<?xml version="1.0"?>
<rdf:RDF xmlns="http://www.semanticweb.org/tylerswheeler/ontologies/2017/7/EmpowerBP#"
     xml:base="http://www.semanticweb.org/tylerswheeler/ontologies/2017/7/EmpowerBP"
     xmlns:rdf="http://www.w3.org/1999/02/22-rdf-syntax-ns#"
     xmlns:owl="http://www.w3.org/2002/07/owl#"
     xmlns:xml="http://www.w3.org/XML/1998/namespace"
     xmlns:xsd="http://www.w3.org/2001/XMLSchema#"
     xmlns:EmpowerBP="http://www.semanticweb.org/tswheeler/ontologies/2016/3/EmpowerBP#"
     xmlns:rdfs="http://www.w3.org/2000/01/rdf-schema#">
    <owl:Ontology rdf:about="http://www.semanticweb.org/tylerswheeler/ontologies/2017/7/EmpowerBP">
        <rdfs:comment>The Behaviour Change Technique Taxonomy</rdfs:comment>
    </owl:Ontology>
    


    <!-- 
    ///////////////////////////////////////////////////////////////////////////////////////
    //
    // Object Properties
    //
    ///////////////////////////////////////////////////////////////////////////////////////
     -->

    


    <!-- http://www.semanticweb.org/tswheeler/ontologies/2016/3/EmpowerBP#canAssessCOMBConstruct -->

    <owl:ObjectProperty rdf:about="http://www.semanticweb.org/tswheeler/ontologies/2016/3/EmpowerBP#canAssessCOMBConstruct">
        <rdfs:domain rdf:resource="http://www.semanticweb.org/tswheeler/ontologies/2016/3/EmpowerBP#COMBAssessmentItem"/>
        <rdfs:range rdf:resource="http://www.semanticweb.org/tswheeler/ontologies/2016/3/EmpowerBP#COMBConstruct"/>
    </owl:ObjectProperty>
    


    <!-- http://www.semanticweb.org/tswheeler/ontologies/2016/3/EmpowerBP#canBlock -->

    <owl:ObjectProperty rdf:about="http://www.semanticweb.org/tswheeler/ontologies/2016/3/EmpowerBP#canBlock">
        <rdfs:domain rdf:resource="http://www.semanticweb.org/tswheeler/ontologies/2016/3/EmpowerBP#Obstacle"/>
        <rdfs:range rdf:resource="http://www.semanticweb.org/tswheeler/ontologies/2016/3/EmpowerBP#InterventionGoal"/>
    </owl:ObjectProperty>
    


    <!-- http://www.semanticweb.org/tswheeler/ontologies/2016/3/EmpowerBP#canResolve -->

    <owl:ObjectProperty rdf:about="http://www.semanticweb.org/tswheeler/ontologies/2016/3/EmpowerBP#canResolve">
        <rdfs:domain rdf:resource="http://www.semanticweb.org/tswheeler/ontologies/2016/3/EmpowerBP#ObstacleTip"/>
        <rdfs:range rdf:resource="http://www.semanticweb.org/tswheeler/ontologies/2016/3/EmpowerBP#Obstacle"/>
    </owl:ObjectProperty>
    


    <!-- http://www.semanticweb.org/tswheeler/ontologies/2016/3/EmpowerBP#evaluatesConstruct -->

    <owl:ObjectProperty rdf:about="http://www.semanticweb.org/tswheeler/ontologies/2016/3/EmpowerBP#evaluatesConstruct">
        <rdfs:domain rdf:resource="http://www.semanticweb.org/tswheeler/ontologies/2016/3/EmpowerBP#Assessment"/>
        <rdfs:range rdf:resource="http://www.semanticweb.org/tswheeler/ontologies/2016/3/EmpowerBP#Construct"/>
    </owl:ObjectProperty>
    


    <!-- http://www.semanticweb.org/tswheeler/ontologies/2016/3/EmpowerBP#hasAssessmentItem -->

    <owl:ObjectProperty rdf:about="http://www.semanticweb.org/tswheeler/ontologies/2016/3/EmpowerBP#hasAssessmentItem">
        <owl:inverseOf rdf:resource="http://www.semanticweb.org/tswheeler/ontologies/2016/3/EmpowerBP#isPartOfAssessment"/>
        <rdfs:domain rdf:resource="http://www.semanticweb.org/tswheeler/ontologies/2016/3/EmpowerBP#Assessment"/>
        <rdfs:range rdf:resource="http://www.semanticweb.org/tswheeler/ontologies/2016/3/EmpowerBP#AssessmentItem"/>
    </owl:ObjectProperty>
    


    <!-- http://www.semanticweb.org/tswheeler/ontologies/2016/3/EmpowerBP#hasAssociatedObstacle -->

    <owl:ObjectProperty rdf:about="http://www.semanticweb.org/tswheeler/ontologies/2016/3/EmpowerBP#hasAssociatedObstacle">
        <rdfs:domain rdf:resource="http://www.semanticweb.org/tswheeler/ontologies/2016/3/EmpowerBP#AssessmentItem"/>
        <rdfs:range rdf:resource="http://www.semanticweb.org/tswheeler/ontologies/2016/3/EmpowerBP#Obstacle"/>
    </owl:ObjectProperty>
    


    <!-- http://www.semanticweb.org/tswheeler/ontologies/2016/3/EmpowerBP#hasCommonBCT -->

    <owl:ObjectProperty rdf:about="http://www.semanticweb.org/tswheeler/ontologies/2016/3/EmpowerBP#hasCommonBCT">
        <owl:inverseOf rdf:resource="http://www.semanticweb.org/tswheeler/ontologies/2016/3/EmpowerBP#isAppropriateForInterventionFunciton"/>
        <rdfs:domain rdf:resource="http://www.semanticweb.org/tswheeler/ontologies/2016/3/EmpowerBP#InterventionFuction"/>
        <rdfs:range rdf:resource="http://purl.bioontology.org/ontology/BCTT#BehaviourChangeTechnique"/>
    </owl:ObjectProperty>
    


    <!-- http://www.semanticweb.org/tswheeler/ontologies/2016/3/EmpowerBP#hasEffectiveInterventionFunction -->

    <owl:ObjectProperty rdf:about="http://www.semanticweb.org/tswheeler/ontologies/2016/3/EmpowerBP#hasEffectiveInterventionFunction">
        <owl:inverseOf rdf:resource="http://www.semanticweb.org/tswheeler/ontologies/2016/3/EmpowerBP#isEffectiveForTDFDomain"/>
        <rdfs:domain rdf:resource="http://www.semanticweb.org/tswheeler/ontologies/2016/3/EmpowerBP#TDFDomain"/>
        <rdfs:range rdf:resource="http://www.semanticweb.org/tswheeler/ontologies/2016/3/EmpowerBP#InterventionFuction"/>
    </owl:ObjectProperty>
    


    <!-- http://www.semanticweb.org/tswheeler/ontologies/2016/3/EmpowerBP#hasHealthCondition -->

    <owl:ObjectProperty rdf:about="http://www.semanticweb.org/tswheeler/ontologies/2016/3/EmpowerBP#hasHealthCondition">
        <rdfs:domain rdf:resource="http://www.semanticweb.org/tswheeler/ontologies/2016/3/EmpowerBP#Patient"/>
    </owl:ObjectProperty>
    


    <!-- http://www.semanticweb.org/tswheeler/ontologies/2016/3/EmpowerBP#hasInterventionGoal -->

    <owl:ObjectProperty rdf:about="http://www.semanticweb.org/tswheeler/ontologies/2016/3/EmpowerBP#hasInterventionGoal">
        <rdfs:domain rdf:resource="http://www.semanticweb.org/tswheeler/ontologies/2016/3/EmpowerBP#Patient"/>
        <rdfs:range rdf:resource="http://www.semanticweb.org/tswheeler/ontologies/2016/3/EmpowerBP#InterventionGoal"/>
    </owl:ObjectProperty>
    


    <!-- http://www.semanticweb.org/tswheeler/ontologies/2016/3/EmpowerBP#hasMostCommonBCT -->

    <owl:ObjectProperty rdf:about="http://www.semanticweb.org/tswheeler/ontologies/2016/3/EmpowerBP#hasMostCommonBCT">
        <owl:inverseOf rdf:resource="http://www.semanticweb.org/tswheeler/ontologies/2016/3/EmpowerBP#isMostAppropriateForInterventionFunction"/>
        <rdfs:domain rdf:resource="http://www.semanticweb.org/tswheeler/ontologies/2016/3/EmpowerBP#InterventionFuction"/>
        <rdfs:range rdf:resource="http://purl.bioontology.org/ontology/BCTT#BehaviourChangeTechnique"/>
    </owl:ObjectProperty>
    


    <!-- http://www.semanticweb.org/tswheeler/ontologies/2016/3/EmpowerBP#hasObstacle -->

    <owl:ObjectProperty rdf:about="http://www.semanticweb.org/tswheeler/ontologies/2016/3/EmpowerBP#hasObstacle">
        <rdfs:domain rdf:resource="http://www.semanticweb.org/tswheeler/ontologies/2016/3/EmpowerBP#Patient"/>
        <rdfs:range rdf:resource="http://www.semanticweb.org/tswheeler/ontologies/2016/3/EmpowerBP#Obstacle"/>
    </owl:ObjectProperty>
    


    <!-- http://www.semanticweb.org/tswheeler/ontologies/2016/3/EmpowerBP#hasRelevantTDF -->

    <owl:ObjectProperty rdf:about="http://www.semanticweb.org/tswheeler/ontologies/2016/3/EmpowerBP#hasRelevantTDF">
        <rdfs:domain rdf:resource="http://www.semanticweb.org/tswheeler/ontologies/2016/3/EmpowerBP#Obstacle"/>
        <rdfs:range rdf:resource="http://www.semanticweb.org/tswheeler/ontologies/2016/3/EmpowerBP#TDFDomain"/>
    </owl:ObjectProperty>
    


    <!-- http://www.semanticweb.org/tswheeler/ontologies/2016/3/EmpowerBP#isAppropriateForInterventionFunciton -->

    <owl:ObjectProperty rdf:about="http://www.semanticweb.org/tswheeler/ontologies/2016/3/EmpowerBP#isAppropriateForInterventionFunciton">
        <rdfs:domain rdf:resource="http://purl.bioontology.org/ontology/BCTT#BehaviourChangeTechnique"/>
        <rdfs:range rdf:resource="http://www.semanticweb.org/tswheeler/ontologies/2016/3/EmpowerBP#InterventionFuction"/>
    </owl:ObjectProperty>
    


    <!-- http://www.semanticweb.org/tswheeler/ontologies/2016/3/EmpowerBP#isAppropriateForInterventionGoal -->

    <owl:ObjectProperty rdf:about="http://www.semanticweb.org/tswheeler/ontologies/2016/3/EmpowerBP#isAppropriateForInterventionGoal">
        <rdfs:domain rdf:resource="http://www.semanticweb.org/tswheeler/ontologies/2016/3/EmpowerBP#InterventionItem"/>
        <rdfs:range rdf:resource="http://www.semanticweb.org/tswheeler/ontologies/2016/3/EmpowerBP#InterventionGoal"/>
    </owl:ObjectProperty>
    


    <!-- http://www.semanticweb.org/tswheeler/ontologies/2016/3/EmpowerBP#isAssessedBy -->

    <owl:ObjectProperty rdf:about="http://www.semanticweb.org/tswheeler/ontologies/2016/3/EmpowerBP#isAssessedBy">
        <rdfs:domain rdf:resource="http://www.semanticweb.org/tswheeler/ontologies/2016/3/EmpowerBP#Patient"/>
        <rdfs:range rdf:resource="http://www.semanticweb.org/tswheeler/ontologies/2016/3/EmpowerBP#Assessment"/>
    </owl:ObjectProperty>
    


    <!-- http://www.semanticweb.org/tswheeler/ontologies/2016/3/EmpowerBP#isEffectiveForTDFDomain -->

    <owl:ObjectProperty rdf:about="http://www.semanticweb.org/tswheeler/ontologies/2016/3/EmpowerBP#isEffectiveForTDFDomain">
        <rdfs:domain rdf:resource="http://www.semanticweb.org/tswheeler/ontologies/2016/3/EmpowerBP#InterventionFuction"/>
        <rdfs:range rdf:resource="http://www.semanticweb.org/tswheeler/ontologies/2016/3/EmpowerBP#TDFDomain"/>
    </owl:ObjectProperty>
    


    <!-- http://www.semanticweb.org/tswheeler/ontologies/2016/3/EmpowerBP#isMostAppropriateForInterventionFunction -->

    <owl:ObjectProperty rdf:about="http://www.semanticweb.org/tswheeler/ontologies/2016/3/EmpowerBP#isMostAppropriateForInterventionFunction">
        <rdfs:domain rdf:resource="http://purl.bioontology.org/ontology/BCTT#BehaviourChangeTechnique"/>
        <rdfs:range rdf:resource="http://www.semanticweb.org/tswheeler/ontologies/2016/3/EmpowerBP#InterventionFuction"/>
    </owl:ObjectProperty>
    


    <!-- http://www.semanticweb.org/tswheeler/ontologies/2016/3/EmpowerBP#isNotAppropriateForHealthCondition -->

    <owl:ObjectProperty rdf:about="http://www.semanticweb.org/tswheeler/ontologies/2016/3/EmpowerBP#isNotAppropriateForHealthCondition">
        <rdfs:domain rdf:resource="http://www.semanticweb.org/tswheeler/ontologies/2016/3/EmpowerBP#InterventionItem"/>
    </owl:ObjectProperty>
    


    <!-- http://www.semanticweb.org/tswheeler/ontologies/2016/3/EmpowerBP#isNotAppropriateForMedication -->

    <owl:ObjectProperty rdf:about="http://www.semanticweb.org/tswheeler/ontologies/2016/3/EmpowerBP#isNotAppropriateForMedication">
        <rdfs:domain rdf:resource="http://www.semanticweb.org/tswheeler/ontologies/2016/3/EmpowerBP#InterventionItem"/>
    </owl:ObjectProperty>
    


    <!-- http://www.semanticweb.org/tswheeler/ontologies/2016/3/EmpowerBP#isPartOfAssessment -->

    <owl:ObjectProperty rdf:about="http://www.semanticweb.org/tswheeler/ontologies/2016/3/EmpowerBP#isPartOfAssessment"/>
    


    <!-- http://www.semanticweb.org/tswheeler/ontologies/2016/3/EmpowerBP#isRelatedToCOMB -->

    <owl:ObjectProperty rdf:about="http://www.semanticweb.org/tswheeler/ontologies/2016/3/EmpowerBP#isRelatedToCOMB">
        <owl:inverseOf rdf:resource="http://www.semanticweb.org/tswheeler/ontologies/2016/3/EmpowerBP#isRelatedToTDF"/>
        <rdfs:domain rdf:resource="http://www.semanticweb.org/tswheeler/ontologies/2016/3/EmpowerBP#TDFDomain"/>
        <rdfs:range rdf:resource="http://www.semanticweb.org/tswheeler/ontologies/2016/3/EmpowerBP#COMBConstruct"/>
    </owl:ObjectProperty>
    


    <!-- http://www.semanticweb.org/tswheeler/ontologies/2016/3/EmpowerBP#isRelatedToTDF -->

    <owl:ObjectProperty rdf:about="http://www.semanticweb.org/tswheeler/ontologies/2016/3/EmpowerBP#isRelatedToTDF">
        <rdfs:domain rdf:resource="http://www.semanticweb.org/tswheeler/ontologies/2016/3/EmpowerBP#COMBConstruct"/>
        <rdfs:range rdf:resource="http://www.semanticweb.org/tswheeler/ontologies/2016/3/EmpowerBP#TDFDomain"/>
    </owl:ObjectProperty>
    


    <!-- http://www.semanticweb.org/tswheeler/ontologies/2016/3/EmpowerBP#isSpecificToGoal -->

    <owl:ObjectProperty rdf:about="http://www.semanticweb.org/tswheeler/ontologies/2016/3/EmpowerBP#isSpecificToGoal">
        <rdfs:domain rdf:resource="http://www.semanticweb.org/tswheeler/ontologies/2016/3/EmpowerBP#AssessmentItem"/>
        <rdfs:range rdf:resource="http://www.semanticweb.org/tswheeler/ontologies/2016/3/EmpowerBP#InterventionGoal"/>
    </owl:ObjectProperty>
    


    <!-- http://www.semanticweb.org/tswheeler/ontologies/2016/3/EmpowerBP#isTakingMedication -->

    <owl:ObjectProperty rdf:about="http://www.semanticweb.org/tswheeler/ontologies/2016/3/EmpowerBP#isTakingMedication">
        <rdfs:domain rdf:resource="http://www.semanticweb.org/tswheeler/ontologies/2016/3/EmpowerBP#Patient"/>
    </owl:ObjectProperty>
    


    <!-- http://www.semanticweb.org/tswheeler/ontologies/2016/3/EmpowerBP#isWarrantedBy -->

    <owl:ObjectProperty rdf:about="http://www.semanticweb.org/tswheeler/ontologies/2016/3/EmpowerBP#isWarrantedBy">
        <rdfs:domain rdf:resource="http://www.semanticweb.org/tswheeler/ontologies/2016/3/EmpowerBP#InterventionItem"/>
        <rdfs:range rdf:resource="http://purl.bioontology.org/ontology/BCTT#BehaviourChangeTechnique"/>
    </owl:ObjectProperty>
    


    <!-- 
    ///////////////////////////////////////////////////////////////////////////////////////
    //
    // Data properties
    //
    ///////////////////////////////////////////////////////////////////////////////////////
     -->

    


    <!-- http://www.semanticweb.org/tswheeler/ontologies/2016/3/EmpowerBP#AutomaticMotivationScore -->

    <owl:DatatypeProperty rdf:about="http://www.semanticweb.org/tswheeler/ontologies/2016/3/EmpowerBP#AutomaticMotivationScore">
        <rdfs:subPropertyOf rdf:resource="http://www.semanticweb.org/tswheeler/ontologies/2016/3/EmpowerBP#COMBScore"/>
        <rdf:type rdf:resource="http://www.w3.org/2002/07/owl#FunctionalProperty"/>
    </owl:DatatypeProperty>
    


    <!-- http://www.semanticweb.org/tswheeler/ontologies/2016/3/EmpowerBP#COMBScore -->

    <owl:DatatypeProperty rdf:about="http://www.semanticweb.org/tswheeler/ontologies/2016/3/EmpowerBP#COMBScore">
        <rdfs:subPropertyOf rdf:resource="http://www.semanticweb.org/tswheeler/ontologies/2016/3/EmpowerBP#assessmentScore"/>
        <rdf:type rdf:resource="http://www.w3.org/2002/07/owl#FunctionalProperty"/>
        <rdfs:range rdf:resource="http://www.w3.org/2001/XMLSchema#integer"/>
    </owl:DatatypeProperty>
    


    <!-- http://www.semanticweb.org/tswheeler/ontologies/2016/3/EmpowerBP#PhyscologicalCapabilityScore -->

    <owl:DatatypeProperty rdf:about="http://www.semanticweb.org/tswheeler/ontologies/2016/3/EmpowerBP#PhyscologicalCapabilityScore">
        <rdfs:subPropertyOf rdf:resource="http://www.semanticweb.org/tswheeler/ontologies/2016/3/EmpowerBP#COMBScore"/>
        <rdf:type rdf:resource="http://www.w3.org/2002/07/owl#FunctionalProperty"/>
    </owl:DatatypeProperty>
    


    <!-- http://www.semanticweb.org/tswheeler/ontologies/2016/3/EmpowerBP#PhysicalCapabilityScore -->

    <owl:DatatypeProperty rdf:about="http://www.semanticweb.org/tswheeler/ontologies/2016/3/EmpowerBP#PhysicalCapabilityScore">
        <rdfs:subPropertyOf rdf:resource="http://www.semanticweb.org/tswheeler/ontologies/2016/3/EmpowerBP#COMBScore"/>
        <rdf:type rdf:resource="http://www.w3.org/2002/07/owl#FunctionalProperty"/>
    </owl:DatatypeProperty>
    


    <!-- http://www.semanticweb.org/tswheeler/ontologies/2016/3/EmpowerBP#PhysicalOpportunityScore -->

    <owl:DatatypeProperty rdf:about="http://www.semanticweb.org/tswheeler/ontologies/2016/3/EmpowerBP#PhysicalOpportunityScore">
        <rdfs:subPropertyOf rdf:resource="http://www.semanticweb.org/tswheeler/ontologies/2016/3/EmpowerBP#COMBScore"/>
        <rdf:type rdf:resource="http://www.w3.org/2002/07/owl#FunctionalProperty"/>
    </owl:DatatypeProperty>
    


    <!-- http://www.semanticweb.org/tswheeler/ontologies/2016/3/EmpowerBP#ReflectiveMotivationScore -->

    <owl:DatatypeProperty rdf:about="http://www.semanticweb.org/tswheeler/ontologies/2016/3/EmpowerBP#ReflectiveMotivationScore">
        <rdfs:subPropertyOf rdf:resource="http://www.semanticweb.org/tswheeler/ontologies/2016/3/EmpowerBP#COMBScore"/>
        <rdf:type rdf:resource="http://www.w3.org/2002/07/owl#FunctionalProperty"/>
    </owl:DatatypeProperty>
    


    <!-- http://www.semanticweb.org/tswheeler/ontologies/2016/3/EmpowerBP#SocialOpportunityScore -->

    <owl:DatatypeProperty rdf:about="http://www.semanticweb.org/tswheeler/ontologies/2016/3/EmpowerBP#SocialOpportunityScore">
        <rdfs:subPropertyOf rdf:resource="http://www.semanticweb.org/tswheeler/ontologies/2016/3/EmpowerBP#COMBScore"/>
        <rdf:type rdf:resource="http://www.w3.org/2002/07/owl#FunctionalProperty"/>
    </owl:DatatypeProperty>
    


    <!-- http://www.semanticweb.org/tswheeler/ontologies/2016/3/EmpowerBP#actorHomeProvince -->

    <owl:DatatypeProperty rdf:about="http://www.semanticweb.org/tswheeler/ontologies/2016/3/EmpowerBP#actorHomeProvince">
        <rdfs:subPropertyOf rdf:resource="http://www.w3.org/2002/07/owl#topDataProperty"/>
        <rdf:type rdf:resource="http://www.w3.org/2002/07/owl#FunctionalProperty"/>
        <rdfs:domain rdf:resource="http://www.semanticweb.org/tswheeler/ontologies/2016/3/EmpowerBP#Patient"/>
        <rdfs:range rdf:resource="http://www.w3.org/2001/XMLSchema#integer"/>
        <rdfs:comment>The Canadian province or territory a patient currently lives in.

1=Alberta
2=British Columbia
3=Manitoba
4=New Brunswick
5=Newfoundland and Labrador
6=Nova Scotia
7=Ontario
8=Prince Edward Island
9=Quebec
10=Saskatchewan
11=Northwest Territories
12=Nunavut
13=Yukon</rdfs:comment>
    </owl:DatatypeProperty>
    


    <!-- http://www.semanticweb.org/tswheeler/ontologies/2016/3/EmpowerBP#actorName -->

    <owl:DatatypeProperty rdf:about="http://www.semanticweb.org/tswheeler/ontologies/2016/3/EmpowerBP#actorName">
        <rdf:type rdf:resource="http://www.w3.org/2002/07/owl#FunctionalProperty"/>
        <rdfs:domain rdf:resource="http://www.semanticweb.org/tswheeler/ontologies/2016/3/EmpowerBP#Actor"/>
        <rdfs:range rdf:resource="http://www.w3.org/2001/XMLSchema#string"/>
        <rdfs:comment>An actor&apos;s preferred name.</rdfs:comment>
    </owl:DatatypeProperty>
    


    <!-- http://www.semanticweb.org/tswheeler/ontologies/2016/3/EmpowerBP#age -->

    <owl:DatatypeProperty rdf:about="http://www.semanticweb.org/tswheeler/ontologies/2016/3/EmpowerBP#age">
        <rdfs:subPropertyOf rdf:resource="http://www.semanticweb.org/tswheeler/ontologies/2016/3/EmpowerBP#non-modifiableElement"/>
        <rdf:type rdf:resource="http://www.w3.org/2002/07/owl#FunctionalProperty"/>
        <rdfs:range rdf:resource="http://www.w3.org/2001/XMLSchema#nonNegativeInteger"/>
        <rdfs:comment>Age in years.</rdfs:comment>
    </owl:DatatypeProperty>
    


    <!-- http://www.semanticweb.org/tswheeler/ontologies/2016/3/EmpowerBP#appropriateForAutomaticMotivation -->

    <owl:DatatypeProperty rdf:about="http://www.semanticweb.org/tswheeler/ontologies/2016/3/EmpowerBP#appropriateForAutomaticMotivation">
        <rdfs:subPropertyOf rdf:resource="http://www.semanticweb.org/tswheeler/ontologies/2016/3/EmpowerBP#interventionItemElement"/>
        <rdf:type rdf:resource="http://www.w3.org/2002/07/owl#FunctionalProperty"/>
        <rdfs:range rdf:resource="http://www.w3.org/2001/XMLSchema#integer"/>
        <rdfs:comment>The minimum user AutomaticMotivation score at which this InterventionItem will be suggested</rdfs:comment>
    </owl:DatatypeProperty>
    


    <!-- http://www.semanticweb.org/tswheeler/ontologies/2016/3/EmpowerBP#appropriateForLocation -->

    <owl:DatatypeProperty rdf:about="http://www.semanticweb.org/tswheeler/ontologies/2016/3/EmpowerBP#appropriateForLocation">
        <rdfs:subPropertyOf rdf:resource="http://www.semanticweb.org/tswheeler/ontologies/2016/3/EmpowerBP#interventionItemElement"/>
        <rdf:type rdf:resource="http://www.w3.org/2002/07/owl#FunctionalProperty"/>
        <rdfs:range rdf:resource="http://www.w3.org/2001/XMLSchema#integer"/>
        <rdfs:comment>The Canadian province or territory an InterventionItem should be suggested in (default 0)

0 = Any
1=Alberta
2=British Columbia
3=Manitoba
4=New Brunswick
5=Newfoundland and Labrador
6=Nova Scotia
7=Ontario
8=Prince Edward Island
9=Quebec
10=Saskatchewan
11=Northwest Territories
12=Nunavut
13=Yukon</rdfs:comment>
    </owl:DatatypeProperty>
    


    <!-- http://www.semanticweb.org/tswheeler/ontologies/2016/3/EmpowerBP#appropriateForPhysicalCapability -->

    <owl:DatatypeProperty rdf:about="http://www.semanticweb.org/tswheeler/ontologies/2016/3/EmpowerBP#appropriateForPhysicalCapability">
        <rdfs:subPropertyOf rdf:resource="http://www.semanticweb.org/tswheeler/ontologies/2016/3/EmpowerBP#interventionItemElement"/>
        <rdf:type rdf:resource="http://www.w3.org/2002/07/owl#FunctionalProperty"/>
        <rdfs:range rdf:resource="http://www.w3.org/2001/XMLSchema#integer"/>
        <rdfs:comment>The minimum user PhysicalCapability score at which this InterventionItem will be suggested</rdfs:comment>
    </owl:DatatypeProperty>
    


    <!-- http://www.semanticweb.org/tswheeler/ontologies/2016/3/EmpowerBP#appropriateForPhysicalOpportunity -->

    <owl:DatatypeProperty rdf:about="http://www.semanticweb.org/tswheeler/ontologies/2016/3/EmpowerBP#appropriateForPhysicalOpportunity">
        <rdfs:subPropertyOf rdf:resource="http://www.semanticweb.org/tswheeler/ontologies/2016/3/EmpowerBP#interventionItemElement"/>
        <rdf:type rdf:resource="http://www.w3.org/2002/07/owl#FunctionalProperty"/>
        <rdfs:range rdf:resource="http://www.w3.org/2001/XMLSchema#integer"/>
        <rdfs:comment>The minimum user PhysicalOpportunity score at which this InterventionItem will be suggested</rdfs:comment>
    </owl:DatatypeProperty>
    


    <!-- http://www.semanticweb.org/tswheeler/ontologies/2016/3/EmpowerBP#appropriateForPsychologicalCapability -->

    <owl:DatatypeProperty rdf:about="http://www.semanticweb.org/tswheeler/ontologies/2016/3/EmpowerBP#appropriateForPsychologicalCapability">
        <rdfs:subPropertyOf rdf:resource="http://www.semanticweb.org/tswheeler/ontologies/2016/3/EmpowerBP#interventionItemElement"/>
        <rdf:type rdf:resource="http://www.w3.org/2002/07/owl#FunctionalProperty"/>
        <rdfs:range rdf:resource="http://www.w3.org/2001/XMLSchema#integer"/>
        <rdfs:comment>The minimum user PsychologicalCapability score at which this InterventionItem will be suggested</rdfs:comment>
    </owl:DatatypeProperty>
    


    <!-- http://www.semanticweb.org/tswheeler/ontologies/2016/3/EmpowerBP#appropriateForReflectiveMotivation -->

    <owl:DatatypeProperty rdf:about="http://www.semanticweb.org/tswheeler/ontologies/2016/3/EmpowerBP#appropriateForReflectiveMotivation">
        <rdfs:subPropertyOf rdf:resource="http://www.semanticweb.org/tswheeler/ontologies/2016/3/EmpowerBP#interventionItemElement"/>
        <rdf:type rdf:resource="http://www.w3.org/2002/07/owl#FunctionalProperty"/>
        <rdfs:range rdf:resource="http://www.w3.org/2001/XMLSchema#integer"/>
        <rdfs:comment>The minimum user ReflexiveMotivation score at which this InterventionItem will be suggested</rdfs:comment>
    </owl:DatatypeProperty>
    


    <!-- http://www.semanticweb.org/tswheeler/ontologies/2016/3/EmpowerBP#appropriateForSocialOpportunity -->

    <owl:DatatypeProperty rdf:about="http://www.semanticweb.org/tswheeler/ontologies/2016/3/EmpowerBP#appropriateForSocialOpportunity">
        <rdfs:subPropertyOf rdf:resource="http://www.semanticweb.org/tswheeler/ontologies/2016/3/EmpowerBP#interventionItemElement"/>
        <rdf:type rdf:resource="http://www.w3.org/2002/07/owl#FunctionalProperty"/>
        <rdfs:range rdf:resource="http://www.w3.org/2001/XMLSchema#integer"/>
        <rdfs:comment>The minimum user SocialOpportunity score at which this InterventionItem will be suggested</rdfs:comment>
    </owl:DatatypeProperty>
    


    <!-- http://www.semanticweb.org/tswheeler/ontologies/2016/3/EmpowerBP#assessmentFinalScore -->

    <owl:DatatypeProperty rdf:about="http://www.semanticweb.org/tswheeler/ontologies/2016/3/EmpowerBP#assessmentFinalScore">
        <rdf:type rdf:resource="http://www.w3.org/2002/07/owl#FunctionalProperty"/>
        <rdfs:domain rdf:resource="http://www.semanticweb.org/tswheeler/ontologies/2016/3/EmpowerBP#Assessment"/>
        <rdfs:range rdf:resource="http://www.w3.org/2001/XMLSchema#integer"/>
        <rdfs:comment>Sum of all AssessmentItem itemScore in an Assessment.</rdfs:comment>
    </owl:DatatypeProperty>
    


    <!-- http://www.semanticweb.org/tswheeler/ontologies/2016/3/EmpowerBP#assessmentItemElement -->

    <owl:DatatypeProperty rdf:about="http://www.semanticweb.org/tswheeler/ontologies/2016/3/EmpowerBP#assessmentItemElement">
        <rdfs:subPropertyOf rdf:resource="http://www.w3.org/2002/07/owl#topDataProperty"/>
    </owl:DatatypeProperty>
    


    <!-- http://www.semanticweb.org/tswheeler/ontologies/2016/3/EmpowerBP#assessmentItemExamples -->

    <owl:DatatypeProperty rdf:about="http://www.semanticweb.org/tswheeler/ontologies/2016/3/EmpowerBP#assessmentItemExamples">
        <rdfs:subPropertyOf rdf:resource="http://www.semanticweb.org/tswheeler/ontologies/2016/3/EmpowerBP#assessmentItemElement"/>
        <rdf:type rdf:resource="http://www.w3.org/2002/07/owl#FunctionalProperty"/>
        <rdfs:domain rdf:resource="http://www.semanticweb.org/tswheeler/ontologies/2016/3/EmpowerBP#AssessmentItem"/>
        <rdfs:range rdf:resource="http://www.w3.org/2001/XMLSchema#string"/>
        <rdfs:comment>Examples provided to the user when asked to rate an assessmentItem.</rdfs:comment>
    </owl:DatatypeProperty>
    


    <!-- http://www.semanticweb.org/tswheeler/ontologies/2016/3/EmpowerBP#assessmentItemID -->

    <owl:DatatypeProperty rdf:about="http://www.semanticweb.org/tswheeler/ontologies/2016/3/EmpowerBP#assessmentItemID">
        <rdfs:subPropertyOf rdf:resource="http://www.semanticweb.org/tswheeler/ontologies/2016/3/EmpowerBP#assessmentItemElement"/>
        <rdf:type rdf:resource="http://www.w3.org/2002/07/owl#FunctionalProperty"/>
        <rdfs:domain rdf:resource="http://www.semanticweb.org/tswheeler/ontologies/2016/3/EmpowerBP#AssessmentItem"/>
        <rdfs:range rdf:resource="http://www.w3.org/2001/XMLSchema#string"/>
    </owl:DatatypeProperty>
    


    <!-- http://www.semanticweb.org/tswheeler/ontologies/2016/3/EmpowerBP#assessmentItemText -->

    <owl:DatatypeProperty rdf:about="http://www.semanticweb.org/tswheeler/ontologies/2016/3/EmpowerBP#assessmentItemText">
        <rdfs:subPropertyOf rdf:resource="http://www.semanticweb.org/tswheeler/ontologies/2016/3/EmpowerBP#assessmentItemElement"/>
        <rdf:type rdf:resource="http://www.w3.org/2002/07/owl#FunctionalProperty"/>
        <rdfs:domain rdf:resource="http://www.semanticweb.org/tswheeler/ontologies/2016/3/EmpowerBP#AssessmentItem"/>
        <rdfs:range rdf:resource="http://www.w3.org/2001/XMLSchema#string"/>
        <rdfs:comment>The text presented to a Patient during an Assessment.</rdfs:comment>
    </owl:DatatypeProperty>
    


    <!-- http://www.semanticweb.org/tswheeler/ontologies/2016/3/EmpowerBP#assessmentScore -->

    <owl:DatatypeProperty rdf:about="http://www.semanticweb.org/tswheeler/ontologies/2016/3/EmpowerBP#assessmentScore">
        <rdfs:subPropertyOf rdf:resource="http://www.semanticweb.org/tswheeler/ontologies/2016/3/EmpowerBP#behaviourProfileElement"/>
    </owl:DatatypeProperty>
    


    <!-- http://www.semanticweb.org/tswheeler/ontologies/2016/3/EmpowerBP#averageDiastolicBP -->

    <owl:DatatypeProperty rdf:about="http://www.semanticweb.org/tswheeler/ontologies/2016/3/EmpowerBP#averageDiastolicBP">
        <rdfs:subPropertyOf rdf:resource="http://www.semanticweb.org/tswheeler/ontologies/2016/3/EmpowerBP#bloodPressure"/>
        <rdf:type rdf:resource="http://www.w3.org/2002/07/owl#FunctionalProperty"/>
        <rdfs:domain rdf:resource="http://www.semanticweb.org/tswheeler/ontologies/2016/3/EmpowerBP#Patient"/>
        <rdfs:range rdf:resource="http://www.w3.org/2001/XMLSchema#nonNegativeInteger"/>
    </owl:DatatypeProperty>
    


    <!-- http://www.semanticweb.org/tswheeler/ontologies/2016/3/EmpowerBP#averageSystolicBP -->

    <owl:DatatypeProperty rdf:about="http://www.semanticweb.org/tswheeler/ontologies/2016/3/EmpowerBP#averageSystolicBP">
        <rdfs:subPropertyOf rdf:resource="http://www.semanticweb.org/tswheeler/ontologies/2016/3/EmpowerBP#bloodPressure"/>
        <rdf:type rdf:resource="http://www.w3.org/2002/07/owl#FunctionalProperty"/>
        <rdfs:domain rdf:resource="http://www.semanticweb.org/tswheeler/ontologies/2016/3/EmpowerBP#Patient"/>
        <rdfs:range rdf:resource="http://www.w3.org/2001/XMLSchema#nonNegativeInteger"/>
    </owl:DatatypeProperty>
    


    <!-- http://www.semanticweb.org/tswheeler/ontologies/2016/3/EmpowerBP#behaviourProfileElement -->

    <owl:DatatypeProperty rdf:about="http://www.semanticweb.org/tswheeler/ontologies/2016/3/EmpowerBP#behaviourProfileElement">
        <rdfs:domain rdf:resource="http://www.semanticweb.org/tswheeler/ontologies/2016/3/EmpowerBP#Patient"/>
    </owl:DatatypeProperty>
    


    <!-- http://www.semanticweb.org/tswheeler/ontologies/2016/3/EmpowerBP#bloodPressure -->

    <owl:DatatypeProperty rdf:about="http://www.semanticweb.org/tswheeler/ontologies/2016/3/EmpowerBP#bloodPressure">
        <rdfs:subPropertyOf rdf:resource="http://www.semanticweb.org/tswheeler/ontologies/2016/3/EmpowerBP#modifiableElement"/>
        <rdfs:comment></rdfs:comment>
    </owl:DatatypeProperty>
    


    <!-- http://www.semanticweb.org/tswheeler/ontologies/2016/3/EmpowerBP#canRepeat -->

    <owl:DatatypeProperty rdf:about="http://www.semanticweb.org/tswheeler/ontologies/2016/3/EmpowerBP#canRepeat">
        <rdfs:subPropertyOf rdf:resource="http://www.semanticweb.org/tswheeler/ontologies/2016/3/EmpowerBP#interventionItemElement"/>
        <rdf:type rdf:resource="http://www.w3.org/2002/07/owl#FunctionalProperty"/>
        <rdfs:range rdf:resource="http://www.w3.org/2001/XMLSchema#integer"/>
        <rdfs:comment>Time (in weeks) after InterventionItem may be repeated</rdfs:comment>
    </owl:DatatypeProperty>
    


    <!-- http://www.semanticweb.org/tswheeler/ontologies/2016/3/EmpowerBP#clinicalProfileElement -->

    <owl:DatatypeProperty rdf:about="http://www.semanticweb.org/tswheeler/ontologies/2016/3/EmpowerBP#clinicalProfileElement">
        <rdfs:subPropertyOf rdf:resource="http://www.w3.org/2002/07/owl#topDataProperty"/>
        <rdfs:domain rdf:resource="http://www.semanticweb.org/tswheeler/ontologies/2016/3/EmpowerBP#Patient"/>
    </owl:DatatypeProperty>
    


    <!-- http://www.semanticweb.org/tswheeler/ontologies/2016/3/EmpowerBP#dailySodiumIntake -->

    <owl:DatatypeProperty rdf:about="http://www.semanticweb.org/tswheeler/ontologies/2016/3/EmpowerBP#dailySodiumIntake">
        <rdfs:subPropertyOf rdf:resource="http://www.semanticweb.org/tswheeler/ontologies/2016/3/EmpowerBP#behaviourProfileElement"/>
        <rdf:type rdf:resource="http://www.w3.org/2002/07/owl#FunctionalProperty"/>
        <rdfs:range rdf:resource="http://www.w3.org/2001/XMLSchema#integer"/>
        <rdfs:comment>Daily estimated sodium intake in milligrams per day, as calculated per BigLife Sodium Calculator</rdfs:comment>
    </owl:DatatypeProperty>
    


    <!-- http://www.semanticweb.org/tswheeler/ontologies/2016/3/EmpowerBP#height -->

    <owl:DatatypeProperty rdf:about="http://www.semanticweb.org/tswheeler/ontologies/2016/3/EmpowerBP#height">
        <rdfs:subPropertyOf rdf:resource="http://www.semanticweb.org/tswheeler/ontologies/2016/3/EmpowerBP#non-modifiableElement"/>
        <rdf:type rdf:resource="http://www.w3.org/2002/07/owl#FunctionalProperty"/>
        <rdfs:domain rdf:resource="http://www.semanticweb.org/tswheeler/ontologies/2016/3/EmpowerBP#Patient"/>
        <rdfs:range rdf:resource="http://www.w3.org/2001/XMLSchema#double"/>
        <rdfs:comment>Height in centimetres.</rdfs:comment>
    </owl:DatatypeProperty>
    


    <!-- http://www.semanticweb.org/tswheeler/ontologies/2016/3/EmpowerBP#interventionItemElement -->

    <owl:DatatypeProperty rdf:about="http://www.semanticweb.org/tswheeler/ontologies/2016/3/EmpowerBP#interventionItemElement">
        <rdfs:subPropertyOf rdf:resource="http://www.w3.org/2002/07/owl#topDataProperty"/>
        <rdfs:domain rdf:resource="http://www.semanticweb.org/tswheeler/ontologies/2016/3/EmpowerBP#InterventionItem"/>
    </owl:DatatypeProperty>
    


    <!-- http://www.semanticweb.org/tswheeler/ontologies/2016/3/EmpowerBP#itemName -->

    <owl:DatatypeProperty rdf:about="http://www.semanticweb.org/tswheeler/ontologies/2016/3/EmpowerBP#itemName">
        <rdfs:subPropertyOf rdf:resource="http://www.semanticweb.org/tswheeler/ontologies/2016/3/EmpowerBP#interventionItemElement"/>
        <rdf:type rdf:resource="http://www.w3.org/2002/07/owl#FunctionalProperty"/>
        <rdfs:domain rdf:resource="http://www.semanticweb.org/tswheeler/ontologies/2016/3/EmpowerBP#InterventionItem"/>
        <rdfs:range rdf:resource="http://www.w3.org/2001/XMLSchema#string"/>
        <rdfs:comment>Name of an InterventionItem</rdfs:comment>
    </owl:DatatypeProperty>
    


    <!-- http://www.semanticweb.org/tswheeler/ontologies/2016/3/EmpowerBP#itemText -->

    <owl:DatatypeProperty rdf:about="http://www.semanticweb.org/tswheeler/ontologies/2016/3/EmpowerBP#itemText">
        <rdfs:subPropertyOf rdf:resource="http://www.semanticweb.org/tswheeler/ontologies/2016/3/EmpowerBP#interventionItemElement"/>
        <rdf:type rdf:resource="http://www.w3.org/2002/07/owl#FunctionalProperty"/>
        <rdfs:domain rdf:resource="http://www.semanticweb.org/tswheeler/ontologies/2016/3/EmpowerBP#InterventionItem"/>
        <rdfs:range rdf:resource="http://www.w3.org/2001/XMLSchema#string"/>
        <rdfs:comment>Text included in an InterventionItem</rdfs:comment>
    </owl:DatatypeProperty>
    


    <!-- http://www.semanticweb.org/tswheeler/ontologies/2016/3/EmpowerBP#maximumUserAge -->

    <owl:DatatypeProperty rdf:about="http://www.semanticweb.org/tswheeler/ontologies/2016/3/EmpowerBP#maximumUserAge">
        <rdfs:subPropertyOf rdf:resource="http://www.semanticweb.org/tswheeler/ontologies/2016/3/EmpowerBP#interventionItemElement"/>
        <rdf:type rdf:resource="http://www.w3.org/2002/07/owl#FunctionalProperty"/>
        <rdfs:range rdf:resource="http://www.w3.org/2001/XMLSchema#integer"/>
        <rdfs:comment>The maximum user age at which this InterventionItem will be suggested (default 120)</rdfs:comment>
    </owl:DatatypeProperty>
    


    <!-- http://www.semanticweb.org/tswheeler/ontologies/2016/3/EmpowerBP#minimumUserAge -->

    <owl:DatatypeProperty rdf:about="http://www.semanticweb.org/tswheeler/ontologies/2016/3/EmpowerBP#minimumUserAge">
        <rdfs:subPropertyOf rdf:resource="http://www.semanticweb.org/tswheeler/ontologies/2016/3/EmpowerBP#interventionItemElement"/>
        <rdf:type rdf:resource="http://www.w3.org/2002/07/owl#FunctionalProperty"/>
        <rdfs:range rdf:resource="http://www.w3.org/2001/XMLSchema#integer"/>
        <rdfs:comment>The minimum user age at which this InterventionItem will be suggested (default 18)</rdfs:comment>
    </owl:DatatypeProperty>
    


    <!-- http://www.semanticweb.org/tswheeler/ontologies/2016/3/EmpowerBP#modifiableElement -->

    <owl:DatatypeProperty rdf:about="http://www.semanticweb.org/tswheeler/ontologies/2016/3/EmpowerBP#modifiableElement">
        <rdfs:subPropertyOf rdf:resource="http://www.semanticweb.org/tswheeler/ontologies/2016/3/EmpowerBP#clinicalProfileElement"/>
        <rdfs:domain rdf:resource="http://www.semanticweb.org/tswheeler/ontologies/2016/3/EmpowerBP#Patient"/>
    </owl:DatatypeProperty>
    


    <!-- http://www.semanticweb.org/tswheeler/ontologies/2016/3/EmpowerBP#non-modifiableElement -->

    <owl:DatatypeProperty rdf:about="http://www.semanticweb.org/tswheeler/ontologies/2016/3/EmpowerBP#non-modifiableElement">
        <rdfs:subPropertyOf rdf:resource="http://www.semanticweb.org/tswheeler/ontologies/2016/3/EmpowerBP#clinicalProfileElement"/>
    </owl:DatatypeProperty>
    


    <!-- http://www.semanticweb.org/tswheeler/ontologies/2016/3/EmpowerBP#physicalActivityLevel -->

    <owl:DatatypeProperty rdf:about="http://www.semanticweb.org/tswheeler/ontologies/2016/3/EmpowerBP#physicalActivityLevel">
        <rdfs:subPropertyOf rdf:resource="http://www.semanticweb.org/tswheeler/ontologies/2016/3/EmpowerBP#behaviourProfileElement"/>
        <rdf:type rdf:resource="http://www.w3.org/2002/07/owl#FunctionalProperty"/>
        <rdfs:range rdf:resource="http://www.w3.org/2001/XMLSchema#integer"/>
        <rdfs:comment>Moderate intensity, dynamic physical exercise (min/week).</rdfs:comment>
    </owl:DatatypeProperty>
    


    <!-- http://www.semanticweb.org/tswheeler/ontologies/2016/3/EmpowerBP#provideJournal -->

    <owl:DatatypeProperty rdf:about="http://www.semanticweb.org/tswheeler/ontologies/2016/3/EmpowerBP#provideJournal">
        <rdfs:subPropertyOf rdf:resource="http://www.semanticweb.org/tswheeler/ontologies/2016/3/EmpowerBP#interventionItemElement"/>
        <rdf:type rdf:resource="http://www.w3.org/2002/07/owl#FunctionalProperty"/>
        <rdfs:domain rdf:resource="http://www.semanticweb.org/tswheeler/ontologies/2016/3/EmpowerBP#InterventionItem"/>
        <rdfs:range rdf:resource="http://www.w3.org/2001/XMLSchema#boolean"/>
        <rdfs:comment>Boolean for whether or not InterventionItem should prompt user to write in reflection journal</rdfs:comment>
    </owl:DatatypeProperty>
    


    <!-- http://www.semanticweb.org/tswheeler/ontologies/2016/3/EmpowerBP#provideLink -->

    <owl:DatatypeProperty rdf:about="http://www.semanticweb.org/tswheeler/ontologies/2016/3/EmpowerBP#provideLink">
        <rdfs:subPropertyOf rdf:resource="http://www.semanticweb.org/tswheeler/ontologies/2016/3/EmpowerBP#interventionItemElement"/>
        <rdf:type rdf:resource="http://www.w3.org/2002/07/owl#FunctionalProperty"/>
        <rdfs:domain rdf:resource="http://www.semanticweb.org/tswheeler/ontologies/2016/3/EmpowerBP#InterventionItem"/>
        <rdfs:range rdf:resource="http://www.w3.org/2001/XMLSchema#boolean"/>
        <rdfs:comment>Boolean for whether or not InterventionItem source should be provided to user</rdfs:comment>
    </owl:DatatypeProperty>
    


    <!-- http://www.semanticweb.org/tswheeler/ontologies/2016/3/EmpowerBP#sex -->

    <owl:DatatypeProperty rdf:about="http://www.semanticweb.org/tswheeler/ontologies/2016/3/EmpowerBP#sex">
        <rdfs:subPropertyOf rdf:resource="http://www.semanticweb.org/tswheeler/ontologies/2016/3/EmpowerBP#non-modifiableElement"/>
        <rdfs:domain rdf:resource="http://www.semanticweb.org/tswheeler/ontologies/2016/3/EmpowerBP#Patient"/>
    </owl:DatatypeProperty>
    


    <!-- http://www.semanticweb.org/tswheeler/ontologies/2016/3/EmpowerBP#sourceURL -->

    <owl:DatatypeProperty rdf:about="http://www.semanticweb.org/tswheeler/ontologies/2016/3/EmpowerBP#sourceURL">
        <rdfs:subPropertyOf rdf:resource="http://www.semanticweb.org/tswheeler/ontologies/2016/3/EmpowerBP#interventionItemElement"/>
        <rdf:type rdf:resource="http://www.w3.org/2002/07/owl#FunctionalProperty"/>
        <rdfs:domain rdf:resource="http://www.semanticweb.org/tswheeler/ontologies/2016/3/EmpowerBP#InterventionItem"/>
        <rdfs:range rdf:resource="http://www.w3.org/2001/XMLSchema#string"/>
        <rdfs:comment>Source URL for an InterventionItem</rdfs:comment>
    </owl:DatatypeProperty>
    


    <!-- http://www.semanticweb.org/tswheeler/ontologies/2016/3/EmpowerBP#weight -->

    <owl:DatatypeProperty rdf:about="http://www.semanticweb.org/tswheeler/ontologies/2016/3/EmpowerBP#weight">
        <rdfs:subPropertyOf rdf:resource="http://www.semanticweb.org/tswheeler/ontologies/2016/3/EmpowerBP#modifiableElement"/>
        <rdf:type rdf:resource="http://www.w3.org/2002/07/owl#FunctionalProperty"/>
        <rdfs:domain rdf:resource="http://www.semanticweb.org/tswheeler/ontologies/2016/3/EmpowerBP#Patient"/>
        <rdfs:range rdf:resource="http://www.w3.org/2001/XMLSchema#double"/>
        <rdfs:comment>Weight in kilograms.</rdfs:comment>
    </owl:DatatypeProperty>
    


    <!-- 
    ///////////////////////////////////////////////////////////////////////////////////////
    //
    // Classes
    //
    ///////////////////////////////////////////////////////////////////////////////////////
     -->

    


    <!-- http://purl.bioontology.org/ontology/BCTT#BehaviourChangeTechnique -->

    <owl:Class rdf:about="http://purl.bioontology.org/ontology/BCTT#BehaviourChangeTechnique">
        <rdfs:comment>The smallest components of a behaviour change intervention that on their own, in favourable circumstances, can bring about change.</rdfs:comment>
    </owl:Class>
    


    <!-- http://purl.bioontology.org/ontology/BCTT#00219 -->

    <owl:Class rdf:about="http://purl.bioontology.org/ontology/BCTT#00219">
        <rdfs:subClassOf rdf:resource="http://purl.bioontology.org/ontology/BCTT#BehaviourChangeTechnique"/>
        <rdfs:label xml:lang="en">Goals and planning</rdfs:label>
    </owl:Class>
    


    <!-- http://purl.bioontology.org/ontology/BCTT#00229 -->

    <owl:Class rdf:about="http://purl.bioontology.org/ontology/BCTT#00229">
        <rdfs:subClassOf rdf:resource="http://purl.bioontology.org/ontology/BCTT#BehaviourChangeTechnique"/>
        <rdfs:label xml:lang="en">Feedback and monitoring</rdfs:label>
    </owl:Class>
    


    <!-- http://purl.bioontology.org/ontology/BCTT#00237 -->

    <owl:Class rdf:about="http://purl.bioontology.org/ontology/BCTT#00237">
        <rdfs:subClassOf rdf:resource="http://purl.bioontology.org/ontology/BCTT#BehaviourChangeTechnique"/>
        <rdfs:label xml:lang="en">Social support</rdfs:label>
    </owl:Class>
    


    <!-- http://purl.bioontology.org/ontology/BCTT#00241 -->

    <owl:Class rdf:about="http://purl.bioontology.org/ontology/BCTT#00241">
        <rdfs:subClassOf rdf:resource="http://purl.bioontology.org/ontology/BCTT#BehaviourChangeTechnique"/>
        <rdfs:label xml:lang="en">Shaping knowledge</rdfs:label>
    </owl:Class>
    


    <!-- http://purl.bioontology.org/ontology/BCTT#00246 -->

    <owl:Class rdf:about="http://purl.bioontology.org/ontology/BCTT#00246">
        <rdfs:subClassOf rdf:resource="http://purl.bioontology.org/ontology/BCTT#BehaviourChangeTechnique"/>
        <rdfs:label xml:lang="en">Natural consequences</rdfs:label>
    </owl:Class>
    


    <!-- http://purl.bioontology.org/ontology/BCTT#00253 -->

    <owl:Class rdf:about="http://purl.bioontology.org/ontology/BCTT#00253">
        <rdfs:subClassOf rdf:resource="http://purl.bioontology.org/ontology/BCTT#BehaviourChangeTechnique"/>
        <rdfs:label xml:lang="en">Comparison of behavior</rdfs:label>
    </owl:Class>
    


    <!-- http://purl.bioontology.org/ontology/BCTT#00257 -->

    <owl:Class rdf:about="http://purl.bioontology.org/ontology/BCTT#00257">
        <rdfs:subClassOf rdf:resource="http://purl.bioontology.org/ontology/BCTT#BehaviourChangeTechnique"/>
        <rdfs:label xml:lang="en">Associations</rdfs:label>
    </owl:Class>
    


    <!-- http://purl.bioontology.org/ontology/BCTT#00266 -->

    <owl:Class rdf:about="http://purl.bioontology.org/ontology/BCTT#00266">
        <rdfs:subClassOf rdf:resource="http://purl.bioontology.org/ontology/BCTT#BehaviourChangeTechnique"/>
        <rdfs:label xml:lang="en">Repetition and substitution</rdfs:label>
    </owl:Class>
    


    <!-- http://purl.bioontology.org/ontology/BCTT#00274 -->

    <owl:Class rdf:about="http://purl.bioontology.org/ontology/BCTT#00274">
        <rdfs:subClassOf rdf:resource="http://purl.bioontology.org/ontology/BCTT#BehaviourChangeTechnique"/>
        <rdfs:label xml:lang="en">Comparison of outcomes</rdfs:label>
    </owl:Class>
    


    <!-- http://purl.bioontology.org/ontology/BCTT#00278 -->

    <owl:Class rdf:about="http://purl.bioontology.org/ontology/BCTT#00278">
        <rdfs:subClassOf rdf:resource="http://purl.bioontology.org/ontology/BCTT#BehaviourChangeTechnique"/>
        <rdfs:label xml:lang="en">Reward and threat</rdfs:label>
    </owl:Class>
    


    <!-- http://purl.bioontology.org/ontology/BCTT#00290 -->

    <owl:Class rdf:about="http://purl.bioontology.org/ontology/BCTT#00290">
        <rdfs:subClassOf rdf:resource="http://purl.bioontology.org/ontology/BCTT#BehaviourChangeTechnique"/>
        <rdfs:label xml:lang="en">Regulation</rdfs:label>
    </owl:Class>
    


    <!-- http://purl.bioontology.org/ontology/BCTT#00295 -->

    <owl:Class rdf:about="http://purl.bioontology.org/ontology/BCTT#00295">
        <rdfs:subClassOf rdf:resource="http://purl.bioontology.org/ontology/BCTT#BehaviourChangeTechnique"/>
        <rdfs:label xml:lang="en">Antecedents</rdfs:label>
    </owl:Class>
    


    <!-- http://purl.bioontology.org/ontology/BCTT#00302 -->

    <owl:Class rdf:about="http://purl.bioontology.org/ontology/BCTT#00302">
        <rdfs:subClassOf rdf:resource="http://purl.bioontology.org/ontology/BCTT#BehaviourChangeTechnique"/>
        <rdfs:label xml:lang="en">Identity</rdfs:label>
    </owl:Class>
    


    <!-- http://purl.bioontology.org/ontology/BCTT#00308 -->

    <owl:Class rdf:about="http://purl.bioontology.org/ontology/BCTT#00308">
        <rdfs:subClassOf rdf:resource="http://purl.bioontology.org/ontology/BCTT#BehaviourChangeTechnique"/>
        <rdfs:label xml:lang="en">Scheduled consequences</rdfs:label>
    </owl:Class>
    


    <!-- http://purl.bioontology.org/ontology/BCTT#00319 -->

    <owl:Class rdf:about="http://purl.bioontology.org/ontology/BCTT#00319">
        <rdfs:subClassOf rdf:resource="http://purl.bioontology.org/ontology/BCTT#BehaviourChangeTechnique"/>
        <rdfs:label xml:lang="en">Self-belief</rdfs:label>
    </owl:Class>
    


    <!-- http://purl.bioontology.org/ontology/BCTT#00324 -->

    <owl:Class rdf:about="http://purl.bioontology.org/ontology/BCTT#00324">
        <rdfs:subClassOf rdf:resource="http://purl.bioontology.org/ontology/BCTT#BehaviourChangeTechnique"/>
        <rdfs:label xml:lang="en">Covert learning</rdfs:label>
    </owl:Class>
    


    <!-- http://www.semanticweb.org/tswheeler/ontologies/2016/3/EmpowerBP#AcquisitionGoal -->

    <owl:Class rdf:about="http://www.semanticweb.org/tswheeler/ontologies/2016/3/EmpowerBP#AcquisitionGoal">
        <rdfs:subClassOf rdf:resource="http://www.semanticweb.org/tswheeler/ontologies/2016/3/EmpowerBP#InterventionGoal"/>
        <rdfs:comment>An InterventionGoal to acquire a behavior the patient currently does not do, or does not do to a criterion (e.g. physical activity).</rdfs:comment>
    </owl:Class>
    


    <!-- http://www.semanticweb.org/tswheeler/ontologies/2016/3/EmpowerBP#Actor -->

    <owl:Class rdf:about="http://www.semanticweb.org/tswheeler/ontologies/2016/3/EmpowerBP#Actor">
        <rdfs:comment>Any individual involved in an intervention.</rdfs:comment>
    </owl:Class>
    


    <!-- http://www.semanticweb.org/tswheeler/ontologies/2016/3/EmpowerBP#Assessment -->

    <owl:Class rdf:about="http://www.semanticweb.org/tswheeler/ontologies/2016/3/EmpowerBP#Assessment">
        <rdfs:comment>A tool consisting of AssessmentItems. Used to evaluate some aspect of a Patient, in regards to a particular Construct. May be specific to particular InterventionGoal.</rdfs:comment>
    </owl:Class>
    


    <!-- http://www.semanticweb.org/tswheeler/ontologies/2016/3/EmpowerBP#AssessmentItem -->

    <owl:Class rdf:about="http://www.semanticweb.org/tswheeler/ontologies/2016/3/EmpowerBP#AssessmentItem">
        <rdfs:comment>A specific question that makes up part of an Assessment.</rdfs:comment>
    </owl:Class>
    


    <!-- http://www.semanticweb.org/tswheeler/ontologies/2016/3/EmpowerBP#AutomaticMotivationAssessment -->

    <owl:Class rdf:about="http://www.semanticweb.org/tswheeler/ontologies/2016/3/EmpowerBP#AutomaticMotivationAssessment">
        <rdfs:subClassOf rdf:resource="http://www.semanticweb.org/tswheeler/ontologies/2016/3/EmpowerBP#COMBAssessment"/>
        <rdfs:comment>A tool to evaluate a Patient&apos;s automatic motivation with respect to a specific InterventionGoal.</rdfs:comment>
    </owl:Class>
    


    <!-- http://www.semanticweb.org/tswheeler/ontologies/2016/3/EmpowerBP#COMBAssessment -->

    <owl:Class rdf:about="http://www.semanticweb.org/tswheeler/ontologies/2016/3/EmpowerBP#COMBAssessment">
        <rdfs:subClassOf rdf:resource="http://www.semanticweb.org/tswheeler/ontologies/2016/3/EmpowerBP#Assessment"/>
        <rdfs:comment>A tool to evaluate one Construct of a Patient&apos;s COM-B profile with respect to a specific InterventionGoal.</rdfs:comment>
    </owl:Class>
    


    <!-- http://www.semanticweb.org/tswheeler/ontologies/2016/3/EmpowerBP#COMBAssessmentItem -->

    <owl:Class rdf:about="http://www.semanticweb.org/tswheeler/ontologies/2016/3/EmpowerBP#COMBAssessmentItem">
        <rdfs:subClassOf rdf:resource="http://www.semanticweb.org/tswheeler/ontologies/2016/3/EmpowerBP#AssessmentItem"/>
        <rdfs:comment>A specific question that makes up part of an COMBAssessment.</rdfs:comment>
    </owl:Class>
    


    <!-- http://www.semanticweb.org/tswheeler/ontologies/2016/3/EmpowerBP#COMBConstruct -->

    <owl:Class rdf:about="http://www.semanticweb.org/tswheeler/ontologies/2016/3/EmpowerBP#COMBConstruct">
        <rdfs:subClassOf rdf:resource="http://www.semanticweb.org/tswheeler/ontologies/2016/3/EmpowerBP#Construct"/>
        <rdfs:comment>Constructs relating to the COM-B Model/Behaviour Change Wheel. These constructs must be present and developed for any behaviour to occur.</rdfs:comment>
    </owl:Class>
    


    <!-- http://www.semanticweb.org/tswheeler/ontologies/2016/3/EmpowerBP#COMBModel -->

    <owl:Class rdf:about="http://www.semanticweb.org/tswheeler/ontologies/2016/3/EmpowerBP#COMBModel">
        <rdfs:subClassOf rdf:resource="http://www.semanticweb.org/tswheeler/ontologies/2016/3/EmpowerBP#Theory"/>
    </owl:Class>
    


    <!-- http://www.semanticweb.org/tswheeler/ontologies/2016/3/EmpowerBP#Capability -->

    <owl:Class rdf:about="http://www.semanticweb.org/tswheeler/ontologies/2016/3/EmpowerBP#Capability">
        <rdfs:subClassOf rdf:resource="http://www.semanticweb.org/tswheeler/ontologies/2016/3/EmpowerBP#COMBConstruct"/>
        <rdfs:comment>Capability can be either ‘physical’ (having the physical skills, strength or stamina) to perform the behaviour or ‘psychological’ (having the knowledge, psychological skills, strength or stamina) to perform the behaviour.</rdfs:comment>
    </owl:Class>
    


    <!-- http://www.semanticweb.org/tswheeler/ontologies/2016/3/EmpowerBP#CessationGoal -->

    <owl:Class rdf:about="http://www.semanticweb.org/tswheeler/ontologies/2016/3/EmpowerBP#CessationGoal">
        <rdfs:subClassOf rdf:resource="http://www.semanticweb.org/tswheeler/ontologies/2016/3/EmpowerBP#InterventionGoal"/>
        <rdfs:comment>An InterventionGoal to cease an undesirable behavior the patient currently engages in (e.g. smoking).</rdfs:comment>
    </owl:Class>
    


    <!-- http://www.semanticweb.org/tswheeler/ontologies/2016/3/EmpowerBP#Construct -->

    <owl:Class rdf:about="http://www.semanticweb.org/tswheeler/ontologies/2016/3/EmpowerBP#Construct">
        <rdfs:comment>A variable, as defined by a Theory, which is not directly observable.</rdfs:comment>
    </owl:Class>
    


    <!-- http://www.semanticweb.org/tswheeler/ontologies/2016/3/EmpowerBP#GradedHealthBehaviour -->

    <owl:Class rdf:about="http://www.semanticweb.org/tswheeler/ontologies/2016/3/EmpowerBP#GradedHealthBehaviour">
        <rdfs:subClassOf rdf:resource="http://www.semanticweb.org/tswheeler/ontologies/2016/3/EmpowerBP#Task"/>
        <rdfs:comment>Tasks that are part of a series with gradual increase in difficulty. A user must complete preceeding tasks to progress to further ones.</rdfs:comment>
    </owl:Class>
    


    <!-- http://www.semanticweb.org/tswheeler/ontologies/2016/3/EmpowerBP#InterventionFuction -->

    <owl:Class rdf:about="http://www.semanticweb.org/tswheeler/ontologies/2016/3/EmpowerBP#InterventionFuction">
        <rdfs:comment>Broad categories of means by which an intervention can change behaviour.</rdfs:comment>
    </owl:Class>
    


    <!-- http://www.semanticweb.org/tswheeler/ontologies/2016/3/EmpowerBP#InterventionGoal -->

    <owl:Class rdf:about="http://www.semanticweb.org/tswheeler/ontologies/2016/3/EmpowerBP#InterventionGoal">
        <rdfs:comment>An overall goal of an intervention (e.g. physical activity promotion, smoking cessation).</rdfs:comment>
    </owl:Class>
    


    <!-- http://www.semanticweb.org/tswheeler/ontologies/2016/3/EmpowerBP#InterventionItem -->

    <owl:Class rdf:about="http://www.semanticweb.org/tswheeler/ontologies/2016/3/EmpowerBP#InterventionItem">
        <rdfs:subClassOf rdf:resource="http://www.w3.org/2002/07/owl#Thing"/>
        <rdfs:comment>Anything that can be provided as part of a counseling intervention (e.g., a recipe).</rdfs:comment>
    </owl:Class>
    


    <!-- http://www.semanticweb.org/tswheeler/ontologies/2016/3/EmpowerBP#Motivation -->

    <owl:Class rdf:about="http://www.semanticweb.org/tswheeler/ontologies/2016/3/EmpowerBP#Motivation">
        <rdfs:subClassOf rdf:resource="http://www.semanticweb.org/tswheeler/ontologies/2016/3/EmpowerBP#COMBConstruct"/>
        <rdfs:comment>Motivation may be ‘reflective’ (involving self-conscious planning and evaluations (beliefs about what is good or bad) or ‘automatic’ (processes involving wants and needs, desires, impulses and reflex responses).</rdfs:comment>
    </owl:Class>
    


    <!-- http://www.semanticweb.org/tswheeler/ontologies/2016/3/EmpowerBP#Obstacle -->

    <owl:Class rdf:about="http://www.semanticweb.org/tswheeler/ontologies/2016/3/EmpowerBP#Obstacle">
        <rdfs:comment>A common barrier to an InterventionGoal. Can be resolved with ObstacleTip.</rdfs:comment>
    </owl:Class>
    


    <!-- http://www.semanticweb.org/tswheeler/ontologies/2016/3/EmpowerBP#ObstacleTip -->

    <owl:Class rdf:about="http://www.semanticweb.org/tswheeler/ontologies/2016/3/EmpowerBP#ObstacleTip">
        <rdfs:subClassOf rdf:resource="http://www.semanticweb.org/tswheeler/ontologies/2016/3/EmpowerBP#Tip"/>
        <rdfs:comment>A Tip intended to address a particular Obstacle.</rdfs:comment>
    </owl:Class>
    


    <!-- http://www.semanticweb.org/tswheeler/ontologies/2016/3/EmpowerBP#Opportunity -->

    <owl:Class rdf:about="http://www.semanticweb.org/tswheeler/ontologies/2016/3/EmpowerBP#Opportunity">
        <rdfs:subClassOf rdf:resource="http://www.semanticweb.org/tswheeler/ontologies/2016/3/EmpowerBP#COMBConstruct"/>
        <rdfs:comment>Opportunity can be ‘physical’ (what the environment allows or facilitates in terms of time, triggers, resources, locations, physical barriers, etc.) or ‘social’ (including interpersonal influences, social cues and cultural norms).</rdfs:comment>
    </owl:Class>
    


    <!-- http://www.semanticweb.org/tswheeler/ontologies/2016/3/EmpowerBP#Patient -->

    <owl:Class rdf:about="http://www.semanticweb.org/tswheeler/ontologies/2016/3/EmpowerBP#Patient">
        <rdfs:subClassOf rdf:resource="http://www.semanticweb.org/tswheeler/ontologies/2016/3/EmpowerBP#Actor"/>
        <rdfs:comment>The individual who is the focus of the intervention.</rdfs:comment>
    </owl:Class>
    


    <!-- http://www.semanticweb.org/tswheeler/ontologies/2016/3/EmpowerBP#PhysicalCapabilityAssessment -->

    <owl:Class rdf:about="http://www.semanticweb.org/tswheeler/ontologies/2016/3/EmpowerBP#PhysicalCapabilityAssessment">
        <rdfs:subClassOf rdf:resource="http://www.semanticweb.org/tswheeler/ontologies/2016/3/EmpowerBP#COMBAssessment"/>
        <rdfs:comment>A tool to evaluate a Patient&apos;s physical capability with respect to a specific InterventionGoal.</rdfs:comment>
    </owl:Class>
    


    <!-- http://www.semanticweb.org/tswheeler/ontologies/2016/3/EmpowerBP#PhysicalOpportunityAssessment -->

    <owl:Class rdf:about="http://www.semanticweb.org/tswheeler/ontologies/2016/3/EmpowerBP#PhysicalOpportunityAssessment">
        <rdfs:subClassOf rdf:resource="http://www.semanticweb.org/tswheeler/ontologies/2016/3/EmpowerBP#COMBAssessment"/>
        <rdfs:comment>A tool to evaluate a Patient&apos;s physical opportunity with respect to a specific InterventionGoal.</rdfs:comment>
    </owl:Class>
    


    <!-- http://www.semanticweb.org/tswheeler/ontologies/2016/3/EmpowerBP#PsychologicalCapabilityAssessment -->

    <owl:Class rdf:about="http://www.semanticweb.org/tswheeler/ontologies/2016/3/EmpowerBP#PsychologicalCapabilityAssessment">
        <rdfs:subClassOf rdf:resource="http://www.semanticweb.org/tswheeler/ontologies/2016/3/EmpowerBP#COMBAssessment"/>
        <rdfs:comment>A tool to evaluate a Patient&apos;s psychologial capability with respect to a specific InterventionGoal.</rdfs:comment>
    </owl:Class>
    


    <!-- http://www.semanticweb.org/tswheeler/ontologies/2016/3/EmpowerBP#ReflectiveMotivationAssessment -->

    <owl:Class rdf:about="http://www.semanticweb.org/tswheeler/ontologies/2016/3/EmpowerBP#ReflectiveMotivationAssessment">
        <rdfs:subClassOf rdf:resource="http://www.semanticweb.org/tswheeler/ontologies/2016/3/EmpowerBP#COMBAssessment"/>
        <rdfs:comment>A tool to evaluate a Patient&apos;s reflective motivation with respect to a specific InterventionGoal.</rdfs:comment>
    </owl:Class>
    


    <!-- http://www.semanticweb.org/tswheeler/ontologies/2016/3/EmpowerBP#Resource -->

    <owl:Class rdf:about="http://www.semanticweb.org/tswheeler/ontologies/2016/3/EmpowerBP#Resource">
        <rdfs:subClassOf rdf:resource="http://www.semanticweb.org/tswheeler/ontologies/2016/3/EmpowerBP#InterventionItem"/>
        <rdfs:comment>Matrial that can be provided to a patient as part of an intervention.</rdfs:comment>
    </owl:Class>
    


    <!-- http://www.semanticweb.org/tswheeler/ontologies/2016/3/EmpowerBP#ShapeableGoal -->

    <owl:Class rdf:about="http://www.semanticweb.org/tswheeler/ontologies/2016/3/EmpowerBP#ShapeableGoal">
        <rdfs:subClassOf rdf:resource="http://www.semanticweb.org/tswheeler/ontologies/2016/3/EmpowerBP#InterventionGoal"/>
    </owl:Class>
    


    <!-- http://www.semanticweb.org/tswheeler/ontologies/2016/3/EmpowerBP#SocialOpportunityAssessment -->

    <owl:Class rdf:about="http://www.semanticweb.org/tswheeler/ontologies/2016/3/EmpowerBP#SocialOpportunityAssessment">
        <rdfs:subClassOf rdf:resource="http://www.semanticweb.org/tswheeler/ontologies/2016/3/EmpowerBP#COMBAssessment"/>
        <rdfs:comment>A tool to evaluate a Patient&apos;s social opportunity with respect to a specific InterventionGoal.</rdfs:comment>
    </owl:Class>
    


    <!-- http://www.semanticweb.org/tswheeler/ontologies/2016/3/EmpowerBP#TDFDomain -->

    <owl:Class rdf:about="http://www.semanticweb.org/tswheeler/ontologies/2016/3/EmpowerBP#TDFDomain">
        <rdfs:subClassOf rdf:resource="http://www.semanticweb.org/tswheeler/ontologies/2016/3/EmpowerBP#Construct"/>
        <rdfs:comment>Key theoretical constructs used in relevant theories as developed in a collaboration between psychologists and implementation researchers.</rdfs:comment>
    </owl:Class>
    


    <!-- http://www.semanticweb.org/tswheeler/ontologies/2016/3/EmpowerBP#Task -->

    <owl:Class rdf:about="http://www.semanticweb.org/tswheeler/ontologies/2016/3/EmpowerBP#Task">
        <rdfs:subClassOf rdf:resource="http://www.semanticweb.org/tswheeler/ontologies/2016/3/EmpowerBP#InterventionItem"/>
        <rdfs:comment>An action intended to be done by the patient, based on a BCT and promote a specific InterventionGoal</rdfs:comment>
    </owl:Class>
    


    <!-- http://www.semanticweb.org/tswheeler/ontologies/2016/3/EmpowerBP#Theory -->

    <owl:Class rdf:about="http://www.semanticweb.org/tswheeler/ontologies/2016/3/EmpowerBP#Theory"/>
    


    <!-- http://www.semanticweb.org/tswheeler/ontologies/2016/3/EmpowerBP#Tip -->

    <owl:Class rdf:about="http://www.semanticweb.org/tswheeler/ontologies/2016/3/EmpowerBP#Tip">
        <rdfs:subClassOf rdf:resource="http://www.semanticweb.org/tswheeler/ontologies/2016/3/EmpowerBP#InterventionItem"/>
        <rdfs:comment>A message delivered as part of an intervention.</rdfs:comment>
    </owl:Class>
    


    <!-- 
    ///////////////////////////////////////////////////////////////////////////////////////
    //
    // Individuals
    //
    ///////////////////////////////////////////////////////////////////////////////////////
     -->

    


    <!-- http://purl.bioontology.org/ontology/BCTT#Action_planning -->

    <owl:NamedIndividual rdf:about="http://purl.bioontology.org/ontology/BCTT#Action_planning">
        <rdf:type rdf:resource="http://purl.bioontology.org/ontology/BCTT#BehaviourChangeTechnique"/>
        <rdf:type rdf:resource="http://purl.bioontology.org/ontology/BCTT#00219"/>
        <EmpowerBP:isMostAppropriateForInterventionFunction rdf:resource="http://www.semanticweb.org/tswheeler/ontologies/2016/3/EmpowerBP#Enablement"/>
        <rdfs:comment>Examples:

Encourage a plan to carry condoms when going out socially at weekends
Prompt planning the performance of a particular physical activity (e.g. running) at a particular time (e.g. before work) on certain days of the week</rdfs:comment>
        <rdfs:comment>Prompt detailed planning of performance of the behaviour (must include at least one of context, frequency, duration and intensity). Context may be environmental (physical or social) or internal (physical, emotional or cognitive) (includes &apos;Implementation Intentions&apos;) 

Note: evidence of action planning does not necessarily imply goal setting, only code latter if sufficient evidence</rdfs:comment>
        <rdfs:label>Action planning</rdfs:label>
    </owl:NamedIndividual>
    


    <!-- http://purl.bioontology.org/ontology/BCTT#Adding_objects_to_the_environment -->

    <owl:NamedIndividual rdf:about="http://purl.bioontology.org/ontology/BCTT#Adding_objects_to_the_environment">
        <rdf:type rdf:resource="http://purl.bioontology.org/ontology/BCTT#BehaviourChangeTechnique"/>
        <rdf:type rdf:resource="http://purl.bioontology.org/ontology/BCTT#00295"/>
        <EmpowerBP:isMostAppropriateForInterventionFunction rdf:resource="http://www.semanticweb.org/tswheeler/ontologies/2016/3/EmpowerBP#Enablement"/>
        <EmpowerBP:isMostAppropriateForInterventionFunction rdf:resource="http://www.semanticweb.org/tswheeler/ontologies/2016/3/EmpowerBP#EnvironmentalRestructuring"/>
        <rdfs:comment>Add objects to the environment in order to facilitate performance of the behavior 

Note: Provision of information (e.g. written, verbal, visual) in a booklet or leaflet is insufficient. If this is accompanied by social support, also code 3.2, Social support (practical); if the environment is changed beyond the addition of objects, also code 12.1, Restructuring the physical environment</rdfs:comment>
        <rdfs:comment>Examples:

Provide free condoms to facilitate safe sex
Provide attractive toothbrush to improve tooth brushing technique</rdfs:comment>
        <rdfs:label>Adding objects to the environment</rdfs:label>
    </owl:NamedIndividual>
    


    <!-- http://purl.bioontology.org/ontology/BCTT#Anticipated_regret -->

    <owl:NamedIndividual rdf:about="http://purl.bioontology.org/ontology/BCTT#Anticipated_regret">
        <rdf:type rdf:resource="http://purl.bioontology.org/ontology/BCTT#BehaviourChangeTechnique"/>
        <rdf:type rdf:resource="http://purl.bioontology.org/ontology/BCTT#00246"/>
        <EmpowerBP:isAppropriateForInterventionFunciton rdf:resource="http://www.semanticweb.org/tswheeler/ontologies/2016/3/EmpowerBP#Coercion"/>
        <EmpowerBP:isAppropriateForInterventionFunciton rdf:resource="http://www.semanticweb.org/tswheeler/ontologies/2016/3/EmpowerBP#Enablement"/>
        <rdfs:comment>Examples:

Ask the person to assess the degree of regret they will feel if they do not quit smoking</rdfs:comment>
        <rdfs:comment>Induce or raise awareness of expectations of future regret about performance of the unwanted behavior

Note: not including 5.6, Information aboutemotionalconsequences; if suggests adoption of a perspective or new perspective in order to change cognitions also code 13.2, Framing/reframing</rdfs:comment>
        <rdfs:label>Anticipated regret</rdfs:label>
    </owl:NamedIndividual>
    


    <!-- http://purl.bioontology.org/ontology/BCTT#Associative_learning -->

    <owl:NamedIndividual rdf:about="http://purl.bioontology.org/ontology/BCTT#Associative_learning">
        <rdf:type rdf:resource="http://purl.bioontology.org/ontology/BCTT#BehaviourChangeTechnique"/>
        <rdf:type rdf:resource="http://purl.bioontology.org/ontology/BCTT#00257"/>
        <EmpowerBP:isAppropriateForInterventionFunciton rdf:resource="http://www.semanticweb.org/tswheeler/ontologies/2016/3/EmpowerBP#EnvironmentalRestructuring"/>
        <rdfs:comment>Examples:

Present repeatedly fatty foods with a disliked sauce to discourage the consumption of fatty foods</rdfs:comment>
        <rdfs:comment>Present a neutral stimulus jointly with a stimulus that already elicits the behavior repeatedly until the neutral stimulus elicits that behavior (includes ‘Classical/Pavlovian Conditioning’)

Note: when a BCT involves reward or punishment, code one or more of: 10.2, Material reward (behavior); 10.3, Non- specific reward; 10.4, Social reward, 10.9, Self-reward; 10.10, Reward (outcome)</rdfs:comment>
        <rdfs:label>Associative learning</rdfs:label>
    </owl:NamedIndividual>
    


    <!-- http://purl.bioontology.org/ontology/BCTT#Avoidance-reducing_exposure_to_cues_for_the_behavior -->

    <owl:NamedIndividual rdf:about="http://purl.bioontology.org/ontology/BCTT#Avoidance-reducing_exposure_to_cues_for_the_behavior">
        <rdf:type rdf:resource="http://purl.bioontology.org/ontology/BCTT#BehaviourChangeTechnique"/>
        <rdf:type rdf:resource="http://purl.bioontology.org/ontology/BCTT#00295"/>
        <EmpowerBP:isAppropriateForInterventionFunciton rdf:resource="http://www.semanticweb.org/tswheeler/ontologies/2016/3/EmpowerBP#Enablement"/>
        <rdfs:comment>Advise on how to avoid exposure to specific social and contextual/physical cues for the behavior, including changing daily or weekly routines

Note: this may also involve 12.1, Restructuring the physical environment and/or 12.2, Restructuring the social environment; if the BCT includes analysing the behavioral problem, only code 1.2, Problem solving</rdfs:comment>
        <rdfs:comment>Examples:

Suggest to a person who wants to quit smoking that their social life focus on activities other than pubs and bars which have been associated with smoking</rdfs:comment>
        <rdfs:label>Avoidance-reducing exposure to cues for the behavior</rdfs:label>
    </owl:NamedIndividual>
    


    <!-- http://purl.bioontology.org/ontology/BCTT#Behavior_cost -->

    <owl:NamedIndividual rdf:about="http://purl.bioontology.org/ontology/BCTT#Behavior_cost">
        <rdf:type rdf:resource="http://purl.bioontology.org/ontology/BCTT#BehaviourChangeTechnique"/>
        <rdf:type rdf:resource="http://purl.bioontology.org/ontology/BCTT#00308"/>
        <EmpowerBP:isAppropriateForInterventionFunciton rdf:resource="http://www.semanticweb.org/tswheeler/ontologies/2016/3/EmpowerBP#Coercion"/>
        <rdfs:comment>Arrange for withdrawal of something valued if and only if an unwanted behavior is performed (includes ‘Response cost’). 

Note if withdrawal of contingent reward code, 14.3, Remove reward</rdfs:comment>
        <rdfs:comment>Examples:

Subtract money from a prepaid refundable deposit when a cigarette is smoked</rdfs:comment>
        <rdfs:label>Behavior cost</rdfs:label>
    </owl:NamedIndividual>
    


    <!-- http://purl.bioontology.org/ontology/BCTT#Behavior_substitution -->

    <owl:NamedIndividual rdf:about="http://purl.bioontology.org/ontology/BCTT#Behavior_substitution">
        <rdf:type rdf:resource="http://purl.bioontology.org/ontology/BCTT#BehaviourChangeTechnique"/>
        <rdf:type rdf:resource="http://purl.bioontology.org/ontology/BCTT#00266"/>
        <EmpowerBP:isAppropriateForInterventionFunciton rdf:resource="http://www.semanticweb.org/tswheeler/ontologies/2016/3/EmpowerBP#Enablement"/>
        <rdfs:comment>Examples:

Suggest that the person goes for a walk rather than watches television</rdfs:comment>
        <rdfs:comment>Prompt substitution of the unwanted behavior with a wanted or neutral behavior

Note: if this occurs regularly, also code 8.4, Habit reversal</rdfs:comment>
        <rdfs:label>Behavior substitution</rdfs:label>
    </owl:NamedIndividual>
    


    <!-- http://purl.bioontology.org/ontology/BCTT#Behavioral_contract -->

    <owl:NamedIndividual rdf:about="http://purl.bioontology.org/ontology/BCTT#Behavioral_contract">
        <rdf:type rdf:resource="http://purl.bioontology.org/ontology/BCTT#BehaviourChangeTechnique"/>
        <rdf:type rdf:resource="http://purl.bioontology.org/ontology/BCTT#00219"/>
        <EmpowerBP:isAppropriateForInterventionFunciton rdf:resource="http://www.semanticweb.org/tswheeler/ontologies/2016/3/EmpowerBP#Coercion"/>
        <EmpowerBP:isAppropriateForInterventionFunciton rdf:resource="http://www.semanticweb.org/tswheeler/ontologies/2016/3/EmpowerBP#Enablement"/>
        <EmpowerBP:isAppropriateForInterventionFunciton rdf:resource="http://www.semanticweb.org/tswheeler/ontologies/2016/3/EmpowerBP#Incentivisation"/>
        <rdfs:comment>Create a written specification of the behaviour to be performed, agreed by the person, and witnessed by another

Note: also code 1.1, Goal setting (behaviour)</rdfs:comment>
        <rdfs:comment>Examples:

Sign a contract with the person e.g. specifying that they will not drink alcohol for one week</rdfs:comment>
        <rdfs:label>Behavioral contract</rdfs:label>
    </owl:NamedIndividual>
    


    <!-- http://purl.bioontology.org/ontology/BCTT#Behavioral_experiments -->

    <owl:NamedIndividual rdf:about="http://purl.bioontology.org/ontology/BCTT#Behavioral_experiments">
        <rdf:type rdf:resource="http://purl.bioontology.org/ontology/BCTT#BehaviourChangeTechnique"/>
        <rdf:type rdf:resource="http://purl.bioontology.org/ontology/BCTT#00241"/>
        <EmpowerBP:isAppropriateForInterventionFunciton rdf:resource="http://www.semanticweb.org/tswheeler/ontologies/2016/3/EmpowerBP#Education"/>
        <EmpowerBP:isAppropriateForInterventionFunciton rdf:resource="http://www.semanticweb.org/tswheeler/ontologies/2016/3/EmpowerBP#Enablement"/>
        <EmpowerBP:isAppropriateForInterventionFunciton rdf:resource="http://www.semanticweb.org/tswheeler/ontologies/2016/3/EmpowerBP#Training"/>
        <rdfs:comment>Advise on how to identify and test hypotheses about the behaviour, its causes and consequences, by collecting and interpreting data</rdfs:comment>
        <rdfs:comment>Examples:

Ask a family physician to give evidence-based advice rather than prescribe antibiotics and to note whether the patients are grateful or annoyed</rdfs:comment>
        <rdfs:label>Behavioral experiments</rdfs:label>
    </owl:NamedIndividual>
    


    <!-- http://purl.bioontology.org/ontology/BCTT#Behavioral_practice-rehearsal -->

    <owl:NamedIndividual rdf:about="http://purl.bioontology.org/ontology/BCTT#Behavioral_practice-rehearsal">
        <rdf:type rdf:resource="http://purl.bioontology.org/ontology/BCTT#BehaviourChangeTechnique"/>
        <rdf:type rdf:resource="http://purl.bioontology.org/ontology/BCTT#00266"/>
        <EmpowerBP:isMostAppropriateForInterventionFunction rdf:resource="http://www.semanticweb.org/tswheeler/ontologies/2016/3/EmpowerBP#Training"/>
        <rdfs:comment>Examples:

Prompt asthma patients to practice measuring their peak flow in the nurse’s consulting room</rdfs:comment>
        <rdfs:comment>Prompt practice or rehearsal of the performance of the behavior one or more times in a context or at a time when the performance may not be necessary, in order to increase habit and skill

Note: if aiming to associate performance with the context, also code 8.3, Habit formation</rdfs:comment>
        <rdfs:label>Behavioral practice-rehearsal</rdfs:label>
    </owl:NamedIndividual>
    


    <!-- http://purl.bioontology.org/ontology/BCTT#Biofeedback -->

    <owl:NamedIndividual rdf:about="http://purl.bioontology.org/ontology/BCTT#Biofeedback">
        <rdf:type rdf:resource="http://purl.bioontology.org/ontology/BCTT#BehaviourChangeTechnique"/>
        <rdf:type rdf:resource="http://purl.bioontology.org/ontology/BCTT#00229"/>
        <EmpowerBP:isAppropriateForInterventionFunciton rdf:resource="http://www.semanticweb.org/tswheeler/ontologies/2016/3/EmpowerBP#Coercion"/>
        <EmpowerBP:isAppropriateForInterventionFunciton rdf:resource="http://www.semanticweb.org/tswheeler/ontologies/2016/3/EmpowerBP#Education"/>
        <EmpowerBP:isAppropriateForInterventionFunciton rdf:resource="http://www.semanticweb.org/tswheeler/ontologies/2016/3/EmpowerBP#Incentivisation"/>
        <EmpowerBP:isAppropriateForInterventionFunciton rdf:resource="http://www.semanticweb.org/tswheeler/ontologies/2016/3/EmpowerBP#Persuasion"/>
        <EmpowerBP:isAppropriateForInterventionFunciton rdf:resource="http://www.semanticweb.org/tswheeler/ontologies/2016/3/EmpowerBP#Training"/>
        <rdfs:comment>Examples:

Inform the person of their blood pressure reading to improve adoption of health behaviors</rdfs:comment>
        <rdfs:comment>Provide feedback about the body (e.g. physiological or biochemical state) using an external monitoring device as part of a behaviour change strategy 

Note: if Biofeedback, code only 2.6, Biofeedback and not 2.2, Feedback on behaviour or 2.7, Feedback on outcome(s) of behaviour</rdfs:comment>
        <rdfs:label>Biofeedback</rdfs:label>
    </owl:NamedIndividual>
    


    <!-- http://purl.bioontology.org/ontology/BCTT#Body_changes -->

    <owl:NamedIndividual rdf:about="http://purl.bioontology.org/ontology/BCTT#Body_changes">
        <rdf:type rdf:resource="http://purl.bioontology.org/ontology/BCTT#BehaviourChangeTechnique"/>
        <rdf:type rdf:resource="http://purl.bioontology.org/ontology/BCTT#00295"/>
        <EmpowerBP:isAppropriateForInterventionFunciton rdf:resource="http://www.semanticweb.org/tswheeler/ontologies/2016/3/EmpowerBP#Enablement"/>
        <rdfs:comment>Alter body structure, functioning or support directly to facilitate behavior change</rdfs:comment>
        <rdfs:comment>Examples:

Prompt strength training, relaxation training or provide assistive aids (e.g. a hearing aid)</rdfs:comment>
        <rdfs:label>Body changes</rdfs:label>
    </owl:NamedIndividual>
    


    <!-- http://purl.bioontology.org/ontology/BCTT#Commitment -->

    <owl:NamedIndividual rdf:about="http://purl.bioontology.org/ontology/BCTT#Commitment">
        <rdf:type rdf:resource="http://purl.bioontology.org/ontology/BCTT#BehaviourChangeTechnique"/>
        <rdf:type rdf:resource="http://purl.bioontology.org/ontology/BCTT#00219"/>
        <EmpowerBP:isAppropriateForInterventionFunciton rdf:resource="http://www.semanticweb.org/tswheeler/ontologies/2016/3/EmpowerBP#Coercion"/>
        <EmpowerBP:isAppropriateForInterventionFunciton rdf:resource="http://www.semanticweb.org/tswheeler/ontologies/2016/3/EmpowerBP#Enablement"/>
        <EmpowerBP:isAppropriateForInterventionFunciton rdf:resource="http://www.semanticweb.org/tswheeler/ontologies/2016/3/EmpowerBP#Incentivisation"/>
        <rdfs:comment>Ask the person to affirm or reaffirm statements indicating commitment to change the behaviour

Note: if defined in terms of the behaviour to be achieved also code 1.1, Goal setting (behaviour)</rdfs:comment>
        <rdfs:comment>Examples:

Ask the person to use an “I will” statement to affirm or reaffirm a strong commitment (i.e. using the words “strongly”, “committed” or “high priority”) to start, continue or restart the attempt to take medication as prescribed</rdfs:comment>
        <rdfs:label>Commitment</rdfs:label>
    </owl:NamedIndividual>
    


    <!-- http://purl.bioontology.org/ontology/BCTT#Comparative_imagining_of_future_outcomes -->

    <owl:NamedIndividual rdf:about="http://purl.bioontology.org/ontology/BCTT#Comparative_imagining_of_future_outcomes">
        <rdf:type rdf:resource="http://purl.bioontology.org/ontology/BCTT#BehaviourChangeTechnique"/>
        <rdf:type rdf:resource="http://purl.bioontology.org/ontology/BCTT#00274"/>
        <EmpowerBP:isAppropriateForInterventionFunciton rdf:resource="http://www.semanticweb.org/tswheeler/ontologies/2016/3/EmpowerBP#Enablement"/>
        <rdfs:comment>Examples:

Prompt the person to imagine and compare likely or possible outcomes following attending versus not attending a screening appointment</rdfs:comment>
        <rdfs:comment>Prompt or advise the imagining and comparing of future outcomes of changed versus unchanged behaviour</rdfs:comment>
        <rdfs:label>Comparative imagining of future outcomes</rdfs:label>
    </owl:NamedIndividual>
    


    <!-- http://purl.bioontology.org/ontology/BCTT#Conserving_mental_resources -->

    <owl:NamedIndividual rdf:about="http://purl.bioontology.org/ontology/BCTT#Conserving_mental_resources">
        <rdf:type rdf:resource="http://purl.bioontology.org/ontology/BCTT#BehaviourChangeTechnique"/>
        <rdf:type rdf:resource="http://purl.bioontology.org/ontology/BCTT#00290"/>
        <EmpowerBP:isAppropriateForInterventionFunciton rdf:resource="http://www.semanticweb.org/tswheeler/ontologies/2016/3/EmpowerBP#Enablement"/>
        <rdfs:comment>Advise on ways of minimising demands on mental resources to facilitate behavior change</rdfs:comment>
        <rdfs:comment>Examples:

Advise to carry food calorie content information to reduce the burden on memory in making food choices</rdfs:comment>
        <rdfs:label>Conserving mental resources</rdfs:label>
    </owl:NamedIndividual>
    


    <!-- http://purl.bioontology.org/ontology/BCTT#Credible_source -->

    <owl:NamedIndividual rdf:about="http://purl.bioontology.org/ontology/BCTT#Credible_source">
        <rdf:type rdf:resource="http://purl.bioontology.org/ontology/BCTT#BehaviourChangeTechnique"/>
        <rdf:type rdf:resource="http://purl.bioontology.org/ontology/BCTT#00274"/>
        <EmpowerBP:isMostAppropriateForInterventionFunction rdf:resource="http://www.semanticweb.org/tswheeler/ontologies/2016/3/EmpowerBP#Persuasion"/>
        <rdfs:comment>Examples:

Present a speech given by a high status professional to emphasise the importance of not exposing patients to unnecessary radiation by ordering x-rays for back pain</rdfs:comment>
        <rdfs:comment>Present verbal or visual communication from a credible source in favour of or against the behavior

Note: code this BCT if source generally agreed on as credible e.g., health professionals, celebrities or words used to indicate expertise or leader in field and if the communication has the aim of persuading; if information about health consequences, also code 5.1, Information about health consequences, if about emotional consequences, also code 5.6, Information about emotional consequences; if about social, environmental or unspecified consequences also code 5.3, Information about social and environmental consequences</rdfs:comment>
        <rdfs:label>Credible source</rdfs:label>
    </owl:NamedIndividual>
    


    <!-- http://purl.bioontology.org/ontology/BCTT#Cue_signalling_reward -->

    <owl:NamedIndividual rdf:about="http://purl.bioontology.org/ontology/BCTT#Cue_signalling_reward">
        <rdf:type rdf:resource="http://purl.bioontology.org/ontology/BCTT#BehaviourChangeTechnique"/>
        <rdf:type rdf:resource="http://purl.bioontology.org/ontology/BCTT#00257"/>
        <EmpowerBP:isAppropriateForInterventionFunciton rdf:resource="http://www.semanticweb.org/tswheeler/ontologies/2016/3/EmpowerBP#Education"/>
        <EmpowerBP:isAppropriateForInterventionFunciton rdf:resource="http://www.semanticweb.org/tswheeler/ontologies/2016/3/EmpowerBP#EnvironmentalRestructuring"/>
        <EmpowerBP:isAppropriateForInterventionFunciton rdf:resource="http://www.semanticweb.org/tswheeler/ontologies/2016/3/EmpowerBP#Incentivisation"/>
        <rdfs:comment>Examples:

Advise that a fee will be paid to dentists for a particular dental treatment of 6-8 year old, but not older, children to encourage delivery of that treatment (the 6- 8 year old children are the environmental stimulus)</rdfs:comment>
        <rdfs:comment>Identify an environmental stimulus that reliably predicts that reward will follow the behavior (includes ‘Discriminative cue’)</rdfs:comment>
        <rdfs:label>Cue signalling reward</rdfs:label>
    </owl:NamedIndividual>
    


    <!-- http://purl.bioontology.org/ontology/BCTT#Demonstration_of_the_behavior -->

    <owl:NamedIndividual rdf:about="http://purl.bioontology.org/ontology/BCTT#Demonstration_of_the_behavior">
        <rdf:type rdf:resource="http://purl.bioontology.org/ontology/BCTT#BehaviourChangeTechnique"/>
        <rdf:type rdf:resource="http://purl.bioontology.org/ontology/BCTT#00253"/>
        <EmpowerBP:isMostAppropriateForInterventionFunction rdf:resource="http://www.semanticweb.org/tswheeler/ontologies/2016/3/EmpowerBP#Modelling"/>
        <EmpowerBP:isMostAppropriateForInterventionFunction rdf:resource="http://www.semanticweb.org/tswheeler/ontologies/2016/3/EmpowerBP#Training"/>
        <rdfs:comment>Examples: 

Demonstrate to nurses how to raise the issue of excessive drinking with patients via a role- play exercise</rdfs:comment>
        <rdfs:comment>Provide an observable sample of the performance of the behaviour, directly in person or indirectly e.g. via film, pictures, for the person to aspire to or imitate (includes ‘Modelling’). 

Note: if advised to practice, also code, 8.1, Behavioural practice and rehearsal; If provided with instructions on how to perform, also code 4.1, Instruction on how to perform the behaviour</rdfs:comment>
        <rdfs:label>Demonstration of the behavior</rdfs:label>
    </owl:NamedIndividual>
    


    <!-- http://purl.bioontology.org/ontology/BCTT#Discrepancy_between_current_behavior_and_goal -->

    <owl:NamedIndividual rdf:about="http://purl.bioontology.org/ontology/BCTT#Discrepancy_between_current_behavior_and_goal">
        <rdf:type rdf:resource="http://purl.bioontology.org/ontology/BCTT#BehaviourChangeTechnique"/>
        <rdf:type rdf:resource="http://purl.bioontology.org/ontology/BCTT#00219"/>
        <EmpowerBP:isAppropriateForInterventionFunciton rdf:resource="http://www.semanticweb.org/tswheeler/ontologies/2016/3/EmpowerBP#Coercion"/>
        <EmpowerBP:isAppropriateForInterventionFunciton rdf:resource="http://www.semanticweb.org/tswheeler/ontologies/2016/3/EmpowerBP#Enablement"/>
        <EmpowerBP:isAppropriateForInterventionFunciton rdf:resource="http://www.semanticweb.org/tswheeler/ontologies/2016/3/EmpowerBP#Incentivisation"/>
        <rdfs:comment>Draw attention to discrepancies between a person&apos;s current behaviour (in terms of the form, frequency, duration, or intensity of that behaviour) and the person&apos;s previously set outcome goals, behavioural goals or action plans (goes beyond self-monitoring of behaviour)
 
Note: if discomfort is created only code 13.3, Incompatible beliefs and not 1.6, Discrepancy between current behaviour and goal; if goals are modified, also code 1.5, Review behaviour goal(s) and/or 1.7, Review outcome goal(s); if feedback is provided, also code 2.2, Feedback on behaviour</rdfs:comment>
        <rdfs:comment>Examples:

Point out that the recorded exercise fell short of the goal set</rdfs:comment>
        <rdfs:label>Discrepancy between current behavior and goal</rdfs:label>
    </owl:NamedIndividual>
    


    <!-- http://purl.bioontology.org/ontology/BCTT#Distraction -->

    <owl:NamedIndividual rdf:about="http://purl.bioontology.org/ontology/BCTT#Distraction">
        <rdf:type rdf:resource="http://purl.bioontology.org/ontology/BCTT#BehaviourChangeTechnique"/>
        <rdf:type rdf:resource="http://purl.bioontology.org/ontology/BCTT#00295"/>
        <EmpowerBP:isAppropriateForInterventionFunciton rdf:resource="http://www.semanticweb.org/tswheeler/ontologies/2016/3/EmpowerBP#Enablement"/>
        <rdfs:comment>Advise or arrange to use an alternative focus for attention to avoid triggers for unwanted behaviour</rdfs:comment>
        <rdfs:comment>Examples:

Suggest to a person who is trying to avoid between-meal snacking to focus on a topic they enjoy (e.g. holiday plans) instead of focusing on food</rdfs:comment>
        <rdfs:label>Distraction</rdfs:label>
    </owl:NamedIndividual>
    


    <!-- http://purl.bioontology.org/ontology/BCTT#Exposure -->

    <owl:NamedIndividual rdf:about="http://purl.bioontology.org/ontology/BCTT#Exposure">
        <rdf:type rdf:resource="http://purl.bioontology.org/ontology/BCTT#BehaviourChangeTechnique"/>
        <rdf:type rdf:resource="http://purl.bioontology.org/ontology/BCTT#00257"/>
        <EmpowerBP:isAppropriateForInterventionFunciton rdf:resource="http://www.semanticweb.org/tswheeler/ontologies/2016/3/EmpowerBP#EnvironmentalRestructuring"/>
        <rdfs:comment>Examples:

Agree a schedule by which the person who is frightened of surgery will visit the hospital where they are scheduled to have surgery</rdfs:comment>
        <rdfs:comment>Provide systematic confrontation with a feared stimulus to reduce the response to a later encounter</rdfs:comment>
        <rdfs:label>Exposure</rdfs:label>
    </owl:NamedIndividual>
    


    <!-- http://purl.bioontology.org/ontology/BCTT#Feedback_on_behaviour -->

    <owl:NamedIndividual rdf:about="http://purl.bioontology.org/ontology/BCTT#Feedback_on_behaviour">
        <rdf:type rdf:resource="http://purl.bioontology.org/ontology/BCTT#BehaviourChangeTechnique"/>
        <rdf:type rdf:resource="http://purl.bioontology.org/ontology/BCTT#00229"/>
        <EmpowerBP:isMostAppropriateForInterventionFunction rdf:resource="http://www.semanticweb.org/tswheeler/ontologies/2016/3/EmpowerBP#Coercion"/>
        <EmpowerBP:isMostAppropriateForInterventionFunction rdf:resource="http://www.semanticweb.org/tswheeler/ontologies/2016/3/EmpowerBP#Education"/>
        <EmpowerBP:isMostAppropriateForInterventionFunction rdf:resource="http://www.semanticweb.org/tswheeler/ontologies/2016/3/EmpowerBP#Incentivisation"/>
        <EmpowerBP:isMostAppropriateForInterventionFunction rdf:resource="http://www.semanticweb.org/tswheeler/ontologies/2016/3/EmpowerBP#Persuasion"/>
        <EmpowerBP:isMostAppropriateForInterventionFunction rdf:resource="http://www.semanticweb.org/tswheeler/ontologies/2016/3/EmpowerBP#Training"/>
        <rdfs:comment>Examples:

Inform the person of how many steps they walked each day (as recorded on a pedometer) or how many calories they ate each day (based on a food consumption questionnaire).</rdfs:comment>
        <rdfs:comment>Monitor and provide informative or evaluative feedback on performance of the behaviour (e.g. form, frequency, duration, intensity)

Note: if Biofeedback, code only 2.6, Biofeedback and not 2.2, Feedback on behaviour; if feedback is on outcome(s) of behaviour, code 2.7, Feedback on outcome(s) of behaviour; if there is no clear evidence that feedback was given, code 2.1, Monitoring of behaviour by others without feedback; if feedback on behaviour is evaluative e.g. praise, also code 10.4, Social reward</rdfs:comment>
        <rdfs:label>Feedback on behaviour</rdfs:label>
    </owl:NamedIndividual>
    


    <!-- http://purl.bioontology.org/ontology/BCTT#Focus_on_past_success -->

    <owl:NamedIndividual rdf:about="http://purl.bioontology.org/ontology/BCTT#Focus_on_past_success">
        <rdf:type rdf:resource="http://purl.bioontology.org/ontology/BCTT#BehaviourChangeTechnique"/>
        <rdf:type rdf:resource="http://purl.bioontology.org/ontology/BCTT#00319"/>
        <EmpowerBP:isAppropriateForInterventionFunciton rdf:resource="http://www.semanticweb.org/tswheeler/ontologies/2016/3/EmpowerBP#Enablement"/>
        <EmpowerBP:isAppropriateForInterventionFunciton rdf:resource="http://www.semanticweb.org/tswheeler/ontologies/2016/3/EmpowerBP#Persuasion"/>
        <rdfs:comment>Advise to think about or list previous successes in performing the behavior (or parts of it)</rdfs:comment>
        <rdfs:comment>Examples:

Advise to describe or list the occasions on which the person had ordered a non-alcoholic drink in a bar</rdfs:comment>
        <rdfs:label>Focus on past success</rdfs:label>
    </owl:NamedIndividual>
    


    <!-- http://purl.bioontology.org/ontology/BCTT#Framing-reframing -->

    <owl:NamedIndividual rdf:about="http://purl.bioontology.org/ontology/BCTT#Framing-reframing">
        <rdf:type rdf:resource="http://purl.bioontology.org/ontology/BCTT#BehaviourChangeTechnique"/>
        <rdf:type rdf:resource="http://purl.bioontology.org/ontology/BCTT#00302"/>
        <EmpowerBP:isAppropriateForInterventionFunciton rdf:resource="http://www.semanticweb.org/tswheeler/ontologies/2016/3/EmpowerBP#Enablement"/>
        <EmpowerBP:isAppropriateForInterventionFunciton rdf:resource="http://www.semanticweb.org/tswheeler/ontologies/2016/3/EmpowerBP#Persuasion"/>
        <rdfs:comment>Examples:

Suggest that the person might think of the tasks as reducing sedentary behavior (rather than increasing activity)</rdfs:comment>
        <rdfs:comment>Suggest the deliberate adoption of a perspective or new perspective on behavior (e.g. its purpose) in order to change cognitions or emotions about performing the behavior (includes ‘Cognitive structuring’)

Note: If information about consequences then code 5.1, Information about health consequences, 5.6, Information about emotional consequences or 5.3, Information about social and environmental consequences instead of 13.2, Framing/reframing</rdfs:comment>
        <rdfs:label>Framing-reframing</rdfs:label>
    </owl:NamedIndividual>
    


    <!-- http://purl.bioontology.org/ontology/BCTT#Future_punishment -->

    <owl:NamedIndividual rdf:about="http://purl.bioontology.org/ontology/BCTT#Future_punishment">
        <rdf:type rdf:resource="http://purl.bioontology.org/ontology/BCTT#BehaviourChangeTechnique"/>
        <rdf:type rdf:resource="http://purl.bioontology.org/ontology/BCTT#00278"/>
        <EmpowerBP:isAppropriateForInterventionFunciton rdf:resource="http://www.semanticweb.org/tswheeler/ontologies/2016/3/EmpowerBP#Coercion"/>
        <rdfs:comment>Examples:

Inform that continuing to consume 30 units of alcohol per day is likely to result in loss of employment if the person continues</rdfs:comment>
        <rdfs:comment>Inform that future punishment or removal of reward will be a consequence of performance of an unwanted behavior (may include fear arousal) (includes ‘Threat’)</rdfs:comment>
        <rdfs:label>Future punishment</rdfs:label>
    </owl:NamedIndividual>
    


    <!-- http://purl.bioontology.org/ontology/BCTT#Generalisation_of_target_behavior -->

    <owl:NamedIndividual rdf:about="http://purl.bioontology.org/ontology/BCTT#Generalisation_of_target_behavior">
        <rdf:type rdf:resource="http://purl.bioontology.org/ontology/BCTT#BehaviourChangeTechnique"/>
        <rdf:type rdf:resource="http://purl.bioontology.org/ontology/BCTT#00266"/>
        <EmpowerBP:isAppropriateForInterventionFunciton rdf:resource="http://www.semanticweb.org/tswheeler/ontologies/2016/3/EmpowerBP#Enablement"/>
        <rdfs:comment>Advise to perform the wanted behaviour, which is already performed in a particular situation, in another situation</rdfs:comment>
        <rdfs:comment>Examples:

Advise to repeat toning exercises learned in the gym when at home</rdfs:comment>
        <rdfs:label>Generalisation of target behavior</rdfs:label>
    </owl:NamedIndividual>
    


    <!-- http://purl.bioontology.org/ontology/BCTT#Graded_tasks -->

    <owl:NamedIndividual rdf:about="http://purl.bioontology.org/ontology/BCTT#Graded_tasks">
        <rdf:type rdf:resource="http://purl.bioontology.org/ontology/BCTT#BehaviourChangeTechnique"/>
        <rdf:type rdf:resource="http://purl.bioontology.org/ontology/BCTT#00266"/>
        <EmpowerBP:isAppropriateForInterventionFunciton rdf:resource="http://www.semanticweb.org/tswheeler/ontologies/2016/3/EmpowerBP#Enablement"/>
        <EmpowerBP:isAppropriateForInterventionFunciton rdf:resource="http://www.semanticweb.org/tswheeler/ontologies/2016/3/EmpowerBP#Training"/>
        <rdfs:comment>Examples:

Ask the person to walk for 100 yards a day for the first week, then half a mile a day after they have successfully achieved 100 yards, then two miles a day after they have successfully achieved one mile</rdfs:comment>
        <rdfs:comment>Set easy-to-perform tasks, making them increasingly difficult, but achievable, until behavior is performed</rdfs:comment>
        <rdfs:label>Graded tasks</rdfs:label>
    </owl:NamedIndividual>
    


    <!-- http://purl.bioontology.org/ontology/BCTT#Habit_formation -->

    <owl:NamedIndividual rdf:about="http://purl.bioontology.org/ontology/BCTT#Habit_formation">
        <rdf:type rdf:resource="http://purl.bioontology.org/ontology/BCTT#BehaviourChangeTechnique"/>
        <rdf:type rdf:resource="http://purl.bioontology.org/ontology/BCTT#00266"/>
        <EmpowerBP:isAppropriateForInterventionFunciton rdf:resource="http://www.semanticweb.org/tswheeler/ontologies/2016/3/EmpowerBP#Training"/>
        <rdfs:comment>Examples:

Prompt patients to take their statin tablet before brushing their teeth every evening</rdfs:comment>
        <rdfs:comment>Prompt rehearsal and repetition of the behavior in the same context repeatedly so that the context elicits the behavior 

Note: also code 8.1, Behavioral practice/rehearsal</rdfs:comment>
        <rdfs:label>Habit formation</rdfs:label>
    </owl:NamedIndividual>
    


    <!-- http://purl.bioontology.org/ontology/BCTT#Habit_reversal -->

    <owl:NamedIndividual rdf:about="http://purl.bioontology.org/ontology/BCTT#Habit_reversal">
        <rdf:type rdf:resource="http://purl.bioontology.org/ontology/BCTT#BehaviourChangeTechnique"/>
        <rdf:type rdf:resource="http://purl.bioontology.org/ontology/BCTT#00266"/>
        <EmpowerBP:isAppropriateForInterventionFunciton rdf:resource="http://www.semanticweb.org/tswheeler/ontologies/2016/3/EmpowerBP#Training"/>
        <rdfs:comment>Examples:

Ask the person to walk up stairs at work where they previously always took the lift</rdfs:comment>
        <rdfs:comment>Prompt rehearsal and repetition of an alternative behavior to replace an unwanted habitual behavior

Note: also code 8.2, Behavior substitution</rdfs:comment>
        <rdfs:label>Habit reversal</rdfs:label>
    </owl:NamedIndividual>
    


    <!-- http://purl.bioontology.org/ontology/BCTT#Identification_of_self_as_role_model -->

    <owl:NamedIndividual rdf:about="http://purl.bioontology.org/ontology/BCTT#Identification_of_self_as_role_model">
        <rdf:type rdf:resource="http://purl.bioontology.org/ontology/BCTT#BehaviourChangeTechnique"/>
        <rdf:type rdf:resource="http://purl.bioontology.org/ontology/BCTT#00302"/>
        <EmpowerBP:isAppropriateForInterventionFunciton rdf:resource="http://www.semanticweb.org/tswheeler/ontologies/2016/3/EmpowerBP#Enablement"/>
        <EmpowerBP:isAppropriateForInterventionFunciton rdf:resource="http://www.semanticweb.org/tswheeler/ontologies/2016/3/EmpowerBP#Persuasion"/>
        <rdfs:comment>Examples:

Inform the person that if they eat healthily, that may be a good example for their children</rdfs:comment>
        <rdfs:comment>Inform that one&apos;s own behavior may be an example to others</rdfs:comment>
        <rdfs:label>Identification of self as role model</rdfs:label>
    </owl:NamedIndividual>
    


    <!-- http://purl.bioontology.org/ontology/BCTT#Identity_associated_with_changed_behavior -->

    <owl:NamedIndividual rdf:about="http://purl.bioontology.org/ontology/BCTT#Identity_associated_with_changed_behavior">
        <rdf:type rdf:resource="http://purl.bioontology.org/ontology/BCTT#BehaviourChangeTechnique"/>
        <rdf:type rdf:resource="http://purl.bioontology.org/ontology/BCTT#00302"/>
        <EmpowerBP:isAppropriateForInterventionFunciton rdf:resource="http://www.semanticweb.org/tswheeler/ontologies/2016/3/EmpowerBP#Enablement"/>
        <EmpowerBP:isAppropriateForInterventionFunciton rdf:resource="http://www.semanticweb.org/tswheeler/ontologies/2016/3/EmpowerBP#Persuasion"/>
        <rdfs:comment>Advise the person to construct a new self- identity as someone who ‘used to engage with the unwanted behavior’</rdfs:comment>
        <rdfs:comment>Examples:

Ask the person to articulate their new identity as an ‘ex-smoker’</rdfs:comment>
        <rdfs:label>Identity associated with changed behavior</rdfs:label>
    </owl:NamedIndividual>
    


    <!-- http://purl.bioontology.org/ontology/BCTT#Imaginary_punishment -->

    <owl:NamedIndividual rdf:about="http://purl.bioontology.org/ontology/BCTT#Imaginary_punishment">
        <rdf:type rdf:resource="http://purl.bioontology.org/ontology/BCTT#BehaviourChangeTechnique"/>
        <rdf:type rdf:resource="http://purl.bioontology.org/ontology/BCTT#00324"/>
        <EmpowerBP:isAppropriateForInterventionFunciton rdf:resource="http://www.semanticweb.org/tswheeler/ontologies/2016/3/EmpowerBP#Coercion"/>
        <EmpowerBP:isAppropriateForInterventionFunciton rdf:resource="http://www.semanticweb.org/tswheeler/ontologies/2016/3/EmpowerBP#Enablement"/>
        <rdfs:comment>Advise to imagine performing the unwanted behaviour in a real-life situation followed by imagining an unpleasant consequence (includes &apos;Covert  sensitisation&apos;)</rdfs:comment>
        <rdfs:comment>Examples:

Advise to imagine overeating and then vomiting</rdfs:comment>
        <rdfs:label>Imaginary punishment</rdfs:label>
    </owl:NamedIndividual>
    


    <!-- http://purl.bioontology.org/ontology/BCTT#Imaginary_reward -->

    <owl:NamedIndividual rdf:about="http://purl.bioontology.org/ontology/BCTT#Imaginary_reward">
        <rdf:type rdf:resource="http://purl.bioontology.org/ontology/BCTT#BehaviourChangeTechnique"/>
        <rdf:type rdf:resource="http://purl.bioontology.org/ontology/BCTT#00324"/>
        <EmpowerBP:isAppropriateForInterventionFunciton rdf:resource="http://www.semanticweb.org/tswheeler/ontologies/2016/3/EmpowerBP#Enablement"/>
        <EmpowerBP:isAppropriateForInterventionFunciton rdf:resource="http://www.semanticweb.org/tswheeler/ontologies/2016/3/EmpowerBP#Incentivisation"/>
        <rdfs:comment>Advise to imagine performing the wanted behaviour in a real-life situation followed by imagining a pleasant consequence (includes &apos;Covert conditioning&apos;)</rdfs:comment>
        <rdfs:comment>Examples:

Advise the health professional to imagine giving dietary advice followed by the patient losing weight and no longer being diabetic</rdfs:comment>
        <rdfs:label>Imaginary reward</rdfs:label>
    </owl:NamedIndividual>
    


    <!-- http://purl.bioontology.org/ontology/BCTT#Incompatible_beliefs -->

    <owl:NamedIndividual rdf:about="http://purl.bioontology.org/ontology/BCTT#Incompatible_beliefs">
        <rdf:type rdf:resource="http://purl.bioontology.org/ontology/BCTT#BehaviourChangeTechnique"/>
        <rdf:type rdf:resource="http://purl.bioontology.org/ontology/BCTT#00302"/>
        <EmpowerBP:isAppropriateForInterventionFunciton rdf:resource="http://www.semanticweb.org/tswheeler/ontologies/2016/3/EmpowerBP#Coercion"/>
        <EmpowerBP:isAppropriateForInterventionFunciton rdf:resource="http://www.semanticweb.org/tswheeler/ontologies/2016/3/EmpowerBP#Enablement"/>
        <rdfs:comment>Draw attention to discrepancies between current or past behavior and self-image, in order to create discomfort (includes ‘Cognitive dissonance’)</rdfs:comment>
        <rdfs:comment>Examples:

Draw attention to a doctor’s liberal use of blood transfusion and their self-identification as a proponent of evidence-based medical practice</rdfs:comment>
        <rdfs:label>Incompatible beliefs</rdfs:label>
    </owl:NamedIndividual>
    


    <!-- http://purl.bioontology.org/ontology/BCTT#Information_about_Antecedents -->

    <owl:NamedIndividual rdf:about="http://purl.bioontology.org/ontology/BCTT#Information_about_Antecedents">
        <rdf:type rdf:resource="http://purl.bioontology.org/ontology/BCTT#BehaviourChangeTechnique"/>
        <rdf:type rdf:resource="http://purl.bioontology.org/ontology/BCTT#00241"/>
        <EmpowerBP:isAppropriateForInterventionFunciton rdf:resource="http://www.semanticweb.org/tswheeler/ontologies/2016/3/EmpowerBP#Education"/>
        <rdfs:comment>Examples:

Advise to keep a record of snacking and of situations or events occurring prior to snacking</rdfs:comment>
        <rdfs:comment>Provide information about antecedents (e.g. social and environmental situations and events, emotions, cognitions) that reliably predict performance of the behaviour</rdfs:comment>
        <rdfs:label>Information about antecedents</rdfs:label>
    </owl:NamedIndividual>
    


    <!-- http://purl.bioontology.org/ontology/BCTT#Information_about_emotional_consequences -->

    <owl:NamedIndividual rdf:about="http://purl.bioontology.org/ontology/BCTT#Information_about_emotional_consequences">
        <rdf:type rdf:resource="http://purl.bioontology.org/ontology/BCTT#BehaviourChangeTechnique"/>
        <rdf:type rdf:resource="http://purl.bioontology.org/ontology/BCTT#00246"/>
        <EmpowerBP:isAppropriateForInterventionFunciton rdf:resource="http://www.semanticweb.org/tswheeler/ontologies/2016/3/EmpowerBP#Education"/>
        <EmpowerBP:isAppropriateForInterventionFunciton rdf:resource="http://www.semanticweb.org/tswheeler/ontologies/2016/3/EmpowerBP#Persuasion"/>
        <rdfs:comment>Examples:

Explain that quitting smoking increases happiness and life satisfaction</rdfs:comment>
        <rdfs:comment>Provide information (e.g. written, verbal, visual) about emotional consequences of performing the behavior

Note: consequences can be related to emotional health disorders (e.g. depression, anxiety) and/or states of mind (e.g. low mood, stress); not including 5.5, Anticipated regret; consequences can be for any target, not just the recipient(s) of the intervention; if information about health consequences code 5.1, Information about health consequences; if about social, environmental or unspecified code 5.3, Information about social and environmental consequences</rdfs:comment>
        <rdfs:label>Information about emotional consequences</rdfs:label>
    </owl:NamedIndividual>
    


    <!-- http://purl.bioontology.org/ontology/BCTT#Information_about_health_consequences -->

    <owl:NamedIndividual rdf:about="http://purl.bioontology.org/ontology/BCTT#Information_about_health_consequences">
        <rdf:type rdf:resource="http://purl.bioontology.org/ontology/BCTT#BehaviourChangeTechnique"/>
        <rdf:type rdf:resource="http://purl.bioontology.org/ontology/BCTT#00246"/>
        <EmpowerBP:isMostAppropriateForInterventionFunction rdf:resource="http://www.semanticweb.org/tswheeler/ontologies/2016/3/EmpowerBP#Education"/>
        <EmpowerBP:isMostAppropriateForInterventionFunction rdf:resource="http://www.semanticweb.org/tswheeler/ontologies/2016/3/EmpowerBP#Persuasion"/>
        <rdfs:comment>Examples:

Explain that not finishing a course of antibiotics can increase susceptibility to future infection
Present the likelihood of contracting a sexually transmitted infection following unprotected sexual behavior</rdfs:comment>
        <rdfs:comment>Provide information (e.g. written, verbal, visual) about health consequences of performing the behavior

Note: consequences can be for any target, not just the recipient(s) of the intervention; emphasising importance of consequences is not sufficient; if information about emotional consequences, code 5.6, Information about emotional consequences; if about social, environmental or unspecified consequences code 5.3, Information about social and environmental consequences</rdfs:comment>
        <rdfs:label>Information about health consequences</rdfs:label>
    </owl:NamedIndividual>
    


    <!-- http://purl.bioontology.org/ontology/BCTT#Information_about_social_and_environmental_consequences -->

    <owl:NamedIndividual rdf:about="http://purl.bioontology.org/ontology/BCTT#Information_about_social_and_environmental_consequences">
        <rdf:type rdf:resource="http://purl.bioontology.org/ontology/BCTT#BehaviourChangeTechnique"/>
        <rdf:type rdf:resource="http://purl.bioontology.org/ontology/BCTT#00246"/>
        <EmpowerBP:isMostAppropriateForInterventionFunction rdf:resource="http://www.semanticweb.org/tswheeler/ontologies/2016/3/EmpowerBP#Education"/>
        <EmpowerBP:isMostAppropriateForInterventionFunction rdf:resource="http://www.semanticweb.org/tswheeler/ontologies/2016/3/EmpowerBP#Persuasion"/>
        <rdfs:comment>Examples:

Tell family physician about financial remuneration for conducting health screening
Inform a smoker that the majority of people disapprove of smoking in public places</rdfs:comment>
        <rdfs:comment>Provide information (e.g. written, verbal, visual) about social and environmental consequences of performing the behavior 

Note: consequences can be for any target, not just the recipient(s) of the intervention; if information about health or consequences, code 5.1, Information about health consequences; if about emotional consequences, code 5.6, Information about emotional consequences; if unspecified, code 5.3, Information about social and environmental consequences</rdfs:comment>
        <rdfs:label>Information about social and environmental consequences</rdfs:label>
    </owl:NamedIndividual>
    


    <!-- http://purl.bioontology.org/ontology/BCTT#Instruction_on_how_to_perform_the_behavior -->

    <owl:NamedIndividual rdf:about="http://purl.bioontology.org/ontology/BCTT#Instruction_on_how_to_perform_the_behavior">
        <rdf:type rdf:resource="http://purl.bioontology.org/ontology/BCTT#BehaviourChangeTechnique"/>
        <rdf:type rdf:resource="http://purl.bioontology.org/ontology/BCTT#00241"/>
        <EmpowerBP:isMostAppropriateForInterventionFunction rdf:resource="http://www.semanticweb.org/tswheeler/ontologies/2016/3/EmpowerBP#Training"/>
        <rdfs:comment>Advise or agree on how to perform the behaviour (includes &apos;Skills training&apos;)

Note: when the person attends classes such as exercise or cookery, code 4.1, Instruction on how to perform the behaviour, 8.1, Behavioural practice/rehearsal and 6.1, Demonstration of the behaviour</rdfs:comment>
        <rdfs:comment>Examples:

Advise the person how to put a condom on a model of a penis correctly</rdfs:comment>
        <rdfs:label>Instruction on how to perform the behavior</rdfs:label>
    </owl:NamedIndividual>
    


    <!-- http://purl.bioontology.org/ontology/BCTT#Mental_rehearsal_of_successful_performance -->

    <owl:NamedIndividual rdf:about="http://purl.bioontology.org/ontology/BCTT#Mental_rehearsal_of_successful_performance">
        <rdf:type rdf:resource="http://purl.bioontology.org/ontology/BCTT#BehaviourChangeTechnique"/>
        <rdf:type rdf:resource="http://purl.bioontology.org/ontology/BCTT#00319"/>
        <EmpowerBP:isAppropriateForInterventionFunciton rdf:resource="http://www.semanticweb.org/tswheeler/ontologies/2016/3/EmpowerBP#Enablement"/>
        <EmpowerBP:isAppropriateForInterventionFunciton rdf:resource="http://www.semanticweb.org/tswheeler/ontologies/2016/3/EmpowerBP#Training"/>
        <rdfs:comment>Advise to practise imagining performing the behavior successfully in relevant contexts</rdfs:comment>
        <rdfs:comment>Examples:

Advise to imagine eating and enjoying a salad in a work canteen</rdfs:comment>
        <rdfs:label>Mental rehearsal of successful performance</rdfs:label>
    </owl:NamedIndividual>
    


    <!-- http://purl.bioontology.org/ontology/BCTT#Monitoring_of_behavior_by_others_without_feedback -->

    <owl:NamedIndividual rdf:about="http://purl.bioontology.org/ontology/BCTT#Monitoring_of_behavior_by_others_without_feedback">
        <rdf:type rdf:resource="http://purl.bioontology.org/ontology/BCTT#BehaviourChangeTechnique"/>
        <rdf:type rdf:resource="http://purl.bioontology.org/ontology/BCTT#00229"/>
        <EmpowerBP:isMostAppropriateForInterventionFunction rdf:resource="http://www.semanticweb.org/tswheeler/ontologies/2016/3/EmpowerBP#Coercion"/>
        <EmpowerBP:isMostAppropriateForInterventionFunction rdf:resource="http://www.semanticweb.org/tswheeler/ontologies/2016/3/EmpowerBP#Incentivisation"/>
        <rdfs:comment>Examples:

Watch hand washing behaviors among health care staff and make notes on context, frequency and technique used</rdfs:comment>
        <rdfs:comment>Observe or record behaviour with the person&apos;s knowledge as part of a behaviour change strategy

Note: if monitoring is part of a data collection procedure rather than a strategy aimed at changing behaviour, do not code; if feedback given, code only 2.2, Feedback on behaviour, and not 2.1, Monitoring of behaviour by others without feedback; if monitoring outcome(s) code 2.5, Monitoring outcome(s) of behaviour by others without feedback; if self-monitoring behaviour, code 2.3, Self-monitoring of behaviour</rdfs:comment>
        <rdfs:label>Monitoring of behavior by others without feedback</rdfs:label>
    </owl:NamedIndividual>
    


    <!-- http://purl.bioontology.org/ontology/BCTT#Monitoring_of_emotional_consequences -->

    <owl:NamedIndividual rdf:about="http://purl.bioontology.org/ontology/BCTT#Monitoring_of_emotional_consequences">
        <rdf:type rdf:resource="http://purl.bioontology.org/ontology/BCTT#BehaviourChangeTechnique"/>
        <rdf:type rdf:resource="http://purl.bioontology.org/ontology/BCTT#00246"/>
        <EmpowerBP:isAppropriateForInterventionFunciton rdf:resource="http://www.semanticweb.org/tswheeler/ontologies/2016/3/EmpowerBP#Enablement"/>
        <rdfs:comment>Examples:

Agree that the person will record how they feel after taking their daily walk</rdfs:comment>
        <rdfs:comment>Prompt assessment of feelings after attempts at performing the behavior</rdfs:comment>
        <rdfs:label>Monitoring of emotional consequences</rdfs:label>
    </owl:NamedIndividual>
    


    <!-- http://purl.bioontology.org/ontology/BCTT#Non-specific_incentive -->

    <owl:NamedIndividual rdf:about="http://purl.bioontology.org/ontology/BCTT#Non-specific_incentive">
        <rdf:type rdf:resource="http://purl.bioontology.org/ontology/BCTT#BehaviourChangeTechnique"/>
        <rdf:type rdf:resource="http://purl.bioontology.org/ontology/BCTT#00278"/>
        <rdfs:comment>Examples:

Identify an activity that the person values and inform them that this will happen if and only if they attend for health screening</rdfs:comment>
        <rdfs:comment>Inform that a reward will be delivered if and only if there has been effort and/or progress in performing the behavior (includes ‘Positive reinforcement’)

Note: if incentive is material, code 10.1, Material incentive (behavior), if social, code 10.5, Social incentive and not 10.6, Non-specific incentive; if incentive is for outcome code 10.8, Incentive (outcome). If reward is delivered also code one of: 10.2, Material reward (behavior); 10.3, Non-specific reward; 10.4, Social reward, 10.9, Self-reward; 10.10, Reward (outcome)</rdfs:comment>
        <rdfs:label>Non-specific incentive</rdfs:label>
    </owl:NamedIndividual>
    


    <!-- http://purl.bioontology.org/ontology/BCTT#Non-specific_reward -->

    <owl:NamedIndividual rdf:about="http://purl.bioontology.org/ontology/BCTT#Non-specific_reward">
        <rdf:type rdf:resource="http://purl.bioontology.org/ontology/BCTT#BehaviourChangeTechnique"/>
        <rdf:type rdf:resource="http://purl.bioontology.org/ontology/BCTT#00278"/>
        <EmpowerBP:isAppropriateForInterventionFunciton rdf:resource="http://www.semanticweb.org/tswheeler/ontologies/2016/3/EmpowerBP#Incentivisation"/>
        <rdfs:comment>Arrange delivery of a reward if and only if there has been effort and/or progress in performing the behavior (includes ‘Positive reinforcement’)

Note: if reward is material, code 10.2, Material reward (behavior), if social, code 10.4, Social reward, and not 10.3, Non- specific reward; if reward is for outcome code 10.10, Reward (outcome). If informed of reward in advance of rewarded behaviour, also code one of: 10.1, Material incentive (behaviour); 10.5, Social incentive; 10.6, Non-specific incentive; 10.7, Self-incentive; 10.8, Incentive (outcome)</rdfs:comment>
        <rdfs:comment>Examples:

Identify something (e.g. an activity such as a visit to the cinema) that the person values and arrange for this to be delivered if and only if they attend for health screening</rdfs:comment>
        <rdfs:label>Non-specific reward</rdfs:label>
    </owl:NamedIndividual>
    


    <!-- http://purl.bioontology.org/ontology/BCTT#Overcorrection -->

    <owl:NamedIndividual rdf:about="http://purl.bioontology.org/ontology/BCTT#Overcorrection">
        <rdf:type rdf:resource="http://purl.bioontology.org/ontology/BCTT#BehaviourChangeTechnique"/>
        <rdf:type rdf:resource="http://purl.bioontology.org/ontology/BCTT#00266"/>
        <EmpowerBP:isAppropriateForInterventionFunciton rdf:resource="http://www.semanticweb.org/tswheeler/ontologies/2016/3/EmpowerBP#Enablement"/>
        <rdfs:comment>Ask to repeat the wanted behavior in an exaggerated way following an unwanted behaviour</rdfs:comment>
        <rdfs:comment>Examples:

Ask to eat only fruit and vegetables the day after a poor diet</rdfs:comment>
        <rdfs:label>Overcorrection</rdfs:label>
    </owl:NamedIndividual>
    


    <!-- http://purl.bioontology.org/ontology/BCTT#Paradoxical_instructions -->

    <owl:NamedIndividual rdf:about="http://purl.bioontology.org/ontology/BCTT#Paradoxical_instructions">
        <rdf:type rdf:resource="http://purl.bioontology.org/ontology/BCTT#BehaviourChangeTechnique"/>
        <rdf:type rdf:resource="http://purl.bioontology.org/ontology/BCTT#00290"/>
        <EmpowerBP:isAppropriateForInterventionFunciton rdf:resource="http://www.semanticweb.org/tswheeler/ontologies/2016/3/EmpowerBP#Incentivisation"/>
        <rdfs:comment>Advise to engage in some form of the unwanted behavior with the aim of reducing motivation to engage in that behaviour</rdfs:comment>
        <rdfs:comment>Examples:

Advise a smoker to smoke twice as many cigarettes a day as they usually do
Tell the person to stay awake as long as possible in order to reduce insomnia</rdfs:comment>
        <rdfs:label>Paradoxical instructions</rdfs:label>
    </owl:NamedIndividual>
    


    <!-- http://purl.bioontology.org/ontology/BCTT#Pharmacological_support -->

    <owl:NamedIndividual rdf:about="http://purl.bioontology.org/ontology/BCTT#Pharmacological_support">
        <rdf:type rdf:resource="http://purl.bioontology.org/ontology/BCTT#BehaviourChangeTechnique"/>
        <rdf:type rdf:resource="http://purl.bioontology.org/ontology/BCTT#00290"/>
        <EmpowerBP:isAppropriateForInterventionFunciton rdf:resource="http://www.semanticweb.org/tswheeler/ontologies/2016/3/EmpowerBP#Enablement"/>
        <rdfs:comment>Examples:

Suggest the patient asks the family physician for nicotine replacement therapy to facilitate smoking cessation</rdfs:comment>
        <rdfs:comment>Provide, or encourage the use of or adherence to, drugs to facilitate behavior change

Note: if pharmacological support to reduce negative emotions (i.e. anxiety) then also code 11.2, Reduce negative emotions</rdfs:comment>
        <rdfs:label>Pharmacological support</rdfs:label>
    </owl:NamedIndividual>
    


    <!-- http://purl.bioontology.org/ontology/BCTT#Problem_solving -->

    <owl:NamedIndividual rdf:about="http://purl.bioontology.org/ontology/BCTT#Problem_solving">
        <rdf:type rdf:resource="http://purl.bioontology.org/ontology/BCTT#BehaviourChangeTechnique"/>
        <rdf:type rdf:resource="http://purl.bioontology.org/ontology/BCTT#00219"/>
        <EmpowerBP:isMostAppropriateForInterventionFunction rdf:resource="http://www.semanticweb.org/tswheeler/ontologies/2016/3/EmpowerBP#Enablement"/>
        <rdfs:comment>Analyse , or prompt the person to analyse, factors influencing the behaviour and generate or select strategies that include overcoming barriers and/or increasing facilitators (includes &apos;Relapse Prevention&apos; and &apos;Coping Planning&apos;).

Note: barrier identification without solutions is not sufficient. If the BCT does not include analysing the behavioural problem, consider 12.3, Avoidance/changing exposure to cues for the behaviour, 12.1, Restructuring the physical environment, 12.2, Restructuring the social environment, or 11.2, Reduce negative emotions</rdfs:comment>
        <rdfs:comment>Examples:

Identify specific triggers (e.g. being in a pub, feeling anxious) that generate the urge/want/need to drink and develop strategies for avoiding environmental triggers or for managing negative emotions, such as anxiety, that motivate drinking
Prompt the patient to identify barriers preventing them from starting a new exercise regime e.g., lack of motivation, and discuss ways in which they could help overcome them e.g., going to the gym with a buddy</rdfs:comment>
        <rdfs:label>Problem solving</rdfs:label>
    </owl:NamedIndividual>
    


    <!-- http://purl.bioontology.org/ontology/BCTT#Prompts-cues -->

    <owl:NamedIndividual rdf:about="http://purl.bioontology.org/ontology/BCTT#Prompts-cues">
        <rdf:type rdf:resource="http://purl.bioontology.org/ontology/BCTT#BehaviourChangeTechnique"/>
        <rdf:type rdf:resource="http://purl.bioontology.org/ontology/BCTT#00257"/>
        <EmpowerBP:isMostAppropriateForInterventionFunction rdf:resource="http://www.semanticweb.org/tswheeler/ontologies/2016/3/EmpowerBP#Education"/>
        <EmpowerBP:isMostAppropriateForInterventionFunction rdf:resource="http://www.semanticweb.org/tswheeler/ontologies/2016/3/EmpowerBP#EnvironmentalRestructuring"/>
        <rdfs:comment>Examples:

Put a sticker on the bathroom mirror to remind people to brush their teeth</rdfs:comment>
        <rdfs:comment>Introduce or define environmental or social stimulus with the purpose of prompting or cueing the behavior. The prompt or cue would normally occur at the time or place of performance

Note: when a stimulus is linked to a specific action in an if-then plan including one or more of frequency, duration or intensity also code 1.4, Action planning.</rdfs:comment>
        <rdfs:label>Prompts-cues</rdfs:label>
    </owl:NamedIndividual>
    


    <!-- http://purl.bioontology.org/ontology/BCTT#Pros_and_cons -->

    <owl:NamedIndividual rdf:about="http://purl.bioontology.org/ontology/BCTT#Pros_and_cons">
        <rdf:type rdf:resource="http://purl.bioontology.org/ontology/BCTT#BehaviourChangeTechnique"/>
        <rdf:type rdf:resource="http://purl.bioontology.org/ontology/BCTT#00274"/>
        <EmpowerBP:isAppropriateForInterventionFunciton rdf:resource="http://www.semanticweb.org/tswheeler/ontologies/2016/3/EmpowerBP#Enablement"/>
        <rdfs:comment>Advise the person to identify and compare reasons for wanting (pros) and not wanting to (cons) change the behavior (includes ‘Decisional balance’)

Note: if providing information about health consequences, also code 5.1, Information about health consequences; if providing information about emotional consequences, also code 5.6, Information about emotional consequences; if providing information about social, environmental or unspecified consequences also code 5.3, Information about social and environmental consequences</rdfs:comment>
        <rdfs:comment>Examples:

Advise the person to list and compare the advantages and disadvantages of prescribing antibiotics for upper respiratory tract infections</rdfs:comment>
        <rdfs:label>Pros and cons</rdfs:label>
    </owl:NamedIndividual>
    


    <!-- http://purl.bioontology.org/ontology/BCTT#Punishment -->

    <owl:NamedIndividual rdf:about="http://purl.bioontology.org/ontology/BCTT#Punishment">
        <rdf:type rdf:resource="http://purl.bioontology.org/ontology/BCTT#BehaviourChangeTechnique"/>
        <rdf:type rdf:resource="http://purl.bioontology.org/ontology/BCTT#00308"/>
        <EmpowerBP:isAppropriateForInterventionFunciton rdf:resource="http://www.semanticweb.org/tswheeler/ontologies/2016/3/EmpowerBP#Coercion"/>
        <rdfs:comment>Arrange for aversive consequence contingent on the performance of the unwanted behavior</rdfs:comment>
        <rdfs:comment>Examples:

Arrange for the person to wear unattractive clothes following consumption of fatty foods</rdfs:comment>
        <rdfs:label>Punishment</rdfs:label>
    </owl:NamedIndividual>
    


    <!-- http://purl.bioontology.org/ontology/BCTT#Re-attribution -->

    <owl:NamedIndividual rdf:about="http://purl.bioontology.org/ontology/BCTT#Re-attribution">
        <rdf:type rdf:resource="http://purl.bioontology.org/ontology/BCTT#BehaviourChangeTechnique"/>
        <rdf:type rdf:resource="http://purl.bioontology.org/ontology/BCTT#00241"/>
        <EmpowerBP:isAppropriateForInterventionFunciton rdf:resource="http://www.semanticweb.org/tswheeler/ontologies/2016/3/EmpowerBP#Education"/>
        <EmpowerBP:isAppropriateForInterventionFunciton rdf:resource="http://www.semanticweb.org/tswheeler/ontologies/2016/3/EmpowerBP#Persuasion"/>
        <rdfs:comment>Elicit perceived causes of behavior and suggest alternative explanations (e.g. external or internal and stable or unstable)</rdfs:comment>
        <rdfs:comment>Examples:

If the person attributes their over-eating to the frequent presence of delicious food, suggest that the ‘real’ cause may be the person’s inattention to bodily signals of hunger and satiety</rdfs:comment>
        <rdfs:label>Re-attribution</rdfs:label>
    </owl:NamedIndividual>
    


    <!-- http://purl.bioontology.org/ontology/BCTT#Reduce_negative_emotions -->

    <owl:NamedIndividual rdf:about="http://purl.bioontology.org/ontology/BCTT#Reduce_negative_emotions">
        <rdf:type rdf:resource="http://purl.bioontology.org/ontology/BCTT#BehaviourChangeTechnique"/>
        <rdf:type rdf:resource="http://purl.bioontology.org/ontology/BCTT#00290"/>
        <EmpowerBP:isAppropriateForInterventionFunciton rdf:resource="http://www.semanticweb.org/tswheeler/ontologies/2016/3/EmpowerBP#Enablement"/>
        <rdfs:comment>Advise on ways of reducing negative emotions to facilitate performance of the behavior (includes ‘Stress Management’) 

Note: if includes analysing the behavioural problem, also code 1.2, Problem solving</rdfs:comment>
        <rdfs:comment>Examples:

Advise on the use of stress management skills, e.g. to reduce anxiety about joining Alcoholics Anonymous</rdfs:comment>
        <rdfs:label>Reduce negative emotions</rdfs:label>
    </owl:NamedIndividual>
    


    <!-- http://purl.bioontology.org/ontology/BCTT#Reduce_prompts-cues -->

    <owl:NamedIndividual rdf:about="http://purl.bioontology.org/ontology/BCTT#Reduce_prompts-cues">
        <rdf:type rdf:resource="http://purl.bioontology.org/ontology/BCTT#BehaviourChangeTechnique"/>
        <rdf:type rdf:resource="http://purl.bioontology.org/ontology/BCTT#00257"/>
        <EmpowerBP:isAppropriateForInterventionFunciton rdf:resource="http://www.semanticweb.org/tswheeler/ontologies/2016/3/EmpowerBP#EnvironmentalRestructuring"/>
        <rdfs:comment>Examples:

Reduce gradually the number of reminders used to take medication</rdfs:comment>
        <rdfs:comment>Withdraw gradually prompts to perform the behavior (includes ‘Fading’)</rdfs:comment>
        <rdfs:label>Reduce prompts-cues</rdfs:label>
    </owl:NamedIndividual>
    


    <!-- http://purl.bioontology.org/ontology/BCTT#Reduce_reward_frequency -->

    <owl:NamedIndividual rdf:about="http://purl.bioontology.org/ontology/BCTT#Reduce_reward_frequency">
        <rdf:type rdf:resource="http://purl.bioontology.org/ontology/BCTT#BehaviourChangeTechnique"/>
        <rdf:type rdf:resource="http://purl.bioontology.org/ontology/BCTT#00308"/>
        <EmpowerBP:isAppropriateForInterventionFunciton rdf:resource="http://www.semanticweb.org/tswheeler/ontologies/2016/3/EmpowerBP#Incentivisation"/>
        <rdfs:comment>Arrange for rewards to be made contingent on increasing duration or frequency of the behavior (includes ‘Thinning’)

Note: also code one of 10.2, Material reward (behavior); 10.3, Non-specific reward; 10.4, Social reward, 10.9, Self- reward; 10.10, Reward (outcome</rdfs:comment>
        <rdfs:comment>Examples:

Arrange reward for each day without smoking, then each week, then each month, then every 2 months and so on</rdfs:comment>
        <rdfs:label>Reduce reward frequency</rdfs:label>
    </owl:NamedIndividual>
    


    <!-- http://purl.bioontology.org/ontology/BCTT#Remove_access_to_the_reward -->

    <owl:NamedIndividual rdf:about="http://purl.bioontology.org/ontology/BCTT#Remove_access_to_the_reward">
        <rdf:type rdf:resource="http://purl.bioontology.org/ontology/BCTT#BehaviourChangeTechnique"/>
        <rdf:type rdf:resource="http://purl.bioontology.org/ontology/BCTT#00257"/>
        <EmpowerBP:isAppropriateForInterventionFunciton rdf:resource="http://www.semanticweb.org/tswheeler/ontologies/2016/3/EmpowerBP#Coercion"/>
        <EmpowerBP:isAppropriateForInterventionFunciton rdf:resource="http://www.semanticweb.org/tswheeler/ontologies/2016/3/EmpowerBP#EnvironmentalRestructuring"/>
        <rdfs:comment>Advise or arrange for the person to be separated from situations in which unwanted behavior can be rewarded in order to reduce the behavior (includes ‘Time out’)</rdfs:comment>
        <rdfs:comment>Examples:

Arrange for cupboard containing high calorie snacks to be locked for a specified period to reduce the consumption of sugary foods in between meals</rdfs:comment>
        <rdfs:label>Remove access to the reward</rdfs:label>
    </owl:NamedIndividual>
    


    <!-- http://purl.bioontology.org/ontology/BCTT#Remove_aversive_stimulus -->

    <owl:NamedIndividual rdf:about="http://purl.bioontology.org/ontology/BCTT#Remove_aversive_stimulus">
        <rdf:type rdf:resource="http://purl.bioontology.org/ontology/BCTT#BehaviourChangeTechnique"/>
        <rdf:type rdf:resource="http://purl.bioontology.org/ontology/BCTT#00257"/>
        <EmpowerBP:isAppropriateForInterventionFunciton rdf:resource="http://www.semanticweb.org/tswheeler/ontologies/2016/3/EmpowerBP#EnvironmentalRestructuring"/>
        <EmpowerBP:isAppropriateForInterventionFunciton rdf:resource="http://www.semanticweb.org/tswheeler/ontologies/2016/3/EmpowerBP#Incentivisation"/>
        <rdfs:comment>Advise or arrange for the removal of an aversive stimulus to facilitate behavior change (includes ‘Escape learning’)</rdfs:comment>
        <rdfs:comment>Examples:

Arrange for a gym-buddy to stop nagging the person to do more exercise in order to increase the desired exercise behaviour</rdfs:comment>
        <rdfs:label>Remove aversive stimulus</rdfs:label>
    </owl:NamedIndividual>
    


    <!-- http://purl.bioontology.org/ontology/BCTT#Remove_punishment -->

    <owl:NamedIndividual rdf:about="http://purl.bioontology.org/ontology/BCTT#Remove_punishment">
        <rdf:type rdf:resource="http://purl.bioontology.org/ontology/BCTT#BehaviourChangeTechnique"/>
        <rdf:type rdf:resource="http://purl.bioontology.org/ontology/BCTT#00308"/>
        <EmpowerBP:isAppropriateForInterventionFunciton rdf:resource="http://www.semanticweb.org/tswheeler/ontologies/2016/3/EmpowerBP#Incentivisation"/>
        <rdfs:comment>Arrange for removal of an unpleasant consequence contingent on performance of the wanted behavior (includes ‘Negative reinforcement’)</rdfs:comment>
        <rdfs:comment>Examples:

Arrange for someone else to do housecleaning only if the person has adhered to the medication regimen for a week</rdfs:comment>
        <rdfs:label>Remove punishment</rdfs:label>
    </owl:NamedIndividual>
    


    <!-- http://purl.bioontology.org/ontology/BCTT#Remove_reward -->

    <owl:NamedIndividual rdf:about="http://purl.bioontology.org/ontology/BCTT#Remove_reward">
        <rdf:type rdf:resource="http://purl.bioontology.org/ontology/BCTT#BehaviourChangeTechnique"/>
        <rdf:type rdf:resource="http://purl.bioontology.org/ontology/BCTT#00308"/>
        <EmpowerBP:isAppropriateForInterventionFunciton rdf:resource="http://www.semanticweb.org/tswheeler/ontologies/2016/3/EmpowerBP#Coercion"/>
        <rdfs:comment>Arrange for discontinuation of contingent reward following performance of the unwanted behavior (includes ‘Extinction’)</rdfs:comment>
        <rdfs:comment>Examples:

Arrange for the other people in the household to ignore the person every time they eat chocolate (rather than attending to them by criticising or persuading)</rdfs:comment>
        <rdfs:label>Remove reward</rdfs:label>
    </owl:NamedIndividual>
    


    <!-- http://purl.bioontology.org/ontology/BCTT#Restructuring_the_physical_environment -->

    <owl:NamedIndividual rdf:about="http://purl.bioontology.org/ontology/BCTT#Restructuring_the_physical_environment">
        <rdf:type rdf:resource="http://purl.bioontology.org/ontology/BCTT#BehaviourChangeTechnique"/>
        <rdf:type rdf:resource="http://purl.bioontology.org/ontology/BCTT#00295"/>
        <EmpowerBP:isMostAppropriateForInterventionFunction rdf:resource="http://www.semanticweb.org/tswheeler/ontologies/2016/3/EmpowerBP#Enablement"/>
        <EmpowerBP:isMostAppropriateForInterventionFunction rdf:resource="http://www.semanticweb.org/tswheeler/ontologies/2016/3/EmpowerBP#EnvironmentalRestructuring"/>
        <rdfs:comment>Change, or advise to change the physical environment in order to facilitate performance of the wanted behavior or create barriers to the unwanted behavior (other than prompts/cues, rewards and punishments)

Note: this may also involve 12.3, Avoidance/reducing exposure to cues for the behavior; if restructuring of the social environment code 12.2, Restructuring the social environment; if only adding objects to the environment, code 12.5, Adding objects to the environment</rdfs:comment>
        <rdfs:comment>Examples:

Advise to keep biscuits and snacks in a cupboard that is inconvenient to get to
Arrange to move vending machine out of the school</rdfs:comment>
        <rdfs:label>Restructuring the physical environment</rdfs:label>
    </owl:NamedIndividual>
    


    <!-- http://purl.bioontology.org/ontology/BCTT#Restructuring_the_social_environment -->

    <owl:NamedIndividual rdf:about="http://purl.bioontology.org/ontology/BCTT#Restructuring_the_social_environment">
        <rdf:type rdf:resource="http://purl.bioontology.org/ontology/BCTT#BehaviourChangeTechnique"/>
        <rdf:type rdf:resource="http://purl.bioontology.org/ontology/BCTT#00295"/>
        <EmpowerBP:isAppropriateForInterventionFunciton rdf:resource="http://www.semanticweb.org/tswheeler/ontologies/2016/3/EmpowerBP#Enablement"/>
        <EmpowerBP:isAppropriateForInterventionFunciton rdf:resource="http://www.semanticweb.org/tswheeler/ontologies/2016/3/EmpowerBP#EnvironmentalRestructuring"/>
        <rdfs:comment>Change, or advise to change the social environment in order to facilitate performance of the wanted behavior or create barriers to the unwanted behavior (other than prompts/cues, rewards and punishments)

Note: this may also involve 12.3, Avoidance/reducing exposure to cues for the behavior; if also restructuring of the physical environment also code 12.1, Restructuring the physical environment</rdfs:comment>
        <rdfs:comment>Examples:

Advise to minimise time spent with friends who drink heavily to reduce alcohol consumption</rdfs:comment>
        <rdfs:label>Restructuring the social environment</rdfs:label>
    </owl:NamedIndividual>
    


    <!-- http://purl.bioontology.org/ontology/BCTT#Reward_alternative_behavior -->

    <owl:NamedIndividual rdf:about="http://purl.bioontology.org/ontology/BCTT#Reward_alternative_behavior">
        <rdf:type rdf:resource="http://purl.bioontology.org/ontology/BCTT#BehaviourChangeTechnique"/>
        <rdf:type rdf:resource="http://purl.bioontology.org/ontology/BCTT#00308"/>
        <EmpowerBP:isAppropriateForInterventionFunciton rdf:resource="http://www.semanticweb.org/tswheeler/ontologies/2016/3/EmpowerBP#Incentivisation"/>
        <rdfs:comment>Arrange reward for performance of an alternative to the unwanted behavior (includes ‘Differential reinforcement’) 

Note: also code one of 10.2, Material reward (behavior); 10.3, Non-specific reward; 10.4, Social reward, 10.9, Self- reward; 10.10, Reward (outcome); consider also coding 1.2, Problem solving</rdfs:comment>
        <rdfs:comment>Examples:

Reward for consumption of low fat foods but not consumption of high fat foods</rdfs:comment>
        <rdfs:label>Reward alternative behavior</rdfs:label>
    </owl:NamedIndividual>
    


    <!-- http://purl.bioontology.org/ontology/BCTT#Reward_approximation -->

    <owl:NamedIndividual rdf:about="http://purl.bioontology.org/ontology/BCTT#Reward_approximation">
        <rdf:type rdf:resource="http://purl.bioontology.org/ontology/BCTT#BehaviourChangeTechnique"/>
        <rdf:type rdf:resource="http://purl.bioontology.org/ontology/BCTT#00308"/>
        <EmpowerBP:isAppropriateForInterventionFunciton rdf:resource="http://www.semanticweb.org/tswheeler/ontologies/2016/3/EmpowerBP#Incentivisation"/>
        <rdfs:comment>Arrange for reward following any approximation to the target behavior, gradually rewarding only performance closer to the wanted behavior (includes ‘Shaping’)</rdfs:comment>
        <rdfs:comment>Examples:

Arrange reward for any reduction in daily calories, gradually requiring the daily calorie count to become closer to the planned calorie intake</rdfs:comment>
        <rdfs:label>Reward approximation</rdfs:label>
    </owl:NamedIndividual>
    


    <!-- http://purl.bioontology.org/ontology/BCTT#Reward_incompatible_behavior -->

    <owl:NamedIndividual rdf:about="http://purl.bioontology.org/ontology/BCTT#Reward_incompatible_behavior">
        <rdf:type rdf:resource="http://purl.bioontology.org/ontology/BCTT#BehaviourChangeTechnique"/>
        <rdf:type rdf:resource="http://purl.bioontology.org/ontology/BCTT#00308"/>
        <EmpowerBP:isAppropriateForInterventionFunciton rdf:resource="http://www.semanticweb.org/tswheeler/ontologies/2016/3/EmpowerBP#Incentivisation"/>
        <rdfs:comment>Arrange reward for responding in a manner that is incompatible with a previous response to that situation (includes ‘Counter-conditioning’) 

Note: also code one of 10.2, Material reward (behavior); 10.3, Non-specific reward; 10.4, Social reward, 10.9, Self- reward; 10.10, Reward (outcome)</rdfs:comment>
        <rdfs:comment>Examples:

Arrange reward for ordering a soft drink at the bar rather than an alcoholic beverage</rdfs:comment>
        <rdfs:label>Reward incompatible behavior</rdfs:label>
    </owl:NamedIndividual>
    


    <!-- http://purl.bioontology.org/ontology/BCTT#Rewarding_completion -->

    <owl:NamedIndividual rdf:about="http://purl.bioontology.org/ontology/BCTT#Rewarding_completion">
        <rdf:type rdf:resource="http://purl.bioontology.org/ontology/BCTT#BehaviourChangeTechnique"/>
        <rdf:type rdf:resource="http://purl.bioontology.org/ontology/BCTT#00308"/>
        <EmpowerBP:isAppropriateForInterventionFunciton rdf:resource="http://www.semanticweb.org/tswheeler/ontologies/2016/3/EmpowerBP#Incentivisation"/>
        <rdfs:comment>Build up behavior by arranging reward following final component of the behavior; gradually add the components of the behavior that occur earlier in the behavioral sequence (includes ‘Backward chaining’)

Note: also code one of 10.2, Material reward (behavior); 10.3, Non-specific reward; 10.4, Social reward, 10.9, Self- reward; 10.10, Reward (outcome)</rdfs:comment>
        <rdfs:comment>Examples:

Reward eating a supplied low calorie meal; then make reward contingent on cooking and eating the meal; then make reward contingent on purchasing, cooking and eating the meal</rdfs:comment>
        <rdfs:label>Rewarding completion</rdfs:label>
    </owl:NamedIndividual>
    


    <!-- http://purl.bioontology.org/ontology/BCTT#Salience_of_consequences -->

    <owl:NamedIndividual rdf:about="http://purl.bioontology.org/ontology/BCTT#Salience_of_consequences">
        <rdf:type rdf:resource="http://purl.bioontology.org/ontology/BCTT#BehaviourChangeTechnique"/>
        <rdf:type rdf:resource="http://purl.bioontology.org/ontology/BCTT#00246"/>
        <EmpowerBP:isAppropriateForInterventionFunciton rdf:resource="http://www.semanticweb.org/tswheeler/ontologies/2016/3/EmpowerBP#Enablement"/>
        <EmpowerBP:isAppropriateForInterventionFunciton rdf:resource="http://www.semanticweb.org/tswheeler/ontologies/2016/3/EmpowerBP#Persuasion"/>
        <rdfs:comment>Examples:

Produce cigarette packets showing pictures of health consequences e.g. diseased lungs, to highlight the dangers of continuing to smoke</rdfs:comment>
        <rdfs:comment>Use methods specifically designed to emphasise the consequences of performing the behaviour with the aim of making them more memorable (goes beyond informing about consequences) 

Note: if information about consequences, also code 5.1, Information about health consequences, 5.6, Information about emotional consequences or 5.3, Information about social and environmental consequences</rdfs:comment>
        <rdfs:label>Salience of consequences</rdfs:label>
    </owl:NamedIndividual>
    


    <!-- http://purl.bioontology.org/ontology/BCTT#Satiation -->

    <owl:NamedIndividual rdf:about="http://purl.bioontology.org/ontology/BCTT#Satiation">
        <rdf:type rdf:resource="http://purl.bioontology.org/ontology/BCTT#BehaviourChangeTechnique"/>
        <rdf:type rdf:resource="http://purl.bioontology.org/ontology/BCTT#00257"/>
        <EmpowerBP:isAppropriateForInterventionFunciton rdf:resource="http://www.semanticweb.org/tswheeler/ontologies/2016/3/EmpowerBP#Education"/>
        <EmpowerBP:isAppropriateForInterventionFunciton rdf:resource="http://www.semanticweb.org/tswheeler/ontologies/2016/3/EmpowerBP#EnvironmentalRestructuring"/>
        <rdfs:comment>Advise or arrange repeated exposure to a stimulus that reduces or extinguishes a drive for the unwanted behavior</rdfs:comment>
        <rdfs:comment>Examples:

Arrange for the person to eat large quantities of chocolate, in order to reduce the person’s appetite for sweet foods</rdfs:comment>
        <rdfs:label>Satiation</rdfs:label>
    </owl:NamedIndividual>
    


    <!-- http://purl.bioontology.org/ontology/BCTT#Self-incentive -->

    <owl:NamedIndividual rdf:about="http://purl.bioontology.org/ontology/BCTT#Self-incentive">
        <rdf:type rdf:resource="http://purl.bioontology.org/ontology/BCTT#BehaviourChangeTechnique"/>
        <rdf:type rdf:resource="http://purl.bioontology.org/ontology/BCTT#00278"/>
        <rdfs:comment>Examples:

Encourage to provide self with material (e.g., new clothes) or other valued objects if and only if they have adhered to a healthy diet</rdfs:comment>
        <rdfs:comment>Plan to reward self in future if and only if there has been effort and/or progress in performing the behavior

Note: if self-reward is material, also code 10.1, Material incentive (behavior), if social, also code 10.5, Social incentive, if unspecified, also code 10.6, Non-specific incentive; if incentive is for outcome code 10.8, Incentive (outcome). If reward is delivered also code one of: 10.2, Material reward (behavior); 10.3, Non-specific reward; 10.4, Social reward, 10.9, Self- reward; 10.10, Reward (outcome)</rdfs:comment>
        <rdfs:label>Self-incentive</rdfs:label>
    </owl:NamedIndividual>
    


    <!-- http://purl.bioontology.org/ontology/BCTT#Self-monitoring_of_behaviour -->

    <owl:NamedIndividual rdf:about="http://purl.bioontology.org/ontology/BCTT#Self-monitoring_of_behaviour">
        <rdf:type rdf:resource="http://purl.bioontology.org/ontology/BCTT#BehaviourChangeTechnique"/>
        <rdf:type rdf:resource="http://purl.bioontology.org/ontology/BCTT#00229"/>
        <EmpowerBP:isMostAppropriateForInterventionFunction rdf:resource="http://www.semanticweb.org/tswheeler/ontologies/2016/3/EmpowerBP#Coercion"/>
        <EmpowerBP:isMostAppropriateForInterventionFunction rdf:resource="http://www.semanticweb.org/tswheeler/ontologies/2016/3/EmpowerBP#Education"/>
        <EmpowerBP:isMostAppropriateForInterventionFunction rdf:resource="http://www.semanticweb.org/tswheeler/ontologies/2016/3/EmpowerBP#Enablement"/>
        <EmpowerBP:isMostAppropriateForInterventionFunction rdf:resource="http://www.semanticweb.org/tswheeler/ontologies/2016/3/EmpowerBP#Incentivisation"/>
        <EmpowerBP:isMostAppropriateForInterventionFunction rdf:resource="http://www.semanticweb.org/tswheeler/ontologies/2016/3/EmpowerBP#Training"/>
        <rdfs:comment>Establish a method for the person to monitor and record their behaviour(s) as part of a behaviour change strategy 

Note: if monitoring is part of a data collection procedure rather than a strategy aimed at changing behaviour, do not code; if monitoring of outcome of behaviour, code 2.4, Self-monitoring of outcome(s) of behaviour; if monitoring is by someone else (without feedback), code 2.1, Monitoring of behaviour by others without feedback</rdfs:comment>
        <rdfs:comment>Examples:

Ask the person to record daily, in a diary, whether they have brushed their teeth for at least two minutes before going to bed
Give patient a pedometer and a form for recording daily total number of steps</rdfs:comment>
        <rdfs:label>Self-monitoring of behaviour</rdfs:label>
    </owl:NamedIndividual>
    


    <!-- http://purl.bioontology.org/ontology/BCTT#Self-reward -->

    <owl:NamedIndividual rdf:about="http://purl.bioontology.org/ontology/BCTT#Self-reward">
        <rdf:type rdf:resource="http://purl.bioontology.org/ontology/BCTT#BehaviourChangeTechnique"/>
        <rdf:type rdf:resource="http://purl.bioontology.org/ontology/BCTT#00278"/>
        <EmpowerBP:isAppropriateForInterventionFunciton rdf:resource="http://www.semanticweb.org/tswheeler/ontologies/2016/3/EmpowerBP#Enablement"/>
        <EmpowerBP:isAppropriateForInterventionFunciton rdf:resource="http://www.semanticweb.org/tswheeler/ontologies/2016/3/EmpowerBP#Incentivisation"/>
        <EmpowerBP:isAppropriateForInterventionFunciton rdf:resource="http://www.semanticweb.org/tswheeler/ontologies/2016/3/EmpowerBP#Training"/>
        <rdfs:comment>Examples:

Encourage to reward self with material (e.g., new clothes) or other valued objects if and only if they have adhered to a healthy diet</rdfs:comment>
        <rdfs:comment>Prompt self-praise or self-reward if and only if there has been effort and/or progress in performing the behavior

Note: if self-reward is material, also code 10.2, Material reward (behavior), if social, also code 10.4, Social reward, if unspecified, also code 10.3, Non-specific reward; if reward is for outcome code 10.10, Reward (outcome). If informed of reward in advance of rewarded behaviour, also code one of: 10.1, Material incentive (behaviour); 10.5, Social incentive; 10.6, Non-specific incentive; 10.7, Self- incentive; 10.8, Incentive (outcome)</rdfs:comment>
        <rdfs:label>Self-reward</rdfs:label>
    </owl:NamedIndividual>
    


    <!-- http://purl.bioontology.org/ontology/BCTT#Self-talk -->

    <owl:NamedIndividual rdf:about="http://purl.bioontology.org/ontology/BCTT#Self-talk">
        <rdf:type rdf:resource="http://purl.bioontology.org/ontology/BCTT#BehaviourChangeTechnique"/>
        <rdf:type rdf:resource="http://purl.bioontology.org/ontology/BCTT#00319"/>
        <EmpowerBP:isAppropriateForInterventionFunciton rdf:resource="http://www.semanticweb.org/tswheeler/ontologies/2016/3/EmpowerBP#Enablement"/>
        <EmpowerBP:isAppropriateForInterventionFunciton rdf:resource="http://www.semanticweb.org/tswheeler/ontologies/2016/3/EmpowerBP#Training"/>
        <rdfs:comment>Examples:

Prompt the person to tell themselves that a walk will be energising</rdfs:comment>
        <rdfs:comment>Prompt positive self-talk (aloud or silently) before and during the behavior</rdfs:comment>
        <rdfs:label>Self-talk</rdfs:label>
    </owl:NamedIndividual>
    


    <!-- http://purl.bioontology.org/ontology/BCTT#Situation-specific_reward -->

    <owl:NamedIndividual rdf:about="http://purl.bioontology.org/ontology/BCTT#Situation-specific_reward">
        <rdf:type rdf:resource="http://purl.bioontology.org/ontology/BCTT#BehaviourChangeTechnique"/>
        <rdf:type rdf:resource="http://purl.bioontology.org/ontology/BCTT#00308"/>
        <EmpowerBP:isAppropriateForInterventionFunciton rdf:resource="http://www.semanticweb.org/tswheeler/ontologies/2016/3/EmpowerBP#Incentivisation"/>
        <rdfs:comment>Arrange for reward following the behavior in one situation but not in another (includes ‘Discrimination training’)

Note: also code one of 10.2, Material reward (behavior); 10.3, Non-specific reward; 10.4, Social reward, 10.9, Self- reward; 10.10, Reward (outcome)</rdfs:comment>
        <rdfs:comment>Examples:

Arrange reward for eating at mealtimes but not between meals</rdfs:comment>
        <rdfs:label>Situation-specific reward</rdfs:label>
    </owl:NamedIndividual>
    


    <!-- http://purl.bioontology.org/ontology/BCTT#Social_comparison -->

    <owl:NamedIndividual rdf:about="http://purl.bioontology.org/ontology/BCTT#Social_comparison">
        <rdf:type rdf:resource="http://purl.bioontology.org/ontology/BCTT#BehaviourChangeTechnique"/>
        <rdf:type rdf:resource="http://purl.bioontology.org/ontology/BCTT#00253"/>
        <EmpowerBP:isAppropriateForInterventionFunciton rdf:resource="http://www.semanticweb.org/tswheeler/ontologies/2016/3/EmpowerBP#Persuasion"/>
        <rdfs:comment>Draw attention to others’ performance to allow comparison with the person’s own performance 

Note: being in a group setting does not necessarily mean that social comparison is actually taking place</rdfs:comment>
        <rdfs:comment>Examples:

Show the doctor the proportion of patients who were prescribed antibiotics for a common cold by other doctors and compare with their own data</rdfs:comment>
        <rdfs:label>Social comparison</rdfs:label>
    </owl:NamedIndividual>
    


    <!-- http://purl.bioontology.org/ontology/BCTT#Social_incentive -->

    <owl:NamedIndividual rdf:about="http://purl.bioontology.org/ontology/BCTT#Social_incentive">
        <rdf:type rdf:resource="http://purl.bioontology.org/ontology/BCTT#BehaviourChangeTechnique"/>
        <rdf:type rdf:resource="http://purl.bioontology.org/ontology/BCTT#00278"/>
        <rdfs:comment>Examples:

Inform that they will be congratulated for each day they eat a reduced fat diet</rdfs:comment>
        <rdfs:comment>Inform that a verbal or non-verbal reward will be delivered if and only if there has been effort and/or progress in performing the behavior (includes ‘Positive reinforcement’)

Note: if incentive is material, code 10.1, Material incentive (behavior), if unspecified code 10.6, Non-specific incentive, and not 10.5, Social incentive; if incentive is for outcome code 10.8, Incentive (outcome). If reward is delivered also code one of: 10.2, Material reward (behavior); 10.3, Non-specific reward; 10.4, Social reward, 10.9, Self-reward; 10.10, Reward (outcome)</rdfs:comment>
        <rdfs:label>Social incentive</rdfs:label>
    </owl:NamedIndividual>
    


    <!-- http://purl.bioontology.org/ontology/BCTT#Social_reward -->

    <owl:NamedIndividual rdf:about="http://purl.bioontology.org/ontology/BCTT#Social_reward">
        <rdf:type rdf:resource="http://purl.bioontology.org/ontology/BCTT#BehaviourChangeTechnique"/>
        <rdf:type rdf:resource="http://purl.bioontology.org/ontology/BCTT#00278"/>
        <EmpowerBP:isAppropriateForInterventionFunciton rdf:resource="http://www.semanticweb.org/tswheeler/ontologies/2016/3/EmpowerBP#Incentivisation"/>
        <rdfs:comment>Arrange verbal or non-verbal reward if and only if there has been effort and/or progress in performing the behavior (includes ‘Positive reinforcement’)

Note: if reward is material, code 10.2, Material reward (behavior), if unspecified code 10.3, Non-specific reward, and not 10.4, Social reward; if reward is for outcome code 10.10, Reward (outcome). If informed of reward in advance of rewarded behaviour, also code one of: 10.1, Material incentive (behaviour); 10.5, Social incentive; 10.6, Non-specific incentive; 10.7, Self-incentive; 10.8, Incentive (outcome)</rdfs:comment>
        <rdfs:comment>Examples:

Congratulate the person for each day they eat a reduced fat diet</rdfs:comment>
        <rdfs:label>Social reward</rdfs:label>
    </owl:NamedIndividual>
    


    <!-- http://purl.bioontology.org/ontology/BCTT#Valued_self-identify -->

    <owl:NamedIndividual rdf:about="http://purl.bioontology.org/ontology/BCTT#Valued_self-identify">
        <rdf:type rdf:resource="http://purl.bioontology.org/ontology/BCTT#BehaviourChangeTechnique"/>
        <rdf:type rdf:resource="http://purl.bioontology.org/ontology/BCTT#00302"/>
        <EmpowerBP:isAppropriateForInterventionFunciton rdf:resource="http://www.semanticweb.org/tswheeler/ontologies/2016/3/EmpowerBP#Enablement"/>
        <rdfs:comment>Advise the person to write or complete rating scales about a cherished value or personal strength as a means of affirming the person’s identity as part of a behavior change strategy (includes ‘Self- affirmation’)</rdfs:comment>
        <rdfs:comment>Examples:

Advise the person to write about their personal strengths before they receive a message advocating the behavior change</rdfs:comment>
        <rdfs:label>Valued self-identify</rdfs:label>
    </owl:NamedIndividual>
    


    <!-- http://purl.bioontology.org/ontology/BCTT#Verbal_persuasion_about_capability -->

    <owl:NamedIndividual rdf:about="http://purl.bioontology.org/ontology/BCTT#Verbal_persuasion_about_capability">
        <rdf:type rdf:resource="http://purl.bioontology.org/ontology/BCTT#BehaviourChangeTechnique"/>
        <rdf:type rdf:resource="http://purl.bioontology.org/ontology/BCTT#00319"/>
        <EmpowerBP:isAppropriateForInterventionFunciton rdf:resource="http://www.semanticweb.org/tswheeler/ontologies/2016/3/EmpowerBP#Enablement"/>
        <EmpowerBP:isAppropriateForInterventionFunciton rdf:resource="http://www.semanticweb.org/tswheeler/ontologies/2016/3/EmpowerBP#Persuasion"/>
        <rdfs:comment>Examples:

Tell the person that they can successfully increase their physical activity, despite their recent heart attack.</rdfs:comment>
        <rdfs:comment>Tell the person that they can successfully perform the wanted behavior, arguing against self-doubts and asserting that they can and will succeed</rdfs:comment>
        <rdfs:label>Verbal persuasion about capability</rdfs:label>
    </owl:NamedIndividual>
    


    <!-- http://purl.bioontology.org/ontology/BCTT#Vicarious_consequences -->

    <owl:NamedIndividual rdf:about="http://purl.bioontology.org/ontology/BCTT#Vicarious_consequences">
        <rdf:type rdf:resource="http://purl.bioontology.org/ontology/BCTT#BehaviourChangeTechnique"/>
        <rdf:type rdf:resource="http://purl.bioontology.org/ontology/BCTT#00324"/>
        <EmpowerBP:isAppropriateForInterventionFunciton rdf:resource="http://www.semanticweb.org/tswheeler/ontologies/2016/3/EmpowerBP#Enablement"/>
        <rdfs:comment>Examples:

Draw attention to the positive comments other staff get when they disinfect their hands regularly</rdfs:comment>
        <rdfs:comment>Prompt observation of the consequences (including rewards and punishments) for others when they perform the behaviour

Note: if observation of health consequences, also code 5.1, Information about health consequences; if of emotional consequences, also code 5.6, Information about emotional consequences, if of social, environmental or unspecified consequences, also code 5.3, Information about social and environmental consequences</rdfs:comment>
        <rdfs:label>Vicarious consequences</rdfs:label>
    </owl:NamedIndividual>
    


    <!-- http://purl.bioontology.org/ontology/BCTT#Feedback_on_outcome(s)_of_behavior -->

    <owl:NamedIndividual rdf:about="http://purl.bioontology.org/ontology/BCTT#Feedback_on_outcome(s)_of_behavior">
        <rdf:type rdf:resource="http://purl.bioontology.org/ontology/BCTT#BehaviourChangeTechnique"/>
        <rdf:type rdf:resource="http://purl.bioontology.org/ontology/BCTT#00229"/>
        <EmpowerBP:isMostAppropriateForInterventionFunction rdf:resource="http://www.semanticweb.org/tswheeler/ontologies/2016/3/EmpowerBP#Coercion"/>
        <EmpowerBP:isMostAppropriateForInterventionFunction rdf:resource="http://www.semanticweb.org/tswheeler/ontologies/2016/3/EmpowerBP#Education"/>
        <EmpowerBP:isMostAppropriateForInterventionFunction rdf:resource="http://www.semanticweb.org/tswheeler/ontologies/2016/3/EmpowerBP#Incentivisation"/>
        <EmpowerBP:isMostAppropriateForInterventionFunction rdf:resource="http://www.semanticweb.org/tswheeler/ontologies/2016/3/EmpowerBP#Persuasion"/>
        <EmpowerBP:isMostAppropriateForInterventionFunction rdf:resource="http://www.semanticweb.org/tswheeler/ontologies/2016/3/EmpowerBP#Training"/>
        <rdfs:comment>Examples:

Inform the person of how much weight they have lost following the implementation of a new exercise regime</rdfs:comment>
        <rdfs:comment>Monitor and provide feedback on the outcome of performance of the behaviour

Note: if Biofeedback, code only 2.6, Biofeedback and not 2.7, Feedback on outcome(s) of behaviour; if feedback is on behaviour code 2.2, Feedback on behaviour; if there is no clear evidence that feedback was given code 2.5, Monitoring outcome(s) of behaviour by others without feedback; i ffeedback on behaviour is evaluative e.g. praise, also code 10.4, Social reward</rdfs:comment>
        <rdfs:label>Feedback on outcome(s) of behavior</rdfs:label>
    </owl:NamedIndividual>
    


    <!-- http://purl.bioontology.org/ontology/BCTT#Goal_setting_(behavior) -->

    <owl:NamedIndividual rdf:about="http://purl.bioontology.org/ontology/BCTT#Goal_setting_(behavior)">
        <rdf:type rdf:resource="http://purl.bioontology.org/ontology/BCTT#BehaviourChangeTechnique"/>
        <rdf:type rdf:resource="http://purl.bioontology.org/ontology/BCTT#00219"/>
        <EmpowerBP:isMostAppropriateForInterventionFunction rdf:resource="http://www.semanticweb.org/tswheeler/ontologies/2016/3/EmpowerBP#Enablement"/>
        <rdfs:comment>Examples:

Agree on a daily walking goal (e.g. 3 miles) with the person and reach agreement about the goal
Set the goal of eating 5 pieces of fruit per day as specified in public health guidelines</rdfs:comment>
        <rdfs:comment>Set or agree a goal defined in terms of the behaviour to be achieved. 

Note: only code g goal-setting if there is sufficient evidence that goal set as part of intervention; if goal unspecified or a behavioural outcome, code 1.3, Goal setting (outcome); if the goal defines a specific context, frequency, duration or intensity for the behaviour, also code 1.4, Action planning</rdfs:comment>
        <rdfs:label>Goal setting (behavior)</rdfs:label>
    </owl:NamedIndividual>
    


    <!-- http://purl.bioontology.org/ontology/BCTT#Goal_setting_(outcome) -->

    <owl:NamedIndividual rdf:about="http://purl.bioontology.org/ontology/BCTT#Goal_setting_(outcome)">
        <rdf:type rdf:resource="http://purl.bioontology.org/ontology/BCTT#BehaviourChangeTechnique"/>
        <rdf:type rdf:resource="http://purl.bioontology.org/ontology/BCTT#00219"/>
        <EmpowerBP:isMostAppropriateForInterventionFunction rdf:resource="http://www.semanticweb.org/tswheeler/ontologies/2016/3/EmpowerBP#Enablement"/>
        <rdfs:comment>Examples:

Set a weight loss goal (e.g. 0.5 kilogram over one week) as an outcome of changed eating patterns</rdfs:comment>
        <rdfs:comment>Set or agree a goal defined in terms of a positive outcome of wanted behaviour

Note: only code guidelines if set as a goal in an intervention context; if goal is a behaviour, code 1.1, Goal setting (behaviour); if goal unspecified code 1.3, Goal setting (outcome)</rdfs:comment>
        <rdfs:label>Goal setting (outcome)</rdfs:label>
    </owl:NamedIndividual>
    


    <!-- http://purl.bioontology.org/ontology/BCTT#Incentive_(outcome) -->

    <owl:NamedIndividual rdf:about="http://purl.bioontology.org/ontology/BCTT#Incentive_(outcome)">
        <rdf:type rdf:resource="http://purl.bioontology.org/ontology/BCTT#BehaviourChangeTechnique"/>
        <rdf:type rdf:resource="http://purl.bioontology.org/ontology/BCTT#00278"/>
        <EmpowerBP:isAppropriateForInterventionFunciton rdf:resource="http://www.semanticweb.org/tswheeler/ontologies/2016/3/EmpowerBP#Incentivisation"/>
        <rdfs:comment>Examples:

Inform the person that they will receive money if and only if a certain amount of weight is lost</rdfs:comment>
        <rdfs:comment>Inform that a reward will be delivered if and only if there has been effort and/or progress in achieving the behavioural outcome (includes ‘Positive reinforcement’)

Note: this includes social, material, self- and non-specific incentives for outcome; if incentive is for the behavior code 10.5, Social incentive, 10.1, Material incentive (behavior), 10.6, Non-specific incentive or 10.7, Self-incentive and not 10.8, Incentive (outcome). If reward is delivered also code one of: 10.2, Material reward (behavior); 10.3, Non-specific reward; 10.4, Social reward, 10.9, Self-reward; 10.10, Reward (outcome)</rdfs:comment>
        <rdfs:label>Incentive (outcome)</rdfs:label>
    </owl:NamedIndividual>
    


    <!-- http://purl.bioontology.org/ontology/BCTT#Information_about_others&apos;_approval -->

    <owl:NamedIndividual rdf:about="http://purl.bioontology.org/ontology/BCTT#Information_about_others&apos;_approval">
        <rdf:type rdf:resource="http://purl.bioontology.org/ontology/BCTT#BehaviourChangeTechnique"/>
        <rdf:type rdf:resource="http://purl.bioontology.org/ontology/BCTT#00253"/>
        <EmpowerBP:isAppropriateForInterventionFunciton rdf:resource="http://www.semanticweb.org/tswheeler/ontologies/2016/3/EmpowerBP#Education"/>
        <EmpowerBP:isAppropriateForInterventionFunciton rdf:resource="http://www.semanticweb.org/tswheeler/ontologies/2016/3/EmpowerBP#Persuasion"/>
        <rdfs:comment>Examples:

Tell the staff at the hospital ward that staff at all other wards approve of washing their hands according to the guidelines</rdfs:comment>
        <rdfs:comment>Provide information about what other people think about the behavior. The information clarifies whether others will like, approve or disapprove of what the person is doing or will do</rdfs:comment>
        <rdfs:label>Information about others&apos; approval</rdfs:label>
    </owl:NamedIndividual>
    


    <!-- http://purl.bioontology.org/ontology/BCTT#Material_incentive_(behavior) -->

    <owl:NamedIndividual rdf:about="http://purl.bioontology.org/ontology/BCTT#Material_incentive_(behavior)">
        <rdf:type rdf:resource="http://purl.bioontology.org/ontology/BCTT#BehaviourChangeTechnique"/>
        <rdf:type rdf:resource="http://purl.bioontology.org/ontology/BCTT#00278"/>
        <rdfs:comment>Examples:

Inform that a financial payment will be made each month in pregnancy that the woman has not smoked</rdfs:comment>
        <rdfs:comment>Inform that money, vouchers or other valued objects will be delivered if and only if there has been effort and/or progress in performing the behavior (includes ‘Positive reinforcement’)

Note: if incentive is social, code 10.5, Social incentive if unspecified code 10.6, Non-specific incentive, and not 10.1, Material incentive (behavior); if incentive is for outcome, code 10.8, Incentive (outcome). If reward is delivered also code one of: 10.2, Material reward (behavior); 10.3, Non-specific reward; 10.4, Social reward, 10.9, Self-reward; 10.10, Reward (outcome)</rdfs:comment>
        <rdfs:label>Material incentive (behavior)</rdfs:label>
    </owl:NamedIndividual>
    


    <!-- http://purl.bioontology.org/ontology/BCTT#Material_reward_(behavior) -->

    <owl:NamedIndividual rdf:about="http://purl.bioontology.org/ontology/BCTT#Material_reward_(behavior)">
        <rdf:type rdf:resource="http://purl.bioontology.org/ontology/BCTT#BehaviourChangeTechnique"/>
        <rdf:type rdf:resource="http://purl.bioontology.org/ontology/BCTT#00278"/>
        <EmpowerBP:isAppropriateForInterventionFunciton rdf:resource="http://www.semanticweb.org/tswheeler/ontologies/2016/3/EmpowerBP#Incentivisation"/>
        <rdfs:comment>Arrange for the delivery of money, vouchers or other valued objects if and only if there has been effort and/or progress in performing the behavior (includes ‘Positive reinforcement’)

Note: If reward is social, code 10.4, Social reward, if unspecified code 10.3, Non- specific reward, and not 10.1, Material reward (behavior); if reward is for outcome, code 10.10, Reward (outcome). If informed of reward in advance of rewarded behaviour, also code one of: 10.1, Material incentive (behaviour); 10.5, Social incentive; 10.6, Non-specific incentive; 10.7, Self-incentive; 10.8, Incentive (outcome)</rdfs:comment>
        <rdfs:comment>Examples:

Arrange for the person to receive money that would have been spent on cigarettes if and only if the smoker has not smoked for one month</rdfs:comment>
        <rdfs:label>Material reward (behavior)</rdfs:label>
    </owl:NamedIndividual>
    


    <!-- http://purl.bioontology.org/ontology/BCTT#Monitoring_of_outcome(s)_of_behavior_without_feedback -->

    <owl:NamedIndividual rdf:about="http://purl.bioontology.org/ontology/BCTT#Monitoring_of_outcome(s)_of_behavior_without_feedback">
        <rdf:type rdf:resource="http://purl.bioontology.org/ontology/BCTT#BehaviourChangeTechnique"/>
        <rdf:type rdf:resource="http://purl.bioontology.org/ontology/BCTT#00229"/>
        <EmpowerBP:isMostAppropriateForInterventionFunction rdf:resource="http://www.semanticweb.org/tswheeler/ontologies/2016/3/EmpowerBP#Coercion"/>
        <EmpowerBP:isMostAppropriateForInterventionFunction rdf:resource="http://www.semanticweb.org/tswheeler/ontologies/2016/3/EmpowerBP#Incentivisation"/>
        <rdfs:comment>Examples:

Record blood pressure, blood glucose, weight loss, or physical fitness</rdfs:comment>
        <rdfs:comment>Observe or record outcomes of behaviour with the person&apos;s knowledge as part of a behaviour change strategy

Note: if monitoring is part of a data collection procedure rather than a strategy aimed at changing behaviour, do not code; if feedback given, code only 2.7, Feedback on outcome(s) of behaviour; if monitoring behaviour code 2.1, Monitoring of behaviour by others without feedback; if self-monitoring outcome(s), code 2.4, Self-monitoring of outcome(s) of behaviour</rdfs:comment>
        <rdfs:label>Monitoring of outcome(s) of behavior without feedback</rdfs:label>
    </owl:NamedIndividual>
    


    <!-- http://purl.bioontology.org/ontology/BCTT#Review_behavior_goal(s) -->

    <owl:NamedIndividual rdf:about="http://purl.bioontology.org/ontology/BCTT#Review_behavior_goal(s)">
        <rdf:type rdf:resource="http://purl.bioontology.org/ontology/BCTT#BehaviourChangeTechnique"/>
        <rdf:type rdf:resource="http://purl.bioontology.org/ontology/BCTT#00219"/>
        <EmpowerBP:isMostAppropriateForInterventionFunction rdf:resource="http://www.semanticweb.org/tswheeler/ontologies/2016/3/EmpowerBP#Enablement"/>
        <rdfs:comment>Examples:

Examine how well a person’s performance corresponds to agreed goals e.g. whether they consumed less than one unit of alcohol per day, and consider modifying future behavioral goals accordingly e.g. by increasing or decreasing alcohol target or changing type of alcohol consumed</rdfs:comment>
        <rdfs:comment>Review behaviour goal(s) jointly with the person and consider modifying goal(s) or behaviour change strategy in light of achievement. This may lead to re-setting the same goal, a small change in that goal or setting a new goal instead of (or in addition to) the first, or no change

Note: if goal specified in terms of behaviour, code 1.5, Review behaviour goal(s), if goal unspecified, code 1.7, Review outcome goal(s); if discrepancy created consider also 1.6, Discrepancy between current behaviour and goal</rdfs:comment>
        <rdfs:label>Review behavior goal(s)</rdfs:label>
    </owl:NamedIndividual>
    


    <!-- http://purl.bioontology.org/ontology/BCTT#Review_outcome_goal(s) -->

    <owl:NamedIndividual rdf:about="http://purl.bioontology.org/ontology/BCTT#Review_outcome_goal(s)">
        <rdf:type rdf:resource="http://purl.bioontology.org/ontology/BCTT#BehaviourChangeTechnique"/>
        <rdf:type rdf:resource="http://purl.bioontology.org/ontology/BCTT#00219"/>
        <EmpowerBP:isMostAppropriateForInterventionFunction rdf:resource="http://www.semanticweb.org/tswheeler/ontologies/2016/3/EmpowerBP#Enablement"/>
        <rdfs:comment>Examples:

Examine how much weight has been lost and consider modifying outcome goal(s) accordingly e.g., by increasing or decreasing subsequent weight loss targets</rdfs:comment>
        <rdfs:comment>Review outcome goal(s) jointly with the person and consider modifying goal(s) in light of achievement. This may lead to re-setting the same goal, a small change in that goal or setting a new goal instead of, or in addition to the first

Note: if goal specified in terms of behaviour, code 1.5, Review behaviour goal(s), if goal unspecified, code 1.7, Review outcome goal(s); if discrepancy created consider also 1.6, Discrepancy between current behaviour and goal</rdfs:comment>
        <rdfs:label>Review outcome goal(s)</rdfs:label>
    </owl:NamedIndividual>
    


    <!-- http://purl.bioontology.org/ontology/BCTT#Reward_(outcome) -->

    <owl:NamedIndividual rdf:about="http://purl.bioontology.org/ontology/BCTT#Reward_(outcome)">
        <rdf:type rdf:resource="http://purl.bioontology.org/ontology/BCTT#BehaviourChangeTechnique"/>
        <rdf:type rdf:resource="http://purl.bioontology.org/ontology/BCTT#00278"/>
        <rdfs:comment>Arrange for the delivery of a reward if and only if there has been effort and/or progress in achieving the behavioral outcome (includes ‘Positive reinforcement’)

Note: this includes social, material, self- and non-specific rewards for outcome; if reward is for the behavior code 10.4, Social reward, 10.2, Material reward (behavior), 10.3, Non-specific reward or 10.9, Self-reward and not 10.10, Reward (outcome). If informed of reward in advance of rewarded behaviour, also code one of: 10.1, Material incentive (behaviour); 10.5, Social incentive; 10.6, Non-specific incentive; 10.7, Self- incentive; 10.8, Incentive (outcome)</rdfs:comment>
        <rdfs:comment>Examples:

Arrange for the person to receive money if and only if a certain amount of weight is lost</rdfs:comment>
        <rdfs:label>Reward (outcome)</rdfs:label>
    </owl:NamedIndividual>
    


    <!-- http://purl.bioontology.org/ontology/BCTT#Self-monitoring_of_outcome(s)_of_behaviour -->

    <owl:NamedIndividual rdf:about="http://purl.bioontology.org/ontology/BCTT#Self-monitoring_of_outcome(s)_of_behaviour">
        <rdf:type rdf:resource="http://purl.bioontology.org/ontology/BCTT#BehaviourChangeTechnique"/>
        <rdf:type rdf:resource="http://purl.bioontology.org/ontology/BCTT#00229"/>
        <EmpowerBP:isAppropriateForInterventionFunciton rdf:resource="http://www.semanticweb.org/tswheeler/ontologies/2016/3/EmpowerBP#Coercion"/>
        <EmpowerBP:isAppropriateForInterventionFunciton rdf:resource="http://www.semanticweb.org/tswheeler/ontologies/2016/3/EmpowerBP#Education"/>
        <EmpowerBP:isAppropriateForInterventionFunciton rdf:resource="http://www.semanticweb.org/tswheeler/ontologies/2016/3/EmpowerBP#Enablement"/>
        <EmpowerBP:isAppropriateForInterventionFunciton rdf:resource="http://www.semanticweb.org/tswheeler/ontologies/2016/3/EmpowerBP#Incentivisation"/>
        <EmpowerBP:isAppropriateForInterventionFunciton rdf:resource="http://www.semanticweb.org/tswheeler/ontologies/2016/3/EmpowerBP#Training"/>
        <rdfs:comment>Establish a method for the person to monitor and record the outcome(s) of their behaviour as part of a behaviour change strategy

Note: if monitoring is part of a data collection procedure rather than a strategy aimed at changing behaviour, do not code ; if monitoring behaviour, code 2.3, Self-monitoring of behaviour; if monitoring is by someone else (without feedback), code 2.5, Monitoring outcome(s) of behaviour by others without feedback</rdfs:comment>
        <rdfs:comment>Examples:

Ask the person to weigh themselves at the end of each day, over a two week period, and record their daily weight on a graph to increase exercise behaviors</rdfs:comment>
        <rdfs:label>Self-monitoring of outcome(s) of behaviour</rdfs:label>
    </owl:NamedIndividual>
    


    <!-- http://purl.bioontology.org/ontology/BCTT#Social_support_(emotional) -->

    <owl:NamedIndividual rdf:about="http://purl.bioontology.org/ontology/BCTT#Social_support_(emotional)">
        <rdf:type rdf:resource="http://purl.bioontology.org/ontology/BCTT#BehaviourChangeTechnique"/>
        <rdf:type rdf:resource="http://purl.bioontology.org/ontology/BCTT#00237"/>
        <EmpowerBP:isAppropriateForInterventionFunciton rdf:resource="http://www.semanticweb.org/tswheeler/ontologies/2016/3/EmpowerBP#Enablement"/>
        <rdfs:comment>Advise on, arrange, or provide emotional social support (e.g. from friends, relatives, colleagues, &apos;buddies&apos; or staff) for performance of the behaviour

Note: if practical, code 3.2, Social support (practical); if unspecified, code 3.1, Social support (unspecified)</rdfs:comment>
        <rdfs:comment>Examples:

Ask the patient to take a partner or friend with them to their colonoscopy appointment</rdfs:comment>
        <rdfs:label>Social support (emotional)</rdfs:label>
    </owl:NamedIndividual>
    


    <!-- http://purl.bioontology.org/ontology/BCTT#Social_support_(practical) -->

    <owl:NamedIndividual rdf:about="http://purl.bioontology.org/ontology/BCTT#Social_support_(practical)">
        <rdf:type rdf:resource="http://purl.bioontology.org/ontology/BCTT#BehaviourChangeTechnique"/>
        <rdf:type rdf:resource="http://purl.bioontology.org/ontology/BCTT#00237"/>
        <EmpowerBP:isMostAppropriateForInterventionFunction rdf:resource="http://www.semanticweb.org/tswheeler/ontologies/2016/3/EmpowerBP#Enablement"/>
        <rdfs:comment>Advise on, arrange, or provide practical help (e.g. from friends, relatives, colleagues, &apos;buddies&apos; or staff) for performance of the behaviour

Note: if emotional, code 3.3, Social support (emotional); if general or unspecified, code 3.1, Social support (unspecified) If only restructuring the physical environment or adding objects to the environment, code 12.1, Restructuring the physical environment or 12.5, Adding objects to the environment; attending a group or class and/or mention of follow-up&apos; does not necessarily apply this BCT, support must be explicitly mentioned.</rdfs:comment>
        <rdfs:comment>Examples:

Ask the partner of the patient to put their tablet on the breakfast tray so that the patient remembers to take it</rdfs:comment>
        <rdfs:label>Social support (practical)</rdfs:label>
    </owl:NamedIndividual>
    


    <!-- http://purl.bioontology.org/ontology/BCTT#Social_support_(unspecified) -->

    <owl:NamedIndividual rdf:about="http://purl.bioontology.org/ontology/BCTT#Social_support_(unspecified)">
        <rdf:type rdf:resource="http://purl.bioontology.org/ontology/BCTT#BehaviourChangeTechnique"/>
        <rdf:type rdf:resource="http://purl.bioontology.org/ontology/BCTT#00237"/>
        <EmpowerBP:isMostAppropriateForInterventionFunction rdf:resource="http://www.semanticweb.org/tswheeler/ontologies/2016/3/EmpowerBP#Enablement"/>
        <rdfs:comment>Advise on, arrange or provide social support (e.g. from friends, relatives, colleagues,&apos; buddies&apos; or staff) or non-contingent praise or reward for performance of the behaviour. It includes encouragement and counselling, but only when it is directed at the behaviour

Note: attending a group class and/ or mention of &apos;follow-up&apos; does not necessarily apply this BCT, support must be explicitly mentioned; if practical, code 3.2, Social support (practical); if emotional, code 3.3, Social support (emotional) (includes &apos;Motivational  interviewing&apos; and &apos;Cognitive  Behavioural Therapy&apos;)</rdfs:comment>
        <rdfs:comment>Examples:

Advise the person to call a ‘buddy’ when they experience an urge to smoke
Arrange for a housemate to encourage continuation with the behavior change programme
Give information about a self- help group that offers support for the behaviour</rdfs:comment>
        <rdfs:label>Social support (unspecified)</rdfs:label>
    </owl:NamedIndividual>
    


    <!-- http://www.semanticweb.org/tswheeler/ontologies/2016/3/EmpowerBP#AgeObstacle -->

    <owl:NamedIndividual rdf:about="http://www.semanticweb.org/tswheeler/ontologies/2016/3/EmpowerBP#AgeObstacle">
        <rdf:type rdf:resource="http://www.semanticweb.org/tswheeler/ontologies/2016/3/EmpowerBP#Obstacle"/>
        <EmpowerBP:hasRelevantTDF rdf:resource="http://www.semanticweb.org/tswheeler/ontologies/2016/3/EmpowerBP#BeliefsAboutCapability"/>
        <EmpowerBP:hasRelevantTDF rdf:resource="http://www.semanticweb.org/tswheeler/ontologies/2016/3/EmpowerBP#Knowledge"/>
        <EmpowerBP:hasRelevantTDF rdf:resource="http://www.semanticweb.org/tswheeler/ontologies/2016/3/EmpowerBP#Optimism"/>
        <EmpowerBP:hasRelevantTDF rdf:resource="http://www.semanticweb.org/tswheeler/ontologies/2016/3/EmpowerBP#PhysicalSkill"/>
        <rdfs:comment>Feels &quot;too old&quot; to perform activity.</rdfs:comment>
    </owl:NamedIndividual>
    


    <!-- http://www.semanticweb.org/tswheeler/ontologies/2016/3/EmpowerBP#AutomaticMotivation -->

    <owl:NamedIndividual rdf:about="http://www.semanticweb.org/tswheeler/ontologies/2016/3/EmpowerBP#AutomaticMotivation">
        <rdf:type rdf:resource="http://www.semanticweb.org/tswheeler/ontologies/2016/3/EmpowerBP#COMBConstruct"/>
        <rdf:type rdf:resource="http://www.semanticweb.org/tswheeler/ontologies/2016/3/EmpowerBP#Construct"/>
        <rdf:type rdf:resource="http://www.semanticweb.org/tswheeler/ontologies/2016/3/EmpowerBP#Motivation"/>
        <EmpowerBP:isRelatedToTDF rdf:resource="http://www.semanticweb.org/tswheeler/ontologies/2016/3/EmpowerBP#Emotion"/>
        <EmpowerBP:isRelatedToTDF rdf:resource="http://www.semanticweb.org/tswheeler/ontologies/2016/3/EmpowerBP#Reinforcement"/>
        <rdfs:comment>Processes involving wants and needs, desires, impulses and reflex responses</rdfs:comment>
    </owl:NamedIndividual>
    


    <!-- http://www.semanticweb.org/tswheeler/ontologies/2016/3/EmpowerBP#BehaviouralRegulation -->

    <owl:NamedIndividual rdf:about="http://www.semanticweb.org/tswheeler/ontologies/2016/3/EmpowerBP#BehaviouralRegulation">
        <rdf:type rdf:resource="http://www.semanticweb.org/tswheeler/ontologies/2016/3/EmpowerBP#Construct"/>
        <rdf:type rdf:resource="http://www.semanticweb.org/tswheeler/ontologies/2016/3/EmpowerBP#TDFDomain"/>
        <EmpowerBP:hasEffectiveInterventionFunction rdf:resource="http://www.semanticweb.org/tswheeler/ontologies/2016/3/EmpowerBP#Education"/>
        <EmpowerBP:hasEffectiveInterventionFunction rdf:resource="http://www.semanticweb.org/tswheeler/ontologies/2016/3/EmpowerBP#Enablement"/>
        <EmpowerBP:hasEffectiveInterventionFunction rdf:resource="http://www.semanticweb.org/tswheeler/ontologies/2016/3/EmpowerBP#Modelling"/>
        <EmpowerBP:hasEffectiveInterventionFunction rdf:resource="http://www.semanticweb.org/tswheeler/ontologies/2016/3/EmpowerBP#Training"/>
        <EmpowerBP:isRelatedToCOMB rdf:resource="http://www.semanticweb.org/tswheeler/ontologies/2016/3/EmpowerBP#PsychologicalCapability"/>
        <rdfs:comment>Anything aimed at managing or changing objectively observed or measured actions</rdfs:comment>
    </owl:NamedIndividual>
    


    <!-- http://www.semanticweb.org/tswheeler/ontologies/2016/3/EmpowerBP#BeliefsAboutCapability -->

    <owl:NamedIndividual rdf:about="http://www.semanticweb.org/tswheeler/ontologies/2016/3/EmpowerBP#BeliefsAboutCapability">
        <rdf:type rdf:resource="http://www.semanticweb.org/tswheeler/ontologies/2016/3/EmpowerBP#Construct"/>
        <rdf:type rdf:resource="http://www.semanticweb.org/tswheeler/ontologies/2016/3/EmpowerBP#TDFDomain"/>
        <EmpowerBP:hasEffectiveInterventionFunction rdf:resource="http://www.semanticweb.org/tswheeler/ontologies/2016/3/EmpowerBP#Education"/>
        <EmpowerBP:hasEffectiveInterventionFunction rdf:resource="http://www.semanticweb.org/tswheeler/ontologies/2016/3/EmpowerBP#Enablement"/>
        <EmpowerBP:hasEffectiveInterventionFunction rdf:resource="http://www.semanticweb.org/tswheeler/ontologies/2016/3/EmpowerBP#Modelling"/>
        <EmpowerBP:hasEffectiveInterventionFunction rdf:resource="http://www.semanticweb.org/tswheeler/ontologies/2016/3/EmpowerBP#Persuasion"/>
        <EmpowerBP:isRelatedToCOMB rdf:resource="http://www.semanticweb.org/tswheeler/ontologies/2016/3/EmpowerBP#ReflectiveMotivation"/>
        <rdfs:comment>Acceptance of the truth, reality, or validity about an ability, talent, or facility that a person can put to constructive use</rdfs:comment>
    </owl:NamedIndividual>
    


    <!-- http://www.semanticweb.org/tswheeler/ontologies/2016/3/EmpowerBP#BeliefsAboutConsequences -->

    <owl:NamedIndividual rdf:about="http://www.semanticweb.org/tswheeler/ontologies/2016/3/EmpowerBP#BeliefsAboutConsequences">
        <rdf:type rdf:resource="http://www.semanticweb.org/tswheeler/ontologies/2016/3/EmpowerBP#Construct"/>
        <rdf:type rdf:resource="http://www.semanticweb.org/tswheeler/ontologies/2016/3/EmpowerBP#TDFDomain"/>
        <EmpowerBP:hasEffectiveInterventionFunction rdf:resource="http://www.semanticweb.org/tswheeler/ontologies/2016/3/EmpowerBP#Education"/>
        <EmpowerBP:hasEffectiveInterventionFunction rdf:resource="http://www.semanticweb.org/tswheeler/ontologies/2016/3/EmpowerBP#Modelling"/>
        <EmpowerBP:hasEffectiveInterventionFunction rdf:resource="http://www.semanticweb.org/tswheeler/ontologies/2016/3/EmpowerBP#Persuasion"/>
        <EmpowerBP:isRelatedToCOMB rdf:resource="http://www.semanticweb.org/tswheeler/ontologies/2016/3/EmpowerBP#ReflectiveMotivation"/>
        <rdfs:comment>Acceptance of the truth, reality, or validity about outcomes of a behaviour in a given situation</rdfs:comment>
    </owl:NamedIndividual>
    


    <!-- http://www.semanticweb.org/tswheeler/ontologies/2016/3/EmpowerBP#Coercion -->

    <owl:NamedIndividual rdf:about="http://www.semanticweb.org/tswheeler/ontologies/2016/3/EmpowerBP#Coercion">
        <rdf:type rdf:resource="http://www.semanticweb.org/tswheeler/ontologies/2016/3/EmpowerBP#InterventionFuction"/>
        <EmpowerBP:hasCommonBCT rdf:resource="http://purl.bioontology.org/ontology/BCTT#Anticipated_regret"/>
        <EmpowerBP:hasCommonBCT rdf:resource="http://purl.bioontology.org/ontology/BCTT#Behavior_cost"/>
        <EmpowerBP:hasCommonBCT rdf:resource="http://purl.bioontology.org/ontology/BCTT#Behavioral_contract"/>
        <EmpowerBP:hasCommonBCT rdf:resource="http://purl.bioontology.org/ontology/BCTT#Biofeedback"/>
        <EmpowerBP:hasCommonBCT rdf:resource="http://purl.bioontology.org/ontology/BCTT#Commitment"/>
        <EmpowerBP:hasCommonBCT rdf:resource="http://purl.bioontology.org/ontology/BCTT#Discrepancy_between_current_behavior_and_goal"/>
        <EmpowerBP:hasCommonBCT rdf:resource="http://purl.bioontology.org/ontology/BCTT#Future_punishment"/>
        <EmpowerBP:hasCommonBCT rdf:resource="http://purl.bioontology.org/ontology/BCTT#Imaginary_punishment"/>
        <EmpowerBP:hasCommonBCT rdf:resource="http://purl.bioontology.org/ontology/BCTT#Incompatible_beliefs"/>
        <EmpowerBP:hasCommonBCT rdf:resource="http://purl.bioontology.org/ontology/BCTT#Punishment"/>
        <EmpowerBP:hasCommonBCT rdf:resource="http://purl.bioontology.org/ontology/BCTT#Remove_access_to_the_reward"/>
        <EmpowerBP:hasCommonBCT rdf:resource="http://purl.bioontology.org/ontology/BCTT#Remove_reward"/>
        <EmpowerBP:hasCommonBCT rdf:resource="http://purl.bioontology.org/ontology/BCTT#Self-monitoring_of_outcome(s)_of_behaviour"/>
        <EmpowerBP:hasMostCommonBCT rdf:resource="http://purl.bioontology.org/ontology/BCTT#Feedback_on_behaviour"/>
        <EmpowerBP:hasMostCommonBCT rdf:resource="http://purl.bioontology.org/ontology/BCTT#Monitoring_of_behavior_by_others_without_feedback"/>
        <EmpowerBP:hasMostCommonBCT rdf:resource="http://purl.bioontology.org/ontology/BCTT#Self-monitoring_of_behaviour"/>
        <EmpowerBP:hasMostCommonBCT rdf:resource="http://purl.bioontology.org/ontology/BCTT#Feedback_on_outcome(s)_of_behavior"/>
        <EmpowerBP:hasMostCommonBCT rdf:resource="http://purl.bioontology.org/ontology/BCTT#Monitoring_of_outcome(s)_of_behavior_without_feedback"/>
        <EmpowerBP:isEffectiveForTDFDomain rdf:resource="http://www.semanticweb.org/tswheeler/ontologies/2016/3/EmpowerBP#Emotion"/>
        <EmpowerBP:isEffectiveForTDFDomain rdf:resource="http://www.semanticweb.org/tswheeler/ontologies/2016/3/EmpowerBP#Goals"/>
        <EmpowerBP:isEffectiveForTDFDomain rdf:resource="http://www.semanticweb.org/tswheeler/ontologies/2016/3/EmpowerBP#Intentions"/>
        <EmpowerBP:isEffectiveForTDFDomain rdf:resource="http://www.semanticweb.org/tswheeler/ontologies/2016/3/EmpowerBP#Reinforcement"/>
        <rdfs:comment>Creating an expectation of punishment or cost.</rdfs:comment>
    </owl:NamedIndividual>
    


    <!-- http://www.semanticweb.org/tswheeler/ontologies/2016/3/EmpowerBP#CognitiveInterpersonalSkills -->

    <owl:NamedIndividual rdf:about="http://www.semanticweb.org/tswheeler/ontologies/2016/3/EmpowerBP#CognitiveInterpersonalSkills">
        <rdf:type rdf:resource="http://www.semanticweb.org/tswheeler/ontologies/2016/3/EmpowerBP#Construct"/>
        <rdf:type rdf:resource="http://www.semanticweb.org/tswheeler/ontologies/2016/3/EmpowerBP#TDFDomain"/>
        <EmpowerBP:hasEffectiveInterventionFunction rdf:resource="http://www.semanticweb.org/tswheeler/ontologies/2016/3/EmpowerBP#Training"/>
        <EmpowerBP:isRelatedToCOMB rdf:resource="http://www.semanticweb.org/tswheeler/ontologies/2016/3/EmpowerBP#PsychologicalCapability"/>
        <rdfs:comment>Cognitive or interpersonal abilities or proficiencies acquired through practice</rdfs:comment>
    </owl:NamedIndividual>
    


    <!-- http://www.semanticweb.org/tswheeler/ontologies/2016/3/EmpowerBP#ConfidenceObstacle -->

    <owl:NamedIndividual rdf:about="http://www.semanticweb.org/tswheeler/ontologies/2016/3/EmpowerBP#ConfidenceObstacle">
        <rdf:type rdf:resource="http://www.semanticweb.org/tswheeler/ontologies/2016/3/EmpowerBP#Obstacle"/>
        <EmpowerBP:hasRelevantTDF rdf:resource="http://www.semanticweb.org/tswheeler/ontologies/2016/3/EmpowerBP#BeliefsAboutCapability"/>
        <EmpowerBP:hasRelevantTDF rdf:resource="http://www.semanticweb.org/tswheeler/ontologies/2016/3/EmpowerBP#Emotion"/>
        <EmpowerBP:hasRelevantTDF rdf:resource="http://www.semanticweb.org/tswheeler/ontologies/2016/3/EmpowerBP#Knowledge"/>
        <EmpowerBP:hasRelevantTDF rdf:resource="http://www.semanticweb.org/tswheeler/ontologies/2016/3/EmpowerBP#Optimism"/>
        <EmpowerBP:hasRelevantTDF rdf:resource="http://www.semanticweb.org/tswheeler/ontologies/2016/3/EmpowerBP#PhysicalSkill"/>
        <rdfs:comment>Lacks confidence in ability to perform activity.</rdfs:comment>
    </owl:NamedIndividual>
    


    <!-- http://www.semanticweb.org/tswheeler/ontologies/2016/3/EmpowerBP#ConvenienceObstacle -->

    <owl:NamedIndividual rdf:about="http://www.semanticweb.org/tswheeler/ontologies/2016/3/EmpowerBP#ConvenienceObstacle">
        <rdf:type rdf:resource="http://www.semanticweb.org/tswheeler/ontologies/2016/3/EmpowerBP#Obstacle"/>
        <EmpowerBP:hasRelevantTDF rdf:resource="http://www.semanticweb.org/tswheeler/ontologies/2016/3/EmpowerBP#BehaviouralRegulation"/>
        <EmpowerBP:hasRelevantTDF rdf:resource="http://www.semanticweb.org/tswheeler/ontologies/2016/3/EmpowerBP#BeliefsAboutConsequences"/>
        <EmpowerBP:hasRelevantTDF rdf:resource="http://www.semanticweb.org/tswheeler/ontologies/2016/3/EmpowerBP#EnvironmentalContextResources"/>
        <EmpowerBP:hasRelevantTDF rdf:resource="http://www.semanticweb.org/tswheeler/ontologies/2016/3/EmpowerBP#Goals"/>
        <EmpowerBP:hasRelevantTDF rdf:resource="http://www.semanticweb.org/tswheeler/ontologies/2016/3/EmpowerBP#Reinforcement"/>
        <rdfs:comment>Feels that activity is too inconvenient. Having time to do the activity is not an issue (see TimeObstacle).</rdfs:comment>
    </owl:NamedIndividual>
    


    <!-- http://www.semanticweb.org/tswheeler/ontologies/2016/3/EmpowerBP#EMAM1 -->

    <owl:NamedIndividual rdf:about="http://www.semanticweb.org/tswheeler/ontologies/2016/3/EmpowerBP#EMAM1">
        <rdf:type rdf:resource="http://www.semanticweb.org/tswheeler/ontologies/2016/3/EmpowerBP#AssessmentItem"/>
        <rdf:type rdf:resource="http://www.semanticweb.org/tswheeler/ontologies/2016/3/EmpowerBP#COMBAssessmentItem"/>
        <EmpowerBP:canAssessCOMBConstruct rdf:resource="http://www.semanticweb.org/tswheeler/ontologies/2016/3/EmpowerBP#AutomaticMotivation"/>
        <EmpowerBP:isSpecificToGoal rdf:resource="http://www.semanticweb.org/tswheeler/ontologies/2016/3/EmpowerBP#ExerciseMore"/>
        <EmpowerBP:assessmentItemExamples rdf:datatype="http://www.w3.org/2001/XMLSchema#string">• Learn how to feel more of a sense of pleasure or satisfaction from exercising.</EmpowerBP:assessmentItemExamples>
        <EmpowerBP:assessmentItemID rdf:datatype="http://www.w3.org/2001/XMLSchema#string">EMAM1</EmpowerBP:assessmentItemID>
        <EmpowerBP:assessmentItemText rdf:datatype="http://www.w3.org/2001/XMLSchema#string">It would help if I could increase my drive or desire to be more active.</EmpowerBP:assessmentItemText>
        <rdfs:comment rdf:datatype="http://www.w3.org/2001/XMLSchema#string">It would help if I could increase my drive or desire to be more active.</rdfs:comment>
        <rdfs:label rdf:datatype="http://www.w3.org/2001/XMLSchema#string">EMAM1</rdfs:label>
    </owl:NamedIndividual>
    


    <!-- http://www.semanticweb.org/tswheeler/ontologies/2016/3/EmpowerBP#EMAM2 -->

    <owl:NamedIndividual rdf:about="http://www.semanticweb.org/tswheeler/ontologies/2016/3/EmpowerBP#EMAM2">
        <rdf:type rdf:resource="http://www.semanticweb.org/tswheeler/ontologies/2016/3/EmpowerBP#AssessmentItem"/>
        <rdf:type rdf:resource="http://www.semanticweb.org/tswheeler/ontologies/2016/3/EmpowerBP#COMBAssessmentItem"/>
        <EmpowerBP:canAssessCOMBConstruct rdf:resource="http://www.semanticweb.org/tswheeler/ontologies/2016/3/EmpowerBP#AutomaticMotivation"/>
        <EmpowerBP:isSpecificToGoal rdf:resource="http://www.semanticweb.org/tswheeler/ontologies/2016/3/EmpowerBP#ExerciseMore"/>
        <EmpowerBP:assessmentItemExamples rdf:datatype="http://www.w3.org/2001/XMLSchema#string">• Learn how to care more about the negative consequences of not exercising regularly.</EmpowerBP:assessmentItemExamples>
        <EmpowerBP:assessmentItemID rdf:datatype="http://www.w3.org/2001/XMLSchema#string">EMAM2</EmpowerBP:assessmentItemID>
        <EmpowerBP:assessmentItemText rdf:datatype="http://www.w3.org/2001/XMLSchema#string">It would help if I could make being active feel more important to me.</EmpowerBP:assessmentItemText>
        <rdfs:comment rdf:datatype="http://www.w3.org/2001/XMLSchema#string">It would help if I could make being active feel more important to me.</rdfs:comment>
        <rdfs:label rdf:datatype="http://www.w3.org/2001/XMLSchema#string">EMAM2</rdfs:label>
    </owl:NamedIndividual>
    


    <!-- http://www.semanticweb.org/tswheeler/ontologies/2016/3/EmpowerBP#EMAM3 -->

    <owl:NamedIndividual rdf:about="http://www.semanticweb.org/tswheeler/ontologies/2016/3/EmpowerBP#EMAM3">
        <rdf:type rdf:resource="http://www.semanticweb.org/tswheeler/ontologies/2016/3/EmpowerBP#AssessmentItem"/>
        <rdf:type rdf:resource="http://www.semanticweb.org/tswheeler/ontologies/2016/3/EmpowerBP#COMBAssessmentItem"/>
        <EmpowerBP:canAssessCOMBConstruct rdf:resource="http://www.semanticweb.org/tswheeler/ontologies/2016/3/EmpowerBP#AutomaticMotivation"/>
        <EmpowerBP:isSpecificToGoal rdf:resource="http://www.semanticweb.org/tswheeler/ontologies/2016/3/EmpowerBP#ExerciseMore"/>
        <EmpowerBP:assessmentItemExamples rdf:datatype="http://www.w3.org/2001/XMLSchema#string">• Get into a pattern of exercising regularly without having to think about it.</EmpowerBP:assessmentItemExamples>
        <EmpowerBP:assessmentItemID rdf:datatype="http://www.w3.org/2001/XMLSchema#string">EMAM3</EmpowerBP:assessmentItemID>
        <EmpowerBP:assessmentItemText rdf:datatype="http://www.w3.org/2001/XMLSchema#string">It would help if I could develop a habit of being physically active.</EmpowerBP:assessmentItemText>
        <rdfs:comment rdf:datatype="http://www.w3.org/2001/XMLSchema#string">It would help if I could develop a habit of being physically active.</rdfs:comment>
        <rdfs:label rdf:datatype="http://www.w3.org/2001/XMLSchema#string">EMAM3</rdfs:label>
    </owl:NamedIndividual>
    


    <!-- http://www.semanticweb.org/tswheeler/ontologies/2016/3/EmpowerBP#EMPO1 -->

    <owl:NamedIndividual rdf:about="http://www.semanticweb.org/tswheeler/ontologies/2016/3/EmpowerBP#EMPO1">
        <rdf:type rdf:resource="http://www.semanticweb.org/tswheeler/ontologies/2016/3/EmpowerBP#AssessmentItem"/>
        <rdf:type rdf:resource="http://www.semanticweb.org/tswheeler/ontologies/2016/3/EmpowerBP#COMBAssessmentItem"/>
        <EmpowerBP:canAssessCOMBConstruct rdf:resource="http://www.semanticweb.org/tswheeler/ontologies/2016/3/EmpowerBP#PhysicalOpportunity"/>
        <EmpowerBP:isSpecificToGoal rdf:resource="http://www.semanticweb.org/tswheeler/ontologies/2016/3/EmpowerBP#ExerciseMore"/>
        <EmpowerBP:assessmentItemExamples rdf:datatype="http://www.w3.org/2001/XMLSchema#string">• Learn how to create time in my day for physical exercise. 
• Learn how to fit physical exercise into my busy schedule.</EmpowerBP:assessmentItemExamples>
        <EmpowerBP:assessmentItemID rdf:datatype="http://www.w3.org/2001/XMLSchema#string">EMPO1</EmpowerBP:assessmentItemID>
        <EmpowerBP:assessmentItemText rdf:datatype="http://www.w3.org/2001/XMLSchema#string">It would help if I had more time to be active.  </EmpowerBP:assessmentItemText>
        <rdfs:comment rdf:datatype="http://www.w3.org/2001/XMLSchema#string">It would help if I had more time to be active.  </rdfs:comment>
        <rdfs:label rdf:datatype="http://www.w3.org/2001/XMLSchema#string">EMPO1</rdfs:label>
    </owl:NamedIndividual>
    


    <!-- http://www.semanticweb.org/tswheeler/ontologies/2016/3/EmpowerBP#EMPO2 -->

    <owl:NamedIndividual rdf:about="http://www.semanticweb.org/tswheeler/ontologies/2016/3/EmpowerBP#EMPO2">
        <rdf:type rdf:resource="http://www.semanticweb.org/tswheeler/ontologies/2016/3/EmpowerBP#AssessmentItem"/>
        <rdf:type rdf:resource="http://www.semanticweb.org/tswheeler/ontologies/2016/3/EmpowerBP#COMBAssessmentItem"/>
        <EmpowerBP:canAssessCOMBConstruct rdf:resource="http://www.semanticweb.org/tswheeler/ontologies/2016/3/EmpowerBP#PhysicalOpportunity"/>
        <EmpowerBP:isSpecificToGoal rdf:resource="http://www.semanticweb.org/tswheeler/ontologies/2016/3/EmpowerBP#ExerciseMore"/>
        <EmpowerBP:assessmentItemExamples rdf:datatype="http://www.w3.org/2001/XMLSchema#string">• Learn how to be physically active with the equipment and clothing that I have.
• Learn how I can get more exercise without spending money.</EmpowerBP:assessmentItemExamples>
        <EmpowerBP:assessmentItemID rdf:datatype="http://www.w3.org/2001/XMLSchema#string">EMPO2</EmpowerBP:assessmentItemID>
        <EmpowerBP:assessmentItemText rdf:datatype="http://www.w3.org/2001/XMLSchema#string">It would help if I had better equipment to exercise with.</EmpowerBP:assessmentItemText>
        <rdfs:comment rdf:datatype="http://www.w3.org/2001/XMLSchema#string">It would help if I had better equipment to exercise with.</rdfs:comment>
        <rdfs:label rdf:datatype="http://www.w3.org/2001/XMLSchema#string">EMPO2</rdfs:label>
    </owl:NamedIndividual>
    


    <!-- http://www.semanticweb.org/tswheeler/ontologies/2016/3/EmpowerBP#EMPO3 -->

    <owl:NamedIndividual rdf:about="http://www.semanticweb.org/tswheeler/ontologies/2016/3/EmpowerBP#EMPO3">
        <rdf:type rdf:resource="http://www.semanticweb.org/tswheeler/ontologies/2016/3/EmpowerBP#AssessmentItem"/>
        <rdf:type rdf:resource="http://www.semanticweb.org/tswheeler/ontologies/2016/3/EmpowerBP#COMBAssessmentItem"/>
        <EmpowerBP:canAssessCOMBConstruct rdf:resource="http://www.semanticweb.org/tswheeler/ontologies/2016/3/EmpowerBP#PhysicalOpportunity"/>
        <EmpowerBP:isSpecificToGoal rdf:resource="http://www.semanticweb.org/tswheeler/ontologies/2016/3/EmpowerBP#ExerciseMore"/>
        <EmpowerBP:assessmentItemExamples rdf:datatype="http://www.w3.org/2001/XMLSchema#string">• Learn where to go to exercise. 
• Learn how to be active at home and at work.</EmpowerBP:assessmentItemExamples>
        <EmpowerBP:assessmentItemID rdf:datatype="http://www.w3.org/2001/XMLSchema#string">EMPO3</EmpowerBP:assessmentItemID>
        <EmpowerBP:assessmentItemText rdf:datatype="http://www.w3.org/2001/XMLSchema#string">It would help if I had more places where I could be active.</EmpowerBP:assessmentItemText>
        <rdfs:comment rdf:datatype="http://www.w3.org/2001/XMLSchema#string">It would help if I had more places where I could be active.</rdfs:comment>
        <rdfs:label rdf:datatype="http://www.w3.org/2001/XMLSchema#string">EMPO3</rdfs:label>
    </owl:NamedIndividual>
    


    <!-- http://www.semanticweb.org/tswheeler/ontologies/2016/3/EmpowerBP#EMPhC1 -->

    <owl:NamedIndividual rdf:about="http://www.semanticweb.org/tswheeler/ontologies/2016/3/EmpowerBP#EMPhC1">
        <rdf:type rdf:resource="http://www.semanticweb.org/tswheeler/ontologies/2016/3/EmpowerBP#AssessmentItem"/>
        <rdf:type rdf:resource="http://www.semanticweb.org/tswheeler/ontologies/2016/3/EmpowerBP#COMBAssessmentItem"/>
        <EmpowerBP:canAssessCOMBConstruct rdf:resource="http://www.semanticweb.org/tswheeler/ontologies/2016/3/EmpowerBP#PhysicalCapability"/>
        <EmpowerBP:isSpecificToGoal rdf:resource="http://www.semanticweb.org/tswheeler/ontologies/2016/3/EmpowerBP#ExerciseMore"/>
        <EmpowerBP:assessmentItemExamples rdf:datatype="http://www.w3.org/2001/XMLSchema#string">• Learn what counts as physical activity.
• Learn different types of exercises.</EmpowerBP:assessmentItemExamples>
        <EmpowerBP:assessmentItemID rdf:datatype="http://www.w3.org/2001/XMLSchema#string">EMPhC1</EmpowerBP:assessmentItemID>
        <EmpowerBP:assessmentItemText rdf:datatype="http://www.w3.org/2001/XMLSchema#string">It would help if I knew more ways to be physically active.</EmpowerBP:assessmentItemText>
        <rdfs:comment rdf:datatype="http://www.w3.org/2001/XMLSchema#string">It would help if I knew more ways to be physically active.</rdfs:comment>
        <rdfs:label rdf:datatype="http://www.w3.org/2001/XMLSchema#string">EMPhC1</rdfs:label>
    </owl:NamedIndividual>
    


    <!-- http://www.semanticweb.org/tswheeler/ontologies/2016/3/EmpowerBP#EMPhC2 -->

    <owl:NamedIndividual rdf:about="http://www.semanticweb.org/tswheeler/ontologies/2016/3/EmpowerBP#EMPhC2">
        <rdf:type rdf:resource="http://www.semanticweb.org/tswheeler/ontologies/2016/3/EmpowerBP#AssessmentItem"/>
        <rdf:type rdf:resource="http://www.semanticweb.org/tswheeler/ontologies/2016/3/EmpowerBP#COMBAssessmentItem"/>
        <EmpowerBP:canAssessCOMBConstruct rdf:resource="http://www.semanticweb.org/tswheeler/ontologies/2016/3/EmpowerBP#PhysicalCapability"/>
        <EmpowerBP:isSpecificToGoal rdf:resource="http://www.semanticweb.org/tswheeler/ontologies/2016/3/EmpowerBP#ExerciseMore"/>
        <EmpowerBP:assessmentItemExamples rdf:datatype="http://www.w3.org/2001/XMLSchema#string">• Learn how to properly start walking or running regularly.
• Learn how to safely do physical activities.</EmpowerBP:assessmentItemExamples>
        <EmpowerBP:assessmentItemID rdf:datatype="http://www.w3.org/2001/XMLSchema#string">EMPhC2</EmpowerBP:assessmentItemID>
        <EmpowerBP:assessmentItemText rdf:datatype="http://www.w3.org/2001/XMLSchema#string">It would help if I learned how to properly perform different physical activities.</EmpowerBP:assessmentItemText>
        <rdfs:comment rdf:datatype="http://www.w3.org/2001/XMLSchema#string">It would help if I learned how to properly perform different physical activities.</rdfs:comment>
        <rdfs:label rdf:datatype="http://www.w3.org/2001/XMLSchema#string">EMPhC2</rdfs:label>
    </owl:NamedIndividual>
    


    <!-- http://www.semanticweb.org/tswheeler/ontologies/2016/3/EmpowerBP#EMPhC3 -->

    <owl:NamedIndividual rdf:about="http://www.semanticweb.org/tswheeler/ontologies/2016/3/EmpowerBP#EMPhC3">
        <rdf:type rdf:resource="http://www.semanticweb.org/tswheeler/ontologies/2016/3/EmpowerBP#AssessmentItem"/>
        <rdf:type rdf:resource="http://www.semanticweb.org/tswheeler/ontologies/2016/3/EmpowerBP#COMBAssessmentItem"/>
        <EmpowerBP:canAssessCOMBConstruct rdf:resource="http://www.semanticweb.org/tswheeler/ontologies/2016/3/EmpowerBP#PhysicalCapability"/>
        <EmpowerBP:isSpecificToGoal rdf:resource="http://www.semanticweb.org/tswheeler/ontologies/2016/3/EmpowerBP#ExerciseMore"/>
        <EmpowerBP:assessmentItemExamples rdf:datatype="http://www.w3.org/2001/XMLSchema#string">• Learn how to build up strength and endurance for physical activity.</EmpowerBP:assessmentItemExamples>
        <EmpowerBP:assessmentItemID rdf:datatype="http://www.w3.org/2001/XMLSchema#string">EMPhC3</EmpowerBP:assessmentItemID>
        <EmpowerBP:assessmentItemText rdf:datatype="http://www.w3.org/2001/XMLSchema#string">It would help if I increased my physical strength and stamina.</EmpowerBP:assessmentItemText>
        <rdfs:comment rdf:datatype="http://www.w3.org/2001/XMLSchema#string">It would help if I increased my physical strength and stamina.</rdfs:comment>
        <rdfs:label rdf:datatype="http://www.w3.org/2001/XMLSchema#string">EMPhC3</rdfs:label>
    </owl:NamedIndividual>
    


    <!-- http://www.semanticweb.org/tswheeler/ontologies/2016/3/EmpowerBP#EMPsC1 -->

    <owl:NamedIndividual rdf:about="http://www.semanticweb.org/tswheeler/ontologies/2016/3/EmpowerBP#EMPsC1">
        <rdf:type rdf:resource="http://www.semanticweb.org/tswheeler/ontologies/2016/3/EmpowerBP#AssessmentItem"/>
        <rdf:type rdf:resource="http://www.semanticweb.org/tswheeler/ontologies/2016/3/EmpowerBP#COMBAssessmentItem"/>
        <EmpowerBP:canAssessCOMBConstruct rdf:resource="http://www.semanticweb.org/tswheeler/ontologies/2016/3/EmpowerBP#PsychologicalCapability"/>
        <EmpowerBP:isSpecificToGoal rdf:resource="http://www.semanticweb.org/tswheeler/ontologies/2016/3/EmpowerBP#ExerciseMore"/>
        <EmpowerBP:assessmentItemExamples rdf:datatype="http://www.w3.org/2001/XMLSchema#string">• Have a better understanding of the benefits of exercise and the risks of not being regularly active.</EmpowerBP:assessmentItemExamples>
        <EmpowerBP:assessmentItemID rdf:datatype="http://www.w3.org/2001/XMLSchema#string">EMPsC1</EmpowerBP:assessmentItemID>
        <EmpowerBP:assessmentItemText rdf:datatype="http://www.w3.org/2001/XMLSchema#string">It would help if I knew more about why physical activity is important.</EmpowerBP:assessmentItemText>
        <rdfs:comment rdf:datatype="http://www.w3.org/2001/XMLSchema#string">It would help if I knew more about why physical activity is important.</rdfs:comment>
        <rdfs:label rdf:datatype="http://www.w3.org/2001/XMLSchema#string">EMPsC1</rdfs:label>
    </owl:NamedIndividual>
    


    <!-- http://www.semanticweb.org/tswheeler/ontologies/2016/3/EmpowerBP#EMPsC2 -->

    <owl:NamedIndividual rdf:about="http://www.semanticweb.org/tswheeler/ontologies/2016/3/EmpowerBP#EMPsC2">
        <rdf:type rdf:resource="http://www.semanticweb.org/tswheeler/ontologies/2016/3/EmpowerBP#AssessmentItem"/>
        <rdf:type rdf:resource="http://www.semanticweb.org/tswheeler/ontologies/2016/3/EmpowerBP#COMBAssessmentItem"/>
        <EmpowerBP:canAssessCOMBConstruct rdf:resource="http://www.semanticweb.org/tswheeler/ontologies/2016/3/EmpowerBP#PsychologicalCapability"/>
        <EmpowerBP:isSpecificToGoal rdf:resource="http://www.semanticweb.org/tswheeler/ontologies/2016/3/EmpowerBP#ExerciseMore"/>
        <EmpowerBP:assessmentItemExamples rdf:datatype="http://www.w3.org/2001/XMLSchema#string">• Learn more about the “proper mindset” to get regular physical exercise.
• Learn how to concentrate on my goals of being more active.</EmpowerBP:assessmentItemExamples>
        <EmpowerBP:assessmentItemID rdf:datatype="http://www.w3.org/2001/XMLSchema#string">EMPsC2</EmpowerBP:assessmentItemID>
        <EmpowerBP:assessmentItemText rdf:datatype="http://www.w3.org/2001/XMLSchema#string">It would help if I changed the way I thought about exercise and being active.</EmpowerBP:assessmentItemText>
        <rdfs:comment rdf:datatype="http://www.w3.org/2001/XMLSchema#string">It would help if I changed the way I thought about exercise and being active.</rdfs:comment>
        <rdfs:label rdf:datatype="http://www.w3.org/2001/XMLSchema#string">EMPsC2</rdfs:label>
    </owl:NamedIndividual>
    


    <!-- http://www.semanticweb.org/tswheeler/ontologies/2016/3/EmpowerBP#EMPsC3 -->

    <owl:NamedIndividual rdf:about="http://www.semanticweb.org/tswheeler/ontologies/2016/3/EmpowerBP#EMPsC3">
        <rdf:type rdf:resource="http://www.semanticweb.org/tswheeler/ontologies/2016/3/EmpowerBP#AssessmentItem"/>
        <rdf:type rdf:resource="http://www.semanticweb.org/tswheeler/ontologies/2016/3/EmpowerBP#COMBAssessmentItem"/>
        <EmpowerBP:canAssessCOMBConstruct rdf:resource="http://www.semanticweb.org/tswheeler/ontologies/2016/3/EmpowerBP#PsychologicalCapability"/>
        <EmpowerBP:isSpecificToGoal rdf:resource="http://www.semanticweb.org/tswheeler/ontologies/2016/3/EmpowerBP#ExerciseMore"/>
        <EmpowerBP:assessmentItemExamples rdf:datatype="http://www.w3.org/2001/XMLSchema#string">• Learn how to reduce unwanted urges or feelings about physical exercise.
• Learn how exercise regularly even when life is stressful.</EmpowerBP:assessmentItemExamples>
        <EmpowerBP:assessmentItemID rdf:datatype="http://www.w3.org/2001/XMLSchema#string">EMPsC3</EmpowerBP:assessmentItemID>
        <EmpowerBP:assessmentItemText rdf:datatype="http://www.w3.org/2001/XMLSchema#string">It would help if I improved my mental strength and stamina.</EmpowerBP:assessmentItemText>
        <rdfs:comment rdf:datatype="http://www.w3.org/2001/XMLSchema#string">It would help if I improved my mental strength and stamina.</rdfs:comment>
        <rdfs:label rdf:datatype="http://www.w3.org/2001/XMLSchema#string">EMPsC3</rdfs:label>
    </owl:NamedIndividual>
    


    <!-- http://www.semanticweb.org/tswheeler/ontologies/2016/3/EmpowerBP#EMRM1 -->

    <owl:NamedIndividual rdf:about="http://www.semanticweb.org/tswheeler/ontologies/2016/3/EmpowerBP#EMRM1">
        <rdf:type rdf:resource="http://www.semanticweb.org/tswheeler/ontologies/2016/3/EmpowerBP#AssessmentItem"/>
        <rdf:type rdf:resource="http://www.semanticweb.org/tswheeler/ontologies/2016/3/EmpowerBP#COMBAssessmentItem"/>
        <EmpowerBP:canAssessCOMBConstruct rdf:resource="http://www.semanticweb.org/tswheeler/ontologies/2016/3/EmpowerBP#ReflectiveMotivation"/>
        <EmpowerBP:isSpecificToGoal rdf:resource="http://www.semanticweb.org/tswheeler/ontologies/2016/3/EmpowerBP#ExerciseMore"/>
        <EmpowerBP:assessmentItemExamples rdf:datatype="http://www.w3.org/2001/XMLSchema#string">• Learn how to weigh the pros and cons of exercising.</EmpowerBP:assessmentItemExamples>
        <EmpowerBP:assessmentItemID rdf:datatype="http://www.w3.org/2001/XMLSchema#string">EMRM1</EmpowerBP:assessmentItemID>
        <EmpowerBP:assessmentItemText rdf:datatype="http://www.w3.org/2001/XMLSchema#string">It would help if could focus more on the reasons to change and not on what is keeping me from changing.</EmpowerBP:assessmentItemText>
        <rdfs:comment rdf:datatype="http://www.w3.org/2001/XMLSchema#string">It would help if could focus more on the reasons to change and not on what is keeping me from changing.</rdfs:comment>
        <rdfs:label rdf:datatype="http://www.w3.org/2001/XMLSchema#string">EMRM1</rdfs:label>
    </owl:NamedIndividual>
    


    <!-- http://www.semanticweb.org/tswheeler/ontologies/2016/3/EmpowerBP#EMRM2 -->

    <owl:NamedIndividual rdf:about="http://www.semanticweb.org/tswheeler/ontologies/2016/3/EmpowerBP#EMRM2">
        <rdf:type rdf:resource="http://www.semanticweb.org/tswheeler/ontologies/2016/3/EmpowerBP#AssessmentItem"/>
        <rdf:type rdf:resource="http://www.semanticweb.org/tswheeler/ontologies/2016/3/EmpowerBP#COMBAssessmentItem"/>
        <EmpowerBP:canAssessCOMBConstruct rdf:resource="http://www.semanticweb.org/tswheeler/ontologies/2016/3/EmpowerBP#ReflectiveMotivation"/>
        <EmpowerBP:isSpecificToGoal rdf:resource="http://www.semanticweb.org/tswheeler/ontologies/2016/3/EmpowerBP#ExerciseMore"/>
        <EmpowerBP:assessmentItemExamples rdf:datatype="http://www.w3.org/2001/XMLSchema#string">• Make clear and thought out plans for exercising more.</EmpowerBP:assessmentItemExamples>
        <EmpowerBP:assessmentItemID rdf:datatype="http://www.w3.org/2001/XMLSchema#string">EMRM2</EmpowerBP:assessmentItemID>
        <EmpowerBP:assessmentItemText rdf:datatype="http://www.w3.org/2001/XMLSchema#string">It would help if I had better plans for being more active.</EmpowerBP:assessmentItemText>
        <rdfs:comment rdf:datatype="http://www.w3.org/2001/XMLSchema#string">It would help if I had better plans for being more active.</rdfs:comment>
        <rdfs:label rdf:datatype="http://www.w3.org/2001/XMLSchema#string">EMRM2</rdfs:label>
    </owl:NamedIndividual>
    


    <!-- http://www.semanticweb.org/tswheeler/ontologies/2016/3/EmpowerBP#EMRM3 -->

    <owl:NamedIndividual rdf:about="http://www.semanticweb.org/tswheeler/ontologies/2016/3/EmpowerBP#EMRM3">
        <rdf:type rdf:resource="http://www.semanticweb.org/tswheeler/ontologies/2016/3/EmpowerBP#AssessmentItem"/>
        <rdf:type rdf:resource="http://www.semanticweb.org/tswheeler/ontologies/2016/3/EmpowerBP#COMBAssessmentItem"/>
        <EmpowerBP:canAssessCOMBConstruct rdf:resource="http://www.semanticweb.org/tswheeler/ontologies/2016/3/EmpowerBP#ReflectiveMotivation"/>
        <EmpowerBP:isSpecificToGoal rdf:resource="http://www.semanticweb.org/tswheeler/ontologies/2016/3/EmpowerBP#ExerciseMore"/>
        <EmpowerBP:assessmentItemExamples rdf:datatype="http://www.w3.org/2001/XMLSchema#string">• Become more confident in my ability to exercise regularly.</EmpowerBP:assessmentItemExamples>
        <EmpowerBP:assessmentItemID rdf:datatype="http://www.w3.org/2001/XMLSchema#string">EMRM3</EmpowerBP:assessmentItemID>
        <EmpowerBP:assessmentItemText rdf:datatype="http://www.w3.org/2001/XMLSchema#string">It would help if I had more self-confidence in my ability to be more active.</EmpowerBP:assessmentItemText>
        <rdfs:comment rdf:datatype="http://www.w3.org/2001/XMLSchema#string">It would help if I had more self-confidence in my ability to be more active.</rdfs:comment>
        <rdfs:label rdf:datatype="http://www.w3.org/2001/XMLSchema#string">EMRM3</rdfs:label>
    </owl:NamedIndividual>
    


    <!-- http://www.semanticweb.org/tswheeler/ontologies/2016/3/EmpowerBP#EMSO1 -->

    <owl:NamedIndividual rdf:about="http://www.semanticweb.org/tswheeler/ontologies/2016/3/EmpowerBP#EMSO1">
        <rdf:type rdf:resource="http://www.semanticweb.org/tswheeler/ontologies/2016/3/EmpowerBP#AssessmentItem"/>
        <rdf:type rdf:resource="http://www.semanticweb.org/tswheeler/ontologies/2016/3/EmpowerBP#COMBAssessmentItem"/>
        <EmpowerBP:canAssessCOMBConstruct rdf:resource="http://www.semanticweb.org/tswheeler/ontologies/2016/3/EmpowerBP#SocialOpportunity"/>
        <EmpowerBP:isSpecificToGoal rdf:resource="http://www.semanticweb.org/tswheeler/ontologies/2016/3/EmpowerBP#ExerciseMore"/>
        <EmpowerBP:assessmentItemExamples rdf:datatype="http://www.w3.org/2001/XMLSchema#string">• Have regular reminders to exercise at strategic times. 
• Learn how to change my home and work environment to support exercising more.</EmpowerBP:assessmentItemExamples>
        <EmpowerBP:assessmentItemID rdf:datatype="http://www.w3.org/2001/XMLSchema#string">EMSO1</EmpowerBP:assessmentItemID>
        <EmpowerBP:assessmentItemText rdf:datatype="http://www.w3.org/2001/XMLSchema#string">It would help if I had more cues to encourage me to exercise.</EmpowerBP:assessmentItemText>
        <rdfs:comment rdf:datatype="http://www.w3.org/2001/XMLSchema#string">It would help if I had more cues to encourage me to exercise.</rdfs:comment>
        <rdfs:label rdf:datatype="http://www.w3.org/2001/XMLSchema#string">EMSO1</rdfs:label>
    </owl:NamedIndividual>
    


    <!-- http://www.semanticweb.org/tswheeler/ontologies/2016/3/EmpowerBP#EMSO2 -->

    <owl:NamedIndividual rdf:about="http://www.semanticweb.org/tswheeler/ontologies/2016/3/EmpowerBP#EMSO2">
        <rdf:type rdf:resource="http://www.semanticweb.org/tswheeler/ontologies/2016/3/EmpowerBP#AssessmentItem"/>
        <rdf:type rdf:resource="http://www.semanticweb.org/tswheeler/ontologies/2016/3/EmpowerBP#COMBAssessmentItem"/>
        <EmpowerBP:canAssessCOMBConstruct rdf:resource="http://www.semanticweb.org/tswheeler/ontologies/2016/3/EmpowerBP#SocialOpportunity"/>
        <EmpowerBP:isSpecificToGoal rdf:resource="http://www.semanticweb.org/tswheeler/ontologies/2016/3/EmpowerBP#ExerciseMore"/>
        <EmpowerBP:assessmentItemExamples rdf:datatype="http://www.w3.org/2001/XMLSchema#string">• Find groups or teams who have similar exercise goals as me.</EmpowerBP:assessmentItemExamples>
        <EmpowerBP:assessmentItemID rdf:datatype="http://www.w3.org/2001/XMLSchema#string">EMSO2</EmpowerBP:assessmentItemID>
        <EmpowerBP:assessmentItemText rdf:datatype="http://www.w3.org/2001/XMLSchema#string">It would help if I had more people around me who were physically active.</EmpowerBP:assessmentItemText>
        <rdfs:comment rdf:datatype="http://www.w3.org/2001/XMLSchema#string">It would help if I had more people around me who were physically active.</rdfs:comment>
        <rdfs:label rdf:datatype="http://www.w3.org/2001/XMLSchema#string">EMSO2</rdfs:label>
    </owl:NamedIndividual>
    


    <!-- http://www.semanticweb.org/tswheeler/ontologies/2016/3/EmpowerBP#EMSO3 -->

    <owl:NamedIndividual rdf:about="http://www.semanticweb.org/tswheeler/ontologies/2016/3/EmpowerBP#EMSO3">
        <rdf:type rdf:resource="http://www.semanticweb.org/tswheeler/ontologies/2016/3/EmpowerBP#AssessmentItem"/>
        <rdf:type rdf:resource="http://www.semanticweb.org/tswheeler/ontologies/2016/3/EmpowerBP#COMBAssessmentItem"/>
        <EmpowerBP:canAssessCOMBConstruct rdf:resource="http://www.semanticweb.org/tswheeler/ontologies/2016/3/EmpowerBP#SocialOpportunity"/>
        <EmpowerBP:isSpecificToGoal rdf:resource="http://www.semanticweb.org/tswheeler/ontologies/2016/3/EmpowerBP#ExerciseMore"/>
        <EmpowerBP:assessmentItemExamples rdf:datatype="http://www.w3.org/2001/XMLSchema#string">• Learn how to have my friends and family help me reach my exercise goals.</EmpowerBP:assessmentItemExamples>
        <EmpowerBP:assessmentItemID rdf:datatype="http://www.w3.org/2001/XMLSchema#string">EMSO3</EmpowerBP:assessmentItemID>
        <EmpowerBP:assessmentItemText rdf:datatype="http://www.w3.org/2001/XMLSchema#string">It would help if I had more people around me supporting my goals.</EmpowerBP:assessmentItemText>
        <rdfs:comment rdf:datatype="http://www.w3.org/2001/XMLSchema#string">It would help if I had more people around me supporting my goals.</rdfs:comment>
        <rdfs:label rdf:datatype="http://www.w3.org/2001/XMLSchema#string">EMSO3</rdfs:label>
    </owl:NamedIndividual>
    


    <!-- http://www.semanticweb.org/tswheeler/ontologies/2016/3/EmpowerBP#Education -->

    <owl:NamedIndividual rdf:about="http://www.semanticweb.org/tswheeler/ontologies/2016/3/EmpowerBP#Education">
        <rdf:type rdf:resource="http://www.semanticweb.org/tswheeler/ontologies/2016/3/EmpowerBP#InterventionFuction"/>
        <EmpowerBP:hasCommonBCT rdf:resource="http://purl.bioontology.org/ontology/BCTT#Behavioral_experiments"/>
        <EmpowerBP:hasCommonBCT rdf:resource="http://purl.bioontology.org/ontology/BCTT#Biofeedback"/>
        <EmpowerBP:hasCommonBCT rdf:resource="http://purl.bioontology.org/ontology/BCTT#Cue_signalling_reward"/>
        <EmpowerBP:hasCommonBCT rdf:resource="http://purl.bioontology.org/ontology/BCTT#Information_about_Antecedents"/>
        <EmpowerBP:hasCommonBCT rdf:resource="http://purl.bioontology.org/ontology/BCTT#Information_about_emotional_consequences"/>
        <EmpowerBP:hasCommonBCT rdf:resource="http://purl.bioontology.org/ontology/BCTT#Re-attribution"/>
        <EmpowerBP:hasCommonBCT rdf:resource="http://purl.bioontology.org/ontology/BCTT#Satiation"/>
        <EmpowerBP:hasCommonBCT rdf:resource="http://purl.bioontology.org/ontology/BCTT#Information_about_others&apos;_approval"/>
        <EmpowerBP:hasCommonBCT rdf:resource="http://purl.bioontology.org/ontology/BCTT#Self-monitoring_of_outcome(s)_of_behaviour"/>
        <EmpowerBP:hasMostCommonBCT rdf:resource="http://purl.bioontology.org/ontology/BCTT#Feedback_on_behaviour"/>
        <EmpowerBP:hasMostCommonBCT rdf:resource="http://purl.bioontology.org/ontology/BCTT#Information_about_health_consequences"/>
        <EmpowerBP:hasMostCommonBCT rdf:resource="http://purl.bioontology.org/ontology/BCTT#Information_about_social_and_environmental_consequences"/>
        <EmpowerBP:hasMostCommonBCT rdf:resource="http://purl.bioontology.org/ontology/BCTT#Prompts-cues"/>
        <EmpowerBP:hasMostCommonBCT rdf:resource="http://purl.bioontology.org/ontology/BCTT#Self-monitoring_of_behaviour"/>
        <EmpowerBP:hasMostCommonBCT rdf:resource="http://purl.bioontology.org/ontology/BCTT#Feedback_on_outcome(s)_of_behavior"/>
        <EmpowerBP:isEffectiveForTDFDomain rdf:resource="http://www.semanticweb.org/tswheeler/ontologies/2016/3/EmpowerBP#BehaviouralRegulation"/>
        <EmpowerBP:isEffectiveForTDFDomain rdf:resource="http://www.semanticweb.org/tswheeler/ontologies/2016/3/EmpowerBP#BeliefsAboutCapability"/>
        <EmpowerBP:isEffectiveForTDFDomain rdf:resource="http://www.semanticweb.org/tswheeler/ontologies/2016/3/EmpowerBP#BeliefsAboutConsequences"/>
        <EmpowerBP:isEffectiveForTDFDomain rdf:resource="http://www.semanticweb.org/tswheeler/ontologies/2016/3/EmpowerBP#Goals"/>
        <EmpowerBP:isEffectiveForTDFDomain rdf:resource="http://www.semanticweb.org/tswheeler/ontologies/2016/3/EmpowerBP#Intentions"/>
        <EmpowerBP:isEffectiveForTDFDomain rdf:resource="http://www.semanticweb.org/tswheeler/ontologies/2016/3/EmpowerBP#Knowledge"/>
        <EmpowerBP:isEffectiveForTDFDomain rdf:resource="http://www.semanticweb.org/tswheeler/ontologies/2016/3/EmpowerBP#Optimism"/>
        <EmpowerBP:isEffectiveForTDFDomain rdf:resource="http://www.semanticweb.org/tswheeler/ontologies/2016/3/EmpowerBP#ProfessionalSocialRoleIdentity"/>
        <rdfs:comment>Increasing knowledge or understanding.</rdfs:comment>
    </owl:NamedIndividual>
    


    <!-- http://www.semanticweb.org/tswheeler/ontologies/2016/3/EmpowerBP#Emotion -->

    <owl:NamedIndividual rdf:about="http://www.semanticweb.org/tswheeler/ontologies/2016/3/EmpowerBP#Emotion">
        <rdf:type rdf:resource="http://www.semanticweb.org/tswheeler/ontologies/2016/3/EmpowerBP#Construct"/>
        <rdf:type rdf:resource="http://www.semanticweb.org/tswheeler/ontologies/2016/3/EmpowerBP#TDFDomain"/>
        <EmpowerBP:hasEffectiveInterventionFunction rdf:resource="http://www.semanticweb.org/tswheeler/ontologies/2016/3/EmpowerBP#Coercion"/>
        <EmpowerBP:hasEffectiveInterventionFunction rdf:resource="http://www.semanticweb.org/tswheeler/ontologies/2016/3/EmpowerBP#Enablement"/>
        <EmpowerBP:hasEffectiveInterventionFunction rdf:resource="http://www.semanticweb.org/tswheeler/ontologies/2016/3/EmpowerBP#Incentivisation"/>
        <EmpowerBP:hasEffectiveInterventionFunction rdf:resource="http://www.semanticweb.org/tswheeler/ontologies/2016/3/EmpowerBP#Modelling"/>
        <EmpowerBP:hasEffectiveInterventionFunction rdf:resource="http://www.semanticweb.org/tswheeler/ontologies/2016/3/EmpowerBP#Persuasion"/>
        <EmpowerBP:isRelatedToCOMB rdf:resource="http://www.semanticweb.org/tswheeler/ontologies/2016/3/EmpowerBP#AutomaticMotivation"/>
        <rdfs:comment>A complex reaction pattern, involving experiential, behavioral, and physiological elements, by which the individual attempts to deal with a personally significant matter or event</rdfs:comment>
    </owl:NamedIndividual>
    


    <!-- http://www.semanticweb.org/tswheeler/ontologies/2016/3/EmpowerBP#Enablement -->

    <owl:NamedIndividual rdf:about="http://www.semanticweb.org/tswheeler/ontologies/2016/3/EmpowerBP#Enablement">
        <rdf:type rdf:resource="http://www.semanticweb.org/tswheeler/ontologies/2016/3/EmpowerBP#InterventionFuction"/>
        <EmpowerBP:hasCommonBCT rdf:resource="http://purl.bioontology.org/ontology/BCTT#Anticipated_regret"/>
        <EmpowerBP:hasCommonBCT rdf:resource="http://purl.bioontology.org/ontology/BCTT#Avoidance-reducing_exposure_to_cues_for_the_behavior"/>
        <EmpowerBP:hasCommonBCT rdf:resource="http://purl.bioontology.org/ontology/BCTT#Behavior_substitution"/>
        <EmpowerBP:hasCommonBCT rdf:resource="http://purl.bioontology.org/ontology/BCTT#Behavioral_contract"/>
        <EmpowerBP:hasCommonBCT rdf:resource="http://purl.bioontology.org/ontology/BCTT#Behavioral_experiments"/>
        <EmpowerBP:hasCommonBCT rdf:resource="http://purl.bioontology.org/ontology/BCTT#Body_changes"/>
        <EmpowerBP:hasCommonBCT rdf:resource="http://purl.bioontology.org/ontology/BCTT#Commitment"/>
        <EmpowerBP:hasCommonBCT rdf:resource="http://purl.bioontology.org/ontology/BCTT#Comparative_imagining_of_future_outcomes"/>
        <EmpowerBP:hasCommonBCT rdf:resource="http://purl.bioontology.org/ontology/BCTT#Conserving_mental_resources"/>
        <EmpowerBP:hasCommonBCT rdf:resource="http://purl.bioontology.org/ontology/BCTT#Discrepancy_between_current_behavior_and_goal"/>
        <EmpowerBP:hasCommonBCT rdf:resource="http://purl.bioontology.org/ontology/BCTT#Distraction"/>
        <EmpowerBP:hasCommonBCT rdf:resource="http://purl.bioontology.org/ontology/BCTT#Focus_on_past_success"/>
        <EmpowerBP:hasCommonBCT rdf:resource="http://purl.bioontology.org/ontology/BCTT#Framing-reframing"/>
        <EmpowerBP:hasCommonBCT rdf:resource="http://purl.bioontology.org/ontology/BCTT#Generalisation_of_target_behavior"/>
        <EmpowerBP:hasCommonBCT rdf:resource="http://purl.bioontology.org/ontology/BCTT#Graded_tasks"/>
        <EmpowerBP:hasCommonBCT rdf:resource="http://purl.bioontology.org/ontology/BCTT#Identification_of_self_as_role_model"/>
        <EmpowerBP:hasCommonBCT rdf:resource="http://purl.bioontology.org/ontology/BCTT#Identity_associated_with_changed_behavior"/>
        <EmpowerBP:hasCommonBCT rdf:resource="http://purl.bioontology.org/ontology/BCTT#Imaginary_punishment"/>
        <EmpowerBP:hasCommonBCT rdf:resource="http://purl.bioontology.org/ontology/BCTT#Imaginary_reward"/>
        <EmpowerBP:hasCommonBCT rdf:resource="http://purl.bioontology.org/ontology/BCTT#Incompatible_beliefs"/>
        <EmpowerBP:hasCommonBCT rdf:resource="http://purl.bioontology.org/ontology/BCTT#Mental_rehearsal_of_successful_performance"/>
        <EmpowerBP:hasCommonBCT rdf:resource="http://purl.bioontology.org/ontology/BCTT#Monitoring_of_emotional_consequences"/>
        <EmpowerBP:hasCommonBCT rdf:resource="http://purl.bioontology.org/ontology/BCTT#Overcorrection"/>
        <EmpowerBP:hasCommonBCT rdf:resource="http://purl.bioontology.org/ontology/BCTT#Pharmacological_support"/>
        <EmpowerBP:hasCommonBCT rdf:resource="http://purl.bioontology.org/ontology/BCTT#Pros_and_cons"/>
        <EmpowerBP:hasCommonBCT rdf:resource="http://purl.bioontology.org/ontology/BCTT#Reduce_negative_emotions"/>
        <EmpowerBP:hasCommonBCT rdf:resource="http://purl.bioontology.org/ontology/BCTT#Restructuring_the_social_environment"/>
        <EmpowerBP:hasCommonBCT rdf:resource="http://purl.bioontology.org/ontology/BCTT#Salience_of_consequences"/>
        <EmpowerBP:hasCommonBCT rdf:resource="http://purl.bioontology.org/ontology/BCTT#Self-reward"/>
        <EmpowerBP:hasCommonBCT rdf:resource="http://purl.bioontology.org/ontology/BCTT#Self-talk"/>
        <EmpowerBP:hasCommonBCT rdf:resource="http://purl.bioontology.org/ontology/BCTT#Valued_self-identify"/>
        <EmpowerBP:hasCommonBCT rdf:resource="http://purl.bioontology.org/ontology/BCTT#Verbal_persuasion_about_capability"/>
        <EmpowerBP:hasCommonBCT rdf:resource="http://purl.bioontology.org/ontology/BCTT#Vicarious_consequences"/>
        <EmpowerBP:hasCommonBCT rdf:resource="http://purl.bioontology.org/ontology/BCTT#Self-monitoring_of_outcome(s)_of_behaviour"/>
        <EmpowerBP:hasCommonBCT rdf:resource="http://purl.bioontology.org/ontology/BCTT#Social_support_(emotional)"/>
        <EmpowerBP:hasMostCommonBCT rdf:resource="http://purl.bioontology.org/ontology/BCTT#Action_planning"/>
        <EmpowerBP:hasMostCommonBCT rdf:resource="http://purl.bioontology.org/ontology/BCTT#Adding_objects_to_the_environment"/>
        <EmpowerBP:hasMostCommonBCT rdf:resource="http://purl.bioontology.org/ontology/BCTT#Problem_solving"/>
        <EmpowerBP:hasMostCommonBCT rdf:resource="http://purl.bioontology.org/ontology/BCTT#Restructuring_the_physical_environment"/>
        <EmpowerBP:hasMostCommonBCT rdf:resource="http://purl.bioontology.org/ontology/BCTT#Self-monitoring_of_behaviour"/>
        <EmpowerBP:hasMostCommonBCT rdf:resource="http://purl.bioontology.org/ontology/BCTT#Goal_setting_(behavior)"/>
        <EmpowerBP:hasMostCommonBCT rdf:resource="http://purl.bioontology.org/ontology/BCTT#Goal_setting_(outcome)"/>
        <EmpowerBP:hasMostCommonBCT rdf:resource="http://purl.bioontology.org/ontology/BCTT#Review_behavior_goal(s)"/>
        <EmpowerBP:hasMostCommonBCT rdf:resource="http://purl.bioontology.org/ontology/BCTT#Review_outcome_goal(s)"/>
        <EmpowerBP:hasMostCommonBCT rdf:resource="http://purl.bioontology.org/ontology/BCTT#Social_support_(practical)"/>
        <EmpowerBP:hasMostCommonBCT rdf:resource="http://purl.bioontology.org/ontology/BCTT#Social_support_(unspecified)"/>
        <EmpowerBP:isEffectiveForTDFDomain rdf:resource="http://www.semanticweb.org/tswheeler/ontologies/2016/3/EmpowerBP#BehaviouralRegulation"/>
        <EmpowerBP:isEffectiveForTDFDomain rdf:resource="http://www.semanticweb.org/tswheeler/ontologies/2016/3/EmpowerBP#BeliefsAboutCapability"/>
        <EmpowerBP:isEffectiveForTDFDomain rdf:resource="http://www.semanticweb.org/tswheeler/ontologies/2016/3/EmpowerBP#Emotion"/>
        <EmpowerBP:isEffectiveForTDFDomain rdf:resource="http://www.semanticweb.org/tswheeler/ontologies/2016/3/EmpowerBP#EnvironmentalContextResources"/>
        <EmpowerBP:isEffectiveForTDFDomain rdf:resource="http://www.semanticweb.org/tswheeler/ontologies/2016/3/EmpowerBP#Goals"/>
        <EmpowerBP:isEffectiveForTDFDomain rdf:resource="http://www.semanticweb.org/tswheeler/ontologies/2016/3/EmpowerBP#MemoryAttentionDecisionProcesses"/>
        <EmpowerBP:isEffectiveForTDFDomain rdf:resource="http://www.semanticweb.org/tswheeler/ontologies/2016/3/EmpowerBP#Optimism"/>
        <EmpowerBP:isEffectiveForTDFDomain rdf:resource="http://www.semanticweb.org/tswheeler/ontologies/2016/3/EmpowerBP#SocialInfluences"/>
        <rdfs:comment>Increasing means/reducing barriers to increase capability (beyond education and training) or opportunity (beyond environmental restructuring). 

E.g. Behavioural support for smoking cessation, medication for cognitive deficits, surgery to reduce obesity, prostheses to promote physical activity.</rdfs:comment>
    </owl:NamedIndividual>
    


    <!-- http://www.semanticweb.org/tswheeler/ontologies/2016/3/EmpowerBP#EnergyObstacle -->

    <owl:NamedIndividual rdf:about="http://www.semanticweb.org/tswheeler/ontologies/2016/3/EmpowerBP#EnergyObstacle">
        <rdf:type rdf:resource="http://www.semanticweb.org/tswheeler/ontologies/2016/3/EmpowerBP#Obstacle"/>
        <EmpowerBP:hasRelevantTDF rdf:resource="http://www.semanticweb.org/tswheeler/ontologies/2016/3/EmpowerBP#EnvironmentalContextResources"/>
        <EmpowerBP:hasRelevantTDF rdf:resource="http://www.semanticweb.org/tswheeler/ontologies/2016/3/EmpowerBP#Goals"/>
        <EmpowerBP:hasRelevantTDF rdf:resource="http://www.semanticweb.org/tswheeler/ontologies/2016/3/EmpowerBP#PhysicalSkill"/>
        <rdfs:comment>Does not have the energy to perform activity.</rdfs:comment>
    </owl:NamedIndividual>
    


    <!-- http://www.semanticweb.org/tswheeler/ontologies/2016/3/EmpowerBP#EnjoymentObstacle -->

    <owl:NamedIndividual rdf:about="http://www.semanticweb.org/tswheeler/ontologies/2016/3/EmpowerBP#EnjoymentObstacle">
        <rdf:type rdf:resource="http://www.semanticweb.org/tswheeler/ontologies/2016/3/EmpowerBP#Obstacle"/>
        <EmpowerBP:hasRelevantTDF rdf:resource="http://www.semanticweb.org/tswheeler/ontologies/2016/3/EmpowerBP#Emotion"/>
        <EmpowerBP:hasRelevantTDF rdf:resource="http://www.semanticweb.org/tswheeler/ontologies/2016/3/EmpowerBP#EnvironmentalContextResources"/>
        <EmpowerBP:hasRelevantTDF rdf:resource="http://www.semanticweb.org/tswheeler/ontologies/2016/3/EmpowerBP#Goals"/>
        <EmpowerBP:hasRelevantTDF rdf:resource="http://www.semanticweb.org/tswheeler/ontologies/2016/3/EmpowerBP#Intentions"/>
        <EmpowerBP:hasRelevantTDF rdf:resource="http://www.semanticweb.org/tswheeler/ontologies/2016/3/EmpowerBP#Reinforcement"/>
        <rdfs:comment>Feels that activity is unenjoyable or boring.</rdfs:comment>
    </owl:NamedIndividual>
    


    <!-- http://www.semanticweb.org/tswheeler/ontologies/2016/3/EmpowerBP#EnvironmentalContextResources -->

    <owl:NamedIndividual rdf:about="http://www.semanticweb.org/tswheeler/ontologies/2016/3/EmpowerBP#EnvironmentalContextResources">
        <rdf:type rdf:resource="http://www.semanticweb.org/tswheeler/ontologies/2016/3/EmpowerBP#Construct"/>
        <rdf:type rdf:resource="http://www.semanticweb.org/tswheeler/ontologies/2016/3/EmpowerBP#TDFDomain"/>
        <EmpowerBP:hasEffectiveInterventionFunction rdf:resource="http://www.semanticweb.org/tswheeler/ontologies/2016/3/EmpowerBP#Enablement"/>
        <EmpowerBP:hasEffectiveInterventionFunction rdf:resource="http://www.semanticweb.org/tswheeler/ontologies/2016/3/EmpowerBP#EnvironmentalRestructuring"/>
        <EmpowerBP:hasEffectiveInterventionFunction rdf:resource="http://www.semanticweb.org/tswheeler/ontologies/2016/3/EmpowerBP#Restriction"/>
        <EmpowerBP:hasEffectiveInterventionFunction rdf:resource="http://www.semanticweb.org/tswheeler/ontologies/2016/3/EmpowerBP#Training"/>
        <EmpowerBP:isRelatedToCOMB rdf:resource="http://www.semanticweb.org/tswheeler/ontologies/2016/3/EmpowerBP#PhysicalOpportunity"/>
        <rdfs:comment>Any circumstance of a person’s situation or environment that discourages or encourages the development of skills and abilities, independence, social competence, and adaptive behavior</rdfs:comment>
        <rdfs:label>Environmental Context and Resources</rdfs:label>
    </owl:NamedIndividual>
    


    <!-- http://www.semanticweb.org/tswheeler/ontologies/2016/3/EmpowerBP#EnvironmentalRestructuring -->

    <owl:NamedIndividual rdf:about="http://www.semanticweb.org/tswheeler/ontologies/2016/3/EmpowerBP#EnvironmentalRestructuring">
        <rdf:type rdf:resource="http://www.semanticweb.org/tswheeler/ontologies/2016/3/EmpowerBP#InterventionFuction"/>
        <EmpowerBP:hasCommonBCT rdf:resource="http://purl.bioontology.org/ontology/BCTT#Associative_learning"/>
        <EmpowerBP:hasCommonBCT rdf:resource="http://purl.bioontology.org/ontology/BCTT#Cue_signalling_reward"/>
        <EmpowerBP:hasCommonBCT rdf:resource="http://purl.bioontology.org/ontology/BCTT#Exposure"/>
        <EmpowerBP:hasCommonBCT rdf:resource="http://purl.bioontology.org/ontology/BCTT#Reduce_prompts-cues"/>
        <EmpowerBP:hasCommonBCT rdf:resource="http://purl.bioontology.org/ontology/BCTT#Remove_access_to_the_reward"/>
        <EmpowerBP:hasCommonBCT rdf:resource="http://purl.bioontology.org/ontology/BCTT#Remove_aversive_stimulus"/>
        <EmpowerBP:hasCommonBCT rdf:resource="http://purl.bioontology.org/ontology/BCTT#Restructuring_the_social_environment"/>
        <EmpowerBP:hasCommonBCT rdf:resource="http://purl.bioontology.org/ontology/BCTT#Satiation"/>
        <EmpowerBP:hasMostCommonBCT rdf:resource="http://purl.bioontology.org/ontology/BCTT#Adding_objects_to_the_environment"/>
        <EmpowerBP:hasMostCommonBCT rdf:resource="http://purl.bioontology.org/ontology/BCTT#Prompts-cues"/>
        <EmpowerBP:hasMostCommonBCT rdf:resource="http://purl.bioontology.org/ontology/BCTT#Restructuring_the_physical_environment"/>
        <EmpowerBP:isEffectiveForTDFDomain rdf:resource="http://www.semanticweb.org/tswheeler/ontologies/2016/3/EmpowerBP#EnvironmentalContextResources"/>
        <EmpowerBP:isEffectiveForTDFDomain rdf:resource="http://www.semanticweb.org/tswheeler/ontologies/2016/3/EmpowerBP#MemoryAttentionDecisionProcesses"/>
        <EmpowerBP:isEffectiveForTDFDomain rdf:resource="http://www.semanticweb.org/tswheeler/ontologies/2016/3/EmpowerBP#Reinforcement"/>
        <EmpowerBP:isEffectiveForTDFDomain rdf:resource="http://www.semanticweb.org/tswheeler/ontologies/2016/3/EmpowerBP#SocialInfluences"/>
        <rdfs:comment>Changing the physical or social context.</rdfs:comment>
    </owl:NamedIndividual>
    


    <!-- http://www.semanticweb.org/tswheeler/ontologies/2016/3/EmpowerBP#ExerciseAMAssessment -->

    <owl:NamedIndividual rdf:about="http://www.semanticweb.org/tswheeler/ontologies/2016/3/EmpowerBP#ExerciseAMAssessment">
        <rdf:type rdf:resource="http://www.semanticweb.org/tswheeler/ontologies/2016/3/EmpowerBP#Assessment"/>
        <rdf:type rdf:resource="http://www.semanticweb.org/tswheeler/ontologies/2016/3/EmpowerBP#AssessmentItem"/>
        <rdf:type rdf:resource="http://www.semanticweb.org/tswheeler/ontologies/2016/3/EmpowerBP#AutomaticMotivationAssessment"/>
        <rdf:type rdf:resource="http://www.semanticweb.org/tswheeler/ontologies/2016/3/EmpowerBP#COMBAssessment"/>
        <EmpowerBP:evaluatesConstruct rdf:resource="http://www.semanticweb.org/tswheeler/ontologies/2016/3/EmpowerBP#AutomaticMotivation"/>
        <EmpowerBP:isSpecificToGoal rdf:resource="http://www.semanticweb.org/tswheeler/ontologies/2016/3/EmpowerBP#ExerciseMore"/>
    </owl:NamedIndividual>
    


    <!-- http://www.semanticweb.org/tswheeler/ontologies/2016/3/EmpowerBP#ExerciseMore -->

    <owl:NamedIndividual rdf:about="http://www.semanticweb.org/tswheeler/ontologies/2016/3/EmpowerBP#ExerciseMore">
        <rdf:type rdf:resource="http://www.semanticweb.org/tswheeler/ontologies/2016/3/EmpowerBP#AcquisitionGoal"/>
        <rdf:type rdf:resource="http://www.semanticweb.org/tswheeler/ontologies/2016/3/EmpowerBP#InterventionGoal"/>
    </owl:NamedIndividual>
    


    <!-- http://www.semanticweb.org/tswheeler/ontologies/2016/3/EmpowerBP#ExercisePOAssessment -->

    <owl:NamedIndividual rdf:about="http://www.semanticweb.org/tswheeler/ontologies/2016/3/EmpowerBP#ExercisePOAssessment">
        <rdf:type rdf:resource="http://www.semanticweb.org/tswheeler/ontologies/2016/3/EmpowerBP#Assessment"/>
        <rdf:type rdf:resource="http://www.semanticweb.org/tswheeler/ontologies/2016/3/EmpowerBP#AssessmentItem"/>
        <rdf:type rdf:resource="http://www.semanticweb.org/tswheeler/ontologies/2016/3/EmpowerBP#COMBAssessment"/>
        <rdf:type rdf:resource="http://www.semanticweb.org/tswheeler/ontologies/2016/3/EmpowerBP#PhysicalOpportunityAssessment"/>
        <EmpowerBP:evaluatesConstruct rdf:resource="http://www.semanticweb.org/tswheeler/ontologies/2016/3/EmpowerBP#PhysicalOpportunity"/>
        <EmpowerBP:isSpecificToGoal rdf:resource="http://www.semanticweb.org/tswheeler/ontologies/2016/3/EmpowerBP#ExerciseMore"/>
    </owl:NamedIndividual>
    


    <!-- http://www.semanticweb.org/tswheeler/ontologies/2016/3/EmpowerBP#ExercisePhysCAssessment -->

    <owl:NamedIndividual rdf:about="http://www.semanticweb.org/tswheeler/ontologies/2016/3/EmpowerBP#ExercisePhysCAssessment">
        <rdf:type rdf:resource="http://www.semanticweb.org/tswheeler/ontologies/2016/3/EmpowerBP#Assessment"/>
        <rdf:type rdf:resource="http://www.semanticweb.org/tswheeler/ontologies/2016/3/EmpowerBP#AssessmentItem"/>
        <rdf:type rdf:resource="http://www.semanticweb.org/tswheeler/ontologies/2016/3/EmpowerBP#COMBAssessment"/>
        <rdf:type rdf:resource="http://www.semanticweb.org/tswheeler/ontologies/2016/3/EmpowerBP#PhysicalCapabilityAssessment"/>
        <EmpowerBP:evaluatesConstruct rdf:resource="http://www.semanticweb.org/tswheeler/ontologies/2016/3/EmpowerBP#PhysicalCapability"/>
        <EmpowerBP:isSpecificToGoal rdf:resource="http://www.semanticweb.org/tswheeler/ontologies/2016/3/EmpowerBP#ExerciseMore"/>
    </owl:NamedIndividual>
    


    <!-- http://www.semanticweb.org/tswheeler/ontologies/2016/3/EmpowerBP#ExercisePsychCAssessment -->

    <owl:NamedIndividual rdf:about="http://www.semanticweb.org/tswheeler/ontologies/2016/3/EmpowerBP#ExercisePsychCAssessment">
        <rdf:type rdf:resource="http://www.semanticweb.org/tswheeler/ontologies/2016/3/EmpowerBP#Assessment"/>
        <rdf:type rdf:resource="http://www.semanticweb.org/tswheeler/ontologies/2016/3/EmpowerBP#AssessmentItem"/>
        <rdf:type rdf:resource="http://www.semanticweb.org/tswheeler/ontologies/2016/3/EmpowerBP#COMBAssessment"/>
        <rdf:type rdf:resource="http://www.semanticweb.org/tswheeler/ontologies/2016/3/EmpowerBP#PsychologicalCapabilityAssessment"/>
        <EmpowerBP:evaluatesConstruct rdf:resource="http://www.semanticweb.org/tswheeler/ontologies/2016/3/EmpowerBP#PsychologicalCapability"/>
        <EmpowerBP:isSpecificToGoal rdf:resource="http://www.semanticweb.org/tswheeler/ontologies/2016/3/EmpowerBP#ExerciseMore"/>
    </owl:NamedIndividual>
    


    <!-- http://www.semanticweb.org/tswheeler/ontologies/2016/3/EmpowerBP#ExerciseRMAssessment -->

    <owl:NamedIndividual rdf:about="http://www.semanticweb.org/tswheeler/ontologies/2016/3/EmpowerBP#ExerciseRMAssessment">
        <rdf:type rdf:resource="http://www.semanticweb.org/tswheeler/ontologies/2016/3/EmpowerBP#Assessment"/>
        <rdf:type rdf:resource="http://www.semanticweb.org/tswheeler/ontologies/2016/3/EmpowerBP#AssessmentItem"/>
        <rdf:type rdf:resource="http://www.semanticweb.org/tswheeler/ontologies/2016/3/EmpowerBP#COMBAssessment"/>
        <rdf:type rdf:resource="http://www.semanticweb.org/tswheeler/ontologies/2016/3/EmpowerBP#ReflectiveMotivationAssessment"/>
        <EmpowerBP:evaluatesConstruct rdf:resource="http://www.semanticweb.org/tswheeler/ontologies/2016/3/EmpowerBP#ReflectiveMotivation"/>
        <EmpowerBP:isSpecificToGoal rdf:resource="http://www.semanticweb.org/tswheeler/ontologies/2016/3/EmpowerBP#ExerciseMore"/>
    </owl:NamedIndividual>
    


    <!-- http://www.semanticweb.org/tswheeler/ontologies/2016/3/EmpowerBP#ExerciseSOAssessment -->

    <owl:NamedIndividual rdf:about="http://www.semanticweb.org/tswheeler/ontologies/2016/3/EmpowerBP#ExerciseSOAssessment">
        <rdf:type rdf:resource="http://www.semanticweb.org/tswheeler/ontologies/2016/3/EmpowerBP#Assessment"/>
        <rdf:type rdf:resource="http://www.semanticweb.org/tswheeler/ontologies/2016/3/EmpowerBP#AssessmentItem"/>
        <rdf:type rdf:resource="http://www.semanticweb.org/tswheeler/ontologies/2016/3/EmpowerBP#COMBAssessment"/>
        <rdf:type rdf:resource="http://www.semanticweb.org/tswheeler/ontologies/2016/3/EmpowerBP#SocialOpportunityAssessment"/>
        <EmpowerBP:evaluatesConstruct rdf:resource="http://www.semanticweb.org/tswheeler/ontologies/2016/3/EmpowerBP#SocialOpportunity"/>
        <EmpowerBP:isSpecificToGoal rdf:resource="http://www.semanticweb.org/tswheeler/ontologies/2016/3/EmpowerBP#ExerciseMore"/>
    </owl:NamedIndividual>
    


    <!-- http://www.semanticweb.org/tswheeler/ontologies/2016/3/EmpowerBP#Goals -->

    <owl:NamedIndividual rdf:about="http://www.semanticweb.org/tswheeler/ontologies/2016/3/EmpowerBP#Goals">
        <rdf:type rdf:resource="http://www.semanticweb.org/tswheeler/ontologies/2016/3/EmpowerBP#Construct"/>
        <rdf:type rdf:resource="http://www.semanticweb.org/tswheeler/ontologies/2016/3/EmpowerBP#TDFDomain"/>
        <EmpowerBP:hasEffectiveInterventionFunction rdf:resource="http://www.semanticweb.org/tswheeler/ontologies/2016/3/EmpowerBP#Coercion"/>
        <EmpowerBP:hasEffectiveInterventionFunction rdf:resource="http://www.semanticweb.org/tswheeler/ontologies/2016/3/EmpowerBP#Education"/>
        <EmpowerBP:hasEffectiveInterventionFunction rdf:resource="http://www.semanticweb.org/tswheeler/ontologies/2016/3/EmpowerBP#Enablement"/>
        <EmpowerBP:hasEffectiveInterventionFunction rdf:resource="http://www.semanticweb.org/tswheeler/ontologies/2016/3/EmpowerBP#Incentivisation"/>
        <EmpowerBP:hasEffectiveInterventionFunction rdf:resource="http://www.semanticweb.org/tswheeler/ontologies/2016/3/EmpowerBP#Modelling"/>
        <EmpowerBP:hasEffectiveInterventionFunction rdf:resource="http://www.semanticweb.org/tswheeler/ontologies/2016/3/EmpowerBP#Persuasion"/>
        <EmpowerBP:isRelatedToCOMB rdf:resource="http://www.semanticweb.org/tswheeler/ontologies/2016/3/EmpowerBP#ReflectiveMotivation"/>
        <rdfs:comment>Mental representation of outcomes or end states that an individual wants to achieve</rdfs:comment>
    </owl:NamedIndividual>
    


    <!-- http://www.semanticweb.org/tswheeler/ontologies/2016/3/EmpowerBP#H1 -->

    <owl:NamedIndividual rdf:about="http://www.semanticweb.org/tswheeler/ontologies/2016/3/EmpowerBP#H1">
        <rdf:type rdf:resource="http://www.semanticweb.org/tswheeler/ontologies/2016/3/EmpowerBP#InterventionItem"/>
        <rdf:type rdf:resource="http://www.semanticweb.org/tswheeler/ontologies/2016/3/EmpowerBP#Task"/>
        <EmpowerBP:isAppropriateForInterventionGoal rdf:resource="http://www.semanticweb.org/tswheeler/ontologies/2016/3/EmpowerBP#ExerciseMore"/>
        <EmpowerBP:isWarrantedBy rdf:resource="http://purl.bioontology.org/ontology/BCTT#Information_about_health_consequences"/>
        <EmpowerBP:appropriateForAutomaticMotivation rdf:datatype="http://www.w3.org/2001/XMLSchema#integer">3</EmpowerBP:appropriateForAutomaticMotivation>
        <EmpowerBP:appropriateForLocation rdf:datatype="http://www.w3.org/2001/XMLSchema#integer">0</EmpowerBP:appropriateForLocation>
        <EmpowerBP:appropriateForPhysicalCapability rdf:datatype="http://www.w3.org/2001/XMLSchema#integer">3</EmpowerBP:appropriateForPhysicalCapability>
        <EmpowerBP:appropriateForPhysicalOpportunity rdf:datatype="http://www.w3.org/2001/XMLSchema#integer">3</EmpowerBP:appropriateForPhysicalOpportunity>
        <EmpowerBP:appropriateForPsychologicalCapability rdf:datatype="http://www.w3.org/2001/XMLSchema#integer">3</EmpowerBP:appropriateForPsychologicalCapability>
        <EmpowerBP:appropriateForReflectiveMotivation rdf:datatype="http://www.w3.org/2001/XMLSchema#integer">3</EmpowerBP:appropriateForReflectiveMotivation>
        <EmpowerBP:appropriateForSocialOpportunity rdf:datatype="http://www.w3.org/2001/XMLSchema#integer">3</EmpowerBP:appropriateForSocialOpportunity>
        <EmpowerBP:canRepeat rdf:datatype="http://www.w3.org/2001/XMLSchema#integer">52</EmpowerBP:canRepeat>
        <EmpowerBP:itemName rdf:datatype="http://www.w3.org/2001/XMLSchema#string">&quot;Be Active!&quot; Quiz</EmpowerBP:itemName>
        <EmpowerBP:itemText rdf:datatype="http://www.w3.org/2001/XMLSchema#string">Take the Public Health Agency of Canada &quot;Be Active!&quot; quiz.</EmpowerBP:itemText>
        <EmpowerBP:maximumUserAge rdf:datatype="http://www.w3.org/2001/XMLSchema#integer">120</EmpowerBP:maximumUserAge>
        <EmpowerBP:minimumUserAge rdf:datatype="http://www.w3.org/2001/XMLSchema#integer">18</EmpowerBP:minimumUserAge>
        <EmpowerBP:provideJournal rdf:datatype="http://www.w3.org/2001/XMLSchema#boolean">false</EmpowerBP:provideJournal>
        <EmpowerBP:provideLink rdf:datatype="http://www.w3.org/2001/XMLSchema#boolean">true</EmpowerBP:provideLink>
        <EmpowerBP:sourceURL rdf:datatype="http://www.w3.org/2001/XMLSchema#string">http://www.phac-aspc.gc.ca/app/pag-gap/facebook/beactive/</EmpowerBP:sourceURL>
        <rdfs:comment rdf:datatype="http://www.w3.org/2001/XMLSchema#string">Take the Public Health Agency of Canada &quot;Be Active!&quot; quiz.</rdfs:comment>
        <rdfs:label rdf:datatype="http://www.w3.org/2001/XMLSchema#string">&quot;Be Active!&quot; Quiz</rdfs:label>
    </owl:NamedIndividual>
    


    <!-- http://www.semanticweb.org/tswheeler/ontologies/2016/3/EmpowerBP#H10 -->

    <owl:NamedIndividual rdf:about="http://www.semanticweb.org/tswheeler/ontologies/2016/3/EmpowerBP#H10">
        <rdf:type rdf:resource="http://www.semanticweb.org/tswheeler/ontologies/2016/3/EmpowerBP#InterventionItem"/>
        <rdf:type rdf:resource="http://www.semanticweb.org/tswheeler/ontologies/2016/3/EmpowerBP#Task"/>
        <EmpowerBP:isAppropriateForInterventionGoal rdf:resource="http://www.semanticweb.org/tswheeler/ontologies/2016/3/EmpowerBP#ReduceSaltIntake"/>
        <EmpowerBP:isWarrantedBy rdf:resource="http://purl.bioontology.org/ontology/BCTT#Behavioral_experiments"/>
        <EmpowerBP:appropriateForAutomaticMotivation rdf:datatype="http://www.w3.org/2001/XMLSchema#integer">6</EmpowerBP:appropriateForAutomaticMotivation>
        <EmpowerBP:appropriateForLocation rdf:datatype="http://www.w3.org/2001/XMLSchema#integer">0</EmpowerBP:appropriateForLocation>
        <EmpowerBP:appropriateForPhysicalCapability rdf:datatype="http://www.w3.org/2001/XMLSchema#integer">3</EmpowerBP:appropriateForPhysicalCapability>
        <EmpowerBP:appropriateForPhysicalOpportunity rdf:datatype="http://www.w3.org/2001/XMLSchema#integer">3</EmpowerBP:appropriateForPhysicalOpportunity>
        <EmpowerBP:appropriateForPsychologicalCapability rdf:datatype="http://www.w3.org/2001/XMLSchema#integer">3</EmpowerBP:appropriateForPsychologicalCapability>
        <EmpowerBP:appropriateForReflectiveMotivation rdf:datatype="http://www.w3.org/2001/XMLSchema#integer">6</EmpowerBP:appropriateForReflectiveMotivation>
        <EmpowerBP:appropriateForSocialOpportunity rdf:datatype="http://www.w3.org/2001/XMLSchema#integer">3</EmpowerBP:appropriateForSocialOpportunity>
        <EmpowerBP:canRepeat rdf:datatype="http://www.w3.org/2001/XMLSchema#integer">52</EmpowerBP:canRepeat>
        <EmpowerBP:itemName rdf:datatype="http://www.w3.org/2001/XMLSchema#string">Sodium Content of Some Common Foods</EmpowerBP:itemName>
        <EmpowerBP:itemText rdf:datatype="http://www.w3.org/2001/XMLSchema#string">Sodium Content of Some Common Foods

Spend a few minutes looking at the chart on the linked page. Itlists how much sodium can be found in some foods and, can help you to choose foods that are lower in sodium. Are you surprised by the amount of sodium in any of the listed foods? </EmpowerBP:itemText>
        <EmpowerBP:maximumUserAge rdf:datatype="http://www.w3.org/2001/XMLSchema#integer">120</EmpowerBP:maximumUserAge>
        <EmpowerBP:minimumUserAge rdf:datatype="http://www.w3.org/2001/XMLSchema#integer">18</EmpowerBP:minimumUserAge>
        <EmpowerBP:provideJournal rdf:datatype="http://www.w3.org/2001/XMLSchema#boolean">false</EmpowerBP:provideJournal>
        <EmpowerBP:provideLink rdf:datatype="http://www.w3.org/2001/XMLSchema#boolean">true</EmpowerBP:provideLink>
        <EmpowerBP:sourceURL rdf:datatype="http://www.w3.org/2001/XMLSchema#string">http://www.dietitians.ca/getattachment/ff62244f-1300-4ba5-bebd-208c3db61adc/FACTSHEET-Food-Sources-of-Sodium.pdf.aspx</EmpowerBP:sourceURL>
        <rdfs:comment rdf:datatype="http://www.w3.org/2001/XMLSchema#string">Sodium Content of Some Common Foods

Spend a few minutes looking at the chart on the linked page. Itlists how much sodium can be found in some foods and, can help you to choose foods that are lower in sodium. Are you surprised by the amount of sodium in any of the listed foods? </rdfs:comment>
        <rdfs:label rdf:datatype="http://www.w3.org/2001/XMLSchema#string">Sodium Content of Some Common Foods</rdfs:label>
    </owl:NamedIndividual>
    


    <!-- http://www.semanticweb.org/tswheeler/ontologies/2016/3/EmpowerBP#H11 -->

    <owl:NamedIndividual rdf:about="http://www.semanticweb.org/tswheeler/ontologies/2016/3/EmpowerBP#H11">
        <rdf:type rdf:resource="http://www.semanticweb.org/tswheeler/ontologies/2016/3/EmpowerBP#InterventionItem"/>
        <rdf:type rdf:resource="http://www.semanticweb.org/tswheeler/ontologies/2016/3/EmpowerBP#Task"/>
        <EmpowerBP:isAppropriateForInterventionGoal rdf:resource="http://www.semanticweb.org/tswheeler/ontologies/2016/3/EmpowerBP#ReduceSaltIntake"/>
        <EmpowerBP:isWarrantedBy rdf:resource="http://purl.bioontology.org/ontology/BCTT#Information_about_health_consequences"/>
        <EmpowerBP:appropriateForAutomaticMotivation rdf:datatype="http://www.w3.org/2001/XMLSchema#integer">3</EmpowerBP:appropriateForAutomaticMotivation>
        <EmpowerBP:appropriateForLocation rdf:datatype="http://www.w3.org/2001/XMLSchema#integer">0</EmpowerBP:appropriateForLocation>
        <EmpowerBP:appropriateForPhysicalCapability rdf:datatype="http://www.w3.org/2001/XMLSchema#integer">3</EmpowerBP:appropriateForPhysicalCapability>
        <EmpowerBP:appropriateForPhysicalOpportunity rdf:datatype="http://www.w3.org/2001/XMLSchema#integer">3</EmpowerBP:appropriateForPhysicalOpportunity>
        <EmpowerBP:appropriateForPsychologicalCapability rdf:datatype="http://www.w3.org/2001/XMLSchema#integer">3</EmpowerBP:appropriateForPsychologicalCapability>
        <EmpowerBP:appropriateForReflectiveMotivation rdf:datatype="http://www.w3.org/2001/XMLSchema#integer">3</EmpowerBP:appropriateForReflectiveMotivation>
        <EmpowerBP:appropriateForSocialOpportunity rdf:datatype="http://www.w3.org/2001/XMLSchema#integer">3</EmpowerBP:appropriateForSocialOpportunity>
        <EmpowerBP:canRepeat rdf:datatype="http://www.w3.org/2001/XMLSchema#integer">52</EmpowerBP:canRepeat>
        <EmpowerBP:itemName rdf:datatype="http://www.w3.org/2001/XMLSchema#string">Hypertension Canada Sodium Quiz</EmpowerBP:itemName>
        <EmpowerBP:itemText rdf:datatype="http://www.w3.org/2001/XMLSchema#string">How much do you know about sodium and your health? Take the quiz and discover if you’re sodium savvy!</EmpowerBP:itemText>
        <EmpowerBP:maximumUserAge rdf:datatype="http://www.w3.org/2001/XMLSchema#integer">120</EmpowerBP:maximumUserAge>
        <EmpowerBP:minimumUserAge rdf:datatype="http://www.w3.org/2001/XMLSchema#integer">18</EmpowerBP:minimumUserAge>
        <EmpowerBP:provideJournal rdf:datatype="http://www.w3.org/2001/XMLSchema#boolean">false</EmpowerBP:provideJournal>
        <EmpowerBP:provideLink rdf:datatype="http://www.w3.org/2001/XMLSchema#boolean">true</EmpowerBP:provideLink>
        <EmpowerBP:sourceURL rdf:datatype="http://www.w3.org/2001/XMLSchema#string">https://www.hypertension.ca/images/2014_EducationalResources/2014_SodiumQuizPaper_P1021_EN.pdf</EmpowerBP:sourceURL>
        <rdfs:comment rdf:datatype="http://www.w3.org/2001/XMLSchema#string">How much do you know about sodium and your health? Take the quiz and discover if you’re sodium savvy!</rdfs:comment>
        <rdfs:label rdf:datatype="http://www.w3.org/2001/XMLSchema#string">Hypertension Canada Sodium Quiz</rdfs:label>
    </owl:NamedIndividual>
    


    <!-- http://www.semanticweb.org/tswheeler/ontologies/2016/3/EmpowerBP#H12 -->

    <owl:NamedIndividual rdf:about="http://www.semanticweb.org/tswheeler/ontologies/2016/3/EmpowerBP#H12">
        <rdf:type rdf:resource="http://www.semanticweb.org/tswheeler/ontologies/2016/3/EmpowerBP#InterventionItem"/>
        <rdf:type rdf:resource="http://www.semanticweb.org/tswheeler/ontologies/2016/3/EmpowerBP#Task"/>
        <EmpowerBP:isAppropriateForInterventionGoal rdf:resource="http://www.semanticweb.org/tswheeler/ontologies/2016/3/EmpowerBP#ReduceSaltIntake"/>
        <EmpowerBP:isWarrantedBy rdf:resource="http://purl.bioontology.org/ontology/BCTT#Instruction_on_how_to_perform_the_behavior"/>
        <EmpowerBP:appropriateForAutomaticMotivation rdf:datatype="http://www.w3.org/2001/XMLSchema#integer">6</EmpowerBP:appropriateForAutomaticMotivation>
        <EmpowerBP:appropriateForLocation rdf:datatype="http://www.w3.org/2001/XMLSchema#integer">0</EmpowerBP:appropriateForLocation>
        <EmpowerBP:appropriateForPhysicalCapability rdf:datatype="http://www.w3.org/2001/XMLSchema#integer">3</EmpowerBP:appropriateForPhysicalCapability>
        <EmpowerBP:appropriateForPhysicalOpportunity rdf:datatype="http://www.w3.org/2001/XMLSchema#integer">3</EmpowerBP:appropriateForPhysicalOpportunity>
        <EmpowerBP:appropriateForPsychologicalCapability rdf:datatype="http://www.w3.org/2001/XMLSchema#integer">3</EmpowerBP:appropriateForPsychologicalCapability>
        <EmpowerBP:appropriateForReflectiveMotivation rdf:datatype="http://www.w3.org/2001/XMLSchema#integer">6</EmpowerBP:appropriateForReflectiveMotivation>
        <EmpowerBP:appropriateForSocialOpportunity rdf:datatype="http://www.w3.org/2001/XMLSchema#integer">3</EmpowerBP:appropriateForSocialOpportunity>
        <EmpowerBP:canRepeat rdf:datatype="http://www.w3.org/2001/XMLSchema#integer">52</EmpowerBP:canRepeat>
        <EmpowerBP:itemName rdf:datatype="http://www.w3.org/2001/XMLSchema#string">Sodium101 Video</EmpowerBP:itemName>
        <EmpowerBP:itemText rdf:datatype="http://www.w3.org/2001/XMLSchema#string">Watch this short 3-minute video from the Canadian Stroke Network on how you can take control of your daily sodium intake. </EmpowerBP:itemText>
        <EmpowerBP:maximumUserAge rdf:datatype="http://www.w3.org/2001/XMLSchema#integer">120</EmpowerBP:maximumUserAge>
        <EmpowerBP:minimumUserAge rdf:datatype="http://www.w3.org/2001/XMLSchema#integer">18</EmpowerBP:minimumUserAge>
        <EmpowerBP:provideJournal rdf:datatype="http://www.w3.org/2001/XMLSchema#boolean">false</EmpowerBP:provideJournal>
        <EmpowerBP:provideLink rdf:datatype="http://www.w3.org/2001/XMLSchema#boolean">true</EmpowerBP:provideLink>
        <EmpowerBP:sourceURL rdf:datatype="http://www.w3.org/2001/XMLSchema#string">https://www.youtube.com/watch?v=6usUql4bpvo</EmpowerBP:sourceURL>
        <rdfs:comment rdf:datatype="http://www.w3.org/2001/XMLSchema#string">Watch this short 3-minute video from the Canadian Stroke Network on how you can take control of your daily sodium intake. </rdfs:comment>
        <rdfs:label rdf:datatype="http://www.w3.org/2001/XMLSchema#string">Sodium101 Video</rdfs:label>
    </owl:NamedIndividual>
    


    <!-- http://www.semanticweb.org/tswheeler/ontologies/2016/3/EmpowerBP#H13 -->

    <owl:NamedIndividual rdf:about="http://www.semanticweb.org/tswheeler/ontologies/2016/3/EmpowerBP#H13">
        <rdf:type rdf:resource="http://www.semanticweb.org/tswheeler/ontologies/2016/3/EmpowerBP#InterventionItem"/>
        <rdf:type rdf:resource="http://www.semanticweb.org/tswheeler/ontologies/2016/3/EmpowerBP#Task"/>
        <EmpowerBP:isAppropriateForInterventionGoal rdf:resource="http://www.semanticweb.org/tswheeler/ontologies/2016/3/EmpowerBP#ReduceSaltIntake"/>
        <EmpowerBP:isWarrantedBy rdf:resource="http://purl.bioontology.org/ontology/BCTT#Instruction_on_how_to_perform_the_behavior"/>
        <EmpowerBP:appropriateForAutomaticMotivation rdf:datatype="http://www.w3.org/2001/XMLSchema#integer">3</EmpowerBP:appropriateForAutomaticMotivation>
        <EmpowerBP:appropriateForLocation rdf:datatype="http://www.w3.org/2001/XMLSchema#integer">0</EmpowerBP:appropriateForLocation>
        <EmpowerBP:appropriateForPhysicalCapability rdf:datatype="http://www.w3.org/2001/XMLSchema#integer">3</EmpowerBP:appropriateForPhysicalCapability>
        <EmpowerBP:appropriateForPhysicalOpportunity rdf:datatype="http://www.w3.org/2001/XMLSchema#integer">3</EmpowerBP:appropriateForPhysicalOpportunity>
        <EmpowerBP:appropriateForPsychologicalCapability rdf:datatype="http://www.w3.org/2001/XMLSchema#integer">3</EmpowerBP:appropriateForPsychologicalCapability>
        <EmpowerBP:appropriateForReflectiveMotivation rdf:datatype="http://www.w3.org/2001/XMLSchema#integer">3</EmpowerBP:appropriateForReflectiveMotivation>
        <EmpowerBP:appropriateForSocialOpportunity rdf:datatype="http://www.w3.org/2001/XMLSchema#integer">3</EmpowerBP:appropriateForSocialOpportunity>
        <EmpowerBP:canRepeat rdf:datatype="http://www.w3.org/2001/XMLSchema#integer">52</EmpowerBP:canRepeat>
        <EmpowerBP:itemName rdf:datatype="http://www.w3.org/2001/XMLSchema#string">Sodium Detector</EmpowerBP:itemName>
        <EmpowerBP:itemText rdf:datatype="http://www.w3.org/2001/XMLSchema#string">Learn how much sodium is in the foods that you eat. Use the Sodium Interactive Tool to find out how much sodium is in processed foods, ingredients high in sodium that are added during cooking and at the table, and foods with naturally occurring sodium.</EmpowerBP:itemText>
        <EmpowerBP:maximumUserAge rdf:datatype="http://www.w3.org/2001/XMLSchema#integer">120</EmpowerBP:maximumUserAge>
        <EmpowerBP:minimumUserAge rdf:datatype="http://www.w3.org/2001/XMLSchema#integer">18</EmpowerBP:minimumUserAge>
        <EmpowerBP:provideJournal rdf:datatype="http://www.w3.org/2001/XMLSchema#boolean">false</EmpowerBP:provideJournal>
        <EmpowerBP:provideLink rdf:datatype="http://www.w3.org/2001/XMLSchema#boolean">true</EmpowerBP:provideLink>
        <EmpowerBP:sourceURL rdf:datatype="http://www.w3.org/2001/XMLSchema#string">http://www.healthycanadians.gc.ca/eating-nutrition/healthy-eating-saine-alimentation/nutrients-nutriments/sodium/detector-depisteur-eng.php</EmpowerBP:sourceURL>
        <rdfs:comment rdf:datatype="http://www.w3.org/2001/XMLSchema#string">Learn how much sodium is in the foods that you eat. Use the Sodium Interactive Tool to find out how much sodium is in processed foods, ingredients high in sodium that are added during cooking and at the table, and foods with naturally occurring sodium.</rdfs:comment>
        <rdfs:label rdf:datatype="http://www.w3.org/2001/XMLSchema#string">Sodium Detector</rdfs:label>
    </owl:NamedIndividual>
    


    <!-- http://www.semanticweb.org/tswheeler/ontologies/2016/3/EmpowerBP#H14 -->

    <owl:NamedIndividual rdf:about="http://www.semanticweb.org/tswheeler/ontologies/2016/3/EmpowerBP#H14">
        <rdf:type rdf:resource="http://www.semanticweb.org/tswheeler/ontologies/2016/3/EmpowerBP#InterventionItem"/>
        <rdf:type rdf:resource="http://www.semanticweb.org/tswheeler/ontologies/2016/3/EmpowerBP#Task"/>
        <EmpowerBP:isAppropriateForInterventionGoal rdf:resource="http://www.semanticweb.org/tswheeler/ontologies/2016/3/EmpowerBP#ReduceSaltIntake"/>
        <EmpowerBP:isWarrantedBy rdf:resource="http://purl.bioontology.org/ontology/BCTT#Prompts-cues"/>
        <EmpowerBP:appropriateForAutomaticMotivation rdf:datatype="http://www.w3.org/2001/XMLSchema#integer">6</EmpowerBP:appropriateForAutomaticMotivation>
        <EmpowerBP:appropriateForLocation rdf:datatype="http://www.w3.org/2001/XMLSchema#integer">0</EmpowerBP:appropriateForLocation>
        <EmpowerBP:appropriateForPhysicalCapability rdf:datatype="http://www.w3.org/2001/XMLSchema#integer">3</EmpowerBP:appropriateForPhysicalCapability>
        <EmpowerBP:appropriateForPhysicalOpportunity rdf:datatype="http://www.w3.org/2001/XMLSchema#integer">3</EmpowerBP:appropriateForPhysicalOpportunity>
        <EmpowerBP:appropriateForPsychologicalCapability rdf:datatype="http://www.w3.org/2001/XMLSchema#integer">3</EmpowerBP:appropriateForPsychologicalCapability>
        <EmpowerBP:appropriateForReflectiveMotivation rdf:datatype="http://www.w3.org/2001/XMLSchema#integer">6</EmpowerBP:appropriateForReflectiveMotivation>
        <EmpowerBP:appropriateForSocialOpportunity rdf:datatype="http://www.w3.org/2001/XMLSchema#integer">3</EmpowerBP:appropriateForSocialOpportunity>
        <EmpowerBP:canRepeat rdf:datatype="http://www.w3.org/2001/XMLSchema#integer">52</EmpowerBP:canRepeat>
        <EmpowerBP:itemName rdf:datatype="http://www.w3.org/2001/XMLSchema#string">Create a personalized food guide</EmpowerBP:itemName>
        <EmpowerBP:itemText rdf:datatype="http://www.w3.org/2001/XMLSchema#string">My Food Guide is an interactive tool that customizes Canada&apos;s Food Guide just for you.

Follow the link to the site and create your personalized guide. It takes about five minutes. You can then print it and stick it on your fridge for quick and easy reference!</EmpowerBP:itemText>
        <EmpowerBP:maximumUserAge rdf:datatype="http://www.w3.org/2001/XMLSchema#integer">120</EmpowerBP:maximumUserAge>
        <EmpowerBP:minimumUserAge rdf:datatype="http://www.w3.org/2001/XMLSchema#integer">18</EmpowerBP:minimumUserAge>
        <EmpowerBP:provideJournal rdf:datatype="http://www.w3.org/2001/XMLSchema#boolean">false</EmpowerBP:provideJournal>
        <EmpowerBP:provideLink rdf:datatype="http://www.w3.org/2001/XMLSchema#boolean">true</EmpowerBP:provideLink>
        <EmpowerBP:sourceURL rdf:datatype="http://www.w3.org/2001/XMLSchema#string">http://www.healthycanadians.gc.ca/eating-nutrition/healthy-eating-saine-alimentation/food-guide-aliment/my-guide-mon-guide/mfg_p1-eng.php</EmpowerBP:sourceURL>
        <rdfs:comment rdf:datatype="http://www.w3.org/2001/XMLSchema#string">My Food Guide is an interactive tool that customizes Canada&apos;s Food Guide just for you.

Follow the link to the site and create your personalized guide. It takes about five minutes. You can then print it and stick it on your fridge for quick and easy reference!</rdfs:comment>
        <rdfs:label rdf:datatype="http://www.w3.org/2001/XMLSchema#string">Create a personalized food guide</rdfs:label>
    </owl:NamedIndividual>
    


    <!-- http://www.semanticweb.org/tswheeler/ontologies/2016/3/EmpowerBP#H15 -->

    <owl:NamedIndividual rdf:about="http://www.semanticweb.org/tswheeler/ontologies/2016/3/EmpowerBP#H15">
        <rdf:type rdf:resource="http://www.semanticweb.org/tswheeler/ontologies/2016/3/EmpowerBP#InterventionItem"/>
        <rdf:type rdf:resource="http://www.semanticweb.org/tswheeler/ontologies/2016/3/EmpowerBP#Task"/>
        <EmpowerBP:isAppropriateForInterventionGoal rdf:resource="http://www.semanticweb.org/tswheeler/ontologies/2016/3/EmpowerBP#ExerciseMore"/>
        <EmpowerBP:isWarrantedBy rdf:resource="http://purl.bioontology.org/ontology/BCTT#Action_planning"/>
        <EmpowerBP:appropriateForAutomaticMotivation rdf:datatype="http://www.w3.org/2001/XMLSchema#integer">6</EmpowerBP:appropriateForAutomaticMotivation>
        <EmpowerBP:appropriateForLocation rdf:datatype="http://www.w3.org/2001/XMLSchema#integer">0</EmpowerBP:appropriateForLocation>
        <EmpowerBP:appropriateForPhysicalCapability rdf:datatype="http://www.w3.org/2001/XMLSchema#integer">6</EmpowerBP:appropriateForPhysicalCapability>
        <EmpowerBP:appropriateForPhysicalOpportunity rdf:datatype="http://www.w3.org/2001/XMLSchema#integer">6</EmpowerBP:appropriateForPhysicalOpportunity>
        <EmpowerBP:appropriateForPsychologicalCapability rdf:datatype="http://www.w3.org/2001/XMLSchema#integer">6</EmpowerBP:appropriateForPsychologicalCapability>
        <EmpowerBP:appropriateForReflectiveMotivation rdf:datatype="http://www.w3.org/2001/XMLSchema#integer">6</EmpowerBP:appropriateForReflectiveMotivation>
        <EmpowerBP:appropriateForSocialOpportunity rdf:datatype="http://www.w3.org/2001/XMLSchema#integer">6</EmpowerBP:appropriateForSocialOpportunity>
        <EmpowerBP:canRepeat rdf:datatype="http://www.w3.org/2001/XMLSchema#integer">52</EmpowerBP:canRepeat>
        <EmpowerBP:itemName rdf:datatype="http://www.w3.org/2001/XMLSchema#string">Nearby Gyms</EmpowerBP:itemName>
        <EmpowerBP:itemText rdf:datatype="http://www.w3.org/2001/XMLSchema#string">Joining a gym can encourage people to become more regularly active. Gyms can be a great place to learn new ways to be active, and professionals are available to offer advice on fitness and exercise. 

Have you considered joining a gym? Why or why not? Try searching online  for gyms near you. </EmpowerBP:itemText>
        <EmpowerBP:maximumUserAge rdf:datatype="http://www.w3.org/2001/XMLSchema#integer">120</EmpowerBP:maximumUserAge>
        <EmpowerBP:minimumUserAge rdf:datatype="http://www.w3.org/2001/XMLSchema#integer">18</EmpowerBP:minimumUserAge>
        <EmpowerBP:provideJournal rdf:datatype="http://www.w3.org/2001/XMLSchema#boolean">false</EmpowerBP:provideJournal>
        <EmpowerBP:provideLink rdf:datatype="http://www.w3.org/2001/XMLSchema#boolean">true</EmpowerBP:provideLink>
        <EmpowerBP:sourceURL rdf:datatype="http://www.w3.org/2001/XMLSchema#string">https://www.google.ca/#q=gyms+near+me</EmpowerBP:sourceURL>
        <rdfs:comment rdf:datatype="http://www.w3.org/2001/XMLSchema#string">Joining a gym can encourage people to become more regularly active. Gyms can be a great place to learn new ways to be active, and professionals are available to offer advice on fitness and exercise. 

Have you considered joining a gym? Why or why not? Try searching online  for gyms near you. </rdfs:comment>
        <rdfs:label rdf:datatype="http://www.w3.org/2001/XMLSchema#string">Nearby Gyms</rdfs:label>
    </owl:NamedIndividual>
    


    <!-- http://www.semanticweb.org/tswheeler/ontologies/2016/3/EmpowerBP#H16 -->

    <owl:NamedIndividual rdf:about="http://www.semanticweb.org/tswheeler/ontologies/2016/3/EmpowerBP#H16">
        <rdf:type rdf:resource="http://www.semanticweb.org/tswheeler/ontologies/2016/3/EmpowerBP#InterventionItem"/>
        <rdf:type rdf:resource="http://www.semanticweb.org/tswheeler/ontologies/2016/3/EmpowerBP#Task"/>
        <EmpowerBP:isAppropriateForInterventionGoal rdf:resource="http://www.semanticweb.org/tswheeler/ontologies/2016/3/EmpowerBP#ExerciseMore"/>
        <EmpowerBP:isWarrantedBy rdf:resource="http://purl.bioontology.org/ontology/BCTT#Instruction_on_how_to_perform_the_behavior"/>
        <EmpowerBP:appropriateForAutomaticMotivation rdf:datatype="http://www.w3.org/2001/XMLSchema#integer">3</EmpowerBP:appropriateForAutomaticMotivation>
        <EmpowerBP:appropriateForLocation rdf:datatype="http://www.w3.org/2001/XMLSchema#integer">0</EmpowerBP:appropriateForLocation>
        <EmpowerBP:appropriateForPhysicalCapability rdf:datatype="http://www.w3.org/2001/XMLSchema#integer">3</EmpowerBP:appropriateForPhysicalCapability>
        <EmpowerBP:appropriateForPhysicalOpportunity rdf:datatype="http://www.w3.org/2001/XMLSchema#integer">3</EmpowerBP:appropriateForPhysicalOpportunity>
        <EmpowerBP:appropriateForPsychologicalCapability rdf:datatype="http://www.w3.org/2001/XMLSchema#integer">3</EmpowerBP:appropriateForPsychologicalCapability>
        <EmpowerBP:appropriateForReflectiveMotivation rdf:datatype="http://www.w3.org/2001/XMLSchema#integer">3</EmpowerBP:appropriateForReflectiveMotivation>
        <EmpowerBP:appropriateForSocialOpportunity rdf:datatype="http://www.w3.org/2001/XMLSchema#integer">3</EmpowerBP:appropriateForSocialOpportunity>
        <EmpowerBP:canRepeat rdf:datatype="http://www.w3.org/2001/XMLSchema#integer">8</EmpowerBP:canRepeat>
        <EmpowerBP:itemName rdf:datatype="http://www.w3.org/2001/XMLSchema#string">Resources</EmpowerBP:itemName>
        <EmpowerBP:itemText rdf:datatype="http://www.w3.org/2001/XMLSchema#string">Take 15 minutes to look through your Resources! Find an interesting resource and read or explore the content.</EmpowerBP:itemText>
        <EmpowerBP:maximumUserAge rdf:datatype="http://www.w3.org/2001/XMLSchema#integer">120</EmpowerBP:maximumUserAge>
        <EmpowerBP:minimumUserAge rdf:datatype="http://www.w3.org/2001/XMLSchema#integer">18</EmpowerBP:minimumUserAge>
        <EmpowerBP:provideJournal rdf:datatype="http://www.w3.org/2001/XMLSchema#boolean">false</EmpowerBP:provideJournal>
        <EmpowerBP:provideLink rdf:datatype="http://www.w3.org/2001/XMLSchema#boolean">true</EmpowerBP:provideLink>
        <EmpowerBP:sourceURL rdf:datatype="http://www.w3.org/2001/XMLSchema#string">&lt;&lt;internal link to Resources&gt;&gt;</EmpowerBP:sourceURL>
        <rdfs:comment rdf:datatype="http://www.w3.org/2001/XMLSchema#string">Take 15 minutes to look through your Resources! Find an interesting resource and read or explore the content.</rdfs:comment>
        <rdfs:label rdf:datatype="http://www.w3.org/2001/XMLSchema#string">Resources</rdfs:label>
    </owl:NamedIndividual>
    


    <!-- http://www.semanticweb.org/tswheeler/ontologies/2016/3/EmpowerBP#H17 -->

    <owl:NamedIndividual rdf:about="http://www.semanticweb.org/tswheeler/ontologies/2016/3/EmpowerBP#H17">
        <rdf:type rdf:resource="http://www.semanticweb.org/tswheeler/ontologies/2016/3/EmpowerBP#InterventionItem"/>
        <rdf:type rdf:resource="http://www.semanticweb.org/tswheeler/ontologies/2016/3/EmpowerBP#Task"/>
        <EmpowerBP:isAppropriateForInterventionGoal rdf:resource="http://www.semanticweb.org/tswheeler/ontologies/2016/3/EmpowerBP#ReduceSaltIntake"/>
        <EmpowerBP:isWarrantedBy rdf:resource="http://purl.bioontology.org/ontology/BCTT#Instruction_on_how_to_perform_the_behavior"/>
        <EmpowerBP:appropriateForAutomaticMotivation rdf:datatype="http://www.w3.org/2001/XMLSchema#integer">3</EmpowerBP:appropriateForAutomaticMotivation>
        <EmpowerBP:appropriateForLocation rdf:datatype="http://www.w3.org/2001/XMLSchema#integer">0</EmpowerBP:appropriateForLocation>
        <EmpowerBP:appropriateForPhysicalCapability rdf:datatype="http://www.w3.org/2001/XMLSchema#integer">3</EmpowerBP:appropriateForPhysicalCapability>
        <EmpowerBP:appropriateForPhysicalOpportunity rdf:datatype="http://www.w3.org/2001/XMLSchema#integer">3</EmpowerBP:appropriateForPhysicalOpportunity>
        <EmpowerBP:appropriateForPsychologicalCapability rdf:datatype="http://www.w3.org/2001/XMLSchema#integer">3</EmpowerBP:appropriateForPsychologicalCapability>
        <EmpowerBP:appropriateForReflectiveMotivation rdf:datatype="http://www.w3.org/2001/XMLSchema#integer">3</EmpowerBP:appropriateForReflectiveMotivation>
        <EmpowerBP:appropriateForSocialOpportunity rdf:datatype="http://www.w3.org/2001/XMLSchema#integer">3</EmpowerBP:appropriateForSocialOpportunity>
        <EmpowerBP:canRepeat rdf:datatype="http://www.w3.org/2001/XMLSchema#integer">8</EmpowerBP:canRepeat>
        <EmpowerBP:itemName rdf:datatype="http://www.w3.org/2001/XMLSchema#string">Resources</EmpowerBP:itemName>
        <EmpowerBP:itemText rdf:datatype="http://www.w3.org/2001/XMLSchema#string">Take 15 minutes to look through your Resources! Find an interesting resource and read or explore the content.</EmpowerBP:itemText>
        <EmpowerBP:maximumUserAge rdf:datatype="http://www.w3.org/2001/XMLSchema#integer">120</EmpowerBP:maximumUserAge>
        <EmpowerBP:minimumUserAge rdf:datatype="http://www.w3.org/2001/XMLSchema#integer">18</EmpowerBP:minimumUserAge>
        <EmpowerBP:provideJournal rdf:datatype="http://www.w3.org/2001/XMLSchema#boolean">false</EmpowerBP:provideJournal>
        <EmpowerBP:provideLink rdf:datatype="http://www.w3.org/2001/XMLSchema#boolean">true</EmpowerBP:provideLink>
        <EmpowerBP:sourceURL rdf:datatype="http://www.w3.org/2001/XMLSchema#string">&lt;&lt;internal link to Resources&gt;&gt;</EmpowerBP:sourceURL>
        <rdfs:comment rdf:datatype="http://www.w3.org/2001/XMLSchema#string">Take 15 minutes to look through your Resources! Find an interesting resource and read or explore the content.</rdfs:comment>
        <rdfs:label rdf:datatype="http://www.w3.org/2001/XMLSchema#string">Resources</rdfs:label>
    </owl:NamedIndividual>
    


    <!-- http://www.semanticweb.org/tswheeler/ontologies/2016/3/EmpowerBP#H18 -->

    <owl:NamedIndividual rdf:about="http://www.semanticweb.org/tswheeler/ontologies/2016/3/EmpowerBP#H18">
        <rdf:type rdf:resource="http://www.semanticweb.org/tswheeler/ontologies/2016/3/EmpowerBP#InterventionItem"/>
        <rdf:type rdf:resource="http://www.semanticweb.org/tswheeler/ontologies/2016/3/EmpowerBP#Task"/>
        <EmpowerBP:isAppropriateForInterventionGoal rdf:resource="http://www.semanticweb.org/tswheeler/ontologies/2016/3/EmpowerBP#ReduceSaltIntake"/>
        <EmpowerBP:isWarrantedBy rdf:resource="http://purl.bioontology.org/ontology/BCTT#Action_planning"/>
        <EmpowerBP:appropriateForAutomaticMotivation rdf:datatype="http://www.w3.org/2001/XMLSchema#integer">6</EmpowerBP:appropriateForAutomaticMotivation>
        <EmpowerBP:appropriateForLocation rdf:datatype="http://www.w3.org/2001/XMLSchema#integer">0</EmpowerBP:appropriateForLocation>
        <EmpowerBP:appropriateForPhysicalCapability rdf:datatype="http://www.w3.org/2001/XMLSchema#integer">6</EmpowerBP:appropriateForPhysicalCapability>
        <EmpowerBP:appropriateForPhysicalOpportunity rdf:datatype="http://www.w3.org/2001/XMLSchema#integer">6</EmpowerBP:appropriateForPhysicalOpportunity>
        <EmpowerBP:appropriateForPsychologicalCapability rdf:datatype="http://www.w3.org/2001/XMLSchema#integer">6</EmpowerBP:appropriateForPsychologicalCapability>
        <EmpowerBP:appropriateForReflectiveMotivation rdf:datatype="http://www.w3.org/2001/XMLSchema#integer">6</EmpowerBP:appropriateForReflectiveMotivation>
        <EmpowerBP:appropriateForSocialOpportunity rdf:datatype="http://www.w3.org/2001/XMLSchema#integer">6</EmpowerBP:appropriateForSocialOpportunity>
        <EmpowerBP:canRepeat rdf:datatype="http://www.w3.org/2001/XMLSchema#integer">4</EmpowerBP:canRepeat>
        <EmpowerBP:itemName rdf:datatype="http://www.w3.org/2001/XMLSchema#string">Healthy Snack</EmpowerBP:itemName>
        <EmpowerBP:itemText rdf:datatype="http://www.w3.org/2001/XMLSchema#string">Pick up a healthy snack!

Head to http://www.cookspiration.com and use the site to look up dietician-approved snack ideas. Is there something that you can add to your next grocery list? </EmpowerBP:itemText>
        <EmpowerBP:maximumUserAge rdf:datatype="http://www.w3.org/2001/XMLSchema#integer">120</EmpowerBP:maximumUserAge>
        <EmpowerBP:minimumUserAge rdf:datatype="http://www.w3.org/2001/XMLSchema#integer">18</EmpowerBP:minimumUserAge>
        <EmpowerBP:provideJournal rdf:datatype="http://www.w3.org/2001/XMLSchema#boolean">false</EmpowerBP:provideJournal>
        <EmpowerBP:provideLink rdf:datatype="http://www.w3.org/2001/XMLSchema#boolean">false</EmpowerBP:provideLink>
        <EmpowerBP:sourceURL rdf:datatype="http://www.w3.org/2001/XMLSchema#string">http://www.cookspiration.com</EmpowerBP:sourceURL>
        <rdfs:comment rdf:datatype="http://www.w3.org/2001/XMLSchema#string">Pick up a healthy snack!

Head to http://www.cookspiration.com and use the site to look up dietician-approved snack ideas. Is there something that you can add to your next grocery list? </rdfs:comment>
        <rdfs:label rdf:datatype="http://www.w3.org/2001/XMLSchema#string">Healthy Snack</rdfs:label>
    </owl:NamedIndividual>
    


    <!-- http://www.semanticweb.org/tswheeler/ontologies/2016/3/EmpowerBP#H19 -->

    <owl:NamedIndividual rdf:about="http://www.semanticweb.org/tswheeler/ontologies/2016/3/EmpowerBP#H19">
        <rdf:type rdf:resource="http://www.semanticweb.org/tswheeler/ontologies/2016/3/EmpowerBP#InterventionItem"/>
        <rdf:type rdf:resource="http://www.semanticweb.org/tswheeler/ontologies/2016/3/EmpowerBP#Task"/>
        <EmpowerBP:isAppropriateForInterventionGoal rdf:resource="http://www.semanticweb.org/tswheeler/ontologies/2016/3/EmpowerBP#ReduceSaltIntake"/>
        <EmpowerBP:isWarrantedBy rdf:resource="http://purl.bioontology.org/ontology/BCTT#Action_planning"/>
        <EmpowerBP:appropriateForAutomaticMotivation rdf:datatype="http://www.w3.org/2001/XMLSchema#integer">6</EmpowerBP:appropriateForAutomaticMotivation>
        <EmpowerBP:appropriateForLocation rdf:datatype="http://www.w3.org/2001/XMLSchema#integer">0</EmpowerBP:appropriateForLocation>
        <EmpowerBP:appropriateForPhysicalCapability rdf:datatype="http://www.w3.org/2001/XMLSchema#integer">6</EmpowerBP:appropriateForPhysicalCapability>
        <EmpowerBP:appropriateForPhysicalOpportunity rdf:datatype="http://www.w3.org/2001/XMLSchema#integer">6</EmpowerBP:appropriateForPhysicalOpportunity>
        <EmpowerBP:appropriateForPsychologicalCapability rdf:datatype="http://www.w3.org/2001/XMLSchema#integer">6</EmpowerBP:appropriateForPsychologicalCapability>
        <EmpowerBP:appropriateForReflectiveMotivation rdf:datatype="http://www.w3.org/2001/XMLSchema#integer">6</EmpowerBP:appropriateForReflectiveMotivation>
        <EmpowerBP:appropriateForSocialOpportunity rdf:datatype="http://www.w3.org/2001/XMLSchema#integer">6</EmpowerBP:appropriateForSocialOpportunity>
        <EmpowerBP:canRepeat rdf:datatype="http://www.w3.org/2001/XMLSchema#integer">4</EmpowerBP:canRepeat>
        <EmpowerBP:itemName rdf:datatype="http://www.w3.org/2001/XMLSchema#string">Healthy Meal</EmpowerBP:itemName>
        <EmpowerBP:itemText rdf:datatype="http://www.w3.org/2001/XMLSchema#string">Plan a healthy meal sometime this week!

Head to http://www.cookspiration.com and use the site to look up dietician-approved meal ideas. Is there something that you can make at home this week?</EmpowerBP:itemText>
        <EmpowerBP:maximumUserAge rdf:datatype="http://www.w3.org/2001/XMLSchema#integer">120</EmpowerBP:maximumUserAge>
        <EmpowerBP:minimumUserAge rdf:datatype="http://www.w3.org/2001/XMLSchema#integer">18</EmpowerBP:minimumUserAge>
        <EmpowerBP:provideJournal rdf:datatype="http://www.w3.org/2001/XMLSchema#boolean">false</EmpowerBP:provideJournal>
        <EmpowerBP:provideLink rdf:datatype="http://www.w3.org/2001/XMLSchema#boolean">false</EmpowerBP:provideLink>
        <EmpowerBP:sourceURL rdf:datatype="http://www.w3.org/2001/XMLSchema#string">http://www.cookspiration.com</EmpowerBP:sourceURL>
        <rdfs:comment rdf:datatype="http://www.w3.org/2001/XMLSchema#string">Plan a healthy meal sometime this week!

Head to http://www.cookspiration.com and use the site to look up dietician-approved meal ideas. Is there something that you can make at home this week?</rdfs:comment>
        <rdfs:label rdf:datatype="http://www.w3.org/2001/XMLSchema#string">Healthy Meal</rdfs:label>
    </owl:NamedIndividual>
    


    <!-- http://www.semanticweb.org/tswheeler/ontologies/2016/3/EmpowerBP#H2 -->

    <owl:NamedIndividual rdf:about="http://www.semanticweb.org/tswheeler/ontologies/2016/3/EmpowerBP#H2">
        <rdf:type rdf:resource="http://www.semanticweb.org/tswheeler/ontologies/2016/3/EmpowerBP#InterventionItem"/>
        <rdf:type rdf:resource="http://www.semanticweb.org/tswheeler/ontologies/2016/3/EmpowerBP#Task"/>
        <EmpowerBP:isAppropriateForInterventionGoal rdf:resource="http://www.semanticweb.org/tswheeler/ontologies/2016/3/EmpowerBP#ExerciseMore"/>
        <EmpowerBP:isWarrantedBy rdf:resource="http://purl.bioontology.org/ontology/BCTT#Instruction_on_how_to_perform_the_behavior"/>
        <EmpowerBP:appropriateForAutomaticMotivation rdf:datatype="http://www.w3.org/2001/XMLSchema#integer">3</EmpowerBP:appropriateForAutomaticMotivation>
        <EmpowerBP:appropriateForLocation rdf:datatype="http://www.w3.org/2001/XMLSchema#integer">0</EmpowerBP:appropriateForLocation>
        <EmpowerBP:appropriateForPhysicalCapability rdf:datatype="http://www.w3.org/2001/XMLSchema#integer">3</EmpowerBP:appropriateForPhysicalCapability>
        <EmpowerBP:appropriateForPhysicalOpportunity rdf:datatype="http://www.w3.org/2001/XMLSchema#integer">3</EmpowerBP:appropriateForPhysicalOpportunity>
        <EmpowerBP:appropriateForPsychologicalCapability rdf:datatype="http://www.w3.org/2001/XMLSchema#integer">3</EmpowerBP:appropriateForPsychologicalCapability>
        <EmpowerBP:appropriateForReflectiveMotivation rdf:datatype="http://www.w3.org/2001/XMLSchema#integer">3</EmpowerBP:appropriateForReflectiveMotivation>
        <EmpowerBP:appropriateForSocialOpportunity rdf:datatype="http://www.w3.org/2001/XMLSchema#integer">3</EmpowerBP:appropriateForSocialOpportunity>
        <EmpowerBP:canRepeat rdf:datatype="http://www.w3.org/2001/XMLSchema#integer">52</EmpowerBP:canRepeat>
        <EmpowerBP:itemName rdf:datatype="http://www.w3.org/2001/XMLSchema#string">Physical Activity Tips for Adults
</EmpowerBP:itemName>
        <EmpowerBP:itemText rdf:datatype="http://www.w3.org/2001/XMLSchema#string">Read the Public Health Agency of Canada&apos;s &quot;Physical activity tips for older adults&quot;.</EmpowerBP:itemText>
        <EmpowerBP:maximumUserAge rdf:datatype="http://www.w3.org/2001/XMLSchema#integer">64</EmpowerBP:maximumUserAge>
        <EmpowerBP:minimumUserAge rdf:datatype="http://www.w3.org/2001/XMLSchema#integer">18</EmpowerBP:minimumUserAge>
        <EmpowerBP:provideJournal rdf:datatype="http://www.w3.org/2001/XMLSchema#boolean">false</EmpowerBP:provideJournal>
        <EmpowerBP:provideLink rdf:datatype="http://www.w3.org/2001/XMLSchema#boolean">true</EmpowerBP:provideLink>
        <EmpowerBP:sourceURL rdf:datatype="http://www.w3.org/2001/XMLSchema#string">http://www.phac-aspc.gc.ca/hp-ps/hl-mvs/pa-ap/07paap-eng.php</EmpowerBP:sourceURL>
        <rdfs:comment rdf:datatype="http://www.w3.org/2001/XMLSchema#string">Read the Public Health Agency of Canada&apos;s &quot;Physical activity tips for older adults&quot;.</rdfs:comment>
        <rdfs:label rdf:datatype="http://www.w3.org/2001/XMLSchema#string">Physical Activity Tips for Adults
</rdfs:label>
    </owl:NamedIndividual>
    


    <!-- http://www.semanticweb.org/tswheeler/ontologies/2016/3/EmpowerBP#H20 -->

    <owl:NamedIndividual rdf:about="http://www.semanticweb.org/tswheeler/ontologies/2016/3/EmpowerBP#H20">
        <rdf:type rdf:resource="http://www.semanticweb.org/tswheeler/ontologies/2016/3/EmpowerBP#InterventionItem"/>
        <rdf:type rdf:resource="http://www.semanticweb.org/tswheeler/ontologies/2016/3/EmpowerBP#Task"/>
        <EmpowerBP:isAppropriateForInterventionGoal rdf:resource="http://www.semanticweb.org/tswheeler/ontologies/2016/3/EmpowerBP#ReduceSaltIntake"/>
        <EmpowerBP:isWarrantedBy rdf:resource="http://purl.bioontology.org/ontology/BCTT#Action_planning"/>
        <EmpowerBP:appropriateForAutomaticMotivation rdf:datatype="http://www.w3.org/2001/XMLSchema#integer">6</EmpowerBP:appropriateForAutomaticMotivation>
        <EmpowerBP:appropriateForLocation rdf:datatype="http://www.w3.org/2001/XMLSchema#integer">0</EmpowerBP:appropriateForLocation>
        <EmpowerBP:appropriateForPhysicalCapability rdf:datatype="http://www.w3.org/2001/XMLSchema#integer">6</EmpowerBP:appropriateForPhysicalCapability>
        <EmpowerBP:appropriateForPhysicalOpportunity rdf:datatype="http://www.w3.org/2001/XMLSchema#integer">6</EmpowerBP:appropriateForPhysicalOpportunity>
        <EmpowerBP:appropriateForPsychologicalCapability rdf:datatype="http://www.w3.org/2001/XMLSchema#integer">6</EmpowerBP:appropriateForPsychologicalCapability>
        <EmpowerBP:appropriateForReflectiveMotivation rdf:datatype="http://www.w3.org/2001/XMLSchema#integer">6</EmpowerBP:appropriateForReflectiveMotivation>
        <EmpowerBP:appropriateForSocialOpportunity rdf:datatype="http://www.w3.org/2001/XMLSchema#integer">6</EmpowerBP:appropriateForSocialOpportunity>
        <EmpowerBP:canRepeat rdf:datatype="http://www.w3.org/2001/XMLSchema#integer">4</EmpowerBP:canRepeat>
        <EmpowerBP:itemName rdf:datatype="http://www.w3.org/2001/XMLSchema#string">Healthy Meal</EmpowerBP:itemName>
        <EmpowerBP:itemText rdf:datatype="http://www.w3.org/2001/XMLSchema#string">Plan a healthy meal sometime this week!

Follow the link to find healhty recipes for every season, submitted by other Canadians. Is there something that you can make at home this week?</EmpowerBP:itemText>
        <EmpowerBP:maximumUserAge rdf:datatype="http://www.w3.org/2001/XMLSchema#integer">120</EmpowerBP:maximumUserAge>
        <EmpowerBP:minimumUserAge rdf:datatype="http://www.w3.org/2001/XMLSchema#integer">18</EmpowerBP:minimumUserAge>
        <EmpowerBP:provideJournal rdf:datatype="http://www.w3.org/2001/XMLSchema#boolean">false</EmpowerBP:provideJournal>
        <EmpowerBP:provideLink rdf:datatype="http://www.w3.org/2001/XMLSchema#boolean">true</EmpowerBP:provideLink>
        <EmpowerBP:sourceURL rdf:datatype="http://www.w3.org/2001/XMLSchema#string">https://www.canada.ca/en/health-canada/services/tips-healthy-eating/eat-well-recipes.html</EmpowerBP:sourceURL>
        <rdfs:comment rdf:datatype="http://www.w3.org/2001/XMLSchema#string">Plan a healthy meal sometime this week!

Follow the link to find healhty recipes for every season, submitted by other Canadians. Is there something that you can make at home this week?</rdfs:comment>
        <rdfs:label rdf:datatype="http://www.w3.org/2001/XMLSchema#string">Healthy Meal</rdfs:label>
    </owl:NamedIndividual>
    


    <!-- http://www.semanticweb.org/tswheeler/ontologies/2016/3/EmpowerBP#H3 -->

    <owl:NamedIndividual rdf:about="http://www.semanticweb.org/tswheeler/ontologies/2016/3/EmpowerBP#H3">
        <rdf:type rdf:resource="http://www.semanticweb.org/tswheeler/ontologies/2016/3/EmpowerBP#InterventionItem"/>
        <rdf:type rdf:resource="http://www.semanticweb.org/tswheeler/ontologies/2016/3/EmpowerBP#Task"/>
        <EmpowerBP:isAppropriateForInterventionGoal rdf:resource="http://www.semanticweb.org/tswheeler/ontologies/2016/3/EmpowerBP#ExerciseMore"/>
        <EmpowerBP:isWarrantedBy rdf:resource="http://purl.bioontology.org/ontology/BCTT#Instruction_on_how_to_perform_the_behavior"/>
        <EmpowerBP:appropriateForAutomaticMotivation rdf:datatype="http://www.w3.org/2001/XMLSchema#integer">3</EmpowerBP:appropriateForAutomaticMotivation>
        <EmpowerBP:appropriateForLocation rdf:datatype="http://www.w3.org/2001/XMLSchema#integer">0</EmpowerBP:appropriateForLocation>
        <EmpowerBP:appropriateForPhysicalCapability rdf:datatype="http://www.w3.org/2001/XMLSchema#integer">3</EmpowerBP:appropriateForPhysicalCapability>
        <EmpowerBP:appropriateForPhysicalOpportunity rdf:datatype="http://www.w3.org/2001/XMLSchema#integer">3</EmpowerBP:appropriateForPhysicalOpportunity>
        <EmpowerBP:appropriateForPsychologicalCapability rdf:datatype="http://www.w3.org/2001/XMLSchema#integer">3</EmpowerBP:appropriateForPsychologicalCapability>
        <EmpowerBP:appropriateForReflectiveMotivation rdf:datatype="http://www.w3.org/2001/XMLSchema#integer">3</EmpowerBP:appropriateForReflectiveMotivation>
        <EmpowerBP:appropriateForSocialOpportunity rdf:datatype="http://www.w3.org/2001/XMLSchema#integer">3</EmpowerBP:appropriateForSocialOpportunity>
        <EmpowerBP:canRepeat rdf:datatype="http://www.w3.org/2001/XMLSchema#integer">52</EmpowerBP:canRepeat>
        <EmpowerBP:itemName rdf:datatype="http://www.w3.org/2001/XMLSchema#string">Physical Activity Tips for Older Adults</EmpowerBP:itemName>
        <EmpowerBP:itemText rdf:datatype="http://www.w3.org/2001/XMLSchema#string">Read the Public Health Agency of Canada&apos;s &quot;Physical activity tips for adults&quot;.</EmpowerBP:itemText>
        <EmpowerBP:maximumUserAge rdf:datatype="http://www.w3.org/2001/XMLSchema#integer">120</EmpowerBP:maximumUserAge>
        <EmpowerBP:minimumUserAge rdf:datatype="http://www.w3.org/2001/XMLSchema#integer">65</EmpowerBP:minimumUserAge>
        <EmpowerBP:provideJournal rdf:datatype="http://www.w3.org/2001/XMLSchema#boolean">false</EmpowerBP:provideJournal>
        <EmpowerBP:provideLink rdf:datatype="http://www.w3.org/2001/XMLSchema#boolean">true</EmpowerBP:provideLink>
        <EmpowerBP:sourceURL rdf:datatype="http://www.w3.org/2001/XMLSchema#string">http://www.phac-aspc.gc.ca/hp-ps/hl-mvs/pa-ap/08paap-eng.php</EmpowerBP:sourceURL>
        <rdfs:comment rdf:datatype="http://www.w3.org/2001/XMLSchema#string">Read the Public Health Agency of Canada&apos;s &quot;Physical activity tips for adults&quot;.</rdfs:comment>
        <rdfs:label rdf:datatype="http://www.w3.org/2001/XMLSchema#string">Physical Activity Tips for Older Adults</rdfs:label>
    </owl:NamedIndividual>
    


    <!-- http://www.semanticweb.org/tswheeler/ontologies/2016/3/EmpowerBP#H4 -->

    <owl:NamedIndividual rdf:about="http://www.semanticweb.org/tswheeler/ontologies/2016/3/EmpowerBP#H4">
        <rdf:type rdf:resource="http://www.semanticweb.org/tswheeler/ontologies/2016/3/EmpowerBP#InterventionItem"/>
        <rdf:type rdf:resource="http://www.semanticweb.org/tswheeler/ontologies/2016/3/EmpowerBP#Task"/>
        <EmpowerBP:isAppropriateForInterventionGoal rdf:resource="http://www.semanticweb.org/tswheeler/ontologies/2016/3/EmpowerBP#ExerciseMore"/>
        <EmpowerBP:isWarrantedBy rdf:resource="http://purl.bioontology.org/ontology/BCTT#Information_about_health_consequences"/>
        <EmpowerBP:appropriateForAutomaticMotivation rdf:datatype="http://www.w3.org/2001/XMLSchema#integer">3</EmpowerBP:appropriateForAutomaticMotivation>
        <EmpowerBP:appropriateForLocation rdf:datatype="http://www.w3.org/2001/XMLSchema#integer">0</EmpowerBP:appropriateForLocation>
        <EmpowerBP:appropriateForPhysicalCapability rdf:datatype="http://www.w3.org/2001/XMLSchema#integer">3</EmpowerBP:appropriateForPhysicalCapability>
        <EmpowerBP:appropriateForPhysicalOpportunity rdf:datatype="http://www.w3.org/2001/XMLSchema#integer">3</EmpowerBP:appropriateForPhysicalOpportunity>
        <EmpowerBP:appropriateForPsychologicalCapability rdf:datatype="http://www.w3.org/2001/XMLSchema#integer">3</EmpowerBP:appropriateForPsychologicalCapability>
        <EmpowerBP:appropriateForReflectiveMotivation rdf:datatype="http://www.w3.org/2001/XMLSchema#integer">3</EmpowerBP:appropriateForReflectiveMotivation>
        <EmpowerBP:appropriateForSocialOpportunity rdf:datatype="http://www.w3.org/2001/XMLSchema#integer">3</EmpowerBP:appropriateForSocialOpportunity>
        <EmpowerBP:canRepeat rdf:datatype="http://www.w3.org/2001/XMLSchema#integer">52</EmpowerBP:canRepeat>
        <EmpowerBP:itemName rdf:datatype="http://www.w3.org/2001/XMLSchema#string">23 and 1/2 Hours</EmpowerBP:itemName>
        <EmpowerBP:itemText rdf:datatype="http://www.w3.org/2001/XMLSchema#string">&quot;23 and 1/2 hours: What is the single best thing we can do for our health?&quot;
Watch this 10 minute video by Dr. Mike Evans about the benefits of walking!</EmpowerBP:itemText>
        <EmpowerBP:maximumUserAge rdf:datatype="http://www.w3.org/2001/XMLSchema#integer">120</EmpowerBP:maximumUserAge>
        <EmpowerBP:minimumUserAge rdf:datatype="http://www.w3.org/2001/XMLSchema#integer">18</EmpowerBP:minimumUserAge>
        <EmpowerBP:provideJournal rdf:datatype="http://www.w3.org/2001/XMLSchema#boolean">false</EmpowerBP:provideJournal>
        <EmpowerBP:provideLink rdf:datatype="http://www.w3.org/2001/XMLSchema#boolean">true</EmpowerBP:provideLink>
        <EmpowerBP:sourceURL rdf:datatype="http://www.w3.org/2001/XMLSchema#string">https://www.youtube.com/watch?v=aUaInS6HIGo</EmpowerBP:sourceURL>
        <rdfs:comment rdf:datatype="http://www.w3.org/2001/XMLSchema#string">&quot;23 and 1/2 hours: What is the single best thing we can do for our health?&quot;
Watch this 10 minute video by Dr. Mike Evans about the benefits of walking!</rdfs:comment>
        <rdfs:label rdf:datatype="http://www.w3.org/2001/XMLSchema#string">23 and 1/2 Hours</rdfs:label>
    </owl:NamedIndividual>
    


    <!-- http://www.semanticweb.org/tswheeler/ontologies/2016/3/EmpowerBP#H5 -->

    <owl:NamedIndividual rdf:about="http://www.semanticweb.org/tswheeler/ontologies/2016/3/EmpowerBP#H5">
        <rdf:type rdf:resource="http://www.semanticweb.org/tswheeler/ontologies/2016/3/EmpowerBP#InterventionItem"/>
        <rdf:type rdf:resource="http://www.semanticweb.org/tswheeler/ontologies/2016/3/EmpowerBP#Task"/>
        <EmpowerBP:isAppropriateForInterventionGoal rdf:resource="http://www.semanticweb.org/tswheeler/ontologies/2016/3/EmpowerBP#ExerciseMore"/>
        <EmpowerBP:isWarrantedBy rdf:resource="http://purl.bioontology.org/ontology/BCTT#Social_support_(unspecified)"/>
        <EmpowerBP:appropriateForAutomaticMotivation rdf:datatype="http://www.w3.org/2001/XMLSchema#integer">6</EmpowerBP:appropriateForAutomaticMotivation>
        <EmpowerBP:appropriateForLocation rdf:datatype="http://www.w3.org/2001/XMLSchema#integer">0</EmpowerBP:appropriateForLocation>
        <EmpowerBP:appropriateForPhysicalCapability rdf:datatype="http://www.w3.org/2001/XMLSchema#integer">3</EmpowerBP:appropriateForPhysicalCapability>
        <EmpowerBP:appropriateForPhysicalOpportunity rdf:datatype="http://www.w3.org/2001/XMLSchema#integer">3</EmpowerBP:appropriateForPhysicalOpportunity>
        <EmpowerBP:appropriateForPsychologicalCapability rdf:datatype="http://www.w3.org/2001/XMLSchema#integer">3</EmpowerBP:appropriateForPsychologicalCapability>
        <EmpowerBP:appropriateForReflectiveMotivation rdf:datatype="http://www.w3.org/2001/XMLSchema#integer">6</EmpowerBP:appropriateForReflectiveMotivation>
        <EmpowerBP:appropriateForSocialOpportunity rdf:datatype="http://www.w3.org/2001/XMLSchema#integer">3</EmpowerBP:appropriateForSocialOpportunity>
        <EmpowerBP:canRepeat rdf:datatype="http://www.w3.org/2001/XMLSchema#integer">52</EmpowerBP:canRepeat>
        <EmpowerBP:itemName rdf:datatype="http://www.w3.org/2001/XMLSchema#string">Head &amp; Stoke Walkabout Video</EmpowerBP:itemName>
        <EmpowerBP:itemText rdf:datatype="http://www.w3.org/2001/XMLSchema#string">Watch this 5 minute video from Heart &amp; Stroke Walkabout about walking groups. Do you know of any walking groups in your area? Maybe you and your friends or coworkers could start one! </EmpowerBP:itemText>
        <EmpowerBP:maximumUserAge rdf:datatype="http://www.w3.org/2001/XMLSchema#integer">120</EmpowerBP:maximumUserAge>
        <EmpowerBP:minimumUserAge rdf:datatype="http://www.w3.org/2001/XMLSchema#integer">18</EmpowerBP:minimumUserAge>
        <EmpowerBP:provideJournal rdf:datatype="http://www.w3.org/2001/XMLSchema#boolean">false</EmpowerBP:provideJournal>
        <EmpowerBP:provideLink rdf:datatype="http://www.w3.org/2001/XMLSchema#boolean">true</EmpowerBP:provideLink>
        <EmpowerBP:sourceURL rdf:datatype="http://www.w3.org/2001/XMLSchema#string">https://www.youtube.com/watch?v=ctHLx9IQhs8</EmpowerBP:sourceURL>
        <rdfs:comment rdf:datatype="http://www.w3.org/2001/XMLSchema#string">Watch this 5 minute video from Heart &amp; Stroke Walkabout about walking groups. Do you know of any walking groups in your area? Maybe you and your friends or coworkers could start one! </rdfs:comment>
        <rdfs:label rdf:datatype="http://www.w3.org/2001/XMLSchema#string">Head &amp; Stoke Walkabout Video</rdfs:label>
    </owl:NamedIndividual>
    


    <!-- http://www.semanticweb.org/tswheeler/ontologies/2016/3/EmpowerBP#H6 -->

    <owl:NamedIndividual rdf:about="http://www.semanticweb.org/tswheeler/ontologies/2016/3/EmpowerBP#H6">
        <rdf:type rdf:resource="http://www.semanticweb.org/tswheeler/ontologies/2016/3/EmpowerBP#InterventionItem"/>
        <rdf:type rdf:resource="http://www.semanticweb.org/tswheeler/ontologies/2016/3/EmpowerBP#Task"/>
        <EmpowerBP:isAppropriateForInterventionGoal rdf:resource="http://www.semanticweb.org/tswheeler/ontologies/2016/3/EmpowerBP#ExerciseMore"/>
        <EmpowerBP:isWarrantedBy rdf:resource="http://purl.bioontology.org/ontology/BCTT#Instruction_on_how_to_perform_the_behavior"/>
        <EmpowerBP:appropriateForAutomaticMotivation rdf:datatype="http://www.w3.org/2001/XMLSchema#integer">6</EmpowerBP:appropriateForAutomaticMotivation>
        <EmpowerBP:appropriateForLocation rdf:datatype="http://www.w3.org/2001/XMLSchema#integer">0</EmpowerBP:appropriateForLocation>
        <EmpowerBP:appropriateForPhysicalCapability rdf:datatype="http://www.w3.org/2001/XMLSchema#integer">3</EmpowerBP:appropriateForPhysicalCapability>
        <EmpowerBP:appropriateForPhysicalOpportunity rdf:datatype="http://www.w3.org/2001/XMLSchema#integer">3</EmpowerBP:appropriateForPhysicalOpportunity>
        <EmpowerBP:appropriateForPsychologicalCapability rdf:datatype="http://www.w3.org/2001/XMLSchema#integer">3</EmpowerBP:appropriateForPsychologicalCapability>
        <EmpowerBP:appropriateForReflectiveMotivation rdf:datatype="http://www.w3.org/2001/XMLSchema#integer">6</EmpowerBP:appropriateForReflectiveMotivation>
        <EmpowerBP:appropriateForSocialOpportunity rdf:datatype="http://www.w3.org/2001/XMLSchema#integer">3</EmpowerBP:appropriateForSocialOpportunity>
        <EmpowerBP:canRepeat rdf:datatype="http://www.w3.org/2001/XMLSchema#integer">52</EmpowerBP:canRepeat>
        <EmpowerBP:itemName rdf:datatype="http://www.w3.org/2001/XMLSchema#string">CSEP Guidelines </EmpowerBP:itemName>
        <EmpowerBP:itemText rdf:datatype="http://www.w3.org/2001/XMLSchema#string">Read &quot;Canadian Physical Activity Guidelines&quot; from the Canadian Society for Exercise Physiology</EmpowerBP:itemText>
        <EmpowerBP:maximumUserAge rdf:datatype="http://www.w3.org/2001/XMLSchema#integer">64</EmpowerBP:maximumUserAge>
        <EmpowerBP:minimumUserAge rdf:datatype="http://www.w3.org/2001/XMLSchema#integer">18</EmpowerBP:minimumUserAge>
        <EmpowerBP:provideJournal rdf:datatype="http://www.w3.org/2001/XMLSchema#boolean">false</EmpowerBP:provideJournal>
        <EmpowerBP:provideLink rdf:datatype="http://www.w3.org/2001/XMLSchema#boolean">true</EmpowerBP:provideLink>
        <EmpowerBP:sourceURL rdf:datatype="http://www.w3.org/2001/XMLSchema#string">http://csep.ca/CMFiles/Guidelines/CSEP_PAGuidelines_adults_en.pdf</EmpowerBP:sourceURL>
        <rdfs:comment rdf:datatype="http://www.w3.org/2001/XMLSchema#string">Read &quot;Canadian Physical Activity Guidelines&quot; from the Canadian Society for Exercise Physiology</rdfs:comment>
        <rdfs:label rdf:datatype="http://www.w3.org/2001/XMLSchema#string">CSEP Guidelines </rdfs:label>
    </owl:NamedIndividual>
    


    <!-- http://www.semanticweb.org/tswheeler/ontologies/2016/3/EmpowerBP#H7 -->

    <owl:NamedIndividual rdf:about="http://www.semanticweb.org/tswheeler/ontologies/2016/3/EmpowerBP#H7">
        <rdf:type rdf:resource="http://www.semanticweb.org/tswheeler/ontologies/2016/3/EmpowerBP#InterventionItem"/>
        <rdf:type rdf:resource="http://www.semanticweb.org/tswheeler/ontologies/2016/3/EmpowerBP#Task"/>
        <EmpowerBP:isAppropriateForInterventionGoal rdf:resource="http://www.semanticweb.org/tswheeler/ontologies/2016/3/EmpowerBP#ExerciseMore"/>
        <EmpowerBP:isWarrantedBy rdf:resource="http://purl.bioontology.org/ontology/BCTT#Instruction_on_how_to_perform_the_behavior"/>
        <EmpowerBP:appropriateForAutomaticMotivation rdf:datatype="http://www.w3.org/2001/XMLSchema#integer">6</EmpowerBP:appropriateForAutomaticMotivation>
        <EmpowerBP:appropriateForLocation rdf:datatype="http://www.w3.org/2001/XMLSchema#integer">0</EmpowerBP:appropriateForLocation>
        <EmpowerBP:appropriateForPhysicalCapability rdf:datatype="http://www.w3.org/2001/XMLSchema#integer">3</EmpowerBP:appropriateForPhysicalCapability>
        <EmpowerBP:appropriateForPhysicalOpportunity rdf:datatype="http://www.w3.org/2001/XMLSchema#integer">3</EmpowerBP:appropriateForPhysicalOpportunity>
        <EmpowerBP:appropriateForPsychologicalCapability rdf:datatype="http://www.w3.org/2001/XMLSchema#integer">3</EmpowerBP:appropriateForPsychologicalCapability>
        <EmpowerBP:appropriateForReflectiveMotivation rdf:datatype="http://www.w3.org/2001/XMLSchema#integer">6</EmpowerBP:appropriateForReflectiveMotivation>
        <EmpowerBP:appropriateForSocialOpportunity rdf:datatype="http://www.w3.org/2001/XMLSchema#integer">3</EmpowerBP:appropriateForSocialOpportunity>
        <EmpowerBP:canRepeat rdf:datatype="http://www.w3.org/2001/XMLSchema#integer">52</EmpowerBP:canRepeat>
        <EmpowerBP:itemName rdf:datatype="http://www.w3.org/2001/XMLSchema#string">CSEP Guidelines</EmpowerBP:itemName>
        <EmpowerBP:itemText rdf:datatype="http://www.w3.org/2001/XMLSchema#string">Read &quot;Canadian Physical Activity Guidelines&quot; from the Canadian Society for Exercise Physiology</EmpowerBP:itemText>
        <EmpowerBP:maximumUserAge rdf:datatype="http://www.w3.org/2001/XMLSchema#integer">120</EmpowerBP:maximumUserAge>
        <EmpowerBP:minimumUserAge rdf:datatype="http://www.w3.org/2001/XMLSchema#integer">65</EmpowerBP:minimumUserAge>
        <EmpowerBP:provideJournal rdf:datatype="http://www.w3.org/2001/XMLSchema#boolean">false</EmpowerBP:provideJournal>
        <EmpowerBP:provideLink rdf:datatype="http://www.w3.org/2001/XMLSchema#boolean">true</EmpowerBP:provideLink>
        <EmpowerBP:sourceURL rdf:datatype="http://www.w3.org/2001/XMLSchema#string">http://csep.ca/CMFiles/Guidelines/CSEP_PAGuidelines_older-adults_en.pdf</EmpowerBP:sourceURL>
        <rdfs:comment rdf:datatype="http://www.w3.org/2001/XMLSchema#string">Read &quot;Canadian Physical Activity Guidelines&quot; from the Canadian Society for Exercise Physiology</rdfs:comment>
        <rdfs:label rdf:datatype="http://www.w3.org/2001/XMLSchema#string">CSEP Guidelines</rdfs:label>
    </owl:NamedIndividual>
    


    <!-- http://www.semanticweb.org/tswheeler/ontologies/2016/3/EmpowerBP#H8 -->

    <owl:NamedIndividual rdf:about="http://www.semanticweb.org/tswheeler/ontologies/2016/3/EmpowerBP#H8">
        <rdf:type rdf:resource="http://www.semanticweb.org/tswheeler/ontologies/2016/3/EmpowerBP#InterventionItem"/>
        <rdf:type rdf:resource="http://www.semanticweb.org/tswheeler/ontologies/2016/3/EmpowerBP#Task"/>
        <EmpowerBP:isAppropriateForInterventionGoal rdf:resource="http://www.semanticweb.org/tswheeler/ontologies/2016/3/EmpowerBP#ReduceSaltIntake"/>
        <EmpowerBP:isWarrantedBy rdf:resource="http://purl.bioontology.org/ontology/BCTT#Instruction_on_how_to_perform_the_behavior"/>
        <EmpowerBP:appropriateForAutomaticMotivation rdf:datatype="http://www.w3.org/2001/XMLSchema#integer">3</EmpowerBP:appropriateForAutomaticMotivation>
        <EmpowerBP:appropriateForLocation rdf:datatype="http://www.w3.org/2001/XMLSchema#integer">0</EmpowerBP:appropriateForLocation>
        <EmpowerBP:appropriateForPhysicalCapability rdf:datatype="http://www.w3.org/2001/XMLSchema#integer">3</EmpowerBP:appropriateForPhysicalCapability>
        <EmpowerBP:appropriateForPhysicalOpportunity rdf:datatype="http://www.w3.org/2001/XMLSchema#integer">3</EmpowerBP:appropriateForPhysicalOpportunity>
        <EmpowerBP:appropriateForPsychologicalCapability rdf:datatype="http://www.w3.org/2001/XMLSchema#integer">3</EmpowerBP:appropriateForPsychologicalCapability>
        <EmpowerBP:appropriateForReflectiveMotivation rdf:datatype="http://www.w3.org/2001/XMLSchema#integer">3</EmpowerBP:appropriateForReflectiveMotivation>
        <EmpowerBP:appropriateForSocialOpportunity rdf:datatype="http://www.w3.org/2001/XMLSchema#integer">3</EmpowerBP:appropriateForSocialOpportunity>
        <EmpowerBP:canRepeat rdf:datatype="http://www.w3.org/2001/XMLSchema#integer">52</EmpowerBP:canRepeat>
        <EmpowerBP:itemName rdf:datatype="http://www.w3.org/2001/XMLSchema#string">Video: Sodium in your diet and how to use %DV</EmpowerBP:itemName>
        <EmpowerBP:itemText rdf:datatype="http://www.w3.org/2001/XMLSchema#string">Click the link and watch the short video &quot;Amanda discusses sodium in your diet and how to use %DV&quot;. It is the last video listed on the page. </EmpowerBP:itemText>
        <EmpowerBP:maximumUserAge rdf:datatype="http://www.w3.org/2001/XMLSchema#integer">120</EmpowerBP:maximumUserAge>
        <EmpowerBP:minimumUserAge rdf:datatype="http://www.w3.org/2001/XMLSchema#integer">18</EmpowerBP:minimumUserAge>
        <EmpowerBP:provideJournal rdf:datatype="http://www.w3.org/2001/XMLSchema#boolean">false</EmpowerBP:provideJournal>
        <EmpowerBP:provideLink rdf:datatype="http://www.w3.org/2001/XMLSchema#boolean">true</EmpowerBP:provideLink>
        <EmpowerBP:sourceURL rdf:datatype="http://www.w3.org/2001/XMLSchema#string">http://www.dietitians.ca/Your-Health/Videos/Videos-2013.aspx</EmpowerBP:sourceURL>
        <rdfs:comment rdf:datatype="http://www.w3.org/2001/XMLSchema#string">Click the link and watch the short video &quot;Amanda discusses sodium in your diet and how to use %DV&quot;. It is the last video listed on the page. </rdfs:comment>
        <rdfs:label rdf:datatype="http://www.w3.org/2001/XMLSchema#string">Video: Sodium in your diet and how to use %DV</rdfs:label>
    </owl:NamedIndividual>
    


    <!-- http://www.semanticweb.org/tswheeler/ontologies/2016/3/EmpowerBP#H9 -->

    <owl:NamedIndividual rdf:about="http://www.semanticweb.org/tswheeler/ontologies/2016/3/EmpowerBP#H9">
        <rdf:type rdf:resource="http://www.semanticweb.org/tswheeler/ontologies/2016/3/EmpowerBP#InterventionItem"/>
        <rdf:type rdf:resource="http://www.semanticweb.org/tswheeler/ontologies/2016/3/EmpowerBP#Task"/>
        <EmpowerBP:isAppropriateForInterventionGoal rdf:resource="http://www.semanticweb.org/tswheeler/ontologies/2016/3/EmpowerBP#ReduceSaltIntake"/>
        <EmpowerBP:isWarrantedBy rdf:resource="http://purl.bioontology.org/ontology/BCTT#Information_about_health_consequences"/>
        <EmpowerBP:appropriateForAutomaticMotivation rdf:datatype="http://www.w3.org/2001/XMLSchema#integer">3</EmpowerBP:appropriateForAutomaticMotivation>
        <EmpowerBP:appropriateForLocation rdf:datatype="http://www.w3.org/2001/XMLSchema#integer">0</EmpowerBP:appropriateForLocation>
        <EmpowerBP:appropriateForPhysicalCapability rdf:datatype="http://www.w3.org/2001/XMLSchema#integer">3</EmpowerBP:appropriateForPhysicalCapability>
        <EmpowerBP:appropriateForPhysicalOpportunity rdf:datatype="http://www.w3.org/2001/XMLSchema#integer">3</EmpowerBP:appropriateForPhysicalOpportunity>
        <EmpowerBP:appropriateForPsychologicalCapability rdf:datatype="http://www.w3.org/2001/XMLSchema#integer">3</EmpowerBP:appropriateForPsychologicalCapability>
        <EmpowerBP:appropriateForReflectiveMotivation rdf:datatype="http://www.w3.org/2001/XMLSchema#integer">3</EmpowerBP:appropriateForReflectiveMotivation>
        <EmpowerBP:appropriateForSocialOpportunity rdf:datatype="http://www.w3.org/2001/XMLSchema#integer">3</EmpowerBP:appropriateForSocialOpportunity>
        <EmpowerBP:canRepeat rdf:datatype="http://www.w3.org/2001/XMLSchema#integer">52</EmpowerBP:canRepeat>
        <EmpowerBP:itemName rdf:datatype="http://www.w3.org/2001/XMLSchema#string">Video: Impact of sodium on your health</EmpowerBP:itemName>
        <EmpowerBP:itemText rdf:datatype="http://www.w3.org/2001/XMLSchema#string">Click the link and watch the short video &quot;Amanda explains the impact of sodium on health and how to decrease your intake&quot;.</EmpowerBP:itemText>
        <EmpowerBP:maximumUserAge rdf:datatype="http://www.w3.org/2001/XMLSchema#integer">120</EmpowerBP:maximumUserAge>
        <EmpowerBP:minimumUserAge rdf:datatype="http://www.w3.org/2001/XMLSchema#integer">18</EmpowerBP:minimumUserAge>
        <EmpowerBP:provideJournal rdf:datatype="http://www.w3.org/2001/XMLSchema#boolean">false</EmpowerBP:provideJournal>
        <EmpowerBP:provideLink rdf:datatype="http://www.w3.org/2001/XMLSchema#boolean">true</EmpowerBP:provideLink>
        <EmpowerBP:sourceURL rdf:datatype="http://www.w3.org/2001/XMLSchema#string">http://www.dietitians.ca/Your-Health/Videos/Videos-2012.aspx</EmpowerBP:sourceURL>
        <rdfs:comment rdf:datatype="http://www.w3.org/2001/XMLSchema#string">Click the link and watch the short video &quot;Amanda explains the impact of sodium on health and how to decrease your intake&quot;.</rdfs:comment>
        <rdfs:label rdf:datatype="http://www.w3.org/2001/XMLSchema#string">Video: Impact of sodium on your health</rdfs:label>
    </owl:NamedIndividual>
    


    <!-- http://www.semanticweb.org/tswheeler/ontologies/2016/3/EmpowerBP#Incentivisation -->

    <owl:NamedIndividual rdf:about="http://www.semanticweb.org/tswheeler/ontologies/2016/3/EmpowerBP#Incentivisation">
        <rdf:type rdf:resource="http://www.semanticweb.org/tswheeler/ontologies/2016/3/EmpowerBP#InterventionFuction"/>
        <EmpowerBP:hasCommonBCT rdf:resource="http://purl.bioontology.org/ontology/BCTT#Behavioral_contract"/>
        <EmpowerBP:hasCommonBCT rdf:resource="http://purl.bioontology.org/ontology/BCTT#Biofeedback"/>
        <EmpowerBP:hasCommonBCT rdf:resource="http://purl.bioontology.org/ontology/BCTT#Commitment"/>
        <EmpowerBP:hasCommonBCT rdf:resource="http://purl.bioontology.org/ontology/BCTT#Cue_signalling_reward"/>
        <EmpowerBP:hasCommonBCT rdf:resource="http://purl.bioontology.org/ontology/BCTT#Discrepancy_between_current_behavior_and_goal"/>
        <EmpowerBP:hasCommonBCT rdf:resource="http://purl.bioontology.org/ontology/BCTT#Imaginary_reward"/>
        <EmpowerBP:hasCommonBCT rdf:resource="http://purl.bioontology.org/ontology/BCTT#Non-specific_reward"/>
        <EmpowerBP:hasCommonBCT rdf:resource="http://purl.bioontology.org/ontology/BCTT#Paradoxical_instructions"/>
        <EmpowerBP:hasCommonBCT rdf:resource="http://purl.bioontology.org/ontology/BCTT#Reduce_reward_frequency"/>
        <EmpowerBP:hasCommonBCT rdf:resource="http://purl.bioontology.org/ontology/BCTT#Remove_aversive_stimulus"/>
        <EmpowerBP:hasCommonBCT rdf:resource="http://purl.bioontology.org/ontology/BCTT#Remove_punishment"/>
        <EmpowerBP:hasCommonBCT rdf:resource="http://purl.bioontology.org/ontology/BCTT#Reward_alternative_behavior"/>
        <EmpowerBP:hasCommonBCT rdf:resource="http://purl.bioontology.org/ontology/BCTT#Reward_approximation"/>
        <EmpowerBP:hasCommonBCT rdf:resource="http://purl.bioontology.org/ontology/BCTT#Reward_incompatible_behavior"/>
        <EmpowerBP:hasCommonBCT rdf:resource="http://purl.bioontology.org/ontology/BCTT#Rewarding_completion"/>
        <EmpowerBP:hasCommonBCT rdf:resource="http://purl.bioontology.org/ontology/BCTT#Self-reward"/>
        <EmpowerBP:hasCommonBCT rdf:resource="http://purl.bioontology.org/ontology/BCTT#Situation-specific_reward"/>
        <EmpowerBP:hasCommonBCT rdf:resource="http://purl.bioontology.org/ontology/BCTT#Social_reward"/>
        <EmpowerBP:hasCommonBCT rdf:resource="http://purl.bioontology.org/ontology/BCTT#Incentive_(outcome)"/>
        <EmpowerBP:hasCommonBCT rdf:resource="http://purl.bioontology.org/ontology/BCTT#Material_reward_(behavior)"/>
        <EmpowerBP:hasCommonBCT rdf:resource="http://purl.bioontology.org/ontology/BCTT#Self-monitoring_of_outcome(s)_of_behaviour"/>
        <EmpowerBP:hasMostCommonBCT rdf:resource="http://purl.bioontology.org/ontology/BCTT#Feedback_on_behaviour"/>
        <EmpowerBP:hasMostCommonBCT rdf:resource="http://purl.bioontology.org/ontology/BCTT#Monitoring_of_behavior_by_others_without_feedback"/>
        <EmpowerBP:hasMostCommonBCT rdf:resource="http://purl.bioontology.org/ontology/BCTT#Self-monitoring_of_behaviour"/>
        <EmpowerBP:hasMostCommonBCT rdf:resource="http://purl.bioontology.org/ontology/BCTT#Feedback_on_outcome(s)_of_behavior"/>
        <EmpowerBP:hasMostCommonBCT rdf:resource="http://purl.bioontology.org/ontology/BCTT#Monitoring_of_outcome(s)_of_behavior_without_feedback"/>
        <EmpowerBP:isEffectiveForTDFDomain rdf:resource="http://www.semanticweb.org/tswheeler/ontologies/2016/3/EmpowerBP#Emotion"/>
        <EmpowerBP:isEffectiveForTDFDomain rdf:resource="http://www.semanticweb.org/tswheeler/ontologies/2016/3/EmpowerBP#Goals"/>
        <EmpowerBP:isEffectiveForTDFDomain rdf:resource="http://www.semanticweb.org/tswheeler/ontologies/2016/3/EmpowerBP#Intentions"/>
        <EmpowerBP:isEffectiveForTDFDomain rdf:resource="http://www.semanticweb.org/tswheeler/ontologies/2016/3/EmpowerBP#Reinforcement"/>
        <rdfs:comment>Creating an expectation of reward.</rdfs:comment>
    </owl:NamedIndividual>
    


    <!-- http://www.semanticweb.org/tswheeler/ontologies/2016/3/EmpowerBP#InjuryObstacle -->

    <owl:NamedIndividual rdf:about="http://www.semanticweb.org/tswheeler/ontologies/2016/3/EmpowerBP#InjuryObstacle">
        <rdf:type rdf:resource="http://www.semanticweb.org/tswheeler/ontologies/2016/3/EmpowerBP#Obstacle"/>
        <EmpowerBP:hasRelevantTDF rdf:resource="http://www.semanticweb.org/tswheeler/ontologies/2016/3/EmpowerBP#BeliefsAboutCapability"/>
        <EmpowerBP:hasRelevantTDF rdf:resource="http://www.semanticweb.org/tswheeler/ontologies/2016/3/EmpowerBP#EnvironmentalContextResources"/>
        <EmpowerBP:hasRelevantTDF rdf:resource="http://www.semanticweb.org/tswheeler/ontologies/2016/3/EmpowerBP#Knowledge"/>
        <EmpowerBP:hasRelevantTDF rdf:resource="http://www.semanticweb.org/tswheeler/ontologies/2016/3/EmpowerBP#Optimism"/>
        <EmpowerBP:hasRelevantTDF rdf:resource="http://www.semanticweb.org/tswheeler/ontologies/2016/3/EmpowerBP#PhysicalSkill"/>
        <rdfs:comment>Unable to perform activity due to injury, or fears future/repeat injury.</rdfs:comment>
    </owl:NamedIndividual>
    


    <!-- http://www.semanticweb.org/tswheeler/ontologies/2016/3/EmpowerBP#Intentions -->

    <owl:NamedIndividual rdf:about="http://www.semanticweb.org/tswheeler/ontologies/2016/3/EmpowerBP#Intentions">
        <rdf:type rdf:resource="http://www.semanticweb.org/tswheeler/ontologies/2016/3/EmpowerBP#Construct"/>
        <rdf:type rdf:resource="http://www.semanticweb.org/tswheeler/ontologies/2016/3/EmpowerBP#TDFDomain"/>
        <EmpowerBP:hasEffectiveInterventionFunction rdf:resource="http://www.semanticweb.org/tswheeler/ontologies/2016/3/EmpowerBP#Coercion"/>
        <EmpowerBP:hasEffectiveInterventionFunction rdf:resource="http://www.semanticweb.org/tswheeler/ontologies/2016/3/EmpowerBP#Education"/>
        <EmpowerBP:hasEffectiveInterventionFunction rdf:resource="http://www.semanticweb.org/tswheeler/ontologies/2016/3/EmpowerBP#Incentivisation"/>
        <EmpowerBP:hasEffectiveInterventionFunction rdf:resource="http://www.semanticweb.org/tswheeler/ontologies/2016/3/EmpowerBP#Modelling"/>
        <EmpowerBP:hasEffectiveInterventionFunction rdf:resource="http://www.semanticweb.org/tswheeler/ontologies/2016/3/EmpowerBP#Persuasion"/>
        <EmpowerBP:isRelatedToCOMB rdf:resource="http://www.semanticweb.org/tswheeler/ontologies/2016/3/EmpowerBP#ReflectiveMotivation"/>
        <rdfs:comment>A conscious decision to perform a behavior or a resolve to act in a certain way</rdfs:comment>
    </owl:NamedIndividual>
    


    <!-- http://www.semanticweb.org/tswheeler/ontologies/2016/3/EmpowerBP#Knowledge -->

    <owl:NamedIndividual rdf:about="http://www.semanticweb.org/tswheeler/ontologies/2016/3/EmpowerBP#Knowledge">
        <rdf:type rdf:resource="http://www.semanticweb.org/tswheeler/ontologies/2016/3/EmpowerBP#Construct"/>
        <rdf:type rdf:resource="http://www.semanticweb.org/tswheeler/ontologies/2016/3/EmpowerBP#TDFDomain"/>
        <EmpowerBP:hasEffectiveInterventionFunction rdf:resource="http://www.semanticweb.org/tswheeler/ontologies/2016/3/EmpowerBP#Education"/>
        <EmpowerBP:isRelatedToCOMB rdf:resource="http://www.semanticweb.org/tswheeler/ontologies/2016/3/EmpowerBP#PsychologicalCapability"/>
        <rdfs:comment>An awareness of the existence of something</rdfs:comment>
    </owl:NamedIndividual>
    


    <!-- http://www.semanticweb.org/tswheeler/ontologies/2016/3/EmpowerBP#LocationObstacle -->

    <owl:NamedIndividual rdf:about="http://www.semanticweb.org/tswheeler/ontologies/2016/3/EmpowerBP#LocationObstacle">
        <rdf:type rdf:resource="http://www.semanticweb.org/tswheeler/ontologies/2016/3/EmpowerBP#Obstacle"/>
        <EmpowerBP:hasRelevantTDF rdf:resource="http://www.semanticweb.org/tswheeler/ontologies/2016/3/EmpowerBP#EnvironmentalContextResources"/>
        <rdfs:comment>Feels they do not have somewhere sto perform activity.</rdfs:comment>
    </owl:NamedIndividual>
    


    <!-- http://www.semanticweb.org/tswheeler/ontologies/2016/3/EmpowerBP#MemoryAttentionDecisionProcesses -->

    <owl:NamedIndividual rdf:about="http://www.semanticweb.org/tswheeler/ontologies/2016/3/EmpowerBP#MemoryAttentionDecisionProcesses">
        <rdf:type rdf:resource="http://www.semanticweb.org/tswheeler/ontologies/2016/3/EmpowerBP#Construct"/>
        <rdf:type rdf:resource="http://www.semanticweb.org/tswheeler/ontologies/2016/3/EmpowerBP#TDFDomain"/>
        <EmpowerBP:hasEffectiveInterventionFunction rdf:resource="http://www.semanticweb.org/tswheeler/ontologies/2016/3/EmpowerBP#Enablement"/>
        <EmpowerBP:hasEffectiveInterventionFunction rdf:resource="http://www.semanticweb.org/tswheeler/ontologies/2016/3/EmpowerBP#EnvironmentalRestructuring"/>
        <EmpowerBP:hasEffectiveInterventionFunction rdf:resource="http://www.semanticweb.org/tswheeler/ontologies/2016/3/EmpowerBP#Training"/>
        <EmpowerBP:isRelatedToCOMB rdf:resource="http://www.semanticweb.org/tswheeler/ontologies/2016/3/EmpowerBP#PsychologicalCapability"/>
        <rdfs:comment>The ability to retain information, focus selectively on aspects of the environment, and choose between two or more alternatives</rdfs:comment>
        <rdfs:label>Memory, Attention, and Decision Processes</rdfs:label>
    </owl:NamedIndividual>
    


    <!-- http://www.semanticweb.org/tswheeler/ontologies/2016/3/EmpowerBP#Modelling -->

    <owl:NamedIndividual rdf:about="http://www.semanticweb.org/tswheeler/ontologies/2016/3/EmpowerBP#Modelling">
        <rdf:type rdf:resource="http://www.semanticweb.org/tswheeler/ontologies/2016/3/EmpowerBP#InterventionFuction"/>
        <EmpowerBP:hasMostCommonBCT rdf:resource="http://purl.bioontology.org/ontology/BCTT#Demonstration_of_the_behavior"/>
        <EmpowerBP:isEffectiveForTDFDomain rdf:resource="http://www.semanticweb.org/tswheeler/ontologies/2016/3/EmpowerBP#BehaviouralRegulation"/>
        <EmpowerBP:isEffectiveForTDFDomain rdf:resource="http://www.semanticweb.org/tswheeler/ontologies/2016/3/EmpowerBP#BeliefsAboutCapability"/>
        <EmpowerBP:isEffectiveForTDFDomain rdf:resource="http://www.semanticweb.org/tswheeler/ontologies/2016/3/EmpowerBP#BeliefsAboutConsequences"/>
        <EmpowerBP:isEffectiveForTDFDomain rdf:resource="http://www.semanticweb.org/tswheeler/ontologies/2016/3/EmpowerBP#Emotion"/>
        <EmpowerBP:isEffectiveForTDFDomain rdf:resource="http://www.semanticweb.org/tswheeler/ontologies/2016/3/EmpowerBP#Goals"/>
        <EmpowerBP:isEffectiveForTDFDomain rdf:resource="http://www.semanticweb.org/tswheeler/ontologies/2016/3/EmpowerBP#Intentions"/>
        <EmpowerBP:isEffectiveForTDFDomain rdf:resource="http://www.semanticweb.org/tswheeler/ontologies/2016/3/EmpowerBP#Optimism"/>
        <EmpowerBP:isEffectiveForTDFDomain rdf:resource="http://www.semanticweb.org/tswheeler/ontologies/2016/3/EmpowerBP#ProfessionalSocialRoleIdentity"/>
        <EmpowerBP:isEffectiveForTDFDomain rdf:resource="http://www.semanticweb.org/tswheeler/ontologies/2016/3/EmpowerBP#SocialInfluences"/>
        <rdfs:comment>Providing an example for pepole to aspire to or imitate.</rdfs:comment>
    </owl:NamedIndividual>
    


    <!-- http://www.semanticweb.org/tswheeler/ontologies/2016/3/EmpowerBP#MoneyObstacle -->

    <owl:NamedIndividual rdf:about="http://www.semanticweb.org/tswheeler/ontologies/2016/3/EmpowerBP#MoneyObstacle">
        <rdf:type rdf:resource="http://www.semanticweb.org/tswheeler/ontologies/2016/3/EmpowerBP#Obstacle"/>
        <EmpowerBP:hasRelevantTDF rdf:resource="http://www.semanticweb.org/tswheeler/ontologies/2016/3/EmpowerBP#EnvironmentalContextResources"/>
        <EmpowerBP:hasRelevantTDF rdf:resource="http://www.semanticweb.org/tswheeler/ontologies/2016/3/EmpowerBP#Knowledge"/>
        <rdfs:comment>Feels activity is too expensive.</rdfs:comment>
    </owl:NamedIndividual>
    


    <!-- http://www.semanticweb.org/tswheeler/ontologies/2016/3/EmpowerBP#MotivationObstacle -->

    <owl:NamedIndividual rdf:about="http://www.semanticweb.org/tswheeler/ontologies/2016/3/EmpowerBP#MotivationObstacle">
        <rdf:type rdf:resource="http://www.semanticweb.org/tswheeler/ontologies/2016/3/EmpowerBP#Obstacle"/>
        <EmpowerBP:hasRelevantTDF rdf:resource="http://www.semanticweb.org/tswheeler/ontologies/2016/3/EmpowerBP#BeliefsAboutConsequences"/>
        <EmpowerBP:hasRelevantTDF rdf:resource="http://www.semanticweb.org/tswheeler/ontologies/2016/3/EmpowerBP#Emotion"/>
        <EmpowerBP:hasRelevantTDF rdf:resource="http://www.semanticweb.org/tswheeler/ontologies/2016/3/EmpowerBP#Goals"/>
        <EmpowerBP:hasRelevantTDF rdf:resource="http://www.semanticweb.org/tswheeler/ontologies/2016/3/EmpowerBP#Intentions"/>
        <EmpowerBP:hasRelevantTDF rdf:resource="http://www.semanticweb.org/tswheeler/ontologies/2016/3/EmpowerBP#Reinforcement"/>
        <EmpowerBP:hasRelevantTDF rdf:resource="http://www.semanticweb.org/tswheeler/ontologies/2016/3/EmpowerBP#SocialInfluences"/>
        <rdfs:comment>Does not have motivation to perform activity.</rdfs:comment>
    </owl:NamedIndividual>
    


    <!-- http://www.semanticweb.org/tswheeler/ontologies/2016/3/EmpowerBP#OT1 -->

    <owl:NamedIndividual rdf:about="http://www.semanticweb.org/tswheeler/ontologies/2016/3/EmpowerBP#OT1">
        <rdf:type rdf:resource="http://www.semanticweb.org/tswheeler/ontologies/2016/3/EmpowerBP#InterventionItem"/>
        <rdf:type rdf:resource="http://www.semanticweb.org/tswheeler/ontologies/2016/3/EmpowerBP#Tip"/>
        <EmpowerBP:isAppropriateForInterventionGoal rdf:resource="http://www.semanticweb.org/tswheeler/ontologies/2016/3/EmpowerBP#ExerciseMore"/>
        <EmpowerBP:isWarrantedBy rdf:resource="http://purl.bioontology.org/ontology/BCTT#Action_planning"/>
        <EmpowerBP:appropriateForAutomaticMotivation rdf:datatype="http://www.w3.org/2001/XMLSchema#integer">6</EmpowerBP:appropriateForAutomaticMotivation>
        <EmpowerBP:appropriateForLocation rdf:datatype="http://www.w3.org/2001/XMLSchema#integer">0</EmpowerBP:appropriateForLocation>
        <EmpowerBP:appropriateForPhysicalCapability rdf:datatype="http://www.w3.org/2001/XMLSchema#integer">3</EmpowerBP:appropriateForPhysicalCapability>
        <EmpowerBP:appropriateForPhysicalOpportunity rdf:datatype="http://www.w3.org/2001/XMLSchema#integer">3</EmpowerBP:appropriateForPhysicalOpportunity>
        <EmpowerBP:appropriateForPsychologicalCapability rdf:datatype="http://www.w3.org/2001/XMLSchema#integer">3</EmpowerBP:appropriateForPsychologicalCapability>
        <EmpowerBP:appropriateForReflectiveMotivation rdf:datatype="http://www.w3.org/2001/XMLSchema#integer">6</EmpowerBP:appropriateForReflectiveMotivation>
        <EmpowerBP:appropriateForSocialOpportunity rdf:datatype="http://www.w3.org/2001/XMLSchema#integer">3</EmpowerBP:appropriateForSocialOpportunity>
        <EmpowerBP:canRepeat rdf:datatype="http://www.w3.org/2001/XMLSchema#integer">26</EmpowerBP:canRepeat>
        <EmpowerBP:itemName rdf:datatype="http://www.w3.org/2001/XMLSchema#string">WalkaboutNS Time Tip</EmpowerBP:itemName>
        <EmpowerBP:itemText rdf:datatype="http://www.w3.org/2001/XMLSchema#string">Make appointments for walking just like you would anything else. Remember that every 10 minute chunk of walking counts! Walking clears your mind and helps you to be more productive, so walking can save time in the end.</EmpowerBP:itemText>
        <EmpowerBP:maximumUserAge rdf:datatype="http://www.w3.org/2001/XMLSchema#integer">120</EmpowerBP:maximumUserAge>
        <EmpowerBP:minimumUserAge rdf:datatype="http://www.w3.org/2001/XMLSchema#integer">18</EmpowerBP:minimumUserAge>
        <EmpowerBP:provideJournal rdf:datatype="http://www.w3.org/2001/XMLSchema#boolean">false</EmpowerBP:provideJournal>
        <EmpowerBP:provideLink rdf:datatype="http://www.w3.org/2001/XMLSchema#boolean">false</EmpowerBP:provideLink>
        <EmpowerBP:sourceURL rdf:datatype="http://www.w3.org/2001/XMLSchema#string">http://walkaboutns.ca/walkabout-info/inspiration/getting-over-barriers/</EmpowerBP:sourceURL>
        <rdfs:comment rdf:datatype="http://www.w3.org/2001/XMLSchema#string">Make appointments for walking just like you would anything else. Remember that every 10 minute chunk of walking counts! Walking clears your mind and helps you to be more productive, so walking can save time in the end.</rdfs:comment>
        <rdfs:label rdf:datatype="http://www.w3.org/2001/XMLSchema#string">WalkaboutNS Time Tip</rdfs:label>
    </owl:NamedIndividual>
    


    <!-- http://www.semanticweb.org/tswheeler/ontologies/2016/3/EmpowerBP#OT10 -->

    <owl:NamedIndividual rdf:about="http://www.semanticweb.org/tswheeler/ontologies/2016/3/EmpowerBP#OT10">
        <rdf:type rdf:resource="http://www.semanticweb.org/tswheeler/ontologies/2016/3/EmpowerBP#InterventionItem"/>
        <rdf:type rdf:resource="http://www.semanticweb.org/tswheeler/ontologies/2016/3/EmpowerBP#Tip"/>
        <EmpowerBP:isAppropriateForInterventionGoal rdf:resource="http://www.semanticweb.org/tswheeler/ontologies/2016/3/EmpowerBP#ExerciseMore"/>
        <EmpowerBP:isWarrantedBy rdf:resource="http://purl.bioontology.org/ontology/BCTT#Information_about_health_consequences"/>
        <EmpowerBP:appropriateForAutomaticMotivation rdf:datatype="http://www.w3.org/2001/XMLSchema#integer">3</EmpowerBP:appropriateForAutomaticMotivation>
        <EmpowerBP:appropriateForLocation rdf:datatype="http://www.w3.org/2001/XMLSchema#integer">0</EmpowerBP:appropriateForLocation>
        <EmpowerBP:appropriateForPhysicalCapability rdf:datatype="http://www.w3.org/2001/XMLSchema#integer">3</EmpowerBP:appropriateForPhysicalCapability>
        <EmpowerBP:appropriateForPhysicalOpportunity rdf:datatype="http://www.w3.org/2001/XMLSchema#integer">3</EmpowerBP:appropriateForPhysicalOpportunity>
        <EmpowerBP:appropriateForPsychologicalCapability rdf:datatype="http://www.w3.org/2001/XMLSchema#integer">3</EmpowerBP:appropriateForPsychologicalCapability>
        <EmpowerBP:appropriateForReflectiveMotivation rdf:datatype="http://www.w3.org/2001/XMLSchema#integer">3</EmpowerBP:appropriateForReflectiveMotivation>
        <EmpowerBP:appropriateForSocialOpportunity rdf:datatype="http://www.w3.org/2001/XMLSchema#integer">3</EmpowerBP:appropriateForSocialOpportunity>
        <EmpowerBP:canRepeat rdf:datatype="http://www.w3.org/2001/XMLSchema#integer">26</EmpowerBP:canRepeat>
        <EmpowerBP:itemName rdf:datatype="http://www.w3.org/2001/XMLSchema#string">PHAC Tip</EmpowerBP:itemName>
        <EmpowerBP:itemText rdf:datatype="http://www.w3.org/2001/XMLSchema#string">Is physical activity safe for everyone?

The recommended level of physical activity applies to all adults aged 65 years and older who do not have a suspected or diagnosed medical condition. Consult a health professional if you are unsure about the types and amounts of physical activity most appropriate for you.</EmpowerBP:itemText>
        <EmpowerBP:maximumUserAge rdf:datatype="http://www.w3.org/2001/XMLSchema#integer">120</EmpowerBP:maximumUserAge>
        <EmpowerBP:minimumUserAge rdf:datatype="http://www.w3.org/2001/XMLSchema#integer">65</EmpowerBP:minimumUserAge>
        <EmpowerBP:provideJournal rdf:datatype="http://www.w3.org/2001/XMLSchema#boolean">false</EmpowerBP:provideJournal>
        <EmpowerBP:provideLink rdf:datatype="http://www.w3.org/2001/XMLSchema#boolean">false</EmpowerBP:provideLink>
        <EmpowerBP:sourceURL rdf:datatype="http://www.w3.org/2001/XMLSchema#string">http://www.phac-aspc.gc.ca/hp-ps/hl-mvs/pa-ap/index-eng.php</EmpowerBP:sourceURL>
        <rdfs:comment rdf:datatype="http://www.w3.org/2001/XMLSchema#string">Is physical activity safe for everyone?

The recommended level of physical activity applies to all adults aged 65 years and older who do not have a suspected or diagnosed medical condition. Consult a health professional if you are unsure about the types and amounts of physical activity most appropriate for you.</rdfs:comment>
        <rdfs:label rdf:datatype="http://www.w3.org/2001/XMLSchema#string">PHAC Tip</rdfs:label>
    </owl:NamedIndividual>
    


    <!-- http://www.semanticweb.org/tswheeler/ontologies/2016/3/EmpowerBP#OT11 -->

    <owl:NamedIndividual rdf:about="http://www.semanticweb.org/tswheeler/ontologies/2016/3/EmpowerBP#OT11">
        <rdf:type rdf:resource="http://www.semanticweb.org/tswheeler/ontologies/2016/3/EmpowerBP#InterventionItem"/>
        <rdf:type rdf:resource="http://www.semanticweb.org/tswheeler/ontologies/2016/3/EmpowerBP#Tip"/>
        <EmpowerBP:isAppropriateForInterventionGoal rdf:resource="http://www.semanticweb.org/tswheeler/ontologies/2016/3/EmpowerBP#ExerciseMore"/>
        <EmpowerBP:isWarrantedBy rdf:resource="http://purl.bioontology.org/ontology/BCTT#Graded_tasks"/>
        <EmpowerBP:appropriateForAutomaticMotivation rdf:datatype="http://www.w3.org/2001/XMLSchema#integer">3</EmpowerBP:appropriateForAutomaticMotivation>
        <EmpowerBP:appropriateForLocation rdf:datatype="http://www.w3.org/2001/XMLSchema#integer">0</EmpowerBP:appropriateForLocation>
        <EmpowerBP:appropriateForPhysicalCapability rdf:datatype="http://www.w3.org/2001/XMLSchema#integer">3</EmpowerBP:appropriateForPhysicalCapability>
        <EmpowerBP:appropriateForPhysicalOpportunity rdf:datatype="http://www.w3.org/2001/XMLSchema#integer">3</EmpowerBP:appropriateForPhysicalOpportunity>
        <EmpowerBP:appropriateForPsychologicalCapability rdf:datatype="http://www.w3.org/2001/XMLSchema#integer">3</EmpowerBP:appropriateForPsychologicalCapability>
        <EmpowerBP:appropriateForReflectiveMotivation rdf:datatype="http://www.w3.org/2001/XMLSchema#integer">3</EmpowerBP:appropriateForReflectiveMotivation>
        <EmpowerBP:appropriateForSocialOpportunity rdf:datatype="http://www.w3.org/2001/XMLSchema#integer">3</EmpowerBP:appropriateForSocialOpportunity>
        <EmpowerBP:canRepeat rdf:datatype="http://www.w3.org/2001/XMLSchema#integer">26</EmpowerBP:canRepeat>
        <EmpowerBP:itemName rdf:datatype="http://www.w3.org/2001/XMLSchema#string">Diabetes.ca Time Tip</EmpowerBP:itemName>
        <EmpowerBP:itemText rdf:datatype="http://www.w3.org/2001/XMLSchema#string">&quot;I have no time&quot;

Every minute of physical activity has health benefits! Start with 5 to 10 minutes at a time; at different times throughout the day. This may be all you need to get going.</EmpowerBP:itemText>
        <EmpowerBP:maximumUserAge rdf:datatype="http://www.w3.org/2001/XMLSchema#integer">120</EmpowerBP:maximumUserAge>
        <EmpowerBP:minimumUserAge rdf:datatype="http://www.w3.org/2001/XMLSchema#integer">18</EmpowerBP:minimumUserAge>
        <EmpowerBP:provideJournal rdf:datatype="http://www.w3.org/2001/XMLSchema#boolean">false</EmpowerBP:provideJournal>
        <EmpowerBP:provideLink rdf:datatype="http://www.w3.org/2001/XMLSchema#boolean">false</EmpowerBP:provideLink>
        <EmpowerBP:sourceURL rdf:datatype="http://www.w3.org/2001/XMLSchema#string">https://www.diabetes.ca/diabetes-and-you/healthy-living-resources/exercise/overcoming-barriers-to-physical-activity</EmpowerBP:sourceURL>
        <rdfs:comment rdf:datatype="http://www.w3.org/2001/XMLSchema#string">&quot;I have no time&quot;

Every minute of physical activity has health benefits! Start with 5 to 10 minutes at a time; at different times throughout the day. This may be all you need to get going.</rdfs:comment>
        <rdfs:label rdf:datatype="http://www.w3.org/2001/XMLSchema#string">Diabetes.ca Time Tip</rdfs:label>
    </owl:NamedIndividual>
    


    <!-- http://www.semanticweb.org/tswheeler/ontologies/2016/3/EmpowerBP#OT12 -->

    <owl:NamedIndividual rdf:about="http://www.semanticweb.org/tswheeler/ontologies/2016/3/EmpowerBP#OT12">
        <rdf:type rdf:resource="http://www.semanticweb.org/tswheeler/ontologies/2016/3/EmpowerBP#InterventionItem"/>
        <rdf:type rdf:resource="http://www.semanticweb.org/tswheeler/ontologies/2016/3/EmpowerBP#Tip"/>
        <EmpowerBP:isAppropriateForInterventionGoal rdf:resource="http://www.semanticweb.org/tswheeler/ontologies/2016/3/EmpowerBP#ExerciseMore"/>
        <EmpowerBP:isWarrantedBy rdf:resource="http://purl.bioontology.org/ontology/BCTT#Non-specific_incentive"/>
        <EmpowerBP:appropriateForAutomaticMotivation rdf:datatype="http://www.w3.org/2001/XMLSchema#integer">3</EmpowerBP:appropriateForAutomaticMotivation>
        <EmpowerBP:appropriateForLocation rdf:datatype="http://www.w3.org/2001/XMLSchema#integer">0</EmpowerBP:appropriateForLocation>
        <EmpowerBP:appropriateForPhysicalCapability rdf:datatype="http://www.w3.org/2001/XMLSchema#integer">3</EmpowerBP:appropriateForPhysicalCapability>
        <EmpowerBP:appropriateForPhysicalOpportunity rdf:datatype="http://www.w3.org/2001/XMLSchema#integer">3</EmpowerBP:appropriateForPhysicalOpportunity>
        <EmpowerBP:appropriateForPsychologicalCapability rdf:datatype="http://www.w3.org/2001/XMLSchema#integer">3</EmpowerBP:appropriateForPsychologicalCapability>
        <EmpowerBP:appropriateForReflectiveMotivation rdf:datatype="http://www.w3.org/2001/XMLSchema#integer">3</EmpowerBP:appropriateForReflectiveMotivation>
        <EmpowerBP:appropriateForSocialOpportunity rdf:datatype="http://www.w3.org/2001/XMLSchema#integer">3</EmpowerBP:appropriateForSocialOpportunity>
        <EmpowerBP:canRepeat rdf:datatype="http://www.w3.org/2001/XMLSchema#integer">26</EmpowerBP:canRepeat>
        <EmpowerBP:itemName rdf:datatype="http://www.w3.org/2001/XMLSchema#string">Diabetes.ca Energy Tip</EmpowerBP:itemName>
        <EmpowerBP:itemText rdf:datatype="http://www.w3.org/2001/XMLSchema#string">&quot;I am too tired&quot;

Regular physical activity will give you more energy and help you sleep better. It may be hard to get started, but once you start, you’ll feel better. In the end, it will be worth the effort.</EmpowerBP:itemText>
        <EmpowerBP:maximumUserAge rdf:datatype="http://www.w3.org/2001/XMLSchema#integer">120</EmpowerBP:maximumUserAge>
        <EmpowerBP:minimumUserAge rdf:datatype="http://www.w3.org/2001/XMLSchema#integer">18</EmpowerBP:minimumUserAge>
        <EmpowerBP:provideJournal rdf:datatype="http://www.w3.org/2001/XMLSchema#boolean">false</EmpowerBP:provideJournal>
        <EmpowerBP:provideLink rdf:datatype="http://www.w3.org/2001/XMLSchema#boolean">false</EmpowerBP:provideLink>
        <EmpowerBP:sourceURL rdf:datatype="http://www.w3.org/2001/XMLSchema#string">https://www.diabetes.ca/diabetes-and-you/healthy-living-resources/exercise/overcoming-barriers-to-physical-activity</EmpowerBP:sourceURL>
        <rdfs:comment rdf:datatype="http://www.w3.org/2001/XMLSchema#string">&quot;I am too tired&quot;

Regular physical activity will give you more energy and help you sleep better. It may be hard to get started, but once you start, you’ll feel better. In the end, it will be worth the effort.</rdfs:comment>
        <rdfs:label rdf:datatype="http://www.w3.org/2001/XMLSchema#string">Diabetes.ca Energy Tip</rdfs:label>
    </owl:NamedIndividual>
    


    <!-- http://www.semanticweb.org/tswheeler/ontologies/2016/3/EmpowerBP#OT13 -->

    <owl:NamedIndividual rdf:about="http://www.semanticweb.org/tswheeler/ontologies/2016/3/EmpowerBP#OT13">
        <rdf:type rdf:resource="http://www.semanticweb.org/tswheeler/ontologies/2016/3/EmpowerBP#InterventionItem"/>
        <rdf:type rdf:resource="http://www.semanticweb.org/tswheeler/ontologies/2016/3/EmpowerBP#Tip"/>
        <EmpowerBP:isAppropriateForInterventionGoal rdf:resource="http://www.semanticweb.org/tswheeler/ontologies/2016/3/EmpowerBP#ExerciseMore"/>
        <EmpowerBP:isWarrantedBy rdf:resource="http://purl.bioontology.org/ontology/BCTT#Graded_tasks"/>
        <EmpowerBP:appropriateForAutomaticMotivation rdf:datatype="http://www.w3.org/2001/XMLSchema#integer">3</EmpowerBP:appropriateForAutomaticMotivation>
        <EmpowerBP:appropriateForLocation rdf:datatype="http://www.w3.org/2001/XMLSchema#integer">0</EmpowerBP:appropriateForLocation>
        <EmpowerBP:appropriateForPhysicalCapability rdf:datatype="http://www.w3.org/2001/XMLSchema#integer">3</EmpowerBP:appropriateForPhysicalCapability>
        <EmpowerBP:appropriateForPhysicalOpportunity rdf:datatype="http://www.w3.org/2001/XMLSchema#integer">3</EmpowerBP:appropriateForPhysicalOpportunity>
        <EmpowerBP:appropriateForPsychologicalCapability rdf:datatype="http://www.w3.org/2001/XMLSchema#integer">3</EmpowerBP:appropriateForPsychologicalCapability>
        <EmpowerBP:appropriateForReflectiveMotivation rdf:datatype="http://www.w3.org/2001/XMLSchema#integer">3</EmpowerBP:appropriateForReflectiveMotivation>
        <EmpowerBP:appropriateForSocialOpportunity rdf:datatype="http://www.w3.org/2001/XMLSchema#integer">3</EmpowerBP:appropriateForSocialOpportunity>
        <EmpowerBP:canRepeat rdf:datatype="http://www.w3.org/2001/XMLSchema#integer">26</EmpowerBP:canRepeat>
        <EmpowerBP:itemName rdf:datatype="http://www.w3.org/2001/XMLSchema#string">Diabetes.ca Motivation Tip</EmpowerBP:itemName>
        <EmpowerBP:itemText rdf:datatype="http://www.w3.org/2001/XMLSchema#string">&quot;I do not have the motivation&quot;

Start with five minutes of physical activity, and allow yourself to stop if you are not enjoying it. That way you can at least start, and once you are into it, you may want to keep going.</EmpowerBP:itemText>
        <EmpowerBP:maximumUserAge rdf:datatype="http://www.w3.org/2001/XMLSchema#integer">120</EmpowerBP:maximumUserAge>
        <EmpowerBP:minimumUserAge rdf:datatype="http://www.w3.org/2001/XMLSchema#integer">18</EmpowerBP:minimumUserAge>
        <EmpowerBP:provideJournal rdf:datatype="http://www.w3.org/2001/XMLSchema#boolean">false</EmpowerBP:provideJournal>
        <EmpowerBP:provideLink rdf:datatype="http://www.w3.org/2001/XMLSchema#boolean">false</EmpowerBP:provideLink>
        <EmpowerBP:sourceURL rdf:datatype="http://www.w3.org/2001/XMLSchema#string">https://www.diabetes.ca/diabetes-and-you/healthy-living-resources/exercise/overcoming-barriers-to-physical-activity</EmpowerBP:sourceURL>
        <rdfs:comment rdf:datatype="http://www.w3.org/2001/XMLSchema#string">&quot;I do not have the motivation&quot;

Start with five minutes of physical activity, and allow yourself to stop if you are not enjoying it. That way you can at least start, and once you are into it, you may want to keep going.</rdfs:comment>
        <rdfs:label rdf:datatype="http://www.w3.org/2001/XMLSchema#string">Diabetes.ca Motivation Tip</rdfs:label>
    </owl:NamedIndividual>
    


    <!-- http://www.semanticweb.org/tswheeler/ontologies/2016/3/EmpowerBP#OT14 -->

    <owl:NamedIndividual rdf:about="http://www.semanticweb.org/tswheeler/ontologies/2016/3/EmpowerBP#OT14">
        <rdf:type rdf:resource="http://www.semanticweb.org/tswheeler/ontologies/2016/3/EmpowerBP#InterventionItem"/>
        <rdf:type rdf:resource="http://www.semanticweb.org/tswheeler/ontologies/2016/3/EmpowerBP#Tip"/>
        <EmpowerBP:isAppropriateForInterventionGoal rdf:resource="http://www.semanticweb.org/tswheeler/ontologies/2016/3/EmpowerBP#ExerciseMore"/>
        <EmpowerBP:isWarrantedBy rdf:resource="http://purl.bioontology.org/ontology/BCTT#Instruction_on_how_to_perform_the_behavior"/>
        <EmpowerBP:appropriateForAutomaticMotivation rdf:datatype="http://www.w3.org/2001/XMLSchema#integer">3</EmpowerBP:appropriateForAutomaticMotivation>
        <EmpowerBP:appropriateForLocation rdf:datatype="http://www.w3.org/2001/XMLSchema#integer">0</EmpowerBP:appropriateForLocation>
        <EmpowerBP:appropriateForPhysicalCapability rdf:datatype="http://www.w3.org/2001/XMLSchema#integer">3</EmpowerBP:appropriateForPhysicalCapability>
        <EmpowerBP:appropriateForPhysicalOpportunity rdf:datatype="http://www.w3.org/2001/XMLSchema#integer">3</EmpowerBP:appropriateForPhysicalOpportunity>
        <EmpowerBP:appropriateForPsychologicalCapability rdf:datatype="http://www.w3.org/2001/XMLSchema#integer">3</EmpowerBP:appropriateForPsychologicalCapability>
        <EmpowerBP:appropriateForReflectiveMotivation rdf:datatype="http://www.w3.org/2001/XMLSchema#integer">3</EmpowerBP:appropriateForReflectiveMotivation>
        <EmpowerBP:appropriateForSocialOpportunity rdf:datatype="http://www.w3.org/2001/XMLSchema#integer">3</EmpowerBP:appropriateForSocialOpportunity>
        <EmpowerBP:canRepeat rdf:datatype="http://www.w3.org/2001/XMLSchema#integer">26</EmpowerBP:canRepeat>
        <EmpowerBP:itemName rdf:datatype="http://www.w3.org/2001/XMLSchema#string">Diabetes.ca Cost Tip</EmpowerBP:itemName>
        <EmpowerBP:itemText rdf:datatype="http://www.w3.org/2001/XMLSchema#string">&quot;It costs too much to join a gym&quot;

You do not need a gym membership or a personal trainer to be active. You can do simple things around the house or in your neighbourhood that do not cost money – go for a short walk or start a project in your yard.</EmpowerBP:itemText>
        <EmpowerBP:maximumUserAge rdf:datatype="http://www.w3.org/2001/XMLSchema#integer">120</EmpowerBP:maximumUserAge>
        <EmpowerBP:minimumUserAge rdf:datatype="http://www.w3.org/2001/XMLSchema#integer">18</EmpowerBP:minimumUserAge>
        <EmpowerBP:provideJournal rdf:datatype="http://www.w3.org/2001/XMLSchema#boolean">false</EmpowerBP:provideJournal>
        <EmpowerBP:provideLink rdf:datatype="http://www.w3.org/2001/XMLSchema#boolean">false</EmpowerBP:provideLink>
        <EmpowerBP:sourceURL rdf:datatype="http://www.w3.org/2001/XMLSchema#string">https://www.diabetes.ca/diabetes-and-you/healthy-living-resources/exercise/overcoming-barriers-to-physical-activity</EmpowerBP:sourceURL>
        <rdfs:comment rdf:datatype="http://www.w3.org/2001/XMLSchema#string">&quot;It costs too much to join a gym&quot;

You do not need a gym membership or a personal trainer to be active. You can do simple things around the house or in your neighbourhood that do not cost money – go for a short walk or start a project in your yard.</rdfs:comment>
        <rdfs:label rdf:datatype="http://www.w3.org/2001/XMLSchema#string">Diabetes.ca Cost Tip</rdfs:label>
    </owl:NamedIndividual>
    


    <!-- http://www.semanticweb.org/tswheeler/ontologies/2016/3/EmpowerBP#OT15 -->

    <owl:NamedIndividual rdf:about="http://www.semanticweb.org/tswheeler/ontologies/2016/3/EmpowerBP#OT15">
        <rdf:type rdf:resource="http://www.semanticweb.org/tswheeler/ontologies/2016/3/EmpowerBP#InterventionItem"/>
        <rdf:type rdf:resource="http://www.semanticweb.org/tswheeler/ontologies/2016/3/EmpowerBP#Tip"/>
        <EmpowerBP:isAppropriateForInterventionGoal rdf:resource="http://www.semanticweb.org/tswheeler/ontologies/2016/3/EmpowerBP#ExerciseMore"/>
        <EmpowerBP:isWarrantedBy rdf:resource="http://purl.bioontology.org/ontology/BCTT#Social_support_(unspecified)"/>
        <EmpowerBP:appropriateForAutomaticMotivation rdf:datatype="http://www.w3.org/2001/XMLSchema#integer">3</EmpowerBP:appropriateForAutomaticMotivation>
        <EmpowerBP:appropriateForLocation rdf:datatype="http://www.w3.org/2001/XMLSchema#integer">0</EmpowerBP:appropriateForLocation>
        <EmpowerBP:appropriateForPhysicalCapability rdf:datatype="http://www.w3.org/2001/XMLSchema#integer">3</EmpowerBP:appropriateForPhysicalCapability>
        <EmpowerBP:appropriateForPhysicalOpportunity rdf:datatype="http://www.w3.org/2001/XMLSchema#integer">3</EmpowerBP:appropriateForPhysicalOpportunity>
        <EmpowerBP:appropriateForPsychologicalCapability rdf:datatype="http://www.w3.org/2001/XMLSchema#integer">3</EmpowerBP:appropriateForPsychologicalCapability>
        <EmpowerBP:appropriateForReflectiveMotivation rdf:datatype="http://www.w3.org/2001/XMLSchema#integer">3</EmpowerBP:appropriateForReflectiveMotivation>
        <EmpowerBP:appropriateForSocialOpportunity rdf:datatype="http://www.w3.org/2001/XMLSchema#integer">3</EmpowerBP:appropriateForSocialOpportunity>
        <EmpowerBP:canRepeat rdf:datatype="http://www.w3.org/2001/XMLSchema#integer">26</EmpowerBP:canRepeat>
        <EmpowerBP:itemName rdf:datatype="http://www.w3.org/2001/XMLSchema#string">Diabetes.ca Social Support Tip</EmpowerBP:itemName>
        <EmpowerBP:itemText rdf:datatype="http://www.w3.org/2001/XMLSchema#string">&quot;I cannot be physically active on my own&quot;

You may be surprised by the support you receive. Doing your activity with others can help to get you started and keep you going. Your local recreation centre may also be able to help you find activity partners.</EmpowerBP:itemText>
        <EmpowerBP:maximumUserAge rdf:datatype="http://www.w3.org/2001/XMLSchema#integer">120</EmpowerBP:maximumUserAge>
        <EmpowerBP:minimumUserAge rdf:datatype="http://www.w3.org/2001/XMLSchema#integer">18</EmpowerBP:minimumUserAge>
        <EmpowerBP:provideJournal rdf:datatype="http://www.w3.org/2001/XMLSchema#boolean">false</EmpowerBP:provideJournal>
        <EmpowerBP:provideLink rdf:datatype="http://www.w3.org/2001/XMLSchema#boolean">false</EmpowerBP:provideLink>
        <EmpowerBP:sourceURL rdf:datatype="http://www.w3.org/2001/XMLSchema#string">https://www.diabetes.ca/diabetes-and-you/healthy-living-resources/exercise/overcoming-barriers-to-physical-activity</EmpowerBP:sourceURL>
        <rdfs:comment rdf:datatype="http://www.w3.org/2001/XMLSchema#string">&quot;I cannot be physically active on my own&quot;

You may be surprised by the support you receive. Doing your activity with others can help to get you started and keep you going. Your local recreation centre may also be able to help you find activity partners.</rdfs:comment>
        <rdfs:label rdf:datatype="http://www.w3.org/2001/XMLSchema#string">Diabetes.ca Social Support Tip</rdfs:label>
    </owl:NamedIndividual>
    


    <!-- http://www.semanticweb.org/tswheeler/ontologies/2016/3/EmpowerBP#OT16 -->

    <owl:NamedIndividual rdf:about="http://www.semanticweb.org/tswheeler/ontologies/2016/3/EmpowerBP#OT16">
        <rdf:type rdf:resource="http://www.semanticweb.org/tswheeler/ontologies/2016/3/EmpowerBP#InterventionItem"/>
        <rdf:type rdf:resource="http://www.semanticweb.org/tswheeler/ontologies/2016/3/EmpowerBP#Tip"/>
        <EmpowerBP:isAppropriateForInterventionGoal rdf:resource="http://www.semanticweb.org/tswheeler/ontologies/2016/3/EmpowerBP#ExerciseMore"/>
        <EmpowerBP:isWarrantedBy rdf:resource="http://purl.bioontology.org/ontology/BCTT#Instruction_on_how_to_perform_the_behavior"/>
        <EmpowerBP:appropriateForAutomaticMotivation rdf:datatype="http://www.w3.org/2001/XMLSchema#integer">3</EmpowerBP:appropriateForAutomaticMotivation>
        <EmpowerBP:appropriateForLocation rdf:datatype="http://www.w3.org/2001/XMLSchema#integer">0</EmpowerBP:appropriateForLocation>
        <EmpowerBP:appropriateForPhysicalCapability rdf:datatype="http://www.w3.org/2001/XMLSchema#integer">3</EmpowerBP:appropriateForPhysicalCapability>
        <EmpowerBP:appropriateForPhysicalOpportunity rdf:datatype="http://www.w3.org/2001/XMLSchema#integer">3</EmpowerBP:appropriateForPhysicalOpportunity>
        <EmpowerBP:appropriateForPsychologicalCapability rdf:datatype="http://www.w3.org/2001/XMLSchema#integer">3</EmpowerBP:appropriateForPsychologicalCapability>
        <EmpowerBP:appropriateForReflectiveMotivation rdf:datatype="http://www.w3.org/2001/XMLSchema#integer">3</EmpowerBP:appropriateForReflectiveMotivation>
        <EmpowerBP:appropriateForSocialOpportunity rdf:datatype="http://www.w3.org/2001/XMLSchema#integer">3</EmpowerBP:appropriateForSocialOpportunity>
        <EmpowerBP:canRepeat rdf:datatype="http://www.w3.org/2001/XMLSchema#integer">26</EmpowerBP:canRepeat>
        <EmpowerBP:itemName rdf:datatype="http://www.w3.org/2001/XMLSchema#string">Diabetes.ca Injury Tip</EmpowerBP:itemName>
        <EmpowerBP:itemText rdf:datatype="http://www.w3.org/2001/XMLSchema#string">&quot;I am afraid of injury or re-injury&quot;

Take care of any injuries. It is difficult to be active if you are hurting. See your doctor or physiotherapist about any nagging pains that may limit your physical activity. Remember to take good care of your body and always wear proper equipment like foot wear.</EmpowerBP:itemText>
        <EmpowerBP:maximumUserAge rdf:datatype="http://www.w3.org/2001/XMLSchema#integer">120</EmpowerBP:maximumUserAge>
        <EmpowerBP:minimumUserAge rdf:datatype="http://www.w3.org/2001/XMLSchema#integer">18</EmpowerBP:minimumUserAge>
        <EmpowerBP:provideJournal rdf:datatype="http://www.w3.org/2001/XMLSchema#boolean">false</EmpowerBP:provideJournal>
        <EmpowerBP:provideLink rdf:datatype="http://www.w3.org/2001/XMLSchema#boolean">false</EmpowerBP:provideLink>
        <EmpowerBP:sourceURL rdf:datatype="http://www.w3.org/2001/XMLSchema#string">https://www.diabetes.ca/diabetes-and-you/healthy-living-resources/exercise/overcoming-barriers-to-physical-activity</EmpowerBP:sourceURL>
        <rdfs:comment rdf:datatype="http://www.w3.org/2001/XMLSchema#string">&quot;I am afraid of injury or re-injury&quot;

Take care of any injuries. It is difficult to be active if you are hurting. See your doctor or physiotherapist about any nagging pains that may limit your physical activity. Remember to take good care of your body and always wear proper equipment like foot wear.</rdfs:comment>
        <rdfs:label rdf:datatype="http://www.w3.org/2001/XMLSchema#string">Diabetes.ca Injury Tip</rdfs:label>
    </owl:NamedIndividual>
    


    <!-- http://www.semanticweb.org/tswheeler/ontologies/2016/3/EmpowerBP#OT17 -->

    <owl:NamedIndividual rdf:about="http://www.semanticweb.org/tswheeler/ontologies/2016/3/EmpowerBP#OT17">
        <rdf:type rdf:resource="http://www.semanticweb.org/tswheeler/ontologies/2016/3/EmpowerBP#InterventionItem"/>
        <rdf:type rdf:resource="http://www.semanticweb.org/tswheeler/ontologies/2016/3/EmpowerBP#Tip"/>
        <EmpowerBP:isAppropriateForInterventionGoal rdf:resource="http://www.semanticweb.org/tswheeler/ontologies/2016/3/EmpowerBP#ReduceSaltIntake"/>
        <EmpowerBP:isWarrantedBy rdf:resource="http://purl.bioontology.org/ontology/BCTT#Instruction_on_how_to_perform_the_behavior"/>
        <EmpowerBP:appropriateForAutomaticMotivation rdf:datatype="http://www.w3.org/2001/XMLSchema#integer">3</EmpowerBP:appropriateForAutomaticMotivation>
        <EmpowerBP:appropriateForLocation rdf:datatype="http://www.w3.org/2001/XMLSchema#integer">0</EmpowerBP:appropriateForLocation>
        <EmpowerBP:appropriateForPhysicalCapability rdf:datatype="http://www.w3.org/2001/XMLSchema#integer">3</EmpowerBP:appropriateForPhysicalCapability>
        <EmpowerBP:appropriateForPhysicalOpportunity rdf:datatype="http://www.w3.org/2001/XMLSchema#integer">3</EmpowerBP:appropriateForPhysicalOpportunity>
        <EmpowerBP:appropriateForPsychologicalCapability rdf:datatype="http://www.w3.org/2001/XMLSchema#integer">3</EmpowerBP:appropriateForPsychologicalCapability>
        <EmpowerBP:appropriateForReflectiveMotivation rdf:datatype="http://www.w3.org/2001/XMLSchema#integer">3</EmpowerBP:appropriateForReflectiveMotivation>
        <EmpowerBP:appropriateForSocialOpportunity rdf:datatype="http://www.w3.org/2001/XMLSchema#integer">3</EmpowerBP:appropriateForSocialOpportunity>
        <EmpowerBP:canRepeat rdf:datatype="http://www.w3.org/2001/XMLSchema#integer">26</EmpowerBP:canRepeat>
        <EmpowerBP:itemName rdf:datatype="http://www.w3.org/2001/XMLSchema#string">Time-Saving Kitchen Tips</EmpowerBP:itemName>
        <EmpowerBP:itemText rdf:datatype="http://www.w3.org/2001/XMLSchema#string">Easy tips to save time in the kitchen:

• Chop extra fruit and vegetables when preparing meals so you have extra for lunches, snacks, and meals the next day.
• Buy pre-cut vegetables such as broccoli, squash, and mushrooms.
• Choose lower-sodium convenience foods to help speed up prep time. Try canned or bottled tomato-based pasta sauces, frozen or canned vegetables and fruit, canned tuna or salmon, and canned beans or lentils.
</EmpowerBP:itemText>
        <EmpowerBP:maximumUserAge rdf:datatype="http://www.w3.org/2001/XMLSchema#integer">120</EmpowerBP:maximumUserAge>
        <EmpowerBP:minimumUserAge rdf:datatype="http://www.w3.org/2001/XMLSchema#integer">18</EmpowerBP:minimumUserAge>
        <EmpowerBP:provideJournal rdf:datatype="http://www.w3.org/2001/XMLSchema#boolean">false</EmpowerBP:provideJournal>
        <EmpowerBP:provideLink rdf:datatype="http://www.w3.org/2001/XMLSchema#boolean">false</EmpowerBP:provideLink>
        <EmpowerBP:sourceURL rdf:datatype="http://www.w3.org/2001/XMLSchema#string">https://www.canada.ca/en/health-canada/services/tips-healthy-eating/time-saving-cooking-tips-healthy-meals.html</EmpowerBP:sourceURL>
        <rdfs:comment rdf:datatype="http://www.w3.org/2001/XMLSchema#string">Easy tips to save time in the kitchen:

• Chop extra fruit and vegetables when preparing meals so you have extra for lunches, snacks, and meals the next day.
• Buy pre-cut vegetables such as broccoli, squash, and mushrooms.
• Choose lower-sodium convenience foods to help speed up prep time. Try canned or bottled tomato-based pasta sauces, frozen or canned vegetables and fruit, canned tuna or salmon, and canned beans or lentils.
</rdfs:comment>
        <rdfs:label rdf:datatype="http://www.w3.org/2001/XMLSchema#string">Time-Saving Kitchen Tips</rdfs:label>
    </owl:NamedIndividual>
    


    <!-- http://www.semanticweb.org/tswheeler/ontologies/2016/3/EmpowerBP#OT18 -->

    <owl:NamedIndividual rdf:about="http://www.semanticweb.org/tswheeler/ontologies/2016/3/EmpowerBP#OT18">
        <rdf:type rdf:resource="http://www.semanticweb.org/tswheeler/ontologies/2016/3/EmpowerBP#InterventionItem"/>
        <rdf:type rdf:resource="http://www.semanticweb.org/tswheeler/ontologies/2016/3/EmpowerBP#Tip"/>
        <EmpowerBP:isAppropriateForInterventionGoal rdf:resource="http://www.semanticweb.org/tswheeler/ontologies/2016/3/EmpowerBP#ReduceSaltIntake"/>
        <EmpowerBP:isWarrantedBy rdf:resource="http://purl.bioontology.org/ontology/BCTT#Instruction_on_how_to_perform_the_behavior"/>
        <EmpowerBP:appropriateForAutomaticMotivation rdf:datatype="http://www.w3.org/2001/XMLSchema#integer">3</EmpowerBP:appropriateForAutomaticMotivation>
        <EmpowerBP:appropriateForLocation rdf:datatype="http://www.w3.org/2001/XMLSchema#integer">0</EmpowerBP:appropriateForLocation>
        <EmpowerBP:appropriateForPhysicalCapability rdf:datatype="http://www.w3.org/2001/XMLSchema#integer">3</EmpowerBP:appropriateForPhysicalCapability>
        <EmpowerBP:appropriateForPhysicalOpportunity rdf:datatype="http://www.w3.org/2001/XMLSchema#integer">3</EmpowerBP:appropriateForPhysicalOpportunity>
        <EmpowerBP:appropriateForPsychologicalCapability rdf:datatype="http://www.w3.org/2001/XMLSchema#integer">3</EmpowerBP:appropriateForPsychologicalCapability>
        <EmpowerBP:appropriateForReflectiveMotivation rdf:datatype="http://www.w3.org/2001/XMLSchema#integer">3</EmpowerBP:appropriateForReflectiveMotivation>
        <EmpowerBP:appropriateForSocialOpportunity rdf:datatype="http://www.w3.org/2001/XMLSchema#integer">3</EmpowerBP:appropriateForSocialOpportunity>
        <EmpowerBP:canRepeat rdf:datatype="http://www.w3.org/2001/XMLSchema#integer">26</EmpowerBP:canRepeat>
        <EmpowerBP:itemName rdf:datatype="http://www.w3.org/2001/XMLSchema#string">Time-Saving Kitchen Tips</EmpowerBP:itemName>
        <EmpowerBP:itemText rdf:datatype="http://www.w3.org/2001/XMLSchema#string">Easy tips to save time in the kitchen:

• Cook on the weekend. Make-then freeze-meals for the upcoming week like soups, stews, casseroles, pasta dishes, and chili. These will come in handy on busy weeknights.
• Cook twice the chicken or ground beef you need and keep extras in the fridge to make chicken salad, enchiladas, chili, or spaghetti sauce the next day.</EmpowerBP:itemText>
        <EmpowerBP:maximumUserAge rdf:datatype="http://www.w3.org/2001/XMLSchema#integer">120</EmpowerBP:maximumUserAge>
        <EmpowerBP:minimumUserAge rdf:datatype="http://www.w3.org/2001/XMLSchema#integer">18</EmpowerBP:minimumUserAge>
        <EmpowerBP:provideJournal rdf:datatype="http://www.w3.org/2001/XMLSchema#boolean">false</EmpowerBP:provideJournal>
        <EmpowerBP:provideLink rdf:datatype="http://www.w3.org/2001/XMLSchema#boolean">false</EmpowerBP:provideLink>
        <EmpowerBP:sourceURL rdf:datatype="http://www.w3.org/2001/XMLSchema#string">https://www.canada.ca/en/health-canada/services/tips-healthy-eating/time-saving-cooking-tips-healthy-meals.html</EmpowerBP:sourceURL>
        <rdfs:comment rdf:datatype="http://www.w3.org/2001/XMLSchema#string">Easy tips to save time in the kitchen:

• Cook on the weekend. Make-then freeze-meals for the upcoming week like soups, stews, casseroles, pasta dishes, and chili. These will come in handy on busy weeknights.
• Cook twice the chicken or ground beef you need and keep extras in the fridge to make chicken salad, enchiladas, chili, or spaghetti sauce the next day.</rdfs:comment>
        <rdfs:label rdf:datatype="http://www.w3.org/2001/XMLSchema#string">Time-Saving Kitchen Tips</rdfs:label>
    </owl:NamedIndividual>
    


    <!-- http://www.semanticweb.org/tswheeler/ontologies/2016/3/EmpowerBP#OT19 -->

    <owl:NamedIndividual rdf:about="http://www.semanticweb.org/tswheeler/ontologies/2016/3/EmpowerBP#OT19">
        <rdf:type rdf:resource="http://www.semanticweb.org/tswheeler/ontologies/2016/3/EmpowerBP#InterventionItem"/>
        <rdf:type rdf:resource="http://www.semanticweb.org/tswheeler/ontologies/2016/3/EmpowerBP#Tip"/>
        <EmpowerBP:isAppropriateForInterventionGoal rdf:resource="http://www.semanticweb.org/tswheeler/ontologies/2016/3/EmpowerBP#ReduceSaltIntake"/>
        <EmpowerBP:isWarrantedBy rdf:resource="http://purl.bioontology.org/ontology/BCTT#Instruction_on_how_to_perform_the_behavior"/>
        <EmpowerBP:appropriateForAutomaticMotivation rdf:datatype="http://www.w3.org/2001/XMLSchema#integer">3</EmpowerBP:appropriateForAutomaticMotivation>
        <EmpowerBP:appropriateForLocation rdf:datatype="http://www.w3.org/2001/XMLSchema#integer">0</EmpowerBP:appropriateForLocation>
        <EmpowerBP:appropriateForPhysicalCapability rdf:datatype="http://www.w3.org/2001/XMLSchema#integer">3</EmpowerBP:appropriateForPhysicalCapability>
        <EmpowerBP:appropriateForPhysicalOpportunity rdf:datatype="http://www.w3.org/2001/XMLSchema#integer">3</EmpowerBP:appropriateForPhysicalOpportunity>
        <EmpowerBP:appropriateForPsychologicalCapability rdf:datatype="http://www.w3.org/2001/XMLSchema#integer">3</EmpowerBP:appropriateForPsychologicalCapability>
        <EmpowerBP:appropriateForReflectiveMotivation rdf:datatype="http://www.w3.org/2001/XMLSchema#integer">3</EmpowerBP:appropriateForReflectiveMotivation>
        <EmpowerBP:appropriateForSocialOpportunity rdf:datatype="http://www.w3.org/2001/XMLSchema#integer">3</EmpowerBP:appropriateForSocialOpportunity>
        <EmpowerBP:canRepeat rdf:datatype="http://www.w3.org/2001/XMLSchema#integer">26</EmpowerBP:canRepeat>
        <EmpowerBP:itemName rdf:datatype="http://www.w3.org/2001/XMLSchema#string">Time-Saving Kitchen Tips</EmpowerBP:itemName>
        <EmpowerBP:itemText rdf:datatype="http://www.w3.org/2001/XMLSchema#string">Easy tip to save time in the kitchen:

• Invest in time-saving appliances. A slow cooker is a great way to come home to a warm meal. A hand blender can help you make quick and easy soups, sauces, and smoothies. Use a mini-chopper to dice up garlic and onions.</EmpowerBP:itemText>
        <EmpowerBP:maximumUserAge rdf:datatype="http://www.w3.org/2001/XMLSchema#integer">120</EmpowerBP:maximumUserAge>
        <EmpowerBP:minimumUserAge rdf:datatype="http://www.w3.org/2001/XMLSchema#integer">18</EmpowerBP:minimumUserAge>
        <EmpowerBP:provideJournal rdf:datatype="http://www.w3.org/2001/XMLSchema#boolean">false</EmpowerBP:provideJournal>
        <EmpowerBP:provideLink rdf:datatype="http://www.w3.org/2001/XMLSchema#boolean">false</EmpowerBP:provideLink>
        <EmpowerBP:sourceURL rdf:datatype="http://www.w3.org/2001/XMLSchema#string">https://www.canada.ca/en/health-canada/services/tips-healthy-eating/time-saving-cooking-tips-healthy-meals.html</EmpowerBP:sourceURL>
        <rdfs:comment rdf:datatype="http://www.w3.org/2001/XMLSchema#string">Easy tip to save time in the kitchen:

• Invest in time-saving appliances. A slow cooker is a great way to come home to a warm meal. A hand blender can help you make quick and easy soups, sauces, and smoothies. Use a mini-chopper to dice up garlic and onions.</rdfs:comment>
        <rdfs:label rdf:datatype="http://www.w3.org/2001/XMLSchema#string">Time-Saving Kitchen Tips</rdfs:label>
    </owl:NamedIndividual>
    


    <!-- http://www.semanticweb.org/tswheeler/ontologies/2016/3/EmpowerBP#OT2 -->

    <owl:NamedIndividual rdf:about="http://www.semanticweb.org/tswheeler/ontologies/2016/3/EmpowerBP#OT2">
        <rdf:type rdf:resource="http://www.semanticweb.org/tswheeler/ontologies/2016/3/EmpowerBP#InterventionItem"/>
        <rdf:type rdf:resource="http://www.semanticweb.org/tswheeler/ontologies/2016/3/EmpowerBP#Tip"/>
        <EmpowerBP:isAppropriateForInterventionGoal rdf:resource="http://www.semanticweb.org/tswheeler/ontologies/2016/3/EmpowerBP#ExerciseMore"/>
        <EmpowerBP:isWarrantedBy rdf:resource="http://purl.bioontology.org/ontology/BCTT#Social_support_(practical)"/>
        <EmpowerBP:appropriateForAutomaticMotivation rdf:datatype="http://www.w3.org/2001/XMLSchema#integer">6</EmpowerBP:appropriateForAutomaticMotivation>
        <EmpowerBP:appropriateForLocation rdf:datatype="http://www.w3.org/2001/XMLSchema#integer">0</EmpowerBP:appropriateForLocation>
        <EmpowerBP:appropriateForPhysicalCapability rdf:datatype="http://www.w3.org/2001/XMLSchema#integer">3</EmpowerBP:appropriateForPhysicalCapability>
        <EmpowerBP:appropriateForPhysicalOpportunity rdf:datatype="http://www.w3.org/2001/XMLSchema#integer">3</EmpowerBP:appropriateForPhysicalOpportunity>
        <EmpowerBP:appropriateForPsychologicalCapability rdf:datatype="http://www.w3.org/2001/XMLSchema#integer">3</EmpowerBP:appropriateForPsychologicalCapability>
        <EmpowerBP:appropriateForReflectiveMotivation rdf:datatype="http://www.w3.org/2001/XMLSchema#integer">6</EmpowerBP:appropriateForReflectiveMotivation>
        <EmpowerBP:appropriateForSocialOpportunity rdf:datatype="http://www.w3.org/2001/XMLSchema#integer">3</EmpowerBP:appropriateForSocialOpportunity>
        <EmpowerBP:canRepeat rdf:datatype="http://www.w3.org/2001/XMLSchema#integer">26</EmpowerBP:canRepeat>
        <EmpowerBP:itemName rdf:datatype="http://www.w3.org/2001/XMLSchema#string">WalkaboutNS Time Tip</EmpowerBP:itemName>
        <EmpowerBP:itemText rdf:datatype="http://www.w3.org/2001/XMLSchema#string">Can&apos;t find time becasue you&apos;re too busy with your family? 

Make walking a family affair. Instead of carpooling, take turns walking your kids to school. Go for a family walk. Walk around the soccer field while the kids are playing. Make plans to incorporate walking into your everyday family activities.</EmpowerBP:itemText>
        <EmpowerBP:maximumUserAge rdf:datatype="http://www.w3.org/2001/XMLSchema#integer">120</EmpowerBP:maximumUserAge>
        <EmpowerBP:minimumUserAge rdf:datatype="http://www.w3.org/2001/XMLSchema#integer">18</EmpowerBP:minimumUserAge>
        <EmpowerBP:provideJournal rdf:datatype="http://www.w3.org/2001/XMLSchema#boolean">false</EmpowerBP:provideJournal>
        <EmpowerBP:provideLink rdf:datatype="http://www.w3.org/2001/XMLSchema#boolean">false</EmpowerBP:provideLink>
        <EmpowerBP:sourceURL rdf:datatype="http://www.w3.org/2001/XMLSchema#string">http://walkaboutns.ca/walkabout-info/inspiration/getting-over-barriers/</EmpowerBP:sourceURL>
        <rdfs:comment rdf:datatype="http://www.w3.org/2001/XMLSchema#string">Can&apos;t find time becasue you&apos;re too busy with your family? 

Make walking a family affair. Instead of carpooling, take turns walking your kids to school. Go for a family walk. Walk around the soccer field while the kids are playing. Make plans to incorporate walking into your everyday family activities.</rdfs:comment>
        <rdfs:label rdf:datatype="http://www.w3.org/2001/XMLSchema#string">WalkaboutNS Time Tip</rdfs:label>
    </owl:NamedIndividual>
    


    <!-- http://www.semanticweb.org/tswheeler/ontologies/2016/3/EmpowerBP#OT20 -->

    <owl:NamedIndividual rdf:about="http://www.semanticweb.org/tswheeler/ontologies/2016/3/EmpowerBP#OT20">
        <rdf:type rdf:resource="http://www.semanticweb.org/tswheeler/ontologies/2016/3/EmpowerBP#InterventionItem"/>
        <rdf:type rdf:resource="http://www.semanticweb.org/tswheeler/ontologies/2016/3/EmpowerBP#Tip"/>
        <EmpowerBP:isAppropriateForInterventionGoal rdf:resource="http://www.semanticweb.org/tswheeler/ontologies/2016/3/EmpowerBP#ReduceSaltIntake"/>
        <EmpowerBP:isWarrantedBy rdf:resource="http://purl.bioontology.org/ontology/BCTT#Restructuring_the_social_environment"/>
        <EmpowerBP:appropriateForAutomaticMotivation rdf:datatype="http://www.w3.org/2001/XMLSchema#integer">3</EmpowerBP:appropriateForAutomaticMotivation>
        <EmpowerBP:appropriateForLocation rdf:datatype="http://www.w3.org/2001/XMLSchema#integer">0</EmpowerBP:appropriateForLocation>
        <EmpowerBP:appropriateForPhysicalCapability rdf:datatype="http://www.w3.org/2001/XMLSchema#integer">3</EmpowerBP:appropriateForPhysicalCapability>
        <EmpowerBP:appropriateForPhysicalOpportunity rdf:datatype="http://www.w3.org/2001/XMLSchema#integer">3</EmpowerBP:appropriateForPhysicalOpportunity>
        <EmpowerBP:appropriateForPsychologicalCapability rdf:datatype="http://www.w3.org/2001/XMLSchema#integer">3</EmpowerBP:appropriateForPsychologicalCapability>
        <EmpowerBP:appropriateForReflectiveMotivation rdf:datatype="http://www.w3.org/2001/XMLSchema#integer">3</EmpowerBP:appropriateForReflectiveMotivation>
        <EmpowerBP:appropriateForSocialOpportunity rdf:datatype="http://www.w3.org/2001/XMLSchema#integer">3</EmpowerBP:appropriateForSocialOpportunity>
        <EmpowerBP:canRepeat rdf:datatype="http://www.w3.org/2001/XMLSchema#integer">26</EmpowerBP:canRepeat>
        <EmpowerBP:itemName rdf:datatype="http://www.w3.org/2001/XMLSchema#string">Time-Saving Kitchen Tip</EmpowerBP:itemName>
        <EmpowerBP:itemText rdf:datatype="http://www.w3.org/2001/XMLSchema#string">Ask the kids to help in the kitchen! By involving children in preparing food, they&apos;ll appreciate meals more and learn important life skills. Depending on their age, kids can wash and peel vegetables, tear up lettuce, mash potatoes, wash and cut fruit, drain and rinse canned beans or lentils, and stir a pot.</EmpowerBP:itemText>
        <EmpowerBP:maximumUserAge rdf:datatype="http://www.w3.org/2001/XMLSchema#integer">120</EmpowerBP:maximumUserAge>
        <EmpowerBP:minimumUserAge rdf:datatype="http://www.w3.org/2001/XMLSchema#integer">18</EmpowerBP:minimumUserAge>
        <EmpowerBP:provideJournal rdf:datatype="http://www.w3.org/2001/XMLSchema#boolean">false</EmpowerBP:provideJournal>
        <EmpowerBP:provideLink rdf:datatype="http://www.w3.org/2001/XMLSchema#boolean">false</EmpowerBP:provideLink>
        <EmpowerBP:sourceURL rdf:datatype="http://www.w3.org/2001/XMLSchema#string">https://www.canada.ca/en/health-canada/services/tips-healthy-eating/time-saving-cooking-tips-healthy-meals.html</EmpowerBP:sourceURL>
        <rdfs:comment rdf:datatype="http://www.w3.org/2001/XMLSchema#string">Ask the kids to help in the kitchen! By involving children in preparing food, they&apos;ll appreciate meals more and learn important life skills. Depending on their age, kids can wash and peel vegetables, tear up lettuce, mash potatoes, wash and cut fruit, drain and rinse canned beans or lentils, and stir a pot.</rdfs:comment>
        <rdfs:label rdf:datatype="http://www.w3.org/2001/XMLSchema#string">Time-Saving Kitchen Tip</rdfs:label>
    </owl:NamedIndividual>
    


    <!-- http://www.semanticweb.org/tswheeler/ontologies/2016/3/EmpowerBP#OT21 -->

    <owl:NamedIndividual rdf:about="http://www.semanticweb.org/tswheeler/ontologies/2016/3/EmpowerBP#OT21">
        <rdf:type rdf:resource="http://www.semanticweb.org/tswheeler/ontologies/2016/3/EmpowerBP#InterventionItem"/>
        <rdf:type rdf:resource="http://www.semanticweb.org/tswheeler/ontologies/2016/3/EmpowerBP#Tip"/>
        <EmpowerBP:isAppropriateForInterventionGoal rdf:resource="http://www.semanticweb.org/tswheeler/ontologies/2016/3/EmpowerBP#ReduceSaltIntake"/>
        <EmpowerBP:isWarrantedBy rdf:resource="http://purl.bioontology.org/ontology/BCTT#Instruction_on_how_to_perform_the_behavior"/>
        <EmpowerBP:appropriateForAutomaticMotivation rdf:datatype="http://www.w3.org/2001/XMLSchema#integer">6</EmpowerBP:appropriateForAutomaticMotivation>
        <EmpowerBP:appropriateForLocation rdf:datatype="http://www.w3.org/2001/XMLSchema#integer">0</EmpowerBP:appropriateForLocation>
        <EmpowerBP:appropriateForPhysicalCapability rdf:datatype="http://www.w3.org/2001/XMLSchema#integer">3</EmpowerBP:appropriateForPhysicalCapability>
        <EmpowerBP:appropriateForPhysicalOpportunity rdf:datatype="http://www.w3.org/2001/XMLSchema#integer">3</EmpowerBP:appropriateForPhysicalOpportunity>
        <EmpowerBP:appropriateForPsychologicalCapability rdf:datatype="http://www.w3.org/2001/XMLSchema#integer">3</EmpowerBP:appropriateForPsychologicalCapability>
        <EmpowerBP:appropriateForReflectiveMotivation rdf:datatype="http://www.w3.org/2001/XMLSchema#integer">6</EmpowerBP:appropriateForReflectiveMotivation>
        <EmpowerBP:appropriateForSocialOpportunity rdf:datatype="http://www.w3.org/2001/XMLSchema#integer">3</EmpowerBP:appropriateForSocialOpportunity>
        <EmpowerBP:canRepeat rdf:datatype="http://www.w3.org/2001/XMLSchema#integer">26</EmpowerBP:canRepeat>
        <EmpowerBP:itemName rdf:datatype="http://www.w3.org/2001/XMLSchema#string">Using Leftovers</EmpowerBP:itemName>
        <EmpowerBP:itemText rdf:datatype="http://www.w3.org/2001/XMLSchema#string">Tired of eating the same meal twice? Get creative with these tips to transform leftovers into a whole new meal.

Salmon:
• Add salmon to a salad or sandwich for a quick lunch.
• Add chunks of salmon to homemade macaroni and cheese.
• Mash to make salmon cakes.
Roast chicken:
• Shred chicken for quick quesadillas.
• Make your own chicken noodle soup with whole grain noodles, lower-sodium broth, and frozen peas and carrots.
• Add chicken to a wholesome white bean chili.
Chili:
• Stuff peppers with chilli and bake.
• Use as a topping for baked sweet potatoes.
• Toss with whole grain pasta for a super speedy meal.</EmpowerBP:itemText>
        <EmpowerBP:maximumUserAge rdf:datatype="http://www.w3.org/2001/XMLSchema#integer">120</EmpowerBP:maximumUserAge>
        <EmpowerBP:minimumUserAge rdf:datatype="http://www.w3.org/2001/XMLSchema#integer">18</EmpowerBP:minimumUserAge>
        <EmpowerBP:provideJournal rdf:datatype="http://www.w3.org/2001/XMLSchema#boolean">false</EmpowerBP:provideJournal>
        <EmpowerBP:provideLink rdf:datatype="http://www.w3.org/2001/XMLSchema#boolean">false</EmpowerBP:provideLink>
        <EmpowerBP:sourceURL rdf:datatype="http://www.w3.org/2001/XMLSchema#string">https://www.canada.ca/en/health-canada/services/tips-healthy-eating/time-saving-cooking-tips-healthy-meals.html</EmpowerBP:sourceURL>
        <rdfs:comment rdf:datatype="http://www.w3.org/2001/XMLSchema#string">Tired of eating the same meal twice? Get creative with these tips to transform leftovers into a whole new meal.

Salmon:
• Add salmon to a salad or sandwich for a quick lunch.
• Add chunks of salmon to homemade macaroni and cheese.
• Mash to make salmon cakes.
Roast chicken:
• Shred chicken for quick quesadillas.
• Make your own chicken noodle soup with whole grain noodles, lower-sodium broth, and frozen peas and carrots.
• Add chicken to a wholesome white bean chili.
Chili:
• Stuff peppers with chilli and bake.
• Use as a topping for baked sweet potatoes.
• Toss with whole grain pasta for a super speedy meal.</rdfs:comment>
        <rdfs:label rdf:datatype="http://www.w3.org/2001/XMLSchema#string">Using Leftovers</rdfs:label>
    </owl:NamedIndividual>
    


    <!-- http://www.semanticweb.org/tswheeler/ontologies/2016/3/EmpowerBP#OT22 -->

    <owl:NamedIndividual rdf:about="http://www.semanticweb.org/tswheeler/ontologies/2016/3/EmpowerBP#OT22">
        <rdf:type rdf:resource="http://www.semanticweb.org/tswheeler/ontologies/2016/3/EmpowerBP#InterventionItem"/>
        <rdf:type rdf:resource="http://www.semanticweb.org/tswheeler/ontologies/2016/3/EmpowerBP#Tip"/>
        <EmpowerBP:isAppropriateForInterventionGoal rdf:resource="http://www.semanticweb.org/tswheeler/ontologies/2016/3/EmpowerBP#ReduceSaltIntake"/>
        <EmpowerBP:isWarrantedBy rdf:resource="http://purl.bioontology.org/ontology/BCTT#Instruction_on_how_to_perform_the_behavior"/>
        <EmpowerBP:appropriateForAutomaticMotivation rdf:datatype="http://www.w3.org/2001/XMLSchema#integer">6</EmpowerBP:appropriateForAutomaticMotivation>
        <EmpowerBP:appropriateForLocation rdf:datatype="http://www.w3.org/2001/XMLSchema#integer">0</EmpowerBP:appropriateForLocation>
        <EmpowerBP:appropriateForPhysicalCapability rdf:datatype="http://www.w3.org/2001/XMLSchema#integer">3</EmpowerBP:appropriateForPhysicalCapability>
        <EmpowerBP:appropriateForPhysicalOpportunity rdf:datatype="http://www.w3.org/2001/XMLSchema#integer">3</EmpowerBP:appropriateForPhysicalOpportunity>
        <EmpowerBP:appropriateForPsychologicalCapability rdf:datatype="http://www.w3.org/2001/XMLSchema#integer">3</EmpowerBP:appropriateForPsychologicalCapability>
        <EmpowerBP:appropriateForReflectiveMotivation rdf:datatype="http://www.w3.org/2001/XMLSchema#integer">6</EmpowerBP:appropriateForReflectiveMotivation>
        <EmpowerBP:appropriateForSocialOpportunity rdf:datatype="http://www.w3.org/2001/XMLSchema#integer">3</EmpowerBP:appropriateForSocialOpportunity>
        <EmpowerBP:canRepeat rdf:datatype="http://www.w3.org/2001/XMLSchema#integer">26</EmpowerBP:canRepeat>
        <EmpowerBP:itemName rdf:datatype="http://www.w3.org/2001/XMLSchema#string">Using Leftovers</EmpowerBP:itemName>
        <EmpowerBP:itemText rdf:datatype="http://www.w3.org/2001/XMLSchema#string">Tired of eating the same meal twice? Get creative with these tips to transform leftovers into a whole new meal.

Pork tenderloin:
• Use in tacos or grilled sandwiches.
• Cook with lower sodium tomato sauce and frozen vegetables and serve over rice.
Cooked vegetables:
• Whip up leftover vegetables in an omelette.
• Add to a pasta dish.
• Top a whole-grain pizza.
Chickpeas:
• Stuff a whole wheat pita pocket.
• Serve over baby spinach.
• Mix with whole grain couscous.</EmpowerBP:itemText>
        <EmpowerBP:maximumUserAge rdf:datatype="http://www.w3.org/2001/XMLSchema#integer">120</EmpowerBP:maximumUserAge>
        <EmpowerBP:minimumUserAge rdf:datatype="http://www.w3.org/2001/XMLSchema#integer">18</EmpowerBP:minimumUserAge>
        <EmpowerBP:provideJournal rdf:datatype="http://www.w3.org/2001/XMLSchema#boolean">false</EmpowerBP:provideJournal>
        <EmpowerBP:provideLink rdf:datatype="http://www.w3.org/2001/XMLSchema#boolean">false</EmpowerBP:provideLink>
        <EmpowerBP:sourceURL rdf:datatype="http://www.w3.org/2001/XMLSchema#string">https://www.canada.ca/en/health-canada/services/tips-healthy-eating/time-saving-cooking-tips-healthy-meals.html</EmpowerBP:sourceURL>
        <rdfs:comment rdf:datatype="http://www.w3.org/2001/XMLSchema#string">Tired of eating the same meal twice? Get creative with these tips to transform leftovers into a whole new meal.

Pork tenderloin:
• Use in tacos or grilled sandwiches.
• Cook with lower sodium tomato sauce and frozen vegetables and serve over rice.
Cooked vegetables:
• Whip up leftover vegetables in an omelette.
• Add to a pasta dish.
• Top a whole-grain pizza.
Chickpeas:
• Stuff a whole wheat pita pocket.
• Serve over baby spinach.
• Mix with whole grain couscous.</rdfs:comment>
        <rdfs:label rdf:datatype="http://www.w3.org/2001/XMLSchema#string">Using Leftovers</rdfs:label>
    </owl:NamedIndividual>
    


    <!-- http://www.semanticweb.org/tswheeler/ontologies/2016/3/EmpowerBP#OT23 -->

    <owl:NamedIndividual rdf:about="http://www.semanticweb.org/tswheeler/ontologies/2016/3/EmpowerBP#OT23">
        <rdf:type rdf:resource="http://www.semanticweb.org/tswheeler/ontologies/2016/3/EmpowerBP#InterventionItem"/>
        <rdf:type rdf:resource="http://www.semanticweb.org/tswheeler/ontologies/2016/3/EmpowerBP#Tip"/>
        <EmpowerBP:isAppropriateForInterventionGoal rdf:resource="http://www.semanticweb.org/tswheeler/ontologies/2016/3/EmpowerBP#ReduceSaltIntake"/>
        <EmpowerBP:isWarrantedBy rdf:resource="http://purl.bioontology.org/ontology/BCTT#Instruction_on_how_to_perform_the_behavior"/>
        <EmpowerBP:appropriateForAutomaticMotivation rdf:datatype="http://www.w3.org/2001/XMLSchema#integer">6</EmpowerBP:appropriateForAutomaticMotivation>
        <EmpowerBP:appropriateForLocation rdf:datatype="http://www.w3.org/2001/XMLSchema#integer">0</EmpowerBP:appropriateForLocation>
        <EmpowerBP:appropriateForPhysicalCapability rdf:datatype="http://www.w3.org/2001/XMLSchema#integer">3</EmpowerBP:appropriateForPhysicalCapability>
        <EmpowerBP:appropriateForPhysicalOpportunity rdf:datatype="http://www.w3.org/2001/XMLSchema#integer">3</EmpowerBP:appropriateForPhysicalOpportunity>
        <EmpowerBP:appropriateForPsychologicalCapability rdf:datatype="http://www.w3.org/2001/XMLSchema#integer">3</EmpowerBP:appropriateForPsychologicalCapability>
        <EmpowerBP:appropriateForReflectiveMotivation rdf:datatype="http://www.w3.org/2001/XMLSchema#integer">6</EmpowerBP:appropriateForReflectiveMotivation>
        <EmpowerBP:appropriateForSocialOpportunity rdf:datatype="http://www.w3.org/2001/XMLSchema#integer">3</EmpowerBP:appropriateForSocialOpportunity>
        <EmpowerBP:canRepeat rdf:datatype="http://www.w3.org/2001/XMLSchema#integer">26</EmpowerBP:canRepeat>
        <EmpowerBP:itemName rdf:datatype="http://www.w3.org/2001/XMLSchema#string">Using Leftovers</EmpowerBP:itemName>
        <EmpowerBP:itemText rdf:datatype="http://www.w3.org/2001/XMLSchema#string">Tired of eating the same meal twice? Get creative with these tips to transform leftovers into a whole new meal.

Cooked brown rice:
• Make a quick stir-fry with frozen vegetables.
• Add to soups and stews.
• Toss together a rice and lentil salad.
Stir-fry:
• Roll up leftover stir-fry in a whole wheat wrap.
• Add stir-fry vegetables and tofu to soup.</EmpowerBP:itemText>
        <EmpowerBP:maximumUserAge rdf:datatype="http://www.w3.org/2001/XMLSchema#integer">120</EmpowerBP:maximumUserAge>
        <EmpowerBP:minimumUserAge rdf:datatype="http://www.w3.org/2001/XMLSchema#integer">18</EmpowerBP:minimumUserAge>
        <EmpowerBP:provideJournal rdf:datatype="http://www.w3.org/2001/XMLSchema#boolean">false</EmpowerBP:provideJournal>
        <EmpowerBP:provideLink rdf:datatype="http://www.w3.org/2001/XMLSchema#boolean">false</EmpowerBP:provideLink>
        <EmpowerBP:sourceURL rdf:datatype="http://www.w3.org/2001/XMLSchema#string">https://www.canada.ca/en/health-canada/services/tips-healthy-eating/time-saving-cooking-tips-healthy-meals.html</EmpowerBP:sourceURL>
        <rdfs:comment rdf:datatype="http://www.w3.org/2001/XMLSchema#string">Tired of eating the same meal twice? Get creative with these tips to transform leftovers into a whole new meal.

Cooked brown rice:
• Make a quick stir-fry with frozen vegetables.
• Add to soups and stews.
• Toss together a rice and lentil salad.
Stir-fry:
• Roll up leftover stir-fry in a whole wheat wrap.
• Add stir-fry vegetables and tofu to soup.</rdfs:comment>
        <rdfs:label rdf:datatype="http://www.w3.org/2001/XMLSchema#string">Using Leftovers</rdfs:label>
    </owl:NamedIndividual>
    


    <!-- http://www.semanticweb.org/tswheeler/ontologies/2016/3/EmpowerBP#OT24 -->

    <owl:NamedIndividual rdf:about="http://www.semanticweb.org/tswheeler/ontologies/2016/3/EmpowerBP#OT24">
        <rdf:type rdf:resource="http://www.semanticweb.org/tswheeler/ontologies/2016/3/EmpowerBP#InterventionItem"/>
        <rdf:type rdf:resource="http://www.semanticweb.org/tswheeler/ontologies/2016/3/EmpowerBP#Tip"/>
        <EmpowerBP:isAppropriateForInterventionGoal rdf:resource="http://www.semanticweb.org/tswheeler/ontologies/2016/3/EmpowerBP#ReduceSaltIntake"/>
        <EmpowerBP:isWarrantedBy rdf:resource="http://purl.bioontology.org/ontology/BCTT#Behavior_substitution"/>
        <EmpowerBP:appropriateForAutomaticMotivation rdf:datatype="http://www.w3.org/2001/XMLSchema#integer">3</EmpowerBP:appropriateForAutomaticMotivation>
        <EmpowerBP:appropriateForLocation rdf:datatype="http://www.w3.org/2001/XMLSchema#integer">0</EmpowerBP:appropriateForLocation>
        <EmpowerBP:appropriateForPhysicalCapability rdf:datatype="http://www.w3.org/2001/XMLSchema#integer">3</EmpowerBP:appropriateForPhysicalCapability>
        <EmpowerBP:appropriateForPhysicalOpportunity rdf:datatype="http://www.w3.org/2001/XMLSchema#integer">3</EmpowerBP:appropriateForPhysicalOpportunity>
        <EmpowerBP:appropriateForPsychologicalCapability rdf:datatype="http://www.w3.org/2001/XMLSchema#integer">3</EmpowerBP:appropriateForPsychologicalCapability>
        <EmpowerBP:appropriateForReflectiveMotivation rdf:datatype="http://www.w3.org/2001/XMLSchema#integer">3</EmpowerBP:appropriateForReflectiveMotivation>
        <EmpowerBP:appropriateForSocialOpportunity rdf:datatype="http://www.w3.org/2001/XMLSchema#integer">3</EmpowerBP:appropriateForSocialOpportunity>
        <EmpowerBP:canRepeat rdf:datatype="http://www.w3.org/2001/XMLSchema#integer">26</EmpowerBP:canRepeat>
        <EmpowerBP:itemName rdf:datatype="http://www.w3.org/2001/XMLSchema#string">Herbs and Spices</EmpowerBP:itemName>
        <EmpowerBP:itemText rdf:datatype="http://www.w3.org/2001/XMLSchema#string">Cooking with herbs and spices instead of salt
Flavour foods with herbs and spices instead of salt. Your taste buds will adjust to less salt in your food. Here are a few ideas to get you started:

• Basil - tastes great with tomatoes and pasta
• Cumin - adds flavour to soup, stews, and sauces
• Curry  powder - good with meat, poultry, soup, and stews
• Dill - pairs well with fish, potatoes, and eggs
• Oregano - perfect in pasta, soup, and salads
• Paprika - good with seafood, vegetables, chicken, and eggs
• Rosemary - delicious with chicken, lamb, and pork
• Thyme - goes well with beef and chicken</EmpowerBP:itemText>
        <EmpowerBP:maximumUserAge rdf:datatype="http://www.w3.org/2001/XMLSchema#integer">120</EmpowerBP:maximumUserAge>
        <EmpowerBP:minimumUserAge rdf:datatype="http://www.w3.org/2001/XMLSchema#integer">18</EmpowerBP:minimumUserAge>
        <EmpowerBP:provideJournal rdf:datatype="http://www.w3.org/2001/XMLSchema#boolean">false</EmpowerBP:provideJournal>
        <EmpowerBP:provideLink rdf:datatype="http://www.w3.org/2001/XMLSchema#boolean">false</EmpowerBP:provideLink>
        <EmpowerBP:sourceURL rdf:datatype="http://www.w3.org/2001/XMLSchema#string">https://www.canada.ca/en/health-canada/services/nutrients/sodium/reducing-sodium-home.html</EmpowerBP:sourceURL>
        <rdfs:comment rdf:datatype="http://www.w3.org/2001/XMLSchema#string">Cooking with herbs and spices instead of salt
Flavour foods with herbs and spices instead of salt. Your taste buds will adjust to less salt in your food. Here are a few ideas to get you started:

• Basil - tastes great with tomatoes and pasta
• Cumin - adds flavour to soup, stews, and sauces
• Curry  powder - good with meat, poultry, soup, and stews
• Dill - pairs well with fish, potatoes, and eggs
• Oregano - perfect in pasta, soup, and salads
• Paprika - good with seafood, vegetables, chicken, and eggs
• Rosemary - delicious with chicken, lamb, and pork
• Thyme - goes well with beef and chicken</rdfs:comment>
        <rdfs:label rdf:datatype="http://www.w3.org/2001/XMLSchema#string">Herbs and Spices</rdfs:label>
    </owl:NamedIndividual>
    


    <!-- http://www.semanticweb.org/tswheeler/ontologies/2016/3/EmpowerBP#OT25 -->

    <owl:NamedIndividual rdf:about="http://www.semanticweb.org/tswheeler/ontologies/2016/3/EmpowerBP#OT25">
        <rdf:type rdf:resource="http://www.semanticweb.org/tswheeler/ontologies/2016/3/EmpowerBP#InterventionItem"/>
        <rdf:type rdf:resource="http://www.semanticweb.org/tswheeler/ontologies/2016/3/EmpowerBP#Tip"/>
        <EmpowerBP:isAppropriateForInterventionGoal rdf:resource="http://www.semanticweb.org/tswheeler/ontologies/2016/3/EmpowerBP#ReduceSaltIntake"/>
        <EmpowerBP:isWarrantedBy rdf:resource="http://purl.bioontology.org/ontology/BCTT#Restructuring_the_social_environment"/>
        <EmpowerBP:appropriateForAutomaticMotivation rdf:datatype="http://www.w3.org/2001/XMLSchema#integer">3</EmpowerBP:appropriateForAutomaticMotivation>
        <EmpowerBP:appropriateForLocation rdf:datatype="http://www.w3.org/2001/XMLSchema#integer">0</EmpowerBP:appropriateForLocation>
        <EmpowerBP:appropriateForPhysicalCapability rdf:datatype="http://www.w3.org/2001/XMLSchema#integer">3</EmpowerBP:appropriateForPhysicalCapability>
        <EmpowerBP:appropriateForPhysicalOpportunity rdf:datatype="http://www.w3.org/2001/XMLSchema#integer">3</EmpowerBP:appropriateForPhysicalOpportunity>
        <EmpowerBP:appropriateForPsychologicalCapability rdf:datatype="http://www.w3.org/2001/XMLSchema#integer">3</EmpowerBP:appropriateForPsychologicalCapability>
        <EmpowerBP:appropriateForReflectiveMotivation rdf:datatype="http://www.w3.org/2001/XMLSchema#integer">3</EmpowerBP:appropriateForReflectiveMotivation>
        <EmpowerBP:appropriateForSocialOpportunity rdf:datatype="http://www.w3.org/2001/XMLSchema#integer">3</EmpowerBP:appropriateForSocialOpportunity>
        <EmpowerBP:canRepeat rdf:datatype="http://www.w3.org/2001/XMLSchema#integer">26</EmpowerBP:canRepeat>
        <EmpowerBP:itemName rdf:datatype="http://www.w3.org/2001/XMLSchema#string">Help from Friends and Family</EmpowerBP:itemName>
        <EmpowerBP:itemText rdf:datatype="http://www.w3.org/2001/XMLSchema#string">Reducing the sodium in your diet is a good idea for everyone! Get your whole household to help plan and create healthy, low-sodium meals. Challenge your friends to make healthy choices too, and share any recipes or tips you may find! </EmpowerBP:itemText>
        <EmpowerBP:maximumUserAge rdf:datatype="http://www.w3.org/2001/XMLSchema#integer">120</EmpowerBP:maximumUserAge>
        <EmpowerBP:minimumUserAge rdf:datatype="http://www.w3.org/2001/XMLSchema#integer">18</EmpowerBP:minimumUserAge>
        <EmpowerBP:provideJournal rdf:datatype="http://www.w3.org/2001/XMLSchema#boolean">false</EmpowerBP:provideJournal>
        <EmpowerBP:provideLink rdf:datatype="http://www.w3.org/2001/XMLSchema#boolean">false</EmpowerBP:provideLink>
        <EmpowerBP:sourceURL rdf:datatype="http://www.w3.org/2001/XMLSchema#string">https://www.canada.ca/en/health-canada/services/tips-healthy-eating/meal-planning-basics.html</EmpowerBP:sourceURL>
        <rdfs:comment rdf:datatype="http://www.w3.org/2001/XMLSchema#string">Reducing the sodium in your diet is a good idea for everyone! Get your whole household to help plan and create healthy, low-sodium meals. Challenge your friends to make healthy choices too, and share any recipes or tips you may find! </rdfs:comment>
        <rdfs:label rdf:datatype="http://www.w3.org/2001/XMLSchema#string">Help from Friends and Family</rdfs:label>
    </owl:NamedIndividual>
    


    <!-- http://www.semanticweb.org/tswheeler/ontologies/2016/3/EmpowerBP#OT26 -->

    <owl:NamedIndividual rdf:about="http://www.semanticweb.org/tswheeler/ontologies/2016/3/EmpowerBP#OT26">
        <rdf:type rdf:resource="http://www.semanticweb.org/tswheeler/ontologies/2016/3/EmpowerBP#InterventionItem"/>
        <rdf:type rdf:resource="http://www.semanticweb.org/tswheeler/ontologies/2016/3/EmpowerBP#Tip"/>
        <EmpowerBP:isAppropriateForInterventionGoal rdf:resource="http://www.semanticweb.org/tswheeler/ontologies/2016/3/EmpowerBP#ReduceSaltIntake"/>
        <EmpowerBP:isWarrantedBy rdf:resource="http://purl.bioontology.org/ontology/BCTT#Instruction_on_how_to_perform_the_behavior"/>
        <EmpowerBP:appropriateForAutomaticMotivation rdf:datatype="http://www.w3.org/2001/XMLSchema#integer">6</EmpowerBP:appropriateForAutomaticMotivation>
        <EmpowerBP:appropriateForLocation rdf:datatype="http://www.w3.org/2001/XMLSchema#integer">0</EmpowerBP:appropriateForLocation>
        <EmpowerBP:appropriateForPhysicalCapability rdf:datatype="http://www.w3.org/2001/XMLSchema#integer">3</EmpowerBP:appropriateForPhysicalCapability>
        <EmpowerBP:appropriateForPhysicalOpportunity rdf:datatype="http://www.w3.org/2001/XMLSchema#integer">3</EmpowerBP:appropriateForPhysicalOpportunity>
        <EmpowerBP:appropriateForPsychologicalCapability rdf:datatype="http://www.w3.org/2001/XMLSchema#integer">3</EmpowerBP:appropriateForPsychologicalCapability>
        <EmpowerBP:appropriateForReflectiveMotivation rdf:datatype="http://www.w3.org/2001/XMLSchema#integer">6</EmpowerBP:appropriateForReflectiveMotivation>
        <EmpowerBP:appropriateForSocialOpportunity rdf:datatype="http://www.w3.org/2001/XMLSchema#integer">3</EmpowerBP:appropriateForSocialOpportunity>
        <EmpowerBP:canRepeat rdf:datatype="http://www.w3.org/2001/XMLSchema#integer">26</EmpowerBP:canRepeat>
        <EmpowerBP:itemName rdf:datatype="http://www.w3.org/2001/XMLSchema#string">Five Simple Meal Planning Tips</EmpowerBP:itemName>
        <EmpowerBP:itemText rdf:datatype="http://www.w3.org/2001/XMLSchema#string">There&apos;s no right or wrong way to plan meals. Some people like to plan for the whole week ahead, while others plan for a couple of days. Do what works for you. Write down your meal and snack ideas on paper or use your Smartphone.

Use these tips to help with your planning:

• Follow Canada&apos;s Food Guide when planning what to eat. Look in your fridge, freezer, and pantry to see what foods you have on hand and what you need to buy.
• Keep a grocery list and jot down items as you run out of them. Add foods based on your meal plan.
• Encourage healthy habits by getting your children involved. Ask them to choose a favourite meal. Encourage your family to try a new food or recipe every now and then.
• Flip through grocery store flyers to take advantage of specials and use coupons to save money. Get healthy recipe ideas from magazines, cookbooks, and websites.
• Think about your family&apos;s schedule. A busy week filled with sports and other activities could mean planning fast and easy meals.</EmpowerBP:itemText>
        <EmpowerBP:maximumUserAge rdf:datatype="http://www.w3.org/2001/XMLSchema#integer">120</EmpowerBP:maximumUserAge>
        <EmpowerBP:minimumUserAge rdf:datatype="http://www.w3.org/2001/XMLSchema#integer">18</EmpowerBP:minimumUserAge>
        <EmpowerBP:provideJournal rdf:datatype="http://www.w3.org/2001/XMLSchema#boolean">false</EmpowerBP:provideJournal>
        <EmpowerBP:provideLink rdf:datatype="http://www.w3.org/2001/XMLSchema#boolean">false</EmpowerBP:provideLink>
        <EmpowerBP:sourceURL rdf:datatype="http://www.w3.org/2001/XMLSchema#string">https://www.canada.ca/en/health-canada/services/tips-healthy-eating/meal-planning-basics.html</EmpowerBP:sourceURL>
        <rdfs:comment rdf:datatype="http://www.w3.org/2001/XMLSchema#string">There&apos;s no right or wrong way to plan meals. Some people like to plan for the whole week ahead, while others plan for a couple of days. Do what works for you. Write down your meal and snack ideas on paper or use your Smartphone.

Use these tips to help with your planning:

• Follow Canada&apos;s Food Guide when planning what to eat. Look in your fridge, freezer, and pantry to see what foods you have on hand and what you need to buy.
• Keep a grocery list and jot down items as you run out of them. Add foods based on your meal plan.
• Encourage healthy habits by getting your children involved. Ask them to choose a favourite meal. Encourage your family to try a new food or recipe every now and then.
• Flip through grocery store flyers to take advantage of specials and use coupons to save money. Get healthy recipe ideas from magazines, cookbooks, and websites.
• Think about your family&apos;s schedule. A busy week filled with sports and other activities could mean planning fast and easy meals.</rdfs:comment>
        <rdfs:label rdf:datatype="http://www.w3.org/2001/XMLSchema#string">Five Simple Meal Planning Tips</rdfs:label>
    </owl:NamedIndividual>
    


    <!-- http://www.semanticweb.org/tswheeler/ontologies/2016/3/EmpowerBP#OT27 -->

    <owl:NamedIndividual rdf:about="http://www.semanticweb.org/tswheeler/ontologies/2016/3/EmpowerBP#OT27">
        <rdf:type rdf:resource="http://www.semanticweb.org/tswheeler/ontologies/2016/3/EmpowerBP#InterventionItem"/>
        <rdf:type rdf:resource="http://www.semanticweb.org/tswheeler/ontologies/2016/3/EmpowerBP#Tip"/>
        <EmpowerBP:isAppropriateForInterventionGoal rdf:resource="http://www.semanticweb.org/tswheeler/ontologies/2016/3/EmpowerBP#ReduceSaltIntake"/>
        <EmpowerBP:isWarrantedBy rdf:resource="http://purl.bioontology.org/ontology/BCTT#Instruction_on_how_to_perform_the_behavior"/>
        <EmpowerBP:appropriateForAutomaticMotivation rdf:datatype="http://www.w3.org/2001/XMLSchema#integer">3</EmpowerBP:appropriateForAutomaticMotivation>
        <EmpowerBP:appropriateForLocation rdf:datatype="http://www.w3.org/2001/XMLSchema#integer">0</EmpowerBP:appropriateForLocation>
        <EmpowerBP:appropriateForPhysicalCapability rdf:datatype="http://www.w3.org/2001/XMLSchema#integer">3</EmpowerBP:appropriateForPhysicalCapability>
        <EmpowerBP:appropriateForPhysicalOpportunity rdf:datatype="http://www.w3.org/2001/XMLSchema#integer">3</EmpowerBP:appropriateForPhysicalOpportunity>
        <EmpowerBP:appropriateForPsychologicalCapability rdf:datatype="http://www.w3.org/2001/XMLSchema#integer">3</EmpowerBP:appropriateForPsychologicalCapability>
        <EmpowerBP:appropriateForReflectiveMotivation rdf:datatype="http://www.w3.org/2001/XMLSchema#integer">3</EmpowerBP:appropriateForReflectiveMotivation>
        <EmpowerBP:appropriateForSocialOpportunity rdf:datatype="http://www.w3.org/2001/XMLSchema#integer">3</EmpowerBP:appropriateForSocialOpportunity>
        <EmpowerBP:canRepeat rdf:datatype="http://www.w3.org/2001/XMLSchema#integer">26</EmpowerBP:canRepeat>
        <EmpowerBP:itemName rdf:datatype="http://www.w3.org/2001/XMLSchema#string">Coupons and Healthy Eating</EmpowerBP:itemName>
        <EmpowerBP:itemText rdf:datatype="http://www.w3.org/2001/XMLSchema#string">It&apos;s possible to eat healthy for cheap!

Flip through grocery store flyers to take advantage of specials and use coupons to save money. Get healthy recipe ideas from magazines, cookbooks, and websites.</EmpowerBP:itemText>
        <EmpowerBP:maximumUserAge rdf:datatype="http://www.w3.org/2001/XMLSchema#integer">120</EmpowerBP:maximumUserAge>
        <EmpowerBP:minimumUserAge rdf:datatype="http://www.w3.org/2001/XMLSchema#integer">18</EmpowerBP:minimumUserAge>
        <EmpowerBP:provideJournal rdf:datatype="http://www.w3.org/2001/XMLSchema#boolean">false</EmpowerBP:provideJournal>
        <EmpowerBP:provideLink rdf:datatype="http://www.w3.org/2001/XMLSchema#boolean">false</EmpowerBP:provideLink>
        <EmpowerBP:sourceURL rdf:datatype="http://www.w3.org/2001/XMLSchema#string">https://www.canada.ca/en/health-canada/services/tips-healthy-eating/meal-planning-basics.html</EmpowerBP:sourceURL>
        <rdfs:comment rdf:datatype="http://www.w3.org/2001/XMLSchema#string">It&apos;s possible to eat healthy for cheap!

Flip through grocery store flyers to take advantage of specials and use coupons to save money. Get healthy recipe ideas from magazines, cookbooks, and websites.</rdfs:comment>
        <rdfs:label rdf:datatype="http://www.w3.org/2001/XMLSchema#string">Coupons and Healthy Eating</rdfs:label>
    </owl:NamedIndividual>
    


    <!-- http://www.semanticweb.org/tswheeler/ontologies/2016/3/EmpowerBP#OT28 -->

    <owl:NamedIndividual rdf:about="http://www.semanticweb.org/tswheeler/ontologies/2016/3/EmpowerBP#OT28">
        <rdf:type rdf:resource="http://www.semanticweb.org/tswheeler/ontologies/2016/3/EmpowerBP#InterventionItem"/>
        <rdf:type rdf:resource="http://www.semanticweb.org/tswheeler/ontologies/2016/3/EmpowerBP#Tip"/>
        <EmpowerBP:isAppropriateForInterventionGoal rdf:resource="http://www.semanticweb.org/tswheeler/ontologies/2016/3/EmpowerBP#ReduceSaltIntake"/>
        <EmpowerBP:isWarrantedBy rdf:resource="http://purl.bioontology.org/ontology/BCTT#Instruction_on_how_to_perform_the_behavior"/>
        <EmpowerBP:appropriateForAutomaticMotivation rdf:datatype="http://www.w3.org/2001/XMLSchema#integer">6</EmpowerBP:appropriateForAutomaticMotivation>
        <EmpowerBP:appropriateForLocation rdf:datatype="http://www.w3.org/2001/XMLSchema#integer">0</EmpowerBP:appropriateForLocation>
        <EmpowerBP:appropriateForPhysicalCapability rdf:datatype="http://www.w3.org/2001/XMLSchema#integer">3</EmpowerBP:appropriateForPhysicalCapability>
        <EmpowerBP:appropriateForPhysicalOpportunity rdf:datatype="http://www.w3.org/2001/XMLSchema#integer">3</EmpowerBP:appropriateForPhysicalOpportunity>
        <EmpowerBP:appropriateForPsychologicalCapability rdf:datatype="http://www.w3.org/2001/XMLSchema#integer">3</EmpowerBP:appropriateForPsychologicalCapability>
        <EmpowerBP:appropriateForReflectiveMotivation rdf:datatype="http://www.w3.org/2001/XMLSchema#integer">6</EmpowerBP:appropriateForReflectiveMotivation>
        <EmpowerBP:appropriateForSocialOpportunity rdf:datatype="http://www.w3.org/2001/XMLSchema#integer">3</EmpowerBP:appropriateForSocialOpportunity>
        <EmpowerBP:canRepeat rdf:datatype="http://www.w3.org/2001/XMLSchema#integer">26</EmpowerBP:canRepeat>
        <EmpowerBP:itemName rdf:datatype="http://www.w3.org/2001/XMLSchema#string">Ideas for planning snacks</EmpowerBP:itemName>
        <EmpowerBP:itemText rdf:datatype="http://www.w3.org/2001/XMLSchema#string">Snacks help keep your energy levels up between meals. Plan to have healthy snacks on hand so you can skip less healthy choices in vending machines or coffee shops.

• Chop extra vegetables when cooking so you&apos;ll have some for snacks. Try different dips with your veggies like hummus, tzatziki, fresh salsa, nut butters, and yogurt.
• Hard-boil eggs on the weekend. They will stay fresh in the fridge for up to one week with the shell on. Pair them with your favourite vegetable.
• Stock up on easy to grab snacks: apples, pears, bananas, plums, grapes, fruit cups (packed in fruit juice), yogurt, granola bars with at least 4 grams of fibre, unsalted nuts, and small cans of low-sodium vegetable juice.
</EmpowerBP:itemText>
        <EmpowerBP:maximumUserAge rdf:datatype="http://www.w3.org/2001/XMLSchema#integer">120</EmpowerBP:maximumUserAge>
        <EmpowerBP:minimumUserAge rdf:datatype="http://www.w3.org/2001/XMLSchema#integer">18</EmpowerBP:minimumUserAge>
        <EmpowerBP:provideJournal rdf:datatype="http://www.w3.org/2001/XMLSchema#boolean">false</EmpowerBP:provideJournal>
        <EmpowerBP:provideLink rdf:datatype="http://www.w3.org/2001/XMLSchema#boolean">false</EmpowerBP:provideLink>
        <EmpowerBP:sourceURL rdf:datatype="http://www.w3.org/2001/XMLSchema#string">https://www.canada.ca/en/health-canada/services/tips-healthy-eating/meal-planning-basics.html</EmpowerBP:sourceURL>
        <rdfs:comment rdf:datatype="http://www.w3.org/2001/XMLSchema#string">Snacks help keep your energy levels up between meals. Plan to have healthy snacks on hand so you can skip less healthy choices in vending machines or coffee shops.

• Chop extra vegetables when cooking so you&apos;ll have some for snacks. Try different dips with your veggies like hummus, tzatziki, fresh salsa, nut butters, and yogurt.
• Hard-boil eggs on the weekend. They will stay fresh in the fridge for up to one week with the shell on. Pair them with your favourite vegetable.
• Stock up on easy to grab snacks: apples, pears, bananas, plums, grapes, fruit cups (packed in fruit juice), yogurt, granola bars with at least 4 grams of fibre, unsalted nuts, and small cans of low-sodium vegetable juice.
</rdfs:comment>
        <rdfs:label rdf:datatype="http://www.w3.org/2001/XMLSchema#string">Ideas for planning snacks</rdfs:label>
    </owl:NamedIndividual>
    


    <!-- http://www.semanticweb.org/tswheeler/ontologies/2016/3/EmpowerBP#OT29 -->

    <owl:NamedIndividual rdf:about="http://www.semanticweb.org/tswheeler/ontologies/2016/3/EmpowerBP#OT29">
        <rdf:type rdf:resource="http://www.semanticweb.org/tswheeler/ontologies/2016/3/EmpowerBP#InterventionItem"/>
        <rdf:type rdf:resource="http://www.semanticweb.org/tswheeler/ontologies/2016/3/EmpowerBP#Tip"/>
        <EmpowerBP:isAppropriateForInterventionGoal rdf:resource="http://www.semanticweb.org/tswheeler/ontologies/2016/3/EmpowerBP#ExerciseMore"/>
        <EmpowerBP:isWarrantedBy rdf:resource="http://purl.bioontology.org/ontology/BCTT#Instruction_on_how_to_perform_the_behavior"/>
        <EmpowerBP:appropriateForAutomaticMotivation rdf:datatype="http://www.w3.org/2001/XMLSchema#integer">9</EmpowerBP:appropriateForAutomaticMotivation>
        <EmpowerBP:appropriateForLocation rdf:datatype="http://www.w3.org/2001/XMLSchema#integer">0</EmpowerBP:appropriateForLocation>
        <EmpowerBP:appropriateForPhysicalCapability rdf:datatype="http://www.w3.org/2001/XMLSchema#integer">6</EmpowerBP:appropriateForPhysicalCapability>
        <EmpowerBP:appropriateForPhysicalOpportunity rdf:datatype="http://www.w3.org/2001/XMLSchema#integer">6</EmpowerBP:appropriateForPhysicalOpportunity>
        <EmpowerBP:appropriateForPsychologicalCapability rdf:datatype="http://www.w3.org/2001/XMLSchema#integer">6</EmpowerBP:appropriateForPsychologicalCapability>
        <EmpowerBP:appropriateForReflectiveMotivation rdf:datatype="http://www.w3.org/2001/XMLSchema#integer">9</EmpowerBP:appropriateForReflectiveMotivation>
        <EmpowerBP:appropriateForSocialOpportunity rdf:datatype="http://www.w3.org/2001/XMLSchema#integer">6</EmpowerBP:appropriateForSocialOpportunity>
        <EmpowerBP:canRepeat rdf:datatype="http://www.w3.org/2001/XMLSchema#integer">26</EmpowerBP:canRepeat>
        <EmpowerBP:itemName rdf:datatype="http://www.w3.org/2001/XMLSchema#string">Playing it Safe</EmpowerBP:itemName>
        <EmpowerBP:itemText rdf:datatype="http://www.w3.org/2001/XMLSchema#string">When adding physical activity into your daily routine, begin with light activities and progress to moderate and vigorous activities later, if you like. This will prevent or minimize any muscle soreness you might experience when you are starting out.

• Use comfortable footwear that provides good cushioning and support
• Wear comfortable clothing that suits your activity – and the weather!
• Wear safety gear approved by the Canadian Standards Association (CSA) whenever appropriate (a helmet for cycling and in-line skating, along with knee, elbow, and wrist protectors; protective eye goggles for squash). </EmpowerBP:itemText>
        <EmpowerBP:maximumUserAge rdf:datatype="http://www.w3.org/2001/XMLSchema#integer">120</EmpowerBP:maximumUserAge>
        <EmpowerBP:minimumUserAge rdf:datatype="http://www.w3.org/2001/XMLSchema#integer">18</EmpowerBP:minimumUserAge>
        <EmpowerBP:provideJournal rdf:datatype="http://www.w3.org/2001/XMLSchema#boolean">false</EmpowerBP:provideJournal>
        <EmpowerBP:provideLink rdf:datatype="http://www.w3.org/2001/XMLSchema#boolean">false</EmpowerBP:provideLink>
        <EmpowerBP:sourceURL rdf:datatype="http://www.w3.org/2001/XMLSchema#string">http://www.physicalactivityplan.org/resources/CPAG.pdf</EmpowerBP:sourceURL>
        <rdfs:comment rdf:datatype="http://www.w3.org/2001/XMLSchema#string">When adding physical activity into your daily routine, begin with light activities and progress to moderate and vigorous activities later, if you like. This will prevent or minimize any muscle soreness you might experience when you are starting out.

• Use comfortable footwear that provides good cushioning and support
• Wear comfortable clothing that suits your activity – and the weather!
• Wear safety gear approved by the Canadian Standards Association (CSA) whenever appropriate (a helmet for cycling and in-line skating, along with knee, elbow, and wrist protectors; protective eye goggles for squash). </rdfs:comment>
        <rdfs:label rdf:datatype="http://www.w3.org/2001/XMLSchema#string">Playing it Safe</rdfs:label>
    </owl:NamedIndividual>
    


    <!-- http://www.semanticweb.org/tswheeler/ontologies/2016/3/EmpowerBP#OT3 -->

    <owl:NamedIndividual rdf:about="http://www.semanticweb.org/tswheeler/ontologies/2016/3/EmpowerBP#OT3">
        <rdf:type rdf:resource="http://www.semanticweb.org/tswheeler/ontologies/2016/3/EmpowerBP#InterventionItem"/>
        <rdf:type rdf:resource="http://www.semanticweb.org/tswheeler/ontologies/2016/3/EmpowerBP#Tip"/>
        <EmpowerBP:isAppropriateForInterventionGoal rdf:resource="http://www.semanticweb.org/tswheeler/ontologies/2016/3/EmpowerBP#ExerciseMore"/>
        <EmpowerBP:isWarrantedBy rdf:resource="http://purl.bioontology.org/ontology/BCTT#Imaginary_reward"/>
        <EmpowerBP:appropriateForAutomaticMotivation rdf:datatype="http://www.w3.org/2001/XMLSchema#integer">3</EmpowerBP:appropriateForAutomaticMotivation>
        <EmpowerBP:appropriateForLocation rdf:datatype="http://www.w3.org/2001/XMLSchema#integer">0</EmpowerBP:appropriateForLocation>
        <EmpowerBP:appropriateForPhysicalCapability rdf:datatype="http://www.w3.org/2001/XMLSchema#integer">3</EmpowerBP:appropriateForPhysicalCapability>
        <EmpowerBP:appropriateForPhysicalOpportunity rdf:datatype="http://www.w3.org/2001/XMLSchema#integer">3</EmpowerBP:appropriateForPhysicalOpportunity>
        <EmpowerBP:appropriateForPsychologicalCapability rdf:datatype="http://www.w3.org/2001/XMLSchema#integer">3</EmpowerBP:appropriateForPsychologicalCapability>
        <EmpowerBP:appropriateForReflectiveMotivation rdf:datatype="http://www.w3.org/2001/XMLSchema#integer">3</EmpowerBP:appropriateForReflectiveMotivation>
        <EmpowerBP:appropriateForSocialOpportunity rdf:datatype="http://www.w3.org/2001/XMLSchema#integer">3</EmpowerBP:appropriateForSocialOpportunity>
        <EmpowerBP:canRepeat rdf:datatype="http://www.w3.org/2001/XMLSchema#integer">26</EmpowerBP:canRepeat>
        <EmpowerBP:itemName rdf:datatype="http://www.w3.org/2001/XMLSchema#string">Self Motivation and Goal Setting</EmpowerBP:itemName>
        <EmpowerBP:itemText rdf:datatype="http://www.w3.org/2001/XMLSchema#string">Get motivated by tracking your progress. Think about rewards for reaching your goals. What is something you hope to gain by exercising more? Write it down in your Journal. </EmpowerBP:itemText>
        <EmpowerBP:maximumUserAge rdf:datatype="http://www.w3.org/2001/XMLSchema#integer">120</EmpowerBP:maximumUserAge>
        <EmpowerBP:minimumUserAge rdf:datatype="http://www.w3.org/2001/XMLSchema#integer">18</EmpowerBP:minimumUserAge>
        <EmpowerBP:provideJournal rdf:datatype="http://www.w3.org/2001/XMLSchema#boolean">true</EmpowerBP:provideJournal>
        <EmpowerBP:provideLink rdf:datatype="http://www.w3.org/2001/XMLSchema#boolean">false</EmpowerBP:provideLink>
        <EmpowerBP:sourceURL rdf:datatype="http://www.w3.org/2001/XMLSchema#string">http://walkaboutns.ca/walkabout-info/inspiration/getting-over-barriers/</EmpowerBP:sourceURL>
        <rdfs:comment rdf:datatype="http://www.w3.org/2001/XMLSchema#string">Get motivated by tracking your progress. Think about rewards for reaching your goals. What is something you hope to gain by exercising more? Write it down in your Journal. </rdfs:comment>
        <rdfs:label rdf:datatype="http://www.w3.org/2001/XMLSchema#string">Self Motivation and Goal Setting</rdfs:label>
    </owl:NamedIndividual>
    


    <!-- http://www.semanticweb.org/tswheeler/ontologies/2016/3/EmpowerBP#OT30 -->

    <owl:NamedIndividual rdf:about="http://www.semanticweb.org/tswheeler/ontologies/2016/3/EmpowerBP#OT30">
        <rdf:type rdf:resource="http://www.semanticweb.org/tswheeler/ontologies/2016/3/EmpowerBP#InterventionItem"/>
        <rdf:type rdf:resource="http://www.semanticweb.org/tswheeler/ontologies/2016/3/EmpowerBP#Tip"/>
        <EmpowerBP:isAppropriateForInterventionGoal rdf:resource="http://www.semanticweb.org/tswheeler/ontologies/2016/3/EmpowerBP#ExerciseMore"/>
        <EmpowerBP:isWarrantedBy rdf:resource="http://purl.bioontology.org/ontology/BCTT#Instruction_on_how_to_perform_the_behavior"/>
        <EmpowerBP:appropriateForAutomaticMotivation rdf:datatype="http://www.w3.org/2001/XMLSchema#integer">6</EmpowerBP:appropriateForAutomaticMotivation>
        <EmpowerBP:appropriateForLocation rdf:datatype="http://www.w3.org/2001/XMLSchema#integer">0</EmpowerBP:appropriateForLocation>
        <EmpowerBP:appropriateForPhysicalCapability rdf:datatype="http://www.w3.org/2001/XMLSchema#integer">3</EmpowerBP:appropriateForPhysicalCapability>
        <EmpowerBP:appropriateForPhysicalOpportunity rdf:datatype="http://www.w3.org/2001/XMLSchema#integer">3</EmpowerBP:appropriateForPhysicalOpportunity>
        <EmpowerBP:appropriateForPsychologicalCapability rdf:datatype="http://www.w3.org/2001/XMLSchema#integer">3</EmpowerBP:appropriateForPsychologicalCapability>
        <EmpowerBP:appropriateForReflectiveMotivation rdf:datatype="http://www.w3.org/2001/XMLSchema#integer">6</EmpowerBP:appropriateForReflectiveMotivation>
        <EmpowerBP:appropriateForSocialOpportunity rdf:datatype="http://www.w3.org/2001/XMLSchema#integer">3</EmpowerBP:appropriateForSocialOpportunity>
        <EmpowerBP:canRepeat rdf:datatype="http://www.w3.org/2001/XMLSchema#integer">26</EmpowerBP:canRepeat>
        <EmpowerBP:itemName rdf:datatype="http://www.w3.org/2001/XMLSchema#string">Increasing Physical Activity</EmpowerBP:itemName>
        <EmpowerBP:itemText rdf:datatype="http://www.w3.org/2001/XMLSchema#string">Some easy ways to be more active:

• Park far away from your building or use public transportation.
• Use a standing or walking desk.
• Have walking meetings, instead of sitting in the conference room.
• Take a brisk walk after lunch.</EmpowerBP:itemText>
        <EmpowerBP:maximumUserAge rdf:datatype="http://www.w3.org/2001/XMLSchema#integer">120</EmpowerBP:maximumUserAge>
        <EmpowerBP:minimumUserAge rdf:datatype="http://www.w3.org/2001/XMLSchema#integer">18</EmpowerBP:minimumUserAge>
        <EmpowerBP:provideJournal rdf:datatype="http://www.w3.org/2001/XMLSchema#boolean">false</EmpowerBP:provideJournal>
        <EmpowerBP:provideLink rdf:datatype="http://www.w3.org/2001/XMLSchema#boolean">false</EmpowerBP:provideLink>
        <EmpowerBP:sourceURL rdf:datatype="http://www.w3.org/2001/XMLSchema#string">http://www.heartandstroke.ca/get-healthy/stay-active/benefits-of-physical-activity</EmpowerBP:sourceURL>
        <rdfs:comment rdf:datatype="http://www.w3.org/2001/XMLSchema#string">Some easy ways to be more active:

• Park far away from your building or use public transportation.
• Use a standing or walking desk.
• Have walking meetings, instead of sitting in the conference room.
• Take a brisk walk after lunch.</rdfs:comment>
        <rdfs:label rdf:datatype="http://www.w3.org/2001/XMLSchema#string">Increasing Physical Activity</rdfs:label>
    </owl:NamedIndividual>
    


    <!-- http://www.semanticweb.org/tswheeler/ontologies/2016/3/EmpowerBP#OT31 -->

    <owl:NamedIndividual rdf:about="http://www.semanticweb.org/tswheeler/ontologies/2016/3/EmpowerBP#OT31">
        <rdf:type rdf:resource="http://www.semanticweb.org/tswheeler/ontologies/2016/3/EmpowerBP#InterventionItem"/>
        <rdf:type rdf:resource="http://www.semanticweb.org/tswheeler/ontologies/2016/3/EmpowerBP#Tip"/>
        <EmpowerBP:isAppropriateForInterventionGoal rdf:resource="http://www.semanticweb.org/tswheeler/ontologies/2016/3/EmpowerBP#ExerciseMore"/>
        <EmpowerBP:isWarrantedBy rdf:resource="http://purl.bioontology.org/ontology/BCTT#Instruction_on_how_to_perform_the_behavior"/>
        <EmpowerBP:appropriateForAutomaticMotivation rdf:datatype="http://www.w3.org/2001/XMLSchema#integer">6</EmpowerBP:appropriateForAutomaticMotivation>
        <EmpowerBP:appropriateForLocation rdf:datatype="http://www.w3.org/2001/XMLSchema#integer">0</EmpowerBP:appropriateForLocation>
        <EmpowerBP:appropriateForPhysicalCapability rdf:datatype="http://www.w3.org/2001/XMLSchema#integer">3</EmpowerBP:appropriateForPhysicalCapability>
        <EmpowerBP:appropriateForPhysicalOpportunity rdf:datatype="http://www.w3.org/2001/XMLSchema#integer">3</EmpowerBP:appropriateForPhysicalOpportunity>
        <EmpowerBP:appropriateForPsychologicalCapability rdf:datatype="http://www.w3.org/2001/XMLSchema#integer">3</EmpowerBP:appropriateForPsychologicalCapability>
        <EmpowerBP:appropriateForReflectiveMotivation rdf:datatype="http://www.w3.org/2001/XMLSchema#integer">6</EmpowerBP:appropriateForReflectiveMotivation>
        <EmpowerBP:appropriateForSocialOpportunity rdf:datatype="http://www.w3.org/2001/XMLSchema#integer">3</EmpowerBP:appropriateForSocialOpportunity>
        <EmpowerBP:canRepeat rdf:datatype="http://www.w3.org/2001/XMLSchema#integer">26</EmpowerBP:canRepeat>
        <EmpowerBP:itemName rdf:datatype="http://www.w3.org/2001/XMLSchema#string">Increasing Physical Activity</EmpowerBP:itemName>
        <EmpowerBP:itemText rdf:datatype="http://www.w3.org/2001/XMLSchema#string">Some easy ways to be more active:

• Rather than send an email, walk to your co-worker.
• Stand during phone calls.
• Drink enough water that you use the restroom often.
• Play pool, go for a walk or play lawn games instead of watching TV.</EmpowerBP:itemText>
        <EmpowerBP:maximumUserAge rdf:datatype="http://www.w3.org/2001/XMLSchema#integer">120</EmpowerBP:maximumUserAge>
        <EmpowerBP:minimumUserAge rdf:datatype="http://www.w3.org/2001/XMLSchema#integer">18</EmpowerBP:minimumUserAge>
        <EmpowerBP:provideJournal rdf:datatype="http://www.w3.org/2001/XMLSchema#boolean">false</EmpowerBP:provideJournal>
        <EmpowerBP:provideLink rdf:datatype="http://www.w3.org/2001/XMLSchema#boolean">false</EmpowerBP:provideLink>
        <EmpowerBP:sourceURL rdf:datatype="http://www.w3.org/2001/XMLSchema#string">http://www.heartandstroke.ca/get-healthy/stay-active/benefits-of-physical-activity</EmpowerBP:sourceURL>
        <rdfs:comment rdf:datatype="http://www.w3.org/2001/XMLSchema#string">Some easy ways to be more active:

• Rather than send an email, walk to your co-worker.
• Stand during phone calls.
• Drink enough water that you use the restroom often.
• Play pool, go for a walk or play lawn games instead of watching TV.</rdfs:comment>
        <rdfs:label rdf:datatype="http://www.w3.org/2001/XMLSchema#string">Increasing Physical Activity</rdfs:label>
    </owl:NamedIndividual>
    


    <!-- http://www.semanticweb.org/tswheeler/ontologies/2016/3/EmpowerBP#OT32 -->

    <owl:NamedIndividual rdf:about="http://www.semanticweb.org/tswheeler/ontologies/2016/3/EmpowerBP#OT32">
        <rdf:type rdf:resource="http://www.semanticweb.org/tswheeler/ontologies/2016/3/EmpowerBP#InterventionItem"/>
        <rdf:type rdf:resource="http://www.semanticweb.org/tswheeler/ontologies/2016/3/EmpowerBP#Tip"/>
        <EmpowerBP:isAppropriateForInterventionGoal rdf:resource="http://www.semanticweb.org/tswheeler/ontologies/2016/3/EmpowerBP#ExerciseMore"/>
        <EmpowerBP:isWarrantedBy rdf:resource="http://purl.bioontology.org/ontology/BCTT#Instruction_on_how_to_perform_the_behavior"/>
        <EmpowerBP:appropriateForAutomaticMotivation rdf:datatype="http://www.w3.org/2001/XMLSchema#integer">6</EmpowerBP:appropriateForAutomaticMotivation>
        <EmpowerBP:appropriateForLocation rdf:datatype="http://www.w3.org/2001/XMLSchema#integer">0</EmpowerBP:appropriateForLocation>
        <EmpowerBP:appropriateForPhysicalCapability rdf:datatype="http://www.w3.org/2001/XMLSchema#integer">3</EmpowerBP:appropriateForPhysicalCapability>
        <EmpowerBP:appropriateForPhysicalOpportunity rdf:datatype="http://www.w3.org/2001/XMLSchema#integer">3</EmpowerBP:appropriateForPhysicalOpportunity>
        <EmpowerBP:appropriateForPsychologicalCapability rdf:datatype="http://www.w3.org/2001/XMLSchema#integer">3</EmpowerBP:appropriateForPsychologicalCapability>
        <EmpowerBP:appropriateForReflectiveMotivation rdf:datatype="http://www.w3.org/2001/XMLSchema#integer">6</EmpowerBP:appropriateForReflectiveMotivation>
        <EmpowerBP:appropriateForSocialOpportunity rdf:datatype="http://www.w3.org/2001/XMLSchema#integer">3</EmpowerBP:appropriateForSocialOpportunity>
        <EmpowerBP:canRepeat rdf:datatype="http://www.w3.org/2001/XMLSchema#integer">26</EmpowerBP:canRepeat>
        <EmpowerBP:itemName rdf:datatype="http://www.w3.org/2001/XMLSchema#string">Increasing Physical Activity</EmpowerBP:itemName>
        <EmpowerBP:itemText rdf:datatype="http://www.w3.org/2001/XMLSchema#string">Here are some ways to fit phsyical activity into your day: 

• Join a weekday community running or walking group.
• Go for a brisk walk around the block after dinner.
• Take a dance class after work. 
• Bike or walk to work every day.</EmpowerBP:itemText>
        <EmpowerBP:maximumUserAge rdf:datatype="http://www.w3.org/2001/XMLSchema#integer">64</EmpowerBP:maximumUserAge>
        <EmpowerBP:minimumUserAge rdf:datatype="http://www.w3.org/2001/XMLSchema#integer">18</EmpowerBP:minimumUserAge>
        <EmpowerBP:provideJournal rdf:datatype="http://www.w3.org/2001/XMLSchema#boolean">false</EmpowerBP:provideJournal>
        <EmpowerBP:provideLink rdf:datatype="http://www.w3.org/2001/XMLSchema#boolean">false</EmpowerBP:provideLink>
        <EmpowerBP:sourceURL rdf:datatype="http://www.w3.org/2001/XMLSchema#string">http://www.csep.ca/cmfiles/guidelines/csep_guidelines_handbook.pdf</EmpowerBP:sourceURL>
        <rdfs:comment rdf:datatype="http://www.w3.org/2001/XMLSchema#string">Here are some ways to fit phsyical activity into your day: 

• Join a weekday community running or walking group.
• Go for a brisk walk around the block after dinner.
• Take a dance class after work. 
• Bike or walk to work every day.</rdfs:comment>
        <rdfs:label rdf:datatype="http://www.w3.org/2001/XMLSchema#string">Increasing Physical Activity</rdfs:label>
    </owl:NamedIndividual>
    


    <!-- http://www.semanticweb.org/tswheeler/ontologies/2016/3/EmpowerBP#OT33 -->

    <owl:NamedIndividual rdf:about="http://www.semanticweb.org/tswheeler/ontologies/2016/3/EmpowerBP#OT33">
        <rdf:type rdf:resource="http://www.semanticweb.org/tswheeler/ontologies/2016/3/EmpowerBP#InterventionItem"/>
        <rdf:type rdf:resource="http://www.semanticweb.org/tswheeler/ontologies/2016/3/EmpowerBP#Tip"/>
        <EmpowerBP:isAppropriateForInterventionGoal rdf:resource="http://www.semanticweb.org/tswheeler/ontologies/2016/3/EmpowerBP#ExerciseMore"/>
        <EmpowerBP:isWarrantedBy rdf:resource="http://purl.bioontology.org/ontology/BCTT#Instruction_on_how_to_perform_the_behavior"/>
        <EmpowerBP:appropriateForAutomaticMotivation rdf:datatype="http://www.w3.org/2001/XMLSchema#integer">6</EmpowerBP:appropriateForAutomaticMotivation>
        <EmpowerBP:appropriateForLocation rdf:datatype="http://www.w3.org/2001/XMLSchema#integer">0</EmpowerBP:appropriateForLocation>
        <EmpowerBP:appropriateForPhysicalCapability rdf:datatype="http://www.w3.org/2001/XMLSchema#integer">3</EmpowerBP:appropriateForPhysicalCapability>
        <EmpowerBP:appropriateForPhysicalOpportunity rdf:datatype="http://www.w3.org/2001/XMLSchema#integer">3</EmpowerBP:appropriateForPhysicalOpportunity>
        <EmpowerBP:appropriateForPsychologicalCapability rdf:datatype="http://www.w3.org/2001/XMLSchema#integer">3</EmpowerBP:appropriateForPsychologicalCapability>
        <EmpowerBP:appropriateForReflectiveMotivation rdf:datatype="http://www.w3.org/2001/XMLSchema#integer">6</EmpowerBP:appropriateForReflectiveMotivation>
        <EmpowerBP:appropriateForSocialOpportunity rdf:datatype="http://www.w3.org/2001/XMLSchema#integer">3</EmpowerBP:appropriateForSocialOpportunity>
        <EmpowerBP:canRepeat rdf:datatype="http://www.w3.org/2001/XMLSchema#integer">26</EmpowerBP:canRepeat>
        <EmpowerBP:itemName rdf:datatype="http://www.w3.org/2001/XMLSchema#string">Increasing Physical Activity</EmpowerBP:itemName>
        <EmpowerBP:itemText rdf:datatype="http://www.w3.org/2001/XMLSchema#string">Here are some ways to fit phsyical activity into your day: 

• Rake the lawn, and then offer to do the same for a neighbour.
• Train for and participate in a run or walk for charity!
• Take up a favourite sport again or try a new sport.
• Be active with the family on the weekend!</EmpowerBP:itemText>
        <EmpowerBP:maximumUserAge rdf:datatype="http://www.w3.org/2001/XMLSchema#integer">64</EmpowerBP:maximumUserAge>
        <EmpowerBP:minimumUserAge rdf:datatype="http://www.w3.org/2001/XMLSchema#integer">18</EmpowerBP:minimumUserAge>
        <EmpowerBP:provideJournal rdf:datatype="http://www.w3.org/2001/XMLSchema#boolean">false</EmpowerBP:provideJournal>
        <EmpowerBP:provideLink rdf:datatype="http://www.w3.org/2001/XMLSchema#boolean">false</EmpowerBP:provideLink>
        <EmpowerBP:sourceURL rdf:datatype="http://www.w3.org/2001/XMLSchema#string">http://www.csep.ca/cmfiles/guidelines/csep_guidelines_handbook.pdf</EmpowerBP:sourceURL>
        <rdfs:comment rdf:datatype="http://www.w3.org/2001/XMLSchema#string">Here are some ways to fit phsyical activity into your day: 

• Rake the lawn, and then offer to do the same for a neighbour.
• Train for and participate in a run or walk for charity!
• Take up a favourite sport again or try a new sport.
• Be active with the family on the weekend!</rdfs:comment>
        <rdfs:label rdf:datatype="http://www.w3.org/2001/XMLSchema#string">Increasing Physical Activity</rdfs:label>
    </owl:NamedIndividual>
    


    <!-- http://www.semanticweb.org/tswheeler/ontologies/2016/3/EmpowerBP#OT34 -->

    <owl:NamedIndividual rdf:about="http://www.semanticweb.org/tswheeler/ontologies/2016/3/EmpowerBP#OT34">
        <rdf:type rdf:resource="http://www.semanticweb.org/tswheeler/ontologies/2016/3/EmpowerBP#InterventionItem"/>
        <rdf:type rdf:resource="http://www.semanticweb.org/tswheeler/ontologies/2016/3/EmpowerBP#Tip"/>
        <EmpowerBP:isAppropriateForInterventionGoal rdf:resource="http://www.semanticweb.org/tswheeler/ontologies/2016/3/EmpowerBP#ExerciseMore"/>
        <EmpowerBP:isWarrantedBy rdf:resource="http://purl.bioontology.org/ontology/BCTT#Instruction_on_how_to_perform_the_behavior"/>
        <EmpowerBP:appropriateForAutomaticMotivation rdf:datatype="http://www.w3.org/2001/XMLSchema#integer">6</EmpowerBP:appropriateForAutomaticMotivation>
        <EmpowerBP:appropriateForLocation rdf:datatype="http://www.w3.org/2001/XMLSchema#integer">0</EmpowerBP:appropriateForLocation>
        <EmpowerBP:appropriateForPhysicalCapability rdf:datatype="http://www.w3.org/2001/XMLSchema#integer">3</EmpowerBP:appropriateForPhysicalCapability>
        <EmpowerBP:appropriateForPhysicalOpportunity rdf:datatype="http://www.w3.org/2001/XMLSchema#integer">3</EmpowerBP:appropriateForPhysicalOpportunity>
        <EmpowerBP:appropriateForPsychologicalCapability rdf:datatype="http://www.w3.org/2001/XMLSchema#integer">3</EmpowerBP:appropriateForPsychologicalCapability>
        <EmpowerBP:appropriateForReflectiveMotivation rdf:datatype="http://www.w3.org/2001/XMLSchema#integer">6</EmpowerBP:appropriateForReflectiveMotivation>
        <EmpowerBP:appropriateForSocialOpportunity rdf:datatype="http://www.w3.org/2001/XMLSchema#integer">3</EmpowerBP:appropriateForSocialOpportunity>
        <EmpowerBP:canRepeat rdf:datatype="http://www.w3.org/2001/XMLSchema#integer">26</EmpowerBP:canRepeat>
        <EmpowerBP:itemName rdf:datatype="http://www.w3.org/2001/XMLSchema#string">Increasing Physical Activity</EmpowerBP:itemName>
        <EmpowerBP:itemText rdf:datatype="http://www.w3.org/2001/XMLSchema#string">Here are some ways to fit physical activity into your day:

• Join a community urban poling or mall walking group.
• Go for a brisk walk around the block after lunch.
• Take a dance class in the afternoon.
• Train for and participate in a run or walk for charity!</EmpowerBP:itemText>
        <EmpowerBP:maximumUserAge rdf:datatype="http://www.w3.org/2001/XMLSchema#integer">120</EmpowerBP:maximumUserAge>
        <EmpowerBP:minimumUserAge rdf:datatype="http://www.w3.org/2001/XMLSchema#integer">65</EmpowerBP:minimumUserAge>
        <EmpowerBP:provideJournal rdf:datatype="http://www.w3.org/2001/XMLSchema#boolean">false</EmpowerBP:provideJournal>
        <EmpowerBP:provideLink rdf:datatype="http://www.w3.org/2001/XMLSchema#boolean">false</EmpowerBP:provideLink>
        <EmpowerBP:sourceURL rdf:datatype="http://www.w3.org/2001/XMLSchema#string">http://www.csep.ca/cmfiles/guidelines/csep_guidelines_handbook.pdf</EmpowerBP:sourceURL>
        <rdfs:comment rdf:datatype="http://www.w3.org/2001/XMLSchema#string">Here are some ways to fit physical activity into your day:

• Join a community urban poling or mall walking group.
• Go for a brisk walk around the block after lunch.
• Take a dance class in the afternoon.
• Train for and participate in a run or walk for charity!</rdfs:comment>
        <rdfs:label rdf:datatype="http://www.w3.org/2001/XMLSchema#string">Increasing Physical Activity</rdfs:label>
    </owl:NamedIndividual>
    


    <!-- http://www.semanticweb.org/tswheeler/ontologies/2016/3/EmpowerBP#OT35 -->

    <owl:NamedIndividual rdf:about="http://www.semanticweb.org/tswheeler/ontologies/2016/3/EmpowerBP#OT35">
        <rdf:type rdf:resource="http://www.semanticweb.org/tswheeler/ontologies/2016/3/EmpowerBP#InterventionItem"/>
        <rdf:type rdf:resource="http://www.semanticweb.org/tswheeler/ontologies/2016/3/EmpowerBP#Tip"/>
        <EmpowerBP:isAppropriateForInterventionGoal rdf:resource="http://www.semanticweb.org/tswheeler/ontologies/2016/3/EmpowerBP#ExerciseMore"/>
        <EmpowerBP:isWarrantedBy rdf:resource="http://purl.bioontology.org/ontology/BCTT#Instruction_on_how_to_perform_the_behavior"/>
        <EmpowerBP:appropriateForAutomaticMotivation rdf:datatype="http://www.w3.org/2001/XMLSchema#integer">6</EmpowerBP:appropriateForAutomaticMotivation>
        <EmpowerBP:appropriateForLocation rdf:datatype="http://www.w3.org/2001/XMLSchema#integer">0</EmpowerBP:appropriateForLocation>
        <EmpowerBP:appropriateForPhysicalCapability rdf:datatype="http://www.w3.org/2001/XMLSchema#integer">3</EmpowerBP:appropriateForPhysicalCapability>
        <EmpowerBP:appropriateForPhysicalOpportunity rdf:datatype="http://www.w3.org/2001/XMLSchema#integer">3</EmpowerBP:appropriateForPhysicalOpportunity>
        <EmpowerBP:appropriateForPsychologicalCapability rdf:datatype="http://www.w3.org/2001/XMLSchema#integer">3</EmpowerBP:appropriateForPsychologicalCapability>
        <EmpowerBP:appropriateForReflectiveMotivation rdf:datatype="http://www.w3.org/2001/XMLSchema#integer">6</EmpowerBP:appropriateForReflectiveMotivation>
        <EmpowerBP:appropriateForSocialOpportunity rdf:datatype="http://www.w3.org/2001/XMLSchema#integer">3</EmpowerBP:appropriateForSocialOpportunity>
        <EmpowerBP:canRepeat rdf:datatype="http://www.w3.org/2001/XMLSchema#integer">26</EmpowerBP:canRepeat>
        <EmpowerBP:itemName rdf:datatype="http://www.w3.org/2001/XMLSchema#string">Increasing Physical Activity</EmpowerBP:itemName>
        <EmpowerBP:itemText rdf:datatype="http://www.w3.org/2001/XMLSchema#string">Here are some ways to fit physical activity into your day: 

• Take up a favourite sport again.
• Be active with the family! Plan to have “active reunions”.
• Go for a nature hike on the weekend. 
• Take the dog for a walk after dinner.</EmpowerBP:itemText>
        <EmpowerBP:maximumUserAge rdf:datatype="http://www.w3.org/2001/XMLSchema#integer">120</EmpowerBP:maximumUserAge>
        <EmpowerBP:minimumUserAge rdf:datatype="http://www.w3.org/2001/XMLSchema#integer">65</EmpowerBP:minimumUserAge>
        <EmpowerBP:provideJournal rdf:datatype="http://www.w3.org/2001/XMLSchema#boolean">false</EmpowerBP:provideJournal>
        <EmpowerBP:provideLink rdf:datatype="http://www.w3.org/2001/XMLSchema#boolean">false</EmpowerBP:provideLink>
        <EmpowerBP:sourceURL rdf:datatype="http://www.w3.org/2001/XMLSchema#string">http://www.csep.ca/cmfiles/guidelines/csep_guidelines_handbook.pdf</EmpowerBP:sourceURL>
        <rdfs:comment rdf:datatype="http://www.w3.org/2001/XMLSchema#string">Here are some ways to fit physical activity into your day: 

• Take up a favourite sport again.
• Be active with the family! Plan to have “active reunions”.
• Go for a nature hike on the weekend. 
• Take the dog for a walk after dinner.</rdfs:comment>
        <rdfs:label rdf:datatype="http://www.w3.org/2001/XMLSchema#string">Increasing Physical Activity</rdfs:label>
    </owl:NamedIndividual>
    


    <!-- http://www.semanticweb.org/tswheeler/ontologies/2016/3/EmpowerBP#OT36 -->

    <owl:NamedIndividual rdf:about="http://www.semanticweb.org/tswheeler/ontologies/2016/3/EmpowerBP#OT36">
        <rdf:type rdf:resource="http://www.semanticweb.org/tswheeler/ontologies/2016/3/EmpowerBP#InterventionItem"/>
        <rdf:type rdf:resource="http://www.semanticweb.org/tswheeler/ontologies/2016/3/EmpowerBP#Tip"/>
        <EmpowerBP:isAppropriateForInterventionGoal rdf:resource="http://www.semanticweb.org/tswheeler/ontologies/2016/3/EmpowerBP#ExerciseMore"/>
        <EmpowerBP:isWarrantedBy rdf:resource="http://purl.bioontology.org/ontology/BCTT#Action_planning"/>
        <EmpowerBP:appropriateForAutomaticMotivation rdf:datatype="http://www.w3.org/2001/XMLSchema#integer">6</EmpowerBP:appropriateForAutomaticMotivation>
        <EmpowerBP:appropriateForLocation rdf:datatype="http://www.w3.org/2001/XMLSchema#integer">6</EmpowerBP:appropriateForLocation>
        <EmpowerBP:appropriateForPhysicalCapability rdf:datatype="http://www.w3.org/2001/XMLSchema#integer">3</EmpowerBP:appropriateForPhysicalCapability>
        <EmpowerBP:appropriateForPhysicalOpportunity rdf:datatype="http://www.w3.org/2001/XMLSchema#integer">3</EmpowerBP:appropriateForPhysicalOpportunity>
        <EmpowerBP:appropriateForPsychologicalCapability rdf:datatype="http://www.w3.org/2001/XMLSchema#integer">3</EmpowerBP:appropriateForPsychologicalCapability>
        <EmpowerBP:appropriateForReflectiveMotivation rdf:datatype="http://www.w3.org/2001/XMLSchema#integer">6</EmpowerBP:appropriateForReflectiveMotivation>
        <EmpowerBP:appropriateForSocialOpportunity rdf:datatype="http://www.w3.org/2001/XMLSchema#integer">3</EmpowerBP:appropriateForSocialOpportunity>
        <EmpowerBP:canRepeat rdf:datatype="http://www.w3.org/2001/XMLSchema#integer">26</EmpowerBP:canRepeat>
        <EmpowerBP:itemName rdf:datatype="http://www.w3.org/2001/XMLSchema#string">Heart &amp; Stroke Walkabout Routes</EmpowerBP:itemName>
        <EmpowerBP:itemText rdf:datatype="http://www.w3.org/2001/XMLSchema#string">Check out this website and find a place to walk near you! Enter your community in the search bar and click Search to find where people go to walk near you. Are there any places you are interested in trying? </EmpowerBP:itemText>
        <EmpowerBP:maximumUserAge rdf:datatype="http://www.w3.org/2001/XMLSchema#integer">120</EmpowerBP:maximumUserAge>
        <EmpowerBP:minimumUserAge rdf:datatype="http://www.w3.org/2001/XMLSchema#integer">18</EmpowerBP:minimumUserAge>
        <EmpowerBP:provideJournal rdf:datatype="http://www.w3.org/2001/XMLSchema#boolean">false</EmpowerBP:provideJournal>
        <EmpowerBP:provideLink rdf:datatype="http://www.w3.org/2001/XMLSchema#boolean">true</EmpowerBP:provideLink>
        <EmpowerBP:sourceURL rdf:datatype="http://www.w3.org/2001/XMLSchema#string">http://walkaboutns.ca/routes/</EmpowerBP:sourceURL>
        <rdfs:comment rdf:datatype="http://www.w3.org/2001/XMLSchema#string">Check out this website and find a place to walk near you! Enter your community in the search bar and click Search to find where people go to walk near you. Are there any places you are interested in trying? </rdfs:comment>
        <rdfs:label rdf:datatype="http://www.w3.org/2001/XMLSchema#string">Heart &amp; Stroke Walkabout Routes</rdfs:label>
    </owl:NamedIndividual>
    


    <!-- http://www.semanticweb.org/tswheeler/ontologies/2016/3/EmpowerBP#OT4 -->

    <owl:NamedIndividual rdf:about="http://www.semanticweb.org/tswheeler/ontologies/2016/3/EmpowerBP#OT4">
        <rdf:type rdf:resource="http://www.semanticweb.org/tswheeler/ontologies/2016/3/EmpowerBP#InterventionItem"/>
        <rdf:type rdf:resource="http://www.semanticweb.org/tswheeler/ontologies/2016/3/EmpowerBP#Tip"/>
        <EmpowerBP:isAppropriateForInterventionGoal rdf:resource="http://www.semanticweb.org/tswheeler/ontologies/2016/3/EmpowerBP#ExerciseMore"/>
        <EmpowerBP:isWarrantedBy rdf:resource="http://purl.bioontology.org/ontology/BCTT#Behavioral_experiments"/>
        <EmpowerBP:appropriateForAutomaticMotivation rdf:datatype="http://www.w3.org/2001/XMLSchema#integer">3</EmpowerBP:appropriateForAutomaticMotivation>
        <EmpowerBP:appropriateForLocation rdf:datatype="http://www.w3.org/2001/XMLSchema#integer">0</EmpowerBP:appropriateForLocation>
        <EmpowerBP:appropriateForPhysicalCapability rdf:datatype="http://www.w3.org/2001/XMLSchema#integer">3</EmpowerBP:appropriateForPhysicalCapability>
        <EmpowerBP:appropriateForPhysicalOpportunity rdf:datatype="http://www.w3.org/2001/XMLSchema#integer">3</EmpowerBP:appropriateForPhysicalOpportunity>
        <EmpowerBP:appropriateForPsychologicalCapability rdf:datatype="http://www.w3.org/2001/XMLSchema#integer">3</EmpowerBP:appropriateForPsychologicalCapability>
        <EmpowerBP:appropriateForReflectiveMotivation rdf:datatype="http://www.w3.org/2001/XMLSchema#integer">3</EmpowerBP:appropriateForReflectiveMotivation>
        <EmpowerBP:appropriateForSocialOpportunity rdf:datatype="http://www.w3.org/2001/XMLSchema#integer">3</EmpowerBP:appropriateForSocialOpportunity>
        <EmpowerBP:canRepeat rdf:datatype="http://www.w3.org/2001/XMLSchema#integer">26</EmpowerBP:canRepeat>
        <EmpowerBP:itemName rdf:datatype="http://www.w3.org/2001/XMLSchema#string">WalkaboutNS Energy Tip</EmpowerBP:itemName>
        <EmpowerBP:itemText rdf:datatype="http://www.w3.org/2001/XMLSchema#string">Too tired to exercise? 

Walking regularly will increase your energy. When you feel tired, your body may benefit from a walk. Test it out! Next time you go for a walk, spend a moment after to think about how your body feels. You can about write it in a Journal entry.</EmpowerBP:itemText>
        <EmpowerBP:maximumUserAge rdf:datatype="http://www.w3.org/2001/XMLSchema#integer">120</EmpowerBP:maximumUserAge>
        <EmpowerBP:minimumUserAge rdf:datatype="http://www.w3.org/2001/XMLSchema#integer">18</EmpowerBP:minimumUserAge>
        <EmpowerBP:provideJournal rdf:datatype="http://www.w3.org/2001/XMLSchema#boolean">true</EmpowerBP:provideJournal>
        <EmpowerBP:provideLink rdf:datatype="http://www.w3.org/2001/XMLSchema#boolean">false</EmpowerBP:provideLink>
        <EmpowerBP:sourceURL rdf:datatype="http://www.w3.org/2001/XMLSchema#string">http://walkaboutns.ca/walkabout-info/inspiration/getting-over-barriers/</EmpowerBP:sourceURL>
        <rdfs:comment rdf:datatype="http://www.w3.org/2001/XMLSchema#string">Too tired to exercise? 

Walking regularly will increase your energy. When you feel tired, your body may benefit from a walk. Test it out! Next time you go for a walk, spend a moment after to think about how your body feels. You can about write it in a Journal entry.</rdfs:comment>
        <rdfs:label rdf:datatype="http://www.w3.org/2001/XMLSchema#string">WalkaboutNS Energy Tip</rdfs:label>
    </owl:NamedIndividual>
    


    <!-- http://www.semanticweb.org/tswheeler/ontologies/2016/3/EmpowerBP#OT5 -->

    <owl:NamedIndividual rdf:about="http://www.semanticweb.org/tswheeler/ontologies/2016/3/EmpowerBP#OT5">
        <rdf:type rdf:resource="http://www.semanticweb.org/tswheeler/ontologies/2016/3/EmpowerBP#InterventionItem"/>
        <rdf:type rdf:resource="http://www.semanticweb.org/tswheeler/ontologies/2016/3/EmpowerBP#Tip"/>
        <EmpowerBP:isAppropriateForInterventionGoal rdf:resource="http://www.semanticweb.org/tswheeler/ontologies/2016/3/EmpowerBP#ExerciseMore"/>
        <EmpowerBP:isWarrantedBy rdf:resource="http://purl.bioontology.org/ontology/BCTT#Social_support_(practical)"/>
        <EmpowerBP:appropriateForAutomaticMotivation rdf:datatype="http://www.w3.org/2001/XMLSchema#integer">3</EmpowerBP:appropriateForAutomaticMotivation>
        <EmpowerBP:appropriateForLocation rdf:datatype="http://www.w3.org/2001/XMLSchema#integer">0</EmpowerBP:appropriateForLocation>
        <EmpowerBP:appropriateForPhysicalCapability rdf:datatype="http://www.w3.org/2001/XMLSchema#integer">3</EmpowerBP:appropriateForPhysicalCapability>
        <EmpowerBP:appropriateForPhysicalOpportunity rdf:datatype="http://www.w3.org/2001/XMLSchema#integer">3</EmpowerBP:appropriateForPhysicalOpportunity>
        <EmpowerBP:appropriateForPsychologicalCapability rdf:datatype="http://www.w3.org/2001/XMLSchema#integer">3</EmpowerBP:appropriateForPsychologicalCapability>
        <EmpowerBP:appropriateForReflectiveMotivation rdf:datatype="http://www.w3.org/2001/XMLSchema#integer">3</EmpowerBP:appropriateForReflectiveMotivation>
        <EmpowerBP:appropriateForSocialOpportunity rdf:datatype="http://www.w3.org/2001/XMLSchema#integer">3</EmpowerBP:appropriateForSocialOpportunity>
        <EmpowerBP:canRepeat rdf:datatype="http://www.w3.org/2001/XMLSchema#integer">26</EmpowerBP:canRepeat>
        <EmpowerBP:itemName rdf:datatype="http://www.w3.org/2001/XMLSchema#string">WalkaboutNS Enjoyment Tip</EmpowerBP:itemName>
        <EmpowerBP:itemText rdf:datatype="http://www.w3.org/2001/XMLSchema#string">Find exercise boring? 

Walking is a great way to spend time with family and friends. You can walk while you discuss business or chat with a friend. Connect with a local walking group here or start your own! </EmpowerBP:itemText>
        <EmpowerBP:maximumUserAge rdf:datatype="http://www.w3.org/2001/XMLSchema#integer">120</EmpowerBP:maximumUserAge>
        <EmpowerBP:minimumUserAge rdf:datatype="http://www.w3.org/2001/XMLSchema#integer">18</EmpowerBP:minimumUserAge>
        <EmpowerBP:provideJournal rdf:datatype="http://www.w3.org/2001/XMLSchema#boolean">false</EmpowerBP:provideJournal>
        <EmpowerBP:provideLink rdf:datatype="http://www.w3.org/2001/XMLSchema#boolean">false</EmpowerBP:provideLink>
        <EmpowerBP:sourceURL rdf:datatype="http://www.w3.org/2001/XMLSchema#string">http://walkaboutns.ca/walkabout-info/inspiration/getting-over-barriers/</EmpowerBP:sourceURL>
        <rdfs:comment rdf:datatype="http://www.w3.org/2001/XMLSchema#string">Find exercise boring? 

Walking is a great way to spend time with family and friends. You can walk while you discuss business or chat with a friend. Connect with a local walking group here or start your own! </rdfs:comment>
        <rdfs:label rdf:datatype="http://www.w3.org/2001/XMLSchema#string">WalkaboutNS Enjoyment Tip</rdfs:label>
    </owl:NamedIndividual>
    


    <!-- http://www.semanticweb.org/tswheeler/ontologies/2016/3/EmpowerBP#OT6 -->

    <owl:NamedIndividual rdf:about="http://www.semanticweb.org/tswheeler/ontologies/2016/3/EmpowerBP#OT6">
        <rdf:type rdf:resource="http://www.semanticweb.org/tswheeler/ontologies/2016/3/EmpowerBP#InterventionItem"/>
        <rdf:type rdf:resource="http://www.semanticweb.org/tswheeler/ontologies/2016/3/EmpowerBP#Tip"/>
        <EmpowerBP:isAppropriateForInterventionGoal rdf:resource="http://www.semanticweb.org/tswheeler/ontologies/2016/3/EmpowerBP#ExerciseMore"/>
        <EmpowerBP:isWarrantedBy rdf:resource="http://purl.bioontology.org/ontology/BCTT#Restructuring_the_physical_environment"/>
        <EmpowerBP:appropriateForAutomaticMotivation rdf:datatype="http://www.w3.org/2001/XMLSchema#integer">3</EmpowerBP:appropriateForAutomaticMotivation>
        <EmpowerBP:appropriateForLocation rdf:datatype="http://www.w3.org/2001/XMLSchema#integer">0</EmpowerBP:appropriateForLocation>
        <EmpowerBP:appropriateForPhysicalCapability rdf:datatype="http://www.w3.org/2001/XMLSchema#integer">3</EmpowerBP:appropriateForPhysicalCapability>
        <EmpowerBP:appropriateForPhysicalOpportunity rdf:datatype="http://www.w3.org/2001/XMLSchema#integer">3</EmpowerBP:appropriateForPhysicalOpportunity>
        <EmpowerBP:appropriateForPsychologicalCapability rdf:datatype="http://www.w3.org/2001/XMLSchema#integer">3</EmpowerBP:appropriateForPsychologicalCapability>
        <EmpowerBP:appropriateForReflectiveMotivation rdf:datatype="http://www.w3.org/2001/XMLSchema#integer">3</EmpowerBP:appropriateForReflectiveMotivation>
        <EmpowerBP:appropriateForSocialOpportunity rdf:datatype="http://www.w3.org/2001/XMLSchema#integer">3</EmpowerBP:appropriateForSocialOpportunity>
        <EmpowerBP:canRepeat rdf:datatype="http://www.w3.org/2001/XMLSchema#integer">26</EmpowerBP:canRepeat>
        <EmpowerBP:itemName rdf:datatype="http://www.w3.org/2001/XMLSchema#string">WalkaboutNS Enjoyment Tip</EmpowerBP:itemName>
        <EmpowerBP:itemText rdf:datatype="http://www.w3.org/2001/XMLSchema#string">Find exercise boring? 

Bring along a music player or audiobook to keep yourself entertained.  Take notice of the area you are walking to appreciate your surroundings. Bring a camera and upload pictures from your walk to social media. </EmpowerBP:itemText>
        <EmpowerBP:maximumUserAge rdf:datatype="http://www.w3.org/2001/XMLSchema#integer">120</EmpowerBP:maximumUserAge>
        <EmpowerBP:minimumUserAge rdf:datatype="http://www.w3.org/2001/XMLSchema#integer">18</EmpowerBP:minimumUserAge>
        <EmpowerBP:provideJournal rdf:datatype="http://www.w3.org/2001/XMLSchema#boolean">false</EmpowerBP:provideJournal>
        <EmpowerBP:provideLink rdf:datatype="http://www.w3.org/2001/XMLSchema#boolean">false</EmpowerBP:provideLink>
        <EmpowerBP:sourceURL rdf:datatype="http://www.w3.org/2001/XMLSchema#string">http://walkaboutns.ca/walkabout-info/inspiration/getting-over-barriers/</EmpowerBP:sourceURL>
        <rdfs:comment rdf:datatype="http://www.w3.org/2001/XMLSchema#string">Find exercise boring? 

Bring along a music player or audiobook to keep yourself entertained.  Take notice of the area you are walking to appreciate your surroundings. Bring a camera and upload pictures from your walk to social media. </rdfs:comment>
        <rdfs:label rdf:datatype="http://www.w3.org/2001/XMLSchema#string">WalkaboutNS Enjoyment Tip</rdfs:label>
    </owl:NamedIndividual>
    


    <!-- http://www.semanticweb.org/tswheeler/ontologies/2016/3/EmpowerBP#OT7 -->

    <owl:NamedIndividual rdf:about="http://www.semanticweb.org/tswheeler/ontologies/2016/3/EmpowerBP#OT7">
        <rdf:type rdf:resource="http://www.semanticweb.org/tswheeler/ontologies/2016/3/EmpowerBP#InterventionItem"/>
        <rdf:type rdf:resource="http://www.semanticweb.org/tswheeler/ontologies/2016/3/EmpowerBP#Tip"/>
        <EmpowerBP:isAppropriateForInterventionGoal rdf:resource="http://www.semanticweb.org/tswheeler/ontologies/2016/3/EmpowerBP#ExerciseMore"/>
        <EmpowerBP:isWarrantedBy rdf:resource="http://purl.bioontology.org/ontology/BCTT#Verbal_persuasion_about_capability"/>
        <EmpowerBP:appropriateForAutomaticMotivation rdf:datatype="http://www.w3.org/2001/XMLSchema#integer">3</EmpowerBP:appropriateForAutomaticMotivation>
        <EmpowerBP:appropriateForLocation rdf:datatype="http://www.w3.org/2001/XMLSchema#integer">0</EmpowerBP:appropriateForLocation>
        <EmpowerBP:appropriateForPhysicalCapability rdf:datatype="http://www.w3.org/2001/XMLSchema#integer">3</EmpowerBP:appropriateForPhysicalCapability>
        <EmpowerBP:appropriateForPhysicalOpportunity rdf:datatype="http://www.w3.org/2001/XMLSchema#integer">3</EmpowerBP:appropriateForPhysicalOpportunity>
        <EmpowerBP:appropriateForPsychologicalCapability rdf:datatype="http://www.w3.org/2001/XMLSchema#integer">3</EmpowerBP:appropriateForPsychologicalCapability>
        <EmpowerBP:appropriateForReflectiveMotivation rdf:datatype="http://www.w3.org/2001/XMLSchema#integer">3</EmpowerBP:appropriateForReflectiveMotivation>
        <EmpowerBP:appropriateForSocialOpportunity rdf:datatype="http://www.w3.org/2001/XMLSchema#integer">3</EmpowerBP:appropriateForSocialOpportunity>
        <EmpowerBP:canRepeat rdf:datatype="http://www.w3.org/2001/XMLSchema#integer">26</EmpowerBP:canRepeat>
        <EmpowerBP:itemName rdf:datatype="http://www.w3.org/2001/XMLSchema#string">WalkaboutNS Confidence Tip</EmpowerBP:itemName>
        <EmpowerBP:itemText rdf:datatype="http://www.w3.org/2001/XMLSchema#string">Unsure of how to start being more active? 

Walking doesn’t require skill or expertise. Building a little more walking into your day, every day, is an easy way to shift into being active again. It can help you accomplish several things at once – run errands, walk your kids to school or meet a friend for coffee.</EmpowerBP:itemText>
        <EmpowerBP:maximumUserAge rdf:datatype="http://www.w3.org/2001/XMLSchema#integer">120</EmpowerBP:maximumUserAge>
        <EmpowerBP:minimumUserAge rdf:datatype="http://www.w3.org/2001/XMLSchema#integer">3</EmpowerBP:minimumUserAge>
        <EmpowerBP:provideJournal rdf:datatype="http://www.w3.org/2001/XMLSchema#boolean">false</EmpowerBP:provideJournal>
        <EmpowerBP:provideLink rdf:datatype="http://www.w3.org/2001/XMLSchema#boolean">false</EmpowerBP:provideLink>
        <EmpowerBP:sourceURL rdf:datatype="http://www.w3.org/2001/XMLSchema#string">http://walkaboutns.ca/walkabout-info/inspiration/getting-over-barriers/</EmpowerBP:sourceURL>
        <rdfs:comment rdf:datatype="http://www.w3.org/2001/XMLSchema#string">Unsure of how to start being more active? 

Walking doesn’t require skill or expertise. Building a little more walking into your day, every day, is an easy way to shift into being active again. It can help you accomplish several things at once – run errands, walk your kids to school or meet a friend for coffee.</rdfs:comment>
        <rdfs:label rdf:datatype="http://www.w3.org/2001/XMLSchema#string">WalkaboutNS Confidence Tip</rdfs:label>
    </owl:NamedIndividual>
    


    <!-- http://www.semanticweb.org/tswheeler/ontologies/2016/3/EmpowerBP#OT8 -->

    <owl:NamedIndividual rdf:about="http://www.semanticweb.org/tswheeler/ontologies/2016/3/EmpowerBP#OT8">
        <rdf:type rdf:resource="http://www.semanticweb.org/tswheeler/ontologies/2016/3/EmpowerBP#InterventionItem"/>
        <rdf:type rdf:resource="http://www.semanticweb.org/tswheeler/ontologies/2016/3/EmpowerBP#Tip"/>
        <EmpowerBP:isAppropriateForInterventionGoal rdf:resource="http://www.semanticweb.org/tswheeler/ontologies/2016/3/EmpowerBP#ExerciseMore"/>
        <EmpowerBP:isWarrantedBy rdf:resource="http://purl.bioontology.org/ontology/BCTT#Verbal_persuasion_about_capability"/>
        <EmpowerBP:appropriateForAutomaticMotivation rdf:datatype="http://www.w3.org/2001/XMLSchema#integer">3</EmpowerBP:appropriateForAutomaticMotivation>
        <EmpowerBP:appropriateForLocation rdf:datatype="http://www.w3.org/2001/XMLSchema#integer">0</EmpowerBP:appropriateForLocation>
        <EmpowerBP:appropriateForPhysicalCapability rdf:datatype="http://www.w3.org/2001/XMLSchema#integer">3</EmpowerBP:appropriateForPhysicalCapability>
        <EmpowerBP:appropriateForPhysicalOpportunity rdf:datatype="http://www.w3.org/2001/XMLSchema#integer">3</EmpowerBP:appropriateForPhysicalOpportunity>
        <EmpowerBP:appropriateForPsychologicalCapability rdf:datatype="http://www.w3.org/2001/XMLSchema#integer">3</EmpowerBP:appropriateForPsychologicalCapability>
        <EmpowerBP:appropriateForReflectiveMotivation rdf:datatype="http://www.w3.org/2001/XMLSchema#integer">3</EmpowerBP:appropriateForReflectiveMotivation>
        <EmpowerBP:appropriateForSocialOpportunity rdf:datatype="http://www.w3.org/2001/XMLSchema#integer">3</EmpowerBP:appropriateForSocialOpportunity>
        <EmpowerBP:canRepeat rdf:datatype="http://www.w3.org/2001/XMLSchema#integer">26</EmpowerBP:canRepeat>
        <EmpowerBP:itemName rdf:datatype="http://www.w3.org/2001/XMLSchema#string">WalkaboutNS Age Tip</EmpowerBP:itemName>
        <EmpowerBP:itemText rdf:datatype="http://www.w3.org/2001/XMLSchema#string">You’re never too old to increase your level of physical activity. Physical activity supports healthy, graceful aging. Many people notice they feel better almost immediately and find that getting around is easier.</EmpowerBP:itemText>
        <EmpowerBP:maximumUserAge rdf:datatype="http://www.w3.org/2001/XMLSchema#integer">120</EmpowerBP:maximumUserAge>
        <EmpowerBP:minimumUserAge rdf:datatype="http://www.w3.org/2001/XMLSchema#integer">18</EmpowerBP:minimumUserAge>
        <EmpowerBP:provideJournal rdf:datatype="http://www.w3.org/2001/XMLSchema#boolean">false</EmpowerBP:provideJournal>
        <EmpowerBP:provideLink rdf:datatype="http://www.w3.org/2001/XMLSchema#boolean">false</EmpowerBP:provideLink>
        <EmpowerBP:sourceURL rdf:datatype="http://www.w3.org/2001/XMLSchema#string">http://walkaboutns.ca/walkabout-info/inspiration/getting-over-barriers/</EmpowerBP:sourceURL>
        <rdfs:comment rdf:datatype="http://www.w3.org/2001/XMLSchema#string">You’re never too old to increase your level of physical activity. Physical activity supports healthy, graceful aging. Many people notice they feel better almost immediately and find that getting around is easier.</rdfs:comment>
        <rdfs:label rdf:datatype="http://www.w3.org/2001/XMLSchema#string">WalkaboutNS Age Tip</rdfs:label>
    </owl:NamedIndividual>
    


    <!-- http://www.semanticweb.org/tswheeler/ontologies/2016/3/EmpowerBP#OT9 -->

    <owl:NamedIndividual rdf:about="http://www.semanticweb.org/tswheeler/ontologies/2016/3/EmpowerBP#OT9">
        <rdf:type rdf:resource="http://www.semanticweb.org/tswheeler/ontologies/2016/3/EmpowerBP#InterventionItem"/>
        <rdf:type rdf:resource="http://www.semanticweb.org/tswheeler/ontologies/2016/3/EmpowerBP#Tip"/>
        <EmpowerBP:isAppropriateForInterventionGoal rdf:resource="http://www.semanticweb.org/tswheeler/ontologies/2016/3/EmpowerBP#ExerciseMore"/>
        <EmpowerBP:isWarrantedBy rdf:resource="http://purl.bioontology.org/ontology/BCTT#Restructuring_the_physical_environment"/>
        <EmpowerBP:appropriateForAutomaticMotivation rdf:datatype="http://www.w3.org/2001/XMLSchema#integer">3</EmpowerBP:appropriateForAutomaticMotivation>
        <EmpowerBP:appropriateForLocation rdf:datatype="http://www.w3.org/2001/XMLSchema#integer">0</EmpowerBP:appropriateForLocation>
        <EmpowerBP:appropriateForPhysicalCapability rdf:datatype="http://www.w3.org/2001/XMLSchema#integer">3</EmpowerBP:appropriateForPhysicalCapability>
        <EmpowerBP:appropriateForPhysicalOpportunity rdf:datatype="http://www.w3.org/2001/XMLSchema#integer">3</EmpowerBP:appropriateForPhysicalOpportunity>
        <EmpowerBP:appropriateForPsychologicalCapability rdf:datatype="http://www.w3.org/2001/XMLSchema#integer">3</EmpowerBP:appropriateForPsychologicalCapability>
        <EmpowerBP:appropriateForReflectiveMotivation rdf:datatype="http://www.w3.org/2001/XMLSchema#integer">3</EmpowerBP:appropriateForReflectiveMotivation>
        <EmpowerBP:appropriateForSocialOpportunity rdf:datatype="http://www.w3.org/2001/XMLSchema#integer">3</EmpowerBP:appropriateForSocialOpportunity>
        <EmpowerBP:canRepeat rdf:datatype="http://www.w3.org/2001/XMLSchema#integer">26</EmpowerBP:canRepeat>
        <EmpowerBP:itemName rdf:datatype="http://www.w3.org/2001/XMLSchema#string">WalkaboutNS Weather Tip</EmpowerBP:itemName>
        <EmpowerBP:itemText rdf:datatype="http://www.w3.org/2001/XMLSchema#string">Worried about the weather? 

Dress for the weather. When you are prepared, you will enjoy being outdoors. If you don’t want to be outside, walk in your office building or go to a mall, arena or other covered location. Indoor tracks are also a great place to walk as well.</EmpowerBP:itemText>
        <EmpowerBP:maximumUserAge rdf:datatype="http://www.w3.org/2001/XMLSchema#integer">120</EmpowerBP:maximumUserAge>
        <EmpowerBP:minimumUserAge rdf:datatype="http://www.w3.org/2001/XMLSchema#integer">18</EmpowerBP:minimumUserAge>
        <EmpowerBP:provideJournal rdf:datatype="http://www.w3.org/2001/XMLSchema#boolean">false</EmpowerBP:provideJournal>
        <EmpowerBP:provideLink rdf:datatype="http://www.w3.org/2001/XMLSchema#boolean">false</EmpowerBP:provideLink>
        <EmpowerBP:sourceURL rdf:datatype="http://www.w3.org/2001/XMLSchema#string">http://walkaboutns.ca/walkabout-info/inspiration/getting-over-barriers/</EmpowerBP:sourceURL>
        <rdfs:comment rdf:datatype="http://www.w3.org/2001/XMLSchema#string">Worried about the weather? 

Dress for the weather. When you are prepared, you will enjoy being outdoors. If you don’t want to be outside, walk in your office building or go to a mall, arena or other covered location. Indoor tracks are also a great place to walk as well.</rdfs:comment>
        <rdfs:label rdf:datatype="http://www.w3.org/2001/XMLSchema#string">WalkaboutNS Weather Tip</rdfs:label>
    </owl:NamedIndividual>
    


    <!-- http://www.semanticweb.org/tswheeler/ontologies/2016/3/EmpowerBP#Optimism -->

    <owl:NamedIndividual rdf:about="http://www.semanticweb.org/tswheeler/ontologies/2016/3/EmpowerBP#Optimism">
        <rdf:type rdf:resource="http://www.semanticweb.org/tswheeler/ontologies/2016/3/EmpowerBP#Construct"/>
        <rdf:type rdf:resource="http://www.semanticweb.org/tswheeler/ontologies/2016/3/EmpowerBP#TDFDomain"/>
        <EmpowerBP:hasEffectiveInterventionFunction rdf:resource="http://www.semanticweb.org/tswheeler/ontologies/2016/3/EmpowerBP#Education"/>
        <EmpowerBP:hasEffectiveInterventionFunction rdf:resource="http://www.semanticweb.org/tswheeler/ontologies/2016/3/EmpowerBP#Enablement"/>
        <EmpowerBP:hasEffectiveInterventionFunction rdf:resource="http://www.semanticweb.org/tswheeler/ontologies/2016/3/EmpowerBP#Modelling"/>
        <EmpowerBP:hasEffectiveInterventionFunction rdf:resource="http://www.semanticweb.org/tswheeler/ontologies/2016/3/EmpowerBP#Persuasion"/>
        <EmpowerBP:isRelatedToCOMB rdf:resource="http://www.semanticweb.org/tswheeler/ontologies/2016/3/EmpowerBP#ReflectiveMotivation"/>
        <rdfs:comment>The confidence that things will happen for the best, or that desired goals will be attained</rdfs:comment>
    </owl:NamedIndividual>
    


    <!-- http://www.semanticweb.org/tswheeler/ontologies/2016/3/EmpowerBP#Persuasion -->

    <owl:NamedIndividual rdf:about="http://www.semanticweb.org/tswheeler/ontologies/2016/3/EmpowerBP#Persuasion">
        <rdf:type rdf:resource="http://www.semanticweb.org/tswheeler/ontologies/2016/3/EmpowerBP#InterventionFuction"/>
        <EmpowerBP:hasCommonBCT rdf:resource="http://purl.bioontology.org/ontology/BCTT#Biofeedback"/>
        <EmpowerBP:hasCommonBCT rdf:resource="http://purl.bioontology.org/ontology/BCTT#Focus_on_past_success"/>
        <EmpowerBP:hasCommonBCT rdf:resource="http://purl.bioontology.org/ontology/BCTT#Framing-reframing"/>
        <EmpowerBP:hasCommonBCT rdf:resource="http://purl.bioontology.org/ontology/BCTT#Identification_of_self_as_role_model"/>
        <EmpowerBP:hasCommonBCT rdf:resource="http://purl.bioontology.org/ontology/BCTT#Identity_associated_with_changed_behavior"/>
        <EmpowerBP:hasCommonBCT rdf:resource="http://purl.bioontology.org/ontology/BCTT#Information_about_emotional_consequences"/>
        <EmpowerBP:hasCommonBCT rdf:resource="http://purl.bioontology.org/ontology/BCTT#Re-attribution"/>
        <EmpowerBP:hasCommonBCT rdf:resource="http://purl.bioontology.org/ontology/BCTT#Salience_of_consequences"/>
        <EmpowerBP:hasCommonBCT rdf:resource="http://purl.bioontology.org/ontology/BCTT#Social_comparison"/>
        <EmpowerBP:hasCommonBCT rdf:resource="http://purl.bioontology.org/ontology/BCTT#Verbal_persuasion_about_capability"/>
        <EmpowerBP:hasCommonBCT rdf:resource="http://purl.bioontology.org/ontology/BCTT#Information_about_others&apos;_approval"/>
        <EmpowerBP:hasMostCommonBCT rdf:resource="http://purl.bioontology.org/ontology/BCTT#Credible_source"/>
        <EmpowerBP:hasMostCommonBCT rdf:resource="http://purl.bioontology.org/ontology/BCTT#Feedback_on_behaviour"/>
        <EmpowerBP:hasMostCommonBCT rdf:resource="http://purl.bioontology.org/ontology/BCTT#Information_about_health_consequences"/>
        <EmpowerBP:hasMostCommonBCT rdf:resource="http://purl.bioontology.org/ontology/BCTT#Information_about_social_and_environmental_consequences"/>
        <EmpowerBP:hasMostCommonBCT rdf:resource="http://purl.bioontology.org/ontology/BCTT#Feedback_on_outcome(s)_of_behavior"/>
        <EmpowerBP:isEffectiveForTDFDomain rdf:resource="http://www.semanticweb.org/tswheeler/ontologies/2016/3/EmpowerBP#BeliefsAboutCapability"/>
        <EmpowerBP:isEffectiveForTDFDomain rdf:resource="http://www.semanticweb.org/tswheeler/ontologies/2016/3/EmpowerBP#BeliefsAboutConsequences"/>
        <EmpowerBP:isEffectiveForTDFDomain rdf:resource="http://www.semanticweb.org/tswheeler/ontologies/2016/3/EmpowerBP#Emotion"/>
        <EmpowerBP:isEffectiveForTDFDomain rdf:resource="http://www.semanticweb.org/tswheeler/ontologies/2016/3/EmpowerBP#Goals"/>
        <EmpowerBP:isEffectiveForTDFDomain rdf:resource="http://www.semanticweb.org/tswheeler/ontologies/2016/3/EmpowerBP#Intentions"/>
        <EmpowerBP:isEffectiveForTDFDomain rdf:resource="http://www.semanticweb.org/tswheeler/ontologies/2016/3/EmpowerBP#Optimism"/>
        <EmpowerBP:isEffectiveForTDFDomain rdf:resource="http://www.semanticweb.org/tswheeler/ontologies/2016/3/EmpowerBP#ProfessionalSocialRoleIdentity"/>
        <rdfs:comment>Using communication to induce positive or negative feelings or stimulate action.</rdfs:comment>
    </owl:NamedIndividual>
    


    <!-- http://www.semanticweb.org/tswheeler/ontologies/2016/3/EmpowerBP#PhysicalCapability -->

    <owl:NamedIndividual rdf:about="http://www.semanticweb.org/tswheeler/ontologies/2016/3/EmpowerBP#PhysicalCapability">
        <rdf:type rdf:resource="http://www.semanticweb.org/tswheeler/ontologies/2016/3/EmpowerBP#COMBConstruct"/>
        <rdf:type rdf:resource="http://www.semanticweb.org/tswheeler/ontologies/2016/3/EmpowerBP#Capability"/>
        <rdf:type rdf:resource="http://www.semanticweb.org/tswheeler/ontologies/2016/3/EmpowerBP#Construct"/>
        <EmpowerBP:isRelatedToTDF rdf:resource="http://www.semanticweb.org/tswheeler/ontologies/2016/3/EmpowerBP#PhysicalSkill"/>
        <rdfs:comment>Having the physical skills, strength or stamina to perform a behaviour</rdfs:comment>
    </owl:NamedIndividual>
    


    <!-- http://www.semanticweb.org/tswheeler/ontologies/2016/3/EmpowerBP#PhysicalHealthObstacle -->

    <owl:NamedIndividual rdf:about="http://www.semanticweb.org/tswheeler/ontologies/2016/3/EmpowerBP#PhysicalHealthObstacle">
        <rdf:type rdf:resource="http://www.semanticweb.org/tswheeler/ontologies/2016/3/EmpowerBP#Obstacle"/>
        <EmpowerBP:hasRelevantTDF rdf:resource="http://www.semanticweb.org/tswheeler/ontologies/2016/3/EmpowerBP#BeliefsAboutCapability"/>
        <EmpowerBP:hasRelevantTDF rdf:resource="http://www.semanticweb.org/tswheeler/ontologies/2016/3/EmpowerBP#EnvironmentalContextResources"/>
        <EmpowerBP:hasRelevantTDF rdf:resource="http://www.semanticweb.org/tswheeler/ontologies/2016/3/EmpowerBP#PhysicalSkill"/>
        <rdfs:comment>Feels they are physically unable to perform activity.</rdfs:comment>
    </owl:NamedIndividual>
    


    <!-- http://www.semanticweb.org/tswheeler/ontologies/2016/3/EmpowerBP#PhysicalOpportunity -->

    <owl:NamedIndividual rdf:about="http://www.semanticweb.org/tswheeler/ontologies/2016/3/EmpowerBP#PhysicalOpportunity">
        <rdf:type rdf:resource="http://www.semanticweb.org/tswheeler/ontologies/2016/3/EmpowerBP#COMBConstruct"/>
        <rdf:type rdf:resource="http://www.semanticweb.org/tswheeler/ontologies/2016/3/EmpowerBP#Construct"/>
        <rdf:type rdf:resource="http://www.semanticweb.org/tswheeler/ontologies/2016/3/EmpowerBP#Opportunity"/>
        <EmpowerBP:isRelatedToTDF rdf:resource="http://www.semanticweb.org/tswheeler/ontologies/2016/3/EmpowerBP#EnvironmentalContextResources"/>
        <rdfs:comment>What the environment allows or facilitates in terms of time, triggers, resources, locations, physical barriers, etc.</rdfs:comment>
    </owl:NamedIndividual>
    


    <!-- http://www.semanticweb.org/tswheeler/ontologies/2016/3/EmpowerBP#PhysicalSkill -->

    <owl:NamedIndividual rdf:about="http://www.semanticweb.org/tswheeler/ontologies/2016/3/EmpowerBP#PhysicalSkill">
        <rdf:type rdf:resource="http://www.semanticweb.org/tswheeler/ontologies/2016/3/EmpowerBP#Construct"/>
        <rdf:type rdf:resource="http://www.semanticweb.org/tswheeler/ontologies/2016/3/EmpowerBP#TDFDomain"/>
        <EmpowerBP:hasEffectiveInterventionFunction rdf:resource="http://www.semanticweb.org/tswheeler/ontologies/2016/3/EmpowerBP#Training"/>
        <EmpowerBP:isRelatedToCOMB rdf:resource="http://www.semanticweb.org/tswheeler/ontologies/2016/3/EmpowerBP#PhysicalCapability"/>
        <rdfs:comment>A physical ability or proficiency acquired through practice</rdfs:comment>
    </owl:NamedIndividual>
    


    <!-- http://www.semanticweb.org/tswheeler/ontologies/2016/3/EmpowerBP#ProfessionalSocialRoleIdentity -->

    <owl:NamedIndividual rdf:about="http://www.semanticweb.org/tswheeler/ontologies/2016/3/EmpowerBP#ProfessionalSocialRoleIdentity">
        <rdf:type rdf:resource="http://www.semanticweb.org/tswheeler/ontologies/2016/3/EmpowerBP#Construct"/>
        <rdf:type rdf:resource="http://www.semanticweb.org/tswheeler/ontologies/2016/3/EmpowerBP#TDFDomain"/>
        <EmpowerBP:hasEffectiveInterventionFunction rdf:resource="http://www.semanticweb.org/tswheeler/ontologies/2016/3/EmpowerBP#Education"/>
        <EmpowerBP:hasEffectiveInterventionFunction rdf:resource="http://www.semanticweb.org/tswheeler/ontologies/2016/3/EmpowerBP#Modelling"/>
        <EmpowerBP:hasEffectiveInterventionFunction rdf:resource="http://www.semanticweb.org/tswheeler/ontologies/2016/3/EmpowerBP#Persuasion"/>
        <EmpowerBP:isRelatedToCOMB rdf:resource="http://www.semanticweb.org/tswheeler/ontologies/2016/3/EmpowerBP#ReflectiveMotivation"/>
        <rdfs:comment>A coherent set of behaviors and displayed personal qualities of an individual in a social or work setting</rdfs:comment>
        <rdfs:label>Professional/Social Role and Identity</rdfs:label>
    </owl:NamedIndividual>
    


    <!-- http://www.semanticweb.org/tswheeler/ontologies/2016/3/EmpowerBP#PsychologicalCapability -->

    <owl:NamedIndividual rdf:about="http://www.semanticweb.org/tswheeler/ontologies/2016/3/EmpowerBP#PsychologicalCapability">
        <rdf:type rdf:resource="http://www.semanticweb.org/tswheeler/ontologies/2016/3/EmpowerBP#COMBConstruct"/>
        <rdf:type rdf:resource="http://www.semanticweb.org/tswheeler/ontologies/2016/3/EmpowerBP#Capability"/>
        <rdf:type rdf:resource="http://www.semanticweb.org/tswheeler/ontologies/2016/3/EmpowerBP#Construct"/>
        <EmpowerBP:isRelatedToTDF rdf:resource="http://www.semanticweb.org/tswheeler/ontologies/2016/3/EmpowerBP#BehaviouralRegulation"/>
        <EmpowerBP:isRelatedToTDF rdf:resource="http://www.semanticweb.org/tswheeler/ontologies/2016/3/EmpowerBP#CognitiveInterpersonalSkills"/>
        <EmpowerBP:isRelatedToTDF rdf:resource="http://www.semanticweb.org/tswheeler/ontologies/2016/3/EmpowerBP#Knowledge"/>
        <EmpowerBP:isRelatedToTDF rdf:resource="http://www.semanticweb.org/tswheeler/ontologies/2016/3/EmpowerBP#MemoryAttentionDecisionProcesses"/>
        <rdfs:comment>Having the knowledge, psychological skills, strength or stamina to perform a behaviour</rdfs:comment>
    </owl:NamedIndividual>
    


    <!-- http://www.semanticweb.org/tswheeler/ontologies/2016/3/EmpowerBP#R1 -->

    <owl:NamedIndividual rdf:about="http://www.semanticweb.org/tswheeler/ontologies/2016/3/EmpowerBP#R1">
        <rdf:type rdf:resource="http://www.semanticweb.org/tswheeler/ontologies/2016/3/EmpowerBP#InterventionItem"/>
        <rdf:type rdf:resource="http://www.semanticweb.org/tswheeler/ontologies/2016/3/EmpowerBP#Resource"/>
        <EmpowerBP:isAppropriateForInterventionGoal rdf:resource="http://www.semanticweb.org/tswheeler/ontologies/2016/3/EmpowerBP#ExerciseMore"/>
        <EmpowerBP:appropriateForAutomaticMotivation rdf:datatype="http://www.w3.org/2001/XMLSchema#integer">3</EmpowerBP:appropriateForAutomaticMotivation>
        <EmpowerBP:appropriateForLocation rdf:datatype="http://www.w3.org/2001/XMLSchema#integer">0</EmpowerBP:appropriateForLocation>
        <EmpowerBP:appropriateForPhysicalCapability rdf:datatype="http://www.w3.org/2001/XMLSchema#integer">3</EmpowerBP:appropriateForPhysicalCapability>
        <EmpowerBP:appropriateForPhysicalOpportunity rdf:datatype="http://www.w3.org/2001/XMLSchema#integer">3</EmpowerBP:appropriateForPhysicalOpportunity>
        <EmpowerBP:appropriateForPsychologicalCapability rdf:datatype="http://www.w3.org/2001/XMLSchema#integer">3</EmpowerBP:appropriateForPsychologicalCapability>
        <EmpowerBP:appropriateForReflectiveMotivation rdf:datatype="http://www.w3.org/2001/XMLSchema#integer">3</EmpowerBP:appropriateForReflectiveMotivation>
        <EmpowerBP:appropriateForSocialOpportunity rdf:datatype="http://www.w3.org/2001/XMLSchema#integer">3</EmpowerBP:appropriateForSocialOpportunity>
        <EmpowerBP:itemName rdf:datatype="http://www.w3.org/2001/XMLSchema#string">Hike Canada</EmpowerBP:itemName>
        <EmpowerBP:itemText rdf:datatype="http://www.w3.org/2001/XMLSchema#string">Looking for a place to place to go walking? Check out Hike Canada and look for a trail near you. </EmpowerBP:itemText>
        <EmpowerBP:maximumUserAge rdf:datatype="http://www.w3.org/2001/XMLSchema#integer">120</EmpowerBP:maximumUserAge>
        <EmpowerBP:minimumUserAge rdf:datatype="http://www.w3.org/2001/XMLSchema#integer">18</EmpowerBP:minimumUserAge>
        <EmpowerBP:provideLink rdf:datatype="http://www.w3.org/2001/XMLSchema#boolean">true</EmpowerBP:provideLink>
        <EmpowerBP:sourceURL rdf:datatype="http://www.w3.org/2001/XMLSchema#string">http://www.hikecanada.org/en</EmpowerBP:sourceURL>
        <rdfs:comment rdf:datatype="http://www.w3.org/2001/XMLSchema#string">Looking for a place to place to go walking? Check out Hike Canada and look for a trail near you. </rdfs:comment>
        <rdfs:label rdf:datatype="http://www.w3.org/2001/XMLSchema#string">Hike Canada</rdfs:label>
    </owl:NamedIndividual>
    


    <!-- http://www.semanticweb.org/tswheeler/ontologies/2016/3/EmpowerBP#R10 -->

    <owl:NamedIndividual rdf:about="http://www.semanticweb.org/tswheeler/ontologies/2016/3/EmpowerBP#R10">
        <rdf:type rdf:resource="http://www.semanticweb.org/tswheeler/ontologies/2016/3/EmpowerBP#InterventionItem"/>
        <rdf:type rdf:resource="http://www.semanticweb.org/tswheeler/ontologies/2016/3/EmpowerBP#Resource"/>
        <EmpowerBP:isAppropriateForInterventionGoal rdf:resource="http://www.semanticweb.org/tswheeler/ontologies/2016/3/EmpowerBP#ReduceSaltIntake"/>
        <EmpowerBP:appropriateForAutomaticMotivation rdf:datatype="http://www.w3.org/2001/XMLSchema#integer">3</EmpowerBP:appropriateForAutomaticMotivation>
        <EmpowerBP:appropriateForLocation rdf:datatype="http://www.w3.org/2001/XMLSchema#integer">0</EmpowerBP:appropriateForLocation>
        <EmpowerBP:appropriateForPhysicalCapability rdf:datatype="http://www.w3.org/2001/XMLSchema#integer">3</EmpowerBP:appropriateForPhysicalCapability>
        <EmpowerBP:appropriateForPhysicalOpportunity rdf:datatype="http://www.w3.org/2001/XMLSchema#integer">3</EmpowerBP:appropriateForPhysicalOpportunity>
        <EmpowerBP:appropriateForPsychologicalCapability rdf:datatype="http://www.w3.org/2001/XMLSchema#integer">3</EmpowerBP:appropriateForPsychologicalCapability>
        <EmpowerBP:appropriateForReflectiveMotivation rdf:datatype="http://www.w3.org/2001/XMLSchema#integer">3</EmpowerBP:appropriateForReflectiveMotivation>
        <EmpowerBP:appropriateForSocialOpportunity rdf:datatype="http://www.w3.org/2001/XMLSchema#integer">3</EmpowerBP:appropriateForSocialOpportunity>
        <EmpowerBP:itemName rdf:datatype="http://www.w3.org/2001/XMLSchema#string">Government of Canada – Healthy Eating</EmpowerBP:itemName>
        <EmpowerBP:itemText rdf:datatype="http://www.w3.org/2001/XMLSchema#string">Health Canada provides tips for healthy eating, information on food allergies, safety standards and labels. Also learn about recalls and how Canada monitors and measures food consumption.</EmpowerBP:itemText>
        <EmpowerBP:maximumUserAge rdf:datatype="http://www.w3.org/2001/XMLSchema#integer">120</EmpowerBP:maximumUserAge>
        <EmpowerBP:minimumUserAge rdf:datatype="http://www.w3.org/2001/XMLSchema#integer">18</EmpowerBP:minimumUserAge>
        <EmpowerBP:provideLink rdf:datatype="http://www.w3.org/2001/XMLSchema#boolean">true</EmpowerBP:provideLink>
        <EmpowerBP:sourceURL rdf:datatype="http://www.w3.org/2001/XMLSchema#string">https://www.canada.ca/en/services/health/healthy-eating.html</EmpowerBP:sourceURL>
        <rdfs:comment rdf:datatype="http://www.w3.org/2001/XMLSchema#string">Health Canada provides tips for healthy eating, information on food allergies, safety standards and labels. Also learn about recalls and how Canada monitors and measures food consumption.</rdfs:comment>
        <rdfs:label rdf:datatype="http://www.w3.org/2001/XMLSchema#string">Government of Canada – Healthy Eating</rdfs:label>
    </owl:NamedIndividual>
    


    <!-- http://www.semanticweb.org/tswheeler/ontologies/2016/3/EmpowerBP#R11 -->

    <owl:NamedIndividual rdf:about="http://www.semanticweb.org/tswheeler/ontologies/2016/3/EmpowerBP#R11">
        <rdf:type rdf:resource="http://www.semanticweb.org/tswheeler/ontologies/2016/3/EmpowerBP#InterventionItem"/>
        <rdf:type rdf:resource="http://www.semanticweb.org/tswheeler/ontologies/2016/3/EmpowerBP#Resource"/>
        <EmpowerBP:isAppropriateForInterventionGoal rdf:resource="http://www.semanticweb.org/tswheeler/ontologies/2016/3/EmpowerBP#ReduceSaltIntake"/>
        <EmpowerBP:appropriateForAutomaticMotivation rdf:datatype="http://www.w3.org/2001/XMLSchema#integer">3</EmpowerBP:appropriateForAutomaticMotivation>
        <EmpowerBP:appropriateForLocation rdf:datatype="http://www.w3.org/2001/XMLSchema#integer">0</EmpowerBP:appropriateForLocation>
        <EmpowerBP:appropriateForPhysicalCapability rdf:datatype="http://www.w3.org/2001/XMLSchema#integer">3</EmpowerBP:appropriateForPhysicalCapability>
        <EmpowerBP:appropriateForPhysicalOpportunity rdf:datatype="http://www.w3.org/2001/XMLSchema#integer">3</EmpowerBP:appropriateForPhysicalOpportunity>
        <EmpowerBP:appropriateForPsychologicalCapability rdf:datatype="http://www.w3.org/2001/XMLSchema#integer">3</EmpowerBP:appropriateForPsychologicalCapability>
        <EmpowerBP:appropriateForReflectiveMotivation rdf:datatype="http://www.w3.org/2001/XMLSchema#integer">3</EmpowerBP:appropriateForReflectiveMotivation>
        <EmpowerBP:appropriateForSocialOpportunity rdf:datatype="http://www.w3.org/2001/XMLSchema#integer">3</EmpowerBP:appropriateForSocialOpportunity>
        <EmpowerBP:itemName rdf:datatype="http://www.w3.org/2001/XMLSchema#string">My Food Guide Mobile App</EmpowerBP:itemName>
        <EmpowerBP:itemText rdf:datatype="http://www.w3.org/2001/XMLSchema#string">The My Food Guide mobile app gives you access to healthy eating information anytime, anywhere. Simply select your age, sex and food preferences to get your own customized Food Guide.</EmpowerBP:itemText>
        <EmpowerBP:maximumUserAge rdf:datatype="http://www.w3.org/2001/XMLSchema#integer">120</EmpowerBP:maximumUserAge>
        <EmpowerBP:minimumUserAge rdf:datatype="http://www.w3.org/2001/XMLSchema#integer">18</EmpowerBP:minimumUserAge>
        <EmpowerBP:provideLink rdf:datatype="http://www.w3.org/2001/XMLSchema#boolean">true</EmpowerBP:provideLink>
        <EmpowerBP:sourceURL rdf:datatype="http://www.w3.org/2001/XMLSchema#string">http://www.healthycanadians.gc.ca/eating-nutrition/healthy-eating-saine-alimentation/food-guide-aliment/my-guide-mon-guide/index-eng.php</EmpowerBP:sourceURL>
        <rdfs:comment rdf:datatype="http://www.w3.org/2001/XMLSchema#string">The My Food Guide mobile app gives you access to healthy eating information anytime, anywhere. Simply select your age, sex and food preferences to get your own customized Food Guide.</rdfs:comment>
        <rdfs:label rdf:datatype="http://www.w3.org/2001/XMLSchema#string">My Food Guide Mobile App</rdfs:label>
    </owl:NamedIndividual>
    


    <!-- http://www.semanticweb.org/tswheeler/ontologies/2016/3/EmpowerBP#R12 -->

    <owl:NamedIndividual rdf:about="http://www.semanticweb.org/tswheeler/ontologies/2016/3/EmpowerBP#R12">
        <rdf:type rdf:resource="http://www.semanticweb.org/tswheeler/ontologies/2016/3/EmpowerBP#InterventionItem"/>
        <rdf:type rdf:resource="http://www.semanticweb.org/tswheeler/ontologies/2016/3/EmpowerBP#Resource"/>
        <EmpowerBP:isAppropriateForInterventionGoal rdf:resource="http://www.semanticweb.org/tswheeler/ontologies/2016/3/EmpowerBP#ReduceSaltIntake"/>
        <EmpowerBP:appropriateForAutomaticMotivation rdf:datatype="http://www.w3.org/2001/XMLSchema#integer">3</EmpowerBP:appropriateForAutomaticMotivation>
        <EmpowerBP:appropriateForLocation rdf:datatype="http://www.w3.org/2001/XMLSchema#integer">0</EmpowerBP:appropriateForLocation>
        <EmpowerBP:appropriateForPhysicalCapability rdf:datatype="http://www.w3.org/2001/XMLSchema#integer">3</EmpowerBP:appropriateForPhysicalCapability>
        <EmpowerBP:appropriateForPhysicalOpportunity rdf:datatype="http://www.w3.org/2001/XMLSchema#integer">3</EmpowerBP:appropriateForPhysicalOpportunity>
        <EmpowerBP:appropriateForPsychologicalCapability rdf:datatype="http://www.w3.org/2001/XMLSchema#integer">3</EmpowerBP:appropriateForPsychologicalCapability>
        <EmpowerBP:appropriateForReflectiveMotivation rdf:datatype="http://www.w3.org/2001/XMLSchema#integer">3</EmpowerBP:appropriateForReflectiveMotivation>
        <EmpowerBP:appropriateForSocialOpportunity rdf:datatype="http://www.w3.org/2001/XMLSchema#integer">3</EmpowerBP:appropriateForSocialOpportunity>
        <EmpowerBP:itemName rdf:datatype="http://www.w3.org/2001/XMLSchema#string">Eat Well Recipes</EmpowerBP:itemName>
        <EmpowerBP:itemText rdf:datatype="http://www.w3.org/2001/XMLSchema#string">Find healthy recipes for every season, submitted by other Canadians</EmpowerBP:itemText>
        <EmpowerBP:maximumUserAge rdf:datatype="http://www.w3.org/2001/XMLSchema#integer">120</EmpowerBP:maximumUserAge>
        <EmpowerBP:minimumUserAge rdf:datatype="http://www.w3.org/2001/XMLSchema#integer">18</EmpowerBP:minimumUserAge>
        <EmpowerBP:provideLink rdf:datatype="http://www.w3.org/2001/XMLSchema#boolean">true</EmpowerBP:provideLink>
        <EmpowerBP:sourceURL rdf:datatype="http://www.w3.org/2001/XMLSchema#string">https://www.canada.ca/en/health-canada/services/tips-healthy-eating/eat-well-recipes.html</EmpowerBP:sourceURL>
        <rdfs:comment rdf:datatype="http://www.w3.org/2001/XMLSchema#string">Find healthy recipes for every season, submitted by other Canadians</rdfs:comment>
        <rdfs:label rdf:datatype="http://www.w3.org/2001/XMLSchema#string">Eat Well Recipes</rdfs:label>
    </owl:NamedIndividual>
    


    <!-- http://www.semanticweb.org/tswheeler/ontologies/2016/3/EmpowerBP#R13 -->

    <owl:NamedIndividual rdf:about="http://www.semanticweb.org/tswheeler/ontologies/2016/3/EmpowerBP#R13">
        <rdf:type rdf:resource="http://www.semanticweb.org/tswheeler/ontologies/2016/3/EmpowerBP#InterventionItem"/>
        <rdf:type rdf:resource="http://www.semanticweb.org/tswheeler/ontologies/2016/3/EmpowerBP#Resource"/>
        <EmpowerBP:isAppropriateForInterventionGoal rdf:resource="http://www.semanticweb.org/tswheeler/ontologies/2016/3/EmpowerBP#ReduceSaltIntake"/>
        <EmpowerBP:appropriateForAutomaticMotivation rdf:datatype="http://www.w3.org/2001/XMLSchema#integer">3</EmpowerBP:appropriateForAutomaticMotivation>
        <EmpowerBP:appropriateForLocation rdf:datatype="http://www.w3.org/2001/XMLSchema#integer">0</EmpowerBP:appropriateForLocation>
        <EmpowerBP:appropriateForPhysicalCapability rdf:datatype="http://www.w3.org/2001/XMLSchema#integer">3</EmpowerBP:appropriateForPhysicalCapability>
        <EmpowerBP:appropriateForPhysicalOpportunity rdf:datatype="http://www.w3.org/2001/XMLSchema#integer">3</EmpowerBP:appropriateForPhysicalOpportunity>
        <EmpowerBP:appropriateForPsychologicalCapability rdf:datatype="http://www.w3.org/2001/XMLSchema#integer">3</EmpowerBP:appropriateForPsychologicalCapability>
        <EmpowerBP:appropriateForReflectiveMotivation rdf:datatype="http://www.w3.org/2001/XMLSchema#integer">3</EmpowerBP:appropriateForReflectiveMotivation>
        <EmpowerBP:appropriateForSocialOpportunity rdf:datatype="http://www.w3.org/2001/XMLSchema#integer">3</EmpowerBP:appropriateForSocialOpportunity>
        <EmpowerBP:itemName rdf:datatype="http://www.w3.org/2001/XMLSchema#string">In Brief: DASH Diet </EmpowerBP:itemName>
        <EmpowerBP:itemText rdf:datatype="http://www.w3.org/2001/XMLSchema#string">An easy-to-read fact sheet about the DASH diet. Includes an overview of DASH research findings and suggestions on how to start and stay on the eating plan.</EmpowerBP:itemText>
        <EmpowerBP:maximumUserAge rdf:datatype="http://www.w3.org/2001/XMLSchema#integer">120</EmpowerBP:maximumUserAge>
        <EmpowerBP:minimumUserAge rdf:datatype="http://www.w3.org/2001/XMLSchema#integer">18</EmpowerBP:minimumUserAge>
        <EmpowerBP:provideLink rdf:datatype="http://www.w3.org/2001/XMLSchema#boolean">true</EmpowerBP:provideLink>
        <EmpowerBP:sourceURL rdf:datatype="http://www.w3.org/2001/XMLSchema#string">https://www.nhlbi.nih.gov/health/resources/heart/hbp-dash-in-brief-html</EmpowerBP:sourceURL>
        <rdfs:comment rdf:datatype="http://www.w3.org/2001/XMLSchema#string">An easy-to-read fact sheet about the DASH diet. Includes an overview of DASH research findings and suggestions on how to start and stay on the eating plan.</rdfs:comment>
        <rdfs:label rdf:datatype="http://www.w3.org/2001/XMLSchema#string">In Brief: DASH Diet </rdfs:label>
    </owl:NamedIndividual>
    


    <!-- http://www.semanticweb.org/tswheeler/ontologies/2016/3/EmpowerBP#R14 -->

    <owl:NamedIndividual rdf:about="http://www.semanticweb.org/tswheeler/ontologies/2016/3/EmpowerBP#R14">
        <rdf:type rdf:resource="http://www.semanticweb.org/tswheeler/ontologies/2016/3/EmpowerBP#InterventionItem"/>
        <rdf:type rdf:resource="http://www.semanticweb.org/tswheeler/ontologies/2016/3/EmpowerBP#Resource"/>
        <EmpowerBP:isAppropriateForInterventionGoal rdf:resource="http://www.semanticweb.org/tswheeler/ontologies/2016/3/EmpowerBP#ReduceSaltIntake"/>
        <EmpowerBP:appropriateForAutomaticMotivation rdf:datatype="http://www.w3.org/2001/XMLSchema#integer">3</EmpowerBP:appropriateForAutomaticMotivation>
        <EmpowerBP:appropriateForLocation rdf:datatype="http://www.w3.org/2001/XMLSchema#integer">0</EmpowerBP:appropriateForLocation>
        <EmpowerBP:appropriateForPhysicalCapability rdf:datatype="http://www.w3.org/2001/XMLSchema#integer">3</EmpowerBP:appropriateForPhysicalCapability>
        <EmpowerBP:appropriateForPhysicalOpportunity rdf:datatype="http://www.w3.org/2001/XMLSchema#integer">3</EmpowerBP:appropriateForPhysicalOpportunity>
        <EmpowerBP:appropriateForPsychologicalCapability rdf:datatype="http://www.w3.org/2001/XMLSchema#integer">3</EmpowerBP:appropriateForPsychologicalCapability>
        <EmpowerBP:appropriateForReflectiveMotivation rdf:datatype="http://www.w3.org/2001/XMLSchema#integer">3</EmpowerBP:appropriateForReflectiveMotivation>
        <EmpowerBP:appropriateForSocialOpportunity rdf:datatype="http://www.w3.org/2001/XMLSchema#integer">3</EmpowerBP:appropriateForSocialOpportunity>
        <EmpowerBP:itemName rdf:datatype="http://www.w3.org/2001/XMLSchema#string">BigLife Sodium Calculator</EmpowerBP:itemName>
        <EmpowerBP:itemText rdf:datatype="http://www.w3.org/2001/XMLSchema#string">
All salt has a lot of sodium and it is in most of the foods we eat – a lot in some and a little in others. Answering the following questions will help you determine how much sodium you consume each day.</EmpowerBP:itemText>
        <EmpowerBP:maximumUserAge rdf:datatype="http://www.w3.org/2001/XMLSchema#integer">120</EmpowerBP:maximumUserAge>
        <EmpowerBP:minimumUserAge rdf:datatype="http://www.w3.org/2001/XMLSchema#integer">18</EmpowerBP:minimumUserAge>
        <EmpowerBP:provideLink rdf:datatype="http://www.w3.org/2001/XMLSchema#boolean">true</EmpowerBP:provideLink>
        <EmpowerBP:sourceURL rdf:datatype="http://www.w3.org/2001/XMLSchema#string">http://www.projectbiglife.ca/sodium/</EmpowerBP:sourceURL>
        <rdfs:comment rdf:datatype="http://www.w3.org/2001/XMLSchema#string">
All salt has a lot of sodium and it is in most of the foods we eat – a lot in some and a little in others. Answering the following questions will help you determine how much sodium you consume each day.</rdfs:comment>
        <rdfs:label rdf:datatype="http://www.w3.org/2001/XMLSchema#string">BigLife Sodium Calculator</rdfs:label>
    </owl:NamedIndividual>
    


    <!-- http://www.semanticweb.org/tswheeler/ontologies/2016/3/EmpowerBP#R2 -->

    <owl:NamedIndividual rdf:about="http://www.semanticweb.org/tswheeler/ontologies/2016/3/EmpowerBP#R2">
        <rdf:type rdf:resource="http://www.semanticweb.org/tswheeler/ontologies/2016/3/EmpowerBP#InterventionItem"/>
        <rdf:type rdf:resource="http://www.semanticweb.org/tswheeler/ontologies/2016/3/EmpowerBP#Resource"/>
        <EmpowerBP:isAppropriateForInterventionGoal rdf:resource="http://www.semanticweb.org/tswheeler/ontologies/2016/3/EmpowerBP#ExerciseMore"/>
        <EmpowerBP:appropriateForAutomaticMotivation rdf:datatype="http://www.w3.org/2001/XMLSchema#integer">3</EmpowerBP:appropriateForAutomaticMotivation>
        <EmpowerBP:appropriateForLocation rdf:datatype="http://www.w3.org/2001/XMLSchema#integer">6</EmpowerBP:appropriateForLocation>
        <EmpowerBP:appropriateForPhysicalCapability rdf:datatype="http://www.w3.org/2001/XMLSchema#integer">3</EmpowerBP:appropriateForPhysicalCapability>
        <EmpowerBP:appropriateForPhysicalOpportunity rdf:datatype="http://www.w3.org/2001/XMLSchema#integer">3</EmpowerBP:appropriateForPhysicalOpportunity>
        <EmpowerBP:appropriateForPsychologicalCapability rdf:datatype="http://www.w3.org/2001/XMLSchema#integer">3</EmpowerBP:appropriateForPsychologicalCapability>
        <EmpowerBP:appropriateForReflectiveMotivation rdf:datatype="http://www.w3.org/2001/XMLSchema#integer">3</EmpowerBP:appropriateForReflectiveMotivation>
        <EmpowerBP:appropriateForSocialOpportunity rdf:datatype="http://www.w3.org/2001/XMLSchema#integer">3</EmpowerBP:appropriateForSocialOpportunity>
        <EmpowerBP:itemName rdf:datatype="http://www.w3.org/2001/XMLSchema#string">Hike Nova Scotia</EmpowerBP:itemName>
        <EmpowerBP:itemText rdf:datatype="http://www.w3.org/2001/XMLSchema#string">Looking for a place to place to go walking? Check out Hike Nova Scotia and look for a trail near you. </EmpowerBP:itemText>
        <EmpowerBP:maximumUserAge rdf:datatype="http://www.w3.org/2001/XMLSchema#integer">120</EmpowerBP:maximumUserAge>
        <EmpowerBP:minimumUserAge rdf:datatype="http://www.w3.org/2001/XMLSchema#integer">18</EmpowerBP:minimumUserAge>
        <EmpowerBP:provideLink rdf:datatype="http://www.w3.org/2001/XMLSchema#boolean">true</EmpowerBP:provideLink>
        <EmpowerBP:sourceURL rdf:datatype="http://www.w3.org/2001/XMLSchema#string">http://www.hikenovascotia.ca</EmpowerBP:sourceURL>
        <rdfs:comment rdf:datatype="http://www.w3.org/2001/XMLSchema#string">Looking for a place to place to go walking? Check out Hike Nova Scotia and look for a trail near you. </rdfs:comment>
        <rdfs:label rdf:datatype="http://www.w3.org/2001/XMLSchema#string">Hike Nova Scotia</rdfs:label>
    </owl:NamedIndividual>
    


    <!-- http://www.semanticweb.org/tswheeler/ontologies/2016/3/EmpowerBP#R3 -->

    <owl:NamedIndividual rdf:about="http://www.semanticweb.org/tswheeler/ontologies/2016/3/EmpowerBP#R3">
        <rdf:type rdf:resource="http://www.semanticweb.org/tswheeler/ontologies/2016/3/EmpowerBP#InterventionItem"/>
        <rdf:type rdf:resource="http://www.semanticweb.org/tswheeler/ontologies/2016/3/EmpowerBP#Resource"/>
        <EmpowerBP:isAppropriateForInterventionGoal rdf:resource="http://www.semanticweb.org/tswheeler/ontologies/2016/3/EmpowerBP#ReduceSaltIntake"/>
        <EmpowerBP:appropriateForAutomaticMotivation rdf:datatype="http://www.w3.org/2001/XMLSchema#integer">3</EmpowerBP:appropriateForAutomaticMotivation>
        <EmpowerBP:appropriateForLocation rdf:datatype="http://www.w3.org/2001/XMLSchema#integer">0</EmpowerBP:appropriateForLocation>
        <EmpowerBP:appropriateForPhysicalCapability rdf:datatype="http://www.w3.org/2001/XMLSchema#integer">3</EmpowerBP:appropriateForPhysicalCapability>
        <EmpowerBP:appropriateForPhysicalOpportunity rdf:datatype="http://www.w3.org/2001/XMLSchema#integer">3</EmpowerBP:appropriateForPhysicalOpportunity>
        <EmpowerBP:appropriateForPsychologicalCapability rdf:datatype="http://www.w3.org/2001/XMLSchema#integer">3</EmpowerBP:appropriateForPsychologicalCapability>
        <EmpowerBP:appropriateForReflectiveMotivation rdf:datatype="http://www.w3.org/2001/XMLSchema#integer">3</EmpowerBP:appropriateForReflectiveMotivation>
        <EmpowerBP:appropriateForSocialOpportunity rdf:datatype="http://www.w3.org/2001/XMLSchema#integer">3</EmpowerBP:appropriateForSocialOpportunity>
        <EmpowerBP:itemName rdf:datatype="http://www.w3.org/2001/XMLSchema#string">Cookspiration</EmpowerBP:itemName>
        <EmpowerBP:itemText rdf:datatype="http://www.w3.org/2001/XMLSchema#string">Need help planning a healthy meal? Find dietitian-approved recipes on the Cookspiration web site with recipe ideas to suite your mood and schedule. Also available as a mobile app!</EmpowerBP:itemText>
        <EmpowerBP:maximumUserAge rdf:datatype="http://www.w3.org/2001/XMLSchema#integer">120</EmpowerBP:maximumUserAge>
        <EmpowerBP:minimumUserAge rdf:datatype="http://www.w3.org/2001/XMLSchema#integer">18</EmpowerBP:minimumUserAge>
        <EmpowerBP:provideLink rdf:datatype="http://www.w3.org/2001/XMLSchema#boolean">true</EmpowerBP:provideLink>
        <EmpowerBP:sourceURL rdf:datatype="http://www.w3.org/2001/XMLSchema#string">http://www.cookspiration.com</EmpowerBP:sourceURL>
        <rdfs:comment rdf:datatype="http://www.w3.org/2001/XMLSchema#string">Need help planning a healthy meal? Find dietitian-approved recipes on the Cookspiration web site with recipe ideas to suite your mood and schedule. Also available as a mobile app!</rdfs:comment>
        <rdfs:label rdf:datatype="http://www.w3.org/2001/XMLSchema#string">Cookspiration</rdfs:label>
    </owl:NamedIndividual>
    


    <!-- http://www.semanticweb.org/tswheeler/ontologies/2016/3/EmpowerBP#R4 -->

    <owl:NamedIndividual rdf:about="http://www.semanticweb.org/tswheeler/ontologies/2016/3/EmpowerBP#R4">
        <rdf:type rdf:resource="http://www.semanticweb.org/tswheeler/ontologies/2016/3/EmpowerBP#InterventionItem"/>
        <rdf:type rdf:resource="http://www.semanticweb.org/tswheeler/ontologies/2016/3/EmpowerBP#Resource"/>
        <EmpowerBP:isAppropriateForInterventionGoal rdf:resource="http://www.semanticweb.org/tswheeler/ontologies/2016/3/EmpowerBP#ReduceSaltIntake"/>
        <EmpowerBP:appropriateForAutomaticMotivation rdf:datatype="http://www.w3.org/2001/XMLSchema#integer">3</EmpowerBP:appropriateForAutomaticMotivation>
        <EmpowerBP:appropriateForLocation rdf:datatype="http://www.w3.org/2001/XMLSchema#integer">0</EmpowerBP:appropriateForLocation>
        <EmpowerBP:appropriateForPhysicalCapability rdf:datatype="http://www.w3.org/2001/XMLSchema#integer">3</EmpowerBP:appropriateForPhysicalCapability>
        <EmpowerBP:appropriateForPhysicalOpportunity rdf:datatype="http://www.w3.org/2001/XMLSchema#integer">3</EmpowerBP:appropriateForPhysicalOpportunity>
        <EmpowerBP:appropriateForPsychologicalCapability rdf:datatype="http://www.w3.org/2001/XMLSchema#integer">3</EmpowerBP:appropriateForPsychologicalCapability>
        <EmpowerBP:appropriateForReflectiveMotivation rdf:datatype="http://www.w3.org/2001/XMLSchema#integer">3</EmpowerBP:appropriateForReflectiveMotivation>
        <EmpowerBP:appropriateForSocialOpportunity rdf:datatype="http://www.w3.org/2001/XMLSchema#integer">3</EmpowerBP:appropriateForSocialOpportunity>
        <EmpowerBP:itemName rdf:datatype="http://www.w3.org/2001/XMLSchema#string">Sodium Sense at Home</EmpowerBP:itemName>
        <EmpowerBP:itemText rdf:datatype="http://www.w3.org/2001/XMLSchema#string">The facts on sodium with tips on making lower sodium choices when eating out and at home</EmpowerBP:itemText>
        <EmpowerBP:maximumUserAge rdf:datatype="http://www.w3.org/2001/XMLSchema#integer">120</EmpowerBP:maximumUserAge>
        <EmpowerBP:minimumUserAge rdf:datatype="http://www.w3.org/2001/XMLSchema#integer">18</EmpowerBP:minimumUserAge>
        <EmpowerBP:provideLink rdf:datatype="http://www.w3.org/2001/XMLSchema#boolean">true</EmpowerBP:provideLink>
        <EmpowerBP:sourceURL rdf:datatype="http://www.w3.org/2001/XMLSchema#string">http://www.dietitians.ca/Downloads/Public/sodium_adults_may2012.aspx</EmpowerBP:sourceURL>
        <rdfs:comment rdf:datatype="http://www.w3.org/2001/XMLSchema#string">The facts on sodium with tips on making lower sodium choices when eating out and at home</rdfs:comment>
        <rdfs:label rdf:datatype="http://www.w3.org/2001/XMLSchema#string">Sodium Sense at Home</rdfs:label>
    </owl:NamedIndividual>
    


    <!-- http://www.semanticweb.org/tswheeler/ontologies/2016/3/EmpowerBP#R5 -->

    <owl:NamedIndividual rdf:about="http://www.semanticweb.org/tswheeler/ontologies/2016/3/EmpowerBP#R5">
        <rdf:type rdf:resource="http://www.semanticweb.org/tswheeler/ontologies/2016/3/EmpowerBP#InterventionItem"/>
        <rdf:type rdf:resource="http://www.semanticweb.org/tswheeler/ontologies/2016/3/EmpowerBP#Resource"/>
        <EmpowerBP:isAppropriateForInterventionGoal rdf:resource="http://www.semanticweb.org/tswheeler/ontologies/2016/3/EmpowerBP#ReduceSaltIntake"/>
        <EmpowerBP:appropriateForAutomaticMotivation rdf:datatype="http://www.w3.org/2001/XMLSchema#integer">3</EmpowerBP:appropriateForAutomaticMotivation>
        <EmpowerBP:appropriateForLocation rdf:datatype="http://www.w3.org/2001/XMLSchema#integer">0</EmpowerBP:appropriateForLocation>
        <EmpowerBP:appropriateForPhysicalCapability rdf:datatype="http://www.w3.org/2001/XMLSchema#integer">3</EmpowerBP:appropriateForPhysicalCapability>
        <EmpowerBP:appropriateForPhysicalOpportunity rdf:datatype="http://www.w3.org/2001/XMLSchema#integer">3</EmpowerBP:appropriateForPhysicalOpportunity>
        <EmpowerBP:appropriateForPsychologicalCapability rdf:datatype="http://www.w3.org/2001/XMLSchema#integer">3</EmpowerBP:appropriateForPsychologicalCapability>
        <EmpowerBP:appropriateForReflectiveMotivation rdf:datatype="http://www.w3.org/2001/XMLSchema#integer">3</EmpowerBP:appropriateForReflectiveMotivation>
        <EmpowerBP:appropriateForSocialOpportunity rdf:datatype="http://www.w3.org/2001/XMLSchema#integer">3</EmpowerBP:appropriateForSocialOpportunity>
        <EmpowerBP:itemName rdf:datatype="http://www.w3.org/2001/XMLSchema#string">Sodium Sense at the Market</EmpowerBP:itemName>
        <EmpowerBP:itemText rdf:datatype="http://www.w3.org/2001/XMLSchema#string">The facts on sodium with tips on making lower sodium choices when shopping for food and at home</EmpowerBP:itemText>
        <EmpowerBP:maximumUserAge rdf:datatype="http://www.w3.org/2001/XMLSchema#integer">120</EmpowerBP:maximumUserAge>
        <EmpowerBP:minimumUserAge rdf:datatype="http://www.w3.org/2001/XMLSchema#integer">18</EmpowerBP:minimumUserAge>
        <EmpowerBP:provideLink rdf:datatype="http://www.w3.org/2001/XMLSchema#boolean">true</EmpowerBP:provideLink>
        <EmpowerBP:sourceURL rdf:datatype="http://www.w3.org/2001/XMLSchema#string">http://www.dietitians.ca/Downloads/Public/sodium_parents_may2012.aspx</EmpowerBP:sourceURL>
        <rdfs:comment rdf:datatype="http://www.w3.org/2001/XMLSchema#string">The facts on sodium with tips on making lower sodium choices when shopping for food and at home</rdfs:comment>
        <rdfs:label rdf:datatype="http://www.w3.org/2001/XMLSchema#string">Sodium Sense at the Market</rdfs:label>
    </owl:NamedIndividual>
    


    <!-- http://www.semanticweb.org/tswheeler/ontologies/2016/3/EmpowerBP#R6 -->

    <owl:NamedIndividual rdf:about="http://www.semanticweb.org/tswheeler/ontologies/2016/3/EmpowerBP#R6">
        <rdf:type rdf:resource="http://www.semanticweb.org/tswheeler/ontologies/2016/3/EmpowerBP#InterventionItem"/>
        <rdf:type rdf:resource="http://www.semanticweb.org/tswheeler/ontologies/2016/3/EmpowerBP#Resource"/>
        <EmpowerBP:isAppropriateForInterventionGoal rdf:resource="http://www.semanticweb.org/tswheeler/ontologies/2016/3/EmpowerBP#ReduceSaltIntake"/>
        <EmpowerBP:appropriateForAutomaticMotivation rdf:datatype="http://www.w3.org/2001/XMLSchema#integer">3</EmpowerBP:appropriateForAutomaticMotivation>
        <EmpowerBP:appropriateForLocation rdf:datatype="http://www.w3.org/2001/XMLSchema#integer">0</EmpowerBP:appropriateForLocation>
        <EmpowerBP:appropriateForPhysicalCapability rdf:datatype="http://www.w3.org/2001/XMLSchema#integer">3</EmpowerBP:appropriateForPhysicalCapability>
        <EmpowerBP:appropriateForPhysicalOpportunity rdf:datatype="http://www.w3.org/2001/XMLSchema#integer">3</EmpowerBP:appropriateForPhysicalOpportunity>
        <EmpowerBP:appropriateForPsychologicalCapability rdf:datatype="http://www.w3.org/2001/XMLSchema#integer">3</EmpowerBP:appropriateForPsychologicalCapability>
        <EmpowerBP:appropriateForReflectiveMotivation rdf:datatype="http://www.w3.org/2001/XMLSchema#integer">3</EmpowerBP:appropriateForReflectiveMotivation>
        <EmpowerBP:appropriateForSocialOpportunity rdf:datatype="http://www.w3.org/2001/XMLSchema#integer">3</EmpowerBP:appropriateForSocialOpportunity>
        <EmpowerBP:itemName rdf:datatype="http://www.w3.org/2001/XMLSchema#string">Sodium Sense and Canada&apos;s Food Guide</EmpowerBP:itemName>
        <EmpowerBP:itemText rdf:datatype="http://www.w3.org/2001/XMLSchema#string">The facts on sodium with tips on making lower sodium food choices</EmpowerBP:itemText>
        <EmpowerBP:maximumUserAge rdf:datatype="http://www.w3.org/2001/XMLSchema#integer">120</EmpowerBP:maximumUserAge>
        <EmpowerBP:minimumUserAge rdf:datatype="http://www.w3.org/2001/XMLSchema#integer">18</EmpowerBP:minimumUserAge>
        <EmpowerBP:provideLink rdf:datatype="http://www.w3.org/2001/XMLSchema#boolean">true</EmpowerBP:provideLink>
        <EmpowerBP:sourceURL rdf:datatype="http://www.w3.org/2001/XMLSchema#string">http://www.dietitians.ca/Downloads/Public/sodium_seniors_may2012.aspx</EmpowerBP:sourceURL>
        <rdfs:comment rdf:datatype="http://www.w3.org/2001/XMLSchema#string">The facts on sodium with tips on making lower sodium food choices</rdfs:comment>
        <rdfs:label rdf:datatype="http://www.w3.org/2001/XMLSchema#string">Sodium Sense and Canada&apos;s Food Guide</rdfs:label>
    </owl:NamedIndividual>
    


    <!-- http://www.semanticweb.org/tswheeler/ontologies/2016/3/EmpowerBP#R7 -->

    <owl:NamedIndividual rdf:about="http://www.semanticweb.org/tswheeler/ontologies/2016/3/EmpowerBP#R7">
        <rdf:type rdf:resource="http://www.semanticweb.org/tswheeler/ontologies/2016/3/EmpowerBP#InterventionItem"/>
        <rdf:type rdf:resource="http://www.semanticweb.org/tswheeler/ontologies/2016/3/EmpowerBP#Resource"/>
        <EmpowerBP:isAppropriateForInterventionGoal rdf:resource="http://www.semanticweb.org/tswheeler/ontologies/2016/3/EmpowerBP#ReduceSaltIntake"/>
        <EmpowerBP:appropriateForAutomaticMotivation rdf:datatype="http://www.w3.org/2001/XMLSchema#integer">3</EmpowerBP:appropriateForAutomaticMotivation>
        <EmpowerBP:appropriateForLocation rdf:datatype="http://www.w3.org/2001/XMLSchema#integer">0</EmpowerBP:appropriateForLocation>
        <EmpowerBP:appropriateForPhysicalCapability rdf:datatype="http://www.w3.org/2001/XMLSchema#integer">3</EmpowerBP:appropriateForPhysicalCapability>
        <EmpowerBP:appropriateForPhysicalOpportunity rdf:datatype="http://www.w3.org/2001/XMLSchema#integer">3</EmpowerBP:appropriateForPhysicalOpportunity>
        <EmpowerBP:appropriateForPsychologicalCapability rdf:datatype="http://www.w3.org/2001/XMLSchema#integer">3</EmpowerBP:appropriateForPsychologicalCapability>
        <EmpowerBP:appropriateForReflectiveMotivation rdf:datatype="http://www.w3.org/2001/XMLSchema#integer">3</EmpowerBP:appropriateForReflectiveMotivation>
        <EmpowerBP:appropriateForSocialOpportunity rdf:datatype="http://www.w3.org/2001/XMLSchema#integer">3</EmpowerBP:appropriateForSocialOpportunity>
        <EmpowerBP:itemName rdf:datatype="http://www.w3.org/2001/XMLSchema#string">Sodium Sense Eating Out</EmpowerBP:itemName>
        <EmpowerBP:itemText rdf:datatype="http://www.w3.org/2001/XMLSchema#string">The facts on sodium with tips on making healthier choices when eating out.</EmpowerBP:itemText>
        <EmpowerBP:maximumUserAge rdf:datatype="http://www.w3.org/2001/XMLSchema#integer">120</EmpowerBP:maximumUserAge>
        <EmpowerBP:minimumUserAge rdf:datatype="http://www.w3.org/2001/XMLSchema#integer">18</EmpowerBP:minimumUserAge>
        <EmpowerBP:provideLink rdf:datatype="http://www.w3.org/2001/XMLSchema#boolean">true</EmpowerBP:provideLink>
        <EmpowerBP:sourceURL rdf:datatype="http://www.w3.org/2001/XMLSchema#string">http://www.dietitians.ca/Downloads/Public/sodium_teens_may2012.aspx</EmpowerBP:sourceURL>
        <rdfs:comment rdf:datatype="http://www.w3.org/2001/XMLSchema#string">The facts on sodium with tips on making healthier choices when eating out.</rdfs:comment>
        <rdfs:label rdf:datatype="http://www.w3.org/2001/XMLSchema#string">Sodium Sense Eating Out</rdfs:label>
    </owl:NamedIndividual>
    


    <!-- http://www.semanticweb.org/tswheeler/ontologies/2016/3/EmpowerBP#R8 -->

    <owl:NamedIndividual rdf:about="http://www.semanticweb.org/tswheeler/ontologies/2016/3/EmpowerBP#R8">
        <rdf:type rdf:resource="http://www.semanticweb.org/tswheeler/ontologies/2016/3/EmpowerBP#InterventionItem"/>
        <rdf:type rdf:resource="http://www.semanticweb.org/tswheeler/ontologies/2016/3/EmpowerBP#Resource"/>
        <EmpowerBP:isAppropriateForInterventionGoal rdf:resource="http://www.semanticweb.org/tswheeler/ontologies/2016/3/EmpowerBP#ReduceSaltIntake"/>
        <EmpowerBP:appropriateForAutomaticMotivation rdf:datatype="http://www.w3.org/2001/XMLSchema#integer">3</EmpowerBP:appropriateForAutomaticMotivation>
        <EmpowerBP:appropriateForLocation rdf:datatype="http://www.w3.org/2001/XMLSchema#integer">0</EmpowerBP:appropriateForLocation>
        <EmpowerBP:appropriateForPhysicalCapability rdf:datatype="http://www.w3.org/2001/XMLSchema#integer">3</EmpowerBP:appropriateForPhysicalCapability>
        <EmpowerBP:appropriateForPhysicalOpportunity rdf:datatype="http://www.w3.org/2001/XMLSchema#integer">3</EmpowerBP:appropriateForPhysicalOpportunity>
        <EmpowerBP:appropriateForPsychologicalCapability rdf:datatype="http://www.w3.org/2001/XMLSchema#integer">3</EmpowerBP:appropriateForPsychologicalCapability>
        <EmpowerBP:appropriateForReflectiveMotivation rdf:datatype="http://www.w3.org/2001/XMLSchema#integer">3</EmpowerBP:appropriateForReflectiveMotivation>
        <EmpowerBP:appropriateForSocialOpportunity rdf:datatype="http://www.w3.org/2001/XMLSchema#integer">3</EmpowerBP:appropriateForSocialOpportunity>
        <EmpowerBP:itemName rdf:datatype="http://www.w3.org/2001/XMLSchema#string">Sodium 101</EmpowerBP:itemName>
        <EmpowerBP:itemText rdf:datatype="http://www.w3.org/2001/XMLSchema#string">Created by the Canadian Stroke Network and now managed by Hypertension Canada, Sodium101 is a website that provides information on how to reduce sodium intake.</EmpowerBP:itemText>
        <EmpowerBP:maximumUserAge rdf:datatype="http://www.w3.org/2001/XMLSchema#integer">120</EmpowerBP:maximumUserAge>
        <EmpowerBP:minimumUserAge rdf:datatype="http://www.w3.org/2001/XMLSchema#integer">18</EmpowerBP:minimumUserAge>
        <EmpowerBP:provideLink rdf:datatype="http://www.w3.org/2001/XMLSchema#boolean">true</EmpowerBP:provideLink>
        <EmpowerBP:sourceURL rdf:datatype="http://www.w3.org/2001/XMLSchema#string">http://www.sodium101.ca</EmpowerBP:sourceURL>
        <rdfs:comment rdf:datatype="http://www.w3.org/2001/XMLSchema#string">Created by the Canadian Stroke Network and now managed by Hypertension Canada, Sodium101 is a website that provides information on how to reduce sodium intake.</rdfs:comment>
        <rdfs:label rdf:datatype="http://www.w3.org/2001/XMLSchema#string">Sodium 101</rdfs:label>
    </owl:NamedIndividual>
    


    <!-- http://www.semanticweb.org/tswheeler/ontologies/2016/3/EmpowerBP#R9 -->

    <owl:NamedIndividual rdf:about="http://www.semanticweb.org/tswheeler/ontologies/2016/3/EmpowerBP#R9">
        <rdf:type rdf:resource="http://www.semanticweb.org/tswheeler/ontologies/2016/3/EmpowerBP#InterventionItem"/>
        <rdf:type rdf:resource="http://www.semanticweb.org/tswheeler/ontologies/2016/3/EmpowerBP#Resource"/>
        <EmpowerBP:isAppropriateForInterventionGoal rdf:resource="http://www.semanticweb.org/tswheeler/ontologies/2016/3/EmpowerBP#ReduceSaltIntake"/>
        <EmpowerBP:appropriateForAutomaticMotivation rdf:datatype="http://www.w3.org/2001/XMLSchema#integer">3</EmpowerBP:appropriateForAutomaticMotivation>
        <EmpowerBP:appropriateForLocation rdf:datatype="http://www.w3.org/2001/XMLSchema#integer">0</EmpowerBP:appropriateForLocation>
        <EmpowerBP:appropriateForPhysicalCapability rdf:datatype="http://www.w3.org/2001/XMLSchema#integer">3</EmpowerBP:appropriateForPhysicalCapability>
        <EmpowerBP:appropriateForPhysicalOpportunity rdf:datatype="http://www.w3.org/2001/XMLSchema#integer">3</EmpowerBP:appropriateForPhysicalOpportunity>
        <EmpowerBP:appropriateForPsychologicalCapability rdf:datatype="http://www.w3.org/2001/XMLSchema#integer">3</EmpowerBP:appropriateForPsychologicalCapability>
        <EmpowerBP:appropriateForReflectiveMotivation rdf:datatype="http://www.w3.org/2001/XMLSchema#integer">3</EmpowerBP:appropriateForReflectiveMotivation>
        <EmpowerBP:appropriateForSocialOpportunity rdf:datatype="http://www.w3.org/2001/XMLSchema#integer">3</EmpowerBP:appropriateForSocialOpportunity>
        <EmpowerBP:itemName rdf:datatype="http://www.w3.org/2001/XMLSchema#string">Government of Canada – Sodum</EmpowerBP:itemName>
        <EmpowerBP:itemText rdf:datatype="http://www.w3.org/2001/XMLSchema#string">Health Canada provides information about sodium, how to lower your intake and a tool for learning how much sodium is in the foods you eat.</EmpowerBP:itemText>
        <EmpowerBP:maximumUserAge rdf:datatype="http://www.w3.org/2001/XMLSchema#integer">120</EmpowerBP:maximumUserAge>
        <EmpowerBP:minimumUserAge rdf:datatype="http://www.w3.org/2001/XMLSchema#integer">18</EmpowerBP:minimumUserAge>
        <EmpowerBP:provideLink rdf:datatype="http://www.w3.org/2001/XMLSchema#boolean">true</EmpowerBP:provideLink>
        <EmpowerBP:sourceURL rdf:datatype="http://www.w3.org/2001/XMLSchema#string">https://www.canada.ca/en/health-canada/services/nutrients/sodium.html</EmpowerBP:sourceURL>
        <rdfs:comment rdf:datatype="http://www.w3.org/2001/XMLSchema#string">Health Canada provides information about sodium, how to lower your intake and a tool for learning how much sodium is in the foods you eat.</rdfs:comment>
        <rdfs:label rdf:datatype="http://www.w3.org/2001/XMLSchema#string">Government of Canada – Sodum</rdfs:label>
    </owl:NamedIndividual>
    


    <!-- http://www.semanticweb.org/tswheeler/ontologies/2016/3/EmpowerBP#RSAM1 -->

    <owl:NamedIndividual rdf:about="http://www.semanticweb.org/tswheeler/ontologies/2016/3/EmpowerBP#RSAM1">
        <rdf:type rdf:resource="http://www.semanticweb.org/tswheeler/ontologies/2016/3/EmpowerBP#AssessmentItem"/>
        <rdf:type rdf:resource="http://www.semanticweb.org/tswheeler/ontologies/2016/3/EmpowerBP#COMBAssessmentItem"/>
        <EmpowerBP:canAssessCOMBConstruct rdf:resource="http://www.semanticweb.org/tswheeler/ontologies/2016/3/EmpowerBP#AutomaticMotivation"/>
        <EmpowerBP:isSpecificToGoal rdf:resource="http://www.semanticweb.org/tswheeler/ontologies/2016/3/EmpowerBP#ReduceSaltIntake"/>
        <EmpowerBP:assessmentItemExamples rdf:datatype="http://www.w3.org/2001/XMLSchema#string">• Learn how to feel more of a sense of pleasure or satisfaction from healthy eating.</EmpowerBP:assessmentItemExamples>
        <EmpowerBP:assessmentItemID rdf:datatype="http://www.w3.org/2001/XMLSchema#string">RSAM1</EmpowerBP:assessmentItemID>
        <EmpowerBP:assessmentItemText rdf:datatype="http://www.w3.org/2001/XMLSchema#string">It would help if I could increase my drive or desire to eat less sodium.</EmpowerBP:assessmentItemText>
        <rdfs:comment rdf:datatype="http://www.w3.org/2001/XMLSchema#string">It would help if I could increase my drive or desire to eat less sodium.</rdfs:comment>
        <rdfs:label rdf:datatype="http://www.w3.org/2001/XMLSchema#string">RSAM1</rdfs:label>
    </owl:NamedIndividual>
    


    <!-- http://www.semanticweb.org/tswheeler/ontologies/2016/3/EmpowerBP#RSAM2 -->

    <owl:NamedIndividual rdf:about="http://www.semanticweb.org/tswheeler/ontologies/2016/3/EmpowerBP#RSAM2">
        <rdf:type rdf:resource="http://www.semanticweb.org/tswheeler/ontologies/2016/3/EmpowerBP#AssessmentItem"/>
        <rdf:type rdf:resource="http://www.semanticweb.org/tswheeler/ontologies/2016/3/EmpowerBP#COMBAssessmentItem"/>
        <EmpowerBP:canAssessCOMBConstruct rdf:resource="http://www.semanticweb.org/tswheeler/ontologies/2016/3/EmpowerBP#AutomaticMotivation"/>
        <EmpowerBP:isSpecificToGoal rdf:resource="http://www.semanticweb.org/tswheeler/ontologies/2016/3/EmpowerBP#ReduceSaltIntake"/>
        <EmpowerBP:assessmentItemExamples rdf:datatype="http://www.w3.org/2001/XMLSchema#string">• Learn how to care more about the negative consequences of eating too much sodium.</EmpowerBP:assessmentItemExamples>
        <EmpowerBP:assessmentItemID rdf:datatype="http://www.w3.org/2001/XMLSchema#string">RSAM2</EmpowerBP:assessmentItemID>
        <EmpowerBP:assessmentItemText rdf:datatype="http://www.w3.org/2001/XMLSchema#string">It would help if I could make being active feel more important to me.</EmpowerBP:assessmentItemText>
        <rdfs:comment rdf:datatype="http://www.w3.org/2001/XMLSchema#string">It would help if I could make being active feel more important to me.</rdfs:comment>
        <rdfs:label rdf:datatype="http://www.w3.org/2001/XMLSchema#string">RSAM2</rdfs:label>
    </owl:NamedIndividual>
    


    <!-- http://www.semanticweb.org/tswheeler/ontologies/2016/3/EmpowerBP#RSAM3 -->

    <owl:NamedIndividual rdf:about="http://www.semanticweb.org/tswheeler/ontologies/2016/3/EmpowerBP#RSAM3">
        <rdf:type rdf:resource="http://www.semanticweb.org/tswheeler/ontologies/2016/3/EmpowerBP#AssessmentItem"/>
        <rdf:type rdf:resource="http://www.semanticweb.org/tswheeler/ontologies/2016/3/EmpowerBP#COMBAssessmentItem"/>
        <EmpowerBP:canAssessCOMBConstruct rdf:resource="http://www.semanticweb.org/tswheeler/ontologies/2016/3/EmpowerBP#AutomaticMotivation"/>
        <EmpowerBP:isSpecificToGoal rdf:resource="http://www.semanticweb.org/tswheeler/ontologies/2016/3/EmpowerBP#ReduceSaltIntake"/>
        <EmpowerBP:assessmentItemExamples rdf:datatype="http://www.w3.org/2001/XMLSchema#string">• Get into a pattern of choosing low-sodium foods regularly without having to think about it.</EmpowerBP:assessmentItemExamples>
        <EmpowerBP:assessmentItemID rdf:datatype="http://www.w3.org/2001/XMLSchema#string">RSAM3</EmpowerBP:assessmentItemID>
        <EmpowerBP:assessmentItemText rdf:datatype="http://www.w3.org/2001/XMLSchema#string">It would help if I could develop a habit of eating healthier.</EmpowerBP:assessmentItemText>
        <rdfs:comment rdf:datatype="http://www.w3.org/2001/XMLSchema#string">It would help if I could develop a habit of eating healthier.</rdfs:comment>
        <rdfs:label rdf:datatype="http://www.w3.org/2001/XMLSchema#string">RSAM3</rdfs:label>
    </owl:NamedIndividual>
    


    <!-- http://www.semanticweb.org/tswheeler/ontologies/2016/3/EmpowerBP#RSPO1 -->

    <owl:NamedIndividual rdf:about="http://www.semanticweb.org/tswheeler/ontologies/2016/3/EmpowerBP#RSPO1">
        <rdf:type rdf:resource="http://www.semanticweb.org/tswheeler/ontologies/2016/3/EmpowerBP#AssessmentItem"/>
        <rdf:type rdf:resource="http://www.semanticweb.org/tswheeler/ontologies/2016/3/EmpowerBP#COMBAssessmentItem"/>
        <EmpowerBP:canAssessCOMBConstruct rdf:resource="http://www.semanticweb.org/tswheeler/ontologies/2016/3/EmpowerBP#PhysicalOpportunity"/>
        <EmpowerBP:isSpecificToGoal rdf:resource="http://www.semanticweb.org/tswheeler/ontologies/2016/3/EmpowerBP#ReduceSaltIntake"/>
        <EmpowerBP:assessmentItemExamples rdf:datatype="http://www.w3.org/2001/XMLSchema#string">• Learn how to make quick and simple low-sodium recipes. 
• Learn how to fit healthy eating into to my busy schedule.</EmpowerBP:assessmentItemExamples>
        <EmpowerBP:assessmentItemID rdf:datatype="http://www.w3.org/2001/XMLSchema#string">RSPO1</EmpowerBP:assessmentItemID>
        <EmpowerBP:assessmentItemText rdf:datatype="http://www.w3.org/2001/XMLSchema#string">It would help if I had more time to make healthier choices. </EmpowerBP:assessmentItemText>
        <rdfs:comment rdf:datatype="http://www.w3.org/2001/XMLSchema#string">It would help if I had more time to make healthier choices. </rdfs:comment>
        <rdfs:label rdf:datatype="http://www.w3.org/2001/XMLSchema#string">RSPO1</rdfs:label>
    </owl:NamedIndividual>
    


    <!-- http://www.semanticweb.org/tswheeler/ontologies/2016/3/EmpowerBP#RSPO2 -->

    <owl:NamedIndividual rdf:about="http://www.semanticweb.org/tswheeler/ontologies/2016/3/EmpowerBP#RSPO2">
        <rdf:type rdf:resource="http://www.semanticweb.org/tswheeler/ontologies/2016/3/EmpowerBP#AssessmentItem"/>
        <rdf:type rdf:resource="http://www.semanticweb.org/tswheeler/ontologies/2016/3/EmpowerBP#COMBAssessmentItem"/>
        <EmpowerBP:canAssessCOMBConstruct rdf:resource="http://www.semanticweb.org/tswheeler/ontologies/2016/3/EmpowerBP#PhysicalOpportunity"/>
        <EmpowerBP:isSpecificToGoal rdf:resource="http://www.semanticweb.org/tswheeler/ontologies/2016/3/EmpowerBP#ReduceSaltIntake"/>
        <EmpowerBP:assessmentItemExamples rdf:datatype="http://www.w3.org/2001/XMLSchema#string">• Learn how to be make healthy meals with the equipment that I have.
• Learn how I can make low-sodium choices without spending extra money.</EmpowerBP:assessmentItemExamples>
        <EmpowerBP:assessmentItemID rdf:datatype="http://www.w3.org/2001/XMLSchema#string">RSPO2</EmpowerBP:assessmentItemID>
        <EmpowerBP:assessmentItemText rdf:datatype="http://www.w3.org/2001/XMLSchema#string">It would help if I had more money or appliances to cook with.</EmpowerBP:assessmentItemText>
        <rdfs:comment rdf:datatype="http://www.w3.org/2001/XMLSchema#string">It would help if I had more money or appliances to cook with.</rdfs:comment>
        <rdfs:label rdf:datatype="http://www.w3.org/2001/XMLSchema#string">RSPO2</rdfs:label>
    </owl:NamedIndividual>
    


    <!-- http://www.semanticweb.org/tswheeler/ontologies/2016/3/EmpowerBP#RSPO3 -->

    <owl:NamedIndividual rdf:about="http://www.semanticweb.org/tswheeler/ontologies/2016/3/EmpowerBP#RSPO3">
        <rdf:type rdf:resource="http://www.semanticweb.org/tswheeler/ontologies/2016/3/EmpowerBP#AssessmentItem"/>
        <rdf:type rdf:resource="http://www.semanticweb.org/tswheeler/ontologies/2016/3/EmpowerBP#COMBAssessmentItem"/>
        <EmpowerBP:canAssessCOMBConstruct rdf:resource="http://www.semanticweb.org/tswheeler/ontologies/2016/3/EmpowerBP#PhysicalOpportunity"/>
        <EmpowerBP:isSpecificToGoal rdf:resource="http://www.semanticweb.org/tswheeler/ontologies/2016/3/EmpowerBP#ReduceSaltIntake"/>
        <EmpowerBP:assessmentItemExamples rdf:datatype="http://www.w3.org/2001/XMLSchema#string">• Learn where to go to find low-sodium options.
• Learn about common low-sodium options for home and when eating out.</EmpowerBP:assessmentItemExamples>
        <EmpowerBP:assessmentItemID rdf:datatype="http://www.w3.org/2001/XMLSchema#string">RSPO3</EmpowerBP:assessmentItemID>
        <EmpowerBP:assessmentItemText rdf:datatype="http://www.w3.org/2001/XMLSchema#string">It would help if I had more places where I could go to find low-sodium choices.</EmpowerBP:assessmentItemText>
        <rdfs:comment rdf:datatype="http://www.w3.org/2001/XMLSchema#string">It would help if I had more places where I could go to find low-sodium choices.</rdfs:comment>
        <rdfs:label rdf:datatype="http://www.w3.org/2001/XMLSchema#string">RSPO3</rdfs:label>
    </owl:NamedIndividual>
    


    <!-- http://www.semanticweb.org/tswheeler/ontologies/2016/3/EmpowerBP#RSPhC1 -->

    <owl:NamedIndividual rdf:about="http://www.semanticweb.org/tswheeler/ontologies/2016/3/EmpowerBP#RSPhC1">
        <rdf:type rdf:resource="http://www.semanticweb.org/tswheeler/ontologies/2016/3/EmpowerBP#AssessmentItem"/>
        <rdf:type rdf:resource="http://www.semanticweb.org/tswheeler/ontologies/2016/3/EmpowerBP#COMBAssessmentItem"/>
        <EmpowerBP:canAssessCOMBConstruct rdf:resource="http://www.semanticweb.org/tswheeler/ontologies/2016/3/EmpowerBP#PhysicalCapability"/>
        <EmpowerBP:isSpecificToGoal rdf:resource="http://www.semanticweb.org/tswheeler/ontologies/2016/3/EmpowerBP#ReduceSaltIntake"/>
        <EmpowerBP:assessmentItemExamples rdf:datatype="http://www.w3.org/2001/XMLSchema#string">• Learn where the sodium in my diet comes from. 
• Learn how to find out about the sodium in the foods I eat.</EmpowerBP:assessmentItemExamples>
        <EmpowerBP:assessmentItemID rdf:datatype="http://www.w3.org/2001/XMLSchema#string">RSPhC1</EmpowerBP:assessmentItemID>
        <EmpowerBP:assessmentItemText rdf:datatype="http://www.w3.org/2001/XMLSchema#string">It would help if I knew more about the sodium in my diet currently.</EmpowerBP:assessmentItemText>
        <rdfs:comment rdf:datatype="http://www.w3.org/2001/XMLSchema#string">It would help if I knew more about the sodium in my diet currently.</rdfs:comment>
        <rdfs:label rdf:datatype="http://www.w3.org/2001/XMLSchema#string">RSPhC1</rdfs:label>
    </owl:NamedIndividual>
    


    <!-- http://www.semanticweb.org/tswheeler/ontologies/2016/3/EmpowerBP#RSPhC2 -->

    <owl:NamedIndividual rdf:about="http://www.semanticweb.org/tswheeler/ontologies/2016/3/EmpowerBP#RSPhC2">
        <rdf:type rdf:resource="http://www.semanticweb.org/tswheeler/ontologies/2016/3/EmpowerBP#AssessmentItem"/>
        <rdf:type rdf:resource="http://www.semanticweb.org/tswheeler/ontologies/2016/3/EmpowerBP#COMBAssessmentItem"/>
        <EmpowerBP:canAssessCOMBConstruct rdf:resource="http://www.semanticweb.org/tswheeler/ontologies/2016/3/EmpowerBP#PhysicalCapability"/>
        <EmpowerBP:isSpecificToGoal rdf:resource="http://www.semanticweb.org/tswheeler/ontologies/2016/3/EmpowerBP#ReduceSaltIntake"/>
        <EmpowerBP:assessmentItemExamples rdf:datatype="http://www.w3.org/2001/XMLSchema#string">• Learn how to find and make low-sodium recipes at home.
• Learn about low-sodium food choices at the store or when eating out.</EmpowerBP:assessmentItemExamples>
        <EmpowerBP:assessmentItemID rdf:datatype="http://www.w3.org/2001/XMLSchema#string">RSPhC2</EmpowerBP:assessmentItemID>
        <EmpowerBP:assessmentItemText rdf:datatype="http://www.w3.org/2001/XMLSchema#string">It would help if I learned about ways of reducing the sodium in my diet.</EmpowerBP:assessmentItemText>
        <rdfs:comment rdf:datatype="http://www.w3.org/2001/XMLSchema#string">It would help if I learned about ways of reducing the sodium in my diet.</rdfs:comment>
        <rdfs:label rdf:datatype="http://www.w3.org/2001/XMLSchema#string">RSPhC2</rdfs:label>
    </owl:NamedIndividual>
    


    <!-- http://www.semanticweb.org/tswheeler/ontologies/2016/3/EmpowerBP#RSPhC3 -->

    <owl:NamedIndividual rdf:about="http://www.semanticweb.org/tswheeler/ontologies/2016/3/EmpowerBP#RSPhC3">
        <rdf:type rdf:resource="http://www.semanticweb.org/tswheeler/ontologies/2016/3/EmpowerBP#AssessmentItem"/>
        <rdf:type rdf:resource="http://www.semanticweb.org/tswheeler/ontologies/2016/3/EmpowerBP#COMBAssessmentItem"/>
        <EmpowerBP:canAssessCOMBConstruct rdf:resource="http://www.semanticweb.org/tswheeler/ontologies/2016/3/EmpowerBP#PhysicalCapability"/>
        <EmpowerBP:isSpecificToGoal rdf:resource="http://www.semanticweb.org/tswheeler/ontologies/2016/3/EmpowerBP#ReduceSaltIntake"/>
        <EmpowerBP:assessmentItemExamples rdf:datatype="http://www.w3.org/2001/XMLSchema#string">• Learn how to find easy and healthy recipes for beginners.</EmpowerBP:assessmentItemExamples>
        <EmpowerBP:assessmentItemID rdf:datatype="http://www.w3.org/2001/XMLSchema#string">RSPhC3</EmpowerBP:assessmentItemID>
        <EmpowerBP:assessmentItemText rdf:datatype="http://www.w3.org/2001/XMLSchema#string">It would help if I had better cooking skills.  </EmpowerBP:assessmentItemText>
        <rdfs:comment rdf:datatype="http://www.w3.org/2001/XMLSchema#string">It would help if I had better cooking skills.  </rdfs:comment>
        <rdfs:label rdf:datatype="http://www.w3.org/2001/XMLSchema#string">RSPhC3</rdfs:label>
    </owl:NamedIndividual>
    


    <!-- http://www.semanticweb.org/tswheeler/ontologies/2016/3/EmpowerBP#RSPsC1 -->

    <owl:NamedIndividual rdf:about="http://www.semanticweb.org/tswheeler/ontologies/2016/3/EmpowerBP#RSPsC1">
        <rdf:type rdf:resource="http://www.semanticweb.org/tswheeler/ontologies/2016/3/EmpowerBP#AssessmentItem"/>
        <rdf:type rdf:resource="http://www.semanticweb.org/tswheeler/ontologies/2016/3/EmpowerBP#COMBAssessmentItem"/>
        <EmpowerBP:canAssessCOMBConstruct rdf:resource="http://www.semanticweb.org/tswheeler/ontologies/2016/3/EmpowerBP#PsychologicalCapability"/>
        <EmpowerBP:isSpecificToGoal rdf:resource="http://www.semanticweb.org/tswheeler/ontologies/2016/3/EmpowerBP#ReduceSaltIntake"/>
        <EmpowerBP:assessmentItemExamples rdf:datatype="http://www.w3.org/2001/XMLSchema#string">• Have a better understanding of the benefits of eating healthy and the risks of having too much sodium.</EmpowerBP:assessmentItemExamples>
        <EmpowerBP:assessmentItemID rdf:datatype="http://www.w3.org/2001/XMLSchema#string">RSPsC1</EmpowerBP:assessmentItemID>
        <EmpowerBP:assessmentItemText rdf:datatype="http://www.w3.org/2001/XMLSchema#string">It would help if I knew more about why a low-sodium diet is important.</EmpowerBP:assessmentItemText>
        <rdfs:comment rdf:datatype="http://www.w3.org/2001/XMLSchema#string">It would help if I knew more about why a low-sodium diet is important.</rdfs:comment>
        <rdfs:label rdf:datatype="http://www.w3.org/2001/XMLSchema#string">RSPsC1</rdfs:label>
    </owl:NamedIndividual>
    


    <!-- http://www.semanticweb.org/tswheeler/ontologies/2016/3/EmpowerBP#RSPsC2 -->

    <owl:NamedIndividual rdf:about="http://www.semanticweb.org/tswheeler/ontologies/2016/3/EmpowerBP#RSPsC2">
        <rdf:type rdf:resource="http://www.semanticweb.org/tswheeler/ontologies/2016/3/EmpowerBP#AssessmentItem"/>
        <rdf:type rdf:resource="http://www.semanticweb.org/tswheeler/ontologies/2016/3/EmpowerBP#COMBAssessmentItem"/>
        <EmpowerBP:canAssessCOMBConstruct rdf:resource="http://www.semanticweb.org/tswheeler/ontologies/2016/3/EmpowerBP#PsychologicalCapability"/>
        <EmpowerBP:isSpecificToGoal rdf:resource="http://www.semanticweb.org/tswheeler/ontologies/2016/3/EmpowerBP#ReduceSaltIntake"/>
        <EmpowerBP:assessmentItemExamples rdf:datatype="http://www.w3.org/2001/XMLSchema#string">• Learn more about the “proper mindset” to making healthy eating choices. 
• Learn how to concentrate on my goals of eating less sodium.</EmpowerBP:assessmentItemExamples>
        <EmpowerBP:assessmentItemID rdf:datatype="http://www.w3.org/2001/XMLSchema#string">RSPsC2</EmpowerBP:assessmentItemID>
        <EmpowerBP:assessmentItemText rdf:datatype="http://www.w3.org/2001/XMLSchema#string">It would help if I changed the way I thought about eating healthier.</EmpowerBP:assessmentItemText>
        <rdfs:comment rdf:datatype="http://www.w3.org/2001/XMLSchema#string">It would help if I changed the way I thought about eating healthier.</rdfs:comment>
        <rdfs:label rdf:datatype="http://www.w3.org/2001/XMLSchema#string">RSPsC2</rdfs:label>
    </owl:NamedIndividual>
    


    <!-- http://www.semanticweb.org/tswheeler/ontologies/2016/3/EmpowerBP#RSPsC3 -->

    <owl:NamedIndividual rdf:about="http://www.semanticweb.org/tswheeler/ontologies/2016/3/EmpowerBP#RSPsC3">
        <rdf:type rdf:resource="http://www.semanticweb.org/tswheeler/ontologies/2016/3/EmpowerBP#AssessmentItem"/>
        <rdf:type rdf:resource="http://www.semanticweb.org/tswheeler/ontologies/2016/3/EmpowerBP#COMBAssessmentItem"/>
        <EmpowerBP:canAssessCOMBConstruct rdf:resource="http://www.semanticweb.org/tswheeler/ontologies/2016/3/EmpowerBP#PsychologicalCapability"/>
        <EmpowerBP:isSpecificToGoal rdf:resource="http://www.semanticweb.org/tswheeler/ontologies/2016/3/EmpowerBP#ReduceSaltIntake"/>
        <EmpowerBP:assessmentItemExamples rdf:datatype="http://www.w3.org/2001/XMLSchema#string">• Learn how to reduce unwanted urges or feelings about healthy eating. 
• Learn how to find and make healthy choices even when life is stressful.</EmpowerBP:assessmentItemExamples>
        <EmpowerBP:assessmentItemID rdf:datatype="http://www.w3.org/2001/XMLSchema#string">RSPsC3</EmpowerBP:assessmentItemID>
        <EmpowerBP:assessmentItemText rdf:datatype="http://www.w3.org/2001/XMLSchema#string">I would like to improve my mental strength and stamina.</EmpowerBP:assessmentItemText>
        <rdfs:comment rdf:datatype="http://www.w3.org/2001/XMLSchema#string">I would like to improve my mental strength and stamina.</rdfs:comment>
        <rdfs:label rdf:datatype="http://www.w3.org/2001/XMLSchema#string">RSPsC3</rdfs:label>
    </owl:NamedIndividual>
    


    <!-- http://www.semanticweb.org/tswheeler/ontologies/2016/3/EmpowerBP#RSRM1 -->

    <owl:NamedIndividual rdf:about="http://www.semanticweb.org/tswheeler/ontologies/2016/3/EmpowerBP#RSRM1">
        <rdf:type rdf:resource="http://www.semanticweb.org/tswheeler/ontologies/2016/3/EmpowerBP#AssessmentItem"/>
        <rdf:type rdf:resource="http://www.semanticweb.org/tswheeler/ontologies/2016/3/EmpowerBP#COMBAssessmentItem"/>
        <EmpowerBP:canAssessCOMBConstruct rdf:resource="http://www.semanticweb.org/tswheeler/ontologies/2016/3/EmpowerBP#ReflectiveMotivation"/>
        <EmpowerBP:isSpecificToGoal rdf:resource="http://www.semanticweb.org/tswheeler/ontologies/2016/3/EmpowerBP#ReduceSaltIntake"/>
        <EmpowerBP:assessmentItemExamples rdf:datatype="http://www.w3.org/2001/XMLSchema#string">• Learn how to weigh the pros and cons of eating less sodium.</EmpowerBP:assessmentItemExamples>
        <EmpowerBP:assessmentItemID rdf:datatype="http://www.w3.org/2001/XMLSchema#string">RSRM1</EmpowerBP:assessmentItemID>
        <EmpowerBP:assessmentItemText rdf:datatype="http://www.w3.org/2001/XMLSchema#string">It would help if could focus more on the reasons to change and not on what is keeping me from changing.</EmpowerBP:assessmentItemText>
        <rdfs:comment rdf:datatype="http://www.w3.org/2001/XMLSchema#string">It would help if could focus more on the reasons to change and not on what is keeping me from changing.</rdfs:comment>
        <rdfs:label rdf:datatype="http://www.w3.org/2001/XMLSchema#string">RSRM1</rdfs:label>
    </owl:NamedIndividual>
    


    <!-- http://www.semanticweb.org/tswheeler/ontologies/2016/3/EmpowerBP#RSRM2 -->

    <owl:NamedIndividual rdf:about="http://www.semanticweb.org/tswheeler/ontologies/2016/3/EmpowerBP#RSRM2">
        <rdf:type rdf:resource="http://www.semanticweb.org/tswheeler/ontologies/2016/3/EmpowerBP#AssessmentItem"/>
        <rdf:type rdf:resource="http://www.semanticweb.org/tswheeler/ontologies/2016/3/EmpowerBP#COMBAssessmentItem"/>
        <EmpowerBP:canAssessCOMBConstruct rdf:resource="http://www.semanticweb.org/tswheeler/ontologies/2016/3/EmpowerBP#ReflectiveMotivation"/>
        <EmpowerBP:isSpecificToGoal rdf:resource="http://www.semanticweb.org/tswheeler/ontologies/2016/3/EmpowerBP#ReduceSaltIntake"/>
        <EmpowerBP:assessmentItemExamples rdf:datatype="http://www.w3.org/2001/XMLSchema#string">• Make clear and thought out plans to limit the amount of sodium in my diet.</EmpowerBP:assessmentItemExamples>
        <EmpowerBP:assessmentItemID rdf:datatype="http://www.w3.org/2001/XMLSchema#string">RSRM2</EmpowerBP:assessmentItemID>
        <EmpowerBP:assessmentItemText rdf:datatype="http://www.w3.org/2001/XMLSchema#string">It would help if I had better plans to eat healthier.</EmpowerBP:assessmentItemText>
        <rdfs:comment rdf:datatype="http://www.w3.org/2001/XMLSchema#string">It would help if I had better plans to eat healthier.</rdfs:comment>
        <rdfs:label rdf:datatype="http://www.w3.org/2001/XMLSchema#string">RSRM2</rdfs:label>
    </owl:NamedIndividual>
    


    <!-- http://www.semanticweb.org/tswheeler/ontologies/2016/3/EmpowerBP#RSRM3 -->

    <owl:NamedIndividual rdf:about="http://www.semanticweb.org/tswheeler/ontologies/2016/3/EmpowerBP#RSRM3">
        <rdf:type rdf:resource="http://www.semanticweb.org/tswheeler/ontologies/2016/3/EmpowerBP#AssessmentItem"/>
        <rdf:type rdf:resource="http://www.semanticweb.org/tswheeler/ontologies/2016/3/EmpowerBP#COMBAssessmentItem"/>
        <EmpowerBP:canAssessCOMBConstruct rdf:resource="http://www.semanticweb.org/tswheeler/ontologies/2016/3/EmpowerBP#ReflectiveMotivation"/>
        <EmpowerBP:isSpecificToGoal rdf:resource="http://www.semanticweb.org/tswheeler/ontologies/2016/3/EmpowerBP#ReduceSaltIntake"/>
        <EmpowerBP:assessmentItemExamples rdf:datatype="http://www.w3.org/2001/XMLSchema#string">• Become more confident in my ability to make low-sodium food choices.</EmpowerBP:assessmentItemExamples>
        <EmpowerBP:assessmentItemID rdf:datatype="http://www.w3.org/2001/XMLSchema#string">RSRM3</EmpowerBP:assessmentItemID>
        <EmpowerBP:assessmentItemText rdf:datatype="http://www.w3.org/2001/XMLSchema#string">It would help if I had more self-confidence in my ability to eat healthier.</EmpowerBP:assessmentItemText>
        <rdfs:comment rdf:datatype="http://www.w3.org/2001/XMLSchema#string">It would help if I had more self-confidence in my ability to eat healthier.</rdfs:comment>
        <rdfs:label rdf:datatype="http://www.w3.org/2001/XMLSchema#string">RSRM3</rdfs:label>
    </owl:NamedIndividual>
    


    <!-- http://www.semanticweb.org/tswheeler/ontologies/2016/3/EmpowerBP#RSSO1 -->

    <owl:NamedIndividual rdf:about="http://www.semanticweb.org/tswheeler/ontologies/2016/3/EmpowerBP#RSSO1">
        <rdf:type rdf:resource="http://www.semanticweb.org/tswheeler/ontologies/2016/3/EmpowerBP#AssessmentItem"/>
        <rdf:type rdf:resource="http://www.semanticweb.org/tswheeler/ontologies/2016/3/EmpowerBP#COMBAssessmentItem"/>
        <EmpowerBP:canAssessCOMBConstruct rdf:resource="http://www.semanticweb.org/tswheeler/ontologies/2016/3/EmpowerBP#SocialOpportunity"/>
        <EmpowerBP:isSpecificToGoal rdf:resource="http://www.semanticweb.org/tswheeler/ontologies/2016/3/EmpowerBP#ReduceSaltIntake"/>
        <EmpowerBP:assessmentItemExamples rdf:datatype="http://www.w3.org/2001/XMLSchema#string">• Have regular reminders to make low-sodium choices at strategic times.
• Learn how to change my home and work environment to support eating healthier.</EmpowerBP:assessmentItemExamples>
        <EmpowerBP:assessmentItemID rdf:datatype="http://www.w3.org/2001/XMLSchema#string">RSSO1</EmpowerBP:assessmentItemID>
        <EmpowerBP:assessmentItemText rdf:datatype="http://www.w3.org/2001/XMLSchema#string">It would help if I had more cues to encourage me to eat healthier.</EmpowerBP:assessmentItemText>
        <rdfs:comment rdf:datatype="http://www.w3.org/2001/XMLSchema#string">It would help if I had more cues to encourage me to eat healthier.</rdfs:comment>
        <rdfs:label rdf:datatype="http://www.w3.org/2001/XMLSchema#string">RSSO1</rdfs:label>
    </owl:NamedIndividual>
    


    <!-- http://www.semanticweb.org/tswheeler/ontologies/2016/3/EmpowerBP#RSSO2 -->

    <owl:NamedIndividual rdf:about="http://www.semanticweb.org/tswheeler/ontologies/2016/3/EmpowerBP#RSSO2">
        <rdf:type rdf:resource="http://www.semanticweb.org/tswheeler/ontologies/2016/3/EmpowerBP#AssessmentItem"/>
        <rdf:type rdf:resource="http://www.semanticweb.org/tswheeler/ontologies/2016/3/EmpowerBP#COMBAssessmentItem"/>
        <EmpowerBP:canAssessCOMBConstruct rdf:resource="http://www.semanticweb.org/tswheeler/ontologies/2016/3/EmpowerBP#SocialOpportunity"/>
        <EmpowerBP:isSpecificToGoal rdf:resource="http://www.semanticweb.org/tswheeler/ontologies/2016/3/EmpowerBP#ReduceSaltIntake"/>
        <EmpowerBP:assessmentItemExamples rdf:datatype="http://www.w3.org/2001/XMLSchema#string">• Find groups or teams who have similar healthy eating goals as me.</EmpowerBP:assessmentItemExamples>
        <EmpowerBP:assessmentItemID rdf:datatype="http://www.w3.org/2001/XMLSchema#string">RSSO2</EmpowerBP:assessmentItemID>
        <EmpowerBP:assessmentItemText rdf:datatype="http://www.w3.org/2001/XMLSchema#string">It would help if I had more people around me who were eating healthy.</EmpowerBP:assessmentItemText>
        <rdfs:comment rdf:datatype="http://www.w3.org/2001/XMLSchema#string">It would help if I had more people around me who were eating healthy.</rdfs:comment>
        <rdfs:label rdf:datatype="http://www.w3.org/2001/XMLSchema#string">RSSO2</rdfs:label>
    </owl:NamedIndividual>
    


    <!-- http://www.semanticweb.org/tswheeler/ontologies/2016/3/EmpowerBP#RSSO3 -->

    <owl:NamedIndividual rdf:about="http://www.semanticweb.org/tswheeler/ontologies/2016/3/EmpowerBP#RSSO3">
        <rdf:type rdf:resource="http://www.semanticweb.org/tswheeler/ontologies/2016/3/EmpowerBP#AssessmentItem"/>
        <rdf:type rdf:resource="http://www.semanticweb.org/tswheeler/ontologies/2016/3/EmpowerBP#COMBAssessmentItem"/>
        <EmpowerBP:canAssessCOMBConstruct rdf:resource="http://www.semanticweb.org/tswheeler/ontologies/2016/3/EmpowerBP#SocialOpportunity"/>
        <EmpowerBP:isSpecificToGoal rdf:resource="http://www.semanticweb.org/tswheeler/ontologies/2016/3/EmpowerBP#ReduceSaltIntake"/>
        <EmpowerBP:assessmentItemExamples rdf:datatype="http://www.w3.org/2001/XMLSchema#string">• Learn how to have my friends and family help me reach my healthy eating goals.</EmpowerBP:assessmentItemExamples>
        <EmpowerBP:assessmentItemID rdf:datatype="http://www.w3.org/2001/XMLSchema#string">RSSO3</EmpowerBP:assessmentItemID>
        <EmpowerBP:assessmentItemText rdf:datatype="http://www.w3.org/2001/XMLSchema#string">It would help if I had more people around me supporting my goals.</EmpowerBP:assessmentItemText>
        <rdfs:comment rdf:datatype="http://www.w3.org/2001/XMLSchema#string">It would help if I had more people around me supporting my goals.</rdfs:comment>
        <rdfs:label rdf:datatype="http://www.w3.org/2001/XMLSchema#string">RSSO3</rdfs:label>
    </owl:NamedIndividual>
    


    <!-- http://www.semanticweb.org/tswheeler/ontologies/2016/3/EmpowerBP#ReduceSaltIntake -->

    <owl:NamedIndividual rdf:about="http://www.semanticweb.org/tswheeler/ontologies/2016/3/EmpowerBP#ReduceSaltIntake">
        <rdf:type rdf:resource="http://www.semanticweb.org/tswheeler/ontologies/2016/3/EmpowerBP#CessationGoal"/>
        <rdf:type rdf:resource="http://www.semanticweb.org/tswheeler/ontologies/2016/3/EmpowerBP#InterventionGoal"/>
    </owl:NamedIndividual>
    


    <!-- http://www.semanticweb.org/tswheeler/ontologies/2016/3/EmpowerBP#ReflectiveMotivation -->

    <owl:NamedIndividual rdf:about="http://www.semanticweb.org/tswheeler/ontologies/2016/3/EmpowerBP#ReflectiveMotivation">
        <rdf:type rdf:resource="http://www.semanticweb.org/tswheeler/ontologies/2016/3/EmpowerBP#COMBConstruct"/>
        <rdf:type rdf:resource="http://www.semanticweb.org/tswheeler/ontologies/2016/3/EmpowerBP#Construct"/>
        <rdf:type rdf:resource="http://www.semanticweb.org/tswheeler/ontologies/2016/3/EmpowerBP#Motivation"/>
        <EmpowerBP:isRelatedToTDF rdf:resource="http://www.semanticweb.org/tswheeler/ontologies/2016/3/EmpowerBP#BeliefsAboutCapability"/>
        <EmpowerBP:isRelatedToTDF rdf:resource="http://www.semanticweb.org/tswheeler/ontologies/2016/3/EmpowerBP#BeliefsAboutConsequences"/>
        <EmpowerBP:isRelatedToTDF rdf:resource="http://www.semanticweb.org/tswheeler/ontologies/2016/3/EmpowerBP#Goals"/>
        <EmpowerBP:isRelatedToTDF rdf:resource="http://www.semanticweb.org/tswheeler/ontologies/2016/3/EmpowerBP#Intentions"/>
        <EmpowerBP:isRelatedToTDF rdf:resource="http://www.semanticweb.org/tswheeler/ontologies/2016/3/EmpowerBP#Optimism"/>
        <EmpowerBP:isRelatedToTDF rdf:resource="http://www.semanticweb.org/tswheeler/ontologies/2016/3/EmpowerBP#ProfessionalSocialRoleIdentity"/>
        <rdfs:comment>Self-concious planning and evaluations (beliefs about what is good or bad)</rdfs:comment>
    </owl:NamedIndividual>
    


    <!-- http://www.semanticweb.org/tswheeler/ontologies/2016/3/EmpowerBP#Reinforcement -->

    <owl:NamedIndividual rdf:about="http://www.semanticweb.org/tswheeler/ontologies/2016/3/EmpowerBP#Reinforcement">
        <rdf:type rdf:resource="http://www.semanticweb.org/tswheeler/ontologies/2016/3/EmpowerBP#Construct"/>
        <rdf:type rdf:resource="http://www.semanticweb.org/tswheeler/ontologies/2016/3/EmpowerBP#TDFDomain"/>
        <EmpowerBP:hasEffectiveInterventionFunction rdf:resource="http://www.semanticweb.org/tswheeler/ontologies/2016/3/EmpowerBP#Coercion"/>
        <EmpowerBP:hasEffectiveInterventionFunction rdf:resource="http://www.semanticweb.org/tswheeler/ontologies/2016/3/EmpowerBP#EnvironmentalRestructuring"/>
        <EmpowerBP:hasEffectiveInterventionFunction rdf:resource="http://www.semanticweb.org/tswheeler/ontologies/2016/3/EmpowerBP#Incentivisation"/>
        <EmpowerBP:hasEffectiveInterventionFunction rdf:resource="http://www.semanticweb.org/tswheeler/ontologies/2016/3/EmpowerBP#Training"/>
        <EmpowerBP:isRelatedToCOMB rdf:resource="http://www.semanticweb.org/tswheeler/ontologies/2016/3/EmpowerBP#AutomaticMotivation"/>
        <rdfs:comment>Increasing the probability of a response by arranging a dependent relationship, or contingency, between the response and a given stimulus</rdfs:comment>
    </owl:NamedIndividual>
    


    <!-- http://www.semanticweb.org/tswheeler/ontologies/2016/3/EmpowerBP#Restriction -->

    <owl:NamedIndividual rdf:about="http://www.semanticweb.org/tswheeler/ontologies/2016/3/EmpowerBP#Restriction">
        <rdf:type rdf:resource="http://www.semanticweb.org/tswheeler/ontologies/2016/3/EmpowerBP#InterventionFuction"/>
        <EmpowerBP:isEffectiveForTDFDomain rdf:resource="http://www.semanticweb.org/tswheeler/ontologies/2016/3/EmpowerBP#EnvironmentalContextResources"/>
        <EmpowerBP:isEffectiveForTDFDomain rdf:resource="http://www.semanticweb.org/tswheeler/ontologies/2016/3/EmpowerBP#SocialInfluences"/>
        <rdfs:comment>Using rules to reduce the opportunity to engage in the target behaviour (or to increase the target behaviour by reducing the opportunity to engage in competing behaviours).</rdfs:comment>
    </owl:NamedIndividual>
    


    <!-- http://www.semanticweb.org/tswheeler/ontologies/2016/3/EmpowerBP#SaltReductionAMAssessment -->

    <owl:NamedIndividual rdf:about="http://www.semanticweb.org/tswheeler/ontologies/2016/3/EmpowerBP#SaltReductionAMAssessment">
        <rdf:type rdf:resource="http://www.semanticweb.org/tswheeler/ontologies/2016/3/EmpowerBP#Assessment"/>
        <rdf:type rdf:resource="http://www.semanticweb.org/tswheeler/ontologies/2016/3/EmpowerBP#AssessmentItem"/>
        <rdf:type rdf:resource="http://www.semanticweb.org/tswheeler/ontologies/2016/3/EmpowerBP#AutomaticMotivationAssessment"/>
        <rdf:type rdf:resource="http://www.semanticweb.org/tswheeler/ontologies/2016/3/EmpowerBP#COMBAssessment"/>
        <EmpowerBP:evaluatesConstruct rdf:resource="http://www.semanticweb.org/tswheeler/ontologies/2016/3/EmpowerBP#AutomaticMotivation"/>
        <EmpowerBP:isSpecificToGoal rdf:resource="http://www.semanticweb.org/tswheeler/ontologies/2016/3/EmpowerBP#ReduceSaltIntake"/>
    </owl:NamedIndividual>
    


    <!-- http://www.semanticweb.org/tswheeler/ontologies/2016/3/EmpowerBP#SaltReductionPOAssessment -->

    <owl:NamedIndividual rdf:about="http://www.semanticweb.org/tswheeler/ontologies/2016/3/EmpowerBP#SaltReductionPOAssessment">
        <rdf:type rdf:resource="http://www.semanticweb.org/tswheeler/ontologies/2016/3/EmpowerBP#Assessment"/>
        <rdf:type rdf:resource="http://www.semanticweb.org/tswheeler/ontologies/2016/3/EmpowerBP#AssessmentItem"/>
        <rdf:type rdf:resource="http://www.semanticweb.org/tswheeler/ontologies/2016/3/EmpowerBP#COMBAssessment"/>
        <rdf:type rdf:resource="http://www.semanticweb.org/tswheeler/ontologies/2016/3/EmpowerBP#PhysicalOpportunityAssessment"/>
        <EmpowerBP:evaluatesConstruct rdf:resource="http://www.semanticweb.org/tswheeler/ontologies/2016/3/EmpowerBP#PhysicalOpportunity"/>
        <EmpowerBP:isSpecificToGoal rdf:resource="http://www.semanticweb.org/tswheeler/ontologies/2016/3/EmpowerBP#ReduceSaltIntake"/>
    </owl:NamedIndividual>
    


    <!-- http://www.semanticweb.org/tswheeler/ontologies/2016/3/EmpowerBP#SaltReductionPhysCAssessment -->

    <owl:NamedIndividual rdf:about="http://www.semanticweb.org/tswheeler/ontologies/2016/3/EmpowerBP#SaltReductionPhysCAssessment">
        <rdf:type rdf:resource="http://www.semanticweb.org/tswheeler/ontologies/2016/3/EmpowerBP#Assessment"/>
        <rdf:type rdf:resource="http://www.semanticweb.org/tswheeler/ontologies/2016/3/EmpowerBP#AssessmentItem"/>
        <rdf:type rdf:resource="http://www.semanticweb.org/tswheeler/ontologies/2016/3/EmpowerBP#COMBAssessment"/>
        <rdf:type rdf:resource="http://www.semanticweb.org/tswheeler/ontologies/2016/3/EmpowerBP#PhysicalCapabilityAssessment"/>
        <EmpowerBP:evaluatesConstruct rdf:resource="http://www.semanticweb.org/tswheeler/ontologies/2016/3/EmpowerBP#PhysicalCapability"/>
        <EmpowerBP:isSpecificToGoal rdf:resource="http://www.semanticweb.org/tswheeler/ontologies/2016/3/EmpowerBP#ReduceSaltIntake"/>
    </owl:NamedIndividual>
    


    <!-- http://www.semanticweb.org/tswheeler/ontologies/2016/3/EmpowerBP#SaltReductionPsychCAssessment -->

    <owl:NamedIndividual rdf:about="http://www.semanticweb.org/tswheeler/ontologies/2016/3/EmpowerBP#SaltReductionPsychCAssessment">
        <rdf:type rdf:resource="http://www.semanticweb.org/tswheeler/ontologies/2016/3/EmpowerBP#Assessment"/>
        <rdf:type rdf:resource="http://www.semanticweb.org/tswheeler/ontologies/2016/3/EmpowerBP#AssessmentItem"/>
        <rdf:type rdf:resource="http://www.semanticweb.org/tswheeler/ontologies/2016/3/EmpowerBP#COMBAssessment"/>
        <rdf:type rdf:resource="http://www.semanticweb.org/tswheeler/ontologies/2016/3/EmpowerBP#PsychologicalCapabilityAssessment"/>
        <EmpowerBP:evaluatesConstruct rdf:resource="http://www.semanticweb.org/tswheeler/ontologies/2016/3/EmpowerBP#PsychologicalCapability"/>
        <EmpowerBP:isSpecificToGoal rdf:resource="http://www.semanticweb.org/tswheeler/ontologies/2016/3/EmpowerBP#ReduceSaltIntake"/>
    </owl:NamedIndividual>
    


    <!-- http://www.semanticweb.org/tswheeler/ontologies/2016/3/EmpowerBP#SaltReductionRMAssessment -->

    <owl:NamedIndividual rdf:about="http://www.semanticweb.org/tswheeler/ontologies/2016/3/EmpowerBP#SaltReductionRMAssessment">
        <rdf:type rdf:resource="http://www.semanticweb.org/tswheeler/ontologies/2016/3/EmpowerBP#Assessment"/>
        <rdf:type rdf:resource="http://www.semanticweb.org/tswheeler/ontologies/2016/3/EmpowerBP#AssessmentItem"/>
        <rdf:type rdf:resource="http://www.semanticweb.org/tswheeler/ontologies/2016/3/EmpowerBP#COMBAssessment"/>
        <rdf:type rdf:resource="http://www.semanticweb.org/tswheeler/ontologies/2016/3/EmpowerBP#ReflectiveMotivationAssessment"/>
        <EmpowerBP:evaluatesConstruct rdf:resource="http://www.semanticweb.org/tswheeler/ontologies/2016/3/EmpowerBP#ReflectiveMotivation"/>
        <EmpowerBP:isSpecificToGoal rdf:resource="http://www.semanticweb.org/tswheeler/ontologies/2016/3/EmpowerBP#ReduceSaltIntake"/>
    </owl:NamedIndividual>
    


    <!-- http://www.semanticweb.org/tswheeler/ontologies/2016/3/EmpowerBP#SaltReductionSOAssessment -->

    <owl:NamedIndividual rdf:about="http://www.semanticweb.org/tswheeler/ontologies/2016/3/EmpowerBP#SaltReductionSOAssessment">
        <rdf:type rdf:resource="http://www.semanticweb.org/tswheeler/ontologies/2016/3/EmpowerBP#Assessment"/>
        <rdf:type rdf:resource="http://www.semanticweb.org/tswheeler/ontologies/2016/3/EmpowerBP#AssessmentItem"/>
        <rdf:type rdf:resource="http://www.semanticweb.org/tswheeler/ontologies/2016/3/EmpowerBP#COMBAssessment"/>
        <rdf:type rdf:resource="http://www.semanticweb.org/tswheeler/ontologies/2016/3/EmpowerBP#SocialOpportunityAssessment"/>
        <EmpowerBP:evaluatesConstruct rdf:resource="http://www.semanticweb.org/tswheeler/ontologies/2016/3/EmpowerBP#SocialOpportunity"/>
        <EmpowerBP:isSpecificToGoal rdf:resource="http://www.semanticweb.org/tswheeler/ontologies/2016/3/EmpowerBP#ReduceSaltIntake"/>
    </owl:NamedIndividual>
    


    <!-- http://www.semanticweb.org/tswheeler/ontologies/2016/3/EmpowerBP#SocialInfluences -->

    <owl:NamedIndividual rdf:about="http://www.semanticweb.org/tswheeler/ontologies/2016/3/EmpowerBP#SocialInfluences">
        <rdf:type rdf:resource="http://www.semanticweb.org/tswheeler/ontologies/2016/3/EmpowerBP#Construct"/>
        <rdf:type rdf:resource="http://www.semanticweb.org/tswheeler/ontologies/2016/3/EmpowerBP#TDFDomain"/>
        <EmpowerBP:hasEffectiveInterventionFunction rdf:resource="http://www.semanticweb.org/tswheeler/ontologies/2016/3/EmpowerBP#Enablement"/>
        <EmpowerBP:hasEffectiveInterventionFunction rdf:resource="http://www.semanticweb.org/tswheeler/ontologies/2016/3/EmpowerBP#EnvironmentalRestructuring"/>
        <EmpowerBP:hasEffectiveInterventionFunction rdf:resource="http://www.semanticweb.org/tswheeler/ontologies/2016/3/EmpowerBP#Modelling"/>
        <EmpowerBP:hasEffectiveInterventionFunction rdf:resource="http://www.semanticweb.org/tswheeler/ontologies/2016/3/EmpowerBP#Restriction"/>
        <EmpowerBP:isRelatedToCOMB rdf:resource="http://www.semanticweb.org/tswheeler/ontologies/2016/3/EmpowerBP#SocialOpportunity"/>
        <rdfs:comment>Those interpersonal processes that can cause an individual to change their thoughts, feelings, or behaviors</rdfs:comment>
    </owl:NamedIndividual>
    


    <!-- http://www.semanticweb.org/tswheeler/ontologies/2016/3/EmpowerBP#SocialOpportunity -->

    <owl:NamedIndividual rdf:about="http://www.semanticweb.org/tswheeler/ontologies/2016/3/EmpowerBP#SocialOpportunity">
        <rdf:type rdf:resource="http://www.semanticweb.org/tswheeler/ontologies/2016/3/EmpowerBP#COMBConstruct"/>
        <rdf:type rdf:resource="http://www.semanticweb.org/tswheeler/ontologies/2016/3/EmpowerBP#Construct"/>
        <rdf:type rdf:resource="http://www.semanticweb.org/tswheeler/ontologies/2016/3/EmpowerBP#Opportunity"/>
        <EmpowerBP:isRelatedToTDF rdf:resource="http://www.semanticweb.org/tswheeler/ontologies/2016/3/EmpowerBP#SocialInfluences"/>
        <rdfs:comment>What is allowed by interpersonal influences, social cues and cultural norms</rdfs:comment>
    </owl:NamedIndividual>
    


    <!-- http://www.semanticweb.org/tswheeler/ontologies/2016/3/EmpowerBP#SocialSupportObstacle -->

    <owl:NamedIndividual rdf:about="http://www.semanticweb.org/tswheeler/ontologies/2016/3/EmpowerBP#SocialSupportObstacle">
        <rdf:type rdf:resource="http://www.semanticweb.org/tswheeler/ontologies/2016/3/EmpowerBP#Obstacle"/>
        <EmpowerBP:hasRelevantTDF rdf:resource="http://www.semanticweb.org/tswheeler/ontologies/2016/3/EmpowerBP#SocialInfluences"/>
        <rdfs:comment>Lack of social support (family, friends).</rdfs:comment>
    </owl:NamedIndividual>
    


    <!-- http://www.semanticweb.org/tswheeler/ontologies/2016/3/EmpowerBP#T1 -->

    <owl:NamedIndividual rdf:about="http://www.semanticweb.org/tswheeler/ontologies/2016/3/EmpowerBP#T1">
        <rdf:type rdf:resource="http://www.semanticweb.org/tswheeler/ontologies/2016/3/EmpowerBP#InterventionItem"/>
        <rdf:type rdf:resource="http://www.semanticweb.org/tswheeler/ontologies/2016/3/EmpowerBP#Tip"/>
        <EmpowerBP:isAppropriateForInterventionGoal rdf:resource="http://www.semanticweb.org/tswheeler/ontologies/2016/3/EmpowerBP#ExerciseMore"/>
        <EmpowerBP:isWarrantedBy rdf:resource="http://purl.bioontology.org/ontology/BCTT#Information_about_health_consequences"/>
        <EmpowerBP:appropriateForAutomaticMotivation rdf:datatype="http://www.w3.org/2001/XMLSchema#integer">3</EmpowerBP:appropriateForAutomaticMotivation>
        <EmpowerBP:appropriateForLocation rdf:datatype="http://www.w3.org/2001/XMLSchema#integer">0</EmpowerBP:appropriateForLocation>
        <EmpowerBP:appropriateForPhysicalCapability rdf:datatype="http://www.w3.org/2001/XMLSchema#integer">3</EmpowerBP:appropriateForPhysicalCapability>
        <EmpowerBP:appropriateForPhysicalOpportunity rdf:datatype="http://www.w3.org/2001/XMLSchema#integer">3</EmpowerBP:appropriateForPhysicalOpportunity>
        <EmpowerBP:appropriateForPsychologicalCapability rdf:datatype="http://www.w3.org/2001/XMLSchema#integer">3</EmpowerBP:appropriateForPsychologicalCapability>
        <EmpowerBP:appropriateForReflectiveMotivation rdf:datatype="http://www.w3.org/2001/XMLSchema#integer">3</EmpowerBP:appropriateForReflectiveMotivation>
        <EmpowerBP:appropriateForSocialOpportunity rdf:datatype="http://www.w3.org/2001/XMLSchema#integer">3</EmpowerBP:appropriateForSocialOpportunity>
        <EmpowerBP:canRepeat rdf:datatype="http://www.w3.org/2001/XMLSchema#integer">26</EmpowerBP:canRepeat>
        <EmpowerBP:itemName rdf:datatype="http://www.w3.org/2001/XMLSchema#string">Risks of Inactivity</EmpowerBP:itemName>
        <EmpowerBP:itemText rdf:datatype="http://www.w3.org/2001/XMLSchema#string">Being inactive is linked to a higher risk of heart disease, stroke and the many disabilities they can cause. In addition, lack of activity may increase your risk for:

• high blood pressure
• high cholesterol
• type 2 diabetes
• osteoporosis
• certain types of cancer
• obesity
• falls and injuries
• depression</EmpowerBP:itemText>
        <EmpowerBP:maximumUserAge rdf:datatype="http://www.w3.org/2001/XMLSchema#integer">120</EmpowerBP:maximumUserAge>
        <EmpowerBP:minimumUserAge rdf:datatype="http://www.w3.org/2001/XMLSchema#integer">18</EmpowerBP:minimumUserAge>
        <EmpowerBP:provideJournal rdf:datatype="http://www.w3.org/2001/XMLSchema#boolean">false</EmpowerBP:provideJournal>
        <EmpowerBP:provideLink rdf:datatype="http://www.w3.org/2001/XMLSchema#boolean">false</EmpowerBP:provideLink>
        <EmpowerBP:sourceURL rdf:datatype="http://www.w3.org/2001/XMLSchema#string">http://www.heartandstroke.ca/get-healthy/stay-active/benefits-of-physical-activity</EmpowerBP:sourceURL>
        <rdfs:comment rdf:datatype="http://www.w3.org/2001/XMLSchema#string">Being inactive is linked to a higher risk of heart disease, stroke and the many disabilities they can cause. In addition, lack of activity may increase your risk for:

• high blood pressure
• high cholesterol
• type 2 diabetes
• osteoporosis
• certain types of cancer
• obesity
• falls and injuries
• depression</rdfs:comment>
        <rdfs:label rdf:datatype="http://www.w3.org/2001/XMLSchema#string">Risks of Inactivity</rdfs:label>
    </owl:NamedIndividual>
    


    <!-- http://www.semanticweb.org/tswheeler/ontologies/2016/3/EmpowerBP#T10 -->

    <owl:NamedIndividual rdf:about="http://www.semanticweb.org/tswheeler/ontologies/2016/3/EmpowerBP#T10">
        <rdf:type rdf:resource="http://www.semanticweb.org/tswheeler/ontologies/2016/3/EmpowerBP#InterventionItem"/>
        <rdf:type rdf:resource="http://www.semanticweb.org/tswheeler/ontologies/2016/3/EmpowerBP#Tip"/>
        <EmpowerBP:isAppropriateForInterventionGoal rdf:resource="http://www.semanticweb.org/tswheeler/ontologies/2016/3/EmpowerBP#ReduceSaltIntake"/>
        <EmpowerBP:isWarrantedBy rdf:resource="http://purl.bioontology.org/ontology/BCTT#Comparative_imagining_of_future_outcomes"/>
        <EmpowerBP:appropriateForAutomaticMotivation rdf:datatype="http://www.w3.org/2001/XMLSchema#integer">3</EmpowerBP:appropriateForAutomaticMotivation>
        <EmpowerBP:appropriateForLocation rdf:datatype="http://www.w3.org/2001/XMLSchema#integer">0</EmpowerBP:appropriateForLocation>
        <EmpowerBP:appropriateForPhysicalCapability rdf:datatype="http://www.w3.org/2001/XMLSchema#integer">3</EmpowerBP:appropriateForPhysicalCapability>
        <EmpowerBP:appropriateForPhysicalOpportunity rdf:datatype="http://www.w3.org/2001/XMLSchema#integer">3</EmpowerBP:appropriateForPhysicalOpportunity>
        <EmpowerBP:appropriateForPsychologicalCapability rdf:datatype="http://www.w3.org/2001/XMLSchema#integer">3</EmpowerBP:appropriateForPsychologicalCapability>
        <EmpowerBP:appropriateForReflectiveMotivation rdf:datatype="http://www.w3.org/2001/XMLSchema#integer">3</EmpowerBP:appropriateForReflectiveMotivation>
        <EmpowerBP:appropriateForSocialOpportunity rdf:datatype="http://www.w3.org/2001/XMLSchema#integer">3</EmpowerBP:appropriateForSocialOpportunity>
        <EmpowerBP:canRepeat rdf:datatype="http://www.w3.org/2001/XMLSchema#integer">26</EmpowerBP:canRepeat>
        <EmpowerBP:itemName rdf:datatype="http://www.w3.org/2001/XMLSchema#string">Sodium and Blood Pressure</EmpowerBP:itemName>
        <EmpowerBP:itemText rdf:datatype="http://www.w3.org/2001/XMLSchema#string">Too much sodium in your diet can lead to high blood pressure

• One of five Canadians have high blood pressure.
• High blood pressure may raise your risk of heart
attack, heart failure, stroke and kidney disease.
• If you have high blood pressure, you may be able
to lower it by cutting back on sodium.
• A healthy, low-sodium diet will also help your blood pressure medications work better</EmpowerBP:itemText>
        <EmpowerBP:maximumUserAge rdf:datatype="http://www.w3.org/2001/XMLSchema#integer">120</EmpowerBP:maximumUserAge>
        <EmpowerBP:minimumUserAge rdf:datatype="http://www.w3.org/2001/XMLSchema#integer">18</EmpowerBP:minimumUserAge>
        <EmpowerBP:provideJournal rdf:datatype="http://www.w3.org/2001/XMLSchema#boolean">false</EmpowerBP:provideJournal>
        <EmpowerBP:provideLink rdf:datatype="http://www.w3.org/2001/XMLSchema#boolean">false</EmpowerBP:provideLink>
        <EmpowerBP:sourceURL rdf:datatype="http://www.w3.org/2001/XMLSchema#string">http://www.hypertension.ca/images/2016_EducationalResources/2015_SaltAndSodiumGetTheFacts_EN_P1004_PREVIEW.pdf</EmpowerBP:sourceURL>
        <rdfs:comment rdf:datatype="http://www.w3.org/2001/XMLSchema#string">Too much sodium in your diet can lead to high blood pressure

• One of five Canadians have high blood pressure.
• High blood pressure may raise your risk of heart
attack, heart failure, stroke and kidney disease.
• If you have high blood pressure, you may be able
to lower it by cutting back on sodium.
• A healthy, low-sodium diet will also help your blood pressure medications work better</rdfs:comment>
        <rdfs:label rdf:datatype="http://www.w3.org/2001/XMLSchema#string">Sodium and Blood Pressure</rdfs:label>
    </owl:NamedIndividual>
    


    <!-- http://www.semanticweb.org/tswheeler/ontologies/2016/3/EmpowerBP#T11 -->

    <owl:NamedIndividual rdf:about="http://www.semanticweb.org/tswheeler/ontologies/2016/3/EmpowerBP#T11">
        <rdf:type rdf:resource="http://www.semanticweb.org/tswheeler/ontologies/2016/3/EmpowerBP#InterventionItem"/>
        <rdf:type rdf:resource="http://www.semanticweb.org/tswheeler/ontologies/2016/3/EmpowerBP#Tip"/>
        <EmpowerBP:isAppropriateForInterventionGoal rdf:resource="http://www.semanticweb.org/tswheeler/ontologies/2016/3/EmpowerBP#ReduceSaltIntake"/>
        <EmpowerBP:isWarrantedBy rdf:resource="http://purl.bioontology.org/ontology/BCTT#Instruction_on_how_to_perform_the_behavior"/>
        <EmpowerBP:appropriateForAutomaticMotivation rdf:datatype="http://www.w3.org/2001/XMLSchema#integer">6</EmpowerBP:appropriateForAutomaticMotivation>
        <EmpowerBP:appropriateForLocation rdf:datatype="http://www.w3.org/2001/XMLSchema#integer">0</EmpowerBP:appropriateForLocation>
        <EmpowerBP:appropriateForPhysicalCapability rdf:datatype="http://www.w3.org/2001/XMLSchema#integer">3</EmpowerBP:appropriateForPhysicalCapability>
        <EmpowerBP:appropriateForPhysicalOpportunity rdf:datatype="http://www.w3.org/2001/XMLSchema#integer">3</EmpowerBP:appropriateForPhysicalOpportunity>
        <EmpowerBP:appropriateForPsychologicalCapability rdf:datatype="http://www.w3.org/2001/XMLSchema#integer">3</EmpowerBP:appropriateForPsychologicalCapability>
        <EmpowerBP:appropriateForReflectiveMotivation rdf:datatype="http://www.w3.org/2001/XMLSchema#integer">6</EmpowerBP:appropriateForReflectiveMotivation>
        <EmpowerBP:appropriateForSocialOpportunity rdf:datatype="http://www.w3.org/2001/XMLSchema#integer">3</EmpowerBP:appropriateForSocialOpportunity>
        <EmpowerBP:canRepeat rdf:datatype="http://www.w3.org/2001/XMLSchema#integer">26</EmpowerBP:canRepeat>
        <EmpowerBP:itemName rdf:datatype="http://www.w3.org/2001/XMLSchema#string">How much sodium do you need each day?</EmpowerBP:itemName>
        <EmpowerBP:itemText rdf:datatype="http://www.w3.org/2001/XMLSchema#string">• Aim to have a daily sodium intake of less than 1500 milligrams (mg). This is equal to the amount of sodium that you would find in 2/3 teaspoon of table salt.
• Most Canadians eat almost double the recommended amount of sodium each day.
• Too much sodium can lead to high blood pressure.</EmpowerBP:itemText>
        <EmpowerBP:maximumUserAge rdf:datatype="http://www.w3.org/2001/XMLSchema#integer">120</EmpowerBP:maximumUserAge>
        <EmpowerBP:minimumUserAge rdf:datatype="http://www.w3.org/2001/XMLSchema#integer">18</EmpowerBP:minimumUserAge>
        <EmpowerBP:provideJournal rdf:datatype="http://www.w3.org/2001/XMLSchema#boolean">false</EmpowerBP:provideJournal>
        <EmpowerBP:provideLink rdf:datatype="http://www.w3.org/2001/XMLSchema#boolean">false</EmpowerBP:provideLink>
        <EmpowerBP:sourceURL rdf:datatype="http://www.w3.org/2001/XMLSchema#string">http://www.hypertension.ca/images/2016_EducationalResources/2015_SaltAndSodiumGetTheFacts_EN_P1004_PREVIEW.pdf</EmpowerBP:sourceURL>
        <rdfs:comment rdf:datatype="http://www.w3.org/2001/XMLSchema#string">• Aim to have a daily sodium intake of less than 1500 milligrams (mg). This is equal to the amount of sodium that you would find in 2/3 teaspoon of table salt.
• Most Canadians eat almost double the recommended amount of sodium each day.
• Too much sodium can lead to high blood pressure.</rdfs:comment>
        <rdfs:label rdf:datatype="http://www.w3.org/2001/XMLSchema#string">How much sodium do you need each day?</rdfs:label>
    </owl:NamedIndividual>
    


    <!-- http://www.semanticweb.org/tswheeler/ontologies/2016/3/EmpowerBP#T12 -->

    <owl:NamedIndividual rdf:about="http://www.semanticweb.org/tswheeler/ontologies/2016/3/EmpowerBP#T12">
        <rdf:type rdf:resource="http://www.semanticweb.org/tswheeler/ontologies/2016/3/EmpowerBP#InterventionItem"/>
        <rdf:type rdf:resource="http://www.semanticweb.org/tswheeler/ontologies/2016/3/EmpowerBP#Tip"/>
        <EmpowerBP:isAppropriateForInterventionGoal rdf:resource="http://www.semanticweb.org/tswheeler/ontologies/2016/3/EmpowerBP#ReduceSaltIntake"/>
        <EmpowerBP:isWarrantedBy rdf:resource="http://purl.bioontology.org/ontology/BCTT#Demonstration_of_the_behavior"/>
        <EmpowerBP:appropriateForAutomaticMotivation rdf:datatype="http://www.w3.org/2001/XMLSchema#integer">6</EmpowerBP:appropriateForAutomaticMotivation>
        <EmpowerBP:appropriateForLocation rdf:datatype="http://www.w3.org/2001/XMLSchema#integer">0</EmpowerBP:appropriateForLocation>
        <EmpowerBP:appropriateForPhysicalCapability rdf:datatype="http://www.w3.org/2001/XMLSchema#integer">3</EmpowerBP:appropriateForPhysicalCapability>
        <EmpowerBP:appropriateForPhysicalOpportunity rdf:datatype="http://www.w3.org/2001/XMLSchema#integer">3</EmpowerBP:appropriateForPhysicalOpportunity>
        <EmpowerBP:appropriateForPsychologicalCapability rdf:datatype="http://www.w3.org/2001/XMLSchema#integer">3</EmpowerBP:appropriateForPsychologicalCapability>
        <EmpowerBP:appropriateForReflectiveMotivation rdf:datatype="http://www.w3.org/2001/XMLSchema#integer">6</EmpowerBP:appropriateForReflectiveMotivation>
        <EmpowerBP:appropriateForSocialOpportunity rdf:datatype="http://www.w3.org/2001/XMLSchema#integer">3</EmpowerBP:appropriateForSocialOpportunity>
        <EmpowerBP:canRepeat rdf:datatype="http://www.w3.org/2001/XMLSchema#integer">26</EmpowerBP:canRepeat>
        <EmpowerBP:itemName rdf:datatype="http://www.w3.org/2001/XMLSchema#string">Healthy Low-Sodium Diets</EmpowerBP:itemName>
        <EmpowerBP:itemText rdf:datatype="http://www.w3.org/2001/XMLSchema#string">A healthy, low-sodium diet includes:

• Lots of vegetables and fruits
• Low-fat milk products or alternatives
• Whole grains
• Lean meats, fish, legumes (beans) and nuts</EmpowerBP:itemText>
        <EmpowerBP:maximumUserAge rdf:datatype="http://www.w3.org/2001/XMLSchema#integer">120</EmpowerBP:maximumUserAge>
        <EmpowerBP:minimumUserAge rdf:datatype="http://www.w3.org/2001/XMLSchema#integer">18</EmpowerBP:minimumUserAge>
        <EmpowerBP:provideJournal rdf:datatype="http://www.w3.org/2001/XMLSchema#boolean">false</EmpowerBP:provideJournal>
        <EmpowerBP:provideLink rdf:datatype="http://www.w3.org/2001/XMLSchema#boolean">false</EmpowerBP:provideLink>
        <EmpowerBP:sourceURL rdf:datatype="http://www.w3.org/2001/XMLSchema#string">http://www.hypertension.ca/images/2016_EducationalResources/2015_SaltAndSodiumGetTheFacts_EN_P1004_PREVIEW.pdf</EmpowerBP:sourceURL>
        <rdfs:comment rdf:datatype="http://www.w3.org/2001/XMLSchema#string">A healthy, low-sodium diet includes:

• Lots of vegetables and fruits
• Low-fat milk products or alternatives
• Whole grains
• Lean meats, fish, legumes (beans) and nuts</rdfs:comment>
        <rdfs:label rdf:datatype="http://www.w3.org/2001/XMLSchema#string">Healthy Low-Sodium Diets</rdfs:label>
    </owl:NamedIndividual>
    


    <!-- http://www.semanticweb.org/tswheeler/ontologies/2016/3/EmpowerBP#T13 -->

    <owl:NamedIndividual rdf:about="http://www.semanticweb.org/tswheeler/ontologies/2016/3/EmpowerBP#T13">
        <rdf:type rdf:resource="http://www.semanticweb.org/tswheeler/ontologies/2016/3/EmpowerBP#InterventionItem"/>
        <rdf:type rdf:resource="http://www.semanticweb.org/tswheeler/ontologies/2016/3/EmpowerBP#Tip"/>
        <EmpowerBP:isAppropriateForInterventionGoal rdf:resource="http://www.semanticweb.org/tswheeler/ontologies/2016/3/EmpowerBP#ReduceSaltIntake"/>
        <EmpowerBP:isWarrantedBy rdf:resource="http://purl.bioontology.org/ontology/BCTT#Information_about_social_and_environmental_consequences"/>
        <EmpowerBP:appropriateForAutomaticMotivation rdf:datatype="http://www.w3.org/2001/XMLSchema#integer">3</EmpowerBP:appropriateForAutomaticMotivation>
        <EmpowerBP:appropriateForLocation rdf:datatype="http://www.w3.org/2001/XMLSchema#integer">0</EmpowerBP:appropriateForLocation>
        <EmpowerBP:appropriateForPhysicalCapability rdf:datatype="http://www.w3.org/2001/XMLSchema#integer">3</EmpowerBP:appropriateForPhysicalCapability>
        <EmpowerBP:appropriateForPhysicalOpportunity rdf:datatype="http://www.w3.org/2001/XMLSchema#integer">3</EmpowerBP:appropriateForPhysicalOpportunity>
        <EmpowerBP:appropriateForPsychologicalCapability rdf:datatype="http://www.w3.org/2001/XMLSchema#integer">3</EmpowerBP:appropriateForPsychologicalCapability>
        <EmpowerBP:appropriateForReflectiveMotivation rdf:datatype="http://www.w3.org/2001/XMLSchema#integer">3</EmpowerBP:appropriateForReflectiveMotivation>
        <EmpowerBP:appropriateForSocialOpportunity rdf:datatype="http://www.w3.org/2001/XMLSchema#integer">3</EmpowerBP:appropriateForSocialOpportunity>
        <EmpowerBP:canRepeat rdf:datatype="http://www.w3.org/2001/XMLSchema#integer">26</EmpowerBP:canRepeat>
        <EmpowerBP:itemName rdf:datatype="http://www.w3.org/2001/XMLSchema#string">Dietary Sodium</EmpowerBP:itemName>
        <EmpowerBP:itemText rdf:datatype="http://www.w3.org/2001/XMLSchema#string">Where does the sodium in your diet come from?

1. Most of the sodium in your diet comes from processed foods and restaurant or take-out meals.
• Breads, breakfast cereals, crackers, sweets and bakery products can contain high levels of sodium even though they may not taste salty.
2. Small amounts of sodium also occur naturally in healthy, unprocessed foods.
3. Another source of sodium is the salt and seasonings added during cooking and when you eat.
• All types of salt are high in sodium, including Kosher salt, sea salt, fleur de sel, gourmet salt and smoked salt. They are not healthier choices.</EmpowerBP:itemText>
        <EmpowerBP:maximumUserAge rdf:datatype="http://www.w3.org/2001/XMLSchema#integer">120</EmpowerBP:maximumUserAge>
        <EmpowerBP:minimumUserAge rdf:datatype="http://www.w3.org/2001/XMLSchema#integer">18</EmpowerBP:minimumUserAge>
        <EmpowerBP:provideJournal rdf:datatype="http://www.w3.org/2001/XMLSchema#boolean">false</EmpowerBP:provideJournal>
        <EmpowerBP:provideLink rdf:datatype="http://www.w3.org/2001/XMLSchema#boolean">false</EmpowerBP:provideLink>
        <EmpowerBP:sourceURL rdf:datatype="http://www.w3.org/2001/XMLSchema#string">http://www.hypertension.ca/images/2016_EducationalResources/2015_SaltAndSodiumGetTheFacts_EN_P1004_PREVIEW.pdf</EmpowerBP:sourceURL>
        <rdfs:comment rdf:datatype="http://www.w3.org/2001/XMLSchema#string">Where does the sodium in your diet come from?

1. Most of the sodium in your diet comes from processed foods and restaurant or take-out meals.
• Breads, breakfast cereals, crackers, sweets and bakery products can contain high levels of sodium even though they may not taste salty.
2. Small amounts of sodium also occur naturally in healthy, unprocessed foods.
3. Another source of sodium is the salt and seasonings added during cooking and when you eat.
• All types of salt are high in sodium, including Kosher salt, sea salt, fleur de sel, gourmet salt and smoked salt. They are not healthier choices.</rdfs:comment>
        <rdfs:label rdf:datatype="http://www.w3.org/2001/XMLSchema#string">Dietary Sodium</rdfs:label>
    </owl:NamedIndividual>
    


    <!-- http://www.semanticweb.org/tswheeler/ontologies/2016/3/EmpowerBP#T14 -->

    <owl:NamedIndividual rdf:about="http://www.semanticweb.org/tswheeler/ontologies/2016/3/EmpowerBP#T14">
        <rdf:type rdf:resource="http://www.semanticweb.org/tswheeler/ontologies/2016/3/EmpowerBP#InterventionItem"/>
        <rdf:type rdf:resource="http://www.semanticweb.org/tswheeler/ontologies/2016/3/EmpowerBP#Tip"/>
        <EmpowerBP:isAppropriateForInterventionGoal rdf:resource="http://www.semanticweb.org/tswheeler/ontologies/2016/3/EmpowerBP#ReduceSaltIntake"/>
        <EmpowerBP:isWarrantedBy rdf:resource="http://purl.bioontology.org/ontology/BCTT#Restructuring_the_physical_environment"/>
        <EmpowerBP:appropriateForAutomaticMotivation rdf:datatype="http://www.w3.org/2001/XMLSchema#integer">6</EmpowerBP:appropriateForAutomaticMotivation>
        <EmpowerBP:appropriateForLocation rdf:datatype="http://www.w3.org/2001/XMLSchema#integer">0</EmpowerBP:appropriateForLocation>
        <EmpowerBP:appropriateForPhysicalCapability rdf:datatype="http://www.w3.org/2001/XMLSchema#integer">3</EmpowerBP:appropriateForPhysicalCapability>
        <EmpowerBP:appropriateForPhysicalOpportunity rdf:datatype="http://www.w3.org/2001/XMLSchema#integer">3</EmpowerBP:appropriateForPhysicalOpportunity>
        <EmpowerBP:appropriateForPsychologicalCapability rdf:datatype="http://www.w3.org/2001/XMLSchema#integer">3</EmpowerBP:appropriateForPsychologicalCapability>
        <EmpowerBP:appropriateForReflectiveMotivation rdf:datatype="http://www.w3.org/2001/XMLSchema#integer">6</EmpowerBP:appropriateForReflectiveMotivation>
        <EmpowerBP:appropriateForSocialOpportunity rdf:datatype="http://www.w3.org/2001/XMLSchema#integer">3</EmpowerBP:appropriateForSocialOpportunity>
        <EmpowerBP:canRepeat rdf:datatype="http://www.w3.org/2001/XMLSchema#integer">26</EmpowerBP:canRepeat>
        <EmpowerBP:itemName rdf:datatype="http://www.w3.org/2001/XMLSchema#string">Sodium at the Grocery Store</EmpowerBP:itemName>
        <EmpowerBP:itemText rdf:datatype="http://www.w3.org/2001/XMLSchema#string">Thinking of sodium at the grocery store: 

• Buy fresh or frozen unprocessed foods most often.
• Choose breads, crackers, baked goods, snack foods, sauces, soups, dressings and “healthy choice” items with the lowest sodium per serving.
• Read food labels to choose packaged foods with the lowest sodium.</EmpowerBP:itemText>
        <EmpowerBP:maximumUserAge rdf:datatype="http://www.w3.org/2001/XMLSchema#integer">120</EmpowerBP:maximumUserAge>
        <EmpowerBP:minimumUserAge rdf:datatype="http://www.w3.org/2001/XMLSchema#integer">18</EmpowerBP:minimumUserAge>
        <EmpowerBP:provideJournal rdf:datatype="http://www.w3.org/2001/XMLSchema#boolean">false</EmpowerBP:provideJournal>
        <EmpowerBP:provideLink rdf:datatype="http://www.w3.org/2001/XMLSchema#boolean">false</EmpowerBP:provideLink>
        <EmpowerBP:sourceURL rdf:datatype="http://www.w3.org/2001/XMLSchema#string">http://www.hypertension.ca/images/2016_EducationalResources/2015_SaltAndSodiumGetTheFacts_EN_P1004_PREVIEW.pdf</EmpowerBP:sourceURL>
        <rdfs:comment rdf:datatype="http://www.w3.org/2001/XMLSchema#string">Thinking of sodium at the grocery store: 

• Buy fresh or frozen unprocessed foods most often.
• Choose breads, crackers, baked goods, snack foods, sauces, soups, dressings and “healthy choice” items with the lowest sodium per serving.
• Read food labels to choose packaged foods with the lowest sodium.</rdfs:comment>
        <rdfs:label rdf:datatype="http://www.w3.org/2001/XMLSchema#string">Sodium at the Grocery Store</rdfs:label>
    </owl:NamedIndividual>
    


    <!-- http://www.semanticweb.org/tswheeler/ontologies/2016/3/EmpowerBP#T15 -->

    <owl:NamedIndividual rdf:about="http://www.semanticweb.org/tswheeler/ontologies/2016/3/EmpowerBP#T15">
        <rdf:type rdf:resource="http://www.semanticweb.org/tswheeler/ontologies/2016/3/EmpowerBP#InterventionItem"/>
        <rdf:type rdf:resource="http://www.semanticweb.org/tswheeler/ontologies/2016/3/EmpowerBP#Tip"/>
        <EmpowerBP:isAppropriateForInterventionGoal rdf:resource="http://www.semanticweb.org/tswheeler/ontologies/2016/3/EmpowerBP#ReduceSaltIntake"/>
        <EmpowerBP:isWarrantedBy rdf:resource="http://purl.bioontology.org/ontology/BCTT#Restructuring_the_physical_environment"/>
        <EmpowerBP:appropriateForAutomaticMotivation rdf:datatype="http://www.w3.org/2001/XMLSchema#integer">6</EmpowerBP:appropriateForAutomaticMotivation>
        <EmpowerBP:appropriateForLocation rdf:datatype="http://www.w3.org/2001/XMLSchema#integer">0</EmpowerBP:appropriateForLocation>
        <EmpowerBP:appropriateForPhysicalCapability rdf:datatype="http://www.w3.org/2001/XMLSchema#integer">3</EmpowerBP:appropriateForPhysicalCapability>
        <EmpowerBP:appropriateForPhysicalOpportunity rdf:datatype="http://www.w3.org/2001/XMLSchema#integer">3</EmpowerBP:appropriateForPhysicalOpportunity>
        <EmpowerBP:appropriateForPsychologicalCapability rdf:datatype="http://www.w3.org/2001/XMLSchema#integer">3</EmpowerBP:appropriateForPsychologicalCapability>
        <EmpowerBP:appropriateForReflectiveMotivation rdf:datatype="http://www.w3.org/2001/XMLSchema#integer">6</EmpowerBP:appropriateForReflectiveMotivation>
        <EmpowerBP:appropriateForSocialOpportunity rdf:datatype="http://www.w3.org/2001/XMLSchema#integer">3</EmpowerBP:appropriateForSocialOpportunity>
        <EmpowerBP:canRepeat rdf:datatype="http://www.w3.org/2001/XMLSchema#integer">26</EmpowerBP:canRepeat>
        <EmpowerBP:itemName rdf:datatype="http://www.w3.org/2001/XMLSchema#string">Nutrition Facts Label</EmpowerBP:itemName>
        <EmpowerBP:itemText rdf:datatype="http://www.w3.org/2001/XMLSchema#string">The Nutrition Facts label can help you choose foods lower in sodium

• Check the serving size and note the amount of sodium.
• Choose foods with less than 120 mg sodium per serving.
• Choose foods with sodium that has a % Daily Value (DV) of 5% or less.</EmpowerBP:itemText>
        <EmpowerBP:maximumUserAge rdf:datatype="http://www.w3.org/2001/XMLSchema#integer">120</EmpowerBP:maximumUserAge>
        <EmpowerBP:minimumUserAge rdf:datatype="http://www.w3.org/2001/XMLSchema#integer">18</EmpowerBP:minimumUserAge>
        <EmpowerBP:provideJournal rdf:datatype="http://www.w3.org/2001/XMLSchema#boolean">false</EmpowerBP:provideJournal>
        <EmpowerBP:provideLink rdf:datatype="http://www.w3.org/2001/XMLSchema#boolean">false</EmpowerBP:provideLink>
        <EmpowerBP:sourceURL rdf:datatype="http://www.w3.org/2001/XMLSchema#string">http://www.hypertension.ca/images/2016_EducationalResources/2015_SaltAndSodiumGetTheFacts_EN_P1004_PREVIEW.pdf</EmpowerBP:sourceURL>
        <rdfs:comment rdf:datatype="http://www.w3.org/2001/XMLSchema#string">The Nutrition Facts label can help you choose foods lower in sodium

• Check the serving size and note the amount of sodium.
• Choose foods with less than 120 mg sodium per serving.
• Choose foods with sodium that has a % Daily Value (DV) of 5% or less.</rdfs:comment>
        <rdfs:label rdf:datatype="http://www.w3.org/2001/XMLSchema#string">Nutrition Facts Label</rdfs:label>
    </owl:NamedIndividual>
    


    <!-- http://www.semanticweb.org/tswheeler/ontologies/2016/3/EmpowerBP#T16 -->

    <owl:NamedIndividual rdf:about="http://www.semanticweb.org/tswheeler/ontologies/2016/3/EmpowerBP#T16">
        <rdf:type rdf:resource="http://www.semanticweb.org/tswheeler/ontologies/2016/3/EmpowerBP#InterventionItem"/>
        <rdf:type rdf:resource="http://www.semanticweb.org/tswheeler/ontologies/2016/3/EmpowerBP#Tip"/>
        <EmpowerBP:isAppropriateForInterventionGoal rdf:resource="http://www.semanticweb.org/tswheeler/ontologies/2016/3/EmpowerBP#ReduceSaltIntake"/>
        <EmpowerBP:isWarrantedBy rdf:resource="http://purl.bioontology.org/ontology/BCTT#Behavior_substitution"/>
        <EmpowerBP:appropriateForAutomaticMotivation rdf:datatype="http://www.w3.org/2001/XMLSchema#integer">6</EmpowerBP:appropriateForAutomaticMotivation>
        <EmpowerBP:appropriateForLocation rdf:datatype="http://www.w3.org/2001/XMLSchema#integer">0</EmpowerBP:appropriateForLocation>
        <EmpowerBP:appropriateForPhysicalCapability rdf:datatype="http://www.w3.org/2001/XMLSchema#integer">3</EmpowerBP:appropriateForPhysicalCapability>
        <EmpowerBP:appropriateForPhysicalOpportunity rdf:datatype="http://www.w3.org/2001/XMLSchema#integer">3</EmpowerBP:appropriateForPhysicalOpportunity>
        <EmpowerBP:appropriateForPsychologicalCapability rdf:datatype="http://www.w3.org/2001/XMLSchema#integer">3</EmpowerBP:appropriateForPsychologicalCapability>
        <EmpowerBP:appropriateForReflectiveMotivation rdf:datatype="http://www.w3.org/2001/XMLSchema#integer">6</EmpowerBP:appropriateForReflectiveMotivation>
        <EmpowerBP:appropriateForSocialOpportunity rdf:datatype="http://www.w3.org/2001/XMLSchema#integer">3</EmpowerBP:appropriateForSocialOpportunity>
        <EmpowerBP:canRepeat rdf:datatype="http://www.w3.org/2001/XMLSchema#integer">26</EmpowerBP:canRepeat>
        <EmpowerBP:itemName rdf:datatype="http://www.w3.org/2001/XMLSchema#string">Sodium at Home</EmpowerBP:itemName>
        <EmpowerBP:itemText rdf:datatype="http://www.w3.org/2001/XMLSchema#string">Thinking of sodium when eating at home:

• Prepare and eat more unprocessed and home made foods. 
• Avoid adding salt when cooking and baking.   
• Use lemon juice, lime, herbs and spices to add flavour without sodium.
• Use less ketchup, mustard, soy sauce, pickles, olives, prepared gravies, sauces and salad dressings.
</EmpowerBP:itemText>
        <EmpowerBP:maximumUserAge rdf:datatype="http://www.w3.org/2001/XMLSchema#integer">120</EmpowerBP:maximumUserAge>
        <EmpowerBP:minimumUserAge rdf:datatype="http://www.w3.org/2001/XMLSchema#integer">18</EmpowerBP:minimumUserAge>
        <EmpowerBP:provideJournal rdf:datatype="http://www.w3.org/2001/XMLSchema#boolean">false</EmpowerBP:provideJournal>
        <EmpowerBP:provideLink rdf:datatype="http://www.w3.org/2001/XMLSchema#boolean">false</EmpowerBP:provideLink>
        <EmpowerBP:sourceURL rdf:datatype="http://www.w3.org/2001/XMLSchema#string">http://www.hypertension.ca/images/2016_EducationalResources/2015_SaltAndSodiumGetTheFacts_EN_P1004_PREVIEW.pdf</EmpowerBP:sourceURL>
        <rdfs:comment rdf:datatype="http://www.w3.org/2001/XMLSchema#string">Thinking of sodium when eating at home:

• Prepare and eat more unprocessed and home made foods. 
• Avoid adding salt when cooking and baking.   
• Use lemon juice, lime, herbs and spices to add flavour without sodium.
• Use less ketchup, mustard, soy sauce, pickles, olives, prepared gravies, sauces and salad dressings.
</rdfs:comment>
        <rdfs:label rdf:datatype="http://www.w3.org/2001/XMLSchema#string">Sodium at Home</rdfs:label>
    </owl:NamedIndividual>
    


    <!-- http://www.semanticweb.org/tswheeler/ontologies/2016/3/EmpowerBP#T17 -->

    <owl:NamedIndividual rdf:about="http://www.semanticweb.org/tswheeler/ontologies/2016/3/EmpowerBP#T17">
        <rdf:type rdf:resource="http://www.semanticweb.org/tswheeler/ontologies/2016/3/EmpowerBP#InterventionItem"/>
        <rdf:type rdf:resource="http://www.semanticweb.org/tswheeler/ontologies/2016/3/EmpowerBP#Tip"/>
        <EmpowerBP:isAppropriateForInterventionGoal rdf:resource="http://www.semanticweb.org/tswheeler/ontologies/2016/3/EmpowerBP#ReduceSaltIntake"/>
        <EmpowerBP:isWarrantedBy rdf:resource="http://purl.bioontology.org/ontology/BCTT#Behavior_substitution"/>
        <EmpowerBP:appropriateForAutomaticMotivation rdf:datatype="http://www.w3.org/2001/XMLSchema#integer">6</EmpowerBP:appropriateForAutomaticMotivation>
        <EmpowerBP:appropriateForLocation rdf:datatype="http://www.w3.org/2001/XMLSchema#integer">0</EmpowerBP:appropriateForLocation>
        <EmpowerBP:appropriateForPhysicalCapability rdf:datatype="http://www.w3.org/2001/XMLSchema#integer">3</EmpowerBP:appropriateForPhysicalCapability>
        <EmpowerBP:appropriateForPhysicalOpportunity rdf:datatype="http://www.w3.org/2001/XMLSchema#integer">3</EmpowerBP:appropriateForPhysicalOpportunity>
        <EmpowerBP:appropriateForPsychologicalCapability rdf:datatype="http://www.w3.org/2001/XMLSchema#integer">3</EmpowerBP:appropriateForPsychologicalCapability>
        <EmpowerBP:appropriateForReflectiveMotivation rdf:datatype="http://www.w3.org/2001/XMLSchema#integer">6</EmpowerBP:appropriateForReflectiveMotivation>
        <EmpowerBP:appropriateForSocialOpportunity rdf:datatype="http://www.w3.org/2001/XMLSchema#integer">3</EmpowerBP:appropriateForSocialOpportunity>
        <EmpowerBP:canRepeat rdf:datatype="http://www.w3.org/2001/XMLSchema#integer">26</EmpowerBP:canRepeat>
        <EmpowerBP:itemName rdf:datatype="http://www.w3.org/2001/XMLSchema#string">Sodium at Home</EmpowerBP:itemName>
        <EmpowerBP:itemText rdf:datatype="http://www.w3.org/2001/XMLSchema#string">Thinking of sodium when eating at home: 

• Avoid cured and deli meats.
• Remove the salt shaker from where you eat.
• Use diluted tomato paste instead of tomato sauce, powdered bouillon or canned soup in recipes.
• Do not use sea salt, fleur de sel or flavoured salts (onion, garlic, celery, BBQ etc.) in recipes; they are also high in sodium</EmpowerBP:itemText>
        <EmpowerBP:maximumUserAge rdf:datatype="http://www.w3.org/2001/XMLSchema#integer">120</EmpowerBP:maximumUserAge>
        <EmpowerBP:minimumUserAge rdf:datatype="http://www.w3.org/2001/XMLSchema#integer">18</EmpowerBP:minimumUserAge>
        <EmpowerBP:provideJournal rdf:datatype="http://www.w3.org/2001/XMLSchema#boolean">false</EmpowerBP:provideJournal>
        <EmpowerBP:provideLink rdf:datatype="http://www.w3.org/2001/XMLSchema#boolean">false</EmpowerBP:provideLink>
        <EmpowerBP:sourceURL rdf:datatype="http://www.w3.org/2001/XMLSchema#string">http://www.hypertension.ca/images/2016_EducationalResources/2015_SaltAndSodiumGetTheFacts_EN_P1004_PREVIEW.pdf</EmpowerBP:sourceURL>
        <rdfs:comment rdf:datatype="http://www.w3.org/2001/XMLSchema#string">Thinking of sodium when eating at home: 

• Avoid cured and deli meats.
• Remove the salt shaker from where you eat.
• Use diluted tomato paste instead of tomato sauce, powdered bouillon or canned soup in recipes.
• Do not use sea salt, fleur de sel or flavoured salts (onion, garlic, celery, BBQ etc.) in recipes; they are also high in sodium</rdfs:comment>
        <rdfs:label rdf:datatype="http://www.w3.org/2001/XMLSchema#string">Sodium at Home</rdfs:label>
    </owl:NamedIndividual>
    


    <!-- http://www.semanticweb.org/tswheeler/ontologies/2016/3/EmpowerBP#T18 -->

    <owl:NamedIndividual rdf:about="http://www.semanticweb.org/tswheeler/ontologies/2016/3/EmpowerBP#T18">
        <rdf:type rdf:resource="http://www.semanticweb.org/tswheeler/ontologies/2016/3/EmpowerBP#InterventionItem"/>
        <rdf:type rdf:resource="http://www.semanticweb.org/tswheeler/ontologies/2016/3/EmpowerBP#Tip"/>
        <EmpowerBP:isAppropriateForInterventionGoal rdf:resource="http://www.semanticweb.org/tswheeler/ontologies/2016/3/EmpowerBP#ReduceSaltIntake"/>
        <EmpowerBP:isWarrantedBy rdf:resource="http://purl.bioontology.org/ontology/BCTT#Behavior_substitution"/>
        <EmpowerBP:appropriateForAutomaticMotivation rdf:datatype="http://www.w3.org/2001/XMLSchema#integer">6</EmpowerBP:appropriateForAutomaticMotivation>
        <EmpowerBP:appropriateForLocation rdf:datatype="http://www.w3.org/2001/XMLSchema#integer">0</EmpowerBP:appropriateForLocation>
        <EmpowerBP:appropriateForPhysicalCapability rdf:datatype="http://www.w3.org/2001/XMLSchema#integer">3</EmpowerBP:appropriateForPhysicalCapability>
        <EmpowerBP:appropriateForPhysicalOpportunity rdf:datatype="http://www.w3.org/2001/XMLSchema#integer">3</EmpowerBP:appropriateForPhysicalOpportunity>
        <EmpowerBP:appropriateForPsychologicalCapability rdf:datatype="http://www.w3.org/2001/XMLSchema#integer">3</EmpowerBP:appropriateForPsychologicalCapability>
        <EmpowerBP:appropriateForReflectiveMotivation rdf:datatype="http://www.w3.org/2001/XMLSchema#integer">6</EmpowerBP:appropriateForReflectiveMotivation>
        <EmpowerBP:appropriateForSocialOpportunity rdf:datatype="http://www.w3.org/2001/XMLSchema#integer">3</EmpowerBP:appropriateForSocialOpportunity>
        <EmpowerBP:canRepeat rdf:datatype="http://www.w3.org/2001/XMLSchema#integer">26</EmpowerBP:canRepeat>
        <EmpowerBP:itemName rdf:datatype="http://www.w3.org/2001/XMLSchema#string">Sodium on the Go</EmpowerBP:itemName>
        <EmpowerBP:itemText rdf:datatype="http://www.w3.org/2001/XMLSchema#string">Thinking of sodium when eating restaurant or take-out meals:

• Choose dishes made from fresh, low-sodium ingredients.
• Ask for less salt and other seasonings, like MSG (monosodium glutamate), to be added to your food.
• Ask for gravy, sauces and salad dressings “on the side”, and use lightly.
• Check the nutrition information of menu items to help you order and choose foods with less sodium. This information may be on a menu, poster or pamphlet at the restaurant or on their website.</EmpowerBP:itemText>
        <EmpowerBP:maximumUserAge rdf:datatype="http://www.w3.org/2001/XMLSchema#integer">120</EmpowerBP:maximumUserAge>
        <EmpowerBP:minimumUserAge rdf:datatype="http://www.w3.org/2001/XMLSchema#integer">18</EmpowerBP:minimumUserAge>
        <EmpowerBP:provideJournal rdf:datatype="http://www.w3.org/2001/XMLSchema#boolean">false</EmpowerBP:provideJournal>
        <EmpowerBP:provideLink rdf:datatype="http://www.w3.org/2001/XMLSchema#boolean">false</EmpowerBP:provideLink>
        <EmpowerBP:sourceURL rdf:datatype="http://www.w3.org/2001/XMLSchema#string">http://www.hypertension.ca/images/2016_EducationalResources/2015_SaltAndSodiumGetTheFacts_EN_P1004_PREVIEW.pdf</EmpowerBP:sourceURL>
        <rdfs:comment rdf:datatype="http://www.w3.org/2001/XMLSchema#string">Thinking of sodium when eating restaurant or take-out meals:

• Choose dishes made from fresh, low-sodium ingredients.
• Ask for less salt and other seasonings, like MSG (monosodium glutamate), to be added to your food.
• Ask for gravy, sauces and salad dressings “on the side”, and use lightly.
• Check the nutrition information of menu items to help you order and choose foods with less sodium. This information may be on a menu, poster or pamphlet at the restaurant or on their website.</rdfs:comment>
        <rdfs:label rdf:datatype="http://www.w3.org/2001/XMLSchema#string">Sodium on the Go</rdfs:label>
    </owl:NamedIndividual>
    


    <!-- http://www.semanticweb.org/tswheeler/ontologies/2016/3/EmpowerBP#T19 -->

    <owl:NamedIndividual rdf:about="http://www.semanticweb.org/tswheeler/ontologies/2016/3/EmpowerBP#T19">
        <rdf:type rdf:resource="http://www.semanticweb.org/tswheeler/ontologies/2016/3/EmpowerBP#InterventionItem"/>
        <rdf:type rdf:resource="http://www.semanticweb.org/tswheeler/ontologies/2016/3/EmpowerBP#Tip"/>
        <EmpowerBP:isAppropriateForInterventionGoal rdf:resource="http://www.semanticweb.org/tswheeler/ontologies/2016/3/EmpowerBP#ReduceSaltIntake"/>
        <EmpowerBP:isWarrantedBy rdf:resource="http://purl.bioontology.org/ontology/BCTT#Information_about_health_consequences"/>
        <EmpowerBP:appropriateForAutomaticMotivation rdf:datatype="http://www.w3.org/2001/XMLSchema#integer">3</EmpowerBP:appropriateForAutomaticMotivation>
        <EmpowerBP:appropriateForLocation rdf:datatype="http://www.w3.org/2001/XMLSchema#integer">0</EmpowerBP:appropriateForLocation>
        <EmpowerBP:appropriateForPhysicalCapability rdf:datatype="http://www.w3.org/2001/XMLSchema#integer">3</EmpowerBP:appropriateForPhysicalCapability>
        <EmpowerBP:appropriateForPhysicalOpportunity rdf:datatype="http://www.w3.org/2001/XMLSchema#integer">3</EmpowerBP:appropriateForPhysicalOpportunity>
        <EmpowerBP:appropriateForPsychologicalCapability rdf:datatype="http://www.w3.org/2001/XMLSchema#integer">3</EmpowerBP:appropriateForPsychologicalCapability>
        <EmpowerBP:appropriateForReflectiveMotivation rdf:datatype="http://www.w3.org/2001/XMLSchema#integer">3</EmpowerBP:appropriateForReflectiveMotivation>
        <EmpowerBP:appropriateForSocialOpportunity rdf:datatype="http://www.w3.org/2001/XMLSchema#integer">3</EmpowerBP:appropriateForSocialOpportunity>
        <EmpowerBP:canRepeat rdf:datatype="http://www.w3.org/2001/XMLSchema#integer">26</EmpowerBP:canRepeat>
        <EmpowerBP:itemName rdf:datatype="http://www.w3.org/2001/XMLSchema#string">Sodium Facts</EmpowerBP:itemName>
        <EmpowerBP:itemText rdf:datatype="http://www.w3.org/2001/XMLSchema#string">Information about Sodium

• Sodium is a mineral found in salt. All salts are high in sodium.
• Sodium is needed by the body to control blood pressure. It also helps with muscle and nerve function.
• Eating too much sodium can lead to health problems. These include high blood pressure, heart disease, stroke and kidney disease. 
 </EmpowerBP:itemText>
        <EmpowerBP:maximumUserAge rdf:datatype="http://www.w3.org/2001/XMLSchema#integer">120</EmpowerBP:maximumUserAge>
        <EmpowerBP:minimumUserAge rdf:datatype="http://www.w3.org/2001/XMLSchema#integer">18</EmpowerBP:minimumUserAge>
        <EmpowerBP:provideJournal rdf:datatype="http://www.w3.org/2001/XMLSchema#boolean">false</EmpowerBP:provideJournal>
        <EmpowerBP:provideLink rdf:datatype="http://www.w3.org/2001/XMLSchema#boolean">false</EmpowerBP:provideLink>
        <EmpowerBP:sourceURL rdf:datatype="http://www.w3.org/2001/XMLSchema#string">http://www.dietitians.ca/Your-Health/Nutrition-A-Z/Minerals/Food-Sources-of-Sodium.aspx</EmpowerBP:sourceURL>
        <rdfs:comment rdf:datatype="http://www.w3.org/2001/XMLSchema#string">Information about Sodium

• Sodium is a mineral found in salt. All salts are high in sodium.
• Sodium is needed by the body to control blood pressure. It also helps with muscle and nerve function.
• Eating too much sodium can lead to health problems. These include high blood pressure, heart disease, stroke and kidney disease. 
 </rdfs:comment>
        <rdfs:label rdf:datatype="http://www.w3.org/2001/XMLSchema#string">Sodium Facts</rdfs:label>
    </owl:NamedIndividual>
    


    <!-- http://www.semanticweb.org/tswheeler/ontologies/2016/3/EmpowerBP#T2 -->

    <owl:NamedIndividual rdf:about="http://www.semanticweb.org/tswheeler/ontologies/2016/3/EmpowerBP#T2">
        <rdf:type rdf:resource="http://www.semanticweb.org/tswheeler/ontologies/2016/3/EmpowerBP#InterventionItem"/>
        <rdf:type rdf:resource="http://www.semanticweb.org/tswheeler/ontologies/2016/3/EmpowerBP#Tip"/>
        <EmpowerBP:isAppropriateForInterventionGoal rdf:resource="http://www.semanticweb.org/tswheeler/ontologies/2016/3/EmpowerBP#ExerciseMore"/>
        <EmpowerBP:isWarrantedBy rdf:resource="http://purl.bioontology.org/ontology/BCTT#Imaginary_reward"/>
        <EmpowerBP:appropriateForAutomaticMotivation rdf:datatype="http://www.w3.org/2001/XMLSchema#integer">3</EmpowerBP:appropriateForAutomaticMotivation>
        <EmpowerBP:appropriateForLocation rdf:datatype="http://www.w3.org/2001/XMLSchema#integer">0</EmpowerBP:appropriateForLocation>
        <EmpowerBP:appropriateForPhysicalCapability rdf:datatype="http://www.w3.org/2001/XMLSchema#integer">3</EmpowerBP:appropriateForPhysicalCapability>
        <EmpowerBP:appropriateForPhysicalOpportunity rdf:datatype="http://www.w3.org/2001/XMLSchema#integer">3</EmpowerBP:appropriateForPhysicalOpportunity>
        <EmpowerBP:appropriateForPsychologicalCapability rdf:datatype="http://www.w3.org/2001/XMLSchema#integer">3</EmpowerBP:appropriateForPsychologicalCapability>
        <EmpowerBP:appropriateForReflectiveMotivation rdf:datatype="http://www.w3.org/2001/XMLSchema#integer">3</EmpowerBP:appropriateForReflectiveMotivation>
        <EmpowerBP:appropriateForSocialOpportunity rdf:datatype="http://www.w3.org/2001/XMLSchema#integer">3</EmpowerBP:appropriateForSocialOpportunity>
        <EmpowerBP:canRepeat rdf:datatype="http://www.w3.org/2001/XMLSchema#integer">26</EmpowerBP:canRepeat>
        <EmpowerBP:itemName rdf:datatype="http://www.w3.org/2001/XMLSchema#string">Benefits of Activity</EmpowerBP:itemName>
        <EmpowerBP:itemText rdf:datatype="http://www.w3.org/2001/XMLSchema#string">You may see benefits of exercise within the first week of regular activity.

For example, your blood pressure may improve and you could start to feel more energetic and relaxed. After three months, you may experience better health, improved posture and balance, stronger muscles and bones, more confidence and a more positive outlook on life.</EmpowerBP:itemText>
        <EmpowerBP:maximumUserAge rdf:datatype="http://www.w3.org/2001/XMLSchema#integer">120</EmpowerBP:maximumUserAge>
        <EmpowerBP:minimumUserAge rdf:datatype="http://www.w3.org/2001/XMLSchema#integer">18</EmpowerBP:minimumUserAge>
        <EmpowerBP:provideJournal rdf:datatype="http://www.w3.org/2001/XMLSchema#boolean">false</EmpowerBP:provideJournal>
        <EmpowerBP:provideLink rdf:datatype="http://www.w3.org/2001/XMLSchema#boolean">false</EmpowerBP:provideLink>
        <EmpowerBP:sourceURL rdf:datatype="http://www.w3.org/2001/XMLSchema#string">http://www.heartandstroke.ca/get-healthy/stay-active/benefits-of-physical-activity</EmpowerBP:sourceURL>
        <rdfs:comment rdf:datatype="http://www.w3.org/2001/XMLSchema#string">You may see benefits of exercise within the first week of regular activity.

For example, your blood pressure may improve and you could start to feel more energetic and relaxed. After three months, you may experience better health, improved posture and balance, stronger muscles and bones, more confidence and a more positive outlook on life.</rdfs:comment>
        <rdfs:label rdf:datatype="http://www.w3.org/2001/XMLSchema#string">Benefits of Activity</rdfs:label>
    </owl:NamedIndividual>
    


    <!-- http://www.semanticweb.org/tswheeler/ontologies/2016/3/EmpowerBP#T20 -->

    <owl:NamedIndividual rdf:about="http://www.semanticweb.org/tswheeler/ontologies/2016/3/EmpowerBP#T20">
        <rdf:type rdf:resource="http://www.semanticweb.org/tswheeler/ontologies/2016/3/EmpowerBP#InterventionItem"/>
        <rdf:type rdf:resource="http://www.semanticweb.org/tswheeler/ontologies/2016/3/EmpowerBP#Tip"/>
        <EmpowerBP:isAppropriateForInterventionGoal rdf:resource="http://www.semanticweb.org/tswheeler/ontologies/2016/3/EmpowerBP#ReduceSaltIntake"/>
        <EmpowerBP:isWarrantedBy rdf:resource="http://purl.bioontology.org/ontology/BCTT#Behavior_substitution"/>
        <EmpowerBP:appropriateForAutomaticMotivation rdf:datatype="http://www.w3.org/2001/XMLSchema#integer">6</EmpowerBP:appropriateForAutomaticMotivation>
        <EmpowerBP:appropriateForLocation rdf:datatype="http://www.w3.org/2001/XMLSchema#integer">0</EmpowerBP:appropriateForLocation>
        <EmpowerBP:appropriateForPhysicalCapability rdf:datatype="http://www.w3.org/2001/XMLSchema#integer">3</EmpowerBP:appropriateForPhysicalCapability>
        <EmpowerBP:appropriateForPhysicalOpportunity rdf:datatype="http://www.w3.org/2001/XMLSchema#integer">3</EmpowerBP:appropriateForPhysicalOpportunity>
        <EmpowerBP:appropriateForPsychologicalCapability rdf:datatype="http://www.w3.org/2001/XMLSchema#integer">3</EmpowerBP:appropriateForPsychologicalCapability>
        <EmpowerBP:appropriateForReflectiveMotivation rdf:datatype="http://www.w3.org/2001/XMLSchema#integer">6</EmpowerBP:appropriateForReflectiveMotivation>
        <EmpowerBP:appropriateForSocialOpportunity rdf:datatype="http://www.w3.org/2001/XMLSchema#integer">3</EmpowerBP:appropriateForSocialOpportunity>
        <EmpowerBP:canRepeat rdf:datatype="http://www.w3.org/2001/XMLSchema#integer">26</EmpowerBP:canRepeat>
        <EmpowerBP:itemName rdf:datatype="http://www.w3.org/2001/XMLSchema#string">Lower sodium options!</EmpowerBP:itemName>
        <EmpowerBP:itemText rdf:datatype="http://www.w3.org/2001/XMLSchema#string">Cut the sodium, keep your health!

Choose more of fresh fruits and vegetables, unsalted popcorn, or unsalted nuts.

Choose less of chips, salted pretzels, or other salty snacks</EmpowerBP:itemText>
        <EmpowerBP:maximumUserAge rdf:datatype="http://www.w3.org/2001/XMLSchema#integer">120</EmpowerBP:maximumUserAge>
        <EmpowerBP:minimumUserAge rdf:datatype="http://www.w3.org/2001/XMLSchema#integer">18</EmpowerBP:minimumUserAge>
        <EmpowerBP:provideJournal rdf:datatype="http://www.w3.org/2001/XMLSchema#boolean">false</EmpowerBP:provideJournal>
        <EmpowerBP:provideLink rdf:datatype="http://www.w3.org/2001/XMLSchema#boolean">false</EmpowerBP:provideLink>
        <EmpowerBP:sourceURL rdf:datatype="http://www.w3.org/2001/XMLSchema#string">http://www.dietitians.ca/Downloads/Factsheets/Sodium-Sense-factsheet-collection.aspx</EmpowerBP:sourceURL>
        <rdfs:comment rdf:datatype="http://www.w3.org/2001/XMLSchema#string">Cut the sodium, keep your health!

Choose more of fresh fruits and vegetables, unsalted popcorn, or unsalted nuts.

Choose less of chips, salted pretzels, or other salty snacks</rdfs:comment>
        <rdfs:label rdf:datatype="http://www.w3.org/2001/XMLSchema#string">Lower sodium options!</rdfs:label>
    </owl:NamedIndividual>
    


    <!-- http://www.semanticweb.org/tswheeler/ontologies/2016/3/EmpowerBP#T21 -->

    <owl:NamedIndividual rdf:about="http://www.semanticweb.org/tswheeler/ontologies/2016/3/EmpowerBP#T21">
        <rdf:type rdf:resource="http://www.semanticweb.org/tswheeler/ontologies/2016/3/EmpowerBP#InterventionItem"/>
        <rdf:type rdf:resource="http://www.semanticweb.org/tswheeler/ontologies/2016/3/EmpowerBP#Tip"/>
        <EmpowerBP:isAppropriateForInterventionGoal rdf:resource="http://www.semanticweb.org/tswheeler/ontologies/2016/3/EmpowerBP#ReduceSaltIntake"/>
        <EmpowerBP:isWarrantedBy rdf:resource="http://purl.bioontology.org/ontology/BCTT#Behavior_substitution"/>
        <EmpowerBP:appropriateForAutomaticMotivation rdf:datatype="http://www.w3.org/2001/XMLSchema#integer">6</EmpowerBP:appropriateForAutomaticMotivation>
        <EmpowerBP:appropriateForLocation rdf:datatype="http://www.w3.org/2001/XMLSchema#integer">0</EmpowerBP:appropriateForLocation>
        <EmpowerBP:appropriateForPhysicalCapability rdf:datatype="http://www.w3.org/2001/XMLSchema#integer">3</EmpowerBP:appropriateForPhysicalCapability>
        <EmpowerBP:appropriateForPhysicalOpportunity rdf:datatype="http://www.w3.org/2001/XMLSchema#integer">3</EmpowerBP:appropriateForPhysicalOpportunity>
        <EmpowerBP:appropriateForPsychologicalCapability rdf:datatype="http://www.w3.org/2001/XMLSchema#integer">3</EmpowerBP:appropriateForPsychologicalCapability>
        <EmpowerBP:appropriateForReflectiveMotivation rdf:datatype="http://www.w3.org/2001/XMLSchema#integer">6</EmpowerBP:appropriateForReflectiveMotivation>
        <EmpowerBP:appropriateForSocialOpportunity rdf:datatype="http://www.w3.org/2001/XMLSchema#integer">3</EmpowerBP:appropriateForSocialOpportunity>
        <EmpowerBP:canRepeat rdf:datatype="http://www.w3.org/2001/XMLSchema#integer">26</EmpowerBP:canRepeat>
        <EmpowerBP:itemName rdf:datatype="http://www.w3.org/2001/XMLSchema#string">Lower sodium options!</EmpowerBP:itemName>
        <EmpowerBP:itemText rdf:datatype="http://www.w3.org/2001/XMLSchema#string">Cut the sodium, keep your health!

Choose more of frice cooked in water or low sodium broth.

Choose less of rice cooked in salty broth.</EmpowerBP:itemText>
        <EmpowerBP:maximumUserAge rdf:datatype="http://www.w3.org/2001/XMLSchema#integer">120</EmpowerBP:maximumUserAge>
        <EmpowerBP:minimumUserAge rdf:datatype="http://www.w3.org/2001/XMLSchema#integer">18</EmpowerBP:minimumUserAge>
        <EmpowerBP:provideJournal rdf:datatype="http://www.w3.org/2001/XMLSchema#boolean">false</EmpowerBP:provideJournal>
        <EmpowerBP:provideLink rdf:datatype="http://www.w3.org/2001/XMLSchema#boolean">false</EmpowerBP:provideLink>
        <EmpowerBP:sourceURL rdf:datatype="http://www.w3.org/2001/XMLSchema#string">http://www.dietitians.ca/Downloads/Factsheets/Sodium-Sense-factsheet-collection.aspx</EmpowerBP:sourceURL>
        <rdfs:comment rdf:datatype="http://www.w3.org/2001/XMLSchema#string">Cut the sodium, keep your health!

Choose more of frice cooked in water or low sodium broth.

Choose less of rice cooked in salty broth.</rdfs:comment>
        <rdfs:label rdf:datatype="http://www.w3.org/2001/XMLSchema#string">Lower sodium options!</rdfs:label>
    </owl:NamedIndividual>
    


    <!-- http://www.semanticweb.org/tswheeler/ontologies/2016/3/EmpowerBP#T22 -->

    <owl:NamedIndividual rdf:about="http://www.semanticweb.org/tswheeler/ontologies/2016/3/EmpowerBP#T22">
        <rdf:type rdf:resource="http://www.semanticweb.org/tswheeler/ontologies/2016/3/EmpowerBP#InterventionItem"/>
        <rdf:type rdf:resource="http://www.semanticweb.org/tswheeler/ontologies/2016/3/EmpowerBP#Tip"/>
        <EmpowerBP:isAppropriateForInterventionGoal rdf:resource="http://www.semanticweb.org/tswheeler/ontologies/2016/3/EmpowerBP#ReduceSaltIntake"/>
        <EmpowerBP:isWarrantedBy rdf:resource="http://purl.bioontology.org/ontology/BCTT#Behavior_substitution"/>
        <EmpowerBP:appropriateForAutomaticMotivation rdf:datatype="http://www.w3.org/2001/XMLSchema#integer">6</EmpowerBP:appropriateForAutomaticMotivation>
        <EmpowerBP:appropriateForLocation rdf:datatype="http://www.w3.org/2001/XMLSchema#integer">0</EmpowerBP:appropriateForLocation>
        <EmpowerBP:appropriateForPhysicalCapability rdf:datatype="http://www.w3.org/2001/XMLSchema#integer">3</EmpowerBP:appropriateForPhysicalCapability>
        <EmpowerBP:appropriateForPhysicalOpportunity rdf:datatype="http://www.w3.org/2001/XMLSchema#integer">3</EmpowerBP:appropriateForPhysicalOpportunity>
        <EmpowerBP:appropriateForPsychologicalCapability rdf:datatype="http://www.w3.org/2001/XMLSchema#integer">3</EmpowerBP:appropriateForPsychologicalCapability>
        <EmpowerBP:appropriateForReflectiveMotivation rdf:datatype="http://www.w3.org/2001/XMLSchema#integer">6</EmpowerBP:appropriateForReflectiveMotivation>
        <EmpowerBP:appropriateForSocialOpportunity rdf:datatype="http://www.w3.org/2001/XMLSchema#integer">3</EmpowerBP:appropriateForSocialOpportunity>
        <EmpowerBP:canRepeat rdf:datatype="http://www.w3.org/2001/XMLSchema#integer">26</EmpowerBP:canRepeat>
        <EmpowerBP:itemName rdf:datatype="http://www.w3.org/2001/XMLSchema#string">Lower sodium options!</EmpowerBP:itemName>
        <EmpowerBP:itemText rdf:datatype="http://www.w3.org/2001/XMLSchema#string">Cut the sodium, keep your health!

Choose more of sandwiches made with roasted meat or poultry, fresh or low sodium canned fish, eggs or natural peanut butter.

Choose less of sandwiches made with canned or deli meats or high sodium canned fish.</EmpowerBP:itemText>
        <EmpowerBP:maximumUserAge rdf:datatype="http://www.w3.org/2001/XMLSchema#integer">120</EmpowerBP:maximumUserAge>
        <EmpowerBP:minimumUserAge rdf:datatype="http://www.w3.org/2001/XMLSchema#integer">18</EmpowerBP:minimumUserAge>
        <EmpowerBP:provideJournal rdf:datatype="http://www.w3.org/2001/XMLSchema#boolean">false</EmpowerBP:provideJournal>
        <EmpowerBP:provideLink rdf:datatype="http://www.w3.org/2001/XMLSchema#boolean">false</EmpowerBP:provideLink>
        <EmpowerBP:sourceURL rdf:datatype="http://www.w3.org/2001/XMLSchema#string">http://www.dietitians.ca/Downloads/Factsheets/Sodium-Sense-factsheet-collection.aspx</EmpowerBP:sourceURL>
        <rdfs:comment rdf:datatype="http://www.w3.org/2001/XMLSchema#string">Cut the sodium, keep your health!

Choose more of sandwiches made with roasted meat or poultry, fresh or low sodium canned fish, eggs or natural peanut butter.

Choose less of sandwiches made with canned or deli meats or high sodium canned fish.</rdfs:comment>
        <rdfs:label rdf:datatype="http://www.w3.org/2001/XMLSchema#string">Lower sodium options!</rdfs:label>
    </owl:NamedIndividual>
    


    <!-- http://www.semanticweb.org/tswheeler/ontologies/2016/3/EmpowerBP#T23 -->

    <owl:NamedIndividual rdf:about="http://www.semanticweb.org/tswheeler/ontologies/2016/3/EmpowerBP#T23">
        <rdf:type rdf:resource="http://www.semanticweb.org/tswheeler/ontologies/2016/3/EmpowerBP#InterventionItem"/>
        <rdf:type rdf:resource="http://www.semanticweb.org/tswheeler/ontologies/2016/3/EmpowerBP#Tip"/>
        <EmpowerBP:isAppropriateForInterventionGoal rdf:resource="http://www.semanticweb.org/tswheeler/ontologies/2016/3/EmpowerBP#ReduceSaltIntake"/>
        <EmpowerBP:isWarrantedBy rdf:resource="http://purl.bioontology.org/ontology/BCTT#Behavior_substitution"/>
        <EmpowerBP:appropriateForAutomaticMotivation rdf:datatype="http://www.w3.org/2001/XMLSchema#integer">6</EmpowerBP:appropriateForAutomaticMotivation>
        <EmpowerBP:appropriateForLocation rdf:datatype="http://www.w3.org/2001/XMLSchema#integer">0</EmpowerBP:appropriateForLocation>
        <EmpowerBP:appropriateForPhysicalCapability rdf:datatype="http://www.w3.org/2001/XMLSchema#integer">3</EmpowerBP:appropriateForPhysicalCapability>
        <EmpowerBP:appropriateForPhysicalOpportunity rdf:datatype="http://www.w3.org/2001/XMLSchema#integer">3</EmpowerBP:appropriateForPhysicalOpportunity>
        <EmpowerBP:appropriateForPsychologicalCapability rdf:datatype="http://www.w3.org/2001/XMLSchema#integer">3</EmpowerBP:appropriateForPsychologicalCapability>
        <EmpowerBP:appropriateForReflectiveMotivation rdf:datatype="http://www.w3.org/2001/XMLSchema#integer">6</EmpowerBP:appropriateForReflectiveMotivation>
        <EmpowerBP:appropriateForSocialOpportunity rdf:datatype="http://www.w3.org/2001/XMLSchema#integer">3</EmpowerBP:appropriateForSocialOpportunity>
        <EmpowerBP:canRepeat rdf:datatype="http://www.w3.org/2001/XMLSchema#integer">26</EmpowerBP:canRepeat>
        <EmpowerBP:itemName rdf:datatype="http://www.w3.org/2001/XMLSchema#string">Lower sodium options!</EmpowerBP:itemName>
        <EmpowerBP:itemText rdf:datatype="http://www.w3.org/2001/XMLSchema#string">Cut the sodium, keep your health!

Choose more of fresh or dried herbs and spices, garlic, ginger, onion, vinegar, lemon and lime juice.

Choose less of salt, kosher salt, sea salt, fleur de sel, gourmet salt, smoked salt, celery salt, garlic salt, or onion salt. </EmpowerBP:itemText>
        <EmpowerBP:maximumUserAge rdf:datatype="http://www.w3.org/2001/XMLSchema#integer">120</EmpowerBP:maximumUserAge>
        <EmpowerBP:minimumUserAge rdf:datatype="http://www.w3.org/2001/XMLSchema#integer">18</EmpowerBP:minimumUserAge>
        <EmpowerBP:provideJournal rdf:datatype="http://www.w3.org/2001/XMLSchema#boolean">false</EmpowerBP:provideJournal>
        <EmpowerBP:provideLink rdf:datatype="http://www.w3.org/2001/XMLSchema#boolean">false</EmpowerBP:provideLink>
        <EmpowerBP:sourceURL rdf:datatype="http://www.w3.org/2001/XMLSchema#string">http://www.dietitians.ca/Downloads/Factsheets/Sodium-Sense-factsheet-collection.aspx</EmpowerBP:sourceURL>
        <rdfs:comment rdf:datatype="http://www.w3.org/2001/XMLSchema#string">Cut the sodium, keep your health!

Choose more of fresh or dried herbs and spices, garlic, ginger, onion, vinegar, lemon and lime juice.

Choose less of salt, kosher salt, sea salt, fleur de sel, gourmet salt, smoked salt, celery salt, garlic salt, or onion salt. </rdfs:comment>
        <rdfs:label rdf:datatype="http://www.w3.org/2001/XMLSchema#string">Lower sodium options!</rdfs:label>
    </owl:NamedIndividual>
    


    <!-- http://www.semanticweb.org/tswheeler/ontologies/2016/3/EmpowerBP#T24 -->

    <owl:NamedIndividual rdf:about="http://www.semanticweb.org/tswheeler/ontologies/2016/3/EmpowerBP#T24">
        <rdf:type rdf:resource="http://www.semanticweb.org/tswheeler/ontologies/2016/3/EmpowerBP#InterventionItem"/>
        <rdf:type rdf:resource="http://www.semanticweb.org/tswheeler/ontologies/2016/3/EmpowerBP#Tip"/>
        <EmpowerBP:isAppropriateForInterventionGoal rdf:resource="http://www.semanticweb.org/tswheeler/ontologies/2016/3/EmpowerBP#ReduceSaltIntake"/>
        <EmpowerBP:isWarrantedBy rdf:resource="http://purl.bioontology.org/ontology/BCTT#Restructuring_the_physical_environment"/>
        <EmpowerBP:appropriateForAutomaticMotivation rdf:datatype="http://www.w3.org/2001/XMLSchema#integer">6</EmpowerBP:appropriateForAutomaticMotivation>
        <EmpowerBP:appropriateForLocation rdf:datatype="http://www.w3.org/2001/XMLSchema#integer">0</EmpowerBP:appropriateForLocation>
        <EmpowerBP:appropriateForPhysicalCapability rdf:datatype="http://www.w3.org/2001/XMLSchema#integer">3</EmpowerBP:appropriateForPhysicalCapability>
        <EmpowerBP:appropriateForPhysicalOpportunity rdf:datatype="http://www.w3.org/2001/XMLSchema#integer">3</EmpowerBP:appropriateForPhysicalOpportunity>
        <EmpowerBP:appropriateForPsychologicalCapability rdf:datatype="http://www.w3.org/2001/XMLSchema#integer">3</EmpowerBP:appropriateForPsychologicalCapability>
        <EmpowerBP:appropriateForReflectiveMotivation rdf:datatype="http://www.w3.org/2001/XMLSchema#integer">6</EmpowerBP:appropriateForReflectiveMotivation>
        <EmpowerBP:appropriateForSocialOpportunity rdf:datatype="http://www.w3.org/2001/XMLSchema#integer">3</EmpowerBP:appropriateForSocialOpportunity>
        <EmpowerBP:canRepeat rdf:datatype="http://www.w3.org/2001/XMLSchema#integer">26</EmpowerBP:canRepeat>
        <EmpowerBP:itemName rdf:datatype="http://www.w3.org/2001/XMLSchema#string">Sodium Sense for Eating Out</EmpowerBP:itemName>
        <EmpowerBP:itemText rdf:datatype="http://www.w3.org/2001/XMLSchema#string">Make healthy choices when eating out!

• Order smaller portions or share with someone
• Ask for gravy, sauces, and salad dressings &quot;on the side&quot; and use only small amounts.
• Balance out your day. If you ate a higher sodium restaurant meal, eat a lower sodium meal at home. 
• Ask for meals to be cooked without salt or monosodium glutamate (MSG), as seasoning that is very high in sodium.
• Many restaurants provide product nutrition information online. Look for the Informed Dining Program at the food establishments you visit. Choose foods with less sodium.</EmpowerBP:itemText>
        <EmpowerBP:maximumUserAge rdf:datatype="http://www.w3.org/2001/XMLSchema#integer">120</EmpowerBP:maximumUserAge>
        <EmpowerBP:minimumUserAge rdf:datatype="http://www.w3.org/2001/XMLSchema#integer">18</EmpowerBP:minimumUserAge>
        <EmpowerBP:provideJournal rdf:datatype="http://www.w3.org/2001/XMLSchema#boolean">false</EmpowerBP:provideJournal>
        <EmpowerBP:provideLink rdf:datatype="http://www.w3.org/2001/XMLSchema#boolean">false</EmpowerBP:provideLink>
        <EmpowerBP:sourceURL rdf:datatype="http://www.w3.org/2001/XMLSchema#string">http://www.dietitians.ca/Downloads/Factsheets/Sodium-Sense-factsheet-collection.aspx</EmpowerBP:sourceURL>
        <rdfs:comment rdf:datatype="http://www.w3.org/2001/XMLSchema#string">Make healthy choices when eating out!

• Order smaller portions or share with someone
• Ask for gravy, sauces, and salad dressings &quot;on the side&quot; and use only small amounts.
• Balance out your day. If you ate a higher sodium restaurant meal, eat a lower sodium meal at home. 
• Ask for meals to be cooked without salt or monosodium glutamate (MSG), as seasoning that is very high in sodium.
• Many restaurants provide product nutrition information online. Look for the Informed Dining Program at the food establishments you visit. Choose foods with less sodium.</rdfs:comment>
        <rdfs:label rdf:datatype="http://www.w3.org/2001/XMLSchema#string">Sodium Sense for Eating Out</rdfs:label>
    </owl:NamedIndividual>
    


    <!-- http://www.semanticweb.org/tswheeler/ontologies/2016/3/EmpowerBP#T25 -->

    <owl:NamedIndividual rdf:about="http://www.semanticweb.org/tswheeler/ontologies/2016/3/EmpowerBP#T25">
        <rdf:type rdf:resource="http://www.semanticweb.org/tswheeler/ontologies/2016/3/EmpowerBP#InterventionItem"/>
        <rdf:type rdf:resource="http://www.semanticweb.org/tswheeler/ontologies/2016/3/EmpowerBP#Tip"/>
        <EmpowerBP:isAppropriateForInterventionGoal rdf:resource="http://www.semanticweb.org/tswheeler/ontologies/2016/3/EmpowerBP#ReduceSaltIntake"/>
        <EmpowerBP:isWarrantedBy rdf:resource="http://purl.bioontology.org/ontology/BCTT#Restructuring_the_physical_environment"/>
        <EmpowerBP:appropriateForAutomaticMotivation rdf:datatype="http://www.w3.org/2001/XMLSchema#integer">6</EmpowerBP:appropriateForAutomaticMotivation>
        <EmpowerBP:appropriateForLocation rdf:datatype="http://www.w3.org/2001/XMLSchema#integer">0</EmpowerBP:appropriateForLocation>
        <EmpowerBP:appropriateForPhysicalCapability rdf:datatype="http://www.w3.org/2001/XMLSchema#integer">3</EmpowerBP:appropriateForPhysicalCapability>
        <EmpowerBP:appropriateForPhysicalOpportunity rdf:datatype="http://www.w3.org/2001/XMLSchema#integer">3</EmpowerBP:appropriateForPhysicalOpportunity>
        <EmpowerBP:appropriateForPsychologicalCapability rdf:datatype="http://www.w3.org/2001/XMLSchema#integer">3</EmpowerBP:appropriateForPsychologicalCapability>
        <EmpowerBP:appropriateForReflectiveMotivation rdf:datatype="http://www.w3.org/2001/XMLSchema#integer">6</EmpowerBP:appropriateForReflectiveMotivation>
        <EmpowerBP:appropriateForSocialOpportunity rdf:datatype="http://www.w3.org/2001/XMLSchema#integer">3</EmpowerBP:appropriateForSocialOpportunity>
        <EmpowerBP:canRepeat rdf:datatype="http://www.w3.org/2001/XMLSchema#integer">26</EmpowerBP:canRepeat>
        <EmpowerBP:itemName rdf:datatype="http://www.w3.org/2001/XMLSchema#string">Sodium Sense at Home</EmpowerBP:itemName>
        <EmpowerBP:itemText rdf:datatype="http://www.w3.org/2001/XMLSchema#string">Experiment with healthy meals and snacks!

• Buy fewer packaged, ready-to-eat and take-out foods.
• Make your own soups, sauces and salad dressings. 
• Buy fresh, frozen, or low sodium canned vegetables whenever possible
• Taste food before adding salt</EmpowerBP:itemText>
        <EmpowerBP:maximumUserAge rdf:datatype="http://www.w3.org/2001/XMLSchema#integer">120</EmpowerBP:maximumUserAge>
        <EmpowerBP:minimumUserAge rdf:datatype="http://www.w3.org/2001/XMLSchema#integer">18</EmpowerBP:minimumUserAge>
        <EmpowerBP:provideJournal rdf:datatype="http://www.w3.org/2001/XMLSchema#boolean">false</EmpowerBP:provideJournal>
        <EmpowerBP:provideLink rdf:datatype="http://www.w3.org/2001/XMLSchema#boolean">false</EmpowerBP:provideLink>
        <EmpowerBP:sourceURL rdf:datatype="http://www.w3.org/2001/XMLSchema#string">http://www.dietitians.ca/Downloads/Factsheets/Sodium-Sense-factsheet-collection.aspx</EmpowerBP:sourceURL>
        <rdfs:comment rdf:datatype="http://www.w3.org/2001/XMLSchema#string">Experiment with healthy meals and snacks!

• Buy fewer packaged, ready-to-eat and take-out foods.
• Make your own soups, sauces and salad dressings. 
• Buy fresh, frozen, or low sodium canned vegetables whenever possible
• Taste food before adding salt</rdfs:comment>
        <rdfs:label rdf:datatype="http://www.w3.org/2001/XMLSchema#string">Sodium Sense at Home</rdfs:label>
    </owl:NamedIndividual>
    


    <!-- http://www.semanticweb.org/tswheeler/ontologies/2016/3/EmpowerBP#T26 -->

    <owl:NamedIndividual rdf:about="http://www.semanticweb.org/tswheeler/ontologies/2016/3/EmpowerBP#T26">
        <rdf:type rdf:resource="http://www.semanticweb.org/tswheeler/ontologies/2016/3/EmpowerBP#InterventionItem"/>
        <rdf:type rdf:resource="http://www.semanticweb.org/tswheeler/ontologies/2016/3/EmpowerBP#Tip"/>
        <EmpowerBP:isAppropriateForInterventionGoal rdf:resource="http://www.semanticweb.org/tswheeler/ontologies/2016/3/EmpowerBP#ReduceSaltIntake"/>
        <EmpowerBP:isWarrantedBy rdf:resource="http://purl.bioontology.org/ontology/BCTT#Restructuring_the_physical_environment"/>
        <EmpowerBP:appropriateForAutomaticMotivation rdf:datatype="http://www.w3.org/2001/XMLSchema#integer">6</EmpowerBP:appropriateForAutomaticMotivation>
        <EmpowerBP:appropriateForLocation rdf:datatype="http://www.w3.org/2001/XMLSchema#integer">0</EmpowerBP:appropriateForLocation>
        <EmpowerBP:appropriateForPhysicalCapability rdf:datatype="http://www.w3.org/2001/XMLSchema#integer">3</EmpowerBP:appropriateForPhysicalCapability>
        <EmpowerBP:appropriateForPhysicalOpportunity rdf:datatype="http://www.w3.org/2001/XMLSchema#integer">3</EmpowerBP:appropriateForPhysicalOpportunity>
        <EmpowerBP:appropriateForPsychologicalCapability rdf:datatype="http://www.w3.org/2001/XMLSchema#integer">3</EmpowerBP:appropriateForPsychologicalCapability>
        <EmpowerBP:appropriateForReflectiveMotivation rdf:datatype="http://www.w3.org/2001/XMLSchema#integer">6</EmpowerBP:appropriateForReflectiveMotivation>
        <EmpowerBP:appropriateForSocialOpportunity rdf:datatype="http://www.w3.org/2001/XMLSchema#integer">3</EmpowerBP:appropriateForSocialOpportunity>
        <EmpowerBP:canRepeat rdf:datatype="http://www.w3.org/2001/XMLSchema#integer">26</EmpowerBP:canRepeat>
        <EmpowerBP:itemName rdf:datatype="http://www.w3.org/2001/XMLSchema#string">Sodium Sense at the Market</EmpowerBP:itemName>
        <EmpowerBP:itemText rdf:datatype="http://www.w3.org/2001/XMLSchema#string">Read the label and find the sodium: 

• Compare food labels and buy products with the lowest amount of sodium
• Use the % Daily Value (%DV) on the label to see if the food has a little or a lot of sodium.
• Here is a useful guide: 5% DV or less is a little, 15% DV or more is a lot.</EmpowerBP:itemText>
        <EmpowerBP:maximumUserAge rdf:datatype="http://www.w3.org/2001/XMLSchema#integer">120</EmpowerBP:maximumUserAge>
        <EmpowerBP:minimumUserAge rdf:datatype="http://www.w3.org/2001/XMLSchema#integer">18</EmpowerBP:minimumUserAge>
        <EmpowerBP:provideJournal rdf:datatype="http://www.w3.org/2001/XMLSchema#boolean">false</EmpowerBP:provideJournal>
        <EmpowerBP:provideLink rdf:datatype="http://www.w3.org/2001/XMLSchema#boolean">false</EmpowerBP:provideLink>
        <EmpowerBP:sourceURL rdf:datatype="http://www.w3.org/2001/XMLSchema#string">http://www.dietitians.ca/Downloads/Factsheets/Sodium-Sense-factsheet-collection.aspx</EmpowerBP:sourceURL>
        <rdfs:comment rdf:datatype="http://www.w3.org/2001/XMLSchema#string">Read the label and find the sodium: 

• Compare food labels and buy products with the lowest amount of sodium
• Use the % Daily Value (%DV) on the label to see if the food has a little or a lot of sodium.
• Here is a useful guide: 5% DV or less is a little, 15% DV or more is a lot.</rdfs:comment>
        <rdfs:label rdf:datatype="http://www.w3.org/2001/XMLSchema#string">Sodium Sense at the Market</rdfs:label>
    </owl:NamedIndividual>
    


    <!-- http://www.semanticweb.org/tswheeler/ontologies/2016/3/EmpowerBP#T27 -->

    <owl:NamedIndividual rdf:about="http://www.semanticweb.org/tswheeler/ontologies/2016/3/EmpowerBP#T27">
        <rdf:type rdf:resource="http://www.semanticweb.org/tswheeler/ontologies/2016/3/EmpowerBP#InterventionItem"/>
        <rdf:type rdf:resource="http://www.semanticweb.org/tswheeler/ontologies/2016/3/EmpowerBP#Tip"/>
        <EmpowerBP:isAppropriateForInterventionGoal rdf:resource="http://www.semanticweb.org/tswheeler/ontologies/2016/3/EmpowerBP#ReduceSaltIntake"/>
        <EmpowerBP:isWarrantedBy rdf:resource="http://purl.bioontology.org/ontology/BCTT#Instruction_on_how_to_perform_the_behavior"/>
        <EmpowerBP:appropriateForAutomaticMotivation rdf:datatype="http://www.w3.org/2001/XMLSchema#integer">6</EmpowerBP:appropriateForAutomaticMotivation>
        <EmpowerBP:appropriateForLocation rdf:datatype="http://www.w3.org/2001/XMLSchema#integer">0</EmpowerBP:appropriateForLocation>
        <EmpowerBP:appropriateForPhysicalCapability rdf:datatype="http://www.w3.org/2001/XMLSchema#integer">3</EmpowerBP:appropriateForPhysicalCapability>
        <EmpowerBP:appropriateForPhysicalOpportunity rdf:datatype="http://www.w3.org/2001/XMLSchema#integer">3</EmpowerBP:appropriateForPhysicalOpportunity>
        <EmpowerBP:appropriateForPsychologicalCapability rdf:datatype="http://www.w3.org/2001/XMLSchema#integer">3</EmpowerBP:appropriateForPsychologicalCapability>
        <EmpowerBP:appropriateForReflectiveMotivation rdf:datatype="http://www.w3.org/2001/XMLSchema#integer">6</EmpowerBP:appropriateForReflectiveMotivation>
        <EmpowerBP:appropriateForSocialOpportunity rdf:datatype="http://www.w3.org/2001/XMLSchema#integer">3</EmpowerBP:appropriateForSocialOpportunity>
        <EmpowerBP:canRepeat rdf:datatype="http://www.w3.org/2001/XMLSchema#integer">26</EmpowerBP:canRepeat>
        <EmpowerBP:itemName rdf:datatype="http://www.w3.org/2001/XMLSchema#string">Reduce the sodium in the foods you use</EmpowerBP:itemName>
        <EmpowerBP:itemText rdf:datatype="http://www.w3.org/2001/XMLSchema#string">Reduce the sodium in the foods you use: 

• Rinse canned vegetables and canned beans, peas, and lentils to wash away some of the sodium. 
• Use less of the seasoning that comes with taco kits, packaged macaroni and cheese, pasta, and rice mixes.
• Use less salt than what the recipe calls for, except when baking.
• Use less ketchup, soy sauce, and other condiments, or try a lower sodium option. </EmpowerBP:itemText>
        <EmpowerBP:maximumUserAge rdf:datatype="http://www.w3.org/2001/XMLSchema#integer">120</EmpowerBP:maximumUserAge>
        <EmpowerBP:minimumUserAge rdf:datatype="http://www.w3.org/2001/XMLSchema#integer">18</EmpowerBP:minimumUserAge>
        <EmpowerBP:provideJournal rdf:datatype="http://www.w3.org/2001/XMLSchema#boolean">false</EmpowerBP:provideJournal>
        <EmpowerBP:provideLink rdf:datatype="http://www.w3.org/2001/XMLSchema#boolean">false</EmpowerBP:provideLink>
        <EmpowerBP:sourceURL rdf:datatype="http://www.w3.org/2001/XMLSchema#string">http://www.dietitians.ca/Downloads/Factsheets/Sodium-Sense-factsheet-collection.aspx</EmpowerBP:sourceURL>
        <rdfs:comment rdf:datatype="http://www.w3.org/2001/XMLSchema#string">Reduce the sodium in the foods you use: 

• Rinse canned vegetables and canned beans, peas, and lentils to wash away some of the sodium. 
• Use less of the seasoning that comes with taco kits, packaged macaroni and cheese, pasta, and rice mixes.
• Use less salt than what the recipe calls for, except when baking.
• Use less ketchup, soy sauce, and other condiments, or try a lower sodium option. </rdfs:comment>
        <rdfs:label rdf:datatype="http://www.w3.org/2001/XMLSchema#string">Reduce the sodium in the foods you use</rdfs:label>
    </owl:NamedIndividual>
    


    <!-- http://www.semanticweb.org/tswheeler/ontologies/2016/3/EmpowerBP#T28 -->

    <owl:NamedIndividual rdf:about="http://www.semanticweb.org/tswheeler/ontologies/2016/3/EmpowerBP#T28">
        <rdf:type rdf:resource="http://www.semanticweb.org/tswheeler/ontologies/2016/3/EmpowerBP#InterventionItem"/>
        <rdf:type rdf:resource="http://www.semanticweb.org/tswheeler/ontologies/2016/3/EmpowerBP#Tip"/>
        <EmpowerBP:isAppropriateForInterventionGoal rdf:resource="http://www.semanticweb.org/tswheeler/ontologies/2016/3/EmpowerBP#ReduceSaltIntake"/>
        <EmpowerBP:isWarrantedBy rdf:resource="http://purl.bioontology.org/ontology/BCTT#Instruction_on_how_to_perform_the_behavior"/>
        <EmpowerBP:appropriateForAutomaticMotivation rdf:datatype="http://www.w3.org/2001/XMLSchema#integer">6</EmpowerBP:appropriateForAutomaticMotivation>
        <EmpowerBP:appropriateForLocation rdf:datatype="http://www.w3.org/2001/XMLSchema#integer">0</EmpowerBP:appropriateForLocation>
        <EmpowerBP:appropriateForPhysicalCapability rdf:datatype="http://www.w3.org/2001/XMLSchema#integer">3</EmpowerBP:appropriateForPhysicalCapability>
        <EmpowerBP:appropriateForPhysicalOpportunity rdf:datatype="http://www.w3.org/2001/XMLSchema#integer">3</EmpowerBP:appropriateForPhysicalOpportunity>
        <EmpowerBP:appropriateForPsychologicalCapability rdf:datatype="http://www.w3.org/2001/XMLSchema#integer">3</EmpowerBP:appropriateForPsychologicalCapability>
        <EmpowerBP:appropriateForReflectiveMotivation rdf:datatype="http://www.w3.org/2001/XMLSchema#integer">6</EmpowerBP:appropriateForReflectiveMotivation>
        <EmpowerBP:appropriateForSocialOpportunity rdf:datatype="http://www.w3.org/2001/XMLSchema#integer">3</EmpowerBP:appropriateForSocialOpportunity>
        <EmpowerBP:canRepeat rdf:datatype="http://www.w3.org/2001/XMLSchema#integer">26</EmpowerBP:canRepeat>
        <EmpowerBP:itemName rdf:datatype="http://www.w3.org/2001/XMLSchema#string">Sodium and Canada&apos;s Food Guide</EmpowerBP:itemName>
        <EmpowerBP:itemText rdf:datatype="http://www.w3.org/2001/XMLSchema#string">1. Vegetables and Fruit

Buy fresh or frozen vegetables whenever possible. Buy canned vegetables and tomato and vegetable juices that are low in sodium. 

2. Grain Products

Choose breads, breakfast cereals, and bakery products that are lowest in sodium. Enjoy a variety of naturally sodium-free grains such as barley, quinoa, and rice.

3. Milk and Alternatives

Enjoy milk, fortified soy beverage, and yogurt because they are low in sodium. 

4. Meat and Alternatives

Buy unseasoned meat, poultry, fish, seafood, and tofu. Choose unsalted nuts. Buy low sodium canned beans or try dried beans, peas, and lentils. </EmpowerBP:itemText>
        <EmpowerBP:maximumUserAge rdf:datatype="http://www.w3.org/2001/XMLSchema#integer">120</EmpowerBP:maximumUserAge>
        <EmpowerBP:minimumUserAge rdf:datatype="http://www.w3.org/2001/XMLSchema#integer">18</EmpowerBP:minimumUserAge>
        <EmpowerBP:provideJournal rdf:datatype="http://www.w3.org/2001/XMLSchema#boolean">false</EmpowerBP:provideJournal>
        <EmpowerBP:provideLink rdf:datatype="http://www.w3.org/2001/XMLSchema#boolean">false</EmpowerBP:provideLink>
        <EmpowerBP:sourceURL rdf:datatype="http://www.w3.org/2001/XMLSchema#string">http://www.dietitians.ca/Downloads/Factsheets/Sodium-Sense-factsheet-collection.aspx</EmpowerBP:sourceURL>
        <rdfs:comment rdf:datatype="http://www.w3.org/2001/XMLSchema#string">1. Vegetables and Fruit

Buy fresh or frozen vegetables whenever possible. Buy canned vegetables and tomato and vegetable juices that are low in sodium. 

2. Grain Products

Choose breads, breakfast cereals, and bakery products that are lowest in sodium. Enjoy a variety of naturally sodium-free grains such as barley, quinoa, and rice.

3. Milk and Alternatives

Enjoy milk, fortified soy beverage, and yogurt because they are low in sodium. 

4. Meat and Alternatives

Buy unseasoned meat, poultry, fish, seafood, and tofu. Choose unsalted nuts. Buy low sodium canned beans or try dried beans, peas, and lentils. </rdfs:comment>
        <rdfs:label rdf:datatype="http://www.w3.org/2001/XMLSchema#string">Sodium and Canada&apos;s Food Guide</rdfs:label>
    </owl:NamedIndividual>
    


    <!-- http://www.semanticweb.org/tswheeler/ontologies/2016/3/EmpowerBP#T29 -->

    <owl:NamedIndividual rdf:about="http://www.semanticweb.org/tswheeler/ontologies/2016/3/EmpowerBP#T29">
        <rdf:type rdf:resource="http://www.semanticweb.org/tswheeler/ontologies/2016/3/EmpowerBP#InterventionItem"/>
        <rdf:type rdf:resource="http://www.semanticweb.org/tswheeler/ontologies/2016/3/EmpowerBP#Tip"/>
        <EmpowerBP:isAppropriateForInterventionGoal rdf:resource="http://www.semanticweb.org/tswheeler/ontologies/2016/3/EmpowerBP#ReduceSaltIntake"/>
        <EmpowerBP:isWarrantedBy rdf:resource="http://purl.bioontology.org/ontology/BCTT#Information_about_social_and_environmental_consequences"/>
        <EmpowerBP:appropriateForAutomaticMotivation rdf:datatype="http://www.w3.org/2001/XMLSchema#integer">3</EmpowerBP:appropriateForAutomaticMotivation>
        <EmpowerBP:appropriateForLocation rdf:datatype="http://www.w3.org/2001/XMLSchema#integer">0</EmpowerBP:appropriateForLocation>
        <EmpowerBP:appropriateForPhysicalCapability rdf:datatype="http://www.w3.org/2001/XMLSchema#integer">3</EmpowerBP:appropriateForPhysicalCapability>
        <EmpowerBP:appropriateForPhysicalOpportunity rdf:datatype="http://www.w3.org/2001/XMLSchema#integer">3</EmpowerBP:appropriateForPhysicalOpportunity>
        <EmpowerBP:appropriateForPsychologicalCapability rdf:datatype="http://www.w3.org/2001/XMLSchema#integer">3</EmpowerBP:appropriateForPsychologicalCapability>
        <EmpowerBP:appropriateForReflectiveMotivation rdf:datatype="http://www.w3.org/2001/XMLSchema#integer">3</EmpowerBP:appropriateForReflectiveMotivation>
        <EmpowerBP:appropriateForSocialOpportunity rdf:datatype="http://www.w3.org/2001/XMLSchema#integer">3</EmpowerBP:appropriateForSocialOpportunity>
        <EmpowerBP:canRepeat rdf:datatype="http://www.w3.org/2001/XMLSchema#integer">26</EmpowerBP:canRepeat>
        <EmpowerBP:itemName rdf:datatype="http://www.w3.org/2001/XMLSchema#string">Sodium-rich Foods</EmpowerBP:itemName>
        <EmpowerBP:itemText rdf:datatype="http://www.w3.org/2001/XMLSchema#string">Most of the foods we eat contain too much sodium:

• Over 75% of the sodium we eat comes from processed foods such as cheese, deli meats, pizza, sauces and soups. 
• Packaged and ready-to-eat foods, fast foods, and restaurant meals are often high in sodium.
• Breads, breakfast cereals and bakery products also contain sodium even though they may not taste salty. </EmpowerBP:itemText>
        <EmpowerBP:maximumUserAge rdf:datatype="http://www.w3.org/2001/XMLSchema#integer">120</EmpowerBP:maximumUserAge>
        <EmpowerBP:minimumUserAge rdf:datatype="http://www.w3.org/2001/XMLSchema#integer">18</EmpowerBP:minimumUserAge>
        <EmpowerBP:provideJournal rdf:datatype="http://www.w3.org/2001/XMLSchema#boolean">false</EmpowerBP:provideJournal>
        <EmpowerBP:provideLink rdf:datatype="http://www.w3.org/2001/XMLSchema#boolean">false</EmpowerBP:provideLink>
        <EmpowerBP:sourceURL rdf:datatype="http://www.w3.org/2001/XMLSchema#string">http://www.dietitians.ca/Downloads/Factsheets/Sodium-Sense-factsheet-collection.aspx</EmpowerBP:sourceURL>
        <rdfs:comment rdf:datatype="http://www.w3.org/2001/XMLSchema#string">Most of the foods we eat contain too much sodium:

• Over 75% of the sodium we eat comes from processed foods such as cheese, deli meats, pizza, sauces and soups. 
• Packaged and ready-to-eat foods, fast foods, and restaurant meals are often high in sodium.
• Breads, breakfast cereals and bakery products also contain sodium even though they may not taste salty. </rdfs:comment>
        <rdfs:label rdf:datatype="http://www.w3.org/2001/XMLSchema#string">Sodium-rich Foods</rdfs:label>
    </owl:NamedIndividual>
    


    <!-- http://www.semanticweb.org/tswheeler/ontologies/2016/3/EmpowerBP#T3 -->

    <owl:NamedIndividual rdf:about="http://www.semanticweb.org/tswheeler/ontologies/2016/3/EmpowerBP#T3">
        <rdf:type rdf:resource="http://www.semanticweb.org/tswheeler/ontologies/2016/3/EmpowerBP#InterventionItem"/>
        <rdf:type rdf:resource="http://www.semanticweb.org/tswheeler/ontologies/2016/3/EmpowerBP#Tip"/>
        <EmpowerBP:isAppropriateForInterventionGoal rdf:resource="http://www.semanticweb.org/tswheeler/ontologies/2016/3/EmpowerBP#ExerciseMore"/>
        <EmpowerBP:isWarrantedBy rdf:resource="http://purl.bioontology.org/ontology/BCTT#Imaginary_reward"/>
        <EmpowerBP:appropriateForAutomaticMotivation rdf:datatype="http://www.w3.org/2001/XMLSchema#integer">3</EmpowerBP:appropriateForAutomaticMotivation>
        <EmpowerBP:appropriateForLocation rdf:datatype="http://www.w3.org/2001/XMLSchema#integer">0</EmpowerBP:appropriateForLocation>
        <EmpowerBP:appropriateForPhysicalCapability rdf:datatype="http://www.w3.org/2001/XMLSchema#integer">3</EmpowerBP:appropriateForPhysicalCapability>
        <EmpowerBP:appropriateForPhysicalOpportunity rdf:datatype="http://www.w3.org/2001/XMLSchema#integer">3</EmpowerBP:appropriateForPhysicalOpportunity>
        <EmpowerBP:appropriateForPsychologicalCapability rdf:datatype="http://www.w3.org/2001/XMLSchema#integer">3</EmpowerBP:appropriateForPsychologicalCapability>
        <EmpowerBP:appropriateForReflectiveMotivation rdf:datatype="http://www.w3.org/2001/XMLSchema#integer">3</EmpowerBP:appropriateForReflectiveMotivation>
        <EmpowerBP:appropriateForSocialOpportunity rdf:datatype="http://www.w3.org/2001/XMLSchema#integer">3</EmpowerBP:appropriateForSocialOpportunity>
        <EmpowerBP:canRepeat rdf:datatype="http://www.w3.org/2001/XMLSchema#integer">26</EmpowerBP:canRepeat>
        <EmpowerBP:itemName rdf:datatype="http://www.w3.org/2001/XMLSchema#string">Benefits of Activity</EmpowerBP:itemName>
        <EmpowerBP:itemText rdf:datatype="http://www.w3.org/2001/XMLSchema#string">Because physical activity makes you feel better about yourself, you&apos;re more likely to make healthy lifestyle choices and avoid unhealthy ones such as smoking, overeating or drinking too much alcohol.</EmpowerBP:itemText>
        <EmpowerBP:maximumUserAge rdf:datatype="http://www.w3.org/2001/XMLSchema#integer">120</EmpowerBP:maximumUserAge>
        <EmpowerBP:minimumUserAge rdf:datatype="http://www.w3.org/2001/XMLSchema#integer">18</EmpowerBP:minimumUserAge>
        <EmpowerBP:provideJournal rdf:datatype="http://www.w3.org/2001/XMLSchema#boolean">false</EmpowerBP:provideJournal>
        <EmpowerBP:provideLink rdf:datatype="http://www.w3.org/2001/XMLSchema#boolean">false</EmpowerBP:provideLink>
        <EmpowerBP:sourceURL rdf:datatype="http://www.w3.org/2001/XMLSchema#string">http://www.heartandstroke.ca/get-healthy/stay-active/benefits-of-physical-activity</EmpowerBP:sourceURL>
        <rdfs:comment rdf:datatype="http://www.w3.org/2001/XMLSchema#string">Because physical activity makes you feel better about yourself, you&apos;re more likely to make healthy lifestyle choices and avoid unhealthy ones such as smoking, overeating or drinking too much alcohol.</rdfs:comment>
        <rdfs:label rdf:datatype="http://www.w3.org/2001/XMLSchema#string">Benefits of Activity</rdfs:label>
    </owl:NamedIndividual>
    


    <!-- http://www.semanticweb.org/tswheeler/ontologies/2016/3/EmpowerBP#T30 -->

    <owl:NamedIndividual rdf:about="http://www.semanticweb.org/tswheeler/ontologies/2016/3/EmpowerBP#T30">
        <rdf:type rdf:resource="http://www.semanticweb.org/tswheeler/ontologies/2016/3/EmpowerBP#InterventionItem"/>
        <rdf:type rdf:resource="http://www.semanticweb.org/tswheeler/ontologies/2016/3/EmpowerBP#Tip"/>
        <EmpowerBP:isAppropriateForInterventionGoal rdf:resource="http://www.semanticweb.org/tswheeler/ontologies/2016/3/EmpowerBP#ReduceSaltIntake"/>
        <EmpowerBP:isWarrantedBy rdf:resource="http://purl.bioontology.org/ontology/BCTT#Behavior_substitution"/>
        <EmpowerBP:appropriateForAutomaticMotivation rdf:datatype="http://www.w3.org/2001/XMLSchema#integer">6</EmpowerBP:appropriateForAutomaticMotivation>
        <EmpowerBP:appropriateForLocation rdf:datatype="http://www.w3.org/2001/XMLSchema#integer">0</EmpowerBP:appropriateForLocation>
        <EmpowerBP:appropriateForPhysicalCapability rdf:datatype="http://www.w3.org/2001/XMLSchema#integer">3</EmpowerBP:appropriateForPhysicalCapability>
        <EmpowerBP:appropriateForPhysicalOpportunity rdf:datatype="http://www.w3.org/2001/XMLSchema#integer">3</EmpowerBP:appropriateForPhysicalOpportunity>
        <EmpowerBP:appropriateForPsychologicalCapability rdf:datatype="http://www.w3.org/2001/XMLSchema#integer">3</EmpowerBP:appropriateForPsychologicalCapability>
        <EmpowerBP:appropriateForReflectiveMotivation rdf:datatype="http://www.w3.org/2001/XMLSchema#integer">6</EmpowerBP:appropriateForReflectiveMotivation>
        <EmpowerBP:appropriateForSocialOpportunity rdf:datatype="http://www.w3.org/2001/XMLSchema#integer">3</EmpowerBP:appropriateForSocialOpportunity>
        <EmpowerBP:canRepeat rdf:datatype="http://www.w3.org/2001/XMLSchema#integer">26</EmpowerBP:canRepeat>
        <EmpowerBP:itemName rdf:datatype="http://www.w3.org/2001/XMLSchema#string">Sodium Sense Eating Out </EmpowerBP:itemName>
        <EmpowerBP:itemText rdf:datatype="http://www.w3.org/2001/XMLSchema#string">Easy ways to cut back on sodium when eating out: 

Choose...
• Lettuce, onions, or tomatoes on burgers and sandwiches
• Salad with dressing on the side or a baked potato

Instead of…
• Cheese, ketchup, mustard, or pickles on burgers and sandwiches
• French fries or fried onion rings</EmpowerBP:itemText>
        <EmpowerBP:maximumUserAge rdf:datatype="http://www.w3.org/2001/XMLSchema#integer">120</EmpowerBP:maximumUserAge>
        <EmpowerBP:minimumUserAge rdf:datatype="http://www.w3.org/2001/XMLSchema#integer">18</EmpowerBP:minimumUserAge>
        <EmpowerBP:provideJournal rdf:datatype="http://www.w3.org/2001/XMLSchema#boolean">false</EmpowerBP:provideJournal>
        <EmpowerBP:provideLink rdf:datatype="http://www.w3.org/2001/XMLSchema#boolean">false</EmpowerBP:provideLink>
        <EmpowerBP:sourceURL rdf:datatype="http://www.w3.org/2001/XMLSchema#string">http://www.dietitians.ca/Downloads/Factsheets/Sodium-Sense-factsheet-collection.aspx</EmpowerBP:sourceURL>
        <rdfs:comment rdf:datatype="http://www.w3.org/2001/XMLSchema#string">Easy ways to cut back on sodium when eating out: 

Choose...
• Lettuce, onions, or tomatoes on burgers and sandwiches
• Salad with dressing on the side or a baked potato

Instead of…
• Cheese, ketchup, mustard, or pickles on burgers and sandwiches
• French fries or fried onion rings</rdfs:comment>
        <rdfs:label rdf:datatype="http://www.w3.org/2001/XMLSchema#string">Sodium Sense Eating Out </rdfs:label>
    </owl:NamedIndividual>
    


    <!-- http://www.semanticweb.org/tswheeler/ontologies/2016/3/EmpowerBP#T31 -->

    <owl:NamedIndividual rdf:about="http://www.semanticweb.org/tswheeler/ontologies/2016/3/EmpowerBP#T31">
        <rdf:type rdf:resource="http://www.semanticweb.org/tswheeler/ontologies/2016/3/EmpowerBP#InterventionItem"/>
        <rdf:type rdf:resource="http://www.semanticweb.org/tswheeler/ontologies/2016/3/EmpowerBP#Tip"/>
        <EmpowerBP:isAppropriateForInterventionGoal rdf:resource="http://www.semanticweb.org/tswheeler/ontologies/2016/3/EmpowerBP#ReduceSaltIntake"/>
        <EmpowerBP:isWarrantedBy rdf:resource="http://purl.bioontology.org/ontology/BCTT#Behavior_substitution"/>
        <EmpowerBP:appropriateForAutomaticMotivation rdf:datatype="http://www.w3.org/2001/XMLSchema#integer">6</EmpowerBP:appropriateForAutomaticMotivation>
        <EmpowerBP:appropriateForLocation rdf:datatype="http://www.w3.org/2001/XMLSchema#integer">0</EmpowerBP:appropriateForLocation>
        <EmpowerBP:appropriateForPhysicalCapability rdf:datatype="http://www.w3.org/2001/XMLSchema#integer">3</EmpowerBP:appropriateForPhysicalCapability>
        <EmpowerBP:appropriateForPhysicalOpportunity rdf:datatype="http://www.w3.org/2001/XMLSchema#integer">3</EmpowerBP:appropriateForPhysicalOpportunity>
        <EmpowerBP:appropriateForPsychologicalCapability rdf:datatype="http://www.w3.org/2001/XMLSchema#integer">3</EmpowerBP:appropriateForPsychologicalCapability>
        <EmpowerBP:appropriateForReflectiveMotivation rdf:datatype="http://www.w3.org/2001/XMLSchema#integer">6</EmpowerBP:appropriateForReflectiveMotivation>
        <EmpowerBP:appropriateForSocialOpportunity rdf:datatype="http://www.w3.org/2001/XMLSchema#integer">3</EmpowerBP:appropriateForSocialOpportunity>
        <EmpowerBP:canRepeat rdf:datatype="http://www.w3.org/2001/XMLSchema#integer">26</EmpowerBP:canRepeat>
        <EmpowerBP:itemName rdf:datatype="http://www.w3.org/2001/XMLSchema#string">Sodium Sense Eating Out </EmpowerBP:itemName>
        <EmpowerBP:itemText rdf:datatype="http://www.w3.org/2001/XMLSchema#string">Easy ways to cut back on sodium when eating out: 

Choose...
• Steamed rice, steamed buns or dim sum rice noodle rolls with sodium-reduced soy sauce on the side
• Stir-fry vegetables with garlic
• Wonton noodles or rice noodles

Instead of…
• Fried rice or dim sum appetizers in soy, hoisin, fish or black bean sauces
• Stir-fry vegetables in oyster sauce
• Chow mein or fried rice noodles</EmpowerBP:itemText>
        <EmpowerBP:maximumUserAge rdf:datatype="http://www.w3.org/2001/XMLSchema#integer">120</EmpowerBP:maximumUserAge>
        <EmpowerBP:minimumUserAge rdf:datatype="http://www.w3.org/2001/XMLSchema#integer">18</EmpowerBP:minimumUserAge>
        <EmpowerBP:provideJournal rdf:datatype="http://www.w3.org/2001/XMLSchema#boolean">false</EmpowerBP:provideJournal>
        <EmpowerBP:provideLink rdf:datatype="http://www.w3.org/2001/XMLSchema#boolean">false</EmpowerBP:provideLink>
        <EmpowerBP:sourceURL rdf:datatype="http://www.w3.org/2001/XMLSchema#string">http://www.dietitians.ca/Downloads/Factsheets/Sodium-Sense-factsheet-collection.aspx</EmpowerBP:sourceURL>
        <rdfs:comment rdf:datatype="http://www.w3.org/2001/XMLSchema#string">Easy ways to cut back on sodium when eating out: 

Choose...
• Steamed rice, steamed buns or dim sum rice noodle rolls with sodium-reduced soy sauce on the side
• Stir-fry vegetables with garlic
• Wonton noodles or rice noodles

Instead of…
• Fried rice or dim sum appetizers in soy, hoisin, fish or black bean sauces
• Stir-fry vegetables in oyster sauce
• Chow mein or fried rice noodles</rdfs:comment>
        <rdfs:label rdf:datatype="http://www.w3.org/2001/XMLSchema#string">Sodium Sense Eating Out </rdfs:label>
    </owl:NamedIndividual>
    


    <!-- http://www.semanticweb.org/tswheeler/ontologies/2016/3/EmpowerBP#T32 -->

    <owl:NamedIndividual rdf:about="http://www.semanticweb.org/tswheeler/ontologies/2016/3/EmpowerBP#T32">
        <rdf:type rdf:resource="http://www.semanticweb.org/tswheeler/ontologies/2016/3/EmpowerBP#InterventionItem"/>
        <rdf:type rdf:resource="http://www.semanticweb.org/tswheeler/ontologies/2016/3/EmpowerBP#Tip"/>
        <EmpowerBP:isAppropriateForInterventionGoal rdf:resource="http://www.semanticweb.org/tswheeler/ontologies/2016/3/EmpowerBP#ReduceSaltIntake"/>
        <EmpowerBP:isWarrantedBy rdf:resource="http://purl.bioontology.org/ontology/BCTT#Behavior_substitution"/>
        <EmpowerBP:appropriateForAutomaticMotivation rdf:datatype="http://www.w3.org/2001/XMLSchema#integer">6</EmpowerBP:appropriateForAutomaticMotivation>
        <EmpowerBP:appropriateForLocation rdf:datatype="http://www.w3.org/2001/XMLSchema#integer">0</EmpowerBP:appropriateForLocation>
        <EmpowerBP:appropriateForPhysicalCapability rdf:datatype="http://www.w3.org/2001/XMLSchema#integer">3</EmpowerBP:appropriateForPhysicalCapability>
        <EmpowerBP:appropriateForPhysicalOpportunity rdf:datatype="http://www.w3.org/2001/XMLSchema#integer">3</EmpowerBP:appropriateForPhysicalOpportunity>
        <EmpowerBP:appropriateForPsychologicalCapability rdf:datatype="http://www.w3.org/2001/XMLSchema#integer">3</EmpowerBP:appropriateForPsychologicalCapability>
        <EmpowerBP:appropriateForReflectiveMotivation rdf:datatype="http://www.w3.org/2001/XMLSchema#integer">6</EmpowerBP:appropriateForReflectiveMotivation>
        <EmpowerBP:appropriateForSocialOpportunity rdf:datatype="http://www.w3.org/2001/XMLSchema#integer">3</EmpowerBP:appropriateForSocialOpportunity>
        <EmpowerBP:canRepeat rdf:datatype="http://www.w3.org/2001/XMLSchema#integer">26</EmpowerBP:canRepeat>
        <EmpowerBP:itemName rdf:datatype="http://www.w3.org/2001/XMLSchema#string">Sodium Sense Eating Out </EmpowerBP:itemName>
        <EmpowerBP:itemText rdf:datatype="http://www.w3.org/2001/XMLSchema#string">Easy ways to cut back on sodium when eating out: 

Choose...
• Raita
• Roti or chapatti
• Tandoori dishes

Instead of…
• Pakoras
• Naan or parantha
• Curry dishes or biryani</EmpowerBP:itemText>
        <EmpowerBP:maximumUserAge rdf:datatype="http://www.w3.org/2001/XMLSchema#integer">120</EmpowerBP:maximumUserAge>
        <EmpowerBP:minimumUserAge rdf:datatype="http://www.w3.org/2001/XMLSchema#integer">18</EmpowerBP:minimumUserAge>
        <EmpowerBP:provideJournal rdf:datatype="http://www.w3.org/2001/XMLSchema#boolean">false</EmpowerBP:provideJournal>
        <EmpowerBP:provideLink rdf:datatype="http://www.w3.org/2001/XMLSchema#boolean">false</EmpowerBP:provideLink>
        <EmpowerBP:sourceURL rdf:datatype="http://www.w3.org/2001/XMLSchema#string">http://www.dietitians.ca/Downloads/Factsheets/Sodium-Sense-factsheet-collection.aspx</EmpowerBP:sourceURL>
        <rdfs:comment rdf:datatype="http://www.w3.org/2001/XMLSchema#string">Easy ways to cut back on sodium when eating out: 

Choose...
• Raita
• Roti or chapatti
• Tandoori dishes

Instead of…
• Pakoras
• Naan or parantha
• Curry dishes or biryani</rdfs:comment>
        <rdfs:label rdf:datatype="http://www.w3.org/2001/XMLSchema#string">Sodium Sense Eating Out </rdfs:label>
    </owl:NamedIndividual>
    


    <!-- http://www.semanticweb.org/tswheeler/ontologies/2016/3/EmpowerBP#T33 -->

    <owl:NamedIndividual rdf:about="http://www.semanticweb.org/tswheeler/ontologies/2016/3/EmpowerBP#T33">
        <rdf:type rdf:resource="http://www.semanticweb.org/tswheeler/ontologies/2016/3/EmpowerBP#InterventionItem"/>
        <rdf:type rdf:resource="http://www.semanticweb.org/tswheeler/ontologies/2016/3/EmpowerBP#Tip"/>
        <EmpowerBP:isAppropriateForInterventionGoal rdf:resource="http://www.semanticweb.org/tswheeler/ontologies/2016/3/EmpowerBP#ReduceSaltIntake"/>
        <EmpowerBP:isWarrantedBy rdf:resource="http://purl.bioontology.org/ontology/BCTT#Behavior_substitution"/>
        <EmpowerBP:appropriateForAutomaticMotivation rdf:datatype="http://www.w3.org/2001/XMLSchema#integer">6</EmpowerBP:appropriateForAutomaticMotivation>
        <EmpowerBP:appropriateForLocation rdf:datatype="http://www.w3.org/2001/XMLSchema#integer">0</EmpowerBP:appropriateForLocation>
        <EmpowerBP:appropriateForPhysicalCapability rdf:datatype="http://www.w3.org/2001/XMLSchema#integer">3</EmpowerBP:appropriateForPhysicalCapability>
        <EmpowerBP:appropriateForPhysicalOpportunity rdf:datatype="http://www.w3.org/2001/XMLSchema#integer">3</EmpowerBP:appropriateForPhysicalOpportunity>
        <EmpowerBP:appropriateForPsychologicalCapability rdf:datatype="http://www.w3.org/2001/XMLSchema#integer">3</EmpowerBP:appropriateForPsychologicalCapability>
        <EmpowerBP:appropriateForReflectiveMotivation rdf:datatype="http://www.w3.org/2001/XMLSchema#integer">6</EmpowerBP:appropriateForReflectiveMotivation>
        <EmpowerBP:appropriateForSocialOpportunity rdf:datatype="http://www.w3.org/2001/XMLSchema#integer">3</EmpowerBP:appropriateForSocialOpportunity>
        <EmpowerBP:canRepeat rdf:datatype="http://www.w3.org/2001/XMLSchema#integer">26</EmpowerBP:canRepeat>
        <EmpowerBP:itemName rdf:datatype="http://www.w3.org/2001/XMLSchema#string">Sodium Sense Eating Out </EmpowerBP:itemName>
        <EmpowerBP:itemText rdf:datatype="http://www.w3.org/2001/XMLSchema#string">Easy ways to cut back on sodium when eating out: 

Choose...
• Grilled fish, meat, or poultry
• Pasta in garlic and olive oil
• Pizza with vegetable toppings

Instead of…
• Lasagna or parmigiana dishes
• Pasta in tomato or marinara sauce
• Pizza with bacon, extra cheese, or pepperoni</EmpowerBP:itemText>
        <EmpowerBP:maximumUserAge rdf:datatype="http://www.w3.org/2001/XMLSchema#integer">120</EmpowerBP:maximumUserAge>
        <EmpowerBP:minimumUserAge rdf:datatype="http://www.w3.org/2001/XMLSchema#integer">18</EmpowerBP:minimumUserAge>
        <EmpowerBP:provideJournal rdf:datatype="http://www.w3.org/2001/XMLSchema#boolean">false</EmpowerBP:provideJournal>
        <EmpowerBP:provideLink rdf:datatype="http://www.w3.org/2001/XMLSchema#boolean">false</EmpowerBP:provideLink>
        <EmpowerBP:sourceURL rdf:datatype="http://www.w3.org/2001/XMLSchema#string">http://www.dietitians.ca/Downloads/Factsheets/Sodium-Sense-factsheet-collection.aspx</EmpowerBP:sourceURL>
        <rdfs:comment rdf:datatype="http://www.w3.org/2001/XMLSchema#string">Easy ways to cut back on sodium when eating out: 

Choose...
• Grilled fish, meat, or poultry
• Pasta in garlic and olive oil
• Pizza with vegetable toppings

Instead of…
• Lasagna or parmigiana dishes
• Pasta in tomato or marinara sauce
• Pizza with bacon, extra cheese, or pepperoni</rdfs:comment>
        <rdfs:label rdf:datatype="http://www.w3.org/2001/XMLSchema#string">Sodium Sense Eating Out </rdfs:label>
    </owl:NamedIndividual>
    


    <!-- http://www.semanticweb.org/tswheeler/ontologies/2016/3/EmpowerBP#T34 -->

    <owl:NamedIndividual rdf:about="http://www.semanticweb.org/tswheeler/ontologies/2016/3/EmpowerBP#T34">
        <rdf:type rdf:resource="http://www.semanticweb.org/tswheeler/ontologies/2016/3/EmpowerBP#InterventionItem"/>
        <rdf:type rdf:resource="http://www.semanticweb.org/tswheeler/ontologies/2016/3/EmpowerBP#Tip"/>
        <EmpowerBP:isAppropriateForInterventionGoal rdf:resource="http://www.semanticweb.org/tswheeler/ontologies/2016/3/EmpowerBP#ExerciseMore"/>
        <EmpowerBP:isWarrantedBy rdf:resource="http://purl.bioontology.org/ontology/BCTT#Information_about_health_consequences"/>
        <EmpowerBP:appropriateForAutomaticMotivation rdf:datatype="http://www.w3.org/2001/XMLSchema#integer">3</EmpowerBP:appropriateForAutomaticMotivation>
        <EmpowerBP:appropriateForLocation rdf:datatype="http://www.w3.org/2001/XMLSchema#integer">0</EmpowerBP:appropriateForLocation>
        <EmpowerBP:appropriateForPhysicalCapability rdf:datatype="http://www.w3.org/2001/XMLSchema#integer">3</EmpowerBP:appropriateForPhysicalCapability>
        <EmpowerBP:appropriateForPhysicalOpportunity rdf:datatype="http://www.w3.org/2001/XMLSchema#integer">3</EmpowerBP:appropriateForPhysicalOpportunity>
        <EmpowerBP:appropriateForPsychologicalCapability rdf:datatype="http://www.w3.org/2001/XMLSchema#integer">3</EmpowerBP:appropriateForPsychologicalCapability>
        <EmpowerBP:appropriateForReflectiveMotivation rdf:datatype="http://www.w3.org/2001/XMLSchema#integer">3</EmpowerBP:appropriateForReflectiveMotivation>
        <EmpowerBP:appropriateForSocialOpportunity rdf:datatype="http://www.w3.org/2001/XMLSchema#integer">3</EmpowerBP:appropriateForSocialOpportunity>
        <EmpowerBP:canRepeat rdf:datatype="http://www.w3.org/2001/XMLSchema#integer">26</EmpowerBP:canRepeat>
        <EmpowerBP:itemName rdf:datatype="http://www.w3.org/2001/XMLSchema#string">Benefits of Regular Activity</EmpowerBP:itemName>
        <EmpowerBP:itemText rdf:datatype="http://www.w3.org/2001/XMLSchema#string">• better health
• improved fitness
• better posture and balance
• better self-esteem
• weight control
• stronger muscles and bones 
• feeling more energetic
• relaxation and reduced stress 
• continued independent living in later life</EmpowerBP:itemText>
        <EmpowerBP:maximumUserAge rdf:datatype="http://www.w3.org/2001/XMLSchema#integer">120</EmpowerBP:maximumUserAge>
        <EmpowerBP:minimumUserAge rdf:datatype="http://www.w3.org/2001/XMLSchema#integer">18</EmpowerBP:minimumUserAge>
        <EmpowerBP:provideJournal rdf:datatype="http://www.w3.org/2001/XMLSchema#boolean">false</EmpowerBP:provideJournal>
        <EmpowerBP:provideLink rdf:datatype="http://www.w3.org/2001/XMLSchema#boolean">false</EmpowerBP:provideLink>
        <EmpowerBP:sourceURL rdf:datatype="http://www.w3.org/2001/XMLSchema#string">http://www.physicalactivityplan.org/resources/CPAG.pdf</EmpowerBP:sourceURL>
        <rdfs:comment rdf:datatype="http://www.w3.org/2001/XMLSchema#string">• better health
• improved fitness
• better posture and balance
• better self-esteem
• weight control
• stronger muscles and bones 
• feeling more energetic
• relaxation and reduced stress 
• continued independent living in later life</rdfs:comment>
        <rdfs:label rdf:datatype="http://www.w3.org/2001/XMLSchema#string">Benefits of Regular Activity</rdfs:label>
    </owl:NamedIndividual>
    


    <!-- http://www.semanticweb.org/tswheeler/ontologies/2016/3/EmpowerBP#T35 -->

    <owl:NamedIndividual rdf:about="http://www.semanticweb.org/tswheeler/ontologies/2016/3/EmpowerBP#T35">
        <rdf:type rdf:resource="http://www.semanticweb.org/tswheeler/ontologies/2016/3/EmpowerBP#InterventionItem"/>
        <rdf:type rdf:resource="http://www.semanticweb.org/tswheeler/ontologies/2016/3/EmpowerBP#Tip"/>
        <EmpowerBP:isAppropriateForInterventionGoal rdf:resource="http://www.semanticweb.org/tswheeler/ontologies/2016/3/EmpowerBP#ExerciseMore"/>
        <EmpowerBP:isWarrantedBy rdf:resource="http://purl.bioontology.org/ontology/BCTT#Information_about_health_consequences"/>
        <EmpowerBP:appropriateForAutomaticMotivation rdf:datatype="http://www.w3.org/2001/XMLSchema#integer">3</EmpowerBP:appropriateForAutomaticMotivation>
        <EmpowerBP:appropriateForLocation rdf:datatype="http://www.w3.org/2001/XMLSchema#integer">0</EmpowerBP:appropriateForLocation>
        <EmpowerBP:appropriateForPhysicalCapability rdf:datatype="http://www.w3.org/2001/XMLSchema#integer">3</EmpowerBP:appropriateForPhysicalCapability>
        <EmpowerBP:appropriateForPhysicalOpportunity rdf:datatype="http://www.w3.org/2001/XMLSchema#integer">3</EmpowerBP:appropriateForPhysicalOpportunity>
        <EmpowerBP:appropriateForPsychologicalCapability rdf:datatype="http://www.w3.org/2001/XMLSchema#integer">3</EmpowerBP:appropriateForPsychologicalCapability>
        <EmpowerBP:appropriateForReflectiveMotivation rdf:datatype="http://www.w3.org/2001/XMLSchema#integer">3</EmpowerBP:appropriateForReflectiveMotivation>
        <EmpowerBP:appropriateForSocialOpportunity rdf:datatype="http://www.w3.org/2001/XMLSchema#integer">3</EmpowerBP:appropriateForSocialOpportunity>
        <EmpowerBP:canRepeat rdf:datatype="http://www.w3.org/2001/XMLSchema#integer">26</EmpowerBP:canRepeat>
        <EmpowerBP:itemName rdf:datatype="http://www.w3.org/2001/XMLSchema#string">Health Risks of Inactivity</EmpowerBP:itemName>
        <EmpowerBP:itemText rdf:datatype="http://www.w3.org/2001/XMLSchema#string">• premature death
• heart disease
• obesity
• high blood pressure 
• adult-onset diabetes 
• osteoporosis
• stroke
• depression 
• colon cancer</EmpowerBP:itemText>
        <EmpowerBP:maximumUserAge rdf:datatype="http://www.w3.org/2001/XMLSchema#integer">120</EmpowerBP:maximumUserAge>
        <EmpowerBP:minimumUserAge rdf:datatype="http://www.w3.org/2001/XMLSchema#integer">18</EmpowerBP:minimumUserAge>
        <EmpowerBP:provideJournal rdf:datatype="http://www.w3.org/2001/XMLSchema#boolean">false</EmpowerBP:provideJournal>
        <EmpowerBP:provideLink rdf:datatype="http://www.w3.org/2001/XMLSchema#boolean">false</EmpowerBP:provideLink>
        <EmpowerBP:sourceURL rdf:datatype="http://www.w3.org/2001/XMLSchema#string">http://www.physicalactivityplan.org/resources/CPAG.pdf</EmpowerBP:sourceURL>
        <rdfs:comment rdf:datatype="http://www.w3.org/2001/XMLSchema#string">• premature death
• heart disease
• obesity
• high blood pressure 
• adult-onset diabetes 
• osteoporosis
• stroke
• depression 
• colon cancer</rdfs:comment>
        <rdfs:label rdf:datatype="http://www.w3.org/2001/XMLSchema#string">Health Risks of Inactivity</rdfs:label>
    </owl:NamedIndividual>
    


    <!-- http://www.semanticweb.org/tswheeler/ontologies/2016/3/EmpowerBP#T36 -->

    <owl:NamedIndividual rdf:about="http://www.semanticweb.org/tswheeler/ontologies/2016/3/EmpowerBP#T36">
        <rdf:type rdf:resource="http://www.semanticweb.org/tswheeler/ontologies/2016/3/EmpowerBP#InterventionItem"/>
        <rdf:type rdf:resource="http://www.semanticweb.org/tswheeler/ontologies/2016/3/EmpowerBP#Tip"/>
        <EmpowerBP:isAppropriateForInterventionGoal rdf:resource="http://www.semanticweb.org/tswheeler/ontologies/2016/3/EmpowerBP#ExerciseMore"/>
        <EmpowerBP:isWarrantedBy rdf:resource="http://purl.bioontology.org/ontology/BCTT#Habit_formation"/>
        <EmpowerBP:appropriateForAutomaticMotivation rdf:datatype="http://www.w3.org/2001/XMLSchema#integer">6</EmpowerBP:appropriateForAutomaticMotivation>
        <EmpowerBP:appropriateForLocation rdf:datatype="http://www.w3.org/2001/XMLSchema#integer">0</EmpowerBP:appropriateForLocation>
        <EmpowerBP:appropriateForPhysicalCapability rdf:datatype="http://www.w3.org/2001/XMLSchema#integer">3</EmpowerBP:appropriateForPhysicalCapability>
        <EmpowerBP:appropriateForPhysicalOpportunity rdf:datatype="http://www.w3.org/2001/XMLSchema#integer">3</EmpowerBP:appropriateForPhysicalOpportunity>
        <EmpowerBP:appropriateForPsychologicalCapability rdf:datatype="http://www.w3.org/2001/XMLSchema#integer">3</EmpowerBP:appropriateForPsychologicalCapability>
        <EmpowerBP:appropriateForReflectiveMotivation rdf:datatype="http://www.w3.org/2001/XMLSchema#integer">6</EmpowerBP:appropriateForReflectiveMotivation>
        <EmpowerBP:appropriateForSocialOpportunity rdf:datatype="http://www.w3.org/2001/XMLSchema#integer">3</EmpowerBP:appropriateForSocialOpportunity>
        <EmpowerBP:canRepeat rdf:datatype="http://www.w3.org/2001/XMLSchema#integer">26</EmpowerBP:canRepeat>
        <EmpowerBP:itemName rdf:datatype="http://www.w3.org/2001/XMLSchema#string">Activities You Can Do at Home</EmpowerBP:itemName>
        <EmpowerBP:itemText rdf:datatype="http://www.w3.org/2001/XMLSchema#string">• Create a new morning routine. Start your day with 10 minutes of movement indoors or outdoors. Some stretching and a short walk first thing in the morning can be better than caffeine.
• Go for a bike ride.
• Park the car 10 minutes away from the store you are going to. Better yet, leave the car at home.
• Dance to your favourite up-beat music for 10 minutes a day.

</EmpowerBP:itemText>
        <EmpowerBP:maximumUserAge rdf:datatype="http://www.w3.org/2001/XMLSchema#integer">120</EmpowerBP:maximumUserAge>
        <EmpowerBP:minimumUserAge rdf:datatype="http://www.w3.org/2001/XMLSchema#integer">18</EmpowerBP:minimumUserAge>
        <EmpowerBP:provideJournal rdf:datatype="http://www.w3.org/2001/XMLSchema#boolean">false</EmpowerBP:provideJournal>
        <EmpowerBP:provideLink rdf:datatype="http://www.w3.org/2001/XMLSchema#boolean">false</EmpowerBP:provideLink>
        <EmpowerBP:sourceURL rdf:datatype="http://www.w3.org/2001/XMLSchema#string">http://www.physicalactivityplan.org/resources/CPAG.pdf</EmpowerBP:sourceURL>
        <rdfs:comment rdf:datatype="http://www.w3.org/2001/XMLSchema#string">• Create a new morning routine. Start your day with 10 minutes of movement indoors or outdoors. Some stretching and a short walk first thing in the morning can be better than caffeine.
• Go for a bike ride.
• Park the car 10 minutes away from the store you are going to. Better yet, leave the car at home.
• Dance to your favourite up-beat music for 10 minutes a day.

</rdfs:comment>
        <rdfs:label rdf:datatype="http://www.w3.org/2001/XMLSchema#string">Activities You Can Do at Home</rdfs:label>
    </owl:NamedIndividual>
    


    <!-- http://www.semanticweb.org/tswheeler/ontologies/2016/3/EmpowerBP#T37 -->

    <owl:NamedIndividual rdf:about="http://www.semanticweb.org/tswheeler/ontologies/2016/3/EmpowerBP#T37">
        <rdf:type rdf:resource="http://www.semanticweb.org/tswheeler/ontologies/2016/3/EmpowerBP#InterventionItem"/>
        <rdf:type rdf:resource="http://www.semanticweb.org/tswheeler/ontologies/2016/3/EmpowerBP#Tip"/>
        <EmpowerBP:isAppropriateForInterventionGoal rdf:resource="http://www.semanticweb.org/tswheeler/ontologies/2016/3/EmpowerBP#ExerciseMore"/>
        <EmpowerBP:isWarrantedBy rdf:resource="http://purl.bioontology.org/ontology/BCTT#Instruction_on_how_to_perform_the_behavior"/>
        <EmpowerBP:appropriateForAutomaticMotivation rdf:datatype="http://www.w3.org/2001/XMLSchema#integer">6</EmpowerBP:appropriateForAutomaticMotivation>
        <EmpowerBP:appropriateForLocation rdf:datatype="http://www.w3.org/2001/XMLSchema#integer">0</EmpowerBP:appropriateForLocation>
        <EmpowerBP:appropriateForPhysicalCapability rdf:datatype="http://www.w3.org/2001/XMLSchema#integer">3</EmpowerBP:appropriateForPhysicalCapability>
        <EmpowerBP:appropriateForPhysicalOpportunity rdf:datatype="http://www.w3.org/2001/XMLSchema#integer">3</EmpowerBP:appropriateForPhysicalOpportunity>
        <EmpowerBP:appropriateForPsychologicalCapability rdf:datatype="http://www.w3.org/2001/XMLSchema#integer">3</EmpowerBP:appropriateForPsychologicalCapability>
        <EmpowerBP:appropriateForReflectiveMotivation rdf:datatype="http://www.w3.org/2001/XMLSchema#integer">6</EmpowerBP:appropriateForReflectiveMotivation>
        <EmpowerBP:appropriateForSocialOpportunity rdf:datatype="http://www.w3.org/2001/XMLSchema#integer">3</EmpowerBP:appropriateForSocialOpportunity>
        <EmpowerBP:canRepeat rdf:datatype="http://www.w3.org/2001/XMLSchema#integer">26</EmpowerBP:canRepeat>
        <EmpowerBP:itemName rdf:datatype="http://www.w3.org/2001/XMLSchema#string">Activities You Can Do at Home</EmpowerBP:itemName>
        <EmpowerBP:itemText rdf:datatype="http://www.w3.org/2001/XMLSchema#string">• If you live in a seniors’ residence, start a hall-walking group. Add to your route each week and pick up friends along the way.
• Parents – play catch or fly a kite with your kids.
• Trade in your power mower for a push mower.
• Do a physical activity routine with leaders on TV or online.</EmpowerBP:itemText>
        <EmpowerBP:maximumUserAge rdf:datatype="http://www.w3.org/2001/XMLSchema#integer">120</EmpowerBP:maximumUserAge>
        <EmpowerBP:minimumUserAge rdf:datatype="http://www.w3.org/2001/XMLSchema#integer">18</EmpowerBP:minimumUserAge>
        <EmpowerBP:provideJournal rdf:datatype="http://www.w3.org/2001/XMLSchema#boolean">false</EmpowerBP:provideJournal>
        <EmpowerBP:provideLink rdf:datatype="http://www.w3.org/2001/XMLSchema#boolean">false</EmpowerBP:provideLink>
        <EmpowerBP:sourceURL rdf:datatype="http://www.w3.org/2001/XMLSchema#string">http://www.physicalactivityplan.org/resources/CPAG.pdf</EmpowerBP:sourceURL>
        <rdfs:comment rdf:datatype="http://www.w3.org/2001/XMLSchema#string">• If you live in a seniors’ residence, start a hall-walking group. Add to your route each week and pick up friends along the way.
• Parents – play catch or fly a kite with your kids.
• Trade in your power mower for a push mower.
• Do a physical activity routine with leaders on TV or online.</rdfs:comment>
        <rdfs:label rdf:datatype="http://www.w3.org/2001/XMLSchema#string">Activities You Can Do at Home</rdfs:label>
    </owl:NamedIndividual>
    


    <!-- http://www.semanticweb.org/tswheeler/ontologies/2016/3/EmpowerBP#T38 -->

    <owl:NamedIndividual rdf:about="http://www.semanticweb.org/tswheeler/ontologies/2016/3/EmpowerBP#T38">
        <rdf:type rdf:resource="http://www.semanticweb.org/tswheeler/ontologies/2016/3/EmpowerBP#InterventionItem"/>
        <rdf:type rdf:resource="http://www.semanticweb.org/tswheeler/ontologies/2016/3/EmpowerBP#Tip"/>
        <EmpowerBP:isAppropriateForInterventionGoal rdf:resource="http://www.semanticweb.org/tswheeler/ontologies/2016/3/EmpowerBP#ExerciseMore"/>
        <EmpowerBP:isWarrantedBy rdf:resource="http://purl.bioontology.org/ontology/BCTT#Instruction_on_how_to_perform_the_behavior"/>
        <EmpowerBP:appropriateForAutomaticMotivation rdf:datatype="http://www.w3.org/2001/XMLSchema#integer">6</EmpowerBP:appropriateForAutomaticMotivation>
        <EmpowerBP:appropriateForLocation rdf:datatype="http://www.w3.org/2001/XMLSchema#integer">0</EmpowerBP:appropriateForLocation>
        <EmpowerBP:appropriateForPhysicalCapability rdf:datatype="http://www.w3.org/2001/XMLSchema#integer">3</EmpowerBP:appropriateForPhysicalCapability>
        <EmpowerBP:appropriateForPhysicalOpportunity rdf:datatype="http://www.w3.org/2001/XMLSchema#integer">3</EmpowerBP:appropriateForPhysicalOpportunity>
        <EmpowerBP:appropriateForPsychologicalCapability rdf:datatype="http://www.w3.org/2001/XMLSchema#integer">3</EmpowerBP:appropriateForPsychologicalCapability>
        <EmpowerBP:appropriateForReflectiveMotivation rdf:datatype="http://www.w3.org/2001/XMLSchema#integer">6</EmpowerBP:appropriateForReflectiveMotivation>
        <EmpowerBP:appropriateForSocialOpportunity rdf:datatype="http://www.w3.org/2001/XMLSchema#integer">3</EmpowerBP:appropriateForSocialOpportunity>
        <EmpowerBP:canRepeat rdf:datatype="http://www.w3.org/2001/XMLSchema#integer">26</EmpowerBP:canRepeat>
        <EmpowerBP:itemName rdf:datatype="http://www.w3.org/2001/XMLSchema#string">Activities You Can Do at Work</EmpowerBP:itemName>
        <EmpowerBP:itemText rdf:datatype="http://www.w3.org/2001/XMLSchema#string">• Take stretch breaks during meetings.
• Have a “walking” meeting – grab your colleague and discuss business while taking a walk.
• Take the stairs. Pretend the elevator is out of service.
• Post a notice near the entrance to the stairway suggesting people take the stairs and have them sign it when they do to encourage others to follow their lead.
</EmpowerBP:itemText>
        <EmpowerBP:maximumUserAge rdf:datatype="http://www.w3.org/2001/XMLSchema#integer">120</EmpowerBP:maximumUserAge>
        <EmpowerBP:minimumUserAge rdf:datatype="http://www.w3.org/2001/XMLSchema#integer">18</EmpowerBP:minimumUserAge>
        <EmpowerBP:provideJournal rdf:datatype="http://www.w3.org/2001/XMLSchema#boolean">false</EmpowerBP:provideJournal>
        <EmpowerBP:provideLink rdf:datatype="http://www.w3.org/2001/XMLSchema#boolean">false</EmpowerBP:provideLink>
        <EmpowerBP:sourceURL rdf:datatype="http://www.w3.org/2001/XMLSchema#string">http://www.physicalactivityplan.org/resources/CPAG.pdf</EmpowerBP:sourceURL>
        <rdfs:comment rdf:datatype="http://www.w3.org/2001/XMLSchema#string">• Take stretch breaks during meetings.
• Have a “walking” meeting – grab your colleague and discuss business while taking a walk.
• Take the stairs. Pretend the elevator is out of service.
• Post a notice near the entrance to the stairway suggesting people take the stairs and have them sign it when they do to encourage others to follow their lead.
</rdfs:comment>
        <rdfs:label rdf:datatype="http://www.w3.org/2001/XMLSchema#string">Activities You Can Do at Work</rdfs:label>
    </owl:NamedIndividual>
    


    <!-- http://www.semanticweb.org/tswheeler/ontologies/2016/3/EmpowerBP#T39 -->

    <owl:NamedIndividual rdf:about="http://www.semanticweb.org/tswheeler/ontologies/2016/3/EmpowerBP#T39">
        <rdf:type rdf:resource="http://www.semanticweb.org/tswheeler/ontologies/2016/3/EmpowerBP#InterventionItem"/>
        <rdf:type rdf:resource="http://www.semanticweb.org/tswheeler/ontologies/2016/3/EmpowerBP#Tip"/>
        <EmpowerBP:isAppropriateForInterventionGoal rdf:resource="http://www.semanticweb.org/tswheeler/ontologies/2016/3/EmpowerBP#ExerciseMore"/>
        <EmpowerBP:isWarrantedBy rdf:resource="http://purl.bioontology.org/ontology/BCTT#Instruction_on_how_to_perform_the_behavior"/>
        <EmpowerBP:appropriateForAutomaticMotivation rdf:datatype="http://www.w3.org/2001/XMLSchema#integer">6</EmpowerBP:appropriateForAutomaticMotivation>
        <EmpowerBP:appropriateForLocation rdf:datatype="http://www.w3.org/2001/XMLSchema#integer">0</EmpowerBP:appropriateForLocation>
        <EmpowerBP:appropriateForPhysicalCapability rdf:datatype="http://www.w3.org/2001/XMLSchema#integer">3</EmpowerBP:appropriateForPhysicalCapability>
        <EmpowerBP:appropriateForPhysicalOpportunity rdf:datatype="http://www.w3.org/2001/XMLSchema#integer">3</EmpowerBP:appropriateForPhysicalOpportunity>
        <EmpowerBP:appropriateForPsychologicalCapability rdf:datatype="http://www.w3.org/2001/XMLSchema#integer">3</EmpowerBP:appropriateForPsychologicalCapability>
        <EmpowerBP:appropriateForReflectiveMotivation rdf:datatype="http://www.w3.org/2001/XMLSchema#integer">6</EmpowerBP:appropriateForReflectiveMotivation>
        <EmpowerBP:appropriateForSocialOpportunity rdf:datatype="http://www.w3.org/2001/XMLSchema#integer">3</EmpowerBP:appropriateForSocialOpportunity>
        <EmpowerBP:canRepeat rdf:datatype="http://www.w3.org/2001/XMLSchema#integer">26</EmpowerBP:canRepeat>
        <EmpowerBP:itemName rdf:datatype="http://www.w3.org/2001/XMLSchema#string">Activities You Can Do at Work</EmpowerBP:itemName>
        <EmpowerBP:itemText rdf:datatype="http://www.w3.org/2001/XMLSchema#string">• Replace your coffee break with a walking/wheeling break.
• Contract your stomach and back muscles while sitting in your chair or on the bus.
• Take a brisk walk before lunch for about 10 minutes.
• Try to make active living one of the goals of your work team. 
• Roll your shoulders and stretch your neck when sitting in front of the computer.</EmpowerBP:itemText>
        <EmpowerBP:maximumUserAge rdf:datatype="http://www.w3.org/2001/XMLSchema#integer">120</EmpowerBP:maximumUserAge>
        <EmpowerBP:minimumUserAge rdf:datatype="http://www.w3.org/2001/XMLSchema#integer">18</EmpowerBP:minimumUserAge>
        <EmpowerBP:provideJournal rdf:datatype="http://www.w3.org/2001/XMLSchema#boolean">false</EmpowerBP:provideJournal>
        <EmpowerBP:provideLink rdf:datatype="http://www.w3.org/2001/XMLSchema#boolean">false</EmpowerBP:provideLink>
        <EmpowerBP:sourceURL rdf:datatype="http://www.w3.org/2001/XMLSchema#string">http://www.physicalactivityplan.org/resources/CPAG.pdf</EmpowerBP:sourceURL>
        <rdfs:comment rdf:datatype="http://www.w3.org/2001/XMLSchema#string">• Replace your coffee break with a walking/wheeling break.
• Contract your stomach and back muscles while sitting in your chair or on the bus.
• Take a brisk walk before lunch for about 10 minutes.
• Try to make active living one of the goals of your work team. 
• Roll your shoulders and stretch your neck when sitting in front of the computer.</rdfs:comment>
        <rdfs:label rdf:datatype="http://www.w3.org/2001/XMLSchema#string">Activities You Can Do at Work</rdfs:label>
    </owl:NamedIndividual>
    


    <!-- http://www.semanticweb.org/tswheeler/ontologies/2016/3/EmpowerBP#T4 -->

    <owl:NamedIndividual rdf:about="http://www.semanticweb.org/tswheeler/ontologies/2016/3/EmpowerBP#T4">
        <rdf:type rdf:resource="http://www.semanticweb.org/tswheeler/ontologies/2016/3/EmpowerBP#InterventionItem"/>
        <rdf:type rdf:resource="http://www.semanticweb.org/tswheeler/ontologies/2016/3/EmpowerBP#Tip"/>
        <EmpowerBP:isAppropriateForInterventionGoal rdf:resource="http://www.semanticweb.org/tswheeler/ontologies/2016/3/EmpowerBP#ExerciseMore"/>
        <EmpowerBP:isWarrantedBy rdf:resource="http://purl.bioontology.org/ontology/BCTT#Information_about_health_consequences"/>
        <EmpowerBP:appropriateForAutomaticMotivation rdf:datatype="http://www.w3.org/2001/XMLSchema#integer">3</EmpowerBP:appropriateForAutomaticMotivation>
        <EmpowerBP:appropriateForLocation rdf:datatype="http://www.w3.org/2001/XMLSchema#integer">0</EmpowerBP:appropriateForLocation>
        <EmpowerBP:appropriateForPhysicalCapability rdf:datatype="http://www.w3.org/2001/XMLSchema#integer">3</EmpowerBP:appropriateForPhysicalCapability>
        <EmpowerBP:appropriateForPhysicalOpportunity rdf:datatype="http://www.w3.org/2001/XMLSchema#integer">3</EmpowerBP:appropriateForPhysicalOpportunity>
        <EmpowerBP:appropriateForPsychologicalCapability rdf:datatype="http://www.w3.org/2001/XMLSchema#integer">3</EmpowerBP:appropriateForPsychologicalCapability>
        <EmpowerBP:appropriateForReflectiveMotivation rdf:datatype="http://www.w3.org/2001/XMLSchema#integer">3</EmpowerBP:appropriateForReflectiveMotivation>
        <EmpowerBP:appropriateForSocialOpportunity rdf:datatype="http://www.w3.org/2001/XMLSchema#integer">3</EmpowerBP:appropriateForSocialOpportunity>
        <EmpowerBP:canRepeat rdf:datatype="http://www.w3.org/2001/XMLSchema#integer">26</EmpowerBP:canRepeat>
        <EmpowerBP:itemName rdf:datatype="http://www.w3.org/2001/XMLSchema#string">Benefits of Activity</EmpowerBP:itemName>
        <EmpowerBP:itemText rdf:datatype="http://www.w3.org/2001/XMLSchema#string">It’s always a good idea to add physical activity to your life, regardless of your age. Physical activity can:

• dramatically lower your risk of heart disease and stroke
• help prevent and control risk factors such as high blood pressure, high cholesterol, type 2 diabetes, osteoporosis, certain types of cancer, and obesity
• reduce stress levels
• increase energy
• improve sleep
• improve digestion</EmpowerBP:itemText>
        <EmpowerBP:maximumUserAge rdf:datatype="http://www.w3.org/2001/XMLSchema#integer">120</EmpowerBP:maximumUserAge>
        <EmpowerBP:minimumUserAge rdf:datatype="http://www.w3.org/2001/XMLSchema#integer">18</EmpowerBP:minimumUserAge>
        <EmpowerBP:provideJournal rdf:datatype="http://www.w3.org/2001/XMLSchema#boolean">false</EmpowerBP:provideJournal>
        <EmpowerBP:provideLink rdf:datatype="http://www.w3.org/2001/XMLSchema#boolean">false</EmpowerBP:provideLink>
        <EmpowerBP:sourceURL rdf:datatype="http://www.w3.org/2001/XMLSchema#string">http://www.heartandstroke.ca/get-healthy/stay-active/benefits-of-physical-activity</EmpowerBP:sourceURL>
        <rdfs:comment rdf:datatype="http://www.w3.org/2001/XMLSchema#string">It’s always a good idea to add physical activity to your life, regardless of your age. Physical activity can:

• dramatically lower your risk of heart disease and stroke
• help prevent and control risk factors such as high blood pressure, high cholesterol, type 2 diabetes, osteoporosis, certain types of cancer, and obesity
• reduce stress levels
• increase energy
• improve sleep
• improve digestion</rdfs:comment>
        <rdfs:label rdf:datatype="http://www.w3.org/2001/XMLSchema#string">Benefits of Activity</rdfs:label>
    </owl:NamedIndividual>
    


    <!-- http://www.semanticweb.org/tswheeler/ontologies/2016/3/EmpowerBP#T40 -->

    <owl:NamedIndividual rdf:about="http://www.semanticweb.org/tswheeler/ontologies/2016/3/EmpowerBP#T40">
        <rdf:type rdf:resource="http://www.semanticweb.org/tswheeler/ontologies/2016/3/EmpowerBP#InterventionItem"/>
        <rdf:type rdf:resource="http://www.semanticweb.org/tswheeler/ontologies/2016/3/EmpowerBP#Tip"/>
        <EmpowerBP:isAppropriateForInterventionGoal rdf:resource="http://www.semanticweb.org/tswheeler/ontologies/2016/3/EmpowerBP#ExerciseMore"/>
        <EmpowerBP:isWarrantedBy rdf:resource="http://purl.bioontology.org/ontology/BCTT#Instruction_on_how_to_perform_the_behavior"/>
        <EmpowerBP:appropriateForAutomaticMotivation rdf:datatype="http://www.w3.org/2001/XMLSchema#integer">6</EmpowerBP:appropriateForAutomaticMotivation>
        <EmpowerBP:appropriateForLocation rdf:datatype="http://www.w3.org/2001/XMLSchema#integer">0</EmpowerBP:appropriateForLocation>
        <EmpowerBP:appropriateForPhysicalCapability rdf:datatype="http://www.w3.org/2001/XMLSchema#integer">3</EmpowerBP:appropriateForPhysicalCapability>
        <EmpowerBP:appropriateForPhysicalOpportunity rdf:datatype="http://www.w3.org/2001/XMLSchema#integer">3</EmpowerBP:appropriateForPhysicalOpportunity>
        <EmpowerBP:appropriateForPsychologicalCapability rdf:datatype="http://www.w3.org/2001/XMLSchema#integer">3</EmpowerBP:appropriateForPsychologicalCapability>
        <EmpowerBP:appropriateForReflectiveMotivation rdf:datatype="http://www.w3.org/2001/XMLSchema#integer">6</EmpowerBP:appropriateForReflectiveMotivation>
        <EmpowerBP:appropriateForSocialOpportunity rdf:datatype="http://www.w3.org/2001/XMLSchema#integer">3</EmpowerBP:appropriateForSocialOpportunity>
        <EmpowerBP:canRepeat rdf:datatype="http://www.w3.org/2001/XMLSchema#integer">26</EmpowerBP:canRepeat>
        <EmpowerBP:itemName rdf:datatype="http://www.w3.org/2001/XMLSchema#string">Activities You Can Do at Play</EmpowerBP:itemName>
        <EmpowerBP:itemText rdf:datatype="http://www.w3.org/2001/XMLSchema#string">• Make a personal or family commitment to try a new activity each season: snowshoe, curl, hike, bike, dance, bowl, fish, camp, ice-skate, ski, swim, in-line skate, walk, run, skip rope, play tag with your kids, or play ball in the park.
• Join a club or organization that coordinates active living events.
• Participate in community programs like SummerActive and
try some new activities.
• Get in the garden and dig, prune, rake and weed.</EmpowerBP:itemText>
        <EmpowerBP:maximumUserAge rdf:datatype="http://www.w3.org/2001/XMLSchema#integer">120</EmpowerBP:maximumUserAge>
        <EmpowerBP:minimumUserAge rdf:datatype="http://www.w3.org/2001/XMLSchema#integer">18</EmpowerBP:minimumUserAge>
        <EmpowerBP:provideJournal rdf:datatype="http://www.w3.org/2001/XMLSchema#boolean">false</EmpowerBP:provideJournal>
        <EmpowerBP:provideLink rdf:datatype="http://www.w3.org/2001/XMLSchema#boolean">false</EmpowerBP:provideLink>
        <EmpowerBP:sourceURL rdf:datatype="http://www.w3.org/2001/XMLSchema#string">http://www.physicalactivityplan.org/resources/CPAG.pdf</EmpowerBP:sourceURL>
        <rdfs:comment rdf:datatype="http://www.w3.org/2001/XMLSchema#string">• Make a personal or family commitment to try a new activity each season: snowshoe, curl, hike, bike, dance, bowl, fish, camp, ice-skate, ski, swim, in-line skate, walk, run, skip rope, play tag with your kids, or play ball in the park.
• Join a club or organization that coordinates active living events.
• Participate in community programs like SummerActive and
try some new activities.
• Get in the garden and dig, prune, rake and weed.</rdfs:comment>
        <rdfs:label rdf:datatype="http://www.w3.org/2001/XMLSchema#string">Activities You Can Do at Play</rdfs:label>
    </owl:NamedIndividual>
    


    <!-- http://www.semanticweb.org/tswheeler/ontologies/2016/3/EmpowerBP#T41 -->

    <owl:NamedIndividual rdf:about="http://www.semanticweb.org/tswheeler/ontologies/2016/3/EmpowerBP#T41">
        <rdf:type rdf:resource="http://www.semanticweb.org/tswheeler/ontologies/2016/3/EmpowerBP#InterventionItem"/>
        <rdf:type rdf:resource="http://www.semanticweb.org/tswheeler/ontologies/2016/3/EmpowerBP#Tip"/>
        <EmpowerBP:isAppropriateForInterventionGoal rdf:resource="http://www.semanticweb.org/tswheeler/ontologies/2016/3/EmpowerBP#ExerciseMore"/>
        <EmpowerBP:isWarrantedBy rdf:resource="http://purl.bioontology.org/ontology/BCTT#Instruction_on_how_to_perform_the_behavior"/>
        <EmpowerBP:appropriateForAutomaticMotivation rdf:datatype="http://www.w3.org/2001/XMLSchema#integer">6</EmpowerBP:appropriateForAutomaticMotivation>
        <EmpowerBP:appropriateForLocation rdf:datatype="http://www.w3.org/2001/XMLSchema#integer">0</EmpowerBP:appropriateForLocation>
        <EmpowerBP:appropriateForPhysicalCapability rdf:datatype="http://www.w3.org/2001/XMLSchema#integer">3</EmpowerBP:appropriateForPhysicalCapability>
        <EmpowerBP:appropriateForPhysicalOpportunity rdf:datatype="http://www.w3.org/2001/XMLSchema#integer">3</EmpowerBP:appropriateForPhysicalOpportunity>
        <EmpowerBP:appropriateForPsychologicalCapability rdf:datatype="http://www.w3.org/2001/XMLSchema#integer">3</EmpowerBP:appropriateForPsychologicalCapability>
        <EmpowerBP:appropriateForReflectiveMotivation rdf:datatype="http://www.w3.org/2001/XMLSchema#integer">6</EmpowerBP:appropriateForReflectiveMotivation>
        <EmpowerBP:appropriateForSocialOpportunity rdf:datatype="http://www.w3.org/2001/XMLSchema#integer">3</EmpowerBP:appropriateForSocialOpportunity>
        <EmpowerBP:canRepeat rdf:datatype="http://www.w3.org/2001/XMLSchema#integer">26</EmpowerBP:canRepeat>
        <EmpowerBP:itemName rdf:datatype="http://www.w3.org/2001/XMLSchema#string">Activities You Can Do at Play</EmpowerBP:itemName>
        <EmpowerBP:itemText rdf:datatype="http://www.w3.org/2001/XMLSchema#string">• See how many different 10-minute walking, wheeling or cycling routes you can find in your neighbourhood.
• Hit a tennis ball with a friend.
• Arrange to meet a couple of friends for a walk every day
at the same time.
• Join a T’ai Chi or yoga class.
• Go line dancing, folk dancing, or square dancing.</EmpowerBP:itemText>
        <EmpowerBP:maximumUserAge rdf:datatype="http://www.w3.org/2001/XMLSchema#integer">120</EmpowerBP:maximumUserAge>
        <EmpowerBP:minimumUserAge rdf:datatype="http://www.w3.org/2001/XMLSchema#integer">18</EmpowerBP:minimumUserAge>
        <EmpowerBP:provideJournal rdf:datatype="http://www.w3.org/2001/XMLSchema#boolean">false</EmpowerBP:provideJournal>
        <EmpowerBP:provideLink rdf:datatype="http://www.w3.org/2001/XMLSchema#boolean">false</EmpowerBP:provideLink>
        <EmpowerBP:sourceURL rdf:datatype="http://www.w3.org/2001/XMLSchema#string">http://www.physicalactivityplan.org/resources/CPAG.pdf</EmpowerBP:sourceURL>
        <rdfs:comment rdf:datatype="http://www.w3.org/2001/XMLSchema#string">• See how many different 10-minute walking, wheeling or cycling routes you can find in your neighbourhood.
• Hit a tennis ball with a friend.
• Arrange to meet a couple of friends for a walk every day
at the same time.
• Join a T’ai Chi or yoga class.
• Go line dancing, folk dancing, or square dancing.</rdfs:comment>
        <rdfs:label rdf:datatype="http://www.w3.org/2001/XMLSchema#string">Activities You Can Do at Play</rdfs:label>
    </owl:NamedIndividual>
    


    <!-- http://www.semanticweb.org/tswheeler/ontologies/2016/3/EmpowerBP#T42 -->

    <owl:NamedIndividual rdf:about="http://www.semanticweb.org/tswheeler/ontologies/2016/3/EmpowerBP#T42">
        <rdf:type rdf:resource="http://www.semanticweb.org/tswheeler/ontologies/2016/3/EmpowerBP#InterventionItem"/>
        <rdf:type rdf:resource="http://www.semanticweb.org/tswheeler/ontologies/2016/3/EmpowerBP#Tip"/>
        <EmpowerBP:isAppropriateForInterventionGoal rdf:resource="http://www.semanticweb.org/tswheeler/ontologies/2016/3/EmpowerBP#ExerciseMore"/>
        <EmpowerBP:isWarrantedBy rdf:resource="http://purl.bioontology.org/ontology/BCTT#Instruction_on_how_to_perform_the_behavior"/>
        <EmpowerBP:appropriateForAutomaticMotivation rdf:datatype="http://www.w3.org/2001/XMLSchema#integer">6</EmpowerBP:appropriateForAutomaticMotivation>
        <EmpowerBP:appropriateForLocation rdf:datatype="http://www.w3.org/2001/XMLSchema#integer">0</EmpowerBP:appropriateForLocation>
        <EmpowerBP:appropriateForPhysicalCapability rdf:datatype="http://www.w3.org/2001/XMLSchema#integer">3</EmpowerBP:appropriateForPhysicalCapability>
        <EmpowerBP:appropriateForPhysicalOpportunity rdf:datatype="http://www.w3.org/2001/XMLSchema#integer">3</EmpowerBP:appropriateForPhysicalOpportunity>
        <EmpowerBP:appropriateForPsychologicalCapability rdf:datatype="http://www.w3.org/2001/XMLSchema#integer">3</EmpowerBP:appropriateForPsychologicalCapability>
        <EmpowerBP:appropriateForReflectiveMotivation rdf:datatype="http://www.w3.org/2001/XMLSchema#integer">6</EmpowerBP:appropriateForReflectiveMotivation>
        <EmpowerBP:appropriateForSocialOpportunity rdf:datatype="http://www.w3.org/2001/XMLSchema#integer">3</EmpowerBP:appropriateForSocialOpportunity>
        <EmpowerBP:canRepeat rdf:datatype="http://www.w3.org/2001/XMLSchema#integer">26</EmpowerBP:canRepeat>
        <EmpowerBP:itemName rdf:datatype="http://www.w3.org/2001/XMLSchema#string">Activities You Can Do on the Way</EmpowerBP:itemName>
        <EmpowerBP:itemText rdf:datatype="http://www.w3.org/2001/XMLSchema#string">• Walk, cycle, in- line skate, or wheel to work or school.
•  Get off the bus two stops early and walk home.
•  Leave the car in a parking lot 10 minutes from work and walk the rest of the way.
• Take your bike to work – you’ll save on gas as well as help to protect the environment and your health.
• If your job involves a lot of driving, plan several short stops in your day. Get out of the car and walk for 10 minutes or more whenever you can.</EmpowerBP:itemText>
        <EmpowerBP:maximumUserAge rdf:datatype="http://www.w3.org/2001/XMLSchema#integer">120</EmpowerBP:maximumUserAge>
        <EmpowerBP:minimumUserAge rdf:datatype="http://www.w3.org/2001/XMLSchema#integer">18</EmpowerBP:minimumUserAge>
        <EmpowerBP:provideJournal rdf:datatype="http://www.w3.org/2001/XMLSchema#boolean">false</EmpowerBP:provideJournal>
        <EmpowerBP:provideLink rdf:datatype="http://www.w3.org/2001/XMLSchema#boolean">false</EmpowerBP:provideLink>
        <EmpowerBP:sourceURL rdf:datatype="http://www.w3.org/2001/XMLSchema#string">http://www.physicalactivityplan.org/resources/CPAG.pdf</EmpowerBP:sourceURL>
        <rdfs:comment rdf:datatype="http://www.w3.org/2001/XMLSchema#string">• Walk, cycle, in- line skate, or wheel to work or school.
•  Get off the bus two stops early and walk home.
•  Leave the car in a parking lot 10 minutes from work and walk the rest of the way.
• Take your bike to work – you’ll save on gas as well as help to protect the environment and your health.
• If your job involves a lot of driving, plan several short stops in your day. Get out of the car and walk for 10 minutes or more whenever you can.</rdfs:comment>
        <rdfs:label rdf:datatype="http://www.w3.org/2001/XMLSchema#string">Activities You Can Do on the Way</rdfs:label>
    </owl:NamedIndividual>
    


    <!-- http://www.semanticweb.org/tswheeler/ontologies/2016/3/EmpowerBP#T43 -->

    <owl:NamedIndividual rdf:about="http://www.semanticweb.org/tswheeler/ontologies/2016/3/EmpowerBP#T43">
        <rdf:type rdf:resource="http://www.semanticweb.org/tswheeler/ontologies/2016/3/EmpowerBP#InterventionItem"/>
        <rdf:type rdf:resource="http://www.semanticweb.org/tswheeler/ontologies/2016/3/EmpowerBP#Tip"/>
        <EmpowerBP:isAppropriateForInterventionGoal rdf:resource="http://www.semanticweb.org/tswheeler/ontologies/2016/3/EmpowerBP#ExerciseMore"/>
        <EmpowerBP:isWarrantedBy rdf:resource="http://purl.bioontology.org/ontology/BCTT#Instruction_on_how_to_perform_the_behavior"/>
        <EmpowerBP:appropriateForAutomaticMotivation rdf:datatype="http://www.w3.org/2001/XMLSchema#integer">6</EmpowerBP:appropriateForAutomaticMotivation>
        <EmpowerBP:appropriateForLocation rdf:datatype="http://www.w3.org/2001/XMLSchema#integer">0</EmpowerBP:appropriateForLocation>
        <EmpowerBP:appropriateForPhysicalCapability rdf:datatype="http://www.w3.org/2001/XMLSchema#integer">3</EmpowerBP:appropriateForPhysicalCapability>
        <EmpowerBP:appropriateForPhysicalOpportunity rdf:datatype="http://www.w3.org/2001/XMLSchema#integer">3</EmpowerBP:appropriateForPhysicalOpportunity>
        <EmpowerBP:appropriateForPsychologicalCapability rdf:datatype="http://www.w3.org/2001/XMLSchema#integer">3</EmpowerBP:appropriateForPsychologicalCapability>
        <EmpowerBP:appropriateForReflectiveMotivation rdf:datatype="http://www.w3.org/2001/XMLSchema#integer">6</EmpowerBP:appropriateForReflectiveMotivation>
        <EmpowerBP:appropriateForSocialOpportunity rdf:datatype="http://www.w3.org/2001/XMLSchema#integer">3</EmpowerBP:appropriateForSocialOpportunity>
        <EmpowerBP:canRepeat rdf:datatype="http://www.w3.org/2001/XMLSchema#integer">26</EmpowerBP:canRepeat>
        <EmpowerBP:itemName rdf:datatype="http://www.w3.org/2001/XMLSchema#string">Strengthening Activities</EmpowerBP:itemName>
        <EmpowerBP:itemText rdf:datatype="http://www.w3.org/2001/XMLSchema#string">What are strengthening activities?

Muscle-strengthening activities build up your muscles. 

Examples of muscle-strengthening activities include push-ups and sit-ups, lifting weights, climbing stairs and digging in the garden.

With bone-strengthening activities,your muscles push and pull against your bones, helping make your bones stronger.

Examples of bone-strengthening activities include running, walking and yoga.

Get stronger by adding activities that target your muscles and bones at least two days per week.


</EmpowerBP:itemText>
        <EmpowerBP:maximumUserAge rdf:datatype="http://www.w3.org/2001/XMLSchema#integer">120</EmpowerBP:maximumUserAge>
        <EmpowerBP:minimumUserAge rdf:datatype="http://www.w3.org/2001/XMLSchema#integer">18</EmpowerBP:minimumUserAge>
        <EmpowerBP:provideJournal rdf:datatype="http://www.w3.org/2001/XMLSchema#boolean">false</EmpowerBP:provideJournal>
        <EmpowerBP:provideLink rdf:datatype="http://www.w3.org/2001/XMLSchema#boolean">false</EmpowerBP:provideLink>
        <EmpowerBP:sourceURL rdf:datatype="http://www.w3.org/2001/XMLSchema#string">http://www.phac-aspc.gc.ca/hp-ps/hl-mvs/pa-ap/07paap-eng.php</EmpowerBP:sourceURL>
        <rdfs:comment rdf:datatype="http://www.w3.org/2001/XMLSchema#string">What are strengthening activities?

Muscle-strengthening activities build up your muscles. 

Examples of muscle-strengthening activities include push-ups and sit-ups, lifting weights, climbing stairs and digging in the garden.

With bone-strengthening activities,your muscles push and pull against your bones, helping make your bones stronger.

Examples of bone-strengthening activities include running, walking and yoga.

Get stronger by adding activities that target your muscles and bones at least two days per week.


</rdfs:comment>
        <rdfs:label rdf:datatype="http://www.w3.org/2001/XMLSchema#string">Strengthening Activities</rdfs:label>
    </owl:NamedIndividual>
    


    <!-- http://www.semanticweb.org/tswheeler/ontologies/2016/3/EmpowerBP#T44 -->

    <owl:NamedIndividual rdf:about="http://www.semanticweb.org/tswheeler/ontologies/2016/3/EmpowerBP#T44">
        <rdf:type rdf:resource="http://www.semanticweb.org/tswheeler/ontologies/2016/3/EmpowerBP#InterventionItem"/>
        <rdf:type rdf:resource="http://www.semanticweb.org/tswheeler/ontologies/2016/3/EmpowerBP#Tip"/>
        <EmpowerBP:isAppropriateForInterventionGoal rdf:resource="http://www.semanticweb.org/tswheeler/ontologies/2016/3/EmpowerBP#ReduceSaltIntake"/>
        <EmpowerBP:isWarrantedBy rdf:resource="http://purl.bioontology.org/ontology/BCTT#Instruction_on_how_to_perform_the_behavior"/>
        <EmpowerBP:appropriateForAutomaticMotivation rdf:datatype="http://www.w3.org/2001/XMLSchema#integer">6</EmpowerBP:appropriateForAutomaticMotivation>
        <EmpowerBP:appropriateForLocation rdf:datatype="http://www.w3.org/2001/XMLSchema#integer">0</EmpowerBP:appropriateForLocation>
        <EmpowerBP:appropriateForPhysicalCapability rdf:datatype="http://www.w3.org/2001/XMLSchema#integer">3</EmpowerBP:appropriateForPhysicalCapability>
        <EmpowerBP:appropriateForPhysicalOpportunity rdf:datatype="http://www.w3.org/2001/XMLSchema#integer">3</EmpowerBP:appropriateForPhysicalOpportunity>
        <EmpowerBP:appropriateForPsychologicalCapability rdf:datatype="http://www.w3.org/2001/XMLSchema#integer">3</EmpowerBP:appropriateForPsychologicalCapability>
        <EmpowerBP:appropriateForReflectiveMotivation rdf:datatype="http://www.w3.org/2001/XMLSchema#integer">6</EmpowerBP:appropriateForReflectiveMotivation>
        <EmpowerBP:appropriateForSocialOpportunity rdf:datatype="http://www.w3.org/2001/XMLSchema#integer">3</EmpowerBP:appropriateForSocialOpportunity>
        <EmpowerBP:canRepeat rdf:datatype="http://www.w3.org/2001/XMLSchema#integer">26</EmpowerBP:canRepeat>
        <EmpowerBP:itemName rdf:datatype="http://www.w3.org/2001/XMLSchema#string">Reading Food Labels</EmpowerBP:itemName>
        <EmpowerBP:itemText rdf:datatype="http://www.w3.org/2001/XMLSchema#string">Other terms for sodium (or salt) to watch for on a label are:

• Celery, garlic or onion salt
• Monosodium glutamate (Accent or MSG)
• Sodium (Sodium Benzoate, Sodium Citrate, Sodium Nitrate)
• Baking soda
• Baking powder
• Brine for pickling
• Soy sauce
• Na (an abbreviation for sodium)

Ingredients are listed in order from most to least. This means the ingredient used in the greatest amount is listed first. Therefore, if sodium or salt appears near the top of the ingredient list, avoid that product. </EmpowerBP:itemText>
        <EmpowerBP:maximumUserAge rdf:datatype="http://www.w3.org/2001/XMLSchema#integer">120</EmpowerBP:maximumUserAge>
        <EmpowerBP:minimumUserAge rdf:datatype="http://www.w3.org/2001/XMLSchema#integer">18</EmpowerBP:minimumUserAge>
        <EmpowerBP:provideJournal rdf:datatype="http://www.w3.org/2001/XMLSchema#boolean">false</EmpowerBP:provideJournal>
        <EmpowerBP:provideLink rdf:datatype="http://www.w3.org/2001/XMLSchema#boolean">false</EmpowerBP:provideLink>
        <EmpowerBP:sourceURL rdf:datatype="http://www.w3.org/2001/XMLSchema#string">https://www.diabetes.ca/diabetes-and-you/healthy-living-resources/diet-nutrition/reducing-salt-intake</EmpowerBP:sourceURL>
        <rdfs:comment rdf:datatype="http://www.w3.org/2001/XMLSchema#string">Other terms for sodium (or salt) to watch for on a label are:

• Celery, garlic or onion salt
• Monosodium glutamate (Accent or MSG)
• Sodium (Sodium Benzoate, Sodium Citrate, Sodium Nitrate)
• Baking soda
• Baking powder
• Brine for pickling
• Soy sauce
• Na (an abbreviation for sodium)

Ingredients are listed in order from most to least. This means the ingredient used in the greatest amount is listed first. Therefore, if sodium or salt appears near the top of the ingredient list, avoid that product. </rdfs:comment>
        <rdfs:label rdf:datatype="http://www.w3.org/2001/XMLSchema#string">Reading Food Labels</rdfs:label>
    </owl:NamedIndividual>
    


    <!-- http://www.semanticweb.org/tswheeler/ontologies/2016/3/EmpowerBP#T45 -->

    <owl:NamedIndividual rdf:about="http://www.semanticweb.org/tswheeler/ontologies/2016/3/EmpowerBP#T45">
        <rdf:type rdf:resource="http://www.semanticweb.org/tswheeler/ontologies/2016/3/EmpowerBP#InterventionItem"/>
        <rdf:type rdf:resource="http://www.semanticweb.org/tswheeler/ontologies/2016/3/EmpowerBP#Tip"/>
        <EmpowerBP:isAppropriateForInterventionGoal rdf:resource="http://www.semanticweb.org/tswheeler/ontologies/2016/3/EmpowerBP#ReduceSaltIntake"/>
        <EmpowerBP:isWarrantedBy rdf:resource="http://purl.bioontology.org/ontology/BCTT#Behavior_substitution"/>
        <EmpowerBP:appropriateForAutomaticMotivation rdf:datatype="http://www.w3.org/2001/XMLSchema#integer">6</EmpowerBP:appropriateForAutomaticMotivation>
        <EmpowerBP:appropriateForLocation rdf:datatype="http://www.w3.org/2001/XMLSchema#integer">0</EmpowerBP:appropriateForLocation>
        <EmpowerBP:appropriateForPhysicalCapability rdf:datatype="http://www.w3.org/2001/XMLSchema#integer">3</EmpowerBP:appropriateForPhysicalCapability>
        <EmpowerBP:appropriateForPhysicalOpportunity rdf:datatype="http://www.w3.org/2001/XMLSchema#integer">3</EmpowerBP:appropriateForPhysicalOpportunity>
        <EmpowerBP:appropriateForPsychologicalCapability rdf:datatype="http://www.w3.org/2001/XMLSchema#integer">3</EmpowerBP:appropriateForPsychologicalCapability>
        <EmpowerBP:appropriateForReflectiveMotivation rdf:datatype="http://www.w3.org/2001/XMLSchema#integer">6</EmpowerBP:appropriateForReflectiveMotivation>
        <EmpowerBP:appropriateForSocialOpportunity rdf:datatype="http://www.w3.org/2001/XMLSchema#integer">3</EmpowerBP:appropriateForSocialOpportunity>
        <EmpowerBP:canRepeat rdf:datatype="http://www.w3.org/2001/XMLSchema#integer">26</EmpowerBP:canRepeat>
        <EmpowerBP:itemName rdf:datatype="http://www.w3.org/2001/XMLSchema#string">Herb Shaker Recipe</EmpowerBP:itemName>
        <EmpowerBP:itemText rdf:datatype="http://www.w3.org/2001/XMLSchema#string">Looking to replace that salt shaker? Try this herb shaker recipe:

2 mL (1/4 tsp) basil
3 mL (1/2 tsp) white pepper
15 mL (1 tbsp) onion powder
15 mL (1 tbsp) garlic powder
2 mL (1/4 tsp) paprika
1 mL (1/8 tsp) rosemary
1 mL (1/8 tsp) celery seed
5 mL (1 tsp) thyme
15 mL (1 tbsp) dry mustard

Blend your ingredients and add to an empty shaker with a few pieces of raw rice to allow for easy flow.</EmpowerBP:itemText>
        <EmpowerBP:maximumUserAge rdf:datatype="http://www.w3.org/2001/XMLSchema#integer">120</EmpowerBP:maximumUserAge>
        <EmpowerBP:minimumUserAge rdf:datatype="http://www.w3.org/2001/XMLSchema#integer">18</EmpowerBP:minimumUserAge>
        <EmpowerBP:provideJournal rdf:datatype="http://www.w3.org/2001/XMLSchema#boolean">false</EmpowerBP:provideJournal>
        <EmpowerBP:provideLink rdf:datatype="http://www.w3.org/2001/XMLSchema#boolean">false</EmpowerBP:provideLink>
        <EmpowerBP:sourceURL rdf:datatype="http://www.w3.org/2001/XMLSchema#string">https://www.diabetes.ca/diabetes-and-you/healthy-living-resources/diet-nutrition/reducing-salt-intake</EmpowerBP:sourceURL>
        <rdfs:comment rdf:datatype="http://www.w3.org/2001/XMLSchema#string">Looking to replace that salt shaker? Try this herb shaker recipe:

2 mL (1/4 tsp) basil
3 mL (1/2 tsp) white pepper
15 mL (1 tbsp) onion powder
15 mL (1 tbsp) garlic powder
2 mL (1/4 tsp) paprika
1 mL (1/8 tsp) rosemary
1 mL (1/8 tsp) celery seed
5 mL (1 tsp) thyme
15 mL (1 tbsp) dry mustard

Blend your ingredients and add to an empty shaker with a few pieces of raw rice to allow for easy flow.</rdfs:comment>
        <rdfs:label rdf:datatype="http://www.w3.org/2001/XMLSchema#string">Herb Shaker Recipe</rdfs:label>
    </owl:NamedIndividual>
    


    <!-- http://www.semanticweb.org/tswheeler/ontologies/2016/3/EmpowerBP#T46 -->

    <owl:NamedIndividual rdf:about="http://www.semanticweb.org/tswheeler/ontologies/2016/3/EmpowerBP#T46">
        <rdf:type rdf:resource="http://www.semanticweb.org/tswheeler/ontologies/2016/3/EmpowerBP#InterventionItem"/>
        <rdf:type rdf:resource="http://www.semanticweb.org/tswheeler/ontologies/2016/3/EmpowerBP#Tip"/>
        <EmpowerBP:isAppropriateForInterventionGoal rdf:resource="http://www.semanticweb.org/tswheeler/ontologies/2016/3/EmpowerBP#ReduceSaltIntake"/>
        <EmpowerBP:isWarrantedBy rdf:resource="http://purl.bioontology.org/ontology/BCTT#Behavior_substitution"/>
        <EmpowerBP:appropriateForAutomaticMotivation rdf:datatype="http://www.w3.org/2001/XMLSchema#integer">6</EmpowerBP:appropriateForAutomaticMotivation>
        <EmpowerBP:appropriateForLocation rdf:datatype="http://www.w3.org/2001/XMLSchema#integer">0</EmpowerBP:appropriateForLocation>
        <EmpowerBP:appropriateForPhysicalCapability rdf:datatype="http://www.w3.org/2001/XMLSchema#integer">3</EmpowerBP:appropriateForPhysicalCapability>
        <EmpowerBP:appropriateForPhysicalOpportunity rdf:datatype="http://www.w3.org/2001/XMLSchema#integer">3</EmpowerBP:appropriateForPhysicalOpportunity>
        <EmpowerBP:appropriateForPsychologicalCapability rdf:datatype="http://www.w3.org/2001/XMLSchema#integer">3</EmpowerBP:appropriateForPsychologicalCapability>
        <EmpowerBP:appropriateForReflectiveMotivation rdf:datatype="http://www.w3.org/2001/XMLSchema#integer">6</EmpowerBP:appropriateForReflectiveMotivation>
        <EmpowerBP:appropriateForSocialOpportunity rdf:datatype="http://www.w3.org/2001/XMLSchema#integer">3</EmpowerBP:appropriateForSocialOpportunity>
        <EmpowerBP:canRepeat rdf:datatype="http://www.w3.org/2001/XMLSchema#integer">26</EmpowerBP:canRepeat>
        <EmpowerBP:itemName rdf:datatype="http://www.w3.org/2001/XMLSchema#string">Sodium - Grains and starches</EmpowerBP:itemName>
        <EmpowerBP:itemText rdf:datatype="http://www.w3.org/2001/XMLSchema#string">Lower sodium foods (choose more of): 

• Whole grains and higher fibre foods such as breads, pasta, cereals, bulk hot cereals
• Grains with no added salt such as unsalted crackers homemade muffins, pancakes, corn breads (made from scratch)
• Homemade soups (can be frozen for later use), or soups that are low sodium or have no added salt

Higher sodium foods (choose less of): 

•   Packaged foods with added salt such as crackers, croutons, seasoned pasta and rice dishes, stuffing, instant hot cereals, instant pancake/waffle mixes
• Canned products such as corn, soups
• Prepared convenience foods such as frozen pizzas, frozen dinners</EmpowerBP:itemText>
        <EmpowerBP:maximumUserAge rdf:datatype="http://www.w3.org/2001/XMLSchema#integer">120</EmpowerBP:maximumUserAge>
        <EmpowerBP:minimumUserAge rdf:datatype="http://www.w3.org/2001/XMLSchema#integer">18</EmpowerBP:minimumUserAge>
        <EmpowerBP:provideJournal rdf:datatype="http://www.w3.org/2001/XMLSchema#boolean">false</EmpowerBP:provideJournal>
        <EmpowerBP:provideLink rdf:datatype="http://www.w3.org/2001/XMLSchema#boolean">false</EmpowerBP:provideLink>
        <EmpowerBP:sourceURL rdf:datatype="http://www.w3.org/2001/XMLSchema#string">https://www.diabetes.ca/diabetes-and-you/healthy-living-resources/diet-nutrition/reducing-salt-intake</EmpowerBP:sourceURL>
        <rdfs:comment rdf:datatype="http://www.w3.org/2001/XMLSchema#string">Lower sodium foods (choose more of): 

• Whole grains and higher fibre foods such as breads, pasta, cereals, bulk hot cereals
• Grains with no added salt such as unsalted crackers homemade muffins, pancakes, corn breads (made from scratch)
• Homemade soups (can be frozen for later use), or soups that are low sodium or have no added salt

Higher sodium foods (choose less of): 

•   Packaged foods with added salt such as crackers, croutons, seasoned pasta and rice dishes, stuffing, instant hot cereals, instant pancake/waffle mixes
• Canned products such as corn, soups
• Prepared convenience foods such as frozen pizzas, frozen dinners</rdfs:comment>
        <rdfs:label rdf:datatype="http://www.w3.org/2001/XMLSchema#string">Sodium - Grains and starches</rdfs:label>
    </owl:NamedIndividual>
    


    <!-- http://www.semanticweb.org/tswheeler/ontologies/2016/3/EmpowerBP#T47 -->

    <owl:NamedIndividual rdf:about="http://www.semanticweb.org/tswheeler/ontologies/2016/3/EmpowerBP#T47">
        <rdf:type rdf:resource="http://www.semanticweb.org/tswheeler/ontologies/2016/3/EmpowerBP#InterventionItem"/>
        <rdf:type rdf:resource="http://www.semanticweb.org/tswheeler/ontologies/2016/3/EmpowerBP#Tip"/>
        <EmpowerBP:isAppropriateForInterventionGoal rdf:resource="http://www.semanticweb.org/tswheeler/ontologies/2016/3/EmpowerBP#ReduceSaltIntake"/>
        <EmpowerBP:isWarrantedBy rdf:resource="http://purl.bioontology.org/ontology/BCTT#Behavior_substitution"/>
        <EmpowerBP:appropriateForAutomaticMotivation rdf:datatype="http://www.w3.org/2001/XMLSchema#integer">6</EmpowerBP:appropriateForAutomaticMotivation>
        <EmpowerBP:appropriateForLocation rdf:datatype="http://www.w3.org/2001/XMLSchema#integer">0</EmpowerBP:appropriateForLocation>
        <EmpowerBP:appropriateForPhysicalCapability rdf:datatype="http://www.w3.org/2001/XMLSchema#integer">3</EmpowerBP:appropriateForPhysicalCapability>
        <EmpowerBP:appropriateForPhysicalOpportunity rdf:datatype="http://www.w3.org/2001/XMLSchema#integer">3</EmpowerBP:appropriateForPhysicalOpportunity>
        <EmpowerBP:appropriateForPsychologicalCapability rdf:datatype="http://www.w3.org/2001/XMLSchema#integer">3</EmpowerBP:appropriateForPsychologicalCapability>
        <EmpowerBP:appropriateForReflectiveMotivation rdf:datatype="http://www.w3.org/2001/XMLSchema#integer">6</EmpowerBP:appropriateForReflectiveMotivation>
        <EmpowerBP:appropriateForSocialOpportunity rdf:datatype="http://www.w3.org/2001/XMLSchema#integer">3</EmpowerBP:appropriateForSocialOpportunity>
        <EmpowerBP:canRepeat rdf:datatype="http://www.w3.org/2001/XMLSchema#integer">26</EmpowerBP:canRepeat>
        <EmpowerBP:itemName rdf:datatype="http://www.w3.org/2001/XMLSchema#string">Sodium Sense - Fruits</EmpowerBP:itemName>
        <EmpowerBP:itemText rdf:datatype="http://www.w3.org/2001/XMLSchema#string">Lower sodium foods (choose more of): 

• Fresh or frozen fruits
• Fruits with their skin

Higher sodium foods (choose less of): 

• Dried fruits processed with salt</EmpowerBP:itemText>
        <EmpowerBP:maximumUserAge rdf:datatype="http://www.w3.org/2001/XMLSchema#integer">120</EmpowerBP:maximumUserAge>
        <EmpowerBP:minimumUserAge rdf:datatype="http://www.w3.org/2001/XMLSchema#integer">18</EmpowerBP:minimumUserAge>
        <EmpowerBP:provideJournal rdf:datatype="http://www.w3.org/2001/XMLSchema#boolean">false</EmpowerBP:provideJournal>
        <EmpowerBP:provideLink rdf:datatype="http://www.w3.org/2001/XMLSchema#boolean">false</EmpowerBP:provideLink>
        <EmpowerBP:sourceURL rdf:datatype="http://www.w3.org/2001/XMLSchema#string">https://www.diabetes.ca/diabetes-and-you/healthy-living-resources/diet-nutrition/reducing-salt-intake</EmpowerBP:sourceURL>
        <rdfs:comment rdf:datatype="http://www.w3.org/2001/XMLSchema#string">Lower sodium foods (choose more of): 

• Fresh or frozen fruits
• Fruits with their skin

Higher sodium foods (choose less of): 

• Dried fruits processed with salt</rdfs:comment>
        <rdfs:label rdf:datatype="http://www.w3.org/2001/XMLSchema#string">Sodium Sense - Fruits</rdfs:label>
    </owl:NamedIndividual>
    


    <!-- http://www.semanticweb.org/tswheeler/ontologies/2016/3/EmpowerBP#T48 -->

    <owl:NamedIndividual rdf:about="http://www.semanticweb.org/tswheeler/ontologies/2016/3/EmpowerBP#T48">
        <rdf:type rdf:resource="http://www.semanticweb.org/tswheeler/ontologies/2016/3/EmpowerBP#InterventionItem"/>
        <rdf:type rdf:resource="http://www.semanticweb.org/tswheeler/ontologies/2016/3/EmpowerBP#Tip"/>
        <EmpowerBP:isAppropriateForInterventionGoal rdf:resource="http://www.semanticweb.org/tswheeler/ontologies/2016/3/EmpowerBP#ReduceSaltIntake"/>
        <EmpowerBP:isWarrantedBy rdf:resource="http://purl.bioontology.org/ontology/BCTT#Behavior_substitution"/>
        <EmpowerBP:appropriateForAutomaticMotivation rdf:datatype="http://www.w3.org/2001/XMLSchema#integer">6</EmpowerBP:appropriateForAutomaticMotivation>
        <EmpowerBP:appropriateForLocation rdf:datatype="http://www.w3.org/2001/XMLSchema#integer">0</EmpowerBP:appropriateForLocation>
        <EmpowerBP:appropriateForPhysicalCapability rdf:datatype="http://www.w3.org/2001/XMLSchema#integer">3</EmpowerBP:appropriateForPhysicalCapability>
        <EmpowerBP:appropriateForPhysicalOpportunity rdf:datatype="http://www.w3.org/2001/XMLSchema#integer">3</EmpowerBP:appropriateForPhysicalOpportunity>
        <EmpowerBP:appropriateForPsychologicalCapability rdf:datatype="http://www.w3.org/2001/XMLSchema#integer">3</EmpowerBP:appropriateForPsychologicalCapability>
        <EmpowerBP:appropriateForReflectiveMotivation rdf:datatype="http://www.w3.org/2001/XMLSchema#integer">6</EmpowerBP:appropriateForReflectiveMotivation>
        <EmpowerBP:appropriateForSocialOpportunity rdf:datatype="http://www.w3.org/2001/XMLSchema#integer">3</EmpowerBP:appropriateForSocialOpportunity>
        <EmpowerBP:canRepeat rdf:datatype="http://www.w3.org/2001/XMLSchema#integer">26</EmpowerBP:canRepeat>
        <EmpowerBP:itemName rdf:datatype="http://www.w3.org/2001/XMLSchema#string">Sodium Sense - Milk and Alternatives</EmpowerBP:itemName>
        <EmpowerBP:itemText rdf:datatype="http://www.w3.org/2001/XMLSchema#string">Lower sodium foods (choose more of): 

• Low fat dairy products such as skim or 1% milk and yogurt or soy milk
• Buttermilk limited to less than 1 cup per week

Higher sodium foods (choose less of): 

•  Malted milk, milkshakes
•  Some chocolate-flavoured mixes
• Canned milk</EmpowerBP:itemText>
        <EmpowerBP:maximumUserAge rdf:datatype="http://www.w3.org/2001/XMLSchema#integer">120</EmpowerBP:maximumUserAge>
        <EmpowerBP:minimumUserAge rdf:datatype="http://www.w3.org/2001/XMLSchema#integer">18</EmpowerBP:minimumUserAge>
        <EmpowerBP:provideJournal rdf:datatype="http://www.w3.org/2001/XMLSchema#boolean">false</EmpowerBP:provideJournal>
        <EmpowerBP:provideLink rdf:datatype="http://www.w3.org/2001/XMLSchema#boolean">false</EmpowerBP:provideLink>
        <EmpowerBP:sourceURL rdf:datatype="http://www.w3.org/2001/XMLSchema#string">https://www.diabetes.ca/diabetes-and-you/healthy-living-resources/diet-nutrition/reducing-salt-intake</EmpowerBP:sourceURL>
        <rdfs:comment rdf:datatype="http://www.w3.org/2001/XMLSchema#string">Lower sodium foods (choose more of): 

• Low fat dairy products such as skim or 1% milk and yogurt or soy milk
• Buttermilk limited to less than 1 cup per week

Higher sodium foods (choose less of): 

•  Malted milk, milkshakes
•  Some chocolate-flavoured mixes
• Canned milk</rdfs:comment>
        <rdfs:label rdf:datatype="http://www.w3.org/2001/XMLSchema#string">Sodium Sense - Milk and Alternatives</rdfs:label>
    </owl:NamedIndividual>
    


    <!-- http://www.semanticweb.org/tswheeler/ontologies/2016/3/EmpowerBP#T49 -->

    <owl:NamedIndividual rdf:about="http://www.semanticweb.org/tswheeler/ontologies/2016/3/EmpowerBP#T49">
        <rdf:type rdf:resource="http://www.semanticweb.org/tswheeler/ontologies/2016/3/EmpowerBP#InterventionItem"/>
        <rdf:type rdf:resource="http://www.semanticweb.org/tswheeler/ontologies/2016/3/EmpowerBP#Tip"/>
        <EmpowerBP:isAppropriateForInterventionGoal rdf:resource="http://www.semanticweb.org/tswheeler/ontologies/2016/3/EmpowerBP#ReduceSaltIntake"/>
        <EmpowerBP:isWarrantedBy rdf:resource="http://purl.bioontology.org/ontology/BCTT#Behavior_substitution"/>
        <EmpowerBP:appropriateForAutomaticMotivation rdf:datatype="http://www.w3.org/2001/XMLSchema#integer">6</EmpowerBP:appropriateForAutomaticMotivation>
        <EmpowerBP:appropriateForLocation rdf:datatype="http://www.w3.org/2001/XMLSchema#integer">0</EmpowerBP:appropriateForLocation>
        <EmpowerBP:appropriateForPhysicalCapability rdf:datatype="http://www.w3.org/2001/XMLSchema#integer">3</EmpowerBP:appropriateForPhysicalCapability>
        <EmpowerBP:appropriateForPhysicalOpportunity rdf:datatype="http://www.w3.org/2001/XMLSchema#integer">3</EmpowerBP:appropriateForPhysicalOpportunity>
        <EmpowerBP:appropriateForPsychologicalCapability rdf:datatype="http://www.w3.org/2001/XMLSchema#integer">3</EmpowerBP:appropriateForPsychologicalCapability>
        <EmpowerBP:appropriateForReflectiveMotivation rdf:datatype="http://www.w3.org/2001/XMLSchema#integer">6</EmpowerBP:appropriateForReflectiveMotivation>
        <EmpowerBP:appropriateForSocialOpportunity rdf:datatype="http://www.w3.org/2001/XMLSchema#integer">3</EmpowerBP:appropriateForSocialOpportunity>
        <EmpowerBP:canRepeat rdf:datatype="http://www.w3.org/2001/XMLSchema#integer">26</EmpowerBP:canRepeat>
        <EmpowerBP:itemName rdf:datatype="http://www.w3.org/2001/XMLSchema#string">Sodium Sense - Sweet Foods and Snacks</EmpowerBP:itemName>
        <EmpowerBP:itemText rdf:datatype="http://www.w3.org/2001/XMLSchema#string">Lower sodium foods (choose more of): 

• Unsalted snack foods like popcorn and chips
• Homemade baked goods (made from scratch)

Higher sodium foods (choose less of): 

• Snack foods like chips and popcorn
• Packaged pudding, cake, pie mixes
</EmpowerBP:itemText>
        <EmpowerBP:maximumUserAge rdf:datatype="http://www.w3.org/2001/XMLSchema#integer">120</EmpowerBP:maximumUserAge>
        <EmpowerBP:minimumUserAge rdf:datatype="http://www.w3.org/2001/XMLSchema#integer">18</EmpowerBP:minimumUserAge>
        <EmpowerBP:provideJournal rdf:datatype="http://www.w3.org/2001/XMLSchema#boolean">false</EmpowerBP:provideJournal>
        <EmpowerBP:provideLink rdf:datatype="http://www.w3.org/2001/XMLSchema#boolean">false</EmpowerBP:provideLink>
        <EmpowerBP:sourceURL rdf:datatype="http://www.w3.org/2001/XMLSchema#string">https://www.diabetes.ca/diabetes-and-you/healthy-living-resources/diet-nutrition/reducing-salt-intake</EmpowerBP:sourceURL>
        <rdfs:comment rdf:datatype="http://www.w3.org/2001/XMLSchema#string">Lower sodium foods (choose more of): 

• Unsalted snack foods like popcorn and chips
• Homemade baked goods (made from scratch)

Higher sodium foods (choose less of): 

• Snack foods like chips and popcorn
• Packaged pudding, cake, pie mixes
</rdfs:comment>
        <rdfs:label rdf:datatype="http://www.w3.org/2001/XMLSchema#string">Sodium Sense - Sweet Foods and Snacks</rdfs:label>
    </owl:NamedIndividual>
    


    <!-- http://www.semanticweb.org/tswheeler/ontologies/2016/3/EmpowerBP#T5 -->

    <owl:NamedIndividual rdf:about="http://www.semanticweb.org/tswheeler/ontologies/2016/3/EmpowerBP#T5">
        <rdf:type rdf:resource="http://www.semanticweb.org/tswheeler/ontologies/2016/3/EmpowerBP#InterventionItem"/>
        <rdf:type rdf:resource="http://www.semanticweb.org/tswheeler/ontologies/2016/3/EmpowerBP#Tip"/>
        <EmpowerBP:isAppropriateForInterventionGoal rdf:resource="http://www.semanticweb.org/tswheeler/ontologies/2016/3/EmpowerBP#ExerciseMore"/>
        <EmpowerBP:isWarrantedBy rdf:resource="http://purl.bioontology.org/ontology/BCTT#Instruction_on_how_to_perform_the_behavior"/>
        <EmpowerBP:appropriateForAutomaticMotivation rdf:datatype="http://www.w3.org/2001/XMLSchema#integer">6</EmpowerBP:appropriateForAutomaticMotivation>
        <EmpowerBP:appropriateForLocation rdf:datatype="http://www.w3.org/2001/XMLSchema#integer">0</EmpowerBP:appropriateForLocation>
        <EmpowerBP:appropriateForPhysicalCapability rdf:datatype="http://www.w3.org/2001/XMLSchema#integer">3</EmpowerBP:appropriateForPhysicalCapability>
        <EmpowerBP:appropriateForPhysicalOpportunity rdf:datatype="http://www.w3.org/2001/XMLSchema#integer">3</EmpowerBP:appropriateForPhysicalOpportunity>
        <EmpowerBP:appropriateForPsychologicalCapability rdf:datatype="http://www.w3.org/2001/XMLSchema#integer">3</EmpowerBP:appropriateForPsychologicalCapability>
        <EmpowerBP:appropriateForReflectiveMotivation rdf:datatype="http://www.w3.org/2001/XMLSchema#integer">6</EmpowerBP:appropriateForReflectiveMotivation>
        <EmpowerBP:appropriateForSocialOpportunity rdf:datatype="http://www.w3.org/2001/XMLSchema#integer">3</EmpowerBP:appropriateForSocialOpportunity>
        <EmpowerBP:canRepeat rdf:datatype="http://www.w3.org/2001/XMLSchema#integer">26</EmpowerBP:canRepeat>
        <EmpowerBP:itemName rdf:datatype="http://www.w3.org/2001/XMLSchema#string">Let&apos;s Talk Intensity!</EmpowerBP:itemName>
        <EmpowerBP:itemText rdf:datatype="http://www.w3.org/2001/XMLSchema#string">Moderate-intensity physical activities will cause adults to sweat a little and to breathe harder. Activities like:
• Walking quickly
• Skating
• Bike riding
Vigorous-intensity physical activities will cause adults to sweat and be ‘out of breath’. Activities like:
• Jogging
• Cross-country skiing
• Basketball
• Soccer</EmpowerBP:itemText>
        <EmpowerBP:maximumUserAge rdf:datatype="http://www.w3.org/2001/XMLSchema#integer">64</EmpowerBP:maximumUserAge>
        <EmpowerBP:minimumUserAge rdf:datatype="http://www.w3.org/2001/XMLSchema#integer">18</EmpowerBP:minimumUserAge>
        <EmpowerBP:provideJournal rdf:datatype="http://www.w3.org/2001/XMLSchema#boolean">false</EmpowerBP:provideJournal>
        <EmpowerBP:provideLink rdf:datatype="http://www.w3.org/2001/XMLSchema#boolean">false</EmpowerBP:provideLink>
        <EmpowerBP:sourceURL rdf:datatype="http://www.w3.org/2001/XMLSchema#string">http://www.csep.ca/cmfiles/guidelines/csep_guidelines_handbook.pdf</EmpowerBP:sourceURL>
        <rdfs:comment rdf:datatype="http://www.w3.org/2001/XMLSchema#string">Moderate-intensity physical activities will cause adults to sweat a little and to breathe harder. Activities like:
• Walking quickly
• Skating
• Bike riding
Vigorous-intensity physical activities will cause adults to sweat and be ‘out of breath’. Activities like:
• Jogging
• Cross-country skiing
• Basketball
• Soccer</rdfs:comment>
        <rdfs:label rdf:datatype="http://www.w3.org/2001/XMLSchema#string">Let&apos;s Talk Intensity!</rdfs:label>
    </owl:NamedIndividual>
    


    <!-- http://www.semanticweb.org/tswheeler/ontologies/2016/3/EmpowerBP#T50 -->

    <owl:NamedIndividual rdf:about="http://www.semanticweb.org/tswheeler/ontologies/2016/3/EmpowerBP#T50">
        <rdf:type rdf:resource="http://www.semanticweb.org/tswheeler/ontologies/2016/3/EmpowerBP#InterventionItem"/>
        <rdf:type rdf:resource="http://www.semanticweb.org/tswheeler/ontologies/2016/3/EmpowerBP#Tip"/>
        <EmpowerBP:isAppropriateForInterventionGoal rdf:resource="http://www.semanticweb.org/tswheeler/ontologies/2016/3/EmpowerBP#ReduceSaltIntake"/>
        <EmpowerBP:isWarrantedBy rdf:resource="http://purl.bioontology.org/ontology/BCTT#Behavior_substitution"/>
        <EmpowerBP:appropriateForAutomaticMotivation rdf:datatype="http://www.w3.org/2001/XMLSchema#integer">6</EmpowerBP:appropriateForAutomaticMotivation>
        <EmpowerBP:appropriateForLocation rdf:datatype="http://www.w3.org/2001/XMLSchema#integer">0</EmpowerBP:appropriateForLocation>
        <EmpowerBP:appropriateForPhysicalCapability rdf:datatype="http://www.w3.org/2001/XMLSchema#integer">3</EmpowerBP:appropriateForPhysicalCapability>
        <EmpowerBP:appropriateForPhysicalOpportunity rdf:datatype="http://www.w3.org/2001/XMLSchema#integer">3</EmpowerBP:appropriateForPhysicalOpportunity>
        <EmpowerBP:appropriateForPsychologicalCapability rdf:datatype="http://www.w3.org/2001/XMLSchema#integer">3</EmpowerBP:appropriateForPsychologicalCapability>
        <EmpowerBP:appropriateForReflectiveMotivation rdf:datatype="http://www.w3.org/2001/XMLSchema#integer">6</EmpowerBP:appropriateForReflectiveMotivation>
        <EmpowerBP:appropriateForSocialOpportunity rdf:datatype="http://www.w3.org/2001/XMLSchema#integer">3</EmpowerBP:appropriateForSocialOpportunity>
        <EmpowerBP:canRepeat rdf:datatype="http://www.w3.org/2001/XMLSchema#integer">26</EmpowerBP:canRepeat>
        <EmpowerBP:itemName rdf:datatype="http://www.w3.org/2001/XMLSchema#string">Sodium Sense - Vegetables</EmpowerBP:itemName>
        <EmpowerBP:itemText rdf:datatype="http://www.w3.org/2001/XMLSchema#string">Lower sodium foods (choose more of): 

• Fresh or frozen vegetables with no sauces
• Low sodium canned vegetables or canned vegetables rinsed with water


Higher sodium foods (choose less of): 

• Canned vegetables
• Sauerkraut, pickled vegetables
• Regular vegetable or tomato juices
• Frozen vegetables with sauces
• Canned tomatoes
</EmpowerBP:itemText>
        <EmpowerBP:maximumUserAge rdf:datatype="http://www.w3.org/2001/XMLSchema#integer">120</EmpowerBP:maximumUserAge>
        <EmpowerBP:minimumUserAge rdf:datatype="http://www.w3.org/2001/XMLSchema#integer">18</EmpowerBP:minimumUserAge>
        <EmpowerBP:provideJournal rdf:datatype="http://www.w3.org/2001/XMLSchema#boolean">false</EmpowerBP:provideJournal>
        <EmpowerBP:provideLink rdf:datatype="http://www.w3.org/2001/XMLSchema#boolean">false</EmpowerBP:provideLink>
        <EmpowerBP:sourceURL rdf:datatype="http://www.w3.org/2001/XMLSchema#string">https://www.diabetes.ca/diabetes-and-you/healthy-living-resources/diet-nutrition/reducing-salt-intake</EmpowerBP:sourceURL>
        <rdfs:comment rdf:datatype="http://www.w3.org/2001/XMLSchema#string">Lower sodium foods (choose more of): 

• Fresh or frozen vegetables with no sauces
• Low sodium canned vegetables or canned vegetables rinsed with water


Higher sodium foods (choose less of): 

• Canned vegetables
• Sauerkraut, pickled vegetables
• Regular vegetable or tomato juices
• Frozen vegetables with sauces
• Canned tomatoes
</rdfs:comment>
        <rdfs:label rdf:datatype="http://www.w3.org/2001/XMLSchema#string">Sodium Sense - Vegetables</rdfs:label>
    </owl:NamedIndividual>
    


    <!-- http://www.semanticweb.org/tswheeler/ontologies/2016/3/EmpowerBP#T51 -->

    <owl:NamedIndividual rdf:about="http://www.semanticweb.org/tswheeler/ontologies/2016/3/EmpowerBP#T51">
        <rdf:type rdf:resource="http://www.semanticweb.org/tswheeler/ontologies/2016/3/EmpowerBP#InterventionItem"/>
        <rdf:type rdf:resource="http://www.semanticweb.org/tswheeler/ontologies/2016/3/EmpowerBP#Tip"/>
        <EmpowerBP:isAppropriateForInterventionGoal rdf:resource="http://www.semanticweb.org/tswheeler/ontologies/2016/3/EmpowerBP#ReduceSaltIntake"/>
        <EmpowerBP:isWarrantedBy rdf:resource="http://purl.bioontology.org/ontology/BCTT#Behavior_substitution"/>
        <EmpowerBP:appropriateForAutomaticMotivation rdf:datatype="http://www.w3.org/2001/XMLSchema#integer">6</EmpowerBP:appropriateForAutomaticMotivation>
        <EmpowerBP:appropriateForLocation rdf:datatype="http://www.w3.org/2001/XMLSchema#integer">0</EmpowerBP:appropriateForLocation>
        <EmpowerBP:appropriateForPhysicalCapability rdf:datatype="http://www.w3.org/2001/XMLSchema#integer">3</EmpowerBP:appropriateForPhysicalCapability>
        <EmpowerBP:appropriateForPhysicalOpportunity rdf:datatype="http://www.w3.org/2001/XMLSchema#integer">3</EmpowerBP:appropriateForPhysicalOpportunity>
        <EmpowerBP:appropriateForPsychologicalCapability rdf:datatype="http://www.w3.org/2001/XMLSchema#integer">3</EmpowerBP:appropriateForPsychologicalCapability>
        <EmpowerBP:appropriateForReflectiveMotivation rdf:datatype="http://www.w3.org/2001/XMLSchema#integer">6</EmpowerBP:appropriateForReflectiveMotivation>
        <EmpowerBP:appropriateForSocialOpportunity rdf:datatype="http://www.w3.org/2001/XMLSchema#integer">3</EmpowerBP:appropriateForSocialOpportunity>
        <EmpowerBP:canRepeat rdf:datatype="http://www.w3.org/2001/XMLSchema#integer">26</EmpowerBP:canRepeat>
        <EmpowerBP:itemName rdf:datatype="http://www.w3.org/2001/XMLSchema#string">Sodium Sense - Meat and Alternatives</EmpowerBP:itemName>
        <EmpowerBP:itemText rdf:datatype="http://www.w3.org/2001/XMLSchema#string">Lower sodium foods (choose more of): 

• Fresh or frozen lean meats and poultry
• Fresh fish or low sodium canned fish at least once a week. Rinse regular canned fish with water to flush the sodium away.
• Dried beans, peas and lentils or canned beans rinsed with water
• Low sodium cheeses such as ricotta, cottage cheese. These are also available as low sodium and low fat.
• Unsalted nuts. Use herbs/spices to flavour nuts &amp; seeds

Higher sodium foods (choose less of): 

• Smoked, cured, canned, koshered meats
• Processed meats like hotdogs, cold cuts, ham, sausage
• Imitation seafood
• Processed cheeses such as cheese slices, cheese sauces and spreads
• Salted nuts and seeds
• Canned beans and lentils
• Pickled eggs</EmpowerBP:itemText>
        <EmpowerBP:maximumUserAge rdf:datatype="http://www.w3.org/2001/XMLSchema#integer">120</EmpowerBP:maximumUserAge>
        <EmpowerBP:minimumUserAge rdf:datatype="http://www.w3.org/2001/XMLSchema#integer">18</EmpowerBP:minimumUserAge>
        <EmpowerBP:provideJournal rdf:datatype="http://www.w3.org/2001/XMLSchema#boolean">false</EmpowerBP:provideJournal>
        <EmpowerBP:provideLink rdf:datatype="http://www.w3.org/2001/XMLSchema#boolean">false</EmpowerBP:provideLink>
        <EmpowerBP:sourceURL rdf:datatype="http://www.w3.org/2001/XMLSchema#string">https://www.diabetes.ca/diabetes-and-you/healthy-living-resources/diet-nutrition/reducing-salt-intake</EmpowerBP:sourceURL>
        <rdfs:comment rdf:datatype="http://www.w3.org/2001/XMLSchema#string">Lower sodium foods (choose more of): 

• Fresh or frozen lean meats and poultry
• Fresh fish or low sodium canned fish at least once a week. Rinse regular canned fish with water to flush the sodium away.
• Dried beans, peas and lentils or canned beans rinsed with water
• Low sodium cheeses such as ricotta, cottage cheese. These are also available as low sodium and low fat.
• Unsalted nuts. Use herbs/spices to flavour nuts &amp; seeds

Higher sodium foods (choose less of): 

• Smoked, cured, canned, koshered meats
• Processed meats like hotdogs, cold cuts, ham, sausage
• Imitation seafood
• Processed cheeses such as cheese slices, cheese sauces and spreads
• Salted nuts and seeds
• Canned beans and lentils
• Pickled eggs</rdfs:comment>
        <rdfs:label rdf:datatype="http://www.w3.org/2001/XMLSchema#string">Sodium Sense - Meat and Alternatives</rdfs:label>
    </owl:NamedIndividual>
    


    <!-- http://www.semanticweb.org/tswheeler/ontologies/2016/3/EmpowerBP#T52 -->

    <owl:NamedIndividual rdf:about="http://www.semanticweb.org/tswheeler/ontologies/2016/3/EmpowerBP#T52">
        <rdf:type rdf:resource="http://www.semanticweb.org/tswheeler/ontologies/2016/3/EmpowerBP#InterventionItem"/>
        <rdf:type rdf:resource="http://www.semanticweb.org/tswheeler/ontologies/2016/3/EmpowerBP#Tip"/>
        <EmpowerBP:isAppropriateForInterventionGoal rdf:resource="http://www.semanticweb.org/tswheeler/ontologies/2016/3/EmpowerBP#ReduceSaltIntake"/>
        <EmpowerBP:isWarrantedBy rdf:resource="http://purl.bioontology.org/ontology/BCTT#Behavior_substitution"/>
        <EmpowerBP:appropriateForAutomaticMotivation rdf:datatype="http://www.w3.org/2001/XMLSchema#integer">6</EmpowerBP:appropriateForAutomaticMotivation>
        <EmpowerBP:appropriateForLocation rdf:datatype="http://www.w3.org/2001/XMLSchema#integer">0</EmpowerBP:appropriateForLocation>
        <EmpowerBP:appropriateForPhysicalCapability rdf:datatype="http://www.w3.org/2001/XMLSchema#integer">3</EmpowerBP:appropriateForPhysicalCapability>
        <EmpowerBP:appropriateForPhysicalOpportunity rdf:datatype="http://www.w3.org/2001/XMLSchema#integer">3</EmpowerBP:appropriateForPhysicalOpportunity>
        <EmpowerBP:appropriateForPsychologicalCapability rdf:datatype="http://www.w3.org/2001/XMLSchema#integer">3</EmpowerBP:appropriateForPsychologicalCapability>
        <EmpowerBP:appropriateForReflectiveMotivation rdf:datatype="http://www.w3.org/2001/XMLSchema#integer">6</EmpowerBP:appropriateForReflectiveMotivation>
        <EmpowerBP:appropriateForSocialOpportunity rdf:datatype="http://www.w3.org/2001/XMLSchema#integer">3</EmpowerBP:appropriateForSocialOpportunity>
        <EmpowerBP:canRepeat rdf:datatype="http://www.w3.org/2001/XMLSchema#integer">26</EmpowerBP:canRepeat>
        <EmpowerBP:itemName rdf:datatype="http://www.w3.org/2001/XMLSchema#string">Sodium Sense - Fats</EmpowerBP:itemName>
        <EmpowerBP:itemText rdf:datatype="http://www.w3.org/2001/XMLSchema#string">Lower sodium foods (choose more of): 

• Canola oil, olive oil, sunflower oil, vegetable oil for cooking
• Non-hydrogenated margarines without added salt
• Unsalted salad dressings or homemade dressings with oil, vinegar and herbs

Higher sodium foods (choose less of): 

• Dips made with soup mixes or processed cheese
• Some salad dressings
• Salted butter</EmpowerBP:itemText>
        <EmpowerBP:maximumUserAge rdf:datatype="http://www.w3.org/2001/XMLSchema#integer">120</EmpowerBP:maximumUserAge>
        <EmpowerBP:minimumUserAge rdf:datatype="http://www.w3.org/2001/XMLSchema#integer">18</EmpowerBP:minimumUserAge>
        <EmpowerBP:provideJournal rdf:datatype="http://www.w3.org/2001/XMLSchema#boolean">false</EmpowerBP:provideJournal>
        <EmpowerBP:provideLink rdf:datatype="http://www.w3.org/2001/XMLSchema#boolean">false</EmpowerBP:provideLink>
        <EmpowerBP:sourceURL rdf:datatype="http://www.w3.org/2001/XMLSchema#string">https://www.diabetes.ca/diabetes-and-you/healthy-living-resources/diet-nutrition/reducing-salt-intake</EmpowerBP:sourceURL>
        <rdfs:comment rdf:datatype="http://www.w3.org/2001/XMLSchema#string">Lower sodium foods (choose more of): 

• Canola oil, olive oil, sunflower oil, vegetable oil for cooking
• Non-hydrogenated margarines without added salt
• Unsalted salad dressings or homemade dressings with oil, vinegar and herbs

Higher sodium foods (choose less of): 

• Dips made with soup mixes or processed cheese
• Some salad dressings
• Salted butter</rdfs:comment>
        <rdfs:label rdf:datatype="http://www.w3.org/2001/XMLSchema#string">Sodium Sense - Fats</rdfs:label>
    </owl:NamedIndividual>
    


    <!-- http://www.semanticweb.org/tswheeler/ontologies/2016/3/EmpowerBP#T53 -->

    <owl:NamedIndividual rdf:about="http://www.semanticweb.org/tswheeler/ontologies/2016/3/EmpowerBP#T53">
        <rdf:type rdf:resource="http://www.semanticweb.org/tswheeler/ontologies/2016/3/EmpowerBP#InterventionItem"/>
        <rdf:type rdf:resource="http://www.semanticweb.org/tswheeler/ontologies/2016/3/EmpowerBP#Tip"/>
        <EmpowerBP:isAppropriateForInterventionGoal rdf:resource="http://www.semanticweb.org/tswheeler/ontologies/2016/3/EmpowerBP#ReduceSaltIntake"/>
        <EmpowerBP:isWarrantedBy rdf:resource="http://purl.bioontology.org/ontology/BCTT#Behavior_substitution"/>
        <EmpowerBP:appropriateForAutomaticMotivation rdf:datatype="http://www.w3.org/2001/XMLSchema#integer">6</EmpowerBP:appropriateForAutomaticMotivation>
        <EmpowerBP:appropriateForLocation rdf:datatype="http://www.w3.org/2001/XMLSchema#integer">0</EmpowerBP:appropriateForLocation>
        <EmpowerBP:appropriateForPhysicalCapability rdf:datatype="http://www.w3.org/2001/XMLSchema#integer">3</EmpowerBP:appropriateForPhysicalCapability>
        <EmpowerBP:appropriateForPhysicalOpportunity rdf:datatype="http://www.w3.org/2001/XMLSchema#integer">3</EmpowerBP:appropriateForPhysicalOpportunity>
        <EmpowerBP:appropriateForPsychologicalCapability rdf:datatype="http://www.w3.org/2001/XMLSchema#integer">3</EmpowerBP:appropriateForPsychologicalCapability>
        <EmpowerBP:appropriateForReflectiveMotivation rdf:datatype="http://www.w3.org/2001/XMLSchema#integer">6</EmpowerBP:appropriateForReflectiveMotivation>
        <EmpowerBP:appropriateForSocialOpportunity rdf:datatype="http://www.w3.org/2001/XMLSchema#integer">3</EmpowerBP:appropriateForSocialOpportunity>
        <EmpowerBP:canRepeat rdf:datatype="http://www.w3.org/2001/XMLSchema#integer">26</EmpowerBP:canRepeat>
        <EmpowerBP:itemName rdf:datatype="http://www.w3.org/2001/XMLSchema#string">Sodium Sense - Extras</EmpowerBP:itemName>
        <EmpowerBP:itemText rdf:datatype="http://www.w3.org/2001/XMLSchema#string">Lower sodium foods (choose more of): 

• Herbs, spices, lemon and vinegar in cooking to flavour your food
• Homemade herb shaker or use herb/spice blends available for purchase
• Low sodium condiments
• Garlic and onion powder

Higher sodium foods (choose less of): 

• Condiments such as ketchup, mustard, and relish
• Sauces such as soy sauce, Worcestershire sauce and barbecue sauce
• Pickles and olives
• Herbs that contain the word salt, such as garlic salt or celery salt
• Kosher salt and sea salt also contain sodium
• Monosodium Glutamate
• Softened water
• Foods described as being smoked, pickled, teriyaki or in broth</EmpowerBP:itemText>
        <EmpowerBP:maximumUserAge rdf:datatype="http://www.w3.org/2001/XMLSchema#integer">120</EmpowerBP:maximumUserAge>
        <EmpowerBP:minimumUserAge rdf:datatype="http://www.w3.org/2001/XMLSchema#integer">18</EmpowerBP:minimumUserAge>
        <EmpowerBP:provideJournal rdf:datatype="http://www.w3.org/2001/XMLSchema#boolean">false</EmpowerBP:provideJournal>
        <EmpowerBP:provideLink rdf:datatype="http://www.w3.org/2001/XMLSchema#boolean">false</EmpowerBP:provideLink>
        <EmpowerBP:sourceURL rdf:datatype="http://www.w3.org/2001/XMLSchema#string">https://www.diabetes.ca/diabetes-and-you/healthy-living-resources/diet-nutrition/reducing-salt-intake</EmpowerBP:sourceURL>
        <rdfs:comment rdf:datatype="http://www.w3.org/2001/XMLSchema#string">Lower sodium foods (choose more of): 

• Herbs, spices, lemon and vinegar in cooking to flavour your food
• Homemade herb shaker or use herb/spice blends available for purchase
• Low sodium condiments
• Garlic and onion powder

Higher sodium foods (choose less of): 

• Condiments such as ketchup, mustard, and relish
• Sauces such as soy sauce, Worcestershire sauce and barbecue sauce
• Pickles and olives
• Herbs that contain the word salt, such as garlic salt or celery salt
• Kosher salt and sea salt also contain sodium
• Monosodium Glutamate
• Softened water
• Foods described as being smoked, pickled, teriyaki or in broth</rdfs:comment>
        <rdfs:label rdf:datatype="http://www.w3.org/2001/XMLSchema#string">Sodium Sense - Extras</rdfs:label>
    </owl:NamedIndividual>
    


    <!-- http://www.semanticweb.org/tswheeler/ontologies/2016/3/EmpowerBP#T54 -->

    <owl:NamedIndividual rdf:about="http://www.semanticweb.org/tswheeler/ontologies/2016/3/EmpowerBP#T54">
        <rdf:type rdf:resource="http://www.semanticweb.org/tswheeler/ontologies/2016/3/EmpowerBP#InterventionItem"/>
        <rdf:type rdf:resource="http://www.semanticweb.org/tswheeler/ontologies/2016/3/EmpowerBP#Tip"/>
        <EmpowerBP:isAppropriateForInterventionGoal rdf:resource="http://www.semanticweb.org/tswheeler/ontologies/2016/3/EmpowerBP#ReduceSaltIntake"/>
        <EmpowerBP:isWarrantedBy rdf:resource="http://purl.bioontology.org/ontology/BCTT#Instruction_on_how_to_perform_the_behavior"/>
        <EmpowerBP:appropriateForAutomaticMotivation rdf:datatype="http://www.w3.org/2001/XMLSchema#integer">6</EmpowerBP:appropriateForAutomaticMotivation>
        <EmpowerBP:appropriateForLocation rdf:datatype="http://www.w3.org/2001/XMLSchema#integer">0</EmpowerBP:appropriateForLocation>
        <EmpowerBP:appropriateForPhysicalCapability rdf:datatype="http://www.w3.org/2001/XMLSchema#integer">3</EmpowerBP:appropriateForPhysicalCapability>
        <EmpowerBP:appropriateForPhysicalOpportunity rdf:datatype="http://www.w3.org/2001/XMLSchema#integer">3</EmpowerBP:appropriateForPhysicalOpportunity>
        <EmpowerBP:appropriateForPsychologicalCapability rdf:datatype="http://www.w3.org/2001/XMLSchema#integer">3</EmpowerBP:appropriateForPsychologicalCapability>
        <EmpowerBP:appropriateForReflectiveMotivation rdf:datatype="http://www.w3.org/2001/XMLSchema#integer">6</EmpowerBP:appropriateForReflectiveMotivation>
        <EmpowerBP:appropriateForSocialOpportunity rdf:datatype="http://www.w3.org/2001/XMLSchema#integer">3</EmpowerBP:appropriateForSocialOpportunity>
        <EmpowerBP:canRepeat rdf:datatype="http://www.w3.org/2001/XMLSchema#integer">26</EmpowerBP:canRepeat>
        <EmpowerBP:itemName rdf:datatype="http://www.w3.org/2001/XMLSchema#string">Add Zip Without Salt!</EmpowerBP:itemName>
        <EmpowerBP:itemText rdf:datatype="http://www.w3.org/2001/XMLSchema#string">Any of the spices in your cupboards can add new flavour to your meals. Here are some ideas to get you started:

• Beef: Bay leaf, chives, parsley, dry mustard powder, marjoram, thyme, oregano, pepper, garlic, onion, fresh mushrooms, sage

• Poultry: Green pepper, fresh mushrooms, parsley, chives, poultry seasoning, lemon juice, paprika, sage, thyme, pepper

• Pork: Applesauce, garlic, onion, pepper, cloves, dill, parsley, pepper, sage

• Fish: Lemon juice, bay leaf, garlic, dill, parsley, pepper, fresh mushrooms, paprika, curry powder

• Vegetables:  Lemon juice, marjoram, dill, parsley, onion, chives, pepper, garlic, vinegar

• Salads:  Dry mustard mixed with vinegar and sugar, lemon juice, chives, parsley, garlic, onion, pepper, oregano

• Soups:  Chives, onion, garlic, chili powder, oregano, thyme, bay leaf, parsley</EmpowerBP:itemText>
        <EmpowerBP:maximumUserAge rdf:datatype="http://www.w3.org/2001/XMLSchema#integer">120</EmpowerBP:maximumUserAge>
        <EmpowerBP:minimumUserAge rdf:datatype="http://www.w3.org/2001/XMLSchema#integer">18</EmpowerBP:minimumUserAge>
        <EmpowerBP:provideJournal rdf:datatype="http://www.w3.org/2001/XMLSchema#boolean">false</EmpowerBP:provideJournal>
        <EmpowerBP:provideLink rdf:datatype="http://www.w3.org/2001/XMLSchema#boolean">false</EmpowerBP:provideLink>
        <EmpowerBP:sourceURL rdf:datatype="http://www.w3.org/2001/XMLSchema#string">https://www.diabetes.ca/diabetes-and-you/healthy-living-resources/diet-nutrition/reducing-salt-intake</EmpowerBP:sourceURL>
        <rdfs:comment rdf:datatype="http://www.w3.org/2001/XMLSchema#string">Any of the spices in your cupboards can add new flavour to your meals. Here are some ideas to get you started:

• Beef: Bay leaf, chives, parsley, dry mustard powder, marjoram, thyme, oregano, pepper, garlic, onion, fresh mushrooms, sage

• Poultry: Green pepper, fresh mushrooms, parsley, chives, poultry seasoning, lemon juice, paprika, sage, thyme, pepper

• Pork: Applesauce, garlic, onion, pepper, cloves, dill, parsley, pepper, sage

• Fish: Lemon juice, bay leaf, garlic, dill, parsley, pepper, fresh mushrooms, paprika, curry powder

• Vegetables:  Lemon juice, marjoram, dill, parsley, onion, chives, pepper, garlic, vinegar

• Salads:  Dry mustard mixed with vinegar and sugar, lemon juice, chives, parsley, garlic, onion, pepper, oregano

• Soups:  Chives, onion, garlic, chili powder, oregano, thyme, bay leaf, parsley</rdfs:comment>
        <rdfs:label rdf:datatype="http://www.w3.org/2001/XMLSchema#string">Add Zip Without Salt!</rdfs:label>
    </owl:NamedIndividual>
    


    <!-- http://www.semanticweb.org/tswheeler/ontologies/2016/3/EmpowerBP#T55 -->

    <owl:NamedIndividual rdf:about="http://www.semanticweb.org/tswheeler/ontologies/2016/3/EmpowerBP#T55">
        <rdf:type rdf:resource="http://www.semanticweb.org/tswheeler/ontologies/2016/3/EmpowerBP#InterventionItem"/>
        <rdf:type rdf:resource="http://www.semanticweb.org/tswheeler/ontologies/2016/3/EmpowerBP#Tip"/>
        <EmpowerBP:isAppropriateForInterventionGoal rdf:resource="http://www.semanticweb.org/tswheeler/ontologies/2016/3/EmpowerBP#ReduceSaltIntake"/>
        <EmpowerBP:isWarrantedBy rdf:resource="http://purl.bioontology.org/ontology/BCTT#Instruction_on_how_to_perform_the_behavior"/>
        <EmpowerBP:appropriateForAutomaticMotivation rdf:datatype="http://www.w3.org/2001/XMLSchema#integer">6</EmpowerBP:appropriateForAutomaticMotivation>
        <EmpowerBP:appropriateForLocation rdf:datatype="http://www.w3.org/2001/XMLSchema#integer">0</EmpowerBP:appropriateForLocation>
        <EmpowerBP:appropriateForPhysicalCapability rdf:datatype="http://www.w3.org/2001/XMLSchema#integer">3</EmpowerBP:appropriateForPhysicalCapability>
        <EmpowerBP:appropriateForPhysicalOpportunity rdf:datatype="http://www.w3.org/2001/XMLSchema#integer">3</EmpowerBP:appropriateForPhysicalOpportunity>
        <EmpowerBP:appropriateForPsychologicalCapability rdf:datatype="http://www.w3.org/2001/XMLSchema#integer">3</EmpowerBP:appropriateForPsychologicalCapability>
        <EmpowerBP:appropriateForReflectiveMotivation rdf:datatype="http://www.w3.org/2001/XMLSchema#integer">6</EmpowerBP:appropriateForReflectiveMotivation>
        <EmpowerBP:appropriateForSocialOpportunity rdf:datatype="http://www.w3.org/2001/XMLSchema#integer">3</EmpowerBP:appropriateForSocialOpportunity>
        <EmpowerBP:canRepeat rdf:datatype="http://www.w3.org/2001/XMLSchema#integer">26</EmpowerBP:canRepeat>
        <EmpowerBP:itemName rdf:datatype="http://www.w3.org/2001/XMLSchema#string">Limit Sodium Intake</EmpowerBP:itemName>
        <EmpowerBP:itemText rdf:datatype="http://www.w3.org/2001/XMLSchema#string">Buy products that are labeled with ≤ 5% daily value (%DV) of sodium

Too much: more than 360 mg or more than 15 %DV
Watch out: between 121 and 360 mg or between 6 and 14%DV
Go ahead: 0 to 120 mg or 0-5 %DV</EmpowerBP:itemText>
        <EmpowerBP:maximumUserAge rdf:datatype="http://www.w3.org/2001/XMLSchema#integer">120</EmpowerBP:maximumUserAge>
        <EmpowerBP:minimumUserAge rdf:datatype="http://www.w3.org/2001/XMLSchema#integer">18</EmpowerBP:minimumUserAge>
        <EmpowerBP:provideJournal rdf:datatype="http://www.w3.org/2001/XMLSchema#boolean">false</EmpowerBP:provideJournal>
        <EmpowerBP:provideLink rdf:datatype="http://www.w3.org/2001/XMLSchema#boolean">false</EmpowerBP:provideLink>
        <EmpowerBP:sourceURL rdf:datatype="http://www.w3.org/2001/XMLSchema#string">https://www.hypertension.ca/en/hypertension/what-can-i-do/limit-saltsodium-intake</EmpowerBP:sourceURL>
        <rdfs:comment rdf:datatype="http://www.w3.org/2001/XMLSchema#string">Buy products that are labeled with ≤ 5% daily value (%DV) of sodium

Too much: more than 360 mg or more than 15 %DV
Watch out: between 121 and 360 mg or between 6 and 14%DV
Go ahead: 0 to 120 mg or 0-5 %DV</rdfs:comment>
        <rdfs:label rdf:datatype="http://www.w3.org/2001/XMLSchema#string">Limit Sodium Intake</rdfs:label>
    </owl:NamedIndividual>
    


    <!-- http://www.semanticweb.org/tswheeler/ontologies/2016/3/EmpowerBP#T56 -->

    <owl:NamedIndividual rdf:about="http://www.semanticweb.org/tswheeler/ontologies/2016/3/EmpowerBP#T56">
        <rdf:type rdf:resource="http://www.semanticweb.org/tswheeler/ontologies/2016/3/EmpowerBP#InterventionItem"/>
        <rdf:type rdf:resource="http://www.semanticweb.org/tswheeler/ontologies/2016/3/EmpowerBP#Tip"/>
        <EmpowerBP:isAppropriateForInterventionGoal rdf:resource="http://www.semanticweb.org/tswheeler/ontologies/2016/3/EmpowerBP#ReduceSaltIntake"/>
        <EmpowerBP:isWarrantedBy rdf:resource="http://purl.bioontology.org/ontology/BCTT#Instruction_on_how_to_perform_the_behavior"/>
        <EmpowerBP:appropriateForAutomaticMotivation rdf:datatype="http://www.w3.org/2001/XMLSchema#integer">6</EmpowerBP:appropriateForAutomaticMotivation>
        <EmpowerBP:appropriateForLocation rdf:datatype="http://www.w3.org/2001/XMLSchema#integer">0</EmpowerBP:appropriateForLocation>
        <EmpowerBP:appropriateForPhysicalCapability rdf:datatype="http://www.w3.org/2001/XMLSchema#integer">3</EmpowerBP:appropriateForPhysicalCapability>
        <EmpowerBP:appropriateForPhysicalOpportunity rdf:datatype="http://www.w3.org/2001/XMLSchema#integer">3</EmpowerBP:appropriateForPhysicalOpportunity>
        <EmpowerBP:appropriateForPsychologicalCapability rdf:datatype="http://www.w3.org/2001/XMLSchema#integer">3</EmpowerBP:appropriateForPsychologicalCapability>
        <EmpowerBP:appropriateForReflectiveMotivation rdf:datatype="http://www.w3.org/2001/XMLSchema#integer">6</EmpowerBP:appropriateForReflectiveMotivation>
        <EmpowerBP:appropriateForSocialOpportunity rdf:datatype="http://www.w3.org/2001/XMLSchema#integer">3</EmpowerBP:appropriateForSocialOpportunity>
        <EmpowerBP:canRepeat rdf:datatype="http://www.w3.org/2001/XMLSchema#integer">26</EmpowerBP:canRepeat>
        <EmpowerBP:itemName rdf:datatype="http://www.w3.org/2001/XMLSchema#string">Sodium101 Health Claims</EmpowerBP:itemName>
        <EmpowerBP:itemText rdf:datatype="http://www.w3.org/2001/XMLSchema#string">Don’t be fooled by health claims marketing “Free”, “Lightly Salted”,“Healthy”, “Lower”, etc.

Get the facts - check the label!</EmpowerBP:itemText>
        <EmpowerBP:maximumUserAge rdf:datatype="http://www.w3.org/2001/XMLSchema#integer">120</EmpowerBP:maximumUserAge>
        <EmpowerBP:minimumUserAge rdf:datatype="http://www.w3.org/2001/XMLSchema#integer">18</EmpowerBP:minimumUserAge>
        <EmpowerBP:provideJournal rdf:datatype="http://www.w3.org/2001/XMLSchema#boolean">false</EmpowerBP:provideJournal>
        <EmpowerBP:provideLink rdf:datatype="http://www.w3.org/2001/XMLSchema#boolean">false</EmpowerBP:provideLink>
        <EmpowerBP:sourceURL rdf:datatype="http://www.w3.org/2001/XMLSchema#string">http://www.sodium101.ca/wp-content/uploads/2012/11/brochure-fullpage-en.pdf</EmpowerBP:sourceURL>
        <rdfs:comment rdf:datatype="http://www.w3.org/2001/XMLSchema#string">Don’t be fooled by health claims marketing “Free”, “Lightly Salted”,“Healthy”, “Lower”, etc.

Get the facts - check the label!</rdfs:comment>
        <rdfs:label rdf:datatype="http://www.w3.org/2001/XMLSchema#string">Sodium101 Health Claims</rdfs:label>
    </owl:NamedIndividual>
    


    <!-- http://www.semanticweb.org/tswheeler/ontologies/2016/3/EmpowerBP#T57 -->

    <owl:NamedIndividual rdf:about="http://www.semanticweb.org/tswheeler/ontologies/2016/3/EmpowerBP#T57">
        <rdf:type rdf:resource="http://www.semanticweb.org/tswheeler/ontologies/2016/3/EmpowerBP#InterventionItem"/>
        <rdf:type rdf:resource="http://www.semanticweb.org/tswheeler/ontologies/2016/3/EmpowerBP#Tip"/>
        <EmpowerBP:isAppropriateForInterventionGoal rdf:resource="http://www.semanticweb.org/tswheeler/ontologies/2016/3/EmpowerBP#ReduceSaltIntake"/>
        <EmpowerBP:isWarrantedBy rdf:resource="http://purl.bioontology.org/ontology/BCTT#Instruction_on_how_to_perform_the_behavior"/>
        <EmpowerBP:appropriateForAutomaticMotivation rdf:datatype="http://www.w3.org/2001/XMLSchema#integer">6</EmpowerBP:appropriateForAutomaticMotivation>
        <EmpowerBP:appropriateForLocation rdf:datatype="http://www.w3.org/2001/XMLSchema#integer">0</EmpowerBP:appropriateForLocation>
        <EmpowerBP:appropriateForPhysicalCapability rdf:datatype="http://www.w3.org/2001/XMLSchema#integer">3</EmpowerBP:appropriateForPhysicalCapability>
        <EmpowerBP:appropriateForPhysicalOpportunity rdf:datatype="http://www.w3.org/2001/XMLSchema#integer">3</EmpowerBP:appropriateForPhysicalOpportunity>
        <EmpowerBP:appropriateForPsychologicalCapability rdf:datatype="http://www.w3.org/2001/XMLSchema#integer">3</EmpowerBP:appropriateForPsychologicalCapability>
        <EmpowerBP:appropriateForReflectiveMotivation rdf:datatype="http://www.w3.org/2001/XMLSchema#integer">6</EmpowerBP:appropriateForReflectiveMotivation>
        <EmpowerBP:appropriateForSocialOpportunity rdf:datatype="http://www.w3.org/2001/XMLSchema#integer">3</EmpowerBP:appropriateForSocialOpportunity>
        <EmpowerBP:canRepeat rdf:datatype="http://www.w3.org/2001/XMLSchema#integer">26</EmpowerBP:canRepeat>
        <EmpowerBP:itemName rdf:datatype="http://www.w3.org/2001/XMLSchema#string">Sodium101 Advice</EmpowerBP:itemName>
        <EmpowerBP:itemText rdf:datatype="http://www.w3.org/2001/XMLSchema#string">Remember that unprocessed, fresh foods such as fruits and vegetables are good for you and are naturally low in sodium.
</EmpowerBP:itemText>
        <EmpowerBP:maximumUserAge rdf:datatype="http://www.w3.org/2001/XMLSchema#integer">120</EmpowerBP:maximumUserAge>
        <EmpowerBP:minimumUserAge rdf:datatype="http://www.w3.org/2001/XMLSchema#integer">18</EmpowerBP:minimumUserAge>
        <EmpowerBP:provideJournal rdf:datatype="http://www.w3.org/2001/XMLSchema#boolean">false</EmpowerBP:provideJournal>
        <EmpowerBP:provideLink rdf:datatype="http://www.w3.org/2001/XMLSchema#boolean">false</EmpowerBP:provideLink>
        <EmpowerBP:sourceURL rdf:datatype="http://www.w3.org/2001/XMLSchema#string">http://www.sodium101.ca/wp-content/uploads/2012/11/brochure-fullpage-en.pdf</EmpowerBP:sourceURL>
        <rdfs:comment rdf:datatype="http://www.w3.org/2001/XMLSchema#string">Remember that unprocessed, fresh foods such as fruits and vegetables are good for you and are naturally low in sodium.
</rdfs:comment>
        <rdfs:label rdf:datatype="http://www.w3.org/2001/XMLSchema#string">Sodium101 Advice</rdfs:label>
    </owl:NamedIndividual>
    


    <!-- http://www.semanticweb.org/tswheeler/ontologies/2016/3/EmpowerBP#T58 -->

    <owl:NamedIndividual rdf:about="http://www.semanticweb.org/tswheeler/ontologies/2016/3/EmpowerBP#T58">
        <rdf:type rdf:resource="http://www.semanticweb.org/tswheeler/ontologies/2016/3/EmpowerBP#InterventionItem"/>
        <rdf:type rdf:resource="http://www.semanticweb.org/tswheeler/ontologies/2016/3/EmpowerBP#Tip"/>
        <EmpowerBP:isAppropriateForInterventionGoal rdf:resource="http://www.semanticweb.org/tswheeler/ontologies/2016/3/EmpowerBP#ReduceSaltIntake"/>
        <EmpowerBP:isWarrantedBy rdf:resource="http://purl.bioontology.org/ontology/BCTT#Instruction_on_how_to_perform_the_behavior"/>
        <EmpowerBP:appropriateForAutomaticMotivation rdf:datatype="http://www.w3.org/2001/XMLSchema#integer">6</EmpowerBP:appropriateForAutomaticMotivation>
        <EmpowerBP:appropriateForLocation rdf:datatype="http://www.w3.org/2001/XMLSchema#integer">0</EmpowerBP:appropriateForLocation>
        <EmpowerBP:appropriateForPhysicalCapability rdf:datatype="http://www.w3.org/2001/XMLSchema#integer">3</EmpowerBP:appropriateForPhysicalCapability>
        <EmpowerBP:appropriateForPhysicalOpportunity rdf:datatype="http://www.w3.org/2001/XMLSchema#integer">3</EmpowerBP:appropriateForPhysicalOpportunity>
        <EmpowerBP:appropriateForPsychologicalCapability rdf:datatype="http://www.w3.org/2001/XMLSchema#integer">3</EmpowerBP:appropriateForPsychologicalCapability>
        <EmpowerBP:appropriateForReflectiveMotivation rdf:datatype="http://www.w3.org/2001/XMLSchema#integer">6</EmpowerBP:appropriateForReflectiveMotivation>
        <EmpowerBP:appropriateForSocialOpportunity rdf:datatype="http://www.w3.org/2001/XMLSchema#integer">3</EmpowerBP:appropriateForSocialOpportunity>
        <EmpowerBP:canRepeat rdf:datatype="http://www.w3.org/2001/XMLSchema#integer">26</EmpowerBP:canRepeat>
        <EmpowerBP:itemName rdf:datatype="http://www.w3.org/2001/XMLSchema#string">Sodium101 Advice</EmpowerBP:itemName>
        <EmpowerBP:itemText rdf:datatype="http://www.w3.org/2001/XMLSchema#string">Try to avoid high sodium products with more than 400 milligrams (mg) sodium per serving. Cut back on those with a sodium content of 200 – 400 mg per serving. Look for those products with less than 200 mg per serving.</EmpowerBP:itemText>
        <EmpowerBP:maximumUserAge rdf:datatype="http://www.w3.org/2001/XMLSchema#integer">120</EmpowerBP:maximumUserAge>
        <EmpowerBP:minimumUserAge rdf:datatype="http://www.w3.org/2001/XMLSchema#integer">18</EmpowerBP:minimumUserAge>
        <EmpowerBP:provideJournal rdf:datatype="http://www.w3.org/2001/XMLSchema#boolean">false</EmpowerBP:provideJournal>
        <EmpowerBP:provideLink rdf:datatype="http://www.w3.org/2001/XMLSchema#boolean">false</EmpowerBP:provideLink>
        <EmpowerBP:sourceURL rdf:datatype="http://www.w3.org/2001/XMLSchema#string">http://www.sodium101.ca/wp-content/uploads/2012/11/brochure-fullpage-en.pdf</EmpowerBP:sourceURL>
        <rdfs:comment rdf:datatype="http://www.w3.org/2001/XMLSchema#string">Try to avoid high sodium products with more than 400 milligrams (mg) sodium per serving. Cut back on those with a sodium content of 200 – 400 mg per serving. Look for those products with less than 200 mg per serving.</rdfs:comment>
        <rdfs:label rdf:datatype="http://www.w3.org/2001/XMLSchema#string">Sodium101 Advice</rdfs:label>
    </owl:NamedIndividual>
    


    <!-- http://www.semanticweb.org/tswheeler/ontologies/2016/3/EmpowerBP#T59 -->

    <owl:NamedIndividual rdf:about="http://www.semanticweb.org/tswheeler/ontologies/2016/3/EmpowerBP#T59">
        <rdf:type rdf:resource="http://www.semanticweb.org/tswheeler/ontologies/2016/3/EmpowerBP#InterventionItem"/>
        <rdf:type rdf:resource="http://www.semanticweb.org/tswheeler/ontologies/2016/3/EmpowerBP#Tip"/>
        <EmpowerBP:isAppropriateForInterventionGoal rdf:resource="http://www.semanticweb.org/tswheeler/ontologies/2016/3/EmpowerBP#ReduceSaltIntake"/>
        <EmpowerBP:isWarrantedBy rdf:resource="http://purl.bioontology.org/ontology/BCTT#Instruction_on_how_to_perform_the_behavior"/>
        <EmpowerBP:appropriateForAutomaticMotivation rdf:datatype="http://www.w3.org/2001/XMLSchema#integer">6</EmpowerBP:appropriateForAutomaticMotivation>
        <EmpowerBP:appropriateForLocation rdf:datatype="http://www.w3.org/2001/XMLSchema#integer">0</EmpowerBP:appropriateForLocation>
        <EmpowerBP:appropriateForPhysicalCapability rdf:datatype="http://www.w3.org/2001/XMLSchema#integer">3</EmpowerBP:appropriateForPhysicalCapability>
        <EmpowerBP:appropriateForPhysicalOpportunity rdf:datatype="http://www.w3.org/2001/XMLSchema#integer">3</EmpowerBP:appropriateForPhysicalOpportunity>
        <EmpowerBP:appropriateForPsychologicalCapability rdf:datatype="http://www.w3.org/2001/XMLSchema#integer">3</EmpowerBP:appropriateForPsychologicalCapability>
        <EmpowerBP:appropriateForReflectiveMotivation rdf:datatype="http://www.w3.org/2001/XMLSchema#integer">6</EmpowerBP:appropriateForReflectiveMotivation>
        <EmpowerBP:appropriateForSocialOpportunity rdf:datatype="http://www.w3.org/2001/XMLSchema#integer">3</EmpowerBP:appropriateForSocialOpportunity>
        <EmpowerBP:canRepeat rdf:datatype="http://www.w3.org/2001/XMLSchema#integer">26</EmpowerBP:canRepeat>
        <EmpowerBP:itemName rdf:datatype="http://www.w3.org/2001/XMLSchema#string">Sodium101 Advice</EmpowerBP:itemName>
        <EmpowerBP:itemText rdf:datatype="http://www.w3.org/2001/XMLSchema#string">Be aware of the serving size – how big a portion and how many servings do you intend to eat?
For example, breads and cereals are a significant source of sodium in our diets because we consume many servings in a day.</EmpowerBP:itemText>
        <EmpowerBP:maximumUserAge rdf:datatype="http://www.w3.org/2001/XMLSchema#integer">120</EmpowerBP:maximumUserAge>
        <EmpowerBP:minimumUserAge rdf:datatype="http://www.w3.org/2001/XMLSchema#integer">18</EmpowerBP:minimumUserAge>
        <EmpowerBP:provideJournal rdf:datatype="http://www.w3.org/2001/XMLSchema#boolean">false</EmpowerBP:provideJournal>
        <EmpowerBP:provideLink rdf:datatype="http://www.w3.org/2001/XMLSchema#boolean">false</EmpowerBP:provideLink>
        <EmpowerBP:sourceURL rdf:datatype="http://www.w3.org/2001/XMLSchema#string">http://www.sodium101.ca/wp-content/uploads/2012/11/brochure-fullpage-en.pdf</EmpowerBP:sourceURL>
        <rdfs:comment rdf:datatype="http://www.w3.org/2001/XMLSchema#string">Be aware of the serving size – how big a portion and how many servings do you intend to eat?
For example, breads and cereals are a significant source of sodium in our diets because we consume many servings in a day.</rdfs:comment>
        <rdfs:label rdf:datatype="http://www.w3.org/2001/XMLSchema#string">Sodium101 Advice</rdfs:label>
    </owl:NamedIndividual>
    


    <!-- http://www.semanticweb.org/tswheeler/ontologies/2016/3/EmpowerBP#T6 -->

    <owl:NamedIndividual rdf:about="http://www.semanticweb.org/tswheeler/ontologies/2016/3/EmpowerBP#T6">
        <rdf:type rdf:resource="http://www.semanticweb.org/tswheeler/ontologies/2016/3/EmpowerBP#InterventionItem"/>
        <rdf:type rdf:resource="http://www.semanticweb.org/tswheeler/ontologies/2016/3/EmpowerBP#Tip"/>
        <EmpowerBP:isAppropriateForInterventionGoal rdf:resource="http://www.semanticweb.org/tswheeler/ontologies/2016/3/EmpowerBP#ExerciseMore"/>
        <EmpowerBP:isWarrantedBy rdf:resource="http://purl.bioontology.org/ontology/BCTT#Instruction_on_how_to_perform_the_behavior"/>
        <EmpowerBP:appropriateForAutomaticMotivation rdf:datatype="http://www.w3.org/2001/XMLSchema#integer">6</EmpowerBP:appropriateForAutomaticMotivation>
        <EmpowerBP:appropriateForLocation rdf:datatype="http://www.w3.org/2001/XMLSchema#integer">0</EmpowerBP:appropriateForLocation>
        <EmpowerBP:appropriateForPhysicalCapability rdf:datatype="http://www.w3.org/2001/XMLSchema#integer">3</EmpowerBP:appropriateForPhysicalCapability>
        <EmpowerBP:appropriateForPhysicalOpportunity rdf:datatype="http://www.w3.org/2001/XMLSchema#integer">3</EmpowerBP:appropriateForPhysicalOpportunity>
        <EmpowerBP:appropriateForPsychologicalCapability rdf:datatype="http://www.w3.org/2001/XMLSchema#integer">3</EmpowerBP:appropriateForPsychologicalCapability>
        <EmpowerBP:appropriateForReflectiveMotivation rdf:datatype="http://www.w3.org/2001/XMLSchema#integer">6</EmpowerBP:appropriateForReflectiveMotivation>
        <EmpowerBP:appropriateForSocialOpportunity rdf:datatype="http://www.w3.org/2001/XMLSchema#integer">3</EmpowerBP:appropriateForSocialOpportunity>
        <EmpowerBP:canRepeat rdf:datatype="http://www.w3.org/2001/XMLSchema#integer">26</EmpowerBP:canRepeat>
        <EmpowerBP:itemName rdf:datatype="http://www.w3.org/2001/XMLSchema#string">Let&apos;s Talk Intensity!</EmpowerBP:itemName>
        <EmpowerBP:itemText rdf:datatype="http://www.w3.org/2001/XMLSchema#string">Moderate-intensity physical activities will cause older adults to sweat a little and to breathe harder. Activities like:
• Walking quickly
• Bicycling
Vigorous-intensity physical activities will cause older adults to sweat and be ‘out of breath’. Activities like:
• Cross-country skiing 
• Swimming</EmpowerBP:itemText>
        <EmpowerBP:maximumUserAge rdf:datatype="http://www.w3.org/2001/XMLSchema#integer">120</EmpowerBP:maximumUserAge>
        <EmpowerBP:minimumUserAge rdf:datatype="http://www.w3.org/2001/XMLSchema#integer">65</EmpowerBP:minimumUserAge>
        <EmpowerBP:provideJournal rdf:datatype="http://www.w3.org/2001/XMLSchema#boolean">false</EmpowerBP:provideJournal>
        <EmpowerBP:provideLink rdf:datatype="http://www.w3.org/2001/XMLSchema#boolean">false</EmpowerBP:provideLink>
        <EmpowerBP:sourceURL rdf:datatype="http://www.w3.org/2001/XMLSchema#string">http://www.csep.ca/cmfiles/guidelines/csep_guidelines_handbook.pdf</EmpowerBP:sourceURL>
        <rdfs:comment rdf:datatype="http://www.w3.org/2001/XMLSchema#string">Moderate-intensity physical activities will cause older adults to sweat a little and to breathe harder. Activities like:
• Walking quickly
• Bicycling
Vigorous-intensity physical activities will cause older adults to sweat and be ‘out of breath’. Activities like:
• Cross-country skiing 
• Swimming</rdfs:comment>
        <rdfs:label rdf:datatype="http://www.w3.org/2001/XMLSchema#string">Let&apos;s Talk Intensity!</rdfs:label>
    </owl:NamedIndividual>
    


    <!-- http://www.semanticweb.org/tswheeler/ontologies/2016/3/EmpowerBP#T60 -->

    <owl:NamedIndividual rdf:about="http://www.semanticweb.org/tswheeler/ontologies/2016/3/EmpowerBP#T60">
        <rdf:type rdf:resource="http://www.semanticweb.org/tswheeler/ontologies/2016/3/EmpowerBP#InterventionItem"/>
        <rdf:type rdf:resource="http://www.semanticweb.org/tswheeler/ontologies/2016/3/EmpowerBP#Tip"/>
        <EmpowerBP:isAppropriateForInterventionGoal rdf:resource="http://www.semanticweb.org/tswheeler/ontologies/2016/3/EmpowerBP#ReduceSaltIntake"/>
        <EmpowerBP:isWarrantedBy rdf:resource="http://purl.bioontology.org/ontology/BCTT#Action_planning"/>
        <EmpowerBP:appropriateForAutomaticMotivation rdf:datatype="http://www.w3.org/2001/XMLSchema#integer">6</EmpowerBP:appropriateForAutomaticMotivation>
        <EmpowerBP:appropriateForLocation rdf:datatype="http://www.w3.org/2001/XMLSchema#integer">0</EmpowerBP:appropriateForLocation>
        <EmpowerBP:appropriateForPhysicalCapability rdf:datatype="http://www.w3.org/2001/XMLSchema#integer">3</EmpowerBP:appropriateForPhysicalCapability>
        <EmpowerBP:appropriateForPhysicalOpportunity rdf:datatype="http://www.w3.org/2001/XMLSchema#integer">3</EmpowerBP:appropriateForPhysicalOpportunity>
        <EmpowerBP:appropriateForPsychologicalCapability rdf:datatype="http://www.w3.org/2001/XMLSchema#integer">3</EmpowerBP:appropriateForPsychologicalCapability>
        <EmpowerBP:appropriateForReflectiveMotivation rdf:datatype="http://www.w3.org/2001/XMLSchema#integer">6</EmpowerBP:appropriateForReflectiveMotivation>
        <EmpowerBP:appropriateForSocialOpportunity rdf:datatype="http://www.w3.org/2001/XMLSchema#integer">3</EmpowerBP:appropriateForSocialOpportunity>
        <EmpowerBP:canRepeat rdf:datatype="http://www.w3.org/2001/XMLSchema#integer">26</EmpowerBP:canRepeat>
        <EmpowerBP:itemName rdf:datatype="http://www.w3.org/2001/XMLSchema#string">Reducing Sodium at Home</EmpowerBP:itemName>
        <EmpowerBP:itemText rdf:datatype="http://www.w3.org/2001/XMLSchema#string">Low-sodium cooking tips

• Cook with little or no salt. Use less salt than what a recipe calls for, and taste your food before adding salt.
• Make your own soup, sauces, and salad dressings.
Rinse canned vegetables, beans, lentils, and chickpeas before using.
• Cook pasta, noodles, and rice in unsalted water
• Use less of the seasoning that comes with taco kits, packaged macaroni and cheese, pasta, and rice mixes.
• Limit high-sodium condiments such as BBQ sauce, soy sauce, ketchup, mustard, relish, pickles, hoisin sauce, fish sauce, and oyster sauce.</EmpowerBP:itemText>
        <EmpowerBP:maximumUserAge rdf:datatype="http://www.w3.org/2001/XMLSchema#integer">120</EmpowerBP:maximumUserAge>
        <EmpowerBP:minimumUserAge rdf:datatype="http://www.w3.org/2001/XMLSchema#integer">18</EmpowerBP:minimumUserAge>
        <EmpowerBP:provideJournal rdf:datatype="http://www.w3.org/2001/XMLSchema#boolean">false</EmpowerBP:provideJournal>
        <EmpowerBP:provideLink rdf:datatype="http://www.w3.org/2001/XMLSchema#boolean">false</EmpowerBP:provideLink>
        <EmpowerBP:sourceURL rdf:datatype="http://www.w3.org/2001/XMLSchema#string">https://www.canada.ca/en/health-canada/services/nutrients/sodium/reducing-sodium-home.html</EmpowerBP:sourceURL>
        <rdfs:comment rdf:datatype="http://www.w3.org/2001/XMLSchema#string">Low-sodium cooking tips

• Cook with little or no salt. Use less salt than what a recipe calls for, and taste your food before adding salt.
• Make your own soup, sauces, and salad dressings.
Rinse canned vegetables, beans, lentils, and chickpeas before using.
• Cook pasta, noodles, and rice in unsalted water
• Use less of the seasoning that comes with taco kits, packaged macaroni and cheese, pasta, and rice mixes.
• Limit high-sodium condiments such as BBQ sauce, soy sauce, ketchup, mustard, relish, pickles, hoisin sauce, fish sauce, and oyster sauce.</rdfs:comment>
        <rdfs:label rdf:datatype="http://www.w3.org/2001/XMLSchema#string">Reducing Sodium at Home</rdfs:label>
    </owl:NamedIndividual>
    


    <!-- http://www.semanticweb.org/tswheeler/ontologies/2016/3/EmpowerBP#T61 -->

    <owl:NamedIndividual rdf:about="http://www.semanticweb.org/tswheeler/ontologies/2016/3/EmpowerBP#T61">
        <rdf:type rdf:resource="http://www.semanticweb.org/tswheeler/ontologies/2016/3/EmpowerBP#InterventionItem"/>
        <rdf:type rdf:resource="http://www.semanticweb.org/tswheeler/ontologies/2016/3/EmpowerBP#Tip"/>
        <EmpowerBP:isAppropriateForInterventionGoal rdf:resource="http://www.semanticweb.org/tswheeler/ontologies/2016/3/EmpowerBP#ReduceSaltIntake"/>
        <EmpowerBP:isWarrantedBy rdf:resource="http://purl.bioontology.org/ontology/BCTT#Action_planning"/>
        <EmpowerBP:appropriateForAutomaticMotivation rdf:datatype="http://www.w3.org/2001/XMLSchema#integer">6</EmpowerBP:appropriateForAutomaticMotivation>
        <EmpowerBP:appropriateForLocation rdf:datatype="http://www.w3.org/2001/XMLSchema#integer">0</EmpowerBP:appropriateForLocation>
        <EmpowerBP:appropriateForPhysicalCapability rdf:datatype="http://www.w3.org/2001/XMLSchema#integer">3</EmpowerBP:appropriateForPhysicalCapability>
        <EmpowerBP:appropriateForPhysicalOpportunity rdf:datatype="http://www.w3.org/2001/XMLSchema#integer">3</EmpowerBP:appropriateForPhysicalOpportunity>
        <EmpowerBP:appropriateForPsychologicalCapability rdf:datatype="http://www.w3.org/2001/XMLSchema#integer">3</EmpowerBP:appropriateForPsychologicalCapability>
        <EmpowerBP:appropriateForReflectiveMotivation rdf:datatype="http://www.w3.org/2001/XMLSchema#integer">6</EmpowerBP:appropriateForReflectiveMotivation>
        <EmpowerBP:appropriateForSocialOpportunity rdf:datatype="http://www.w3.org/2001/XMLSchema#integer">3</EmpowerBP:appropriateForSocialOpportunity>
        <EmpowerBP:canRepeat rdf:datatype="http://www.w3.org/2001/XMLSchema#integer">26</EmpowerBP:canRepeat>
        <EmpowerBP:itemName rdf:datatype="http://www.w3.org/2001/XMLSchema#string">Herbs and Spices</EmpowerBP:itemName>
        <EmpowerBP:itemText rdf:datatype="http://www.w3.org/2001/XMLSchema#string">Cooking with herbs and spices instead of salt
Flavour foods with herbs and spices instead of salt. Your taste buds will adjust to less salt in your food. Here are a few ideas to get you started:

• Basil - tastes great with tomatoes and pasta
• Cumin - adds flavour to soup, stews, and sauces
• Curry  powder - good with meat, poultry, soup, and stews
• Dill - pairs well with fish, potatoes, and eggs
• Oregano - perfect in pasta, soup, and salads
• Paprika - good with seafood, vegetables, chicken, and eggs
• Rosemary - delicious with chicken, lamb, and pork
• Thyme - goes well with beef and chicken</EmpowerBP:itemText>
        <EmpowerBP:maximumUserAge rdf:datatype="http://www.w3.org/2001/XMLSchema#integer">120</EmpowerBP:maximumUserAge>
        <EmpowerBP:minimumUserAge rdf:datatype="http://www.w3.org/2001/XMLSchema#integer">18</EmpowerBP:minimumUserAge>
        <EmpowerBP:provideJournal rdf:datatype="http://www.w3.org/2001/XMLSchema#boolean">false</EmpowerBP:provideJournal>
        <EmpowerBP:provideLink rdf:datatype="http://www.w3.org/2001/XMLSchema#boolean">false</EmpowerBP:provideLink>
        <EmpowerBP:sourceURL rdf:datatype="http://www.w3.org/2001/XMLSchema#string">https://www.canada.ca/en/health-canada/services/nutrients/sodium/reducing-sodium-home.html</EmpowerBP:sourceURL>
        <rdfs:comment rdf:datatype="http://www.w3.org/2001/XMLSchema#string">Cooking with herbs and spices instead of salt
Flavour foods with herbs and spices instead of salt. Your taste buds will adjust to less salt in your food. Here are a few ideas to get you started:

• Basil - tastes great with tomatoes and pasta
• Cumin - adds flavour to soup, stews, and sauces
• Curry  powder - good with meat, poultry, soup, and stews
• Dill - pairs well with fish, potatoes, and eggs
• Oregano - perfect in pasta, soup, and salads
• Paprika - good with seafood, vegetables, chicken, and eggs
• Rosemary - delicious with chicken, lamb, and pork
• Thyme - goes well with beef and chicken</rdfs:comment>
        <rdfs:label rdf:datatype="http://www.w3.org/2001/XMLSchema#string">Herbs and Spices</rdfs:label>
    </owl:NamedIndividual>
    


    <!-- http://www.semanticweb.org/tswheeler/ontologies/2016/3/EmpowerBP#T62 -->

    <owl:NamedIndividual rdf:about="http://www.semanticweb.org/tswheeler/ontologies/2016/3/EmpowerBP#T62">
        <rdf:type rdf:resource="http://www.semanticweb.org/tswheeler/ontologies/2016/3/EmpowerBP#InterventionItem"/>
        <rdf:type rdf:resource="http://www.semanticweb.org/tswheeler/ontologies/2016/3/EmpowerBP#Tip"/>
        <EmpowerBP:isAppropriateForInterventionGoal rdf:resource="http://www.semanticweb.org/tswheeler/ontologies/2016/3/EmpowerBP#ReduceSaltIntake"/>
        <EmpowerBP:isWarrantedBy rdf:resource="http://purl.bioontology.org/ontology/BCTT#Information_about_social_and_environmental_consequences"/>
        <EmpowerBP:appropriateForAutomaticMotivation rdf:datatype="http://www.w3.org/2001/XMLSchema#integer">3</EmpowerBP:appropriateForAutomaticMotivation>
        <EmpowerBP:appropriateForLocation rdf:datatype="http://www.w3.org/2001/XMLSchema#integer">0</EmpowerBP:appropriateForLocation>
        <EmpowerBP:appropriateForPhysicalCapability rdf:datatype="http://www.w3.org/2001/XMLSchema#integer">3</EmpowerBP:appropriateForPhysicalCapability>
        <EmpowerBP:appropriateForPhysicalOpportunity rdf:datatype="http://www.w3.org/2001/XMLSchema#integer">3</EmpowerBP:appropriateForPhysicalOpportunity>
        <EmpowerBP:appropriateForPsychologicalCapability rdf:datatype="http://www.w3.org/2001/XMLSchema#integer">3</EmpowerBP:appropriateForPsychologicalCapability>
        <EmpowerBP:appropriateForReflectiveMotivation rdf:datatype="http://www.w3.org/2001/XMLSchema#integer">3</EmpowerBP:appropriateForReflectiveMotivation>
        <EmpowerBP:appropriateForSocialOpportunity rdf:datatype="http://www.w3.org/2001/XMLSchema#integer">3</EmpowerBP:appropriateForSocialOpportunity>
        <EmpowerBP:canRepeat rdf:datatype="http://www.w3.org/2001/XMLSchema#integer">26</EmpowerBP:canRepeat>
        <EmpowerBP:itemName rdf:datatype="http://www.w3.org/2001/XMLSchema#string">Top Five Food Sources of Sodium</EmpowerBP:itemName>
        <EmpowerBP:itemText rdf:datatype="http://www.w3.org/2001/XMLSchema#string">Almost 80% of the sodium we eat comes from processed and packaged foods, not the salt shaker. Here&apos;s a list of the top five food sources of sodium:
1. Mixed dishes such as macaroni &amp; cheese, lasagne, beef stew, etc.
2. Baked goods such as bread , buns, muffins, and biscuits
3. Processed meat such as deli meat, hotdogs, seasoned meat, etc.
4. Soup
5. Cheese</EmpowerBP:itemText>
        <EmpowerBP:maximumUserAge rdf:datatype="http://www.w3.org/2001/XMLSchema#integer">120</EmpowerBP:maximumUserAge>
        <EmpowerBP:minimumUserAge rdf:datatype="http://www.w3.org/2001/XMLSchema#integer">18</EmpowerBP:minimumUserAge>
        <EmpowerBP:provideJournal rdf:datatype="http://www.w3.org/2001/XMLSchema#boolean">false</EmpowerBP:provideJournal>
        <EmpowerBP:provideLink rdf:datatype="http://www.w3.org/2001/XMLSchema#boolean">false</EmpowerBP:provideLink>
        <EmpowerBP:sourceURL rdf:datatype="http://www.w3.org/2001/XMLSchema#string">https://www.canada.ca/en/health-canada/services/nutrients/sodium/sodium-basics.html#a3</EmpowerBP:sourceURL>
        <rdfs:comment rdf:datatype="http://www.w3.org/2001/XMLSchema#string">Almost 80% of the sodium we eat comes from processed and packaged foods, not the salt shaker. Here&apos;s a list of the top five food sources of sodium:
1. Mixed dishes such as macaroni &amp; cheese, lasagne, beef stew, etc.
2. Baked goods such as bread , buns, muffins, and biscuits
3. Processed meat such as deli meat, hotdogs, seasoned meat, etc.
4. Soup
5. Cheese</rdfs:comment>
        <rdfs:label rdf:datatype="http://www.w3.org/2001/XMLSchema#string">Top Five Food Sources of Sodium</rdfs:label>
    </owl:NamedIndividual>
    


    <!-- http://www.semanticweb.org/tswheeler/ontologies/2016/3/EmpowerBP#T63 -->

    <owl:NamedIndividual rdf:about="http://www.semanticweb.org/tswheeler/ontologies/2016/3/EmpowerBP#T63">
        <rdf:type rdf:resource="http://www.semanticweb.org/tswheeler/ontologies/2016/3/EmpowerBP#InterventionItem"/>
        <rdf:type rdf:resource="http://www.semanticweb.org/tswheeler/ontologies/2016/3/EmpowerBP#Tip"/>
        <EmpowerBP:isAppropriateForInterventionGoal rdf:resource="http://www.semanticweb.org/tswheeler/ontologies/2016/3/EmpowerBP#ExerciseMore"/>
        <EmpowerBP:isWarrantedBy rdf:resource="http://purl.bioontology.org/ontology/BCTT#Information_about_social_and_environmental_consequences"/>
        <EmpowerBP:appropriateForAutomaticMotivation rdf:datatype="http://www.w3.org/2001/XMLSchema#integer">3</EmpowerBP:appropriateForAutomaticMotivation>
        <EmpowerBP:appropriateForLocation rdf:datatype="http://www.w3.org/2001/XMLSchema#integer">0</EmpowerBP:appropriateForLocation>
        <EmpowerBP:appropriateForPhysicalCapability rdf:datatype="http://www.w3.org/2001/XMLSchema#integer">3</EmpowerBP:appropriateForPhysicalCapability>
        <EmpowerBP:appropriateForPhysicalOpportunity rdf:datatype="http://www.w3.org/2001/XMLSchema#integer">3</EmpowerBP:appropriateForPhysicalOpportunity>
        <EmpowerBP:appropriateForPsychologicalCapability rdf:datatype="http://www.w3.org/2001/XMLSchema#integer">3</EmpowerBP:appropriateForPsychologicalCapability>
        <EmpowerBP:appropriateForReflectiveMotivation rdf:datatype="http://www.w3.org/2001/XMLSchema#integer">3</EmpowerBP:appropriateForReflectiveMotivation>
        <EmpowerBP:appropriateForSocialOpportunity rdf:datatype="http://www.w3.org/2001/XMLSchema#integer">3</EmpowerBP:appropriateForSocialOpportunity>
        <EmpowerBP:canRepeat rdf:datatype="http://www.w3.org/2001/XMLSchema#integer">26</EmpowerBP:canRepeat>
        <EmpowerBP:itemName rdf:datatype="http://www.w3.org/2001/XMLSchema#string">Walking and the Environment</EmpowerBP:itemName>
        <EmpowerBP:itemText rdf:datatype="http://www.w3.org/2001/XMLSchema#string">Walking is an environmentally sustainable form of transportation. Climate change is one of the most pressing issues facing communities, our nation and the international community. Walking is one easy way to replace a car trip and reduce greenhouse gas emissions.

According to Environment Canada, 27% of Canada’s greenhouse gas emissions come from transportation, the daily use of cars and trucks make up 12% of our total.</EmpowerBP:itemText>
        <EmpowerBP:maximumUserAge rdf:datatype="http://www.w3.org/2001/XMLSchema#integer">120</EmpowerBP:maximumUserAge>
        <EmpowerBP:minimumUserAge rdf:datatype="http://www.w3.org/2001/XMLSchema#integer">18</EmpowerBP:minimumUserAge>
        <EmpowerBP:provideJournal rdf:datatype="http://www.w3.org/2001/XMLSchema#boolean">false</EmpowerBP:provideJournal>
        <EmpowerBP:provideLink rdf:datatype="http://www.w3.org/2001/XMLSchema#boolean">false</EmpowerBP:provideLink>
        <EmpowerBP:sourceURL rdf:datatype="http://www.w3.org/2001/XMLSchema#string">http://walkaboutns.ca/walkabout-info/about/</EmpowerBP:sourceURL>
        <rdfs:comment rdf:datatype="http://www.w3.org/2001/XMLSchema#string">Walking is an environmentally sustainable form of transportation. Climate change is one of the most pressing issues facing communities, our nation and the international community. Walking is one easy way to replace a car trip and reduce greenhouse gas emissions.

According to Environment Canada, 27% of Canada’s greenhouse gas emissions come from transportation, the daily use of cars and trucks make up 12% of our total.</rdfs:comment>
        <rdfs:label rdf:datatype="http://www.w3.org/2001/XMLSchema#string">Walking and the Environment</rdfs:label>
    </owl:NamedIndividual>
    


    <!-- http://www.semanticweb.org/tswheeler/ontologies/2016/3/EmpowerBP#T64 -->

    <owl:NamedIndividual rdf:about="http://www.semanticweb.org/tswheeler/ontologies/2016/3/EmpowerBP#T64">
        <rdf:type rdf:resource="http://www.semanticweb.org/tswheeler/ontologies/2016/3/EmpowerBP#InterventionItem"/>
        <rdf:type rdf:resource="http://www.semanticweb.org/tswheeler/ontologies/2016/3/EmpowerBP#Tip"/>
        <EmpowerBP:isAppropriateForInterventionGoal rdf:resource="http://www.semanticweb.org/tswheeler/ontologies/2016/3/EmpowerBP#ReduceSaltIntake"/>
        <EmpowerBP:isWarrantedBy rdf:resource="http://purl.bioontology.org/ontology/BCTT#Restructuring_the_physical_environment"/>
        <EmpowerBP:appropriateForAutomaticMotivation rdf:datatype="http://www.w3.org/2001/XMLSchema#integer">6</EmpowerBP:appropriateForAutomaticMotivation>
        <EmpowerBP:appropriateForLocation rdf:datatype="http://www.w3.org/2001/XMLSchema#integer">0</EmpowerBP:appropriateForLocation>
        <EmpowerBP:appropriateForPhysicalCapability rdf:datatype="http://www.w3.org/2001/XMLSchema#integer">3</EmpowerBP:appropriateForPhysicalCapability>
        <EmpowerBP:appropriateForPhysicalOpportunity rdf:datatype="http://www.w3.org/2001/XMLSchema#integer">3</EmpowerBP:appropriateForPhysicalOpportunity>
        <EmpowerBP:appropriateForPsychologicalCapability rdf:datatype="http://www.w3.org/2001/XMLSchema#integer">3</EmpowerBP:appropriateForPsychologicalCapability>
        <EmpowerBP:appropriateForReflectiveMotivation rdf:datatype="http://www.w3.org/2001/XMLSchema#integer">6</EmpowerBP:appropriateForReflectiveMotivation>
        <EmpowerBP:appropriateForSocialOpportunity rdf:datatype="http://www.w3.org/2001/XMLSchema#integer">3</EmpowerBP:appropriateForSocialOpportunity>
        <EmpowerBP:canRepeat rdf:datatype="http://www.w3.org/2001/XMLSchema#integer">26</EmpowerBP:canRepeat>
        <EmpowerBP:itemName rdf:datatype="http://www.w3.org/2001/XMLSchema#string">Move the Salt Shaker</EmpowerBP:itemName>
        <EmpowerBP:itemText rdf:datatype="http://www.w3.org/2001/XMLSchema#string">Try keeping your salt shaker in a cupboard instead of on the table or countertop! You&apos;ll be less likely to reach for it when eating or preparing a meal. </EmpowerBP:itemText>
        <EmpowerBP:maximumUserAge rdf:datatype="http://www.w3.org/2001/XMLSchema#integer">120</EmpowerBP:maximumUserAge>
        <EmpowerBP:minimumUserAge rdf:datatype="http://www.w3.org/2001/XMLSchema#integer">18</EmpowerBP:minimumUserAge>
        <EmpowerBP:provideJournal rdf:datatype="http://www.w3.org/2001/XMLSchema#boolean">false</EmpowerBP:provideJournal>
        <EmpowerBP:provideLink rdf:datatype="http://www.w3.org/2001/XMLSchema#boolean">false</EmpowerBP:provideLink>
        <EmpowerBP:sourceURL rdf:datatype="http://www.w3.org/2001/XMLSchema#string">https://www.diabetes.ca/diabetes-and-you/healthy-living-resources/diet-nutrition/reducing-salt-intake</EmpowerBP:sourceURL>
        <rdfs:comment rdf:datatype="http://www.w3.org/2001/XMLSchema#string">Try keeping your salt shaker in a cupboard instead of on the table or countertop! You&apos;ll be less likely to reach for it when eating or preparing a meal. </rdfs:comment>
        <rdfs:label rdf:datatype="http://www.w3.org/2001/XMLSchema#string">Move the Salt Shaker</rdfs:label>
    </owl:NamedIndividual>
    


    <!-- http://www.semanticweb.org/tswheeler/ontologies/2016/3/EmpowerBP#T7 -->

    <owl:NamedIndividual rdf:about="http://www.semanticweb.org/tswheeler/ontologies/2016/3/EmpowerBP#T7">
        <rdf:type rdf:resource="http://www.semanticweb.org/tswheeler/ontologies/2016/3/EmpowerBP#InterventionItem"/>
        <rdf:type rdf:resource="http://www.semanticweb.org/tswheeler/ontologies/2016/3/EmpowerBP#Tip"/>
        <EmpowerBP:isAppropriateForInterventionGoal rdf:resource="http://www.semanticweb.org/tswheeler/ontologies/2016/3/EmpowerBP#ExerciseMore"/>
        <EmpowerBP:isWarrantedBy rdf:resource="http://purl.bioontology.org/ontology/BCTT#Graded_tasks"/>
        <EmpowerBP:appropriateForAutomaticMotivation rdf:datatype="http://www.w3.org/2001/XMLSchema#integer">6</EmpowerBP:appropriateForAutomaticMotivation>
        <EmpowerBP:appropriateForLocation rdf:datatype="http://www.w3.org/2001/XMLSchema#integer">0</EmpowerBP:appropriateForLocation>
        <EmpowerBP:appropriateForPhysicalCapability rdf:datatype="http://www.w3.org/2001/XMLSchema#integer">3</EmpowerBP:appropriateForPhysicalCapability>
        <EmpowerBP:appropriateForPhysicalOpportunity rdf:datatype="http://www.w3.org/2001/XMLSchema#integer">3</EmpowerBP:appropriateForPhysicalOpportunity>
        <EmpowerBP:appropriateForPsychologicalCapability rdf:datatype="http://www.w3.org/2001/XMLSchema#integer">3</EmpowerBP:appropriateForPsychologicalCapability>
        <EmpowerBP:appropriateForReflectiveMotivation rdf:datatype="http://www.w3.org/2001/XMLSchema#integer">6</EmpowerBP:appropriateForReflectiveMotivation>
        <EmpowerBP:appropriateForSocialOpportunity rdf:datatype="http://www.w3.org/2001/XMLSchema#integer">3</EmpowerBP:appropriateForSocialOpportunity>
        <EmpowerBP:canRepeat rdf:datatype="http://www.w3.org/2001/XMLSchema#integer">26</EmpowerBP:canRepeat>
        <EmpowerBP:itemName rdf:datatype="http://www.w3.org/2001/XMLSchema#string">Every Step Counts!</EmpowerBP:itemName>
        <EmpowerBP:itemText rdf:datatype="http://www.w3.org/2001/XMLSchema#string">If you’re not active now, adding any amount of physical activity can bring some health bene ts. Take a step in the right direction. Start now and slowly increase your physical activity to meet the recommendations.</EmpowerBP:itemText>
        <EmpowerBP:maximumUserAge rdf:datatype="http://www.w3.org/2001/XMLSchema#integer">120</EmpowerBP:maximumUserAge>
        <EmpowerBP:minimumUserAge rdf:datatype="http://www.w3.org/2001/XMLSchema#integer">18</EmpowerBP:minimumUserAge>
        <EmpowerBP:provideJournal rdf:datatype="http://www.w3.org/2001/XMLSchema#boolean">false</EmpowerBP:provideJournal>
        <EmpowerBP:provideLink rdf:datatype="http://www.w3.org/2001/XMLSchema#boolean">false</EmpowerBP:provideLink>
        <EmpowerBP:sourceURL rdf:datatype="http://www.w3.org/2001/XMLSchema#string">http://www.phac-aspc.gc.ca/hp-ps/hl-mvs/pa-ap/index-eng.php</EmpowerBP:sourceURL>
        <rdfs:comment rdf:datatype="http://www.w3.org/2001/XMLSchema#string">If you’re not active now, adding any amount of physical activity can bring some health bene ts. Take a step in the right direction. Start now and slowly increase your physical activity to meet the recommendations.</rdfs:comment>
        <rdfs:label rdf:datatype="http://www.w3.org/2001/XMLSchema#string">Every Step Counts!</rdfs:label>
    </owl:NamedIndividual>
    


    <!-- http://www.semanticweb.org/tswheeler/ontologies/2016/3/EmpowerBP#T8 -->

    <owl:NamedIndividual rdf:about="http://www.semanticweb.org/tswheeler/ontologies/2016/3/EmpowerBP#T8">
        <rdf:type rdf:resource="http://www.semanticweb.org/tswheeler/ontologies/2016/3/EmpowerBP#InterventionItem"/>
        <rdf:type rdf:resource="http://www.semanticweb.org/tswheeler/ontologies/2016/3/EmpowerBP#Tip"/>
        <EmpowerBP:isAppropriateForInterventionGoal rdf:resource="http://www.semanticweb.org/tswheeler/ontologies/2016/3/EmpowerBP#ExerciseMore"/>
        <EmpowerBP:isWarrantedBy rdf:resource="http://purl.bioontology.org/ontology/BCTT#Instruction_on_how_to_perform_the_behavior"/>
        <EmpowerBP:appropriateForAutomaticMotivation rdf:datatype="http://www.w3.org/2001/XMLSchema#integer">6</EmpowerBP:appropriateForAutomaticMotivation>
        <EmpowerBP:appropriateForLocation rdf:datatype="http://www.w3.org/2001/XMLSchema#integer">0</EmpowerBP:appropriateForLocation>
        <EmpowerBP:appropriateForPhysicalCapability rdf:datatype="http://www.w3.org/2001/XMLSchema#integer">3</EmpowerBP:appropriateForPhysicalCapability>
        <EmpowerBP:appropriateForPhysicalOpportunity rdf:datatype="http://www.w3.org/2001/XMLSchema#integer">3</EmpowerBP:appropriateForPhysicalOpportunity>
        <EmpowerBP:appropriateForPsychologicalCapability rdf:datatype="http://www.w3.org/2001/XMLSchema#integer">3</EmpowerBP:appropriateForPsychologicalCapability>
        <EmpowerBP:appropriateForReflectiveMotivation rdf:datatype="http://www.w3.org/2001/XMLSchema#integer">6</EmpowerBP:appropriateForReflectiveMotivation>
        <EmpowerBP:appropriateForSocialOpportunity rdf:datatype="http://www.w3.org/2001/XMLSchema#integer">3</EmpowerBP:appropriateForSocialOpportunity>
        <EmpowerBP:canRepeat rdf:datatype="http://www.w3.org/2001/XMLSchema#integer">26</EmpowerBP:canRepeat>
        <EmpowerBP:itemName rdf:datatype="http://www.w3.org/2001/XMLSchema#string">Types of Aerobic Activities</EmpowerBP:itemName>
        <EmpowerBP:itemText rdf:datatype="http://www.w3.org/2001/XMLSchema#string">Aerobic activity moves your large muscles, such as those in your arms and legs. Running, swimming, walking, bicycling, dancing, and doing jumping jacks are examples of aerobic activity. Aerobic activity also is called endurance activity.

Aerobic activity makes your heart beat faster than usual. You also breathe harder during this type of activity. Over time, regular aerobic activity makes your heart and lungs stronger and able to work better.

Below are examples of aerobic activities. Depending on your level of fitness, they can be light, moderate, or vigorous in intensity:

• Pushing a grocery cart around a store
• Gardening, such as digging or hoeing that causes your heart rate to go up
• Walking, hiking, jogging, running
• Water aerobics or swimming laps
• Bicycling, skateboarding, rollerblading, and jumping rope
• Ballroom dancing and aerobic dancing
• Tennis, soccer, hockey, and basketball</EmpowerBP:itemText>
        <EmpowerBP:maximumUserAge rdf:datatype="http://www.w3.org/2001/XMLSchema#integer">64</EmpowerBP:maximumUserAge>
        <EmpowerBP:minimumUserAge rdf:datatype="http://www.w3.org/2001/XMLSchema#integer">18</EmpowerBP:minimumUserAge>
        <EmpowerBP:provideJournal rdf:datatype="http://www.w3.org/2001/XMLSchema#boolean">false</EmpowerBP:provideJournal>
        <EmpowerBP:provideLink rdf:datatype="http://www.w3.org/2001/XMLSchema#boolean">false</EmpowerBP:provideLink>
        <EmpowerBP:sourceURL rdf:datatype="http://www.w3.org/2001/XMLSchema#string">https://www.nhlbi.nih.gov/health/health-topics/topics/phys/types</EmpowerBP:sourceURL>
        <rdfs:comment rdf:datatype="http://www.w3.org/2001/XMLSchema#string">Aerobic activity moves your large muscles, such as those in your arms and legs. Running, swimming, walking, bicycling, dancing, and doing jumping jacks are examples of aerobic activity. Aerobic activity also is called endurance activity.

Aerobic activity makes your heart beat faster than usual. You also breathe harder during this type of activity. Over time, regular aerobic activity makes your heart and lungs stronger and able to work better.

Below are examples of aerobic activities. Depending on your level of fitness, they can be light, moderate, or vigorous in intensity:

• Pushing a grocery cart around a store
• Gardening, such as digging or hoeing that causes your heart rate to go up
• Walking, hiking, jogging, running
• Water aerobics or swimming laps
• Bicycling, skateboarding, rollerblading, and jumping rope
• Ballroom dancing and aerobic dancing
• Tennis, soccer, hockey, and basketball</rdfs:comment>
        <rdfs:label rdf:datatype="http://www.w3.org/2001/XMLSchema#string">Types of Aerobic Activities</rdfs:label>
    </owl:NamedIndividual>
    


    <!-- http://www.semanticweb.org/tswheeler/ontologies/2016/3/EmpowerBP#T9 -->

    <owl:NamedIndividual rdf:about="http://www.semanticweb.org/tswheeler/ontologies/2016/3/EmpowerBP#T9">
        <rdf:type rdf:resource="http://www.semanticweb.org/tswheeler/ontologies/2016/3/EmpowerBP#InterventionItem"/>
        <rdf:type rdf:resource="http://www.semanticweb.org/tswheeler/ontologies/2016/3/EmpowerBP#Tip"/>
        <EmpowerBP:isAppropriateForInterventionGoal rdf:resource="http://www.semanticweb.org/tswheeler/ontologies/2016/3/EmpowerBP#ReduceSaltIntake"/>
        <EmpowerBP:isWarrantedBy rdf:resource="http://purl.bioontology.org/ontology/BCTT#Information_about_social_and_environmental_consequences"/>
        <EmpowerBP:appropriateForAutomaticMotivation rdf:datatype="http://www.w3.org/2001/XMLSchema#integer">3</EmpowerBP:appropriateForAutomaticMotivation>
        <EmpowerBP:appropriateForLocation rdf:datatype="http://www.w3.org/2001/XMLSchema#integer">0</EmpowerBP:appropriateForLocation>
        <EmpowerBP:appropriateForPhysicalCapability rdf:datatype="http://www.w3.org/2001/XMLSchema#integer">3</EmpowerBP:appropriateForPhysicalCapability>
        <EmpowerBP:appropriateForPhysicalOpportunity rdf:datatype="http://www.w3.org/2001/XMLSchema#integer">3</EmpowerBP:appropriateForPhysicalOpportunity>
        <EmpowerBP:appropriateForPsychologicalCapability rdf:datatype="http://www.w3.org/2001/XMLSchema#integer">3</EmpowerBP:appropriateForPsychologicalCapability>
        <EmpowerBP:appropriateForReflectiveMotivation rdf:datatype="http://www.w3.org/2001/XMLSchema#integer">3</EmpowerBP:appropriateForReflectiveMotivation>
        <EmpowerBP:appropriateForSocialOpportunity rdf:datatype="http://www.w3.org/2001/XMLSchema#integer">3</EmpowerBP:appropriateForSocialOpportunity>
        <EmpowerBP:canRepeat rdf:datatype="http://www.w3.org/2001/XMLSchema#integer">26</EmpowerBP:canRepeat>
        <EmpowerBP:itemName rdf:datatype="http://www.w3.org/2001/XMLSchema#string">Salt and sodium - What’s the difference?</EmpowerBP:itemName>
        <EmpowerBP:itemText rdf:datatype="http://www.w3.org/2001/XMLSchema#string">• Salt is an ingredient we add to our food. We use it in the form of table salt, sea salt and in some seasonings.
• Sodium is one of the mineral nutrients. Sodium is found mainly in salt but it is also part of some food additives, such as MSG.
• We can find out the total amount of sodium in our foods by checking the Nutrition Facts label.</EmpowerBP:itemText>
        <EmpowerBP:maximumUserAge rdf:datatype="http://www.w3.org/2001/XMLSchema#integer">120</EmpowerBP:maximumUserAge>
        <EmpowerBP:minimumUserAge rdf:datatype="http://www.w3.org/2001/XMLSchema#integer">18</EmpowerBP:minimumUserAge>
        <EmpowerBP:provideJournal rdf:datatype="http://www.w3.org/2001/XMLSchema#boolean">false</EmpowerBP:provideJournal>
        <EmpowerBP:provideLink rdf:datatype="http://www.w3.org/2001/XMLSchema#boolean">false</EmpowerBP:provideLink>
        <EmpowerBP:sourceURL rdf:datatype="http://www.w3.org/2001/XMLSchema#string">http://www.hypertension.ca/images/2016_EducationalResources/2015_SaltAndSodiumGetTheFacts_EN_P1004_PREVIEW.pdf</EmpowerBP:sourceURL>
        <rdfs:comment rdf:datatype="http://www.w3.org/2001/XMLSchema#string">• Salt is an ingredient we add to our food. We use it in the form of table salt, sea salt and in some seasonings.
• Sodium is one of the mineral nutrients. Sodium is found mainly in salt but it is also part of some food additives, such as MSG.
• We can find out the total amount of sodium in our foods by checking the Nutrition Facts label.</rdfs:comment>
        <rdfs:label rdf:datatype="http://www.w3.org/2001/XMLSchema#string">Salt and sodium - What’s the difference?</rdfs:label>
    </owl:NamedIndividual>
    


    <!-- http://www.semanticweb.org/tswheeler/ontologies/2016/3/EmpowerBP#TPBadExercise -->

    <owl:NamedIndividual rdf:about="http://www.semanticweb.org/tswheeler/ontologies/2016/3/EmpowerBP#TPBadExercise">
        <rdf:type rdf:resource="http://www.semanticweb.org/tswheeler/ontologies/2016/3/EmpowerBP#Actor"/>
        <rdf:type rdf:resource="http://www.semanticweb.org/tswheeler/ontologies/2016/3/EmpowerBP#Patient"/>
        <EmpowerBP:hasInterventionGoal rdf:resource="http://www.semanticweb.org/tswheeler/ontologies/2016/3/EmpowerBP#ExerciseMore"/>
        <EmpowerBP:hasObstacle rdf:resource="http://www.semanticweb.org/tswheeler/ontologies/2016/3/EmpowerBP#MotivationObstacle"/>
        <EmpowerBP:hasObstacle rdf:resource="http://www.semanticweb.org/tswheeler/ontologies/2016/3/EmpowerBP#TimeObstacle"/>
        <EmpowerBP:AutomaticMotivationScore rdf:datatype="http://www.w3.org/2001/XMLSchema#integer">3</EmpowerBP:AutomaticMotivationScore>
        <EmpowerBP:PhyscologicalCapabilityScore rdf:datatype="http://www.w3.org/2001/XMLSchema#integer">3</EmpowerBP:PhyscologicalCapabilityScore>
        <EmpowerBP:PhysicalCapabilityScore rdf:datatype="http://www.w3.org/2001/XMLSchema#integer">3</EmpowerBP:PhysicalCapabilityScore>
        <EmpowerBP:PhysicalOpportunityScore rdf:datatype="http://www.w3.org/2001/XMLSchema#integer">3</EmpowerBP:PhysicalOpportunityScore>
        <EmpowerBP:ReflectiveMotivationScore rdf:datatype="http://www.w3.org/2001/XMLSchema#integer">3</EmpowerBP:ReflectiveMotivationScore>
        <EmpowerBP:SocialOpportunityScore rdf:datatype="http://www.w3.org/2001/XMLSchema#integer">3</EmpowerBP:SocialOpportunityScore>
        <EmpowerBP:actorHomeProvince rdf:datatype="http://www.w3.org/2001/XMLSchema#integer">6</EmpowerBP:actorHomeProvince>
        <EmpowerBP:actorName rdf:datatype="http://www.w3.org/2001/XMLSchema#string">Bad Runner</EmpowerBP:actorName>
        <EmpowerBP:age rdf:datatype="http://www.w3.org/2001/XMLSchema#integer">30</EmpowerBP:age>
        <EmpowerBP:dailySodiumIntake rdf:datatype="http://www.w3.org/2001/XMLSchema#integer">4000</EmpowerBP:dailySodiumIntake>
        <EmpowerBP:physicalActivityLevel rdf:datatype="http://www.w3.org/2001/XMLSchema#integer">30</EmpowerBP:physicalActivityLevel>
    </owl:NamedIndividual>
    


    <!-- http://www.semanticweb.org/tswheeler/ontologies/2016/3/EmpowerBP#TimeObstacle -->

    <owl:NamedIndividual rdf:about="http://www.semanticweb.org/tswheeler/ontologies/2016/3/EmpowerBP#TimeObstacle">
        <rdf:type rdf:resource="http://www.semanticweb.org/tswheeler/ontologies/2016/3/EmpowerBP#Obstacle"/>
        <EmpowerBP:hasRelevantTDF rdf:resource="http://www.semanticweb.org/tswheeler/ontologies/2016/3/EmpowerBP#BeliefsAboutConsequences"/>
        <EmpowerBP:hasRelevantTDF rdf:resource="http://www.semanticweb.org/tswheeler/ontologies/2016/3/EmpowerBP#EnvironmentalContextResources"/>
        <EmpowerBP:hasRelevantTDF rdf:resource="http://www.semanticweb.org/tswheeler/ontologies/2016/3/EmpowerBP#Goals"/>
        <EmpowerBP:hasRelevantTDF rdf:resource="http://www.semanticweb.org/tswheeler/ontologies/2016/3/EmpowerBP#Intentions"/>
        <EmpowerBP:hasRelevantTDF rdf:resource="http://www.semanticweb.org/tswheeler/ontologies/2016/3/EmpowerBP#Reinforcement"/>
        <rdfs:comment>Does not have enough time to perform activity.</rdfs:comment>
    </owl:NamedIndividual>
    


    <!-- http://www.semanticweb.org/tswheeler/ontologies/2016/3/EmpowerBP#Training -->

    <owl:NamedIndividual rdf:about="http://www.semanticweb.org/tswheeler/ontologies/2016/3/EmpowerBP#Training">
        <rdf:type rdf:resource="http://www.semanticweb.org/tswheeler/ontologies/2016/3/EmpowerBP#InterventionFuction"/>
        <EmpowerBP:hasCommonBCT rdf:resource="http://purl.bioontology.org/ontology/BCTT#Behavioral_experiments"/>
        <EmpowerBP:hasCommonBCT rdf:resource="http://purl.bioontology.org/ontology/BCTT#Biofeedback"/>
        <EmpowerBP:hasCommonBCT rdf:resource="http://purl.bioontology.org/ontology/BCTT#Graded_tasks"/>
        <EmpowerBP:hasCommonBCT rdf:resource="http://purl.bioontology.org/ontology/BCTT#Habit_formation"/>
        <EmpowerBP:hasCommonBCT rdf:resource="http://purl.bioontology.org/ontology/BCTT#Habit_reversal"/>
        <EmpowerBP:hasCommonBCT rdf:resource="http://purl.bioontology.org/ontology/BCTT#Mental_rehearsal_of_successful_performance"/>
        <EmpowerBP:hasCommonBCT rdf:resource="http://purl.bioontology.org/ontology/BCTT#Self-reward"/>
        <EmpowerBP:hasCommonBCT rdf:resource="http://purl.bioontology.org/ontology/BCTT#Self-talk"/>
        <EmpowerBP:hasCommonBCT rdf:resource="http://purl.bioontology.org/ontology/BCTT#Self-monitoring_of_outcome(s)_of_behaviour"/>
        <EmpowerBP:hasMostCommonBCT rdf:resource="http://purl.bioontology.org/ontology/BCTT#Behavioral_practice-rehearsal"/>
        <EmpowerBP:hasMostCommonBCT rdf:resource="http://purl.bioontology.org/ontology/BCTT#Demonstration_of_the_behavior"/>
        <EmpowerBP:hasMostCommonBCT rdf:resource="http://purl.bioontology.org/ontology/BCTT#Feedback_on_behaviour"/>
        <EmpowerBP:hasMostCommonBCT rdf:resource="http://purl.bioontology.org/ontology/BCTT#Instruction_on_how_to_perform_the_behavior"/>
        <EmpowerBP:hasMostCommonBCT rdf:resource="http://purl.bioontology.org/ontology/BCTT#Self-monitoring_of_behaviour"/>
        <EmpowerBP:hasMostCommonBCT rdf:resource="http://purl.bioontology.org/ontology/BCTT#Feedback_on_outcome(s)_of_behavior"/>
        <EmpowerBP:isEffectiveForTDFDomain rdf:resource="http://www.semanticweb.org/tswheeler/ontologies/2016/3/EmpowerBP#BehaviouralRegulation"/>
        <EmpowerBP:isEffectiveForTDFDomain rdf:resource="http://www.semanticweb.org/tswheeler/ontologies/2016/3/EmpowerBP#CognitiveInterpersonalSkills"/>
        <EmpowerBP:isEffectiveForTDFDomain rdf:resource="http://www.semanticweb.org/tswheeler/ontologies/2016/3/EmpowerBP#EnvironmentalContextResources"/>
        <EmpowerBP:isEffectiveForTDFDomain rdf:resource="http://www.semanticweb.org/tswheeler/ontologies/2016/3/EmpowerBP#MemoryAttentionDecisionProcesses"/>
        <EmpowerBP:isEffectiveForTDFDomain rdf:resource="http://www.semanticweb.org/tswheeler/ontologies/2016/3/EmpowerBP#PhysicalSkill"/>
        <EmpowerBP:isEffectiveForTDFDomain rdf:resource="http://www.semanticweb.org/tswheeler/ontologies/2016/3/EmpowerBP#Reinforcement"/>
        <rdfs:comment>Imparting skills.</rdfs:comment>
    </owl:NamedIndividual>
    


    <!-- http://www.semanticweb.org/tswheeler/ontologies/2016/3/EmpowerBP#WeatherObstacle -->

    <owl:NamedIndividual rdf:about="http://www.semanticweb.org/tswheeler/ontologies/2016/3/EmpowerBP#WeatherObstacle">
        <rdf:type rdf:resource="http://www.semanticweb.org/tswheeler/ontologies/2016/3/EmpowerBP#Obstacle"/>
        <EmpowerBP:hasRelevantTDF rdf:resource="http://www.semanticweb.org/tswheeler/ontologies/2016/3/EmpowerBP#EnvironmentalContextResources"/>
        <EmpowerBP:hasRelevantTDF rdf:resource="http://www.semanticweb.org/tswheeler/ontologies/2016/3/EmpowerBP#Knowledge"/>
        <rdfs:comment>Feels that weather prevents them from performing activity.</rdfs:comment>
    </owl:NamedIndividual>
    


    <!-- 
    ///////////////////////////////////////////////////////////////////////////////////////
    //
    // Annotations
    //
    ///////////////////////////////////////////////////////////////////////////////////////
     -->

    <rdf:Description rdf:about="http://www.w3.org/2000/01/rdf-schema#OWLAnnotationPropertyImpl_7da5e65b_da82_4f08_8ecf_0fc25b3b1e8c">
        <rdfs:label xml:lang="en">label</rdfs:label>
    </rdf:Description>
    <rdf:Description rdf:about="http://www.w3.org/2001/XMLSchema#OWLDatatypeImpl_0cca81fc_384b_4012_954f_29dc40ba7d2a">
        <rdfs:label xml:lang="en">string</rdfs:label>
    </rdf:Description>
</rdf:RDF>



<!-- Generated by the OWL API (version 4.2.8.20170104-2310) https://github.com/owlcs/owlapi -->

