<?xml version="1.0" encoding="UTF-8"?>
<rdf:RDF
   xmlns:owl="http://www.w3.org/2002/07/owl#"
   xmlns:rdf="http://www.w3.org/1999/02/22-rdf-syntax-ns#"
   xmlns:rdfs="http://www.w3.org/2000/01/rdf-schema#"
   xmlns:skos="http://www.w3.org/2004/02/skos/core#"
>
  <rdf:Description rdf:about="http://vocabularies.wikipathways.org/gpml#hasAnchor">
    <rdfs:range rdf:resource="http://vocabularies.wikipathways.org/gpml#GraphicalLine"/>
    <rdf:type rdf:resource="http://www.w3.org/2002/07/owl#ObjectProperty"/>
    <rdfs:comment xml:lang="en">Boolean property for the existence of an Anchor on a given line or interaction.</rdfs:comment>
    <rdfs:label xml:lang="en">hasAnchor</rdfs:label>
    <skos:inScheme rdf:resource="http://vocabularies.wikipathways.org/gpml#"/>
    <rdfs:range rdf:resource="http://vocabularies.wikipathways.org/gpml#Interaction"/>
    <rdfs:range rdf:resource="http://vocabularies.wikipathways.org/gpml#Anchor"/>
  </rdf:Description>
  <rdf:Description rdf:about="http://vocabularies.wikipathways.org/gpml#align">
    <rdfs:range rdf:resource="http://www.w3.org/2001/XMLSchema#string"/>
    <rdf:type rdf:resource="http://www.w3.org/2002/07/owl#DatatypeProperty"/>
    <rdfs:range rdf:resource="http://vocabularies.wikipathways.org/gpml#Label"/>
    <rdfs:range rdf:resource="http://vocabularies.wikipathways.org/gpml#Shape"/>
    <skos:inScheme rdf:resource="http://vocabularies.wikipathways.org/gpml#"/>
    <rdfs:label xml:lang="en">align</rdfs:label>
    <rdfs:comment xml:lang="en">Horizontal alignment of displayed text, e.g., Left, Center, Right.</rdfs:comment>
    <rdfs:range rdf:resource="http://vocabularies.wikipathways.org/gpml#DataNode"/>
  </rdf:Description>
  <rdf:Description rdf:about="http://vocabularies.wikipathways.org/gpml#">
    <rdf:type rdf:resource="http://www.w3.org/2004/02/skos/core#ConceptScheme"/>
    <owl:versionIRI rdf:resource="http://www.w3.org/2012/pyRdfa/extract?uri=http://vocabularies.wikipathways.org/gpml#"/>
    <rdfs:seeAlso rdf:resource="http://www.wikipathways.org/"/>
    <rdfs:label xml:lang="en">WikiPathways GPML Vocabulary</rdfs:label>
    <rdf:type rdf:resource="http://www.w3.org/2002/07/owl#Ontology"/>
  </rdf:Description>
  <rdf:Description rdf:about="http://vocabularies.wikipathways.org/gpml#Xref">
    <rdfs:comment xml:lang="en">Reference to a database entry that matches the node
in the pathway. It is a combination of an identifier of the entity and an
identifier of the database in which the entity is found.</rdfs:comment>
    <skos:inScheme rdf:resource="http://vocabularies.wikipathways.org/gpml#"/>
    <rdfs:label xml:lang="en">Xref</rdfs:label>
    <rdf:type rdf:resource="http://www.w3.org/2002/07/owl#Class"/>
  </rdf:Description>
  <rdf:Description rdf:about="http://vocabularies.wikipathways.org/gpml#GraphicalLine">
    <skos:inScheme rdf:resource="http://vocabularies.wikipathways.org/gpml#"/>
    <rdf:type rdf:resource="http://www.w3.org/2002/07/owl#Class"/>
    <rdfs:label xml:lang="en">GraphicalLine</rdfs:label>
    <rdfs:comment xml:lang="en">A visual annotation, often used to partition space or connect other annotation, e.g., Shapes. An Xref can not be specified for GraphicalLines (in contrast to Interactions).</rdfs:comment>
  </rdf:Description>
  <rdf:Description rdf:about="http://vocabularies.wikipathways.org/gpml#width">
    <rdfs:comment xml:lang="en">The pixel value for the x-dimensional length of a given object.</rdfs:comment>
    <rdfs:range rdf:resource="http://www.w3.org/2001/XMLSchema#float"/>
    <rdfs:range rdf:resource="http://vocabularies.wikipathways.org/gpml#State"/>
    <rdfs:range rdf:resource="http://vocabularies.wikipathways.org/gpml#Shape"/>
    <rdfs:range rdf:resource="http://vocabularies.wikipathways.org/gpml#Label"/>
    <skos:inScheme rdf:resource="http://vocabularies.wikipathways.org/gpml#"/>
    <rdf:type rdf:resource="http://www.w3.org/2002/07/owl#DatatypeProperty"/>
    <rdfs:label xml:lang="en">width</rdfs:label>
    <rdfs:range rdf:resource="http://vocabularies.wikipathways.org/gpml#DataNode"/>
  </rdf:Description>
  <rdf:Description rdf:about="http://vocabularies.wikipathways.org/gpml#centerY">
    <rdfs:range rdf:resource="http://vocabularies.wikipathways.org/gpml#InfoBox"/>
    <rdfs:range rdf:resource="http://www.w3.org/2001/XMLSchema#float"/>
    <rdfs:label xml:lang="en">centerY</rdfs:label>
    <rdf:type rdf:resource="http://www.w3.org/2002/07/owl#DatatypeProperty"/>
    <rdfs:range rdf:resource="http://vocabularies.wikipathways.org/gpml#DataNode"/>
    <rdfs:range rdf:resource="http://vocabularies.wikipathways.org/gpml#Legend"/>
    <skos:inScheme rdf:resource="http://vocabularies.wikipathways.org/gpml#"/>
    <rdfs:range rdf:resource="http://vocabularies.wikipathways.org/gpml#Label"/>
    <rdfs:comment xml:lang="en">Middle of a pathway element in the y-direction.</rdfs:comment>
    <rdfs:range rdf:resource="http://vocabularies.wikipathways.org/gpml#Shape"/>
  </rdf:Description>
  <rdf:Description rdf:about="http://vocabularies.wikipathways.org/gpml#hasPoint">
    <rdfs:range rdf:resource="http://vocabularies.wikipathways.org/gpml#Interaction"/>
    <rdfs:range rdf:resource="http://vocabularies.wikipathways.org/gpml#Point"/>
    <rdf:type rdf:resource="http://www.w3.org/2002/07/owl#ObjectProperty"/>
    <rdfs:label xml:lang="en">hasPoint</rdfs:label>
    <skos:inScheme rdf:resource="http://vocabularies.wikipathways.org/gpml#"/>
    <rdfs:comment xml:lang="en">Boolean property for the existence of a Point in a given line or interaction.</rdfs:comment>
    <rdfs:range rdf:resource="http://vocabularies.wikipathways.org/gpml#GraphicalLine"/>
  </rdf:Description>
  <rdf:Description rdf:about="http://vocabularies.wikipathways.org/gpml#fontDecoration">
    <rdfs:label xml:lang="en">fontDecoration</rdfs:label>
    <skos:inScheme rdf:resource="http://vocabularies.wikipathways.org/gpml#"/>
    <rdfs:range rdf:resource="http://www.w3.org/2001/XMLSchema#string"/>
    <rdf:type rdf:resource="http://www.w3.org/2002/07/owl#DatatypeProperty"/>
    <rdfs:range rdf:resource="http://vocabularies.wikipathways.org/gpml#Shape"/>
    <rdfs:comment xml:lang="en">Deprecated: Not in use.</rdfs:comment>
    <rdfs:range rdf:resource="http://vocabularies.wikipathways.org/gpml#Label"/>
  </rdf:Description>
  <rdf:Description rdf:about="http://vocabularies.wikipathways.org/gpml#fontStyle">
    <skos:inScheme rdf:resource="http://vocabularies.wikipathways.org/gpml#"/>
    <rdfs:range rdf:resource="http://vocabularies.wikipathways.org/gpml#DataNode"/>
    <rdf:type rdf:resource="http://www.w3.org/2002/07/owl#DatatypeProperty"/>
    <rdfs:comment xml:lang="en">The typographic style or font face applied to displayed text, e.g., Arial.</rdfs:comment>
    <rdfs:range rdf:resource="http://vocabularies.wikipathways.org/gpml#Shape"/>
    <rdfs:range rdf:resource="http://www.w3.org/2001/XMLSchema#string"/>
    <rdfs:range rdf:resource="http://vocabularies.wikipathways.org/gpml#Label"/>
    <rdfs:label xml:lang="en">fontStyle</rdfs:label>
  </rdf:Description>
  <rdf:Description rdf:about="http://vocabularies.wikipathways.org/gpml#textlabel">
    <rdfs:range rdf:resource="http://vocabularies.wikipathways.org/gpml#DataNode"/>
    <rdfs:range rdf:resource="http://vocabularies.wikipathways.org/gpml#State"/>
    <rdfs:label xml:lang="en">textlabel</rdfs:label>
    <rdfs:range rdf:resource="http://vocabularies.wikipathways.org/gpml#Group"/>
    <rdfs:range rdf:resource="http://www.w3.org/2001/XMLSchema#string"/>
    <rdf:type rdf:resource="http://www.w3.org/2002/07/owl#DatatypeProperty"/>
    <skos:inScheme rdf:resource="http://vocabularies.wikipathways.org/gpml#"/>
    <rdfs:range rdf:resource="http://vocabularies.wikipathways.org/gpml#Label"/>
    <rdfs:range rdf:resource="http://vocabularies.wikipathways.org/gpml#Shape"/>
    <rdfs:comment xml:lang="en">TextLabel of an object (DataNode, Group, Label, Shape, State).</rdfs:comment>
  </rdf:Description>
  <rdf:Description rdf:about="http://vocabularies.wikipathways.org/gpml#State">
    <rdfs:comment xml:lang="en">A particular condition, mode or modification of an entity, e.g., phosphorylated, activated, mutated, SNP, etc.</rdfs:comment>
    <skos:inScheme rdf:resource="http://vocabularies.wikipathways.org/gpml#"/>
    <rdf:type rdf:resource="http://www.w3.org/2002/07/owl#Class"/>
    <rdfs:label xml:lang="en">State</rdfs:label>
  </rdf:Description>
  <rdf:Description rdf:about="http://vocabularies.wikipathways.org/gpml#hasInfoBox">
    <rdfs:range rdf:resource="http://vocabularies.wikipathways.org/gpml#Pathway"/>
    <skos:inScheme rdf:resource="http://vocabularies.wikipathways.org/gpml#"/>
    <rdfs:range rdf:resource="http://vocabularies.wikipathways.org/gpml#InfoBox"/>
    <rdfs:comment xml:lang="en">Boolean property for the existence of an InfroBox in a given pathway.</rdfs:comment>
    <rdf:type rdf:resource="http://www.w3.org/2002/07/owl#ObjectProperty"/>
    <rdfs:label xml:lang="en">hasInfoBox</rdfs:label>
  </rdf:Description>
  <rdf:Description rdf:about="http://vocabularies.wikipathways.org/gpml#name">
    <rdfs:label xml:lang="en">name</rdfs:label>
    <rdf:type rdf:resource="http://www.w3.org/2002/07/owl#DatatypeProperty"/>
    <rdfs:comment xml:lang="en">The name of a pathway.</rdfs:comment>
    <rdfs:range rdf:resource="http://www.w3.org/2001/XMLSchema#string"/>
    <rdfs:range rdf:resource="http://vocabularies.wikipathways.org/gpml#Pathway"/>
    <skos:inScheme rdf:resource="http://vocabularies.wikipathways.org/gpml#"/>
  </rdf:Description>
  <rdf:Description rdf:about="http://vocabularies.wikipathways.org/gpml#last-Modified">
    <rdfs:range rdf:resource="http://www.w3.org/2001/XMLSchema#string"/>
    <rdfs:comment xml:lang="en">The date of the last modification of the pathway.</rdfs:comment>
    <rdf:type rdf:resource="http://www.w3.org/2002/07/owl#DatatypeProperty"/>
    <rdfs:range rdf:resource="http://vocabularies.wikipathways.org/gpml#Pathway"/>
    <skos:inScheme rdf:resource="http://vocabularies.wikipathways.org/gpml#"/>
    <rdfs:label xml:lang="en">last-Modified</rdfs:label>
  </rdf:Description>
  <rdf:Description rdf:about="http://vocabularies.wikipathways.org/gpml#value">
    <rdfs:range rdf:resource="http://vocabularies.wikipathways.org/gpml#Attribute"/>
    <rdfs:comment xml:lang="en">Value of the key/value pair in the Attribute class.</rdfs:comment>
    <rdfs:range rdf:resource="http://www.w3.org/2001/XMLSchema#string"/>
    <rdf:type rdf:resource="http://www.w3.org/2002/07/owl#DatatypeProperty"/>
    <rdfs:label xml:lang="en">value</rdfs:label>
    <skos:inScheme rdf:resource="http://vocabularies.wikipathways.org/gpml#"/>
  </rdf:Description>
  <rdf:Description rdf:about="http://vocabularies.wikipathways.org/gpml#Label">
    <rdf:type rdf:resource="http://www.w3.org/2002/07/owl#Class"/>
    <rdfs:Label xml:lang="en">Label</rdfs:Label>
    <rdfs:comment xml:lang="en">A text field which can be used to annotate any aspect of a pathway.</rdfs:comment>
    <skos:inScheme rdf:resource="http://vocabularies.wikipathways.org/gpml#"/>
  </rdf:Description>
  <rdf:Description rdf:about="http://vocabularies.wikipathways.org/gpml#color">
    <rdfs:range rdf:resource="http://vocabularies.wikipathways.org/gpml#Shape"/>
    <rdfs:range rdf:resource="http://vocabularies.wikipathways.org/gpml#Label"/>
    <rdfs:comment xml:lang="en">The color to be used for visualization.</rdfs:comment>
    <rdfs:range rdf:resource="http://www.w3.org/2001/XMLSchema#hexBinary"/>
    <rdf:type rdf:resource="http://www.w3.org/2002/07/owl#DatatypeProperty"/>
    <rdfs:range rdf:resource="http://vocabularies.wikipathways.org/gpml#GraphicalLine"/>
    <skos:inScheme rdf:resource="http://vocabularies.wikipathways.org/gpml#"/>
    <rdfs:label xml:lang="en">color</rdfs:label>
    <rdfs:range rdf:resource="http://vocabularies.wikipathways.org/gpml#State"/>
    <rdfs:range rdf:resource="http://vocabularies.wikipathways.org/gpml#DataNode"/>
    <rdfs:range rdf:resource="http://vocabularies.wikipathways.org/gpml#Interaction"/>
  </rdf:Description>
  <rdf:Description rdf:about="http://vocabularies.wikipathways.org/gpml#x">
    <rdfs:range rdf:resource="http://www.w3.org/2001/XMLSchema#float"/>
    <rdfs:comment xml:lang="en">The x-coordinate of a point in the 2-dimensional plane in which a pathway is drawn.</rdfs:comment>
    <rdfs:label xml:lang="en">x</rdfs:label>
    <rdfs:range rdf:resource="http://vocabularies.wikipathways.org/gpml#Point"/>
    <rdf:type rdf:resource="http://www.w3.org/2002/07/owl#DatatypeProperty"/>
    <skos:inScheme rdf:resource="http://vocabularies.wikipathways.org/gpml#"/>
  </rdf:Description>
  <rdf:Description rdf:about="http://vocabularies.wikipathways.org/gpml#groupRef">
    <rdfs:label xml:lang="en">groupRef</rdfs:label>
    <rdfs:range rdf:resource="http://www.w3.org/2001/XMLSchema#string"/>
    <rdf:type rdf:resource="http://www.w3.org/2002/07/owl#DatatypeProperty"/>
    <skos:inScheme rdf:resource="http://vocabularies.wikipathways.org/gpml#"/>
    <rdfs:range rdf:resource="http://vocabularies.wikipathways.org/gpml#DataNode"/>
    <rdfs:range rdf:resource="http://vocabularies.wikipathways.org/gpml#Shape"/>
    <rdfs:range rdf:resource="http://vocabularies.wikipathways.org/gpml#Group"/>
    <rdfs:range rdf:resource="http://vocabularies.wikipathways.org/gpml#Label"/>
    <rdfs:comment xml:lang="en">A GroupRef indicates that its element is part of the gpml:Group with the specified GroupId.
DataNode, GraphicalLine, Group, Interaction, Label and Shape can be part of a group.</rdfs:comment>
    <rdfs:range rdf:resource="http://vocabularies.wikipathways.org/gpml#Interaction"/>
    <rdfs:range rdf:resource="http://vocabularies.wikipathways.org/gpml#GraphicalLine"/>
  </rdf:Description>
  <rdf:Description rdf:about="http://vocabularies.wikipathways.org/gpml#href">
    <rdf:type rdf:resource="http://www.w3.org/2002/07/owl#DatatypeProperty"/>
    <rdfs:range rdf:resource="http://www.w3.org/2001/XMLSchema#string"/>
    <rdfs:label xml:lang="en">href</rdfs:label>
    <rdfs:range rdf:resource="http://vocabularies.wikipathways.org/gpml#Label"/>
    <skos:inScheme rdf:resource="http://vocabularies.wikipathways.org/gpml#"/>
    <rdfs:comment xml:lang="en">The hyperlink optionally specified in a Label.</rdfs:comment>
  </rdf:Description>
  <rdf:Description rdf:about="http://vocabularies.wikipathways.org/gpml#hasLabel">
    <rdfs:range rdf:resource="http://vocabularies.wikipathways.org/gpml#Pathway"/>
    <rdfs:range rdf:resource="http://vocabularies.wikipathways.org/gpml#Label"/>
    <rdfs:comment xml:lang="en">Boolean property for the existence of a Label in a given pathway.</rdfs:comment>
    <rdf:type rdf:resource="http://www.w3.org/2002/07/owl#ObjectProperty"/>
    <rdfs:label xml:lang="en">hasLabel</rdfs:label>
    <skos:inScheme rdf:resource="http://vocabularies.wikipathways.org/gpml#"/>
  </rdf:Description>
  <rdf:Description rdf:about="http://vocabularies.wikipathways.org/gpml#biopaxRef">
    <rdfs:label xml:lang="en">biopaxRef</rdfs:label>
    <rdfs:range rdf:resource="http://vocabularies.wikipathways.org/gpml#Interaction"/>
    <rdfs:range rdf:resource="http://www.w3.org/2001/XMLSchema#string"/>
    <rdf:type rdf:resource="http://www.w3.org/2002/07/owl#DatatypeProperty"/>
    <rdfs:range rdf:resource="http://vocabularies.wikipathways.org/gpml#Label"/>
    <rdfs:range rdf:resource="http://vocabularies.wikipathways.org/gpml#Shape"/>
    <rdfs:range rdf:resource="http://vocabularies.wikipathways.org/gpml#GraphicalLine"/>
    <rdfs:range rdf:resource="http://vocabularies.wikipathways.org/gpml#Pathway"/>
    <rdfs:range rdf:resource="http://vocabularies.wikipathways.org/gpml#DataNode"/>
    <rdfs:range rdf:resource="http://vocabularies.wikipathways.org/gpml#State"/>
    <rdfs:seeAlso rdf:resource="http://www.biopax.org/release/biopax-level3.owl#PublicationXref"/>
    <rdfs:comment xml:lang="en">Reuse of references defined by BioPAX.</rdfs:comment>
    <skos:inScheme rdf:resource="http://vocabularies.wikipathways.org/gpml#"/>
    <rdfs:range rdf:resource="http://vocabularies.wikipathways.org/gpml#Group"/>
  </rdf:Description>
  <rdf:Description rdf:about="http://vocabularies.wikipathways.org/gpml#Attribute">
    <rdfs:comment xml:lang="en">Element used to specify key/value paired information for a given object.</rdfs:comment>
    <skos:inScheme rdf:resource="http://vocabularies.wikipathways.org/gpml#"/>
    <rdfs:label xml:lang="en">Attribute</rdfs:label>
    <rdf:type rdf:resource="http://www.w3.org/2002/07/owl#Class"/>
  </rdf:Description>
  <rdf:Description rdf:about="http://vocabularies.wikipathways.org/gpml#boardHeight">
    <rdfs:comment xml:lang="en">Range minimum is zero.</rdfs:comment>
    <rdfs:range rdf:resource="http://www.w3.org/2001/XMLSchema#float"/>
    <skos:inScheme rdf:resource="http://vocabularies.wikipathways.org/gpml#"/>
    <rdfs:range rdf:resource="http://vocabularies.wikipathways.org/gpml#Pathway"/>
    <rdf:type rdf:resource="http://www.w3.org/2002/07/owl#DatatypeProperty"/>
    <rdfs:label xml:lang="en">boardHeight</rdfs:label>
  </rdf:Description>
  <rdf:Description rdf:about="http://vocabularies.wikipathways.org/gpml#valign">
    <rdf:type rdf:resource="http://www.w3.org/2002/07/owl#DatatypeProperty"/>
    <rdfs:range rdf:resource="http://vocabularies.wikipathways.org/gpml#DataNode"/>
    <rdfs:label xml:lang="en">valign</rdfs:label>
    <skos:inScheme rdf:resource="http://vocabularies.wikipathways.org/gpml#"/>
    <rdfs:comment xml:lang="en"> Vertical alignment of displayed text, e.g., Top, Middle, Bottom.</rdfs:comment>
    <rdfs:range rdf:resource="http://vocabularies.wikipathways.org/gpml#Shape"/>
    <rdfs:range rdf:resource="http://vocabularies.wikipathways.org/gpml#Label"/>
    <rdfs:range rdf:resource="http://www.w3.org/2001/XMLSchema#string"/>
  </rdf:Description>
  <rdf:Description rdf:about="http://vocabularies.wikipathways.org/gpml#fillColor">
    <rdfs:range rdf:resource="http://vocabularies.wikipathways.org/gpml#DataNode"/>
    <rdfs:label xml:lang="en">fillColor</rdfs:label>
    <rdfs:range rdf:resource="http://vocabularies.wikipathways.org/gpml#Shape"/>
    <rdfs:range rdf:resource="http://vocabularies.wikipathways.org/gpml#Label"/>
    <rdfs:comment xml:lang="en">The hexidecimal color value used to paint the area of an object, not including its border.</rdfs:comment>
    <skos:inScheme rdf:resource="http://vocabularies.wikipathways.org/gpml#"/>
    <rdf:type rdf:resource="http://www.w3.org/2002/07/owl#DatatypeProperty"/>
    <rdfs:range rdf:resource="http://www.w3.org/2001/XMLSchema#hexBinary"/>
    <rdfs:range rdf:resource="http://vocabularies.wikipathways.org/gpml#State"/>
  </rdf:Description>
  <rdf:Description rdf:about="http://vocabularies.wikipathways.org/gpml#style">
    <rdf:type rdf:resource="http://www.w3.org/2002/07/owl#DatatypeProperty"/>
    <rdfs:label xml:lang="en">style</rdfs:label>
    <rdfs:range rdf:resource="http://www.w3.org/2001/XMLSchema#string"/>
    <rdfs:range rdf:resource="http://vocabularies.wikipathways.org/gpml#Group"/>
    <skos:inScheme rdf:resource="http://vocabularies.wikipathways.org/gpml#"/>
    <rdfs:comment xml:lang="en">The type of Group, e.g., Complex.</rdfs:comment>
  </rdf:Description>
  <rdf:Description rdf:about="http://vocabularies.wikipathways.org/gpml#email">
    <rdfs:range rdf:resource="http://vocabularies.wikipathways.org/gpml#Pathway"/>
    <rdfs:range rdf:resource="http://www.w3.org/2001/XMLSchema#string"/>
    <rdf:type rdf:resource="http://www.w3.org/2002/07/owl#DatatypeProperty"/>
    <rdfs:label xml:lang="en">email</rdfs:label>
    <rdfs:comment xml:lang="en">Deprecated: An electronic mail address. Used to reference the author or maintainer of a pathway prior to WikiPathways.</rdfs:comment>
    <skos:inScheme rdf:resource="http://vocabularies.wikipathways.org/gpml#"/>
  </rdf:Description>
  <rdf:Description rdf:about="http://vocabularies.wikipathways.org/gpml#hasGraphicalLine">
    <rdfs:range rdf:resource="http://vocabularies.wikipathways.org/gpml#Pathway"/>
    <rdfs:label xml:lang="en">hasGraphicalLine</rdfs:label>
    <rdfs:comment xml:lang="en">Boolean property for the existence of a GraphicalLine in a given pathway.</rdfs:comment>
    <rdfs:range rdf:resource="http://vocabularies.wikipathways.org/gpml#GraphicalLine"/>
    <rdf:type rdf:resource="http://www.w3.org/2002/07/owl#ObjectProperty"/>
    <skos:inScheme rdf:resource="http://vocabularies.wikipathways.org/gpml#"/>
  </rdf:Description>
  <rdf:Description rdf:about="http://vocabularies.wikipathways.org/gpml#author">
    <rdfs:range rdf:resource="http://www.w3.org/2001/XMLSchema#string"/>
    <rdf:type rdf:resource="http://www.w3.org/2002/07/owl#DatatypeProperty"/>
    <rdfs:range rdf:resource="http://vocabularies.wikipathways.org/gpml#Pathway"/>
    <skos:inScheme rdf:resource="http://vocabularies.wikipathways.org/gpml#"/>
    <rdfs:label xml:lang="en">author</rdfs:label>
    <rdfs:comment xml:lang="en">The person who created or edited the pathway in question.</rdfs:comment>
  </rdf:Description>
  <rdf:Description rdf:about="http://vocabularies.wikipathways.org/gpml#graphRef">
    <rdfs:comment xml:lang="en">A GraphRef indicates a "depends on" or child/parent relationship between two Pathway elements. The element with the GraphRef is the child, and the element referred to by the GraphRef is the parent. The parent's GraphId will be specified by the child's GraphRef.</rdfs:comment>
    <rdfs:label xml:lang="en">graphRef</rdfs:label>
    <rdfs:range rdf:resource="http://www.w3.org/2001/XMLSchema#string"/>
    <skos:inScheme rdf:resource="http://vocabularies.wikipathways.org/gpml#"/>
    <rdfs:range rdf:resource="http://vocabularies.wikipathways.org/gpml#Point"/>
    <rdf:type rdf:resource="http://www.w3.org/2002/07/owl#DatatypeProperty"/>
    <rdfs:range rdf:resource="http://vocabularies.wikipathways.org/gpml#State"/>
  </rdf:Description>
  <rdf:Description rdf:about="http://vocabularies.wikipathways.org/gpml#Legend">
    <rdfs:comment xml:lang="en">An explanatory list of the colors used for visualizing data on the pathway. Not currently used.</rdfs:comment>
    <rdf:type rdf:resource="http://www.w3.org/2002/07/owl#Class"/>
    <rdfs:label xml:lang="en">Legend</rdfs:label>
    <skos:inScheme rdf:resource="http://vocabularies.wikipathways.org/gpml#"/>
  </rdf:Description>
  <rdf:Description rdf:about="http://vocabularies.wikipathways.org/gpml#fontWeight">
    <rdfs:range rdf:resource="http://www.w3.org/2001/XMLSchema#string"/>
    <rdf:type rdf:resource="http://www.w3.org/2002/07/owl#DatatypeProperty"/>
    <rdfs:range rdf:resource="http://vocabularies.wikipathways.org/gpml#Label"/>
    <rdfs:range rdf:resource="http://vocabularies.wikipathways.org/gpml#Shape"/>
    <rdfs:comment xml:lang="en">Thickness of the font used, e.g a bold font would have more weight. Used for DataNodes, Labels and Shapes.</rdfs:comment>
    <skos:inScheme rdf:resource="http://vocabularies.wikipathways.org/gpml#"/>
    <rdfs:label xml:lang="en">fontWeight</rdfs:label>
    <rdfs:range rdf:resource="http://vocabularies.wikipathways.org/gpml#DataNode"/>
  </rdf:Description>
  <rdf:Description rdf:about="http://vocabularies.wikipathways.org/gpml#hasDataNode">
    <rdfs:label xml:lang="en">hasDataNode</rdfs:label>
    <skos:inScheme rdf:resource="http://vocabularies.wikipathways.org/gpml#"/>
    <rdfs:range rdf:resource="http://vocabularies.wikipathways.org/gpml#Pathway"/>
    <rdfs:range rdf:resource="http://vocabularies.wikipathways.org/gpml#DataNode"/>
    <rdfs:comment xml:lang="en">Boolean property for the existence of a DataNode in a given pathway.</rdfs:comment>
    <rdf:type rdf:resource="http://www.w3.org/2002/07/owl#ObjectProperty"/>
  </rdf:Description>
  <rdf:Description rdf:about="http://vocabularies.wikipathways.org/gpml#relY">
    <rdfs:range rdf:resource="http://vocabularies.wikipathways.org/gpml#State"/>
    <rdfs:label xml:lang="en">relY</rdfs:label>
    <rdfs:range rdf:resource="http://vocabularies.wikipathways.org/gpml#Point"/>
    <rdf:type rdf:resource="http://www.w3.org/2002/07/owl#DatatypeProperty"/>
    <skos:inScheme rdf:resource="http://vocabularies.wikipathways.org/gpml#"/>
    <rdfs:comment xml:lang="en">RelY is the y-coordinate used when a point or state is linked to a another object - relative coordinate to the object that it is linked to (0,0 - center, 1,1 - bottom-right).</rdfs:comment>
    <rdfs:range rdf:resource="http://www.w3.org/2001/XMLSchema#float"/>
  </rdf:Description>
  <rdf:Description rdf:about="http://vocabularies.wikipathways.org/gpml#hasInteraction">
    <skos:inScheme rdf:resource="http://vocabularies.wikipathways.org/gpml#"/>
    <rdfs:label xml:lang="en">hasInteraction</rdfs:label>
    <rdfs:comment xml:lang="en">Boolean property for the existence of an Interaction in a given pathway.</rdfs:comment>
    <rdfs:range rdf:resource="http://vocabularies.wikipathways.org/gpml#Pathway"/>
    <rdf:type rdf:resource="http://www.w3.org/2002/07/owl#ObjectProperty"/>
    <rdfs:range rdf:resource="http://vocabularies.wikipathways.org/gpml#Interaction"/>
  </rdf:Description>
  <rdf:Description rdf:about="http://vocabularies.wikipathways.org/gpml#position">
    <rdfs:range rdf:resource="http://vocabularies.wikipathways.org/gpml#Anchor"/>
    <skos:inScheme rdf:resource="http://vocabularies.wikipathways.org/gpml#"/>
    <rdfs:range rdf:resource="http://www.w3.org/2001/XMLSchema#float"/>
    <rdf:type rdf:resource="http://www.w3.org/2002/07/owl#DatatypeProperty"/>
    <rdfs:comment xml:lang="en">Proportional distance of an anchor along the line it belongs to, between 0 and 1.</rdfs:comment>
    <rdfs:label xml:lang="en">position</rdfs:label>
  </rdf:Description>
  <rdf:Description rdf:about="http://vocabularies.wikipathways.org/gpml#hasPublicationXref">
    <rdfs:range rdf:resource="http://vocabularies.wikipathways.org/gpml#Interaction"/>
    <rdfs:range rdf:resource="http://vocabularies.wikipathways.org/gpml#Group"/>
    <rdfs:range rdf:resource="http://vocabularies.wikipathways.org/gpml#State"/>
    <rdfs:range rdf:resource="http://vocabularies.wikipathways.org/gpml#DataNode"/>
    <skos:inScheme rdf:resource="http://vocabularies.wikipathways.org/gpml#"/>
    <rdfs:comment xml:lang="en">Boolean property for the existence of a PublicationXref associated with a given object.</rdfs:comment>
    <rdfs:range rdf:resource="http://vocabularies.wikipathways.org/gpml#PublicationXref"/>
    <rdfs:range rdf:resource="http://vocabularies.wikipathways.org/gpml#GraphicalLine"/>
    <rdfs:label xml:lang="en">hasPublicationXref</rdfs:label>
    <rdf:type rdf:resource="http://www.w3.org/2002/07/owl#ObjectProperty"/>
    <rdfs:range rdf:resource="http://vocabularies.wikipathways.org/gpml#Shape"/>
    <rdfs:range rdf:resource="http://vocabularies.wikipathways.org/gpml#Label"/>
    <rdfs:range rdf:resource="http://vocabularies.wikipathways.org/gpml#Pathway"/>
  </rdf:Description>
  <rdf:Description rdf:about="http://vocabularies.wikipathways.org/gpml#source">
    <rdf:type rdf:resource="http://www.w3.org/2002/07/owl#DatatypeProperty"/>
    <rdfs:comment xml:lang="en">The author, reference or category of a comment. Used to help parse pathway-level comments, e.g., the descriptions displayed at WikiPathways.org are comments with source="WikiPathways-description".</rdfs:comment>
    <rdfs:label xml:lang="en">source</rdfs:label>
    <skos:inScheme rdf:resource="http://vocabularies.wikipathways.org/gpml#"/>
    <rdfs:range rdf:resource="http://www.w3.org/2001/XMLSchema#string"/>
    <rdfs:range rdf:resource="http://vocabularies.wikipathways.org/gpml#Commnet"/>
  </rdf:Description>
  <rdf:Description rdf:about="http://vocabularies.wikipathways.org/gpml#boardWidth">
    <rdfs:label xml:lang="en">boardWidth</rdfs:label>
    <rdf:type rdf:resource="http://www.w3.org/2002/07/owl#DatatypeProperty"/>
    <rdfs:comment xml:lang="en">Range minimum is zero.</rdfs:comment>
    <skos:inScheme rdf:resource="http://vocabularies.wikipathways.org/gpml#"/>
    <rdfs:range rdf:resource="http://www.w3.org/2001/XMLSchema#float"/>
    <rdfs:range rdf:resource="http://vocabularies.wikipathways.org/gpml#Pathway"/>
  </rdf:Description>
  <rdf:Description rdf:about="http://vocabularies.wikipathways.org/gpml#PublicationXref">
    <rdfs:label xml:lang="en">PublicationXref</rdfs:label>
    <rdfs:comment xml:lang="en">Defines a literature reference. Refers to a BioPAX definition.</rdfs:comment>
    <skos:inScheme rdf:resource="http://vocabularies.wikipathways.org/gpml#"/>
    <rdfs:seeAlso rdf:resource="http://www.biopax.org/owldoc/Level3/classes/PublicationXref___-1968381200.html"/>
    <rdf:type rdf:resource="http://www.w3.org/2002/07/owl#Class"/>
  </rdf:Description>
  <rdf:Description rdf:about="http://vocabularies.wikipathways.org/gpml#RequiresCurationAttention">
    <rdfs:label xml:lang="en">RequiresCurationAttention</rdfs:label>
    <skos:inScheme rdf:resource="http://vocabularies.wikipathways.org/gpml#"/>
    <rdfs:comment xml:lang="en">Deprecated: Not in use.</rdfs:comment>
    <rdf:type rdf:resource="http://www.w3.org/2002/07/owl#Class"/>
  </rdf:Description>
  <rdf:Description rdf:about="http://vocabularies.wikipathways.org/gpml#groupId">
    <rdfs:label xml:lang="en">groupId</rdfs:label>
    <skos:inScheme rdf:resource="http://vocabularies.wikipathways.org/gpml#"/>
    <rdfs:range rdf:resource="http://vocabularies.wikipathways.org/gpml#Group"/>
    <rdfs:range rdf:resource="http://www.w3.org/2001/XMLSchema#string"/>
    <rdf:type rdf:resource="http://www.w3.org/2002/07/owl#DatatypeProperty"/>
    <rdfs:comment xml:lang="en">Uniquely identifies a gpml:Group in a gpml:Pathway.</rdfs:comment>
  </rdf:Description>
  <rdf:Description rdf:about="http://vocabularies.wikipathways.org/gpml#hasXref">
    <rdfs:range rdf:resource="http://vocabularies.wikipathways.org/gpml#Xref"/>
    <rdfs:range rdf:resource="http://vocabularies.wikipathways.org/gpml#State"/>
    <skos:inScheme rdf:resource="http://vocabularies.wikipathways.org/gpml#"/>
    <rdfs:range rdf:resource="http://vocabularies.wikipathways.org/gpml#DataNode"/>
    <rdfs:label xml:lang="en">hasXref</rdfs:label>
    <rdfs:range rdf:resource="http://vocabularies.wikipathways.org/gpml#Interaction"/>
    <rdf:type rdf:resource="http://www.w3.org/2002/07/owl#ObjectProperty"/>
    <rdfs:comment xml:lang="en">Boolean property for the existence of an Xref associated with a given object.</rdfs:comment>
  </rdf:Description>
  <rdf:Description rdf:about="http://vocabularies.wikipathways.org/gpml#graphId">
    <rdfs:range rdf:resource="http://vocabularies.wikipathways.org/gpml#Label"/>
    <rdfs:range rdf:resource="http://vocabularies.wikipathways.org/gpml#Shape"/>
    <rdfs:range rdf:resource="http://www.w3.org/2001/XMLSchema#string"/>
    <rdfs:range rdf:resource="http://vocabularies.wikipathways.org/gpml#Anchor"/>
    <rdf:type rdf:resource="http://www.w3.org/2002/07/owl#DatatypeProperty"/>
    <rdfs:range rdf:resource="http://vocabularies.wikipathways.org/gpml#Point"/>
    <rdfs:range rdf:resource="http://vocabularies.wikipathways.org/gpml#GraphicalLine"/>
    <rdfs:label xml:lang="en">graphId</rdfs:label>
    <skos:inScheme rdf:resource="http://vocabularies.wikipathways.org/gpml#"/>
    <rdfs:range rdf:resource="http://vocabularies.wikipathways.org/gpml#DataNode"/>
    <rdfs:range rdf:resource="http://vocabularies.wikipathways.org/gpml#State"/>
    <rdfs:range rdf:resource="http://vocabularies.wikipathways.org/gpml#Group"/>
    <rdfs:range rdf:resource="http://vocabularies.wikipathways.org/gpml#Interaction"/>
    <rdfs:comment xml:lang="en">A GraphId is a unique (per Pathway) identifier for a pathway element, such as DataNode, Interaction, GraphicalLine, Label, Point, Group, Shape, State and Anchor.</rdfs:comment>
  </rdf:Description>
  <rdf:Description rdf:about="http://vocabularies.wikipathways.org/gpml#id">
    <rdfs:comment xml:lang="en">The identifier of a PublicationXref or Xref object.</rdfs:comment>
    <rdf:type rdf:resource="http://www.w3.org/2002/07/owl#DatatypeProperty"/>
    <rdfs:range rdf:resource="http://vocabularies.wikipathways.org/gpml#Xref"/>
    <rdfs:seeAlso rdf:resource="http://www.biopax.org/release/biopax-level3.owl#id"/>
    <rdfs:label xml:lang="en">id</rdfs:label>
    <rdfs:range rdf:resource="http://vocabularies.wikipathways.org/gpml#PublicationXref"/>
    <rdfs:range rdf:resource="http://www.w3.org/2001/XMLSchema#string"/>
    <skos:inScheme rdf:resource="http://vocabularies.wikipathways.org/gpml#"/>
  </rdf:Description>
  <rdf:Description rdf:about="http://vocabularies.wikipathways.org/gpml#hasBiopax">
    <rdfs:comment xml:lang="en">Boolean property for the existence of a BioPax class associated with a given pathway.</rdfs:comment>
    <rdfs:label xml:lang="en">hasBiopax</rdfs:label>
    <rdfs:range rdf:resource="http://vocabularies.wikipathways.org/gpml#Biopax"/>
    <skos:inScheme rdf:resource="http://vocabularies.wikipathways.org/gpml#"/>
    <rdf:type rdf:resource="http://www.w3.org/2002/07/owl#ObjectProperty"/>
    <rdfs:range rdf:resource="http://vocabularies.wikipathways.org/gpml#Pathway"/>
  </rdf:Description>
  <rdf:Description rdf:about="http://vocabularies.wikipathways.org/gpml#version">
    <rdfs:label xml:lang="en">version</rdfs:label>
    <skos:inScheme rdf:resource="http://vocabularies.wikipathways.org/gpml#"/>
    <rdfs:range rdf:resource="http://vocabularies.wikipathways.org/gpml#Pathway"/>
    <rdfs:range rdf:resource="http://www.w3.org/2001/XMLSchema#string"/>
    <rdfs:comment xml:lang="en">The version of a Pathway (currently not used in WP).</rdfs:comment>
    <rdf:type rdf:resource="http://www.w3.org/2002/07/owl#DatatypeProperty"/>
  </rdf:Description>
  <rdf:Description rdf:about="http://vocabularies.wikipathways.org/gpml#Group">
    <rdfs:comment xml:lang="en">A collection of structurally or functionally similar or related pathway elements.</rdfs:comment>
    <rdfs:label xml:lang="en">Group</rdfs:label>
    <skos:inScheme rdf:resource="http://vocabularies.wikipathways.org/gpml#"/>
    <rdf:type rdf:resource="http://www.w3.org/2002/07/owl#Class"/>
  </rdf:Description>
  <rdf:Description rdf:about="http://vocabularies.wikipathways.org/gpml#hasLegend">
    <skos:inScheme rdf:resource="http://vocabularies.wikipathways.org/gpml#"/>
    <rdfs:range rdf:resource="http://vocabularies.wikipathways.org/gpml#Pathway"/>
    <rdf:type rdf:resource="http://www.w3.org/2002/07/owl#ObjectProperty"/>
    <rdfs:label xml:lang="en">hasLegend</rdfs:label>
    <rdfs:range rdf:resource="http://vocabularies.wikipathways.org/gpml#Legend"/>
    <rdfs:comment xml:lang="en">Boolean property for the existence of a Legend in a given pathway.</rdfs:comment>
  </rdf:Description>
  <rdf:Description rdf:about="http://vocabularies.wikipathways.org/gpml#height">
    <rdfs:range rdf:resource="http://vocabularies.wikipathways.org/gpml#State"/>
    <rdf:type rdf:resource="http://www.w3.org/2002/07/owl#DatatypeProperty"/>
    <rdfs:range rdf:resource="http://vocabularies.wikipathways.org/gpml#Label"/>
    <rdfs:range rdf:resource="http://vocabularies.wikipathways.org/gpml#Shape"/>
    <rdfs:comment xml:lang="en">The pixel value for the y-dimensional length of a given object.</rdfs:comment>
    <rdfs:range rdf:resource="http://www.w3.org/2001/XMLSchema#float"/>
    <rdfs:label xml:lang="en">height</rdfs:label>
    <skos:inScheme rdf:resource="http://vocabularies.wikipathways.org/gpml#"/>
    <rdfs:range rdf:resource="http://vocabularies.wikipathways.org/gpml#DataNode"/>
  </rdf:Description>
  <rdf:Description rdf:about="http://vocabularies.wikipathways.org/gpml#hasAttribute">
    <skos:inScheme rdf:resource="http://vocabularies.wikipathways.org/gpml#"/>
    <rdfs:range rdf:resource="http://vocabularies.wikipathways.org/gpml#Shape"/>
    <rdfs:range rdf:resource="http://vocabularies.wikipathways.org/gpml#DataNode"/>
    <rdfs:range rdf:resource="http://vocabularies.wikipathways.org/gpml#Pathway"/>
    <rdfs:range rdf:resource="http://vocabularies.wikipathways.org/gpml#State"/>
    <rdfs:comment xml:lang="en">Boolean property for the existence of an Attribute class associated with a given object.</rdfs:comment>
    <rdf:type rdf:resource="http://www.w3.org/2002/07/owl#ObjectProperty"/>
    <rdfs:label xml:lang="en">hasAttribute</rdfs:label>
    <rdfs:range rdf:resource="http://vocabularies.wikipathways.org/gpml#Label"/>
    <rdfs:range rdf:resource="http://vocabularies.wikipathways.org/gpml#GraphicalLine"/>
    <rdfs:range rdf:resource="http://vocabularies.wikipathways.org/gpml#Group"/>
    <rdfs:range rdf:resource="http://vocabularies.wikipathways.org/gpml#Attribute"/>
    <rdfs:range rdf:resource="http://vocabularies.wikipathways.org/gpml#Interaction"/>
  </rdf:Description>
  <rdf:Description rdf:about="http://vocabularies.wikipathways.org/gpml#lineStyle">
    <skos:inScheme rdf:resource="http://vocabularies.wikipathways.org/gpml#"/>
    <rdfs:range rdf:resource="http://vocabularies.wikipathways.org/gpml#State"/>
    <rdfs:range rdf:resource="http://vocabularies.wikipathways.org/gpml#DataNode"/>
    <rdfs:label xml:lang="en">lineStyle</rdfs:label>
    <rdfs:range rdf:resource="http://vocabularies.wikipathways.org/gpml#Label"/>
    <rdfs:range rdf:resource="http://vocabularies.wikipathways.org/gpml#Interaction"/>
    <rdfs:range rdf:resource="http://vocabularies.wikipathways.org/gpml#Shape"/>
    <rdfs:comment xml:lang="en">The visual appearance of a line or border, e.g., Solid or Broken.</rdfs:comment>
    <rdf:type rdf:resource="http://www.w3.org/2002/07/owl#DatatypeProperty"/>
    <rdfs:range rdf:resource="http://www.w3.org/2001/XMLSchema#string"/>
    <rdfs:range rdf:resource="http://vocabularies.wikipathways.org/gpml#GraphicalLine"/>
  </rdf:Description>
  <rdf:Description rdf:about="http://vocabularies.wikipathways.org/gpml#hasState">
    <rdfs:range rdf:resource="http://vocabularies.wikipathways.org/gpml#Pathway"/>
    <skos:inScheme rdf:resource="http://vocabularies.wikipathways.org/gpml#"/>
    <rdfs:label xml:lang="en">hasState</rdfs:label>
    <rdf:type rdf:resource="http://www.w3.org/2002/07/owl#ObjectProperty"/>
    <rdfs:comment xml:lang="en">Boolean property for the existence of a State in a given pathway.</rdfs:comment>
    <rdfs:range rdf:resource="http://vocabularies.wikipathways.org/gpml#State"/>
  </rdf:Description>
  <rdf:Description rdf:about="http://vocabularies.wikipathways.org/gpml#arrowHead">
    <skos:inScheme rdf:resource="http://vocabularies.wikipathways.org/gpml#"/>
    <rdf:type rdf:resource="http://www.w3.org/2002/07/owl#DatatypeProperty"/>
    <rdfs:label xml:lang="en">arrowHead</rdfs:label>
    <rdfs:range rdf:resource="http://vocabularies.wikipathways.org/gpml#Point"/>
    <rdfs:range rdf:resource="http://www.w3.org/2001/XMLSchema#string"/>
    <rdfs:comment xml:lang="en">Specifies the glyph at the ends of lines and interactions.</rdfs:comment>
  </rdf:Description>
  <rdf:Description rdf:about="http://vocabularies.wikipathways.org/gpml#hasGroup">
    <rdfs:comment xml:lang="en">Boolean property for the existence of a Group in a given pathway.</rdfs:comment>
    <rdfs:range rdf:resource="http://vocabularies.wikipathways.org/gpml#Pathway"/>
    <skos:inScheme rdf:resource="http://vocabularies.wikipathways.org/gpml#"/>
    <rdf:type rdf:resource="http://www.w3.org/2002/07/owl#ObjectProperty"/>
    <rdfs:label xml:lang="en">hasGroup</rdfs:label>
    <rdfs:range rdf:resource="http://vocabularies.wikipathways.org/gpml#Group"/>
  </rdf:Description>
  <rdf:Description rdf:about="http://vocabularies.wikipathways.org/gpml#database">
    <rdfs:range rdf:resource="http://www.w3.org/2001/XMLSchema#string"/>
    <rdfs:seeAlso rdf:resource="http://vocabularies.bridgedb.org/ops#DataSource"/>
    <rdfs:range rdf:resource="http://vocabularies.wikipathways.org/gpml#Xref"/>
    <rdf:type rdf:resource="http://www.w3.org/2002/07/owl#DatatypeProperty"/>
    <rdfs:comment xml:lang="en">Specifies the datasource for the identifier provided as an Xref.  Equivalent to http://vocabularies.bridgedb.org/ops#DataSource conventional name .</rdfs:comment>
    <skos:inScheme rdf:resource="http://vocabularies.wikipathways.org/gpml#"/>
    <rdfs:label xml:lang="en">database</rdfs:label>
  </rdf:Description>
  <rdf:Description rdf:about="http://vocabularies.wikipathways.org/gpml#hasComment">
    <rdfs:comment xml:lang="en">Boolean property for the existence of a Comment class associated with a given object.</rdfs:comment>
    <skos:inScheme rdf:resource="http://vocabularies.wikipathways.org/gpml#"/>
    <rdfs:range rdf:resource="http://vocabularies.wikipathways.org/gpml#State"/>
    <rdfs:label xml:lang="en">hasComment</rdfs:label>
    <rdfs:range rdf:resource="http://vocabularies.wikipathways.org/gpml#GraphicalLine"/>
    <rdfs:range rdf:resource="http://vocabularies.wikipathways.org/gpml#Shape"/>
    <rdfs:range rdf:resource="http://vocabularies.wikipathways.org/gpml#Pathway"/>
    <rdf:type rdf:resource="http://www.w3.org/2002/07/owl#ObjectProperty"/>
    <rdfs:range rdf:resource="http://vocabularies.wikipathways.org/gpml#DataNode"/>
    <rdfs:range rdf:resource="http://vocabularies.wikipathways.org/gpml#Comment"/>
    <rdfs:range rdf:resource="http://vocabularies.wikipathways.org/gpml#Label"/>
    <rdfs:range rdf:resource="http://vocabularies.wikipathways.org/gpml#Group"/>
    <rdfs:range rdf:resource="http://vocabularies.wikipathways.org/gpml#Interaction"/>
  </rdf:Description>
  <rdf:Description rdf:about="http://vocabularies.wikipathways.org/gpml#InfoBox">
    <rdf:type rdf:resource="http://www.w3.org/2002/07/owl#Class"/>
    <rdfs:comment xml:lang="en">Currently just a placeholder -- not used.</rdfs:comment>
    <skos:inScheme rdf:resource="http://vocabularies.wikipathways.org/gpml#"/>
    <rdfs:label xml:lang="en">InfoBox</rdfs:label>
  </rdf:Description>
  <rdf:Description rdf:about="http://vocabularies.wikipathways.org/gpml#zorder">
    <rdfs:range rdf:resource="http://vocabularies.wikipathways.org/gpml#Label"/>
    <rdfs:range rdf:resource="http://vocabularies.wikipathways.org/gpml#Shape"/>
    <rdf:type rdf:resource="http://www.w3.org/2002/07/owl#DatatypeProperty"/>
    <rdfs:range rdf:resource="http://vocabularies.wikipathways.org/gpml#GraphicalLine"/>
    <rdfs:label xml:lang="en">zorder</rdfs:label>
    <skos:inScheme rdf:resource="http://vocabularies.wikipathways.org/gpml#"/>
    <rdfs:range rdf:resource="http://vocabularies.wikipathways.org/gpml#DataNode"/>
    <rdfs:range rdf:resource="http://vocabularies.wikipathways.org/gpml#State"/>
    <rdfs:range rdf:resource="http://www.w3.org/2001/XMLSchema#integer"/>
    <rdfs:range rdf:resource="http://vocabularies.wikipathways.org/gpml#Interaction"/>
    <rdfs:comment xml:lang="en">Indicates the zorder of the object in the pathway.</rdfs:comment>
  </rdf:Description>
  <rdf:Description rdf:about="http://vocabularies.wikipathways.org/gpml#lineThickness">
    <rdfs:range rdf:resource="http://vocabularies.wikipathways.org/gpml#State"/>
    <rdfs:range rdf:resource="http://vocabularies.wikipathways.org/gpml#DataNode"/>
    <skos:inScheme rdf:resource="http://vocabularies.wikipathways.org/gpml#"/>
    <rdf:type rdf:resource="http://www.w3.org/2002/07/owl#DatatypeProperty"/>
    <rdfs:comment xml:lang="en">The pixel value for the width of a given line, interaction or border.</rdfs:comment>
    <rdfs:label xml:lang="en">lineThickness</rdfs:label>
    <rdfs:range rdf:resource="http://vocabularies.wikipathways.org/gpml#Interaction"/>
    <rdfs:range rdf:resource="http://www.w3.org/2001/XMLSchema#string"/>
    <rdfs:range rdf:resource="http://vocabularies.wikipathways.org/gpml#Shape"/>
    <rdfs:range rdf:resource="http://vocabularies.wikipathways.org/gpml#GraphicalLine"/>
    <rdfs:range rdf:resource="http://vocabularies.wikipathways.org/gpml#Label"/>
  </rdf:Description>
  <rdf:Description rdf:about="http://vocabularies.wikipathways.org/gpml#key">
    <rdfs:range rdf:resource="http://vocabularies.wikipathways.org/gpml#Attribute"/>
    <skos:inScheme rdf:resource="http://vocabularies.wikipathways.org/gpml#"/>
    <rdfs:label xml:lang="en">key</rdfs:label>
    <rdfs:comment xml:lang="en">Key of the key/value pair in the Attribute class.</rdfs:comment>
    <rdfs:range rdf:resource="http://www.w3.org/2001/XMLSchema#string"/>
    <rdf:type rdf:resource="http://www.w3.org/2002/07/owl#DatatypeProperty"/>
  </rdf:Description>
  <rdf:Description rdf:about="http://vocabularies.wikipathways.org/gpml#relX">
    <rdfs:range rdf:resource="http://www.w3.org/2001/XMLSchema#float"/>
    <rdfs:comment xml:lang="en">RelX is the x-coordinate used when a point or state is linked to a another object - relative coordinate to the object that it is linked to (0,0 - center, 1,1 - bottom-right).</rdfs:comment>
    <rdfs:label xml:lang="en">relX</rdfs:label>
    <rdfs:range rdf:resource="http://vocabularies.wikipathways.org/gpml#Point"/>
    <rdf:type rdf:resource="http://www.w3.org/2002/07/owl#DatatypeProperty"/>
    <skos:inScheme rdf:resource="http://vocabularies.wikipathways.org/gpml#"/>
    <rdfs:range rdf:resource="http://vocabularies.wikipathways.org/gpml#State"/>
  </rdf:Description>
  <rdf:Description rdf:about="http://vocabularies.wikipathways.org/gpml#Shape">
    <rdf:type rdf:resource="http://www.w3.org/2002/07/owl#Class"/>
    <skos:inScheme rdf:resource="http://vocabularies.wikipathways.org/gpml#"/>
    <rdfs:label xml:lang="en">Shape</rdfs:label>
    <rdfs:comment xml:lang="en">Shape can refer to two different things in GPML, both of which are associated with graphical elements.</rdfs:comment>
  </rdf:Description>
  <rdf:Description rdf:about="http://vocabularies.wikipathways.org/gpml#centerX">
    <rdfs:label xml:lang="en">centerX</rdfs:label>
    <rdfs:range rdf:resource="http://vocabularies.wikipathways.org/gpml#Legend"/>
    <rdfs:range rdf:resource="http://vocabularies.wikipathways.org/gpml#InfoBox"/>
    <skos:inScheme rdf:resource="http://vocabularies.wikipathways.org/gpml#"/>
    <rdfs:range rdf:resource="http://vocabularies.wikipathways.org/gpml#Shape"/>
    <rdf:type rdf:resource="http://www.w3.org/2002/07/owl#DatatypeProperty"/>
    <rdfs:range rdf:resource="http://vocabularies.wikipathways.org/gpml#Label"/>
    <rdfs:comment xml:lang="en">Middle of a pathway element in the x-direction.</rdfs:comment>
    <rdfs:range rdf:resource="http://www.w3.org/2001/XMLSchema#float"/>
    <rdfs:range rdf:resource="http://vocabularies.wikipathways.org/gpml#DataNode"/>
  </rdf:Description>
  <rdf:Description rdf:about="http://vocabularies.wikipathways.org/gpml#shapeType">
    <rdfs:comment xml:lang="en">Currently: Specifies the glyph (graphical representation) to use for GPML elements (DataNode, Label, Shape, State).

Proposed: Expand it to also describe Anchors. It should replace the term currently used to specify the graphical representation of an Anchor. The current term is "Shape," which conflicts with the GPML element named "Shape." See details for term "Shape."</rdfs:comment>
    <rdfs:range rdf:resource="http://www.w3.org/2001/XMLSchema#string"/>
    <skos:inScheme rdf:resource="http://vocabularies.wikipathways.org/gpml#"/>
    <rdfs:range rdf:resource="http://vocabularies.wikipathways.org/gpml#DataNode"/>
    <rdfs:range rdf:resource="http://vocabularies.wikipathways.org/gpml#State"/>
    <rdfs:range rdf:resource="http://vocabularies.wikipathways.org/gpml#Label"/>
    <rdfs:range rdf:resource="http://vocabularies.wikipathways.org/gpml#Shape"/>
    <rdfs:label xml:lang="en">shapeType</rdfs:label>
    <rdf:type rdf:resource="http://www.w3.org/2002/07/owl#DatatypeProperty"/>
  </rdf:Description>
  <rdf:Description rdf:about="http://vocabularies.wikipathways.org/gpml#hasShape">
    <rdfs:comment xml:lang="en">Boolean property for the existence of a Shape in a given pathway.</rdfs:comment>
    <rdfs:range rdf:resource="http://vocabularies.wikipathways.org/gpml#Pathway"/>
    <skos:inScheme rdf:resource="http://vocabularies.wikipathways.org/gpml#"/>
    <rdf:type rdf:resource="http://www.w3.org/2002/07/owl#ObjectProperty"/>
    <rdfs:label xml:lang="en">hasShape</rdfs:label>
    <rdfs:range rdf:resource="http://vocabularies.wikipathways.org/gpml#Shape"/>
  </rdf:Description>
  <rdf:Description rdf:about="http://vocabularies.wikipathways.org/gpml#organism">
    <rdfs:range rdf:resource="http://www.w3.org/2001/XMLSchema#string"/>
    <rdfs:label xml:lang="en">organism</rdfs:label>
    <rdfs:range rdf:resource="http://vocabularies.wikipathways.org/gpml#Pathway"/>
    <skos:inScheme rdf:resource="http://vocabularies.wikipathways.org/gpml#"/>
    <rdf:type rdf:resource="http://www.w3.org/2002/07/owl#DatatypeProperty"/>
    <rdfs:comment xml:lang="en">The scientific name (e.g., Homo sapiens) of the species being described by the pathway.</rdfs:comment>
  </rdf:Description>
  <rdf:Description rdf:about="http://vocabularies.wikipathways.org/gpml#data-Source">
    <rdf:type rdf:resource="http://www.w3.org/2002/07/owl#DatatypeProperty"/>
    <rdfs:comment xml:lang="en">Deprecated: Not in use.</rdfs:comment>
    <rdfs:range rdf:resource="http://vocabularies.wikipathways.org/gpml#Pathway"/>
    <skos:inScheme rdf:resource="http://vocabularies.wikipathways.org/gpml#"/>
    <rdfs:label xml:lang="en">data-Source</rdfs:label>
    <rdfs:range rdf:resource="http://www.w3.org/2001/XMLSchema#string"/>
  </rdf:Description>
  <rdf:Description rdf:about="http://vocabularies.wikipathways.org/gpml#connectorType">
    <skos:inScheme rdf:resource="http://vocabularies.wikipathways.org/gpml#"/>
    <rdfs:comment xml:lang="en">Specifies a set of rules to govern layout of Graphical Lines and Interactions.  PathVisio (Java): Line Type and GPML: ConnectorType</rdfs:comment>
    <rdf:type rdf:resource="http://www.w3.org/2002/07/owl#DatatypeProperty"/>
    <rdfs:range rdf:resource="http://vocabularies.wikipathways.org/gpml#GraphicalLine"/>
    <rdfs:range rdf:resource="http://www.w3.org/2001/XMLSchema#string"/>
    <rdfs:range rdf:resource="http://vocabularies.wikipathways.org/gpml#Interaction"/>
    <rdfs:label xml:lang="en">connectorType</rdfs:label>
  </rdf:Description>
  <rdf:Description rdf:about="http://vocabularies.wikipathways.org/gpml#DataNode">
    <rdfs:comment xml:lang="en">Denotes a biological entity that forms a node in a pathway and has some biological meaning associated with it. For a list of the gpml:DataNode types supported at WikiPathways, see subclasses of wp:DataNode or the wpTypes vocabulary defined for use in applications..</rdfs:comment>
    <rdfs:label xml:lang="en">DataNode</rdfs:label>
    <rdf:type rdf:resource="http://www.w3.org/2002/07/owl#Class"/>
    <skos:inScheme rdf:resource="http://vocabularies.wikipathways.org/gpml#"/>
  </rdf:Description>
  <rdf:Description rdf:about="http://vocabularies.wikipathways.org/gpml#y">
    <rdfs:comment xml:lang="en">The y-coordinate of a point in the 2-dimensional plane in which a pathway is drawn.</rdfs:comment>
    <rdfs:label xml:lang="en">y</rdfs:label>
    <skos:inScheme rdf:resource="http://vocabularies.wikipathways.org/gpml#"/>
    <rdf:type rdf:resource="http://www.w3.org/2002/07/owl#DatatypeProperty"/>
    <rdfs:range rdf:resource="http://www.w3.org/2001/XMLSchema#float"/>
    <rdfs:range rdf:resource="http://vocabularies.wikipathways.org/gpml#Point"/>
  </rdf:Description>
  <rdf:Description rdf:about="http://vocabularies.wikipathways.org/gpml#license">
    <rdf:type rdf:resource="http://www.w3.org/2002/07/owl#DatatypeProperty"/>
    <rdfs:range rdf:resource="http://vocabularies.wikipathways.org/gpml#Pathway"/>
    <rdfs:comment xml:lang="en">The license of a pathway.</rdfs:comment>
    <rdfs:range rdf:resource="http://www.w3.org/2001/XMLSchema#string"/>
    <skos:inScheme rdf:resource="http://vocabularies.wikipathways.org/gpml#"/>
    <rdfs:label xml:lang="en">license</rdfs:label>
  </rdf:Description>
  <rdf:Description rdf:about="http://vocabularies.wikipathways.org/gpml#Pathway">
    <rdf:type rdf:resource="http://www.w3.org/2002/07/owl#Class"/>
    <rdfs:label xml:lang="en">Pathway</rdfs:label>
    <rdfs:comment xml:lang="en">A graph diagram representing a biological process as a set of interactions and relationships among genes, proteins, metabolites, and other factors in the context of cellular compartments, tissues and organisms.</rdfs:comment>
    <skos:inScheme rdf:resource="http://vocabularies.wikipathways.org/gpml#"/>
  </rdf:Description>
  <rdf:Description rdf:about="http://vocabularies.wikipathways.org/gpml#shape">
    <rdfs:label xml:lang="en">shape</rdfs:label>
    <rdfs:range rdf:resource="http://www.w3.org/2001/XMLSchema#string"/>
    <rdf:type rdf:resource="http://www.w3.org/2002/07/owl#DatatypeProperty"/>
    <rdfs:comment xml:lang="en">The visual representation of an anchor, e.g., Circle or None.</rdfs:comment>
    <skos:inScheme rdf:resource="http://vocabularies.wikipathways.org/gpml#"/>
    <rdfs:range rdf:resource="http://vocabularies.wikipathways.org/gpml#Anchor"/>
  </rdf:Description>
  <rdf:Description rdf:about="http://vocabularies.wikipathways.org/gpml#fontSize">
    <skos:inScheme rdf:resource="http://vocabularies.wikipathways.org/gpml#"/>
    <rdfs:label xml:lang="en">fontSize</rdfs:label>
    <rdfs:range rdf:resource="http://vocabularies.wikipathways.org/gpml#Label"/>
    <rdfs:range rdf:resource="http://vocabularies.wikipathways.org/gpml#Shape"/>
    <rdfs:comment xml:lang="en">The point value for the size of the font.</rdfs:comment>
    <rdf:type rdf:resource="http://www.w3.org/2002/07/owl#DatatypeProperty"/>
    <rdfs:range rdf:resource="http://www.w3.org/2001/XMLSchema#nonNegativeInteger"/>
  </rdf:Description>
  <rdf:Description rdf:about="http://vocabularies.wikipathways.org/gpml#rotation">
    <rdf:type rdf:resource="http://www.w3.org/2002/07/owl#DatatypeProperty"/>
    <rdfs:label xml:lang="en">rotation</rdfs:label>
    <rdfs:comment xml:lang="en">The degree value of angular offset relative to the center of a given object.</rdfs:comment>
    <rdfs:range rdf:resource="http://vocabularies.wikipathways.org/gpml#Shape"/>
    <rdfs:range rdf:resource="http://www.w3.org/2001/XMLSchema#float"/>
    <skos:inScheme rdf:resource="http://vocabularies.wikipathways.org/gpml#"/>
  </rdf:Description>
  <rdf:Description rdf:about="http://vocabularies.wikipathways.org/gpml#Anchor">
    <skos:inScheme rdf:resource="http://vocabularies.wikipathways.org/gpml#"/>
    <rdfs:comment xml:lang="en">A connection point on a graphical line or an interaction, where another graphical line or interaction can be connected.</rdfs:comment>
    <rdfs:label xml:lang="en">Anchor</rdfs:label>
    <rdf:type rdf:resource="http://www.w3.org/2002/07/owl#Class"/>
  </rdf:Description>
  <rdf:Description rdf:about="http://vocabularies.wikipathways.org/gpml#fontStrikethru">
    <rdfs:range rdf:resource="http://www.w3.org/2001/XMLSchema#string"/>
    <rdf:type rdf:resource="http://www.w3.org/2002/07/owl#DatatypeProperty"/>
    <rdfs:label xml:lang="en">fontStrikethru</rdfs:label>
    <rdfs:range rdf:resource="http://vocabularies.wikipathways.org/gpml#Label"/>
    <rdfs:range rdf:resource="http://vocabularies.wikipathways.org/gpml#Shape"/>
    <rdfs:range rdf:resource="http://vocabularies.wikipathways.org/gpml#DataNode"/>
    <skos:inScheme rdf:resource="http://vocabularies.wikipathways.org/gpml#"/>
    <rdfs:comment xml:lang="en">Deprecated: Not in use.</rdfs:comment>
  </rdf:Description>
  <rdf:Description rdf:about="http://vocabularies.wikipathways.org/gpml#type">
    <rdfs:range rdf:resource="http://vocabularies.wikipathways.org/gpml#DataNode"/>
    <rdfs:label xml:lang="en">type</rdfs:label>
    <rdfs:range rdf:resource="http://www.w3.org/2001/XMLSchema#string"/>
    <rdfs:range rdf:resource="http://vocabularies.wikipathways.org/gpml#Interaction"/>
    <rdfs:range rdf:resource="http://vocabularies.wikipathways.org/gpml#GraphicalLine"/>
    <skos:inScheme rdf:resource="http://vocabularies.wikipathways.org/gpml#"/>
    <rdfs:comment xml:lang="en">Specifies the type of an object (DataNode, GraphicalLine, Interaction).</rdfs:comment>
    <rdf:type rdf:resource="http://www.w3.org/2002/07/owl#DatatypeProperty"/>
  </rdf:Description>
  <rdf:Description rdf:about="http://vocabularies.wikipathways.org/gpml#Point">
    <skos:inScheme rdf:resource="http://vocabularies.wikipathways.org/gpml#"/>
    <rdfs:label xml:lang="en">Point</rdfs:label>
    <rdfs:comment xml:lang="en">A location in 2-dimensional space defined by x and y coordinates.</rdfs:comment>
    <rdf:type rdf:resource="http://www.w3.org/2002/07/owl#Class"/>
  </rdf:Description>
  <rdf:Description rdf:about="http://vocabularies.wikipathways.org/gpml#Interaction">
    <skos:inScheme rdf:resource="http://vocabularies.wikipathways.org/gpml#"/>
    <rdf:type rdf:resource="http://www.w3.org/2002/07/owl#Class"/>
    <rdfs:comment xml:lang="en">Defines the biochemical relationship between DataNodes or with Anchors on other Interactions. An Xref can be specified for Interactions (in contrast to GraphicalLines).</rdfs:comment>
    <rdfs:label xml:lang="en">Interaction</rdfs:label>
  </rdf:Description>
  <rdf:Description rdf:about="http://vocabularies.wikipathways.org/gpml#maintainer">
    <rdfs:label xml:lang="en">maintainer</rdfs:label>
    <skos:inScheme rdf:resource="http://vocabularies.wikipathways.org/gpml#"/>
    <rdfs:comment xml:lang="en">The maintainer of the pathway. Currently not used in WP.</rdfs:comment>
    <rdf:type rdf:resource="http://www.w3.org/2002/07/owl#DatatypeProperty"/>
    <rdfs:range rdf:resource="http://vocabularies.wikipathways.org/gpml#Pathway"/>
    <rdfs:range rdf:resource="http://www.w3.org/2001/XMLSchema#string"/>
  </rdf:Description>
  <rdf:Description rdf:about="http://vocabularies.wikipathways.org/gpml#Comment">
    <rdfs:label xml:lang="en">Comment</rdfs:label>
    <skos:inScheme rdf:resource="http://vocabularies.wikipathways.org/gpml#"/>
    <rdfs:comment xml:lang="en">Elements used to provide descriptions and arbitrary notes for a given object.</rdfs:comment>
    <rdf:type rdf:resource="http://www.w3.org/2002/07/owl#Class"/>
  </rdf:Description>
  <rdf:Description rdf:about="http://vocabularies.wikipathways.org/gpml#fontName">
    <rdfs:range rdf:resource="http://vocabularies.wikipathways.org/gpml#Label"/>
    <rdfs:label xml:lang="en">fontName</rdfs:label>
    <skos:inScheme rdf:resource="http://vocabularies.wikipathways.org/gpml#"/>
    <rdf:type rdf:resource="http://www.w3.org/2002/07/owl#DatatypeProperty"/>
    <rdfs:comment xml:lang="en">The name of the set of printable text characters to be used for visualization.</rdfs:comment>
    <rdfs:range rdf:resource="http://www.w3.org/2001/XMLSchema#string"/>
    <rdfs:range rdf:resource="http://vocabularies.wikipathways.org/gpml#Shape"/>
  </rdf:Description>
  <rdf:Description rdf:about="http://vocabularies.wikipathways.org/gpml#stateType">
    <skos:inScheme rdf:resource="http://vocabularies.wikipathways.org/gpml#"/>
    <rdfs:comment xml:lang="en">A free text field to describe the nature or category of a given state.</rdfs:comment>
    <rdf:type rdf:resource="http://www.w3.org/2002/07/owl#DatatypeProperty"/>
    <rdfs:range rdf:resource="http://vocabularies.wikipathways.org/gpml#State"/>
    <rdfs:range rdf:resource="http://www.w3.org/2001/XMLSchema#string"/>
    <rdfs:label xml:lang="en">stateType</rdfs:label>
  </rdf:Description>
  <rdf:Description rdf:about="http://vocabularies.wikipathways.org/gpml#Biopax">
    <rdf:type rdf:resource="http://www.w3.org/2002/07/owl#Class"/>
    <skos:inScheme rdf:resource="http://vocabularies.wikipathways.org/gpml#"/>
    <rdfs:comment xml:lang="en">Element used to embed Biopax (namespace: http://www.biopax.org/release/biopax-level3.owl) content in a GPML document.</rdfs:comment>
    <rdfs:label xml:lang="en">Biopax</rdfs:label>
  </rdf:Description>
</rdf:RDF>
