@prefix : <file:///ERROR/EMPTY/PREFIX/BANNED/> .
@prefix BFO: <http://purl.obolibrary.org/obo/BFO_> .
@prefix BIRNLEX: <http://uri.neuinfo.org/nif/nifstd/birnlex_> .
@prefix dc: <http://purl.org/dc/elements/1.1/> .
@prefix NIFRID: <http://uri.neuinfo.org/nif/nifstd/readable/> .
@prefix NLX: <http://uri.neuinfo.org/nif/nifstd/nlx_> .
@prefix NLXDYS: <http://uri.neuinfo.org/nif/nifstd/nlx_dys_> .
@prefix owl: <http://www.w3.org/2002/07/owl#> .
@prefix PROTEGE: <http://protege.stanford.edu/plugins/owl/protege#> .
@prefix rdf: <http://www.w3.org/1999/02/22-rdf-syntax-ns#> .
@prefix rdfs: <http://www.w3.org/2000/01/rdf-schema#> .
@prefix skos: <http://www.w3.org/2004/02/skos/core#> .
@prefix xml: <http://www.w3.org/XML/1998/namespace> .
@prefix xsd: <http://www.w3.org/2001/XMLSchema#> .

<http://ontology.neuinfo.org/NIF/ttl/NIF-Dysfunction.ttl> a owl:Ontology ;
    owl:imports <http://ontology.neuinfo.org/NIF/ttl/nif_backend.ttl> ;
    dc:title "NIF-Dysfunction (formally BIRNLex-Disease)"^^xsd:string ;
    skos:definition "This ontology contains the former BIRNLex-Disease, version 1.3.2. -- The BIRN Project lexicon will provide entities for data and database annotation for the BIRN project, covering anatomy, disease, data collection, project management and experimental design.  It is built using the organizational framework provided by the foundational Basic Formal Ontology (BFO).  It uses an abstract biomedical layer on top of that - OBO-UBO which has been constructed  as a proposal to the OBO Foundry.  This is meant to support creating a sharable view of core biomedical objects such as biomaterial_entity, and organismal_entity that all biomedical ontologies are likely to need and want to use with the same intended meaning.  The BIRNLex biomaterial entities have already been factored to separately maintained ontology - BIRNLexBiomaterialEntity.owl which this BIRNLex-Main.owl file imports.  The Ontology of Biomedical Investigation (OBI) is also imported and forms the foundation for the formal description of all experiment-related artifacts.  The BIRNLex will serve as the basis for construction of a formal ontology for the multiscale investigation of neurological disease."^^xsd:string ;
    skos:editorialNote "ID use: 2086, 2104; 12500 - 12831"^^xsd:string,
        "next ID: birnlex_12832"^^xsd:string,
        "Using birnlex IDs starting with 12500."^^xsd:string ;
    owl:versionInfo "1.5 (December, 2012)"^^xsd:string ;
    dc:contributor "Amarnath Gupta"^^xsd:string,
        "Bill Bug"^^xsd:string,
        "Carol Bean"^^xsd:string,
        "Christine Fennema-Notestine"^^xsd:string,
        "David Kennedy"^^xsd:string,
        "Fahim Imam"^^xsd:string,
        "Jeff Grethe"^^xsd:string,
        "Jessica Turner"^^xsd:string,
        "Maryann Martone"^^xsd:string ;
    dc:creator "The BIRN Ontology Task Force"^^xsd:string ;
    dc:subject "The BIRN project lexicon"^^xsd:string ;
    PROTEGE:defaultLanguage "en"^^xsd:string ;
    skos:historyNote """v1.3.1 - moved disease from BIRNLex-Other to to this stand-alone module. (BB: 2007-10-05)
v1.4  (May 2012) - Addition of DOID as an imported module. Addition of a bridging module that assigns equivalencies between DOID and NIF-Dysfunction classes.
v1.5 (December 2012) - Additional classes from NeuroLex: Neuropathy, Giant axonal neuropathy etc. and some hierarchical changes. Importing the newer version of doid <http://purl.obolibrary.org/obo/doid/2012-12-07/doid.owl>
v1.6 (January 2013) - Additional classes from NeuroLex: Traumatic brain injury."""^^xsd:string,
        "v1.3.2 - moved neuro diseases under Nervous system disease class and added eye and multisystem diseases (BB: 2007-11-18)."^^xsd:string,
        "v1.3.3 - added all three variants as synonyms for the disease names (or their synonyms) with (or sometimes without) an apostrophe (’s), e.g.,  “Batten disease”, “Batten’s disease” and “Battens disease” are kept as synonymous terms. (Fahim Imam: April 14, 2009)"^^xsd:string .

### Classes

BIRNLEX:2086 a owl:Class ;
    rdfs:label "Neurodegenerative disease"^^xsd:string ;
    skos:prefLabel "Neurodegenerative disease"^^xsd:string ;
    NIFRID:synonym "Degenerative Neurologic Disease"^^xsd:string,
        "Degenerative Neurologic Disorder"^^xsd:string,
        "Nervous System Degenerative Disease"^^xsd:string,
        "Neurodegenerative Disorder"^^xsd:string,
        "Neurologic Degenerative Condition"^^xsd:string ;
    skos:definition "Hereditary and sporadic conditions which are characterized by progressive nervous system dysfunction. These disorders are often associated with atrophy of the affected central or peripheral nervous system structures. (MeSH)."^^xsd:string ;
    rdfs:subClassOf BIRNLEX:12796 ;
    skos:editorialNote "Note BIRNLex seeks to evolve a core subsumptive disease hierarchy based first on the effected function, then the effected structure, the latter for those categories of nervous system disease that have typically been associated with structural abnormalities or trauma (e.g., Motor neuron diseases, cerebrovascular trauma, etc.). Disease causation is in fact the ultimate goal of much biomedical research, and our recognitition of ALL the driving causes of a particular disease - and the ways in which these causes inter-relate with each other and with effected structures to cause a change in normal function is a critical representational task BIRNlex will increasingly take on to provide an evolving, nuanced functional reconstruction of disease as a process and an outcome.  These relations will be represented using OWL ObjectProperties.  Function is the most sensible context to drive the asserted subsumptive hierarchy for representing nervous system disease, since it is with the clinical description of altered, impaired, decreased, or lost function that the diagnosis - and the research - of disease is rooted.  Much has already been described regarding both the effected biomaterial entities and the causes of disease.  However, it is because understanding of such relations still is far from comprehensive, that biomedical investigation into nervous system disease continues.  Finally, given the \"realist\" ontology design approach being used to construct BIRNLex, function must be represented as inhering in some biomaterial entity from molecules and their controlling elements on up through gross anatomical structures.  Over time, BIRNLex will provide the required relations to depict these functionally-related structures for both the normal and pathological function of the nervous system.  This will be true both for the causes and for the outcomes of nervous system disease.  Initial work to extend this expressive representation will focus on the neurodegenerative diseases being studied by BIRN researchers.  Though this will be te case, BIRNLex still needs to provide a core asserted hierarchy for a broad swarth of nervous system disease, so as to enable BIRN researchers to link to the breadth of disorders that may impact or relate to those directly under study."^^xsd:string ;
    NIFRID:createdDate "2006-07-15"^^xsd:string ;
    NIFRID:modifiedDate "2007-11-18"^^xsd:string ;
    NIFRID:hasBirnlexCurator NIFRID:BIRN_OTF ;
    NIFRID:hasCurationStatus NIFRID:uncurated ;
    NIFRID:hasDefinitionSource NIFRID:MeSH_defSource ;
    NIFRID:hasExternalSource NIFRID:MeSH ;
    NIFRID:MeshUid "D019636"^^xsd:string ;
    NIFRID:nifID "_8.3_2"^^xsd:string .

BIRNLEX:2092 a owl:Class ;
    rdfs:label "Alzheimers disease"^^xsd:string ;
    skos:prefLabel "Alzheimers disease"^^xsd:string ;
    NIFRID:synonym "Alzheimer Dementia"^^xsd:string,
        "Alzheimer disease"^^xsd:string,
        "Alzheimer Senile Dementia"^^xsd:string,
        "Alzheimer Type Dementia"^^xsd:string,
        "Alzheimer Type Senile Dementia"^^xsd:string,
        "Alzheimer's"^^xsd:string,
        "Alzheimer's Dementia"^^xsd:string,
        "Alzheimer's disease"^^xsd:string,
        "Alzheimers"^^xsd:string ;
    NIFRID:abbrev "AD"^^xsd:string ;
    rdfs:subClassOf BIRNLEX:12696 ;
    NIFRID:createdDate "2006-04-04"^^xsd:string ;
    NIFRID:modifiedDate "April 11, 2009"^^xsd:string ;
    NIFRID:birnlexDefinition "A neurodegenerative disease resulting in the insidious onset of dementia. Impairment of memory, judgement, attention span, and problem solving skills are followed by severe APRAXIAS and a global loss of cognitive abilities. The condition primarily occurs after age 60, and is marked pathologically by severe cortical atrophy and the triad of SENILE PLAQUES; NEUROFIBRILLARY TANGLES; and NEUROPIL THREADS. (adapted from MSH)"^^xsd:string ;
    NIFRID:definingCitation "Adams et al., Principles of Neurology, 6th ed, pp1049-57"^^xsd:string ;
    NIFRID:definingCitationURI <http://www.ninds.nih.gov/disorders/alzheimersdisease/alzheimersdisease.htm> ;
    NIFRID:hasBirnlexCurator NIFRID:BIRN_OTF ;
    NIFRID:hasCurationStatus NIFRID:curation_complete ;
    NIFRID:hasDefinitionSource NIFRID:MeSH_defSource ;
    NIFRID:hasExternalSource NIFRID:MeSH ;
    NIFRID:MeshUid "D000544"^^xsd:string ;
    NIFRID:nifID "_8.3_2.1"^^xsd:string ;
    NIFRID:putativeClassExtension "Acute Confusional Senile Dementia"^^xsd:string,
        "Early Onset Alzheimer Disease"^^xsd:string,
        "Focal Onset Alzheimer's Disease"^^xsd:string,
        "Late Onset Alzheimer Disease"^^xsd:string,
        "Presenile Dementia"^^xsd:string,
        "Primary Senile Degenerative Dementia"^^xsd:string ;
    NIFRID:UmlsCui "C0002395"^^xsd:string ;
    NIFRID:usageNote "MeSH includes implied subtypes based mostly on chronological time of onset"^^xsd:string .

BIRNLEX:2098 a owl:Class ;
    rdfs:label "Parkinsons disease"^^xsd:string ;
    skos:prefLabel "Parkinsons disease"^^xsd:string ;
    NIFRID:synonym "Idiopathic PD"^^xsd:string,
        "Paralysis Agitans"^^xsd:string,
        "Parkinson disease"^^xsd:string,
        "Parkinson syndrome"^^xsd:string,
        "Parkinson's"^^xsd:string,
        "Parkinson's disease"^^xsd:string,
        "Parkinson's syndrome"^^xsd:string,
        "Parkinsonian disorder"^^xsd:string,
        "Parkinsons"^^xsd:string ;
    rdfs:subClassOf BIRNLEX:2086 ;
    NIFRID:createdDate "2007-03-05"^^xsd:string ;
    NIFRID:modifiedDate "June 24, 2009"^^xsd:string ;
    NIFRID:acronym "PD"^^xsd:string ;
    NIFRID:birnlexDefinition """* A disease characterized as a progressive motor disability manifested by tremors, shaking, muscular rigidity, and lack of postural reflexes. (PSY)
* A progressive, degenerative neurologic disease characterized by a TREMOR that is maximal at rest, retropulsion (i.e. a tendency to fall backwards), rigidity, stooped posture, slowness of voluntary movements, and a masklike facial expression. Pathologic features include loss of melanin containing neurons in the substantia nigra and other pigmented nuclei of the brainstem. LEWY BODIES are present in the substantia nigra and locus coeruleus but may also be found in a related condition (LEWY BODY DISEASE, DIFFUSE) characterized by dementia in combination with varying degrees of parkinsonism. (Adams et al., Principles of Neurology, 6th ed, p1059, pp1067-75) (MSH)
* progressive, degenerative disorder of the nervous system characterized by tremors, rigidity, bradykinesia, postural instability, and gait abnormalities; caused by a loss of neurons and a decrease of dopamine in the basal ganglia. (CSP)"""^^xsd:string ;
    NIFRID:definingCitationURI <http://www.ninds.nih.gov/disorders/parkinsons_disease/parkinsons_disease.htm> ;
    NIFRID:hasBirnlexCurator NIFRID:Bill_Bug ;
    NIFRID:hasDefinitionSource NIFRID:UMLS_defSource ;
    NIFRID:nifID "_8.3_2.7"^^xsd:string ;
    NIFRID:putativeClassExtension "Idiopathic Parkinson Disease"^^xsd:string,
        "Lewy Body Parkinson Disease"^^xsd:string,
        "Primary Parkinsonism"^^xsd:string ;
    NIFRID:UmlsCui "C0030567"^^xsd:string ;
    NIFRID:usageNote "MeSH includes several implied subtypes based primarily on causation"^^xsd:string .

BIRNLEX:2104 a owl:Class ;
    rdfs:label "Schizophrenia"^^xsd:string ;
    skos:prefLabel "Schizophrenia"^^xsd:string ;
    NIFRID:synonym "Dementia Praecox"^^xsd:string,
        "Schizophrenic Disorder"^^xsd:string ;
    rdfs:subClassOf BIRNLEX:12761 ;
    NIFRID:createdDate "2006-06-01"^^xsd:string ;
    NIFRID:modifiedDate "2007-10-08"^^xsd:string ;
    NIFRID:externallySourcedDefinition "A severe emotional disorder of psychotic depth characteristically marked by a retreat from reality with delusion formation, hallucinations, emotional disharmony, and regressive behavior. (MeSH)"^^xsd:string ;
    NIFRID:hasBirnlexCurator NIFRID:Jessica_Turner ;
    NIFRID:hasCurationStatus NIFRID:uncurated ;
    NIFRID:hasExternalSource NIFRID:UMLS ;
    NIFRID:nifID "_8.3_11.6"^^xsd:string ;
    NIFRID:UmlsCui "C0036341"^^xsd:string .

BIRNLEX:11013 a owl:Class ;
    rdfs:label "Disease"^^xsd:string ;
    rdfs:subClassOf BFO:0000016 .

BIRNLEX:12500 a owl:Class ;
    rdfs:label "Huntingtons disease"^^xsd:string ;
    skos:prefLabel "Huntingtons disease"^^xsd:string ;
    NIFRID:synonym "Chronic Progressive Hereditary Chorea (Huntington)"^^xsd:string,
        "Huntington Chronic Progressive Hereditary Chorea"^^xsd:string,
        "Huntington disease"^^xsd:string,
        "Huntington's"^^xsd:string,
        "Huntington's Chorea"^^xsd:string,
        "Huntington's disease"^^xsd:string ;
    skos:definition "A familial disorder inherited as an autosomal dominant trait and characterized by the onset of progressive CHOREA and DEMENTIA in the fourth or fifth decade of life. Common initial manifestations include paranoia; poor impulse control; DEPRESSION; HALLUCINATIONS; and DELUSIONS. Eventually intellectual impairment; loss of fine motor control; ATHETOSIS; and diffuse chorea involving axial and limb musculature develops, leading to a vegetative state within 10-15 years of disease onset. The juvenile variant has a more fulminant course including SEIZURES; ATAXIA; dementia; and chorea."^^xsd:string ;
    rdfs:subClassOf BIRNLEX:2086 ;
    NIFRID:createdDate "2007-10-05"^^xsd:string ;
    NIFRID:modifiedDate "April 11, 2009"^^xsd:string ;
    NIFRID:acronym "HD"^^xsd:string ;
    NIFRID:definingCitation "Adams et al., Principles of Neurology, 6th ed, pp1060-4"^^xsd:string ;
    NIFRID:definingCitationURI <http://www.ninds.nih.gov/disorders/huntington/huntington.htm> ;
    NIFRID:hasBirnlexCurator NIFRID:Bill_Bug ;
    NIFRID:hasCurationStatus NIFRID:uncurated ;
    NIFRID:hasDefinitionSource NIFRID:MeSH_defSource ;
    NIFRID:hasExternalSource NIFRID:MeSH ;
    NIFRID:MeshUid "D006816"^^xsd:string ;
    NIFRID:nifID "_8.3_2.10"^^xsd:string .

BIRNLEX:12501 a owl:Class ;
    rdfs:label "Autistic Disorder"^^xsd:string ;
    skos:prefLabel "Autistic Disorder"^^xsd:string ;
    NIFRID:synonym "Autism"^^xsd:string,
        "Early Infantile Autism"^^xsd:string,
        "Infantile Autism"^^xsd:string,
        "Kanner's Syndrome"^^xsd:string ;
    rdfs:subClassOf BIRNLEX:12768 ;
    NIFRID:createdDate "2007-10-01"^^xsd:string ;
    NIFRID:modifiedDate "2007-10-08"^^xsd:string ;
    NIFRID:definingCitation "DSM-IV"^^xsd:string ;
    NIFRID:definingCitationURI <http://www.ninds.nih.gov/disorders/autism/autism.htm> ;
    NIFRID:hasBirnlexCurator NIFRID:Bill_Bug ;
    NIFRID:hasCurationStatus NIFRID:uncurated ;
    NIFRID:nifID "_8.3_11.7"^^xsd:string .

BIRNLEX:12502 a owl:Class ;
    rdfs:label "Lewy Body Disease"^^xsd:string ;
    skos:prefLabel "Lewy Body Disease"^^xsd:string ;
    skos:definition "A neurodegenerative disease characterized by dementia, mild parkinsonism, and fluctuations in attention and alertness. The neuropsychiatric manifestations tend to precede the onset of bradykinesia, MUSCLE RIGIDITY, and other extrapyramidal signs. DELUSIONS and visual HALLUCINATIONS are relatively frequent in this condition. Histologic examination reveals LEWY BODIES in the CEREBRAL CORTEX and BRAIN STEM. SENILE PLAQUES and other pathologic features characteristic of ALZHEIMER DISEASE may also be present."^^xsd:string ;
    rdfs:subClassOf BIRNLEX:2086 ;
    NIFRID:createdDate "2007-10-05"^^xsd:string ;
    NIFRID:modifiedDate "2007-10-05"^^xsd:string ;
    NIFRID:acronym "LBD"^^xsd:string ;
    NIFRID:definingCitation "Neurology 1997;48:376-380; Neurology 1996;47:1113-1124"^^xsd:string ;
    NIFRID:hasBirnlexCurator NIFRID:Bill_Bug ;
    NIFRID:hasCurationStatus NIFRID:uncurated ;
    NIFRID:hasDefinitionSource NIFRID:MeSH_defSource ;
    NIFRID:hasExternalSource NIFRID:MeSH ;
    NIFRID:MeshUid "D020961"^^xsd:string ;
    NIFRID:nifID "_8.3_2.9"^^xsd:string ;
    NIFRID:usageNote "There are two MeSH terms for this general term that indicate there are infact subtypes of Lewy Body Disease (i.e., Diffuse Lewy Body Disease; Cortical Lewy Body Disease)"^^xsd:string .

BIRNLEX:12504 a owl:Class ;
    rdfs:label "Akinetic-Rigid Variant of Huntington Disease"^^xsd:string ;
    skos:prefLabel "Akinetic-Rigid Variant of Huntington Disease"^^xsd:string ;
    NIFRID:synonym "Akinetic-Rigid Variant of Huntington's Disease"^^xsd:string,
        "Akinetic-Rigid Variant of Huntingtons Disease"^^xsd:string,
        "Huntington Disease, Akinetic-Rigid Variant"^^xsd:string ;
    rdfs:subClassOf BIRNLEX:12500 ;
    NIFRID:createdDate "2007-10-05"^^xsd:string ;
    NIFRID:modifiedDate "April 11, 2009"^^xsd:string ;
    NIFRID:hasBirnlexCurator NIFRID:Bill_Bug ;
    NIFRID:hasCurationStatus NIFRID:uncurated ;
    NIFRID:hasExternalSource NIFRID:MeSH ;
    NIFRID:MeshUid "D006816"^^xsd:string .

BIRNLEX:12505 a owl:Class ;
    rdfs:label "Juvenile-Onset Huntington Disease"^^xsd:string ;
    skos:prefLabel "Juvenile-Onset Huntington Disease"^^xsd:string ;
    NIFRID:synonym "Juvenile Huntington Disease"^^xsd:string,
        "Juvenile Onset Huntington's Disease"^^xsd:string,
        "Juvenile-Onset Huntington's Disease"^^xsd:string,
        "Juvenile-Onset Huntingtons Disease"^^xsd:string ;
    rdfs:subClassOf BIRNLEX:12500 ;
    NIFRID:createdDate "2007-10-05"^^xsd:string ;
    NIFRID:modifiedDate "April 11, 2009"^^xsd:string ;
    NIFRID:hasBirnlexCurator NIFRID:Bill_Bug ;
    NIFRID:hasCurationStatus NIFRID:uncurated ;
    NIFRID:hasExternalSource NIFRID:MeSH ;
    NIFRID:MeshUid "D006816"^^xsd:string .

BIRNLEX:12506 a owl:Class ;
    rdfs:label "Late-Onset Huntington Disease"^^xsd:string ;
    skos:prefLabel "Late-Onset Huntington Disease"^^xsd:string ;
    NIFRID:synonym "Late Onset Huntington Disease"^^xsd:string,
        "Late Onset Huntingtons Disease"^^xsd:string,
        "Late-Onset Huntington's Disease"^^xsd:string,
        "Late-Onset Huntingtons Disease"^^xsd:string ;
    rdfs:subClassOf BIRNLEX:12500 ;
    NIFRID:createdDate "2007-10-05"^^xsd:string ;
    NIFRID:modifiedDate "2007-10-05"^^xsd:string ;
    NIFRID:hasBirnlexCurator NIFRID:Bill_Bug ;
    NIFRID:hasCurationStatus NIFRID:uncurated ;
    NIFRID:hasExternalSource NIFRID:MeSH ;
    NIFRID:MeshUid "D006816"^^xsd:string .

BIRNLEX:12507 a owl:Class ;
    rdfs:label "Demyelinating disease"^^xsd:string ;
    skos:prefLabel "Demyelinating disease"^^xsd:string ;
    NIFRID:synonym "Demyelinating disorder"^^xsd:string ;
    skos:definition "Diseases characterized by loss or dysfunction of myelin in the central or peripheral nervous system."^^xsd:string ;
    rdfs:subClassOf BIRNLEX:12796 ;
    NIFRID:createdDate "2007-10-05"^^xsd:string ;
    NIFRID:modifiedDate "2007-11-18"^^xsd:string ;
    NIFRID:hasBirnlexCurator NIFRID:Bill_Bug ;
    NIFRID:hasCurationStatus NIFRID:uncurated ;
    NIFRID:hasDefinitionSource NIFRID:MeSH_defSource ;
    NIFRID:hasExternalSource NIFRID:MeSH ;
    NIFRID:MeshUid "D003711"^^xsd:string ;
    NIFRID:nifID "_8.3_3"^^xsd:string ;
    NIFRID:UmlsCui "C0011303"^^xsd:string .

BIRNLEX:12508 a owl:Class ;
    rdfs:label "Demyelinating Autoimmune Disease"^^xsd:string ;
    skos:prefLabel "Demyelinating Autoimmune Disease"^^xsd:string ;
    NIFRID:synonym "Autoimmune Demyelinating Diseases, Central Nervous System"^^xsd:string,
        "CNS Autoimmune Demyelinating Disorders"^^xsd:string,
        "CNS Demyelinating Autoimmune Diseases"^^xsd:string ;
    skos:definition "Conditions characterized by loss or dysfunction of myelin (see MYELIN SHEATH) in the brain, spinal cord, or optic nerves secondary to autoimmune mediated processes. This may take the form of a humoral or cellular immune response directed toward myelin or OLIGODENDROGLIA associated autoantigens (MeSH)."^^xsd:string ;
    rdfs:subClassOf BIRNLEX:12507 ;
    NIFRID:createdDate "2007-10-05"^^xsd:string ;
    NIFRID:modifiedDate "2007-10-05"^^xsd:string ;
    NIFRID:hasBirnlexCurator NIFRID:Bill_Bug ;
    NIFRID:hasCurationStatus NIFRID:uncurated ;
    NIFRID:hasExternalSource NIFRID:MeSH ;
    NIFRID:MeshUid "D020278"^^xsd:string ;
    skos:scopeNote "For central nervous system diseases only; for demyelinating diseases of the peripheral nervous system consider POLYRADICULONEURITIS; GUILLAIN-BARRE SYNDROME; and CHRONIC INFLAMMATORY POLYRADICULONEUROPATHY; for demyelinating autoimmune diseases of the brain or spinal cord not otherwise specified coord with BRAIN DISEASES or SPINAL CORD DISEASES (MeSH)."^^xsd:string .

BIRNLEX:12509 a owl:Class ;
    rdfs:label "Diffuse Cerebral Sclerosis of Schilder"^^xsd:string ;
    skos:prefLabel "Diffuse Cerebral Sclerosis of Schilder"^^xsd:string ;
    NIFRID:synonym "Alpers Disease"^^xsd:string,
        "Alpers Syndrome"^^xsd:string,
        "Alpers' Disease"^^xsd:string,
        "Balo's Concentric Sclerosis"^^xsd:string,
        "Cerebral Sclerosis, Diffuse"^^xsd:string,
        "Encephalitis Periaxialis"^^xsd:string,
        "Encephalitis Periaxialis Concentrica"^^xsd:string,
        "Encephalitis Periaxialis Diffusa"^^xsd:string,
        "Myelinoclastic Diffuse Sclerosis"^^xsd:string,
        "Poliodystrophia Cerebri"^^xsd:string,
        "Schilder Disease"^^xsd:string,
        "Schilder's Disease"^^xsd:string,
        "Schilders Disease"^^xsd:string ;
    skos:definition "A rare central nervous system demyelinating condition affecting children and young adults. Pathologic findings include a large, sharply defined, asymmetric focus of myelin destruction that may involve an entire lobe or cerebral hemisphere. The clinical course tends to be progressive and includes dementia, cortical blindness, cortical deafness, spastic hemiplegia, and pseudobulbar palsy. Concentric sclerosis of Balo is differentiated from diffuse cerebral sclerosis of Schilder by the pathologic finding of alternating bands of destruction and preservation of myelin in concentric rings. Alpers' Syndrome refers to a heterogeneous group of diseases that feature progressive cerebral deterioration and liver disease. (MeSH)."^^xsd:string ;
    rdfs:subClassOf BIRNLEX:12508 ;
    NIFRID:createdDate "2007-10-05"^^xsd:string ;
    NIFRID:modifiedDate "April 11, 2009"^^xsd:string ;
    NIFRID:definingCitation "Adams et al., Principles of Neurology, 6th ed, p914; Dev Neurosci 1991;13(4-5):267-73"^^xsd:string ;
    NIFRID:definingCitationURI <http://www.ninds.nih.gov/disorders/schilders/schilders.htm> ;
    NIFRID:hasBirnlexCurator NIFRID:Bill_Bug ;
    NIFRID:hasCurationStatus NIFRID:uncurated ;
    NIFRID:hasExternalSource NIFRID:MeSH ;
    NIFRID:MeshUid "D002549"^^xsd:string .

BIRNLEX:12510 a owl:Class ;
    rdfs:label "Acute Disseminated Encephalomyelitis"^^xsd:string ;
    skos:prefLabel "Acute Disseminated Encephalomyelitis"^^xsd:string ;
    NIFRID:synonym "Postinfectious Encephalomyelitis"^^xsd:string ;
    skos:definition "An acute or subacute inflammatory process of the CENTRAL NERVOUS SYSTEM characterized histologically by multiple foci of perivascular demyelination. Symptom onset usually occurs several days after an acute viral infection or immunization, but it may coincide with the onset of infection or rarely no antecedent event can be identified. Clinical manifestations include CONFUSION, somnolence, FEVER, nuchal rigidity, and involuntary movements. The illness may progress to COMA and eventually be fatal (MeSH)."^^xsd:string ;
    rdfs:subClassOf BIRNLEX:12508 ;
    NIFRID:createdDate "2007-10-05"^^xsd:string ;
    NIFRID:modifiedDate "2007-10-05"^^xsd:string ;
    NIFRID:definingCitation "Adams et al., Principles of Neurology, 6th ed, p921"^^xsd:string ;
    NIFRID:definingCitationURI <http://www.ninds.nih.gov/disorders/encephalomyelitis/acute_encephalomyelitis.htm> ;
    NIFRID:hasBirnlexCurator NIFRID:Bill_Bug ;
    NIFRID:hasCurationStatus NIFRID:uncurated ;
    NIFRID:hasExternalSource NIFRID:MeSH ;
    NIFRID:MeshUid "D004673"^^xsd:string ;
    skos:scopeNote "When post-vaccinal (note X ref) coord IM with vaccine source if pertinent (IM or NIM); for post-vaccinal or postinfectious inflammation of the spinal cord only, use MYELITIS, TRANSVERSE; (MeSH)."^^xsd:string .

BIRNLEX:12511 a owl:Class ;
    rdfs:label "Post-Vaccinal Encephalomyelitis"^^xsd:string ;
    skos:prefLabel "Post-Vaccinal Encephalomyelitis"^^xsd:string ;
    NIFRID:synonym "Post-Vaccinal Encephalitis"^^xsd:string,
        "Postvaccinal Encephalitis"^^xsd:string,
        "Vaccination Encephalitis"^^xsd:string ;
    skos:definition "Form of Acute Disseminated Encephalomyelitis induced by a vacine-related infection."^^xsd:string ;
    rdfs:subClassOf BIRNLEX:12510 ;
    NIFRID:createdDate "2007-10-05"^^xsd:string ;
    NIFRID:modifiedDate "2007-10-05"^^xsd:string ;
    NIFRID:hasBirnlexCurator NIFRID:Bill_Bug ;
    NIFRID:hasCurationStatus NIFRID:uncurated ;
    NIFRID:hasExternalSource NIFRID:MeSH ;
    NIFRID:MeshUid "D004673"^^xsd:string .

BIRNLEX:12512 a owl:Class ;
    rdfs:label "Postexanthem Encephalomyelitis"^^xsd:string ;
    skos:prefLabel "Postexanthem Encephalomyelitis"^^xsd:string ;
    skos:definition "Form of Acute Disseminated Encephalomyelitis following an exanthem infection (exanthem or exanthema = an eruptive disease (as measles) or its symptomatic eruption [Merriam-Webster Online Dictonary, c. 2006-2007])."^^xsd:string ;
    rdfs:subClassOf BIRNLEX:12510 ;
    NIFRID:createdDate "2007-10-05"^^xsd:string ;
    NIFRID:modifiedDate "2007-10-05"^^xsd:string ;
    NIFRID:hasBirnlexCurator NIFRID:Bill_Bug ;
    NIFRID:hasCurationStatus NIFRID:uncurated ;
    NIFRID:hasExternalSource NIFRID:MeSH ;
    NIFRID:MeshUid "D004673"^^xsd:string .

BIRNLEX:12513 a owl:Class ;
    rdfs:label "Acute Hemorrhagic Leukoencephalitis"^^xsd:string ;
    skos:prefLabel "Acute Hemorrhagic Leukoencephalitis"^^xsd:string ;
    NIFRID:synonym "Acute Necrotizing Encephalitis"^^xsd:string,
        "Acute Necrotizing Hemorrhagic Encephalomyelitis"^^xsd:string,
        "Hemorrhagic Necrotizing Encephalomyelitis"^^xsd:string,
        "Hurst's Disease"^^xsd:string,
        "Leukoencephalitis Acuta Hemorrhagica"^^xsd:string,
        "Subacute Hemorrhagic Leukoencephalitis"^^xsd:string ;
    skos:definition "A fulminant and often fatal demyelinating disease of the brain which primarily affects young adults and children. Clinical features include the rapid onset of weakness, SEIZURES, and COMA. It may follow a viral illness or MYCOPLASMA PNEUMONIAE infections but in most instances there is no precipitating event. Pathologic examination reveals marked perivascular demyelination and necrosis of white matter with microhemorrhages (MeSH)."^^xsd:string ;
    rdfs:subClassOf BIRNLEX:12508 ;
    NIFRID:createdDate "2007-10-05"^^xsd:string ;
    NIFRID:modifiedDate "2007-10-05"^^xsd:string ;
    NIFRID:definingCitation "Adams et al., Principles of Neurology, 6th ed, pp924-5"^^xsd:string ;
    NIFRID:hasBirnlexCurator NIFRID:Bill_Bug ;
    NIFRID:hasCurationStatus NIFRID:uncurated ;
    NIFRID:hasExternalSource NIFRID:MeSH ;
    NIFRID:MeshUid "D004684"^^xsd:string .

BIRNLEX:12514 a owl:Class ;
    rdfs:label "Multiple Sclerosis"^^xsd:string ;
    skos:prefLabel "Multiple Sclerosis"^^xsd:string ;
    NIFRID:synonym "Acute Fulminating Multiple Sclerosis"^^xsd:string,
        "Disseminated Sclerosis"^^xsd:string ;
    skos:definition "An autoimmune disorder mainly affecting young adults and characterized by destruction of myelin in the central nervous system. Pathologic findings include multiple sharply demarcated areas of demyelination throughout the white matter of the central nervous system. Clinical manifestations include visual loss, extra-ocular movement disorders, paresthesias, loss of sensation, weakness, dysarthria, spasticity, ataxia, and bladder dysfunction. The usual pattern is one of recurrent attacks followed by partial recovery (see MULTIPLE SCLEROSIS, RELAPSING-REMITTING), but acute fulminating and chronic progressive forms (see MULTIPLE SCLEROSIS, CHRONIC PROGRESSIVE) also occur (MeSH)."^^xsd:string ;
    rdfs:subClassOf BIRNLEX:12508 ;
    NIFRID:createdDate "2007-10-05"^^xsd:string ;
    NIFRID:modifiedDate "2007-10-05"^^xsd:string ;
    NIFRID:acronym "MS"^^xsd:string ;
    NIFRID:definingCitation "Adams et al., Principles of Neurology, 6th ed, p903"^^xsd:string ;
    NIFRID:definingCitationURI <http://www.ninds.nih.gov/disorders/multiple_sclerosis/multiple_sclerosis.htm> ;
    NIFRID:hasBirnlexCurator NIFRID:Bill_Bug ;
    NIFRID:hasCurationStatus NIFRID:uncurated ;
    NIFRID:hasExternalSource NIFRID:MeSH ;
    NIFRID:MeshUid "D009103"^^xsd:string ;
    NIFRID:nifID "_8.3_3.1"^^xsd:string .

BIRNLEX:12515 a owl:Class ;
    rdfs:label "Chronic Progressive Multiple Sclerosis"^^xsd:string ;
    skos:prefLabel "Chronic Progressive Multiple Sclerosis"^^xsd:string ;
    NIFRID:synonym "Progressive Relapsing Multiple Sclerosis"^^xsd:string,
        "Remittent Progressive Multiple Sclerosis"^^xsd:string ;
    skos:definition "A form of multiple sclerosis characterized by a progressive deterioration in neurologic function which is in contrast to the more typical relapsing remitting form. If the clinical course is free of distinct remissions, it is referred to as primary progressive multiple sclerosis. When the progressive decline is punctuated by acute exacerbations, it is referred to as progressive relapsing multiple sclerosis. The term secondary progressive multiple sclerosis is used when relapsing remitting multiple sclerosis evolves into the chronic progressive form (MeSH)."^^xsd:string ;
    rdfs:subClassOf BIRNLEX:12514 ;
    NIFRID:createdDate "2007-10-05"^^xsd:string ;
    NIFRID:modifiedDate "2007-10-05"^^xsd:string ;
    NIFRID:definingCitation "Ann Neurol 1994;36 Suppl:S73-S79; Adams et al., Principles of Neurology, 6th ed, pp903-914"^^xsd:string ;
    NIFRID:hasBirnlexCurator NIFRID:Bill_Bug ;
    NIFRID:hasCurationStatus NIFRID:uncurated ;
    NIFRID:hasExternalSource NIFRID:MeSH ;
    NIFRID:MeshUid "D020528"^^xsd:string .

BIRNLEX:12516 a owl:Class ;
    rdfs:label "Primary Progressive Multiple Sclerosis"^^xsd:string ;
    skos:prefLabel "Primary Progressive Multiple Sclerosis"^^xsd:string ;
    rdfs:subClassOf BIRNLEX:12515 ;
    NIFRID:createdDate "2007-10-05"^^xsd:string ;
    NIFRID:modifiedDate "2007-10-05"^^xsd:string ;
    NIFRID:hasBirnlexCurator NIFRID:Bill_Bug ;
    NIFRID:hasCurationStatus NIFRID:uncurated ;
    NIFRID:hasExternalSource NIFRID:MeSH ;
    NIFRID:MeshUid "D020528"^^xsd:string .

BIRNLEX:12517 a owl:Class ;
    rdfs:label "Secondary Progressive Multiple Sclerosis"^^xsd:string ;
    skos:prefLabel "Secondary Progressive Multiple Sclerosis"^^xsd:string ;
    rdfs:subClassOf BIRNLEX:12515 ;
    NIFRID:createdDate "2007-10-05"^^xsd:string ;
    NIFRID:modifiedDate "2007-10-05"^^xsd:string ;
    NIFRID:hasBirnlexCurator NIFRID:Bill_Bug ;
    NIFRID:hasCurationStatus NIFRID:uncurated ;
    NIFRID:hasExternalSource NIFRID:MeSH ;
    NIFRID:MeshUid "D020528"^^xsd:string .

BIRNLEX:12518 a owl:Class ;
    rdfs:label "Relapsing-Remitting Multiple Sclerosis"^^xsd:string ;
    skos:prefLabel "Relapsing-Remitting Multiple Sclerosis"^^xsd:string ;
    NIFRID:synonym "Acute Relapsing Multiple Sclerosis"^^xsd:string,
        "Remitting-Relapsing Multiple Sclerosis"^^xsd:string ;
    skos:definition "The most common clinical variant of MULTIPLE SCLEROSIS, characterized by recurrent acute exacerbations of neurologic dysfunction followed by partial or complete recovery. Common clinical manifestations include loss of visual (see OPTIC NEURITIS), motor, sensory, or bladder function. Acute episodes of demyelination may occur at any site in the central nervous system, and commonly involve the optic nerves, spinal cord, brain stem, and cerebellum (MeSH)."^^xsd:string ;
    rdfs:subClassOf BIRNLEX:12514 ;
    NIFRID:createdDate "2007-10-05"^^xsd:string ;
    NIFRID:modifiedDate "2007-10-05"^^xsd:string ;
    NIFRID:definingCitation "Adams et al., Principles of Neurology, 6th ed, pp903-914"^^xsd:string ;
    NIFRID:hasBirnlexCurator NIFRID:Bill_Bug ;
    NIFRID:hasCurationStatus NIFRID:uncurated ;
    NIFRID:hasExternalSource NIFRID:MeSH ;
    NIFRID:MeshUid "D020529"^^xsd:string .

BIRNLEX:12519 a owl:Class ;
    rdfs:label "Neuromyelitis Optica"^^xsd:string ;
    skos:prefLabel "Neuromyelitis Optica"^^xsd:string ;
    NIFRID:synonym "Devic Disease"^^xsd:string,
        "Devic Syndrome"^^xsd:string,
        "Devic's Disease"^^xsd:string,
        "Devic's Syndrome"^^xsd:string,
        "Devics Disease"^^xsd:string,
        "Devics Syndrome"^^xsd:string ;
    skos:definition "A syndrome characterized by acute OPTIC NEURITIS in combination with acute MYELITIS, TRANSVERSE. Demyelinating and/or necrotizing lesions form in one or both optic nerves and in the spinal cord. The onset of optic neuritis and myelitis may be simultaneous or separated by several months (MeSH)."^^xsd:string ;
    rdfs:subClassOf BIRNLEX:12508 ;
    NIFRID:createdDate "2007-10-05"^^xsd:string ;
    NIFRID:modifiedDate "April 11, 2009"^^xsd:string ;
    NIFRID:definingCitation "J Neurol Neurosurg Psychiatry 1996 Apr;60(4):382-387"^^xsd:string ;
    NIFRID:definingCitationURI <http://www.ninds.nih.gov/disorders/neuromyelitis_optica/neuromyelitis_optica.htm> ;
    NIFRID:hasBirnlexCurator NIFRID:Bill_Bug ;
    NIFRID:hasCurationStatus NIFRID:uncurated ;
    NIFRID:hasExternalSource NIFRID:MeSH ;
    NIFRID:MeshUid "D009471"^^xsd:string .

BIRNLEX:12520 a owl:Class ;
    rdfs:label "Transverse Myelitis"^^xsd:string ;
    skos:prefLabel "Transverse Myelitis"^^xsd:string ;
    NIFRID:synonym "Acute Transverse Myelitis"^^xsd:string,
        "Demyelinative Myelitis"^^xsd:string,
        "Necrotizing Myelitis"^^xsd:string,
        "Subacute Transverse Myelitis"^^xsd:string,
        "Transverse Myelopathy Syndrome"^^xsd:string ;
    skos:definition "Inflammation of a transverse portion of the spinal cord characterized by acute or subacute segmental demyelination or necrosis. The condition may occur sporadically, follow an infection or vaccination, or present as a paraneoplastic syndrome (see also ENCEPHALOMYELITIS, ACUTE DISSEMINATED). Clinical manifestations include motor weakness, sensory loss, and incontinence (MeSH)."^^xsd:string ;
    rdfs:subClassOf BIRNLEX:12508 ;
    NIFRID:createdDate "2007-10-05"^^xsd:string ;
    NIFRID:modifiedDate "2007-10-05"^^xsd:string ;
    NIFRID:definingCitation "Adams et al., Principles of Neurology, 6th ed, pp1242-6"^^xsd:string ;
    NIFRID:definingCitationURI <http://www.ninds.nih.gov/disorders/transversemyelitis/transversemyelitis.htm> ;
    NIFRID:hasBirnlexCurator NIFRID:Bill_Bug ;
    NIFRID:hasCurationStatus NIFRID:uncurated ;
    NIFRID:hasExternalSource NIFRID:MeSH ;
    NIFRID:MeshUid "D009188"^^xsd:string ;
    skos:scopeNote "Post-vaccinal or postinfectious inflammation of the spinal cord only goes here, in central nervous system or brain see X refs at ENCEPHALOMYELITIS, ACUTE DISSEMINATED (MeSH)."^^xsd:string .

BIRNLEX:12521 a owl:Class ;
    rdfs:label "Postinfectious Myelitis"^^xsd:string ;
    skos:prefLabel "Postinfectious Myelitis"^^xsd:string ;
    skos:definition "A form of Transverse Myelitis induced by an infection.(MeSH)."^^xsd:string ;
    rdfs:subClassOf BIRNLEX:12520 ;
    NIFRID:createdDate "2007-10-05"^^xsd:string ;
    NIFRID:modifiedDate "2007-10-05"^^xsd:string ;
    NIFRID:hasBirnlexCurator NIFRID:Bill_Bug ;
    NIFRID:hasCurationStatus NIFRID:uncurated ;
    NIFRID:hasExternalSource NIFRID:MeSH ;
    NIFRID:MeshUid "D009188"^^xsd:string .

BIRNLEX:12522 a owl:Class ;
    rdfs:label "Postvaccinal Myelitis"^^xsd:string ;
    skos:prefLabel "Postvaccinal Myelitis"^^xsd:string ;
    skos:definition "A form of Transverse Myelitis induced by a vaccine-induced infection.(MeSH)."^^xsd:string ;
    rdfs:subClassOf BIRNLEX:12521 ;
    NIFRID:createdDate "2007-10-05"^^xsd:string ;
    NIFRID:modifiedDate "2007-10-05"^^xsd:string ;
    NIFRID:hasBirnlexCurator NIFRID:Bill_Bug ;
    NIFRID:hasCurationStatus NIFRID:uncurated ;
    NIFRID:hasExternalSource NIFRID:MeSH ;
    NIFRID:MeshUid "D009188"^^xsd:string .

BIRNLEX:12523 a owl:Class ;
    rdfs:label "Paraneoplastic Myelitis"^^xsd:string ;
    skos:prefLabel "Paraneoplastic Myelitis"^^xsd:string ;
    skos:definition "A form of Transverse Myelitis associated with a neoplastic condition.(MeSH)."^^xsd:string ;
    rdfs:subClassOf BIRNLEX:12520 ;
    NIFRID:createdDate "2007-10-05"^^xsd:string ;
    NIFRID:modifiedDate "2007-10-05"^^xsd:string ;
    NIFRID:hasBirnlexCurator NIFRID:Bill_Bug ;
    NIFRID:hasCurationStatus NIFRID:uncurated ;
    NIFRID:hasExternalSource NIFRID:MeSH ;
    NIFRID:MeshUid "D009188"^^xsd:string .

BIRNLEX:12524 a owl:Class ;
    rdfs:label "Neurodevelopmental disease"^^xsd:string ;
    skos:prefLabel "Neurodevelopmental disease"^^xsd:string ;
    skos:definition "Hereditary and sporadic conditions which are characterized by progressive nervous system dysfunction. These disorders are often associated with atrophy of the affected central or peripheral nervous system structures. (MeSH)."^^xsd:string ;
    rdfs:subClassOf BIRNLEX:12796 ;
    skos:editorialNote "Note BIRNLex seeks to evolve a core subsumptive disease hierarchy based first on the effected function, then the effected structure, the latter for those categories of nervous system disease that have typically been associated with structural abnormalities or trauma (e.g., Motor neuron diseases, cerebrovascular trauma, etc.). Disease causation is in fact the ultimate goal of much biomedical research, and our recognitition of ALL the driving causes of a particular disease - and the ways in which these causes inter-relate with each other and with effected structures to cause a change in normal function is a critical representational task BIRNlex will increasingly take on to provide an evolving, nuanced functional reconstruction of disease as a process and an outcome.  These relations will be represented using OWL ObjectProperties.  Function is the most sensible context to drive the asserted subsumptive hierarchy for representing nervous system disease, since it is with the clinical description of altered, impaired, decreased, or lost function that the diagnosis - and the research - of disease is rooted.  Much has already been described regarding both the effected biomaterial entities and the causes of disease.  However, it is because understanding of such relations still is far from comprehensive, that biomedical investigation into nervous system disease continues.  Finally, given the \"realist\" ontology design approach being used to construct BIRNLex, function must be represented as inhering in some biomaterial entity from molecules and their controlling elements on up through gross anatomical structures.  Over time, BIRNLex will provide the required relations to depict these functionally-related structures for both the normal and pathological function of the nervous system.  This will be true both for the causes and for the outcomes of nervous system disease.  Initial work to extend this expressive representation will focus on the neurodegenerative diseases being studied by BIRN researchers.  Though this will be te case, BIRNLex still needs to provide a core asserted hierarchy for a broad swarth of nervous system disease, so as to enable BIRN researchers to link to the breadth of disorders that may impact or relate to those directly under study."^^xsd:string ;
    NIFRID:createdDate "2007-10-05"^^xsd:string ;
    NIFRID:modifiedDate "2007-11-18"^^xsd:string ;
    NIFRID:hasBirnlexCurator NIFRID:Bill_Bug ;
    NIFRID:hasCurationStatus NIFRID:uncurated ;
    NIFRID:hasDefinitionSource NIFRID:MeSH_defSource ;
    NIFRID:hasExternalSource NIFRID:MeSH ;
    NIFRID:nifID "_8.3_4"^^xsd:string .

BIRNLEX:12525 a owl:Class ;
    rdfs:label "Nervous system neoplastic disease"^^xsd:string ;
    skos:prefLabel "Nervous system neoplastic disease"^^xsd:string ;
    NIFRID:synonym "Cancer"^^xsd:string ;
    skos:definition "Abnormal mass of tissue in the nervous system."^^xsd:string ;
    rdfs:subClassOf BIRNLEX:12796 ;
    skos:editorialNote "Despite the fact most of the subclasses for neoplastic disease appear to be representing an object (the neoplasm itself), they should be considered to be representing the disposition for a given tissue to develop such a neoplasm.  It is left for the future as to how this disposition will be linked to the tissue bearing that disposition.  Again - we will consult those working on a realist representation of neoplastic disorders for insight and guidance on this task (BB: 2007-10-05)."^^xsd:string,
        "This entire branch will ultimately be vetted against the NCI Thesaurus and reviewed with NCICB staff working on representation for nervous system neoplasms (2007-10-05)."^^xsd:string ;
    NIFRID:createdDate "2007-10-05"^^xsd:string ;
    NIFRID:modifiedDate "April 29, 2010"^^xsd:string ;
    NIFRID:hasBirnlexCurator NIFRID:Bill_Bug ;
    NIFRID:hasCurationStatus NIFRID:uncurated ;
    NIFRID:hasExternalSource NIFRID:MeSH ;
    NIFRID:MeshUid "D009423"^^xsd:string ;
    NIFRID:nifID "_8.3_10"^^xsd:string .

BIRNLEX:12526 a owl:Class ;
    rdfs:label "Hereditary Central Nervous System Demyelinating Diseases"^^xsd:string ;
    skos:prefLabel "Hereditary Central Nervous System Demyelinating Diseases"^^xsd:string ;
    rdfs:subClassOf BIRNLEX:12507 ;
    NIFRID:createdDate "2007-10-05"^^xsd:string ;
    NIFRID:modifiedDate "2007-10-05"^^xsd:string ;
    NIFRID:hasBirnlexCurator NIFRID:Bill_Bug ;
    NIFRID:hasCurationStatus NIFRID:uncurated ;
    NIFRID:hasExternalSource NIFRID:MeSH ;
    NIFRID:MeshUid "D020279"^^xsd:string .

BIRNLEX:12527 a owl:Class ;
    rdfs:label "Adrenoleukodystrophy"^^xsd:string ;
    skos:prefLabel "Adrenoleukodystrophy"^^xsd:string ;
    NIFRID:synonym "Adrenomyeloneuropathy"^^xsd:string,
        "Schilder-Addison Complex"^^xsd:string,
        "X-Linked Adrenoleukodystrophy"^^xsd:string ;
    skos:definition "An X-linked recessive disorder characterized by the accumulation of saturated very long chain fatty acids in the LYSOSOMES of ADRENAL CORTEX and the white matter of CENTRAL NERVOUS SYSTEM. This disease occurs almost exclusively in the males. Clinical features include the childhood onset of ATAXIA; NEUROBEHAVIORAL MANIFESTATIONS; HYPERPIGMENTATION; ADRENAL INSUFFICIENCY; SEIZURES; MUSCLE SPASTICITY; and DEMENTIA. The slowly progressive adult form is called adrenomyeloneuropathy. The defective gene ABCD1 is located at Xq28, and encodes the adrenoleukodystrophy protein ( ATP-BINDING CASSETTE TRANSPORTERS) (MeSH)."^^xsd:string ;
    rdfs:subClassOf BIRNLEX:12526 ;
    NIFRID:createdDate "2007-10-05"^^xsd:string ;
    NIFRID:modifiedDate "2007-10-05"^^xsd:string ;
    NIFRID:acronym "ALD"^^xsd:string ;
    NIFRID:definingCitationURI <http://www.ninds.nih.gov/disorders/adrenoleukodystrophy/adrenoleukodystrophy.htm> ;
    NIFRID:hasBirnlexCurator NIFRID:Bill_Bug ;
    NIFRID:hasCurationStatus NIFRID:uncurated ;
    NIFRID:hasExternalSource NIFRID:MeSH ;
    NIFRID:MeshUid "D000326"^^xsd:string ;
    skos:scopeNote "Do not confuse with ADRENOLEUKODYSTROPHY, NEONATAL see PEROXISOMAL DISORDERS (MeSH)"^^xsd:string .

BIRNLEX:12528 a owl:Class ;
    rdfs:label "Alexander Disease"^^xsd:string ;
    skos:prefLabel "Alexander Disease"^^xsd:string ;
    NIFRID:synonym "Alexander's Disease"^^xsd:string,
        "Alexanders Disease"^^xsd:string ;
    skos:definition "A rare inherited disorder of myelin formation. Alexander disease is a progressive leukoencephalopathy whose hallmark is the widespread accumulation of cytoplasmic inclusions called Rosenthal fibers. The fibers contain GLIAL FIBRILLARY ACIDIC PROTEIN in association with ALPHA-CRYSTALLIN B CHAIN. Rosenthal fibers are found predominantly in ASTROCYTES located in the subependymal, subpial, and periventricular areas of the BRAIN (MeSH)."^^xsd:string ;
    rdfs:subClassOf BIRNLEX:12526 ;
    NIFRID:createdDate "2007-10-05"^^xsd:string ;
    NIFRID:modifiedDate "April 11, 2009"^^xsd:string ;
    NIFRID:definingCitationURI <http://www.ninds.nih.gov/disorders/alexander_disease/alexander_disease.htm> ;
    NIFRID:hasBirnlexCurator NIFRID:Bill_Bug ;
    NIFRID:hasCurationStatus NIFRID:uncurated ;
    NIFRID:hasExternalSource NIFRID:MeSH ;
    NIFRID:MeshUid "D038261"^^xsd:string .

BIRNLEX:12529 a owl:Class ;
    rdfs:label "Canavan Disease"^^xsd:string ;
    skos:prefLabel "Canavan Disease"^^xsd:string ;
    NIFRID:synonym "Aspartoacylase Deficiency Disease"^^xsd:string,
        "Canavan's Disease"^^xsd:string,
        "Canavan-van Bogaert-Bertrand Disease"^^xsd:string,
        "Canavans Disease"^^xsd:string,
        "Familial Form of Canavan Disease"^^xsd:string,
        "Leukodystrophy, Spongiform"^^xsd:string,
        "Spongy Disease of Central Nervous System"^^xsd:string,
        "Spongy Disease of White Matter"^^xsd:string ;
    skos:definition "A rare neurodegenerative condition of infancy or childhood characterized by white matter vacuolization and demeylination that gives rise to a spongy appearance. Aspartoacylase deficiency leads to an accumulation of N-acetylaspartate in astrocytes. Inheritance may be autosomal recessive or the illness may occur sporadically. This illness occurs more frequently in individuals of Ashkenazic Jewish descent. The neonatal form features the onset of hypotonia and lethargy at birth, rapidly progressing to coma and death. The infantile form features developmental delay, DYSKINESIAS, hypotonia, spasticity, blindness, and megalencephaly. The juvenile form is characterized by ATAXIA; OPTIC ATROPHY; and DEMENTIA (MeSH)."^^xsd:string ;
    rdfs:subClassOf BIRNLEX:12526 ;
    NIFRID:createdDate "2007-10-05"^^xsd:string ;
    NIFRID:modifiedDate "April 11, 2009"^^xsd:string ;
    NIFRID:definingCitation "Adams et al., Principles of Neurology, 6th ed, p944; Am J Med Genet 1988 Feb;29(2):463-71"^^xsd:string ;
    NIFRID:definingCitationURI <http://www.ninds.nih.gov/disorders/canavan/canavan.htm> ;
    NIFRID:hasBirnlexCurator NIFRID:Bill_Bug ;
    NIFRID:hasCurationStatus NIFRID:uncurated ;
    NIFRID:hasExternalSource NIFRID:MeSH ;
    NIFRID:MeshUid "D017825"^^xsd:string ;
    skos:scopeNote "Do not confuse X ref CANAVAN-VAN BOGAERT-BERTRAND DISEASE with VAN BOGAERT'S LEUKOENCEPHALITIS see SUBACUTE SCLEROSING PANENCEPHALITIS (MeSH)."^^xsd:string .

BIRNLEX:12530 a owl:Class ;
    rdfs:label "Type I Canavan Disease"^^xsd:string ;
    skos:prefLabel "Type I Canavan Disease"^^xsd:string ;
    NIFRID:synonym "Neonatal Canavan Disease"^^xsd:string,
        "Type I Canavan's Disease"^^xsd:string,
        "Type I Canavans Disease"^^xsd:string ;
    rdfs:subClassOf BIRNLEX:12529 ;
    NIFRID:createdDate "2007-10-05"^^xsd:string ;
    NIFRID:modifiedDate "April 11, 2009"^^xsd:string ;
    NIFRID:hasBirnlexCurator NIFRID:Bill_Bug ;
    NIFRID:hasCurationStatus NIFRID:uncurated ;
    NIFRID:hasExternalSource NIFRID:MeSH ;
    NIFRID:MeshUid "D017825"^^xsd:string .

BIRNLEX:12531 a owl:Class ;
    rdfs:label "Type II Canavan Disease"^^xsd:string ;
    skos:prefLabel "Type II Canavan Disease"^^xsd:string ;
    NIFRID:synonym "Infantile Canavan Disease"^^xsd:string,
        "Spongy Degeneration of Infancy"^^xsd:string,
        "Type II Canavan's Disease"^^xsd:string,
        "Type II Canavans Disease"^^xsd:string ;
    rdfs:subClassOf BIRNLEX:12529 ;
    NIFRID:createdDate "2007-10-05"^^xsd:string ;
    NIFRID:modifiedDate "April 11, 2009"^^xsd:string ;
    NIFRID:hasBirnlexCurator NIFRID:Bill_Bug ;
    NIFRID:hasCurationStatus NIFRID:uncurated ;
    NIFRID:hasExternalSource NIFRID:MeSH ;
    NIFRID:MeshUid "D017825"^^xsd:string .

BIRNLEX:12532 a owl:Class ;
    rdfs:label "Type III Canavan Disease"^^xsd:string ;
    skos:prefLabel "Type III Canavan Disease"^^xsd:string ;
    NIFRID:synonym "Juvenile Canavan Disease"^^xsd:string,
        "Type III Canavan's Disease"^^xsd:string,
        "Type III Canavans Disease"^^xsd:string ;
    rdfs:subClassOf BIRNLEX:12529 ;
    NIFRID:createdDate "2007-10-05"^^xsd:string ;
    NIFRID:modifiedDate "April 11, 2009"^^xsd:string ;
    NIFRID:hasBirnlexCurator NIFRID:Bill_Bug ;
    NIFRID:hasCurationStatus NIFRID:uncurated ;
    NIFRID:hasExternalSource NIFRID:MeSH ;
    NIFRID:MeshUid "D017825"^^xsd:string .

BIRNLEX:12533 a owl:Class ;
    rdfs:label "Globoid Cell Leukodystrophy"^^xsd:string ;
    skos:prefLabel "Globoid Cell Leukodystrophy"^^xsd:string ;
    NIFRID:synonym "Diffuse Globoid Body Sclerosis"^^xsd:string,
        "Galactosylceramidase Deficiency Disease"^^xsd:string,
        "Galactosylceramide-beta-Galactosidase Deficiency Disease"^^xsd:string,
        "Globoid Leukodystrophy"^^xsd:string,
        "Krabbe Disease"^^xsd:string,
        "Krabbe's Disease"^^xsd:string,
        "Krabbe's Leukodystrophy"^^xsd:string,
        "Krabbes Disease"^^xsd:string ;
    skos:definition "An autosomal recessive metabolic disorder caused by a deficiency of GALACTOSYLCERAMIDASE leading to intralysosomal accumulation of galactolipids such as GALACTOSYLCERAMIDES and PSYCHOSINE. It is characterized by demyelination associated with large multinucleated globoid cells, predominantly involving the white matter of the central nervous system. The loss of MYELIN disrupts normal conduction of nerve impulses (MeSH)."^^xsd:string ;
    rdfs:subClassOf BIRNLEX:12526 ;
    NIFRID:createdDate "2007-10-05"^^xsd:string ;
    NIFRID:modifiedDate "April 11, 2009"^^xsd:string ;
    NIFRID:definingCitationURI <http://www.ninds.nih.gov/disorders/krabbe/krabbe.htm> ;
    NIFRID:hasBirnlexCurator NIFRID:Bill_Bug ;
    NIFRID:hasCurationStatus NIFRID:uncurated ;
    NIFRID:hasExternalSource NIFRID:MeSH ;
    NIFRID:MeshUid "D007965"^^xsd:string .

BIRNLEX:12534 a owl:Class ;
    rdfs:label "Classic Globoid Cell Leukodystrophy"^^xsd:string ;
    skos:prefLabel "Classic Globoid Cell Leukodystrophy"^^xsd:string ;
    rdfs:subClassOf BIRNLEX:12533 ;
    NIFRID:createdDate "2007-10-05"^^xsd:string ;
    NIFRID:modifiedDate "2007-10-05"^^xsd:string ;
    NIFRID:hasBirnlexCurator NIFRID:Bill_Bug ;
    NIFRID:hasCurationStatus NIFRID:uncurated ;
    NIFRID:hasExternalSource NIFRID:MeSH ;
    NIFRID:MeshUid "D007965"^^xsd:string .

BIRNLEX:12535 a owl:Class ;
    rdfs:label "Infantile Globoid Cell Leukodystrophy"^^xsd:string ;
    skos:prefLabel "Infantile Globoid Cell Leukodystrophy"^^xsd:string ;
    rdfs:subClassOf BIRNLEX:12533 ;
    NIFRID:createdDate "2007-10-05"^^xsd:string ;
    NIFRID:modifiedDate "2007-10-05"^^xsd:string ;
    NIFRID:hasBirnlexCurator NIFRID:Bill_Bug ;
    NIFRID:hasCurationStatus NIFRID:uncurated ;
    NIFRID:hasExternalSource NIFRID:MeSH ;
    NIFRID:MeshUid "D007965"^^xsd:string .

BIRNLEX:12536 a owl:Class ;
    rdfs:label "Early-Onset Globoid Cell Leukodystrophy"^^xsd:string ;
    skos:prefLabel "Early-Onset Globoid Cell Leukodystrophy"^^xsd:string ;
    rdfs:subClassOf BIRNLEX:12533 ;
    NIFRID:createdDate "2007-10-05"^^xsd:string ;
    NIFRID:modifiedDate "2007-10-05"^^xsd:string ;
    NIFRID:hasBirnlexCurator NIFRID:Bill_Bug ;
    NIFRID:hasCurationStatus NIFRID:uncurated ;
    NIFRID:hasExternalSource NIFRID:MeSH ;
    NIFRID:MeshUid "D007965"^^xsd:string .

BIRNLEX:12537 a owl:Class ;
    rdfs:label "Late-Onset Globoid Cell Leukodystrophy"^^xsd:string ;
    skos:prefLabel "Late-Onset Globoid Cell Leukodystrophy"^^xsd:string ;
    rdfs:subClassOf BIRNLEX:12533 ;
    NIFRID:createdDate "2007-10-05"^^xsd:string ;
    NIFRID:modifiedDate "2007-10-05"^^xsd:string ;
    NIFRID:hasBirnlexCurator NIFRID:Bill_Bug ;
    NIFRID:hasCurationStatus NIFRID:uncurated ;
    NIFRID:hasExternalSource NIFRID:MeSH ;
    NIFRID:MeshUid "D007965"^^xsd:string .

BIRNLEX:12538 a owl:Class ;
    rdfs:label "Niemann-Pick Disease"^^xsd:string ;
    skos:prefLabel "Niemann-Pick Disease"^^xsd:string ;
    NIFRID:synonym "Niemann Pick Disease"^^xsd:string,
        "Niemann Pick's Disease"^^xsd:string,
        "Niemann-Pick Diseases"^^xsd:string,
        "Niemann-Pick's Disease"^^xsd:string ;
    skos:definition "A group of autosomal recessive disorders in which harmful quantities of lipids accumulate in the viscera and the central nervous system. They can be caused by deficiencies of enzyme activities ( SPHINGOMYELIN PHOSPHODIESTERASE) or defects in intracellular transport, resulting in the accumulation of SPHINGOMYELINS and CHOLESTEROL. There are various subtypes based on their clinical and genetic differences (MeSH)."^^xsd:string ;
    rdfs:subClassOf BIRNLEX:12526 ;
    NIFRID:createdDate "2007-10-05"^^xsd:string ;
    NIFRID:modifiedDate "April 11, 2009"^^xsd:string ;
    NIFRID:definingCitationURI <http://www.ninds.nih.gov/disorders/niemann/niemann.htm> ;
    NIFRID:hasBirnlexCurator NIFRID:Bill_Bug ;
    NIFRID:hasCurationStatus NIFRID:uncurated ;
    NIFRID:hasExternalSource NIFRID:MeSH ;
    NIFRID:MeshUid "D009542"^^xsd:string .

BIRNLEX:12539 a owl:Class ;
    rdfs:label "Niemann-Pick Disease, Type A"^^xsd:string ;
    skos:prefLabel "Niemann-Pick Disease, Type A"^^xsd:string ;
    NIFRID:synonym "Classical Niemann-Pick Disease"^^xsd:string,
        "Niemann Pick's Disease, Type A"^^xsd:string,
        "Niemann-Pick Disease, Acute Neuronopathic Form"^^xsd:string,
        "Niemann-Pick Disease, Acute Neurovisceral Form"^^xsd:string,
        "Niemann-Pick Disease, Neuronopathic Type"^^xsd:string,
        "Niemann-Pick's Disease, Type A"^^xsd:string,
        "Sphingomyelinase Deficiency Disease"^^xsd:string ;
    skos:definition "The classic infantile form of Niemann-Pick Disease, caused by mutation in SPHINGOMYELIN PHOSPHODIESTERASE. It is characterized by accumulation of SPHINGOMYELINS in the cells of the RETICULOENDOTHELIAL SYSTEM and other cell throughout the body leading to cell death. Clinical signs include JAUNDICE, hepatosplenomegaly, and severe brain damage (MeSH)."^^xsd:string ;
    rdfs:subClassOf BIRNLEX:12538 ;
    NIFRID:createdDate "2007-10-05"^^xsd:string ;
    NIFRID:modifiedDate "April 11, 2009"^^xsd:string ;
    NIFRID:hasBirnlexCurator NIFRID:Bill_Bug ;
    NIFRID:hasCurationStatus NIFRID:uncurated ;
    NIFRID:hasExternalSource NIFRID:MeSH ;
    NIFRID:MeshUid "D052536"^^xsd:string .

BIRNLEX:12540 a owl:Class ;
    rdfs:label "Niemann-Pick Disease, Type B"^^xsd:string ;
    skos:prefLabel "Niemann-Pick Disease, Type B"^^xsd:string ;
    NIFRID:synonym "Niemann Pick's Disease, Type B"^^xsd:string,
        "Niemann-Pick Disease, Adult Non-Neuronopathic"^^xsd:string,
        "Niemann-Pick Disease, Non-Neuronopathic Type"^^xsd:string,
        "Niemann-Pick Disease, Type E"^^xsd:string,
        "Niemann-Pick Disease, Visceral"^^xsd:string,
        "Niemann-Pick's Disease, Type B"^^xsd:string ;
    skos:definition "An allelic disorder of TYPE A NIEMANN-PICK DISEASE, a late-onset form. It is also caused by mutation in SPHINGOMYELIN PHOSPHODIESTERASE but clinical signs involve only visceral organs (non-neuropathic type) (MeSH)."^^xsd:string ;
    rdfs:subClassOf BIRNLEX:12538 ;
    NIFRID:createdDate "2007-10-05"^^xsd:string ;
    NIFRID:modifiedDate "April 11, 2009"^^xsd:string ;
    NIFRID:hasBirnlexCurator NIFRID:Bill_Bug ;
    NIFRID:hasCurationStatus NIFRID:uncurated ;
    NIFRID:hasExternalSource NIFRID:MeSH ;
    NIFRID:MeshUid "D052537"^^xsd:string .

BIRNLEX:12541 a owl:Class ;
    rdfs:label "Niemann-Pick Disease, Type C"^^xsd:string ;
    skos:prefLabel "Niemann-Pick Disease, Type C"^^xsd:string ;
    NIFRID:synonym "Neurovisceral Storage Disease with Vertical Supranuclear Ophthalmoplegia"^^xsd:string,
        "Niemann Pick Disease, Type C"^^xsd:string,
        "Niemann Pick's Disease, Type C"^^xsd:string,
        "Niemann-Pick Disease with Cholesterol Esterification Block"^^xsd:string,
        "Niemann-Pick Disease without Sphingomyelinase Deficiency"^^xsd:string,
        "Niemann-Pick Disease, Chronic Neuronopathic Form"^^xsd:string,
        "Niemann-Pick Disease, Nova Scotian"^^xsd:string,
        "Niemann-Pick Disease, Type D"^^xsd:string,
        "Niemann-Pick's Disease, Type C"^^xsd:string ;
    skos:definition "An autosomal recessive lipid storage disorder that is characterized by accumulation of CHOLESTEROL and SPHINGOMYELINS in cells of the VISCERA and the CENTRAL NERVOUS SYSTEM. Type C (or C1) and type D are allelic disorders caused by mutation of gene (NPC1) encoding a protein that mediate intracellular cholesterol transport from lysosomes. Clinical signs include hepatosplenomegaly and chronic neurological symptoms. Type D is a variant in people with a Nova Scotia ancestry (MeSH)."^^xsd:string ;
    rdfs:subClassOf BIRNLEX:12538 ;
    NIFRID:createdDate "2007-10-05"^^xsd:string ;
    NIFRID:modifiedDate "April 11, 2009"^^xsd:string ;
    NIFRID:hasBirnlexCurator NIFRID:Bill_Bug ;
    NIFRID:hasCurationStatus NIFRID:uncurated ;
    NIFRID:hasExternalSource NIFRID:MeSH ;
    NIFRID:MeshUid "D052556"^^xsd:string .

BIRNLEX:12542 a owl:Class ;
    rdfs:label "Metachromatic Leukodystrophy"^^xsd:string ;
    skos:prefLabel "Metachromatic Leukodystrophy"^^xsd:string ;
    NIFRID:synonym "Arylsulfatase A Deficiency Disease"^^xsd:string,
        "Cerebroside Sulphatase Deficiency Disease"^^xsd:string,
        "Greenfield's Disease"^^xsd:string,
        "Sulfatide Lipidosis"^^xsd:string ;
    skos:definition "An autosomal recessive metabolic disease caused by a deficiency of arylsulfatase A (CEREBROSIDE-SULFATASE) leading to intralysosomal accumulation of cerebroside sulfate ( SULFOGLYCOSPHINGOLIPIDS) in the nervous system and other organs. Pathological features include diffuse demyelination, and metachromatically-staining granules in many cell types such as the GLIAL CELLS. There are several allelic and nonallelic forms with a variety of neurological symptoms (MeSH)."^^xsd:string ;
    rdfs:subClassOf BIRNLEX:12526 ;
    NIFRID:createdDate "2007-10-05"^^xsd:string ;
    NIFRID:modifiedDate "2007-10-05"^^xsd:string ;
    NIFRID:definingCitationURI <http://www.ninds.nih.gov/disorders/metachromatic_leukodystrophy/metachromatic_leukodystrophy.htm> ;
    NIFRID:hasBirnlexCurator NIFRID:Bill_Bug ;
    NIFRID:hasCurationStatus NIFRID:uncurated ;
    NIFRID:hasExternalSource NIFRID:MeSH ;
    NIFRID:MeshUid "D007966"^^xsd:string .

BIRNLEX:12543 a owl:Class ;
    rdfs:label "Metachromatic Leukodystrophy, Infant-Type"^^xsd:string ;
    skos:prefLabel "Metachromatic Leukodystrophy, Infant-Type"^^xsd:string ;
    rdfs:subClassOf BIRNLEX:12542 ;
    NIFRID:createdDate "2007-10-05"^^xsd:string ;
    NIFRID:modifiedDate "2007-10-05"^^xsd:string ;
    NIFRID:hasBirnlexCurator NIFRID:Bill_Bug ;
    NIFRID:hasCurationStatus NIFRID:uncurated ;
    NIFRID:hasExternalSource NIFRID:MeSH ;
    NIFRID:MeshUid "D007966"^^xsd:string .

BIRNLEX:12544 a owl:Class ;
    rdfs:label "Metachromatic Leukodystrophy, Juvenile-Type"^^xsd:string ;
    skos:prefLabel "Metachromatic Leukodystrophy, Juvenile-Type"^^xsd:string ;
    rdfs:subClassOf BIRNLEX:12542 ;
    NIFRID:createdDate "2007-10-05"^^xsd:string ;
    NIFRID:modifiedDate "2007-10-05"^^xsd:string ;
    NIFRID:hasBirnlexCurator NIFRID:Bill_Bug ;
    NIFRID:hasCurationStatus NIFRID:uncurated ;
    NIFRID:hasExternalSource NIFRID:MeSH ;
    NIFRID:MeshUid "D007966"^^xsd:string .

BIRNLEX:12545 a owl:Class ;
    rdfs:label "Metachromatic Leukodystrophy, Adult-Type"^^xsd:string ;
    skos:prefLabel "Metachromatic Leukodystrophy, Adult-Type"^^xsd:string ;
    rdfs:subClassOf BIRNLEX:12542 ;
    NIFRID:createdDate "2007-10-05"^^xsd:string ;
    NIFRID:modifiedDate "2007-10-05"^^xsd:string ;
    NIFRID:hasBirnlexCurator NIFRID:Bill_Bug ;
    NIFRID:hasCurationStatus NIFRID:uncurated ;
    NIFRID:hasExternalSource NIFRID:MeSH ;
    NIFRID:MeshUid "D007966"^^xsd:string .

BIRNLEX:12546 a owl:Class ;
    rdfs:label "Pelizaeus-Merzbacher Disease"^^xsd:string ;
    skos:prefLabel "Pelizaeus-Merzbacher Disease"^^xsd:string ;
    NIFRID:synonym "Cockayne-Pelizaeus-Merzbacher Disease"^^xsd:string,
        "Pelizaeus Merzbacher's Disease"^^xsd:string,
        "Pelizaeus-Merzbacher's Disease"^^xsd:string ;
    skos:definition "A rare, slowly progressive disorder of myelin formation. Subtypes are referred to as classic, congenital, transitional, and adult forms of this disease. The classic form is X-chromosome linked, has its onset in infancy and is associated with a mutation of the proteolipid protein gene. Clinical manifestations include TREMOR, spasmus nutans, roving eye movements, ATAXIA, spasticity, and NYSTAGMUS, CONGENITAL. Death occurs by the third decade of life. The congenital form has similar characteristics but presents early in infancy and features rapid disease progression. Transitional and adult subtypes have a later onset and less severe symptomatology. Pathologic features include patchy areas of demyelination with preservation of perivascular islands (trigoid appearance) (MeSH)."^^xsd:string ;
    rdfs:subClassOf BIRNLEX:12526 ;
    NIFRID:createdDate "2007-10-05"^^xsd:string ;
    NIFRID:modifiedDate "April 11, 2009"^^xsd:string ;
    NIFRID:definingCitationURI <http://www.ninds.nih.gov/disorders/pelizaeus_merzbacher/pelizaeus_merzbacher.htm> ;
    NIFRID:hasBirnlexCurator NIFRID:Bill_Bug ;
    NIFRID:hasCurationStatus NIFRID:uncurated ;
    NIFRID:hasExternalSource NIFRID:MeSH ;
    NIFRID:MeshUid "D020371"^^xsd:string .

BIRNLEX:12547 a owl:Class ;
    rdfs:label "Classic Pelizaeus-Merzbacher Disease"^^xsd:string ;
    skos:prefLabel "Classic Pelizaeus-Merzbacher Disease"^^xsd:string ;
    NIFRID:synonym "Classic Pelizaeus Merzbacher's Disease"^^xsd:string,
        "Classic Pelizaeus-Merzbacher's Disease"^^xsd:string ;
    rdfs:subClassOf BIRNLEX:12546 ;
    NIFRID:createdDate "2007-10-05"^^xsd:string ;
    NIFRID:modifiedDate "April 11, 2009"^^xsd:string ;
    NIFRID:hasBirnlexCurator NIFRID:Bill_Bug ;
    NIFRID:hasCurationStatus NIFRID:uncurated ;
    NIFRID:hasExternalSource NIFRID:MeSH ;
    NIFRID:MeshUid "D020371"^^xsd:string .

BIRNLEX:12548 a owl:Class ;
    rdfs:label "Transitional Pelizaeus-Merzbacher Disease"^^xsd:string ;
    skos:prefLabel "Transitional Pelizaeus-Merzbacher Disease"^^xsd:string ;
    NIFRID:synonym "Transitional Pelizaeus Merzbacher's Disease"^^xsd:string,
        "Transitional Pelizaeus-Merzbacher's Disease"^^xsd:string ;
    rdfs:subClassOf BIRNLEX:12546 ;
    NIFRID:createdDate "2007-10-05"^^xsd:string ;
    NIFRID:modifiedDate "April 11, 2009"^^xsd:string ;
    NIFRID:hasBirnlexCurator NIFRID:Bill_Bug ;
    NIFRID:hasCurationStatus NIFRID:uncurated ;
    NIFRID:hasExternalSource NIFRID:MeSH ;
    NIFRID:MeshUid "D020371"^^xsd:string .

BIRNLEX:12550 a owl:Class ;
    rdfs:label "Adult Pelizaeus-Merzbacher Disease"^^xsd:string ;
    skos:prefLabel "Adult Pelizaeus-Merzbacher Disease"^^xsd:string ;
    NIFRID:synonym "Adult Pelizaeus-Merzbacher's Disease"^^xsd:string,
        "Adult Pelizaeus-Merzbachers Disease"^^xsd:string ;
    rdfs:subClassOf BIRNLEX:12546 ;
    NIFRID:createdDate "2007-10-05"^^xsd:string ;
    NIFRID:modifiedDate "April 11, 2009"^^xsd:string ;
    NIFRID:hasBirnlexCurator NIFRID:Bill_Bug ;
    NIFRID:hasCurationStatus NIFRID:uncurated ;
    NIFRID:hasExternalSource NIFRID:MeSH ;
    NIFRID:MeshUid "D020371"^^xsd:string .

BIRNLEX:12551 a owl:Class ;
    rdfs:label "Progressive Multifocal Leukoencephalopathy"^^xsd:string ;
    skos:prefLabel "Progressive Multifocal Leukoencephalopathy"^^xsd:string ;
    NIFRID:synonym "JC Polyomavirus Encephalopathy"^^xsd:string,
        "PML"^^xsd:string ;
    skos:definition "An opportunistic viral infection of the central nervous system associated with conditions that impair cell-mediated immunity (e.g., ACQUIRED IMMUNODEFICIENCY SYNDROME and other IMMUNOLOGIC DEFICIENCY SYNDROMES; HEMATOLOGIC NEOPLASMS; IMMUNOSUPPRESSION; and COLLAGEN DISEASES). The causative organism is JC Polyomavirus ( JC VIRUS) which primarily affects oligodendrocytes, resulting in multiple areas of demyelination. Clinical manifestations include DEMENTIA; ATAXIA; visual disturbances; and other focal neurologic deficits, generally progressing to a vegetative state within 6 months (MeSH)."^^xsd:string ;
    rdfs:subClassOf BIRNLEX:12507 ;
    NIFRID:createdDate "2007-10-05"^^xsd:string ;
    NIFRID:modifiedDate "2007-10-05"^^xsd:string ;
    NIFRID:definingCitationURI <http://www.ninds.nih.gov/disorders/pml/pml.htm> ;
    NIFRID:hasBirnlexCurator NIFRID:Bill_Bug ;
    NIFRID:hasCurationStatus NIFRID:uncurated ;
    NIFRID:hasExternalSource NIFRID:MeSH ;
    NIFRID:MeshUid "D007968"^^xsd:string .

BIRNLEX:12552 a owl:Class ;
    rdfs:label "Central Pontine Myelinolysis"^^xsd:string ;
    skos:prefLabel "Central Pontine Myelinolysis"^^xsd:string ;
    NIFRID:synonym "Extrapontine Myelinoclasis"^^xsd:string,
        "Extrapontine Myelinolysis"^^xsd:string ;
    skos:definition "A demyelinating condition affecting the PONS and characterized clinically by an acute progressive QUADRIPLEGIA; DYSARTHRIA; DYSPHAGIA; and alterations of consciousness. Pathologic features include prominent demyelination in the central PONS with sparing of axons and neurons. This condition is usually associated with systemic disorders such as HYPONATREMIA; chronic ALCOHOLISM; LIVER FAILURE; severe BURNS; malignant NEOPLASMS; hemorrhagic PANCREATITIS; HEMODIALYSIS; and SEPSIS. The rapid medical correction of hyponatremia has been cited as a cause of this condition (MeSH)."^^xsd:string ;
    rdfs:subClassOf BIRNLEX:12507 ;
    NIFRID:createdDate "2007-10-05"^^xsd:string ;
    NIFRID:modifiedDate "2007-10-05"^^xsd:string ;
    NIFRID:definingCitation "Adams et al., Principles of Neurology, 6th ed, pp1125-6"^^xsd:string ;
    NIFRID:definingCitationURI <http://www.ninds.nih.gov/disorders/central_pontine_myelinolysis.htm> ;
    NIFRID:hasBirnlexCurator NIFRID:Bill_Bug ;
    NIFRID:hasCurationStatus NIFRID:uncurated ;
    NIFRID:hasExternalSource NIFRID:MeSH ;
    NIFRID:MeshUid "D017590"^^xsd:string .

BIRNLEX:12553 a owl:Class ;
    rdfs:label "Polyradiculoneuropathy"^^xsd:string ;
    skos:prefLabel "Polyradiculoneuropathy"^^xsd:string ;
    NIFRID:synonym "Peripheral Autoimmune Demyelinating Disease"^^xsd:string,
        "Polyneuropathy"^^xsd:string,
        "Polyradiculoneuritis"^^xsd:string ;
    skos:definition "Diseases characterized by injury or dysfunction involving multiple peripheral nerves and nerve roots. The process may primarily affect myelin or nerve axons. Two of the more common demyelinating forms are acute inflammatory polyradiculopathy ( GUILLAIN-BARRE SYNDROME) and POLYRADICULONEUROPATHY, CHRONIC INFLAMMATORY DEMYELINATING. Polyradiculoneuritis refers to inflammation of multiple peripheral nerves and spinal nerve roots (MeSH)."^^xsd:string ;
    rdfs:subClassOf BIRNLEX:12507 ;
    NIFRID:createdDate "2007-10-05"^^xsd:string ;
    NIFRID:modifiedDate "2007-10-05"^^xsd:string ;
    NIFRID:hasBirnlexCurator NIFRID:Bill_Bug ;
    NIFRID:hasCurationStatus NIFRID:uncurated ;
    NIFRID:hasExternalSource NIFRID:MeSH ;
    NIFRID:MeshUid "D011129"^^xsd:string ;
    NIFRID:nifID "_8.3_3.2"^^xsd:string ;
    skos:scopeNote "Do not confuse with POLYRADICULOPATHY (disease of multiple nerve roots) nor with RADICULOPATHY (disease of a single nerve root)"^^xsd:string .

BIRNLEX:12554 a owl:Class ;
    rdfs:label "Guillain-Barre Syndrome"^^xsd:string ;
    skos:prefLabel "Guillain-Barre Syndrome"^^xsd:string ;
    NIFRID:synonym "Acute Autoimmune Neuropathy"^^xsd:string,
        "Acute Inflammatory Demyelinating Polyradiculoneuropathy"^^xsd:string,
        "Acute Inflammatory Polyneuropathy"^^xsd:string,
        "Acute Inflammatory Polyradiculoneuropathy"^^xsd:string,
        "Guillaine-Barre Syndrome"^^xsd:string,
        "Landry-Guillain-Barre Syndrome"^^xsd:string ;
    skos:definition "An acute inflammatory autoimmune neuritis caused by T cell- mediated cellular immune response directed towards peripheral myelin. Demyelination occurs in peripheral nerves and nerve roots. The process is often preceded by a viral or bacterial infection, surgery, immunization, lymphoma, or exposure to toxins. Common clinical manifestations include progressive weakness, loss of sensation, and loss of deep tendon reflexes. Weakness of respiratory muscles and autonomic dysfunction may occur (MeSH)."^^xsd:string ;
    rdfs:subClassOf BIRNLEX:12553 ;
    NIFRID:createdDate "2007-10-05"^^xsd:string ;
    NIFRID:modifiedDate "2007-10-05"^^xsd:string ;
    NIFRID:acronym "AIDP"^^xsd:string ;
    NIFRID:definingCitation "Adams et al., Principles of Neurology, 6th ed, pp1312-1314"^^xsd:string ;
    NIFRID:definingCitationURI <http://www.ninds.nih.gov/disorders/gbs/gbs.htm> ;
    NIFRID:hasBirnlexCurator NIFRID:Bill_Bug ;
    NIFRID:hasCurationStatus NIFRID:uncurated ;
    NIFRID:hasExternalSource NIFRID:MeSH ;
    NIFRID:MeshUid "D020275"^^xsd:string ;
    skos:scopeNote "Do not confuse X ref POLYRADICULONEUROPATHY, ACUTE INFLAMMATORY with POLYRADICULONEUROPATHY, CHRONIC INFLAMMATORY see POLYRADICULONEUROPATHY, CHRONIC INFLAMMATORY DEMYELINATING"^^xsd:string .

BIRNLEX:12555 a owl:Class ;
    rdfs:label "Miller Fisher Syndrome"^^xsd:string ;
    skos:prefLabel "Miller Fisher Syndrome"^^xsd:string ;
    NIFRID:synonym "Fisher Syndrome"^^xsd:string,
        "Guillain Barre Syndrome, Miller Fisher Variant"^^xsd:string,
        "Ophthalmoplegia, Ataxia and Areflexia Syndrome"^^xsd:string ;
    skos:definition "A variant of the GUILLAIN-BARRE SYNDROME characterized by the acute onset of oculomotor dysfunction, ataxia, and loss of deep tendon reflexes with relative sparing of strength in the extremities and trunk. The ataxia is produced by peripheral sensory nerve dysfunction and not by cerebellar injury. Facial weakness and sensory loss may also occur. The process is mediated by autoantibodies directed against a component of myelin found in peripheral nerves (MeSH)."^^xsd:string ;
    rdfs:subClassOf BIRNLEX:12554 ;
    NIFRID:createdDate "2007-10-05"^^xsd:string ;
    NIFRID:modifiedDate "2007-10-05"^^xsd:string ;
    NIFRID:definingCitation "Adams et al., Principles of Neurology, 6th ed, p1313; Neurology 1987 Sep;37(9):1493-8"^^xsd:string ;
    NIFRID:definingCitationURI <http://www.ninds.nih.gov/disorders/miller_fisher/miller_fisher.htm> ;
    NIFRID:hasBirnlexCurator NIFRID:Bill_Bug ;
    NIFRID:hasCurationStatus NIFRID:uncurated ;
    NIFRID:hasExternalSource NIFRID:MeSH ;
    NIFRID:MeshUid "D019846"^^xsd:string ;
    skos:scopeNote "X ref FISHER SYNDROME: do not confuse with the Fisher one-and-a-half syndrome, an eye movement disorder caused by a brain stem lesion."^^xsd:string .

BIRNLEX:12556 a owl:Class ;
    rdfs:label "Hereditary Sensory and Autonomic Neuropathies"^^xsd:string ;
    skos:prefLabel "Hereditary Sensory and Autonomic Neuropathies"^^xsd:string ;
    NIFRID:synonym "Congenital Insensitivity to Pain with Anhidrosis"^^xsd:string,
        "Hereditary Sensory Radicular Neuropathy"^^xsd:string ;
    skos:definition "A group of inherited disorders characterized by degeneration of dorsal root and autonomic ganglion cells, and clinically by loss of sensation and autonomic dysfunction. There are five subtypes. Type I features autosomal dominant inheritance and distal sensory involvement. Type II is characterized by autosomal inheritance and distal and proximal sensory loss. Type III is DYSAUTONOMIA, FAMILIAL. Type IV features insensitivity to pain, heat intolerance, and mental deficiency. Type V is characterized by a selective loss of pain with intact light touch and vibratory sensation (MeSH)."^^xsd:string ;
    rdfs:subClassOf BIRNLEX:12553 ;
    NIFRID:createdDate "2007-10-05"^^xsd:string ;
    NIFRID:modifiedDate "2007-10-05"^^xsd:string ;
    NIFRID:acronym "HSAN"^^xsd:string ;
    NIFRID:definingCitation "Joynt, Clinical Neurology, 1995, Ch51, pp142-4"^^xsd:string ;
    NIFRID:definingCitationURI <http://www.ninds.nih.gov/disorders/neuropathy_hereditary/neuropathy_hereditary.htm> ;
    NIFRID:hasBirnlexCurator NIFRID:Bill_Bug ;
    NIFRID:hasCurationStatus NIFRID:uncurated ;
    NIFRID:hasExternalSource NIFRID:MeSH ;
    NIFRID:MeshUid "D009477"^^xsd:string ;
    skos:scopeNote "Do not confuse with HEREDITARY MOTOR AND SENSORY NEUROPATHIES; for X refs to HSAN types: HSAN TYPE III is see DYSAUTONOMIA, FAMILIAL."^^xsd:string .

BIRNLEX:12557 a owl:Class ;
    rdfs:label "Hereditary Sensory Autonomic Neuropathy, Type 1"^^xsd:string ;
    skos:prefLabel "Hereditary Sensory Autonomic Neuropathy, Type 1"^^xsd:string ;
    NIFRID:abbrev "HSAN Type I"^^xsd:string,
        "HSN Type I"^^xsd:string ;
    rdfs:subClassOf BIRNLEX:12556 ;
    NIFRID:createdDate "2007-10-05"^^xsd:string ;
    NIFRID:modifiedDate "2007-10-05"^^xsd:string ;
    NIFRID:hasBirnlexCurator NIFRID:Bill_Bug ;
    NIFRID:hasCurationStatus NIFRID:uncurated ;
    NIFRID:hasExternalSource NIFRID:MeSH ;
    NIFRID:MeshUid "D009477"^^xsd:string .

BIRNLEX:12558 a owl:Class ;
    rdfs:label "Hereditary Sensory Autonomic Neuropathy, Type 2"^^xsd:string ;
    skos:prefLabel "Hereditary Sensory Autonomic Neuropathy, Type 2"^^xsd:string ;
    NIFRID:abbrev "HSAN Type II"^^xsd:string,
        "HSN Type II"^^xsd:string ;
    rdfs:subClassOf BIRNLEX:12556 ;
    NIFRID:createdDate "2007-10-05"^^xsd:string ;
    NIFRID:modifiedDate "2007-10-05"^^xsd:string ;
    NIFRID:hasBirnlexCurator NIFRID:Bill_Bug ;
    NIFRID:hasCurationStatus NIFRID:uncurated ;
    NIFRID:hasExternalSource NIFRID:MeSH ;
    NIFRID:MeshUid "D009477"^^xsd:string .

BIRNLEX:12559 a owl:Class ;
    rdfs:label "Hereditary Sensory Autonomic Neuropathy, Type 4"^^xsd:string ;
    skos:prefLabel "Hereditary Sensory Autonomic Neuropathy, Type 4"^^xsd:string ;
    NIFRID:abbrev "HSAN Type IV"^^xsd:string,
        "HSN Type IV"^^xsd:string ;
    rdfs:subClassOf BIRNLEX:12556 ;
    NIFRID:createdDate "2007-10-05"^^xsd:string ;
    NIFRID:modifiedDate "2007-10-05"^^xsd:string ;
    NIFRID:hasBirnlexCurator NIFRID:Bill_Bug ;
    NIFRID:hasCurationStatus NIFRID:uncurated ;
    NIFRID:hasExternalSource NIFRID:MeSH ;
    NIFRID:MeshUid "D009477"^^xsd:string .

BIRNLEX:12560 a owl:Class ;
    rdfs:label "Hereditary Sensory Autonomic Neuropathy, Type 5"^^xsd:string ;
    skos:prefLabel "Hereditary Sensory Autonomic Neuropathy, Type 5"^^xsd:string ;
    NIFRID:abbrev "HSAN Type V"^^xsd:string,
        "HSN Type V"^^xsd:string ;
    rdfs:subClassOf BIRNLEX:12556 ;
    NIFRID:createdDate "2007-10-05"^^xsd:string ;
    NIFRID:modifiedDate "2007-10-05"^^xsd:string ;
    NIFRID:hasBirnlexCurator NIFRID:Bill_Bug ;
    NIFRID:hasCurationStatus NIFRID:uncurated ;
    NIFRID:hasExternalSource NIFRID:MeSH ;
    NIFRID:MeshUid "D009477"^^xsd:string .

BIRNLEX:12561 a owl:Class ;
    rdfs:label "Familial Dysautonomia"^^xsd:string ;
    skos:prefLabel "Familial Dysautonomia"^^xsd:string ;
    NIFRID:synonym "Dominant Hereditary Sensory Neuropathy, Type 3"^^xsd:string,
        "Hereditary-Sensory and Autonomic Neuropathy Type III"^^xsd:string,
        "Neuropathy, Hereditary and Autonomic, Type III"^^xsd:string,
        "Riley-Day Syndrome"^^xsd:string ;
    NIFRID:abbrev "HSAN Type III"^^xsd:string ;
    skos:definition "An autosomal disorder of the peripheral and autonomic nervous systems limited to individuals of Ashkenazic Jewish descent. Clinical manifestations are present at birth and include diminished lacrimation, defective thermoregulation, orthostatic hypotension ( HYPOTENSION, ORTHOSTATIC), fixed pupils, excessive SWEATING, loss of pain and temperature sensation, and absent reflexes. Pathologic features include reduced numbers of small diameter peripheral nerve fibers and autonomic ganglion neurons (MeSH)."^^xsd:string ;
    rdfs:subClassOf BIRNLEX:12579 ;
    NIFRID:createdDate "2007-10-05"^^xsd:string ;
    NIFRID:modifiedDate "2007-10-05"^^xsd:string ;
    NIFRID:definingCitation "Adams et al., Principles of Neurology, 6th ed, p1348; Nat Genet 1993;4(2):160-4"^^xsd:string ;
    NIFRID:definingCitationURI <http://www.ninds.nih.gov/disorders/dysautonomia/dysautonomia.htm> ;
    NIFRID:hasBirnlexCurator NIFRID:Bill_Bug ;
    NIFRID:hasCurationStatus NIFRID:uncurated ;
    NIFRID:hasExternalSource NIFRID:MeSH ;
    NIFRID:MeshUid "D004402"^^xsd:string ;
    skos:scopeNote "Do not confuse with DYSAUTONOMIA see AUTONOMIC NERVOUS SYSTEM DISEASES."^^xsd:string .

BIRNLEX:12562 a owl:Class ;
    rdfs:label "Atypical Pelizaeus-Merzbacher Disease"^^xsd:string ;
    skos:prefLabel "Atypical Pelizaeus-Merzbacher Disease"^^xsd:string ;
    NIFRID:synonym "Atypical Pelizaeus Merzbacher's Disease"^^xsd:string,
        "Atypical Pelizaeus-Merzbacher's Disease"^^xsd:string ;
    rdfs:subClassOf BIRNLEX:12546 ;
    NIFRID:createdDate "2007-10-05"^^xsd:string ;
    NIFRID:modifiedDate "April 11, 2009"^^xsd:string ;
    NIFRID:hasBirnlexCurator NIFRID:Bill_Bug ;
    NIFRID:hasCurationStatus NIFRID:uncurated ;
    NIFRID:hasExternalSource NIFRID:MeSH ;
    NIFRID:MeshUid "D020371"^^xsd:string .

BIRNLEX:12563 a owl:Class ;
    rdfs:label "Chronic Inflammatory Demyelinating Polyradiculoneuropathy"^^xsd:string ;
    skos:prefLabel "Chronic Inflammatory Demyelinating Polyradiculoneuropathy"^^xsd:string ;
    NIFRID:synonym "Chronic Inflammatory Demyelinating Polyneuropathy"^^xsd:string,
        "Chronic Inflammatory Polyradiculoneuropathy"^^xsd:string,
        "Chronic Inflammatory Polyradiculopathy"^^xsd:string ;
    skos:definition "A slowly progressive autoimmune demyelinating disease of peripheral nerves and nerve roots. Clinical manifestations include weakness and sensory loss in the extremities and enlargement of peripheral nerves. The course may be relapsing-remitting or demonstrate a step-wise progression. Protein is usually elevated in the spinal fluid and cranial nerves are typically spared. GUILLAIN-BARRE SYNDROME features a relatively rapid progression of disease which distinguishes it from this condition (MeSH)."^^xsd:string ;
    rdfs:subClassOf BIRNLEX:12553 ;
    NIFRID:createdDate "2007-10-05"^^xsd:string ;
    NIFRID:modifiedDate "2007-10-05"^^xsd:string ;
    NIFRID:acronym "CIDP"^^xsd:string ;
    NIFRID:definingCitation "Adams et al., Principles of Neurology, 6th ed, p1337"^^xsd:string ;
    NIFRID:definingCitationURI <http://www.ninds.nih.gov/disorders/cidp/cidp.htm> ;
    NIFRID:hasBirnlexCurator NIFRID:Bill_Bug ;
    NIFRID:hasCurationStatus NIFRID:uncurated ;
    NIFRID:hasExternalSource NIFRID:MeSH ;
    NIFRID:MeshUid "D020277"^^xsd:string ;
    skos:scopeNote "Do do not confuse X ref CHRONIC INFLAMMATORY POLYRADICULONEUROPATHY with POLYRADICULONEUROPATHY, ACUTE INFLAMMATORY see GUILLAIN-BARRE SYNDROME."^^xsd:string .

BIRNLEX:12564 a owl:Class ;
    rdfs:label "Subacute Combined Degeneration"^^xsd:string ;
    skos:prefLabel "Subacute Combined Degeneration"^^xsd:string ;
    NIFRID:synonym "Subacute Combined Neuropathy Degeneration"^^xsd:string ;
    skos:definition "A neuropathy due to VITAMIN B 12 DEFICIENCY or to excessive NITROUS OXIDE inhalation. It is associated with overproduction of the myelinolytic TUMOR NECROSIS FACTOR-ALPHA (MeSH)."^^xsd:string ;
    rdfs:subClassOf BIRNLEX:12507 ;
    NIFRID:createdDate "2007-10-05"^^xsd:string ;
    NIFRID:modifiedDate "2007-10-05"^^xsd:string ;
    NIFRID:hasBirnlexCurator NIFRID:Bill_Bug ;
    NIFRID:hasCurationStatus NIFRID:uncurated ;
    NIFRID:hasExternalSource NIFRID:MeSH ;
    NIFRID:MeshUid "D052879"^^xsd:string .

BIRNLEX:12565 a owl:Class ;
    rdfs:label "Motor Neuron Disease"^^xsd:string ;
    skos:prefLabel "Motor Neuron Disease"^^xsd:string ;
    NIFRID:synonym "Motor System Disease"^^xsd:string ;
    skos:definition "Diseases characterized by a selective degeneration of the motor neurons of the spinal cord, brainstem, or motor cortex. Clinical subtypes are distinguished by the major site of degeneration. In AMYOTROPHIC LATERAL SCLEROSIS there is involvement of upper, lower, and brainstem motor neurons. In progressive muscular atrophy and related syndromes (see MUSCULAR ATROPHY, SPINAL) the motor neurons in the spinal cord are primarily affected. With progressive bulbar palsy ( BULBAR PALSY, PROGRESSIVE), the initial degeneration occurs in the brainstem. In primary lateral sclerosis, the cortical neurons are affected in isolation (MeSH)."^^xsd:string ;
    rdfs:subClassOf BIRNLEX:2086 ;
    NIFRID:createdDate "2007-10-05"^^xsd:string ;
    NIFRID:modifiedDate "2007-11-18"^^xsd:string ;
    NIFRID:definingCitation "Adams et al., Principles of Neurology, 6th ed, p1089"^^xsd:string ;
    NIFRID:definingCitationURI <http://www.ninds.nih.gov/disorders/motor_neuron_diseases/motor_neuron_diseases.htm> ;
    NIFRID:hasBirnlexCurator NIFRID:Bill_Bug ;
    NIFRID:hasCurationStatus NIFRID:uncurated ;
    NIFRID:hasDefinitionSource NIFRID:MeSH_defSource ;
    NIFRID:hasExternalSource NIFRID:MeSH ;
    NIFRID:MeshUid "D016472"^^xsd:string ;
    NIFRID:nifID "_8.3_2.5"^^xsd:string ;
    NIFRID:UmlsCui "C0085084"^^xsd:string ;
    NIFRID:usageNote "Note that MeSH includes the following sub-types which cannot easily be specified as subtypes without leading to multiple inheritance (e.g., Anterior Horn Cell Disease; Familial Motor Neuron Disease; Lateral Sclerosis; Lower Motor Neuron Disease; Upper Motor Neuron Disease; Primary Lateral Sclerosis; Secondary Motor Neuron Disease).  These subtypes describe either the location within the CNS axis where motor neuron degeneration is observed, the complex temporal development of that degeneration, and the hereditory nature of the disorder.  In the course of many specific patient cases, the location of degenerating MNs starts in one location and then procedes to others, as is the case for some of the concrete child classess created for this parent class.  In the end, a more detailed OWL representation would need to be employed where the location, timing, and putative casue of degenerating MNs is specified using ObjectProperties, and such subtypes as LOWER MOTOR NEURON DISEASE would then be inferred types.  The practical problem with this approach is that terms such as ALS and LOWER MN DISEASE have a particular meaning in a clinical context.  Though ALS might be inferred to be a member of the set of LOWER MN DISEASEs, since there is loss of MNs in the lower spinal cord, clinicians typically consider LOWER MN DISEASE to have a distinct set of presenting signs when compared to ALS.  Clinicians do not typically consider ALS to be a type of LOWER MN DISEASE (BB: 2007-10-05)"^^xsd:string .

BIRNLEX:12566 a owl:Class ;
    rdfs:label "Amyotrophic Lateral Sclerosis"^^xsd:string ;
    skos:prefLabel "Amyotrophic Lateral Sclerosis"^^xsd:string ;
    NIFRID:synonym "Gehrig's Disease"^^xsd:string,
        "Gehrigs Disease"^^xsd:string,
        "Lou Gehrig Disease"^^xsd:string,
        "Lou Gehrig's Disease"^^xsd:string,
        "Lou Gehrigs Disease"^^xsd:string ;
    skos:definition "A degenerative disorder affecting upper MOTOR NEURONS in the brain and lower motor neurons in the brain stem and SPINAL CORD. Disease onset is usually after the age of 50 and the process is usually fatal within 3 to 6 years. Clinical manifestations include progressive weakness, atrophy, FASCICULATION, hyperreflexia, DYSARTHRIA, dysphagia, and eventual paralysis of respiratory function. Pathologic features include the replacement of motor neurons with fibrous ASTROCYTES and atrophy of anterior SPINAL NERVE ROOTS and corticospinal tracts (MeSH)."^^xsd:string ;
    rdfs:subClassOf BIRNLEX:12565 ;
    NIFRID:createdDate "2007-10-05"^^xsd:string ;
    NIFRID:modifiedDate "April 11, 2009"^^xsd:string ;
    NIFRID:acronym "ALS"^^xsd:string ;
    NIFRID:definingCitation "Adams et al., Principles of Neurology, 6th ed, pp1089-94"^^xsd:string ;
    NIFRID:definingCitationURI <http://www.ninds.nih.gov/disorders/amyotrophiclateralsclerosis/amyotrophiclateralsclerosis.htm> ;
    NIFRID:hasBirnlexCurator NIFRID:Bill_Bug ;
    NIFRID:hasCurationStatus NIFRID:uncurated ;
    NIFRID:hasDefinitionSource NIFRID:MeSH_defSource ;
    NIFRID:hasExternalSource NIFRID:MeSH ;
    NIFRID:MeshUid "D000690"^^xsd:string ;
    NIFRID:nifID "_8.3_2.5.1"^^xsd:string .

BIRNLEX:12567 a owl:Class ;
    rdfs:label "Progressive Bulbar Palsy"^^xsd:string ;
    skos:prefLabel "Progressive Bulbar Palsy"^^xsd:string ;
    NIFRID:synonym "Bulbar Palsy"^^xsd:string,
        "Bulbar paralysis"^^xsd:string,
        "Fazio-Londe Syndrome"^^xsd:string,
        "Fazio-Londe's Syndrome"^^xsd:string ;
    skos:definition "A motor neuron disease marked by progressive weakness of the muscles innervated by cranial nerves of the lower brain stem. Clinical manifestations include dysarthria, dysphagia, facial weakness, tongue weakness, and fasciculations of the tongue and facial muscles. The adult form of the disease is marked initially by bulbar weakness which progresses to involve motor neurons throughout the neuroaxis. Eventually this condition may become indistinguishable from AMYOTROPHIC LATERAL SCLEROSIS. Fazio-Londe syndrome is an inherited form of this illness which occurs in children and young adults (MeSH)."^^xsd:string ;
    rdfs:subClassOf BIRNLEX:12565 ;
    NIFRID:createdDate "2007-10-05"^^xsd:string ;
    NIFRID:modifiedDate "2007-11-18"^^xsd:string ;
    NIFRID:definingCitation "Adams et al., Principles of Neurology, 6th ed, p1091; Brain 1992 Dec;115(Pt 6):1889-1900"^^xsd:string ;
    NIFRID:hasBirnlexCurator NIFRID:Bill_Bug ;
    NIFRID:hasCurationStatus NIFRID:uncurated ;
    NIFRID:hasDefinitionSource NIFRID:MeSH_defSource ;
    NIFRID:hasExternalSource NIFRID:MeSH ;
    NIFRID:MeshUid "D010244"^^xsd:string ;
    NIFRID:UmlsCui "C0030442"^^xsd:string .

BIRNLEX:12568 a owl:Class ;
    rdfs:label "Spinal muscular atrophy"^^xsd:string ;
    skos:prefLabel "Spinal Muscular Atrophy"^^xsd:string ;
    NIFRID:synonym "Bulbospinal Neuronopathy"^^xsd:string,
        "Kennedy Syndrome"^^xsd:string,
        "Kennedy's Syndrome"^^xsd:string,
        "Progressive Myelopathic Muscular Atrophy"^^xsd:string ;
    skos:definition "A group of disorders marked by progressive degeneration of motor neurons in the spinal cord resulting in weakness and muscular atrophy, usually without evidence of injury to the corticospinal tracts. Diseases in this category include Werdnig-Hoffmann disease and later onset SPINAL MUSCULAR ATROPHIES OF CHILDHOOD, most of which are hereditary (MeSH)."^^xsd:string ;
    rdfs:subClassOf BIRNLEX:12565 ;
    NIFRID:createdDate "2007-10-05"^^xsd:string ;
    NIFRID:modifiedDate "April 11, 2009"^^xsd:string ;
    NIFRID:acronym "SMA"^^xsd:string ;
    NIFRID:definingCitation "Adams et al., Principles of Neurology, 6th ed, p1089"^^xsd:string ;
    NIFRID:definingCitationURI <http://www.ninds.nih.gov/disorders/sma/sma.htm> ;
    NIFRID:hasBirnlexCurator NIFRID:Bill_Bug ;
    NIFRID:hasCurationStatus NIFRID:uncurated ;
    NIFRID:hasDefinitionSource NIFRID:MeSH_defSource ;
    NIFRID:hasExternalSource NIFRID:MeSH ;
    NIFRID:MeshUid "D009134"^^xsd:string ;
    NIFRID:nifID "_8.3_2.5.2"^^xsd:string ;
    NIFRID:putativeClassExtension "Adult Spinal Muscular Atrophy"^^xsd:string,
        "Distal Spinal Muscular Atrophy"^^xsd:string,
        "Oculopharyngeal Spinal Muscular Atrophy"^^xsd:string,
        "Progressive Proximal Myelopathic Muscular Atrophy"^^xsd:string,
        "Scapuloperoneal Form of Spinal Muscular Atrophy"^^xsd:string ;
    NIFRID:UmlsCui "C0026847"^^xsd:string .

BIRNLEX:12569 a owl:Class ;
    rdfs:label "Spinal Muscular Atrophies of Childhood"^^xsd:string ;
    skos:prefLabel "Spinal Muscular Atrophies of Childhood"^^xsd:string ;
    NIFRID:synonym "Bulbospinal Neuronopathy"^^xsd:string,
        "Kennedy Syndrome"^^xsd:string,
        "Kennedy's Syndrome"^^xsd:string,
        "Progressive Myelopathic Muscular Atrophy"^^xsd:string ;
    skos:definition "A group of recessively inherited diseases that feature progressive muscular atrophy and hypotonia. They are classified as type I (Werdnig-Hoffman disease), type II (intermediate form), and type III (Kugelberg-Welander disease). Type I is fatal in infancy, type II has a late infantile onset and is associated with survival into the second or third decade. Type III has its onset in childhood, and is slowly progressive (MeSH)."^^xsd:string ;
    rdfs:subClassOf BIRNLEX:12568 ;
    NIFRID:createdDate "2007-10-05"^^xsd:string ;
    NIFRID:modifiedDate "April 11, 2009"^^xsd:string ;
    NIFRID:definingCitation "J Med Genet 1996 Apr:33(4):281-3"^^xsd:string ;
    NIFRID:definingCitationURI <http://www.ninds.nih.gov/disorders/kennedys/kennedys.htm> ;
    NIFRID:hasBirnlexCurator NIFRID:Bill_Bug ;
    NIFRID:hasCurationStatus NIFRID:uncurated ;
    NIFRID:hasDefinitionSource NIFRID:MeSH_defSource ;
    NIFRID:hasExternalSource NIFRID:MeSH ;
    NIFRID:MeshUid "D009134"^^xsd:string ;
    skos:scopeNote "Infantile, childhood or adolescent: for other, MUSCULAR ATROPHY, SPINAL is available (MeSH)."^^xsd:string .

BIRNLEX:12570 a owl:Class ;
    rdfs:label "Type I Spinal Muscular Atrophy"^^xsd:string ;
    skos:prefLabel "Type I Spinal Muscular Atrophy"^^xsd:string ;
    NIFRID:synonym "Hereditary Motor Neuropathy Proximal Type I"^^xsd:string,
        "Infantile Spinal Muscular Atrophy"^^xsd:string,
        "Werdnig-Hoffmann Disease"^^xsd:string ;
    NIFRID:abbrev "HMN Proximal Type I"^^xsd:string ;
    rdfs:subClassOf BIRNLEX:12569 ;
    NIFRID:createdDate "2007-10-05"^^xsd:string ;
    NIFRID:modifiedDate "2007-11-18"^^xsd:string ;
    NIFRID:acronym "WHD"^^xsd:string ;
    NIFRID:definingCitation "J Med Genet 1996 Apr:33(4):281-3"^^xsd:string ;
    NIFRID:hasBirnlexCurator NIFRID:Bill_Bug ;
    NIFRID:hasCurationStatus NIFRID:uncurated ;
    NIFRID:hasDefinitionSource NIFRID:MeSH_defSource ;
    NIFRID:hasExternalSource NIFRID:MeSH ;
    NIFRID:MeshUid "D014897"^^xsd:string ;
    NIFRID:UmlsCui "C0043116"^^xsd:string ;
    NIFRID:usageNote "Type I is fatal in infancy (MeSH)."^^xsd:string ;
    skos:scopeNote "Additional MeSH entry terms imply there are subtypes based on the location of the motor neuron degeneration - e.g.: Proximal Hereditary Motor Neuropathy (HMN) Type I"^^xsd:string .

BIRNLEX:12571 a owl:Class ;
    rdfs:label "Type II Spinal Muscular Atrophy"^^xsd:string ;
    skos:prefLabel "Type II Spinal Muscular Atrophy"^^xsd:string ;
    NIFRID:synonym "Late infantile spinal muscular atrophy"^^xsd:string ;
    NIFRID:abbrev "SMA2"^^xsd:string ;
    rdfs:subClassOf BIRNLEX:12569 ;
    NIFRID:createdDate "2007-10-05"^^xsd:string ;
    NIFRID:modifiedDate "2007-11-18"^^xsd:string ;
    NIFRID:definingCitation "J Med Genet 1996 Apr:33(4):281-3"^^xsd:string ;
    NIFRID:hasBirnlexCurator NIFRID:Bill_Bug ;
    NIFRID:hasCurationStatus NIFRID:uncurated ;
    NIFRID:hasDefinitionSource NIFRID:MeSH_defSource ;
    NIFRID:hasExternalSource NIFRID:MeSH ;
    NIFRID:MeshUid "D014897"^^xsd:string ;
    NIFRID:UmlsCui "C0393538"^^xsd:string ;
    skos:scopeNote "Type II has a late infantile onset and is associated with survival into the second or third decade (MeSH)."^^xsd:string .

BIRNLEX:12572 a owl:Class ;
    rdfs:label "Type III Spinal Muscular Atrophy"^^xsd:string ;
    skos:prefLabel "Type III Spinal Muscular Atrophy"^^xsd:string ;
    NIFRID:synonym "Juvenile Spinal Muscular Atrophy"^^xsd:string,
        "Kugelberg-Welander Disease"^^xsd:string ;
    NIFRID:abbrev "SMA3"^^xsd:string,
        "SMA type III"^^xsd:string ;
    rdfs:subClassOf BIRNLEX:12569 ;
    NIFRID:createdDate "2007-10-05"^^xsd:string ;
    NIFRID:modifiedDate "2007-11-18"^^xsd:string ;
    NIFRID:definingCitation "J Med Genet 1996 Apr:33(4):281-3"^^xsd:string ;
    NIFRID:hasBirnlexCurator NIFRID:Bill_Bug ;
    NIFRID:hasCurationStatus NIFRID:uncurated ;
    NIFRID:hasDefinitionSource NIFRID:MeSH_defSource ;
    NIFRID:hasExternalSource NIFRID:MeSH ;
    NIFRID:MeshUid "D014897"^^xsd:string ;
    NIFRID:UmlsCui "C0152109"^^xsd:string ;
    skos:scopeNote "Type III has its onset in childhood and is slowly progressive (MeSH)."^^xsd:string .

BIRNLEX:12573 a owl:Class ;
    rdfs:label "Multiple System Atrophy"^^xsd:string ;
    skos:prefLabel "Multiple System Atrophy"^^xsd:string ;
    NIFRID:synonym "Multiple System Atrophy Syndrome"^^xsd:string,
        "Multisystem Atrophy"^^xsd:string,
        "Multisystemic Atrophy"^^xsd:string ;
    skos:definition "A syndrome complex composed of three conditions which represent clinical variants of the same disease process: STRIATONIGRAL DEGENERATION; SHY-DRAGER SYNDROME; and the sporadic form of OLIVOPONTOCEREBELLAR ATROPHIES. Clinical features include autonomic, cerebellar, and basal ganglia dysfunction. Pathologic examination reveals atrophy of the basal ganglia, cerebellum, pons, and medulla, with prominent loss of autonomic neurons in the brain stem and spinal cord (MeSH)."^^xsd:string ;
    rdfs:subClassOf BIRNLEX:2086 ;
    NIFRID:createdDate "2007-10-05"^^xsd:string ;
    NIFRID:modifiedDate "2007-10-05"^^xsd:string ;
    NIFRID:definingCitation "Adams et al., Principles of Neurology, 6th ed, p1076; Baillieres Clin Neurol 1997 Apr;6(1):187-204; Med Clin North Am 1999 Mar;83(2):381-92"^^xsd:string ;
    NIFRID:definingCitationURI <http://www.ninds.nih.gov/disorders/msa/msa.htm> ;
    NIFRID:hasBirnlexCurator NIFRID:Bill_Bug ;
    NIFRID:hasCurationStatus NIFRID:uncurated ;
    NIFRID:hasDefinitionSource NIFRID:MeSH_defSource ;
    NIFRID:hasExternalSource NIFRID:MeSH ;
    NIFRID:MeshUid "D019578"^^xsd:string ;
    NIFRID:nifID "_8.3_2.11"^^xsd:string ;
    skos:scopeNote "A specific neurodegenerative syndrome complex; not for atrophy in other systems (BB: 2007-10-05)"^^xsd:string .

BIRNLEX:12574 a owl:Class ;
    rdfs:label "Olivopontocerebellar Atrophy"^^xsd:string ;
    skos:prefLabel "Olivopontocerebellar Atrophy"^^xsd:string ;
    NIFRID:synonym "Dejerine-Thomas Syndrome"^^xsd:string,
        "Olivo-Ponto-Cerebellar Atrophy"^^xsd:string,
        "Olivo-Ponto-Cerebellar Degeneration"^^xsd:string,
        "Olivopontocerebellar Atrophies"^^xsd:string,
        "Olivopontocerebellar Atrophy"^^xsd:string,
        "Olivopontocerebellar Degeneration"^^xsd:string,
        "Pontoolivocerebellar Atrophy"^^xsd:string,
        "Presenile Ataxia"^^xsd:string ;
    skos:definition "A group of inherited and sporadic disorders which share progressive ataxia in combination with atrophy of the CEREBELLUM; PONS; and inferior olivary nuclei. Additional clinical features may include MUSCLE RIGIDITY; NYSTAGMUS, PATHOLOGIC; RETINAL DEGENERATION; MUSCLE SPASTICITY; DEMENTIA; URINARY INCONTINENCE; and OPHTHALMOPLEGIA. The familial form has an earlier onset (second decade) and may feature spinal cord atrophy. The sporadic form tends to present in the fifth or sixth decade, and is considered a clinical subtype of MULTIPLE SYSTEM ATROPHY (MeSH)."^^xsd:string ;
    rdfs:subClassOf BIRNLEX:12573 ;
    NIFRID:createdDate "2007-10-05"^^xsd:string ;
    NIFRID:modifiedDate "2007-10-05"^^xsd:string ;
    NIFRID:definingCitation "Adams et al., Principles of Neurology, 6th ed, p1085"^^xsd:string ;
    NIFRID:definingCitationURI <http://www.ninds.nih.gov/disorders/opca/opca.htm> ;
    NIFRID:hasBirnlexCurator NIFRID:Bill_Bug ;
    NIFRID:hasCurationStatus NIFRID:uncurated ;
    NIFRID:hasDefinitionSource NIFRID:MeSH_defSource ;
    NIFRID:hasExternalSource NIFRID:MeSH ;
    NIFRID:MeshUid "D009849"^^xsd:string ;
    NIFRID:UmlsCui "C0028968"^^xsd:string ;
    NIFRID:usageNote "The MeSH term has the following implied subtypes: Nonfamilial Olivopontocerebellar Atrophy; Idiopathic Olivopontocerebellar Atrophy"^^xsd:string .

BIRNLEX:12575 a owl:Class ;
    rdfs:label "Familial Olivopontocerebellar Atrophy"^^xsd:string ;
    skos:prefLabel "Familial Olivopontocerebellar Atrophy"^^xsd:string ;
    NIFRID:synonym "Inherited Olivopontocerebellar Atrophy"^^xsd:string ;
    rdfs:subClassOf BIRNLEX:12574 ;
    NIFRID:createdDate "2007-10-05"^^xsd:string ;
    NIFRID:modifiedDate "2007-10-05"^^xsd:string ;
    NIFRID:definingCitation "Adams et al., Principles of Neurology, 6th ed, p1085"^^xsd:string ;
    NIFRID:hasBirnlexCurator NIFRID:Bill_Bug ;
    NIFRID:hasCurationStatus NIFRID:uncurated ;
    NIFRID:hasDefinitionSource NIFRID:MeSH_defSource ;
    NIFRID:hasExternalSource NIFRID:MeSH ;
    NIFRID:MeshUid "D009849"^^xsd:string ;
    skos:scopeNote "The familial form has an earlier onset (second decade) and may feature spinal cord atrophy. (BB: 2007-10-05)"^^xsd:string .

BIRNLEX:12576 a owl:Class ;
    rdfs:label "Shy-Drager Syndrome"^^xsd:string ;
    skos:prefLabel "Shy-Drager Syndrome"^^xsd:string ;
    NIFRID:synonym "Dysautonomia-Orthostatic Hypotension Syndrome"^^xsd:string,
        "Dysautonomic Orthostatic Hypotension"^^xsd:string,
        "Idiopathic Orthostatic Hypotension, Shy-Drager Type"^^xsd:string,
        "Multiple System Atrophy with Orthostatic Hypotension"^^xsd:string,
        "Progressive Autonomic Failure"^^xsd:string ;
    skos:definition "A progressive neurodegenerative condition of the central and autonomic nervous systems characterized by atrophy of the preganglionic lateral horn neurons of the thoracic spinal cord, which differentiates this condition from other forms of idiopathic orthostatic hypotension ( HYPOTENSION, ORTHOSTATIC). This disease is generally considered a clinical variant of MULTIPLE SYSTEM ATROPHY. Affected individuals present in the fifth or sixth decade with orthostasis and bladder dysfunction; and later develop FECAL INCONTINENCE; anhidrosis; ATAXIA; IMPOTENCE; and alterations of tone suggestive of basal ganglia dysfunction (MeSH)."^^xsd:string ;
    rdfs:subClassOf BIRNLEX:12579 ;
    NIFRID:createdDate "2007-10-05"^^xsd:string ;
    NIFRID:modifiedDate "2007-10-05"^^xsd:string ;
    NIFRID:definingCitation "Adams et al., Principles of Neurology, 6th ed, p536"^^xsd:string ;
    NIFRID:definingCitationURI <http://www.ninds.nih.gov/disorders/striatonigral_degeneration/striatonigral_degeneration.htm> ;
    NIFRID:hasBirnlexCurator NIFRID:Bill_Bug ;
    NIFRID:hasCurationStatus NIFRID:uncurated ;
    NIFRID:hasDefinitionSource NIFRID:MeSH_defSource ;
    NIFRID:hasExternalSource NIFRID:MeSH ;
    NIFRID:MeshUid "D012791"^^xsd:string .

BIRNLEX:12577 a owl:Class ;
    rdfs:label "Striatonigral Degeneration"^^xsd:string ;
    skos:prefLabel "Striatonigral Degeneration"^^xsd:string ;
    NIFRID:synonym "Striatonigral Atrophy"^^xsd:string ;
    skos:definition "A sporadic neurodegenerative disease with onset in middle-age characterized clinically by Parkinsonian features (e.g., MUSCLE RIGIDITY; HYPOKINESIA; stooped posture) and HYPOTENSION. This condition is considered a clinical variant of MULTIPLE SYSTEM ATROPHY. Pathologic features include a prominent loss of neurons in the zona compacta of the SUBSTANTIA NIGRA and PUTAMEN (MeSH)."^^xsd:string ;
    rdfs:subClassOf BIRNLEX:12573 ;
    NIFRID:createdDate "2007-10-05"^^xsd:string ;
    NIFRID:modifiedDate "2007-10-05"^^xsd:string ;
    NIFRID:definingCitation "Adams et al., Principles of Neurology, 6th ed, p1075-6"^^xsd:string ;
    NIFRID:definingCitationURI <http://www.ninds.nih.gov/disorders/msa_orthostatic_hypotension/msa_orthostatic_hypotension.htm> ;
    NIFRID:hasBirnlexCurator NIFRID:Bill_Bug ;
    NIFRID:hasCurationStatus NIFRID:uncurated ;
    NIFRID:hasDefinitionSource NIFRID:MeSH_defSource ;
    NIFRID:hasExternalSource NIFRID:MeSH ;
    NIFRID:MeshUid "D020955"^^xsd:string ;
    NIFRID:UmlsCui "C0270733"^^xsd:string .

BIRNLEX:12578 a owl:Class ;
    rdfs:label "Neuromuscular Disease"^^xsd:string ;
    skos:prefLabel "Neuromuscular Disease"^^xsd:string ;
    skos:definition "A general term encompassing lower MOTOR NEURON DISEASE; PERIPHERAL NERVOUS SYSTEM DISEASES; and certain MUSCULAR DISEASES. Manifestations include MUSCLE WEAKNESS; FASCICULATION; muscle ATROPHY; SPASM; MYOKYMIA; MUSCLE HYPERTONIA, myalgias, and MUSCLE HYPOTONIA (MeSH)."^^xsd:string ;
    rdfs:subClassOf BIRNLEX:12822 ;
    NIFRID:createdDate "2007-10-05"^^xsd:string ;
    NIFRID:modifiedDate "2007-11-18"^^xsd:string ;
    NIFRID:hasBirnlexCurator NIFRID:Bill_Bug ;
    NIFRID:hasCurationStatus NIFRID:uncurated ;
    NIFRID:hasDefinitionSource NIFRID:MeSH_defSource ;
    NIFRID:hasExternalSource NIFRID:MeSH ;
    NIFRID:MeshUid "D009468"^^xsd:string ;
    NIFRID:nifID "_8.3_9"^^xsd:string .

BIRNLEX:12579 a owl:Class ;
    rdfs:label "Autonomic Nervous System Disease"^^xsd:string ;
    skos:prefLabel "Autonomic Nervous System Disease"^^xsd:string ;
    NIFRID:synonym "ANS Diseases"^^xsd:string,
        "Autonomic Diseases"^^xsd:string,
        "Autonomic Nervous System Disorders"^^xsd:string,
        "Autonomic Peripheral Nervous System Diseases"^^xsd:string,
        "Dysautonomia"^^xsd:string ;
    skos:definition "Diseases of the parasympathetic or sympathetic divisions of the AUTONOMIC NERVOUS SYSTEM; which has components located in the CENTRAL NERVOUS SYSTEM and PERIPHERAL NERVOUS SYSTEM. Autonomic dysfunction may be associated with HYPOTHALAMIC DISEASES; BRAIN STEM disorders; SPINAL CORD DISEASES; and PERIPHERAL NERVOUS SYSTEM DISEASES. Manifestations include impairments of vegetative functions including the maintenance of BLOOD PRESSURE; HEART RATE; pupil function; SWEATING; REPRODUCTIVE AND URINARY PHYSIOLOGY; and DIGESTION (MeSH)."^^xsd:string ;
    rdfs:subClassOf BIRNLEX:12796 ;
    skos:editorialNote "MeSH includes synonyms for two implied sub-types: Pure Autonomic Failure; Segmental Autonomic Dysfunction"^^xsd:string ;
    NIFRID:createdDate "2007-10-05"^^xsd:string ;
    NIFRID:modifiedDate "2007-11-18"^^xsd:string ;
    NIFRID:definingCitationURI <http://www.ninds.nih.gov/disorders/dysautonomia/dysautonomia.htm> ;
    NIFRID:hasBirnlexCurator NIFRID:Bill_Bug ;
    NIFRID:hasCurationStatus NIFRID:uncurated ;
    NIFRID:hasDefinitionSource NIFRID:MeSH_defSource ;
    NIFRID:hasExternalSource NIFRID:MeSH ;
    NIFRID:MeshUid "D001342"^^xsd:string .

BIRNLEX:12580 a owl:Class ;
    rdfs:label "Parasympathetic Nervous System Disease"^^xsd:string ;
    skos:prefLabel "Parasympathetic Nervous System Disease"^^xsd:string ;
    rdfs:subClassOf BIRNLEX:12579 ;
    NIFRID:createdDate "2007-10-05"^^xsd:string ;
    NIFRID:modifiedDate "2007-10-05"^^xsd:string ;
    NIFRID:hasBirnlexCurator NIFRID:Bill_Bug ;
    NIFRID:hasCurationStatus NIFRID:uncurated ;
    NIFRID:hasDefinitionSource NIFRID:MeSH_defSource ;
    NIFRID:hasExternalSource NIFRID:MeSH ;
    NIFRID:MeshUid "D001342"^^xsd:string .

BIRNLEX:12581 a owl:Class ;
    rdfs:label "Holmes-Adie Syndrome"^^xsd:string ;
    skos:prefLabel "Holmes-Adie Syndrome"^^xsd:string ;
    NIFRID:synonym "Adie Syndrome"^^xsd:string ;
    rdfs:subClassOf BIRNLEX:12579 ;
    NIFRID:createdDate "2007-10-05"^^xsd:string ;
    NIFRID:modifiedDate "2007-10-05"^^xsd:string ;
    NIFRID:definingCitationURI <http://www.ninds.nih.gov/disorders/holmes_adie/holmes_adie.htm> ;
    NIFRID:hasBirnlexCurator NIFRID:Bill_Bug ;
    NIFRID:hasCurationStatus NIFRID:uncurated ;
    NIFRID:hasDefinitionSource NIFRID:MeSH_defSource ;
    NIFRID:hasExternalSource NIFRID:MeSH ;
    NIFRID:MeshUid "D000270"^^xsd:string .

BIRNLEX:12582 a owl:Class ;
    rdfs:label "Autonomic Dysreflexia"^^xsd:string ;
    skos:prefLabel "Autonomic Dysreflexia"^^xsd:string ;
    NIFRID:synonym "Autonomic Hyperreflexia"^^xsd:string,
        "Spinal Autonomic Dysreflexia"^^xsd:string ;
    skos:definition "A syndrome associated with damage to the spinal cord above the mid thoracic level (see SPINAL CORD INJURIES) characterized by a marked increase in the sympathetic response to minor stimuli such as bladder or rectal distention. Manifestations include HYPERTENSION; TACHYCARDIA (or reflex bradycardia); FEVER; FLUSHING; and HYPERHIDROSIS. Extreme hypertension may be associated with a CEREBROVASCULAR ACCIDENT (MeSH)."^^xsd:string ;
    rdfs:subClassOf BIRNLEX:12579 ;
    NIFRID:createdDate "2007-10-05"^^xsd:string ;
    NIFRID:modifiedDate "2007-10-05"^^xsd:string ;
    NIFRID:definingCitation "Adams et al., Principles of Neurology, 6th ed, pp538 and 1232; J Spinal Cord Med 1997;20(3):355-60"^^xsd:string ;
    NIFRID:hasBirnlexCurator NIFRID:Bill_Bug ;
    NIFRID:hasCurationStatus NIFRID:uncurated ;
    NIFRID:hasDefinitionSource NIFRID:MeSH_defSource ;
    NIFRID:hasExternalSource NIFRID:MeSH ;
    NIFRID:MeshUid "D020211"^^xsd:string .

BIRNLEX:12583 a owl:Class ;
    rdfs:label "Complex Regional Pain Syndrome"^^xsd:string ;
    skos:prefLabel "Complex Regional Pain Syndrome"^^xsd:string ;
    NIFRID:synonym "Autonomic Hyperreflexia"^^xsd:string ;
    skos:definition "Conditions characterized by pain involving an extremity or other body region, HYPERESTHESIA, and localized autonomic dysfunction following injury to soft tissue or nerve. The pain is usually associated with ERYTHEMA; SKIN TEMPERATURE changes, abnormal sudomotor activity (i.e., changes in sweating due to altered sympathetic innervation) or edema. The degree of pain and other manifestations is out of proportion to that expected from the inciting event. Two subtypes of this condition have been described: type I; ( REFLEX SYMPATHETIC DYSTROPHY) and type II; (CAUSALGIA) (MeSH)."^^xsd:string ;
    rdfs:subClassOf BIRNLEX:12579 ;
    NIFRID:createdDate "2007-10-05"^^xsd:string ;
    NIFRID:modifiedDate "2007-10-05"^^xsd:string ;
    NIFRID:acronym "CRPS"^^xsd:string ;
    NIFRID:definingCitation "Pain 1995 Oct;63(1):127-33"^^xsd:string ;
    NIFRID:definingCitationURI <http://www.ninds.nih.gov/disorders/reflex_sympathetic_dystrophy/reflex_sympathetic_dystrophy.htm> ;
    NIFRID:hasBirnlexCurator NIFRID:Bill_Bug ;
    NIFRID:hasCurationStatus NIFRID:uncurated ;
    NIFRID:hasDefinitionSource NIFRID:MeSH_defSource ;
    NIFRID:hasExternalSource NIFRID:MeSH ;
    NIFRID:MeshUid "D020918"^^xsd:string .

BIRNLEX:12584 a owl:Class ;
    rdfs:label "Causalgia"^^xsd:string ;
    skos:prefLabel "Causalgia"^^xsd:string ;
    NIFRID:synonym "Causalgia Syndrome"^^xsd:string,
        "Complex Regional Pain Syndrome Type II"^^xsd:string,
        "Deafferentation Pain"^^xsd:string ;
    NIFRID:abbrev "CRPS Type II"^^xsd:string ;
    skos:definition "A complex regional pain syndrome characterized by burning pain and marked sensitivity to touch ( HYPERESTHESIA) in the distribution of an injured peripheral nerve. Autonomic dysfunction in the form of sudomotor (i.e., sympathetic innervation to sweat glands), vasomotor, and trophic skin changes may also occur (MeSH)."^^xsd:string ;
    rdfs:subClassOf BIRNLEX:12583 ;
    NIFRID:createdDate "2007-10-05"^^xsd:string ;
    NIFRID:modifiedDate "2007-10-05"^^xsd:string ;
    NIFRID:definingCitation "Adams et al., Principles of Neurology, 6th ed, p1359"^^xsd:string ;
    NIFRID:hasBirnlexCurator NIFRID:Bill_Bug ;
    NIFRID:hasCurationStatus NIFRID:uncurated ;
    NIFRID:hasDefinitionSource NIFRID:MeSH_defSource ;
    NIFRID:hasExternalSource NIFRID:MeSH ;
    NIFRID:MeshUid "D002422"^^xsd:string .

BIRNLEX:12585 a owl:Class ;
    rdfs:label "Reflex Sympathetic Dystrophy"^^xsd:string ;
    skos:prefLabel "Reflex Sympathetic Dystrophy"^^xsd:string ;
    NIFRID:synonym "Algodystrophic Syndrome"^^xsd:string,
        "Algodystrophy"^^xsd:string,
        "Cervical Sympathetic Dystrophy"^^xsd:string,
        "Complex Regional Pain Syndrome Type I"^^xsd:string,
        "Reflex Sympathetic Dystrophy Syndrome"^^xsd:string,
        "Shoulder-Hand Syndrome"^^xsd:string,
        "Sudek Atrophy"^^xsd:string,
        "Sympathetic Reflex Dystrophia"^^xsd:string ;
    NIFRID:abbrev "CRPS Type I"^^xsd:string ;
    skos:definition "A syndrome characterized by severe burning pain in an extremity accompanied by sudomotor, vasomotor, and trophic changes in bone without an associated specific nerve injury. This condition is most often precipitated by trauma to soft tissue or nerve complexes. The skin over the affected region is usually erythematous and demonstrates hypersensitivity to tactile stimuli and erythema (MeSH)."^^xsd:string ;
    rdfs:subClassOf BIRNLEX:12583 ;
    NIFRID:createdDate "2007-10-05"^^xsd:string ;
    NIFRID:modifiedDate "2007-10-05"^^xsd:string ;
    NIFRID:acronym "RSD"^^xsd:string ;
    NIFRID:definingCitation "Adams et al., Principles of Neurology, 6th ed, p1360; Pain 1995 Oct;63(1):127-33"^^xsd:string ;
    NIFRID:hasBirnlexCurator NIFRID:Bill_Bug ;
    NIFRID:hasCurationStatus NIFRID:uncurated ;
    NIFRID:hasDefinitionSource NIFRID:MeSH_defSource ;
    NIFRID:hasExternalSource NIFRID:MeSH ;
    NIFRID:MeshUid "D012019"^^xsd:string .

BIRNLEX:12586 a owl:Class ;
    rdfs:label "Horner Syndrome"^^xsd:string ;
    skos:prefLabel "Horner Syndrome"^^xsd:string ;
    NIFRID:synonym "Bernard Syndrome"^^xsd:string,
        "Claude Bernard-Horner Syndrome"^^xsd:string,
        "Miosis, Innervational Defect"^^xsd:string,
        "Oculosympathetic Syndrome"^^xsd:string,
        "Ptosis Sympathetic"^^xsd:string,
        "Sympathetic Ocular-Ophthalmoplegia"^^xsd:string ;
    skos:definition "A syndrome associated with defective sympathetic innervation to one side of the face, including the eye. Clinical features include MIOSIS; mild BLEPHAROPTOSIS; and hemifacial ANHIDROSIS (decreased sweating)(see HYPOHIDROSIS). Lesions of the BRAIN STEM; cervical SPINAL CORD; first thoracic nerve root; apex of the LUNG; CAROTID ARTERY; CAVERNOUS SINUS; and apex of the ORBIT may cause this condition (MeSH)."^^xsd:string ;
    rdfs:subClassOf BIRNLEX:12579 ;
    NIFRID:createdDate "2007-10-05"^^xsd:string ;
    NIFRID:modifiedDate "2007-10-05"^^xsd:string ;
    NIFRID:definingCitation "Miller et al., Clinical Neuro-Ophthalmology, 4th ed, pp500-11"^^xsd:string ;
    NIFRID:definingCitationURI <http://www.ninds.nih.gov/disorders/reflex_sympathetic_dystrophy/reflex_sympathetic_dystrophy.htm> ;
    NIFRID:hasBirnlexCurator NIFRID:Bill_Bug ;
    NIFRID:hasCurationStatus NIFRID:uncurated ;
    NIFRID:hasDefinitionSource NIFRID:MeSH_defSource ;
    NIFRID:hasExternalSource NIFRID:MeSH ;
    NIFRID:MeshUid "D006732"^^xsd:string .

BIRNLEX:12587 a owl:Class ;
    rdfs:label "Frey Syndrome"^^xsd:string ;
    skos:prefLabel "Frey Syndrome"^^xsd:string ;
    NIFRID:synonym "Auriculotemporal Syndrome"^^xsd:string,
        "Baillarger Syndrome"^^xsd:string,
        "Frey's Syndrome"^^xsd:string,
        "Freys Syndrome"^^xsd:string,
        "Gustatory Hyperhidrosis"^^xsd:string,
        "Salivosudoriparous Syndrome"^^xsd:string,
        "Sympathetic Ocular-Ophthalmoplegia"^^xsd:string,
        "Von Frey Syndrome"^^xsd:string,
        "Von Frey's Syndrome"^^xsd:string ;
    skos:definition "An autonomic disorder characterized by excessive sweating of the forehead, upper lip, perioral region, or sternum subsequent to gustatory stimuli. The auriculotemporal syndrome features facial flushing or sweating limited to the distribution of the auriculotemporal nerve and may develop after trauma to the parotid gland, in association with PAROTID NEOPLASMS, or following their surgical removal (MeSH)."^^xsd:string ;
    rdfs:subClassOf BIRNLEX:12579 ;
    NIFRID:createdDate "2007-10-05"^^xsd:string ;
    NIFRID:modifiedDate "April 11, 2009"^^xsd:string ;
    NIFRID:definingCitation "Ann Neurol 1997 Dec;42(6):973-5"^^xsd:string ;
    NIFRID:definingCitationURI <http://www.ninds.nih.gov/disorders/reflex_sympathetic_dystrophy/reflex_sympathetic_dystrophy.htm> ;
    NIFRID:hasBirnlexCurator NIFRID:Bill_Bug ;
    NIFRID:hasCurationStatus NIFRID:uncurated ;
    NIFRID:hasDefinitionSource NIFRID:MeSH_defSource ;
    NIFRID:hasExternalSource NIFRID:MeSH ;
    NIFRID:MeshUid "D013547"^^xsd:string .

BIRNLEX:12588 a owl:Class ;
    rdfs:label "Isaacs Syndrome"^^xsd:string ;
    skos:prefLabel "Isaacs Syndrome"^^xsd:string ;
    NIFRID:synonym "Acquired Neuromyotonia"^^xsd:string,
        "Continuous Muscle Activity Syndrome"^^xsd:string,
        "Continuous Myokymia"^^xsd:string,
        "Gamstorp-Wohlfart Syndrome"^^xsd:string,
        "Isaac Syndrome"^^xsd:string,
        "Isaac's Syndrome"^^xsd:string,
        "Isaacs-Mertens Syndrome"^^xsd:string,
        "Neuromyotonia"^^xsd:string,
        "Pseudomyotonia"^^xsd:string,
        "Pseudomyotonia Syndrome of Isaacs"^^xsd:string,
        "Quantal Squander"^^xsd:string ;
    skos:definition "A rare neuromuscular disorder with onset usually in late childhood or early adulthood, characterized by intermittent or continuous widespread involuntary muscle contractions; FASCICULATION; hyporeflexia; MUSCLE CRAMP; MUSCLE WEAKNESS; HYPERHIDROSIS; TACHYCARDIA; and MYOKYMIA. Involvement of pharyngeal or laryngeal muscles may interfere with speech and breathing. The continuous motor activity persists during sleep and general anesthesia (distinguishing this condition from STIFF-PERSON SYNDROME). Familial and acquired (primarily autoimmune) forms have been reported (MeSH)."^^xsd:string ;
    rdfs:subClassOf BIRNLEX:12578 ;
    NIFRID:createdDate "2007-10-05"^^xsd:string ;
    NIFRID:modifiedDate "April 11, 2009"^^xsd:string ;
    NIFRID:definingCitation "Ann NY Acad Sci 1998 May 13;841:482-496; Adams et al., Principles of Neurology, 6th ed, p1491"^^xsd:string ;
    NIFRID:definingCitationURI <http://www.ninds.nih.gov/disorders/isaacs_syndrome/isaacs_syndrome.htm> ;
    NIFRID:hasBirnlexCurator NIFRID:Bill_Bug ;
    NIFRID:hasCurationStatus NIFRID:uncurated ;
    NIFRID:hasDefinitionSource NIFRID:MeSH_defSource ;
    NIFRID:hasExternalSource NIFRID:MeSH ;
    NIFRID:MeshUid "D020386"^^xsd:string .

BIRNLEX:12589 a owl:Class ;
    rdfs:label "Sympathetic Nervous System Diseases"^^xsd:string ;
    skos:prefLabel "Sympathetic Nervous System Diseases"^^xsd:string ;
    rdfs:subClassOf BIRNLEX:12579 ;
    NIFRID:createdDate "2007-10-05"^^xsd:string ;
    NIFRID:modifiedDate "2007-10-05"^^xsd:string ;
    NIFRID:hasBirnlexCurator NIFRID:Bill_Bug ;
    NIFRID:hasCurationStatus NIFRID:uncurated ;
    NIFRID:hasDefinitionSource NIFRID:MeSH_defSource ;
    NIFRID:hasExternalSource NIFRID:MeSH ;
    NIFRID:MeshUid "D001342"^^xsd:string .

BIRNLEX:12590 a owl:Class ;
    rdfs:label "Neuromuscular Junction Diseases"^^xsd:string ;
    skos:prefLabel "Neuromuscular Junction Diseases"^^xsd:string ;
    NIFRID:synonym "Neuromuscular Junction Disorders"^^xsd:string,
        "Neuromuscular Transmission Disorders"^^xsd:string ;
    skos:definition "Conditions characterized by impaired transmission of impulses at the NEUROMUSCULAR JUNCTION. This may result from disorders that affect receptor function, pre- or postsynaptic membrane function, or ACETYLCHOLINESTERASE activity. The majority of diseases in this category are associated with autoimmune, toxic, or inherited conditions (MeSH)."^^xsd:string ;
    rdfs:subClassOf BIRNLEX:12578 ;
    NIFRID:createdDate "2007-10-05"^^xsd:string ;
    NIFRID:modifiedDate "2007-10-05"^^xsd:string ;
    NIFRID:hasBirnlexCurator NIFRID:Bill_Bug ;
    NIFRID:hasCurationStatus NIFRID:uncurated ;
    NIFRID:hasDefinitionSource NIFRID:MeSH_defSource ;
    NIFRID:hasExternalSource NIFRID:MeSH ;
    NIFRID:MeshUid "D020511"^^xsd:string .

BIRNLEX:12591 a owl:Class ;
    rdfs:label "Botulism"^^xsd:string ;
    skos:prefLabel "Botulism"^^xsd:string ;
    NIFRID:synonym "Toxico-Infectious Botulism"^^xsd:string ;
    skos:definition "A disease caused by potent protein NEUROTOXINS produced by CLOSTRIDIUM BOTULINUM which interfere with the presynaptic release of ACETYLCHOLINE at the NEUROMUSCULAR JUNCTION. Clinical features include abdominal pain, vomiting, acute PARALYSIS (including respiratory paralysis), blurred vision, and DIPLOPIA. Botulism may be classified into several subtypes (e.g., food-borne, infant, wound, and others) (MeSH)."^^xsd:string ;
    rdfs:subClassOf BIRNLEX:12590 ;
    NIFRID:createdDate "2007-10-05"^^xsd:string ;
    NIFRID:modifiedDate "2007-10-05"^^xsd:string ;
    NIFRID:hasBirnlexCurator NIFRID:Bill_Bug ;
    NIFRID:hasCurationStatus NIFRID:uncurated ;
    NIFRID:hasDefinitionSource NIFRID:MeSH_defSource ;
    NIFRID:hasExternalSource NIFRID:MeSH ;
    NIFRID:MeshUid "D001906"^^xsd:string .

BIRNLEX:12592 a owl:Class ;
    rdfs:label "Lambert-Eaton Myasthenic Syndrome"^^xsd:string ;
    skos:prefLabel "Lambert-Eaton Myasthenic Syndrome"^^xsd:string ;
    NIFRID:synonym "Eaton-Lambert Myasthenic Syndrome"^^xsd:string,
        "Eaton-Lambert Syndrome"^^xsd:string,
        "Lambert-Eaton Syndrome"^^xsd:string,
        "Lambert-Eaton's Syndrome"^^xsd:string,
        "Myasthenic-Myopathic Syndrome of Eaton-Lambert"^^xsd:string,
        "Myasthenic-Myopathic Syndrome of Lambert-Eaton"^^xsd:string ;
    skos:definition "An autoimmune disease characterized by weakness and fatigability of proximal muscles, particularly of the pelvic girdle, lower extremities, trunk, and shoulder girdle. There is relative sparing of extraocular and bulbar muscles. CARCINOMA, SMALL CELL of the lung is a frequently associated condition, although other malignancies and autoimmune diseases may be associated. Muscular weakness results from impaired impulse transmission at the NEUROMUSCULAR JUNCTION. Presynaptic calcium channel dysfunction leads to a reduced amount of acetylcholine being released in response to stimulation of the nerve (MeSH)."^^xsd:string ;
    rdfs:subClassOf BIRNLEX:12590 ;
    NIFRID:createdDate "2007-10-05"^^xsd:string ;
    NIFRID:modifiedDate "2007-10-05"^^xsd:string ;
    NIFRID:definingCitation "Adams et al., Principles of Neurology, 6th ed, pp 1471"^^xsd:string ;
    NIFRID:definingCitationURI <http://www.ninds.nih.gov/disorders/lambert_eaton/lambert_eaton.htm> ;
    NIFRID:hasBirnlexCurator NIFRID:Bill_Bug ;
    NIFRID:hasCurationStatus NIFRID:uncurated ;
    NIFRID:hasDefinitionSource NIFRID:MeSH_defSource ;
    NIFRID:hasExternalSource NIFRID:MeSH ;
    NIFRID:MeshUid "D015624"^^xsd:string ;
    NIFRID:nifID "_8.3_9.2"^^xsd:string .

BIRNLEX:12593 a owl:Class ;
    rdfs:label "Myasthenia Gravis"^^xsd:string ;
    skos:prefLabel "Myasthenia Gravis"^^xsd:string ;
    NIFRID:synonym "Myasthenia Gravis, Generalized"^^xsd:string ;
    skos:definition "A disorder of neuromuscular transmission characterized by weakness of cranial and skeletal muscles. Autoantibodies directed against acetylcholine receptors damage the motor endplate portion of the NEUROMUSCULAR JUNCTION, impairing the transmission of impulses to skeletal muscles. Clinical manifestations may include diplopia, ptosis, and weakness of facial, bulbar, respiratory, and proximal limb muscles. The disease may remain limited to the ocular muscles. THYMOMA is commonly associated with this condition (MeSH)."^^xsd:string ;
    rdfs:subClassOf BIRNLEX:12590 ;
    NIFRID:createdDate "2007-10-05"^^xsd:string ;
    NIFRID:modifiedDate "2007-10-05"^^xsd:string ;
    NIFRID:definingCitation "Adams et al., Principles of Neurology, 6th ed, p1459"^^xsd:string ;
    NIFRID:definingCitationURI <http://www.ninds.nih.gov/disorders/myasthenia_gravis/myasthenia_gravis.htm> ;
    NIFRID:hasBirnlexCurator NIFRID:Bill_Bug ;
    NIFRID:hasCurationStatus NIFRID:uncurated ;
    NIFRID:hasDefinitionSource NIFRID:MeSH_defSource ;
    NIFRID:hasExternalSource NIFRID:MeSH ;
    NIFRID:MeshUid "D009157"^^xsd:string ;
    NIFRID:nifID "_8.3_9.1"^^xsd:string .

BIRNLEX:12594 a owl:Class ;
    rdfs:label "Myasthenia Gravis, Ocular"^^xsd:string ;
    skos:prefLabel "Myasthenia Gravis, Ocular"^^xsd:string ;
    rdfs:subClassOf BIRNLEX:12593 ;
    NIFRID:createdDate "2007-10-05"^^xsd:string ;
    NIFRID:modifiedDate "2007-10-05"^^xsd:string ;
    NIFRID:hasBirnlexCurator NIFRID:Bill_Bug ;
    NIFRID:hasCurationStatus NIFRID:uncurated ;
    NIFRID:hasExternalSource NIFRID:MeSH ;
    NIFRID:MeshUid "D009157"^^xsd:string .

BIRNLEX:12595 a owl:Class ;
    rdfs:label "Autoimmune Experimental Myasthenia Gravis"^^xsd:string ;
    skos:prefLabel "Autoimmune Experimental Myasthenia Gravis"^^xsd:string ;
    NIFRID:synonym "Experimental Myasthenia"^^xsd:string,
        "Experimental Myasthenia Gravis"^^xsd:string ;
    skos:definition "Any autoimmune animal disease model used in the study of MYASTHENIA GRAVIS. Injection with purified neuromuscular junction acetylcholine receptor (AChR) (see RECEPTORS, CHOLINERGIC) components results in a myasthenic syndrome that has acute and chronic phases. The motor endplate pathology, loss of acetylcholine receptors, presence of circulating anti-AChR antibodies, and electrophysiologic changes make this condition virtually identical to human myasthenia gravis (MeSH)."^^xsd:string ;
    rdfs:subClassOf BIRNLEX:12593 ;
    NIFRID:createdDate "2007-10-05"^^xsd:string ;
    NIFRID:modifiedDate "2007-10-05"^^xsd:string ;
    NIFRID:definingCitation "Joynt, Clinical Neurology, 1997, Ch 54, p3"^^xsd:string ;
    NIFRID:hasBirnlexCurator NIFRID:Bill_Bug ;
    NIFRID:hasCurationStatus NIFRID:uncurated ;
    NIFRID:hasDefinitionSource NIFRID:MeSH_defSource ;
    NIFRID:hasExternalSource NIFRID:MeSH ;
    NIFRID:MeshUid "D020720"^^xsd:string ;
    NIFRID:usageNote "Passive transfer of AChR antibodies or lymphocytes from afflicted animals to normals induces passive transfer experimental autoimmune myasthenia gravis (i.e., Passive Transfer Experimental Autoimmune Myasthenia Gravis) (MeSH)."^^xsd:string .

BIRNLEX:12596 a owl:Class ;
    rdfs:label "Neonatal Myasthenia Gravis"^^xsd:string ;
    skos:prefLabel "Neonatal Myasthenia Gravis"^^xsd:string ;
    NIFRID:synonym "Antenatal Myasthenia Gravis"^^xsd:string ;
    skos:definition "A disorder of neuromuscular transmission that occurs in a minority of newborns born to women with myasthenia gravis. Clinical features are usually present at birth or develop in the first 3 days of life and consist of hypotonia and impaired respiratory, suck, and swallowing abilities. This condition is associated with the passive transfer of acetylcholine receptor antibodies through the placenta.  (MeSH)."^^xsd:string ;
    rdfs:subClassOf BIRNLEX:12593 ;
    NIFRID:createdDate "2007-10-05"^^xsd:string ;
    NIFRID:modifiedDate "2007-10-05"^^xsd:string ;
    NIFRID:definingCitation "Menkes, Textbook of Child Neurology, 5th ed, p823; Neurology 1997 Jan;48(1):50-4"^^xsd:string ;
    NIFRID:hasBirnlexCurator NIFRID:Bill_Bug ;
    NIFRID:hasCurationStatus NIFRID:uncurated ;
    NIFRID:hasDefinitionSource NIFRID:MeSH_defSource ;
    NIFRID:hasExternalSource NIFRID:MeSH ;
    NIFRID:MeshUid "D020941"^^xsd:string ;
    NIFRID:usageNote "In the majority of infants the myasthenic weakness resolves (i.e., Transient neonatal myasthenia gravis) although this disorder may rarely continue beyond the neonatal period (i.e., Persistent neonatal myasthenia gravis) (MeSH)."^^xsd:string .

BIRNLEX:12597 a owl:Class ;
    rdfs:label "Congenital Myasthenic Syndrome"^^xsd:string ;
    skos:prefLabel "Congenital Myasthenic Syndrome"^^xsd:string ;
    NIFRID:synonym "Congenital Myasthenia Gravis"^^xsd:string ;
    skos:definition "A heterogeneous group of disorders characterized by a congenital defect in neuromuscular transmission at the NEUROMUSCULAR JUNCTION. This includes presynaptic, synaptic, and postsynaptic disorders (that are not of autoimmune origin). The majority of these diseases are caused by mutations of various subunits of the nicotinic acetylcholine receptor ( RECEPTORS, NICOTINIC) on the postsynaptic surface of the junction (MeSH)."^^xsd:string ;
    rdfs:subClassOf BIRNLEX:12590 ;
    NIFRID:createdDate "2007-10-05"^^xsd:string ;
    NIFRID:modifiedDate "2007-10-05"^^xsd:string ;
    NIFRID:definingCitation "Arch Neurol 1999 Feb;56(2):163-7"^^xsd:string ;
    NIFRID:hasBirnlexCurator NIFRID:Bill_Bug ;
    NIFRID:hasCurationStatus NIFRID:uncurated ;
    NIFRID:hasDefinitionSource NIFRID:MeSH_defSource ;
    NIFRID:hasExternalSource NIFRID:MeSH ;
    NIFRID:MeshUid "D020294"^^xsd:string ;
    NIFRID:usageNote "Do not confuse with MYASTHENIA GRAVIS, NEONATAL, a transient condition seen in neonates born to myasthenic mothers (MeSH)."^^xsd:string .

BIRNLEX:12598 a owl:Class ;
    rdfs:label "Postsynaptic Congenital Myasthenic Syndrome"^^xsd:string ;
    skos:prefLabel "Postsynaptic Congenital Myasthenic Syndrome"^^xsd:string ;
    NIFRID:synonym "Slow-Channel Congenital Myasthenic Syndrome"^^xsd:string ;
    rdfs:subClassOf BIRNLEX:12597 ;
    NIFRID:createdDate "2007-10-05"^^xsd:string ;
    NIFRID:modifiedDate "2007-10-05"^^xsd:string ;
    NIFRID:hasBirnlexCurator NIFRID:Bill_Bug ;
    NIFRID:hasCurationStatus NIFRID:uncurated ;
    NIFRID:hasDefinitionSource NIFRID:MeSH_defSource ;
    NIFRID:hasExternalSource NIFRID:MeSH ;
    NIFRID:MeshUid "D020294"^^xsd:string .

BIRNLEX:12599 a owl:Class ;
    rdfs:label "Presynaptic Congenital Myasthenic Syndrome"^^xsd:string ;
    skos:prefLabel "Presynaptic Congenital Myasthenic Syndrome"^^xsd:string ;
    rdfs:subClassOf BIRNLEX:12597 ;
    NIFRID:createdDate "2007-10-05"^^xsd:string ;
    NIFRID:modifiedDate "2007-10-05"^^xsd:string ;
    NIFRID:hasBirnlexCurator NIFRID:Bill_Bug ;
    NIFRID:hasCurationStatus NIFRID:uncurated ;
    NIFRID:hasDefinitionSource NIFRID:MeSH_defSource ;
    NIFRID:hasExternalSource NIFRID:MeSH ;
    NIFRID:MeshUid "D020294"^^xsd:string .

BIRNLEX:12600 a owl:Class ;
    rdfs:label "Primary nervous system neoplastic disease"^^xsd:string ;
    skos:prefLabel "Primary nervous system neoplastic disease"^^xsd:string ;
    NIFRID:synonym "Nerve Tissue Neoplasm"^^xsd:string,
        "Nervous Tissue Neoplasm"^^xsd:string ;
    skos:definition "Neoplasms composed of nerve tissue. This concept does not refer to neoplasms located in the nervous system or its component nerves (MeSH)."^^xsd:string ;
    rdfs:subClassOf BIRNLEX:12525 ;
    NIFRID:createdDate "2007-10-05"^^xsd:string ;
    NIFRID:modifiedDate "2007-10-05"^^xsd:string ;
    NIFRID:hasBirnlexCurator NIFRID:Bill_Bug ;
    NIFRID:hasCurationStatus NIFRID:uncurated ;
    NIFRID:hasDefinitionSource NIFRID:MeSH_defSource ;
    NIFRID:hasExternalSource NIFRID:MeSH ;
    NIFRID:MeshUid "D009380"^^xsd:string ;
    NIFRID:nifID "_8.3_10.1"^^xsd:string .

BIRNLEX:12601 a owl:Class ;
    rdfs:label "Meningioma"^^xsd:string ;
    skos:prefLabel "Meningioma"^^xsd:string ;
    skos:definition "A relatively common neoplasm of the CENTRAL NERVOUS SYSTEM that arises from arachnoidal cells. The majority are well differentiated vascular tumors which grow slowly and have a low potential to be invasive, although malignant subtypes occur. Meningiomas have a predilection to arise from the parasagittal region, cerebral convexity, sphenoidal ridge, olfactory groove, and SPINAL CANAL (MeSH)."^^xsd:string ;
    rdfs:subClassOf BIRNLEX:12600 ;
    NIFRID:createdDate "2007-10-05"^^xsd:string ;
    NIFRID:modifiedDate "2007-10-05"^^xsd:string ;
    NIFRID:hasBirnlexCurator NIFRID:Bill_Bug ;
    NIFRID:hasCurationStatus NIFRID:uncurated ;
    NIFRID:hasDefinitionSource NIFRID:MeSH_defSource ;
    NIFRID:hasExternalSource NIFRID:MeSH ;
    NIFRID:MeshUid "D008579"^^xsd:string ;
    NIFRID:nifID "_8.3_10.1.2"^^xsd:string ;
    NIFRID:usageNote "MeSH lists a large variety of Meningioma types categorized largely by anatomic location, histologic characteristics, or benign vs. malignant (i.e.: Angioblastic Meningioma; Angiomatous Meningioma; Benign Meningioma; Cerebral Convexity Meningioma; Clear Cell Meningioma; Fibrous Meningioma; Hemangioblastic Meningioma; Hemangiopericytic Meningioma; Intracranial Meningioma; Intraorbital Meningioma; Intraventricular Meningioma; Malignant Meningioma; Meningiomas, Multiple; Meningiomatosis; Meningotheliomatous Meningioma; Microcystic Meningioma; Olfactory Groove Meningioma; Papillary Meningioma; Parasagittal Meningioma; Posterior Fossa Meningioma; Psammomatous Meningioma; Secretory Meningioma; Sphenoid Wing Meningioma; Spinal Meningioma; Transitional Meningioma; Xanthomatous Meningioma)."^^xsd:string .

BIRNLEX:12602 a owl:Class ;
    rdfs:label "Nerve Sheath Neoplasms"^^xsd:string ;
    skos:prefLabel "Nerve Sheath Neoplasms"^^xsd:string ;
    skos:definition "Neoplasms which arise from nerve sheaths formed by SCHWANN CELLS in the PERIPHERAL NERVOUS SYSTEM or by OLIGODENDROCYTES in the CENTRAL NERVOUS SYSTEM. Malignant peripheral nerve sheath tumors, NEUROFIBROMA, and NEURILEMMOMA are relatively common tumors in this category (MeSH)."^^xsd:string ;
    rdfs:subClassOf BIRNLEX:12600 ;
    NIFRID:createdDate "2007-10-05"^^xsd:string ;
    NIFRID:modifiedDate "2007-10-05"^^xsd:string ;
    NIFRID:hasBirnlexCurator NIFRID:Bill_Bug ;
    NIFRID:hasCurationStatus NIFRID:uncurated ;
    NIFRID:hasDefinitionSource NIFRID:MeSH_defSource ;
    NIFRID:hasExternalSource NIFRID:MeSH ;
    NIFRID:MeshUid "D018317"^^xsd:string .

BIRNLEX:12603 a owl:Class ;
    rdfs:label "Neurilemmoma"^^xsd:string ;
    skos:prefLabel "Neurilemmoma"^^xsd:string ;
    NIFRID:synonym "Neurilemmosarcoma"^^xsd:string,
        "Neurilemoma"^^xsd:string,
        "Neurinoma"^^xsd:string,
        "Schwannoma"^^xsd:string ;
    skos:definition "A neoplasm that arises from SCHWANN CELLS of the cranial, peripheral, and autonomic nerves. Clinically, these tumors may present as a cranial neuropathy, abdominal or soft tissue mass, intracranial lesion, or with spinal cord compression. Histologically, these tumors are encapsulated, highly vascular, and composed of a homogenous pattern of biphasic fusiform-shaped cells that may have a palisaded appearance (MeSH)."^^xsd:string ;
    rdfs:subClassOf BIRNLEX:12610 ;
    NIFRID:createdDate "2007-10-05"^^xsd:string ;
    NIFRID:modifiedDate "2007-10-05"^^xsd:string ;
    NIFRID:definingCitation "DeVita Jr et al., Cancer: Principles and Practice of Oncology, 5th ed, pp964-5"^^xsd:string ;
    NIFRID:hasBirnlexCurator NIFRID:Bill_Bug ;
    NIFRID:hasCurationStatus NIFRID:uncurated ;
    NIFRID:hasDefinitionSource NIFRID:MeSH_defSource ;
    NIFRID:hasExternalSource NIFRID:MeSH ;
    NIFRID:MeshUid "D009442"^^xsd:string ;
    NIFRID:usageNote "May be benign or malignant."^^xsd:string .

BIRNLEX:12604 a owl:Class ;
    rdfs:label "Neurofibroma"^^xsd:string ;
    skos:prefLabel "Neurofibroma"^^xsd:string ;
    skos:definition "A moderately firm, benign, encapsulated tumor resulting from proliferation of SCHWANN CELLS and FIBROBLASTS that includes portions of nerve fibers. The tumors usually develop along peripheral or cranial nerves and are a central feature of NEUROFIBROMATOSIS 1, where they may occur intracranially or involve spinal roots. Pathologic features include fusiform enlargement of the involved nerve. Microscopic examination reveals a disorganized and loose cellular pattern with elongated nuclei intermixed with fibrous strands (MeSH)."^^xsd:string ;
    rdfs:subClassOf BIRNLEX:12602 ;
    NIFRID:createdDate "2007-10-05"^^xsd:string ;
    NIFRID:modifiedDate "2007-10-05"^^xsd:string ;
    NIFRID:definingCitation "Adams et al., Principles of Neurology, 6th ed, p1016"^^xsd:string ;
    NIFRID:hasBirnlexCurator NIFRID:Bill_Bug ;
    NIFRID:hasCurationStatus NIFRID:uncurated ;
    NIFRID:hasDefinitionSource NIFRID:MeSH_defSource ;
    NIFRID:hasExternalSource NIFRID:MeSH ;
    NIFRID:MeshUid "D009455"^^xsd:string ;
    NIFRID:usageNote "May be benign or malignant."^^xsd:string .

BIRNLEX:12605 a owl:Class ;
    rdfs:label "Neurofibromatosis"^^xsd:string ;
    skos:prefLabel "Neurofibromatosis"^^xsd:string ;
    NIFRID:synonym "Multiple Neurofibromas"^^xsd:string,
        "Neurofibromatosis Syndrome"^^xsd:string ;
    skos:definition "A group of disorders characterized by an autosomal dominant pattern of inheritance with high rates of spontaneous mutation and multiple neurofibromas or neurilemmomas. NEUROFIBROMATOSIS 1 (generalized neurofibromatosis) accounts for approximately 95% of cases, although multiple additional subtypes (e.g., NEUROFIBROMATOSIS 2, neurofibromatosis 3, etc.) have been described (MeSH)."^^xsd:string ;
    rdfs:subClassOf BIRNLEX:12604 ;
    NIFRID:createdDate "2007-10-05"^^xsd:string ;
    NIFRID:modifiedDate "2007-10-05"^^xsd:string ;
    NIFRID:definingCitation "Adams et al., Principles of Neurology, 6th ed, p1016"^^xsd:string ;
    NIFRID:hasBirnlexCurator NIFRID:Bill_Bug ;
    NIFRID:hasCurationStatus NIFRID:uncurated ;
    NIFRID:hasDefinitionSource NIFRID:MeSH_defSource ;
    NIFRID:hasExternalSource NIFRID:MeSH ;
    NIFRID:MeshUid "D017253"^^xsd:string ;
    NIFRID:usageNote "May be benign or malignant."^^xsd:string .

BIRNLEX:12606 a owl:Class ;
    rdfs:label "Neurofibroma, Plexiform"^^xsd:string ;
    skos:prefLabel "Neurofibroma, Plexiform"^^xsd:string ;
    NIFRID:synonym "Elephantiasis Neuromatosis"^^xsd:string,
        "Pachydermatocele"^^xsd:string,
        "Tumor Royale"^^xsd:string ;
    skos:definition "A type of neurofibroma manifesting as a diffuse overgrowth of subcutaneous tissue, usually involving the face, scalp, neck, and chest but occasionally occurring in the abdomen or pelvis. The tumors tend to progress, and may extend along nerve roots to eventually involve the spinal roots and spinal cord. This process is almost always a manifestation of NEUROFIBROMATOSIS 1 (MeSH)."^^xsd:string ;
    rdfs:subClassOf BIRNLEX:12604 ;
    NIFRID:createdDate "2007-10-05"^^xsd:string ;
    NIFRID:modifiedDate "2007-10-05"^^xsd:string ;
    NIFRID:definingCitation "Adams et al., Principles of Neurology, 6th ed, p1016; J Pediatr 1997 Nov;131(5):678-82"^^xsd:string ;
    NIFRID:hasBirnlexCurator NIFRID:Bill_Bug ;
    NIFRID:hasCurationStatus NIFRID:uncurated ;
    NIFRID:hasDefinitionSource NIFRID:MeSH_defSource ;
    NIFRID:hasExternalSource NIFRID:MeSH ;
    NIFRID:MeshUid "D018318"^^xsd:string .

BIRNLEX:12607 a owl:Class ;
    rdfs:label "Neurofibromatosis 1"^^xsd:string ;
    skos:prefLabel "Neurofibromatosis 1"^^xsd:string ;
    NIFRID:synonym "Neurofibromatosis I"^^xsd:string,
        "Neurofibromatosis Type 1"^^xsd:string,
        "Neurofibromatosis Type I"^^xsd:string,
        "Recklinghausen Disease of Nerve"^^xsd:string,
        "von Recklinghausen Disease"^^xsd:string ;
    skos:definition "An autosomal dominant inherited disorder (with a high frequency of spontaneous mutations) that features developmental changes in the nervous system, muscles, bones, and skin, most notably in tissue derived from the embryonic NEURAL CREST. Multiple hyperpigmented skin lesions and subcutaneous tumors are the hallmark of this disease. Peripheral and central nervous system neoplasms occur frequently, especially OPTIC NERVE GLIOMA and NEUROFIBROSARCOMA. NF1 is caused by mutations which inactivate the NF1 gene (GENES, NEUROFIBROMATOSIS 1) on chromosome 17q. The incidence of learning disabilities is also elevated in this condition. A syndrome characterized by the presence of PULMONARY STENOSIS; CAFE-AU-LAIT SPOTS; MENTAL RETARDATION; and short stature caused by mutations in the NF1 gene (GENES, NEUROFIBROMATOSIS 1). There is overlap of clinical features with NOONAN SYNDROME in a syndrome called neurofibromatosis-Noonan syndrome. Both the PTPN11 and NF1 gene products are involved in the SIGNAL TRANSDUCTION pathway of Ras ( RAS PROTEINS) (MeSH)."^^xsd:string ;
    rdfs:subClassOf BIRNLEX:12605 ;
    NIFRID:createdDate "2007-10-05"^^xsd:string ;
    NIFRID:modifiedDate "2007-10-05"^^xsd:string ;
    NIFRID:acronym "NF1"^^xsd:string ;
    NIFRID:definingCitation "Adams et al., Principles of Neurology, 6th ed, pp1014-18"^^xsd:string ;
    NIFRID:hasBirnlexCurator NIFRID:Bill_Bug ;
    NIFRID:hasCurationStatus NIFRID:uncurated ;
    NIFRID:hasDefinitionSource NIFRID:MeSH_defSource ;
    NIFRID:hasExternalSource NIFRID:MeSH ;
    NIFRID:MeshUid "D009456"^^xsd:string .

BIRNLEX:12608 a owl:Class ;
    rdfs:label "Neurofibromatosis 2"^^xsd:string ;
    skos:prefLabel "Neurofibromatosis 2"^^xsd:string ;
    NIFRID:synonym "Bilateral Acoustic Neurofibromatosis"^^xsd:string,
        "Bilateral Acoustic Neuroma"^^xsd:string,
        "Bilateral Acoustic Schwannoma"^^xsd:string,
        "Familial Acoustic Neuroma"^^xsd:string,
        "Neurofibromatosis II"^^xsd:string,
        "Neurofibromatosis Type 2"^^xsd:string,
        "Neurofibromatosis Type II"^^xsd:string ;
    skos:definition "An autosomal dominant disorder characterized by a high incidence of bilateral acoustic neuromas as well as schwannomas ( NEURILEMMOMA) of other cranial and peripheral nerves, and other benign intracranial tumors including meningiomas, ependymomas, spinal neurofibromas, and gliomas. The disease has been linked to mutations of the NF2 gene (GENES, NEUROFIBROMATOSIS 2) on chromosome 22 (22q12) and usually presents clinically in the first or second decade of life.(MeSH)."^^xsd:string ;
    rdfs:subClassOf BIRNLEX:12605 ;
    NIFRID:createdDate "2007-10-05"^^xsd:string ;
    NIFRID:modifiedDate "2007-10-05"^^xsd:string ;
    NIFRID:acronym "NF2"^^xsd:string ;
    NIFRID:hasBirnlexCurator NIFRID:Bill_Bug ;
    NIFRID:hasCurationStatus NIFRID:uncurated ;
    NIFRID:hasDefinitionSource NIFRID:MeSH_defSource ;
    NIFRID:hasExternalSource NIFRID:MeSH ;
    NIFRID:MeshUid "D016518"^^xsd:string .

BIRNLEX:12609 a owl:Class ;
    rdfs:label "Neurofibrosarcoma"^^xsd:string ;
    skos:prefLabel "Neurofibrosarcoma"^^xsd:string ;
    NIFRID:synonym "Neurogenic Sarcoma"^^xsd:string ;
    skos:definition "A malignant tumor that arises from small cutaneous nerves, is locally aggressive, and has a potential for metastasis. Characteristic histopathologic features include proliferating atypical spindle cells with slender wavy and pointed nuclei, hypocellular areas, and areas featuring organized whorls of fibroblastic proliferation. The most common primary sites are the extremities, retroperitoneum, and trunk. These tumors tend to present in childhood, often in association with NEUROFIBROMATOSIS 1 (MeSH)."^^xsd:string ;
    rdfs:subClassOf BIRNLEX:12602 ;
    NIFRID:createdDate "2007-10-05"^^xsd:string ;
    NIFRID:modifiedDate "2007-10-05"^^xsd:string ;
    NIFRID:definingCitation "DeVita et al., Cancer: Principles & Practice of Oncology, 5th ed, p1662; Mayo Clin Proc 1990 Feb;65(2):164-72"^^xsd:string ;
    NIFRID:hasBirnlexCurator NIFRID:Bill_Bug ;
    NIFRID:hasCurationStatus NIFRID:uncurated ;
    NIFRID:hasDefinitionSource NIFRID:MeSH_defSource ;
    NIFRID:hasExternalSource NIFRID:MeSH ;
    NIFRID:MeshUid "D018319"^^xsd:string .

BIRNLEX:12610 a owl:Class ;
    rdfs:label "Neuroma"^^xsd:string ;
    skos:prefLabel "Neuroma"^^xsd:string ;
    skos:definition "A tumor made up of nerve cells and nerve fibers (MeSH)."^^xsd:string ;
    rdfs:subClassOf BIRNLEX:12602 ;
    NIFRID:createdDate "2007-10-05"^^xsd:string ;
    NIFRID:modifiedDate "2007-10-05"^^xsd:string ;
    NIFRID:definingCitation "Stedman, 25th ed"^^xsd:string ;
    NIFRID:hasBirnlexCurator NIFRID:Bill_Bug ;
    NIFRID:hasCurationStatus NIFRID:uncurated ;
    NIFRID:hasDefinitionSource NIFRID:MeSH_defSource ;
    NIFRID:hasExternalSource NIFRID:MeSH ;
    NIFRID:MeshUid "D009463"^^xsd:string .

BIRNLEX:12611 a owl:Class ;
    rdfs:label "Neurothekeoma"^^xsd:string ;
    skos:prefLabel "Neurothekeoma"^^xsd:string ;
    NIFRID:synonym "Myxoma, Nerve Sheath"^^xsd:string,
        "Neurotheceoma"^^xsd:string,
        "Neurothecoma"^^xsd:string ;
    skos:definition "A benign myxoma of cutaneous nerve sheath origin. Theke is from the Greek theke, sheath (MeSH)."^^xsd:string ;
    rdfs:subClassOf BIRNLEX:12602 ;
    NIFRID:createdDate "2007-10-05"^^xsd:string ;
    NIFRID:modifiedDate "2007-10-05"^^xsd:string ;
    NIFRID:definingCitation "Stedman, 25th ed"^^xsd:string ;
    NIFRID:hasBirnlexCurator NIFRID:Bill_Bug ;
    NIFRID:hasCurationStatus NIFRID:uncurated ;
    NIFRID:hasDefinitionSource NIFRID:MeSH_defSource ;
    NIFRID:hasExternalSource NIFRID:MeSH ;
    NIFRID:MeshUid "D018321"^^xsd:string .

BIRNLEX:12612 a owl:Class ;
    rdfs:label "Neuroectodermal Neoplasm"^^xsd:string ;
    skos:prefLabel "Neuroectodermal Neoplasm"^^xsd:string ;
    NIFRID:synonym "Neuroectodermal Tumor"^^xsd:string ;
    skos:definition "Malignant neoplasms arising in the neuroectoderm, the portion of the ectoderm of the early embryo that gives rise to the central and peripheral nervous systems, including some glial cells.(MeSH)."^^xsd:string ;
    rdfs:subClassOf BIRNLEX:12600 ;
    NIFRID:createdDate "2007-10-05"^^xsd:string ;
    NIFRID:modifiedDate "2007-10-05"^^xsd:string ;
    NIFRID:hasBirnlexCurator NIFRID:Bill_Bug ;
    NIFRID:hasCurationStatus NIFRID:uncurated ;
    NIFRID:hasDefinitionSource NIFRID:MeSH_defSource ;
    NIFRID:hasExternalSource NIFRID:MeSH ;
    NIFRID:MeshUid "D017599"^^xsd:string .

BIRNLEX:12613 a owl:Class ;
    rdfs:label "Craniopharyngioma"^^xsd:string ;
    skos:prefLabel "Craniopharyngioma"^^xsd:string ;
    NIFRID:synonym "Rathke Cleft Neoplasm"^^xsd:string,
        "Rathke Pouch Tumor"^^xsd:string ;
    skos:definition "A benign pituitary-region neoplasm that originates from Rathke's pouch. The two major histologic and clinical subtypes are adamantinous (or classical) craniopharyngioma and papillary craniopharyngioma. The adamantinous form presents in children and adolescents as an expanding cystic lesion in the pituitary region. The cystic cavity is filled with a black viscous substance and histologically the tumor is composed of adamantinomatous epithelium and areas of calcification and necrosis. Papillary craniopharyngiomas occur in adults, and histologically feature a squamous epithelium with papillations (MeSH)."^^xsd:string ;
    rdfs:subClassOf BIRNLEX:12600 ;
    NIFRID:createdDate "2007-10-05"^^xsd:string ;
    NIFRID:modifiedDate "2007-10-05"^^xsd:string ;
    NIFRID:hasBirnlexCurator NIFRID:Bill_Bug ;
    NIFRID:hasCurationStatus NIFRID:uncurated ;
    NIFRID:hasDefinitionSource NIFRID:MeSH_defSource ;
    NIFRID:hasExternalSource NIFRID:MeSH ;
    NIFRID:MeshUid "D003397"^^xsd:string .

BIRNLEX:12614 a owl:Class ;
    rdfs:label "Adamantinous Craniopharyngioma"^^xsd:string ;
    skos:prefLabel "Adamantinous Craniopharyngioma"^^xsd:string ;
    NIFRID:synonym "Craniopharyngioma, Child"^^xsd:string ;
    skos:definition "The adamantinous form presents in children and adolescents as an expanding cystic lesion in the pituitary region. The cystic cavity is filled with a black viscous substance and histologically the tumor is composed of adamantinomatous epithelium and areas of calcification and necrosis. Papillary craniopharyngiomas occur in adults, and histologically feature a squamous epithelium with papillations (MeSH)."^^xsd:string ;
    rdfs:subClassOf BIRNLEX:12613 ;
    NIFRID:createdDate "2007-10-05"^^xsd:string ;
    NIFRID:modifiedDate "2007-10-05"^^xsd:string ;
    NIFRID:hasBirnlexCurator NIFRID:Bill_Bug ;
    NIFRID:hasCurationStatus NIFRID:uncurated ;
    NIFRID:hasDefinitionSource NIFRID:MeSH_defSource ;
    NIFRID:hasExternalSource NIFRID:MeSH ;
    NIFRID:MeshUid "D003397"^^xsd:string .

BIRNLEX:12615 a owl:Class ;
    rdfs:label "Papillary Craniopharyngioma"^^xsd:string ;
    skos:prefLabel "Papillary Craniopharyngioma"^^xsd:string ;
    NIFRID:synonym "Craniopharyngioma, Adult"^^xsd:string ;
    skos:definition "Papillary craniopharyngiomas occur in adults, and histologically feature a squamous epithelium with papillations (MeSH)."^^xsd:string ;
    rdfs:subClassOf BIRNLEX:12613 ;
    NIFRID:createdDate "2007-10-05"^^xsd:string ;
    NIFRID:modifiedDate "2007-10-05"^^xsd:string ;
    NIFRID:hasBirnlexCurator NIFRID:Bill_Bug ;
    NIFRID:hasCurationStatus NIFRID:uncurated ;
    NIFRID:hasDefinitionSource NIFRID:MeSH_defSource ;
    NIFRID:hasExternalSource NIFRID:MeSH ;
    NIFRID:MeshUid "D003397"^^xsd:string .

BIRNLEX:12616 a owl:Class ;
    rdfs:label "Neuroepithelial Neoplasm"^^xsd:string ;
    skos:prefLabel "Neuroepithelial Neoplasm"^^xsd:string ;
    NIFRID:synonym "Neuroepithelial Tumor"^^xsd:string ;
    skos:definition "Neoplasms composed of neuroepithelial cells, which have the capacity to differentiate into NEURONS, oligodendrocytes, and ASTROCYTES. The majority of craniospinal tumors are of neuroepithelial origin (MeSH)."^^xsd:string ;
    rdfs:subClassOf BIRNLEX:12600 ;
    NIFRID:createdDate "2007-10-05"^^xsd:string ;
    NIFRID:modifiedDate "2007-10-05"^^xsd:string ;
    NIFRID:hasBirnlexCurator NIFRID:Bill_Bug ;
    NIFRID:hasCurationStatus NIFRID:uncurated ;
    NIFRID:hasDefinitionSource NIFRID:MeSH_defSource ;
    NIFRID:hasExternalSource NIFRID:MeSH ;
    NIFRID:MeshUid "D018302"^^xsd:string .

BIRNLEX:12617 a owl:Class ;
    rdfs:label "Ganglioneuroma"^^xsd:string ;
    skos:prefLabel "Ganglioneuroma"^^xsd:string ;
    NIFRID:synonym "Gangliocytoma"^^xsd:string ;
    skos:definition "A benign neoplasm that usually arises from the sympathetic trunk in the mediastinum. Histologic features include spindle cell proliferation (resembling a neurofibroma) and the presence of large ganglion cells. The tumor may present clinically with HORNER SYNDROME or diarrhea due to ectopic production of vasoactive intestinal peptide (MeSH)."^^xsd:string ;
    rdfs:subClassOf BIRNLEX:12600 ;
    NIFRID:createdDate "2007-10-05"^^xsd:string ;
    NIFRID:modifiedDate "2007-10-05"^^xsd:string ;
    NIFRID:hasBirnlexCurator NIFRID:Bill_Bug ;
    NIFRID:hasCurationStatus NIFRID:uncurated ;
    NIFRID:hasDefinitionSource NIFRID:MeSH_defSource ;
    NIFRID:hasExternalSource NIFRID:MeSH ;
    NIFRID:MeshUid "D005729"^^xsd:string .

BIRNLEX:12618 a owl:Class ;
    rdfs:label "Glioma"^^xsd:string ;
    skos:prefLabel "Glioma"^^xsd:string ;
    NIFRID:synonym "Glial Cell Tumor"^^xsd:string ;
    skos:definition "Benign and malignant central nervous system neoplasms derived from glial cells (i.e., astrocytes, oligodendrocytes, and ependymocytes). Astrocytes may give rise to astrocytomas ( ASTROCYTOMA) or glioblastoma multiforme (see GLIOBLASTOMA). Oligodendrocytes give rise to oligodendrogliomas ( OLIGODENDROGLIOMA) and ependymocytes may undergo transformation to become EPENDYMOMA; CHOROID PLEXUS NEOPLASMS; or colloid cysts of the third ventricle (MeSH)."^^xsd:string ;
    rdfs:subClassOf BIRNLEX:12600 ;
    NIFRID:createdDate "2007-10-05"^^xsd:string ;
    NIFRID:modifiedDate "2007-10-05"^^xsd:string ;
    NIFRID:definingCitation "Escourolle et al., Manual of Basic Neuropathology, 2nd ed, p21"^^xsd:string ;
    NIFRID:hasBirnlexCurator NIFRID:Bill_Bug ;
    NIFRID:hasCurationStatus NIFRID:uncurated ;
    NIFRID:hasDefinitionSource NIFRID:MeSH_defSource ;
    NIFRID:hasExternalSource NIFRID:MeSH ;
    NIFRID:MeshUid "D005910"^^xsd:string ;
    NIFRID:nifID "_8.3_10.1.1"^^xsd:string .

BIRNLEX:12619 a owl:Class ;
    rdfs:label "Astrocytoma"^^xsd:string ;
    skos:prefLabel "Astrocytoma"^^xsd:string ;
    NIFRID:synonym "Astrocytic Glioma"^^xsd:string,
        "Astroglioma"^^xsd:string ;
    skos:definition "Neoplasms of the brain and spinal cord derived from glial cells which vary from histologically benign forms to highly anaplastic and malignant tumors. Fibrillary astrocytomas are the most common type and may be classified in order of increasing malignancy (grades I through IV). In the first two decades of life, astrocytomas tend to originate in the cerebellar hemispheres; in adults, they most frequently arise in the cerebrum and frequently undergo malignant transformation (MeSH)."^^xsd:string ;
    rdfs:subClassOf BIRNLEX:12600 ;
    NIFRID:createdDate "2007-10-05"^^xsd:string ;
    NIFRID:modifiedDate "2007-10-05"^^xsd:string ;
    NIFRID:definingCitation "Devita et al., Cancer: Principles and Practice of Oncology, 5th ed, pp2013-7; Holland et al., Cancer Medicine, 3d ed, p1082"^^xsd:string ;
    NIFRID:hasBirnlexCurator NIFRID:Bill_Bug ;
    NIFRID:hasCurationStatus NIFRID:uncurated ;
    NIFRID:hasDefinitionSource NIFRID:MeSH_defSource ;
    NIFRID:hasExternalSource NIFRID:MeSH ;
    NIFRID:MeshUid "D001254"^^xsd:string ;
    NIFRID:usageNote "The following Entry Terms in MeSH imply a series of sub-types based on anatomical location, developmental onset, histological profile, and neoplastic state: Astrocytoma, Grade I; Astrocytoma, Grade II; Astrocytoma, Grade III; Astrocytoma, Protoplasmic; Astrocytoma, Subependymal Giant Cell; Cerebral Astrocytoma; Childhood Cerebral Astrocytoma; Fibrillary Astrocytoma; Gemistocytic Astrocytoma; Intracranial Astrocytoma; Juvenile Pilocytic Astrocytoma; Oligoastrocytoma, Mixed; Pilocytic Astrocytoma; Subependymal Giant Cell Astrocytoma"^^xsd:string ;
    skos:scopeNote "Grades I-III go here, with pathol"^^xsd:string .

BIRNLEX:12620 a owl:Class ;
    rdfs:label "Glioblastoma"^^xsd:string ;
    skos:prefLabel "Glioblastoma"^^xsd:string ;
    NIFRID:synonym "Astrocytoma, Grade IV"^^xsd:string,
        "Giant Cell Glioblastoma"^^xsd:string,
        "Glioblastoma Multiforme"^^xsd:string ;
    skos:definition "A malignant form of astrocytoma histologically characterized by pleomorphism of cells, nuclear atypia, microhemorrhage, and necrosis. They may arise in any region of the central nervous system, with a predilection for the cerebral hemispheres, basal ganglia, and commissural pathways. Clinical presentation most frequently occurs in the fifth or sixth decade of life with focal neurologic signs or seizures (MeSH)."^^xsd:string ;
    rdfs:subClassOf BIRNLEX:12619 ;
    NIFRID:createdDate "2007-10-05"^^xsd:string ;
    NIFRID:modifiedDate "2007-10-05"^^xsd:string ;
    NIFRID:hasBirnlexCurator NIFRID:Bill_Bug ;
    NIFRID:hasCurationStatus NIFRID:uncurated ;
    NIFRID:hasDefinitionSource NIFRID:MeSH_defSource ;
    NIFRID:hasExternalSource NIFRID:MeSH ;
    NIFRID:MeshUid "D005909"^^xsd:string ;
    skos:scopeNote "for GLIOBLASTOMA, RETINAL see RETINOBLASTOMA"^^xsd:string .

BIRNLEX:12621 a owl:Class ;
    rdfs:label "Optic Nerve Glioma"^^xsd:string ;
    skos:prefLabel "Optic Nerve Glioma"^^xsd:string ;
    NIFRID:synonym "Glioblastoma Multiforme"^^xsd:string,
        "Malignant Optic Nerve Astrocytoma"^^xsd:string,
        "Optic Glioma"^^xsd:string ;
    skos:definition "Glial cell derived tumors arising from the optic nerve, usually presenting in childhood. Roughly 50% are associated with NEUROFIBROMATOSIS 1. Clinical manifestations include decreased visual acuity; EXOPHTHALMOS; NYSTAGMUS, PATHOLOGIC; STRABISMUS; pallor or swelling of the optic disc; and INTRACRANIAL HYPERTENSION. The tumor may extend into the optic chiasm and hypothalamus (MeSH)."^^xsd:string ;
    rdfs:subClassOf BIRNLEX:12619 ;
    NIFRID:createdDate "2007-10-05"^^xsd:string ;
    NIFRID:modifiedDate "2007-10-05"^^xsd:string ;
    NIFRID:definingCitation "Adams et al., Principles of Neurology, 6th ed, p681"^^xsd:string ;
    NIFRID:hasBirnlexCurator NIFRID:Bill_Bug ;
    NIFRID:hasCurationStatus NIFRID:uncurated ;
    NIFRID:hasDefinitionSource NIFRID:MeSH_defSource ;
    NIFRID:hasExternalSource NIFRID:MeSH ;
    NIFRID:MeshUid "D020339"^^xsd:string .

BIRNLEX:12622 a owl:Class ;
    rdfs:label "Ependymoma"^^xsd:string ;
    skos:prefLabel "Ependymoma"^^xsd:string ;
    skos:definition "Glioma derived from ependymocytes that tend to present as malignant intracranial tumors in children and as benign intraspinal neoplasms in adults. It may arise from any level of the ventricular system or central canal of the spinal cord. Intracranial ependymomas most frequently originate in the FOURTH VENTRICLE and histologically are densely cellular tumors which may contain ependymal tubules and perivascular pseudorosettes. Spinal ependymomas are usually benign papillary or myxopapillary tumors (MeSH)."^^xsd:string ;
    rdfs:subClassOf BIRNLEX:12618 ;
    NIFRID:createdDate "2007-10-05"^^xsd:string ;
    NIFRID:modifiedDate "2007-10-05"^^xsd:string ;
    NIFRID:definingCitation "DeVita et al., Principles and Practice of Oncology, 5th ed, p2018; Escourolle et al., Manual of Basic Neuropathology, 2nd ed, pp28-9"^^xsd:string ;
    NIFRID:hasBirnlexCurator NIFRID:Bill_Bug ;
    NIFRID:hasCurationStatus NIFRID:uncurated ;
    NIFRID:hasDefinitionSource NIFRID:MeSH_defSource ;
    NIFRID:hasExternalSource NIFRID:MeSH ;
    NIFRID:MeshUid "D004806"^^xsd:string ;
    NIFRID:usageNote "The following Entry Terms in MeSH imply a series of sub-types based on gross anatomy, histological profile, and neoplastic state: Anaplastic Ependymoma; Cellular Ependymoma; Clear Cell Ependymoma; Ependymoma, Myxopapillary; Ependymoma, Papillary; Papillary Ependymoma"^^xsd:string .

BIRNLEX:12623 a owl:Class ;
    rdfs:label "Subependymal Glioma"^^xsd:string ;
    skos:prefLabel "Subependymal Glioma"^^xsd:string ;
    NIFRID:synonym "Subependymal Astrocytoma"^^xsd:string,
        "Subependymal Gliosis"^^xsd:string,
        "Subependymoma"^^xsd:string ;
    skos:definition "Rare, slow-growing, benign intraventricular tumors, often asymptomatic and discovered incidentally. The tumors are classified histologically as ependymomas and demonstrate a proliferation of subependymal fibrillary astrocytes among the ependymal tumor cells (MeSH)."^^xsd:string ;
    rdfs:subClassOf BIRNLEX:12622 ;
    NIFRID:createdDate "2007-10-05"^^xsd:string ;
    NIFRID:modifiedDate "2007-10-05"^^xsd:string ;
    NIFRID:definingCitation "Clin Neurol Neurosurg 1997 Feb;99(1):17-22"^^xsd:string ;
    NIFRID:hasBirnlexCurator NIFRID:Bill_Bug ;
    NIFRID:hasCurationStatus NIFRID:uncurated ;
    NIFRID:hasDefinitionSource NIFRID:MeSH_defSource ;
    NIFRID:hasExternalSource NIFRID:MeSH ;
    NIFRID:MeshUid "D004806"^^xsd:string ;
    NIFRID:usageNote "The following Entry Terms in MeSH imply a series of sub-types based on gross anatomy, histological profile, and neoplastic state: Anaplastic Ependymoma; Cellular Ependymoma; Clear Cell Ependymoma; Ependymoma, Myxopapillary; Ependymoma, Papillary; Papillary Ependymoma"^^xsd:string .

BIRNLEX:12624 a owl:Class ;
    rdfs:label "Ganglioglioma"^^xsd:string ;
    skos:prefLabel "Ganglioglioma"^^xsd:string ;
    skos:definition "Rare indolent tumors comprised of neoplastic glial and neuronal cells which occur primarily in children and young adults. Benign lesions tend to be associated with long survival unless the tumor degenerates into a histologically malignant form. They tend to occur in the optic nerve and white matter of the brain and spinal cord (MeSH)."^^xsd:string ;
    rdfs:subClassOf BIRNLEX:12618 ;
    NIFRID:createdDate "2007-10-05"^^xsd:string ;
    NIFRID:modifiedDate "2007-10-05"^^xsd:string ;
    NIFRID:hasBirnlexCurator NIFRID:Bill_Bug ;
    NIFRID:hasCurationStatus NIFRID:uncurated ;
    NIFRID:hasDefinitionSource NIFRID:MeSH_defSource ;
    NIFRID:hasExternalSource NIFRID:MeSH ;
    NIFRID:MeshUid "D018303"^^xsd:string ;
    NIFRID:putativeClassExtension "Benign ganglioglioma"^^xsd:string,
        "Intracranial ganglioglioma"^^xsd:string,
        "Malignant ganglioglioma"^^xsd:string ;
    NIFRID:usageNote "MeSH includes qualified subtypes"^^xsd:string .

BIRNLEX:12625 a owl:Class ;
    rdfs:label "Gliosarcoma"^^xsd:string ;
    skos:prefLabel "Gliosarcoma"^^xsd:string ;
    NIFRID:synonym "Glioblastoma with Sarcomatous Component"^^xsd:string,
        "Sarcomatous Glioma"^^xsd:string ;
    skos:definition "Rare mixed tumors of the brain and rarely the spinal cord which contain malignant neuroectodermal (glial) and mesenchymal components, including spindle-shaped fibrosarcoma cells. These tumors are highly aggressive and present primarily in adults as rapidly expanding mass lesions. They may arise in tissue that has been previously irradiated (MeSH)."^^xsd:string ;
    rdfs:subClassOf BIRNLEX:12618 ;
    NIFRID:createdDate "2007-10-05"^^xsd:string ;
    NIFRID:modifiedDate "2007-10-05"^^xsd:string ;
    NIFRID:definingCitation "Br J Neurosurg 1995 Apr;9(2):171-8"^^xsd:string ;
    NIFRID:hasBirnlexCurator NIFRID:Bill_Bug ;
    NIFRID:hasCurationStatus NIFRID:uncurated ;
    NIFRID:hasDefinitionSource NIFRID:MeSH_defSource ;
    NIFRID:hasExternalSource NIFRID:MeSH ;
    NIFRID:MeshUid "D018316"^^xsd:string .

BIRNLEX:12626 a owl:Class ;
    rdfs:label "Medulloblastoma"^^xsd:string ;
    skos:prefLabel "Medulloblastoma"^^xsd:string ;
    NIFRID:synonym "Medullomyoblastoma"^^xsd:string ;
    skos:definition "A malignant neoplasm that may be classified either as a glioma or as a primitive neuroectodermal tumor of childhood (see NEUROECTODERMAL TUMOR, PRIMITIVE). The tumor occurs most frequently in the first decade of life with the most typical location being the cerebellar vermis. Histologic features include a high degree of cellularity, frequent mitotic figures, and a tendency for the cells to organize into sheets or form rosettes. Medulloblastoma have a high propensity to spread throughout the craniospinal intradural axis (MeSH)."^^xsd:string ;
    rdfs:subClassOf BIRNLEX:12618 ;
    NIFRID:createdDate "2007-10-05"^^xsd:string ;
    NIFRID:modifiedDate "2007-10-05"^^xsd:string ;
    NIFRID:definingCitation "DeVita et al., Cancer: Principles and Practice of Oncology, 5th ed, pp2060-1"^^xsd:string ;
    NIFRID:hasBirnlexCurator NIFRID:Bill_Bug ;
    NIFRID:hasCurationStatus NIFRID:uncurated ;
    NIFRID:hasDefinitionSource NIFRID:MeSH_defSource ;
    NIFRID:hasExternalSource NIFRID:MeSH ;
    NIFRID:MeshUid "D008527"^^xsd:string ;
    NIFRID:putativeClassExtension "Adult medulloblastoma"^^xsd:string,
        "Childhood medulloblastoma"^^xsd:string,
        "Circumscribed arachnoidal cerebellar sarcoma"^^xsd:string,
        "Desmoplastic medulloblastoma"^^xsd:string,
        "Melanocytic medulloblastoma"^^xsd:string ;
    NIFRID:usageNote "MeSH includes qualified subtypes"^^xsd:string .

BIRNLEX:12627 a owl:Class ;
    rdfs:label "Oligodendroglioma"^^xsd:string ;
    skos:prefLabel "Oligodendroglioma"^^xsd:string ;
    NIFRID:synonym "Mixed Oligodendroglioma-Astrocytoma"^^xsd:string,
        "Mixed Oligodendroglioma-Ependymoma"^^xsd:string,
        "Oligodendroblastoma"^^xsd:string ;
    skos:definition "A relatively slow-growing glioma that is derived from oligodendrocytes and tends to occur in the cerebral hemispheres, thalamus, or lateral ventricle. They may present at any age, but are most frequent in the third to fifth decades, with an earlier incidence peak in the first decade. Histologically, these tumors are encapsulated, relatively avascular, and tend to form cysts and microcalcifications. Neoplastic cells tend to have small round nuclei surrounded by unstained nuclei. The tumors may vary from well-differentiated to highly anaplastic forms (MeSH)."^^xsd:string ;
    rdfs:subClassOf BIRNLEX:12618 ;
    NIFRID:createdDate "2007-10-05"^^xsd:string ;
    NIFRID:modifiedDate "2007-10-05"^^xsd:string ;
    NIFRID:definingCitation "DeVita et al., Cancer: Principles and Practice of Oncology, 5th edOncology, p2052; Adams et al., Principles of Neurology, 6th ed, p655"^^xsd:string ;
    NIFRID:hasBirnlexCurator NIFRID:Bill_Bug ;
    NIFRID:hasCurationStatus NIFRID:uncurated ;
    NIFRID:hasDefinitionSource NIFRID:MeSH_defSource ;
    NIFRID:hasExternalSource NIFRID:MeSH ;
    NIFRID:MeshUid "D009837"^^xsd:string ;
    NIFRID:putativeClassExtension "Adult oligodendroglioma"^^xsd:string,
        "Anaplastic oligodendroglioma"^^xsd:string,
        "Childhood oligodendroglioma"^^xsd:string,
        "Well-differentiated oligodendroglioma"^^xsd:string ;
    NIFRID:usageNote "MeSH includes qualified subtypes"^^xsd:string .

BIRNLEX:12628 a owl:Class ;
    rdfs:label "Neurocytoma"^^xsd:string ;
    skos:prefLabel "Neurocytoma"^^xsd:string ;
    NIFRID:synonym "Central Neurocytoma"^^xsd:string ;
    skos:definition "A benign brain tumor composed of neural elements which most often arise from the SEPTUM PELLUCIDUM and the walls of the lateral ventricles. Immunohistochemistry and electron microscopy evaluations may reveal expression of neuron specific enolase and synaptophysin and cells containing microtubuli, neurosecretory granules, and presynaptic vesicles (MeSH)."^^xsd:string ;
    rdfs:subClassOf BIRNLEX:12600 ;
    NIFRID:createdDate "2007-10-05"^^xsd:string ;
    NIFRID:modifiedDate "2007-10-05"^^xsd:string ;
    NIFRID:definingCitation "Acta Med Port 1994 Feb;7(2):113-9"^^xsd:string ;
    NIFRID:hasBirnlexCurator NIFRID:Bill_Bug ;
    NIFRID:hasCurationStatus NIFRID:uncurated ;
    NIFRID:hasDefinitionSource NIFRID:MeSH_defSource ;
    NIFRID:hasExternalSource NIFRID:MeSH ;
    NIFRID:MeshUid "D018306"^^xsd:string .

BIRNLEX:12629 a owl:Class ;
    rdfs:label "Primitive Neuroectodermal Neoplasm"^^xsd:string ;
    skos:prefLabel "Primitive Neuroectodermal Neoplasm"^^xsd:string ;
    NIFRID:synonym "Primitive Neuroectodermal Tumor"^^xsd:string,
        "Primitive Neuroepithelial Neoplasm"^^xsd:string,
        "Primitive Neuroepithelial Tumor"^^xsd:string ;
    skos:definition "A group of malignant tumors of the nervous system that feature primitive cells with elements of neuronal and/or glial differentiation. Use of this term is limited by some authors to central nervous system tumors and others include neoplasms of similar origin which arise extracranially (i.e., NEUROECTODERMAL TUMORS, PRIMITIVE, PERIPHERAL). This term is also occasionally used as a synonym for MEDULLOBLASTOMA. In general, these tumors arise in the first decade of life and tend to be highly malignant (MeSH)."^^xsd:string ;
    rdfs:subClassOf BIRNLEX:12600 ;
    NIFRID:createdDate "2007-10-05"^^xsd:string ;
    NIFRID:modifiedDate "2007-10-05"^^xsd:string ;
    NIFRID:acronym "PNET"^^xsd:string ;
    NIFRID:definingCitation "DeVita et al., Cancer: Principles and Practice of Oncology, 5th ed, p2059"^^xsd:string ;
    NIFRID:hasBirnlexCurator NIFRID:Bill_Bug ;
    NIFRID:hasCurationStatus NIFRID:uncurated ;
    NIFRID:hasDefinitionSource NIFRID:MeSH_defSource ;
    NIFRID:hasExternalSource NIFRID:MeSH ;
    NIFRID:MeshUid "D018242"^^xsd:string ;
    NIFRID:putativeClassExtension "Ependymoblastoma"^^xsd:string,
        "Medulloepithelioma"^^xsd:string,
        "Spongioblastoma"^^xsd:string ;
    NIFRID:usageNote "MeSH includes qualified subtypes."^^xsd:string .

BIRNLEX:12630 a owl:Class ;
    rdfs:label "Peripheral Primitive Neuroectodermal Neoplasm"^^xsd:string ;
    skos:prefLabel "Peripheral Primitive Neuroectodermal Neoplasm"^^xsd:string ;
    NIFRID:synonym "Extracranial Primitive Neuroectodermal Tumor"^^xsd:string,
        "Neuroepithelioma"^^xsd:string,
        "Peripheral Neuroectodermal Tumor"^^xsd:string,
        "Peripheral Primitive Neuroectodermal Tumor"^^xsd:string ;
    skos:definition "A group of highly cellular primitive round cell neoplasms which occur extracranially in soft tissue and bone and are derived from embryonal neural crest cells. These tumors occur primarily in children and adolescents and share a number of characteristics with Ewing's Sarcoma ( SARCOMA, EWING'S). They may arise from the chest wall, skin, orbit, kidney, and other structures and tend to be locally invasive or metastasize, although relatively benign forms may occur. Characteristic histologic features include a tendency to form Homer-Wright rosettes and to stain positively with neuron-specific enolase and vimentin (MeSH)."^^xsd:string ;
    rdfs:subClassOf BIRNLEX:12629 ;
    NIFRID:createdDate "2007-10-05"^^xsd:string ;
    NIFRID:modifiedDate "2007-10-05"^^xsd:string ;
    NIFRID:acronym "pPNET"^^xsd:string ;
    NIFRID:definingCitation "DeVita et al., Cancer: Principles and Practice of Oncology, 5th ed, p2113; J Clin Oncol 1998 Mar;16(3):1150-7"^^xsd:string ;
    NIFRID:hasBirnlexCurator NIFRID:Bill_Bug ;
    NIFRID:hasCurationStatus NIFRID:uncurated ;
    NIFRID:hasDefinitionSource NIFRID:MeSH_defSource ;
    NIFRID:hasExternalSource NIFRID:MeSH ;
    NIFRID:MeshUid "D018241"^^xsd:string .

BIRNLEX:12631 a owl:Class ;
    rdfs:label "Neuroblastoma"^^xsd:string ;
    skos:prefLabel "Neuroblastoma"^^xsd:string ;
    skos:definition "A common neoplasm of early childhood arising from neural crest cells in the sympathetic nervous system, and characterized by diverse clinical behavior, ranging from spontaneous remission to rapid metastatic progression and death. This tumor is the most common intraabdominal malignancy of childhood, but it may also arise from thorax, neck, or rarely occur in the central nervous system. Histologic features include uniform round cells with hyperchromatic nuclei arranged in nests and separated by fibrovascular septa. Neuroblastomas may be associated with the opsoclonus-myoclonus syndrome (MeSH)."^^xsd:string ;
    rdfs:subClassOf BIRNLEX:12630 ;
    NIFRID:createdDate "2007-10-05"^^xsd:string ;
    NIFRID:modifiedDate "2007-10-05"^^xsd:string ;
    NIFRID:definingCitation "DeVita et al., Cancer: Principles and Practice of Oncology, 5th ed, pp2099-2101; Curr Opin Oncol 1998 Jan;10(1):43-51"^^xsd:string ;
    NIFRID:hasBirnlexCurator NIFRID:Bill_Bug ;
    NIFRID:hasCurationStatus NIFRID:uncurated ;
    NIFRID:hasDefinitionSource NIFRID:MeSH_defSource ;
    NIFRID:hasExternalSource NIFRID:MeSH ;
    NIFRID:MeshUid "D009447"^^xsd:string .

BIRNLEX:12632 a owl:Class ;
    rdfs:label "Olfactory Esthesioneuroblastoma"^^xsd:string ;
    skos:prefLabel "Olfactory Esthesioneuroblastoma"^^xsd:string ;
    NIFRID:synonym "Aesthesioneuroblastoma"^^xsd:string,
        "Esthesioneuroblastoma"^^xsd:string,
        "Olfactory Neuroblastoma"^^xsd:string,
        "Paranasal Sinus-Nasal Cavity Esthesioneuroblastoma"^^xsd:string ;
    skos:definition "A malignant olfactory neuroblastoma arising from the olfactory epithelium of the superior nasal cavity and cribriform plate. It is uncommon (3% of nasal tumors) and rarely is associated with the production of excess hormones (e.g., SIADH, Cushing Syndrome). It has a high propensity for multiple local recurrences and bony metastases (MeSH)."^^xsd:string ;
    rdfs:subClassOf BIRNLEX:12631 ;
    NIFRID:createdDate "2007-10-05"^^xsd:string ;
    NIFRID:modifiedDate "2007-10-05"^^xsd:string ;
    NIFRID:definingCitation "Holland et al., Cancer Medicine, 3rd ed, p1245; J Laryngol Otol 1998 Jul;112(7):628-33"^^xsd:string ;
    NIFRID:hasBirnlexCurator NIFRID:Bill_Bug ;
    NIFRID:hasCurationStatus NIFRID:uncurated ;
    NIFRID:hasDefinitionSource NIFRID:MeSH_defSource ;
    NIFRID:hasExternalSource NIFRID:MeSH ;
    NIFRID:MeshUid "D018304"^^xsd:string .

BIRNLEX:12633 a owl:Class ;
    rdfs:label "Ganglioneuroblastoma"^^xsd:string ;
    skos:prefLabel "Ganglioneuroblastoma"^^xsd:string ;
    skos:definition "A moderately malignant neoplasm composed of primitive neuroectodermal cells dispersed in myxomatous or fibrous stroma intermixed with mature ganglion cells. It may undergo transformation into a neuroblastoma. It arises from the sympathetic trunk or less frequently from the adrenal medulla, cerebral cortex, and other locations. Cervical ganglioneuroblastomas may be associated with HORNER SYNDROME and the tumor may occasionally secrete vasoactive intestinal peptide, resulting in chronic diarrhea (MeSH)."^^xsd:string ;
    rdfs:subClassOf BIRNLEX:12631 ;
    NIFRID:createdDate "2007-10-05"^^xsd:string ;
    NIFRID:modifiedDate "2007-10-05"^^xsd:string ;
    NIFRID:hasBirnlexCurator NIFRID:Bill_Bug ;
    NIFRID:hasCurationStatus NIFRID:uncurated ;
    NIFRID:hasDefinitionSource NIFRID:MeSH_defSource ;
    NIFRID:hasExternalSource NIFRID:MeSH ;
    NIFRID:MeshUid "D018305"^^xsd:string .

BIRNLEX:12634 a owl:Class ;
    rdfs:label "Pinealoma"^^xsd:string ;
    skos:prefLabel "Pinealoma"^^xsd:string ;
    NIFRID:synonym "Pineal Neoplasm"^^xsd:string,
        "Pineal Parenchymal Tumor"^^xsd:string,
        "Pineal Tumor"^^xsd:string,
        "Pinealocytoma"^^xsd:string,
        "Pineoblastoma"^^xsd:string,
        "Pineocytoma"^^xsd:string ;
    skos:definition "Neoplasms which originate from pineal parenchymal cells that tend to enlarge the gland and be locally invasive. The two major forms are pineocytoma and the more malignant pineoblastoma. Pineocytomas have moderate cellularity and tend to form rosette patterns. Pineoblastomas are highly cellular tumors containing small, poorly differentiated cells. These tumors occasionally seed the neuroaxis or cause obstructive HYDROCEPHALUS or Parinaud's syndrome. GERMINOMA; CARCINOMA, EMBRYONAL; GLIOMA; and other neoplasms may arise in the pineal region with germinoma being the most common pineal region tumor (MeSH)."^^xsd:string ;
    rdfs:subClassOf BIRNLEX:12600 ;
    NIFRID:createdDate "2007-10-05"^^xsd:string ;
    NIFRID:modifiedDate "2007-10-05"^^xsd:string ;
    NIFRID:definingCitation "DeVita et al., Cancer: Principles and Practice of Oncology, 5th ed, p2064; Adams et al., Principles of Neurology, 6th ed, p670"^^xsd:string ;
    NIFRID:hasBirnlexCurator NIFRID:Bill_Bug ;
    NIFRID:hasCurationStatus NIFRID:uncurated ;
    NIFRID:hasDefinitionSource NIFRID:MeSH_defSource ;
    NIFRID:hasExternalSource NIFRID:MeSH ;
    NIFRID:MeshUid "D010871"^^xsd:string .

BIRNLEX:12635 a owl:Class ;
    rdfs:label "Retinoblastoma"^^xsd:string ;
    skos:prefLabel "Retinoblastoma"^^xsd:string ;
    NIFRID:synonym "Retinal Glioblastoma"^^xsd:string,
        "Retinal Glioma"^^xsd:string,
        "Retinal Neuroblastoma"^^xsd:string ;
    skos:definition "A malignant tumor arising from the nuclear layer of the retina that is the most common primary tumor of the eye in children. The tumor tends to occur in early childhood or infancy and may be present at birth. The majority are sporadic, but the condition may be transmitted as an autosomal dominant trait. Histologic features include dense cellularity, small round polygonal cells, and areas of calcification and necrosis. An abnormal pupil reflex (leukokoria); NYSTAGMUS, PATHOLOGIC; STRABISMUS; and visual loss represent common clinical characteristics of this condition (MeSH)."^^xsd:string ;
    rdfs:subClassOf BIRNLEX:12600 ;
    NIFRID:createdDate "2007-10-05"^^xsd:string ;
    NIFRID:modifiedDate "2007-10-05"^^xsd:string ;
    NIFRID:definingCitation "DeVita et al., Cancer: Principles and Practice of Oncology, 5th ed, p2104"^^xsd:string ;
    NIFRID:hasBirnlexCurator NIFRID:Bill_Bug ;
    NIFRID:hasCurationStatus NIFRID:uncurated ;
    NIFRID:hasDefinitionSource NIFRID:MeSH_defSource ;
    NIFRID:hasExternalSource NIFRID:MeSH ;
    NIFRID:MeshUid "D012175"^^xsd:string .

BIRNLEX:12636 a owl:Class ;
    rdfs:label "Familial Retinoblastoma"^^xsd:string ;
    skos:prefLabel "Familial Retinoblastoma"^^xsd:string ;
    NIFRID:synonym "Hereditary Retinoblastoma"^^xsd:string ;
    rdfs:subClassOf BIRNLEX:12635 ;
    NIFRID:createdDate "2007-10-05"^^xsd:string ;
    NIFRID:modifiedDate "2007-10-05"^^xsd:string ;
    NIFRID:hasBirnlexCurator NIFRID:Bill_Bug ;
    NIFRID:hasCurationStatus NIFRID:uncurated ;
    NIFRID:hasExternalSource NIFRID:MeSH ;
    NIFRID:MeshUid "D012175"^^xsd:string .

BIRNLEX:12637 a owl:Class ;
    rdfs:label "Sporadic Retinoblastoma"^^xsd:string ;
    skos:prefLabel "Sporadic Retinoblastoma"^^xsd:string ;
    rdfs:subClassOf BIRNLEX:12635 ;
    NIFRID:createdDate "2007-10-05"^^xsd:string ;
    NIFRID:modifiedDate "2007-10-05"^^xsd:string ;
    NIFRID:hasBirnlexCurator NIFRID:Bill_Bug ;
    NIFRID:hasCurationStatus NIFRID:uncurated ;
    NIFRID:hasExternalSource NIFRID:MeSH ;
    NIFRID:MeshUid "D012175"^^xsd:string .

BIRNLEX:12638 a owl:Class ;
    rdfs:label "Dyskinesia"^^xsd:string ;
    skos:prefLabel "Dyskinesia"^^xsd:string ;
    NIFRID:synonym "Abnormal Movements"^^xsd:string,
        "Asterixis"^^xsd:string,
        "Ballismus"^^xsd:string,
        "Hemiballism"^^xsd:string,
        "Hemiballismus"^^xsd:string,
        "Involuntary Movements"^^xsd:string ;
    skos:definition "Abnormal involuntary movements which primarily affect the extremities, trunk, or jaw that occur as a manifestation of an underlying disease process. Conditions which feature recurrent or persistent episodes of dyskinesia as a primary manifestation of disease may be referred to as dyskinesia syndromes (see MOVEMENT DISORDERS). Dyskinesias are also a relatively common manifestation of BASAL GANGLIA DISEASES (MeSH)."^^xsd:string ;
    rdfs:subClassOf BIRNLEX:12796 ;
    skos:editorialNote "May need to create a \"malfunction\" dependent_continuant or disposition to accomodate most of the Dyskinesias which are more functional presenting signs in a complex disease process than a disease in and of themselves (BB:2007-10-05)."^^xsd:string,
        "Note BIRNLex seeks to evolve a core subsumptive disease hierarchy based first on the effected function, then the effected structure, the latter for those categories of nervous system disease that have typically been associated with structural abnormalities or trauma (e.g., Motor neuron diseases, cerebrovascular trauma, etc.). Disease causation is in fact the ultimate goal of much biomedical research, and our recognitition of ALL the driving causes of a particular disease - and the ways in which these causes inter-relate with each other and with effected structures to cause a change in normal function is a critical representational task BIRNlex will increasingly take on to provide an evolving, nuanced functional reconstruction of disease as a process and an outcome.  These relations will be represented using OWL ObjectProperties.  Function is the most sensible context to drive the asserted subsumptive hierarchy for representing nervous system disease, since it is with the clinical description of altered, impaired, decreased, or lost function that the diagnosis - and the research - of disease is rooted.  Much has already been described regarding both the effected biomaterial entities and the causes of disease.  However, it is because understanding of such relations still is far from comprehensive, that biomedical investigation into nervous system disease continues.  Finally, given the \"realist\" ontology design approach being used to construct BIRNLex, function must be represented as inhering in some biomaterial entity from molecules and their controlling elements on up through gross anatomical structures.  Over time, BIRNLex will provide the required relations to depict these functionally-related structures for both the normal and pathological function of the nervous system.  This will be true both for the causes and for the outcomes of nervous system disease.  Initial work to extend this expressive representation will focus on the neurodegenerative diseases being studied by BIRN researchers.  Though this will be te case, BIRNLex still needs to provide a core asserted hierarchy for a broad swarth of nervous system disease, so as to enable BIRN researchers to link to the breadth of disorders that may impact or relate to those directly under study."^^xsd:string ;
    NIFRID:createdDate "2007-10-05"^^xsd:string ;
    NIFRID:modifiedDate "2007-11-18"^^xsd:string ;
    NIFRID:hasBirnlexCurator NIFRID:Bill_Bug ;
    NIFRID:hasCurationStatus NIFRID:uncurated ;
    NIFRID:hasDefinitionSource NIFRID:MeSH_defSource ;
    NIFRID:hasExternalSource NIFRID:MeSH ;
    NIFRID:MeshUid "D020820"^^xsd:string ;
    NIFRID:nifID "_8.3_2.3"^^xsd:string .

BIRNLEX:12639 a owl:Class ;
    rdfs:label "Ataxia"^^xsd:string ;
    skos:prefLabel "Ataxia"^^xsd:string ;
    skos:definition "Impairment of the ability to perform smoothly coordinated voluntary movements. This condition may affect the limbs, trunk, eyes, pharynx, larynx, and other structures. Ataxia may result from impaired sensory or motor function. Sensory ataxia may result from posterior column injury or PERIPHERAL NERVE DISEASES. Motor ataxia may be associated with CEREBELLAR DISEASES; CEREBRAL CORTEX diseases; THALAMIC DISEASES; BASAL GANGLIA DISEASES; injury to the RED NUCLEUS; and other conditions (MeSH)."^^xsd:string ;
    rdfs:subClassOf BIRNLEX:12638 ;
    NIFRID:createdDate "2007-10-05"^^xsd:string ;
    NIFRID:modifiedDate "2007-10-05"^^xsd:string ;
    NIFRID:definingCitationURI <http://www.ninds.nih.gov/disorders/ataxia/ataxia.htm> ;
    NIFRID:hasBirnlexCurator NIFRID:Bill_Bug ;
    NIFRID:hasCurationStatus NIFRID:uncurated ;
    NIFRID:hasDefinitionSource NIFRID:MeSH_defSource ;
    NIFRID:hasExternalSource NIFRID:MeSH ;
    NIFRID:MeshUid "D001259"^^xsd:string ;
    NIFRID:nifID "_8.3_2.4"^^xsd:string .

BIRNLEX:12640 a owl:Class ;
    rdfs:label "Paresis"^^xsd:string ;
    skos:prefLabel "Paresis"^^xsd:string ;
    skos:definition "A general term referring to a mild to moderate degree of muscular weakness, occasionally used as a synonym for PARALYSIS (severe or complete loss of motor function). In the older literature, paresis often referred specifically to paretic neurosyphilis (see NEUROSYPHILIS). \"General paresis\" and \"general paralysis\" may still carry that connotation. Bilateral lower extremity paresis is referred to as PARAPARESIS (MeSH)."^^xsd:string ;
    rdfs:subClassOf BIRNLEX:12796 ;
    skos:editorialNote "Note BIRNLex seeks to evolve a core subsumptive disease hierarchy based first on the effected function, then the effected structure, the latter for those categories of nervous system disease that have typically been associated with structural abnormalities or trauma (e.g., Motor neuron diseases, cerebrovascular trauma, etc.). Disease causation is in fact the ultimate goal of much biomedical research, and our recognitition of ALL the driving causes of a particular disease - and the ways in which these causes inter-relate with each other and with effected structures to cause a change in normal function is a critical representational task BIRNlex will increasingly take on to provide an evolving, nuanced functional reconstruction of disease as a process and an outcome.  These relations will be represented using OWL ObjectProperties.  Function is the most sensible context to drive the asserted subsumptive hierarchy for representing nervous system disease, since it is with the clinical description of altered, impaired, decreased, or lost function that the diagnosis - and the research - of disease is rooted.  Much has already been described regarding both the effected biomaterial entities and the causes of disease.  However, it is because understanding of such relations still is far from comprehensive, that biomedical investigation into nervous system disease continues.  Finally, given the \"realist\" ontology design approach being used to construct BIRNLex, function must be represented as inhering in some biomaterial entity from molecules and their controlling elements on up through gross anatomical structures.  Over time, BIRNLex will provide the required relations to depict these functionally-related structures for both the normal and pathological function of the nervous system.  This will be true both for the causes and for the outcomes of nervous system disease.  Initial work to extend this expressive representation will focus on the neurodegenerative diseases being studied by BIRN researchers.  Though this will be te case, BIRNLex still needs to provide a core asserted hierarchy for a broad swarth of nervous system disease, so as to enable BIRN researchers to link to the breadth of disorders that may impact or relate to those directly under study."^^xsd:string ;
    NIFRID:createdDate "2007-11-18"^^xsd:string ;
    NIFRID:modifiedDate "2007-10-05"^^xsd:string ;
    NIFRID:hasBirnlexCurator NIFRID:Bill_Bug ;
    NIFRID:hasCurationStatus NIFRID:uncurated ;
    NIFRID:hasDefinitionSource NIFRID:MeSH_defSource ;
    NIFRID:hasExternalSource NIFRID:MeSH ;
    NIFRID:MeshUid "D010291"^^xsd:string ;
    NIFRID:putativeClassExtension "Brachial Paresis"^^xsd:string,
        "Crural Paresis"^^xsd:string,
        "Hemiparesis"^^xsd:string,
        "Lower Extremity Paresis"^^xsd:string,
        "Monoparesis"^^xsd:string,
        "Muscle Paresis"^^xsd:string,
        "Muscular Paresis"^^xsd:string,
        "Upper Extremity Paresis"^^xsd:string ;
    NIFRID:usageNote "MeSH includes qualified subtypes"^^xsd:string .

BIRNLEX:12641 a owl:Class ;
    rdfs:label "Paralysis"^^xsd:string ;
    skos:prefLabel "Paralysis"^^xsd:string ;
    NIFRID:synonym "Palsy"^^xsd:string,
        "Plegia"^^xsd:string ;
    skos:definition "Severe loss of motor function as compared with PARESIS, a slight loss; GENERAL PARALYSIS see NEUROSYPHILIS does not mean \"generalized paralysis\" ( = PARALYSIS); spastic paralysis = PARALYSIS (IM) + MUSCLE SPASTICITY (NIM); flaccid paralysis = PARALYSIS (IM) + MUSCLE FLACCIDITY (NIM) (MeSH)."^^xsd:string ;
    rdfs:subClassOf BIRNLEX:12796 ;
    skos:editorialNote "Note BIRNLex seeks to evolve a core subsumptive disease hierarchy based first on the effected function, then the effected structure, the latter for those categories of nervous system disease that have typically been associated with structural abnormalities or trauma (e.g., Motor neuron diseases, cerebrovascular trauma, etc.). Disease causation is in fact the ultimate goal of much biomedical research, and our recognitition of ALL the driving causes of a particular disease - and the ways in which these causes inter-relate with each other and with effected structures to cause a change in normal function is a critical representational task BIRNlex will increasingly take on to provide an evolving, nuanced functional reconstruction of disease as a process and an outcome.  These relations will be represented using OWL ObjectProperties.  Function is the most sensible context to drive the asserted subsumptive hierarchy for representing nervous system disease, since it is with the clinical description of altered, impaired, decreased, or lost function that the diagnosis - and the research - of disease is rooted.  Much has already been described regarding both the effected biomaterial entities and the causes of disease.  However, it is because understanding of such relations still is far from comprehensive, that biomedical investigation into nervous system disease continues.  Finally, given the \"realist\" ontology design approach being used to construct BIRNLex, function must be represented as inhering in some biomaterial entity from molecules and their controlling elements on up through gross anatomical structures.  Over time, BIRNLex will provide the required relations to depict these functionally-related structures for both the normal and pathological function of the nervous system.  This will be true both for the causes and for the outcomes of nervous system disease.  Initial work to extend this expressive representation will focus on the neurodegenerative diseases being studied by BIRN researchers.  Though this will be te case, BIRNLex still needs to provide a core asserted hierarchy for a broad swarth of nervous system disease, so as to enable BIRN researchers to link to the breadth of disorders that may impact or relate to those directly under study."^^xsd:string ;
    NIFRID:createdDate "2007-10-05"^^xsd:string ;
    NIFRID:modifiedDate "2007-11-18"^^xsd:string ;
    NIFRID:definingCitation "Adams et al., Principles of Neurology, 6th ed, p45"^^xsd:string ;
    NIFRID:hasBirnlexCurator NIFRID:Bill_Bug ;
    NIFRID:hasCurationStatus NIFRID:uncurated ;
    NIFRID:hasDefinitionSource NIFRID:MeSH_defSource ;
    NIFRID:hasExternalSource NIFRID:MeSH ;
    NIFRID:MeshUid "D010243"^^xsd:string ;
    NIFRID:nifID "_8.3_2.3"^^xsd:string ;
    NIFRID:putativeClassExtension "Todd Paralysis"^^xsd:string ;
    NIFRID:usageNote "MeSH includes qualified subtypes"^^xsd:string .

BIRNLEX:12642 a owl:Class ;
    rdfs:label "Metastatic nervous system neoplastic disease"^^xsd:string ;
    skos:prefLabel "Metastatic nervous system neoplastic disease"^^xsd:string ;
    skos:definition "Neoplasms not composed of nerve tissue located in the nervous system or its component nerves."^^xsd:string ;
    rdfs:subClassOf BIRNLEX:12525 ;
    NIFRID:createdDate "2007-10-05"^^xsd:string ;
    NIFRID:modifiedDate "2007-10-05"^^xsd:string ;
    NIFRID:hasBirnlexCurator NIFRID:Bill_Bug ;
    NIFRID:hasCurationStatus NIFRID:uncurated ;
    NIFRID:nifID "_8.3_10.2"^^xsd:string .

BIRNLEX:12643 a owl:Class ;
    rdfs:label "Nervous System Paraneoplastic Syndrome"^^xsd:string ;
    skos:prefLabel "Nervous System Paraneoplastic Syndrome"^^xsd:string ;
    skos:definition "Degenerative or inflammatory conditions affecting the central or peripheral nervous system that develop in association with a systemic neoplasm without direct invasion by tumor. They may be associated with circulating antibodies that react with the affected neural tissue (MeSH)."^^xsd:string ;
    rdfs:subClassOf BIRNLEX:2086 ;
    skos:editorialNote "Note that all of teh progeny of this class are in fact neurodegenerative diseases.  In holding  with the \"realist\" orientation and the effort to represent the CORE subsumptive hierarchy as a related set of functional or function-structure classes - as opposed to using causal relations to specify nervous system disease - Nervous System Paraneoplastic Syndromes have been made a sub-class of neurodegerative disease as opposed to metastatic nervous system neoplastic disease.  Causal relations - such as specify a specific neoplastic condition as the cause for the resulting degeration of nervous system structure and function - will be provided via ObjectProperties.  Certain disorders which are in fact Nervous System Paraneoplastic Syndromes - e.g., Lambert-Eaton Myasthenic Syndrome, Transverse Myelitis, Opsoclonus-Myoclonus Syndrome - are left as children of the functional disease categories based on the affected function (BB: 2007-10-06)."^^xsd:string ;
    NIFRID:createdDate "2007-10-05"^^xsd:string ;
    NIFRID:modifiedDate "2007-10-05"^^xsd:string ;
    NIFRID:definingCitation "Intern Med 1996 Dec;35(12):925-9"^^xsd:string ;
    NIFRID:hasBirnlexCurator NIFRID:Bill_Bug ;
    NIFRID:hasCurationStatus NIFRID:uncurated ;
    NIFRID:hasDefinitionSource NIFRID:MeSH_defSource ;
    NIFRID:hasExternalSource NIFRID:MeSH ;
    NIFRID:MeshUid "D020361"^^xsd:string ;
    NIFRID:nifID "_8.3_10.3"^^xsd:string ;
    NIFRID:putativeClassExtension "Paraneoplastic Autonomic Dysfunction"^^xsd:string,
        "Paraneoplastic Encephalomyelitis"^^xsd:string ;
    NIFRID:usageNote "MeSH includes qualified subtypes"^^xsd:string .

BIRNLEX:12644 a owl:Class ;
    rdfs:label "Limbic Encephalitis"^^xsd:string ;
    skos:prefLabel "Limbic Encephalitis"^^xsd:string ;
    NIFRID:synonym "Paraneoplastic Limbic Encephalitis"^^xsd:string ;
    skos:definition "A paraneoplastic syndrome marked by degeneration of neurons in the medial temporal lobe. Clinical features include behavioral changes, HALLUCINATIONS, loss of short term memory, anosmia, AGEUSIA, and DEMENTIA. Circulating anti-neuronal antibodies (anti-Hu; also called ANNA 1) and small cell lung carcinomas are frequently associated with this condition (MeSH)."^^xsd:string ;
    rdfs:subClassOf BIRNLEX:12643 ;
    NIFRID:createdDate "2007-10-05"^^xsd:string ;
    NIFRID:modifiedDate "2007-10-05"^^xsd:string ;
    NIFRID:definingCitation "Pathologe 1997 Sep;18(5):406-10; J Int Neuropsychol Soc 1996 Sep;2(5):460-6; Brain 1997 Jun;120(Pt 6):923-8"^^xsd:string ;
    NIFRID:hasBirnlexCurator NIFRID:Bill_Bug ;
    NIFRID:hasCurationStatus NIFRID:uncurated ;
    NIFRID:hasDefinitionSource NIFRID:MeSH_defSource ;
    NIFRID:hasExternalSource NIFRID:MeSH ;
    NIFRID:MeshUid "D020363"^^xsd:string .

BIRNLEX:12645 a owl:Class ;
    rdfs:label "Paraneoplastic Cerebellar Degeneration"^^xsd:string ;
    skos:prefLabel "Paraneoplastic Cerebellar Degeneration"^^xsd:string ;
    NIFRID:synonym "Paraneoplastic Cerebellar Syndrome"^^xsd:string ;
    skos:definition "Cerebellar degeneration associated with a remote neoplasm. Clinical manifestations include progressive limb and GAIT ATAXIA; DYSARTHRIA; and NYSTAGMUS, PATHOLOGIC. The histologic type of the associated neoplasm is usually carcinoma or lymphoma. Pathologically the cerebellar cortex and subcortical nuclei demonstrate diffuse degenerative changes. Anti-Purkinje cell antibodies (anti-Yo) are found in the serum of approximately 50% of affected individuals (MeSH)."^^xsd:string ;
    rdfs:subClassOf BIRNLEX:12643 ;
    NIFRID:createdDate "2007-10-05"^^xsd:string ;
    NIFRID:modifiedDate "2007-10-05"^^xsd:string ;
    NIFRID:definingCitation "Adams et al., Principles of Neurology, 6th ed, p686"^^xsd:string ;
    NIFRID:hasBirnlexCurator NIFRID:Bill_Bug ;
    NIFRID:hasCurationStatus NIFRID:uncurated ;
    NIFRID:hasDefinitionSource NIFRID:MeSH_defSource ;
    NIFRID:hasExternalSource NIFRID:MeSH ;
    NIFRID:MeshUid "D020362"^^xsd:string ;
    NIFRID:putativeClassExtension "Anti-Yo-Associated Paraneoplastic Cerebellar Degeneration"^^xsd:string ;
    NIFRID:usageNote "MeSH includes qualified subtypes"^^xsd:string .

BIRNLEX:12646 a owl:Class ;
    rdfs:label "Paraneoplastic Polyneuropathy"^^xsd:string ;
    skos:prefLabel "Paraneoplastic Polyneuropathy"^^xsd:string ;
    NIFRID:synonym "Paraneoplastic Neuropathy"^^xsd:string,
        "Paraneoplastic Peripheral Neuropathy"^^xsd:string ;
    skos:definition "A diffuse or multifocal peripheral neuropathy related to the remote effects of a neoplasm, most often carcinoma or lymphoma. Pathologically, there are inflammatory changes in peripheral nerves. The most common clinical presentation is a symmetric distal mixed sensorimotor polyneuropathy (MeSH)."^^xsd:string ;
    rdfs:subClassOf BIRNLEX:12643 ;
    NIFRID:createdDate "2007-10-05"^^xsd:string ;
    NIFRID:modifiedDate "2007-10-05"^^xsd:string ;
    NIFRID:definingCitation "Adams et al., Principles of Neurology, 6th ed, p1334"^^xsd:string ;
    NIFRID:hasBirnlexCurator NIFRID:Bill_Bug ;
    NIFRID:hasCurationStatus NIFRID:uncurated ;
    NIFRID:hasDefinitionSource NIFRID:MeSH_defSource ;
    NIFRID:hasExternalSource NIFRID:MeSH ;
    NIFRID:MeshUid "D020364"^^xsd:string .

BIRNLEX:12647 a owl:Class ;
    rdfs:label "Cerebellar Ataxia"^^xsd:string ;
    skos:prefLabel "Cerebellar Ataxia"^^xsd:string ;
    NIFRID:synonym "Adiadochokinesis"^^xsd:string,
        "Cerebellar Dysmetria"^^xsd:string,
        "Cerebellar Hemiataxia"^^xsd:string,
        "Cerebellar Incoordination"^^xsd:string,
        "Dysmetria"^^xsd:string ;
    skos:definition "Incoordination of voluntary movements that occur as a manifestation of CEREBELLAR DISEASES. Characteristic features include a tendency for limb movements to overshoot or undershoot a target (dysmetria), a tremor that occurs during attempted movements (intention TREMOR), impaired force and rhythm of diadochokinesis (rapidly alternating movements), and GAIT ATAXIA (MeSH)."^^xsd:string ;
    rdfs:subClassOf BIRNLEX:12639 ;
    NIFRID:createdDate "2007-10-05"^^xsd:string ;
    NIFRID:modifiedDate "2007-10-05"^^xsd:string ;
    NIFRID:definingCitation "Adams et al., Principles of Neurology, 6th ed, p90"^^xsd:string ;
    NIFRID:hasBirnlexCurator NIFRID:Bill_Bug ;
    NIFRID:hasCurationStatus NIFRID:uncurated ;
    NIFRID:hasDefinitionSource NIFRID:MeSH_defSource ;
    NIFRID:hasExternalSource NIFRID:MeSH ;
    NIFRID:MeshUid "D002524"^^xsd:string .

BIRNLEX:12648 a owl:Class ;
    rdfs:label "Spinocerebellar Ataxia"^^xsd:string ;
    skos:prefLabel "Spinocerebellar Ataxia"^^xsd:string ;
    NIFRID:synonym "Dominantly-Inherited Spinocerebellar Ataxia"^^xsd:string,
        "Spinocerebellar Atrophy"^^xsd:string ;
    skos:definition "A group of dominantly inherited, predominatly late-onset, cerebellar ataxias which have been divided into multiple subtypes based on clinical features and genetic mapping. Progressive ataxia is a central feature of these conditions, and in certain subtypes POLYNEUROPATHY; DYSARTHRIA; visual loss; and other disorders may develop (MeSH)."^^xsd:string ;
    rdfs:subClassOf BIRNLEX:12647 ;
    NIFRID:createdDate "2007-10-05"^^xsd:string ;
    NIFRID:modifiedDate "2007-10-05"^^xsd:string ;
    NIFRID:definingCitation "Joynt, Clinical Neurology, 1997, Ch65, pp 12-17; J Neuropathol Exp Neurol 1998 Jun;57(6):531-43"^^xsd:string ;
    NIFRID:definingCitationURI <http://www.ninds.nih.gov/disorders/ataxia/ataxia.htm> ;
    NIFRID:hasBirnlexCurator NIFRID:Bill_Bug ;
    NIFRID:hasCurationStatus NIFRID:uncurated ;
    NIFRID:hasDefinitionSource NIFRID:MeSH_defSource ;
    NIFRID:hasExternalSource NIFRID:MeSH ;
    NIFRID:MeshUid "D020754"^^xsd:string ;
    NIFRID:putativeClassExtension "Spinocerebellar Ataxia Type 1"^^xsd:string,
        "Spinocerebellar Ataxia Type 2"^^xsd:string,
        "Spinocerebellar Ataxia Type 4"^^xsd:string,
        "Spinocerebellar Ataxia Type 5"^^xsd:string,
        "Spinocerebellar Ataxia Type 6"^^xsd:string,
        "Spinocerebellar Ataxia Type 7"^^xsd:string ;
    NIFRID:usageNote "MeSH includes qualified subtypes"^^xsd:string .

BIRNLEX:12649 a owl:Class ;
    rdfs:label "Ataxia Telangiectasia"^^xsd:string ;
    skos:prefLabel "Ataxia Telangiectasia"^^xsd:string ;
    NIFRID:synonym "Ataxia Telangiectasia Syndrome"^^xsd:string,
        "Louis-Bar Syndrome"^^xsd:string ;
    skos:definition "An autosomal recessive inherited disorder characterized by choreoathetosis beginning in childhood, progressive CEREBELLAR ATAXIA; TELANGIECTASIS of CONJUNCTIVA and SKIN; DYSARTHRIA; B- and T-cell immunodeficiency, and RADIOSENSITIVITY to IONIZING RADIATION. Affected individuals are prone to recurrent sinobronchopulmonary infections, lymphoreticular neoplasms, and other malignancies. Serum ALPHA-FETOPROTEINS are usually elevated. The gene for this disorder (ATM) encodes a cell cycle checkpoint protein kinase and has been mapped to chromosome 11 (11q22-q23) (MeSH)."^^xsd:string ;
    rdfs:subClassOf BIRNLEX:12648 ;
    NIFRID:createdDate "2007-10-05"^^xsd:string ;
    NIFRID:modifiedDate "2007-10-05"^^xsd:string ;
    NIFRID:definingCitation "Menkes, Textbook of Child Neurology, 5th ed, p688"^^xsd:string ;
    NIFRID:definingCitationURI <http://www.ninds.nih.gov/disorders/a_t/a-t.htm> ;
    NIFRID:hasBirnlexCurator NIFRID:Bill_Bug ;
    NIFRID:hasCurationStatus NIFRID:uncurated ;
    NIFRID:hasDefinitionSource NIFRID:MeSH_defSource ;
    NIFRID:hasExternalSource NIFRID:MeSH ;
    NIFRID:MeshUid "D001260"^^xsd:string .

BIRNLEX:12650 a owl:Class ;
    rdfs:label "Machado-Joseph Disease"^^xsd:string ;
    skos:prefLabel "Machado-Joseph Disease"^^xsd:string ;
    NIFRID:synonym "Autosomal Dominant Striatonigral Degeneration"^^xsd:string,
        "Joseph Azorean Disease"^^xsd:string,
        "Joseph Disease"^^xsd:string,
        "Joseph's Disease"^^xsd:string,
        "Josephs Disease"^^xsd:string,
        "Machado-Joseph Azorean Disease"^^xsd:string,
        "Machado-Joseph's Disease"^^xsd:string,
        "Machado-Josephs Disease"^^xsd:string,
        "Nervous System Azorean Disease"^^xsd:string,
        "Spinocerebellar Ataxia Type 3"^^xsd:string ;
    skos:definition "A dominantly-inherited ATAXIA first described in people of Azorean and Portuguese descent, and subsequently identified in Brazil, Japan, China, and Australia. This disorder is classified as one of the SPINOCEREBELLAR ATAXIAS (Type 3) and has been associated with a mutation of the MJD1 gene on chromosome 14. Clinical features include progressive ataxia, DYSARTHRIA, postural instability, nystagmus, eyelid retraction, and facial FASCICULATIONS. DYSTONIA is prominent in younger patients (referred to as Type I Machado-Joseph Disease). Type II features ataxia and ocular signs; Type III features MUSCULAR ATROPHY and a sensorimotor neuropathy; and Type IV features extrapyramidal signs combined with a sensorimotor neuropathy (MeSH)."^^xsd:string ;
    rdfs:subClassOf BIRNLEX:12648 ;
    NIFRID:createdDate "2007-10-05"^^xsd:string ;
    NIFRID:modifiedDate "April 11, 2009"^^xsd:string ;
    NIFRID:definingCitation "Clin Neurosci 1995;3(1):17-22; Ann Neurol 1998 Mar;43(3):288-96"^^xsd:string ;
    NIFRID:definingCitationURI <http://www.ninds.nih.gov/disorders/machado_joseph/machado_joseph.htm> ;
    NIFRID:hasBirnlexCurator NIFRID:Bill_Bug ;
    NIFRID:hasCurationStatus NIFRID:uncurated ;
    NIFRID:hasDefinitionSource NIFRID:MeSH_defSource ;
    NIFRID:hasExternalSource NIFRID:MeSH ;
    NIFRID:MeshUid "D017827"^^xsd:string ;
    NIFRID:putativeClassExtension "Machado-Joseph Disease Type I"^^xsd:string,
        "Machado-Joseph Disease Type II"^^xsd:string,
        "Machado-Joseph Disease Type III"^^xsd:string,
        "Machado-Joseph Disease Type IV"^^xsd:string ;
    NIFRID:usageNote "MeSH includes qualified subtypes"^^xsd:string .

BIRNLEX:12651 a owl:Class ;
    rdfs:label "Gait Ataxia"^^xsd:string ;
    skos:prefLabel "Gait Ataxia"^^xsd:string ;
    NIFRID:synonym "Ataxia of Gait"^^xsd:string,
        "Cerebellar Gait"^^xsd:string,
        "Cerebellar Gait Ataxia"^^xsd:string ;
    skos:definition "Impairment of the ability to coordinate the movements required for normal ambulation ( WALKING) which may result from impairments of motor function or sensory feedback. This condition may be associated with BRAIN DISEASES (including CEREBELLAR DISEASES and BASAL GANGLIA DISEASES); SPINAL CORD DISEASES; or PERIPHERAL NERVOUS SYSTEM DISEASES (MeSH)."^^xsd:string ;
    rdfs:subClassOf BIRNLEX:12639 ;
    NIFRID:createdDate "2007-10-05"^^xsd:string ;
    NIFRID:modifiedDate "2007-10-05"^^xsd:string ;
    NIFRID:hasBirnlexCurator NIFRID:Bill_Bug ;
    NIFRID:hasCurationStatus NIFRID:uncurated ;
    NIFRID:hasDefinitionSource NIFRID:MeSH_defSource ;
    NIFRID:hasExternalSource NIFRID:MeSH ;
    NIFRID:MeshUid "D020234"^^xsd:string .

BIRNLEX:12652 a owl:Class ;
    rdfs:label "Athetosis"^^xsd:string ;
    skos:prefLabel "Athetosis"^^xsd:string ;
    NIFRID:synonym "Athetoid Movements"^^xsd:string,
        "Hammond Disease"^^xsd:string,
        "Hammond's Disease"^^xsd:string,
        "Hammonds Disease"^^xsd:string ;
    skos:definition "A dyskinesia characterized by an inability to maintain the fingers, toes, tongue, or other body parts in a stable position, resulting in continuous slow, sinusoidal, and flowing involuntary movements. This condition is frequently accompanied by CHOREA, where it is referred to as choreoathetosis. Athetosis may occur as a manifestation of BASAL GANGLIA DISEASES or DRUG TOXICITY (MeSH)."^^xsd:string ;
    rdfs:subClassOf BIRNLEX:12638 ;
    NIFRID:createdDate "2007-10-05"^^xsd:string ;
    NIFRID:modifiedDate "April 11, 2009"^^xsd:string ;
    NIFRID:definingCitation "Adams et al., Principles of Neurology, 6th ed, p76"^^xsd:string ;
    NIFRID:hasBirnlexCurator NIFRID:Bill_Bug ;
    NIFRID:hasCurationStatus NIFRID:uncurated ;
    NIFRID:hasDefinitionSource NIFRID:MeSH_defSource ;
    NIFRID:hasExternalSource NIFRID:MeSH ;
    NIFRID:MeshUid "D001264"^^xsd:string .

BIRNLEX:12653 a owl:Class ;
    rdfs:label "Catalepsy"^^xsd:string ;
    skos:prefLabel "Catalepsy"^^xsd:string ;
    NIFRID:synonym "Anochlesia"^^xsd:string,
        "Cerea Flexibilitas"^^xsd:string,
        "Flexibility, Waxy"^^xsd:string ;
    skos:definition "A condition characterized by inactivity, decreased responsiveness to stimuli, and a tendency to maintain an immobile posture. The limbs tend to remain in whatever position they are placed (waxy flexibility). Catalepsy may be associated with PSYCHOTIC DISORDERS (e.g., SCHIZOPHRENIA, CATATONIC), nervous system drug toxicity, and other conditions (MeSH)."^^xsd:string ;
    rdfs:subClassOf BIRNLEX:12638 ;
    NIFRID:createdDate "2007-10-05"^^xsd:string ;
    NIFRID:modifiedDate "2007-10-05"^^xsd:string ;
    NIFRID:hasBirnlexCurator NIFRID:Bill_Bug ;
    NIFRID:hasCurationStatus NIFRID:uncurated ;
    NIFRID:hasDefinitionSource NIFRID:MeSH_defSource ;
    NIFRID:hasExternalSource NIFRID:MeSH ;
    NIFRID:MeshUid "D002375"^^xsd:string .

BIRNLEX:12654 a owl:Class ;
    rdfs:label "Chorea"^^xsd:string ;
    skos:prefLabel "Chorea"^^xsd:string ;
    NIFRID:synonym "Choreic Movement"^^xsd:string,
        "Choreiform Movement"^^xsd:string ;
    skos:definition "Involuntary, forcible, rapid, jerky movements that may be subtle or become confluent, markedly altering normal patterns of movement. Hypotonia and pendular reflexes are often associated. Conditions which feature recurrent or persistent episodes of chorea as a primary manifestation of disease are referred to as CHOREATIC DISORDERS. Chorea is also a frequent manifestation of BASAL GANGLIA DISEASES (MeSH)."^^xsd:string ;
    rdfs:subClassOf BIRNLEX:12638 ;
    NIFRID:createdDate "2007-10-05"^^xsd:string ;
    NIFRID:modifiedDate "2007-10-05"^^xsd:string ;
    NIFRID:hasBirnlexCurator NIFRID:Bill_Bug ;
    NIFRID:hasCurationStatus NIFRID:uncurated ;
    NIFRID:hasDefinitionSource NIFRID:MeSH_defSource ;
    NIFRID:hasExternalSource NIFRID:MeSH ;
    NIFRID:MeshUid "D002819"^^xsd:string ;
    NIFRID:usageNote "choreoathetosis = CHOREA (IM) + ATHETOSIS (IM); MORVAN'S CHOREA see MYOKYMIA and CHOREATIC DISORDERS are also available"^^xsd:string .

BIRNLEX:12655 a owl:Class ;
    rdfs:label "Dystonia"^^xsd:string ;
    skos:prefLabel "Dystonia"^^xsd:string ;
    NIFRID:synonym "Muscle Dystonia"^^xsd:string ;
    skos:definition "A persistent attitude or posture due to the co-contraction of agonists and antagonist muscles in one region of the body. It most often affects the large axial muscles of the trunk and limb girdles. Conditions which feature persistent or recurrent episodes of dystonia as a primary manifestation of disease are referred to as DYSTONIC DISORDERS (MeSH)."^^xsd:string ;
    rdfs:subClassOf BIRNLEX:12638 ;
    NIFRID:createdDate "2007-10-05"^^xsd:string ;
    NIFRID:modifiedDate "2007-10-05"^^xsd:string ;
    NIFRID:definingCitation "Adams et al., Principles of Neurology, 6th ed, p77"^^xsd:string ;
    NIFRID:hasBirnlexCurator NIFRID:Bill_Bug ;
    NIFRID:hasCurationStatus NIFRID:uncurated ;
    NIFRID:hasDefinitionSource NIFRID:MeSH_defSource ;
    NIFRID:hasExternalSource NIFRID:MeSH ;
    NIFRID:MeshUid "D004421"^^xsd:string ;
    NIFRID:putativeClassExtension "Diurnal Dystonia"^^xsd:string,
        "Limb Dystonia"^^xsd:string,
        "Paroxysmal Dystonia"^^xsd:string ;
    NIFRID:usageNote "Do not confuse with MUSCLE HYPERTONIA or MUSCLE HYPOTONIA; DYSTONIC DISORDERS is available"^^xsd:string,
        "MeSH includes qualified subtypes"^^xsd:string .

BIRNLEX:12656 a owl:Class ;
    rdfs:label "Torticollis"^^xsd:string ;
    skos:prefLabel "Torticollis"^^xsd:string ;
    NIFRID:synonym "Cervical Dystonia"^^xsd:string,
        "Wryneck"^^xsd:string ;
    skos:definition "A common form of DYSTONIA due to involuntary sustained or spasmodic, repetitive muscle contractions in the neck region. According to the position of the twisted neck and head, cervical dystonia can be categorized as torticollis, laterocollis, retrocollis, and a combination of these abnormal postures; A symptom, not a disease, of a twisted neck. In most instances, the head is tipped toward one side and the chin rotated toward the other. The involuntary muscle contractions in the neck region of patients with torticollis can be due to congenital defects, trauma, inflammation, tumors, and neurological or other factors. (MeSH)."^^xsd:string ;
    rdfs:subClassOf BIRNLEX:12655 ;
    NIFRID:createdDate "2007-10-05"^^xsd:string ;
    NIFRID:modifiedDate "2007-10-05"^^xsd:string ;
    NIFRID:hasBirnlexCurator NIFRID:Bill_Bug ;
    NIFRID:hasCurationStatus NIFRID:uncurated ;
    NIFRID:hasDefinitionSource NIFRID:MeSH_defSource ;
    NIFRID:hasExternalSource NIFRID:MeSH ;
    NIFRID:MeshUid "D014103"^^xsd:string ;
    NIFRID:putativeClassExtension "Intermittent Torticollis"^^xsd:string,
        "Psychogenic Torticollis"^^xsd:string,
        "Spasmodic Torticollis"^^xsd:string ;
    NIFRID:usageNote "MeSH includes qualified subtypes"^^xsd:string .

BIRNLEX:12657 a owl:Class ;
    rdfs:label "Hyperkinesis"^^xsd:string ;
    skos:prefLabel "Hyperkinesis"^^xsd:string ;
    NIFRID:synonym "Generalized Hyperkinesia"^^xsd:string,
        "Hyperkinesia"^^xsd:string,
        "Hyperkinetic Movements"^^xsd:string,
        "Motor Hyperactivity"^^xsd:string ;
    skos:definition "Excessive movement of muscles of the body as a whole, which may be associated with organic or psychological disorders (MeSH)."^^xsd:string ;
    rdfs:subClassOf BIRNLEX:12638 ;
    NIFRID:createdDate "2007-10-05"^^xsd:string ;
    NIFRID:modifiedDate "2007-10-05"^^xsd:string ;
    NIFRID:hasBirnlexCurator NIFRID:Bill_Bug ;
    NIFRID:hasCurationStatus NIFRID:uncurated ;
    NIFRID:hasDefinitionSource NIFRID:MeSH_defSource ;
    NIFRID:hasExternalSource NIFRID:MeSH ;
    NIFRID:MeshUid "D006948"^^xsd:string ;
    skos:scopeNote "Do not confuse with MYOKYMIA or ISAACS SYNDROME"^^xsd:string .

BIRNLEX:12658 a owl:Class ;
    rdfs:label "Hypokinesia"^^xsd:string ;
    skos:prefLabel "Hypokinesia"^^xsd:string ;
    NIFRID:synonym "Bradykinesia"^^xsd:string,
        "Hypodynamia"^^xsd:string ;
    skos:definition "Slow or diminished movement of body musculature. It may be associated with BASAL GANGLIA DISEASES; MENTAL DISORDERS; prolonged inactivity due to illness; and other conditions (MeSH)."^^xsd:string ;
    rdfs:subClassOf BIRNLEX:12638 ;
    NIFRID:createdDate "2007-10-05"^^xsd:string ;
    NIFRID:modifiedDate "2007-10-05"^^xsd:string ;
    NIFRID:hasBirnlexCurator NIFRID:Bill_Bug ;
    NIFRID:hasCurationStatus NIFRID:uncurated ;
    NIFRID:hasDefinitionSource NIFRID:MeSH_defSource ;
    NIFRID:hasExternalSource NIFRID:MeSH ;
    NIFRID:MeshUid "D018476"^^xsd:string ;
    NIFRID:putativeClassExtension "Antiorthostatic Hypokinesia"^^xsd:string ;
    NIFRID:usageNote "MeSH includes qualified subtypes"^^xsd:string .

BIRNLEX:12659 a owl:Class ;
    rdfs:label "Myoclonus"^^xsd:string ;
    skos:prefLabel "Myoclonus"^^xsd:string ;
    NIFRID:synonym "Myoclonic Jerking"^^xsd:string ;
    skos:definition "Involuntary shock-like contractions, irregular in rhythm and amplitude, followed by relaxation, of a muscle or a group of muscles. This condition may be a feature of some CENTRAL NERVOUS SYSTEM DISEASES; (e.g., EPILEPSY, MYOCLONIC). Nocturnal myoclonus is the principal feature of the NOCTURNAL MYOCLONUS SYNDROME (MeSH)."^^xsd:string ;
    rdfs:subClassOf BIRNLEX:12638 ;
    NIFRID:createdDate "2007-10-05"^^xsd:string ;
    NIFRID:modifiedDate "2007-10-05"^^xsd:string ;
    NIFRID:hasBirnlexCurator NIFRID:Bill_Bug ;
    NIFRID:hasCurationStatus NIFRID:uncurated ;
    NIFRID:hasDefinitionSource NIFRID:MeSH_defSource ;
    NIFRID:hasExternalSource NIFRID:MeSH ;
    NIFRID:MeshUid "D009207"^^xsd:string ;
    NIFRID:putativeClassExtension "Action Myoclonus"^^xsd:string,
        "Eyelid Myoclonus"^^xsd:string,
        "Intention Myoclonus"^^xsd:string,
        "Lower Extremity Myoclonus"^^xsd:string,
        "Myoclonus Simplex"^^xsd:string,
        "Nocturnal Myoclonus"^^xsd:string,
        "Oculopalatal Myoclonus"^^xsd:string,
        "Palatal Myoclonus"^^xsd:string,
        "Polymyoclonus"^^xsd:string,
        "Segmental Myoclonus"^^xsd:string,
        "Sleep Myoclonus"^^xsd:string,
        "Upper Extremity Myoclonus"^^xsd:string ;
    NIFRID:usageNote "MeSH includes qualified subtypes"^^xsd:string ;
    skos:scopeNote "For \"myoclonic seizure\" consider MYOCLONUS or EPILEPSY, MYOCLONIC or SPASMS, INFANTILE; note other myoclonus terms are also available"^^xsd:string .

BIRNLEX:12660 a owl:Class ;
    rdfs:label "Opsoclonus-Myoclonus Syndrome"^^xsd:string ;
    skos:prefLabel "Opsoclonus-Myoclonus Syndrome"^^xsd:string ;
    NIFRID:synonym "Dancing Eyes-Dancing Feet Syndrome"^^xsd:string,
        "Kinsbourne Syndrome"^^xsd:string,
        "Opsoclonus Myoclonus Ataxia"^^xsd:string,
        "Paraneoplastic Opsoclonus-Myoclonus Ataxia"^^xsd:string ;
    skos:definition "A neurological condition that is characterized by uncontrolled rapid irregular movements of the eye ( OPSOCLONUS) and the muscle ( MYOCLONUS) causing unsteady, trembling gait. It is also known as dancing eyes-dancing feet syndrome and is often associated with neoplasms, viral infections, or autoimmune disorders involving the nervous system (MeSH)."^^xsd:string ;
    rdfs:subClassOf BIRNLEX:12638 ;
    NIFRID:createdDate "2007-10-05"^^xsd:string ;
    NIFRID:modifiedDate "2007-10-05"^^xsd:string ;
    NIFRID:definingCitationURI <http://www.ninds.nih.gov/disorders/opsoclonus_myoclonus/opsoclonus_myoclonus.htm> ;
    NIFRID:hasBirnlexCurator NIFRID:Bill_Bug ;
    NIFRID:hasCurationStatus NIFRID:uncurated ;
    NIFRID:hasDefinitionSource NIFRID:MeSH_defSource ;
    NIFRID:hasExternalSource NIFRID:MeSH ;
    NIFRID:MeshUid "D053578"^^xsd:string .

BIRNLEX:12661 a owl:Class ;
    rdfs:label "Psychomotor Agitation"^^xsd:string ;
    skos:prefLabel "Psychomotor Agitation"^^xsd:string ;
    NIFRID:synonym "Akathisia"^^xsd:string,
        "Psychomotor Excitement"^^xsd:string,
        "Psychomotor Hyperactivity"^^xsd:string,
        "Psychomotor Restlessness"^^xsd:string,
        "Restlessness"^^xsd:string ;
    skos:definition "A feeling of restlessness associated with increased motor activity. This may occur as a manifestation of nervous system drug toxicity or other conditions (MeSH)."^^xsd:string ;
    rdfs:subClassOf BIRNLEX:12638 ;
    NIFRID:createdDate "2007-10-05"^^xsd:string ;
    NIFRID:modifiedDate "2007-10-05"^^xsd:string ;
    NIFRID:hasBirnlexCurator NIFRID:Bill_Bug ;
    NIFRID:hasCurationStatus NIFRID:uncurated ;
    NIFRID:hasDefinitionSource NIFRID:MeSH_defSource ;
    NIFRID:hasExternalSource NIFRID:MeSH ;
    NIFRID:MeshUid "D011595"^^xsd:string ;
    skos:scopeNote "Do not confuse X ref AKATHISIA with AKATHISIA, DRUG-INDUCED: see note there"^^xsd:string .

BIRNLEX:12662 a owl:Class ;
    rdfs:label "Synkinesis"^^xsd:string ;
    skos:prefLabel "Synkinesis"^^xsd:string ;
    skos:definition "An involuntary movement accompanying a volitional movement. It often refers to facial movements that accompany FACIAL PARALYSIS (MeSH)."^^xsd:string ;
    rdfs:subClassOf BIRNLEX:12638 ;
    NIFRID:createdDate "2007-10-05"^^xsd:string ;
    NIFRID:modifiedDate "2007-10-05"^^xsd:string ;
    NIFRID:hasBirnlexCurator NIFRID:Bill_Bug ;
    NIFRID:hasCurationStatus NIFRID:uncurated ;
    NIFRID:hasDefinitionSource NIFRID:MeSH_defSource ;
    NIFRID:hasExternalSource NIFRID:MeSH ;
    NIFRID:MeshUid "D046608"^^xsd:string .

BIRNLEX:12663 a owl:Class ;
    rdfs:label "Tic"^^xsd:string ;
    skos:prefLabel "Tic"^^xsd:string ;
    NIFRID:synonym "Habit Chorea"^^xsd:string,
        "Habit Spasm"^^xsd:string,
        "Habituation Spasm"^^xsd:string ;
    skos:definition "Habitual, repeated, rapid contraction of certain muscles, resulting in stereotyped individualized actions that can be voluntarily suppressed for only brief periods. They often involve the face, vocal cords, neck, and less often the extremities. Examples include repetitive throat clearing, vocalizations, sniffing, pursing the lips, and excessive blinking. Tics tend to be aggravated by emotional stress. When frequent they may interfere with speech and INTERPERSONAL RELATIONS. Conditions which feature frequent and prominent tics as a primary manifestation of disease are referred to as TIC DISORDERS (MeSH)."^^xsd:string ;
    rdfs:subClassOf BIRNLEX:12638 ;
    NIFRID:createdDate "2007-10-05"^^xsd:string ;
    NIFRID:modifiedDate "2007-10-05"^^xsd:string ;
    NIFRID:definingCitation "Adams et al., Principles of Neurology, 6th ed, pp109-10"^^xsd:string ;
    NIFRID:hasBirnlexCurator NIFRID:Bill_Bug ;
    NIFRID:hasCurationStatus NIFRID:uncurated ;
    NIFRID:hasDefinitionSource NIFRID:MeSH_defSource ;
    NIFRID:hasExternalSource NIFRID:MeSH ;
    NIFRID:MeshUid "D020323"^^xsd:string ;
    NIFRID:putativeClassExtension "Motor Tic"^^xsd:string,
        "Transient Tic"^^xsd:string,
        "Vocal Tic"^^xsd:string ;
    NIFRID:usageNote "MeSH includes qualified subtypes"^^xsd:string .

BIRNLEX:12664 a owl:Class ;
    rdfs:label "Tremor"^^xsd:string ;
    skos:prefLabel "Tremor"^^xsd:string ;
    skos:definition "Cyclical movement of a body part that can represent either a physiologic process or a manifestation of disease. Intention or action tremor, a common manifestation of CEREBELLAR DISEASES, is aggravated by movement. In contrast, resting tremor is maximal when there is no attempt at voluntary movement, and occurs as a relatively frequent manifestation of PARKINSON DISEASE (MeSH)."^^xsd:string ;
    rdfs:subClassOf BIRNLEX:12638 ;
    NIFRID:createdDate "2007-10-05"^^xsd:string ;
    NIFRID:modifiedDate "2007-10-05"^^xsd:string ;
    NIFRID:hasBirnlexCurator NIFRID:Bill_Bug ;
    NIFRID:hasCurationStatus NIFRID:uncurated ;
    NIFRID:hasDefinitionSource NIFRID:MeSH_defSource ;
    NIFRID:hasExternalSource NIFRID:MeSH ;
    NIFRID:MeshUid "D014202"^^xsd:string ;
    NIFRID:putativeClassExtension "Action Tremor"^^xsd:string,
        "Coarse Tremor"^^xsd:string,
        "Continuous Tremor"^^xsd:string,
        "Darkness Tremor"^^xsd:string,
        "Fine Tremor"^^xsd:string,
        "Intention Tremor"^^xsd:string,
        "Intermittent Tremor"^^xsd:string,
        "Involuntary Quiver"^^xsd:string,
        "Limb Tremor"^^xsd:string,
        "Massive Tremor"^^xsd:string,
        "Muscle Tremor"^^xsd:string,
        "Neonatal Tremor"^^xsd:string,
        "Nerve Tremor"^^xsd:string,
        "Passive Tremor"^^xsd:string,
        "Perioral Tremor"^^xsd:string,
        "Persistent Tremor"^^xsd:string,
        "Pill Rolling Tremor"^^xsd:string,
        "Rest Tremor"^^xsd:string,
        "Resting Tremor"^^xsd:string,
        "Saturnine Tremor"^^xsd:string,
        "Semirhythmic Tremor"^^xsd:string,
        "Senile Tremor"^^xsd:string,
        "Static Tremor"^^xsd:string ;
    NIFRID:usageNote "MeSH includes qualified subtypes"^^xsd:string .

BIRNLEX:12665 a owl:Class ;
    rdfs:label "Nervous System Trauma"^^xsd:string ;
    skos:prefLabel "Nervous System Trauma"^^xsd:string ;
    NIFRID:synonym "Craniocervical Injury"^^xsd:string,
        "Nervous System Injury"^^xsd:string ;
    skos:definition "Traumatic injuries to the brain, cranial nerves, spinal cord, autonomic nervous system, or neuromuscular system, including iatrogenic injuries induced by surgical procedures (MeSH)."^^xsd:string ;
    rdfs:subClassOf BIRNLEX:12796 ;
    skos:editorialNote "Note BIRNLex seeks to evolve a core subsumptive disease hierarchy based first on the effected function, then the effected structure, the latter for those categories of nervous system disease that have typically been associated with structural abnormalities or trauma (e.g., Motor neuron diseases, cerebrovascular trauma, etc.). Disease causation is in fact the ultimate goal of much biomedical research, and our recognitition of ALL the driving causes of a particular disease - and the ways in which these causes inter-relate with each other and with effected structures to cause a change in normal function is a critical representational task BIRNlex will increasingly take on to provide an evolving, nuanced functional reconstruction of disease as a process and an outcome.  These relations will be represented using OWL ObjectProperties.  Function is the most sensible context to drive the asserted subsumptive hierarchy for representing nervous system disease, since it is with the clinical description of altered, impaired, decreased, or lost function that the diagnosis - and the research - of disease is rooted.  Much has already been described regarding both the effected biomaterial entities and the causes of disease.  However, it is because understanding of such relations still is far from comprehensive, that biomedical investigation into nervous system disease continues.  Finally, given the \"realist\" ontology design approach being used to construct BIRNLex, function must be represented as inhering in some biomaterial entity from molecules and their controlling elements on up through gross anatomical structures.  Over time, BIRNLex will provide the required relations to depict these functionally-related structures for both the normal and pathological function of the nervous system.  This will be true both for the causes and for the outcomes of nervous system disease.  Initial work to extend this expressive representation will focus on the neurodegenerative diseases being studied by BIRN researchers.  Though this will be te case, BIRNLex still needs to provide a core asserted hierarchy for a broad swarth of nervous system disease, so as to enable BIRN researchers to link to the breadth of disorders that may impact or relate to those directly under study."^^xsd:string ;
    NIFRID:createdDate "2007-10-05"^^xsd:string ;
    NIFRID:modifiedDate "2007-11-18"^^xsd:string ;
    NIFRID:hasBirnlexCurator NIFRID:Bill_Bug ;
    NIFRID:hasCurationStatus NIFRID:uncurated ;
    NIFRID:hasDefinitionSource NIFRID:MeSH_defSource ;
    NIFRID:hasExternalSource NIFRID:MeSH ;
    NIFRID:MeshUid "D020196"^^xsd:string ;
    NIFRID:nifID "_8.3_12"^^xsd:string .

BIRNLEX:12666 a owl:Class ;
    rdfs:label "Cerebrovascular Trauma"^^xsd:string ;
    skos:prefLabel "Cerebrovascular Trauma"^^xsd:string ;
    NIFRID:synonym "Vascular Brain Injury"^^xsd:string,
        "Vascular Brain Trauma"^^xsd:string ;
    skos:definition "Penetrating and nonpenetrating traumatic injuries to an extracranial or intracranial blood vessel that supplies the brain. This includes the CAROTID ARTERIES, vertebral arteries ( VERTEBRAL ARTERY), and intracranial arteries, veins, and venous sinuses (MeSH)."^^xsd:string ;
    rdfs:subClassOf BIRNLEX:12665 ;
    NIFRID:createdDate "2007-10-05"^^xsd:string ;
    NIFRID:modifiedDate "2007-10-05"^^xsd:string ;
    NIFRID:hasBirnlexCurator NIFRID:Bill_Bug ;
    NIFRID:hasCurationStatus NIFRID:uncurated ;
    NIFRID:hasDefinitionSource NIFRID:MeSH_defSource ;
    NIFRID:hasExternalSource NIFRID:MeSH ;
    NIFRID:MeshUid "D020214"^^xsd:string .

BIRNLEX:12667 a owl:Class ;
    rdfs:label "Craniocerebral Trauma"^^xsd:string ;
    skos:prefLabel "Craniocerebral Trauma"^^xsd:string ;
    NIFRID:synonym "Craniocerebral Injury"^^xsd:string,
        "Head Injury"^^xsd:string,
        "Head Trauma"^^xsd:string ;
    skos:definition "Traumatic injuries involving the cranium and intracranial structures (i.e., BRAIN; CRANIAL NERVES; MENINGES; and other structures). Injuries may be classified by whether or not the skull is penetrated (i.e., penetrating vs. nonpenetrating) or whether there is an associated hemorrhage (MeSH)."^^xsd:string ;
    rdfs:subClassOf BIRNLEX:12665 ;
    NIFRID:createdDate "2007-10-05"^^xsd:string ;
    NIFRID:modifiedDate "2007-10-05"^^xsd:string ;
    NIFRID:hasBirnlexCurator NIFRID:Bill_Bug ;
    NIFRID:hasCurationStatus NIFRID:uncurated ;
    NIFRID:hasDefinitionSource NIFRID:MeSH_defSource ;
    NIFRID:hasExternalSource NIFRID:MeSH ;
    NIFRID:MeshUid "D006259"^^xsd:string ;
    NIFRID:putativeClassExtension "Crushing Skull Injury"^^xsd:string,
        "Forehead Trauma"^^xsd:string,
        "Frontal Region Trauma"^^xsd:string,
        "Minor Head Injury"^^xsd:string,
        "Multiple Head Injury"^^xsd:string,
        "Occipital Region Trauma"^^xsd:string,
        "Open Head Injury"^^xsd:string,
        "Parietal Region Trauma"^^xsd:string,
        "Superficial Head Injury"^^xsd:string,
        "Temporal Region Trauma"^^xsd:string ;
    NIFRID:usageNote "MeSH includes qualified subtypes based on the severity, invasiveness, or gross anatomical location of the head injury"^^xsd:string .

BIRNLEX:12668 a owl:Class ;
    rdfs:label "Spinal Cord Trauma"^^xsd:string ;
    skos:prefLabel "Spinal Cord Trauma"^^xsd:string ;
    NIFRID:synonym "Spinal Cord Injury"^^xsd:string ;
    skos:definition "Penetrating and non-penetrating injuries to the spinal cord resulting from traumatic external forces (e.g., WOUNDS, GUNSHOT; WHIPLASH INJURIES; etc.) (MeSH)."^^xsd:string ;
    rdfs:subClassOf BIRNLEX:12665 ;
    NIFRID:createdDate "2007-10-05"^^xsd:string ;
    NIFRID:modifiedDate "2007-10-05"^^xsd:string ;
    NIFRID:hasBirnlexCurator NIFRID:Bill_Bug ;
    NIFRID:hasCurationStatus NIFRID:uncurated ;
    NIFRID:hasDefinitionSource NIFRID:MeSH_defSource ;
    NIFRID:hasExternalSource NIFRID:MeSH ;
    NIFRID:MeshUid "D013119"^^xsd:string ;
    NIFRID:putativeClassExtension "Post-Traumatic Myelopathy"^^xsd:string,
        "Spinal Cord Contusion"^^xsd:string,
        "Spinal Cord Laceration"^^xsd:string,
        "Spinal Cord Transection"^^xsd:string,
        "Traumatic Myelopathy"^^xsd:string ;
    NIFRID:usageNote "MeSH includes qualified subtypes based on the severity or invasiveness of the spinal cord injury"^^xsd:string .

BIRNLEX:12669 a owl:Class ;
    rdfs:label "Mental Disorder"^^xsd:string ;
    skos:prefLabel "Mental Disorder"^^xsd:string ;
    NIFRID:synonym "Behavior Disorder"^^xsd:string,
        "Psychiatric Disorder"^^xsd:string ;
    skos:definition "Psychiatric illness or diseases manifested by breakdowns in the adaptational process expressed primarily as abnormalities of thought, feeling, and behavior producing either distress or impairment of function (MeSH)."^^xsd:string ;
    rdfs:subClassOf BIRNLEX:12796 ;
    skos:editorialNote "Note BIRNLex seeks to evolve a core subsumptive disease hierarchy based first on the effected function, then the effected structure, the latter for those categories of nervous system disease that have typically been associated with structural abnormalities or trauma (e.g., Motor neuron diseases, cerebrovascular trauma, etc.). Disease causation is in fact the ultimate goal of much biomedical research, and our recognitition of ALL the driving causes of a particular disease - and the ways in which these causes inter-relate with each other and with effected structures to cause a change in normal function is a critical representational task BIRNlex will increasingly take on to provide an evolving, nuanced functional reconstruction of disease as a process and an outcome.  These relations will be represented using OWL ObjectProperties.  Function is the most sensible context to drive the asserted subsumptive hierarchy for representing nervous system disease, since it is with the clinical description of altered, impaired, decreased, or lost function that the diagnosis - and the research - of disease is rooted.  Much has already been described regarding both the effected biomaterial entities and the causes of disease.  However, it is because understanding of such relations still is far from comprehensive, that biomedical investigation into nervous system disease continues.  Finally, given the \"realist\" ontology design approach being used to construct BIRNLex, function must be represented as inhering in some biomaterial entity from molecules and their controlling elements on up through gross anatomical structures.  Over time, BIRNLex will provide the required relations to depict these functionally-related structures for both the normal and pathological function of the nervous system.  This will be true both for the causes and for the outcomes of nervous system disease.  Initial work to extend this expressive representation will focus on the neurodegenerative diseases being studied by BIRN researchers.  Though this will be te case, BIRNLex still needs to provide a core asserted hierarchy for a broad swarth of nervous system disease, so as to enable BIRN researchers to link to the breadth of disorders that may impact or relate to those directly under study."^^xsd:string ;
    NIFRID:createdDate "2007-10-05"^^xsd:string ;
    NIFRID:modifiedDate "2007-11-18"^^xsd:string ;
    NIFRID:hasBirnlexCurator NIFRID:Bill_Bug ;
    NIFRID:hasCurationStatus NIFRID:uncurated ;
    NIFRID:hasDefinitionSource NIFRID:MeSH_defSource ;
    NIFRID:hasExternalSource NIFRID:MeSH ;
    NIFRID:MeshUid "D001523"^^xsd:string ;
    NIFRID:nifID "_8.3_11"^^xsd:string .

BIRNLEX:12670 a owl:Class ;
    rdfs:label "Adjustment Disorder"^^xsd:string ;
    skos:prefLabel "Adjustment Disorder"^^xsd:string ;
    NIFRID:synonym "Anniversary Reaction"^^xsd:string,
        "Reactive Depression"^^xsd:string,
        "Reactive Disorder"^^xsd:string,
        "Transient Situational Disturbance"^^xsd:string ;
    skos:definition "Maladaptive reactions to identifiable psychosocial stressors occurring within a short time after onset of the stressor. They are manifested by either impairment in social or occupational functioning or by symptoms (depression, anxiety, etc.) that are in excess of a normal and expected reaction to the stressor (MeSH)."^^xsd:string ;
    rdfs:subClassOf BIRNLEX:12669 ;
    NIFRID:createdDate "2007-10-05"^^xsd:string ;
    NIFRID:modifiedDate "2007-10-05"^^xsd:string ;
    NIFRID:hasBirnlexCurator NIFRID:Bill_Bug ;
    NIFRID:hasCurationStatus NIFRID:uncurated ;
    NIFRID:hasDefinitionSource NIFRID:MeSH_defSource ;
    NIFRID:hasExternalSource NIFRID:MeSH ;
    NIFRID:MeshUid "D000275"^^xsd:string .

BIRNLEX:12671 a owl:Class ;
    rdfs:label "Anxiety Disorder"^^xsd:string ;
    skos:prefLabel "Anxiety Disorder"^^xsd:string ;
    NIFRID:synonym "Anxiety Neurosis"^^xsd:string,
        "Neurotic Anxiety State"^^xsd:string ;
    skos:definition "Persistent and disabling ANXIETY (MeSH)."^^xsd:string ;
    rdfs:subClassOf BIRNLEX:12669 ;
    NIFRID:createdDate "2007-10-05"^^xsd:string ;
    NIFRID:modifiedDate "2007-10-05"^^xsd:string ;
    NIFRID:hasBirnlexCurator NIFRID:Bill_Bug ;
    NIFRID:hasCurationStatus NIFRID:uncurated ;
    NIFRID:hasDefinitionSource NIFRID:MeSH_defSource ;
    NIFRID:hasExternalSource NIFRID:MeSH ;
    NIFRID:MeshUid "D001008"^^xsd:string ;
    NIFRID:nifID "_8.3_11.4"^^xsd:string .

BIRNLEX:12672 a owl:Class ;
    rdfs:label "Agoraphobia"^^xsd:string ;
    skos:prefLabel "Agoraphobia"^^xsd:string ;
    skos:definition "Obsessive, persistent, intense fear of open places (MeSH)."^^xsd:string ;
    rdfs:subClassOf BIRNLEX:12671 ;
    NIFRID:createdDate "2007-10-05"^^xsd:string ;
    NIFRID:modifiedDate "2007-10-05"^^xsd:string ;
    NIFRID:hasBirnlexCurator NIFRID:Bill_Bug ;
    NIFRID:hasCurationStatus NIFRID:uncurated ;
    NIFRID:hasDefinitionSource NIFRID:MeSH_defSource ;
    NIFRID:hasExternalSource NIFRID:MeSH ;
    NIFRID:MeshUid "D000379"^^xsd:string .

BIRNLEX:12673 a owl:Class ;
    rdfs:label "Neurocirculatory Asthenia"^^xsd:string ;
    skos:prefLabel "Neurocirculatory Asthenia"^^xsd:string ;
    NIFRID:synonym "Cardiac Neurosis"^^xsd:string,
        "Effort Syndrome"^^xsd:string,
        "Hyperkinetic Heart Syndrome"^^xsd:string ;
    skos:definition "A clinical syndrome characterized by palpitation, SHORTNESS OF BREATH, labored breathing, subjective complaints of effort and discomfort, all following slight EXERTION. Other symptoms may be DIZZINESS, tremulousness, SWEATING, and INSOMNIA. Neurocirculatory asthenia is most typically seen as a form of anxiety disorder (MeSH)."^^xsd:string ;
    rdfs:subClassOf BIRNLEX:12671 ;
    NIFRID:createdDate "2007-10-05"^^xsd:string ;
    NIFRID:modifiedDate "2007-10-05"^^xsd:string ;
    NIFRID:hasBirnlexCurator NIFRID:Bill_Bug ;
    NIFRID:hasCurationStatus NIFRID:uncurated ;
    NIFRID:hasDefinitionSource NIFRID:MeSH_defSource ;
    NIFRID:hasExternalSource NIFRID:MeSH ;
    NIFRID:MeshUid "D009449"^^xsd:string .

BIRNLEX:12674 a owl:Class ;
    rdfs:label "Obsessive-Compulsive Disorder"^^xsd:string ;
    skos:prefLabel "Obsessive-Compulsive Disorder"^^xsd:string ;
    NIFRID:synonym "Obsessive-Compulsive Neurosis"^^xsd:string ;
    skos:definition "An anxiety disorder characterized by recurrent, persistent obsessions or compulsions. Obsessions are the intrusive ideas, thoughts, or images that are experienced as senseless or repugnant. Compulsions are repetitive and seemingly purposeful behavior which the individual generally recognizes as senseless and from which the individual does not derive pleasure although it may provide a release from tension (MeSH)."^^xsd:string ;
    rdfs:subClassOf BIRNLEX:12671 ;
    NIFRID:createdDate "2007-10-05"^^xsd:string ;
    NIFRID:modifiedDate "2007-10-05"^^xsd:string ;
    NIFRID:hasBirnlexCurator NIFRID:Bill_Bug ;
    NIFRID:hasCurationStatus NIFRID:uncurated ;
    NIFRID:hasDefinitionSource NIFRID:MeSH_defSource ;
    NIFRID:hasExternalSource NIFRID:MeSH ;
    NIFRID:MeshUid "D009771"^^xsd:string .

BIRNLEX:12675 a owl:Class ;
    rdfs:label "Phobic Disorder"^^xsd:string ;
    skos:prefLabel "Phobic Disorder"^^xsd:string ;
    NIFRID:synonym "Phobia"^^xsd:string,
        "Phobic Neurosis"^^xsd:string ;
    skos:definition "Anxiety disorders in which the essential feature is persistent and irrational fear of a specific object, activity, or situation that the individual feels compelled to avoid. The individual recognizes the fear as excessive or unreasonable (MeSH)."^^xsd:string ;
    rdfs:subClassOf BIRNLEX:12671 ;
    NIFRID:createdDate "2007-10-05"^^xsd:string ;
    NIFRID:modifiedDate "2007-10-05"^^xsd:string ;
    NIFRID:hasBirnlexCurator NIFRID:Bill_Bug ;
    NIFRID:hasCurationStatus NIFRID:uncurated ;
    NIFRID:hasDefinitionSource NIFRID:MeSH_defSource ;
    NIFRID:hasExternalSource NIFRID:MeSH ;
    NIFRID:MeshUid "D010698"^^xsd:string ;
    NIFRID:putativeClassExtension "Claustrophobia"^^xsd:string,
        "School Phobia"^^xsd:string,
        "Social Phobia"^^xsd:string ;
    NIFRID:usageNote "MeSH includes the following qualified subtypes based on the type of object or experience inducing the fear reaction: ; ; "^^xsd:string .

BIRNLEX:12676 a owl:Class ;
    rdfs:label "Panic Disorder"^^xsd:string ;
    skos:prefLabel "Panic Disorder"^^xsd:string ;
    NIFRID:synonym "Panic Attack"^^xsd:string ;
    skos:definition "A type of anxiety disorder characterized by unexpected panic attacks that last minutes or, rarely, hours. Panic attacks begin with intense apprehension, fear or terror and, often, a feeling of impending doom. Symptoms experienced during a panic attack include dyspnea or sensations of being smothered; dizziness, loss of balance or faintness; choking sensations; palpitations or accelerated heart rate; shakiness; sweating; nausea or other form of abdominal distress; depersonalization or derealization; paresthesias; hot flashes or chills; chest discomfort or pain; fear of dying and fear of not being in control of oneself or going crazy. Agoraphobia may also develop. Similar to other anxiety disorders, it may be inherited as an autosomal dominant trait (MeSH)."^^xsd:string ;
    rdfs:subClassOf BIRNLEX:12671 ;
    NIFRID:createdDate "2007-10-05"^^xsd:string ;
    NIFRID:modifiedDate "2007-10-05"^^xsd:string ;
    NIFRID:hasBirnlexCurator NIFRID:Bill_Bug ;
    NIFRID:hasCurationStatus NIFRID:uncurated ;
    NIFRID:hasDefinitionSource NIFRID:MeSH_defSource ;
    NIFRID:hasExternalSource NIFRID:MeSH ;
    NIFRID:MeshUid "D016584"^^xsd:string .

BIRNLEX:12677 a owl:Class ;
    rdfs:label "Traumatic Stress Disorder"^^xsd:string ;
    skos:prefLabel "Traumatic Stress Disorder"^^xsd:string ;
    NIFRID:synonym "Stress Disorder"^^xsd:string ;
    skos:definition "Anxiety disorders manifested by the development of characteristic symptoms following a psychologically traumatic event that is outside the normal range of usual human experience. Symptoms include re-experiencing the traumatic event, increased arousal, and numbing of responsiveness to or reduced involvement with the external world. Traumatic stress disorders can be further classified by the time of onset and the duration of these symptoms (MeSH)."^^xsd:string ;
    rdfs:subClassOf BIRNLEX:12671 ;
    NIFRID:createdDate "2007-10-05"^^xsd:string ;
    NIFRID:modifiedDate "2007-10-05"^^xsd:string ;
    NIFRID:hasBirnlexCurator NIFRID:Bill_Bug ;
    NIFRID:hasCurationStatus NIFRID:uncurated ;
    NIFRID:hasDefinitionSource NIFRID:MeSH_defSource ;
    NIFRID:hasExternalSource NIFRID:MeSH ;
    NIFRID:MeshUid "D040921"^^xsd:string .

BIRNLEX:12678 a owl:Class ;
    rdfs:label "Combat Disorder"^^xsd:string ;
    skos:prefLabel "Combat Disorder"^^xsd:string ;
    NIFRID:synonym "Combat Neurosis"^^xsd:string,
        "War Neurosis"^^xsd:string ;
    skos:definition "Neurotic reactions to unusual, severe, or overwhelming military stress (MeSH)."^^xsd:string ;
    rdfs:subClassOf BIRNLEX:12677 ;
    NIFRID:createdDate "2007-10-05"^^xsd:string ;
    NIFRID:modifiedDate "2007-10-05"^^xsd:string ;
    NIFRID:hasBirnlexCurator NIFRID:Bill_Bug ;
    NIFRID:hasCurationStatus NIFRID:uncurated ;
    NIFRID:hasDefinitionSource NIFRID:MeSH_defSource ;
    NIFRID:hasExternalSource NIFRID:MeSH ;
    NIFRID:MeshUid "D003130"^^xsd:string .

BIRNLEX:12679 a owl:Class ;
    rdfs:label "Post-Traumatic Stress Disorder"^^xsd:string ;
    skos:prefLabel "Post-Traumatic Stress Disorder"^^xsd:string ;
    NIFRID:synonym "Post-Traumatic Neurosis"^^xsd:string ;
    skos:definition "A class of traumatic stress disorders with symptoms that last more than one month. There are various forms of post-traumatic stress disorder, depending on the time of onset and the duration of these stress symptoms. In the acute form, the duration of the symptoms is between 1 to 3 months. In the chronic form, symptoms last more than 3 months. With delayed onset, symptoms develop more than 6 months after the traumatic event (MeSH)."^^xsd:string ;
    rdfs:subClassOf BIRNLEX:12677 ;
    NIFRID:createdDate "2007-10-05"^^xsd:string ;
    NIFRID:modifiedDate "2007-10-05"^^xsd:string ;
    NIFRID:acronym "PTSD"^^xsd:string ;
    NIFRID:hasBirnlexCurator NIFRID:Bill_Bug ;
    NIFRID:hasCurationStatus NIFRID:uncurated ;
    NIFRID:hasDefinitionSource NIFRID:MeSH_defSource ;
    NIFRID:hasExternalSource NIFRID:MeSH ;
    NIFRID:MeshUid "D013313"^^xsd:string ;
    NIFRID:putativeClassExtension "Acute Post-Traumatic Stress Disorder"^^xsd:string,
        "Chronic Post-Traumatic Stress Disorder"^^xsd:string,
        "Delayed Onset Post-Traumatic Stress Disorder"^^xsd:string ;
    NIFRID:usageNote "MeSH includes qualified subtypes based on the time of onset or temporal extent of the stress reaction"^^xsd:string .

BIRNLEX:12680 a owl:Class ;
    rdfs:label "Acute Traumatic Stress Disorder"^^xsd:string ;
    skos:prefLabel "Acute Traumatic Stress Disorder"^^xsd:string ;
    NIFRID:synonym "Acute Stress Disorder"^^xsd:string ;
    skos:definition "A class of traumatic stress disorders that is characterized by the significant dissociative states seen immediately after overwhelming trauma. By definition it cannot last longer than 1 month, if it persists, a diagnosis of post-traumatic stress disorder ( STRESS DISORDERS, POST-TRAUMATIC) is more appropriate (MeSH)."^^xsd:string ;
    rdfs:subClassOf BIRNLEX:12677 ;
    NIFRID:createdDate "2007-10-05"^^xsd:string ;
    NIFRID:modifiedDate "2007-10-05"^^xsd:string ;
    NIFRID:hasBirnlexCurator NIFRID:Bill_Bug ;
    NIFRID:hasCurationStatus NIFRID:uncurated ;
    NIFRID:hasDefinitionSource NIFRID:MeSH_defSource ;
    NIFRID:hasExternalSource NIFRID:MeSH ;
    NIFRID:MeshUid "D040701"^^xsd:string .

BIRNLEX:12681 a owl:Class ;
    rdfs:label "Central Nervous System Infection"^^xsd:string ;
    skos:prefLabel "Central Nervous System Infection"^^xsd:string ;
    skos:definition "Pathogenic infections of the brain, spinal cord, and meninges. DNA VIRUS INFECTIONS; RNA VIRUS INFECTIONS; BACTERIAL INFECTIONS; MYCOPLASMA INFECTIONS; SPIROCHAETALES INFECTIONS; fungal infections; PROTOZOAN INFECTIONS; HELMINTHIASIS; and PRION DISEASES may involve the central nervous system as a primary or secondary process (MeSH)."^^xsd:string ;
    rdfs:subClassOf BIRNLEX:12796 ;
    NIFRID:createdDate "2007-10-05"^^xsd:string ;
    NIFRID:modifiedDate "2007-11-18"^^xsd:string ;
    NIFRID:hasBirnlexCurator NIFRID:Bill_Bug ;
    NIFRID:hasCurationStatus NIFRID:uncurated ;
    NIFRID:hasDefinitionSource NIFRID:MeSH_defSource ;
    NIFRID:hasExternalSource NIFRID:MeSH ;
    NIFRID:MeshUid "D002494"^^xsd:string ;
    NIFRID:nifID "_8.3_6"^^xsd:string .

BIRNLEX:12682 a owl:Class ;
    rdfs:label "Central Nervous System Bacterial Infection"^^xsd:string ;
    skos:prefLabel "Central Nervous System Bacterial Infection"^^xsd:string ;
    skos:definition "Bacterial infections of the brain, spinal cord, and meninges, including infections involving the perimeningeal spaces (MeSH)."^^xsd:string ;
    rdfs:subClassOf BIRNLEX:12681 ;
    NIFRID:createdDate "2007-10-05"^^xsd:string ;
    NIFRID:modifiedDate "2007-10-05"^^xsd:string ;
    NIFRID:hasBirnlexCurator NIFRID:Bill_Bug ;
    NIFRID:hasCurationStatus NIFRID:uncurated ;
    NIFRID:hasDefinitionSource NIFRID:MeSH_defSource ;
    NIFRID:hasExternalSource NIFRID:MeSH ;
    NIFRID:MeshUid "D020806"^^xsd:string ;
    NIFRID:nifID "_8.3_6.1"^^xsd:string .

BIRNLEX:12683 a owl:Class ;
    rdfs:label "Central Nervous System Fungal Infection"^^xsd:string ;
    skos:prefLabel "Central Nervous System Fungal Infection"^^xsd:string ;
    NIFRID:synonym "Acute Stress Disorder"^^xsd:string,
        "Central Nervous System Mycosis"^^xsd:string ;
    skos:definition "MYCOSES of the brain, spinal cord, and meninges which may result in ENCEPHALITIS; MENINGITIS, FUNGAL; MYELITIS; BRAIN ABSCESS; and EPIDURAL ABSCESS. Certain types of fungi may produce disease in immunologically normal hosts, while others are classified as opportunistic pathogens, causing illness primarily in immunocompromised individuals (e.g., ACQUIRED IMMUNODEFICIENCY SYNDROME) (MeSH)."^^xsd:string ;
    rdfs:subClassOf BIRNLEX:12681 ;
    NIFRID:createdDate "2007-10-05"^^xsd:string ;
    NIFRID:modifiedDate "2007-10-05"^^xsd:string ;
    NIFRID:hasBirnlexCurator NIFRID:Bill_Bug ;
    NIFRID:hasCurationStatus NIFRID:uncurated ;
    NIFRID:hasDefinitionSource NIFRID:MeSH_defSource ;
    NIFRID:hasExternalSource NIFRID:MeSH ;
    NIFRID:MeshUid "D020314"^^xsd:string .

BIRNLEX:12684 a owl:Class ;
    rdfs:label "Central Nervous System Parasitic Infection"^^xsd:string ;
    skos:prefLabel "Central Nervous System Parasitic Infection"^^xsd:string ;
    skos:definition "Infections of the brain, spinal cord, and meninges caused by parasites, primarily PROTOZOA and HELMINTHS (MeSH)."^^xsd:string ;
    rdfs:subClassOf BIRNLEX:12681 ;
    NIFRID:createdDate "2007-10-05"^^xsd:string ;
    NIFRID:modifiedDate "2007-10-05"^^xsd:string ;
    NIFRID:hasBirnlexCurator NIFRID:Bill_Bug ;
    NIFRID:hasCurationStatus NIFRID:uncurated ;
    NIFRID:hasDefinitionSource NIFRID:MeSH_defSource ;
    NIFRID:hasExternalSource NIFRID:MeSH ;
    NIFRID:MeshUid "D020807"^^xsd:string .

BIRNLEX:12685 a owl:Class ;
    rdfs:label "Central Nervous System Viral Infection"^^xsd:string ;
    skos:prefLabel "Central Nervous System Viral Infection"^^xsd:string ;
    NIFRID:synonym "Viral CNS Infection"^^xsd:string ;
    skos:definition "Viral infections of the brain, spinal cord, meninges, or perimeningeal spaces (MeSH)."^^xsd:string ;
    rdfs:subClassOf BIRNLEX:12681 ;
    NIFRID:createdDate "2007-10-05"^^xsd:string ;
    NIFRID:modifiedDate "2007-10-05"^^xsd:string ;
    NIFRID:hasBirnlexCurator NIFRID:Bill_Bug ;
    NIFRID:hasCurationStatus NIFRID:uncurated ;
    NIFRID:hasDefinitionSource NIFRID:MeSH_defSource ;
    NIFRID:hasExternalSource NIFRID:MeSH ;
    NIFRID:MeshUid "D020805"^^xsd:string ;
    NIFRID:nifID "_8.3_6.2"^^xsd:string .

BIRNLEX:12686 a owl:Class ;
    rdfs:label "Prion Disease"^^xsd:string ;
    skos:prefLabel "Prion Disease"^^xsd:string ;
    NIFRID:synonym "Prion Protein Disease"^^xsd:string,
        "Prion-Induced Disorder"^^xsd:string,
        "Transmissible Dementia"^^xsd:string,
        "Transmissible Spongiform Encephalopathy"^^xsd:string ;
    skos:definition "A group of genetic, infectious, or sporadic degenerative human and animal nervous system disorders associated with abnormal PRIONS. These diseases are characterized by conversion of the normal prion protein to an abnormal configuration via a post-translational process. In humans, these conditions generally feature DEMENTIA; ATAXIA; and a fatal outcome. Pathologic features include a spongiform encephalopathy without evidence of inflammation. The older literature occasionally refers to these as unconventional SLOW VIRUS DISEASES (MeSH)."^^xsd:string ;
    rdfs:subClassOf BIRNLEX:2086 ;
    NIFRID:createdDate "2007-10-05"^^xsd:string ;
    NIFRID:modifiedDate "2007-10-05"^^xsd:string ;
    NIFRID:definingCitation "Proc Natl Acad Sci USA 1998 Nov 10;95(23):13363-83"^^xsd:string ;
    NIFRID:hasBirnlexCurator NIFRID:Bill_Bug ;
    NIFRID:hasCurationStatus NIFRID:uncurated ;
    NIFRID:hasDefinitionSource NIFRID:MeSH_defSource ;
    NIFRID:hasExternalSource NIFRID:MeSH ;
    NIFRID:MeshUid "D017096"^^xsd:string ;
    NIFRID:nifID "_8.3_2.8"^^xsd:string ;
    NIFRID:putativeClassExtension "Inherited Human Transmissible Spongiform Encephalopathy"^^xsd:string ;
    NIFRID:usageNote "MeSH includes qualified subtype limiting to humans"^^xsd:string .

BIRNLEX:12687 a owl:Class ;
    rdfs:label "Creutzfeldt-Jakob Syndrome"^^xsd:string ;
    skos:prefLabel "Creutzfeldt-Jakob Syndrome"^^xsd:string ;
    NIFRID:synonym "Creutzfeldt-Jakob Disease"^^xsd:string,
        "Jakob Creutzfeldt Disease"^^xsd:string,
        "Jakob-Creutzfeldt Disease"^^xsd:string,
        "Jakob-Creutzfeldt Syndrome"^^xsd:string ;
    skos:definition "A rare transmissible encephalopathy most prevalent between the ages of 50 and 70 years. Affected individuals may present with sleep disturbances, personality changes, ATAXIA; APHASIA, visual loss, weakness, muscle atrophy, MYOCLONUS, progressive dementia, and death within one year of disease onset. A familial form exhibiting autosomal dominant inheritance and a new variant CJD (potentially associated with ENCEPHALOPATHY, BOVINE SPONGIFORM) have been described. Pathological features include prominent cerebellar and cerebral cortical spongiform degeneration and the presence of PRIONS (MeSH)."^^xsd:string ;
    rdfs:subClassOf BIRNLEX:12686 ;
    NIFRID:createdDate "2007-10-05"^^xsd:string ;
    NIFRID:modifiedDate "April 11, 2009"^^xsd:string ;
    NIFRID:acronym "CJD"^^xsd:string ;
    NIFRID:definingCitation "N Engl J Med, 1998 Dec 31;339(27)"^^xsd:string ;
    NIFRID:hasBirnlexCurator NIFRID:Bill_Bug ;
    NIFRID:hasCurationStatus NIFRID:uncurated ;
    NIFRID:hasDefinitionSource NIFRID:MeSH_defSource ;
    NIFRID:hasExternalSource NIFRID:MeSH ;
    NIFRID:MeshUid "D007562"^^xsd:string ;
    NIFRID:nifID "_8.3_2.8.1"^^xsd:string .

BIRNLEX:12688 a owl:Class ;
    rdfs:label "Familial Creutzfeldt-Jakob Disease"^^xsd:string ;
    skos:prefLabel "Familial Creutzfeldt-Jakob Disease"^^xsd:string ;
    skos:definition "A familial form exhibiting autosomal dominant inheritance has been described. Pathological features include prominent cerebellar and cerebral cortical spongiform degeneration and the presence of PRIONS (MeSH)."^^xsd:string ;
    rdfs:subClassOf BIRNLEX:12687 ;
    NIFRID:createdDate "2007-10-05"^^xsd:string ;
    NIFRID:modifiedDate "2007-10-05"^^xsd:string ;
    NIFRID:definingCitation "N Engl J Med, 1998 Dec 31;339(27)"^^xsd:string ;
    NIFRID:hasBirnlexCurator NIFRID:Bill_Bug ;
    NIFRID:hasCurationStatus NIFRID:uncurated ;
    NIFRID:hasDefinitionSource NIFRID:MeSH_defSource ;
    NIFRID:hasExternalSource NIFRID:MeSH ;
    NIFRID:MeshUid "D007562"^^xsd:string .

BIRNLEX:12689 a owl:Class ;
    rdfs:label "Variant-Creutzfeldt-Jakob Disease"^^xsd:string ;
    skos:prefLabel "Variant-Creutzfeldt-Jakob Disease"^^xsd:string ;
    NIFRID:synonym "CJD Variant"^^xsd:string,
        "New Variant Creutzfeldt-Jakob Disease"^^xsd:string,
        "Variant Creutzfeldt-Jakob Disease"^^xsd:string,
        "Variant-Creutzfeldt-Jakob's Disease"^^xsd:string ;
    skos:definition "A new variant CJD (potentially associated with ENCEPHALOPATHY, BOVINE SPONGIFORM) has been described. Pathological features include prominent cerebellar and cerebral cortical spongiform degeneration and the presence of PRIONS (MeSH)."^^xsd:string ;
    rdfs:subClassOf BIRNLEX:12687 ;
    NIFRID:createdDate "2007-10-05"^^xsd:string ;
    NIFRID:modifiedDate "April 11, 2009"^^xsd:string ;
    NIFRID:acronym "V-CJD"^^xsd:string ;
    NIFRID:definingCitation "N Engl J Med, 1998 Dec 31;339(27)"^^xsd:string ;
    NIFRID:hasBirnlexCurator NIFRID:Bill_Bug ;
    NIFRID:hasCurationStatus NIFRID:uncurated ;
    NIFRID:hasDefinitionSource NIFRID:MeSH_defSource ;
    NIFRID:hasExternalSource NIFRID:MeSH ;
    NIFRID:MeshUid "D007562"^^xsd:string .

BIRNLEX:12690 a owl:Class ;
    rdfs:label "Bovine Spongiform Encephalopathy"^^xsd:string ;
    skos:prefLabel "Bovine Spongiform Encephalopathy"^^xsd:string ;
    NIFRID:synonym "Mad Cow Disease"^^xsd:string ;
    skos:definition "A transmissible spongiform encephalopathy of cattle associated with abnormal prion proteins in the brain. Affected animals develop excitability and salivation followed by ATAXIA. This disorder has been associated with consumption of SCRAPIE infected ruminant derived protein. This condition may be transmitted to humans, where it is referred to as variant or new variant CREUTZFELDT-JAKOB SYNDROME (MeSH)."^^xsd:string ;
    rdfs:subClassOf BIRNLEX:12686 ;
    NIFRID:createdDate "2007-10-05"^^xsd:string ;
    NIFRID:modifiedDate "2007-10-05"^^xsd:string ;
    NIFRID:acronym "BSE"^^xsd:string ;
    NIFRID:definingCitation "Vet Rec 1998 Jul 25;143(41):101-5"^^xsd:string ;
    NIFRID:hasBirnlexCurator NIFRID:Bill_Bug ;
    NIFRID:hasCurationStatus NIFRID:uncurated ;
    NIFRID:hasDefinitionSource NIFRID:MeSH_defSource ;
    NIFRID:hasExternalSource NIFRID:MeSH ;
    NIFRID:MeshUid "D016643"^^xsd:string .

BIRNLEX:12691 a owl:Class ;
    rdfs:label "Gerstmann-Straussler-Scheinker Disease"^^xsd:string ;
    skos:prefLabel "Gerstmann-Straussler-Scheinker Disease"^^xsd:string ;
    NIFRID:synonym "Gerstmann-Straussler Inherited Spongiform Encephalopathy"^^xsd:string,
        "Gerstmann-Straussler Syndrome"^^xsd:string,
        "Gerstmann-Straussler-Scheinker's Disease"^^xsd:string ;
    skos:definition "An autosomal dominant familial prion disease with a wide spectrum of clinical presentations including ATAXIA, spastic paraparesis, extrapyramidal signs, and DEMENTIA. Clinical onset is in the third to sixth decade of life and the mean duration of illness prior to death is five years. Several kindreds with variable clinical and pathologic features have been described. Pathologic features include cerebral prion protein amyloidosis, and spongiform or neurofibrillary degeneration (MeSH)."^^xsd:string ;
    rdfs:subClassOf BIRNLEX:12686 ;
    NIFRID:createdDate "2007-10-05"^^xsd:string ;
    NIFRID:modifiedDate "April 11, 2009"^^xsd:string ;
    NIFRID:definingCitation "Brain Pathol 1998 Jul;8(3):499-513; Brain Pathol 1995 Jan;5(1):61-75"^^xsd:string ;
    NIFRID:hasBirnlexCurator NIFRID:Bill_Bug ;
    NIFRID:hasCurationStatus NIFRID:uncurated ;
    NIFRID:hasDefinitionSource NIFRID:MeSH_defSource ;
    NIFRID:hasExternalSource NIFRID:MeSH ;
    NIFRID:MeshUid "D016098"^^xsd:string .

BIRNLEX:12692 a owl:Class ;
    rdfs:label "Fatal Familial Insomnia"^^xsd:string ;
    skos:prefLabel "Fatal Familial Insomnia"^^xsd:string ;
    skos:definition "An autosomal dominant disorder characterized by degeneration of the THALAMUS and progressive insomnia. It is caused by a mutation in the prion protein ( PRIONS) (MeSH)."^^xsd:string ;
    rdfs:subClassOf BIRNLEX:12686 ;
    NIFRID:createdDate "2007-10-05"^^xsd:string ;
    NIFRID:modifiedDate "2007-10-05"^^xsd:string ;
    NIFRID:hasBirnlexCurator NIFRID:Bill_Bug ;
    NIFRID:hasCurationStatus NIFRID:uncurated ;
    NIFRID:hasDefinitionSource NIFRID:MeSH_defSource ;
    NIFRID:hasExternalSource NIFRID:MeSH ;
    NIFRID:MeshUid "D034062"^^xsd:string .

BIRNLEX:12693 a owl:Class ;
    rdfs:label "Kuru"^^xsd:string ;
    skos:prefLabel "Kuru"^^xsd:string ;
    NIFRID:synonym "Kuru Encephalopathy"^^xsd:string ;
    skos:definition "A prion disease found exclusively among the Fore linguistic group natives of the highlands of NEW GUINEA. The illness is primarily restricted to adult females and children of both sexes. It is marked by the subacute onset of tremor and ataxia followed by motor weakness and incontinence. Death occurs within 3-6 months of disease onset. The condition is associated with ritual cannibalism, and has become rare since this practice has been discontinued. Pathologic features include a noninflammatory loss of neurons that is most prominent in the cerebellum, glial proliferation, and amyloid plaques (MeSH)."^^xsd:string ;
    rdfs:subClassOf BIRNLEX:12686 ;
    NIFRID:createdDate "2007-10-05"^^xsd:string ;
    NIFRID:modifiedDate "2007-10-05"^^xsd:string ;
    NIFRID:hasBirnlexCurator NIFRID:Bill_Bug ;
    NIFRID:hasCurationStatus NIFRID:uncurated ;
    NIFRID:hasDefinitionSource NIFRID:MeSH_defSource ;
    NIFRID:hasExternalSource NIFRID:MeSH ;
    NIFRID:MeshUid "D007729"^^xsd:string .

BIRNLEX:12694 a owl:Class ;
    rdfs:label "Scrapie"^^xsd:string ;
    skos:prefLabel "Scrapie"^^xsd:string ;
    NIFRID:synonym "Rida"^^xsd:string ;
    skos:definition "A prion disease found exclusively among the Fore linguistic group natives of the highlands of NEW GUINEA. The illness is primarily restricted to adult females and children of both sexes. It is marked by the subacute onset of tremor and ataxia followed by motor weakness and incontinence. Death occurs within 3-6 months of disease onset. The condition is associated with ritual cannibalism, and has become rare since this practice has been discontinued. Pathologic features include a noninflammatory loss of neurons that is most prominent in the cerebellum, glial proliferation, and amyloid plaques (MeSH)."^^xsd:string ;
    rdfs:subClassOf BIRNLEX:12686 ;
    NIFRID:createdDate "2007-10-05"^^xsd:string ;
    NIFRID:modifiedDate "2007-10-05"^^xsd:string ;
    NIFRID:hasBirnlexCurator NIFRID:Bill_Bug ;
    NIFRID:hasCurationStatus NIFRID:uncurated ;
    NIFRID:hasDefinitionSource NIFRID:MeSH_defSource ;
    NIFRID:hasExternalSource NIFRID:MeSH ;
    NIFRID:MeshUid "D012608"^^xsd:string .

BIRNLEX:12695 a owl:Class ;
    rdfs:label "Chronic Wasting Disease"^^xsd:string ;
    skos:prefLabel "Chronic Wasting Disease"^^xsd:string ;
    skos:definition "A transmissible spongiform encephalopathy (prion disease) of DEER and elk characterized by chronic weight loss leading to death. It is thought to spread by direct contact between animals or through environmental contamination with the prion protein ( PRIONS) (MeSH)."^^xsd:string ;
    rdfs:subClassOf BIRNLEX:12686 ;
    NIFRID:createdDate "2007-10-05"^^xsd:string ;
    NIFRID:modifiedDate "2007-10-05"^^xsd:string ;
    NIFRID:hasBirnlexCurator NIFRID:Bill_Bug ;
    NIFRID:hasCurationStatus NIFRID:uncurated ;
    NIFRID:hasDefinitionSource NIFRID:MeSH_defSource ;
    NIFRID:hasExternalSource NIFRID:MeSH ;
    NIFRID:MeshUid "D034081"^^xsd:string .

BIRNLEX:12696 a owl:Class ;
    rdfs:label "Tauopathy"^^xsd:string ;
    skos:prefLabel "Tauopathy"^^xsd:string ;
    skos:definition "Neurodegenerative disorders involving deposition of abnormal tau protein isoforms ( TAU PROTEINS) in neurons and glial cells in the brain. Pathological aggregations of tau proteins are associated with mutation of the tau gene on chromosome 17 in patients with ALZHEIMER DISEASE; DEMENTIA; PARKINSONIAN DISORDERS; progressive supranuclear palsy ( SUPRANUCLEAR PALSY, PROGRESSIVE); and corticobasal degeneration (MeSH)."^^xsd:string ;
    rdfs:subClassOf BIRNLEX:2086 ;
    NIFRID:createdDate "2007-10-05"^^xsd:string ;
    NIFRID:modifiedDate "2007-10-05"^^xsd:string ;
    NIFRID:hasBirnlexCurator NIFRID:Bill_Bug ;
    NIFRID:hasCurationStatus NIFRID:uncurated ;
    NIFRID:hasDefinitionSource NIFRID:MeSH_defSource ;
    NIFRID:hasExternalSource NIFRID:MeSH ;
    NIFRID:MeshUid "D024801"^^xsd:string .

BIRNLEX:12697 a owl:Class ;
    rdfs:label "Progressive Supranuclear Palsy"^^xsd:string ;
    skos:prefLabel "Progressive Supranuclear Palsy"^^xsd:string ;
    NIFRID:synonym "Progressive Supranuclear Ophthalmoplegia"^^xsd:string,
        "Steele-Richardson-Olszewski Disease"^^xsd:string,
        "Steele-Richardson-Olszewski Syndrome"^^xsd:string ;
    skos:definition "A degenerative disease of the central nervous system characterized by balance difficulties; OCULAR MOTILITY DISORDERS (supranuclear ophthalmoplegia); DYSARTHRIA; swallowing difficulties; and axial DYSTONIA. Onset is usually in the fifth decade and disease progression occurs over several years. Pathologic findings include neurofibrillary degeneration and neuronal loss in the dorsal MESENCEPHALON; SUBTHALAMIC NUCLEUS; RED NUCLEUS; pallidum; dentate nucleus; and vestibular nuclei (MeSH)."^^xsd:string ;
    rdfs:subClassOf BIRNLEX:12696 ;
    NIFRID:createdDate "2007-10-08"^^xsd:string ;
    NIFRID:modifiedDate "2007-10-08"^^xsd:string ;
    NIFRID:hasBirnlexCurator NIFRID:Bill_Bug ;
    NIFRID:hasCurationStatus NIFRID:uncurated ;
    NIFRID:hasDefinitionSource NIFRID:MeSH_defSource ;
    NIFRID:hasExternalSource NIFRID:MeSH ;
    NIFRID:MeshUid "D013494"^^xsd:string ;
    NIFRID:nifID "_8.3_2.12"^^xsd:string .

BIRNLEX:12698 a owl:Class ;
    rdfs:label "Substance-Related Disorder"^^xsd:string ;
    skos:prefLabel "Substance-Related Disorder"^^xsd:string ;
    NIFRID:synonym "Addiction"^^xsd:string,
        "Drug Abuse"^^xsd:string,
        "Drug Usage"^^xsd:string,
        "drug use"^^xsd:string,
        "Drug Use Disorder"^^xsd:string,
        "Substance Abuse"^^xsd:string,
        "Substance Disorder"^^xsd:string,
        "Substance use"^^xsd:string,
        "Substance Use Disorder"^^xsd:string,
        "Substance-Induced Organic Mental Disorder"^^xsd:string ;
    skos:definition "Disorder related to substance abuse, the side effects of a medication, toxin exposure, and ALCOHOL-RELATED DISORDERS (MeSH)."^^xsd:string ;
    rdfs:subClassOf BIRNLEX:12669 ;
    NIFRID:createdDate "2007-10-08"^^xsd:string ;
    NIFRID:modifiedDate "March 18, 2009"^^xsd:string ;
    NIFRID:hasBirnlexCurator NIFRID:Bill_Bug ;
    NIFRID:hasCurationStatus NIFRID:uncurated ;
    NIFRID:hasDefinitionSource NIFRID:MeSH_defSource ;
    NIFRID:hasExternalSource NIFRID:MeSH ;
    NIFRID:MeshUid "D019966"^^xsd:string ;
    NIFRID:nifID "_8.3_11.1"^^xsd:string ;
    NIFRID:putativeClassExtension "Drug Addiction"^^xsd:string,
        "Drug Dependence"^^xsd:string,
        "Drug Habituation"^^xsd:string,
        "Glue Sniffing"^^xsd:string,
        "Substance Addiction"^^xsd:string,
        "Substance Dependence"^^xsd:string ;
    NIFRID:usageNote "MeSH includes the following entry terms that are either implied sub-types or components of the overall spectrum of functional manifestations of Substance-Related Disorder"^^xsd:string .

BIRNLEX:12699 a owl:Class ;
    rdfs:label "Alcohol-Related Disorder"^^xsd:string ;
    skos:prefLabel "Alcohol-Related Disorder"^^xsd:string ;
    skos:definition "Disorder related to or resulting from abuse or mis-use of alcohol (MeSH)."^^xsd:string ;
    rdfs:subClassOf BIRNLEX:12698 ;
    NIFRID:createdDate "2007-10-08"^^xsd:string ;
    NIFRID:modifiedDate "2007-10-08"^^xsd:string ;
    NIFRID:hasBirnlexCurator NIFRID:Bill_Bug ;
    NIFRID:hasCurationStatus NIFRID:uncurated ;
    NIFRID:hasDefinitionSource NIFRID:MeSH_defSource ;
    NIFRID:hasExternalSource NIFRID:MeSH ;
    NIFRID:MeshUid "D019973"^^xsd:string ;
    NIFRID:nifID "_8.3_11.1.1"^^xsd:string .

BIRNLEX:12700 a owl:Class ;
    rdfs:label "Alcohol Amnestic Disorder"^^xsd:string ;
    skos:prefLabel "Alcohol Amnestic Disorder"^^xsd:string ;
    NIFRID:synonym "Alcohol Amnestic Syndrome"^^xsd:string,
        "Alcohol-Induced Amnestic Psychosis"^^xsd:string,
        "Alcohol-Induced Amnestic Syndrome"^^xsd:string,
        "Alcohol-Induced Dysmnesic Psychosis"^^xsd:string,
        "Alcohol-Induced Dysmnesic Syndrome"^^xsd:string ;
    skos:definition "A mental disorder associated with chronic ethanol abuse ( ALCOHOLISM) and nutritional deficiencies characterized by short term memory loss, confabulations, and disturbances of attention (MeSH)."^^xsd:string ;
    rdfs:subClassOf BIRNLEX:12699 ;
    NIFRID:createdDate "2007-10-08"^^xsd:string ;
    NIFRID:modifiedDate "2007-10-08"^^xsd:string ;
    NIFRID:definingCitation "Adams et al., Principles of Neurology, 6th ed, p1139"^^xsd:string ;
    NIFRID:hasBirnlexCurator NIFRID:Bill_Bug ;
    NIFRID:hasCurationStatus NIFRID:uncurated ;
    NIFRID:hasDefinitionSource NIFRID:MeSH_defSource ;
    NIFRID:hasExternalSource NIFRID:MeSH ;
    NIFRID:MeshUid "D000425"^^xsd:string .

BIRNLEX:12701 a owl:Class ;
    rdfs:label "Korsakoff Syndrome"^^xsd:string ;
    skos:prefLabel "Korsakoff Syndrome"^^xsd:string ;
    NIFRID:synonym "Korsakoff Psychosis"^^xsd:string,
        "Wernicke-Korsakoff Syndrome"^^xsd:string ;
    skos:definition "An acquired cognitive disorder characterized by inattentiveness and the inability to form short term memories. This disorder is frequently associated with chronic ALCOHOLISM; but it may also result from dietary deficiencies; CRANIOCEREBRAL TRAUMA; NEOPLASMS; CEREBROVASCULAR DISORDERS; ENCEPHALITIS; EPILEPSY; and other conditions (MeSH)."^^xsd:string ;
    rdfs:subClassOf BIRNLEX:12700 ;
    NIFRID:createdDate "2007-10-08"^^xsd:string ;
    NIFRID:modifiedDate "2007-10-08"^^xsd:string ;
    NIFRID:definingCitation "Adams et al., Principles of Neurology, 6th ed, p1139"^^xsd:string ;
    NIFRID:hasBirnlexCurator NIFRID:Bill_Bug ;
    NIFRID:hasCurationStatus NIFRID:uncurated ;
    NIFRID:hasDefinitionSource NIFRID:MeSH_defSource ;
    NIFRID:hasExternalSource NIFRID:MeSH ;
    NIFRID:MeshUid "D019973"^^xsd:string .

BIRNLEX:12702 a owl:Class ;
    rdfs:label "Alcohol Withdrawal Delirium"^^xsd:string ;
    skos:prefLabel "Alcohol Withdrawal Delirium"^^xsd:string ;
    NIFRID:synonym "Alcohol Withdrawal Associated Autonomic Hyperactivity"^^xsd:string,
        "Alcohol Withdrawal Hallucinosis"^^xsd:string,
        "Alcohol Withdrawal-Induced Delirium Tremens"^^xsd:string,
        "Delirium Tremens"^^xsd:string ;
    skos:definition "An acute organic mental disorder induced by cessation or reduction in chronic alcohol consumption. Clinical characteristics include CONFUSION; DELUSIONS; vivid HALLUCINATIONS; TREMOR; agitation; insomnia; and signs of autonomic hyperactivity (e.g., elevated blood pressure and heart rate, dilated pupils, and diaphoresis). This condition may occasionally be fatal. It was formerly called delirium tremens (MeSH)."^^xsd:string ;
    rdfs:subClassOf BIRNLEX:12699 ;
    NIFRID:createdDate "2007-10-08"^^xsd:string ;
    NIFRID:modifiedDate "2007-10-08"^^xsd:string ;
    NIFRID:definingCitation "Adams et al., Principles of Neurology, 6th ed, p1175"^^xsd:string ;
    NIFRID:hasBirnlexCurator NIFRID:Bill_Bug ;
    NIFRID:hasCurationStatus NIFRID:uncurated ;
    NIFRID:hasDefinitionSource NIFRID:MeSH_defSource ;
    NIFRID:hasExternalSource NIFRID:MeSH ;
    NIFRID:MeshUid "D000430"^^xsd:string .

BIRNLEX:12703 a owl:Class ;
    rdfs:label "Alcoholic Intoxication"^^xsd:string ;
    skos:prefLabel "Alcoholic Intoxication"^^xsd:string ;
    NIFRID:synonym "Drunkenness"^^xsd:string ;
    skos:definition "An acute brain syndrome which results from the excessive ingestion of ETHANOL or ALCOHOLIC BEVERAGES (MeSH)."^^xsd:string ;
    rdfs:subClassOf BIRNLEX:12699 ;
    NIFRID:createdDate "2007-10-08"^^xsd:string ;
    NIFRID:modifiedDate "2007-10-08"^^xsd:string ;
    NIFRID:hasBirnlexCurator NIFRID:Bill_Bug ;
    NIFRID:hasCurationStatus NIFRID:uncurated ;
    NIFRID:hasDefinitionSource NIFRID:MeSH_defSource ;
    NIFRID:hasExternalSource NIFRID:MeSH ;
    NIFRID:MeshUid "D000435"^^xsd:string .

BIRNLEX:12704 a owl:Class ;
    rdfs:label "Alcoholism"^^xsd:string ;
    skos:prefLabel "Alcoholism"^^xsd:string ;
    NIFRID:synonym "Alcohol Abuse"^^xsd:string,
        "Chronic Alcoholic Intoxication"^^xsd:string ;
    skos:definition "A primary, chronic disease with genetic, psychosocial, and environmental factors influencing its development and manifestations. The disease is often progressive and fatal. It is characterized by impaired control over drinking, preoccupation with the drug alcohol, use of alcohol despite adverse consequences, and distortions in thinking, most notably denial. Each of these symptoms may be continuous or periodic (MeSH)."^^xsd:string ;
    rdfs:subClassOf BIRNLEX:12699 ;
    NIFRID:createdDate "2007-10-08"^^xsd:string ;
    NIFRID:modifiedDate "2007-10-08"^^xsd:string ;
    NIFRID:definingCitation "Morse and Flavin for the Joint Commission of the National Council on Alcoholism and Drug Dependence and the American Society of Addiction Medicine to Study the Definition and Criteria for the Diagnosis of Alcoholism: in JAMA 1992;268:1012-4"^^xsd:string ;
    NIFRID:hasBirnlexCurator NIFRID:Bill_Bug ;
    NIFRID:hasCurationStatus NIFRID:uncurated ;
    NIFRID:hasDefinitionSource NIFRID:MeSH_defSource ;
    NIFRID:hasExternalSource NIFRID:MeSH ;
    NIFRID:MeshUid "D000437"^^xsd:string .

BIRNLEX:12705 a owl:Class ;
    rdfs:label "Metabolic Nervous System Disease"^^xsd:string ;
    skos:prefLabel "Metabolic Nervous System Disease"^^xsd:string ;
    NIFRID:synonym "Central Nervous System Metabolic Disorder"^^xsd:string,
        "CNS Metabolic Disorder"^^xsd:string,
        "Metabolic Brain Disease"^^xsd:string,
        "Metabolic Brain Disorder"^^xsd:string,
        "Metabolic Brain Syndrome"^^xsd:string,
        "Metabolic Encephalopathy"^^xsd:string,
        "Metabolic Nervous System Disorder"^^xsd:string,
        "Metabolic Nervous System Syndrome"^^xsd:string ;
    skos:definition "Brain dysfunction or damage caused by acquired (i.e., non-inborn) metabolic disorders. Associated conditions include ENDOCRINE DISEASES; WATER-ELECTROLYTE IMBALANCE; KIDNEY DISEASES; LIVER DISEASES; anoxia ( HYPOXIA, BRAIN); nutritional disorders (see NUTRITIONAL AND METABOLIC DISEASES); an encephalopathy associated with HEMODIALYSIS; and other disorders (MeSH)."^^xsd:string ;
    rdfs:subClassOf BIRNLEX:12796 ;
    skos:editorialNote "Note BIRNLex seeks to evolve a core subsumptive disease hierarchy based first on the effected function, then the effected structure, the latter for those categories of nervous system disease that have typically been associated with structural abnormalities or trauma (e.g., Motor neuron diseases, cerebrovascular trauma, etc.). Disease causation is in fact the ultimate goal of much biomedical research, and our recognitition of ALL the driving causes of a particular disease - and the ways in which these causes inter-relate with each other and with effected structures to cause a change in normal function is a critical representational task BIRNlex will increasingly take on to provide an evolving, nuanced functional reconstruction of disease as a process and an outcome.  These relations will be represented using OWL ObjectProperties.  Function is the most sensible context to drive the asserted subsumptive hierarchy for representing nervous system disease, since it is with the clinical description of altered, impaired, decreased, or lost function that the diagnosis - and the research - of disease is rooted.  Much has already been described regarding both the effected biomaterial entities and the causes of disease.  However, it is because understanding of such relations still is far from comprehensive, that biomedical investigation into nervous system disease continues.  Finally, given the \"realist\" ontology design approach being used to construct BIRNLex, function must be represented as inhering in some biomaterial entity from molecules and their controlling elements on up through gross anatomical structures.  Over time, BIRNLex will provide the required relations to depict these functionally-related structures for both the normal and pathological function of the nervous system.  This will be true both for the causes and for the outcomes of nervous system disease.  Initial work to extend this expressive representation will focus on the neurodegenerative diseases being studied by BIRN researchers.  Though this will be te case, BIRNLex still needs to provide a core asserted hierarchy for a broad swarth of nervous system disease, so as to enable BIRN researchers to link to the breadth of disorders that may impact or relate to those directly under study."^^xsd:string ;
    NIFRID:createdDate "2007-10-08"^^xsd:string ;
    NIFRID:modifiedDate "2007-11-18"^^xsd:string ;
    NIFRID:definingCitation "Plum & Posner, Diagnosis of Stupor and Coma, 3rd ed, pp208-260"^^xsd:string ;
    NIFRID:hasBirnlexCurator NIFRID:Bill_Bug ;
    NIFRID:hasCurationStatus NIFRID:uncurated ;
    NIFRID:hasDefinitionSource NIFRID:MeSH_defSource ;
    NIFRID:hasExternalSource NIFRID:MeSH ;
    NIFRID:MeshUid "D001928"^^xsd:string ;
    NIFRID:nifID "_8.3_7"^^xsd:string ;
    NIFRID:usageNote "Acquired or inborn metabolic diseases that produce brain dysfunction or damage. These include primary (i.e., disorders intrinsic to the brain) and secondary (i.e., extracranial) metabolic conditions that adversely affect cerebral function (MeSH)."^^xsd:string,
        "MeSH includes all the listed synonyms with ACQUIRED pre-pended, indicating a non-hereditary subtype."^^xsd:string .

BIRNLEX:12706 a owl:Class ;
    rdfs:label "Inborn Metabolic Brain Disease"^^xsd:string ;
    skos:prefLabel "Inborn Metabolic Brain Disease"^^xsd:string ;
    NIFRID:synonym "Familial Metabolic Brain Disease"^^xsd:string,
        "Familial Metabolic Brain Disorder"^^xsd:string,
        "Inborn Errors of Metabolism, Brain"^^xsd:string,
        "Inborn Metabolic Brain Disorder"^^xsd:string,
        "Inborn Metabolic Central Nervous System Disease"^^xsd:string,
        "Inborn Metabolic Central Nervous System Disorder"^^xsd:string,
        "Inborn Metabolic CNS Disease"^^xsd:string,
        "Inborn Metabolic CNS Disorder"^^xsd:string,
        "Inborn Metabolic Encephalopathy"^^xsd:string,
        "Inherited Metabolic Brain Disease"^^xsd:string,
        "Inherited Metabolic Brain Disorder"^^xsd:string ;
    skos:definition "Brain disorders resulting from inborn metabolic errors, primarily from enzymatic defects which lead to substrate accumulation, product reduction, or increase in toxic metabolites through alternate pathways. The majority of these conditions are familial, however spontaneous mutation may also occur in utero (MeSH)."^^xsd:string ;
    rdfs:subClassOf BIRNLEX:12705 ;
    NIFRID:createdDate "2007-10-08"^^xsd:string ;
    NIFRID:modifiedDate "2007-10-08"^^xsd:string ;
    NIFRID:hasBirnlexCurator NIFRID:Bill_Bug ;
    NIFRID:hasCurationStatus NIFRID:uncurated ;
    NIFRID:hasDefinitionSource NIFRID:MeSH_defSource ;
    NIFRID:hasExternalSource NIFRID:MeSH ;
    NIFRID:MeshUid "D020739"^^xsd:string .

BIRNLEX:12707 a owl:Class ;
    rdfs:label "Alcoholic Psychosis"^^xsd:string ;
    skos:prefLabel "Alcoholic Psychosis"^^xsd:string ;
    skos:definition "A group of mental disorders associated with organic brain damage and caused by poisoning from alcohol (MeSH)."^^xsd:string ;
    rdfs:subClassOf BIRNLEX:12699 ;
    skos:editorialNote "This class will utlimately be moved to a position reflecting the effected function, as opposed to one reflecting causation (BB: 2007-10-08)"^^xsd:string ;
    NIFRID:createdDate "2007-10-08"^^xsd:string ;
    NIFRID:modifiedDate "2007-10-08"^^xsd:string ;
    NIFRID:hasBirnlexCurator NIFRID:Bill_Bug ;
    NIFRID:hasCurationStatus NIFRID:graph_position_temporary ;
    NIFRID:hasDefinitionSource NIFRID:MeSH_defSource ;
    NIFRID:hasExternalSource NIFRID:MeSH ;
    NIFRID:MeshUid "D011604"^^xsd:string .

BIRNLEX:12708 a owl:Class ;
    rdfs:label "Wernicke Encephalopathy"^^xsd:string ;
    skos:prefLabel "Wernicke Encephalopathy"^^xsd:string ;
    NIFRID:synonym "Cerebral Beriberi"^^xsd:string,
        "Gayet-Wernicke Encephalopathy"^^xsd:string,
        "Wernicke Disease"^^xsd:string,
        "Wernicke Syndrome"^^xsd:string ;
    skos:definition "An acute neurological disorder characterized by the triad of ophthalmoplegia, ataxia, and disturbances of mental activity or consciousness. Eye movement abnormalities include nystagmus, external rectus palsies, and reduced conjugate gaze. THIAMINE DEFICIENCY and chronic ALCOHOLISM are associated conditions. Pathologic features include periventricular petechial hemorrhages and neuropil breakdown in the diencephalon and brainstem. Chronic thiamine deficiency may lead to KORSAKOFF SYNDROME (MeSH)."^^xsd:string ;
    rdfs:subClassOf BIRNLEX:12699 ;
    skos:editorialNote "This class will utlimately be moved to a position reflecting the effected function, as opposed to one reflecting causation (BB: 2007-10-08)"^^xsd:string ;
    NIFRID:createdDate "2007-10-08"^^xsd:string ;
    NIFRID:modifiedDate "2007-10-08"^^xsd:string ;
    NIFRID:definingCitation "Adams et al., Principles of Neurology, 6th ed, pp1139-42; Davis & Robertson, Textbook of Neuropathology, 2nd ed, pp452-3"^^xsd:string ;
    NIFRID:hasBirnlexCurator NIFRID:Bill_Bug ;
    NIFRID:hasCurationStatus NIFRID:graph_position_temporary ;
    NIFRID:hasDefinitionSource NIFRID:MeSH_defSource ;
    NIFRID:hasExternalSource NIFRID:MeSH ;
    NIFRID:MeshUid "D011604"^^xsd:string .

BIRNLEX:12709 a owl:Class ;
    rdfs:label "Amphetamine-Related Disorder"^^xsd:string ;
    skos:prefLabel "Amphetamine-Related Disorder"^^xsd:string ;
    NIFRID:synonym "Amphetamine Abuse"^^xsd:string,
        "Amphetamine Usage"^^xsd:string ;
    skos:definition "Disorders related or resulting from use of amphetamines (MeSH)."^^xsd:string ;
    rdfs:subClassOf BIRNLEX:12698 ;
    NIFRID:createdDate "2007-10-08"^^xsd:string ;
    NIFRID:modifiedDate "2007-10-08"^^xsd:string ;
    NIFRID:hasBirnlexCurator NIFRID:Bill_Bug ;
    NIFRID:hasCurationStatus NIFRID:uncurated ;
    NIFRID:hasDefinitionSource NIFRID:MeSH_defSource ;
    NIFRID:hasExternalSource NIFRID:MeSH ;
    NIFRID:MeshUid "D019969"^^xsd:string ;
    NIFRID:putativeClassExtension "Amphetamine Addiction"^^xsd:string,
        "Amphetamine Dependence"^^xsd:string ;
    NIFRID:usageNote "MeSH includes implied components of the overall spectrum of functional manifestations of Amphetamine-Related Disorder"^^xsd:string .

BIRNLEX:12710 a owl:Class ;
    rdfs:label "Cocaine-Related Disorder"^^xsd:string ;
    skos:prefLabel "Cocaine-Related Disorder"^^xsd:string ;
    NIFRID:synonym "Cocaine Abuse"^^xsd:string,
        "Cocaine Usage"^^xsd:string ;
    skos:definition "Disorders related or resulting from use of amphetamines (MeSH)."^^xsd:string ;
    rdfs:subClassOf BIRNLEX:12698 ;
    NIFRID:createdDate "2007-10-08"^^xsd:string ;
    NIFRID:modifiedDate "2007-10-08"^^xsd:string ;
    NIFRID:hasBirnlexCurator NIFRID:Bill_Bug ;
    NIFRID:hasCurationStatus NIFRID:uncurated ;
    NIFRID:hasDefinitionSource NIFRID:MeSH_defSource ;
    NIFRID:hasExternalSource NIFRID:MeSH ;
    NIFRID:MeshUid "D019970"^^xsd:string ;
    NIFRID:nifID "_8.3_11.1.3"^^xsd:string ;
    NIFRID:putativeClassExtension "Cocaine Addiction"^^xsd:string,
        "Cocaine Dependence"^^xsd:string ;
    NIFRID:usageNote "MeSH includes implied components of the overall spectrum of functional manifestations of Cocaine-Related Disorder"^^xsd:string .

BIRNLEX:12711 a owl:Class ;
    rdfs:label "Cannabis-Related Disorder"^^xsd:string ;
    skos:prefLabel "Cannabis-Related Disorder"^^xsd:string ;
    NIFRID:synonym "Cannabinoid Abuse"^^xsd:string,
        "Cannabis Abuse"^^xsd:string,
        "Hashish Abuse"^^xsd:string,
        "Marijuana Abuse"^^xsd:string ;
    skos:definition "The excessive use of marijuana with associated psychological symptoms and impairment in social or occupational functioning (MeSH)."^^xsd:string ;
    rdfs:subClassOf BIRNLEX:12698 ;
    NIFRID:createdDate "2007-10-08"^^xsd:string ;
    NIFRID:modifiedDate "2007-10-08"^^xsd:string ;
    NIFRID:hasBirnlexCurator NIFRID:Bill_Bug ;
    NIFRID:hasCurationStatus NIFRID:uncurated ;
    NIFRID:hasDefinitionSource NIFRID:MeSH_defSource ;
    NIFRID:hasExternalSource NIFRID:MeSH ;
    NIFRID:MeshUid "D002189"^^xsd:string ;
    NIFRID:nifID "_8.3_11.1.2"^^xsd:string ;
    NIFRID:putativeClassExtension "Cannabis Dependence"^^xsd:string,
        "Marijuana Dependence"^^xsd:string ;
    NIFRID:usageNote "MeSH includes implied components of the overall spectrum of functional manifestations of Cannabis-Related Disorder"^^xsd:string .

BIRNLEX:12712 a owl:Class ;
    rdfs:label "Neonatal Abstinence Syndrome"^^xsd:string ;
    skos:prefLabel "Neonatal Abstinence Syndrome"^^xsd:string ;
    skos:definition "Fetal and neonatal addiction and withdrawal as a result of the mother's dependence on drugs during pregnancy. Withdrawal or abstinence symptoms develop shortly after birth. Symptoms exhibited are loud, high-pitched crying, sweating, yawning and gastrointestinal disturbances (MeSH)."^^xsd:string ;
    rdfs:subClassOf BIRNLEX:12698 ;
    NIFRID:createdDate "2007-10-08"^^xsd:string ;
    NIFRID:modifiedDate "2007-10-08"^^xsd:string ;
    NIFRID:hasBirnlexCurator NIFRID:Bill_Bug ;
    NIFRID:hasCurationStatus NIFRID:uncurated ;
    NIFRID:hasDefinitionSource NIFRID:MeSH_defSource ;
    NIFRID:hasExternalSource NIFRID:MeSH ;
    NIFRID:MeshUid "D009357"^^xsd:string ;
    NIFRID:putativeClassExtension "Neonatal Passive Addiction"^^xsd:string,
        "Neonatal Substance Withdrawal"^^xsd:string,
        "Neonatal Withdrawal Syndrome"^^xsd:string ;
    NIFRID:usageNote "MeSH includes implied components of the overall spectrum of functional manifestations of Neonatal Abstinence Syndrome"^^xsd:string .

BIRNLEX:12713 a owl:Class ;
    rdfs:label "Opioid-Related Disorder"^^xsd:string ;
    skos:prefLabel "Opioid-Related Disorder"^^xsd:string ;
    NIFRID:synonym "Narcotic Abuse"^^xsd:string ;
    skos:definition "Disorders related or resulting from abuse or mis-use of opioids (MeSH)."^^xsd:string ;
    rdfs:subClassOf BIRNLEX:12698 ;
    NIFRID:createdDate "2007-10-08"^^xsd:string ;
    NIFRID:modifiedDate "2007-10-08"^^xsd:string ;
    NIFRID:hasBirnlexCurator NIFRID:Bill_Bug ;
    NIFRID:hasCurationStatus NIFRID:uncurated ;
    NIFRID:hasDefinitionSource NIFRID:MeSH_defSource ;
    NIFRID:hasExternalSource NIFRID:MeSH ;
    NIFRID:MeshUid "D009293"^^xsd:string ;
    NIFRID:nifID "_8.3_11.1.5"^^xsd:string ;
    NIFRID:putativeClassExtension "Narcotic Addiction"^^xsd:string,
        "Narcotic Dependence"^^xsd:string,
        "Opiate Addiction"^^xsd:string,
        "Opiate Dependence"^^xsd:string ;
    NIFRID:usageNote "MeSH includes implied components of the overall spectrum of functional manifestations of Opioid-Related Disorder"^^xsd:string .

BIRNLEX:12714 a owl:Class ;
    rdfs:label "Heroin-Related Disorder"^^xsd:string ;
    skos:prefLabel "Heroin-Related Disorder"^^xsd:string ;
    NIFRID:synonym "Heroin Abuse"^^xsd:string,
        "Heroin Usage"^^xsd:string ;
    skos:definition "Disorders related or resulting from abuse or mis-use of heroin."^^xsd:string ;
    rdfs:subClassOf BIRNLEX:12713 ;
    NIFRID:createdDate "2007-10-08"^^xsd:string ;
    NIFRID:modifiedDate "2007-10-08"^^xsd:string ;
    NIFRID:hasBirnlexCurator NIFRID:Bill_Bug ;
    NIFRID:hasCurationStatus NIFRID:uncurated ;
    NIFRID:hasDefinitionSource NIFRID:MeSH_defSource ;
    NIFRID:hasExternalSource NIFRID:MeSH ;
    NIFRID:MeshUid "D006556"^^xsd:string ;
    NIFRID:putativeClassExtension "Heroin Addiction"^^xsd:string,
        "Heroin Dependence"^^xsd:string ;
    NIFRID:usageNote "MeSH includes implied components of the overall spectrum of functional manifestations of Opioid-Related Disorder"^^xsd:string .

BIRNLEX:12715 a owl:Class ;
    rdfs:label "Morphine-Related Disorder"^^xsd:string ;
    skos:prefLabel "Morphine-Related Disorder"^^xsd:string ;
    NIFRID:synonym "Morphine Abuse"^^xsd:string,
        "Morphine Usage"^^xsd:string ;
    skos:definition "Disorders related or resulting from abuse or mis-use of morphine."^^xsd:string ;
    rdfs:subClassOf BIRNLEX:12713 ;
    NIFRID:createdDate "2007-10-08"^^xsd:string ;
    NIFRID:modifiedDate "2007-10-08"^^xsd:string ;
    NIFRID:hasBirnlexCurator NIFRID:Bill_Bug ;
    NIFRID:hasCurationStatus NIFRID:uncurated ;
    NIFRID:hasDefinitionSource NIFRID:MeSH_defSource ;
    NIFRID:hasExternalSource NIFRID:MeSH ;
    NIFRID:MeshUid "D009021"^^xsd:string ;
    NIFRID:putativeClassExtension "Morphine Addiction"^^xsd:string,
        "Morphine Dependence"^^xsd:string ;
    NIFRID:usageNote "MeSH includes implied components of the overall spectrum of functional manifestations of Morphine-Related Disorder"^^xsd:string .

BIRNLEX:12716 a owl:Class ;
    rdfs:label "Nicotine Use Disorder"^^xsd:string ;
    skos:prefLabel "Nicotine Use Disorder"^^xsd:string ;
    NIFRID:synonym "Tobacco Use Disorder"^^xsd:string ;
    skos:definition "Tobacco used to the detriment of a person's health or social functioning. Tobacco dependence is included (MeSH)."^^xsd:string ;
    rdfs:subClassOf BIRNLEX:12698 ;
    NIFRID:createdDate "2007-10-08"^^xsd:string ;
    NIFRID:modifiedDate "2007-10-08"^^xsd:string ;
    NIFRID:hasBirnlexCurator NIFRID:Bill_Bug ;
    NIFRID:hasCurationStatus NIFRID:uncurated ;
    NIFRID:hasDefinitionSource NIFRID:MeSH_defSource ;
    NIFRID:hasExternalSource NIFRID:MeSH ;
    NIFRID:MeshUid "D014029"^^xsd:string ;
    NIFRID:nifID "_8.3_11.1.4"^^xsd:string ;
    NIFRID:putativeClassExtension "Nicotine Addiction"^^xsd:string,
        "Nicotine Dependence"^^xsd:string ;
    NIFRID:usageNote "MeSH includes implied components of the overall spectrum of functional manifestations of Nicotine Use Disorder"^^xsd:string ;
    skos:scopeNote "includes cigarettes, cigars, chewing tobacco & snuff; a psychiatric diag: do not confuse with SMOKING / adv eff; note X ref NICOTINE DEPENDENCE: do not coord with NICOTINE unless nicotine is substantially discussed as a chemical"^^xsd:string .

BIRNLEX:12717 a owl:Class ;
    rdfs:label "Phencyclidine-Related Disorder"^^xsd:string ;
    skos:prefLabel "Phencyclidine-Related Disorder"^^xsd:string ;
    NIFRID:synonym "Angel Dust Abuse"^^xsd:string,
        "PCP Abuse"^^xsd:string ;
    skos:definition "The misuse of phencyclidine with associated psychological symptoms and impairment in social or occupational functioning (MeSH)."^^xsd:string ;
    rdfs:subClassOf BIRNLEX:12698 ;
    NIFRID:createdDate "2007-10-08"^^xsd:string ;
    NIFRID:modifiedDate "2007-10-08"^^xsd:string ;
    NIFRID:hasBirnlexCurator NIFRID:Bill_Bug ;
    NIFRID:hasCurationStatus NIFRID:uncurated ;
    NIFRID:hasDefinitionSource NIFRID:MeSH_defSource ;
    NIFRID:hasExternalSource NIFRID:MeSH ;
    NIFRID:MeshUid "D010623"^^xsd:string .

BIRNLEX:12718 a owl:Class ;
    rdfs:label "Epilepsy"^^xsd:string ;
    skos:prefLabel "Epilepsy"^^xsd:string ;
    NIFRID:synonym "Epileptic Seizure"^^xsd:string,
        "Seizure Disorder"^^xsd:string ;
    skos:definition "A disorder characterized by recurrent episodes of paroxysmal brain dysfunction due to a sudden, disorderly, and excessive neuronal discharge. Epilepsy classification systems are generally based upon: (1) clinical features of the seizure episodes (e.g., motor seizure), (2) etiology (e.g., post-traumatic), (3) anatomic site of seizure origin (e.g., frontal lobe seizure), (4) tendency to spread to other structures in the brain, and (5) temporal patterns (e.g., nocturnal epilepsy) (MeSH)."^^xsd:string ;
    rdfs:subClassOf BIRNLEX:12796 ;
    skos:editorialNote "Note BIRNLex seeks to evolve a core subsumptive disease hierarchy based first on the effected function, then the effected structure, the latter for those categories of nervous system disease that have typically been associated with structural abnormalities or trauma (e.g., Motor neuron diseases, cerebrovascular trauma, etc.). Disease causation is in fact the ultimate goal of much biomedical research, and our recognitition of ALL the driving causes of a particular disease - and the ways in which these causes inter-relate with each other and with effected structures to cause a change in normal function is a critical representational task BIRNlex will increasingly take on to provide an evolving, nuanced functional reconstruction of disease as a process and an outcome.  These relations will be represented using OWL ObjectProperties.  Function is the most sensible context to drive the asserted subsumptive hierarchy for representing nervous system disease, since it is with the clinical description of altered, impaired, decreased, or lost function that the diagnosis - and the research - of disease is rooted.  Much has already been described regarding both the effected biomaterial entities and the causes of disease.  However, it is because understanding of such relations still is far from comprehensive, that biomedical investigation into nervous system disease continues.  Finally, given the \"realist\" ontology design approach being used to construct BIRNLex, function must be represented as inhering in some biomaterial entity from molecules and their controlling elements on up through gross anatomical structures.  Over time, BIRNLex will provide the required relations to depict these functionally-related structures for both the normal and pathological function of the nervous system.  This will be true both for the causes and for the outcomes of nervous system disease.  Initial work to extend this expressive representation will focus on the neurodegenerative diseases being studied by BIRN researchers.  Though this will be te case, BIRNLex still needs to provide a core asserted hierarchy for a broad swarth of nervous system disease, so as to enable BIRN researchers to link to the breadth of disorders that may impact or relate to those directly under study."^^xsd:string ;
    NIFRID:createdDate "2007-10-08"^^xsd:string ;
    NIFRID:modifiedDate "2007-11-18"^^xsd:string ;
    NIFRID:hasBirnlexCurator NIFRID:Bill_Bug ;
    NIFRID:hasCurationStatus NIFRID:uncurated ;
    NIFRID:hasDefinitionSource NIFRID:MeSH_defSource ;
    NIFRID:hasExternalSource NIFRID:MeSH ;
    NIFRID:MeshUid "D004827"^^xsd:string ;
    NIFRID:nifID "_8.3_5"^^xsd:string .

BIRNLEX:12719 a owl:Class ;
    rdfs:label "Myoclonic Epilepsy"^^xsd:string ;
    skos:prefLabel "Myoclonic Epilepsy"^^xsd:string ;
    NIFRID:synonym "Myoclonic Encephalopathy"^^xsd:string,
        "Myoclonic Seizure Disorder"^^xsd:string,
        "Symptomatic Myoclonic Epilepsy"^^xsd:string ;
    skos:definition "A clinically diverse group of epilepsy syndromes characterized either by myoclonic seizures or by myoclonus in association with other seizure types. Myoclonic epilepsy syndromes are divided into three subtypes based on etiology: familial, cryptogenic, and symptomatic (i.e., occurring secondary to known disease processes such as infections, hypoxic-ischemic injuries, trauma, etc.) (MeSH)."^^xsd:string ;
    rdfs:subClassOf BIRNLEX:12718 ;
    NIFRID:createdDate "2007-10-08"^^xsd:string ;
    NIFRID:modifiedDate "2007-10-08"^^xsd:string ;
    NIFRID:hasBirnlexCurator NIFRID:Bill_Bug ;
    NIFRID:hasCurationStatus NIFRID:uncurated ;
    NIFRID:hasDefinitionSource NIFRID:MeSH_defSource ;
    NIFRID:hasExternalSource NIFRID:MeSH ;
    NIFRID:MeshUid "D020190"^^xsd:string ;
    NIFRID:nifID "_8.3_5.2.3"^^xsd:string ;
    NIFRID:putativeClassExtension "Cryptogenic Myoclonic Epilepsy"^^xsd:string,
        "Idiopathic Myoclonic Epilepsy"^^xsd:string,
        "Myoclonic Absence Epilepsy"^^xsd:string,
        "Myoclonic Astatic Epilepsy"^^xsd:string ;
    NIFRID:usageNote "MeSH includes implied subtypes"^^xsd:string .

BIRNLEX:12720 a owl:Class ;
    rdfs:label "Infantile Myoclonic Epilepsy"^^xsd:string ;
    skos:prefLabel "Infantile Myoclonic Epilepsy"^^xsd:string ;
    NIFRID:synonym "Early Childhood Myoclonic Epilepsy"^^xsd:string ;
    rdfs:subClassOf BIRNLEX:12719 ;
    NIFRID:createdDate "2007-10-08"^^xsd:string ;
    NIFRID:modifiedDate "2007-10-08"^^xsd:string ;
    NIFRID:hasBirnlexCurator NIFRID:Bill_Bug ;
    NIFRID:hasCurationStatus NIFRID:uncurated ;
    NIFRID:hasDefinitionSource NIFRID:MeSH_defSource ;
    NIFRID:hasExternalSource NIFRID:MeSH ;
    NIFRID:MeshUid "D004831"^^xsd:string ;
    NIFRID:putativeClassExtension "Benign Infantile Myoclonic Epilepsy"^^xsd:string,
        "Severe Infantile Myoclonic Epilepsy"^^xsd:string ;
    NIFRID:usageNote "MeSH includes implied subtypes based on disease severity"^^xsd:string .

BIRNLEX:12721 a owl:Class ;
    rdfs:label "Juvenile Myoclonic Epilepsy"^^xsd:string ;
    skos:prefLabel "Juvenile Myoclonic Epilepsy"^^xsd:string ;
    NIFRID:synonym "Adolescent Myoclonic Epilepsy"^^xsd:string,
        "Impulsive Petit Mal Epilepsy"^^xsd:string,
        "Janz Impulsive Petit Mal"^^xsd:string,
        "Janz Juvenile Myoclonic Epilepsy"^^xsd:string,
        "Janz Syndrome"^^xsd:string,
        "Juvenile Myoclonic Epilepsy of Janz"^^xsd:string ;
    skos:definition "A disorder characterized by the onset of myoclonus in adolescence, a marked increase in the incidence of absence seizures (see EPILEPSY, ABSENCE), and generalized major motor seizures (see EPILEPSY, TONIC-CLONIC). The myoclonic episodes tend to occur shortly after awakening. Seizures tend to be aggravated by sleep deprivation and alcohol consumption. Hereditary and sporadic forms have been identified (MeSH)."^^xsd:string ;
    rdfs:subClassOf BIRNLEX:12719 ;
    NIFRID:createdDate "2007-10-08"^^xsd:string ;
    NIFRID:modifiedDate "2007-10-08"^^xsd:string ;
    NIFRID:acronym "JME"^^xsd:string ;
    NIFRID:definingCitation "Adams et al., Principles of Neurology, 6th ed, p323"^^xsd:string ;
    NIFRID:hasBirnlexCurator NIFRID:Bill_Bug ;
    NIFRID:hasCurationStatus NIFRID:uncurated ;
    NIFRID:hasDefinitionSource NIFRID:MeSH_defSource ;
    NIFRID:hasExternalSource NIFRID:MeSH ;
    NIFRID:MeshUid "D020190"^^xsd:string .

BIRNLEX:12722 a owl:Class ;
    rdfs:label "Progressive Myoclonic Epilepsy"^^xsd:string ;
    skos:prefLabel "Progressive Myoclonic Epilepsy"^^xsd:string ;
    skos:definition "A heterogeneous group of primarily familial disorders characterized by myoclonic seizures, tonic-clonic seizures, ataxia, progressive intellectual deterioration, and neuronal degeneration. These include LAFORA DISEASE; MERRF SYNDROME; NEURONAL CEROID-LIPOFUSCINOSIS; sialidosis (see MUCOLIPIDOSES), and UNVERRICHT-LUNDBORG SYNDROME (MeSH)."^^xsd:string ;
    rdfs:subClassOf BIRNLEX:12719 ;
    NIFRID:createdDate "2007-10-08"^^xsd:string ;
    NIFRID:modifiedDate "2007-10-08"^^xsd:string ;
    NIFRID:hasBirnlexCurator NIFRID:Bill_Bug ;
    NIFRID:hasCurationStatus NIFRID:uncurated ;
    NIFRID:hasDefinitionSource NIFRID:MeSH_defSource ;
    NIFRID:hasExternalSource NIFRID:MeSH ;
    NIFRID:MeshUid "D020191"^^xsd:string ;
    NIFRID:putativeClassExtension "Action Myoclonus-Renal Failure Syndrome"^^xsd:string,
        "Atypical Inclusion-Body Disease"^^xsd:string,
        "Biotin-Responsive Encephalopathy"^^xsd:string,
        "Dentatorubral-Pallidoluysian Atrophy"^^xsd:string,
        "Familial Progressive Myoclonic Epilepsy"^^xsd:string,
        "May-White Syndrome"^^xsd:string ;
    NIFRID:usageNote "MeSH includes implied subtypes"^^xsd:string .

BIRNLEX:12723 a owl:Class ;
    rdfs:label "Lafora Progressive Myoclonic Epilepsy"^^xsd:string ;
    skos:prefLabel "Lafora Progressive Myoclonic Epilepsy"^^xsd:string ;
    NIFRID:synonym "Lafora Body Disease"^^xsd:string,
        "Lafora Disease"^^xsd:string,
        "Lafora Type Progressive Myoclonic Epilepsy"^^xsd:string,
        "Late Onset Lafora Body Disease"^^xsd:string ;
    skos:definition "A form of stimulus sensitive myoclonic epilepsy inherited as an autosomal recessive condition. The most common presenting feature is a single seizure in the second decade of life. This is followed by progressive myoclonus, myoclonic seizures, tonic-clonic seizures, focal occipital seizures, intellectual decline, and severe motor and coordination impairments. Most affected individuals do not live past the age of 25 years. Concentric amyloid (Lafora) bodies are found in neurons, liver, skin, bone, and muscle (MeSH)."^^xsd:string ;
    rdfs:subClassOf BIRNLEX:12722 ;
    NIFRID:createdDate "2007-10-08"^^xsd:string ;
    NIFRID:modifiedDate "2007-10-08"^^xsd:string ;
    NIFRID:definingCitation "Menkes, Textbook of Childhood Neurology, 5th ed, pp111-110"^^xsd:string ;
    NIFRID:hasBirnlexCurator NIFRID:Bill_Bug ;
    NIFRID:hasCurationStatus NIFRID:uncurated ;
    NIFRID:hasDefinitionSource NIFRID:MeSH_defSource ;
    NIFRID:hasExternalSource NIFRID:MeSH ;
    NIFRID:MeshUid "D020192"^^xsd:string ;
    NIFRID:usageNote "MeSH includes the following implied subtypes: Action Myoclonus-Renal Failure Syndrome; Atypical Inclusion-Body Disease; Biotin-Responsive Encephalopathy; Dentatorubral-Pallidoluysian Atrophy; Familial Progressive Myoclonic Epilepsy; May-White Syndrome"^^xsd:string .

BIRNLEX:12724 a owl:Class ;
    rdfs:label "MERRF Syndrome"^^xsd:string ;
    skos:prefLabel "MERRF Syndrome"^^xsd:string ;
    NIFRID:synonym "Fukuhara Disease"^^xsd:string,
        "Fukuhara Syndrome"^^xsd:string,
        "Myoclonic Epilepsy and Ragged Red Fibers"^^xsd:string,
        "Myoclonic Epilepsy with Ragged Red Fibers"^^xsd:string ;
    skos:definition "A mitochondrial encephalomyopathy characterized clinically by a mixed seizure disorder, myoclonus, progressive ataxia, spasticity, and a mild myopathy. Dysarthria, optic atrophy, growth retardation, deafness, and dementia may also occur. This condition tends to present in childhood and to be transmitted via maternal lineage. Muscle biopsies reveal ragged-red fibers and respiratory chain enzymatic defects (MeSH)."^^xsd:string ;
    rdfs:subClassOf BIRNLEX:12722 ;
    NIFRID:createdDate "2007-10-08"^^xsd:string ;
    NIFRID:modifiedDate "2007-10-08"^^xsd:string ;
    NIFRID:definingCitation "Adams et al., Principles of Neurology, 6th ed, p986"^^xsd:string ;
    NIFRID:hasBirnlexCurator NIFRID:Bill_Bug ;
    NIFRID:hasCurationStatus NIFRID:uncurated ;
    NIFRID:hasDefinitionSource NIFRID:MeSH_defSource ;
    NIFRID:hasExternalSource NIFRID:MeSH ;
    NIFRID:MeshUid "D017243"^^xsd:string .

BIRNLEX:12725 a owl:Class ;
    rdfs:label "Unverricht-Lundborg Syndrome"^^xsd:string ;
    skos:prefLabel "Unverricht-Lundborg Syndrome"^^xsd:string ;
    NIFRID:synonym "Baltic Myoclonus"^^xsd:string,
        "Baltic Myoclonus Epilepsy"^^xsd:string,
        "Lundborg-Unverricht Syndrome"^^xsd:string,
        "Mediterranean Myoclonic Epilepsy"^^xsd:string,
        "Unverricht Disease"^^xsd:string ;
    skos:definition "An autosomal recessive condition characterized by recurrent myoclonic and generalized seizures, ATAXIA, slowly progressive intellectual deterioration, dysarthria, and intention tremor. Myoclonic seizures are severe and continuous, and tend to be triggered by movement, stress, and sensory stimuli. The age of onset is between 8 and 13 years, and the condition is relatively frequent in the Baltic region, especially Finland (MeSH)."^^xsd:string ;
    rdfs:subClassOf BIRNLEX:12722 ;
    NIFRID:createdDate "2007-10-08"^^xsd:string ;
    NIFRID:modifiedDate "2007-10-08"^^xsd:string ;
    NIFRID:definingCitation "Menkes, Textbook of Child Neurology, 5th ed, pp109-110"^^xsd:string ;
    NIFRID:hasBirnlexCurator NIFRID:Bill_Bug ;
    NIFRID:hasCurationStatus NIFRID:uncurated ;
    NIFRID:hasDefinitionSource NIFRID:MeSH_defSource ;
    NIFRID:hasExternalSource NIFRID:MeSH ;
    NIFRID:MeshUid "D020194"^^xsd:string .

BIRNLEX:12726 a owl:Class ;
    rdfs:label "Partial Epilepsy"^^xsd:string ;
    skos:prefLabel "Partial Epilepsy"^^xsd:string ;
    NIFRID:synonym "Focal Epilepsy"^^xsd:string,
        "Focal Seizure Disorder"^^xsd:string,
        "Localization-Related Epilepsy"^^xsd:string,
        "Partial Seizure Disorder"^^xsd:string,
        "Simple Partial Epilepsy"^^xsd:string,
        "Simple Partial Seizure"^^xsd:string,
        "Simple Partial Seizure, Consciousness Preserved"^^xsd:string ;
    skos:definition "Conditions characterized by recurrent paroxysmal neuronal discharges which arise from a focal region of the brain. Partial seizures are divided into simple and complex, depending on whether consciousness is unaltered (simple partial seizure) or disturbed (complex partial seizure). Both types may feature a wide variety of motor, sensory, and autonomic symptoms. Partial seizures may be classified by associated clinical features or anatomic location of the seizure focus. A secondary generalized seizure refers to a partial seizure that spreads to involve the brain diffusely (MeSH)."^^xsd:string ;
    rdfs:subClassOf BIRNLEX:12718 ;
    NIFRID:createdDate "2007-10-08"^^xsd:string ;
    NIFRID:modifiedDate "2007-10-08"^^xsd:string ;
    NIFRID:definingCitation "Adams et al., Principles of Neurology, 6th ed, pp317"^^xsd:string ;
    NIFRID:hasBirnlexCurator NIFRID:Bill_Bug ;
    NIFRID:hasCurationStatus NIFRID:uncurated ;
    NIFRID:hasDefinitionSource NIFRID:MeSH_defSource ;
    NIFRID:hasExternalSource NIFRID:MeSH ;
    NIFRID:MeshUid "D004828"^^xsd:string ;
    NIFRID:nifID "_8.3_5.1"^^xsd:string ;
    NIFRID:putativeClassExtension "Abdominal Epilepsy"^^xsd:string,
        "Amygdalo-Hippocampal Epilepsy"^^xsd:string,
        "Childhood Benign Focal Epilepsy"^^xsd:string,
        "Childhood Benign Occipital Epilepsy"^^xsd:string,
        "Digestive Epilepsy; Gelastic Epilepsy"^^xsd:string,
        "Occipital Lobe Epilepsy"^^xsd:string,
        "Rhinencephalic Epilepsy"^^xsd:string,
        "Subclinical Seizures"^^xsd:string,
        "Uncinate Seizures"^^xsd:string ;
    NIFRID:usageNote "MeSH includes implied subtypes"^^xsd:string .

BIRNLEX:12727 a owl:Class ;
    rdfs:label "Simple Partial Epilepsy"^^xsd:string ;
    skos:prefLabel "Simple Partial Epilepsy"^^xsd:string ;
    NIFRID:synonym "Simple Partial Seizure"^^xsd:string,
        "Simple Partial Seizure, Consciousness Preserved"^^xsd:string ;
    rdfs:subClassOf BIRNLEX:12726 ;
    NIFRID:createdDate "2007-10-08"^^xsd:string ;
    NIFRID:modifiedDate "2007-10-08"^^xsd:string ;
    NIFRID:definingCitation "Adams et al., Principles of Neurology, 6th ed, pp317"^^xsd:string ;
    NIFRID:hasBirnlexCurator NIFRID:Bill_Bug ;
    NIFRID:hasCurationStatus NIFRID:uncurated ;
    NIFRID:hasDefinitionSource NIFRID:MeSH_defSource ;
    NIFRID:hasExternalSource NIFRID:MeSH ;
    NIFRID:MeshUid "D004828"^^xsd:string ;
    NIFRID:nifID "_8.3_5.1.1"^^xsd:string .

BIRNLEX:12728 a owl:Class ;
    rdfs:label "Complex Partial Epilepsy"^^xsd:string ;
    skos:prefLabel "Complex Partial Epilepsy"^^xsd:string ;
    NIFRID:synonym "Complex Partial Seizure Disorder"^^xsd:string ;
    skos:definition "A disorder characterized by recurrent partial seizures marked by impairment of cognition. During the seizure the individual may experience a wide variety of psychic phenomenon including formed hallucinations, illusions, deja vu, intense emotional feelings, confusion, and spatial disorientation. Focal motor activity, sensory alterations and AUTOMATISM may also occur. Complex partial seizures often originate from foci in one or both temporal lobes. The etiology may be idiopathic (cryptogenic partial complex epilepsy) or occur as a secondary manifestation of a focal cortical lesion (symptomatic partial complex epilepsy) (MeSH)."^^xsd:string ;
    rdfs:subClassOf BIRNLEX:12726 ;
    NIFRID:createdDate "2007-10-08"^^xsd:string ;
    NIFRID:modifiedDate "2007-10-08"^^xsd:string ;
    NIFRID:definingCitation "Adams et al., Principles of Neurology, 6th ed, pp317-8"^^xsd:string ;
    NIFRID:hasBirnlexCurator NIFRID:Bill_Bug ;
    NIFRID:hasCurationStatus NIFRID:uncurated ;
    NIFRID:hasDefinitionSource NIFRID:MeSH_defSource ;
    NIFRID:hasExternalSource NIFRID:MeSH ;
    NIFRID:MeshUid "D017029"^^xsd:string ;
    NIFRID:nifID "_8.3_5.1.2"^^xsd:string ;
    NIFRID:putativeClassExtension "Cryptogenic Partial Complex Epilepsy"^^xsd:string,
        "Psychic Equivalent Epilepsy"^^xsd:string,
        "Psychomotor Epilepsy"^^xsd:string,
        "Symptomatic Partial Complex Epilepsy"^^xsd:string ;
    NIFRID:usageNote "MeSH includes implied subtypes"^^xsd:string .

BIRNLEX:12729 a owl:Class ;
    rdfs:label "Frontal Lobe Epilepsy"^^xsd:string ;
    skos:prefLabel "Frontal Lobe Epilepsy"^^xsd:string ;
    NIFRID:synonym "Complex Partial Seizure Disorder"^^xsd:string ;
    skos:definition "A localization-related (focal) form of epilepsy characterized by seizures which arise in the frontal lobe. A variety of clinical syndromes exist depending on the exact location of the seizure focus. Simple or complex motor movements may occur, and most commonly involve the face and upper extremities. Seizures in the anterior frontal regions may be associated with head and eye turning, typically away from the side of origin of the seizure. Frontal lobe seizures may be idiopathic (cryptogenic) or caused by an identifiable disease process such as traumatic injuries, neoplasms, or other macroscopic or microscopic lesions of the frontal lobes (symptomatic frontal lobe seizures) (MeSH)."^^xsd:string ;
    rdfs:subClassOf BIRNLEX:12726 ;
    NIFRID:createdDate "2007-10-08"^^xsd:string ;
    NIFRID:modifiedDate "2007-10-08"^^xsd:string ;
    NIFRID:definingCitation "Adams et al., Principles of Neurology, 6th ed, pp318-9"^^xsd:string ;
    NIFRID:hasBirnlexCurator NIFRID:Bill_Bug ;
    NIFRID:hasCurationStatus NIFRID:uncurated ;
    NIFRID:hasDefinitionSource NIFRID:MeSH_defSource ;
    NIFRID:hasExternalSource NIFRID:MeSH ;
    NIFRID:MeshUid "D017034"^^xsd:string ;
    NIFRID:putativeClassExtension "Anterior Fronto-Polar Epilepsy"^^xsd:string,
        "Benign Frontal Childhood Epilepsy"^^xsd:string,
        "Cingulate Epilepsy"^^xsd:string,
        "Opercular Epilepsy"^^xsd:string,
        "Orbito-Frontal Epilepsy"^^xsd:string,
        "Supplementary Motor Epilepsy"^^xsd:string ;
    NIFRID:usageNote "MeSH includes implied subtypes"^^xsd:string .

BIRNLEX:12730 a owl:Class ;
    rdfs:label "Motor Partial Epilepsy"^^xsd:string ;
    skos:prefLabel "Motor Partial Epilepsy"^^xsd:string ;
    NIFRID:synonym "Focal Motor Epilepsy"^^xsd:string,
        "Hemimotor Epilepsy"^^xsd:string,
        "Hemimotor Seizure Disorder"^^xsd:string,
        "Motor Partial Seizure Disorder"^^xsd:string,
        "Motor Seizure Disorder"^^xsd:string,
        "Versive Seizures"^^xsd:string ;
    skos:definition "A disorder characterized by recurrent localized paroxysmal discharges of cerebral neurons that give rise to seizures that have motor manifestations. The majority of partial motor seizures originate in the FRONTAL LOBE (see also EPILEPSY, FRONTAL LOBE). Motor seizures may manifest as tonic or clonic movements involving the face, one limb or one side of the body. A variety of more complex patterns of movement, including abnormal posturing of extremities, may also occur (MeSH)."^^xsd:string ;
    rdfs:subClassOf BIRNLEX:12726 ;
    NIFRID:createdDate "2007-10-08"^^xsd:string ;
    NIFRID:modifiedDate "2007-10-08"^^xsd:string ;
    NIFRID:hasBirnlexCurator NIFRID:Bill_Bug ;
    NIFRID:hasCurationStatus NIFRID:uncurated ;
    NIFRID:hasDefinitionSource NIFRID:MeSH_defSource ;
    NIFRID:hasExternalSource NIFRID:MeSH ;
    NIFRID:MeshUid "D020938"^^xsd:string ;
    NIFRID:putativeClassExtension "Focal Clonic Seizure"^^xsd:string,
        "Focal Tonic Seizure"^^xsd:string ;
    NIFRID:usageNote "MeSH includes implied subtypes"^^xsd:string .

BIRNLEX:12731 a owl:Class ;
    rdfs:label "Sensory Partial Epilepsy"^^xsd:string ;
    skos:prefLabel "Sensory Partial Epilepsy"^^xsd:string ;
    NIFRID:synonym "Focal Sensory Seizure"^^xsd:string,
        "Partial Sensory Seizure"^^xsd:string,
        "Sensory Epilepsy"^^xsd:string,
        "Sensory Focal Seizure Disorder"^^xsd:string,
        "Sensory Partial Seizure Disorder"^^xsd:string,
        "Sensory Seizure Disorder"^^xsd:string,
        "Simple Partial Seizure, Special Sensory Symptoms"^^xsd:string ;
    skos:definition "A disorder characterized by recurrent focal onset seizures which have sensory (i.e., olfactory, visual, tactile, gustatory, or auditory) manifestations. Partial seizures that feature alterations of consciousness are referred to as complex partial seizures ( EPILEPSY, COMPLEX PARTIAL) (MeSH)."^^xsd:string ;
    rdfs:subClassOf BIRNLEX:12726 ;
    NIFRID:createdDate "2007-10-08"^^xsd:string ;
    NIFRID:modifiedDate "2007-10-08"^^xsd:string ;
    NIFRID:hasBirnlexCurator NIFRID:Bill_Bug ;
    NIFRID:hasCurationStatus NIFRID:uncurated ;
    NIFRID:hasDefinitionSource NIFRID:MeSH_defSource ;
    NIFRID:hasExternalSource NIFRID:MeSH ;
    NIFRID:MeshUid "D020937"^^xsd:string ;
    NIFRID:putativeClassExtension "Gustatory Partial Seizure"^^xsd:string,
        "Olfactory Partial Seizure"^^xsd:string,
        "Vertiginous Partial Seizure"^^xsd:string,
        "Visual Partial Seizure"^^xsd:string ;
    NIFRID:usageNote "MeSH includes implied subtypes based on effected sensory modality"^^xsd:string .

BIRNLEX:12732 a owl:Class ;
    rdfs:label "Rolandic Epilepsy"^^xsd:string ;
    skos:prefLabel "Rolandic Epilepsy"^^xsd:string ;
    NIFRID:synonym "Benign Childhood Epilepsy With Centro-Temporal Spikes"^^xsd:string,
        "Benign Rolandic Epilepsy"^^xsd:string,
        "Benign Rolandic Epilepsy of Childhood"^^xsd:string,
        "Centralopathic Epilepsy"^^xsd:string,
        "Centrotemporal Epilepsy"^^xsd:string,
        "Rolands Epilepsy"^^xsd:string,
        "Sylvian Epilepsy"^^xsd:string ;
    skos:definition "An autosomal dominant inherited partial epilepsy syndrome with onset between age 3 and 13 years. Seizures are characterized by PARESTHESIA and tonic or clonic activity of the lower face associated with drooling and dysarthria. The episodes tend to occur at night and may become secondarily generalized. In most cases, affected children are neurologically and developmentally normal. The electroencephalogram shows characteristic high-voltage sharp waves over the central temporal regions, which are more prominent during drowsiness and sleep. In general, seizures do not continue beyond mid-adolescence (MeSH)."^^xsd:string ;
    rdfs:subClassOf BIRNLEX:12726 ;
    NIFRID:createdDate "2007-10-08"^^xsd:string ;
    NIFRID:modifiedDate "2007-10-08"^^xsd:string ;
    NIFRID:definingCitation "Epilepsia 1998 39;Suppl 4:S32-S41"^^xsd:string ;
    NIFRID:hasBirnlexCurator NIFRID:Bill_Bug ;
    NIFRID:hasCurationStatus NIFRID:uncurated ;
    NIFRID:hasDefinitionSource NIFRID:MeSH_defSource ;
    NIFRID:hasExternalSource NIFRID:MeSH ;
    NIFRID:MeshUid "D019305"^^xsd:string .

BIRNLEX:12733 a owl:Class ;
    rdfs:label "Temporal Lobe Epilepsy"^^xsd:string ;
    skos:prefLabel "Temporal Lobe Epilepsy"^^xsd:string ;
    NIFRID:synonym "Childhood Benign Psychomotor Epilepsy"^^xsd:string,
        "Lateral Temporal Epilepsy"^^xsd:string,
        "Uncinate Epilepsy"^^xsd:string ;
    skos:definition "A localization-related (focal) form of epilepsy characterized by recurrent seizures that arise from foci within the temporal lobe, most commonly from its mesial aspect. A wide variety of psychic phenomena may be associated, including illusions, hallucinations, dyscognitive states, and affective experiences. The majority of complex partial seizures (see EPILEPSY, COMPLEX PARTIAL) originate from the temporal lobes. Temporal lobe seizures may be classified by etiology as cryptogenic, familial, or symptomatic (i.e., related to an identified disease process or lesion) (MeSH)."^^xsd:string ;
    rdfs:subClassOf BIRNLEX:12726 ;
    NIFRID:createdDate "2007-10-08"^^xsd:string ;
    NIFRID:modifiedDate "2007-10-08"^^xsd:string ;
    NIFRID:definingCitation "Adams et al., Principles of Neurology, 6th ed, p321"^^xsd:string ;
    NIFRID:hasBirnlexCurator NIFRID:Bill_Bug ;
    NIFRID:hasCurationStatus NIFRID:uncurated ;
    NIFRID:hasDefinitionSource NIFRID:MeSH_defSource ;
    NIFRID:hasExternalSource NIFRID:MeSH ;
    NIFRID:MeshUid "D004833"^^xsd:string .

BIRNLEX:12734 a owl:Class ;
    rdfs:label "Benign Neonatal Epilepsy"^^xsd:string ;
    skos:prefLabel "Benign Neonatal Epilepsy"^^xsd:string ;
    NIFRID:synonym "Benign Neonatal Convulsions"^^xsd:string ;
    skos:definition "A condition marked by recurrent seizures that occur during the first 4-6 weeks of life despite an otherwise benign neonatal course. Autosomal dominant familial and sporadic forms have been identified. Seizures generally consist of brief episodes of tonic posturing and other movements, apnea, eye deviations, and blood pressure fluctuations. These tend to remit after the 6th week of life. The risk of developing epilepsy at an older age is moderately increased in the familial form of this disorder (MeSH)."^^xsd:string ;
    rdfs:subClassOf BIRNLEX:12718 ;
    NIFRID:createdDate "2007-10-08"^^xsd:string ;
    NIFRID:modifiedDate "2007-10-08"^^xsd:string ;
    NIFRID:definingCitation "Adams et al., Principles of Neurology, 6th ed, pp317"^^xsd:string ;
    NIFRID:hasBirnlexCurator NIFRID:Bill_Bug ;
    NIFRID:hasCurationStatus NIFRID:uncurated ;
    NIFRID:hasDefinitionSource NIFRID:MeSH_defSource ;
    NIFRID:hasExternalSource NIFRID:MeSH ;
    NIFRID:MeshUid "D020936"^^xsd:string ;
    NIFRID:putativeClassExtension "Benign Familial Neonatal Epilepsy"^^xsd:string,
        "Benign Non-Familial Neonatal Convulsions"^^xsd:string,
        "Familial Benign Neonatal Convulsions"^^xsd:string,
        "Non-Familial Benign Neonatal Convulsions"^^xsd:string ;
    NIFRID:usageNote "MeSH includes implied subtypes based on genetic factors."^^xsd:string .

BIRNLEX:12735 a owl:Class ;
    rdfs:label "Familial Benign Neonatal Epilepsy"^^xsd:string ;
    skos:prefLabel "Familial Benign Neonatal Epilepsy"^^xsd:string ;
    NIFRID:synonym "Familial Benign Neonatal Convulsions"^^xsd:string ;
    rdfs:subClassOf BIRNLEX:12734 ;
    NIFRID:createdDate "2007-10-08"^^xsd:string ;
    NIFRID:modifiedDate "2007-10-08"^^xsd:string ;
    NIFRID:hasBirnlexCurator NIFRID:Bill_Bug ;
    NIFRID:hasCurationStatus NIFRID:uncurated ;
    NIFRID:hasDefinitionSource NIFRID:MeSH_defSource ;
    NIFRID:hasExternalSource NIFRID:MeSH ;
    NIFRID:MeshUid "D020936"^^xsd:string .

BIRNLEX:12736 a owl:Class ;
    rdfs:label "Non-Familial Benign Neonatal Epilepsy"^^xsd:string ;
    skos:prefLabel "Non-Familial Benign Neonatal Epilepsy"^^xsd:string ;
    NIFRID:synonym "Non-Familial Benign Neonatal Convulsions"^^xsd:string ;
    rdfs:subClassOf BIRNLEX:12734 ;
    NIFRID:createdDate "2007-10-08"^^xsd:string ;
    NIFRID:modifiedDate "2007-10-08"^^xsd:string ;
    NIFRID:hasBirnlexCurator NIFRID:Bill_Bug ;
    NIFRID:hasCurationStatus NIFRID:uncurated ;
    NIFRID:hasDefinitionSource NIFRID:MeSH_defSource ;
    NIFRID:hasExternalSource NIFRID:MeSH ;
    NIFRID:MeshUid "D020936"^^xsd:string .

BIRNLEX:12737 a owl:Class ;
    rdfs:label "Generalized Epilepsy"^^xsd:string ;
    skos:prefLabel "Generalized Epilepsy"^^xsd:string ;
    NIFRID:synonym "Generalized Onset Seizure Disorder"^^xsd:string,
        "Generalized Seizure Disorder"^^xsd:string,
        "Symptomatic Generalized Epilepsy"^^xsd:string ;
    skos:definition "Recurrent conditions characterized by epileptic seizures which arise diffusely and simultaneously from both hemispheres of the brain. Classification is generally based upon motor manifestations of the seizure (e.g., convulsive, nonconvulsive, akinetic, atonic, etc.) or etiology (e.g., idiopathic, cryptogenic, and symptomatic) (MeSH)."^^xsd:string ;
    rdfs:subClassOf BIRNLEX:12718 ;
    NIFRID:createdDate "2007-10-08"^^xsd:string ;
    NIFRID:modifiedDate "2007-10-08"^^xsd:string ;
    NIFRID:definingCitation "Mayo Clin Proc, 1996 Apr;71(4):405-14"^^xsd:string ;
    NIFRID:hasBirnlexCurator NIFRID:Bill_Bug ;
    NIFRID:hasCurationStatus NIFRID:uncurated ;
    NIFRID:hasDefinitionSource NIFRID:MeSH_defSource ;
    NIFRID:hasExternalSource NIFRID:MeSH ;
    NIFRID:MeshUid "D004829"^^xsd:string ;
    NIFRID:nifID "_8.3_5.2"^^xsd:string ;
    NIFRID:usageNote "\"generalized\" as opposed to \"focal\" or partial ( = EPILEPSIES, PARTIAL); prefer specific indentions; note X ref EPILEPSY, TONIC: do not confuse with EPILEPSY, TONIC-CLONIC"^^xsd:string,
        "MeSH includes implied subtypes"^^xsd:string .

BIRNLEX:12738 a owl:Class ;
    rdfs:label "Generalized Convulsive Epilepsy"^^xsd:string ;
    skos:prefLabel "Generalized Convulsive Epilepsy"^^xsd:string ;
    NIFRID:synonym "Convulsive Generalized Seizure Disorder"^^xsd:string ;
    rdfs:subClassOf BIRNLEX:12737 ;
    NIFRID:createdDate "2007-10-08"^^xsd:string ;
    NIFRID:modifiedDate "2007-10-08"^^xsd:string ;
    NIFRID:hasBirnlexCurator NIFRID:Bill_Bug ;
    NIFRID:hasCurationStatus NIFRID:uncurated ;
    NIFRID:hasDefinitionSource NIFRID:MeSH_defSource ;
    NIFRID:hasExternalSource NIFRID:MeSH ;
    NIFRID:MeshUid "D004829"^^xsd:string .

BIRNLEX:12739 a owl:Class ;
    rdfs:label "Generalized Nonconvulsive Epilepsy"^^xsd:string ;
    skos:prefLabel "Generalized Nonconvulsive Epilepsy"^^xsd:string ;
    NIFRID:synonym "Nonconvulsive Generalized Seizure Disorder"^^xsd:string ;
    rdfs:subClassOf BIRNLEX:12737 ;
    NIFRID:createdDate "2007-10-08"^^xsd:string ;
    NIFRID:modifiedDate "2007-10-08"^^xsd:string ;
    NIFRID:hasBirnlexCurator NIFRID:Bill_Bug ;
    NIFRID:hasCurationStatus NIFRID:uncurated ;
    NIFRID:hasDefinitionSource NIFRID:MeSH_defSource ;
    NIFRID:hasExternalSource NIFRID:MeSH ;
    NIFRID:MeshUid "D004829"^^xsd:string .

BIRNLEX:12740 a owl:Class ;
    rdfs:label "Atonic Epilepsy"^^xsd:string ;
    skos:prefLabel "Atonic Epilepsy"^^xsd:string ;
    NIFRID:synonym "Akinetic Epilepsy"^^xsd:string ;
    rdfs:subClassOf BIRNLEX:12739 ;
    NIFRID:createdDate "2007-10-08"^^xsd:string ;
    NIFRID:modifiedDate "2007-10-08"^^xsd:string ;
    NIFRID:hasBirnlexCurator NIFRID:Bill_Bug ;
    NIFRID:hasCurationStatus NIFRID:uncurated ;
    NIFRID:hasDefinitionSource NIFRID:MeSH_defSource ;
    NIFRID:hasExternalSource NIFRID:MeSH ;
    NIFRID:MeshUid "D004829"^^xsd:string ;
    NIFRID:nifID "_8.3_5.2.4"^^xsd:string .

BIRNLEX:12741 a owl:Class ;
    rdfs:label "Tonic Epilepsy"^^xsd:string ;
    skos:prefLabel "Tonic Epilepsy"^^xsd:string ;
    rdfs:subClassOf BIRNLEX:12739 ;
    NIFRID:createdDate "2007-10-08"^^xsd:string ;
    NIFRID:modifiedDate "2007-10-08"^^xsd:string ;
    NIFRID:hasBirnlexCurator NIFRID:Bill_Bug ;
    NIFRID:hasCurationStatus NIFRID:uncurated ;
    NIFRID:hasDefinitionSource NIFRID:MeSH_defSource ;
    NIFRID:hasExternalSource NIFRID:MeSH ;
    NIFRID:MeshUid "D004829"^^xsd:string .

BIRNLEX:12742 a owl:Class ;
    rdfs:label "Absence Epilepsy"^^xsd:string ;
    skos:prefLabel "Absence Epilepsy"^^xsd:string ;
    NIFRID:synonym "Absence Seizure"^^xsd:string,
        "Absence Seizure Disorder"^^xsd:string,
        "Akinetic Petit Mal"^^xsd:string,
        "Atonic Absence Seizure"^^xsd:string,
        "Childhood Absence Epilepsy"^^xsd:string,
        "Juvenile Absence Epilepsy"^^xsd:string,
        "Minor Epilepsy"^^xsd:string,
        "Petit Mal Convulsion"^^xsd:string,
        "Petit Mal Epilepsy"^^xsd:string,
        "Pykno-Epilepsy"^^xsd:string,
        "Pyknolepsy"^^xsd:string ;
    skos:definition "A childhood seizure disorder characterized by rhythmic electrical brain discharges of generalized onset. Clinical features include a sudden cessation of ongoing activity usually without loss of postural tone. Rhythmic blinking of the eyelids or lip smacking frequently accompanies the SEIZURES. The usual duration is 5-10 seconds, and multiple episodes may occur daily. Juvenile absence epilepsy is characterized by the juvenile onset of absence seizures and an increased incidence of myoclonus and tonic-clonic seizures (MeSH)."^^xsd:string ;
    rdfs:subClassOf BIRNLEX:12737 ;
    NIFRID:createdDate "2007-10-08"^^xsd:string ;
    NIFRID:modifiedDate "2007-10-08"^^xsd:string ;
    NIFRID:definingCitation "Menkes, Textbook of Child Neurology, 5th ed, p736"^^xsd:string ;
    NIFRID:hasBirnlexCurator NIFRID:Bill_Bug ;
    NIFRID:hasCurationStatus NIFRID:uncurated ;
    NIFRID:hasDefinitionSource NIFRID:MeSH_defSource ;
    NIFRID:hasExternalSource NIFRID:MeSH ;
    NIFRID:MeshUid "D004832"^^xsd:string ;
    NIFRID:nifID "_8.3_5.2.2"^^xsd:string ;
    NIFRID:putativeClassExtension "Atypical Absence Epilepsy"^^xsd:string ;
    NIFRID:usageNote "MeSH includes implied subtypes"^^xsd:string .

BIRNLEX:12743 a owl:Class ;
    rdfs:label "Tonic-Clonic Epilepsy"^^xsd:string ;
    skos:prefLabel "Tonic-Clonic Epilepsy"^^xsd:string ;
    NIFRID:synonym "Grand Mal Convulsions"^^xsd:string,
        "Grand Mal Convulsions Epilepsy"^^xsd:string,
        "Grand Mal Seizure Disorder"^^xsd:string,
        "Grand Mal Seizures Disorder"^^xsd:string,
        "Major Epilepsy"^^xsd:string,
        "Major Motor Seizure Disorder"^^xsd:string,
        "Tonic-Clonic Convulsion Disorder"^^xsd:string,
        "Tonic-Clonic Convulsion Syndrome"^^xsd:string,
        "Tonic-Clonic Convulsions"^^xsd:string,
        "Tonic-Clonic Seizure Disorder"^^xsd:string,
        "Tonic-Clonic Seizure Syndrome"^^xsd:string ;
    skos:definition "A generalized seizure disorder characterized by recurrent major motor seizures. The initial brief tonic phase is marked by trunk flexion followed by diffuse extension of the trunk and extremities. The clonic phase features rhythmic flexor contractions of the trunk and limbs, pupillary dilation, elevations of blood pressure and pulse, urinary incontinence, and tongue biting. This is followed by a profound state of depressed consciousness (post-ictal state) which gradually improves over minutes to hours. The disorder may be cryptogenic, familial, or symptomatic (caused by an identified disease process) (MeSH)."^^xsd:string ;
    rdfs:subClassOf BIRNLEX:12737 ;
    NIFRID:createdDate "2007-10-08"^^xsd:string ;
    NIFRID:modifiedDate "2007-10-08"^^xsd:string ;
    NIFRID:definingCitation "Adams et al., Principles of Neurology, 6th ed, p329"^^xsd:string ;
    NIFRID:hasBirnlexCurator NIFRID:Bill_Bug ;
    NIFRID:hasCurationStatus NIFRID:uncurated ;
    NIFRID:hasDefinitionSource NIFRID:MeSH_defSource ;
    NIFRID:hasExternalSource NIFRID:MeSH ;
    NIFRID:MeshUid "D004830"^^xsd:string ;
    NIFRID:nifID "_8.3_5.2.1"^^xsd:string ;
    NIFRID:putativeClassExtension "Cryptogenic Tonic-Clonic Epilepsy"^^xsd:string,
        "Symptomatic Tonic-Clonic Epilepsy"^^xsd:string ;
    NIFRID:usageNote "MeSH includes implied subtypes"^^xsd:string .

BIRNLEX:12744 a owl:Class ;
    rdfs:label "Infantile Spasms"^^xsd:string ;
    skos:prefLabel "Infantile Spasms"^^xsd:string ;
    NIFRID:synonym "Hypsarrhythmia"^^xsd:string,
        "Jackknife Seizures"^^xsd:string,
        "Lightning Attacks"^^xsd:string,
        "Nodding Spasm"^^xsd:string,
        "Salaam Attacks"^^xsd:string,
        "Salaam Seizures"^^xsd:string,
        "Spasmus Nutans"^^xsd:string,
        "West Syndrome"^^xsd:string ;
    skos:definition "An epileptic syndrome characterized by the triad of infantile spasms, hypsarrhythmia, and arrest of psychomotor development at seizure onset. The majority present between 3-12 months of age, with spasms consisting of combinations of brief flexor or extensor movements of the head, trunk, and limbs. The condition is divided into two forms: cryptogenic (idiopathic) and symptomatic (secondary to a known disease process such as intrauterine infections; nervous system abnormalities; BRAIN DISEASES, METABOLIC, INBORN; prematurity; perinatal asphyxia; TUBEROUS SCLEROSIS; etc.) (MeSH)."^^xsd:string ;
    rdfs:subClassOf BIRNLEX:12737 ;
    NIFRID:createdDate "2007-10-08"^^xsd:string ;
    NIFRID:modifiedDate "2007-10-08"^^xsd:string ;
    NIFRID:definingCitation "Menkes, Textbook of Child Neurology, 5th ed, pp744-8"^^xsd:string ;
    NIFRID:hasBirnlexCurator NIFRID:Bill_Bug ;
    NIFRID:hasCurationStatus NIFRID:uncurated ;
    NIFRID:hasDefinitionSource NIFRID:MeSH_defSource ;
    NIFRID:hasExternalSource NIFRID:MeSH ;
    NIFRID:MeshUid "D013036"^^xsd:string ;
    NIFRID:putativeClassExtension "Cryptogenic Infantile Spasms"^^xsd:string,
        "Cryptogenic West Syndrome"^^xsd:string,
        "Symptomatic Infantile Spasms"^^xsd:string,
        "Symptomatic West Syndrome"^^xsd:string ;
    NIFRID:usageNote "MeSH includes implied subtypes"^^xsd:string .

BIRNLEX:12745 a owl:Class ;
    rdfs:label "Post-Traumatic Epilepsy"^^xsd:string ;
    skos:prefLabel "Post-Traumatic Epilepsy"^^xsd:string ;
    NIFRID:synonym "Concussive Convulsion"^^xsd:string,
        "Impact Seizure"^^xsd:string,
        "Post-Traumatic Seizure Disorder"^^xsd:string,
        "Traumatic Epilepsy"^^xsd:string ;
    skos:definition "Recurrent seizures causally related to CRANIOCEREBRAL TRAUMA. Seizure onset may be immediate but is typically delayed for several days after the injury and may not occur for up to two years. The majority of seizures have a focal onset that correlates clinically with the site of brain injury. Cerebral cortex injuries caused by a penetrating foreign object ( CRANIOCEREBRAL TRAUMA, PENETRATING) are more likely than closed head injuries ( HEAD INJURIES, CLOSED) to be associated with epilepsy. Concussive convulsions are nonepileptic phenomena that occur immediately after head injury and are characterized by tonic and clonic movements (MeSH)."^^xsd:string ;
    rdfs:subClassOf BIRNLEX:12718 ;
    NIFRID:createdDate "2007-10-08"^^xsd:string ;
    NIFRID:modifiedDate "2007-10-08"^^xsd:string ;
    NIFRID:definingCitation "Rev Neurol 1998 Feb;26(150):256-261; Sports Med 1998 Feb;25(2):131-6"^^xsd:string ;
    NIFRID:hasBirnlexCurator NIFRID:Bill_Bug ;
    NIFRID:hasCurationStatus NIFRID:uncurated ;
    NIFRID:hasDefinitionSource NIFRID:MeSH_defSource ;
    NIFRID:hasExternalSource NIFRID:MeSH ;
    NIFRID:MeshUid "D004834"^^xsd:string ;
    NIFRID:putativeClassExtension "Early Post-Traumatic Seizures"^^xsd:string,
        "Late Post-Traumatic Seizures"^^xsd:string ;
    NIFRID:usageNote "MeSH includes implied subtypes"^^xsd:string .

BIRNLEX:12746 a owl:Class ;
    rdfs:label "Reflex Epilepsy"^^xsd:string ;
    skos:prefLabel "Reflex Epilepsy"^^xsd:string ;
    skos:definition "A subtype of epilepsy characterized by seizures that are consistently provoked by a certain specific stimulus. Auditory, visual, and somatosensory stimuli as well as the acts of writing, reading, eating, and decision making are examples of events or activities that may induce seizure activity in affected individuals (MeSH)."^^xsd:string ;
    rdfs:subClassOf BIRNLEX:12718 ;
    NIFRID:createdDate "2007-10-08"^^xsd:string ;
    NIFRID:modifiedDate "2007-10-08"^^xsd:string ;
    NIFRID:definingCitation "Neurol Clin 1994 Feb;12(1):57-8"^^xsd:string ;
    NIFRID:hasBirnlexCurator NIFRID:Bill_Bug ;
    NIFRID:hasCurationStatus NIFRID:uncurated ;
    NIFRID:hasDefinitionSource NIFRID:MeSH_defSource ;
    NIFRID:hasExternalSource NIFRID:MeSH ;
    NIFRID:MeshUid "D020195"^^xsd:string ;
    NIFRID:putativeClassExtension "Audiogenic Epilepsy"^^xsd:string,
        "Cursive Epilepsy"^^xsd:string,
        "Decision Making Reflex Epilepsy"^^xsd:string,
        "Eating-Induced Epilepsy"^^xsd:string,
        "Immersion Related Epilepsy"^^xsd:string,
        "Musicogenic Epilepsy"^^xsd:string,
        "Photosensitive Epilepsy"^^xsd:string,
        "Reading Epilepsy"^^xsd:string,
        "Tactile Reflex Epilepsy"^^xsd:string,
        "Visual Pattern Reflex Epilepsy"^^xsd:string,
        "Writing-Induced Reflex Epilepsy"^^xsd:string ;
    NIFRID:usageNote "MeSH includes implied subtypes based on the inducing stimulus"^^xsd:string .

BIRNLEX:12747 a owl:Class ;
    rdfs:label "Landau-Kleffner Syndrome"^^xsd:string ;
    skos:prefLabel "Landau-Kleffner Syndrome"^^xsd:string ;
    NIFRID:synonym "Acquired Childhoood Aphasia with Convulsive Disorder"^^xsd:string,
        "Acquired Epileptic Aphasia"^^xsd:string,
        "Landau-Kleffner Acquired Epileptiform Aphasia"^^xsd:string ;
    skos:definition "A syndrome characterized by the onset of isolated language dysfunction in otherwise normal children (age of onset 4-7 years) and epileptiform discharges on ELECTROENCEPHALOGRAPHY. Seizures, including atypical absence ( EPILEPSY, ABSENCE), complex partial ( EPILEPSY, COMPLEX PARTIAL), and other types may occur. The electroencephalographic abnormalities and seizures tend to resolve by puberty. The language disorder may also resolve although some individuals are left with severe language dysfunction, including APHASIA and auditory AGNOSIA (MeSH)."^^xsd:string ;
    rdfs:subClassOf BIRNLEX:12718 ;
    NIFRID:createdDate "2007-10-08"^^xsd:string ;
    NIFRID:modifiedDate "2007-10-08"^^xsd:string ;
    NIFRID:definingCitation "Menkes, Textbook of Child Neurology, 5th ed, pp749-50; J Child Neurol 1997 Nov;12(8):489-495"^^xsd:string ;
    NIFRID:hasBirnlexCurator NIFRID:Bill_Bug ;
    NIFRID:hasCurationStatus NIFRID:uncurated ;
    NIFRID:hasDefinitionSource NIFRID:MeSH_defSource ;
    NIFRID:hasExternalSource NIFRID:MeSH ;
    NIFRID:MeshUid "D018887"^^xsd:string .

BIRNLEX:12748 a owl:Class ;
    rdfs:label "Seizures"^^xsd:string ;
    skos:prefLabel "Seizures"^^xsd:string ;
    NIFRID:synonym "Convulsions"^^xsd:string,
        "Convulsive Seizures"^^xsd:string,
        "Non-Epileptic Convulsion"^^xsd:string ;
    skos:definition "Clinical or subclinical disturbances of cortical function due to a sudden, abnormal, excessive, and disorganized discharge of brain cells. Clinical manifestations include abnormal motor, sensory and psychic phenomena. Recurrent seizures are usually referred to as EPILEPSY or \"seizure disorder.\" (MeSH)."^^xsd:string ;
    rdfs:subClassOf BIRNLEX:12718 ;
    NIFRID:createdDate "2007-10-08"^^xsd:string ;
    NIFRID:modifiedDate "2007-10-08"^^xsd:string ;
    NIFRID:hasBirnlexCurator NIFRID:Bill_Bug ;
    NIFRID:hasCurationStatus NIFRID:uncurated ;
    NIFRID:hasDefinitionSource NIFRID:MeSH_defSource ;
    NIFRID:hasExternalSource NIFRID:MeSH ;
    NIFRID:MeshUid "D012640"^^xsd:string ;
    NIFRID:putativeClassExtension "Auditory Seizures"^^xsd:string,
        "Clonic Seizures"^^xsd:string,
        "Focal Seizures"^^xsd:string,
        "Generalized Seizures"^^xsd:string,
        "Gustatory Seizures"^^xsd:string,
        "Jacksonian Seizure"^^xsd:string,
        "Motor Seizures"^^xsd:string,
        "Olfactory Seizures"^^xsd:string,
        "Sensory Seizures"^^xsd:string,
        "Somatosensory Seizures"^^xsd:string,
        "Tonic Seizures"^^xsd:string,
        "Tonic-Clonic Seizures"^^xsd:string,
        "Vertiginous Seizures"^^xsd:string,
        "Vestibular Seizures"^^xsd:string,
        "Visual Seizures"^^xsd:string ;
    NIFRID:usageNote "MeSH includes implied subtypes based on the inducing stimulus"^^xsd:string .

BIRNLEX:12749 a owl:Class ;
    rdfs:label "Febrile Seizures"^^xsd:string ;
    skos:prefLabel "Febrile Seizures"^^xsd:string ;
    NIFRID:synonym "Febrile Convulsion Seizure"^^xsd:string,
        "Febrile Convulsions"^^xsd:string,
        "Febrile Fit"^^xsd:string,
        "Fever Convulsion"^^xsd:string,
        "Fever Seizure"^^xsd:string,
        "Pyrexial Convulsion"^^xsd:string,
        "Pyrexial Seizure"^^xsd:string ;
    skos:definition "Clinical or subclinical disturbances of cortical function due to a sudden, abnormal, excessive, and disorganized discharge of brain cells. Clinical manifestations include abnormal motor, sensory and psychic phenomena. Recurrent seizures are usually referred to as EPILEPSY or \"seizure disorder.\" (MeSH)."^^xsd:string ;
    rdfs:subClassOf BIRNLEX:12718 ;
    NIFRID:createdDate "2007-10-08"^^xsd:string ;
    NIFRID:modifiedDate "2007-10-08"^^xsd:string ;
    NIFRID:hasBirnlexCurator NIFRID:Bill_Bug ;
    NIFRID:hasCurationStatus NIFRID:uncurated ;
    NIFRID:hasDefinitionSource NIFRID:MeSH_defSource ;
    NIFRID:hasExternalSource NIFRID:MeSH ;
    NIFRID:MeshUid "D003294"^^xsd:string ;
    NIFRID:putativeClassExtension "Complex Febrile Seizure"^^xsd:string,
        "Simple Febrile Seizure"^^xsd:string ;
    NIFRID:usageNote "MeSH includes implied subtypes"^^xsd:string .

BIRNLEX:12750 a owl:Class ;
    rdfs:label "Status Epilepticus"^^xsd:string ;
    skos:prefLabel "Status Epilepticus"^^xsd:string ;
    skos:definition "A prolonged seizure or seizures repeated frequently enough to prevent recovery between episodes occurring over a period of 20-30 minutes. The most common subtype is generalized tonic-clonic status epilepticus, a potentially fatal condition associated with neuronal injury and respiratory and metabolic dysfunction. Nonconvulsive forms include petit mal status and complex partial status, which may manifest as behavioral disturbances. Simple partial status epilepticus consists of persistent motor, sensory, or autonomic seizures that do not impair cognition (see also EPILEPSIA PARTIALIS CONTINUA). Subclinical status epilepticus generally refers to seizures occurring in an unresponsive or comatose individual in the absence of overt signs of seizure activity (MeSH)."^^xsd:string ;
    rdfs:subClassOf BIRNLEX:12718 ;
    NIFRID:createdDate "2007-10-08"^^xsd:string ;
    NIFRID:modifiedDate "2007-10-08"^^xsd:string ;
    NIFRID:definingCitation "N Engl J Med 1998 Apr 2;338(14):970-6; Neurologia 1997 Dec;12 Suppl 6:25-30"^^xsd:string ;
    NIFRID:hasBirnlexCurator NIFRID:Bill_Bug ;
    NIFRID:hasCurationStatus NIFRID:uncurated ;
    NIFRID:hasDefinitionSource NIFRID:MeSH_defSource ;
    NIFRID:hasExternalSource NIFRID:MeSH ;
    NIFRID:MeshUid "D013226"^^xsd:string ;
    NIFRID:nifID "_8.3_5.3"^^xsd:string ;
    NIFRID:putativeClassExtension "Absence Status"^^xsd:string,
        "Complex Partial Status Epilepticus"^^xsd:string,
        "Electrographic Status Epilepticus"^^xsd:string,
        "Generalized Convulsive Status Epilepticus"^^xsd:string,
        "Generalized Status Epilepticus"^^xsd:string,
        "Grand Mal Status Epilepticus"^^xsd:string,
        "Non-Convulsive Status Epilepticus"^^xsd:string,
        "Petit Mal Status"^^xsd:string,
        "Simple Partial Status Epilepticus"^^xsd:string,
        "Subclinical Status Epilepticus"^^xsd:string ;
    NIFRID:usageNote "MeSH includes implied subtypes"^^xsd:string .

BIRNLEX:12751 a owl:Class ;
    rdfs:label "Epilepsia Partialis Continua"^^xsd:string ;
    skos:prefLabel "Epilepsia Partialis Continua"^^xsd:string ;
    NIFRID:synonym "Kojevnikov's Epilepsy"^^xsd:string,
        "Kojewnikow Syndrome"^^xsd:string,
        "Kozhevnikov Syndrome"^^xsd:string ;
    skos:definition "A variant of epilepsy characterized by continuous focal jerking of a body part over a period of hours, days, or even years without spreading to other body regions. Contractions may be aggravated by movement and are reduced, but not abolished during sleep. ELECTROENCEPHALOGRAPHY demonstrates epileptiform (spike and wave) discharges over the hemisphere opposite to the affected limb in most instances. The repetitive movements may originate from the CEREBRAL CORTEX or from subcortical structures (e.g., BRAIN STEM; BASAL GANGLIA). This condition is associated with Russian Spring and Summer encephalitis (see ENCEPHALITIS, TICK BORNE); Rasmussen syndrome (see ENCEPHALITIS); MULTIPLE SCLEROSIS; DIABETES MELLITUS; BRAIN NEOPLASMS; and CEREBROVASCULAR DISORDERS (MeSH)."^^xsd:string ;
    rdfs:subClassOf BIRNLEX:12750 ;
    NIFRID:createdDate "2007-10-08"^^xsd:string ;
    NIFRID:modifiedDate "2007-10-08"^^xsd:string ;
    NIFRID:definingCitation "Brain, 1996 April;119(pt2):393-407; Epilepsia 1993;34;Suppl 1:S29-S36; and Adams et al., Principles of Neurology, 6th ed, p319"^^xsd:string ;
    NIFRID:hasBirnlexCurator NIFRID:Bill_Bug ;
    NIFRID:hasCurationStatus NIFRID:uncurated ;
    NIFRID:hasDefinitionSource NIFRID:MeSH_defSource ;
    NIFRID:hasExternalSource NIFRID:MeSH ;
    NIFRID:MeshUid "D017036"^^xsd:string ;
    NIFRID:putativeClassExtension "Chronic Progressive Epilepsia Partialis Continua"^^xsd:string,
        "Progressive Variant Kozhevnikow Syndrome"^^xsd:string ;
    NIFRID:usageNote "MeSH includes implied subtypes"^^xsd:string .

BIRNLEX:12752 a owl:Class ;
    rdfs:label "Mood Disorder"^^xsd:string ;
    skos:prefLabel "Mood Disorder"^^xsd:string ;
    NIFRID:synonym "Affective Disorder"^^xsd:string ;
    skos:definition "Those disorders that have a disturbance in mood as their predominant feature. (MeSH)."^^xsd:string ;
    rdfs:subClassOf BIRNLEX:12669 ;
    skos:editorialNote "human only; do not confuse with AFFECTIVE SYMPTOMS (MeSH)."^^xsd:string ;
    NIFRID:createdDate "2007-10-05"^^xsd:string ;
    NIFRID:modifiedDate "2007-10-05"^^xsd:string ;
    NIFRID:hasBirnlexCurator NIFRID:Bill_Bug ;
    NIFRID:hasCurationStatus NIFRID:uncurated ;
    NIFRID:hasDefinitionSource NIFRID:MeSH_defSource ;
    NIFRID:hasExternalSource NIFRID:MeSH ;
    NIFRID:MeshUid "D019964"^^xsd:string .

BIRNLEX:12753 a owl:Class ;
    rdfs:label "Affective Psychotic Disorder"^^xsd:string ;
    skos:prefLabel "Affective Psychotic Disorder"^^xsd:string ;
    NIFRID:synonym "Affective Psychosis"^^xsd:string,
        "Psychotic Mood Disorder"^^xsd:string,
        "Reactive Psychotic Depression"^^xsd:string ;
    skos:definition "Disorders in which the essential feature is a severe disturbance in mood (depression, anxiety, elation, and excitement) accompanied by psychotic symptoms such as delusions, hallucinations, gross impairment in reality testing, etc. (MeSH)."^^xsd:string ;
    rdfs:subClassOf BIRNLEX:12752 ;
    NIFRID:createdDate "2007-10-08"^^xsd:string ;
    NIFRID:modifiedDate "2007-10-08"^^xsd:string ;
    NIFRID:hasBirnlexCurator NIFRID:Bill_Bug ;
    NIFRID:hasCurationStatus NIFRID:uncurated ;
    NIFRID:hasDefinitionSource NIFRID:MeSH_defSource ;
    NIFRID:hasExternalSource NIFRID:MeSH ;
    NIFRID:MeshUid "D000341"^^xsd:string .

BIRNLEX:12754 a owl:Class ;
    rdfs:label "Bipolar Disorder"^^xsd:string ;
    skos:prefLabel "Bipolar Disorder"^^xsd:string ;
    NIFRID:synonym "Affective Bipolar Psychosis"^^xsd:string,
        "Bipolar Depression"^^xsd:string,
        "Manic-Depressive Psychosis"^^xsd:string ;
    skos:definition "A major affective disorder marked by severe mood swings (manic or major depressive episodes) and a tendency to remission and recurrence (MeSH)."^^xsd:string ;
    rdfs:subClassOf BIRNLEX:12753 ;
    NIFRID:createdDate "2007-10-08"^^xsd:string ;
    NIFRID:modifiedDate "2007-10-08"^^xsd:string ;
    NIFRID:hasBirnlexCurator NIFRID:Bill_Bug ;
    NIFRID:hasCurationStatus NIFRID:uncurated ;
    NIFRID:hasDefinitionSource NIFRID:MeSH_defSource ;
    NIFRID:hasExternalSource NIFRID:MeSH ;
    NIFRID:MeshUid "D001714"^^xsd:string ;
    NIFRID:nifID "_8.3_11.3"^^xsd:string ;
    NIFRID:putativeClassExtension "Mania"^^xsd:string,
        "Manic Disorder"^^xsd:string,
        "Manic State"^^xsd:string ;
    NIFRID:usageNote "MeSH includes implied subcomponents"^^xsd:string .

BIRNLEX:12755 a owl:Class ;
    rdfs:label "Cyclothymic Disorder"^^xsd:string ;
    skos:prefLabel "Cyclothymic Disorder"^^xsd:string ;
    NIFRID:synonym "Cyclothymic Personality"^^xsd:string ;
    skos:definition "An affective disorder characterized by periods of depression and hypomania. These may be separated by periods of normal mood (MeSH)."^^xsd:string ;
    rdfs:subClassOf BIRNLEX:12754 ;
    NIFRID:createdDate "2007-10-08"^^xsd:string ;
    NIFRID:modifiedDate "2007-10-08"^^xsd:string ;
    NIFRID:hasBirnlexCurator NIFRID:Bill_Bug ;
    NIFRID:hasCurationStatus NIFRID:uncurated ;
    NIFRID:hasDefinitionSource NIFRID:MeSH_defSource ;
    NIFRID:hasExternalSource NIFRID:MeSH ;
    NIFRID:MeshUid "D003527"^^xsd:string .

BIRNLEX:12756 a owl:Class ;
    rdfs:label "Depressive Disorder"^^xsd:string ;
    skos:prefLabel "Depressive Disorder"^^xsd:string ;
    NIFRID:synonym "Depressive Neurosis"^^xsd:string,
        "Depressive Syndrome"^^xsd:string,
        "Endogenous Depression"^^xsd:string,
        "Melancholia"^^xsd:string,
        "Neurotic Depression"^^xsd:string,
        "Unipolar Depression"^^xsd:string ;
    skos:definition "An affective disorder manifested by either a dysphoric mood or loss of interest or pleasure in usual activities. The mood disturbance is prominent and relatively persistent (MeSH)."^^xsd:string ;
    rdfs:subClassOf BIRNLEX:12752 ;
    NIFRID:createdDate "2007-10-08"^^xsd:string ;
    NIFRID:modifiedDate "2007-10-08"^^xsd:string ;
    NIFRID:hasBirnlexCurator NIFRID:Bill_Bug ;
    NIFRID:hasCurationStatus NIFRID:uncurated ;
    NIFRID:hasDefinitionSource NIFRID:MeSH_defSource ;
    NIFRID:hasExternalSource NIFRID:MeSH ;
    NIFRID:MeshUid "D003866"^^xsd:string ;
    NIFRID:nifID "_8.3_11.2"^^xsd:string .

BIRNLEX:12757 a owl:Class ;
    rdfs:label "Postpartum Depression"^^xsd:string ;
    skos:prefLabel "Postpartum Depression"^^xsd:string ;
    NIFRID:synonym "Post-Natal Depression"^^xsd:string,
        "Post-Partum Depression"^^xsd:string ;
    skos:definition "Depression in POSTPARTUM WOMEN, usually within four weeks after giving birth ( PARTURITION). The degree of depression ranges from mild transient depression to neurotic or psychotic depressive disorders (MeSH)."^^xsd:string ;
    rdfs:subClassOf BIRNLEX:12756 ;
    NIFRID:createdDate "2007-10-08"^^xsd:string ;
    NIFRID:modifiedDate "2007-10-08"^^xsd:string ;
    NIFRID:definingCitation "DSM-IV, p386"^^xsd:string ;
    NIFRID:hasBirnlexCurator NIFRID:Bill_Bug ;
    NIFRID:hasCurationStatus NIFRID:uncurated ;
    NIFRID:hasDefinitionSource NIFRID:MeSH_defSource ;
    NIFRID:hasExternalSource NIFRID:MeSH ;
    NIFRID:MeshUid "D019052"^^xsd:string .

BIRNLEX:12758 a owl:Class ;
    rdfs:label "Major Depressive Disorder"^^xsd:string ;
    skos:prefLabel "Major Depressive Disorder"^^xsd:string ;
    NIFRID:synonym "Involutional Depression"^^xsd:string,
        "Involutional Melancholia"^^xsd:string,
        "Involutional Paraphrenia"^^xsd:string,
        "Involutional Psychosis"^^xsd:string ;
    skos:definition "Marked depression appearing in the involution period and characterized by hallucinations, delusions, paranoia, and agitation. (MeSH)."^^xsd:string ;
    rdfs:subClassOf BIRNLEX:12756 ;
    NIFRID:createdDate "2007-10-08"^^xsd:string ;
    NIFRID:modifiedDate "2007-10-08"^^xsd:string ;
    NIFRID:hasBirnlexCurator NIFRID:Bill_Bug ;
    NIFRID:hasCurationStatus NIFRID:uncurated ;
    NIFRID:hasDefinitionSource NIFRID:MeSH_defSource ;
    NIFRID:hasExternalSource NIFRID:MeSH ;
    NIFRID:MeshUid "D003865"^^xsd:string .

BIRNLEX:12759 a owl:Class ;
    rdfs:label "Dysthymic Disorder"^^xsd:string ;
    skos:prefLabel "Dysthymic Disorder"^^xsd:string ;
    skos:definition "Chronically depressed mood that occurs for most of the day more days than not for at least 2 years. The required minimum duration in children to make this diagnosis is 1 year. During periods of depressed mood, at least 2 of the following additional symptoms are present: poor appetite or overeating, insomnia or hypersomnia, low energy or fatigue, low self esteem, poor concentration or difficulty making decisions, and feelings of hopelessness (MeSH)."^^xsd:string ;
    rdfs:subClassOf BIRNLEX:12756 ;
    NIFRID:createdDate "2007-10-08"^^xsd:string ;
    NIFRID:modifiedDate "2007-10-08"^^xsd:string ;
    NIFRID:hasBirnlexCurator NIFRID:Bill_Bug ;
    NIFRID:hasCurationStatus NIFRID:uncurated ;
    NIFRID:hasDefinitionSource NIFRID:MeSH_defSource ;
    NIFRID:hasExternalSource NIFRID:MeSH ;
    NIFRID:MeshUid "D019263"^^xsd:string .

BIRNLEX:12760 a owl:Class ;
    rdfs:label "Seasonal Affective Disorder"^^xsd:string ;
    skos:prefLabel "Seasonal Affective Disorder"^^xsd:string ;
    NIFRID:synonym "Seasonal Mood Disorder"^^xsd:string ;
    skos:definition "A syndrome characterized by depressions that recur annually at the same time each year, usually during the winter months. Other symptoms include anxiety, irritability, decreased energy, increased appetite (carbohydrate cravings), increased duration of sleep, and weight gain. SAD (seasonal affective disorder) can be treated by daily exposure to bright artificial lights ( PHOTOTHERAPY), during the season of recurrence (MeSH)."^^xsd:string ;
    rdfs:subClassOf BIRNLEX:12756 ;
    NIFRID:createdDate "2007-10-08"^^xsd:string ;
    NIFRID:modifiedDate "2007-10-08"^^xsd:string ;
    NIFRID:hasBirnlexCurator NIFRID:Bill_Bug ;
    NIFRID:hasCurationStatus NIFRID:uncurated ;
    NIFRID:hasDefinitionSource NIFRID:MeSH_defSource ;
    NIFRID:hasExternalSource NIFRID:MeSH ;
    NIFRID:MeshUid "D016574"^^xsd:string .

BIRNLEX:12761 a owl:Class ;
    rdfs:label "Psychotic Disorder"^^xsd:string ;
    skos:prefLabel "Psychotic Disorder"^^xsd:string ;
    NIFRID:synonym "Psychosis"^^xsd:string ;
    skos:definition "Those disorders that have a disturbance in mood as their predominant feature. (MeSH)."^^xsd:string ;
    rdfs:subClassOf BIRNLEX:12669 ;
    NIFRID:createdDate "2007-10-08"^^xsd:string ;
    NIFRID:modifiedDate "2007-10-08"^^xsd:string ;
    NIFRID:hasBirnlexCurator NIFRID:Bill_Bug ;
    NIFRID:hasCurationStatus NIFRID:uncurated ;
    NIFRID:hasDefinitionSource NIFRID:MeSH_defSource ;
    NIFRID:hasExternalSource NIFRID:MeSH ;
    NIFRID:MeshUid "D011618"^^xsd:string ;
    NIFRID:nifID "_8.3_11.5"^^xsd:string ;
    NIFRID:putativeClassExtension "Brief Reactive Psychosis"^^xsd:string,
        "Schizoaffective Disorder"^^xsd:string,
        "Schizophreniform Disorder"^^xsd:string ;
    NIFRID:usageNote "MeSH includes implied subcomponents"^^xsd:string .

BIRNLEX:12762 a owl:Class ;
    rdfs:label "Capgras Syndrome"^^xsd:string ;
    skos:prefLabel "Capgras Syndrome"^^xsd:string ;
    rdfs:subClassOf BIRNLEX:12761 ;
    NIFRID:createdDate "2007-10-08"^^xsd:string ;
    NIFRID:modifiedDate "2007-10-08"^^xsd:string ;
    NIFRID:externallySourcedDefinition "A psychotic disorder characterized by the patient's belief that acquaintances or closely related persons have been replaced by doubles or imposters. (MeSH)"^^xsd:string ;
    NIFRID:hasBirnlexCurator NIFRID:Jessica_Turner ;
    NIFRID:hasCurationStatus NIFRID:uncurated ;
    NIFRID:hasExternalSource NIFRID:UMLS ;
    NIFRID:MeshUid "D002194"^^xsd:string .

BIRNLEX:12763 a owl:Class ;
    rdfs:label "Paranoid Disorder"^^xsd:string ;
    skos:prefLabel "Paranoid Disorder"^^xsd:string ;
    NIFRID:synonym "Paranoia"^^xsd:string,
        "Paranoid Psychosis"^^xsd:string,
        "Psychosis"^^xsd:string ;
    rdfs:subClassOf BIRNLEX:12761 ;
    NIFRID:createdDate "2007-10-08"^^xsd:string ;
    NIFRID:modifiedDate "2007-10-08"^^xsd:string ;
    NIFRID:externallySourcedDefinition "Chronic mental disorders in which there has been an insidious development of a permanent and unshakeable delusional system (persecutory delusions or delusions of jealousy), accompanied by preservation of clear and orderly thinking. Emotional responses and behavior are consistent with the delusional state. (MeSH)"^^xsd:string ;
    NIFRID:hasBirnlexCurator NIFRID:Jessica_Turner ;
    NIFRID:hasCurationStatus NIFRID:uncurated ;
    NIFRID:hasExternalSource NIFRID:UMLS ;
    NIFRID:MeshUid "D010259"^^xsd:string .

BIRNLEX:12764 a owl:Class ;
    rdfs:label "Catatonic Schizophrenia"^^xsd:string ;
    skos:prefLabel "Catatonic Schizophrenia"^^xsd:string ;
    rdfs:subClassOf BIRNLEX:2104 ;
    NIFRID:createdDate "2007-10-08"^^xsd:string ;
    NIFRID:modifiedDate "2007-10-08"^^xsd:string ;
    NIFRID:externallySourcedDefinition "A type of schizophrenia characterized by abnormality of motor behavior which may involve particular forms of stupor, rigidity, excitement or inappropriate posture (MeSH)"^^xsd:string ;
    NIFRID:hasBirnlexCurator NIFRID:Jessica_Turner ;
    NIFRID:hasCurationStatus NIFRID:uncurated ;
    NIFRID:hasExternalSource NIFRID:UMLS ;
    NIFRID:MeshUid "D012560"^^xsd:string .

BIRNLEX:12765 a owl:Class ;
    rdfs:label "Disorganized Schizophrenia"^^xsd:string ;
    skos:prefLabel "Disorganized Schizophrenia"^^xsd:string ;
    NIFRID:synonym "Hebephrenic Schizophrenia"^^xsd:string ;
    rdfs:subClassOf BIRNLEX:2104 ;
    NIFRID:createdDate "2007-10-08"^^xsd:string ;
    NIFRID:modifiedDate "2007-10-08"^^xsd:string ;
    NIFRID:definingCitation "Dorland, 27th ed"^^xsd:string ;
    NIFRID:externallySourcedDefinition "A type of schizophrenia characterized by frequent incoherence; marked loosening of associations, or grossly disorganized behavior and flat or grossly inappropriate affect that does not meet the criteria for the catatonic type; associated features include extreme social withdrawal, grimacing, mannerisms, mirror gazing, inappropriate giggling, and other odd behavior (MeSH)"^^xsd:string ;
    NIFRID:hasBirnlexCurator NIFRID:Jessica_Turner ;
    NIFRID:hasCurationStatus NIFRID:uncurated ;
    NIFRID:hasExternalSource NIFRID:UMLS ;
    NIFRID:MeshUid "D012562"^^xsd:string .

BIRNLEX:12766 a owl:Class ;
    rdfs:label "Paranoid Schizophrenia"^^xsd:string ;
    skos:prefLabel "Paranoid Schizophrenia"^^xsd:string ;
    NIFRID:synonym "Delusional Disorder"^^xsd:string ;
    rdfs:subClassOf BIRNLEX:2104 ;
    NIFRID:createdDate "2007-10-08"^^xsd:string ;
    NIFRID:modifiedDate "2007-10-08"^^xsd:string ;
    NIFRID:externallySourcedDefinition "A chronic form of schizophrenia characterized primarily by the presence of persecutory or grandiose delusions, often associated with hallucination (MeSH)"^^xsd:string ;
    NIFRID:hasBirnlexCurator NIFRID:Jessica_Turner ;
    NIFRID:hasCurationStatus NIFRID:uncurated ;
    NIFRID:hasExternalSource NIFRID:UMLS ;
    NIFRID:MeshUid "D012563"^^xsd:string .

BIRNLEX:12767 a owl:Class ;
    rdfs:label "Shared Paranoid Disorder"^^xsd:string ;
    skos:prefLabel "Shared Paranoid Disorder"^^xsd:string ;
    NIFRID:synonym "Folie a Deux"^^xsd:string,
        "Folie a Trois"^^xsd:string,
        "Shared Psychotic Disorder"^^xsd:string ;
    rdfs:subClassOf BIRNLEX:2104 ;
    NIFRID:createdDate "2007-10-08"^^xsd:string ;
    NIFRID:modifiedDate "2007-10-08"^^xsd:string ;
    NIFRID:externallySourcedDefinition "A condition in which two closely related persons, usually in the same family, share the same delusions. (MeSH)"^^xsd:string ;
    NIFRID:hasBirnlexCurator NIFRID:Jessica_Turner ;
    NIFRID:hasCurationStatus NIFRID:uncurated ;
    NIFRID:hasExternalSource NIFRID:UMLS ;
    NIFRID:MeshUid "D012753"^^xsd:string .

BIRNLEX:12768 a owl:Class ;
    rdfs:label "Pervasive Development Disorder"^^xsd:string ;
    skos:prefLabel "Pervasive Development Disorder"^^xsd:string ;
    NIFRID:synonym "Pervasive Child Development Disorder"^^xsd:string ;
    skos:definition "Severe distortions in the development of many basic psychological functions that are not normal for any stage in development. These distortions are manifested in sustained social impairment, speech abnormalities, and peculiar motor movements (MeSH)."^^xsd:string ;
    rdfs:subClassOf BIRNLEX:12669 ;
    NIFRID:createdDate "2007-10-08"^^xsd:string ;
    NIFRID:modifiedDate "2007-10-08"^^xsd:string ;
    NIFRID:hasBirnlexCurator NIFRID:Bill_Bug ;
    NIFRID:hasCurationStatus NIFRID:uncurated ;
    NIFRID:hasDefinitionSource NIFRID:MeSH_defSource ;
    NIFRID:hasExternalSource NIFRID:MeSH ;
    NIFRID:MeshUid "D002659"^^xsd:string .

BIRNLEX:12769 a owl:Class ;
    rdfs:label "Asperger Syndrome"^^xsd:string ;
    skos:prefLabel "Asperger Syndrome"^^xsd:string ;
    NIFRID:synonym "Asperger's Disorder"^^xsd:string ;
    skos:definition "A childhood disorder predominately affecting boys and similar to autism ( AUTISTIC DISORDER). It is characterized by severe, sustained, clinically significant impairment of social interaction, and restricted repetitive and stereotyped patterns of behavior. In contrast to autism, there are no clinically significant delays in language or cognitive development (MeSH)."^^xsd:string ;
    rdfs:subClassOf BIRNLEX:12768 ;
    NIFRID:createdDate "2007-10-08"^^xsd:string ;
    NIFRID:modifiedDate "2007-10-08"^^xsd:string ;
    NIFRID:definingCitation "DSM-IV"^^xsd:string ;
    NIFRID:hasBirnlexCurator NIFRID:Bill_Bug ;
    NIFRID:hasCurationStatus NIFRID:uncurated ;
    NIFRID:hasDefinitionSource NIFRID:MeSH_defSource ;
    NIFRID:hasExternalSource NIFRID:MeSH ;
    NIFRID:MeshUid "D020817"^^xsd:string .

BIRNLEX:12770 a owl:Class ;
    rdfs:label "Rett Syndrome"^^xsd:string ;
    skos:prefLabel "Rett Syndrome"^^xsd:string ;
    NIFRID:synonym "Autism-Dementia-Ataxia-Loss of Purposeful Hand Use Syndrome"^^xsd:string,
        "Cerebroatrophic Hyperammonemia"^^xsd:string,
        "Rett Disorder"^^xsd:string ;
    skos:definition "An inherited neurological developmental disorder that is associated with X-LINKED INHERITANCE and may be lethal in utero to hemizygous males. The affected female is normal until the age of 6-25 months when progressive loss of voluntary control of hand movements and communication skills; ATAXIA; SEIZURES; autistic behavior; intermittent HYPERVENTILATION; and HYPERAMMONEMIA appear (MeSH)."^^xsd:string ;
    rdfs:subClassOf BIRNLEX:12768 ;
    NIFRID:createdDate "2007-10-08"^^xsd:string ;
    NIFRID:modifiedDate "2007-10-08"^^xsd:string ;
    NIFRID:definingCitation "Menkes, Textbook of Child Neurology, 5th ed, p199"^^xsd:string ;
    NIFRID:hasBirnlexCurator NIFRID:Bill_Bug ;
    NIFRID:hasCurationStatus NIFRID:uncurated ;
    NIFRID:hasDefinitionSource NIFRID:MeSH_defSource ;
    NIFRID:hasExternalSource NIFRID:MeSH ;
    NIFRID:MeshUid "D015518"^^xsd:string .

BIRNLEX:12771 a owl:Class ;
    rdfs:label "Consciousness Disorder"^^xsd:string ;
    skos:prefLabel "Consciousness Disorder"^^xsd:string ;
    NIFRID:synonym "Altered Level of Consciousness"^^xsd:string,
        "Depressed Level of Consciousness"^^xsd:string,
        "Semiconsciousness"^^xsd:string ;
    skos:definition "Organic mental disorders in which there is impairment of the ability to maintain awareness of self and environment and to respond to environmental stimuli. Dysfunction of the cerebral hemispheres or brain stem RETICULAR FORMATION may result in this condition (MeSH)."^^xsd:string ;
    rdfs:subClassOf BIRNLEX:12669 ;
    NIFRID:createdDate "2007-10-08"^^xsd:string ;
    NIFRID:modifiedDate "2007-10-08"^^xsd:string ;
    NIFRID:hasBirnlexCurator NIFRID:Bill_Bug ;
    NIFRID:hasCurationStatus NIFRID:uncurated ;
    NIFRID:hasDefinitionSource NIFRID:MeSH_defSource ;
    NIFRID:hasExternalSource NIFRID:MeSH ;
    NIFRID:MeshUid "D003244"^^xsd:string ;
    NIFRID:nifID "_8.3_17"^^xsd:string .

BIRNLEX:12772 a owl:Class ;
    rdfs:label "Unconsciousness"^^xsd:string ;
    skos:prefLabel "Unconsciousness"^^xsd:string ;
    NIFRID:synonym "Loss of Consciousness"^^xsd:string,
        "Unconscious State"^^xsd:string ;
    skos:definition "Organic mental disorders in which there is impairment of the ability to maintain awareness of self and environment and to respond to environmental stimuli. Dysfunction of the cerebral hemispheres or brain stem RETICULAR FORMATION may result in this condition (MeSH)."^^xsd:string ;
    rdfs:subClassOf BIRNLEX:12669 ;
    NIFRID:createdDate "2007-10-08"^^xsd:string ;
    NIFRID:modifiedDate "2007-10-08"^^xsd:string ;
    NIFRID:hasBirnlexCurator NIFRID:Bill_Bug ;
    NIFRID:hasCurationStatus NIFRID:uncurated ;
    NIFRID:hasDefinitionSource NIFRID:MeSH_defSource ;
    NIFRID:hasExternalSource NIFRID:MeSH ;
    NIFRID:MeshUid "D014474"^^xsd:string .

BIRNLEX:12773 a owl:Class ;
    rdfs:label "Coma"^^xsd:string ;
    skos:prefLabel "Coma"^^xsd:string ;
    NIFRID:synonym "Comatose"^^xsd:string,
        "Loss of Consciousness"^^xsd:string,
        "Pseudocoma"^^xsd:string ;
    skos:definition "A profound state of unconsciousness associated with depressed cerebral activity from which the individual cannot be aroused. Coma generally occurs when there is dysfunction or injury involving both cerebral hemispheres or the brain stem RETICULAR FORMATION.  This includes Feigned coma or psychogenic coma. These patients appear comatose (i.e., unresponsive, unarousable, or both) but have no structural lesion, metabolic or toxic disorder (MeSH)."^^xsd:string ;
    rdfs:subClassOf BIRNLEX:12669 ;
    NIFRID:createdDate "2007-10-08"^^xsd:string ;
    NIFRID:modifiedDate "2007-10-08"^^xsd:string ;
    NIFRID:hasBirnlexCurator NIFRID:Bill_Bug ;
    NIFRID:hasCurationStatus NIFRID:uncurated ;
    NIFRID:hasDefinitionSource NIFRID:MeSH_defSource ;
    NIFRID:hasExternalSource NIFRID:MeSH ;
    NIFRID:MeshUid "D003128"^^xsd:string ;
    NIFRID:nifID "_8.3_17.3"^^xsd:string .

BIRNLEX:12774 a owl:Class ;
    rdfs:label "Persistent Vegetative State"^^xsd:string ;
    skos:prefLabel "Persistent Vegetative State"^^xsd:string ;
    NIFRID:synonym "Permanent Vegetative State"^^xsd:string,
        "Postcomatose Unawareness State"^^xsd:string,
        "Posttraumatic Unawareness State"^^xsd:string,
        "Posttraumatic Vegetative State"^^xsd:string,
        "Prolonged Posttraumatic Unawareness"^^xsd:string,
        "Vegetative State"^^xsd:string ;
    skos:definition "Vegetative state refers to the neurocognitive status of individuals with severe brain damage, in whom physiologic functions (sleep-wake cycles, autonomic control, and breathing) persist, but awareness (including all cognitive function and emotion) is abolished (MeSH)."^^xsd:string ;
    rdfs:subClassOf BIRNLEX:12669 ;
    NIFRID:createdDate "2007-10-08"^^xsd:string ;
    NIFRID:modifiedDate "2007-10-08"^^xsd:string ;
    NIFRID:acronym "PVS"^^xsd:string ;
    NIFRID:hasBirnlexCurator NIFRID:Bill_Bug ;
    NIFRID:hasCurationStatus NIFRID:uncurated ;
    NIFRID:hasDefinitionSource NIFRID:MeSH_defSource ;
    NIFRID:hasExternalSource NIFRID:MeSH ;
    NIFRID:MeshUid "D018458"^^xsd:string ;
    NIFRID:nifID "_8.3_17.2"^^xsd:string ;
    NIFRID:putativeClassExtension "Transient Vegetative State"^^xsd:string ;
    NIFRID:usageNote "MeSH includes implied subtypes"^^xsd:string .

BIRNLEX:12775 a owl:Class ;
    rdfs:label "Stupor"^^xsd:string ;
    skos:prefLabel "Stupor"^^xsd:string ;
    NIFRID:synonym "Narcosis"^^xsd:string ;
    skos:definition "A state of reduced sensibility and response to stimuli which is distinguished from COMA in that the person can be aroused by vigorous and repeated stimulation. The person is still conscious and can make voluntary movements. It can be induced by CENTRAL NERVOUS SYSTEM AGENTS. The word derives from Latin stupere and is related to stunned, stupid, dazed or LETHARGY (MeSH)."^^xsd:string ;
    rdfs:subClassOf BIRNLEX:12669 ;
    NIFRID:createdDate "2007-10-08"^^xsd:string ;
    NIFRID:modifiedDate "2007-10-08"^^xsd:string ;
    NIFRID:hasBirnlexCurator NIFRID:Bill_Bug ;
    NIFRID:hasCurationStatus NIFRID:uncurated ;
    NIFRID:hasDefinitionSource NIFRID:MeSH_defSource ;
    NIFRID:hasExternalSource NIFRID:MeSH ;
    NIFRID:MeshUid "D053608"^^xsd:string .

BIRNLEX:12776 a owl:Class ;
    rdfs:label "Syncope"^^xsd:string ;
    skos:prefLabel "Syncope"^^xsd:string ;
    NIFRID:synonym "Drop Attack"^^xsd:string,
        "Syncopal Episode"^^xsd:string,
        "Syncopal Vertigo"^^xsd:string ;
    skos:definition "A transient loss of consciousness and postural tone caused by diminished blood flow to the brain (i.e., BRAIN ISCHEMIA). Presyncope refers to the sensation of lightheadedness and loss of strength that precedes a syncopal event or accompanies an incomplete syncope (MeSH)."^^xsd:string ;
    rdfs:subClassOf BIRNLEX:12669 ;
    NIFRID:createdDate "2007-10-08"^^xsd:string ;
    NIFRID:modifiedDate "2007-10-08"^^xsd:string ;
    NIFRID:definingCitation "Adams et al., Principles of Neurology, 6th ed, pp367-9"^^xsd:string ;
    NIFRID:hasBirnlexCurator NIFRID:Bill_Bug ;
    NIFRID:hasCurationStatus NIFRID:uncurated ;
    NIFRID:hasDefinitionSource NIFRID:MeSH_defSource ;
    NIFRID:hasExternalSource NIFRID:MeSH ;
    NIFRID:MeshUid "D013575"^^xsd:string ;
    NIFRID:putativeClassExtension "Cardiogenic Syncope"^^xsd:string,
        "Carotid Sinus Syncope"^^xsd:string,
        "Convulsive Syncope"^^xsd:string,
        "Deglutitional Syncope"^^xsd:string,
        "Effort Syncope"^^xsd:string,
        "Hyperventilation Syncope"^^xsd:string,
        "Micturition Syncope"^^xsd:string,
        "Postural Syncope"^^xsd:string,
        "Situational Syncope"^^xsd:string,
        "Stokes-Adams Syncope"^^xsd:string,
        "Tussive Syncope"^^xsd:string ;
    NIFRID:usageNote "MeSH includes implied subtypes based mostly on cause"^^xsd:string .

BIRNLEX:12777 a owl:Class ;
    rdfs:label "Vasovagal Syncope"^^xsd:string ;
    skos:prefLabel "Vasovagal Syncope"^^xsd:string ;
    NIFRID:synonym "Cerebral Syncope"^^xsd:string,
        "Malignant Neurocardiogenic Syncope"^^xsd:string,
        "Neurally Mediated Faint"^^xsd:string,
        "Neurally-Mediated Vasovagal Syncope"^^xsd:string,
        "Neurocardiogenic Syncope"^^xsd:string,
        "Neurogenic Syncope"^^xsd:string,
        "Supine Syncope"^^xsd:string,
        "Vasodepressor Syncope"^^xsd:string ;
    skos:definition "Loss of consciousness due to a reduction in blood pressure that is associated with an increase in vagal tone and peripheral vasodilation (MeSH)."^^xsd:string ;
    rdfs:subClassOf BIRNLEX:12776 ;
    NIFRID:createdDate "2007-10-08"^^xsd:string ;
    NIFRID:modifiedDate "2007-10-08"^^xsd:string ;
    NIFRID:hasBirnlexCurator NIFRID:Bill_Bug ;
    NIFRID:hasCurationStatus NIFRID:uncurated ;
    NIFRID:hasDefinitionSource NIFRID:MeSH_defSource ;
    NIFRID:hasExternalSource NIFRID:MeSH ;
    NIFRID:MeshUid "D019462"^^xsd:string .

BIRNLEX:12778 a owl:Class ;
    rdfs:label "Minimally Conscious State"^^xsd:string ;
    skos:prefLabel "Minimally Conscious State"^^xsd:string ;
    rdfs:subClassOf BIRNLEX:12669 ;
    NIFRID:createdDate "2007-10-08"^^xsd:string ;
    NIFRID:modifiedDate "2007-10-08"^^xsd:string ;
    NIFRID:hasBirnlexCurator NIFRID:Bill_Bug ;
    NIFRID:hasCurationStatus NIFRID:uncurated ;
    NIFRID:hasDefinitionSource NIFRID:MeSH_defSource ;
    NIFRID:hasExternalSource NIFRID:MeSH ;
    NIFRID:MeshUid "D018458"^^xsd:string ;
    NIFRID:nifID "_8.3_17.1"^^xsd:string .

BIRNLEX:12779 a owl:Class ;
    rdfs:label "Muscular Disease"^^xsd:string ;
    skos:prefLabel "Muscular Disease"^^xsd:string ;
    NIFRID:synonym "Muscle Disorder"^^xsd:string,
        "Myopathy"^^xsd:string ;
    skos:definition "Acquired, familial, and congenital disorders of skeletal muscle ( MUSCLE, SKELETAL) and smooth muscle ( MUSCLE, SMOOTH) (MeSH)."^^xsd:string ;
    rdfs:subClassOf BIRNLEX:11013 ;
    skos:editorialNote "Note BIRNLex seeks to evolve a core subsumptive disease hierarchy based first on the effected function, then the effected structure, the latter for those categories of nervous system disease that have typically been associated with structural abnormalities or trauma (e.g., Motor neuron diseases, cerebrovascular trauma, etc.). Disease causation is in fact the ultimate goal of much biomedical research, and our recognitition of ALL the driving causes of a particular disease - and the ways in which these causes inter-relate with each other and with effected structures to cause a change in normal function is a critical representational task BIRNlex will increasingly take on to provide an evolving, nuanced functional reconstruction of disease as a process and an outcome.  These relations will be represented using OWL ObjectProperties.  Function is the most sensible context to drive the asserted subsumptive hierarchy for representing nervous system disease, since it is with the clinical description of altered, impaired, decreased, or lost function that the diagnosis - and the research - of disease is rooted.  Much has already been described regarding both the effected biomaterial entities and the causes of disease.  However, it is because understanding of such relations still is far from comprehensive, that biomedical investigation into nervous system disease continues.  Finally, given the \"realist\" ontology design approach being used to construct BIRNLex, function must be represented as inhering in some biomaterial entity from molecules and their controlling elements on up through gross anatomical structures.  Over time, BIRNLex will provide the required relations to depict these functionally-related structures for both the normal and pathological function of the nervous system.  This will be true both for the causes and for the outcomes of nervous system disease.  Initial work to extend this expressive representation will focus on the neurodegenerative diseases being studied by BIRN researchers.  Though this will be te case, BIRNLex still needs to provide a core asserted hierarchy for a broad swarth of nervous system disease, so as to enable BIRN researchers to link to the breadth of disorders that may impact or relate to those directly under study."^^xsd:string ;
    NIFRID:createdDate "2007-10-08"^^xsd:string ;
    NIFRID:modifiedDate "2007-10-08"^^xsd:string ;
    NIFRID:hasBirnlexCurator NIFRID:Bill_Bug ;
    NIFRID:hasCurationStatus NIFRID:uncurated ;
    NIFRID:hasDefinitionSource NIFRID:MeSH_defSource ;
    NIFRID:hasExternalSource NIFRID:MeSH ;
    NIFRID:MeshUid "D009135"^^xsd:string ;
    NIFRID:nifID "_8.3_8"^^xsd:string .

BIRNLEX:12780 a owl:Class ;
    rdfs:label "Cerebrovascular Disorder"^^xsd:string ;
    skos:prefLabel "Cerebrovascular Disorder"^^xsd:string ;
    NIFRID:synonym "Brain Vascular Disorder"^^xsd:string,
        "Cerebrovascular Insufficiency"^^xsd:string,
        "Intracranial Vascular Disorder"^^xsd:string ;
    skos:definition "A broad category of disorders characterized by impairment of blood flow in the arteries and veins which supply the brain. These include CEREBRAL INFARCTION; BRAIN ISCHEMIA; HYPOXIA, BRAIN; INTRACRANIAL EMBOLISM AND THROMBOSIS; INTRACRANIAL ARTERIOVENOUS MALFORMATIONS; and VASCULITIS, CENTRAL NERVOUS SYSTEM. In common usage, the term cerebrovascular disorders is not limited to conditions that affect the cerebrum, but refers to vascular disorders of the entire brain including the DIENCEPHALON; BRAIN STEM; and CEREBELLUM (MeSH)."^^xsd:string ;
    rdfs:subClassOf BIRNLEX:12796 ;
    skos:editorialNote "Note BIRNLex seeks to evolve a core subsumptive disease hierarchy based first on the effected function, then the effected structure, the latter for those categories of nervous system disease that have typically been associated with structural abnormalities or trauma (e.g., Motor neuron diseases, cerebrovascular trauma, etc.). Disease causation is in fact the ultimate goal of much biomedical research, and our recognitition of ALL the driving causes of a particular disease - and the ways in which these causes inter-relate with each other and with effected structures to cause a change in normal function is a critical representational task BIRNlex will increasingly take on to provide an evolving, nuanced functional reconstruction of disease as a process and an outcome.  These relations will be represented using OWL ObjectProperties.  Function is the most sensible context to drive the asserted subsumptive hierarchy for representing nervous system disease, since it is with the clinical description of altered, impaired, decreased, or lost function that the diagnosis - and the research - of disease is rooted.  Much has already been described regarding both the effected biomaterial entities and the causes of disease.  However, it is because understanding of such relations still is far from comprehensive, that biomedical investigation into nervous system disease continues.  Finally, given the \"realist\" ontology design approach being used to construct BIRNLex, function must be represented as inhering in some biomaterial entity from molecules and their controlling elements on up through gross anatomical structures.  Over time, BIRNLex will provide the required relations to depict these functionally-related structures for both the normal and pathological function of the nervous system.  This will be true both for the causes and for the outcomes of nervous system disease.  Initial work to extend this expressive representation will focus on the neurodegenerative diseases being studied by BIRN researchers.  Though this will be te case, BIRNLex still needs to provide a core asserted hierarchy for a broad swarth of nervous system disease, so as to enable BIRN researchers to link to the breadth of disorders that may impact or relate to those directly under study."^^xsd:string ;
    NIFRID:createdDate "2007-10-08"^^xsd:string ;
    NIFRID:modifiedDate "2007-11-18"^^xsd:string ;
    NIFRID:hasBirnlexCurator NIFRID:Bill_Bug ;
    NIFRID:hasCurationStatus NIFRID:uncurated ;
    NIFRID:hasDefinitionSource NIFRID:MeSH_defSource ;
    NIFRID:hasExternalSource NIFRID:MeSH ;
    NIFRID:MeshUid "D002561"^^xsd:string ;
    NIFRID:nifID "_8.3_1"^^xsd:string .

BIRNLEX:12781 a owl:Class ;
    rdfs:label "Brain Ischemia"^^xsd:string ;
    skos:prefLabel "Brain Ischemia"^^xsd:string ;
    NIFRID:synonym "Cerebral Ischemia"^^xsd:string,
        "Ischemic Brain Injury"^^xsd:string,
        "Ischemic Encephalopathy"^^xsd:string ;
    skos:definition "Localized reduction of blood flow to brain tissue due to arterial obstruction or systemic hypoperfusion. This frequently occurs in conjunction with brain hypoxia ( HYPOXIA, BRAIN). Prolonged ischemia is associated with BRAIN INFARCTION (MeSH)."^^xsd:string ;
    rdfs:subClassOf BIRNLEX:12780 ;
    NIFRID:createdDate "2007-10-08"^^xsd:string ;
    NIFRID:modifiedDate "2007-10-08"^^xsd:string ;
    NIFRID:hasBirnlexCurator NIFRID:Bill_Bug ;
    NIFRID:hasCurationStatus NIFRID:uncurated ;
    NIFRID:hasDefinitionSource NIFRID:MeSH_defSource ;
    NIFRID:hasExternalSource NIFRID:MeSH ;
    NIFRID:MeshUid "D002545"^^xsd:string ;
    NIFRID:nifID "_8.3_1.1"^^xsd:string .

BIRNLEX:12783 a owl:Class ;
    rdfs:label "Cerebrovascular Accident"^^xsd:string ;
    skos:prefLabel "Cerebrovascular Accident"^^xsd:string ;
    NIFRID:synonym "Apoplexy"^^xsd:string,
        "Cerebral Stroke"^^xsd:string,
        "Cerebrovascular Apoplexya"^^xsd:string,
        "Cerebrovascular Stroke"^^xsd:string,
        "Stroke"^^xsd:string ;
    skos:definition "A sudden, nonconvulsive loss of neurologic function due to an ischemic or hemorrhagic intracranial vascular event. In general, cerebrovascular accidents are classified by anatomic location in the brain, vascular distribution, etiology, age of the affected individual, and hemorrhagic vs. nonhemorrhagic nature (MeSH)."^^xsd:string ;
    rdfs:subClassOf BIRNLEX:12780 ;
    NIFRID:createdDate "2007-10-08"^^xsd:string ;
    NIFRID:modifiedDate "2007-10-08"^^xsd:string ;
    NIFRID:acronym "CVA"^^xsd:string ;
    NIFRID:definingCitation "Adams et al., Principles of Neurology, 6th ed, pp777-810"^^xsd:string ;
    NIFRID:hasBirnlexCurator NIFRID:Bill_Bug ;
    NIFRID:hasCurationStatus NIFRID:uncurated ;
    NIFRID:hasDefinitionSource NIFRID:MeSH_defSource ;
    NIFRID:hasExternalSource NIFRID:MeSH ;
    NIFRID:MeshUid "D020521"^^xsd:string ;
    NIFRID:nifID "_8.3_1"^^xsd:string .

BIRNLEX:12784 a owl:Class ;
    rdfs:label "Brain Infarction"^^xsd:string ;
    skos:prefLabel "Brain Infarction"^^xsd:string ;
    skos:definition "The formation of an area of necrosis in the brain, including the cerebral hemispheres (see CEREBRAL INFARCTION), thalami, basal ganglia, brain stem ( BRAIN STEM INFARCTIONS), or cerebellum secondary to an insufficiency of arterial or venous blood flow (MeSH)."^^xsd:string ;
    rdfs:subClassOf BIRNLEX:12783 ;
    NIFRID:createdDate "2007-10-08"^^xsd:string ;
    NIFRID:modifiedDate "2007-10-08"^^xsd:string ;
    NIFRID:hasBirnlexCurator NIFRID:Bill_Bug ;
    NIFRID:hasCurationStatus NIFRID:uncurated ;
    NIFRID:hasDefinitionSource NIFRID:MeSH_defSource ;
    NIFRID:hasExternalSource NIFRID:MeSH ;
    NIFRID:MeshUid "D020520"^^xsd:string ;
    NIFRID:putativeClassExtension "Anterior Cerebral Circulation Infarction"^^xsd:string,
        "Anterior Circulation Brain Infarction"^^xsd:string,
        "Lacunar Infarction"^^xsd:string,
        "Posterior Circulation Brain Infarction"^^xsd:string,
        "Venous Brain Infarction"^^xsd:string ;
    NIFRID:usageNote "MeSH includes implied subtypes based on the effected vessels"^^xsd:string .

BIRNLEX:12785 a owl:Class ;
    rdfs:label "Brain Stem Infarction"^^xsd:string ;
    skos:prefLabel "Brain Stem Infarction"^^xsd:string ;
    NIFRID:synonym "Brainstem Stroke"^^xsd:string ;
    skos:definition "Infarctions that occur in the brain stem which is comprised of the midbrain, pons, and medulla. There are several named syndromes characterized by their distinctive clinical manifestations and specific sites of ischemic injury (MeSH)."^^xsd:string ;
    rdfs:subClassOf BIRNLEX:12784 ;
    NIFRID:createdDate "2007-10-08"^^xsd:string ;
    NIFRID:modifiedDate "2007-10-08"^^xsd:string ;
    NIFRID:hasBirnlexCurator NIFRID:Bill_Bug ;
    NIFRID:hasCurationStatus NIFRID:uncurated ;
    NIFRID:hasDefinitionSource NIFRID:MeSH_defSource ;
    NIFRID:hasExternalSource NIFRID:MeSH ;
    NIFRID:MeshUid "D020526"^^xsd:string .

BIRNLEX:12786 a owl:Class ;
    rdfs:label "Claude Syndrome"^^xsd:string ;
    skos:prefLabel "Claude Syndrome"^^xsd:string ;
    skos:definition "Anatomical location: Midbrain Tegmentum; Vasculature: Posterior cerebral artery; Symptoms: Ataxia - arm and leg - also Oculomotor palsy with contralateral tremor and ataxia"^^xsd:string ;
    rdfs:subClassOf BIRNLEX:12785 ;
    NIFRID:createdDate "2007-10-08"^^xsd:string ;
    NIFRID:modifiedDate "2007-10-08"^^xsd:string ;
    NIFRID:definingCitationURI <http://www.strokecenter.org/prof/syndromes/syndromePage15.htm> ;
    NIFRID:hasBirnlexCurator NIFRID:Bill_Bug ;
    NIFRID:hasCurationStatus NIFRID:uncurated ;
    NIFRID:hasDefinitionSource NIFRID:MeSH_defSource ;
    NIFRID:hasExternalSource NIFRID:MeSH ;
    NIFRID:MeshUid "D020526"^^xsd:string .

BIRNLEX:12787 a owl:Class ;
    rdfs:label "Foville Syndrome"^^xsd:string ;
    skos:prefLabel "Foville Syndrome"^^xsd:string ;
    NIFRID:synonym "Inferior medial pontine syndrome"^^xsd:string ;
    skos:definition "Anatomical location: Pons - Unilateral lesion in the dorsal pontine tegmentum in the caudal third of the pons; Vasculature: Basilar artery, Paramedian and Short circumferential branches; Symptoms: contralateral - weakness in upper and lower extremity - ipsilateral: weakness in entire side of face, as well as lateral gaze weakness"^^xsd:string ;
    rdfs:subClassOf BIRNLEX:12785 ;
    NIFRID:createdDate "2007-10-08"^^xsd:string ;
    NIFRID:modifiedDate "2007-10-08"^^xsd:string ;
    NIFRID:definingCitationURI <http://www.strokecenter.org/prof/syndromes/syndromePage24.htm> ;
    NIFRID:hasBirnlexCurator NIFRID:Bill_Bug ;
    NIFRID:hasCurationStatus NIFRID:uncurated ;
    NIFRID:hasDefinitionSource NIFRID:MeSH_defSource ;
    NIFRID:hasExternalSource NIFRID:MeSH ;
    NIFRID:MeshUid "D020526"^^xsd:string .

BIRNLEX:12788 a owl:Class ;
    rdfs:label "Millard-Gubler Syndrome"^^xsd:string ;
    skos:prefLabel "Millard-Gubler Syndrome"^^xsd:string ;
    NIFRID:synonym "Ventral pontine syndrome"^^xsd:string ;
    skos:definition "Anatomical location: Pons - Basis pontis and fascicles of CN VI amd VII; Vasculature: Basilar artery, Paramedian and Short circumferential branches; Symptoms: contralateral - weakness in upper and lower extremity - ipsilateral: weakness in entire side of face, as well as lateral gaze weakness"^^xsd:string ;
    rdfs:subClassOf BIRNLEX:12785 ;
    NIFRID:createdDate "2007-10-08"^^xsd:string ;
    NIFRID:modifiedDate "2007-10-08"^^xsd:string ;
    NIFRID:definingCitationURI <http://www.strokecenter.org/prof/syndromes/syndromePage23.htm> ;
    NIFRID:hasBirnlexCurator NIFRID:Bill_Bug ;
    NIFRID:hasCurationStatus NIFRID:uncurated ;
    NIFRID:hasDefinitionSource NIFRID:MeSH_defSource ;
    NIFRID:hasExternalSource NIFRID:MeSH ;
    NIFRID:MeshUid "D020526"^^xsd:string .

BIRNLEX:12789 a owl:Class ;
    rdfs:label "Weber Syndrome"^^xsd:string ;
    skos:prefLabel "Weber Syndrome"^^xsd:string ;
    skos:definition "Anatomical location: Base of Midbrain; Vasculature: Posterior cerebral artery: Penetrating branches to midbrain; Symptoms: contralateral - weakness in upper and lower extremity - ipsilateral: lateral gaze weakness"^^xsd:string ;
    rdfs:subClassOf BIRNLEX:12785 ;
    NIFRID:createdDate "2007-10-08"^^xsd:string ;
    NIFRID:modifiedDate "2007-10-08"^^xsd:string ;
    NIFRID:definingCitationURI <http://www.strokecenter.org/prof/syndromes/syndromePage11.htm> ;
    NIFRID:hasBirnlexCurator NIFRID:Bill_Bug ;
    NIFRID:hasCurationStatus NIFRID:uncurated ;
    NIFRID:hasDefinitionSource NIFRID:MeSH_defSource ;
    NIFRID:hasExternalSource NIFRID:MeSH ;
    NIFRID:MeshUid "D020526"^^xsd:string .

BIRNLEX:12790 a owl:Class ;
    rdfs:label "Wallenberg Syndrome"^^xsd:string ;
    skos:prefLabel "Wallenberg Syndrome"^^xsd:string ;
    NIFRID:synonym "Dorsolateral Medullary Syndrome"^^xsd:string,
        "Lateral Bulbar syndrome"^^xsd:string,
        "Lateral medullary syndrome"^^xsd:string,
        "Posterior Inferior Cerebellar Artery Syndrome"^^xsd:string,
        "Vieseaux-Wallenberg Syndrome"^^xsd:string ;
    skos:definition "Infarction of the dorsolateral aspect of the medulla due to occlusion of the vertebral artery and/or the posterior inferior cerebellar artery. Clinical manifestations vary with the size of infarction, but may include loss of pain and temperature sensation in the ipsilateral face and contralateral body below the chin; ipsilateral HORNER SYNDROME; ipsilateral ATAXIA; DYSARTHRIA; VERTIGO; nausea, hiccup; dysphagia; and VOCAL CORD PARALYSIS (MeSH)"^^xsd:string ;
    rdfs:subClassOf BIRNLEX:12785 ;
    NIFRID:createdDate "2007-10-08"^^xsd:string ;
    NIFRID:modifiedDate "2007-10-08"^^xsd:string ;
    NIFRID:definingCitationURI <http://www.strokecenter.org/prof/syndromes/syndromePage9.htm> ;
    NIFRID:hasBirnlexCurator NIFRID:Bill_Bug ;
    NIFRID:hasCurationStatus NIFRID:uncurated ;
    NIFRID:hasDefinitionSource NIFRID:MeSH_defSource ;
    NIFRID:hasExternalSource NIFRID:MeSH ;
    NIFRID:MeshUid "D014854"^^xsd:string .

BIRNLEX:12791 a owl:Class ;
    rdfs:label "Cerebral Infarction"^^xsd:string ;
    skos:prefLabel "Cerebral Infarction"^^xsd:string ;
    skos:definition "The formation of an area of necrosis in the cerebrum caused by an insufficiency of arterial or venous blood flow. Infarcts of the cerebrum are generally classified by hemisphere (i.e., left vs. right), lobe (e.g., frontal lobe infarction), arterial distribution (e.g., INFARCTION, ANTERIOR CEREBRAL ARTERY), and etiology (e.g., embolic infarction) (MeSH)."^^xsd:string ;
    rdfs:subClassOf BIRNLEX:12784 ;
    NIFRID:createdDate "2007-10-08"^^xsd:string ;
    NIFRID:modifiedDate "2007-10-08"^^xsd:string ;
    NIFRID:hasBirnlexCurator NIFRID:Bill_Bug ;
    NIFRID:hasCurationStatus NIFRID:uncurated ;
    NIFRID:hasDefinitionSource NIFRID:MeSH_defSource ;
    NIFRID:hasExternalSource NIFRID:MeSH ;
    NIFRID:MeshUid "D002544"^^xsd:string ;
    NIFRID:putativeClassExtension "Anterior Choroidal Artery Infarction"^^xsd:string,
        "Left Hemisphere Cerebral Infarction"^^xsd:string,
        "Right Hemisphere Cerebral Infarction"^^xsd:string,
        "Subcortical Infarction"^^xsd:string ;
    NIFRID:usageNote "MeSH includes implied subtypes based mostly on gross anatomical location or effected vessel"^^xsd:string .

BIRNLEX:12792 a owl:Class ;
    rdfs:label "Anterior Cerebral Artery Infarction"^^xsd:string ;
    skos:prefLabel "Anterior Cerebral Artery Infarction"^^xsd:string ;
    NIFRID:synonym "ACA Infarction"^^xsd:string,
        "Anterior Cerebral Artery Circulation Infarction"^^xsd:string,
        "Anterior Cerebral Artery Distribution Infarction"^^xsd:string,
        "Anterior Cerebral Artery Stroke"^^xsd:string,
        "Anterior Cerebral Artery Syndrome"^^xsd:string,
        "Heubner Artery Infarction"^^xsd:string ;
    skos:definition "An infarction in the vascular distribution of the anterior cerebral artery which supplies the majority of the medial surface of the cerebral hemispheres, and provides branches (including Heubner's artery) to the anterior limb of the internal capsule, head of the CAUDATE NUCLEUS, and anterior GLOBUS PALLIDUS. Clinical manifestations may include contralateral lower extremity weakness and sensory loss. Bilateral anterior cerebral artery infarctions are associated with abulia, PARAPLEGIA, and URINARY INCONTINENCE (MeSH)."^^xsd:string ;
    rdfs:subClassOf BIRNLEX:12791 ;
    NIFRID:createdDate "2007-10-08"^^xsd:string ;
    NIFRID:modifiedDate "2007-10-08"^^xsd:string ;
    NIFRID:definingCitation "Adams et al., Principles of Neurology, 6th ed, pp789-93"^^xsd:string ;
    NIFRID:hasBirnlexCurator NIFRID:Bill_Bug ;
    NIFRID:hasCurationStatus NIFRID:uncurated ;
    NIFRID:hasDefinitionSource NIFRID:MeSH_defSource ;
    NIFRID:hasExternalSource NIFRID:MeSH ;
    NIFRID:MeshUid "D020243"^^xsd:string .

BIRNLEX:12793 a owl:Class ;
    rdfs:label "Middle Cerebral Artery Infarction"^^xsd:string ;
    skos:prefLabel "Middle Cerebral Artery Infarction"^^xsd:string ;
    NIFRID:synonym "MCA Infarction"^^xsd:string,
        "Middle Cerebral Artery Circulation Infarction"^^xsd:string,
        "Middle Cerebral Artery Stroke"^^xsd:string,
        "Middle Cerebral Artery Syndrome"^^xsd:string ;
    skos:definition "The formation of an area of necrosis in the cerebrum caused by an insufficiency of arterial or venous blood flow. Infarcts of the cerebrum are generally classified by hemisphere (i.e., left vs. right), lobe (e.g., frontal lobe infarction), arterial distribution (e.g., INFARCTION, ANTERIOR CEREBRAL ARTERY), and etiology (e.g., embolic infarction) (MeSH)."^^xsd:string ;
    rdfs:subClassOf BIRNLEX:12791 ;
    NIFRID:createdDate "2007-10-08"^^xsd:string ;
    NIFRID:modifiedDate "2007-10-08"^^xsd:string ;
    NIFRID:definingCitation "Adams et al., Principles of Neurology, 6th ed, pp793-8"^^xsd:string ;
    NIFRID:hasBirnlexCurator NIFRID:Bill_Bug ;
    NIFRID:hasCurationStatus NIFRID:uncurated ;
    NIFRID:hasDefinitionSource NIFRID:MeSH_defSource ;
    NIFRID:hasExternalSource NIFRID:MeSH ;
    NIFRID:MeshUid "D020244"^^xsd:string ;
    NIFRID:putativeClassExtension "Left Middle Cerebral Artery Infarction"^^xsd:string,
        "Middle Cerebral Artery Embolic Infarction"^^xsd:string,
        "Middle Cerebral Artery Embolus"^^xsd:string,
        "Middle Cerebral Artery Occlusion"^^xsd:string,
        "Middle Cerebral Artery Thrombosis"^^xsd:string,
        "Middle Cerebral Artery Thrombotic Infarction"^^xsd:string,
        "Right Middle Cerebral Artery Infarction"^^xsd:string ;
    NIFRID:usageNote "MeSH includes implied subtypes based mostly on cause or effected vessel"^^xsd:string .

BIRNLEX:12794 a owl:Class ;
    rdfs:label "Posterior Cerebral Artery Infarction"^^xsd:string ;
    skos:prefLabel "Posterior Cerebral Artery Infarction"^^xsd:string ;
    NIFRID:synonym "PCA Infarction"^^xsd:string,
        "Posterior Cerebral Artery Stroke"^^xsd:string,
        "Posterior Cerebral Artery Syndrome"^^xsd:string ;
    skos:definition "Formation of an area of coagulation necrosis induced by ischemia in the vascular distribution of the posterior cerebral artery. This artery supplies portions of the MESENCEPHALON (see also BRAIN STEM INFARCTIONS) and thalamus, inferomedial TEMPORAL LOBE, and medial OCCIPITAL LOBE. Clinical manifestations vary with the size and location of infarction, but include a variety of midbrain and thalamic syndromes, HEMIANOPSIA, and behavioral syndromes related to memory and processing visual information (MeSH)."^^xsd:string ;
    rdfs:subClassOf BIRNLEX:12791 ;
    NIFRID:createdDate "2007-10-08"^^xsd:string ;
    NIFRID:modifiedDate "2007-10-08"^^xsd:string ;
    NIFRID:definingCitation "Adams et al., Principles of Neurology, 6th ed, p786"^^xsd:string ;
    NIFRID:hasBirnlexCurator NIFRID:Bill_Bug ;
    NIFRID:hasCurationStatus NIFRID:uncurated ;
    NIFRID:hasDefinitionSource NIFRID:MeSH_defSource ;
    NIFRID:hasExternalSource NIFRID:MeSH ;
    NIFRID:MeshUid "D020762"^^xsd:string ;
    NIFRID:putativeClassExtension "Posterior Cerebral Artery Embolic Infarction"^^xsd:string,
        "Posterior Cerebral Artery Thrombotic Infarction"^^xsd:string ;
    NIFRID:usageNote "MeSH includes the following implied subtypes based mostly on cause or effected vessel: ; "^^xsd:string .

BIRNLEX:12795 a owl:Class ;
    rdfs:label "Cerebral Hemorrhage"^^xsd:string ;
    skos:prefLabel "Cerebral Hemorrhage"^^xsd:string ;
    NIFRID:synonym "Cerebral Brain Hemorrhage"^^xsd:string,
        "Cerebral Parenchymal Hemorrhage"^^xsd:string,
        "Cerebrum Hemorrhage"^^xsd:string,
        "Intracerebral Hemorrhage"^^xsd:string ;
    skos:definition "Bleeding into a cerebral hemisphere of the brain, including lobar, subcortical white matter, and basal ganglia hemorrhages. Commonly associated conditions include HYPERTENSION; INTRACRANIAL ARTERIOSCLEROSIS; INTRACRANIAL ANEURYSM; CRANIOCEREBRAL TRAUMA; INTRACRANIAL ARTERIOVENOUS MALFORMATIONS; CEREBRAL AMYLOID ANGIOPATHY; and CEREBRAL INFARCTION (MeSH)."^^xsd:string ;
    rdfs:subClassOf BIRNLEX:12780 ;
    NIFRID:createdDate "2007-10-08"^^xsd:string ;
    NIFRID:modifiedDate "2007-10-08"^^xsd:string ;
    NIFRID:hasBirnlexCurator NIFRID:Bill_Bug ;
    NIFRID:hasCurationStatus NIFRID:uncurated ;
    NIFRID:hasDefinitionSource NIFRID:MeSH_defSource ;
    NIFRID:hasExternalSource NIFRID:MeSH ;
    NIFRID:MeshUid "D002543"^^xsd:string ;
    NIFRID:nifID "_8.3_1.2"^^xsd:string .

BIRNLEX:12796 a owl:Class ;
    rdfs:label "Nervous system disease"^^xsd:string ;
    skos:prefLabel "Nervous system disease"^^xsd:string ;
    NIFRID:synonym "Nervous system disorder"^^xsd:string ;
    skos:definition "Diseases of the central and peripheral nervous system. This includes disorders of the brain, spinal cord, cranial nerves, peripheral nerves, nerve roots, autonomic nervous system, neuromuscular junction, and muscle (MeSH)."^^xsd:string ;
    rdfs:subClassOf BIRNLEX:11013 ;
    skos:editorialNote "Note BIRNLex seeks to evolve a core subsumptive disease hierarchy based first on the effected function, then the effected structure, the latter for those categories of nervous system disease that have typically been associated with structural abnormalities or trauma (e.g., Motor neuron diseases, cerebrovascular trauma, etc.). Disease causation is in fact the ultimate goal of much biomedical research, and our recognitition of ALL the driving causes of a particular disease - and the ways in which these causes inter-relate with each other and with effected structures to cause a change in normal function is a critical representational task BIRNlex will increasingly take on to provide an evolving, nuanced functional reconstruction of disease as a process and an outcome.  These relations will be represented using OWL ObjectProperties.  Function is the most sensible context to drive the asserted subsumptive hierarchy for representing nervous system disease, since it is with the clinical description of altered, impaired, decreased, or lost function that the diagnosis - and the research - of disease is rooted.  Much has already been described regarding both the effected biomaterial entities and the causes of disease.  However, it is because understanding of such relations still is far from comprehensive, that biomedical investigation into nervous system disease continues.  Finally, given the \"realist\" ontology design approach being used to construct BIRNLex, function must be represented as inhering in some biomaterial entity from molecules and their controlling elements on up through gross anatomical structures.  Over time, BIRNLex will provide the required relations to depict these functionally-related structures for both the normal and pathological function of the nervous system.  This will be true both for the causes and for the outcomes of nervous system disease.  Initial work to extend this expressive representation will focus on the neurodegenerative diseases being studied by BIRN researchers.  Though this will be te case, BIRNLex still needs to provide a core asserted hierarchy for a broad swarth of nervous system disease, so as to enable BIRN researchers to link to the breadth of disorders that may impact or relate to those directly under study."^^xsd:string ;
    NIFRID:createdDate "2007-11-18"^^xsd:string ;
    NIFRID:modifiedDate "2007-11-18"^^xsd:string ;
    NIFRID:hasBirnlexCurator NIFRID:Bill_Bug ;
    NIFRID:hasCurationStatus NIFRID:uncurated ;
    NIFRID:hasDefinitionSource NIFRID:MeSH_defSource ;
    NIFRID:hasExternalSource NIFRID:MeSH ;
    NIFRID:MeshUid "D009422"^^xsd:string ;
    NIFRID:UmlsCui "C0027765"^^xsd:string .

BIRNLEX:12797 a owl:Class ;
    rdfs:label "Eye disease"^^xsd:string ;
    skos:prefLabel "Eye disease"^^xsd:string ;
    NIFRID:synonym "Disease of eye"^^xsd:string,
        "Eye disorder"^^xsd:string,
        "Occular disease"^^xsd:string,
        "Ophthalmic disorder"^^xsd:string,
        "Ophthalmological disorder"^^xsd:string ;
    skos:definition """* Diseases or defects of the eye. Use VISION DISORDERS for other pathology involving visual neural pathways. (PSY)
* impairment of health or a condition of abnormal functioning of the organ of sight. (CSP)"""^^xsd:string ;
    rdfs:subClassOf BIRNLEX:11013 ;
    skos:editorialNote "Note BIRNLex seeks to evolve a core subsumptive disease hierarchy based first on the effected function, then the effected structure, the latter for those categories of nervous system disease that have typically been associated with structural abnormalities or trauma (e.g., Motor neuron diseases, cerebrovascular trauma, etc.). Disease causation is in fact the ultimate goal of much biomedical research, and our recognitition of ALL the driving causes of a particular disease - and the ways in which these causes inter-relate with each other and with effected structures to cause a change in normal function is a critical representational task BIRNlex will increasingly take on to provide an evolving, nuanced functional reconstruction of disease as a process and an outcome.  These relations will be represented using OWL ObjectProperties.  Function is the most sensible context to drive the asserted subsumptive hierarchy for representing nervous system disease, since it is with the clinical description of altered, impaired, decreased, or lost function that the diagnosis - and the research - of disease is rooted.  Much has already been described regarding both the effected biomaterial entities and the causes of disease.  However, it is because understanding of such relations still is far from comprehensive, that biomedical investigation into nervous system disease continues.  Finally, given the \"realist\" ontology design approach being used to construct BIRNLex, function must be represented as inhering in some biomaterial entity from molecules and their controlling elements on up through gross anatomical structures.  Over time, BIRNLex will provide the required relations to depict these functionally-related structures for both the normal and pathological function of the nervous system.  This will be true both for the causes and for the outcomes of nervous system disease.  Initial work to extend this expressive representation will focus on the neurodegenerative diseases being studied by BIRN researchers.  Though this will be te case, BIRNLex still needs to provide a core asserted hierarchy for a broad swarth of nervous system disease, so as to enable BIRN researchers to link to the breadth of disorders that may impact or relate to those directly under study."^^xsd:string ;
    NIFRID:createdDate "2007-11-18"^^xsd:string ;
    NIFRID:modifiedDate "2007-11-18"^^xsd:string ;
    NIFRID:hasBirnlexCurator NIFRID:Bill_Bug ;
    NIFRID:hasCurationStatus NIFRID:uncurated ;
    NIFRID:hasDefinitionSource NIFRID:UMLS_defSource ;
    NIFRID:hasExternalSource NIFRID:UMLS ;
    NIFRID:MeshUid "D005128"^^xsd:string ;
    NIFRID:UmlsCui "C0015397"^^xsd:string .

BIRNLEX:12798 a owl:Class ;
    rdfs:label "Retinal disease"^^xsd:string ;
    skos:prefLabel "Retinal disease"^^xsd:string ;
    NIFRID:synonym "retinal disorder"^^xsd:string,
        "retinopathia"^^xsd:string,
        "retinopathy"^^xsd:string ;
    skos:definition "Pathologic condition of the innermost of the three tunics of the eyeball or retina. (CSP)"^^xsd:string ;
    rdfs:subClassOf BIRNLEX:12797 ;
    NIFRID:createdDate "2007-11-18"^^xsd:string ;
    NIFRID:modifiedDate "2007-11-18"^^xsd:string ;
    NIFRID:hasBirnlexCurator NIFRID:Bill_Bug ;
    NIFRID:hasCurationStatus NIFRID:uncurated ;
    NIFRID:hasDefinitionSource NIFRID:UMLS_defSource ;
    NIFRID:hasExternalSource NIFRID:UMLS ;
    NIFRID:MeshUid "D012164"^^xsd:string ;
    NIFRID:UmlsCui "C0035309"^^xsd:string .

BIRNLEX:12799 a owl:Class ;
    rdfs:label "Retinal degeneration"^^xsd:string ;
    skos:prefLabel "Retinal degeneration"^^xsd:string ;
    NIFRID:synonym "degeneration of retina"^^xsd:string ;
    skos:definition """* a retrogressive pathological change in the retina, focal or generalized, caused by genetic defects, inflammation, trauma, vascular disease, or aging. Degeneration affecting predominantly the macula lutea of the retina is MACULAR DEGENERATION. (Newell, Ophthalmology: Principles and Concepts, 7th ed, p304) (MSH)
* retrogressive pathological change in the retina, focal or generalized, caused by genetic defects, inflammation, trauma, vascular disease, or aging. (CSP)"""^^xsd:string ;
    rdfs:subClassOf BIRNLEX:12798 ;
    NIFRID:createdDate "2007-11-18"^^xsd:string ;
    NIFRID:modifiedDate "2007-11-18"^^xsd:string ;
    NIFRID:definingCitation "Newell, Ophthalmology: Principles and Concepts, 7th ed, p304"^^xsd:string ;
    NIFRID:hasBirnlexCurator NIFRID:Bill_Bug ;
    NIFRID:hasCurationStatus NIFRID:uncurated ;
    NIFRID:hasDefinitionSource NIFRID:UMLS_defSource ;
    NIFRID:hasExternalSource NIFRID:UMLS ;
    NIFRID:MeshUid "D012162"^^xsd:string ;
    NIFRID:putativeClassExtension "Generalized retinal degeneration"^^xsd:string,
        "Ophthalmoplegic-retinal degeneration syndrome"^^xsd:string ;
    NIFRID:UmlsCui "C0035304"^^xsd:string .

BIRNLEX:12800 a owl:Class ;
    rdfs:label "Paving stone retinal degeneration"^^xsd:string ;
    skos:prefLabel "Paving stone retinal degeneration"^^xsd:string ;
    NIFRID:synonym "Cobblestone retinal degeneration"^^xsd:string ;
    rdfs:subClassOf BIRNLEX:12799 ;
    NIFRID:createdDate "2007-11-18"^^xsd:string ;
    NIFRID:modifiedDate "2007-11-18"^^xsd:string ;
    NIFRID:hasBirnlexCurator NIFRID:Bill_Bug ;
    NIFRID:hasCurationStatus NIFRID:uncurated ;
    NIFRID:hasExternalSource NIFRID:UMLS ;
    NIFRID:UmlsCui "C0154854"^^xsd:string .

BIRNLEX:12801 a owl:Class ;
    rdfs:label "Deafmutism-retinal degeneration syndrome"^^xsd:string ;
    skos:prefLabel "Deafmutism-retinal degeneration syndrome"^^xsd:string ;
    NIFRID:synonym "Dalinas-Amalric syndrome"^^xsd:string,
        "Diallinas-Amalric syndrome"^^xsd:string ;
    rdfs:subClassOf BIRNLEX:12799 ;
    NIFRID:createdDate "2007-11-18"^^xsd:string ;
    NIFRID:modifiedDate "2007-11-18"^^xsd:string ;
    NIFRID:hasBirnlexCurator NIFRID:Bill_Bug ;
    NIFRID:hasCurationStatus NIFRID:uncurated ;
    NIFRID:hasExternalSource NIFRID:UMLS ;
    NIFRID:UmlsCui "C0271504"^^xsd:string .

BIRNLEX:12802 a owl:Class ;
    rdfs:label "Glaucomatous retinal degeneration"^^xsd:string ;
    skos:prefLabel "Glaucomatous retinal degeneration"^^xsd:string ;
    NIFRID:synonym "Glaucomatous retinal degeneration syndrome"^^xsd:string ;
    rdfs:subClassOf BIRNLEX:12799 ;
    NIFRID:createdDate "2007-11-18"^^xsd:string ;
    NIFRID:modifiedDate "2007-11-18"^^xsd:string ;
    NIFRID:hasBirnlexCurator NIFRID:Bill_Bug ;
    NIFRID:hasCurationStatus NIFRID:uncurated ;
    NIFRID:hasExternalSource NIFRID:UMLS ;
    NIFRID:UmlsCui "C0521686"^^xsd:string .

BIRNLEX:12803 a owl:Class ;
    rdfs:label "Myopic chorioretinal atrophy"^^xsd:string ;
    skos:prefLabel "Myopic chorioretinal atrophy"^^xsd:string ;
    NIFRID:synonym "Gross myopic retinal degeneration"^^xsd:string,
        "Myopic chorioretinal atrophy disorder"^^xsd:string,
        "Myopic chorioretinal degeneration"^^xsd:string,
        "Peripheral myopic atrophy"^^xsd:string ;
    rdfs:subClassOf BIRNLEX:12799 ;
    NIFRID:createdDate "2007-11-18"^^xsd:string ;
    NIFRID:modifiedDate "2007-11-18"^^xsd:string ;
    NIFRID:hasBirnlexCurator NIFRID:Bill_Bug ;
    NIFRID:hasCurationStatus NIFRID:uncurated ;
    NIFRID:hasExternalSource NIFRID:UMLS ;
    NIFRID:UmlsCui "C0339422"^^xsd:string .

BIRNLEX:12804 a owl:Class ;
    rdfs:label "Retinal lattice degeneration"^^xsd:string ;
    skos:prefLabel "Retinal lattice degeneration"^^xsd:string ;
    NIFRID:synonym "Lattice retinal degeneration"^^xsd:string,
        "Palisade degeneration of retina"^^xsd:string,
        "Retinal lattice degeneration disorder"^^xsd:string ;
    rdfs:subClassOf BIRNLEX:12799 ;
    NIFRID:createdDate "2007-11-18"^^xsd:string ;
    NIFRID:modifiedDate "2007-11-18"^^xsd:string ;
    NIFRID:hasBirnlexCurator NIFRID:Bill_Bug ;
    NIFRID:hasCurationStatus NIFRID:uncurated ;
    NIFRID:hasExternalSource NIFRID:UMLS ;
    NIFRID:UmlsCui "C0154856"^^xsd:string .

BIRNLEX:12805 a owl:Class ;
    rdfs:label "Multifocal retinal degeneration"^^xsd:string ;
    skos:prefLabel "Multifocal retinal degeneration"^^xsd:string ;
    NIFRID:synonym "Multifocal retinal degeneration disorder"^^xsd:string ;
    rdfs:subClassOf BIRNLEX:12799 ;
    NIFRID:createdDate "2007-11-18"^^xsd:string ;
    NIFRID:modifiedDate "2007-11-18"^^xsd:string ;
    NIFRID:hasBirnlexCurator NIFRID:Bill_Bug ;
    NIFRID:hasCurationStatus NIFRID:uncurated ;
    NIFRID:hasExternalSource NIFRID:UMLS ;
    NIFRID:UmlsCui "C0521689"^^xsd:string .

BIRNLEX:12806 a owl:Class ;
    rdfs:label "Peripheral retinal degeneration"^^xsd:string ;
    skos:prefLabel "Peripheral retinal degeneration"^^xsd:string ;
    NIFRID:synonym "Peripheral degeneration of retina"^^xsd:string,
        "Peripheral retinal degeneration disorder"^^xsd:string ;
    rdfs:subClassOf BIRNLEX:12799 ;
    NIFRID:createdDate "2007-11-18"^^xsd:string ;
    NIFRID:modifiedDate "2007-11-18"^^xsd:string ;
    NIFRID:hasBirnlexCurator NIFRID:Bill_Bug ;
    NIFRID:hasCurationStatus NIFRID:uncurated ;
    NIFRID:hasExternalSource NIFRID:UMLS ;
    NIFRID:UmlsCui "C1320640"^^xsd:string .

BIRNLEX:12807 a owl:Class ;
    rdfs:label "Snowflake retinal degeneration"^^xsd:string ;
    skos:prefLabel "Snowflake retinal degeneration"^^xsd:string ;
    NIFRID:synonym "Snowflake retinal degeneration disorder"^^xsd:string ;
    rdfs:subClassOf BIRNLEX:12799 ;
    NIFRID:createdDate "2007-11-18"^^xsd:string ;
    NIFRID:modifiedDate "2007-11-18"^^xsd:string ;
    NIFRID:hasBirnlexCurator NIFRID:Bill_Bug ;
    NIFRID:hasCurationStatus NIFRID:uncurated ;
    NIFRID:hasExternalSource NIFRID:UMLS ;
    NIFRID:UmlsCui "C0339443"^^xsd:string .

BIRNLEX:12808 a owl:Class ;
    rdfs:label "Peripheral snowflake retinal degeneration"^^xsd:string ;
    skos:prefLabel "Peripheral snowflake retinal degeneration"^^xsd:string ;
    NIFRID:synonym "Peripheral snowflake retinal degeneration disorder"^^xsd:string,
        "Snowflake retinal degeneration"^^xsd:string ;
    rdfs:subClassOf BIRNLEX:12807 ;
    NIFRID:createdDate "2007-11-18"^^xsd:string ;
    NIFRID:modifiedDate "2007-11-18"^^xsd:string ;
    NIFRID:hasBirnlexCurator NIFRID:Bill_Bug ;
    NIFRID:hasCurationStatus NIFRID:uncurated ;
    NIFRID:hasExternalSource NIFRID:UMLS ;
    NIFRID:UmlsCui "C0344291"^^xsd:string .

BIRNLEX:12809 a owl:Class ;
    rdfs:label "Snail-track retinal degeneration"^^xsd:string ;
    skos:prefLabel "Snail-track retinal degeneration"^^xsd:string ;
    NIFRID:synonym "Snail-track retinal degeneration disorder"^^xsd:string ;
    rdfs:subClassOf BIRNLEX:12799 ;
    NIFRID:createdDate "2007-11-18"^^xsd:string ;
    NIFRID:modifiedDate "2007-11-18"^^xsd:string ;
    NIFRID:hasBirnlexCurator NIFRID:Bill_Bug ;
    NIFRID:hasCurationStatus NIFRID:uncurated ;
    NIFRID:hasExternalSource NIFRID:UMLS ;
    NIFRID:UmlsCui "C0339442"^^xsd:string .

BIRNLEX:12810 a owl:Class ;
    rdfs:label "Sudden acquired retinal degeneration"^^xsd:string ;
    skos:prefLabel "Sudden acquired retinal degeneration"^^xsd:string ;
    NIFRID:synonym "Sudden acquired retinal degeneration disorder"^^xsd:string ;
    rdfs:subClassOf BIRNLEX:12799 ;
    NIFRID:createdDate "2007-11-18"^^xsd:string ;
    NIFRID:modifiedDate "2007-11-18"^^xsd:string ;
    NIFRID:hasBirnlexCurator NIFRID:Bill_Bug ;
    NIFRID:hasCurationStatus NIFRID:uncurated ;
    NIFRID:hasExternalSource NIFRID:UMLS ;
    NIFRID:UmlsCui "C0521690"^^xsd:string .

BIRNLEX:12811 a owl:Class ;
    rdfs:label "Macular degeneration"^^xsd:string ;
    skos:prefLabel "Macular degeneration"^^xsd:string ;
    NIFRID:synonym "Maculadegeneration"^^xsd:string ;
    skos:definition """* degenerative changes in the macula lutea of the retina. (MSH)
* deterioration of the macula lutea in the retina; may be inherited, drug induced, or due to aging; leads to a severe loss of central vision while peripheral vision is retained. (CSP)"""^^xsd:string ;
    rdfs:subClassOf BIRNLEX:12799 ;
    NIFRID:createdDate "2007-11-18"^^xsd:string ;
    NIFRID:modifiedDate "2007-11-18"^^xsd:string ;
    NIFRID:hasBirnlexCurator NIFRID:Bill_Bug ;
    NIFRID:hasCurationStatus NIFRID:uncurated ;
    NIFRID:hasDefinitionSource NIFRID:UMLS_defSource ;
    NIFRID:hasExternalSource NIFRID:MeSH ;
    NIFRID:MeshUid "D008268"^^xsd:string ;
    NIFRID:UmlsCui "C0024437"^^xsd:string .

BIRNLEX:12812 a owl:Class ;
    rdfs:label "Age-related macular degeneration"^^xsd:string ;
    skos:prefLabel "Age-related macular degeneration"^^xsd:string ;
    NIFRID:synonym "Age related maculopathy"^^xsd:string,
        "Senile macular degeneration"^^xsd:string,
        "Senile macular degeneration of retina"^^xsd:string ;
    rdfs:subClassOf BIRNLEX:12811 ;
    NIFRID:createdDate "2007-11-18"^^xsd:string ;
    NIFRID:modifiedDate "2007-11-18"^^xsd:string ;
    NIFRID:acronym "AMD"^^xsd:string,
        "ARMD"^^xsd:string,
        "SMD"^^xsd:string ;
    NIFRID:hasBirnlexCurator NIFRID:Bill_Bug ;
    NIFRID:hasCurationStatus NIFRID:uncurated ;
    NIFRID:hasExternalSource NIFRID:UMLS ;
    NIFRID:putativeClassExtension "Degeneration of macula and posterior pole"^^xsd:string ;
    NIFRID:UmlsCui "C0242383"^^xsd:string .

BIRNLEX:12813 a owl:Class ;
    rdfs:label "Dry senile macular retinal degeneration"^^xsd:string ;
    skos:prefLabel "Dry senile macular retinal degeneration"^^xsd:string ;
    NIFRID:synonym "Atrophic age-related macular degeneration"^^xsd:string,
        "Atrophic senile macular retinal degeneration"^^xsd:string,
        "Geographic atrophy of macula"^^xsd:string,
        "Nonexudative age-related macular degeneration"^^xsd:string,
        "Nonexudative age-related macular degeneration disorder"^^xsd:string,
        "Nonexudative senile macular degeneration"^^xsd:string,
        "Nonexudative senile macular retinal degeneration disorder"^^xsd:string,
        "Nonneovascular age-related macular degeneration"^^xsd:string ;
    rdfs:subClassOf BIRNLEX:12812 ;
    NIFRID:createdDate "2007-11-18"^^xsd:string ;
    NIFRID:modifiedDate "2007-11-18"^^xsd:string ;
    NIFRID:hasBirnlexCurator NIFRID:Bill_Bug ;
    NIFRID:hasCurationStatus NIFRID:uncurated ;
    NIFRID:hasExternalSource NIFRID:UMLS ;
    NIFRID:UmlsCui "C0271083"^^xsd:string .

BIRNLEX:12814 a owl:Class ;
    rdfs:label "Cystoid macular retinal degeneration"^^xsd:string ;
    skos:prefLabel "Cystoid macular retinal degeneration"^^xsd:string ;
    NIFRID:synonym "Central cystoid Retinal Edema"^^xsd:string,
        "Cystoid Macular Edema"^^xsd:string ;
    skos:definition "Fluid accumulation in the outer layer of the MACULA LUTEA at the center of the RETINA. Cystic spaces are formed and may lead to a macular depression or hole."^^xsd:string ;
    rdfs:subClassOf BIRNLEX:12811 ;
    NIFRID:createdDate "2007-11-18"^^xsd:string ;
    NIFRID:modifiedDate "2007-11-18"^^xsd:string ;
    NIFRID:hasBirnlexCurator NIFRID:Bill_Bug ;
    NIFRID:hasCurationStatus NIFRID:uncurated ;
    NIFRID:hasDefinitionSource NIFRID:MeSH_defSource ;
    NIFRID:hasExternalSource NIFRID:MeSH ;
    NIFRID:MeshUid "D008269"^^xsd:string ;
    NIFRID:UmlsCui "C0154850"^^xsd:string,
        "C0546382"^^xsd:string .

BIRNLEX:12815 a owl:Class ;
    rdfs:label "Wet senile macular retinal degeneration"^^xsd:string ;
    skos:prefLabel "Wet senile macular retinal degeneration"^^xsd:string ;
    NIFRID:synonym "Disciform senile macular retinal degeneration"^^xsd:string,
        "Exudative age-related macular degeneration disorder"^^xsd:string,
        "Exudative senile macular degeneration of retina"^^xsd:string,
        "Exudative senile macular retinal degeneration"^^xsd:string,
        "Junius-Kuhnt degeneration"^^xsd:string,
        "Kuhnt-Junius degeneration"^^xsd:string,
        "Kuhnt-Junius degeneration disorder"^^xsd:string,
        "Subretinal neovascularization of macula"^^xsd:string ;
    rdfs:subClassOf BIRNLEX:12812 ;
    NIFRID:createdDate "2007-11-18"^^xsd:string ;
    NIFRID:modifiedDate "2007-11-18"^^xsd:string ;
    NIFRID:hasBirnlexCurator NIFRID:Bill_Bug ;
    NIFRID:hasCurationStatus NIFRID:uncurated ;
    NIFRID:hasExternalSource NIFRID:UMLS ;
    NIFRID:UmlsCui "C0271084"^^xsd:string .

BIRNLEX:12816 a owl:Class ;
    rdfs:label "Familial macular degeneration"^^xsd:string ;
    skos:prefLabel "Familial macular degeneration"^^xsd:string ;
    rdfs:subClassOf BIRNLEX:12811 ;
    NIFRID:createdDate "2007-11-18"^^xsd:string ;
    NIFRID:modifiedDate "2007-11-18"^^xsd:string ;
    NIFRID:hasBirnlexCurator NIFRID:Bill_Bug ;
    NIFRID:hasCurationStatus NIFRID:uncurated .

BIRNLEX:12817 a owl:Class ;
    rdfs:label "Familial juvenile macular degeneration"^^xsd:string ;
    skos:prefLabel "Familial juvenile macular degeneration"^^xsd:string ;
    NIFRID:synonym "Familial juvenile macular degeneration syndrome"^^xsd:string,
        "Fundus flavimaculatus"^^xsd:string,
        "Stargardts disease"^^xsd:string ;
    rdfs:subClassOf BIRNLEX:12816 ;
    NIFRID:createdDate "2007-11-18"^^xsd:string ;
    NIFRID:modifiedDate "2007-11-18"^^xsd:string ;
    NIFRID:acronym "FFM"^^xsd:string ;
    NIFRID:hasBirnlexCurator NIFRID:Bill_Bug ;
    NIFRID:hasCurationStatus NIFRID:uncurated ;
    NIFRID:hasExternalSource NIFRID:UMLS ;
    NIFRID:UmlsCui "C0271093"^^xsd:string .

BIRNLEX:12818 a owl:Class ;
    rdfs:label "Familial pseudoinflammatory macular degeneration"^^xsd:string ;
    skos:prefLabel "Familial pseudoinflammatory macular degeneration"^^xsd:string ;
    NIFRID:synonym "Familial pseudoinflammatory macular degeneration disorder"^^xsd:string,
        "Sorsbys macular degeneration"^^xsd:string ;
    rdfs:subClassOf BIRNLEX:12816 ;
    NIFRID:createdDate "2007-11-18"^^xsd:string ;
    NIFRID:modifiedDate "2007-11-18"^^xsd:string ;
    NIFRID:hasBirnlexCurator NIFRID:Bill_Bug ;
    NIFRID:hasCurationStatus NIFRID:uncurated ;
    NIFRID:hasExternalSource NIFRID:UMLS ;
    NIFRID:UmlsCui "C0520726"^^xsd:string .

BIRNLEX:12819 a owl:Class ;
    rdfs:label "Retinal drusen"^^xsd:string ;
    skos:prefLabel "Retinal drusen"^^xsd:string ;
    NIFRID:synonym "Colloid bodies in retina"^^xsd:string,
        "Degenerative drusen of retina"^^xsd:string,
        "Drusen of retina"^^xsd:string ;
    skos:definition "Colloid or hyaline bodies lying beneath the retinal pigment epithelium. They may occur either secondary to changes in the choroid that affect the pigment epithelium or as an autosomal dominant disorder of the retinal pigment epithelium."^^xsd:string ;
    rdfs:subClassOf BIRNLEX:12799 ;
    NIFRID:createdDate "2007-11-18"^^xsd:string ;
    NIFRID:modifiedDate "2007-11-18"^^xsd:string ;
    NIFRID:hasBirnlexCurator NIFRID:Bill_Bug ;
    NIFRID:hasCurationStatus NIFRID:uncurated ;
    NIFRID:hasDefinitionSource NIFRID:MeSH_defSource ;
    NIFRID:hasExternalSource NIFRID:MeSH ;
    NIFRID:MeshUid "D015593"^^xsd:string ;
    NIFRID:UmlsCui "C0035312"^^xsd:string .

BIRNLEX:12820 a owl:Class ;
    rdfs:label "Retinitis Pigmentosa"^^xsd:string ;
    skos:prefLabel "Retinitis Pigmentosa"^^xsd:string ;
    NIFRID:synonym "Chorioretinal heredodystrophy"^^xsd:string,
        "Pigmentary retinopathy"^^xsd:string,
        "Rod cone Dystrophy"^^xsd:string,
        "Tapetoretinal degeneration"^^xsd:string ;
    skos:definition """* hereditary, progressive degeneration of the neuroepithelium of the retina characterized by night blindness and progressive contraction of the visual field. (MSH)
* group of inherited abnormalities in the retina; characterized by night blindness, retinal atrophy, weakening of the retinal vessels, pigment clumping, and contraction of the visual field. (CSP)"""^^xsd:string ;
    rdfs:subClassOf BIRNLEX:12799 ;
    NIFRID:createdDate "2007-11-18"^^xsd:string ;
    NIFRID:modifiedDate "2007-11-18"^^xsd:string ;
    NIFRID:hasBirnlexCurator NIFRID:Bill_Bug ;
    NIFRID:hasCurationStatus NIFRID:uncurated ;
    NIFRID:hasDefinitionSource NIFRID:UMLS_defSource ;
    NIFRID:hasExternalSource NIFRID:UMLS ;
    NIFRID:MeshUid "D012174"^^xsd:string ;
    NIFRID:UmlsCui "C0035334"^^xsd:string .

BIRNLEX:12821 a owl:Class ;
    rdfs:label "Usher Syndrome"^^xsd:string ;
    skos:prefLabel "Usher Syndrome"^^xsd:string ;
    NIFRID:synonym "dystrophia retinae pigmentosa-dysostosis syndrome"^^xsd:string,
        "dystrophia retinae-dysacousis syndrome"^^xsd:string,
        "Graefe-Usher syndrome"^^xsd:string,
        "Hallgren syndrome"^^xsd:string,
        "Hallgren's syndrome"^^xsd:string,
        "Hallgrens syndrome"^^xsd:string,
        "retinitis pigmentosa-congenital deafness syndrome"^^xsd:string,
        "Retinitis pigmentosa-deafness syndrome"^^xsd:string,
        "Usher's Syndrome"^^xsd:string,
        "Ushers Syndrome"^^xsd:string ;
    skos:definition """* a hereditary disorder characterized by deaf-mutism, retinitis pigmentosa, and occasional mental retardation. Early cases were reported mainly in Jews in Germany but later observations came from Finland, Norway, France, England, Israel, Louisiana. (the Acadian type affecting 4.4 per 100,000), and other parts. Several types are recognized: Type I. Synonyms: Usher syndrome type I (US1, USH1) Usher syndrome type IA (US1A, USH1A) Usher syndrome, French type Type IB Synonyms: Usher syndrome type IB (US1B, USH1B) Usher syndrome, non-Acadian variety Type IC Synonyms: Usher syndrome type IC (US1C, USH1C) Usher syndrome, Acadian variety Profound congenital deafness with onset of retinitis pigmentosa by the age of 10 years. Type II Synonyms: Usher syndrome type II (US2, USH2) Type IIB Synonyms: Usher syndrome IIB (US2B, USH2B) Type III Synonyms: Usher syndrome type III (US3, USH3) Retinitis pigmentosa first noted at puberty with progressive hearing loss. Schizophrenia reported in some cases. Type IV Synonyms: Usher syndrome type IV (US4, USH4) Retinitis pigmentosa and deafness possibly transmitted as an X-linked trait. (JABL)
* autosomal recessive hereditary disorders characterized by congenital SENSORINEURAL HEARING LOSS and RETINITIS PIGMENTOSA. Genetically and symptomatically heterogeneous, clinical classes include type I, type II, and type III. Their severity, age of onset of retinitis pigmentosa and the degree of vestibular dysfunction are variable. (MSH)
* hereditary disorder believed to occur in two forms: (1) characterized by congenital deafness and severe retinitis pigmentosa, and (2) in which the inner ear and retina are less severely affected; most cases are transmitted as autosomal recessive trait, but some forms are X-linked. (CSP)"""^^xsd:string ;
    rdfs:subClassOf BIRNLEX:12822 ;
    NIFRID:createdDate "2007-11-18"^^xsd:string ;
    NIFRID:modifiedDate "April 11, 2009"^^xsd:string ;
    NIFRID:acronym "DRD"^^xsd:string,
        "US"^^xsd:string ;
    NIFRID:hasBirnlexCurator NIFRID:Bill_Bug ;
    NIFRID:hasCurationStatus NIFRID:uncurated ;
    NIFRID:hasDefinitionSource NIFRID:UMLS_defSource ;
    NIFRID:hasExternalSource NIFRID:UMLS ;
    NIFRID:MeshUid "D052245"^^xsd:string ;
    NIFRID:UmlsCui "C0271097"^^xsd:string .

BIRNLEX:12822 a owl:Class ;
    rdfs:label "Multisystem disease"^^xsd:string ;
    skos:prefLabel "Multisystem disease"^^xsd:string ;
    rdfs:subClassOf skos:ConceptScheme ;
    skos:editorialNote "Note BIRNLex seeks to evolve a core subsumptive disease hierarchy based first on the effected function, then the effected structure, the latter for those categories of nervous system disease that have typically been associated with structural abnormalities or trauma (e.g., Motor neuron diseases, cerebrovascular trauma, etc.). Disease causation is in fact the ultimate goal of much biomedical research, and our recognitition of ALL the driving causes of a particular disease - and the ways in which these causes inter-relate with each other and with effected structures to cause a change in normal function is a critical representational task BIRNlex will increasingly take on to provide an evolving, nuanced functional reconstruction of disease as a process and an outcome.  These relations will be represented using OWL ObjectProperties.  Function is the most sensible context to drive the asserted subsumptive hierarchy for representing nervous system disease, since it is with the clinical description of altered, impaired, decreased, or lost function that the diagnosis - and the research - of disease is rooted.  Much has already been described regarding both the effected biomaterial entities and the causes of disease.  However, it is because understanding of such relations still is far from comprehensive, that biomedical investigation into nervous system disease continues.  Finally, given the \"realist\" ontology design approach being used to construct BIRNLex, function must be represented as inhering in some biomaterial entity from molecules and their controlling elements on up through gross anatomical structures.  Over time, BIRNLex will provide the required relations to depict these functionally-related structures for both the normal and pathological function of the nervous system.  This will be true both for the causes and for the outcomes of nervous system disease.  Initial work to extend this expressive representation will focus on the neurodegenerative diseases being studied by BIRN researchers.  Though this will be te case, BIRNLex still needs to provide a core asserted hierarchy for a broad swarth of nervous system disease, so as to enable BIRN researchers to link to the breadth of disorders that may impact or relate to those directly under study."^^xsd:string ;
    NIFRID:createdDate "2007-11-18"^^xsd:string ;
    NIFRID:modifiedDate "2007-11-18"^^xsd:string ;
    NIFRID:hasBirnlexCurator NIFRID:Bill_Bug ;
    NIFRID:hasCurationStatus NIFRID:uncurated ;
    skos:scopeNote "Diseases whose constellation of symptoms occurs across multiple body systems."^^xsd:string .

BIRNLEX:12823 a owl:Class ;
    rdfs:label "Usher syndrome type I"^^xsd:string ;
    skos:prefLabel "Usher syndrome type I"^^xsd:string ;
    NIFRID:synonym "Usher syndrome type 1"^^xsd:string,
        "Usher's syndrome type 1"^^xsd:string ;
    rdfs:subClassOf BIRNLEX:12821 ;
    NIFRID:createdDate "2007-11-18"^^xsd:string ;
    NIFRID:modifiedDate "2007-11-18"^^xsd:string ;
    NIFRID:hasBirnlexCurator NIFRID:Bill_Bug ;
    NIFRID:hasCurationStatus NIFRID:uncurated ;
    NIFRID:hasExternalSource NIFRID:UMLS ;
    NIFRID:MeshUid "D052245"^^xsd:string ;
    NIFRID:UmlsCui "C0339533"^^xsd:string,
        "C1568247"^^xsd:string .

BIRNLEX:12824 a owl:Class ;
    rdfs:label "Usher syndrome type II"^^xsd:string ;
    skos:prefLabel "Usher syndrome type II"^^xsd:string ;
    NIFRID:synonym "Usher syndrome type 2"^^xsd:string,
        "Usher's syndrome type II"^^xsd:string ;
    rdfs:subClassOf BIRNLEX:12821 ;
    NIFRID:createdDate "2007-11-18"^^xsd:string ;
    NIFRID:modifiedDate "2007-11-18"^^xsd:string ;
    NIFRID:hasBirnlexCurator NIFRID:Bill_Bug ;
    NIFRID:hasCurationStatus NIFRID:uncurated ;
    NIFRID:hasDefinitionSource NIFRID:UMLS_defSource ;
    NIFRID:hasExternalSource NIFRID:UMLS ;
    NIFRID:MeshUid "D052245"^^xsd:string ;
    NIFRID:UmlsCui "C0339534"^^xsd:string,
        "C1568249"^^xsd:string .

BIRNLEX:12825 a owl:Class ;
    rdfs:label "Usher syndrome type III"^^xsd:string ;
    skos:prefLabel "Usher syndrome type III"^^xsd:string ;
    NIFRID:synonym "Usher syndrome type 3"^^xsd:string,
        "Usher's syndrome type III"^^xsd:string ;
    rdfs:subClassOf BIRNLEX:12821 ;
    NIFRID:createdDate "2007-11-18"^^xsd:string ;
    NIFRID:modifiedDate "2007-11-18"^^xsd:string ;
    NIFRID:hasBirnlexCurator NIFRID:Bill_Bug ;
    NIFRID:hasCurationStatus NIFRID:uncurated ;
    NIFRID:hasDefinitionSource NIFRID:UMLS_defSource ;
    NIFRID:hasExternalSource NIFRID:UMLS ;
    NIFRID:MeshUid "D052245"^^xsd:string ;
    NIFRID:UmlsCui "C1568248"^^xsd:string .

BIRNLEX:12826 a owl:Class ;
    rdfs:label "Kearns-Sayer Syndrome"^^xsd:string ;
    skos:prefLabel "Kearns-Sayer Syndrome"^^xsd:string ;
    NIFRID:synonym "Kearn-Sayre Mitochondrial Cytopathy"^^xsd:string,
        "Kearns Syndrome"^^xsd:string,
        "Kearns-Sayre-Shy-Daroff Syndrome"^^xsd:string,
        "Mitochondrial ocular myopathy"^^xsd:string,
        "Pigmentary degeneration of the retina plus heart block syndrome"^^xsd:string ;
    skos:definition "A mitochondrial disorder featuring the triad of chronic progressive EXTERNAL OPHTHALMOPLEGIA, cardiomyopathy ( CARDIOMYOPATHIES) with conduction block ( HEART BLOCK), and RETINITIS PIGMENTOSA. Disease onset is in the first or second decade. Elevated CSF protein, sensorineural deafness, seizures, and pyramidal signs may also be present. Ragged-red fibers are found on muscle biopsy."^^xsd:string ;
    rdfs:subClassOf BIRNLEX:12822 ;
    NIFRID:createdDate "2007-11-18"^^xsd:string ;
    NIFRID:modifiedDate "2007-11-18"^^xsd:string ;
    NIFRID:acronym "KSS"^^xsd:string ;
    NIFRID:definingCitation "Adams et al., Principles of Neurology, 6th ed, p984"^^xsd:string ;
    NIFRID:hasBirnlexCurator NIFRID:Bill_Bug ;
    NIFRID:hasCurationStatus NIFRID:uncurated ;
    NIFRID:hasDefinitionSource NIFRID:UMLS_defSource ;
    NIFRID:hasExternalSource NIFRID:UMLS ;
    NIFRID:MeshUid "D007625"^^xsd:string ;
    NIFRID:UmlsCui "C0022541"^^xsd:string .

BIRNLEX:12827 a owl:Class ;
    rdfs:label "Retinoschisis"^^xsd:string ;
    skos:prefLabel "Retinoschisis"^^xsd:string ;
    NIFRID:synonym "Retinoschisis disorder"^^xsd:string,
        "Schisis of retina"^^xsd:string ;
    skos:definition "A vitreoretinal dystrophy characterized by splitting of the neuroretinal layers. It occurs in two forms: degenerative retinoschisis and X chromosome-linked juvenile retinoschisis."^^xsd:string ;
    rdfs:subClassOf BIRNLEX:12799 ;
    NIFRID:createdDate "2007-11-18"^^xsd:string ;
    NIFRID:modifiedDate "2007-11-18"^^xsd:string ;
    NIFRID:acronym "RS"^^xsd:string ;
    NIFRID:hasBirnlexCurator NIFRID:Bill_Bug ;
    NIFRID:hasCurationStatus NIFRID:uncurated ;
    NIFRID:hasDefinitionSource NIFRID:MeSH_defSource ;
    NIFRID:hasExternalSource NIFRID:UMLS ;
    NIFRID:MeshUid "D041441"^^xsd:string ;
    NIFRID:putativeClassExtension "Breaks in retinoschisis"^^xsd:string,
        "Bullous retinoschisis"^^xsd:string,
        "Diffuse peripheral retinoschisis"^^xsd:string,
        "Flat retinoschisis"^^xsd:string,
        "Macular and peripheral retinoschisis"^^xsd:string,
        "Macular retinoschisis"^^xsd:string,
        "Peripheral retinoschisis"^^xsd:string,
        "Retinoschisis inner leaf break"^^xsd:string,
        "Retinoschisis outer leaf break"^^xsd:string,
        "Senile retinoschisis"^^xsd:string ;
    NIFRID:UmlsCui "C0152439"^^xsd:string .

BIRNLEX:12828 a owl:Class ;
    rdfs:label "X-Linked Retinoschisis"^^xsd:string ;
    skos:prefLabel "X-Linked Retinoschisis"^^xsd:string ;
    NIFRID:synonym "Juvenile retinoschisis"^^xsd:string,
        "Retinoschisis disorder"^^xsd:string ;
    skos:definition "X chromosome recessive disorder, found nearly exclusively in males and becoming apparent around puberty. Characterized initially by a cystlike structure involving the FOVEA CENTRALIS, a peripheral retinoschisis occurs in about half the patients."^^xsd:string ;
    rdfs:subClassOf BIRNLEX:12829 ;
    NIFRID:createdDate "2007-11-18"^^xsd:string ;
    NIFRID:modifiedDate "2007-11-18"^^xsd:string ;
    NIFRID:hasBirnlexCurator NIFRID:Bill_Bug ;
    NIFRID:hasCurationStatus NIFRID:uncurated ;
    NIFRID:hasDefinitionSource NIFRID:MeSH_defSource ;
    NIFRID:hasExternalSource NIFRID:UMLS ;
    NIFRID:MeshUid "D041441"^^xsd:string ;
    NIFRID:UmlsCui "C0271091"^^xsd:string .

BIRNLEX:12829 a owl:Class ;
    rdfs:label "Congenital retinoschisis"^^xsd:string ;
    skos:prefLabel "Congenital retinoschisis"^^xsd:string ;
    NIFRID:synonym "Congenital retinoschisis disorder"^^xsd:string ;
    rdfs:subClassOf BIRNLEX:12827 ;
    NIFRID:createdDate "2007-11-18"^^xsd:string ;
    NIFRID:modifiedDate "2007-11-18"^^xsd:string ;
    NIFRID:hasBirnlexCurator NIFRID:Bill_Bug ;
    NIFRID:hasCurationStatus NIFRID:uncurated ;
    NIFRID:hasExternalSource NIFRID:UMLS ;
    NIFRID:UmlsCui "C0344551"^^xsd:string .

BIRNLEX:12830 a owl:Class ;
    rdfs:label "Degenerative Retinoschis"^^xsd:string ;
    skos:prefLabel "Degenerative Retinoschis"^^xsd:string ;
    skos:definition "Splitting of the RETINA into two layers at the level of the outer plexiform layer, beginning as a cystic degeneration in the extreme retinal periphery. It usually occurs after 40 years of age and is generally not progressive."^^xsd:string ;
    rdfs:subClassOf BIRNLEX:12827 ;
    NIFRID:createdDate "2007-11-18"^^xsd:string ;
    NIFRID:modifiedDate "2007-11-18"^^xsd:string ;
    NIFRID:hasBirnlexCurator NIFRID:Bill_Bug ;
    NIFRID:hasCurationStatus NIFRID:uncurated ;
    NIFRID:hasDefinitionSource NIFRID:MeSH_defSource ;
    NIFRID:hasExternalSource NIFRID:UMLS ;
    NIFRID:UmlsCui "C1137478"^^xsd:string .

BIRNLEX:12831 a owl:Class ;
    rdfs:label "Neuronal Ceroid Lipofuscinosis"^^xsd:string ;
    skos:prefLabel "Neuronal Ceroid Lipofuscinosis"^^xsd:string ;
    NIFRID:synonym "Batten"^^xsd:string,
        "Batten Disease"^^xsd:string,
        "Batten's Disease"^^xsd:string,
        "Batten-Mayou Disease"^^xsd:string,
        "Batten-Spielmeyer-Vogt Disease"^^xsd:string,
        "Battens Disease"^^xsd:string,
        "Spielmeyer-Vogt Disease"^^xsd:string ;
    skos:definition "* A group of severe neurodegenerative diseases characterized by intracellular accumulation of autofluorescent wax-like lipid materials ( CEROID; LIPOFUSCIN) in neurons. There are several subtypes based on mutations of the various genes, time of disease onset, and severity of the neurological defects such as progressive DEMENTIA; SEIZURES; and visual failure (MeSH). * Batten disease is a fatal, inherited disorder of the nervous system that begins in childhood. In some cases, the early signs are subtle, taking the form of personality and behavior changes, slow learning, clumsiness, or stumbling. Symptoms of Batten disease are linked to a buildup of substances called lipopigments in the body's tissues. Lipopigments are made up of fats and proteins. Because vision loss is often an early sign, Batten disease may be first suspected during an eye exam. Often, an eye specialist or other physician may refer the child to a neurologist. Diagnostic tests for Batten disease include blood or urine tests, skin or tissue sampling, an electroencephalogram (EEG), electrical studies of the eyes, and brain scans (NINDS Disease page)."^^xsd:string ;
    rdfs:subClassOf BIRNLEX:2086 ;
    NIFRID:createdDate "2008-01-18"^^xsd:string ;
    NIFRID:modifiedDate "April 27, 2010"^^xsd:string ;
    NIFRID:birnlexDefinition """* A group of severe neurodegenerative diseases characterized by intracellular accumulation of autofluorescent wax-like lipid materials ( CEROID; LIPOFUSCIN) in neurons. There are several subtypes based on mutations of the various genes, time of disease onset, and severity of the neurological defects such as progressive DEMENTIA; SEIZURES; and visual failure (MeSH).
 * Batten disease is a fatal, inherited disorder of the nervous system that begins in childhood. In some cases, the early signs are subtle, taking the form of personality and behavior changes, slow learning, clumsiness, or stumbling. Symptoms of Batten disease are linked to a buildup of substances called lipopigments in the body's tissues. Lipopigments are made up of fats and proteins. Because vision loss is often an early sign, Batten disease may be first suspected during an eye exam. Often, an eye specialist or other physician may refer the child to a neurologist. Diagnostic tests for Batten disease include blood or urine tests, skin or tissue sampling, an electroencephalogram (EEG), electrical studies of the eyes, and brain scans (NINDS Disease page)."""^^xsd:string ;
    NIFRID:definingCitationURI <http://www.ninds.nih.gov/disorders/batten/batten.htm> ;
    NIFRID:hasBirnlexCurator NIFRID:Bill_Bug ;
    NIFRID:hasDefinitionSource NIFRID:UMLS_defSource ;
    NIFRID:MeshUid "D009472"^^xsd:string ;
    NIFRID:putativeClassExtension "Adult Neuronal Ceroid Lipofuscinosis"^^xsd:string,
        "Jansky-Bielschowsky Disease"^^xsd:string,
        "Juvenile Cerebroretinal Degeneration"^^xsd:string,
        "Kufs Disease"^^xsd:string,
        "Santavuori-Haltia Disease"^^xsd:string ;
    NIFRID:UmlsCui "C0751383"^^xsd:string ;
    NIFRID:usageNote "MeSH includes several implied subtypes based primarily on causation"^^xsd:string,
        "The MeSH term includes implied subtypes related to developmental stage at time of diagnosis: Infantile Neuronal Ceroid Lipofuscinosis, Late-Infantile Neuronal Ceroid Lipofuscinosis, Juvenile Neuronal Ceroid Lipofuscinosis, and Adult Neuronal Ceroid Lipofuscinosis"^^xsd:string .

NLX:143898 a owl:Class ;
    rdfs:label "Traumatic brain injury" ;
    NIFRID:synonym "intracranial injury",
        "TBI",
        "tbi" ;
    dc:description "Traumatic brain injury (TBI), also known as intracranial injury, occurs when an external force traumatically injures the brain. TBI can be classified based on severity, mechanism (closed or penetrating head injury), or other features (e.g. occurring in a specific location or over a widespread area). Head injury usually refers to TBI, but is a broader category because it can involve damage to structures other than the brain, such as the scalp and skull. (Wikipedia)" ;
    rdfs:subClassOf BIRNLEX:12667 ;
    owl:versionInfo "174637" ;
    NIFRID:createdDate "May 17, 2012" ;
    NIFRID:MeshUid "D001930"^^xsd:string .

NLX:151498 a owl:Class ;
    rdfs:label "Neuropathy"^^xsd:string ;
    dc:description "Medical term referring to disorders of the nerves of the peripheral nervous system (specifically excluding encephalopathy and myelopathy, which pertain to the central nervous system.) It is usually considered equivalent to peripheral neuropathy, which is defined as deranged function and structure of peripheral motor, sensory, and autonomic neurons, involving either the entire neuron or selected levels. According to some sources, a disorder of the cranial nerves can be considered a neuropathy. - adapted from Wikipedia"^^xsd:string ;
    rdfs:subClassOf BIRNLEX:12796 ;
    NIFRID:createdDate "August 20, 2012"^^xsd:string ;
    dc:contributor "Maryann Martone"^^xsd:string .

NLX:151499 a owl:Class ;
    rdfs:label "Giant axonal neuropathy"^^xsd:string ;
    NIFRID:abbrev "GAN"^^xsd:string ;
    dc:description "A progressive hereditary disease that affects the peripheral and central nervous systems. It is characterized morphologically by aggregates of intermediate filaments in different tissues. Mutations have been reported in the gene that codes for gigaxonin. Morphologically, GAN is characterized by the presence of giant axons filled with densely packed accumulations of neurofilaments (NF). Affected axons have a thin myelin sheath, do not transmit signals properly, and eventually perish. Unique to GAN is that in addition to the inclusions in neurons, astrocytes can be filled with glial filament bodies, fibroblasts with vimentin clusters and muscle fibers with desmin accumulations."^^xsd:string ;
    rdfs:subClassOf NLX:151498 ;
    NIFRID:createdDate "August 20, 2012"^^xsd:string ;
    dc:contributor "Maryann Martone"^^xsd:string ;
    NIFRID:definingCitation "Mussche S et al. (2012) Proteomic analysis in giant axonal neuropathy: new insights into disease mechanisms. Muscle Nerve 46: 246-56"^^xsd:string ;
    NIFRID:umls_ID "C1850386"^^xsd:string .

NLXDYS:090801 a owl:Class ;
    rdfs:label "Pick's Disease"^^xsd:string ;
    NIFRID:synonym "Picks Disease"^^xsd:string ;
    rdfs:subClassOf BIRNLEX:2086 ;
    NIFRID:createdDate "August 11, 2009"^^xsd:string ;
    dc:contributor "Jane Bugea"^^xsd:string .

NLXDYS:100201 a owl:Class ;
    rdfs:label "Neuronal intranuclear hyaline inclusion disease"^^xsd:string ;
    NIFRID:synonym "intranuclear inclusion body disease"^^xsd:string,
        "neuronal intranuclear inclusion disease"^^xsd:string ;
    NIFRID:abbrev "NIHID"^^xsd:string ;
    skos:definition "Neuronal intranuclear hyaline inclusion disease is a rare neurodegenerative disease characterized pathologically by the presence of eosinophilic intranuclear inclusions in neuronal cells"^^xsd:string ;
    rdfs:subClassOf BIRNLEX:2086 ;
    NIFRID:createdDate "February 17, 2010"^^xsd:string ;
    dc:contributor "Maryann Martone"^^xsd:string .

NLXDYS:100301 a owl:Class ;
    rdfs:label "Tic disorder"^^xsd:string ;
    skos:definition "Tic disorders are defined in the Diagnostic and Statistical Manual of Mental Disorders (DSM) based on type (motor or phonic) and duration of tics (sudden, rapid, nonrhythmic, stereotyped, involuntary movements). Tic disorders are defined similarly by the World Health Organization (ICD-10 codes).\\\\n\\\\nDSM-IV-TR diagnosis codes for the tic disorders are:\\\\n\\\\n307.20 Tic Disorder NOS (Not Otherwise Specified)\\\\n\\\\n307.21 Transient Tic Disorder\\\\n\\\\n307.22 Chronic Motor or Vocal Tic Disorder\\\\n\\\\n307.23 Tourette's Disorder\\\\n\\\\n\\\\nICD10 diagnosis codes are:\\\\n\\\\nF95.0 Transient tic disorder\\\\n\\\\nF95.1 Chronic motor or vocal tic disorder\\\\n\\\\nF95.2 Combined vocal and multiple motor tic disorder (de la Tourette)\\\\n\\\\nF95.8 Other tic disorders\\\\n\\\\nF95.9 Tic disorder, unspecified, Tic disorders are defined in the Diagnostic and Statistical Manual of Mental Disorders (DSM) based on type (motor or phonic) and duration of tics (sudden, rapid, nonrhythmic, stereotyped, involuntary movements). Tic disorders are defined similarly by the World Health Organization (ICD-10 codes).\\\\\\\\n\\\\\\\\nDSM-IV-TR diagnosis codes for the tic disorders are:\\\\\\\\n\\\\\\\\n307.20 Tic Disorder NOS (Not Otherwise Specified)\\\\\\\\n\\\\\\\\n307.21 Transient Tic Disorder\\\\\\\\n\\\\\\\\n307.22 Chronic Motor or Vocal Tic Disorder\\\\\\\\n\\\\\\\\n307.23 Tourette's Disorder\\\\\\\\n\\\\\\\\n\\\\\\\\nICD10 diagnosis codes are:\\\\\\\\n\\\\\\\\nF95.0 Transient tic disorder\\\\\\\\n\\\\\\\\nF95.1 Chronic motor or vocal tic disorder\\\\\\\\n\\\\\\\\nF95.2 Combined vocal and multiple motor tic disorder (de la Tourette)\\\\\\\\n\\\\\\\\nF95.8 Other tic disorders\\\\\\\\n\\\\\\\\nF95.9 Tic disorder, unspecified, Tic disorders are defined in the Diagnostic and Statistical Manual of Mental Disorders (DSM) based on type (motor or phonic) and duration of tics (sudden, rapid, nonrhythmic, stereotyped, involuntary movements). Tic disorders are defined similarly by the World Health Organization (ICD-10 codes).\\n\\nDSM-IV-TR diagnosis codes for the tic disorders are:\\n\\n307.20 Tic Disorder NOS (Not Otherwise Specified)\\n\\n307.21 Transient Tic Disorder\\n\\n307.22 Chronic Motor or Vocal Tic Disorder\\n\\n307.23 Tourette's Disorder\\n\\n\\nICD10 diagnosis codes are:\\n\\nF95.0 Transient tic disorder\\n\\nF95.1 Chronic motor or vocal tic disorder\\n\\nF95.2 Combined vocal and multiple motor tic disorder (de la Tourette)\\n\\nF95.8 Other tic disorders\\n\\nF95.9 Tic disorder, unspecified"^^xsd:string ;
    rdfs:subClassOf BIRNLEX:12669 ;
    NIFRID:createdDate "March 19, 2010"^^xsd:string ;
    NIFRID:definingCitation "American Psychiatric Association (2000). \"Diagnostic criteria for tic disorders\". Diagnostic and Statistical Manual of Mental Disorders, 4th ed., text revision (DSM-IV-TR), ISBN 0890420254. Retrieved on July 22, 2008."^^xsd:string .

NLXDYS:100302 a owl:Class ;
    rdfs:label "Chronic Tic Disorder"^^xsd:string ;
    skos:definition "Chronic tic disorder is either single or multiple motor or phonic tics, but not both, which are present for more than a year."^^xsd:string ;
    rdfs:subClassOf NLXDYS:100301 ;
    NIFRID:createdDate "March 19, 2010"^^xsd:string ;
    NIFRID:definingCitation "Evidente VG. \"Is it a tic or Tourette's? Clues for differentiating simple from more complex tic disorders\". Postgraduate medicine108 (5): 175-6, 179-82. PMID 11043089 Retrieved on 2007-05-24"^^xsd:string .

NLXDYS:100303 a owl:Class ;
    rdfs:label "Tourette's Disorder"^^xsd:string ;
    NIFRID:synonym "Gilles de la Tourette syndrome"^^xsd:string,
        "Tourette Disorder"^^xsd:string,
        "Tourette syndrome"^^xsd:string,
        "Tourette's Syndrome"^^xsd:string,
        "Tourettes Disorder"^^xsd:string,
        "TS"^^xsd:string ;
    skos:definition "Both multiple motor and one or more vocal tics have been present at some time during the illness. A tic is a sudden rapid recurrent, non rhythmic, stereotyped motor movement or vocalization.\\n\\nTourette syndrome (TS) is a neurological disorder characterized by repetitive, stereotyped, involuntary movements and vocalizations called tics. The disorder is named for Dr. Georges Gilles de la Tourette, the pioneering French neurologist who in 1885 first described the condition in an 86-year-old French noblewoman., Both multiple motor and one or more vocal tics have been present at some time during the illness. A tic is a sudden rapid recurrent, non rhythmic, stereotyped motor movement or vocalization.\\\\\\\\n\\\\\\\\nTourette syndrome (TS) is a neurological disorder characterized by repetitive, stereotyped, involuntary movements and vocalizations called tics. The disorder is named for Dr. Georges Gilles de la Tourette, the pioneering French neurologist who in 1885 first described the condition in an 86-year-old French noblewoman., Both multiple motor and one or more vocal tics have been present at some time during the illness. A tic is a sudden rapid recurrent, non rhythmic, stereotyped motor movement or vocalization.\\\\n\\\\nTourette syndrome (TS) is a neurological disorder characterized by repetitive, stereotyped, involuntary movements and vocalizations called tics. The disorder is named for Dr. Georges Gilles de la Tourette, the pioneering French neurologist who in 1885 first described the condition in an 86-year-old French noblewoman."^^xsd:string ;
    rdfs:subClassOf NLXDYS:100301 ;
    NIFRID:createdDate "March 19, 2010"^^xsd:string ;
    NIFRID:definingCitation "Diagnostic and Statistical Manual of Mental Disorders. 4th ed."^^xsd:string ;
    NIFRID:definingCitationURI <http://medical-dictionary.thefreedictionary.com/Tourette+syndrome> .

NLXDYS:100304 a owl:Class ;
    rdfs:label "Transient Tic Disorder"^^xsd:string ;
    skos:definition "Transient tic disorder consists of multiple motor and/or phonic tics with duration of at least 4 weeks, but less than 12 months."^^xsd:string ;
    rdfs:subClassOf NLXDYS:100301 ;
    NIFRID:createdDate "March 19, 2010"^^xsd:string ;
    NIFRID:definingCitation "Evidente VG. \"Is it a tic or Tourette's? Clues for differentiating simple from more complex tic disorders\". Postgraduate medicine108 (5): 175-6, 179-82. PMID 11043089 Retrieved on 2007-05-24"^^xsd:string .

NLXDYS:100316 a owl:Class ;
    rdfs:label "Charcot Marie Tooth disease"^^xsd:string ;
    NIFRID:synonym "hereditary motor and sensory neuropathy"^^xsd:string,
        "peroneal muscular atrophy"^^xsd:string ;
    NIFRID:abbrev "CMT"^^xsd:string,
        "HMSN"^^xsd:string ;
    skos:definition "A common inherited neurological disorders, affecting approximately 1 in 2,500 people in the United States, comprising a group of disorders caused by mutations in genes that affect the normal function of the peripheral nerves. A typical feature includes weakness of the foot and lower leg muscles, which may result in foot drop and a high-stepped gait with frequent tripping or falls. Foot deformities, such as high arches and hammertoes (a condition in which the middle joint of a toe bends upwards), are also characteristic due to weakness of the small muscles in the feet. In addition, the lower legs may take on an \"inverted champagne bottle\" appearance due to the loss of muscle bulk. Later in the disease, weakness and muscle atrophy may occur in the hands, resulting in difficulty with fine motor skills. (adapted from NINDS disease pages)"^^xsd:string ;
    rdfs:subClassOf BIRNLEX:12796 ;
    NIFRID:createdDate "March 17, 2010"^^xsd:string ;
    NIFRID:definingCitationURI <http://www.ninds.nih.gov/disorders/charcot_marie_tooth/charcot_marie_tooth.htm> .

NLXDYS:2011001 a owl:Class ;
    rdfs:label "Kennedy Syndrome"^^xsd:string ;
    NIFRID:synonym "Bulbospinal Neuronopathy"^^xsd:string,
        "Progressive Myelopathic Muscular Atrophy"^^xsd:string ;
    skos:definition "Kennedy's disease is an inherited motor neuron disease that affects males. It is one of a group of disorders called spinal muscular atrophy (SMA). Onset of the disease is usually between the ages of 20 and 40, although it has been diagnosed in men from their teens to their 70s. Early symptoms include tremor of the outstretched hands, muscle cramps with exertion, and fasciculations (fleeting muscle twitches visible under the skin). Eventually, individuals develop limb weakness which usually begins in the pelvic or shoulder regions. Weakness of the facial and tongue muscles may occur later in the course of the disease and often leads to dysphagia (difficulty in swallowing), dysarthria (slurring of speech), and recurrent aspiration pneumonia. Some individuals develop gynecomastia (excessive enlargement of male breasts) and low sperm count or infertility. Still others develop non-insulin-dependent diabetes mellitus. Kennedy's disease is an x-linked recessive disease, which means the patient's mother carries the defective gene on one of her X chromosomes. Daughters of patients with Kennedy's disease are also carriers and have a 1 in 2 chance of having a son affected with the disease. Parents with concerns about their children may wish to talk to a genetic counselor. (http://www.ninds.nih.gov/disorders/kennedys/kennedys.htm)"^^xsd:string ;
    rdfs:subClassOf BIRNLEX:12568 ;
    owl:versionInfo "140443"^^xsd:string ;
    NIFRID:createdDate "March 3, 2011"^^xsd:string ;
    NIFRID:modifiedDate "March 3, 2011"^^xsd:string .

NLXDYS:2011002 a owl:Class ;
    rdfs:label "Type IV Spinal Muscular Atrophy"^^xsd:string ;
    NIFRID:synonym "Finkey late-adult type SMA"^^xsd:string,
        "late-onset Finkel-type spinal muscular atrophy"^^xsd:string ;
    skos:definition "Adult onset spinal muscular atrophy due to autosomal dominant mutation in the vesicle-associated membrane protein-associated protein B gene (VAPB, {605704.0001} (adapted from OMIM)"^^xsd:string ;
    rdfs:subClassOf BIRNLEX:12568 ;
    owl:versionInfo "141143"^^xsd:string ;
    NIFRID:createdDate "March 3, 2011"^^xsd:string ;
    NIFRID:modifiedDate "March 3, 2011"^^xsd:string .

NLXDYS:20090301 a owl:Class ;
    rdfs:label "Eating disorder"^^xsd:string ;
    skos:prefLabel "Eating disorder"^^xsd:string ;
    NIFRID:synonym "Eating related disorder"^^xsd:string,
        "Eating-related disorder"^^xsd:string ;
    skos:definition "A type of disorder involving the results of eating behavior, e.g., eating too much or eating too little."^^xsd:string ;
    rdfs:subClassOf BIRNLEX:11013 ;
    rdfs:comment "This can be considered a proxy class for conditions like obesity which really are more qualities than diseases; but until the correct classification is in place, we will use it because it is useful. (Maryann Martone, February, 2009)"^^xsd:string ;
    NIFRID:createdDate "March 18, 2009"^^xsd:string ;
    skos:example "Obesity"^^xsd:string .

NLXDYS:20090302 a owl:Class ;
    rdfs:label "Obesity"^^xsd:string ;
    skos:prefLabel "Obesity"^^xsd:string ;
    skos:definition "An eating-related disorder in which excess body fat has accumulated to such an extent that health may be negatively affected. It is commonly defined as a body mass index (weight divided by height squared) of 30 kg/m2 or higher."^^xsd:string ;
    rdfs:subClassOf NLXDYS:20090301 ;
    NIFRID:createdDate "March 18, 2009"^^xsd:string ;
    NIFRID:hasDefinitionSource <http://en.wikipedia.org/wiki/Obesity> .

NLXDYS:20090303 a owl:Class ;
    rdfs:label "Morbid obesity"^^xsd:string ;
    skos:prefLabel "Morbid obesity"^^xsd:string ;
    NIFRID:synonym "Obesity"^^xsd:string ;
    skos:definition "Extreme form of obesity where body bass index is 40 or more, which is roughly equivalent to 100 pounds or more over ideal body weight."^^xsd:string ;
    rdfs:subClassOf NLXDYS:20090302 ;
    NIFRID:createdDate "March 18, 2009"^^xsd:string ;
    NIFRID:modifiedDate "April 8, 2010"^^xsd:string .

NLXDYS:20090501 a owl:Class ;
    rdfs:label "Mental retardation disorder"^^xsd:string ;
    skos:definition "According to the latest edition of the Diagnostic and Statistical Manual of Mental Disorders (DSM-IV), there are three criteria before a person is considered to have a mental retardation: an IQ below 70, significant limitations in two or more areas of adaptive behavior (as measured by an adaptive behavior rating scale, i.e. communication, self-help skills, interpersonal skills, and more), and evidence that the limitations became apparent before the age of 18."^^xsd:string ;
    rdfs:subClassOf BIRNLEX:12796 ;
    NIFRID:createdDate "May 14, 2009"^^xsd:string ;
    dc:contributor "Maryann Martone"^^xsd:string .

NLXDYS:20090502 a owl:Class ;
    rdfs:label "Downs syndrome"^^xsd:string ;
    NIFRID:synonym "Down syndrome"^^xsd:string,
        "Down's syndrome"^^xsd:string,
        "Trisomy 21"^^xsd:string ;
    skos:definition "A disorder caused by the presence of all or part of an extra 21st chromosome, characterized by structural abnormalities throughout the body. Often Down syndrome is associated with some impairment of cognitive ability and physical growth as well as facial appearance. (Adapted from Wikipedia)"^^xsd:string ;
    rdfs:subClassOf NLXDYS:20090501 ;
    NIFRID:createdDate "May 14, 2009"^^xsd:string ;
    dc:contributor "Maryann Martone"^^xsd:string .

NLXDYS:20090601 a owl:Class ;
    rdfs:label "Fragile X syndrome"^^xsd:string ;
    NIFRID:synonym "Escalante's syndrome"^^xsd:string,
        "FRAXA syndrome"^^xsd:string,
        "Marker X syndrome"^^xsd:string,
        "Martin-Bell syndrome"^^xsd:string ;
    skos:definition "Fragile X syndrome is an X linked inherited form of mental impairment. The syndrome occurs in approximately 1 in 3600 males and 1 in 4000 to 6000 females. The majority of males with fragile X syndrome will have a significant intellectual disability. The spectrum ranges from learning disabilities to severe mental retardation and autism. In addition, males have a variety of physical and behavioral characteristics, including enlarged ears, long face with prominent chin, and large testicles (in post pubertal males). Connective tissue problems may include ear infections, mitral valve prolapse, flat feet, double-jointed fingers, hyperflexible joints and a variety of skeletal problems. Behavioral characteristics in males include attention deficit disorders, speech disturbances, hand biting, hand flapping, autistic behaviors, poor eye contact, and unusual responses to various touch, auditory or visual stimuli. The characteristics seen in males can also be seen in females, though females often have milder intellectual disability and a milder presentation of the behavioral or physical features. (from http://www.fragilex.org/)"^^xsd:string ;
    rdfs:subClassOf NLXDYS:20090501 ;
    NIFRID:createdDate "June 20, 2009"^^xsd:string ;
    dc:contributor "Maryann Martone"^^xsd:string .

NLXDYS:20090602 a owl:Class ;
    rdfs:label "Fetal alcohol syndrome"^^xsd:string ;
    NIFRID:synonym "FAS"^^xsd:string ;
    skos:definition "A condition occurring in FETUS or NEWBORN due to in utero ETHANOL exposure when mother consumed alcohol during PREGNANCY. It is characterized by a cluster of irreversible BIRTH DEFECTS including abnormalities in physical, mental, and behavior development (such as FETAL GROWTH RETARDATION; MENTAL RETARDATION; ATTENTION DEFICIT AND DISRUPTIVE BEHAVIOR DISORDERS) with varied degree of severity in an individual.(MeSH)"^^xsd:string ;
    rdfs:subClassOf BIRNLEX:11013 ;
    NIFRID:createdDate "June 21, 2009"^^xsd:string ;
    dc:contributor "Maryann Martone"^^xsd:string ;
    NIFRID:MeshUid "D005310"^^xsd:string .

skos:ConceptScheme a owl:Class ;
    rdfs:isDefinedBy <http://www.w3.org/2004/02/skos/core> .

### Annotations

dc:creator rdfs:isDefinedBy dc: .

dc:description rdfs:isDefinedBy dc: .

dc:subject rdfs:isDefinedBy dc: .

dc:title rdfs:isDefinedBy dc: .

skos:historyNote rdfs:isDefinedBy <http://www.w3.org/2004/02/skos/core> .

### Serialized using the pyontutils deterministic serializer v1.1.3
