<?xml version="1.0"?>


<!DOCTYPE rdf:RDF [
    <!ENTITY pathLex "http://www.semanticweb.org/david/ontologies/2013/0/pathLex.owl#1.3.6.1.4.1.19376.1.8.2.1." >
    <!ENTITY owl "http://www.w3.org/2002/07/owl#" >
    <!ENTITY dc "http://purl.org/dc/elements/1.1/" >
    <!ENTITY xsd "http://www.w3.org/2001/XMLSchema#" >
    <!ENTITY skos "http://www.w3.org/2004/02/skos/core#" >
    <!ENTITY rdfs "http://www.w3.org/2000/01/rdf-schema#" >
    <!ENTITY rdf "http://www.w3.org/1999/02/22-rdf-syntax-ns#" >
]>


<rdf:RDF xmlns="http://www.semanticweb.org/david/ontologies/2013/0/pathLex.owl#"
     xml:base="http://www.semanticweb.org/david/ontologies/2013/0/pathLex.owl"
     xmlns:dc="http://purl.org/dc/elements/1.1/"
     xmlns:pathLex="http://www.semanticweb.org/david/ontologies/2013/0/pathLex.owl#1.3.6.1.4.1.19376.1.8.2.1."
     xmlns:rdfs="http://www.w3.org/2000/01/rdf-schema#"
     xmlns:owl="http://www.w3.org/2002/07/owl#"
     xmlns:xsd="http://www.w3.org/2001/XMLSchema#"
     xmlns:rdf="http://www.w3.org/1999/02/22-rdf-syntax-ns#"
     xmlns:skos="http://www.w3.org/2004/02/skos/core#">
    <owl:Ontology rdf:about="http://www.semanticweb.org/david/ontologies/2013/0/pathLex.owl">
        <dc:creator>David Ouagne</dc:creator>
        <dc:creator>Christel Daniel</dc:creator>
        <skos:prefLabel xml:lang="en">PATHLEX</skos:prefLabel>
    </owl:Ontology>
    


    <!-- 
    ///////////////////////////////////////////////////////////////////////////////////////
    //
    // Annotation properties
    //
    ///////////////////////////////////////////////////////////////////////////////////////
     -->

    <owl:AnnotationProperty rdf:about="&dc;creator"/>
    <owl:AnnotationProperty rdf:about="&skos;prefLabel"/>
    <owl:AnnotationProperty rdf:about="&skos;definition"/>
    <owl:AnnotationProperty rdf:about="&skos;altLabel">
        <rdfs:subPropertyOf rdf:resource="&rdfs;label"/>
    </owl:AnnotationProperty>
    


    <!-- 
    ///////////////////////////////////////////////////////////////////////////////////////
    //
    // Datatypes
    //
    ///////////////////////////////////////////////////////////////////////////////////////
     -->

    


    <!-- 
    ///////////////////////////////////////////////////////////////////////////////////////
    //
    // Classes
    //
    ///////////////////////////////////////////////////////////////////////////////////////
     -->

    


    <!-- http://www.semanticweb.org/david/ontologies/2013/0/1.3.6.1.4.1.19376.1.8.2.1.1 -->

    <owl:Class rdf:about="&pathLex;1">
        <rdfs:subClassOf rdf:resource="&pathLex;99999"/>
        <skos:definition xml:lang="en">Generic-Infiltrating malignant neoplasm-Specimen weight</skos:definition>
        <skos:prefLabel xml:lang="en">Specimen weight</skos:prefLabel>
    </owl:Class>
    


    <!-- http://www.semanticweb.org/david/ontologies/2013/0/1.3.6.1.4.1.19376.1.8.2.1.10 -->

    <owl:Class rdf:about="&pathLex;10">
        <rdfs:subClassOf rdf:resource="&pathLex;10010"/>
        <skos:definition xml:lang="en">Generic-Infiltrating malignant neoplasm-Lesion size, largest dimension</skos:definition>
        <skos:prefLabel xml:lang="en">Lesion size, largest dimension</skos:prefLabel>
    </owl:Class>
    


    <!-- http://www.semanticweb.org/david/ontologies/2013/0/1.3.6.1.4.1.19376.1.8.2.1.10000 -->

    <owl:Class rdf:about="&pathLex;10000">
        <rdfs:subClassOf rdf:resource="&pathLex;10011"/>
        <skos:prefLabel xml:lang="en">Histologic grade</skos:prefLabel>
    </owl:Class>
    


    <!-- http://www.semanticweb.org/david/ontologies/2013/0/1.3.6.1.4.1.19376.1.8.2.1.10003 -->

    <owl:Class rdf:about="&pathLex;10003">
        <rdfs:subClassOf rdf:resource="&pathLex;10010"/>
        <skos:prefLabel xml:lang="en">Ancillary techniques</skos:prefLabel>
    </owl:Class>
    


    <!-- http://www.semanticweb.org/david/ontologies/2013/0/1.3.6.1.4.1.19376.1.8.2.1.10005 -->

    <owl:Class rdf:about="&pathLex;10005">
        <rdfs:subClassOf rdf:resource="&pathLex;10010"/>
        <skos:prefLabel xml:lang="en">Histologic grade</skos:prefLabel>
    </owl:Class>
    


    <!-- http://www.semanticweb.org/david/ontologies/2013/0/1.3.6.1.4.1.19376.1.8.2.1.10008 -->

    <owl:Class rdf:about="&pathLex;10008">
        <rdfs:subClassOf rdf:resource="&pathLex;10013"/>
        <skos:prefLabel xml:lang="en">Target site</skos:prefLabel>
    </owl:Class>
    


    <!-- http://www.semanticweb.org/david/ontologies/2013/0/1.3.6.1.4.1.19376.1.8.2.1.10009 -->

    <owl:Class rdf:about="&pathLex;10009">
        <rdfs:subClassOf rdf:resource="&pathLex;10013"/>
        <skos:prefLabel xml:lang="en">Specimen collection procedure</skos:prefLabel>
    </owl:Class>
    


    <!-- http://www.semanticweb.org/david/ontologies/2013/0/1.3.6.1.4.1.19376.1.8.2.1.10010 -->

    <owl:Class rdf:about="&pathLex;10010">
        <skos:prefLabel xml:lang="en">Generic-Infiltrating malignant neoplasm</skos:prefLabel>
    </owl:Class>
    


    <!-- http://www.semanticweb.org/david/ontologies/2013/0/1.3.6.1.4.1.19376.1.8.2.1.10011 -->

    <owl:Class rdf:about="&pathLex;10011">
        <skos:prefLabel xml:lang="en">Generic-In situ neoplasm</skos:prefLabel>
    </owl:Class>
    


    <!-- http://www.semanticweb.org/david/ontologies/2013/0/1.3.6.1.4.1.19376.1.8.2.1.10012 -->

    <owl:Class rdf:about="&pathLex;10012">
        <rdfs:subClassOf rdf:resource="&owl;Thing"/>
        <skos:prefLabel xml:lang="en">Generic-Lesion</skos:prefLabel>
    </owl:Class>
    


    <!-- http://www.semanticweb.org/david/ontologies/2013/0/1.3.6.1.4.1.19376.1.8.2.1.10013 -->

    <owl:Class rdf:about="&pathLex;10013">
        <rdfs:subClassOf rdf:resource="&owl;Thing"/>
        <skos:prefLabel xml:lang="en">Generic-Specimen</skos:prefLabel>
    </owl:Class>
    


    <!-- http://www.semanticweb.org/david/ontologies/2013/0/1.3.6.1.4.1.19376.1.8.2.1.1006 -->

    <owl:Class rdf:about="&pathLex;1006">
        <rdfs:subClassOf rdf:resource="&pathLex;99999"/>
        <skos:prefLabel xml:lang="en">Adenocarcinoma (acinar, not otherwise specified)</skos:prefLabel>
        <skos:definition xml:lang="en">Prostate-Infiltrating malignant neoplasm-Histologic type-Adenocarcinoma (acinar, not otherwise specified)</skos:definition>
    </owl:Class>
    


    <!-- http://www.semanticweb.org/david/ontologies/2013/0/1.3.6.1.4.1.19376.1.8.2.1.1007 -->

    <owl:Class rdf:about="&pathLex;1007">
        <rdfs:subClassOf rdf:resource="&pathLex;99999"/>
        <skos:definition xml:lang="en">Prostate-Infiltrating malignant neoplasm-Histologic type-Prostatic duct adenocarcinoma</skos:definition>
        <skos:prefLabel xml:lang="en">Prostatic duct adenocarcinoma</skos:prefLabel>
    </owl:Class>
    


    <!-- http://www.semanticweb.org/david/ontologies/2013/0/1.3.6.1.4.1.19376.1.8.2.1.1008 -->

    <owl:Class rdf:about="&pathLex;1008">
        <rdfs:subClassOf rdf:resource="&pathLex;99999"/>
        <skos:prefLabel xml:lang="en">Mucinous (colloid) adenocarcinoma</skos:prefLabel>
        <skos:definition xml:lang="en">Prostate-Infiltrating malignant neoplasm-Histologic type-Mucinous (colloid) adenocarcinoma</skos:definition>
    </owl:Class>
    


    <!-- http://www.semanticweb.org/david/ontologies/2013/0/1.3.6.1.4.1.19376.1.8.2.1.1012 -->

    <owl:Class rdf:about="&pathLex;1012">
        <rdfs:subClassOf rdf:resource="&pathLex;99999"/>
        <skos:prefLabel xml:lang="en">Grade 1</skos:prefLabel>
        <skos:definition xml:lang="en">Prostate-Infiltrating malignant neoplasm-Histologic grade (Gleason-Primary (Predominant) Pattern)-Grade 1</skos:definition>
    </owl:Class>
    


    <!-- http://www.semanticweb.org/david/ontologies/2013/0/1.3.6.1.4.1.19376.1.8.2.1.1013 -->

    <owl:Class rdf:about="&pathLex;1013">
        <rdfs:subClassOf rdf:resource="&pathLex;99999"/>
        <skos:prefLabel xml:lang="en">Grade 2</skos:prefLabel>
        <skos:definition xml:lang="en">Prostate-Infiltrating malignant neoplasm-Histologic grade (Gleason-Primary (Predominant) Pattern)-Grade 2</skos:definition>
    </owl:Class>
    


    <!-- http://www.semanticweb.org/david/ontologies/2013/0/1.3.6.1.4.1.19376.1.8.2.1.1014 -->

    <owl:Class rdf:about="&pathLex;1014">
        <rdfs:subClassOf rdf:resource="&pathLex;99999"/>
        <skos:prefLabel xml:lang="en">Grade 3</skos:prefLabel>
        <skos:definition xml:lang="en">Prostate-Infiltrating malignant neoplasm-Histologic grade (Gleason-Primary (Predominant) Pattern)-Grade 3</skos:definition>
    </owl:Class>
    


    <!-- http://www.semanticweb.org/david/ontologies/2013/0/1.3.6.1.4.1.19376.1.8.2.1.1015 -->

    <owl:Class rdf:about="&pathLex;1015">
        <rdfs:subClassOf rdf:resource="&pathLex;99999"/>
        <skos:prefLabel xml:lang="en">Grade 4</skos:prefLabel>
        <skos:definition xml:lang="en">Prostate-Infiltrating malignant neoplasm-Histologic grade (Gleason-Primary (Predominant) Pattern)-Grade 4</skos:definition>
    </owl:Class>
    


    <!-- http://www.semanticweb.org/david/ontologies/2013/0/1.3.6.1.4.1.19376.1.8.2.1.1016 -->

    <owl:Class rdf:about="&pathLex;1016">
        <rdfs:subClassOf rdf:resource="&pathLex;99999"/>
        <skos:prefLabel xml:lang="en">Grade 5</skos:prefLabel>
        <skos:definition xml:lang="en">Prostate-Infiltrating malignant neoplasm-Histologic grade (Gleason-Primary (Predominant) Pattern)-Grade 5</skos:definition>
    </owl:Class>
    


    <!-- http://www.semanticweb.org/david/ontologies/2013/0/1.3.6.1.4.1.19376.1.8.2.1.1017 -->

    <owl:Class rdf:about="&pathLex;1017">
        <rdfs:subClassOf rdf:resource="&pathLex;99999"/>
        <skos:prefLabel xml:lang="en">Grade 1</skos:prefLabel>
        <skos:definition xml:lang="en">Prostate-Infiltrating malignant neoplasm-Histologic grade (Gleason-Secondary (Worst Remaining) Pattern)-Grade 1</skos:definition>
    </owl:Class>
    


    <!-- http://www.semanticweb.org/david/ontologies/2013/0/1.3.6.1.4.1.19376.1.8.2.1.1018 -->

    <owl:Class rdf:about="&pathLex;1018">
        <rdfs:subClassOf rdf:resource="&pathLex;99999"/>
        <skos:prefLabel xml:lang="en">Grade 2</skos:prefLabel>
        <skos:definition xml:lang="en">Prostate-Infiltrating malignant neoplasm-Histologic grade (Gleason-Secondary (Worst Remaining) Pattern)-Grade 2</skos:definition>
    </owl:Class>
    


    <!-- http://www.semanticweb.org/david/ontologies/2013/0/1.3.6.1.4.1.19376.1.8.2.1.1019 -->

    <owl:Class rdf:about="&pathLex;1019">
        <rdfs:subClassOf rdf:resource="&pathLex;99999"/>
        <skos:prefLabel xml:lang="en">Grade 3</skos:prefLabel>
        <skos:definition xml:lang="en">Prostate-Infiltrating malignant neoplasm-Histologic grade (Gleason-Secondary (Worst Remaining) Pattern)-Grade 3</skos:definition>
    </owl:Class>
    


    <!-- http://www.semanticweb.org/david/ontologies/2013/0/1.3.6.1.4.1.19376.1.8.2.1.1020 -->

    <owl:Class rdf:about="&pathLex;1020">
        <rdfs:subClassOf rdf:resource="&pathLex;99999"/>
        <skos:prefLabel xml:lang="en">Grade 4</skos:prefLabel>
        <skos:definition xml:lang="en">Prostate-Infiltrating malignant neoplasm-Histologic grade (Gleason-Secondary (Worst Remaining) Pattern)-Grade 4</skos:definition>
    </owl:Class>
    


    <!-- http://www.semanticweb.org/david/ontologies/2013/0/1.3.6.1.4.1.19376.1.8.2.1.1021 -->

    <owl:Class rdf:about="&pathLex;1021">
        <rdfs:subClassOf rdf:resource="&pathLex;99999"/>
        <skos:prefLabel xml:lang="en">Grade 5</skos:prefLabel>
        <skos:definition xml:lang="en">Prostate-Infiltrating malignant neoplasm-Histologic grade (Gleason-Secondary (Worst Remaining) Pattern)-Grade 5</skos:definition>
    </owl:Class>
    


    <!-- http://www.semanticweb.org/david/ontologies/2013/0/1.3.6.1.4.1.19376.1.8.2.1.1022 -->

    <owl:Class rdf:about="&pathLex;1022">
        <rdfs:subClassOf rdf:resource="&pathLex;99999"/>
        <skos:prefLabel xml:lang="en">Grade 3</skos:prefLabel>
        <skos:definition xml:lang="en">Prostate-Infiltrating malignant neoplasm-Histologic grade (Gleason-Tertiary Pattern)-Grade 3</skos:definition>
    </owl:Class>
    


    <!-- http://www.semanticweb.org/david/ontologies/2013/0/1.3.6.1.4.1.19376.1.8.2.1.1023 -->

    <owl:Class rdf:about="&pathLex;1023">
        <rdfs:subClassOf rdf:resource="&pathLex;99999"/>
        <skos:prefLabel xml:lang="en">Grade 4</skos:prefLabel>
        <skos:definition xml:lang="en">Prostate-Infiltrating malignant neoplasm-Histologic grade (Gleason-Tertiary Pattern)-Grade 4</skos:definition>
    </owl:Class>
    


    <!-- http://www.semanticweb.org/david/ontologies/2013/0/1.3.6.1.4.1.19376.1.8.2.1.1024 -->

    <owl:Class rdf:about="&pathLex;1024">
        <rdfs:subClassOf rdf:resource="&pathLex;99999"/>
        <skos:prefLabel xml:lang="en">Grade 5</skos:prefLabel>
        <skos:definition xml:lang="en">Prostate-Infiltrating malignant neoplasm-Histologic grade (Gleason-Tertiary Pattern)-Grade 5</skos:definition>
    </owl:Class>
    


    <!-- http://www.semanticweb.org/david/ontologies/2013/0/1.3.6.1.4.1.19376.1.8.2.1.1025 -->

    <owl:Class rdf:about="&pathLex;1025">
        <rdfs:subClassOf rdf:resource="&pathLex;99999"/>
        <skos:prefLabel xml:lang="en">2</skos:prefLabel>
        <skos:definition xml:lang="en">Prostate-Infiltrating malignant neoplasm-Histologic grade (Gleason-Total Gleason Score)-2</skos:definition>
    </owl:Class>
    


    <!-- http://www.semanticweb.org/david/ontologies/2013/0/1.3.6.1.4.1.19376.1.8.2.1.1026 -->

    <owl:Class rdf:about="&pathLex;1026">
        <rdfs:subClassOf rdf:resource="&pathLex;99999"/>
        <skos:prefLabel xml:lang="en">3</skos:prefLabel>
        <skos:definition xml:lang="en">Prostate-Infiltrating malignant neoplasm-Histologic grade (Gleason-Total Gleason Score)-3</skos:definition>
    </owl:Class>
    


    <!-- http://www.semanticweb.org/david/ontologies/2013/0/1.3.6.1.4.1.19376.1.8.2.1.1027 -->

    <owl:Class rdf:about="&pathLex;1027">
        <rdfs:subClassOf rdf:resource="&pathLex;99999"/>
        <skos:prefLabel xml:lang="en">4</skos:prefLabel>
        <skos:definition xml:lang="en">Prostate-Infiltrating malignant neoplasm-Histologic grade (Gleason-Total Gleason Score)-4</skos:definition>
    </owl:Class>
    


    <!-- http://www.semanticweb.org/david/ontologies/2013/0/1.3.6.1.4.1.19376.1.8.2.1.1028 -->

    <owl:Class rdf:about="&pathLex;1028">
        <rdfs:subClassOf rdf:resource="&pathLex;99999"/>
        <skos:prefLabel xml:lang="en">5</skos:prefLabel>
        <skos:definition xml:lang="en">Prostate-Infiltrating malignant neoplasm-Histologic grade (Gleason-Total Gleason Score)-5</skos:definition>
    </owl:Class>
    


    <!-- http://www.semanticweb.org/david/ontologies/2013/0/1.3.6.1.4.1.19376.1.8.2.1.1029 -->

    <owl:Class rdf:about="&pathLex;1029">
        <rdfs:subClassOf rdf:resource="&pathLex;99999"/>
        <skos:prefLabel xml:lang="en">6</skos:prefLabel>
        <skos:definition xml:lang="en">Prostate-Infiltrating malignant neoplasm-Histologic grade (Gleason-Total Gleason Score)-6</skos:definition>
    </owl:Class>
    


    <!-- http://www.semanticweb.org/david/ontologies/2013/0/1.3.6.1.4.1.19376.1.8.2.1.1030 -->

    <owl:Class rdf:about="&pathLex;1030">
        <rdfs:subClassOf rdf:resource="&pathLex;99999"/>
        <skos:prefLabel xml:lang="en">7</skos:prefLabel>
        <skos:definition xml:lang="en">Prostate-Infiltrating malignant neoplasm-Histologic grade (Gleason-Total Gleason Score)-7</skos:definition>
    </owl:Class>
    


    <!-- http://www.semanticweb.org/david/ontologies/2013/0/1.3.6.1.4.1.19376.1.8.2.1.1031 -->

    <owl:Class rdf:about="&pathLex;1031">
        <rdfs:subClassOf rdf:resource="&pathLex;99999"/>
        <skos:prefLabel xml:lang="en">8</skos:prefLabel>
        <skos:definition xml:lang="en">Prostate-Infiltrating malignant neoplasm-Histologic grade (Gleason-Total Gleason Score)-8</skos:definition>
    </owl:Class>
    


    <!-- http://www.semanticweb.org/david/ontologies/2013/0/1.3.6.1.4.1.19376.1.8.2.1.1032 -->

    <owl:Class rdf:about="&pathLex;1032">
        <rdfs:subClassOf rdf:resource="&pathLex;99999"/>
        <skos:prefLabel xml:lang="en">9</skos:prefLabel>
        <skos:definition xml:lang="en">Prostate-Infiltrating malignant neoplasm-Histologic grade (Gleason-Total Gleason Score)-9</skos:definition>
    </owl:Class>
    


    <!-- http://www.semanticweb.org/david/ontologies/2013/0/1.3.6.1.4.1.19376.1.8.2.1.1033 -->

    <owl:Class rdf:about="&pathLex;1033">
        <rdfs:subClassOf rdf:resource="&pathLex;99999"/>
        <skos:prefLabel xml:lang="en">10</skos:prefLabel>
        <skos:definition xml:lang="en">Prostate-Infiltrating malignant neoplasm-Histologic grade (Gleason-Total Gleason Score)-10</skos:definition>
    </owl:Class>
    


    <!-- http://www.semanticweb.org/david/ontologies/2013/0/1.3.6.1.4.1.19376.1.8.2.1.1036 -->

    <owl:Class rdf:about="&pathLex;1036">
        <rdfs:subClassOf rdf:resource="&pathLex;99999"/>
        <skos:definition xml:lang="en">Prostate-Infiltrating malignant neoplasm-pT-pT2: Organ confined</skos:definition>
        <skos:prefLabel xml:lang="en">pT2: Organ confined</skos:prefLabel>
    </owl:Class>
    


    <!-- http://www.semanticweb.org/david/ontologies/2013/0/1.3.6.1.4.1.19376.1.8.2.1.1037 -->

    <owl:Class rdf:about="&pathLex;1037">
        <rdfs:subClassOf rdf:resource="&pathLex;99999"/>
        <skos:definition xml:lang="en">Prostate-Infiltrating malignant neoplasm-pT-pT2a: Unilateral, involving one-half of 1 side or less</skos:definition>
        <skos:prefLabel xml:lang="en">pT2a: Unilateral, involving one-half of 1 side or less</skos:prefLabel>
    </owl:Class>
    


    <!-- http://www.semanticweb.org/david/ontologies/2013/0/1.3.6.1.4.1.19376.1.8.2.1.1038 -->

    <owl:Class rdf:about="&pathLex;1038">
        <rdfs:subClassOf rdf:resource="&pathLex;99999"/>
        <skos:definition xml:lang="en">Prostate-Infiltrating malignant neoplasm-pT-pT2b: Unilateral, involving more than one-half of 1 side but not both sides</skos:definition>
        <skos:prefLabel xml:lang="en">pT2b: Unilateral, involving more than one-half of 1 side but not both sides</skos:prefLabel>
    </owl:Class>
    


    <!-- http://www.semanticweb.org/david/ontologies/2013/0/1.3.6.1.4.1.19376.1.8.2.1.1039 -->

    <owl:Class rdf:about="&pathLex;1039">
        <rdfs:subClassOf rdf:resource="&pathLex;99999"/>
        <skos:definition xml:lang="en">Prostate-Infiltrating malignant neoplasm-pT-pT2c: Bilateral disease</skos:definition>
        <skos:prefLabel xml:lang="en">pT2c: Bilateral disease</skos:prefLabel>
    </owl:Class>
    


    <!-- http://www.semanticweb.org/david/ontologies/2013/0/1.3.6.1.4.1.19376.1.8.2.1.1040 -->

    <owl:Class rdf:about="&pathLex;1040">
        <rdfs:subClassOf rdf:resource="&pathLex;99999"/>
        <skos:definition xml:lang="en">Prostate-Infiltrating malignant neoplasm-pT-pT3: Extraprostatic extension</skos:definition>
        <skos:prefLabel xml:lang="en">pT3: Extraprostatic extension</skos:prefLabel>
    </owl:Class>
    


    <!-- http://www.semanticweb.org/david/ontologies/2013/0/1.3.6.1.4.1.19376.1.8.2.1.1041 -->

    <owl:Class rdf:about="&pathLex;1041">
        <rdfs:subClassOf rdf:resource="&pathLex;99999"/>
        <skos:definition xml:lang="en">Prostate-Infiltrating malignant neoplasm-pT-pT3a: Extraprostatic extension or microscopic invasion of bladder neck</skos:definition>
        <skos:prefLabel xml:lang="en">pT3a: Extraprostatic extension or microscopic invasion of bladder neck</skos:prefLabel>
    </owl:Class>
    


    <!-- http://www.semanticweb.org/david/ontologies/2013/0/1.3.6.1.4.1.19376.1.8.2.1.1042 -->

    <owl:Class rdf:about="&pathLex;1042">
        <rdfs:subClassOf rdf:resource="&pathLex;99999"/>
        <skos:definition xml:lang="en">Prostate-Infiltrating malignant neoplasm-pT-pT3b: Seminal vesicle invasion</skos:definition>
        <skos:prefLabel xml:lang="en">pT3b: Seminal vesicle invasion</skos:prefLabel>
    </owl:Class>
    


    <!-- http://www.semanticweb.org/david/ontologies/2013/0/1.3.6.1.4.1.19376.1.8.2.1.1043 -->

    <owl:Class rdf:about="&pathLex;1043">
        <rdfs:subClassOf rdf:resource="&pathLex;99999"/>
        <skos:definition xml:lang="en">Prostate-Infiltrating malignant neoplasm-pT-pT4: Invasion of rectum, levator muscles and/or pelvic wall (Note J)</skos:definition>
        <skos:prefLabel xml:lang="en">pT4: Invasion of rectum, levator muscles and/or pelvic wall (Note J)</skos:prefLabel>
    </owl:Class>
    


    <!-- http://www.semanticweb.org/david/ontologies/2013/0/1.3.6.1.4.1.19376.1.8.2.1.1044 -->

    <owl:Class rdf:about="&pathLex;1044">
        <rdfs:subClassOf rdf:resource="&pathLex;99999"/>
        <skos:definition xml:lang="en">Prostate-Infiltrating malignant neoplasm-pN-pN0: No regional lymph node metastasis</skos:definition>
        <skos:prefLabel xml:lang="en">pN0: No regional lymph node metastasis</skos:prefLabel>
    </owl:Class>
    


    <!-- http://www.semanticweb.org/david/ontologies/2013/0/1.3.6.1.4.1.19376.1.8.2.1.1045 -->

    <owl:Class rdf:about="&pathLex;1045">
        <rdfs:subClassOf rdf:resource="&pathLex;99999"/>
        <skos:definition xml:lang="en">Prostate-Infiltrating malignant neoplasm-pN-pN1: Metastasis in regional lymph node or nodes</skos:definition>
        <skos:prefLabel xml:lang="en">pN1: Metastasis in regional lymph node or nodes</skos:prefLabel>
    </owl:Class>
    


    <!-- http://www.semanticweb.org/david/ontologies/2013/0/1.3.6.1.4.1.19376.1.8.2.1.1046 -->

    <owl:Class rdf:about="&pathLex;1046">
        <rdfs:subClassOf rdf:resource="&pathLex;99999"/>
        <skos:prefLabel xml:lang="en">Testis</skos:prefLabel>
        <skos:definition xml:lang="en">Testis-Specimen-Target site-Testis</skos:definition>
    </owl:Class>
    


    <!-- http://www.semanticweb.org/david/ontologies/2013/0/1.3.6.1.4.1.19376.1.8.2.1.1047 -->

    <owl:Class rdf:about="&pathLex;1047">
        <rdfs:subClassOf rdf:resource="&pathLex;99999"/>
        <skos:prefLabel xml:lang="en">Radical Orchiectomy</skos:prefLabel>
        <skos:definition xml:lang="en">Testis-Specimen-Specimen collection procedure-Radical Orchiectomy</skos:definition>
    </owl:Class>
    


    <!-- http://www.semanticweb.org/david/ontologies/2013/0/1.3.6.1.4.1.19376.1.8.2.1.1049 -->

    <owl:Class rdf:about="&pathLex;1049">
        <rdfs:subClassOf rdf:resource="&pathLex;99999"/>
        <skos:prefLabel xml:lang="en">Teratoma</skos:prefLabel>
        <skos:definition xml:lang="en">Testis-Infiltrating malignant neoplasm-Histologic type-Teratoma</skos:definition>
    </owl:Class>
    


    <!-- http://www.semanticweb.org/david/ontologies/2013/0/1.3.6.1.4.1.19376.1.8.2.1.1050 -->

    <owl:Class rdf:about="&pathLex;1050">
        <rdfs:subClassOf rdf:resource="&pathLex;99999"/>
        <skos:prefLabel xml:lang="en">Intratubular germ cell neoplasia, unclassified only</skos:prefLabel>
        <skos:definition xml:lang="en">Testis-Infiltrating malignant neoplasm-Histologic type-Intratubular germ cell neoplasia, unclassified only</skos:definition>
    </owl:Class>
    


    <!-- http://www.semanticweb.org/david/ontologies/2013/0/1.3.6.1.4.1.19376.1.8.2.1.1051 -->

    <owl:Class rdf:about="&pathLex;1051">
        <rdfs:subClassOf rdf:resource="&pathLex;99999"/>
        <skos:prefLabel xml:lang="en">Seminoma, classic type</skos:prefLabel>
        <skos:definition xml:lang="en">Testis-Infiltrating malignant neoplasm-Histologic type-Seminoma, classic type</skos:definition>
    </owl:Class>
    


    <!-- http://www.semanticweb.org/david/ontologies/2013/0/1.3.6.1.4.1.19376.1.8.2.1.1052 -->

    <owl:Class rdf:about="&pathLex;1052">
        <rdfs:subClassOf rdf:resource="&pathLex;99999"/>
        <skos:prefLabel xml:lang="en">Mixed germ cell tumor</skos:prefLabel>
        <skos:definition xml:lang="en">Testis-Infiltrating malignant neoplasm-Histologic type-Mixed germ cell tumor</skos:definition>
    </owl:Class>
    


    <!-- http://www.semanticweb.org/david/ontologies/2013/0/1.3.6.1.4.1.19376.1.8.2.1.1054 -->

    <owl:Class rdf:about="&pathLex;1054">
        <rdfs:subClassOf rdf:resource="&pathLex;99999"/>
        <skos:definition xml:lang="en">Testis-Infiltrating malignant neoplasm-Histologic type-Yolk sac tumor</skos:definition>
        <skos:prefLabel xml:lang="en">Yolk sac tumor</skos:prefLabel>
    </owl:Class>
    


    <!-- http://www.semanticweb.org/david/ontologies/2013/0/1.3.6.1.4.1.19376.1.8.2.1.1056 -->

    <owl:Class rdf:about="&pathLex;1056">
        <rdfs:subClassOf rdf:resource="&pathLex;99999"/>
        <skos:prefLabel xml:lang="en">Testicular scar only</skos:prefLabel>
        <skos:definition xml:lang="en">Testis-Infiltrating malignant neoplasm-Histologic type-Testicular scar only</skos:definition>
    </owl:Class>
    


    <!-- http://www.semanticweb.org/david/ontologies/2013/0/1.3.6.1.4.1.19376.1.8.2.1.1060 -->

    <owl:Class rdf:about="&pathLex;1060">
        <rdfs:subClassOf rdf:resource="&pathLex;99999"/>
        <skos:prefLabel xml:lang="en">Spermatic Cord Margin</skos:prefLabel>
        <skos:definition xml:lang="en">Testis-Infiltrating malignant neoplasm-Margin site-Spermatic Cord Margin</skos:definition>
    </owl:Class>
    


    <!-- http://www.semanticweb.org/david/ontologies/2013/0/1.3.6.1.4.1.19376.1.8.2.1.1061 -->

    <owl:Class rdf:about="&pathLex;1061">
        <rdfs:subClassOf rdf:resource="&pathLex;99999"/>
        <skos:definition xml:lang="en">Testis-Infiltrating malignant neoplasm-pT-pT0: No evidence of primary tumor</skos:definition>
        <skos:prefLabel xml:lang="en">pT0: No evidence of primary tumor</skos:prefLabel>
    </owl:Class>
    


    <!-- http://www.semanticweb.org/david/ontologies/2013/0/1.3.6.1.4.1.19376.1.8.2.1.1062 -->

    <owl:Class rdf:about="&pathLex;1062">
        <rdfs:subClassOf rdf:resource="&pathLex;99999"/>
        <skos:definition xml:lang="en">Testis-Infiltrating malignant neoplasm-pT-pTis: Intratubular germ cell neoplasia (carcinoma in situ)</skos:definition>
        <skos:prefLabel xml:lang="en">pTis: Intratubular germ cell neoplasia (carcinoma in situ)</skos:prefLabel>
    </owl:Class>
    


    <!-- http://www.semanticweb.org/david/ontologies/2013/0/1.3.6.1.4.1.19376.1.8.2.1.1063 -->

    <owl:Class rdf:about="&pathLex;1063">
        <rdfs:subClassOf rdf:resource="&pathLex;99999"/>
        <skos:definition xml:lang="en">Testis-Infiltrating malignant neoplasm-pT-pT1: Tumor limited to the testis and epididymis without vascular/lymphatic invasion; tumor may invade tunica albuginea but not tunica vaginalis</skos:definition>
        <skos:prefLabel xml:lang="en">pT1: Tumor limited to the testis and epididymis without vascular/lymphatic invasion; tumor may invade tunica albuginea but not tunica vaginalis</skos:prefLabel>
    </owl:Class>
    


    <!-- http://www.semanticweb.org/david/ontologies/2013/0/1.3.6.1.4.1.19376.1.8.2.1.1064 -->

    <owl:Class rdf:about="&pathLex;1064">
        <rdfs:subClassOf rdf:resource="&pathLex;99999"/>
        <skos:definition xml:lang="en">Testis-Infiltrating malignant neoplasm-pT-pT2: Tumor limited to the testis and epididymis with vascular/lymphatic invasion, or tumor extending through the tunica albuginea with involvement of the tunica vaginalis</skos:definition>
        <skos:prefLabel xml:lang="en">pT2: Tumor limited to the testis and epididymis with vascular/lymphatic invasion, or tumor extending through the tunica albuginea with involvement of the tunica vaginalis</skos:prefLabel>
    </owl:Class>
    


    <!-- http://www.semanticweb.org/david/ontologies/2013/0/1.3.6.1.4.1.19376.1.8.2.1.1065 -->

    <owl:Class rdf:about="&pathLex;1065">
        <rdfs:subClassOf rdf:resource="&pathLex;99999"/>
        <skos:definition xml:lang="en">Testis-Infiltrating malignant neoplasm-pT-pT3: Tumor invades the spermatic cord with or without vascular/lymphatic invasion</skos:definition>
        <skos:prefLabel xml:lang="en">pT3: Tumor invades the spermatic cord with or without vascular/lymphatic invasion</skos:prefLabel>
    </owl:Class>
    


    <!-- http://www.semanticweb.org/david/ontologies/2013/0/1.3.6.1.4.1.19376.1.8.2.1.1066 -->

    <owl:Class rdf:about="&pathLex;1066">
        <rdfs:subClassOf rdf:resource="&pathLex;99999"/>
        <skos:definition xml:lang="en">Testis-Infiltrating malignant neoplasm-pT-pTX: Cannot be assessed
pT0: No evidence of primary tumor
pTis: Intratubular germ cell neoplasia (carcinoma in situ)
pT1: Tumor limited to the testis and epididymis without vascular/lymphatic
invasion; tumor may invade tunica albuginea but not tunica vaginalis
pT2: Tumor limited to the testis and epididymis with vascular/lymphatic invasion, or
tumor extending through the tunica albuginea with involvement of the tunica
vaginalis
pT3: Tumor invades the spermatic cord with or without vascular/lymphatic invasion
pT4: Tumor invades the scrotum with or without vascular/lymphatic invasion</skos:definition>
        <skos:prefLabel xml:lang="en">pTX: Cannot be assessed
pT0: No evidence of primary tumor
pTis: Intratubular germ cell neoplasia (carcinoma in situ)
pT1: Tumor limited to the testis and epididymis without vascular/lymphatic
invasion; tumor may invade tunica albuginea but not tunica vaginalis
pT2: Tumor limited to the testis and epididymis with vascular/lymphatic invasion, or
tumor extending through the tunica albuginea with involvement of the tunica
vaginalis
pT3: Tumor invades the spermatic cord with or without vascular/lymphatic invasion
pT4: Tumor invades the scrotum with or without vascular/lymphatic invasion</skos:prefLabel>
    </owl:Class>
    


    <!-- http://www.semanticweb.org/david/ontologies/2013/0/1.3.6.1.4.1.19376.1.8.2.1.1067 -->

    <owl:Class rdf:about="&pathLex;1067">
        <rdfs:subClassOf rdf:resource="&pathLex;99999"/>
        <skos:definition xml:lang="en">Testis-Infiltrating malignant neoplasm-pN-pN0: No regional lymph node metastasis</skos:definition>
        <skos:prefLabel xml:lang="en">pN0: No regional lymph node metastasis</skos:prefLabel>
    </owl:Class>
    


    <!-- http://www.semanticweb.org/david/ontologies/2013/0/1.3.6.1.4.1.19376.1.8.2.1.1068 -->

    <owl:Class rdf:about="&pathLex;1068">
        <rdfs:subClassOf rdf:resource="&pathLex;99999"/>
        <skos:definition xml:lang="en">Testis-Infiltrating malignant neoplasm-pN-pN1: Metastasis with a lymph node mass 2 cm or less in greatest dimension, or 5 or fewer positive nodes, none more than 2 cm in greatest dimension</skos:definition>
        <skos:prefLabel xml:lang="en">pN1: Metastasis with a lymph node mass 2 cm or less in greatest dimension, or 5 or fewer positive nodes, none more than 2 cm in greatest dimension</skos:prefLabel>
    </owl:Class>
    


    <!-- http://www.semanticweb.org/david/ontologies/2013/0/1.3.6.1.4.1.19376.1.8.2.1.1069 -->

    <owl:Class rdf:about="&pathLex;1069">
        <rdfs:subClassOf rdf:resource="&pathLex;99999"/>
        <skos:definition xml:lang="en">Testis-Infiltrating malignant neoplasm-pN-pN2: Metastasis with a lymph node mass greater than 2 cm but not more than 5 cm in greatest dimension; or more than 5 nodes positive, none greater than 5 cm; or evidence of extranodal extension of tumor</skos:definition>
        <skos:prefLabel xml:lang="en">pN2: Metastasis with a lymph node mass greater than 2 cm but not more than 5 cm in greatest dimension; or more than 5 nodes positive, none greater than 5 cm; or evidence of extranodal extension of tumor</skos:prefLabel>
    </owl:Class>
    


    <!-- http://www.semanticweb.org/david/ontologies/2013/0/1.3.6.1.4.1.19376.1.8.2.1.1070 -->

    <owl:Class rdf:about="&pathLex;1070">
        <rdfs:subClassOf rdf:resource="&pathLex;99999"/>
        <skos:definition xml:lang="en">Testis-Infiltrating malignant neoplasm-pN-pN3: Metastasis with a lymph node mass greater than 5 cm in greatest dimension</skos:definition>
        <skos:prefLabel xml:lang="en">pN3: Metastasis with a lymph node mass greater than 5 cm in greatest dimension</skos:prefLabel>
    </owl:Class>
    


    <!-- http://www.semanticweb.org/david/ontologies/2013/0/1.3.6.1.4.1.19376.1.8.2.1.1071 -->

    <owl:Class rdf:about="&pathLex;1071">
        <rdfs:subClassOf rdf:resource="&pathLex;99999"/>
        <skos:definition xml:lang="en">Kidney-Specimen-Specimen collection procedure-Partial nephrectomy</skos:definition>
        <skos:prefLabel xml:lang="en">Partial nephrectomy</skos:prefLabel>
    </owl:Class>
    


    <!-- http://www.semanticweb.org/david/ontologies/2013/0/1.3.6.1.4.1.19376.1.8.2.1.1072 -->

    <owl:Class rdf:about="&pathLex;1072">
        <rdfs:subClassOf rdf:resource="&pathLex;99999"/>
        <skos:definition xml:lang="en">Kidney-Specimen-Specimen collection procedure-Radical nephrectomy</skos:definition>
        <skos:prefLabel xml:lang="en">Radical nephrectomy</skos:prefLabel>
    </owl:Class>
    


    <!-- http://www.semanticweb.org/david/ontologies/2013/0/1.3.6.1.4.1.19376.1.8.2.1.1074 -->

    <owl:Class rdf:about="&pathLex;1074">
        <rdfs:subClassOf rdf:resource="&pathLex;99999"/>
        <skos:definition xml:lang="en">Kidney-Infiltrating malignant neoplasm-Lesion site-Upper pole</skos:definition>
        <skos:prefLabel xml:lang="en">Upper pole</skos:prefLabel>
    </owl:Class>
    


    <!-- http://www.semanticweb.org/david/ontologies/2013/0/1.3.6.1.4.1.19376.1.8.2.1.1075 -->

    <owl:Class rdf:about="&pathLex;1075">
        <rdfs:subClassOf rdf:resource="&pathLex;99999"/>
        <skos:definition xml:lang="en">Kidney-Infiltrating malignant neoplasm-Lesion site-Middle</skos:definition>
        <skos:prefLabel xml:lang="en">Middle</skos:prefLabel>
    </owl:Class>
    


    <!-- http://www.semanticweb.org/david/ontologies/2013/0/1.3.6.1.4.1.19376.1.8.2.1.1076 -->

    <owl:Class rdf:about="&pathLex;1076">
        <rdfs:subClassOf rdf:resource="&pathLex;99999"/>
        <skos:definition xml:lang="en">Kidney-Infiltrating malignant neoplasm-Lesion site-Lower pole</skos:definition>
        <skos:prefLabel xml:lang="en">Lower pole</skos:prefLabel>
    </owl:Class>
    


    <!-- http://www.semanticweb.org/david/ontologies/2013/0/1.3.6.1.4.1.19376.1.8.2.1.1077 -->

    <owl:Class rdf:about="&pathLex;1077">
        <rdfs:subClassOf rdf:resource="&pathLex;99999"/>
        <skos:prefLabel xml:lang="en">Kidney</skos:prefLabel>
        <skos:definition xml:lang="en">Kidney-Infiltrating malignant neoplasm-Lesion site-Kidney</skos:definition>
    </owl:Class>
    


    <!-- http://www.semanticweb.org/david/ontologies/2013/0/1.3.6.1.4.1.19376.1.8.2.1.1078 -->

    <owl:Class rdf:about="&pathLex;1078">
        <rdfs:subClassOf rdf:resource="&pathLex;99999"/>
        <skos:prefLabel xml:lang="en">Clear cell renal cell carcinoma</skos:prefLabel>
        <skos:definition xml:lang="en">Kidney-Infiltrating malignant neoplasm-Histologic type-Clear cell renal cell carcinoma</skos:definition>
    </owl:Class>
    


    <!-- http://www.semanticweb.org/david/ontologies/2013/0/1.3.6.1.4.1.19376.1.8.2.1.1079 -->

    <owl:Class rdf:about="&pathLex;1079">
        <rdfs:subClassOf rdf:resource="&pathLex;99999"/>
        <skos:prefLabel xml:lang="en">Chromophobe renal cell carcinoma</skos:prefLabel>
        <skos:definition xml:lang="en">Kidney-Infiltrating malignant neoplasm-Histologic type-Chromophobe renal cell carcinoma</skos:definition>
    </owl:Class>
    


    <!-- http://www.semanticweb.org/david/ontologies/2013/0/1.3.6.1.4.1.19376.1.8.2.1.1080 -->

    <owl:Class rdf:about="&pathLex;1080">
        <rdfs:subClassOf rdf:resource="&pathLex;99999"/>
        <skos:prefLabel xml:lang="en">Carcinoma of the collecting ducts of Bellini</skos:prefLabel>
        <skos:definition xml:lang="en">Kidney-Infiltrating malignant neoplasm-Histologic type-Carcinoma of the collecting ducts of Bellini</skos:definition>
    </owl:Class>
    


    <!-- http://www.semanticweb.org/david/ontologies/2013/0/1.3.6.1.4.1.19376.1.8.2.1.1081 -->

    <owl:Class rdf:about="&pathLex;1081">
        <rdfs:subClassOf rdf:resource="&pathLex;99999"/>
        <skos:definition xml:lang="en">Kidney-Infiltrating malignant neoplasm-Histologic type-Renal medullary carcinoma</skos:definition>
        <skos:prefLabel xml:lang="en">Renal medullary carcinoma</skos:prefLabel>
    </owl:Class>
    


    <!-- http://www.semanticweb.org/david/ontologies/2013/0/1.3.6.1.4.1.19376.1.8.2.1.1084 -->

    <owl:Class rdf:about="&pathLex;1084">
        <rdfs:subClassOf rdf:resource="&pathLex;99999"/>
        <skos:prefLabel xml:lang="en">G1: Nuclei round, uniform, approximately 10 mm; nucleoli inconspicuous or absent</skos:prefLabel>
        <skos:definition xml:lang="en">Kidney-Infiltrating malignant neoplasm-Histologic grade (Fuhrman Nuclear Grade)-G1: Nuclei round, uniform, approximately 10 mm; nucleoli inconspicuous or absent</skos:definition>
    </owl:Class>
    


    <!-- http://www.semanticweb.org/david/ontologies/2013/0/1.3.6.1.4.1.19376.1.8.2.1.1085 -->

    <owl:Class rdf:about="&pathLex;1085">
        <rdfs:subClassOf rdf:resource="&pathLex;99999"/>
        <skos:prefLabel xml:lang="en">G2: Nuclei slightly irregular, approximately 15 mm; nucleoli evident</skos:prefLabel>
        <skos:definition xml:lang="en">Kidney-Infiltrating malignant neoplasm-Histologic grade (Fuhrman Nuclear Grade)-G2: Nuclei slightly irregular, approximately 15 mm; nucleoli evident</skos:definition>
    </owl:Class>
    


    <!-- http://www.semanticweb.org/david/ontologies/2013/0/1.3.6.1.4.1.19376.1.8.2.1.1086 -->

    <owl:Class rdf:about="&pathLex;1086">
        <rdfs:subClassOf rdf:resource="&pathLex;99999"/>
        <skos:prefLabel xml:lang="en">G3: Nuclei very irregular, approximately 20 mm; nucleoli large and proeminent</skos:prefLabel>
        <skos:definition xml:lang="en">Kidney-Infiltrating malignant neoplasm-Histologic grade (Fuhrman Nuclear Grade)-G3: Nuclei very irregular, approximately 20 mm; nucleoli large and proeminent</skos:definition>
    </owl:Class>
    


    <!-- http://www.semanticweb.org/david/ontologies/2013/0/1.3.6.1.4.1.19376.1.8.2.1.1087 -->

    <owl:Class rdf:about="&pathLex;1087">
        <rdfs:subClassOf rdf:resource="&pathLex;99999"/>
        <skos:prefLabel xml:lang="en">G4: Nuclei bizarre and multilobated, 20 mm or greater, nucleoli prominent, chromatin clumped</skos:prefLabel>
        <skos:definition xml:lang="en">Kidney-Infiltrating malignant neoplasm-Histologic grade (Fuhrman Nuclear Grade)-G4: Nuclei bizarre and multilobated, 20 mm or greater, nucleoli prominent, chromatin clumped</skos:definition>
    </owl:Class>
    


    <!-- http://www.semanticweb.org/david/ontologies/2013/0/1.3.6.1.4.1.19376.1.8.2.1.1093 -->

    <owl:Class rdf:about="&pathLex;1093">
        <rdfs:subClassOf rdf:resource="&pathLex;99999"/>
        <skos:definition xml:lang="en">Kidney-Infiltrating malignant neoplasm-Margin site-Renal parenchymal margin (partial nephrectomy only)</skos:definition>
        <skos:prefLabel xml:lang="en">Renal parenchymal margin (partial nephrectomy only)</skos:prefLabel>
    </owl:Class>
    


    <!-- http://www.semanticweb.org/david/ontologies/2013/0/1.3.6.1.4.1.19376.1.8.2.1.1094 -->

    <owl:Class rdf:about="&pathLex;1094">
        <rdfs:subClassOf rdf:resource="&pathLex;99999"/>
        <skos:definition xml:lang="en">Kidney-Infiltrating malignant neoplasm-Margin site-Renal vein margin</skos:definition>
        <skos:prefLabel xml:lang="en">Renal vein margin</skos:prefLabel>
    </owl:Class>
    


    <!-- http://www.semanticweb.org/david/ontologies/2013/0/1.3.6.1.4.1.19376.1.8.2.1.1095 -->

    <owl:Class rdf:about="&pathLex;1095">
        <rdfs:subClassOf rdf:resource="&pathLex;99999"/>
        <skos:definition xml:lang="en">Kidney-Infiltrating malignant neoplasm-pT-pT0: No evidence of primary tumor</skos:definition>
        <skos:prefLabel xml:lang="en">pT0: No evidence of primary tumor</skos:prefLabel>
    </owl:Class>
    


    <!-- http://www.semanticweb.org/david/ontologies/2013/0/1.3.6.1.4.1.19376.1.8.2.1.1096 -->

    <owl:Class rdf:about="&pathLex;1096">
        <rdfs:subClassOf rdf:resource="&pathLex;99999"/>
        <skos:definition xml:lang="en">Kidney-Infiltrating malignant neoplasm-pT-pT1: Tumor 7 cm or less in greatest dimension, limited to the kidney</skos:definition>
        <skos:prefLabel xml:lang="en">pT1: Tumor 7 cm or less in greatest dimension, limited to the kidney</skos:prefLabel>
    </owl:Class>
    


    <!-- http://www.semanticweb.org/david/ontologies/2013/0/1.3.6.1.4.1.19376.1.8.2.1.1097 -->

    <owl:Class rdf:about="&pathLex;1097">
        <rdfs:subClassOf rdf:resource="&pathLex;99999"/>
        <skos:definition xml:lang="en">Kidney-Infiltrating malignant neoplasm-pT-pT1a: Tumor 4 cm or less in greatest dimension, limited to the kidney</skos:definition>
        <skos:prefLabel xml:lang="en">pT1a: Tumor 4 cm or less in greatest dimension, limited to the kidney</skos:prefLabel>
    </owl:Class>
    


    <!-- http://www.semanticweb.org/david/ontologies/2013/0/1.3.6.1.4.1.19376.1.8.2.1.1098 -->

    <owl:Class rdf:about="&pathLex;1098">
        <rdfs:subClassOf rdf:resource="&pathLex;99999"/>
        <skos:definition xml:lang="en">Kidney-Infiltrating malignant neoplasm-pT-pT1b: Tumor more than 4 cm but not more than 7 cm in greatest dimension, limited to the kidney</skos:definition>
        <skos:prefLabel xml:lang="en">pT1b: Tumor more than 4 cm but not more than 7 cm in greatest dimension, limited to the kidney</skos:prefLabel>
    </owl:Class>
    


    <!-- http://www.semanticweb.org/david/ontologies/2013/0/1.3.6.1.4.1.19376.1.8.2.1.1099 -->

    <owl:Class rdf:about="&pathLex;1099">
        <rdfs:subClassOf rdf:resource="&pathLex;99999"/>
        <skos:definition xml:lang="en">Kidney-Infiltrating malignant neoplasm-pT-pT2: Tumor more than 7 cm in greatest dimension, limited to the kidney</skos:definition>
        <skos:prefLabel xml:lang="en">pT2: Tumor more than 7 cm in greatest dimension, limited to the kidney</skos:prefLabel>
    </owl:Class>
    


    <!-- http://www.semanticweb.org/david/ontologies/2013/0/1.3.6.1.4.1.19376.1.8.2.1.11 -->

    <owl:Class rdf:about="&pathLex;11">
        <rdfs:subClassOf rdf:resource="&pathLex;99999"/>
        <skos:definition xml:lang="en">Generic-Infiltrating malignant neoplasm-Lesion size, additional dimension</skos:definition>
        <skos:prefLabel xml:lang="en">Lesion size, additional dimension</skos:prefLabel>
    </owl:Class>
    


    <!-- http://www.semanticweb.org/david/ontologies/2013/0/1.3.6.1.4.1.19376.1.8.2.1.1100 -->

    <owl:Class rdf:about="&pathLex;1100">
        <rdfs:subClassOf rdf:resource="&pathLex;99999"/>
        <skos:definition xml:lang="en">Kidney-Infiltrating malignant neoplasm-pT-pT2a: Tumor more than 7 cm but less than or equal to 10 cm in greatest dimension, limited to the kidney</skos:definition>
        <skos:prefLabel xml:lang="en">pT2a: Tumor more than 7 cm but less than or equal to 10 cm in greatest dimension, limited to the kidney</skos:prefLabel>
    </owl:Class>
    


    <!-- http://www.semanticweb.org/david/ontologies/2013/0/1.3.6.1.4.1.19376.1.8.2.1.1101 -->

    <owl:Class rdf:about="&pathLex;1101">
        <rdfs:subClassOf rdf:resource="&pathLex;99999"/>
        <skos:definition xml:lang="en">Kidney-Infiltrating malignant neoplasm-pT-pT2b: Tumor more than 10 cm, limited to the kidney</skos:definition>
        <skos:prefLabel xml:lang="en">pT2b: Tumor more than 10 cm, limited to the kidney</skos:prefLabel>
    </owl:Class>
    


    <!-- http://www.semanticweb.org/david/ontologies/2013/0/1.3.6.1.4.1.19376.1.8.2.1.1102 -->

    <owl:Class rdf:about="&pathLex;1102">
        <rdfs:subClassOf rdf:resource="&pathLex;99999"/>
        <skos:definition xml:lang="en">Kidney-Infiltrating malignant neoplasm-pT-pT3: Tumor extends into major veins or perinephric tissues but not into the ipsilateral adrenal gland and not beyond Gerota’s fascia</skos:definition>
        <skos:prefLabel xml:lang="en">pT3: Tumor extends into major veins or perinephric tissues but not into the ipsilateral adrenal gland and not beyond Gerota’s fascia</skos:prefLabel>
    </owl:Class>
    


    <!-- http://www.semanticweb.org/david/ontologies/2013/0/1.3.6.1.4.1.19376.1.8.2.1.1103 -->

    <owl:Class rdf:about="&pathLex;1103">
        <rdfs:subClassOf rdf:resource="&pathLex;99999"/>
        <skos:definition xml:lang="en">Kidney-Infiltrating malignant neoplasm-pT-pT3a: Tumor grossly extends into the renal vein or its segmental (muscle containing) branches, or tumor invades perirenal and/or renal sinus fat but not beyond Gerota’s fascia</skos:definition>
        <skos:prefLabel xml:lang="en">pT3a: Tumor grossly extends into the renal vein or its segmental (muscle containing) branches, or tumor invades perirenal and/or renal sinus fat but not beyond Gerota’s fascia</skos:prefLabel>
    </owl:Class>
    


    <!-- http://www.semanticweb.org/david/ontologies/2013/0/1.3.6.1.4.1.19376.1.8.2.1.1104 -->

    <owl:Class rdf:about="&pathLex;1104">
        <rdfs:subClassOf rdf:resource="&pathLex;99999"/>
        <skos:definition xml:lang="en">Kidney-Infiltrating malignant neoplasm-pT-pT3b: Tumor grossly extends into the vena cava below the diaphragm</skos:definition>
        <skos:prefLabel xml:lang="en">pT3b: Tumor grossly extends into the vena cava below the diaphragm</skos:prefLabel>
    </owl:Class>
    


    <!-- http://www.semanticweb.org/david/ontologies/2013/0/1.3.6.1.4.1.19376.1.8.2.1.1105 -->

    <owl:Class rdf:about="&pathLex;1105">
        <rdfs:subClassOf rdf:resource="&pathLex;99999"/>
        <skos:definition xml:lang="en">Kidney-Infiltrating malignant neoplasm-pT-pT3c: Tumor grossly extends into vena cava above diaphragm or invades the wall of the vena cava</skos:definition>
        <skos:prefLabel xml:lang="en">pT3c: Tumor grossly extends into vena cava above diaphragm or invades the wall of the vena cava</skos:prefLabel>
    </owl:Class>
    


    <!-- http://www.semanticweb.org/david/ontologies/2013/0/1.3.6.1.4.1.19376.1.8.2.1.1106 -->

    <owl:Class rdf:about="&pathLex;1106">
        <rdfs:subClassOf rdf:resource="&pathLex;99999"/>
        <skos:definition xml:lang="en">Kidney-Infiltrating malignant neoplasm-pT-pT4: Tumor invades beyond Gerota’s fascia (including contiguous extension into the ipsilateral adrenal gland)</skos:definition>
        <skos:prefLabel xml:lang="en">pT4: Tumor invades beyond Gerota’s fascia (including contiguous extension into the ipsilateral adrenal gland)</skos:prefLabel>
    </owl:Class>
    


    <!-- http://www.semanticweb.org/david/ontologies/2013/0/1.3.6.1.4.1.19376.1.8.2.1.1107 -->

    <owl:Class rdf:about="&pathLex;1107">
        <rdfs:subClassOf rdf:resource="&pathLex;99999"/>
        <skos:definition xml:lang="en">Kidney-Infiltrating malignant neoplasm-pN-pN0: No regional lymph node metastasis</skos:definition>
        <skos:prefLabel xml:lang="en">pN0: No regional lymph node metastasis</skos:prefLabel>
    </owl:Class>
    


    <!-- http://www.semanticweb.org/david/ontologies/2013/0/1.3.6.1.4.1.19376.1.8.2.1.1108 -->

    <owl:Class rdf:about="&pathLex;1108">
        <rdfs:subClassOf rdf:resource="&pathLex;99999"/>
        <skos:definition xml:lang="en">Kidney-Infiltrating malignant neoplasm-pN-pN1: Metastasis in regional lymph node(s)</skos:definition>
        <skos:prefLabel xml:lang="en">pN1: Metastasis in regional lymph node(s)</skos:prefLabel>
    </owl:Class>
    


    <!-- http://www.semanticweb.org/david/ontologies/2013/0/1.3.6.1.4.1.19376.1.8.2.1.1117 -->

    <owl:Class rdf:about="&pathLex;1117">
        <rdfs:subClassOf rdf:resource="&pathLex;99999"/>
        <skos:definition xml:lang="en">Urinary bladder-Infiltrating malignant neoplasm-Histologic type-Urothelial (transitional cell) carcinoma</skos:definition>
        <skos:prefLabel xml:lang="en">Urothelial (transitional cell) carcinoma</skos:prefLabel>
    </owl:Class>
    


    <!-- http://www.semanticweb.org/david/ontologies/2013/0/1.3.6.1.4.1.19376.1.8.2.1.1118 -->

    <owl:Class rdf:about="&pathLex;1118">
        <rdfs:subClassOf rdf:resource="&pathLex;99999"/>
        <skos:prefLabel xml:lang="en">Small cell carcinoma</skos:prefLabel>
        <skos:definition xml:lang="en">Urinary bladder-Infiltrating malignant neoplasm-Histologic type-Small cell carcinoma</skos:definition>
    </owl:Class>
    


    <!-- http://www.semanticweb.org/david/ontologies/2013/0/1.3.6.1.4.1.19376.1.8.2.1.1133 -->

    <owl:Class rdf:about="&pathLex;1133">
        <rdfs:subClassOf rdf:resource="&pathLex;99999"/>
        <skos:definition xml:lang="en">Urinary bladder-Infiltrating malignant neoplasm-pT-pT0: No evidence of primary tumor</skos:definition>
        <skos:prefLabel xml:lang="en">pT0: No evidence of primary tumor</skos:prefLabel>
    </owl:Class>
    


    <!-- http://www.semanticweb.org/david/ontologies/2013/0/1.3.6.1.4.1.19376.1.8.2.1.1134 -->

    <owl:Class rdf:about="&pathLex;1134">
        <rdfs:subClassOf rdf:resource="&pathLex;99999"/>
        <skos:definition xml:lang="en">Urinary bladder-Infiltrating malignant neoplasm-pT-pTa: Noninvasive papillary carcinoma</skos:definition>
        <skos:prefLabel xml:lang="en">pTa: Noninvasive papillary carcinoma</skos:prefLabel>
    </owl:Class>
    


    <!-- http://www.semanticweb.org/david/ontologies/2013/0/1.3.6.1.4.1.19376.1.8.2.1.1135 -->

    <owl:Class rdf:about="&pathLex;1135">
        <rdfs:subClassOf rdf:resource="&pathLex;99999"/>
        <skos:definition xml:lang="en">Urinary bladder-Infiltrating malignant neoplasm-pT-pTis: Carcinoma in situ: “flat tumor”</skos:definition>
        <skos:prefLabel xml:lang="en">pTis: Carcinoma in situ: “flat tumor”</skos:prefLabel>
    </owl:Class>
    


    <!-- http://www.semanticweb.org/david/ontologies/2013/0/1.3.6.1.4.1.19376.1.8.2.1.1136 -->

    <owl:Class rdf:about="&pathLex;1136">
        <rdfs:subClassOf rdf:resource="&pathLex;99999"/>
        <skos:definition xml:lang="en">Urinary bladder-Infiltrating malignant neoplasm-pT-pT1: Tumor invades subepithelial connective tissue (lamina propria)</skos:definition>
        <skos:prefLabel xml:lang="en">pT1: Tumor invades subepithelial connective tissue (lamina propria)</skos:prefLabel>
    </owl:Class>
    


    <!-- http://www.semanticweb.org/david/ontologies/2013/0/1.3.6.1.4.1.19376.1.8.2.1.1137 -->

    <owl:Class rdf:about="&pathLex;1137">
        <rdfs:subClassOf rdf:resource="&pathLex;99999"/>
        <skos:definition xml:lang="en">Urinary bladder-Infiltrating malignant neoplasm-pT-pT2: Tumor invades muscularis propria (detrusor muscle)</skos:definition>
        <skos:prefLabel xml:lang="en">pT2: Tumor invades muscularis propria (detrusor muscle)</skos:prefLabel>
    </owl:Class>
    


    <!-- http://www.semanticweb.org/david/ontologies/2013/0/1.3.6.1.4.1.19376.1.8.2.1.1138 -->

    <owl:Class rdf:about="&pathLex;1138">
        <rdfs:subClassOf rdf:resource="&pathLex;99999"/>
        <skos:definition xml:lang="en">Urinary bladder-Infiltrating malignant neoplasm-pT-pT2a: Tumor invades superficial muscularis propria (inner half)</skos:definition>
        <skos:prefLabel xml:lang="en">pT2a: Tumor invades superficial muscularis propria (inner half)</skos:prefLabel>
    </owl:Class>
    


    <!-- http://www.semanticweb.org/david/ontologies/2013/0/1.3.6.1.4.1.19376.1.8.2.1.1139 -->

    <owl:Class rdf:about="&pathLex;1139">
        <rdfs:subClassOf rdf:resource="&pathLex;99999"/>
        <skos:definition xml:lang="en">Urinary bladder-Infiltrating malignant neoplasm-pT-pT2b: Tumor invades deep muscularis propria (outer half)</skos:definition>
        <skos:prefLabel xml:lang="en">pT2b: Tumor invades deep muscularis propria (outer half)</skos:prefLabel>
    </owl:Class>
    


    <!-- http://www.semanticweb.org/david/ontologies/2013/0/1.3.6.1.4.1.19376.1.8.2.1.1140 -->

    <owl:Class rdf:about="&pathLex;1140">
        <rdfs:subClassOf rdf:resource="&pathLex;99999"/>
        <skos:definition xml:lang="en">Urinary bladder-Infiltrating malignant neoplasm-pT-pT3: Tumor invades perivesical tissue</skos:definition>
        <skos:prefLabel xml:lang="en">pT3: Tumor invades perivesical tissue</skos:prefLabel>
    </owl:Class>
    


    <!-- http://www.semanticweb.org/david/ontologies/2013/0/1.3.6.1.4.1.19376.1.8.2.1.1141 -->

    <owl:Class rdf:about="&pathLex;1141">
        <rdfs:subClassOf rdf:resource="&pathLex;99999"/>
        <skos:definition xml:lang="en">Urinary bladder-Infiltrating malignant neoplasm-pT-pT3a: Microscopically</skos:definition>
        <skos:prefLabel xml:lang="en">pT3a: Microscopically</skos:prefLabel>
    </owl:Class>
    


    <!-- http://www.semanticweb.org/david/ontologies/2013/0/1.3.6.1.4.1.19376.1.8.2.1.1142 -->

    <owl:Class rdf:about="&pathLex;1142">
        <rdfs:subClassOf rdf:resource="&pathLex;99999"/>
        <skos:definition xml:lang="en">Urinary bladder-Infiltrating malignant neoplasm-pT-pT3b: Macroscopically (extravesicular mass)</skos:definition>
        <skos:prefLabel xml:lang="en">pT3b: Macroscopically (extravesicular mass)</skos:prefLabel>
    </owl:Class>
    


    <!-- http://www.semanticweb.org/david/ontologies/2013/0/1.3.6.1.4.1.19376.1.8.2.1.1143 -->

    <owl:Class rdf:about="&pathLex;1143">
        <rdfs:subClassOf rdf:resource="&pathLex;99999"/>
        <skos:definition xml:lang="en">Urinary bladder-Infiltrating malignant neoplasm-pT-pT4: Tumor invades any of the following: prostatic stroma, seminal vesicles, uterus,vagina, pelvic wall, abdominal wall</skos:definition>
        <skos:prefLabel xml:lang="en">pT4: Tumor invades any of the following: prostatic stroma, seminal vesicles, uterus,vagina, pelvic wall, abdominal wall</skos:prefLabel>
    </owl:Class>
    


    <!-- http://www.semanticweb.org/david/ontologies/2013/0/1.3.6.1.4.1.19376.1.8.2.1.1144 -->

    <owl:Class rdf:about="&pathLex;1144">
        <rdfs:subClassOf rdf:resource="&pathLex;99999"/>
        <skos:definition xml:lang="en">Urinary bladder-Infiltrating malignant neoplasm-pT-pT4a: Tumor invades prostatic stroma or uterus or vagina</skos:definition>
        <skos:prefLabel xml:lang="en">pT4a: Tumor invades prostatic stroma or uterus or vagina</skos:prefLabel>
    </owl:Class>
    


    <!-- http://www.semanticweb.org/david/ontologies/2013/0/1.3.6.1.4.1.19376.1.8.2.1.1145 -->

    <owl:Class rdf:about="&pathLex;1145">
        <rdfs:subClassOf rdf:resource="&pathLex;99999"/>
        <skos:definition xml:lang="en">Urinary bladder-Infiltrating malignant neoplasm-pT-pT4b: Tumor invades pelvic wall or abdominal wall</skos:definition>
        <skos:prefLabel xml:lang="en">pT4b: Tumor invades pelvic wall or abdominal wall</skos:prefLabel>
    </owl:Class>
    


    <!-- http://www.semanticweb.org/david/ontologies/2013/0/1.3.6.1.4.1.19376.1.8.2.1.1147 -->

    <owl:Class rdf:about="&pathLex;1147">
        <rdfs:subClassOf rdf:resource="&pathLex;99999"/>
        <skos:definition xml:lang="en">Urinary bladder-Infiltrating malignant neoplasm-pN-pN1: Single regional lymph node metastasis in the true pelvis (hypogastric, obturator, external iliac or presacral lymph node)</skos:definition>
        <skos:prefLabel xml:lang="en">pN1: Single regional lymph node metastasis in the true pelvis (hypogastric, obturator, external iliac or presacral lymph node)</skos:prefLabel>
    </owl:Class>
    


    <!-- http://www.semanticweb.org/david/ontologies/2013/0/1.3.6.1.4.1.19376.1.8.2.1.1148 -->

    <owl:Class rdf:about="&pathLex;1148">
        <rdfs:subClassOf rdf:resource="&pathLex;99999"/>
        <skos:definition xml:lang="en">Urinary bladder-Infiltrating malignant neoplasm-pN-pN2: Multiple regional lymph node metastasis in the true pelvis (hypogastric, obrutrator, external iliac or presacral lymph node metastasis)</skos:definition>
        <skos:prefLabel xml:lang="en">pN2: Multiple regional lymph node metastasis in the true pelvis (hypogastric, obrutrator, external iliac or presacral lymph node metastasis)</skos:prefLabel>
    </owl:Class>
    


    <!-- http://www.semanticweb.org/david/ontologies/2013/0/1.3.6.1.4.1.19376.1.8.2.1.1149 -->

    <owl:Class rdf:about="&pathLex;1149">
        <rdfs:subClassOf rdf:resource="&pathLex;99999"/>
        <skos:definition xml:lang="en">Urinary bladder-Infiltrating malignant neoplasm-pN-pN3: Lymph node metastasis to the common iliac lymph nodes</skos:definition>
        <skos:prefLabel xml:lang="en">pN3: Lymph node metastasis to the common iliac lymph nodes</skos:prefLabel>
    </owl:Class>
    


    <!-- http://www.semanticweb.org/david/ontologies/2013/0/1.3.6.1.4.1.19376.1.8.2.1.1150 -->

    <owl:Class rdf:about="&pathLex;1150">
        <rdfs:subClassOf rdf:resource="&pathLex;99999"/>
        <skos:prefLabel xml:lang="en">Body</skos:prefLabel>
        <skos:definition xml:lang="en">Skin (melanoma)-Infiltrating malignant neoplasm-Lesion site-Body</skos:definition>
    </owl:Class>
    


    <!-- http://www.semanticweb.org/david/ontologies/2013/0/1.3.6.1.4.1.19376.1.8.2.1.1152 -->

    <owl:Class rdf:about="&pathLex;1152">
        <rdfs:subClassOf rdf:resource="&pathLex;99999"/>
        <skos:prefLabel xml:lang="en">Excision</skos:prefLabel>
        <skos:definition xml:lang="en">Skin (melanoma)-Specimen-Specimen collection procedure-Excision</skos:definition>
    </owl:Class>
    


    <!-- http://www.semanticweb.org/david/ontologies/2013/0/1.3.6.1.4.1.19376.1.8.2.1.1156 -->

    <owl:Class rdf:about="&pathLex;1156">
        <rdfs:subClassOf rdf:resource="&pathLex;99999"/>
        <skos:definition xml:lang="en">Skin (melanoma)-Infiltrating malignant neoplasm-Histologic type-Superficial spreading melanoma</skos:definition>
        <skos:prefLabel xml:lang="en">Superficial spreading melanoma</skos:prefLabel>
    </owl:Class>
    


    <!-- http://www.semanticweb.org/david/ontologies/2013/0/1.3.6.1.4.1.19376.1.8.2.1.1157 -->

    <owl:Class rdf:about="&pathLex;1157">
        <rdfs:subClassOf rdf:resource="&pathLex;99999"/>
        <skos:prefLabel xml:lang="en">Nodular melanoma</skos:prefLabel>
        <skos:definition xml:lang="en">Skin (melanoma)-Infiltrating malignant neoplasm-Histologic type-Nodular melanoma</skos:definition>
    </owl:Class>
    


    <!-- http://www.semanticweb.org/david/ontologies/2013/0/1.3.6.1.4.1.19376.1.8.2.1.1160 -->

    <owl:Class rdf:about="&pathLex;1160">
        <rdfs:subClassOf rdf:resource="&pathLex;99999"/>
        <skos:prefLabel xml:lang="en">I (Melanoma in situ)</skos:prefLabel>
        <skos:definition xml:lang="en">Skin (melanoma)-Infiltrating malignant neoplasm-Histologic grade (Clark)-I (Melanoma in situ)</skos:definition>
    </owl:Class>
    


    <!-- http://www.semanticweb.org/david/ontologies/2013/0/1.3.6.1.4.1.19376.1.8.2.1.1161 -->

    <owl:Class rdf:about="&pathLex;1161">
        <rdfs:subClassOf rdf:resource="&pathLex;99999"/>
        <skos:prefLabel xml:lang="en">II (Melanoma present in but does not fill and expand papillary dermis)</skos:prefLabel>
        <skos:definition xml:lang="en">Skin (melanoma)-Infiltrating malignant neoplasm-Histologic grade (Clark)-II (Melanoma present in but does not fill and expand papillary dermis)</skos:definition>
    </owl:Class>
    


    <!-- http://www.semanticweb.org/david/ontologies/2013/0/1.3.6.1.4.1.19376.1.8.2.1.1162 -->

    <owl:Class rdf:about="&pathLex;1162">
        <rdfs:subClassOf rdf:resource="&pathLex;99999"/>
        <skos:prefLabel xml:lang="en">III (Melanoma fills and expands papillary dermis)</skos:prefLabel>
        <skos:definition xml:lang="en">Skin (melanoma)-Infiltrating malignant neoplasm-Histologic grade (Clark)-III (Melanoma fills and expands papillary dermis)</skos:definition>
    </owl:Class>
    


    <!-- http://www.semanticweb.org/david/ontologies/2013/0/1.3.6.1.4.1.19376.1.8.2.1.1163 -->

    <owl:Class rdf:about="&pathLex;1163">
        <rdfs:subClassOf rdf:resource="&pathLex;99999"/>
        <skos:prefLabel xml:lang="en">IV (Melanoma invades reticular dermis)</skos:prefLabel>
        <skos:definition xml:lang="en">Skin (melanoma)-Infiltrating malignant neoplasm-Histologic grade (Clark)-IV (Melanoma invades reticular dermis)</skos:definition>
    </owl:Class>
    


    <!-- http://www.semanticweb.org/david/ontologies/2013/0/1.3.6.1.4.1.19376.1.8.2.1.1164 -->

    <owl:Class rdf:about="&pathLex;1164">
        <rdfs:subClassOf rdf:resource="&pathLex;99999"/>
        <skos:definition xml:lang="en">Skin (melanoma)-Infiltrating malignant neoplasm-Histologic grade (Clark)-V (Melanoma invades subcutaneum)</skos:definition>
        <skos:prefLabel xml:lang="en">V (Melanoma invades subcutaneum)</skos:prefLabel>
    </owl:Class>
    


    <!-- http://www.semanticweb.org/david/ontologies/2013/0/1.3.6.1.4.1.19376.1.8.2.1.1165 -->

    <owl:Class rdf:about="&pathLex;1165">
        <rdfs:subClassOf rdf:resource="&pathLex;99999"/>
        <skos:prefLabel xml:lang="en">Deep margin</skos:prefLabel>
        <skos:definition xml:lang="en">Skin (melanoma)-Infiltrating malignant neoplasm-Margin site-Deep margin</skos:definition>
    </owl:Class>
    


    <!-- http://www.semanticweb.org/david/ontologies/2013/0/1.3.6.1.4.1.19376.1.8.2.1.1166 -->

    <owl:Class rdf:about="&pathLex;1166">
        <rdfs:subClassOf rdf:resource="&pathLex;99999"/>
        <skos:prefLabel xml:lang="en">Peripheral margins</skos:prefLabel>
        <skos:definition xml:lang="en">Skin (melanoma)-Infiltrating malignant neoplasm-Margin site-Peripheral margins</skos:definition>
    </owl:Class>
    


    <!-- http://www.semanticweb.org/david/ontologies/2013/0/1.3.6.1.4.1.19376.1.8.2.1.1167 -->

    <owl:Class rdf:about="&pathLex;1167">
        <rdfs:subClassOf rdf:resource="&pathLex;99999"/>
        <skos:definition xml:lang="en">Skin (melanoma)-Infiltrating malignant neoplasm-pT-pT0: No evidence of primary tumor</skos:definition>
        <skos:prefLabel xml:lang="en">pT0: No evidence of primary tumor</skos:prefLabel>
    </owl:Class>
    


    <!-- http://www.semanticweb.org/david/ontologies/2013/0/1.3.6.1.4.1.19376.1.8.2.1.1168 -->

    <owl:Class rdf:about="&pathLex;1168">
        <rdfs:subClassOf rdf:resource="&pathLex;99999"/>
        <skos:definition xml:lang="en">Skin (melanoma)-Infiltrating malignant neoplasm-pT-pTis: Melanoma in situ (ie, not an invasive tumor: anatomic level I)</skos:definition>
        <skos:prefLabel xml:lang="en">pTis: Melanoma in situ (ie, not an invasive tumor: anatomic level I)</skos:prefLabel>
    </owl:Class>
    


    <!-- http://www.semanticweb.org/david/ontologies/2013/0/1.3.6.1.4.1.19376.1.8.2.1.1169 -->

    <owl:Class rdf:about="&pathLex;1169">
        <rdfs:subClassOf rdf:resource="&pathLex;99999"/>
        <skos:definition xml:lang="en">Skin (melanoma)-Infiltrating malignant neoplasm-pT-pT1: Melanoma 1.0 mm or less in thickness, with or without ulceration (see Note D)</skos:definition>
        <skos:prefLabel xml:lang="en">pT1: Melanoma 1.0 mm or less in thickness, with or without ulceration (see Note D)</skos:prefLabel>
    </owl:Class>
    


    <!-- http://www.semanticweb.org/david/ontologies/2013/0/1.3.6.1.4.1.19376.1.8.2.1.1170 -->

    <owl:Class rdf:about="&pathLex;1170">
        <rdfs:subClassOf rdf:resource="&pathLex;99999"/>
        <skos:definition xml:lang="en">Skin (melanoma)-Infiltrating malignant neoplasm-pT-pT1a: Melanoma 1.0 mm or less in thickness, no ulceration, &lt;1 mitoses/mm2</skos:definition>
        <skos:prefLabel xml:lang="en">pT1a: Melanoma 1.0 mm or less in thickness, no ulceration, &lt;1 mitoses/mm2</skos:prefLabel>
    </owl:Class>
    


    <!-- http://www.semanticweb.org/david/ontologies/2013/0/1.3.6.1.4.1.19376.1.8.2.1.1171 -->

    <owl:Class rdf:about="&pathLex;1171">
        <rdfs:subClassOf rdf:resource="&pathLex;99999"/>
        <skos:definition xml:lang="en">Skin (melanoma)-Infiltrating malignant neoplasm-pT-pT1b: Melanoma 1.0 mm or less in thickness with ulceration and/or 1 or more mitoses/mm2</skos:definition>
        <skos:prefLabel xml:lang="en">pT1b: Melanoma 1.0 mm or less in thickness with ulceration and/or 1 or more mitoses/mm2</skos:prefLabel>
    </owl:Class>
    


    <!-- http://www.semanticweb.org/david/ontologies/2013/0/1.3.6.1.4.1.19376.1.8.2.1.1172 -->

    <owl:Class rdf:about="&pathLex;1172">
        <rdfs:subClassOf rdf:resource="&pathLex;99999"/>
        <skos:definition xml:lang="en">Skin (melanoma)-Infiltrating malignant neoplasm-pT-pT2: Melanoma 1.01 to 2 mm in thickness, with or without ulceration</skos:definition>
        <skos:prefLabel xml:lang="en">pT2: Melanoma 1.01 to 2 mm in thickness, with or without ulceration</skos:prefLabel>
    </owl:Class>
    


    <!-- http://www.semanticweb.org/david/ontologies/2013/0/1.3.6.1.4.1.19376.1.8.2.1.1173 -->

    <owl:Class rdf:about="&pathLex;1173">
        <rdfs:subClassOf rdf:resource="&pathLex;99999"/>
        <skos:definition xml:lang="en">Skin (melanoma)-Infiltrating malignant neoplasm-pT-pT2a: Melanoma 1.01 to 2.0 mm in thickness, no ulceration</skos:definition>
        <skos:prefLabel xml:lang="en">pT2a: Melanoma 1.01 to 2.0 mm in thickness, no ulceration</skos:prefLabel>
    </owl:Class>
    


    <!-- http://www.semanticweb.org/david/ontologies/2013/0/1.3.6.1.4.1.19376.1.8.2.1.1174 -->

    <owl:Class rdf:about="&pathLex;1174">
        <rdfs:subClassOf rdf:resource="&pathLex;99999"/>
        <skos:definition xml:lang="en">Skin (melanoma)-Infiltrating malignant neoplasm-pT-pT2b: Melanoma 1.01 to 2.0 mm in thickness, with ulceration</skos:definition>
        <skos:prefLabel xml:lang="en">pT2b: Melanoma 1.01 to 2.0 mm in thickness, with ulceration</skos:prefLabel>
    </owl:Class>
    


    <!-- http://www.semanticweb.org/david/ontologies/2013/0/1.3.6.1.4.1.19376.1.8.2.1.1175 -->

    <owl:Class rdf:about="&pathLex;1175">
        <rdfs:subClassOf rdf:resource="&pathLex;99999"/>
        <skos:definition xml:lang="en">Skin (melanoma)-Infiltrating malignant neoplasm-pT-pT3: Melanoma 2.01 to 4.0 mm in thickness, with or without ulceration</skos:definition>
        <skos:prefLabel xml:lang="en">pT3: Melanoma 2.01 to 4.0 mm in thickness, with or without ulceration</skos:prefLabel>
    </owl:Class>
    


    <!-- http://www.semanticweb.org/david/ontologies/2013/0/1.3.6.1.4.1.19376.1.8.2.1.1176 -->

    <owl:Class rdf:about="&pathLex;1176">
        <rdfs:subClassOf rdf:resource="&pathLex;99999"/>
        <skos:definition xml:lang="en">Skin (melanoma)-Infiltrating malignant neoplasm-pT-pT3a: Melanoma 2.01 to 4.0 mm in thickness, no ulceration</skos:definition>
        <skos:prefLabel xml:lang="en">pT3a: Melanoma 2.01 to 4.0 mm in thickness, no ulceration</skos:prefLabel>
    </owl:Class>
    


    <!-- http://www.semanticweb.org/david/ontologies/2013/0/1.3.6.1.4.1.19376.1.8.2.1.1177 -->

    <owl:Class rdf:about="&pathLex;1177">
        <rdfs:subClassOf rdf:resource="&pathLex;99999"/>
        <skos:definition xml:lang="en">Skin (melanoma)-Infiltrating malignant neoplasm-pT-pT3b: Melanoma 2.01 to 4.0 mm in thickness, with ulceration</skos:definition>
        <skos:prefLabel xml:lang="en">pT3b: Melanoma 2.01 to 4.0 mm in thickness, with ulceration</skos:prefLabel>
    </owl:Class>
    


    <!-- http://www.semanticweb.org/david/ontologies/2013/0/1.3.6.1.4.1.19376.1.8.2.1.1178 -->

    <owl:Class rdf:about="&pathLex;1178">
        <rdfs:subClassOf rdf:resource="&pathLex;99999"/>
        <skos:definition xml:lang="en">Skin (melanoma)-Infiltrating malignant neoplasm-pT-pT4: Melanoma greater than 4.0 mm in thickness, with or without ulceration</skos:definition>
        <skos:prefLabel xml:lang="en">pT4: Melanoma greater than 4.0 mm in thickness, with or without ulceration</skos:prefLabel>
    </owl:Class>
    


    <!-- http://www.semanticweb.org/david/ontologies/2013/0/1.3.6.1.4.1.19376.1.8.2.1.1179 -->

    <owl:Class rdf:about="&pathLex;1179">
        <rdfs:subClassOf rdf:resource="&pathLex;99999"/>
        <skos:definition xml:lang="en">Skin (melanoma)-Infiltrating malignant neoplasm-pT-pT4a: Melanoma greater than 4.0 mm in thickness, no ulceration</skos:definition>
        <skos:prefLabel xml:lang="en">pT4a: Melanoma greater than 4.0 mm in thickness, no ulceration</skos:prefLabel>
    </owl:Class>
    


    <!-- http://www.semanticweb.org/david/ontologies/2013/0/1.3.6.1.4.1.19376.1.8.2.1.1180 -->

    <owl:Class rdf:about="&pathLex;1180">
        <rdfs:subClassOf rdf:resource="&pathLex;99999"/>
        <skos:definition xml:lang="en">Skin (melanoma)-Infiltrating malignant neoplasm-pT-pT4b: Melanoma greater than 4.0 mm in thickness, with ulceration</skos:definition>
        <skos:prefLabel xml:lang="en">pT4b: Melanoma greater than 4.0 mm in thickness, with ulceration</skos:prefLabel>
    </owl:Class>
    


    <!-- http://www.semanticweb.org/david/ontologies/2013/0/1.3.6.1.4.1.19376.1.8.2.1.1181 -->

    <owl:Class rdf:about="&pathLex;1181">
        <rdfs:subClassOf rdf:resource="&pathLex;99999"/>
        <skos:definition xml:lang="en">Skin (melanoma)-Infiltrating malignant neoplasm-pN-pN0: No regional lymph node metastasis</skos:definition>
        <skos:prefLabel xml:lang="en">pN0: No regional lymph node metastasis</skos:prefLabel>
    </owl:Class>
    


    <!-- http://www.semanticweb.org/david/ontologies/2013/0/1.3.6.1.4.1.19376.1.8.2.1.1182 -->

    <owl:Class rdf:about="&pathLex;1182">
        <rdfs:subClassOf rdf:resource="&pathLex;99999"/>
        <skos:definition xml:lang="en">Skin (melanoma)-Infiltrating malignant neoplasm-pN-pN1: Metastasis in 1 regional lymph node</skos:definition>
        <skos:prefLabel xml:lang="en">pN1: Metastasis in 1 regional lymph node</skos:prefLabel>
    </owl:Class>
    


    <!-- http://www.semanticweb.org/david/ontologies/2013/0/1.3.6.1.4.1.19376.1.8.2.1.1183 -->

    <owl:Class rdf:about="&pathLex;1183">
        <rdfs:subClassOf rdf:resource="&pathLex;99999"/>
        <skos:definition xml:lang="en">Skin (melanoma)-Infiltrating malignant neoplasm-pN-pN1a: Clinically occult (microscopic) metastasis</skos:definition>
        <skos:prefLabel xml:lang="en">pN1a: Clinically occult (microscopic) metastasis</skos:prefLabel>
    </owl:Class>
    


    <!-- http://www.semanticweb.org/david/ontologies/2013/0/1.3.6.1.4.1.19376.1.8.2.1.1184 -->

    <owl:Class rdf:about="&pathLex;1184">
        <rdfs:subClassOf rdf:resource="&pathLex;99999"/>
        <skos:definition xml:lang="en">Skin (melanoma)-Infiltrating malignant neoplasm-pN-pN1b: Clinically apparent (macroscopic) metastasis</skos:definition>
        <skos:prefLabel xml:lang="en">pN1b: Clinically apparent (macroscopic) metastasis</skos:prefLabel>
    </owl:Class>
    


    <!-- http://www.semanticweb.org/david/ontologies/2013/0/1.3.6.1.4.1.19376.1.8.2.1.1185 -->

    <owl:Class rdf:about="&pathLex;1185">
        <rdfs:subClassOf rdf:resource="&pathLex;99999"/>
        <skos:definition xml:lang="en">Skin (melanoma)-Infiltrating malignant neoplasm-pN-pN2: Metastasis in 2 to 3 regional nodes or intralymphatic regional metastasis without nodal metastasis</skos:definition>
        <skos:prefLabel xml:lang="en">pN2: Metastasis in 2 to 3 regional nodes or intralymphatic regional metastasis without nodal metastasis</skos:prefLabel>
    </owl:Class>
    


    <!-- http://www.semanticweb.org/david/ontologies/2013/0/1.3.6.1.4.1.19376.1.8.2.1.1186 -->

    <owl:Class rdf:about="&pathLex;1186">
        <rdfs:subClassOf rdf:resource="&pathLex;99999"/>
        <skos:definition xml:lang="en">Skin (melanoma)-Infiltrating malignant neoplasm-pN-pN2a: Clinically occult (microscopic) metastasis</skos:definition>
        <skos:prefLabel xml:lang="en">pN2a: Clinically occult (microscopic) metastasis</skos:prefLabel>
    </owl:Class>
    


    <!-- http://www.semanticweb.org/david/ontologies/2013/0/1.3.6.1.4.1.19376.1.8.2.1.1187 -->

    <owl:Class rdf:about="&pathLex;1187">
        <rdfs:subClassOf rdf:resource="&pathLex;99999"/>
        <skos:definition xml:lang="en">Skin (melanoma)-Infiltrating malignant neoplasm-pN-pN2b: Clinically apparent (macroscopic) metastasis</skos:definition>
        <skos:prefLabel xml:lang="en">pN2b: Clinically apparent (macroscopic) metastasis</skos:prefLabel>
    </owl:Class>
    


    <!-- http://www.semanticweb.org/david/ontologies/2013/0/1.3.6.1.4.1.19376.1.8.2.1.1188 -->

    <owl:Class rdf:about="&pathLex;1188">
        <rdfs:subClassOf rdf:resource="&pathLex;99999"/>
        <skos:definition xml:lang="en">Skin (melanoma)-Infiltrating malignant neoplasm-pN-pN2c: Satellite or in-transit metastasis without nodal metastasis</skos:definition>
        <skos:prefLabel xml:lang="en">pN2c: Satellite or in-transit metastasis without nodal metastasis</skos:prefLabel>
    </owl:Class>
    


    <!-- http://www.semanticweb.org/david/ontologies/2013/0/1.3.6.1.4.1.19376.1.8.2.1.1189 -->

    <owl:Class rdf:about="&pathLex;1189">
        <rdfs:subClassOf rdf:resource="&pathLex;99999"/>
        <skos:definition xml:lang="en">Skin (melanoma)-Infiltrating malignant neoplasm-pN-pN3: Metastasis in 4 or more regional lymph nodes, or matted metastatic nodes, or in-transit metastasis or satellites(s) with metastasis in regional node(s)</skos:definition>
        <skos:prefLabel xml:lang="en">pN3: Metastasis in 4 or more regional lymph nodes, or matted metastatic nodes, or in-transit metastasis or satellites(s) with metastasis in regional node(s)</skos:prefLabel>
    </owl:Class>
    


    <!-- http://www.semanticweb.org/david/ontologies/2013/0/1.3.6.1.4.1.19376.1.8.2.1.1190 -->

    <owl:Class rdf:about="&pathLex;1190">
        <rdfs:subClassOf rdf:resource="&pathLex;99999"/>
        <skos:prefLabel xml:lang="en">Thyroid</skos:prefLabel>
        <skos:definition xml:lang="en">Thyroid-Infiltrating malignant neoplasm-Lesion site-Thyroid</skos:definition>
    </owl:Class>
    


    <!-- http://www.semanticweb.org/david/ontologies/2013/0/1.3.6.1.4.1.19376.1.8.2.1.1191 -->

    <owl:Class rdf:about="&pathLex;1191">
        <rdfs:subClassOf rdf:resource="&pathLex;99999"/>
        <skos:prefLabel xml:lang="en">Thyroid lobectomy</skos:prefLabel>
        <skos:definition xml:lang="en">Thyroid-Specimen-Specimen collection procedure-Thyroid lobectomy</skos:definition>
    </owl:Class>
    


    <!-- http://www.semanticweb.org/david/ontologies/2013/0/1.3.6.1.4.1.19376.1.8.2.1.1192 -->

    <owl:Class rdf:about="&pathLex;1192">
        <rdfs:subClassOf rdf:resource="&pathLex;99999"/>
        <skos:prefLabel xml:lang="en">Partial thyroidectomy (anything less than a lobectomy)</skos:prefLabel>
        <skos:definition xml:lang="en">Thyroid-Specimen-Specimen collection procedure-Partial thyroidectomy (anything less than a lobectomy)</skos:definition>
    </owl:Class>
    


    <!-- http://www.semanticweb.org/david/ontologies/2013/0/1.3.6.1.4.1.19376.1.8.2.1.1193 -->

    <owl:Class rdf:about="&pathLex;1193">
        <rdfs:subClassOf rdf:resource="&pathLex;99999"/>
        <skos:prefLabel xml:lang="en">Hemithyroidectomy (lobe and part or all of isthmus)</skos:prefLabel>
        <skos:definition xml:lang="en">Thyroid-Specimen-Specimen collection procedure-Hemithyroidectomy (lobe and part or all of isthmus)</skos:definition>
    </owl:Class>
    


    <!-- http://www.semanticweb.org/david/ontologies/2013/0/1.3.6.1.4.1.19376.1.8.2.1.1194 -->

    <owl:Class rdf:about="&pathLex;1194">
        <rdfs:subClassOf rdf:resource="&pathLex;99999"/>
        <skos:definition xml:lang="en">Thyroid-Specimen-Specimen collection procedure-Total thyroidectomy</skos:definition>
        <skos:prefLabel xml:lang="en">Total thyroidectomy</skos:prefLabel>
    </owl:Class>
    


    <!-- http://www.semanticweb.org/david/ontologies/2013/0/1.3.6.1.4.1.19376.1.8.2.1.120 -->

    <owl:Class rdf:about="&pathLex;120">
        <rdfs:subClassOf rdf:resource="&pathLex;54"/>
        <skos:definition xml:lang="en">Cervix-Infiltrating malignant neoplasm-Margins involvement</skos:definition>
        <skos:prefLabel xml:lang="en">Cervix-Margins involvement</skos:prefLabel>
        <skos:altLabel xml:lang="en">Margins involvement</skos:altLabel>
    </owl:Class>
    


    <!-- http://www.semanticweb.org/david/ontologies/2013/0/1.3.6.1.4.1.19376.1.8.2.1.1200 -->

    <owl:Class rdf:about="&pathLex;1200">
        <rdfs:subClassOf rdf:resource="&pathLex;99999"/>
        <skos:prefLabel xml:lang="en">Papillary carcinoma</skos:prefLabel>
        <skos:definition xml:lang="en">Thyroid-Infiltrating malignant neoplasm-Histologic type-Papillary carcinoma</skos:definition>
    </owl:Class>
    


    <!-- http://www.semanticweb.org/david/ontologies/2013/0/1.3.6.1.4.1.19376.1.8.2.1.1201 -->

    <owl:Class rdf:about="&pathLex;1201">
        <rdfs:subClassOf rdf:resource="&pathLex;99999"/>
        <skos:prefLabel xml:lang="en">Follicular carcinoma</skos:prefLabel>
        <skos:definition xml:lang="en">Thyroid-Infiltrating malignant neoplasm-Histologic type-Follicular carcinoma</skos:definition>
    </owl:Class>
    


    <!-- http://www.semanticweb.org/david/ontologies/2013/0/1.3.6.1.4.1.19376.1.8.2.1.1202 -->

    <owl:Class rdf:about="&pathLex;1202">
        <rdfs:subClassOf rdf:resource="&pathLex;99999"/>
        <skos:prefLabel xml:lang="en">Poorly differentiated thyroid Carcinoma, including insular carcinoma</skos:prefLabel>
        <skos:definition xml:lang="en">Thyroid-Infiltrating malignant neoplasm-Histologic type-Poorly differentiated thyroid Carcinoma, including insular carcinoma</skos:definition>
    </owl:Class>
    


    <!-- http://www.semanticweb.org/david/ontologies/2013/0/1.3.6.1.4.1.19376.1.8.2.1.1203 -->

    <owl:Class rdf:about="&pathLex;1203">
        <rdfs:subClassOf rdf:resource="&pathLex;99999"/>
        <skos:prefLabel xml:lang="en">Medullary carcinoma</skos:prefLabel>
        <skos:definition xml:lang="en">Thyroid-Infiltrating malignant neoplasm-Histologic type-Medullary carcinoma</skos:definition>
    </owl:Class>
    


    <!-- http://www.semanticweb.org/david/ontologies/2013/0/1.3.6.1.4.1.19376.1.8.2.1.1204 -->

    <owl:Class rdf:about="&pathLex;1204">
        <rdfs:subClassOf rdf:resource="&pathLex;99999"/>
        <skos:definition xml:lang="en">Thyroid-Infiltrating malignant neoplasm-Histologic type-Undifferentiated (anaplastic) carcinoma</skos:definition>
        <skos:prefLabel xml:lang="en">Undifferentiated (anaplastic) carcinoma</skos:prefLabel>
    </owl:Class>
    


    <!-- http://www.semanticweb.org/david/ontologies/2013/0/1.3.6.1.4.1.19376.1.8.2.1.1209 -->

    <owl:Class rdf:about="&pathLex;1209">
        <rdfs:subClassOf rdf:resource="&pathLex;99999"/>
        <skos:definition xml:lang="en">Thyroid-Infiltrating malignant neoplasm-pT-pT0: No evidence of primary tumor</skos:definition>
        <skos:prefLabel xml:lang="en">pT0: No evidence of primary tumor</skos:prefLabel>
    </owl:Class>
    


    <!-- http://www.semanticweb.org/david/ontologies/2013/0/1.3.6.1.4.1.19376.1.8.2.1.121 -->

    <owl:Class rdf:about="&pathLex;121">
        <rdfs:subClassOf rdf:resource="&pathLex;69"/>
        <skos:definition xml:lang="en">Cervix-In situ neoplasm-Margins involvement</skos:definition>
        <skos:prefLabel xml:lang="en">Cervix-Margins involvement</skos:prefLabel>
        <skos:altLabel xml:lang="en">Margins involvement</skos:altLabel>
    </owl:Class>
    


    <!-- http://www.semanticweb.org/david/ontologies/2013/0/1.3.6.1.4.1.19376.1.8.2.1.1210 -->

    <owl:Class rdf:about="&pathLex;1210">
        <rdfs:subClassOf rdf:resource="&pathLex;99999"/>
        <skos:definition xml:lang="en">Thyroid-Infiltrating malignant neoplasm-pT-pT1: Tumor size 2 cm or less, limited to thyroid</skos:definition>
        <skos:prefLabel xml:lang="en">pT1: Tumor size 2 cm or less, limited to thyroid</skos:prefLabel>
    </owl:Class>
    


    <!-- http://www.semanticweb.org/david/ontologies/2013/0/1.3.6.1.4.1.19376.1.8.2.1.1211 -->

    <owl:Class rdf:about="&pathLex;1211">
        <rdfs:subClassOf rdf:resource="&pathLex;99999"/>
        <skos:definition xml:lang="en">Thyroid-Infiltrating malignant neoplasm-pT-pT1a: Tumor 1 cm or less in greatest dimension limited to the thyroid.</skos:definition>
        <skos:prefLabel xml:lang="en">pT1a: Tumor 1 cm or less in greatest dimension limited to the thyroid.</skos:prefLabel>
    </owl:Class>
    


    <!-- http://www.semanticweb.org/david/ontologies/2013/0/1.3.6.1.4.1.19376.1.8.2.1.1212 -->

    <owl:Class rdf:about="&pathLex;1212">
        <rdfs:subClassOf rdf:resource="&pathLex;99999"/>
        <skos:definition xml:lang="en">Thyroid-Infiltrating malignant neoplasm-pT-pT1b: Tumor more than 1 cm but not more than 2 cm in greatest dimension, limited to the thyroid</skos:definition>
        <skos:prefLabel xml:lang="en">pT1b: Tumor more than 1 cm but not more than 2 cm in greatest dimension, limited to the thyroid</skos:prefLabel>
    </owl:Class>
    


    <!-- http://www.semanticweb.org/david/ontologies/2013/0/1.3.6.1.4.1.19376.1.8.2.1.1213 -->

    <owl:Class rdf:about="&pathLex;1213">
        <rdfs:subClassOf rdf:resource="&pathLex;99999"/>
        <skos:definition xml:lang="en">Thyroid-Infiltrating malignant neoplasm-pT-pT2: Tumor more than 2 cm, but not more than 4 cm, limited to thyroid</skos:definition>
        <skos:prefLabel xml:lang="en">pT2: Tumor more than 2 cm, but not more than 4 cm, limited to thyroid</skos:prefLabel>
    </owl:Class>
    


    <!-- http://www.semanticweb.org/david/ontologies/2013/0/1.3.6.1.4.1.19376.1.8.2.1.1214 -->

    <owl:Class rdf:about="&pathLex;1214">
        <rdfs:subClassOf rdf:resource="&pathLex;99999"/>
        <skos:definition xml:lang="en">Thyroid-Infiltrating malignant neoplasm-pT-pT3: Tumor more than 4 cm limited to thyroid or any tumor with minimal extrathyroid extension (eg, extension to sternothyroid muscle or perithyroid soft tissues)</skos:definition>
        <skos:prefLabel xml:lang="en">pT3: Tumor more than 4 cm limited to thyroid or any tumor with minimal extrathyroid extension (eg, extension to sternothyroid muscle or perithyroid soft tissues)</skos:prefLabel>
    </owl:Class>
    


    <!-- http://www.semanticweb.org/david/ontologies/2013/0/1.3.6.1.4.1.19376.1.8.2.1.1215 -->

    <owl:Class rdf:about="&pathLex;1215">
        <rdfs:subClassOf rdf:resource="&pathLex;99999"/>
        <skos:definition xml:lang="en">Thyroid-Infiltrating malignant neoplasm-pT-pT4a: Moderately advanced disease. Tumor of any size extending beyond the thyroid capsule to invade subcutaneous soft tissues, larynx, trachea, esophagus or recurrent laryngeal nerve</skos:definition>
        <skos:prefLabel xml:lang="en">pT4a: Moderately advanced disease. Tumor of any size extending beyond the thyroid capsule to invade subcutaneous soft tissues, larynx, trachea, esophagus or recurrent laryngeal nerve</skos:prefLabel>
    </owl:Class>
    


    <!-- http://www.semanticweb.org/david/ontologies/2013/0/1.3.6.1.4.1.19376.1.8.2.1.1216 -->

    <owl:Class rdf:about="&pathLex;1216">
        <rdfs:subClassOf rdf:resource="&pathLex;99999"/>
        <skos:definition xml:lang="en">Thyroid-Infiltrating malignant neoplasm-pT-pT4b: Very advanced disease. Tumor invades prevertebral fascia or encases carotid artery or mediastinal vessels</skos:definition>
        <skos:prefLabel xml:lang="en">pT4b: Very advanced disease. Tumor invades prevertebral fascia or encases carotid artery or mediastinal vessels</skos:prefLabel>
    </owl:Class>
    


    <!-- http://www.semanticweb.org/david/ontologies/2013/0/1.3.6.1.4.1.19376.1.8.2.1.1217 -->

    <owl:Class rdf:about="&pathLex;1217">
        <rdfs:subClassOf rdf:resource="&pathLex;99999"/>
        <skos:definition xml:lang="en">Thyroid-Infiltrating malignant neoplasm-pT-pT0: No evidence of primary tumor</skos:definition>
        <skos:prefLabel xml:lang="en">pT0: No evidence of primary tumor</skos:prefLabel>
    </owl:Class>
    


    <!-- http://www.semanticweb.org/david/ontologies/2013/0/1.3.6.1.4.1.19376.1.8.2.1.1218 -->

    <owl:Class rdf:about="&pathLex;1218">
        <rdfs:subClassOf rdf:resource="&pathLex;99999"/>
        <skos:definition xml:lang="en">Thyroid-Infiltrating malignant neoplasm-pT-pT1: Tumor size 2 cm or less, limited to thyroid</skos:definition>
        <skos:prefLabel xml:lang="en">pT1: Tumor size 2 cm or less, limited to thyroid</skos:prefLabel>
    </owl:Class>
    


    <!-- http://www.semanticweb.org/david/ontologies/2013/0/1.3.6.1.4.1.19376.1.8.2.1.1219 -->

    <owl:Class rdf:about="&pathLex;1219">
        <rdfs:subClassOf rdf:resource="&pathLex;99999"/>
        <skos:definition xml:lang="en">Thyroid-Infiltrating malignant neoplasm-pT-pT1a: Tumor 1 cm or less in greatest dimension limited to the thyroid.</skos:definition>
        <skos:prefLabel xml:lang="en">pT1a: Tumor 1 cm or less in greatest dimension limited to the thyroid.</skos:prefLabel>
    </owl:Class>
    


    <!-- http://www.semanticweb.org/david/ontologies/2013/0/1.3.6.1.4.1.19376.1.8.2.1.122 -->

    <owl:Class rdf:about="&pathLex;122">
        <rdfs:subClassOf rdf:resource="&pathLex;60"/>
        <skos:definition xml:lang="en">Cervix-Infiltrating malignant neoplasm-Distance of lesion from closest uninvolved margin</skos:definition>
        <skos:prefLabel xml:lang="en">Distance of lesion from closest uninvolved margin</skos:prefLabel>
    </owl:Class>
    


    <!-- http://www.semanticweb.org/david/ontologies/2013/0/1.3.6.1.4.1.19376.1.8.2.1.1220 -->

    <owl:Class rdf:about="&pathLex;1220">
        <rdfs:subClassOf rdf:resource="&pathLex;99999"/>
        <skos:definition xml:lang="en">Thyroid-Infiltrating malignant neoplasm-pT-pT1b: Tumor more than 1 cm but not more than 2 cm in greatest dimension, limited to the thyroid</skos:definition>
        <skos:prefLabel xml:lang="en">pT1b: Tumor more than 1 cm but not more than 2 cm in greatest dimension, limited to the thyroid</skos:prefLabel>
    </owl:Class>
    


    <!-- http://www.semanticweb.org/david/ontologies/2013/0/1.3.6.1.4.1.19376.1.8.2.1.1221 -->

    <owl:Class rdf:about="&pathLex;1221">
        <rdfs:subClassOf rdf:resource="&pathLex;99999"/>
        <skos:definition xml:lang="en">Thyroid-Infiltrating malignant neoplasm-pT-pT2: Tumor more than 2 cm, but not more than 4 cm, limited to thyroid</skos:definition>
        <skos:prefLabel xml:lang="en">pT2: Tumor more than 2 cm, but not more than 4 cm, limited to thyroid</skos:prefLabel>
    </owl:Class>
    


    <!-- http://www.semanticweb.org/david/ontologies/2013/0/1.3.6.1.4.1.19376.1.8.2.1.1222 -->

    <owl:Class rdf:about="&pathLex;1222">
        <rdfs:subClassOf rdf:resource="&pathLex;99999"/>
        <skos:definition xml:lang="en">Thyroid-Infiltrating malignant neoplasm-pT-pT3: Tumor more than 4 cm limited to thyroid or any tumor with minimal extrathyroid extension (eg, extension to sternothyroid muscle or perithyroid soft tissues)</skos:definition>
        <skos:prefLabel xml:lang="en">pT3: Tumor more than 4 cm limited to thyroid or any tumor with minimal extrathyroid extension (eg, extension to sternothyroid muscle or perithyroid soft tissues)</skos:prefLabel>
    </owl:Class>
    


    <!-- http://www.semanticweb.org/david/ontologies/2013/0/1.3.6.1.4.1.19376.1.8.2.1.1223 -->

    <owl:Class rdf:about="&pathLex;1223">
        <rdfs:subClassOf rdf:resource="&pathLex;99999"/>
        <skos:definition xml:lang="en">Thyroid-Infiltrating malignant neoplasm-pT-pT4a: Intrathyroidal anaplastic carcinoma—surgically resectable</skos:definition>
        <skos:prefLabel xml:lang="en">pT4a: Intrathyroidal anaplastic carcinoma—surgically resectable</skos:prefLabel>
    </owl:Class>
    


    <!-- http://www.semanticweb.org/david/ontologies/2013/0/1.3.6.1.4.1.19376.1.8.2.1.1224 -->

    <owl:Class rdf:about="&pathLex;1224">
        <rdfs:subClassOf rdf:resource="&pathLex;99999"/>
        <skos:definition xml:lang="en">Thyroid-Infiltrating malignant neoplasm-pT-pT4b: Extrathyroidal anaplastic carcinoma—surgically unresectable</skos:definition>
        <skos:prefLabel xml:lang="en">pT4b: Extrathyroidal anaplastic carcinoma—surgically unresectable</skos:prefLabel>
    </owl:Class>
    


    <!-- http://www.semanticweb.org/david/ontologies/2013/0/1.3.6.1.4.1.19376.1.8.2.1.1225 -->

    <owl:Class rdf:about="&pathLex;1225">
        <rdfs:subClassOf rdf:resource="&pathLex;99999"/>
        <skos:definition xml:lang="en">Thyroid-Infiltrating malignant neoplasm-pN-pN0: No regional lymph node metastasis</skos:definition>
        <skos:prefLabel xml:lang="en">pN0: No regional lymph node metastasis</skos:prefLabel>
    </owl:Class>
    


    <!-- http://www.semanticweb.org/david/ontologies/2013/0/1.3.6.1.4.1.19376.1.8.2.1.1226 -->

    <owl:Class rdf:about="&pathLex;1226">
        <rdfs:subClassOf rdf:resource="&pathLex;99999"/>
        <skos:definition xml:lang="en">Thyroid-Infiltrating malignant neoplasm-pN-pN1a: Nodal metastases to Level VI (pretracheal, paratracheal and prelaryngeal/Delphian) lymph nodes</skos:definition>
        <skos:prefLabel xml:lang="en">pN1a: Nodal metastases to Level VI (pretracheal, paratracheal and prelaryngeal/Delphian) lymph nodes</skos:prefLabel>
    </owl:Class>
    


    <!-- http://www.semanticweb.org/david/ontologies/2013/0/1.3.6.1.4.1.19376.1.8.2.1.1227 -->

    <owl:Class rdf:about="&pathLex;1227">
        <rdfs:subClassOf rdf:resource="&pathLex;99999"/>
        <skos:definition xml:lang="en">Thyroid-Infiltrating malignant neoplasm-pN-pN1b: Metastases to unilateral, bilateral or contralateral cervical (Levels I, II, III, IV,V) or retropharyngeal or superior mediastinal lymph nodes (Level VII).</skos:definition>
        <skos:prefLabel xml:lang="en">pN1b: Metastases to unilateral, bilateral or contralateral cervical (Levels I, II, III, IV,V) or retropharyngeal or superior mediastinal lymph nodes (Level VII).</skos:prefLabel>
    </owl:Class>
    


    <!-- http://www.semanticweb.org/david/ontologies/2013/0/1.3.6.1.4.1.19376.1.8.2.1.123 -->

    <owl:Class rdf:about="&pathLex;123">
        <rdfs:subClassOf rdf:resource="&pathLex;137"/>
        <skos:definition xml:lang="en">Cervix-In situ neoplasm-Distance of lesion from closest uninvolved margin</skos:definition>
        <skos:prefLabel xml:lang="en">Distance of lesion from closest uninvolved margin</skos:prefLabel>
    </owl:Class>
    


    <!-- http://www.semanticweb.org/david/ontologies/2013/0/1.3.6.1.4.1.19376.1.8.2.1.1239 -->

    <owl:Class rdf:about="&pathLex;1239">
        <rdfs:subClassOf rdf:resource="&pathLex;99999"/>
        <skos:definition xml:lang="en">Lip, oral cavity-Infiltrating malignant neoplasm-Histologic type-Squamous cell carcinoma, conventional</skos:definition>
        <skos:prefLabel xml:lang="en">Squamous cell carcinoma, conventional</skos:prefLabel>
    </owl:Class>
    


    <!-- http://www.semanticweb.org/david/ontologies/2013/0/1.3.6.1.4.1.19376.1.8.2.1.124 -->

    <owl:Class rdf:about="&pathLex;124">
        <rdfs:subClassOf rdf:resource="&pathLex;62"/>
        <skos:definition xml:lang="en">Cervix-Infiltrating malignant neoplasm-Lymph-vascular invasion</skos:definition>
        <skos:prefLabel xml:lang="en">Cervix-Lymph-vascular invasion</skos:prefLabel>
        <skos:altLabel xml:lang="en">Lymph-vascular invasion</skos:altLabel>
    </owl:Class>
    


    <!-- http://www.semanticweb.org/david/ontologies/2013/0/1.3.6.1.4.1.19376.1.8.2.1.1240 -->

    <owl:Class rdf:about="&pathLex;1240">
        <rdfs:subClassOf rdf:resource="&pathLex;99999"/>
        <skos:prefLabel xml:lang="en">Basaloid squamous cell carcinoma</skos:prefLabel>
        <skos:definition xml:lang="en">Lip, oral cavity-Infiltrating malignant neoplasm-Histologic type-Basaloid squamous cell carcinoma</skos:definition>
    </owl:Class>
    


    <!-- http://www.semanticweb.org/david/ontologies/2013/0/1.3.6.1.4.1.19376.1.8.2.1.1241 -->

    <owl:Class rdf:about="&pathLex;1241">
        <rdfs:subClassOf rdf:resource="&pathLex;99999"/>
        <skos:definition xml:lang="en">Lip, oral cavity-Infiltrating malignant neoplasm-Histologic type-Spindle cell squamous carcinoma</skos:definition>
        <skos:prefLabel xml:lang="en">Spindle cell squamous carcinoma</skos:prefLabel>
    </owl:Class>
    


    <!-- http://www.semanticweb.org/david/ontologies/2013/0/1.3.6.1.4.1.19376.1.8.2.1.1242 -->

    <owl:Class rdf:about="&pathLex;1242">
        <rdfs:subClassOf rdf:resource="&pathLex;99999"/>
        <skos:definition xml:lang="en">Lip, oral cavity-Infiltrating malignant neoplasm-Histologic type-Verrucous carcinoma</skos:definition>
        <skos:prefLabel xml:lang="en">Verrucous carcinoma</skos:prefLabel>
    </owl:Class>
    


    <!-- http://www.semanticweb.org/david/ontologies/2013/0/1.3.6.1.4.1.19376.1.8.2.1.1245 -->

    <owl:Class rdf:about="&pathLex;1245">
        <rdfs:subClassOf rdf:resource="&pathLex;99999"/>
        <skos:prefLabel xml:lang="en">Adenosquamous carcinoma</skos:prefLabel>
        <skos:definition xml:lang="en">Lip, oral cavity-Infiltrating malignant neoplasm-Histologic type-Adenosquamous carcinoma</skos:definition>
    </owl:Class>
    


    <!-- http://www.semanticweb.org/david/ontologies/2013/0/1.3.6.1.4.1.19376.1.8.2.1.125 -->

    <owl:Class rdf:about="&pathLex;125">
        <rdfs:subClassOf rdf:resource="&pathLex;209"/>
        <skos:definition xml:lang="en">Cervix-Infiltrating malignant neoplasm-Lymph node sampling</skos:definition>
        <skos:prefLabel xml:lang="en">Cervix-Lymph node sampling</skos:prefLabel>
        <skos:altLabel xml:lang="en">Lymph node sampling</skos:altLabel>
    </owl:Class>
    


    <!-- http://www.semanticweb.org/david/ontologies/2013/0/1.3.6.1.4.1.19376.1.8.2.1.1258 -->

    <owl:Class rdf:about="&pathLex;1258">
        <rdfs:subClassOf rdf:resource="&pathLex;99999"/>
        <skos:definition xml:lang="en">Lip, oral cavity-Infiltrating malignant neoplasm-pT carcinoma-pT0: No evidence of primary tumor</skos:definition>
        <skos:prefLabel xml:lang="en">pT0: No evidence of primary tumor</skos:prefLabel>
    </owl:Class>
    


    <!-- http://www.semanticweb.org/david/ontologies/2013/0/1.3.6.1.4.1.19376.1.8.2.1.1259 -->

    <owl:Class rdf:about="&pathLex;1259">
        <rdfs:subClassOf rdf:resource="&pathLex;99999"/>
        <skos:definition xml:lang="en">Lip, oral cavity-Infiltrating malignant neoplasm-pT carcinoma-pTis: Carcinoma in situ</skos:definition>
        <skos:prefLabel xml:lang="en">pTis: Carcinoma in situ</skos:prefLabel>
    </owl:Class>
    


    <!-- http://www.semanticweb.org/david/ontologies/2013/0/1.3.6.1.4.1.19376.1.8.2.1.126 -->

    <owl:Class rdf:about="&pathLex;126">
        <rdfs:subClassOf rdf:resource="&pathLex;36"/>
        <skos:prefLabel xml:lang="en">Cervix-Extent</skos:prefLabel>
        <skos:definition xml:lang="en">Cervix-Infiltrating malignant neoplasm-Extent</skos:definition>
        <skos:altLabel xml:lang="en">Extent</skos:altLabel>
    </owl:Class>
    


    <!-- http://www.semanticweb.org/david/ontologies/2013/0/1.3.6.1.4.1.19376.1.8.2.1.1260 -->

    <owl:Class rdf:about="&pathLex;1260">
        <rdfs:subClassOf rdf:resource="&pathLex;99999"/>
        <skos:definition xml:lang="en">Lip, oral cavity-Infiltrating malignant neoplasm-pT carcinoma-pT1: Tumor 2 cm or less in greatest dimension</skos:definition>
        <skos:prefLabel xml:lang="en">pT1: Tumor 2 cm or less in greatest dimension</skos:prefLabel>
    </owl:Class>
    


    <!-- http://www.semanticweb.org/david/ontologies/2013/0/1.3.6.1.4.1.19376.1.8.2.1.1261 -->

    <owl:Class rdf:about="&pathLex;1261">
        <rdfs:subClassOf rdf:resource="&pathLex;99999"/>
        <skos:definition xml:lang="en">Lip, oral cavity-Infiltrating malignant neoplasm-pT carcinoma-pT2: Tumor more than 2 cm but not more than 4 cm in greatest dimension</skos:definition>
        <skos:prefLabel xml:lang="en">pT2: Tumor more than 2 cm but not more than 4 cm in greatest dimension</skos:prefLabel>
    </owl:Class>
    


    <!-- http://www.semanticweb.org/david/ontologies/2013/0/1.3.6.1.4.1.19376.1.8.2.1.1262 -->

    <owl:Class rdf:about="&pathLex;1262">
        <rdfs:subClassOf rdf:resource="&pathLex;99999"/>
        <skos:definition xml:lang="en">Lip, oral cavity-Infiltrating malignant neoplasm-pT carcinoma-pT3: Tumor more than 4 cm in greatest dimension - Oropharynx : or extension to lingual surface of epiglottis</skos:definition>
        <skos:prefLabel xml:lang="en">pT3: Tumor more than 4 cm in greatest dimension - Oropharynx : or extension to lingual surface of epiglottis</skos:prefLabel>
    </owl:Class>
    


    <!-- http://www.semanticweb.org/david/ontologies/2013/0/1.3.6.1.4.1.19376.1.8.2.1.1263 -->

    <owl:Class rdf:about="&pathLex;1263">
        <rdfs:subClassOf rdf:resource="&pathLex;99999"/>
        <skos:definition xml:lang="en">Lip, oral cavity-Infiltrating malignant neoplasm-pT carcinoma-pT4a: Moderately advanced local disease. Lip: Tumor invades through cortical bone, inferior alveolar nerve, floor of mouth, or skin of face, ie, chin or nose - Oral cavity: Tumor invades adjacent structures only (eg, through cortical bone [mandible, maxilla], into deep [extrinsic] muscle of tongue [genioglossus, hyoglossus, palatoglossus, and styloglossus], maxillary sinus, skin of face) - Oropharynx : Tumor invades larynx, deep/extrinsic muscle of tongue, medial pterygoid muscles, hard palate, or mandible</skos:definition>
        <skos:prefLabel xml:lang="en">pT4a: Moderately advanced local disease. Lip: Tumor invades through cortical bone, inferior alveolar nerve, floor of mouth, or skin of face, ie, chin or nose - Oral cavity: Tumor invades adjacent structures only (eg, through cortical bone [mandible, maxilla], into deep [extrinsic] muscle of tongue [genioglossus, hyoglossus, palatoglossus, and styloglossus], maxillary sinus, skin of face) - Oropharynx : Tumor invades larynx, deep/extrinsic muscle of tongue, medial pterygoid muscles, hard palate, or mandible</skos:prefLabel>
    </owl:Class>
    


    <!-- http://www.semanticweb.org/david/ontologies/2013/0/1.3.6.1.4.1.19376.1.8.2.1.1264 -->

    <owl:Class rdf:about="&pathLex;1264">
        <rdfs:subClassOf rdf:resource="&pathLex;99999"/>
        <skos:definition xml:lang="en">Lip, oral cavity-Infiltrating malignant neoplasm-pT carcinoma-pT4b: Very advanced local disease. Tumor invades masticator space, pterygoid plates, or skull base, and/or encases internal carotid artery - Oropharynx: Tumor invades lateral pterygoid muscle, pterygoid plates, lateral nasopharynx, or skull base, or encases carotid artery</skos:definition>
        <skos:prefLabel xml:lang="en">pT4b: Very advanced local disease. Tumor invades masticator space, pterygoid plates, or skull base, and/or encases internal carotid artery - Oropharynx: Tumor invades lateral pterygoid muscle, pterygoid plates, lateral nasopharynx, or skull base, or encases carotid artery</skos:prefLabel>
    </owl:Class>
    


    <!-- http://www.semanticweb.org/david/ontologies/2013/0/1.3.6.1.4.1.19376.1.8.2.1.1265 -->

    <owl:Class rdf:about="&pathLex;1265">
        <rdfs:subClassOf rdf:resource="&pathLex;99999"/>
        <skos:definition xml:lang="en">Lip, oral cavity-Infiltrating malignant neoplasm-pN-pN0: No regional lymph node metastasis</skos:definition>
        <skos:prefLabel xml:lang="en">pN0: No regional lymph node metastasis</skos:prefLabel>
    </owl:Class>
    


    <!-- http://www.semanticweb.org/david/ontologies/2013/0/1.3.6.1.4.1.19376.1.8.2.1.1266 -->

    <owl:Class rdf:about="&pathLex;1266">
        <rdfs:subClassOf rdf:resource="&pathLex;99999"/>
        <skos:definition xml:lang="en">Lip, oral cavity-Infiltrating malignant neoplasm-pN-pN1: Metastasis in a single ipsilateral lymph node, 3 cm or less in greatest dimension</skos:definition>
        <skos:prefLabel xml:lang="en">pN1: Metastasis in a single ipsilateral lymph node, 3 cm or less in greatest dimension</skos:prefLabel>
    </owl:Class>
    


    <!-- http://www.semanticweb.org/david/ontologies/2013/0/1.3.6.1.4.1.19376.1.8.2.1.1267 -->

    <owl:Class rdf:about="&pathLex;1267">
        <rdfs:subClassOf rdf:resource="&pathLex;99999"/>
        <skos:definition xml:lang="en">Lip, oral cavity-Infiltrating malignant neoplasm-pN-pN2a: Metastasis in a single ipsilateral lymph node, more than 3 cm but not more than 6 cm in greatest dimension</skos:definition>
        <skos:prefLabel xml:lang="en">pN2a: Metastasis in a single ipsilateral lymph node, more than 3 cm but not more than 6 cm in greatest dimension</skos:prefLabel>
    </owl:Class>
    


    <!-- http://www.semanticweb.org/david/ontologies/2013/0/1.3.6.1.4.1.19376.1.8.2.1.1268 -->

    <owl:Class rdf:about="&pathLex;1268">
        <rdfs:subClassOf rdf:resource="&pathLex;99999"/>
        <skos:definition xml:lang="en">Lip, oral cavity-Infiltrating malignant neoplasm-pN-pN2b: Metastasis in multiple ipsilateral lymph nodes, none more than 6 cm in greatest dimension</skos:definition>
        <skos:prefLabel xml:lang="en">pN2b: Metastasis in multiple ipsilateral lymph nodes, none more than 6 cm in greatest dimension</skos:prefLabel>
    </owl:Class>
    


    <!-- http://www.semanticweb.org/david/ontologies/2013/0/1.3.6.1.4.1.19376.1.8.2.1.1269 -->

    <owl:Class rdf:about="&pathLex;1269">
        <rdfs:subClassOf rdf:resource="&pathLex;99999"/>
        <skos:definition xml:lang="en">Lip, oral cavity-Infiltrating malignant neoplasm-pN-pN2c: Metastasis in bilateral or contralateral lymph nodes, none more than 6 cm in greatest dimension</skos:definition>
        <skos:prefLabel xml:lang="en">pN2c: Metastasis in bilateral or contralateral lymph nodes, none more than 6 cm in greatest dimension</skos:prefLabel>
    </owl:Class>
    


    <!-- http://www.semanticweb.org/david/ontologies/2013/0/1.3.6.1.4.1.19376.1.8.2.1.127 -->

    <owl:Class rdf:about="&pathLex;127">
        <rdfs:subClassOf rdf:resource="&pathLex;10012"/>
        <skos:definition xml:lang="en">Cervix-Lesion-Identification of pathogen agents</skos:definition>
        <skos:prefLabel xml:lang="en">Identification of pathogen agents</skos:prefLabel>
    </owl:Class>
    


    <!-- http://www.semanticweb.org/david/ontologies/2013/0/1.3.6.1.4.1.19376.1.8.2.1.1270 -->

    <owl:Class rdf:about="&pathLex;1270">
        <rdfs:subClassOf rdf:resource="&pathLex;99999"/>
        <skos:definition xml:lang="en">Lip, oral cavity-Infiltrating malignant neoplasm-pN-pN3: Metastasis in a lymph node more than 6 cm in greatest dimension</skos:definition>
        <skos:prefLabel xml:lang="en">pN3: Metastasis in a lymph node more than 6 cm in greatest dimension</skos:prefLabel>
    </owl:Class>
    


    <!-- http://www.semanticweb.org/david/ontologies/2013/0/1.3.6.1.4.1.19376.1.8.2.1.1271 -->

    <owl:Class rdf:about="&pathLex;1271">
        <rdfs:subClassOf rdf:resource="&pathLex;99999"/>
        <skos:prefLabel xml:lang="en">Nasopharynx</skos:prefLabel>
        <skos:definition xml:lang="en">Pharynx-Specimen-Target site-Nasopharynx</skos:definition>
    </owl:Class>
    


    <!-- http://www.semanticweb.org/david/ontologies/2013/0/1.3.6.1.4.1.19376.1.8.2.1.1272 -->

    <owl:Class rdf:about="&pathLex;1272">
        <rdfs:subClassOf rdf:resource="&pathLex;99999"/>
        <skos:prefLabel xml:lang="en">Hypopharynx</skos:prefLabel>
        <skos:definition xml:lang="en">Pharynx-Specimen-Target site-Hypopharynx</skos:definition>
    </owl:Class>
    


    <!-- http://www.semanticweb.org/david/ontologies/2013/0/1.3.6.1.4.1.19376.1.8.2.1.1277 -->

    <owl:Class rdf:about="&pathLex;1277">
        <rdfs:subClassOf rdf:resource="&pathLex;99999"/>
        <skos:prefLabel xml:lang="en">Laryngopharyngectomy</skos:prefLabel>
        <skos:definition xml:lang="en">Pharynx-Specimen-Specimen collection procedure-Laryngopharyngectomy</skos:definition>
    </owl:Class>
    


    <!-- http://www.semanticweb.org/david/ontologies/2013/0/1.3.6.1.4.1.19376.1.8.2.1.128 -->

    <owl:Class rdf:about="&pathLex;128">
        <rdfs:subClassOf rdf:resource="&pathLex;7"/>
        <skos:definition xml:lang="en">Cervix-Infiltrating malignant neoplasm-Lesion site</skos:definition>
        <skos:prefLabel xml:lang="en">Cervix-Lesion site</skos:prefLabel>
        <skos:altLabel xml:lang="en">Lesion site</skos:altLabel>
    </owl:Class>
    


    <!-- http://www.semanticweb.org/david/ontologies/2013/0/1.3.6.1.4.1.19376.1.8.2.1.1280 -->

    <owl:Class rdf:about="&pathLex;1280">
        <rdfs:subClassOf rdf:resource="&pathLex;99999"/>
        <skos:prefLabel xml:lang="en">Hypopharynx: Piriform sinus</skos:prefLabel>
        <skos:definition xml:lang="en">Pharynx-Infiltrating malignant neoplasm-Lesion site-Hypopharynx: Piriform sinus</skos:definition>
    </owl:Class>
    


    <!-- http://www.semanticweb.org/david/ontologies/2013/0/1.3.6.1.4.1.19376.1.8.2.1.1281 -->

    <owl:Class rdf:about="&pathLex;1281">
        <rdfs:subClassOf rdf:resource="&pathLex;99999"/>
        <skos:prefLabel xml:lang="en">Hypopharynx: Postcricoid</skos:prefLabel>
        <skos:definition xml:lang="en">Pharynx-Infiltrating malignant neoplasm-Lesion site-Hypopharynx: Postcricoid</skos:definition>
    </owl:Class>
    


    <!-- http://www.semanticweb.org/david/ontologies/2013/0/1.3.6.1.4.1.19376.1.8.2.1.1282 -->

    <owl:Class rdf:about="&pathLex;1282">
        <rdfs:subClassOf rdf:resource="&pathLex;99999"/>
        <skos:prefLabel xml:lang="en">Hypopharynx: Pharyngeal wall (posterior and/or lateral)</skos:prefLabel>
        <skos:definition xml:lang="en">Pharynx-Infiltrating malignant neoplasm-Lesion site-Hypopharynx: Pharyngeal wall (posterior and/or lateral)</skos:definition>
    </owl:Class>
    


    <!-- http://www.semanticweb.org/david/ontologies/2013/0/1.3.6.1.4.1.19376.1.8.2.1.129 -->

    <owl:Class rdf:about="&pathLex;129">
        <rdfs:subClassOf rdf:resource="&pathLex;45"/>
        <skos:definition xml:lang="en">Cervix-Infiltrating malignant neoplasm-Lymph node site</skos:definition>
        <skos:prefLabel xml:lang="en">Cervix-Lymph node site</skos:prefLabel>
        <skos:altLabel xml:lang="en">Lymph node site</skos:altLabel>
    </owl:Class>
    


    <!-- http://www.semanticweb.org/david/ontologies/2013/0/1.3.6.1.4.1.19376.1.8.2.1.130 -->

    <owl:Class rdf:about="&pathLex;130">
        <rdfs:subClassOf rdf:resource="&pathLex;39"/>
        <skos:definition xml:lang="en">Cervix-Infiltrating malignant neoplasm-Number of lymph nodes involved</skos:definition>
        <skos:prefLabel xml:lang="en">Cervix-Number of lymph nodes involved</skos:prefLabel>
        <skos:altLabel xml:lang="en">Number of lymph nodes involved</skos:altLabel>
    </owl:Class>
    


    <!-- http://www.semanticweb.org/david/ontologies/2013/0/1.3.6.1.4.1.19376.1.8.2.1.131 -->

    <owl:Class rdf:about="&pathLex;131">
        <rdfs:subClassOf rdf:resource="&pathLex;38"/>
        <skos:definition xml:lang="en">Cervix-Infiltrating malignant neoplasm-Number of lymph nodes examined</skos:definition>
        <skos:prefLabel xml:lang="en">Cervix-Number of lymph nodes examined</skos:prefLabel>
        <skos:altLabel xml:lang="en">Number of lymph nodes examined</skos:altLabel>
    </owl:Class>
    


    <!-- http://www.semanticweb.org/david/ontologies/2013/0/1.3.6.1.4.1.19376.1.8.2.1.1312 -->

    <owl:Class rdf:about="&pathLex;1312">
        <rdfs:subClassOf rdf:resource="&pathLex;99999"/>
        <skos:definition xml:lang="en">Salivary gland-Specimen-Target site-Total parotid gland (qualifier : right, left)</skos:definition>
        <skos:prefLabel xml:lang="en">Total parotid gland (qualifier : right, left)</skos:prefLabel>
    </owl:Class>
    


    <!-- http://www.semanticweb.org/david/ontologies/2013/0/1.3.6.1.4.1.19376.1.8.2.1.1313 -->

    <owl:Class rdf:about="&pathLex;1313">
        <rdfs:subClassOf rdf:resource="&pathLex;99999"/>
        <skos:definition xml:lang="en">Salivary gland-Infiltrating malignant neoplasm-Lesion site-Submandibular gland</skos:definition>
        <skos:prefLabel xml:lang="en">Submandibular gland</skos:prefLabel>
    </owl:Class>
    


    <!-- http://www.semanticweb.org/david/ontologies/2013/0/1.3.6.1.4.1.19376.1.8.2.1.1314 -->

    <owl:Class rdf:about="&pathLex;1314">
        <rdfs:subClassOf rdf:resource="&pathLex;99999"/>
        <skos:definition xml:lang="en">Salivary gland-Infiltrating malignant neoplasm-Lesion site-Sublingual gland</skos:definition>
        <skos:prefLabel xml:lang="en">Sublingual gland</skos:prefLabel>
    </owl:Class>
    


    <!-- http://www.semanticweb.org/david/ontologies/2013/0/1.3.6.1.4.1.19376.1.8.2.1.1316 -->

    <owl:Class rdf:about="&pathLex;1316">
        <rdfs:subClassOf rdf:resource="&pathLex;99999"/>
        <skos:definition xml:lang="en">Salivary gland-Specimen-Specimen collection procedure-Superficial parotidectomy (qualifier: right, left)</skos:definition>
        <skos:prefLabel xml:lang="en">Superficial parotidectomy (qualifier: right, left)</skos:prefLabel>
    </owl:Class>
    


    <!-- http://www.semanticweb.org/david/ontologies/2013/0/1.3.6.1.4.1.19376.1.8.2.1.1318 -->

    <owl:Class rdf:about="&pathLex;1318">
        <rdfs:subClassOf rdf:resource="&pathLex;99999"/>
        <skos:definition xml:lang="en">Salivary gland-Specimen-Specimen collection procedure-Total parotidectomy (qualifier: right, left)</skos:definition>
        <skos:prefLabel xml:lang="en">Total parotidectomy (qualifier: right, left)</skos:prefLabel>
    </owl:Class>
    


    <!-- http://www.semanticweb.org/david/ontologies/2013/0/1.3.6.1.4.1.19376.1.8.2.1.1321 -->

    <owl:Class rdf:about="&pathLex;1321">
        <rdfs:subClassOf rdf:resource="&pathLex;99999"/>
        <skos:prefLabel xml:lang="en">Adenoid cystic carcinoma</skos:prefLabel>
        <skos:definition xml:lang="en">Salivary gland-Infiltrating malignant neoplasm-Histologic type-Adenoid cystic carcinoma</skos:definition>
    </owl:Class>
    


    <!-- http://www.semanticweb.org/david/ontologies/2013/0/1.3.6.1.4.1.19376.1.8.2.1.1322 -->

    <owl:Class rdf:about="&pathLex;1322">
        <rdfs:subClassOf rdf:resource="&pathLex;99999"/>
        <skos:prefLabel xml:lang="en">Adenocarcinoma, not otherwise specified (NOS)</skos:prefLabel>
        <skos:definition xml:lang="en">Salivary gland-Infiltrating malignant neoplasm-Histologic type-Adenocarcinoma, not otherwise specified (NOS)</skos:definition>
    </owl:Class>
    


    <!-- http://www.semanticweb.org/david/ontologies/2013/0/1.3.6.1.4.1.19376.1.8.2.1.1323 -->

    <owl:Class rdf:about="&pathLex;1323">
        <rdfs:subClassOf rdf:resource="&pathLex;99999"/>
        <skos:prefLabel xml:lang="en">Basal cell adenocarcinoma</skos:prefLabel>
        <skos:definition xml:lang="en">Salivary gland-Infiltrating malignant neoplasm-Histologic type-Basal cell adenocarcinoma</skos:definition>
    </owl:Class>
    


    <!-- http://www.semanticweb.org/david/ontologies/2013/0/1.3.6.1.4.1.19376.1.8.2.1.1324 -->

    <owl:Class rdf:about="&pathLex;1324">
        <rdfs:subClassOf rdf:resource="&pathLex;99999"/>
        <skos:prefLabel xml:lang="en">Carcinoma ex pleomorphic adenoma (malignant mixed tumor)</skos:prefLabel>
        <skos:definition xml:lang="en">Salivary gland-Infiltrating malignant neoplasm-Histologic type-Carcinoma ex pleomorphic adenoma (malignant mixed tumor)</skos:definition>
    </owl:Class>
    


    <!-- http://www.semanticweb.org/david/ontologies/2013/0/1.3.6.1.4.1.19376.1.8.2.1.1325 -->

    <owl:Class rdf:about="&pathLex;1325">
        <rdfs:subClassOf rdf:resource="&pathLex;99999"/>
        <skos:prefLabel xml:lang="en">Carcinosarcoma (true malignant mixed tumor)</skos:prefLabel>
        <skos:definition xml:lang="en">Salivary gland-Infiltrating malignant neoplasm-Histologic type-Carcinosarcoma (true malignant mixed tumor)</skos:definition>
    </owl:Class>
    


    <!-- http://www.semanticweb.org/david/ontologies/2013/0/1.3.6.1.4.1.19376.1.8.2.1.1328 -->

    <owl:Class rdf:about="&pathLex;1328">
        <rdfs:subClassOf rdf:resource="&pathLex;99999"/>
        <skos:prefLabel xml:lang="en">Mucoepidermoid carcinoma</skos:prefLabel>
        <skos:definition xml:lang="en">Salivary gland-Infiltrating malignant neoplasm-Histologic type-Mucoepidermoid carcinoma</skos:definition>
    </owl:Class>
    


    <!-- http://www.semanticweb.org/david/ontologies/2013/0/1.3.6.1.4.1.19376.1.8.2.1.133 -->

    <owl:Class rdf:about="&pathLex;133">
        <rdfs:subClassOf rdf:resource="&pathLex;1432"/>
        <skos:definition xml:lang="en">Cervix-Infiltrating malignant neoplasm-pN</skos:definition>
        <skos:prefLabel xml:lang="en">Cervix-Infiltrating malignant neoplasm-pN</skos:prefLabel>
        <skos:altLabel xml:lang="en">pN</skos:altLabel>
    </owl:Class>
    


    <!-- http://www.semanticweb.org/david/ontologies/2013/0/1.3.6.1.4.1.19376.1.8.2.1.1330 -->

    <owl:Class rdf:about="&pathLex;1330">
        <rdfs:subClassOf rdf:resource="&pathLex;99999"/>
        <skos:definition xml:lang="en">Salivary gland-Infiltrating malignant neoplasm-Histologic type-Sebaceous adenocarcinoma</skos:definition>
        <skos:prefLabel xml:lang="en">Sebaceous adenocarcinoma</skos:prefLabel>
    </owl:Class>
    


    <!-- http://www.semanticweb.org/david/ontologies/2013/0/1.3.6.1.4.1.19376.1.8.2.1.1331 -->

    <owl:Class rdf:about="&pathLex;1331">
        <rdfs:subClassOf rdf:resource="&pathLex;99999"/>
        <skos:definition xml:lang="en">Salivary gland-Infiltrating malignant neoplasm-Histologic type-Small cell (neuroendocrine) carcinoma</skos:definition>
        <skos:prefLabel xml:lang="en">Small cell (neuroendocrine) carcinoma</skos:prefLabel>
    </owl:Class>
    


    <!-- http://www.semanticweb.org/david/ontologies/2013/0/1.3.6.1.4.1.19376.1.8.2.1.1332 -->

    <owl:Class rdf:about="&pathLex;1332">
        <rdfs:subClassOf rdf:resource="&pathLex;99999"/>
        <skos:definition xml:lang="en">Salivary gland-Infiltrating malignant neoplasm-Histologic type-Undifferentiated carcinoma, large cell type</skos:definition>
        <skos:prefLabel xml:lang="en">Undifferentiated carcinoma, large cell type</skos:prefLabel>
    </owl:Class>
    


    <!-- http://www.semanticweb.org/david/ontologies/2013/0/1.3.6.1.4.1.19376.1.8.2.1.1340 -->

    <owl:Class rdf:about="&pathLex;1340">
        <rdfs:subClassOf rdf:resource="&pathLex;99999"/>
        <skos:definition xml:lang="en">Salivary gland-Infiltrating malignant neoplasm-pT-pTX: Cannot be assessed</skos:definition>
        <skos:prefLabel xml:lang="en">pTX: Cannot be assessed</skos:prefLabel>
    </owl:Class>
    


    <!-- http://www.semanticweb.org/david/ontologies/2013/0/1.3.6.1.4.1.19376.1.8.2.1.1341 -->

    <owl:Class rdf:about="&pathLex;1341">
        <rdfs:subClassOf rdf:resource="&pathLex;99999"/>
        <skos:definition xml:lang="en">Salivary gland-Infiltrating malignant neoplasm-pT-pT0: No evidence of primary tumor</skos:definition>
        <skos:prefLabel xml:lang="en">pT0: No evidence of primary tumor</skos:prefLabel>
    </owl:Class>
    


    <!-- http://www.semanticweb.org/david/ontologies/2013/0/1.3.6.1.4.1.19376.1.8.2.1.1342 -->

    <owl:Class rdf:about="&pathLex;1342">
        <rdfs:subClassOf rdf:resource="&pathLex;99999"/>
        <skos:definition xml:lang="en">Salivary gland-Infiltrating malignant neoplasm-pT-pT1: Tumor 2 cm or less in greatest dimension without extraparenchymal extension</skos:definition>
        <skos:prefLabel xml:lang="en">pT1: Tumor 2 cm or less in greatest dimension without extraparenchymal extension</skos:prefLabel>
    </owl:Class>
    


    <!-- http://www.semanticweb.org/david/ontologies/2013/0/1.3.6.1.4.1.19376.1.8.2.1.1343 -->

    <owl:Class rdf:about="&pathLex;1343">
        <rdfs:subClassOf rdf:resource="&pathLex;99999"/>
        <skos:definition xml:lang="en">Salivary gland-Infiltrating malignant neoplasm-pT-pT2: Tumor more than 2 cm but not more than 4 cm in greatest dimension without extraparenchymal extension</skos:definition>
        <skos:prefLabel xml:lang="en">pT2: Tumor more than 2 cm but not more than 4 cm in greatest dimension without extraparenchymal extension</skos:prefLabel>
    </owl:Class>
    


    <!-- http://www.semanticweb.org/david/ontologies/2013/0/1.3.6.1.4.1.19376.1.8.2.1.1344 -->

    <owl:Class rdf:about="&pathLex;1344">
        <rdfs:subClassOf rdf:resource="&pathLex;99999"/>
        <skos:definition xml:lang="en">Salivary gland-Infiltrating malignant neoplasm-pT-pT3: Tumor more than 4 cm and/or tumor having extraparenchymal extension</skos:definition>
        <skos:prefLabel xml:lang="en">pT3: Tumor more than 4 cm and/or tumor having extraparenchymal extension</skos:prefLabel>
    </owl:Class>
    


    <!-- http://www.semanticweb.org/david/ontologies/2013/0/1.3.6.1.4.1.19376.1.8.2.1.1345 -->

    <owl:Class rdf:about="&pathLex;1345">
        <rdfs:subClassOf rdf:resource="&pathLex;99999"/>
        <skos:definition xml:lang="en">Salivary gland-Infiltrating malignant neoplasm-pT-pT4a: Moderately advanced disease. Tumor invades skin, mandible, ear canal, and/or facial nerve.</skos:definition>
        <skos:prefLabel xml:lang="en">pT4a: Moderately advanced disease. Tumor invades skin, mandible, ear canal, and/or facial nerve.</skos:prefLabel>
    </owl:Class>
    


    <!-- http://www.semanticweb.org/david/ontologies/2013/0/1.3.6.1.4.1.19376.1.8.2.1.1346 -->

    <owl:Class rdf:about="&pathLex;1346">
        <rdfs:subClassOf rdf:resource="&pathLex;99999"/>
        <skos:definition xml:lang="en">Salivary gland-Infiltrating malignant neoplasm-pT-pT4b: Very advanced local disease. Tumor invades skull base and/or pterygoid plates and/or encases carotid artery</skos:definition>
        <skos:prefLabel xml:lang="en">pT4b: Very advanced local disease. Tumor invades skull base and/or pterygoid plates and/or encases carotid artery</skos:prefLabel>
    </owl:Class>
    


    <!-- http://www.semanticweb.org/david/ontologies/2013/0/1.3.6.1.4.1.19376.1.8.2.1.1347 -->

    <owl:Class rdf:about="&pathLex;1347">
        <rdfs:subClassOf rdf:resource="&pathLex;99999"/>
        <skos:definition xml:lang="en">Salivary gland-Infiltrating malignant neoplasm-pN-pN0: No regional lymph node metastasis</skos:definition>
        <skos:prefLabel xml:lang="en">pN0: No regional lymph node metastasis</skos:prefLabel>
    </owl:Class>
    


    <!-- http://www.semanticweb.org/david/ontologies/2013/0/1.3.6.1.4.1.19376.1.8.2.1.1348 -->

    <owl:Class rdf:about="&pathLex;1348">
        <rdfs:subClassOf rdf:resource="&pathLex;99999"/>
        <skos:definition xml:lang="en">Salivary gland-Infiltrating malignant neoplasm-pN-pN1: Metastasis in a single ipsilateral lymph node, 3 cm or less in greatest dimension</skos:definition>
        <skos:prefLabel xml:lang="en">pN1: Metastasis in a single ipsilateral lymph node, 3 cm or less in greatest dimension</skos:prefLabel>
    </owl:Class>
    


    <!-- http://www.semanticweb.org/david/ontologies/2013/0/1.3.6.1.4.1.19376.1.8.2.1.1349 -->

    <owl:Class rdf:about="&pathLex;1349">
        <rdfs:subClassOf rdf:resource="&pathLex;99999"/>
        <skos:definition xml:lang="en">Salivary gland-Infiltrating malignant neoplasm-pN-pN2a: Metastasis in a single ipsilateral lymph node, more than 3 cm but not more than 6 cm in greatest dimension</skos:definition>
        <skos:prefLabel xml:lang="en">pN2a: Metastasis in a single ipsilateral lymph node, more than 3 cm but not more than 6 cm in greatest dimension</skos:prefLabel>
    </owl:Class>
    


    <!-- http://www.semanticweb.org/david/ontologies/2013/0/1.3.6.1.4.1.19376.1.8.2.1.135 -->

    <owl:Class rdf:about="&pathLex;135">
        <rdfs:subClassOf rdf:resource="&pathLex;1431"/>
        <skos:definition xml:lang="en">Cervix-Infiltrating malignant neoplasm-pT</skos:definition>
        <skos:prefLabel xml:lang="en">Cervix-Infiltrating malignant neoplasm-pT</skos:prefLabel>
        <skos:altLabel xml:lang="en">pT</skos:altLabel>
    </owl:Class>
    


    <!-- http://www.semanticweb.org/david/ontologies/2013/0/1.3.6.1.4.1.19376.1.8.2.1.1350 -->

    <owl:Class rdf:about="&pathLex;1350">
        <rdfs:subClassOf rdf:resource="&pathLex;99999"/>
        <skos:definition xml:lang="en">Salivary gland-Infiltrating malignant neoplasm-pN-pN2b: Metastasis in multiple ipsilateral lymph nodes, none more than 6 cm in greatest dimension</skos:definition>
        <skos:prefLabel xml:lang="en">pN2b: Metastasis in multiple ipsilateral lymph nodes, none more than 6 cm in greatest dimension</skos:prefLabel>
    </owl:Class>
    


    <!-- http://www.semanticweb.org/david/ontologies/2013/0/1.3.6.1.4.1.19376.1.8.2.1.1351 -->

    <owl:Class rdf:about="&pathLex;1351">
        <rdfs:subClassOf rdf:resource="&pathLex;99999"/>
        <skos:definition xml:lang="en">Salivary gland-Infiltrating malignant neoplasm-pN-pN2c: Metastasis in bilateral or contralateral lymph nodes, none more than 6 cm in greatest dimension</skos:definition>
        <skos:prefLabel xml:lang="en">pN2c: Metastasis in bilateral or contralateral lymph nodes, none more than 6 cm in greatest dimension</skos:prefLabel>
    </owl:Class>
    


    <!-- http://www.semanticweb.org/david/ontologies/2013/0/1.3.6.1.4.1.19376.1.8.2.1.1352 -->

    <owl:Class rdf:about="&pathLex;1352">
        <rdfs:subClassOf rdf:resource="&pathLex;99999"/>
        <skos:definition xml:lang="en">Salivary gland-Infiltrating malignant neoplasm-pN-pN3: Metastasis in a lymph node, more than 6 cm in greatest dimension</skos:definition>
        <skos:prefLabel xml:lang="en">pN3: Metastasis in a lymph node, more than 6 cm in greatest dimension</skos:prefLabel>
    </owl:Class>
    


    <!-- http://www.semanticweb.org/david/ontologies/2013/0/1.3.6.1.4.1.19376.1.8.2.1.1354 -->

    <owl:Class rdf:about="&pathLex;1354">
        <rdfs:subClassOf rdf:resource="&pathLex;99999"/>
        <skos:definition xml:lang="en">Larynx-Specimen-Specimen collection procedure-Partial laryngectomy (specify type)</skos:definition>
        <skos:prefLabel xml:lang="en">Partial laryngectomy (specify type)</skos:prefLabel>
    </owl:Class>
    


    <!-- http://www.semanticweb.org/david/ontologies/2013/0/1.3.6.1.4.1.19376.1.8.2.1.1355 -->

    <owl:Class rdf:about="&pathLex;1355">
        <rdfs:subClassOf rdf:resource="&pathLex;99999"/>
        <skos:definition xml:lang="en">Larynx-Specimen-Specimen collection procedure-Total laryngectomy</skos:definition>
        <skos:prefLabel xml:lang="en">Total laryngectomy</skos:prefLabel>
    </owl:Class>
    


    <!-- http://www.semanticweb.org/david/ontologies/2013/0/1.3.6.1.4.1.19376.1.8.2.1.136 -->

    <owl:Class rdf:about="&pathLex;136">
        <rdfs:subClassOf rdf:resource="&pathLex;10"/>
        <skos:definition xml:lang="en">Cervix-Infiltrating malignant neoplasm-Lesion size, largest dimension</skos:definition>
        <skos:prefLabel xml:lang="en">Cervix-Lesion size, largest dimension</skos:prefLabel>
        <skos:altLabel xml:lang="en">Lesion size, largest dimension</skos:altLabel>
    </owl:Class>
    


    <!-- http://www.semanticweb.org/david/ontologies/2013/0/1.3.6.1.4.1.19376.1.8.2.1.1362 -->

    <owl:Class rdf:about="&pathLex;1362">
        <rdfs:subClassOf rdf:resource="&pathLex;99999"/>
        <skos:definition xml:lang="en">Larynx-Infiltrating malignant neoplasm-Histologic type-Squamous cell carcinoma, conventional</skos:definition>
        <skos:prefLabel xml:lang="en">Squamous cell carcinoma, conventional</skos:prefLabel>
    </owl:Class>
    


    <!-- http://www.semanticweb.org/david/ontologies/2013/0/1.3.6.1.4.1.19376.1.8.2.1.1363 -->

    <owl:Class rdf:about="&pathLex;1363">
        <rdfs:subClassOf rdf:resource="&pathLex;99999"/>
        <skos:prefLabel xml:lang="en">Adenosquamous carcinoma</skos:prefLabel>
        <skos:definition xml:lang="en">Larynx-Infiltrating malignant neoplasm-Histologic type-Adenosquamous carcinoma</skos:definition>
    </owl:Class>
    


    <!-- http://www.semanticweb.org/david/ontologies/2013/0/1.3.6.1.4.1.19376.1.8.2.1.1364 -->

    <owl:Class rdf:about="&pathLex;1364">
        <rdfs:subClassOf rdf:resource="&pathLex;99999"/>
        <skos:definition xml:lang="en">Larynx-Infiltrating malignant neoplasm-Histologic type-Verrucous carcinoma</skos:definition>
        <skos:prefLabel xml:lang="en">Verrucous carcinoma</skos:prefLabel>
    </owl:Class>
    


    <!-- http://www.semanticweb.org/david/ontologies/2013/0/1.3.6.1.4.1.19376.1.8.2.1.1365 -->

    <owl:Class rdf:about="&pathLex;1365">
        <rdfs:subClassOf rdf:resource="&pathLex;99999"/>
        <skos:definition xml:lang="en">Larynx-Infiltrating malignant neoplasm-Histologic type-Lymphoepithelial carcinoma (non-nasopharyngeal)</skos:definition>
        <skos:prefLabel xml:lang="en">Lymphoepithelial carcinoma (non-nasopharyngeal)</skos:prefLabel>
    </owl:Class>
    


    <!-- http://www.semanticweb.org/david/ontologies/2013/0/1.3.6.1.4.1.19376.1.8.2.1.1366 -->

    <owl:Class rdf:about="&pathLex;1366">
        <rdfs:subClassOf rdf:resource="&pathLex;99999"/>
        <skos:prefLabel xml:lang="en">Carcinoma of Minor Salivary Glands</skos:prefLabel>
        <skos:definition xml:lang="en">Larynx-Infiltrating malignant neoplasm-Histologic type-Carcinoma of Minor Salivary Glands</skos:definition>
    </owl:Class>
    


    <!-- http://www.semanticweb.org/david/ontologies/2013/0/1.3.6.1.4.1.19376.1.8.2.1.137 -->

    <owl:Class rdf:about="&pathLex;137">
        <rdfs:subClassOf rdf:resource="&pathLex;10011"/>
        <skos:definition xml:lang="en">Cervix-In situ neoplasm-Cytologic type</skos:definition>
        <skos:prefLabel xml:lang="en">Cytologic type</skos:prefLabel>
    </owl:Class>
    


    <!-- http://www.semanticweb.org/david/ontologies/2013/0/1.3.6.1.4.1.19376.1.8.2.1.1376 -->

    <owl:Class rdf:about="&pathLex;1376">
        <rdfs:subClassOf rdf:resource="&pathLex;99999"/>
        <skos:definition xml:lang="en">Larynx-Infiltrating malignant neoplasm-pT supra glottis carcinoma-pT0: No evidence of primary tumor</skos:definition>
        <skos:prefLabel xml:lang="en">pT0: No evidence of primary tumor</skos:prefLabel>
    </owl:Class>
    


    <!-- http://www.semanticweb.org/david/ontologies/2013/0/1.3.6.1.4.1.19376.1.8.2.1.1377 -->

    <owl:Class rdf:about="&pathLex;1377">
        <rdfs:subClassOf rdf:resource="&pathLex;99999"/>
        <skos:definition xml:lang="en">Larynx-Infiltrating malignant neoplasm-pT supra glottis carcinoma-pTis: Carcinoma in situ</skos:definition>
        <skos:prefLabel xml:lang="en">pTis: Carcinoma in situ</skos:prefLabel>
    </owl:Class>
    


    <!-- http://www.semanticweb.org/david/ontologies/2013/0/1.3.6.1.4.1.19376.1.8.2.1.1378 -->

    <owl:Class rdf:about="&pathLex;1378">
        <rdfs:subClassOf rdf:resource="&pathLex;99999"/>
        <skos:definition xml:lang="en">Larynx-Infiltrating malignant neoplasm-pT supra glottis carcinoma-pT1: Tumor limited to one subsite of supraglottis with normal vocal cord mobility</skos:definition>
        <skos:prefLabel xml:lang="en">pT1: Tumor limited to one subsite of supraglottis with normal vocal cord mobility</skos:prefLabel>
    </owl:Class>
    


    <!-- http://www.semanticweb.org/david/ontologies/2013/0/1.3.6.1.4.1.19376.1.8.2.1.1379 -->

    <owl:Class rdf:about="&pathLex;1379">
        <rdfs:subClassOf rdf:resource="&pathLex;99999"/>
        <skos:definition xml:lang="en">Larynx-Infiltrating malignant neoplasm-pT supra glottis carcinoma-pT2: Tumor invades mucosa of more than one adjacent subsite of supraglottis or glottis or region outside the supraglottis (eg, mucosa of base of tongue, vallecula, medial wall of pyriform sinus) without fixation of the larynx</skos:definition>
        <skos:prefLabel xml:lang="en">pT2: Tumor invades mucosa of more than one adjacent subsite of supraglottis or glottis or region outside the supraglottis (eg, mucosa of base of tongue, vallecula, medial wall of pyriform sinus) without fixation of the larynx</skos:prefLabel>
    </owl:Class>
    


    <!-- http://www.semanticweb.org/david/ontologies/2013/0/1.3.6.1.4.1.19376.1.8.2.1.138 -->

    <owl:Class rdf:about="&pathLex;138">
        <rdfs:subClassOf rdf:resource="&pathLex;10010"/>
        <skos:definition xml:lang="en">Cervix-Infiltrating malignant neoplasm-Cytologic type</skos:definition>
        <skos:prefLabel xml:lang="en">Cytologic type</skos:prefLabel>
    </owl:Class>
    


    <!-- http://www.semanticweb.org/david/ontologies/2013/0/1.3.6.1.4.1.19376.1.8.2.1.1380 -->

    <owl:Class rdf:about="&pathLex;1380">
        <rdfs:subClassOf rdf:resource="&pathLex;99999"/>
        <skos:definition xml:lang="en">Larynx-Infiltrating malignant neoplasm-pT supra glottis carcinoma-pT3: Tumor limited to larynx with vocal cord fixation and/or invades any of the following: postcricoid area, preepiglottic space, paraglottic space, and/or inner cortex of thyroid cartilage</skos:definition>
        <skos:prefLabel xml:lang="en">pT3: Tumor limited to larynx with vocal cord fixation and/or invades any of the following: postcricoid area, preepiglottic space, paraglottic space, and/or inner cortex of thyroid cartilage</skos:prefLabel>
    </owl:Class>
    


    <!-- http://www.semanticweb.org/david/ontologies/2013/0/1.3.6.1.4.1.19376.1.8.2.1.1381 -->

    <owl:Class rdf:about="&pathLex;1381">
        <rdfs:subClassOf rdf:resource="&pathLex;99999"/>
        <skos:definition xml:lang="en">Larynx-Infiltrating malignant neoplasm-pT supra glottis carcinoma-pT4a: Moderately advanced local disease. Tumor invades through the thyroid cartilage and/or invades tissues beyond the larynx (eg, trachea, soft tissues of neck including deep extrinsic muscle of tongue, strap muscles, thyroid, or esophagus)</skos:definition>
        <skos:prefLabel xml:lang="en">pT4a: Moderately advanced local disease. Tumor invades through the thyroid cartilage and/or invades tissues beyond the larynx (eg, trachea, soft tissues of neck including deep extrinsic muscle of tongue, strap muscles, thyroid, or esophagus)</skos:prefLabel>
    </owl:Class>
    


    <!-- http://www.semanticweb.org/david/ontologies/2013/0/1.3.6.1.4.1.19376.1.8.2.1.1382 -->

    <owl:Class rdf:about="&pathLex;1382">
        <rdfs:subClassOf rdf:resource="&pathLex;99999"/>
        <skos:definition xml:lang="en">Larynx-Infiltrating malignant neoplasm-pT supra glottis carcinoma-pT4b: Very advanced local disease. Tumor invades prevertebral space, encases carotid artery, or invades mediastinal structures</skos:definition>
        <skos:prefLabel xml:lang="en">pT4b: Very advanced local disease. Tumor invades prevertebral space, encases carotid artery, or invades mediastinal structures</skos:prefLabel>
    </owl:Class>
    


    <!-- http://www.semanticweb.org/david/ontologies/2013/0/1.3.6.1.4.1.19376.1.8.2.1.1383 -->

    <owl:Class rdf:about="&pathLex;1383">
        <rdfs:subClassOf rdf:resource="&pathLex;99999"/>
        <skos:definition xml:lang="en">Larynx-Infiltrating malignant neoplasm-pT glottis carcinoma-pT0: No evidence of primary tumor</skos:definition>
        <skos:prefLabel xml:lang="en">pT0: No evidence of primary tumor</skos:prefLabel>
    </owl:Class>
    


    <!-- http://www.semanticweb.org/david/ontologies/2013/0/1.3.6.1.4.1.19376.1.8.2.1.1384 -->

    <owl:Class rdf:about="&pathLex;1384">
        <rdfs:subClassOf rdf:resource="&pathLex;99999"/>
        <skos:definition xml:lang="en">Larynx-Infiltrating malignant neoplasm-pT glottis carcinoma-pTis: Carcinoma in situ</skos:definition>
        <skos:prefLabel xml:lang="en">pTis: Carcinoma in situ</skos:prefLabel>
    </owl:Class>
    


    <!-- http://www.semanticweb.org/david/ontologies/2013/0/1.3.6.1.4.1.19376.1.8.2.1.1385 -->

    <owl:Class rdf:about="&pathLex;1385">
        <rdfs:subClassOf rdf:resource="&pathLex;99999"/>
        <skos:definition xml:lang="en">Larynx-Infiltrating malignant neoplasm-pT glottis carcinoma-pT1: Tumor limited to the vocal cord(s) (may involve anterior or posterior commissure) with normal mobility</skos:definition>
        <skos:prefLabel xml:lang="en">pT1: Tumor limited to the vocal cord(s) (may involve anterior or posterior commissure) with normal mobility</skos:prefLabel>
    </owl:Class>
    


    <!-- http://www.semanticweb.org/david/ontologies/2013/0/1.3.6.1.4.1.19376.1.8.2.1.1386 -->

    <owl:Class rdf:about="&pathLex;1386">
        <rdfs:subClassOf rdf:resource="&pathLex;99999"/>
        <skos:definition xml:lang="en">Larynx-Infiltrating malignant neoplasm-pT glottis carcinoma-pT1a: Tumor limited to one vocal cord</skos:definition>
        <skos:prefLabel xml:lang="en">pT1a: Tumor limited to one vocal cord</skos:prefLabel>
    </owl:Class>
    


    <!-- http://www.semanticweb.org/david/ontologies/2013/0/1.3.6.1.4.1.19376.1.8.2.1.1387 -->

    <owl:Class rdf:about="&pathLex;1387">
        <rdfs:subClassOf rdf:resource="&pathLex;99999"/>
        <skos:definition xml:lang="en">Larynx-Infiltrating malignant neoplasm-pT glottis carcinoma-pT1b: Tumor involves both vocal cords</skos:definition>
        <skos:prefLabel xml:lang="en">pT1b: Tumor involves both vocal cords</skos:prefLabel>
    </owl:Class>
    


    <!-- http://www.semanticweb.org/david/ontologies/2013/0/1.3.6.1.4.1.19376.1.8.2.1.1388 -->

    <owl:Class rdf:about="&pathLex;1388">
        <rdfs:subClassOf rdf:resource="&pathLex;99999"/>
        <skos:definition xml:lang="en">Larynx-Infiltrating malignant neoplasm-pT glottis carcinoma-pT2: Tumor extends to supraglottis and/or subglottis and/or with impaired vocal cord mobility</skos:definition>
        <skos:prefLabel xml:lang="en">pT2: Tumor extends to supraglottis and/or subglottis and/or with impaired vocal cord mobility</skos:prefLabel>
    </owl:Class>
    


    <!-- http://www.semanticweb.org/david/ontologies/2013/0/1.3.6.1.4.1.19376.1.8.2.1.1389 -->

    <owl:Class rdf:about="&pathLex;1389">
        <rdfs:subClassOf rdf:resource="&pathLex;99999"/>
        <skos:definition xml:lang="en">Larynx-Infiltrating malignant neoplasm-pT glottis carcinoma-pT3: Tumor limited to the larynx with vocal cord fixation and/or invades paraglottic space and/or minor thyroid cartilage erosion (eg, inner cortex) (Note H)</skos:definition>
        <skos:prefLabel xml:lang="en">pT3: Tumor limited to the larynx with vocal cord fixation and/or invades paraglottic space and/or minor thyroid cartilage erosion (eg, inner cortex) (Note H)</skos:prefLabel>
    </owl:Class>
    


    <!-- http://www.semanticweb.org/david/ontologies/2013/0/1.3.6.1.4.1.19376.1.8.2.1.139 -->

    <owl:Class rdf:about="&pathLex;139">
        <rdfs:subClassOf rdf:resource="&pathLex;23"/>
        <skos:prefLabel xml:lang="en">Cervix-Histologic type</skos:prefLabel>
        <skos:definition xml:lang="en">Cervix-Lesion-Histologic type</skos:definition>
        <skos:altLabel xml:lang="en">Histologic type</skos:altLabel>
    </owl:Class>
    


    <!-- http://www.semanticweb.org/david/ontologies/2013/0/1.3.6.1.4.1.19376.1.8.2.1.1390 -->

    <owl:Class rdf:about="&pathLex;1390">
        <rdfs:subClassOf rdf:resource="&pathLex;99999"/>
        <skos:definition xml:lang="en">Larynx-Infiltrating malignant neoplasm-pT glottis carcinoma-pT4a: Moderately advanced local disease. Tumor invades through the outer cortex of the thyroid cartilage and/or invades tissues beyond the larynx (eg, trachea, soft tissues of neck including deep extrinsic muscle of the tongue, strap muscles, thyroid, or esophagus) (Note H)</skos:definition>
        <skos:prefLabel xml:lang="en">pT4a: Moderately advanced local disease. Tumor invades through the outer cortex of the thyroid cartilage and/or invades tissues beyond the larynx (eg, trachea, soft tissues of neck including deep extrinsic muscle of the tongue, strap muscles, thyroid, or esophagus) (Note H)</skos:prefLabel>
    </owl:Class>
    


    <!-- http://www.semanticweb.org/david/ontologies/2013/0/1.3.6.1.4.1.19376.1.8.2.1.1391 -->

    <owl:Class rdf:about="&pathLex;1391">
        <rdfs:subClassOf rdf:resource="&pathLex;99999"/>
        <skos:definition xml:lang="en">Larynx-Infiltrating malignant neoplasm-pT glottis carcinoma-pT4b: Very advanced local disease. Tumor invades prevertebral space, encases carotid artery, or invades mediastinal structures</skos:definition>
        <skos:prefLabel xml:lang="en">pT4b: Very advanced local disease. Tumor invades prevertebral space, encases carotid artery, or invades mediastinal structures</skos:prefLabel>
    </owl:Class>
    


    <!-- http://www.semanticweb.org/david/ontologies/2013/0/1.3.6.1.4.1.19376.1.8.2.1.1392 -->

    <owl:Class rdf:about="&pathLex;1392">
        <rdfs:subClassOf rdf:resource="&pathLex;99999"/>
        <skos:definition xml:lang="en">Larynx-Infiltrating malignant neoplasm-pT sub glottis carcinoma-pT0: No evidence of primary tumor</skos:definition>
        <skos:prefLabel xml:lang="en">pT0: No evidence of primary tumor</skos:prefLabel>
    </owl:Class>
    


    <!-- http://www.semanticweb.org/david/ontologies/2013/0/1.3.6.1.4.1.19376.1.8.2.1.1393 -->

    <owl:Class rdf:about="&pathLex;1393">
        <rdfs:subClassOf rdf:resource="&pathLex;99999"/>
        <skos:definition xml:lang="en">Larynx-Infiltrating malignant neoplasm-pT sub glottis carcinoma-pTis: Carcinoma in situ</skos:definition>
        <skos:prefLabel xml:lang="en">pTis: Carcinoma in situ</skos:prefLabel>
    </owl:Class>
    


    <!-- http://www.semanticweb.org/david/ontologies/2013/0/1.3.6.1.4.1.19376.1.8.2.1.1394 -->

    <owl:Class rdf:about="&pathLex;1394">
        <rdfs:subClassOf rdf:resource="&pathLex;99999"/>
        <skos:definition xml:lang="en">Larynx-Infiltrating malignant neoplasm-pT sub glottis carcinoma-pT1: Tumor limited to subglottis</skos:definition>
        <skos:prefLabel xml:lang="en">pT1: Tumor limited to subglottis</skos:prefLabel>
    </owl:Class>
    


    <!-- http://www.semanticweb.org/david/ontologies/2013/0/1.3.6.1.4.1.19376.1.8.2.1.1395 -->

    <owl:Class rdf:about="&pathLex;1395">
        <rdfs:subClassOf rdf:resource="&pathLex;99999"/>
        <skos:definition xml:lang="en">Larynx-Infiltrating malignant neoplasm-pT sub glottis carcinoma-pT2: Tumor extends to vocal cord(s) with normal or impaired mobility</skos:definition>
        <skos:prefLabel xml:lang="en">pT2: Tumor extends to vocal cord(s) with normal or impaired mobility</skos:prefLabel>
    </owl:Class>
    


    <!-- http://www.semanticweb.org/david/ontologies/2013/0/1.3.6.1.4.1.19376.1.8.2.1.1396 -->

    <owl:Class rdf:about="&pathLex;1396">
        <rdfs:subClassOf rdf:resource="&pathLex;99999"/>
        <skos:definition xml:lang="en">Larynx-Infiltrating malignant neoplasm-pT sub glottis carcinoma-pT3: Tumor limited to larynx with vocal cord fixation</skos:definition>
        <skos:prefLabel xml:lang="en">pT3: Tumor limited to larynx with vocal cord fixation</skos:prefLabel>
    </owl:Class>
    


    <!-- http://www.semanticweb.org/david/ontologies/2013/0/1.3.6.1.4.1.19376.1.8.2.1.1397 -->

    <owl:Class rdf:about="&pathLex;1397">
        <rdfs:subClassOf rdf:resource="&pathLex;99999"/>
        <skos:definition xml:lang="en">Larynx-Infiltrating malignant neoplasm-pT sub glottis carcinoma-pT4a: Moderately advanced local disease. Tumor invades cricoid or thyroid cartilage and/or invades tissues beyond the larynx (eg, trachea, soft tissues of neck including deep extrinsic muscles of the tongue, strap muscles, thyroid, or esophagus)</skos:definition>
        <skos:prefLabel xml:lang="en">pT4a: Moderately advanced local disease. Tumor invades cricoid or thyroid cartilage and/or invades tissues beyond the larynx (eg, trachea, soft tissues of neck including deep extrinsic muscles of the tongue, strap muscles, thyroid, or esophagus)</skos:prefLabel>
    </owl:Class>
    


    <!-- http://www.semanticweb.org/david/ontologies/2013/0/1.3.6.1.4.1.19376.1.8.2.1.1398 -->

    <owl:Class rdf:about="&pathLex;1398">
        <rdfs:subClassOf rdf:resource="&pathLex;99999"/>
        <skos:definition xml:lang="en">Larynx-Infiltrating malignant neoplasm-pT sub glottis carcinoma-pT4b: Very advanced local disease. Tumor invades prevertebral space, encases carotid artery, or invades mediastinal structures</skos:definition>
        <skos:prefLabel xml:lang="en">pT4b: Very advanced local disease. Tumor invades prevertebral space, encases carotid artery, or invades mediastinal structures</skos:prefLabel>
    </owl:Class>
    


    <!-- http://www.semanticweb.org/david/ontologies/2013/0/1.3.6.1.4.1.19376.1.8.2.1.1399 -->

    <owl:Class rdf:about="&pathLex;1399">
        <rdfs:subClassOf rdf:resource="&pathLex;99999"/>
        <skos:definition xml:lang="en">Larynx-Infiltrating malignant neoplasm-pT mucosal malignant melanoma-pT0: No evidence of primary tumor</skos:definition>
        <skos:prefLabel xml:lang="en">pT0: No evidence of primary tumor</skos:prefLabel>
    </owl:Class>
    


    <!-- http://www.semanticweb.org/david/ontologies/2013/0/1.3.6.1.4.1.19376.1.8.2.1.14 -->

    <owl:Class rdf:about="&pathLex;14">
        <rdfs:subClassOf rdf:resource="&pathLex;99999"/>
        <skos:prefLabel xml:lang="en">Lesion size, largest dimension</skos:prefLabel>
        <skos:definition xml:lang="en">Prostate-Infiltrating malignant neoplasm-Lesion size, largest dimension</skos:definition>
    </owl:Class>
    


    <!-- http://www.semanticweb.org/david/ontologies/2013/0/1.3.6.1.4.1.19376.1.8.2.1.140 -->

    <owl:Class rdf:about="&pathLex;140">
        <rdfs:subClassOf rdf:resource="&pathLex;1840"/>
        <skos:prefLabel xml:lang="en">Cervix-Histologic type</skos:prefLabel>
        <skos:definition xml:lang="en">Cervix-In situ neoplasm-Histologic type</skos:definition>
        <skos:altLabel xml:lang="en">Histologic type</skos:altLabel>
    </owl:Class>
    


    <!-- http://www.semanticweb.org/david/ontologies/2013/0/1.3.6.1.4.1.19376.1.8.2.1.1400 -->

    <owl:Class rdf:about="&pathLex;1400">
        <rdfs:subClassOf rdf:resource="&pathLex;99999"/>
        <skos:definition xml:lang="en">Larynx-Infiltrating malignant neoplasm-pT mucosal malignant melanoma-pTis: Carcinoma in situ</skos:definition>
        <skos:prefLabel xml:lang="en">pTis: Carcinoma in situ</skos:prefLabel>
    </owl:Class>
    


    <!-- http://www.semanticweb.org/david/ontologies/2013/0/1.3.6.1.4.1.19376.1.8.2.1.1401 -->

    <owl:Class rdf:about="&pathLex;1401">
        <rdfs:subClassOf rdf:resource="&pathLex;99999"/>
        <skos:definition xml:lang="en">Larynx-Infiltrating malignant neoplasm-pT mucosal malignant melanoma-pT3: Mucosal disease</skos:definition>
        <skos:prefLabel xml:lang="en">pT3: Mucosal disease</skos:prefLabel>
    </owl:Class>
    


    <!-- http://www.semanticweb.org/david/ontologies/2013/0/1.3.6.1.4.1.19376.1.8.2.1.1402 -->

    <owl:Class rdf:about="&pathLex;1402">
        <rdfs:subClassOf rdf:resource="&pathLex;99999"/>
        <skos:definition xml:lang="en">Larynx-Infiltrating malignant neoplasm-pT mucosal malignant melanoma-pT4a: Moderately advanced disease. Tumor involving deep soft tissue, cartilage, bone, or overlying skin</skos:definition>
        <skos:prefLabel xml:lang="en">pT4a: Moderately advanced disease. Tumor involving deep soft tissue, cartilage, bone, or overlying skin</skos:prefLabel>
    </owl:Class>
    


    <!-- http://www.semanticweb.org/david/ontologies/2013/0/1.3.6.1.4.1.19376.1.8.2.1.1403 -->

    <owl:Class rdf:about="&pathLex;1403">
        <rdfs:subClassOf rdf:resource="&pathLex;99999"/>
        <skos:definition xml:lang="en">Larynx-Infiltrating malignant neoplasm-pT mucosal malignant melanoma-pT4b: Very advanced disease. Tumor involving brain, dura, skull base, lower cranial nerves (IX, X, XI, XII), masticator space, carotid artery, prevertebral space, or mediastinal structures</skos:definition>
        <skos:prefLabel xml:lang="en">pT4b: Very advanced disease. Tumor involving brain, dura, skull base, lower cranial nerves (IX, X, XI, XII), masticator space, carotid artery, prevertebral space, or mediastinal structures</skos:prefLabel>
    </owl:Class>
    


    <!-- http://www.semanticweb.org/david/ontologies/2013/0/1.3.6.1.4.1.19376.1.8.2.1.1404 -->

    <owl:Class rdf:about="&pathLex;1404">
        <rdfs:subClassOf rdf:resource="&pathLex;99999"/>
        <skos:definition xml:lang="en">Larynx-Infiltrating malignant neoplasm-pN carcinoma-pN0: No regional lymph node metastasis</skos:definition>
        <skos:prefLabel xml:lang="en">pN0: No regional lymph node metastasis</skos:prefLabel>
    </owl:Class>
    


    <!-- http://www.semanticweb.org/david/ontologies/2013/0/1.3.6.1.4.1.19376.1.8.2.1.1405 -->

    <owl:Class rdf:about="&pathLex;1405">
        <rdfs:subClassOf rdf:resource="&pathLex;99999"/>
        <skos:definition xml:lang="en">Larynx-Infiltrating malignant neoplasm-pN carcinoma-pN1: Metastasis in a single ipsilateral lymph node, 3 cm or less in greatest dimension</skos:definition>
        <skos:prefLabel xml:lang="en">pN1: Metastasis in a single ipsilateral lymph node, 3 cm or less in greatest dimension</skos:prefLabel>
    </owl:Class>
    


    <!-- http://www.semanticweb.org/david/ontologies/2013/0/1.3.6.1.4.1.19376.1.8.2.1.1406 -->

    <owl:Class rdf:about="&pathLex;1406">
        <rdfs:subClassOf rdf:resource="&pathLex;99999"/>
        <skos:definition xml:lang="en">Larynx-Infiltrating malignant neoplasm-pN carcinoma-pN2: Metastasis in a single ipsilateral lymph node, more than 3 cm but not more than 6 cm in greatest dimension, or in multiple ipsilateral lymph nodes, none more than 6 cm in greatest dimension, or in bilateral or contralateral lymph nodes, none more than 6 cm in greatest dimension</skos:definition>
        <skos:prefLabel xml:lang="en">pN2: Metastasis in a single ipsilateral lymph node, more than 3 cm but not more than 6 cm in greatest dimension, or in multiple ipsilateral lymph nodes, none more than 6 cm in greatest dimension, or in bilateral or contralateral lymph nodes, none more than 6 cm in greatest dimension</skos:prefLabel>
    </owl:Class>
    


    <!-- http://www.semanticweb.org/david/ontologies/2013/0/1.3.6.1.4.1.19376.1.8.2.1.1407 -->

    <owl:Class rdf:about="&pathLex;1407">
        <rdfs:subClassOf rdf:resource="&pathLex;99999"/>
        <skos:definition xml:lang="en">Larynx-Infiltrating malignant neoplasm-pN carcinoma-pN2a: Metastasis in a single ipsilateral lymph node, more than 3 cm but not more than 6 cm in greatest dimension</skos:definition>
        <skos:prefLabel xml:lang="en">pN2a: Metastasis in a single ipsilateral lymph node, more than 3 cm but not more than 6 cm in greatest dimension</skos:prefLabel>
    </owl:Class>
    


    <!-- http://www.semanticweb.org/david/ontologies/2013/0/1.3.6.1.4.1.19376.1.8.2.1.1408 -->

    <owl:Class rdf:about="&pathLex;1408">
        <rdfs:subClassOf rdf:resource="&pathLex;99999"/>
        <skos:definition xml:lang="en">Larynx-Infiltrating malignant neoplasm-pN carcinoma-pN2b: Metastasis in multiple ipsilateral lymph nodes, none more than 6 cm in greatest dimension</skos:definition>
        <skos:prefLabel xml:lang="en">pN2b: Metastasis in multiple ipsilateral lymph nodes, none more than 6 cm in greatest dimension</skos:prefLabel>
    </owl:Class>
    


    <!-- http://www.semanticweb.org/david/ontologies/2013/0/1.3.6.1.4.1.19376.1.8.2.1.1409 -->

    <owl:Class rdf:about="&pathLex;1409">
        <rdfs:subClassOf rdf:resource="&pathLex;99999"/>
        <skos:definition xml:lang="en">Larynx-Infiltrating malignant neoplasm-pN carcinoma-pN2c: Metastasis in bilateral or contralateral lymph nodes, none more than 6 cm in greatest dimension</skos:definition>
        <skos:prefLabel xml:lang="en">pN2c: Metastasis in bilateral or contralateral lymph nodes, none more than 6 cm in greatest dimension</skos:prefLabel>
    </owl:Class>
    


    <!-- http://www.semanticweb.org/david/ontologies/2013/0/1.3.6.1.4.1.19376.1.8.2.1.141 -->

    <owl:Class rdf:about="&pathLex;141">
        <rdfs:subClassOf rdf:resource="&pathLex;21"/>
        <skos:prefLabel xml:lang="en">Cervix-Histologic type</skos:prefLabel>
        <skos:definition xml:lang="en">Cervix-Infiltrating malignant neoplasm-Histologic type</skos:definition>
        <skos:altLabel xml:lang="en">Histologic type</skos:altLabel>
    </owl:Class>
    


    <!-- http://www.semanticweb.org/david/ontologies/2013/0/1.3.6.1.4.1.19376.1.8.2.1.1410 -->

    <owl:Class rdf:about="&pathLex;1410">
        <rdfs:subClassOf rdf:resource="&pathLex;99999"/>
        <skos:definition xml:lang="en">Larynx-Infiltrating malignant neoplasm-pN carcinoma-pN3: Metastasis in a lymph node more than 6 cm in greatest dimension</skos:definition>
        <skos:prefLabel xml:lang="en">pN3: Metastasis in a lymph node more than 6 cm in greatest dimension</skos:prefLabel>
    </owl:Class>
    


    <!-- http://www.semanticweb.org/david/ontologies/2013/0/1.3.6.1.4.1.19376.1.8.2.1.1411 -->

    <owl:Class rdf:about="&pathLex;1411">
        <rdfs:subClassOf rdf:resource="&pathLex;99999"/>
        <skos:definition xml:lang="en">Larynx-Infiltrating malignant neoplasm-pN mucosal malignant melanoma-pN0: No regional lymph node metastases</skos:definition>
        <skos:prefLabel xml:lang="en">pN0: No regional lymph node metastases</skos:prefLabel>
    </owl:Class>
    


    <!-- http://www.semanticweb.org/david/ontologies/2013/0/1.3.6.1.4.1.19376.1.8.2.1.1412 -->

    <owl:Class rdf:about="&pathLex;1412">
        <rdfs:subClassOf rdf:resource="&pathLex;99999"/>
        <skos:definition xml:lang="en">Larynx-Infiltrating malignant neoplasm-pN mucosal malignant melanoma-pN1: Regional lymph node metastases present</skos:definition>
        <skos:prefLabel xml:lang="en">pN1: Regional lymph node metastases present</skos:prefLabel>
    </owl:Class>
    


    <!-- http://www.semanticweb.org/david/ontologies/2013/0/1.3.6.1.4.1.19376.1.8.2.1.1413 -->

    <owl:Class rdf:about="&pathLex;1413">
        <rdfs:subClassOf rdf:resource="&pathLex;99999"/>
        <skos:prefLabel xml:lang="en">Endoscopic resection</skos:prefLabel>
        <skos:definition xml:lang="en">Esophagus-Specimen-Specimen collection procedure-Endoscopic resection</skos:definition>
    </owl:Class>
    


    <!-- http://www.semanticweb.org/david/ontologies/2013/0/1.3.6.1.4.1.19376.1.8.2.1.1415 -->

    <owl:Class rdf:about="&pathLex;1415">
        <rdfs:subClassOf rdf:resource="&pathLex;99999"/>
        <skos:prefLabel xml:lang="en">Urinary bladder</skos:prefLabel>
        <skos:definition xml:lang="en">Urinary bladder-Specimen-Target site-Urinary bladder</skos:definition>
    </owl:Class>
    


    <!-- http://www.semanticweb.org/david/ontologies/2013/0/1.3.6.1.4.1.19376.1.8.2.1.1431 -->

    <owl:Class rdf:about="&pathLex;1431">
        <rdfs:subClassOf rdf:resource="&pathLex;10010"/>
        <skos:altLabel xml:lang="en">Concept pT UICC TNM  7ème édition</skos:altLabel>
        <skos:definition xml:lang="en">Generic-Infiltrating malignant neoplasm-pT-Concept pT UICC TNM  7ème édition</skos:definition>
        <skos:prefLabel xml:lang="en">pT-Concept pT UICC TNM  7ème édition</skos:prefLabel>
    </owl:Class>
    


    <!-- http://www.semanticweb.org/david/ontologies/2013/0/1.3.6.1.4.1.19376.1.8.2.1.1432 -->

    <owl:Class rdf:about="&pathLex;1432">
        <rdfs:subClassOf rdf:resource="&pathLex;10010"/>
        <skos:altLabel xml:lang="en">Concept pN UICC TNM  7ème édition</skos:altLabel>
        <skos:definition xml:lang="en">Generic-Infiltrating malignant neoplasm-pN-Concept pN UICC TNM  7ème édition</skos:definition>
        <skos:prefLabel xml:lang="en">pN-Concept pN UICC TNM  7ème édition</skos:prefLabel>
    </owl:Class>
    


    <!-- http://www.semanticweb.org/david/ontologies/2013/0/1.3.6.1.4.1.19376.1.8.2.1.1433 -->

    <owl:Class rdf:about="&pathLex;1433">
        <rdfs:subClassOf rdf:resource="&pathLex;10010"/>
        <skos:altLabel xml:lang="en">Concept pM UICC TNM  7ème édition</skos:altLabel>
        <skos:definition xml:lang="en">Generic-Infiltrating malignant neoplasm-pM-Concept pM UICC TNM  7ème édition</skos:definition>
        <skos:prefLabel xml:lang="en">pM-Concept pM UICC TNM  7ème édition</skos:prefLabel>
    </owl:Class>
    


    <!-- http://www.semanticweb.org/david/ontologies/2013/0/1.3.6.1.4.1.19376.1.8.2.1.1437 -->

    <owl:Class rdf:about="&pathLex;1437">
        <rdfs:subClassOf rdf:resource="&pathLex;138"/>
        <skos:definition xml:lang="en">Cervix-Infiltrating malignant neoplasm-Cytologic type-Squamous cell carcinoma</skos:definition>
        <skos:prefLabel xml:lang="en">Squamous cell carcinoma</skos:prefLabel>
    </owl:Class>
    


    <!-- http://www.semanticweb.org/david/ontologies/2013/0/1.3.6.1.4.1.19376.1.8.2.1.1438 -->

    <owl:Class rdf:about="&pathLex;1438">
        <rdfs:subClassOf rdf:resource="&pathLex;138"/>
        <skos:prefLabel xml:lang="en">Adenocarcinoma</skos:prefLabel>
        <skos:definition xml:lang="en">Cervix-Infiltrating malignant neoplasm-Cytologic type-Adenocarcinoma</skos:definition>
    </owl:Class>
    


    <!-- http://www.semanticweb.org/david/ontologies/2013/0/1.3.6.1.4.1.19376.1.8.2.1.1439 -->

    <owl:Class rdf:about="&pathLex;1439">
        <rdfs:subClassOf rdf:resource="&pathLex;137"/>
        <skos:prefLabel xml:lang="en">Atypical squamous cells</skos:prefLabel>
        <skos:definition xml:lang="en">Cervix-In situ neoplasm-Cytologic type-Atypical squamous cells</skos:definition>
    </owl:Class>
    


    <!-- http://www.semanticweb.org/david/ontologies/2013/0/1.3.6.1.4.1.19376.1.8.2.1.1440 -->

    <owl:Class rdf:about="&pathLex;1440">
        <rdfs:subClassOf rdf:resource="&pathLex;137"/>
        <skos:prefLabel xml:lang="en">Atypical squamous cells of undetermined significance (ASC-US)</skos:prefLabel>
        <skos:definition xml:lang="en">Cervix-In situ neoplasm-Cytologic type-Atypical squamous cells of undetermined significance (ASC-US)</skos:definition>
    </owl:Class>
    


    <!-- http://www.semanticweb.org/david/ontologies/2013/0/1.3.6.1.4.1.19376.1.8.2.1.1441 -->

    <owl:Class rdf:about="&pathLex;1441">
        <rdfs:subClassOf rdf:resource="&pathLex;137"/>
        <skos:prefLabel xml:lang="en">Atypical squamous cells for which a high-grade lesion cannot be excluded (ASC-H)</skos:prefLabel>
        <skos:definition xml:lang="en">Cervix-In situ neoplasm-Cytologic type-Atypical squamous cells for which a high-grade lesion cannot be excluded (ASC-H)</skos:definition>
    </owl:Class>
    


    <!-- http://www.semanticweb.org/david/ontologies/2013/0/1.3.6.1.4.1.19376.1.8.2.1.1443 -->

    <owl:Class rdf:about="&pathLex;1443">
        <rdfs:subClassOf rdf:resource="&pathLex;137"/>
        <skos:definition xml:lang="en">Cervix-In situ neoplasm-Cytologic type-Low-grade squamous intraepithelial lesion encompassing HPV infection or mild dysplasia (CIN 1)</skos:definition>
        <skos:prefLabel xml:lang="en">Low-grade squamous intraepithelial lesion encompassing HPV infection or mild dysplasia (CIN 1)</skos:prefLabel>
    </owl:Class>
    


    <!-- http://www.semanticweb.org/david/ontologies/2013/0/1.3.6.1.4.1.19376.1.8.2.1.1444 -->

    <owl:Class rdf:about="&pathLex;1444">
        <rdfs:subClassOf rdf:resource="&pathLex;137"/>
        <skos:definition xml:lang="en">Cervix-In situ neoplasm-Cytologic type-High-grade squamous intraepithelial lesion encompassing moderate (CIN 2) and severe dysplasia (CIN 3/CIS); whether the lesion has features suggesting invasion is noted</skos:definition>
        <skos:prefLabel xml:lang="en">High-grade squamous intraepithelial lesion encompassing moderate (CIN 2) and severe dysplasia (CIN 3/CIS); whether the lesion has features suggesting invasion is noted</skos:prefLabel>
    </owl:Class>
    


    <!-- http://www.semanticweb.org/david/ontologies/2013/0/1.3.6.1.4.1.19376.1.8.2.1.1446 -->

    <owl:Class rdf:about="&pathLex;1446">
        <rdfs:subClassOf rdf:resource="&pathLex;137"/>
        <skos:prefLabel xml:lang="en">Atypical glandular cells</skos:prefLabel>
        <skos:definition xml:lang="en">Cervix-In situ neoplasm-Cytologic type-Atypical glandular cells</skos:definition>
    </owl:Class>
    


    <!-- http://www.semanticweb.org/david/ontologies/2013/0/1.3.6.1.4.1.19376.1.8.2.1.1447 -->

    <owl:Class rdf:about="&pathLex;1447">
        <rdfs:subClassOf rdf:resource="&pathLex;137"/>
        <skos:prefLabel xml:lang="en">Atypical endocervical cells</skos:prefLabel>
        <skos:definition xml:lang="en">Cervix-In situ neoplasm-Cytologic type-Atypical endocervical cells</skos:definition>
    </owl:Class>
    


    <!-- http://www.semanticweb.org/david/ontologies/2013/0/1.3.6.1.4.1.19376.1.8.2.1.1448 -->

    <owl:Class rdf:about="&pathLex;1448">
        <rdfs:subClassOf rdf:resource="&pathLex;137"/>
        <skos:prefLabel xml:lang="en">Atypical endometrial cells</skos:prefLabel>
        <skos:definition xml:lang="en">Cervix-In situ neoplasm-Cytologic type-Atypical endometrial cells</skos:definition>
    </owl:Class>
    


    <!-- http://www.semanticweb.org/david/ontologies/2013/0/1.3.6.1.4.1.19376.1.8.2.1.1449 -->

    <owl:Class rdf:about="&pathLex;1449">
        <rdfs:subClassOf rdf:resource="&pathLex;137"/>
        <skos:prefLabel xml:lang="en">Atypical glandular cells likely to be
cancerous</skos:prefLabel>
        <skos:definition xml:lang="en">Cervix-In situ neoplasm-Cytologic type-Atypical glandular cells likely to be
cancerous</skos:definition>
    </owl:Class>
    


    <!-- http://www.semanticweb.org/david/ontologies/2013/0/1.3.6.1.4.1.19376.1.8.2.1.145 -->

    <owl:Class rdf:about="&pathLex;145">
        <rdfs:subClassOf rdf:resource="&pathLex;99999"/>
        <skos:definition xml:lang="en">Colon-Infiltrating malignant neoplasm-Distance of lesion from closest uninvolved margin</skos:definition>
        <skos:prefLabel xml:lang="en">Distance of lesion from closest uninvolved margin</skos:prefLabel>
    </owl:Class>
    


    <!-- http://www.semanticweb.org/david/ontologies/2013/0/1.3.6.1.4.1.19376.1.8.2.1.1450 -->

    <owl:Class rdf:about="&pathLex;1450">
        <rdfs:subClassOf rdf:resource="&pathLex;137"/>
        <skos:prefLabel xml:lang="en">Atypical endocervical cells likely to be
cancerou
</skos:prefLabel>
        <skos:definition xml:lang="en">Cervix-In situ neoplasm-Cytologic type-Atypical endocervical cells likely to be
cancerou
</skos:definition>
    </owl:Class>
    


    <!-- http://www.semanticweb.org/david/ontologies/2013/0/1.3.6.1.4.1.19376.1.8.2.1.1451 -->

    <owl:Class rdf:about="&pathLex;1451">
        <rdfs:subClassOf rdf:resource="&pathLex;137"/>
        <skos:prefLabel xml:lang="en">Adenocarcinoma endocervical in situ </skos:prefLabel>
        <skos:definition xml:lang="en">Cervix-In situ neoplasm-Cytologic type-Adenocarcinoma endocervical in situ </skos:definition>
    </owl:Class>
    


    <!-- http://www.semanticweb.org/david/ontologies/2013/0/1.3.6.1.4.1.19376.1.8.2.1.1455 -->

    <owl:Class rdf:about="&pathLex;1455">
        <rdfs:subClassOf rdf:resource="&pathLex;139"/>
        <skos:definition xml:lang="en">Cervix-Lesion-Histologic type-Inflammation</skos:definition>
        <skos:prefLabel xml:lang="en">Inflammation</skos:prefLabel>
    </owl:Class>
    


    <!-- http://www.semanticweb.org/david/ontologies/2013/0/1.3.6.1.4.1.19376.1.8.2.1.147 -->

    <owl:Class rdf:about="&pathLex;147">
        <rdfs:subClassOf rdf:resource="&pathLex;99999"/>
        <skos:definition xml:lang="en">Colon-Infiltrating malignant neoplasm-Lymph-vascular invasion</skos:definition>
        <skos:prefLabel xml:lang="en">Lymph-vascular invasion</skos:prefLabel>
    </owl:Class>
    


    <!-- http://www.semanticweb.org/david/ontologies/2013/0/1.3.6.1.4.1.19376.1.8.2.1.1472 -->

    <owl:Class rdf:about="&pathLex;1472">
        <rdfs:subClassOf rdf:resource="&pathLex;434"/>
        <skos:definition xml:lang="en">Breast-Infiltrating malignant neoplasm-HER2/neu (immunoperoxidase study)-Positive (Score 3+)</skos:definition>
        <skos:prefLabel xml:lang="en">Positive (Score 3+)</skos:prefLabel>
    </owl:Class>
    


    <!-- http://www.semanticweb.org/david/ontologies/2013/0/1.3.6.1.4.1.19376.1.8.2.1.1473 -->

    <owl:Class rdf:about="&pathLex;1473">
        <rdfs:subClassOf rdf:resource="&pathLex;434"/>
        <skos:definition xml:lang="en">Breast-Infiltrating malignant neoplasm-HER2/neu (immunoperoxidase study)-Negative (Score 0)</skos:definition>
        <skos:prefLabel xml:lang="en">Negative (Score 0)</skos:prefLabel>
    </owl:Class>
    


    <!-- http://www.semanticweb.org/david/ontologies/2013/0/1.3.6.1.4.1.19376.1.8.2.1.148 -->

    <owl:Class rdf:about="&pathLex;148">
        <rdfs:subClassOf rdf:resource="&pathLex;99999"/>
        <skos:definition xml:lang="en">Colon-Infiltrating malignant neoplasm-Extent</skos:definition>
        <skos:prefLabel xml:lang="en">Extent</skos:prefLabel>
    </owl:Class>
    


    <!-- http://www.semanticweb.org/david/ontologies/2013/0/1.3.6.1.4.1.19376.1.8.2.1.149 -->

    <owl:Class rdf:about="&pathLex;149">
        <rdfs:subClassOf rdf:resource="&pathLex;99999"/>
        <skos:definition xml:lang="en">Colon-Infiltrating malignant neoplasm-Perineural invasion</skos:definition>
        <skos:prefLabel xml:lang="en">Perineural invasion</skos:prefLabel>
    </owl:Class>
    


    <!-- http://www.semanticweb.org/david/ontologies/2013/0/1.3.6.1.4.1.19376.1.8.2.1.15 -->

    <owl:Class rdf:about="&pathLex;15">
        <rdfs:subClassOf rdf:resource="&pathLex;99999"/>
        <skos:prefLabel xml:lang="en">Lesion size, largest dimension</skos:prefLabel>
        <skos:definition xml:lang="en">Prostate-Infiltrating malignant neoplasm-Lesion size, largest dimension</skos:definition>
    </owl:Class>
    


    <!-- http://www.semanticweb.org/david/ontologies/2013/0/1.3.6.1.4.1.19376.1.8.2.1.150 -->

    <owl:Class rdf:about="&pathLex;150">
        <rdfs:subClassOf rdf:resource="&pathLex;99999"/>
        <skos:definition xml:lang="en">Colon-Infiltrating malignant neoplasm-Lesion site</skos:definition>
        <skos:prefLabel xml:lang="en">Lesion site</skos:prefLabel>
    </owl:Class>
    


    <!-- http://www.semanticweb.org/david/ontologies/2013/0/1.3.6.1.4.1.19376.1.8.2.1.151 -->

    <owl:Class rdf:about="&pathLex;151">
        <rdfs:subClassOf rdf:resource="&pathLex;99999"/>
        <skos:definition xml:lang="en">Colon-Infiltrating malignant neoplasm-Margin site</skos:definition>
        <skos:prefLabel xml:lang="en">Margin site</skos:prefLabel>
    </owl:Class>
    


    <!-- http://www.semanticweb.org/david/ontologies/2013/0/1.3.6.1.4.1.19376.1.8.2.1.152 -->

    <owl:Class rdf:about="&pathLex;152">
        <rdfs:subClassOf rdf:resource="&pathLex;99999"/>
        <skos:definition xml:lang="en">Colon-Infiltrating malignant neoplasm-Number of lymph nodes involved</skos:definition>
        <skos:prefLabel xml:lang="en">Number of lymph nodes involved</skos:prefLabel>
    </owl:Class>
    


    <!-- http://www.semanticweb.org/david/ontologies/2013/0/1.3.6.1.4.1.19376.1.8.2.1.153 -->

    <owl:Class rdf:about="&pathLex;153">
        <rdfs:subClassOf rdf:resource="&pathLex;99999"/>
        <skos:definition xml:lang="en">Colon-Infiltrating malignant neoplasm-Number of lymph nodes examined</skos:definition>
        <skos:prefLabel xml:lang="en">Number of lymph nodes examined</skos:prefLabel>
    </owl:Class>
    


    <!-- http://www.semanticweb.org/david/ontologies/2013/0/1.3.6.1.4.1.19376.1.8.2.1.155 -->

    <owl:Class rdf:about="&pathLex;155">
        <rdfs:subClassOf rdf:resource="&pathLex;99999"/>
        <skos:definition xml:lang="en">Colon-Infiltrating malignant neoplasm-pN</skos:definition>
        <skos:prefLabel xml:lang="en">pN</skos:prefLabel>
    </owl:Class>
    


    <!-- http://www.semanticweb.org/david/ontologies/2013/0/1.3.6.1.4.1.19376.1.8.2.1.157 -->

    <owl:Class rdf:about="&pathLex;157">
        <rdfs:subClassOf rdf:resource="&pathLex;99999"/>
        <skos:definition xml:lang="en">Colon-Infiltrating malignant neoplasm-pT</skos:definition>
        <skos:prefLabel xml:lang="en">pT</skos:prefLabel>
    </owl:Class>
    


    <!-- http://www.semanticweb.org/david/ontologies/2013/0/1.3.6.1.4.1.19376.1.8.2.1.158 -->

    <owl:Class rdf:about="&pathLex;158">
        <rdfs:subClassOf rdf:resource="&pathLex;99999"/>
        <skos:definition xml:lang="en">Colon-Infiltrating malignant neoplasm-Lesion size, largest dimension</skos:definition>
        <skos:prefLabel xml:lang="en">Lesion size, largest dimension</skos:prefLabel>
    </owl:Class>
    


    <!-- http://www.semanticweb.org/david/ontologies/2013/0/1.3.6.1.4.1.19376.1.8.2.1.159 -->

    <owl:Class rdf:about="&pathLex;159">
        <rdfs:subClassOf rdf:resource="&pathLex;99999"/>
        <skos:definition xml:lang="en">Colon-Infiltrating malignant neoplasm-Specimen size, largest dimension</skos:definition>
        <skos:prefLabel xml:lang="en">Specimen size, largest dimension</skos:prefLabel>
    </owl:Class>
    


    <!-- http://www.semanticweb.org/david/ontologies/2013/0/1.3.6.1.4.1.19376.1.8.2.1.1597 -->

    <owl:Class rdf:about="&pathLex;1597">
        <rdfs:subClassOf rdf:resource="&pathLex;99999"/>
        <skos:definition xml:lang="en">Generic-Infiltrating malignant neoplasm-TNM Descriptors -Multiple primary tumors</skos:definition>
        <skos:prefLabel xml:lang="en">Multiple primary tumors</skos:prefLabel>
    </owl:Class>
    


    <!-- http://www.semanticweb.org/david/ontologies/2013/0/1.3.6.1.4.1.19376.1.8.2.1.1598 -->

    <owl:Class rdf:about="&pathLex;1598">
        <rdfs:subClassOf rdf:resource="&pathLex;99999"/>
        <skos:definition xml:lang="en">Generic-Infiltrating malignant neoplasm-TNM Descriptors -Recurrent</skos:definition>
        <skos:prefLabel xml:lang="en">Recurrent</skos:prefLabel>
    </owl:Class>
    


    <!-- http://www.semanticweb.org/david/ontologies/2013/0/1.3.6.1.4.1.19376.1.8.2.1.1599 -->

    <owl:Class rdf:about="&pathLex;1599">
        <rdfs:subClassOf rdf:resource="&pathLex;99999"/>
        <skos:definition xml:lang="en">Generic-Infiltrating malignant neoplasm-TNM Descriptors -Post-treatment</skos:definition>
        <skos:prefLabel xml:lang="en">Post-treatment</skos:prefLabel>
    </owl:Class>
    


    <!-- http://www.semanticweb.org/david/ontologies/2013/0/1.3.6.1.4.1.19376.1.8.2.1.16 -->

    <owl:Class rdf:about="&pathLex;16">
        <rdfs:subClassOf rdf:resource="&pathLex;99999"/>
        <skos:prefLabel xml:lang="en">Lesion size, largest dimension</skos:prefLabel>
        <skos:definition xml:lang="en">Skin (melanoma)-Infiltrating malignant neoplasm-Lesion size, largest dimension</skos:definition>
    </owl:Class>
    


    <!-- http://www.semanticweb.org/david/ontologies/2013/0/1.3.6.1.4.1.19376.1.8.2.1.160 -->

    <owl:Class rdf:about="&pathLex;160">
        <rdfs:subClassOf rdf:resource="&pathLex;99999"/>
        <skos:definition xml:lang="en">Colon-Infiltrating malignant neoplasm-Histologic type</skos:definition>
        <skos:prefLabel xml:lang="en">Histologic type</skos:prefLabel>
    </owl:Class>
    


    <!-- http://www.semanticweb.org/david/ontologies/2013/0/1.3.6.1.4.1.19376.1.8.2.1.1602 -->

    <owl:Class rdf:about="&pathLex;1602">
        <rdfs:subClassOf rdf:resource="&pathLex;432"/>
        <skos:definition xml:lang="en">Breast-Infiltrating malignant neoplasm-Estrogen receptor-No immunoreactive tumor cells present</skos:definition>
        <skos:prefLabel xml:lang="en">No immunoreactive tumor cells present</skos:prefLabel>
    </owl:Class>
    


    <!-- http://www.semanticweb.org/david/ontologies/2013/0/1.3.6.1.4.1.19376.1.8.2.1.161 -->

    <owl:Class rdf:about="&pathLex;161">
        <rdfs:subClassOf rdf:resource="&pathLex;99999"/>
        <skos:definition xml:lang="en">Endometrium-Infiltrating malignant neoplasm-Margins involvement</skos:definition>
        <skos:prefLabel xml:lang="en">Margins involvement</skos:prefLabel>
    </owl:Class>
    


    <!-- http://www.semanticweb.org/david/ontologies/2013/0/1.3.6.1.4.1.19376.1.8.2.1.1619 -->

    <owl:Class rdf:about="&pathLex;1619">
        <rdfs:subClassOf rdf:resource="&pathLex;99999"/>
        <skos:definition xml:lang="en">Pharynx-Infiltrating malignant neoplasm-pN hypopharynx carcinoma-pN0: No regional lymph node metastasis</skos:definition>
        <skos:prefLabel xml:lang="en">pN0: No regional lymph node metastasis</skos:prefLabel>
    </owl:Class>
    


    <!-- http://www.semanticweb.org/david/ontologies/2013/0/1.3.6.1.4.1.19376.1.8.2.1.162 -->

    <owl:Class rdf:about="&pathLex;162">
        <rdfs:subClassOf rdf:resource="&pathLex;99999"/>
        <skos:prefLabel xml:lang="en">Distance of lesion from closest uninvolved margin</skos:prefLabel>
        <skos:definition xml:lang="en">Endometrium-Infiltrating malignant neoplasm-Distance of lesion from closest uninvolved margin</skos:definition>
    </owl:Class>
    


    <!-- http://www.semanticweb.org/david/ontologies/2013/0/1.3.6.1.4.1.19376.1.8.2.1.1620 -->

    <owl:Class rdf:about="&pathLex;1620">
        <rdfs:subClassOf rdf:resource="&pathLex;99999"/>
        <skos:definition xml:lang="en">Pharynx-Infiltrating malignant neoplasm-pN hypopharynx carcinoma-pN1: Metastasis in a single ipsilateral lymph node, 3 cm or less in greatest dimension</skos:definition>
        <skos:prefLabel xml:lang="en">pN1: Metastasis in a single ipsilateral lymph node, 3 cm or less in greatest dimension</skos:prefLabel>
    </owl:Class>
    


    <!-- http://www.semanticweb.org/david/ontologies/2013/0/1.3.6.1.4.1.19376.1.8.2.1.1621 -->

    <owl:Class rdf:about="&pathLex;1621">
        <rdfs:subClassOf rdf:resource="&pathLex;99999"/>
        <skos:definition xml:lang="en">Pharynx-Infiltrating malignant neoplasm-pN hypopharynx carcinoma-pN2: Metastasis in a single ipsilateral lymph node, more than 3 cm but not more than 6 cm in greatest dimension, or in multiple ipsilateral lymph nodes, none more than 6 cm in greatest dimension, or in bilateral or contralateral lymph nodes, none more than 6 cm in greatest dimension</skos:definition>
        <skos:prefLabel xml:lang="en">pN2: Metastasis in a single ipsilateral lymph node, more than 3 cm but not more than 6 cm in greatest dimension, or in multiple ipsilateral lymph nodes, none more than 6 cm in greatest dimension, or in bilateral or contralateral lymph nodes, none more than 6 cm in greatest dimension</skos:prefLabel>
    </owl:Class>
    


    <!-- http://www.semanticweb.org/david/ontologies/2013/0/1.3.6.1.4.1.19376.1.8.2.1.1622 -->

    <owl:Class rdf:about="&pathLex;1622">
        <rdfs:subClassOf rdf:resource="&pathLex;99999"/>
        <skos:definition xml:lang="en">Pharynx-Infiltrating malignant neoplasm-pN hypopharynx carcinoma-pN2a: Metastasis in a single ipsilateral lymph node, more than 3 cm but not more than 6 cm in greatest dimension</skos:definition>
        <skos:prefLabel xml:lang="en">pN2a: Metastasis in a single ipsilateral lymph node, more than 3 cm but not more than 6 cm in greatest dimension</skos:prefLabel>
    </owl:Class>
    


    <!-- http://www.semanticweb.org/david/ontologies/2013/0/1.3.6.1.4.1.19376.1.8.2.1.1623 -->

    <owl:Class rdf:about="&pathLex;1623">
        <rdfs:subClassOf rdf:resource="&pathLex;99999"/>
        <skos:definition xml:lang="en">Pharynx-Infiltrating malignant neoplasm-pN hypopharynx carcinoma-pN2b: Metastasis in multiple ipsilateral lymph nodes, none more than 6 cm in greatest dimension</skos:definition>
        <skos:prefLabel xml:lang="en">pN2b: Metastasis in multiple ipsilateral lymph nodes, none more than 6 cm in greatest dimension</skos:prefLabel>
    </owl:Class>
    


    <!-- http://www.semanticweb.org/david/ontologies/2013/0/1.3.6.1.4.1.19376.1.8.2.1.1624 -->

    <owl:Class rdf:about="&pathLex;1624">
        <rdfs:subClassOf rdf:resource="&pathLex;99999"/>
        <skos:definition xml:lang="en">Pharynx-Infiltrating malignant neoplasm-pN hypopharynx carcinoma-pN2c: Metastasis in bilateral or contralateral lymph nodes, none more than 6 cm in greatest dimension</skos:definition>
        <skos:prefLabel xml:lang="en">pN2c: Metastasis in bilateral or contralateral lymph nodes, none more than 6 cm in greatest dimension</skos:prefLabel>
    </owl:Class>
    


    <!-- http://www.semanticweb.org/david/ontologies/2013/0/1.3.6.1.4.1.19376.1.8.2.1.1625 -->

    <owl:Class rdf:about="&pathLex;1625">
        <rdfs:subClassOf rdf:resource="&pathLex;99999"/>
        <skos:definition xml:lang="en">Pharynx-Infiltrating malignant neoplasm-pN hypopharynx carcinoma-pN3: Metastasis in a lymph node more than 6 cm in greatest dimension</skos:definition>
        <skos:prefLabel xml:lang="en">pN3: Metastasis in a lymph node more than 6 cm in greatest dimension</skos:prefLabel>
    </owl:Class>
    


    <!-- http://www.semanticweb.org/david/ontologies/2013/0/1.3.6.1.4.1.19376.1.8.2.1.1626 -->

    <owl:Class rdf:about="&pathLex;1626">
        <rdfs:subClassOf rdf:resource="&pathLex;99999"/>
        <skos:definition xml:lang="en">Pharynx-Infiltrating malignant neoplasm-pN nasopharynx carcinoma-pN0: No regional lymph node metastasis</skos:definition>
        <skos:prefLabel xml:lang="en">pN0: No regional lymph node metastasis</skos:prefLabel>
    </owl:Class>
    


    <!-- http://www.semanticweb.org/david/ontologies/2013/0/1.3.6.1.4.1.19376.1.8.2.1.1627 -->

    <owl:Class rdf:about="&pathLex;1627">
        <rdfs:subClassOf rdf:resource="&pathLex;99999"/>
        <skos:definition xml:lang="en">Pharynx-Infiltrating malignant neoplasm-pN nasopharynx carcinoma-pN1: Unilateral metastasis in lymph node(s), 6 cm or less in greatest dimension, above the supraclavicular fossa</skos:definition>
        <skos:prefLabel xml:lang="en">pN1: Unilateral metastasis in lymph node(s), 6 cm or less in greatest dimension, above the supraclavicular fossa</skos:prefLabel>
    </owl:Class>
    


    <!-- http://www.semanticweb.org/david/ontologies/2013/0/1.3.6.1.4.1.19376.1.8.2.1.1628 -->

    <owl:Class rdf:about="&pathLex;1628">
        <rdfs:subClassOf rdf:resource="&pathLex;99999"/>
        <skos:definition xml:lang="en">Pharynx-Infiltrating malignant neoplasm-pN nasopharynx carcinoma-pN2: Bilateral metastasis in lymph node(s), 6 cm or less in greatest dimension, above the supraclavicular fossa</skos:definition>
        <skos:prefLabel xml:lang="en">pN2: Bilateral metastasis in lymph node(s), 6 cm or less in greatest dimension, above the supraclavicular fossa</skos:prefLabel>
    </owl:Class>
    


    <!-- http://www.semanticweb.org/david/ontologies/2013/0/1.3.6.1.4.1.19376.1.8.2.1.1629 -->

    <owl:Class rdf:about="&pathLex;1629">
        <rdfs:subClassOf rdf:resource="&pathLex;99999"/>
        <skos:definition xml:lang="en">Pharynx-Infiltrating malignant neoplasm-pN nasopharynx carcinoma-pN3: Metastasis in a lymph node greater than 6 cm and/or to supraclavicular fossa</skos:definition>
        <skos:prefLabel xml:lang="en">pN3: Metastasis in a lymph node greater than 6 cm and/or to supraclavicular fossa</skos:prefLabel>
    </owl:Class>
    


    <!-- http://www.semanticweb.org/david/ontologies/2013/0/1.3.6.1.4.1.19376.1.8.2.1.163 -->

    <owl:Class rdf:about="&pathLex;163">
        <rdfs:subClassOf rdf:resource="&pathLex;99999"/>
        <skos:definition xml:lang="en">Endometrium-Infiltrating malignant neoplasm-Lymph-vascular invasion</skos:definition>
        <skos:prefLabel xml:lang="en">Lymph-vascular invasion</skos:prefLabel>
    </owl:Class>
    


    <!-- http://www.semanticweb.org/david/ontologies/2013/0/1.3.6.1.4.1.19376.1.8.2.1.1630 -->

    <owl:Class rdf:about="&pathLex;1630">
        <rdfs:subClassOf rdf:resource="&pathLex;99999"/>
        <skos:definition xml:lang="en">Pharynx-Infiltrating malignant neoplasm-pN nasopharynx carcinoma-pN3a: Greater than 6 cm in dimension</skos:definition>
        <skos:prefLabel xml:lang="en">pN3a: Greater than 6 cm in dimension</skos:prefLabel>
    </owl:Class>
    


    <!-- http://www.semanticweb.org/david/ontologies/2013/0/1.3.6.1.4.1.19376.1.8.2.1.1631 -->

    <owl:Class rdf:about="&pathLex;1631">
        <rdfs:subClassOf rdf:resource="&pathLex;99999"/>
        <skos:definition xml:lang="en">Pharynx-Infiltrating malignant neoplasm-pN nasopharynx carcinoma-pN3b: Extension to the supraclavicular fossa</skos:definition>
        <skos:prefLabel xml:lang="en">pN3b: Extension to the supraclavicular fossa</skos:prefLabel>
    </owl:Class>
    


    <!-- http://www.semanticweb.org/david/ontologies/2013/0/1.3.6.1.4.1.19376.1.8.2.1.1632 -->

    <owl:Class rdf:about="&pathLex;1632">
        <rdfs:subClassOf rdf:resource="&pathLex;99999"/>
        <skos:definition xml:lang="en">Pharynx-Infiltrating malignant neoplasm-pN mucosal malignant melanoma-pN0: No regional lymph node metastases</skos:definition>
        <skos:prefLabel xml:lang="en">pN0: No regional lymph node metastases</skos:prefLabel>
    </owl:Class>
    


    <!-- http://www.semanticweb.org/david/ontologies/2013/0/1.3.6.1.4.1.19376.1.8.2.1.1633 -->

    <owl:Class rdf:about="&pathLex;1633">
        <rdfs:subClassOf rdf:resource="&pathLex;99999"/>
        <skos:definition xml:lang="en">Pharynx-Infiltrating malignant neoplasm-pN mucosal malignant melanoma-pN1: Regional lymph node metastases present</skos:definition>
        <skos:prefLabel xml:lang="en">pN1: Regional lymph node metastases present</skos:prefLabel>
    </owl:Class>
    


    <!-- http://www.semanticweb.org/david/ontologies/2013/0/1.3.6.1.4.1.19376.1.8.2.1.1634 -->

    <owl:Class rdf:about="&pathLex;1634">
        <rdfs:subClassOf rdf:resource="&pathLex;99999"/>
        <skos:definition xml:lang="en">Pharynx-Infiltrating malignant neoplasm-pT hypopharynx carcinoma-pT0: No evidence of primary tumor</skos:definition>
        <skos:prefLabel xml:lang="en">pT0: No evidence of primary tumor</skos:prefLabel>
    </owl:Class>
    


    <!-- http://www.semanticweb.org/david/ontologies/2013/0/1.3.6.1.4.1.19376.1.8.2.1.1635 -->

    <owl:Class rdf:about="&pathLex;1635">
        <rdfs:subClassOf rdf:resource="&pathLex;99999"/>
        <skos:definition xml:lang="en">Pharynx-Infiltrating malignant neoplasm-pT hypopharynx carcinoma-pTis: Carcinoma in situ</skos:definition>
        <skos:prefLabel xml:lang="en">pTis: Carcinoma in situ</skos:prefLabel>
    </owl:Class>
    


    <!-- http://www.semanticweb.org/david/ontologies/2013/0/1.3.6.1.4.1.19376.1.8.2.1.1636 -->

    <owl:Class rdf:about="&pathLex;1636">
        <rdfs:subClassOf rdf:resource="&pathLex;99999"/>
        <skos:definition xml:lang="en">Pharynx-Infiltrating malignant neoplasm-pT hypopharynx carcinoma-pT1: Tumor limited to one subsite of hypopharynx and/or 2 cm or less in greatest dimension</skos:definition>
        <skos:prefLabel xml:lang="en">pT1: Tumor limited to one subsite of hypopharynx and/or 2 cm or less in greatest dimension</skos:prefLabel>
    </owl:Class>
    


    <!-- http://www.semanticweb.org/david/ontologies/2013/0/1.3.6.1.4.1.19376.1.8.2.1.1637 -->

    <owl:Class rdf:about="&pathLex;1637">
        <rdfs:subClassOf rdf:resource="&pathLex;99999"/>
        <skos:definition xml:lang="en">Pharynx-Infiltrating malignant neoplasm-pT hypopharynx carcinoma-pT2: Tumor invades more than one subsite of hypopharynx or an adjacent site, or measures more than 2 cm but not more than 4 cm in greatest dimension without fixation of hemilarynx</skos:definition>
        <skos:prefLabel xml:lang="en">pT2: Tumor invades more than one subsite of hypopharynx or an adjacent site, or measures more than 2 cm but not more than 4 cm in greatest dimension without fixation of hemilarynx</skos:prefLabel>
    </owl:Class>
    


    <!-- http://www.semanticweb.org/david/ontologies/2013/0/1.3.6.1.4.1.19376.1.8.2.1.1638 -->

    <owl:Class rdf:about="&pathLex;1638">
        <rdfs:subClassOf rdf:resource="&pathLex;99999"/>
        <skos:definition xml:lang="en">Pharynx-Infiltrating malignant neoplasm-pT hypopharynx carcinoma-pT3: Tumor measures more than 4 cm in greatest dimension or with fixation of hemilarynx or extension to esophagus</skos:definition>
        <skos:prefLabel xml:lang="en">pT3: Tumor measures more than 4 cm in greatest dimension or with fixation of hemilarynx or extension to esophagus</skos:prefLabel>
    </owl:Class>
    


    <!-- http://www.semanticweb.org/david/ontologies/2013/0/1.3.6.1.4.1.19376.1.8.2.1.1639 -->

    <owl:Class rdf:about="&pathLex;1639">
        <rdfs:subClassOf rdf:resource="&pathLex;99999"/>
        <skos:definition xml:lang="en">Pharynx-Infiltrating malignant neoplasm-pT hypopharynx carcinoma-pT4a: Moderately advanced local disease. Tumor invades thyroid/cricoid cartilage, hyoid bone, thyroid gland, or central compartment soft tissue#</skos:definition>
        <skos:prefLabel xml:lang="en">pT4a: Moderately advanced local disease. Tumor invades thyroid/cricoid cartilage, hyoid bone, thyroid gland, or central compartment soft tissue#</skos:prefLabel>
    </owl:Class>
    


    <!-- http://www.semanticweb.org/david/ontologies/2013/0/1.3.6.1.4.1.19376.1.8.2.1.164 -->

    <owl:Class rdf:about="&pathLex;164">
        <rdfs:subClassOf rdf:resource="&pathLex;99999"/>
        <skos:definition xml:lang="en">Endometrium-Infiltrating malignant neoplasm-Lymph node sampling</skos:definition>
        <skos:prefLabel xml:lang="en">Lymph node sampling</skos:prefLabel>
    </owl:Class>
    


    <!-- http://www.semanticweb.org/david/ontologies/2013/0/1.3.6.1.4.1.19376.1.8.2.1.1640 -->

    <owl:Class rdf:about="&pathLex;1640">
        <rdfs:subClassOf rdf:resource="&pathLex;99999"/>
        <skos:definition xml:lang="en">Pharynx-Infiltrating malignant neoplasm-pT hypopharynx carcinoma-pT4b: Very advanced local disease. Tumor invades prevertebral</skos:definition>
        <skos:prefLabel xml:lang="en">pT4b: Very advanced local disease. Tumor invades prevertebral</skos:prefLabel>
    </owl:Class>
    


    <!-- http://www.semanticweb.org/david/ontologies/2013/0/1.3.6.1.4.1.19376.1.8.2.1.1641 -->

    <owl:Class rdf:about="&pathLex;1641">
        <rdfs:subClassOf rdf:resource="&pathLex;99999"/>
        <skos:definition xml:lang="en">Pharynx-Infiltrating malignant neoplasm-pT mucosal malignant melanoma-pT3: Mucosal disease</skos:definition>
        <skos:prefLabel xml:lang="en">pT3: Mucosal disease</skos:prefLabel>
    </owl:Class>
    


    <!-- http://www.semanticweb.org/david/ontologies/2013/0/1.3.6.1.4.1.19376.1.8.2.1.1642 -->

    <owl:Class rdf:about="&pathLex;1642">
        <rdfs:subClassOf rdf:resource="&pathLex;99999"/>
        <skos:definition xml:lang="en">Pharynx-Infiltrating malignant neoplasm-pT mucosal malignant melanoma-pT4a: Moderately advanced disease. Tumor involving deep soft tissue, cartilage,bone, or overlying skin.</skos:definition>
        <skos:prefLabel xml:lang="en">pT4a: Moderately advanced disease. Tumor involving deep soft tissue, cartilage,bone, or overlying skin.</skos:prefLabel>
    </owl:Class>
    


    <!-- http://www.semanticweb.org/david/ontologies/2013/0/1.3.6.1.4.1.19376.1.8.2.1.1643 -->

    <owl:Class rdf:about="&pathLex;1643">
        <rdfs:subClassOf rdf:resource="&pathLex;99999"/>
        <skos:definition xml:lang="en">Pharynx-Infiltrating malignant neoplasm-pT mucosal malignant melanoma-pT4b: Very advanced disease. Tumor involving brain, dura, skull base, lower cranial nerves (IX, X, XI, XII), masticator space, carotid artery, prevertebral space, or mediastinal structures.</skos:definition>
        <skos:prefLabel xml:lang="en">pT4b: Very advanced disease. Tumor involving brain, dura, skull base, lower cranial nerves (IX, X, XI, XII), masticator space, carotid artery, prevertebral space, or mediastinal structures.</skos:prefLabel>
    </owl:Class>
    


    <!-- http://www.semanticweb.org/david/ontologies/2013/0/1.3.6.1.4.1.19376.1.8.2.1.1644 -->

    <owl:Class rdf:about="&pathLex;1644">
        <rdfs:subClassOf rdf:resource="&pathLex;99999"/>
        <skos:definition xml:lang="en">Pharynx-Infiltrating malignant neoplasm-pT nasopharynx carcinoma-pT0: No evidence of primary tumor</skos:definition>
        <skos:prefLabel xml:lang="en">pT0: No evidence of primary tumor</skos:prefLabel>
    </owl:Class>
    


    <!-- http://www.semanticweb.org/david/ontologies/2013/0/1.3.6.1.4.1.19376.1.8.2.1.1645 -->

    <owl:Class rdf:about="&pathLex;1645">
        <rdfs:subClassOf rdf:resource="&pathLex;99999"/>
        <skos:definition xml:lang="en">Pharynx-Infiltrating malignant neoplasm-pT nasopharynx carcinoma-pTis: Carcinoma in situ</skos:definition>
        <skos:prefLabel xml:lang="en">pTis: Carcinoma in situ</skos:prefLabel>
    </owl:Class>
    


    <!-- http://www.semanticweb.org/david/ontologies/2013/0/1.3.6.1.4.1.19376.1.8.2.1.1646 -->

    <owl:Class rdf:about="&pathLex;1646">
        <rdfs:subClassOf rdf:resource="&pathLex;99999"/>
        <skos:definition xml:lang="en">Pharynx-Infiltrating malignant neoplasm-pT nasopharynx carcinoma-pT1: Tumor confined to nasopharynx, or tumor extends to oropharynx and/or nasal cavity without parapharyngeal extension#</skos:definition>
        <skos:prefLabel xml:lang="en">pT1: Tumor confined to nasopharynx, or tumor extends to oropharynx and/or nasal cavity without parapharyngeal extension#</skos:prefLabel>
    </owl:Class>
    


    <!-- http://www.semanticweb.org/david/ontologies/2013/0/1.3.6.1.4.1.19376.1.8.2.1.1647 -->

    <owl:Class rdf:about="&pathLex;1647">
        <rdfs:subClassOf rdf:resource="&pathLex;99999"/>
        <skos:definition xml:lang="en">Pharynx-Infiltrating malignant neoplasm-pT nasopharynx carcinoma-pT2: Tumor with parapharyngeal extension</skos:definition>
        <skos:prefLabel xml:lang="en">pT2: Tumor with parapharyngeal extension</skos:prefLabel>
    </owl:Class>
    


    <!-- http://www.semanticweb.org/david/ontologies/2013/0/1.3.6.1.4.1.19376.1.8.2.1.1648 -->

    <owl:Class rdf:about="&pathLex;1648">
        <rdfs:subClassOf rdf:resource="&pathLex;99999"/>
        <skos:definition xml:lang="en">Pharynx-Infiltrating malignant neoplasm-pT nasopharynx carcinoma-pT3: Tumor invades bony structures of skull base and/or paranasal sinuses</skos:definition>
        <skos:prefLabel xml:lang="en">pT3: Tumor invades bony structures of skull base and/or paranasal sinuses</skos:prefLabel>
    </owl:Class>
    


    <!-- http://www.semanticweb.org/david/ontologies/2013/0/1.3.6.1.4.1.19376.1.8.2.1.1649 -->

    <owl:Class rdf:about="&pathLex;1649">
        <rdfs:subClassOf rdf:resource="&pathLex;99999"/>
        <skos:definition xml:lang="en">Pharynx-Infiltrating malignant neoplasm-pT nasopharynx carcinoma-pT4: Tumor with intracranial extension and/or involvement of cranial nerves, hypopharynx, orbit, or with extension to the infratemporal fossa/masticator space</skos:definition>
        <skos:prefLabel xml:lang="en">pT4: Tumor with intracranial extension and/or involvement of cranial nerves, hypopharynx, orbit, or with extension to the infratemporal fossa/masticator space</skos:prefLabel>
    </owl:Class>
    


    <!-- http://www.semanticweb.org/david/ontologies/2013/0/1.3.6.1.4.1.19376.1.8.2.1.165 -->

    <owl:Class rdf:about="&pathLex;165">
        <rdfs:subClassOf rdf:resource="&pathLex;99999"/>
        <skos:definition xml:lang="en">Endometrium-Infiltrating malignant neoplasm-Extent</skos:definition>
        <skos:prefLabel xml:lang="en">Extent</skos:prefLabel>
    </owl:Class>
    


    <!-- http://www.semanticweb.org/david/ontologies/2013/0/1.3.6.1.4.1.19376.1.8.2.1.1650 -->

    <owl:Class rdf:about="&pathLex;1650">
        <rdfs:subClassOf rdf:resource="&pathLex;99999"/>
        <skos:prefLabel xml:lang="en">Epiglottis</skos:prefLabel>
        <skos:definition xml:lang="en">Larynx-Infiltrating malignant neoplasm-Lesion site-Epiglottis</skos:definition>
    </owl:Class>
    


    <!-- http://www.semanticweb.org/david/ontologies/2013/0/1.3.6.1.4.1.19376.1.8.2.1.1651 -->

    <owl:Class rdf:about="&pathLex;1651">
        <rdfs:subClassOf rdf:resource="&pathLex;99999"/>
        <skos:prefLabel xml:lang="en">Aryepiglottic folds</skos:prefLabel>
        <skos:definition xml:lang="en">Larynx-Infiltrating malignant neoplasm-Lesion site-Aryepiglottic folds</skos:definition>
    </owl:Class>
    


    <!-- http://www.semanticweb.org/david/ontologies/2013/0/1.3.6.1.4.1.19376.1.8.2.1.1652 -->

    <owl:Class rdf:about="&pathLex;1652">
        <rdfs:subClassOf rdf:resource="&pathLex;99999"/>
        <skos:prefLabel xml:lang="en">Arytenoid(s)</skos:prefLabel>
        <skos:definition xml:lang="en">Larynx-Infiltrating malignant neoplasm-Lesion site-Arytenoid(s)</skos:definition>
    </owl:Class>
    


    <!-- http://www.semanticweb.org/david/ontologies/2013/0/1.3.6.1.4.1.19376.1.8.2.1.1653 -->

    <owl:Class rdf:about="&pathLex;1653">
        <rdfs:subClassOf rdf:resource="&pathLex;99999"/>
        <skos:prefLabel xml:lang="en">False vocal cord</skos:prefLabel>
        <skos:definition xml:lang="en">Larynx-Infiltrating malignant neoplasm-Lesion site-False vocal cord</skos:definition>
    </owl:Class>
    


    <!-- http://www.semanticweb.org/david/ontologies/2013/0/1.3.6.1.4.1.19376.1.8.2.1.1654 -->

    <owl:Class rdf:about="&pathLex;1654">
        <rdfs:subClassOf rdf:resource="&pathLex;99999"/>
        <skos:definition xml:lang="en">Larynx-Infiltrating malignant neoplasm-Lesion site-Ventricle</skos:definition>
        <skos:prefLabel xml:lang="en">Ventricle</skos:prefLabel>
    </owl:Class>
    


    <!-- http://www.semanticweb.org/david/ontologies/2013/0/1.3.6.1.4.1.19376.1.8.2.1.1655 -->

    <owl:Class rdf:about="&pathLex;1655">
        <rdfs:subClassOf rdf:resource="&pathLex;99999"/>
        <skos:definition xml:lang="en">Larynx-Infiltrating malignant neoplasm-Lesion site-True vocal cord</skos:definition>
        <skos:prefLabel xml:lang="en">True vocal cord</skos:prefLabel>
    </owl:Class>
    


    <!-- http://www.semanticweb.org/david/ontologies/2013/0/1.3.6.1.4.1.19376.1.8.2.1.1656 -->

    <owl:Class rdf:about="&pathLex;1656">
        <rdfs:subClassOf rdf:resource="&pathLex;99999"/>
        <skos:definition xml:lang="en">Larynx-Infiltrating malignant neoplasm-Lesion site-Posterior commissure</skos:definition>
        <skos:prefLabel xml:lang="en">Posterior commissure</skos:prefLabel>
    </owl:Class>
    


    <!-- http://www.semanticweb.org/david/ontologies/2013/0/1.3.6.1.4.1.19376.1.8.2.1.1657 -->

    <owl:Class rdf:about="&pathLex;1657">
        <rdfs:subClassOf rdf:resource="&pathLex;99999"/>
        <skos:prefLabel xml:lang="en">Anterior commissure</skos:prefLabel>
        <skos:definition xml:lang="en">Larynx-Infiltrating malignant neoplasm-Lesion site-Anterior commissure</skos:definition>
    </owl:Class>
    


    <!-- http://www.semanticweb.org/david/ontologies/2013/0/1.3.6.1.4.1.19376.1.8.2.1.1658 -->

    <owl:Class rdf:about="&pathLex;1658">
        <rdfs:subClassOf rdf:resource="&pathLex;99999"/>
        <skos:prefLabel xml:lang="en">Larynx, subglottis</skos:prefLabel>
        <skos:definition xml:lang="en">Larynx-Infiltrating malignant neoplasm-Lesion site-Larynx, subglottis</skos:definition>
    </owl:Class>
    


    <!-- http://www.semanticweb.org/david/ontologies/2013/0/1.3.6.1.4.1.19376.1.8.2.1.166 -->

    <owl:Class rdf:about="&pathLex;166">
        <rdfs:subClassOf rdf:resource="&pathLex;99999"/>
        <skos:definition xml:lang="en">Endometrium-Infiltrating malignant neoplasm-Histologic grade (FIGO)</skos:definition>
        <skos:prefLabel xml:lang="en">Histologic grade (FIGO)</skos:prefLabel>
    </owl:Class>
    


    <!-- http://www.semanticweb.org/david/ontologies/2013/0/1.3.6.1.4.1.19376.1.8.2.1.167 -->

    <owl:Class rdf:about="&pathLex;167">
        <rdfs:subClassOf rdf:resource="&pathLex;99999"/>
        <skos:definition xml:lang="en">Endometrium-Infiltrating malignant neoplasm-Lesion site</skos:definition>
        <skos:prefLabel xml:lang="en">Lesion site</skos:prefLabel>
    </owl:Class>
    


    <!-- http://www.semanticweb.org/david/ontologies/2013/0/1.3.6.1.4.1.19376.1.8.2.1.168 -->

    <owl:Class rdf:about="&pathLex;168">
        <rdfs:subClassOf rdf:resource="&pathLex;99999"/>
        <skos:definition xml:lang="en">Endometrium-Infiltrating malignant neoplasm-Lymph node site</skos:definition>
        <skos:prefLabel xml:lang="en">Lymph node site</skos:prefLabel>
    </owl:Class>
    


    <!-- http://www.semanticweb.org/david/ontologies/2013/0/1.3.6.1.4.1.19376.1.8.2.1.169 -->

    <owl:Class rdf:about="&pathLex;169">
        <rdfs:subClassOf rdf:resource="&pathLex;99999"/>
        <skos:definition xml:lang="en">Endometrium-Infiltrating malignant neoplasm-Number of lymph nodes involved</skos:definition>
        <skos:prefLabel xml:lang="en">Number of lymph nodes involved</skos:prefLabel>
    </owl:Class>
    


    <!-- http://www.semanticweb.org/david/ontologies/2013/0/1.3.6.1.4.1.19376.1.8.2.1.17 -->

    <owl:Class rdf:about="&pathLex;17">
        <rdfs:subClassOf rdf:resource="&pathLex;21"/>
        <skos:definition xml:lang="en">Breast-Infiltrating malignant neoplasm-Extensive intraductal component </skos:definition>
        <skos:prefLabel xml:lang="en">Extensive intraductal component </skos:prefLabel>
    </owl:Class>
    


    <!-- http://www.semanticweb.org/david/ontologies/2013/0/1.3.6.1.4.1.19376.1.8.2.1.170 -->

    <owl:Class rdf:about="&pathLex;170">
        <rdfs:subClassOf rdf:resource="&pathLex;99999"/>
        <skos:definition xml:lang="en">Endometrium-Infiltrating malignant neoplasm-Number of lymph nodes examined</skos:definition>
        <skos:prefLabel xml:lang="en">Number of lymph nodes examined</skos:prefLabel>
    </owl:Class>
    


    <!-- http://www.semanticweb.org/david/ontologies/2013/0/1.3.6.1.4.1.19376.1.8.2.1.172 -->

    <owl:Class rdf:about="&pathLex;172">
        <rdfs:subClassOf rdf:resource="&pathLex;99999"/>
        <skos:definition xml:lang="en">Endometrium-Infiltrating malignant neoplasm-pN</skos:definition>
        <skos:prefLabel xml:lang="en">pN</skos:prefLabel>
    </owl:Class>
    


    <!-- http://www.semanticweb.org/david/ontologies/2013/0/1.3.6.1.4.1.19376.1.8.2.1.174 -->

    <owl:Class rdf:about="&pathLex;174">
        <rdfs:subClassOf rdf:resource="&pathLex;99999"/>
        <skos:definition xml:lang="en">Endometrium-Infiltrating malignant neoplasm-pT</skos:definition>
        <skos:prefLabel xml:lang="en">pT</skos:prefLabel>
    </owl:Class>
    


    <!-- http://www.semanticweb.org/david/ontologies/2013/0/1.3.6.1.4.1.19376.1.8.2.1.175 -->

    <owl:Class rdf:about="&pathLex;175">
        <rdfs:subClassOf rdf:resource="&pathLex;99999"/>
        <skos:definition xml:lang="en">Endometrium-Infiltrating malignant neoplasm-Lesion size, largest dimension</skos:definition>
        <skos:prefLabel xml:lang="en">Lesion size, largest dimension</skos:prefLabel>
    </owl:Class>
    


    <!-- http://www.semanticweb.org/david/ontologies/2013/0/1.3.6.1.4.1.19376.1.8.2.1.176 -->

    <owl:Class rdf:about="&pathLex;176">
        <rdfs:subClassOf rdf:resource="&pathLex;99999"/>
        <skos:definition xml:lang="en">Endometrium-Infiltrating malignant neoplasm-Histologic type</skos:definition>
        <skos:prefLabel xml:lang="en">Histologic type</skos:prefLabel>
    </owl:Class>
    


    <!-- http://www.semanticweb.org/david/ontologies/2013/0/1.3.6.1.4.1.19376.1.8.2.1.1765 -->

    <owl:Class rdf:about="&pathLex;1765">
        <rdfs:subClassOf rdf:resource="&pathLex;99999"/>
        <skos:prefLabel xml:lang="en">Basaloid squamous cell carcinoma</skos:prefLabel>
        <skos:definition xml:lang="en">Larynx-Infiltrating malignant neoplasm-Histologic type-Basaloid squamous cell carcinoma</skos:definition>
    </owl:Class>
    


    <!-- http://www.semanticweb.org/david/ontologies/2013/0/1.3.6.1.4.1.19376.1.8.2.1.1767 -->

    <owl:Class rdf:about="&pathLex;1767">
        <rdfs:subClassOf rdf:resource="&pathLex;99999"/>
        <skos:definition xml:lang="en">Larynx-Infiltrating malignant neoplasm-Histologic type-Spindle cell squamous cell carcinoma</skos:definition>
        <skos:prefLabel xml:lang="en">Spindle cell squamous cell carcinoma</skos:prefLabel>
    </owl:Class>
    


    <!-- http://www.semanticweb.org/david/ontologies/2013/0/1.3.6.1.4.1.19376.1.8.2.1.177 -->

    <owl:Class rdf:about="&pathLex;177">
        <rdfs:subClassOf rdf:resource="&pathLex;99999"/>
        <skos:prefLabel xml:lang="en">Margins involvement</skos:prefLabel>
        <skos:definition xml:lang="en">Stomach-Infiltrating malignant neoplasm-Margins involvement</skos:definition>
    </owl:Class>
    


    <!-- http://www.semanticweb.org/david/ontologies/2013/0/1.3.6.1.4.1.19376.1.8.2.1.178 -->

    <owl:Class rdf:about="&pathLex;178">
        <rdfs:subClassOf rdf:resource="&pathLex;99999"/>
        <skos:prefLabel xml:lang="en">Margins involvement</skos:prefLabel>
        <skos:definition xml:lang="en">Stomach-Infiltrating malignant neoplasm-Margins involvement</skos:definition>
    </owl:Class>
    


    <!-- http://www.semanticweb.org/david/ontologies/2013/0/1.3.6.1.4.1.19376.1.8.2.1.179 -->

    <owl:Class rdf:about="&pathLex;179">
        <rdfs:subClassOf rdf:resource="&pathLex;99999"/>
        <skos:prefLabel xml:lang="en">Margins involvement</skos:prefLabel>
        <skos:definition xml:lang="en">Stomach-Infiltrating malignant neoplasm-Margins involvement</skos:definition>
    </owl:Class>
    


    <!-- http://www.semanticweb.org/david/ontologies/2013/0/1.3.6.1.4.1.19376.1.8.2.1.180 -->

    <owl:Class rdf:about="&pathLex;180">
        <rdfs:subClassOf rdf:resource="&pathLex;99999"/>
        <skos:prefLabel xml:lang="en">Distance of lesion from closest uninvolved margin</skos:prefLabel>
        <skos:definition xml:lang="en">Stomach-Infiltrating malignant neoplasm-Distance of lesion from closest uninvolved margin</skos:definition>
    </owl:Class>
    


    <!-- http://www.semanticweb.org/david/ontologies/2013/0/1.3.6.1.4.1.19376.1.8.2.1.181 -->

    <owl:Class rdf:about="&pathLex;181">
        <rdfs:subClassOf rdf:resource="&pathLex;99999"/>
        <skos:prefLabel xml:lang="en">Lymph-vascular invasion</skos:prefLabel>
        <skos:definition xml:lang="en">Stomach-Infiltrating malignant neoplasm-Lymph-vascular invasion</skos:definition>
    </owl:Class>
    


    <!-- http://www.semanticweb.org/david/ontologies/2013/0/1.3.6.1.4.1.19376.1.8.2.1.1812 -->

    <owl:Class rdf:about="&pathLex;1812">
        <rdfs:subClassOf rdf:resource="&pathLex;99999"/>
        <skos:definition xml:lang="en">Lip, oral cavity-Infiltrating malignant neoplasm-pT mucosal malignant melanoma-pT3: Mucosal disease</skos:definition>
        <skos:prefLabel xml:lang="en">pT3: Mucosal disease</skos:prefLabel>
    </owl:Class>
    


    <!-- http://www.semanticweb.org/david/ontologies/2013/0/1.3.6.1.4.1.19376.1.8.2.1.1813 -->

    <owl:Class rdf:about="&pathLex;1813">
        <rdfs:subClassOf rdf:resource="&pathLex;99999"/>
        <skos:definition xml:lang="en">Lip, oral cavity-Infiltrating malignant neoplasm-pT mucosal malignant melanoma-pT4a: Moderately advanced disease. Tumor involving deep soft tissue, cartilage, or overlying skin</skos:definition>
        <skos:prefLabel xml:lang="en">pT4a: Moderately advanced disease. Tumor involving deep soft tissue, cartilage, or overlying skin</skos:prefLabel>
    </owl:Class>
    


    <!-- http://www.semanticweb.org/david/ontologies/2013/0/1.3.6.1.4.1.19376.1.8.2.1.1814 -->

    <owl:Class rdf:about="&pathLex;1814">
        <rdfs:subClassOf rdf:resource="&pathLex;99999"/>
        <skos:definition xml:lang="en">Lip, oral cavity-Infiltrating malignant neoplasm-pT mucosal malignant melanoma-pT4b: Very advanced disease. Tumor involving brain, dura, skull base, lower cranial nerves (IX, X, XI, XII), masticator space, carotid artery, prevertebral space, or mediastinal structures</skos:definition>
        <skos:prefLabel xml:lang="en">pT4b: Very advanced disease. Tumor involving brain, dura, skull base, lower cranial nerves (IX, X, XI, XII), masticator space, carotid artery, prevertebral space, or mediastinal structures</skos:prefLabel>
    </owl:Class>
    


    <!-- http://www.semanticweb.org/david/ontologies/2013/0/1.3.6.1.4.1.19376.1.8.2.1.1815 -->

    <owl:Class rdf:about="&pathLex;1815">
        <rdfs:subClassOf rdf:resource="&pathLex;99999"/>
        <skos:definition xml:lang="en">Colon-Infiltrating malignant neoplasm-Histologic grade (Two-Tier Grading System)</skos:definition>
        <skos:prefLabel xml:lang="en">Histologic grade (Two-Tier Grading System)</skos:prefLabel>
    </owl:Class>
    


    <!-- http://www.semanticweb.org/david/ontologies/2013/0/1.3.6.1.4.1.19376.1.8.2.1.1817 -->

    <owl:Class rdf:about="&pathLex;1817">
        <rdfs:subClassOf rdf:resource="&pathLex;99999"/>
        <skos:definition xml:lang="en">Colon-Infiltrating malignant neoplasm-pM</skos:definition>
        <skos:prefLabel xml:lang="en">pM</skos:prefLabel>
    </owl:Class>
    


    <!-- http://www.semanticweb.org/david/ontologies/2013/0/1.3.6.1.4.1.19376.1.8.2.1.1818 -->

    <owl:Class rdf:about="&pathLex;1818">
        <rdfs:subClassOf rdf:resource="&pathLex;99999"/>
        <skos:definition xml:lang="en">Colon-Infiltrating malignant neoplasm-Histologic Features Suggestive of Microsatellite Instability</skos:definition>
        <skos:prefLabel xml:lang="en">Histologic Features Suggestive of Microsatellite Instability</skos:prefLabel>
    </owl:Class>
    


    <!-- http://www.semanticweb.org/david/ontologies/2013/0/1.3.6.1.4.1.19376.1.8.2.1.1819 -->

    <owl:Class rdf:about="&pathLex;1819">
        <rdfs:subClassOf rdf:resource="&pathLex;99999"/>
        <skos:definition xml:lang="en">Colon-Infiltrating malignant neoplasm-Macroscopic type</skos:definition>
        <skos:prefLabel xml:lang="en">Macroscopic type</skos:prefLabel>
    </owl:Class>
    


    <!-- http://www.semanticweb.org/david/ontologies/2013/0/1.3.6.1.4.1.19376.1.8.2.1.182 -->

    <owl:Class rdf:about="&pathLex;182">
        <rdfs:subClassOf rdf:resource="&pathLex;99999"/>
        <skos:prefLabel xml:lang="en">Extent</skos:prefLabel>
        <skos:definition xml:lang="en">Stomach-Infiltrating malignant neoplasm-Extent</skos:definition>
    </owl:Class>
    


    <!-- http://www.semanticweb.org/david/ontologies/2013/0/1.3.6.1.4.1.19376.1.8.2.1.1820 -->

    <owl:Class rdf:about="&pathLex;1820">
        <rdfs:subClassOf rdf:resource="&pathLex;99999"/>
        <skos:definition xml:lang="en">Colon-Lesion-Histologic type</skos:definition>
        <skos:prefLabel xml:lang="en">Histologic type</skos:prefLabel>
    </owl:Class>
    


    <!-- http://www.semanticweb.org/david/ontologies/2013/0/1.3.6.1.4.1.19376.1.8.2.1.1821 -->

    <owl:Class rdf:about="&pathLex;1821">
        <rdfs:subClassOf rdf:resource="&pathLex;99999"/>
        <skos:definition xml:lang="en">Colon-Lesion-Macroscopic type</skos:definition>
        <skos:prefLabel xml:lang="en">Macroscopic type</skos:prefLabel>
    </owl:Class>
    


    <!-- http://www.semanticweb.org/david/ontologies/2013/0/1.3.6.1.4.1.19376.1.8.2.1.1822 -->

    <owl:Class rdf:about="&pathLex;1822">
        <rdfs:subClassOf rdf:resource="&pathLex;99999"/>
        <skos:definition xml:lang="en">Endometrium-Infiltrating malignant neoplasm-Histologic grade (WHO)</skos:definition>
        <skos:prefLabel xml:lang="en">Histologic grade (WHO)</skos:prefLabel>
    </owl:Class>
    


    <!-- http://www.semanticweb.org/david/ontologies/2013/0/1.3.6.1.4.1.19376.1.8.2.1.1824 -->

    <owl:Class rdf:about="&pathLex;1824">
        <rdfs:subClassOf rdf:resource="&pathLex;99999"/>
        <skos:definition xml:lang="en">Endometrium-Infiltrating malignant neoplasm-pM</skos:definition>
        <skos:prefLabel xml:lang="en">pM</skos:prefLabel>
    </owl:Class>
    


    <!-- http://www.semanticweb.org/david/ontologies/2013/0/1.3.6.1.4.1.19376.1.8.2.1.1825 -->

    <owl:Class rdf:about="&pathLex;1825">
        <rdfs:subClassOf rdf:resource="&pathLex;99999"/>
        <skos:definition xml:lang="en">Endometrium-Lesion-Histologic type</skos:definition>
        <skos:prefLabel xml:lang="en">Histologic type</skos:prefLabel>
    </owl:Class>
    


    <!-- http://www.semanticweb.org/david/ontologies/2013/0/1.3.6.1.4.1.19376.1.8.2.1.1826 -->

    <owl:Class rdf:about="&pathLex;1826">
        <rdfs:subClassOf rdf:resource="&pathLex;99999"/>
        <skos:definition xml:lang="en">Endometrium-Lesion-Lesion site</skos:definition>
        <skos:prefLabel xml:lang="en">Lesion site</skos:prefLabel>
    </owl:Class>
    


    <!-- http://www.semanticweb.org/david/ontologies/2013/0/1.3.6.1.4.1.19376.1.8.2.1.1828 -->

    <owl:Class rdf:about="&pathLex;1828">
        <rdfs:subClassOf rdf:resource="&pathLex;99999"/>
        <skos:definition xml:lang="en">Stomach-Infiltrating malignant neoplasm-pM</skos:definition>
        <skos:prefLabel xml:lang="en">pM</skos:prefLabel>
    </owl:Class>
    


    <!-- http://www.semanticweb.org/david/ontologies/2013/0/1.3.6.1.4.1.19376.1.8.2.1.1829 -->

    <owl:Class rdf:about="&pathLex;1829">
        <rdfs:subClassOf rdf:resource="&pathLex;99999"/>
        <skos:prefLabel xml:lang="en">Histologic type</skos:prefLabel>
        <skos:definition xml:lang="en">Stomach-Lesion-Histologic type</skos:definition>
    </owl:Class>
    


    <!-- http://www.semanticweb.org/david/ontologies/2013/0/1.3.6.1.4.1.19376.1.8.2.1.183 -->

    <owl:Class rdf:about="&pathLex;183">
        <rdfs:subClassOf rdf:resource="&pathLex;99999"/>
        <skos:prefLabel xml:lang="en">Perineural invasion</skos:prefLabel>
        <skos:definition xml:lang="en">Stomach-Infiltrating malignant neoplasm-Perineural invasion</skos:definition>
    </owl:Class>
    


    <!-- http://www.semanticweb.org/david/ontologies/2013/0/1.3.6.1.4.1.19376.1.8.2.1.1830 -->

    <owl:Class rdf:about="&pathLex;1830">
        <rdfs:subClassOf rdf:resource="&pathLex;99999"/>
        <skos:prefLabel xml:lang="en">Lesion site</skos:prefLabel>
        <skos:definition xml:lang="en">Stomach-Lesion-Lesion site</skos:definition>
    </owl:Class>
    


    <!-- http://www.semanticweb.org/david/ontologies/2013/0/1.3.6.1.4.1.19376.1.8.2.1.1832 -->

    <owl:Class rdf:about="&pathLex;1832">
        <rdfs:subClassOf rdf:resource="&pathLex;99999"/>
        <skos:definition xml:lang="en">Liver-Infiltrating malignant neoplasm-pM</skos:definition>
        <skos:prefLabel xml:lang="en">pM</skos:prefLabel>
    </owl:Class>
    


    <!-- http://www.semanticweb.org/david/ontologies/2013/0/1.3.6.1.4.1.19376.1.8.2.1.1833 -->

    <owl:Class rdf:about="&pathLex;1833">
        <rdfs:subClassOf rdf:resource="&pathLex;99999"/>
        <skos:prefLabel xml:lang="en">Histologic type</skos:prefLabel>
        <skos:definition xml:lang="en">Liver-Lesion-Histologic type</skos:definition>
    </owl:Class>
    


    <!-- http://www.semanticweb.org/david/ontologies/2013/0/1.3.6.1.4.1.19376.1.8.2.1.1834 -->

    <owl:Class rdf:about="&pathLex;1834">
        <rdfs:subClassOf rdf:resource="&pathLex;99999"/>
        <skos:prefLabel xml:lang="en">Lesion site</skos:prefLabel>
        <skos:definition xml:lang="en">Liver-Lesion-Lesion site</skos:definition>
    </owl:Class>
    


    <!-- http://www.semanticweb.org/david/ontologies/2013/0/1.3.6.1.4.1.19376.1.8.2.1.1835 -->

    <owl:Class rdf:about="&pathLex;1835">
        <rdfs:subClassOf rdf:resource="&pathLex;99999"/>
        <skos:definition xml:lang="en">Generic-Infiltrating malignant neoplasm-TNM Descriptors </skos:definition>
        <skos:prefLabel xml:lang="en">TNM Descriptors </skos:prefLabel>
    </owl:Class>
    


    <!-- http://www.semanticweb.org/david/ontologies/2013/0/1.3.6.1.4.1.19376.1.8.2.1.1836 -->

    <owl:Class rdf:about="&pathLex;1836">
        <rdfs:subClassOf rdf:resource="&pathLex;10010"/>
        <skos:definition xml:lang="en">Generic-Infiltrating malignant neoplasm-Margin site</skos:definition>
        <skos:prefLabel xml:lang="en">Margin site</skos:prefLabel>
    </owl:Class>
    


    <!-- http://www.semanticweb.org/david/ontologies/2013/0/1.3.6.1.4.1.19376.1.8.2.1.184 -->

    <owl:Class rdf:about="&pathLex;184">
        <rdfs:subClassOf rdf:resource="&pathLex;99999"/>
        <skos:prefLabel xml:lang="en">Lesion site</skos:prefLabel>
        <skos:definition xml:lang="en">Stomach-Infiltrating malignant neoplasm-Lesion site</skos:definition>
    </owl:Class>
    


    <!-- http://www.semanticweb.org/david/ontologies/2013/0/1.3.6.1.4.1.19376.1.8.2.1.1840 -->

    <owl:Class rdf:about="&pathLex;1840">
        <rdfs:subClassOf rdf:resource="&pathLex;10011"/>
        <skos:definition xml:lang="en">Generic-In situ neoplasm-Histologic type</skos:definition>
        <skos:prefLabel xml:lang="en">Histologic type</skos:prefLabel>
    </owl:Class>
    


    <!-- http://www.semanticweb.org/david/ontologies/2013/0/1.3.6.1.4.1.19376.1.8.2.1.1841 -->

    <owl:Class rdf:about="&pathLex;1841">
        <rdfs:subClassOf rdf:resource="&pathLex;10011"/>
        <skos:definition xml:lang="en">Generic-In situ neoplasm-Lesion site</skos:definition>
        <skos:prefLabel xml:lang="en">Lesion site</skos:prefLabel>
    </owl:Class>
    


    <!-- http://www.semanticweb.org/david/ontologies/2013/0/1.3.6.1.4.1.19376.1.8.2.1.1842 -->

    <owl:Class rdf:about="&pathLex;1842">
        <rdfs:subClassOf rdf:resource="&pathLex;99999"/>
        <skos:prefLabel xml:lang="en">Lesion site</skos:prefLabel>
        <skos:definition xml:lang="en">Salivary gland-Infiltrating malignant neoplasm-Lesion site</skos:definition>
    </owl:Class>
    


    <!-- http://www.semanticweb.org/david/ontologies/2013/0/1.3.6.1.4.1.19376.1.8.2.1.1844 -->

    <owl:Class rdf:about="&pathLex;1844">
        <rdfs:subClassOf rdf:resource="&pathLex;99999"/>
        <skos:prefLabel xml:lang="en">Macroscopic type</skos:prefLabel>
        <skos:definition xml:lang="en">Salivary gland-Infiltrating malignant neoplasm-Macroscopic type</skos:definition>
    </owl:Class>
    


    <!-- http://www.semanticweb.org/david/ontologies/2013/0/1.3.6.1.4.1.19376.1.8.2.1.1845 -->

    <owl:Class rdf:about="&pathLex;1845">
        <rdfs:subClassOf rdf:resource="&pathLex;99999"/>
        <skos:prefLabel xml:lang="en">Histologic type</skos:prefLabel>
        <skos:definition xml:lang="en">Salivary gland-Lesion-Histologic type</skos:definition>
    </owl:Class>
    


    <!-- http://www.semanticweb.org/david/ontologies/2013/0/1.3.6.1.4.1.19376.1.8.2.1.1846 -->

    <owl:Class rdf:about="&pathLex;1846">
        <rdfs:subClassOf rdf:resource="&pathLex;99999"/>
        <skos:prefLabel xml:lang="en">Lesion site</skos:prefLabel>
        <skos:definition xml:lang="en">Salivary gland-Lesion-Lesion site</skos:definition>
    </owl:Class>
    


    <!-- http://www.semanticweb.org/david/ontologies/2013/0/1.3.6.1.4.1.19376.1.8.2.1.1848 -->

    <owl:Class rdf:about="&pathLex;1848">
        <rdfs:subClassOf rdf:resource="&pathLex;99999"/>
        <skos:definition xml:lang="en">Larynx-Infiltrating malignant neoplasm-pM</skos:definition>
        <skos:prefLabel xml:lang="en">pM</skos:prefLabel>
    </owl:Class>
    


    <!-- http://www.semanticweb.org/david/ontologies/2013/0/1.3.6.1.4.1.19376.1.8.2.1.1849 -->

    <owl:Class rdf:about="&pathLex;1849">
        <rdfs:subClassOf rdf:resource="&pathLex;99999"/>
        <skos:definition xml:lang="en">Larynx-Infiltrating malignant neoplasm-Macroscopic type</skos:definition>
        <skos:prefLabel xml:lang="en">Macroscopic type</skos:prefLabel>
    </owl:Class>
    


    <!-- http://www.semanticweb.org/david/ontologies/2013/0/1.3.6.1.4.1.19376.1.8.2.1.185 -->

    <owl:Class rdf:about="&pathLex;185">
        <rdfs:subClassOf rdf:resource="&pathLex;99999"/>
        <skos:prefLabel xml:lang="en">Margin site</skos:prefLabel>
        <skos:definition xml:lang="en">Stomach-Infiltrating malignant neoplasm-Margin site</skos:definition>
    </owl:Class>
    


    <!-- http://www.semanticweb.org/david/ontologies/2013/0/1.3.6.1.4.1.19376.1.8.2.1.1850 -->

    <owl:Class rdf:about="&pathLex;1850">
        <rdfs:subClassOf rdf:resource="&pathLex;99999"/>
        <skos:prefLabel xml:lang="en">Histologic type</skos:prefLabel>
        <skos:definition xml:lang="en">Larynx-Lesion-Histologic type</skos:definition>
    </owl:Class>
    


    <!-- http://www.semanticweb.org/david/ontologies/2013/0/1.3.6.1.4.1.19376.1.8.2.1.1851 -->

    <owl:Class rdf:about="&pathLex;1851">
        <rdfs:subClassOf rdf:resource="&pathLex;99999"/>
        <skos:definition xml:lang="en">Larynx-Lesion-Lesion site</skos:definition>
        <skos:prefLabel xml:lang="en">Lesion site</skos:prefLabel>
    </owl:Class>
    


    <!-- http://www.semanticweb.org/david/ontologies/2013/0/1.3.6.1.4.1.19376.1.8.2.1.1852 -->

    <owl:Class rdf:about="&pathLex;1852">
        <rdfs:subClassOf rdf:resource="&pathLex;99999"/>
        <skos:prefLabel xml:lang="en">Lesion site</skos:prefLabel>
        <skos:definition xml:lang="en">Lip, oral cavity-Infiltrating malignant neoplasm-Lesion site</skos:definition>
    </owl:Class>
    


    <!-- http://www.semanticweb.org/david/ontologies/2013/0/1.3.6.1.4.1.19376.1.8.2.1.1854 -->

    <owl:Class rdf:about="&pathLex;1854">
        <rdfs:subClassOf rdf:resource="&pathLex;99999"/>
        <skos:prefLabel xml:lang="en">Histologic type</skos:prefLabel>
        <skos:definition xml:lang="en">Lip, oral cavity-Lesion-Histologic type</skos:definition>
    </owl:Class>
    


    <!-- http://www.semanticweb.org/david/ontologies/2013/0/1.3.6.1.4.1.19376.1.8.2.1.1855 -->

    <owl:Class rdf:about="&pathLex;1855">
        <rdfs:subClassOf rdf:resource="&pathLex;99999"/>
        <skos:prefLabel xml:lang="en">Lesion site</skos:prefLabel>
        <skos:definition xml:lang="en">Lip, oral cavity-Lesion-Lesion site</skos:definition>
    </owl:Class>
    


    <!-- http://www.semanticweb.org/david/ontologies/2013/0/1.3.6.1.4.1.19376.1.8.2.1.1856 -->

    <owl:Class rdf:about="&pathLex;1856">
        <rdfs:subClassOf rdf:resource="&pathLex;99999"/>
        <skos:definition xml:lang="en">Esophagus-Infiltrating malignant neoplasm-Histologic grade (WHO)</skos:definition>
        <skos:prefLabel xml:lang="en">Histologic grade (WHO)</skos:prefLabel>
    </owl:Class>
    


    <!-- http://www.semanticweb.org/david/ontologies/2013/0/1.3.6.1.4.1.19376.1.8.2.1.1858 -->

    <owl:Class rdf:about="&pathLex;1858">
        <rdfs:subClassOf rdf:resource="&pathLex;99999"/>
        <skos:definition xml:lang="en">Esophagus-Infiltrating malignant neoplasm-pM</skos:definition>
        <skos:prefLabel xml:lang="en">pM</skos:prefLabel>
    </owl:Class>
    


    <!-- http://www.semanticweb.org/david/ontologies/2013/0/1.3.6.1.4.1.19376.1.8.2.1.1859 -->

    <owl:Class rdf:about="&pathLex;1859">
        <rdfs:subClassOf rdf:resource="&pathLex;99999"/>
        <skos:definition xml:lang="en">Esophagus-Lesion-Histologic type</skos:definition>
        <skos:prefLabel xml:lang="en">Histologic type</skos:prefLabel>
    </owl:Class>
    


    <!-- http://www.semanticweb.org/david/ontologies/2013/0/1.3.6.1.4.1.19376.1.8.2.1.186 -->

    <owl:Class rdf:about="&pathLex;186">
        <rdfs:subClassOf rdf:resource="&pathLex;99999"/>
        <skos:prefLabel xml:lang="en">Number of lymph nodes involved</skos:prefLabel>
        <skos:definition xml:lang="en">Stomach-Infiltrating malignant neoplasm-Number of lymph nodes involved</skos:definition>
    </owl:Class>
    


    <!-- http://www.semanticweb.org/david/ontologies/2013/0/1.3.6.1.4.1.19376.1.8.2.1.1860 -->

    <owl:Class rdf:about="&pathLex;1860">
        <rdfs:subClassOf rdf:resource="&pathLex;99999"/>
        <skos:definition xml:lang="en">Esophagus-Lesion-Lesion site</skos:definition>
        <skos:prefLabel xml:lang="en">Lesion site</skos:prefLabel>
    </owl:Class>
    


    <!-- http://www.semanticweb.org/david/ontologies/2013/0/1.3.6.1.4.1.19376.1.8.2.1.1861 -->

    <owl:Class rdf:about="&pathLex;1861">
        <rdfs:subClassOf rdf:resource="&pathLex;99999"/>
        <skos:prefLabel xml:lang="en">Histologic grade (WHO)</skos:prefLabel>
        <skos:definition xml:lang="en">Ovary-Infiltrating malignant neoplasm-Histologic grade (WHO)</skos:definition>
    </owl:Class>
    


    <!-- http://www.semanticweb.org/david/ontologies/2013/0/1.3.6.1.4.1.19376.1.8.2.1.1862 -->

    <owl:Class rdf:about="&pathLex;1862">
        <rdfs:subClassOf rdf:resource="&pathLex;99999"/>
        <skos:prefLabel xml:lang="en">Lesion site</skos:prefLabel>
        <skos:definition xml:lang="en">Ovary-Infiltrating malignant neoplasm-Lesion site</skos:definition>
    </owl:Class>
    


    <!-- http://www.semanticweb.org/david/ontologies/2013/0/1.3.6.1.4.1.19376.1.8.2.1.1864 -->

    <owl:Class rdf:about="&pathLex;1864">
        <rdfs:subClassOf rdf:resource="&pathLex;99999"/>
        <skos:definition xml:lang="en">Ovary-Infiltrating malignant neoplasm-pM</skos:definition>
        <skos:prefLabel xml:lang="en">pM</skos:prefLabel>
    </owl:Class>
    


    <!-- http://www.semanticweb.org/david/ontologies/2013/0/1.3.6.1.4.1.19376.1.8.2.1.1865 -->

    <owl:Class rdf:about="&pathLex;1865">
        <rdfs:subClassOf rdf:resource="&pathLex;99999"/>
        <skos:prefLabel xml:lang="en">Histologic type</skos:prefLabel>
        <skos:definition xml:lang="en">Ovary-Lesion-Histologic type</skos:definition>
    </owl:Class>
    


    <!-- http://www.semanticweb.org/david/ontologies/2013/0/1.3.6.1.4.1.19376.1.8.2.1.1866 -->

    <owl:Class rdf:about="&pathLex;1866">
        <rdfs:subClassOf rdf:resource="&pathLex;99999"/>
        <skos:prefLabel xml:lang="en">Lesion site</skos:prefLabel>
        <skos:definition xml:lang="en">Ovary-Lesion-Lesion site</skos:definition>
    </owl:Class>
    


    <!-- http://www.semanticweb.org/david/ontologies/2013/0/1.3.6.1.4.1.19376.1.8.2.1.1868 -->

    <owl:Class rdf:about="&pathLex;1868">
        <rdfs:subClassOf rdf:resource="&pathLex;99999"/>
        <skos:definition xml:lang="en">Pancreas-Infiltrating malignant neoplasm-pM</skos:definition>
        <skos:prefLabel xml:lang="en">pM</skos:prefLabel>
    </owl:Class>
    


    <!-- http://www.semanticweb.org/david/ontologies/2013/0/1.3.6.1.4.1.19376.1.8.2.1.1869 -->

    <owl:Class rdf:about="&pathLex;1869">
        <rdfs:subClassOf rdf:resource="&pathLex;99999"/>
        <skos:prefLabel xml:lang="en">Histologic type</skos:prefLabel>
        <skos:definition xml:lang="en">Pancreas-Lesion-Histologic type</skos:definition>
    </owl:Class>
    


    <!-- http://www.semanticweb.org/david/ontologies/2013/0/1.3.6.1.4.1.19376.1.8.2.1.187 -->

    <owl:Class rdf:about="&pathLex;187">
        <rdfs:subClassOf rdf:resource="&pathLex;99999"/>
        <skos:prefLabel xml:lang="en">Number of lymph nodes examined</skos:prefLabel>
        <skos:definition xml:lang="en">Stomach-Infiltrating malignant neoplasm-Number of lymph nodes examined</skos:definition>
    </owl:Class>
    


    <!-- http://www.semanticweb.org/david/ontologies/2013/0/1.3.6.1.4.1.19376.1.8.2.1.1870 -->

    <owl:Class rdf:about="&pathLex;1870">
        <rdfs:subClassOf rdf:resource="&pathLex;99999"/>
        <skos:prefLabel xml:lang="en">Lesion site</skos:prefLabel>
        <skos:definition xml:lang="en">Pancreas-Lesion-Lesion site</skos:definition>
    </owl:Class>
    


    <!-- http://www.semanticweb.org/david/ontologies/2013/0/1.3.6.1.4.1.19376.1.8.2.1.1871 -->

    <owl:Class rdf:about="&pathLex;1871">
        <rdfs:subClassOf rdf:resource="&pathLex;99999"/>
        <skos:prefLabel xml:lang="en">Lymph node site</skos:prefLabel>
        <skos:definition xml:lang="en">Skin (melanoma)-Infiltrating malignant neoplasm-Lymph node site</skos:definition>
    </owl:Class>
    


    <!-- http://www.semanticweb.org/david/ontologies/2013/0/1.3.6.1.4.1.19376.1.8.2.1.1873 -->

    <owl:Class rdf:about="&pathLex;1873">
        <rdfs:subClassOf rdf:resource="&pathLex;99999"/>
        <skos:definition xml:lang="en">Skin (melanoma)-Infiltrating malignant neoplasm-pM</skos:definition>
        <skos:prefLabel xml:lang="en">pM</skos:prefLabel>
    </owl:Class>
    


    <!-- http://www.semanticweb.org/david/ontologies/2013/0/1.3.6.1.4.1.19376.1.8.2.1.1874 -->

    <owl:Class rdf:about="&pathLex;1874">
        <rdfs:subClassOf rdf:resource="&pathLex;99999"/>
        <skos:prefLabel xml:lang="en">Histologic type</skos:prefLabel>
        <skos:definition xml:lang="en">Skin (melanoma)-Lesion-Histologic type</skos:definition>
    </owl:Class>
    


    <!-- http://www.semanticweb.org/david/ontologies/2013/0/1.3.6.1.4.1.19376.1.8.2.1.1875 -->

    <owl:Class rdf:about="&pathLex;1875">
        <rdfs:subClassOf rdf:resource="&pathLex;99999"/>
        <skos:prefLabel xml:lang="en">Lesion site</skos:prefLabel>
        <skos:definition xml:lang="en">Skin (melanoma)-Lesion-Lesion site</skos:definition>
    </owl:Class>
    


    <!-- http://www.semanticweb.org/david/ontologies/2013/0/1.3.6.1.4.1.19376.1.8.2.1.1876 -->

    <owl:Class rdf:about="&pathLex;1876">
        <rdfs:subClassOf rdf:resource="&pathLex;99999"/>
        <skos:prefLabel xml:lang="en">EBV (Epstein Barr virus encoded RNA [EBER], other)</skos:prefLabel>
        <skos:definition xml:lang="en">Pharynx-Infiltrating malignant neoplasm-EBV (Epstein Barr virus encoded RNA [EBER], other)</skos:definition>
    </owl:Class>
    


    <!-- http://www.semanticweb.org/david/ontologies/2013/0/1.3.6.1.4.1.19376.1.8.2.1.1877 -->

    <owl:Class rdf:about="&pathLex;1877">
        <rdfs:subClassOf rdf:resource="&pathLex;99999"/>
        <skos:prefLabel xml:lang="en">HPV (p16 immunoreactivity, in situ)</skos:prefLabel>
        <skos:definition xml:lang="en">Pharynx-Infiltrating malignant neoplasm-HPV (p16 immunoreactivity, in situ)</skos:definition>
    </owl:Class>
    


    <!-- http://www.semanticweb.org/david/ontologies/2013/0/1.3.6.1.4.1.19376.1.8.2.1.1879 -->

    <owl:Class rdf:about="&pathLex;1879">
        <rdfs:subClassOf rdf:resource="&pathLex;99999"/>
        <skos:definition xml:lang="en">Pharynx-Infiltrating malignant neoplasm-pM</skos:definition>
        <skos:prefLabel xml:lang="en">pM</skos:prefLabel>
    </owl:Class>
    


    <!-- http://www.semanticweb.org/david/ontologies/2013/0/1.3.6.1.4.1.19376.1.8.2.1.1880 -->

    <owl:Class rdf:about="&pathLex;1880">
        <rdfs:subClassOf rdf:resource="&pathLex;99999"/>
        <skos:definition xml:lang="en">Pharynx-Infiltrating malignant neoplasm-pT oropharynx carcinoma</skos:definition>
        <skos:prefLabel xml:lang="en">pT oropharynx carcinoma</skos:prefLabel>
    </owl:Class>
    


    <!-- http://www.semanticweb.org/david/ontologies/2013/0/1.3.6.1.4.1.19376.1.8.2.1.1882 -->

    <owl:Class rdf:about="&pathLex;1882">
        <rdfs:subClassOf rdf:resource="&pathLex;99999"/>
        <skos:prefLabel xml:lang="en">Histologic type</skos:prefLabel>
        <skos:definition xml:lang="en">Pharynx-Lesion-Histologic type</skos:definition>
    </owl:Class>
    


    <!-- http://www.semanticweb.org/david/ontologies/2013/0/1.3.6.1.4.1.19376.1.8.2.1.1883 -->

    <owl:Class rdf:about="&pathLex;1883">
        <rdfs:subClassOf rdf:resource="&pathLex;99999"/>
        <skos:prefLabel xml:lang="en">Lesion site</skos:prefLabel>
        <skos:definition xml:lang="en">Pharynx-Lesion-Lesion site</skos:definition>
    </owl:Class>
    


    <!-- http://www.semanticweb.org/david/ontologies/2013/0/1.3.6.1.4.1.19376.1.8.2.1.1884 -->

    <owl:Class rdf:about="&pathLex;1884">
        <rdfs:subClassOf rdf:resource="&pathLex;99999"/>
        <skos:prefLabel xml:lang="en">Epidermal growth factor receptor (EGFR)</skos:prefLabel>
        <skos:definition xml:lang="en">Lung-Infiltrating malignant neoplasm-Epidermal growth factor receptor (EGFR)</skos:definition>
    </owl:Class>
    


    <!-- http://www.semanticweb.org/david/ontologies/2013/0/1.3.6.1.4.1.19376.1.8.2.1.1885 -->

    <owl:Class rdf:about="&pathLex;1885">
        <rdfs:subClassOf rdf:resource="&pathLex;99999"/>
        <skos:prefLabel xml:lang="en">KRAS mutational analysis</skos:prefLabel>
        <skos:definition xml:lang="en">Lung-Infiltrating malignant neoplasm-KRAS mutational analysis</skos:definition>
    </owl:Class>
    


    <!-- http://www.semanticweb.org/david/ontologies/2013/0/1.3.6.1.4.1.19376.1.8.2.1.1886 -->

    <owl:Class rdf:about="&pathLex;1886">
        <rdfs:subClassOf rdf:resource="&pathLex;99999"/>
        <skos:prefLabel xml:lang="en">Histologic grade (WHO)</skos:prefLabel>
        <skos:definition xml:lang="en">Lung-Infiltrating malignant neoplasm-Histologic grade (WHO)</skos:definition>
    </owl:Class>
    


    <!-- http://www.semanticweb.org/david/ontologies/2013/0/1.3.6.1.4.1.19376.1.8.2.1.1887 -->

    <owl:Class rdf:about="&pathLex;1887">
        <rdfs:subClassOf rdf:resource="&pathLex;99999"/>
        <skos:prefLabel xml:lang="en">Lesion site</skos:prefLabel>
        <skos:definition xml:lang="en">Lung-Infiltrating malignant neoplasm-Lesion site</skos:definition>
    </owl:Class>
    


    <!-- http://www.semanticweb.org/david/ontologies/2013/0/1.3.6.1.4.1.19376.1.8.2.1.1889 -->

    <owl:Class rdf:about="&pathLex;1889">
        <rdfs:subClassOf rdf:resource="&pathLex;99999"/>
        <skos:definition xml:lang="en">Lung-Infiltrating malignant neoplasm-pM</skos:definition>
        <skos:prefLabel xml:lang="en">pM</skos:prefLabel>
    </owl:Class>
    


    <!-- http://www.semanticweb.org/david/ontologies/2013/0/1.3.6.1.4.1.19376.1.8.2.1.189 -->

    <owl:Class rdf:about="&pathLex;189">
        <rdfs:subClassOf rdf:resource="&pathLex;99999"/>
        <skos:definition xml:lang="en">Stomach-Infiltrating malignant neoplasm-pN</skos:definition>
        <skos:prefLabel xml:lang="en">pN</skos:prefLabel>
    </owl:Class>
    


    <!-- http://www.semanticweb.org/david/ontologies/2013/0/1.3.6.1.4.1.19376.1.8.2.1.1890 -->

    <owl:Class rdf:about="&pathLex;1890">
        <rdfs:subClassOf rdf:resource="&pathLex;99999"/>
        <skos:prefLabel xml:lang="en">Histologic type</skos:prefLabel>
        <skos:definition xml:lang="en">Lung-Lesion-Histologic type</skos:definition>
    </owl:Class>
    


    <!-- http://www.semanticweb.org/david/ontologies/2013/0/1.3.6.1.4.1.19376.1.8.2.1.1891 -->

    <owl:Class rdf:about="&pathLex;1891">
        <rdfs:subClassOf rdf:resource="&pathLex;99999"/>
        <skos:prefLabel xml:lang="en">Lesion site</skos:prefLabel>
        <skos:definition xml:lang="en">Lung-Lesion-Lesion site</skos:definition>
    </owl:Class>
    


    <!-- http://www.semanticweb.org/david/ontologies/2013/0/1.3.6.1.4.1.19376.1.8.2.1.1892 -->

    <owl:Class rdf:about="&pathLex;1892">
        <rdfs:subClassOf rdf:resource="&pathLex;99999"/>
        <skos:prefLabel xml:lang="en">Margin site</skos:prefLabel>
        <skos:definition xml:lang="en">Prostate-Infiltrating malignant neoplasm-Margin site</skos:definition>
    </owl:Class>
    


    <!-- http://www.semanticweb.org/david/ontologies/2013/0/1.3.6.1.4.1.19376.1.8.2.1.1894 -->

    <owl:Class rdf:about="&pathLex;1894">
        <rdfs:subClassOf rdf:resource="&pathLex;99999"/>
        <skos:definition xml:lang="en">Prostate-Infiltrating malignant neoplasm-pM</skos:definition>
        <skos:prefLabel xml:lang="en">pM</skos:prefLabel>
    </owl:Class>
    


    <!-- http://www.semanticweb.org/david/ontologies/2013/0/1.3.6.1.4.1.19376.1.8.2.1.1895 -->

    <owl:Class rdf:about="&pathLex;1895">
        <rdfs:subClassOf rdf:resource="&pathLex;99999"/>
        <skos:prefLabel xml:lang="en">Histologic type</skos:prefLabel>
        <skos:definition xml:lang="en">Prostate-Lesion-Histologic type</skos:definition>
    </owl:Class>
    


    <!-- http://www.semanticweb.org/david/ontologies/2013/0/1.3.6.1.4.1.19376.1.8.2.1.1896 -->

    <owl:Class rdf:about="&pathLex;1896">
        <rdfs:subClassOf rdf:resource="&pathLex;99999"/>
        <skos:prefLabel xml:lang="en">Lesion site</skos:prefLabel>
        <skos:definition xml:lang="en">Prostate-Lesion-Lesion site</skos:definition>
    </owl:Class>
    


    <!-- http://www.semanticweb.org/david/ontologies/2013/0/1.3.6.1.4.1.19376.1.8.2.1.1898 -->

    <owl:Class rdf:about="&pathLex;1898">
        <rdfs:subClassOf rdf:resource="&pathLex;99999"/>
        <skos:definition xml:lang="en">Kidney-Infiltrating malignant neoplasm-pM</skos:definition>
        <skos:prefLabel xml:lang="en">pM</skos:prefLabel>
    </owl:Class>
    


    <!-- http://www.semanticweb.org/david/ontologies/2013/0/1.3.6.1.4.1.19376.1.8.2.1.1899 -->

    <owl:Class rdf:about="&pathLex;1899">
        <rdfs:subClassOf rdf:resource="&pathLex;99999"/>
        <skos:prefLabel xml:lang="en">Histologic type</skos:prefLabel>
        <skos:definition xml:lang="en">Kidney-Lesion-Histologic type</skos:definition>
    </owl:Class>
    


    <!-- http://www.semanticweb.org/david/ontologies/2013/0/1.3.6.1.4.1.19376.1.8.2.1.1900 -->

    <owl:Class rdf:about="&pathLex;1900">
        <rdfs:subClassOf rdf:resource="&pathLex;99999"/>
        <skos:definition xml:lang="en">Kidney-Lesion-Lesion site</skos:definition>
        <skos:prefLabel xml:lang="en">Lesion site</skos:prefLabel>
    </owl:Class>
    


    <!-- http://www.semanticweb.org/david/ontologies/2013/0/1.3.6.1.4.1.19376.1.8.2.1.1901 -->

    <owl:Class rdf:about="&pathLex;1901">
        <rdfs:subClassOf rdf:resource="&pathLex;1840"/>
        <skos:definition xml:lang="en">Breast-In situ neoplasm-Necrosis of ductal carcinoma in situ (DCIS)</skos:definition>
        <skos:prefLabel xml:lang="en">Necrosis of ductal carcinoma in situ (DCIS)</skos:prefLabel>
    </owl:Class>
    


    <!-- http://www.semanticweb.org/david/ontologies/2013/0/1.3.6.1.4.1.19376.1.8.2.1.1903 -->

    <owl:Class rdf:about="&pathLex;1903">
        <rdfs:subClassOf rdf:resource="&pathLex;1433"/>
        <skos:prefLabel xml:lang="en">Breast-Infiltrating malignant neoplasm-pM</skos:prefLabel>
        <skos:definition xml:lang="en">Breast-Infiltrating malignant neoplasm-pM</skos:definition>
        <skos:altLabel xml:lang="en">pM</skos:altLabel>
    </owl:Class>
    


    <!-- http://www.semanticweb.org/david/ontologies/2013/0/1.3.6.1.4.1.19376.1.8.2.1.1904 -->

    <owl:Class rdf:about="&pathLex;1904">
        <rdfs:subClassOf rdf:resource="&pathLex;23"/>
        <skos:prefLabel xml:lang="en">Breast-Histologic type</skos:prefLabel>
        <skos:definition xml:lang="en">Breast-Lesion-Histologic type</skos:definition>
        <skos:altLabel xml:lang="en">Histologic type</skos:altLabel>
    </owl:Class>
    


    <!-- http://www.semanticweb.org/david/ontologies/2013/0/1.3.6.1.4.1.19376.1.8.2.1.1905 -->

    <owl:Class rdf:about="&pathLex;1905">
        <rdfs:subClassOf rdf:resource="&pathLex;6"/>
        <skos:prefLabel xml:lang="en">Breast-Lesion site</skos:prefLabel>
        <skos:definition xml:lang="en">Breast-Lesion-Lesion site</skos:definition>
        <skos:altLabel xml:lang="en">Lesion site</skos:altLabel>
    </owl:Class>
    


    <!-- http://www.semanticweb.org/david/ontologies/2013/0/1.3.6.1.4.1.19376.1.8.2.1.1906 -->

    <owl:Class rdf:about="&pathLex;1906">
        <rdfs:subClassOf rdf:resource="&pathLex;1841"/>
        <skos:definition xml:lang="en">Breast-In situ neoplasm-Lesion site</skos:definition>
        <skos:prefLabel xml:lang="en">Breast-Lesion site</skos:prefLabel>
        <skos:altLabel xml:lang="en">Lesion site</skos:altLabel>
    </owl:Class>
    


    <!-- http://www.semanticweb.org/david/ontologies/2013/0/1.3.6.1.4.1.19376.1.8.2.1.1908 -->

    <owl:Class rdf:about="&pathLex;1908">
        <rdfs:subClassOf rdf:resource="&pathLex;99999"/>
        <skos:definition xml:lang="en">Testis-Infiltrating malignant neoplasm-pM</skos:definition>
        <skos:prefLabel xml:lang="en">pM</skos:prefLabel>
    </owl:Class>
    


    <!-- http://www.semanticweb.org/david/ontologies/2013/0/1.3.6.1.4.1.19376.1.8.2.1.1909 -->

    <owl:Class rdf:about="&pathLex;1909">
        <rdfs:subClassOf rdf:resource="&pathLex;99999"/>
        <skos:prefLabel xml:lang="en">Histologic type</skos:prefLabel>
        <skos:definition xml:lang="en">Testis-Lesion-Histologic type</skos:definition>
    </owl:Class>
    


    <!-- http://www.semanticweb.org/david/ontologies/2013/0/1.3.6.1.4.1.19376.1.8.2.1.191 -->

    <owl:Class rdf:about="&pathLex;191">
        <rdfs:subClassOf rdf:resource="&pathLex;99999"/>
        <skos:definition xml:lang="en">Stomach-Infiltrating malignant neoplasm-pT</skos:definition>
        <skos:prefLabel xml:lang="en">pT</skos:prefLabel>
    </owl:Class>
    


    <!-- http://www.semanticweb.org/david/ontologies/2013/0/1.3.6.1.4.1.19376.1.8.2.1.1910 -->

    <owl:Class rdf:about="&pathLex;1910">
        <rdfs:subClassOf rdf:resource="&pathLex;99999"/>
        <skos:prefLabel xml:lang="en">Lesion site</skos:prefLabel>
        <skos:definition xml:lang="en">Testis-Lesion-Lesion site</skos:definition>
    </owl:Class>
    


    <!-- http://www.semanticweb.org/david/ontologies/2013/0/1.3.6.1.4.1.19376.1.8.2.1.1911 -->

    <owl:Class rdf:about="&pathLex;1911">
        <rdfs:subClassOf rdf:resource="&pathLex;99999"/>
        <skos:prefLabel xml:lang="en">Histologic grade (WHO)</skos:prefLabel>
        <skos:definition xml:lang="en">Thyroid-Infiltrating malignant neoplasm-Histologic grade (WHO)</skos:definition>
    </owl:Class>
    


    <!-- http://www.semanticweb.org/david/ontologies/2013/0/1.3.6.1.4.1.19376.1.8.2.1.1913 -->

    <owl:Class rdf:about="&pathLex;1913">
        <rdfs:subClassOf rdf:resource="&pathLex;99999"/>
        <skos:definition xml:lang="en">Thyroid-Infiltrating malignant neoplasm-pM</skos:definition>
        <skos:prefLabel xml:lang="en">pM</skos:prefLabel>
    </owl:Class>
    


    <!-- http://www.semanticweb.org/david/ontologies/2013/0/1.3.6.1.4.1.19376.1.8.2.1.1914 -->

    <owl:Class rdf:about="&pathLex;1914">
        <rdfs:subClassOf rdf:resource="&pathLex;99999"/>
        <skos:prefLabel xml:lang="en">Histologic type</skos:prefLabel>
        <skos:definition xml:lang="en">Thyroid-Lesion-Histologic type</skos:definition>
    </owl:Class>
    


    <!-- http://www.semanticweb.org/david/ontologies/2013/0/1.3.6.1.4.1.19376.1.8.2.1.1915 -->

    <owl:Class rdf:about="&pathLex;1915">
        <rdfs:subClassOf rdf:resource="&pathLex;99999"/>
        <skos:prefLabel xml:lang="en">Lesion site</skos:prefLabel>
        <skos:definition xml:lang="en">Thyroid-Lesion-Lesion site</skos:definition>
    </owl:Class>
    


    <!-- http://www.semanticweb.org/david/ontologies/2013/0/1.3.6.1.4.1.19376.1.8.2.1.1917 -->

    <owl:Class rdf:about="&pathLex;1917">
        <rdfs:subClassOf rdf:resource="&pathLex;99999"/>
        <skos:definition xml:lang="en">Urinary bladder-Infiltrating malignant neoplasm-pM</skos:definition>
        <skos:prefLabel xml:lang="en">pM</skos:prefLabel>
    </owl:Class>
    


    <!-- http://www.semanticweb.org/david/ontologies/2013/0/1.3.6.1.4.1.19376.1.8.2.1.1918 -->

    <owl:Class rdf:about="&pathLex;1918">
        <rdfs:subClassOf rdf:resource="&pathLex;99999"/>
        <skos:prefLabel xml:lang="en">Macroscopic type</skos:prefLabel>
        <skos:definition xml:lang="en">Urinary bladder-Infiltrating malignant neoplasm-Macroscopic type</skos:definition>
    </owl:Class>
    


    <!-- http://www.semanticweb.org/david/ontologies/2013/0/1.3.6.1.4.1.19376.1.8.2.1.1919 -->

    <owl:Class rdf:about="&pathLex;1919">
        <rdfs:subClassOf rdf:resource="&pathLex;99999"/>
        <skos:prefLabel xml:lang="en">Histologic type</skos:prefLabel>
        <skos:definition xml:lang="en">Urinary bladder-Lesion-Histologic type</skos:definition>
    </owl:Class>
    


    <!-- http://www.semanticweb.org/david/ontologies/2013/0/1.3.6.1.4.1.19376.1.8.2.1.192 -->

    <owl:Class rdf:about="&pathLex;192">
        <rdfs:subClassOf rdf:resource="&pathLex;99999"/>
        <skos:prefLabel xml:lang="en">Lesion size, largest dimension</skos:prefLabel>
        <skos:definition xml:lang="en">Stomach-Infiltrating malignant neoplasm-Lesion size, largest dimension</skos:definition>
    </owl:Class>
    


    <!-- http://www.semanticweb.org/david/ontologies/2013/0/1.3.6.1.4.1.19376.1.8.2.1.1920 -->

    <owl:Class rdf:about="&pathLex;1920">
        <rdfs:subClassOf rdf:resource="&pathLex;99999"/>
        <skos:prefLabel xml:lang="en">Lesion site</skos:prefLabel>
        <skos:definition xml:lang="en">Urinary bladder-Lesion-Lesion site</skos:definition>
    </owl:Class>
    


    <!-- http://www.semanticweb.org/david/ontologies/2013/0/1.3.6.1.4.1.19376.1.8.2.1.1921 -->

    <owl:Class rdf:about="&pathLex;1921">
        <rdfs:subClassOf rdf:resource="&pathLex;99999"/>
        <skos:definition xml:lang="en">Pharynx-Infiltrating malignant neoplasm-Epstein-Barr virus (Epstein Barr virus encoded RNA [EBER], other)-Present</skos:definition>
        <skos:prefLabel xml:lang="en">Present</skos:prefLabel>
    </owl:Class>
    


    <!-- http://www.semanticweb.org/david/ontologies/2013/0/1.3.6.1.4.1.19376.1.8.2.1.1922 -->

    <owl:Class rdf:about="&pathLex;1922">
        <rdfs:subClassOf rdf:resource="&pathLex;99999"/>
        <skos:prefLabel xml:lang="en">Negative</skos:prefLabel>
        <skos:definition xml:lang="en">Pharynx-Infiltrating malignant neoplasm-Epstein-Barr virus (Epstein Barr virus encoded RNA [EBER], other)-Negative</skos:definition>
    </owl:Class>
    


    <!-- http://www.semanticweb.org/david/ontologies/2013/0/1.3.6.1.4.1.19376.1.8.2.1.1923 -->

    <owl:Class rdf:about="&pathLex;1923">
        <rdfs:subClassOf rdf:resource="&pathLex;99999"/>
        <skos:definition xml:lang="en">Pharynx-Infiltrating malignant neoplasm-Human papillomavirus (p16 immunoreactivity, in situ)-Present</skos:definition>
        <skos:prefLabel xml:lang="en">Present</skos:prefLabel>
    </owl:Class>
    


    <!-- http://www.semanticweb.org/david/ontologies/2013/0/1.3.6.1.4.1.19376.1.8.2.1.1924 -->

    <owl:Class rdf:about="&pathLex;1924">
        <rdfs:subClassOf rdf:resource="&pathLex;99999"/>
        <skos:prefLabel xml:lang="en">Negative</skos:prefLabel>
        <skos:definition xml:lang="en">Pharynx-Infiltrating malignant neoplasm-Human papillomavirus (p16 immunoreactivity, in situ)-Negative</skos:definition>
    </owl:Class>
    


    <!-- http://www.semanticweb.org/david/ontologies/2013/0/1.3.6.1.4.1.19376.1.8.2.1.1925 -->

    <owl:Class rdf:about="&pathLex;1925">
        <rdfs:subClassOf rdf:resource="&pathLex;433"/>
        <skos:definition xml:lang="en">Breast-Infiltrating malignant neoplasm-HER2/neu (FISH method)-Equivocal (HER2 gene copy 4.0 to 6.0 or ratio 1.8 to 2.2)</skos:definition>
        <skos:prefLabel xml:lang="en">Equivocal (HER2 gene copy 4.0 to 6.0 or ratio 1.8 to 2.2)</skos:prefLabel>
    </owl:Class>
    


    <!-- http://www.semanticweb.org/david/ontologies/2013/0/1.3.6.1.4.1.19376.1.8.2.1.1926 -->

    <owl:Class rdf:about="&pathLex;1926">
        <rdfs:subClassOf rdf:resource="&pathLex;434"/>
        <skos:definition xml:lang="en">Breast-Infiltrating malignant neoplasm-HER2/neu (immunoperoxidase study)-Negative (Score 1+)</skos:definition>
        <skos:prefLabel xml:lang="en">Negative (Score 1+)</skos:prefLabel>
    </owl:Class>
    


    <!-- http://www.semanticweb.org/david/ontologies/2013/0/1.3.6.1.4.1.19376.1.8.2.1.1927 -->

    <owl:Class rdf:about="&pathLex;1927">
        <rdfs:subClassOf rdf:resource="&pathLex;434"/>
        <skos:definition xml:lang="en">Breast-Infiltrating malignant neoplasm-HER2/neu (immunoperoxidase study)-Equivocal (Score 2+)</skos:definition>
        <skos:prefLabel xml:lang="en">Equivocal (Score 2+)</skos:prefLabel>
    </owl:Class>
    


    <!-- http://www.semanticweb.org/david/ontologies/2013/0/1.3.6.1.4.1.19376.1.8.2.1.1928 -->

    <owl:Class rdf:about="&pathLex;1928">
        <rdfs:subClassOf rdf:resource="&pathLex;99999"/>
        <skos:definition xml:lang="en">Colon-Infiltrating malignant neoplasm-Microsatellite instability-Stable</skos:definition>
        <skos:prefLabel xml:lang="en">Stable</skos:prefLabel>
    </owl:Class>
    


    <!-- http://www.semanticweb.org/david/ontologies/2013/0/1.3.6.1.4.1.19376.1.8.2.1.1929 -->

    <owl:Class rdf:about="&pathLex;1929">
        <rdfs:subClassOf rdf:resource="&pathLex;99999"/>
        <skos:definition xml:lang="en">Colon-Infiltrating malignant neoplasm-Microsatellite instability-Low</skos:definition>
        <skos:prefLabel xml:lang="en">Low</skos:prefLabel>
    </owl:Class>
    


    <!-- http://www.semanticweb.org/david/ontologies/2013/0/1.3.6.1.4.1.19376.1.8.2.1.193 -->

    <owl:Class rdf:about="&pathLex;193">
        <rdfs:subClassOf rdf:resource="&pathLex;99999"/>
        <skos:prefLabel xml:lang="en">Histologic type</skos:prefLabel>
        <skos:definition xml:lang="en">Stomach-Infiltrating malignant neoplasm-Histologic type</skos:definition>
    </owl:Class>
    


    <!-- http://www.semanticweb.org/david/ontologies/2013/0/1.3.6.1.4.1.19376.1.8.2.1.1930 -->

    <owl:Class rdf:about="&pathLex;1930">
        <rdfs:subClassOf rdf:resource="&pathLex;99999"/>
        <skos:definition xml:lang="en">Colon-Infiltrating malignant neoplasm-Microsatellite instability-High</skos:definition>
        <skos:prefLabel xml:lang="en">High</skos:prefLabel>
    </owl:Class>
    


    <!-- http://www.semanticweb.org/david/ontologies/2013/0/1.3.6.1.4.1.19376.1.8.2.1.1931 -->

    <owl:Class rdf:about="&pathLex;1931">
        <rdfs:subClassOf rdf:resource="&pathLex;99999"/>
        <skos:definition xml:lang="en">Lung-Infiltrating malignant neoplasm-Epidermal growth factor receptor (EGFR)-Positive</skos:definition>
        <skos:prefLabel xml:lang="en">Positive</skos:prefLabel>
    </owl:Class>
    


    <!-- http://www.semanticweb.org/david/ontologies/2013/0/1.3.6.1.4.1.19376.1.8.2.1.1932 -->

    <owl:Class rdf:about="&pathLex;1932">
        <rdfs:subClassOf rdf:resource="&pathLex;99999"/>
        <skos:definition xml:lang="en">Lung-Infiltrating malignant neoplasm-Epidermal growth factor receptor (EGFR)-Negative</skos:definition>
        <skos:prefLabel xml:lang="en">Negative</skos:prefLabel>
    </owl:Class>
    


    <!-- http://www.semanticweb.org/david/ontologies/2013/0/1.3.6.1.4.1.19376.1.8.2.1.1933 -->

    <owl:Class rdf:about="&pathLex;1933">
        <rdfs:subClassOf rdf:resource="&pathLex;99999"/>
        <skos:definition xml:lang="en">Colon-Infiltrating malignant neoplasm-Mismatch Repair Proteins-MLH1 (Immunohistochemistry Study)-Intact nuclear positivity, tumor cells</skos:definition>
        <skos:prefLabel xml:lang="en">Intact nuclear positivity, tumor cells</skos:prefLabel>
    </owl:Class>
    


    <!-- http://www.semanticweb.org/david/ontologies/2013/0/1.3.6.1.4.1.19376.1.8.2.1.1934 -->

    <owl:Class rdf:about="&pathLex;1934">
        <rdfs:subClassOf rdf:resource="&pathLex;99999"/>
        <skos:definition xml:lang="en">Colon-Infiltrating malignant neoplasm-Mismatch Repair Proteins-MLH1 (Immunohistochemistry Study)-Loss of nuclear positivity, tumor cells</skos:definition>
        <skos:prefLabel xml:lang="en">Loss of nuclear positivity, tumor cells</skos:prefLabel>
    </owl:Class>
    


    <!-- http://www.semanticweb.org/david/ontologies/2013/0/1.3.6.1.4.1.19376.1.8.2.1.1935 -->

    <owl:Class rdf:about="&pathLex;1935">
        <rdfs:subClassOf rdf:resource="&pathLex;99999"/>
        <skos:definition xml:lang="en">Colon-Infiltrating malignant neoplasm-Mismatch Repair Proteins-MLH2 (Immunohistochemistry Study)-Intact nuclear positivity, tumor cells</skos:definition>
        <skos:prefLabel xml:lang="en">Intact nuclear positivity, tumor cells</skos:prefLabel>
    </owl:Class>
    


    <!-- http://www.semanticweb.org/david/ontologies/2013/0/1.3.6.1.4.1.19376.1.8.2.1.1936 -->

    <owl:Class rdf:about="&pathLex;1936">
        <rdfs:subClassOf rdf:resource="&pathLex;99999"/>
        <skos:definition xml:lang="en">Colon-Infiltrating malignant neoplasm-Mismatch Repair Proteins-MLH2 (Immunohistochemistry Study)-Loss of nuclear positivity, tumor cells</skos:definition>
        <skos:prefLabel xml:lang="en">Loss of nuclear positivity, tumor cells</skos:prefLabel>
    </owl:Class>
    


    <!-- http://www.semanticweb.org/david/ontologies/2013/0/1.3.6.1.4.1.19376.1.8.2.1.1937 -->

    <owl:Class rdf:about="&pathLex;1937">
        <rdfs:subClassOf rdf:resource="&pathLex;99999"/>
        <skos:definition xml:lang="en">Colon-Infiltrating malignant neoplasm-Mismatch Repair Proteins-MLH6 (Immunohistochemistry Study)-Intact nuclear positivity, tumor cells</skos:definition>
        <skos:prefLabel xml:lang="en">Intact nuclear positivity, tumor cells</skos:prefLabel>
    </owl:Class>
    


    <!-- http://www.semanticweb.org/david/ontologies/2013/0/1.3.6.1.4.1.19376.1.8.2.1.1938 -->

    <owl:Class rdf:about="&pathLex;1938">
        <rdfs:subClassOf rdf:resource="&pathLex;99999"/>
        <skos:definition xml:lang="en">Colon-Infiltrating malignant neoplasm-Mismatch Repair Proteins-MLH6 (Immunohistochemistry Study)-Loss of nuclear positivity, tumor cells</skos:definition>
        <skos:prefLabel xml:lang="en">Loss of nuclear positivity, tumor cells</skos:prefLabel>
    </owl:Class>
    


    <!-- http://www.semanticweb.org/david/ontologies/2013/0/1.3.6.1.4.1.19376.1.8.2.1.1939 -->

    <owl:Class rdf:about="&pathLex;1939">
        <rdfs:subClassOf rdf:resource="&pathLex;99999"/>
        <skos:definition xml:lang="en">Colon-Infiltrating malignant neoplasm-BRAF V600E mutational analysis-Mutant detected</skos:definition>
        <skos:prefLabel xml:lang="en">Mutant detected</skos:prefLabel>
    </owl:Class>
    


    <!-- http://www.semanticweb.org/david/ontologies/2013/0/1.3.6.1.4.1.19376.1.8.2.1.194 -->

    <owl:Class rdf:about="&pathLex;194">
        <rdfs:subClassOf rdf:resource="&pathLex;99999"/>
        <skos:definition xml:lang="en">Liver-Infiltrating malignant neoplasm-Margins involvement</skos:definition>
        <skos:prefLabel xml:lang="en">Margins involvement</skos:prefLabel>
    </owl:Class>
    


    <!-- http://www.semanticweb.org/david/ontologies/2013/0/1.3.6.1.4.1.19376.1.8.2.1.1940 -->

    <owl:Class rdf:about="&pathLex;1940">
        <rdfs:subClassOf rdf:resource="&pathLex;99999"/>
        <skos:definition xml:lang="en">Colon-Infiltrating malignant neoplasm-BRAF V600E mutational analysis-No mutant detected</skos:definition>
        <skos:prefLabel xml:lang="en">No mutant detected</skos:prefLabel>
    </owl:Class>
    


    <!-- http://www.semanticweb.org/david/ontologies/2013/0/1.3.6.1.4.1.19376.1.8.2.1.1941 -->

    <owl:Class rdf:about="&pathLex;1941">
        <rdfs:subClassOf rdf:resource="&pathLex;99999"/>
        <skos:definition xml:lang="en">Colon-Infiltrating malignant neoplasm-KRAS mutational analysis-Intact nuclear positivity, tumor cells</skos:definition>
        <skos:prefLabel xml:lang="en">Intact nuclear positivity, tumor cells</skos:prefLabel>
    </owl:Class>
    


    <!-- http://www.semanticweb.org/david/ontologies/2013/0/1.3.6.1.4.1.19376.1.8.2.1.1942 -->

    <owl:Class rdf:about="&pathLex;1942">
        <rdfs:subClassOf rdf:resource="&pathLex;99999"/>
        <skos:definition xml:lang="en">Colon-Infiltrating malignant neoplasm-KRAS mutational analysis-Loss of nuclear positivity, tumor cells</skos:definition>
        <skos:prefLabel xml:lang="en">Loss of nuclear positivity, tumor cells</skos:prefLabel>
    </owl:Class>
    


    <!-- http://www.semanticweb.org/david/ontologies/2013/0/1.3.6.1.4.1.19376.1.8.2.1.1943 -->

    <owl:Class rdf:about="&pathLex;1943">
        <rdfs:subClassOf rdf:resource="&pathLex;99999"/>
        <skos:definition xml:lang="en">Lung-Infiltrating malignant neoplasm-KRAS mutational analysis-Mutant detected</skos:definition>
        <skos:prefLabel xml:lang="en">Mutant detected</skos:prefLabel>
    </owl:Class>
    


    <!-- http://www.semanticweb.org/david/ontologies/2013/0/1.3.6.1.4.1.19376.1.8.2.1.1944 -->

    <owl:Class rdf:about="&pathLex;1944">
        <rdfs:subClassOf rdf:resource="&pathLex;99999"/>
        <skos:definition xml:lang="en">Lung-Infiltrating malignant neoplasm-KRAS mutational analysis-No mutant detected</skos:definition>
        <skos:prefLabel xml:lang="en">No mutant detected</skos:prefLabel>
    </owl:Class>
    


    <!-- http://www.semanticweb.org/david/ontologies/2013/0/1.3.6.1.4.1.19376.1.8.2.1.1945 -->

    <owl:Class rdf:about="&pathLex;1945">
        <rdfs:subClassOf rdf:resource="&pathLex;99999"/>
        <skos:definition xml:lang="en">Colon-Infiltrating malignant neoplasm-Mismatch Repair Proteins-PMS2 (Immunohistochemistry Study)-Intact nuclear positivity, tumor cells</skos:definition>
        <skos:prefLabel xml:lang="en">Intact nuclear positivity, tumor cells</skos:prefLabel>
    </owl:Class>
    


    <!-- http://www.semanticweb.org/david/ontologies/2013/0/1.3.6.1.4.1.19376.1.8.2.1.1946 -->

    <owl:Class rdf:about="&pathLex;1946">
        <rdfs:subClassOf rdf:resource="&pathLex;99999"/>
        <skos:definition xml:lang="en">Colon-Infiltrating malignant neoplasm-Mismatch Repair Proteins-PMS2 (Immunohistochemistry Study)-Loss of nuclear positivity, tumor cells</skos:definition>
        <skos:prefLabel xml:lang="en">Loss of nuclear positivity, tumor cells</skos:prefLabel>
    </owl:Class>
    


    <!-- http://www.semanticweb.org/david/ontologies/2013/0/1.3.6.1.4.1.19376.1.8.2.1.1947 -->

    <owl:Class rdf:about="&pathLex;1947">
        <rdfs:subClassOf rdf:resource="&pathLex;99999"/>
        <skos:definition xml:lang="en">Colon-Infiltrating malignant neoplasm-Extent-No evidence of primary tumor</skos:definition>
        <skos:prefLabel xml:lang="en">No evidence of primary tumor</skos:prefLabel>
    </owl:Class>
    


    <!-- http://www.semanticweb.org/david/ontologies/2013/0/1.3.6.1.4.1.19376.1.8.2.1.1948 -->

    <owl:Class rdf:about="&pathLex;1948">
        <rdfs:subClassOf rdf:resource="&pathLex;99999"/>
        <skos:definition xml:lang="en">Colon-Infiltrating malignant neoplasm-Extent-Intramucosal carcinoma, invasion of lamina propria</skos:definition>
        <skos:prefLabel xml:lang="en">Intramucosal carcinoma, invasion of lamina propria</skos:prefLabel>
    </owl:Class>
    


    <!-- http://www.semanticweb.org/david/ontologies/2013/0/1.3.6.1.4.1.19376.1.8.2.1.1949 -->

    <owl:Class rdf:about="&pathLex;1949">
        <rdfs:subClassOf rdf:resource="&pathLex;99999"/>
        <skos:definition xml:lang="en">Colon-Infiltrating malignant neoplasm-Extent-Tumor invades submucosa</skos:definition>
        <skos:prefLabel xml:lang="en">Tumor invades submucosa</skos:prefLabel>
    </owl:Class>
    


    <!-- http://www.semanticweb.org/david/ontologies/2013/0/1.3.6.1.4.1.19376.1.8.2.1.195 -->

    <owl:Class rdf:about="&pathLex;195">
        <rdfs:subClassOf rdf:resource="&pathLex;99999"/>
        <skos:prefLabel xml:lang="en">Distance of lesion from closest uninvolved margin</skos:prefLabel>
        <skos:definition xml:lang="en">Liver-Infiltrating malignant neoplasm-Distance of lesion from closest uninvolved margin</skos:definition>
    </owl:Class>
    


    <!-- http://www.semanticweb.org/david/ontologies/2013/0/1.3.6.1.4.1.19376.1.8.2.1.1950 -->

    <owl:Class rdf:about="&pathLex;1950">
        <rdfs:subClassOf rdf:resource="&pathLex;99999"/>
        <skos:definition xml:lang="en">Colon-Infiltrating malignant neoplasm-Extent-Tumor invades muscularis propria</skos:definition>
        <skos:prefLabel xml:lang="en">Tumor invades muscularis propria</skos:prefLabel>
    </owl:Class>
    


    <!-- http://www.semanticweb.org/david/ontologies/2013/0/1.3.6.1.4.1.19376.1.8.2.1.1951 -->

    <owl:Class rdf:about="&pathLex;1951">
        <rdfs:subClassOf rdf:resource="&pathLex;99999"/>
        <skos:definition xml:lang="en">Colon-Infiltrating malignant neoplasm-Extent-Tumor invades through the muscularis propria into the subserosal adipose tissue or the nonperitonealized pericolic or perirectal soft tissues but does not extend to the serosal surface</skos:definition>
        <skos:prefLabel xml:lang="en">Tumor invades through the muscularis propria into the subserosal adipose tissue or the nonperitonealized pericolic or perirectal soft tissues but does not extend to the serosal surface</skos:prefLabel>
    </owl:Class>
    


    <!-- http://www.semanticweb.org/david/ontologies/2013/0/1.3.6.1.4.1.19376.1.8.2.1.1952 -->

    <owl:Class rdf:about="&pathLex;1952">
        <rdfs:subClassOf rdf:resource="&pathLex;99999"/>
        <skos:definition xml:lang="en">Colon-Infiltrating malignant neoplasm-Extent-Tumor penetrates to the surface of the visceral peritoneum (serosa)</skos:definition>
        <skos:prefLabel xml:lang="en">Tumor penetrates to the surface of the visceral peritoneum (serosa)</skos:prefLabel>
    </owl:Class>
    


    <!-- http://www.semanticweb.org/david/ontologies/2013/0/1.3.6.1.4.1.19376.1.8.2.1.1953 -->

    <owl:Class rdf:about="&pathLex;1953">
        <rdfs:subClassOf rdf:resource="&pathLex;99999"/>
        <skos:definition xml:lang="en">Colon-Infiltrating malignant neoplasm-Extent-Tumor is adherent to other organs or structures (specify: _________________)</skos:definition>
        <skos:prefLabel xml:lang="en">Tumor is adherent to other organs or structures (specify: _________________)</skos:prefLabel>
    </owl:Class>
    


    <!-- http://www.semanticweb.org/david/ontologies/2013/0/1.3.6.1.4.1.19376.1.8.2.1.1954 -->

    <owl:Class rdf:about="&pathLex;1954">
        <rdfs:subClassOf rdf:resource="&pathLex;99999"/>
        <skos:definition xml:lang="en">Colon-Infiltrating malignant neoplasm-Extent-Tumor directly invades adjacent structures (specify: __________________)</skos:definition>
        <skos:prefLabel xml:lang="en">Tumor directly invades adjacent structures (specify: __________________)</skos:prefLabel>
    </owl:Class>
    


    <!-- http://www.semanticweb.org/david/ontologies/2013/0/1.3.6.1.4.1.19376.1.8.2.1.1955 -->

    <owl:Class rdf:about="&pathLex;1955">
        <rdfs:subClassOf rdf:resource="&pathLex;99999"/>
        <skos:definition xml:lang="en">Colon-Infiltrating malignant neoplasm-Extent-Tumor penetrates to the surface of the visceral peritoneum (serosa) and directly invades adjacent structures (specify: _____________________)</skos:definition>
        <skos:prefLabel xml:lang="en">Tumor penetrates to the surface of the visceral peritoneum (serosa) and directly invades adjacent structures (specify: _____________________)</skos:prefLabel>
    </owl:Class>
    


    <!-- http://www.semanticweb.org/david/ontologies/2013/0/1.3.6.1.4.1.19376.1.8.2.1.1956 -->

    <owl:Class rdf:about="&pathLex;1956">
        <rdfs:subClassOf rdf:resource="&pathLex;99999"/>
        <skos:prefLabel xml:lang="en">&lt;50% myometrial invasion</skos:prefLabel>
        <skos:definition xml:lang="en">Endometrium-Infiltrating malignant neoplasm-Extent-&lt;50% myometrial invasion</skos:definition>
    </owl:Class>
    


    <!-- http://www.semanticweb.org/david/ontologies/2013/0/1.3.6.1.4.1.19376.1.8.2.1.1957 -->

    <owl:Class rdf:about="&pathLex;1957">
        <rdfs:subClassOf rdf:resource="&pathLex;99999"/>
        <skos:prefLabel xml:lang="en">&gt;=50% myometrial invasion</skos:prefLabel>
        <skos:definition xml:lang="en">Endometrium-Infiltrating malignant neoplasm-Extent-&gt;=50% myometrial invasion</skos:definition>
    </owl:Class>
    


    <!-- http://www.semanticweb.org/david/ontologies/2013/0/1.3.6.1.4.1.19376.1.8.2.1.1959 -->

    <owl:Class rdf:about="&pathLex;1959">
        <rdfs:subClassOf rdf:resource="&pathLex;99999"/>
        <skos:definition xml:lang="en">Colon-Infiltrating malignant neoplasm-Histologic grade (Two-Tier Grading System)-Low-grade (well-differentiated to moderately differentiated)</skos:definition>
        <skos:prefLabel xml:lang="en">Low-grade (well-differentiated to moderately differentiated)</skos:prefLabel>
    </owl:Class>
    


    <!-- http://www.semanticweb.org/david/ontologies/2013/0/1.3.6.1.4.1.19376.1.8.2.1.196 -->

    <owl:Class rdf:about="&pathLex;196">
        <rdfs:subClassOf rdf:resource="&pathLex;99999"/>
        <skos:definition xml:lang="en">Liver-Infiltrating malignant neoplasm-Lymph-vascular invasion</skos:definition>
        <skos:prefLabel xml:lang="en">Lymph-vascular invasion</skos:prefLabel>
    </owl:Class>
    


    <!-- http://www.semanticweb.org/david/ontologies/2013/0/1.3.6.1.4.1.19376.1.8.2.1.1960 -->

    <owl:Class rdf:about="&pathLex;1960">
        <rdfs:subClassOf rdf:resource="&pathLex;99999"/>
        <skos:definition xml:lang="en">Colon-Infiltrating malignant neoplasm-Histologic grade (Two-Tier Grading System)-High-grade (poorly differentiated to undifferentiated)</skos:definition>
        <skos:prefLabel xml:lang="en">High-grade (poorly differentiated to undifferentiated)</skos:prefLabel>
    </owl:Class>
    


    <!-- http://www.semanticweb.org/david/ontologies/2013/0/1.3.6.1.4.1.19376.1.8.2.1.1961 -->

    <owl:Class rdf:about="&pathLex;1961">
        <rdfs:subClassOf rdf:resource="&pathLex;486"/>
        <skos:definition xml:lang="en">Cervix-Infiltrating malignant neoplasm-Histologic grade (WHO)-G1: Well differentiated</skos:definition>
        <skos:prefLabel xml:lang="en">G1: Well differentiated</skos:prefLabel>
    </owl:Class>
    


    <!-- http://www.semanticweb.org/david/ontologies/2013/0/1.3.6.1.4.1.19376.1.8.2.1.1962 -->

    <owl:Class rdf:about="&pathLex;1962">
        <rdfs:subClassOf rdf:resource="&pathLex;486"/>
        <skos:definition xml:lang="en">Cervix-Infiltrating malignant neoplasm-Histologic grade (WHO)-G2: Moderately differentiated</skos:definition>
        <skos:prefLabel xml:lang="en">G2: Moderately differentiated</skos:prefLabel>
    </owl:Class>
    


    <!-- http://www.semanticweb.org/david/ontologies/2013/0/1.3.6.1.4.1.19376.1.8.2.1.1963 -->

    <owl:Class rdf:about="&pathLex;1963">
        <rdfs:subClassOf rdf:resource="&pathLex;486"/>
        <skos:definition xml:lang="en">Cervix-Infiltrating malignant neoplasm-Histologic grade (WHO)-G3: Poorly differentiated</skos:definition>
        <skos:prefLabel xml:lang="en">G3: Poorly differentiated</skos:prefLabel>
    </owl:Class>
    


    <!-- http://www.semanticweb.org/david/ontologies/2013/0/1.3.6.1.4.1.19376.1.8.2.1.1964 -->

    <owl:Class rdf:about="&pathLex;1964">
        <rdfs:subClassOf rdf:resource="&pathLex;99999"/>
        <skos:definition xml:lang="en">Endometrium-Infiltrating malignant neoplasm-Histologic grade (WHO)-G1: Well differentiated</skos:definition>
        <skos:prefLabel xml:lang="en">G1: Well differentiated</skos:prefLabel>
    </owl:Class>
    


    <!-- http://www.semanticweb.org/david/ontologies/2013/0/1.3.6.1.4.1.19376.1.8.2.1.1965 -->

    <owl:Class rdf:about="&pathLex;1965">
        <rdfs:subClassOf rdf:resource="&pathLex;99999"/>
        <skos:definition xml:lang="en">Endometrium-Infiltrating malignant neoplasm-Histologic grade (WHO)-G2: Moderately differentiated</skos:definition>
        <skos:prefLabel xml:lang="en">G2: Moderately differentiated</skos:prefLabel>
    </owl:Class>
    


    <!-- http://www.semanticweb.org/david/ontologies/2013/0/1.3.6.1.4.1.19376.1.8.2.1.1966 -->

    <owl:Class rdf:about="&pathLex;1966">
        <rdfs:subClassOf rdf:resource="&pathLex;99999"/>
        <skos:definition xml:lang="en">Endometrium-Infiltrating malignant neoplasm-Histologic grade (WHO)-G3: Poorly differentiated</skos:definition>
        <skos:prefLabel xml:lang="en">G3: Poorly differentiated</skos:prefLabel>
    </owl:Class>
    


    <!-- http://www.semanticweb.org/david/ontologies/2013/0/1.3.6.1.4.1.19376.1.8.2.1.1967 -->

    <owl:Class rdf:about="&pathLex;1967">
        <rdfs:subClassOf rdf:resource="&pathLex;99999"/>
        <skos:definition xml:lang="en">Esophagus-Infiltrating malignant neoplasm-Histologic grade (WHO)-G1: Well differentiated</skos:definition>
        <skos:prefLabel xml:lang="en">G1: Well differentiated</skos:prefLabel>
    </owl:Class>
    


    <!-- http://www.semanticweb.org/david/ontologies/2013/0/1.3.6.1.4.1.19376.1.8.2.1.1968 -->

    <owl:Class rdf:about="&pathLex;1968">
        <rdfs:subClassOf rdf:resource="&pathLex;99999"/>
        <skos:definition xml:lang="en">Esophagus-Infiltrating malignant neoplasm-Histologic grade (WHO)-G2: Moderately differentiated</skos:definition>
        <skos:prefLabel xml:lang="en">G2: Moderately differentiated</skos:prefLabel>
    </owl:Class>
    


    <!-- http://www.semanticweb.org/david/ontologies/2013/0/1.3.6.1.4.1.19376.1.8.2.1.1969 -->

    <owl:Class rdf:about="&pathLex;1969">
        <rdfs:subClassOf rdf:resource="&pathLex;99999"/>
        <skos:definition xml:lang="en">Esophagus-Infiltrating malignant neoplasm-Histologic grade (WHO)-G3: Poorly differentiated</skos:definition>
        <skos:prefLabel xml:lang="en">G3: Poorly differentiated</skos:prefLabel>
    </owl:Class>
    


    <!-- http://www.semanticweb.org/david/ontologies/2013/0/1.3.6.1.4.1.19376.1.8.2.1.197 -->

    <owl:Class rdf:about="&pathLex;197">
        <rdfs:subClassOf rdf:resource="&pathLex;99999"/>
        <skos:prefLabel xml:lang="en">Extent</skos:prefLabel>
        <skos:definition xml:lang="en">Liver-Infiltrating malignant neoplasm-Extent</skos:definition>
    </owl:Class>
    


    <!-- http://www.semanticweb.org/david/ontologies/2013/0/1.3.6.1.4.1.19376.1.8.2.1.1970 -->

    <owl:Class rdf:about="&pathLex;1970">
        <rdfs:subClassOf rdf:resource="&pathLex;99999"/>
        <skos:definition xml:lang="en">Esophagus-Infiltrating malignant neoplasm-Histologic grade (WHO)-G4: Undifferentiated</skos:definition>
        <skos:prefLabel xml:lang="en">G4: Undifferentiated</skos:prefLabel>
    </owl:Class>
    


    <!-- http://www.semanticweb.org/david/ontologies/2013/0/1.3.6.1.4.1.19376.1.8.2.1.1971 -->

    <owl:Class rdf:about="&pathLex;1971">
        <rdfs:subClassOf rdf:resource="&pathLex;99999"/>
        <skos:prefLabel xml:lang="en">G1: Well differentiated</skos:prefLabel>
        <skos:definition xml:lang="en">Ovary-Infiltrating malignant neoplasm-Histologic grade (WHO)-G1: Well differentiated</skos:definition>
    </owl:Class>
    


    <!-- http://www.semanticweb.org/david/ontologies/2013/0/1.3.6.1.4.1.19376.1.8.2.1.1972 -->

    <owl:Class rdf:about="&pathLex;1972">
        <rdfs:subClassOf rdf:resource="&pathLex;99999"/>
        <skos:prefLabel xml:lang="en">G2: Moderately differentiated</skos:prefLabel>
        <skos:definition xml:lang="en">Ovary-Infiltrating malignant neoplasm-Histologic grade (WHO)-G2: Moderately differentiated</skos:definition>
    </owl:Class>
    


    <!-- http://www.semanticweb.org/david/ontologies/2013/0/1.3.6.1.4.1.19376.1.8.2.1.1973 -->

    <owl:Class rdf:about="&pathLex;1973">
        <rdfs:subClassOf rdf:resource="&pathLex;99999"/>
        <skos:prefLabel xml:lang="en">G3: Poorly differentiated</skos:prefLabel>
        <skos:definition xml:lang="en">Ovary-Infiltrating malignant neoplasm-Histologic grade (WHO)-G3: Poorly differentiated</skos:definition>
    </owl:Class>
    


    <!-- http://www.semanticweb.org/david/ontologies/2013/0/1.3.6.1.4.1.19376.1.8.2.1.1974 -->

    <owl:Class rdf:about="&pathLex;1974">
        <rdfs:subClassOf rdf:resource="&pathLex;99999"/>
        <skos:prefLabel xml:lang="en">G1: Well differentiated</skos:prefLabel>
        <skos:definition xml:lang="en">Lung-Infiltrating malignant neoplasm-Histologic grade (WHO)-G1: Well differentiated</skos:definition>
    </owl:Class>
    


    <!-- http://www.semanticweb.org/david/ontologies/2013/0/1.3.6.1.4.1.19376.1.8.2.1.1975 -->

    <owl:Class rdf:about="&pathLex;1975">
        <rdfs:subClassOf rdf:resource="&pathLex;99999"/>
        <skos:prefLabel xml:lang="en">G2: Moderately differentiated</skos:prefLabel>
        <skos:definition xml:lang="en">Lung-Infiltrating malignant neoplasm-Histologic grade (WHO)-G2: Moderately differentiated</skos:definition>
    </owl:Class>
    


    <!-- http://www.semanticweb.org/david/ontologies/2013/0/1.3.6.1.4.1.19376.1.8.2.1.1976 -->

    <owl:Class rdf:about="&pathLex;1976">
        <rdfs:subClassOf rdf:resource="&pathLex;99999"/>
        <skos:prefLabel xml:lang="en">G3: Poorly differentiated</skos:prefLabel>
        <skos:definition xml:lang="en">Lung-Infiltrating malignant neoplasm-Histologic grade (WHO)-G3: Poorly differentiated</skos:definition>
    </owl:Class>
    


    <!-- http://www.semanticweb.org/david/ontologies/2013/0/1.3.6.1.4.1.19376.1.8.2.1.1977 -->

    <owl:Class rdf:about="&pathLex;1977">
        <rdfs:subClassOf rdf:resource="&pathLex;99999"/>
        <skos:prefLabel xml:lang="en">G4: Undifferentiated</skos:prefLabel>
        <skos:definition xml:lang="en">Lung-Infiltrating malignant neoplasm-Histologic grade (WHO)-G4: Undifferentiated</skos:definition>
    </owl:Class>
    


    <!-- http://www.semanticweb.org/david/ontologies/2013/0/1.3.6.1.4.1.19376.1.8.2.1.1978 -->

    <owl:Class rdf:about="&pathLex;1978">
        <rdfs:subClassOf rdf:resource="&pathLex;99999"/>
        <skos:prefLabel xml:lang="en">G1: Well differentiated</skos:prefLabel>
        <skos:definition xml:lang="en">Thyroid-Infiltrating malignant neoplasm-Histologic grade (WHO)-G1: Well differentiated</skos:definition>
    </owl:Class>
    


    <!-- http://www.semanticweb.org/david/ontologies/2013/0/1.3.6.1.4.1.19376.1.8.2.1.1979 -->

    <owl:Class rdf:about="&pathLex;1979">
        <rdfs:subClassOf rdf:resource="&pathLex;99999"/>
        <skos:prefLabel xml:lang="en">G2: Moderately differentiated</skos:prefLabel>
        <skos:definition xml:lang="en">Thyroid-Infiltrating malignant neoplasm-Histologic grade (WHO)-G2: Moderately differentiated</skos:definition>
    </owl:Class>
    


    <!-- http://www.semanticweb.org/david/ontologies/2013/0/1.3.6.1.4.1.19376.1.8.2.1.198 -->

    <owl:Class rdf:about="&pathLex;198">
        <rdfs:subClassOf rdf:resource="&pathLex;99999"/>
        <skos:definition xml:lang="en">Liver-Infiltrating malignant neoplasm-Perineural invasion</skos:definition>
        <skos:prefLabel xml:lang="en">Perineural invasion</skos:prefLabel>
    </owl:Class>
    


    <!-- http://www.semanticweb.org/david/ontologies/2013/0/1.3.6.1.4.1.19376.1.8.2.1.1980 -->

    <owl:Class rdf:about="&pathLex;1980">
        <rdfs:subClassOf rdf:resource="&pathLex;99999"/>
        <skos:prefLabel xml:lang="en">G3: Poorly differentiated</skos:prefLabel>
        <skos:definition xml:lang="en">Thyroid-Infiltrating malignant neoplasm-Histologic grade (WHO)-G3: Poorly differentiated</skos:definition>
    </owl:Class>
    


    <!-- http://www.semanticweb.org/david/ontologies/2013/0/1.3.6.1.4.1.19376.1.8.2.1.1981 -->

    <owl:Class rdf:about="&pathLex;1981">
        <rdfs:subClassOf rdf:resource="&pathLex;99999"/>
        <skos:prefLabel xml:lang="en">G4: Undifferentiated</skos:prefLabel>
        <skos:definition xml:lang="en">Thyroid-Infiltrating malignant neoplasm-Histologic grade (WHO)-G4: Undifferentiated</skos:definition>
    </owl:Class>
    


    <!-- http://www.semanticweb.org/david/ontologies/2013/0/1.3.6.1.4.1.19376.1.8.2.1.1984 -->

    <owl:Class rdf:about="&pathLex;1984">
        <rdfs:subClassOf rdf:resource="&pathLex;99999"/>
        <skos:definition xml:lang="en">Skin (melanoma)-Infiltrating malignant neoplasm-Lymph node site-Subcapsular</skos:definition>
        <skos:prefLabel xml:lang="en">Subcapsular</skos:prefLabel>
    </owl:Class>
    


    <!-- http://www.semanticweb.org/david/ontologies/2013/0/1.3.6.1.4.1.19376.1.8.2.1.1985 -->

    <owl:Class rdf:about="&pathLex;1985">
        <rdfs:subClassOf rdf:resource="&pathLex;99999"/>
        <skos:prefLabel xml:lang="en">Intramedullary</skos:prefLabel>
        <skos:definition xml:lang="en">Skin (melanoma)-Infiltrating malignant neoplasm-Lymph node site-Intramedullary</skos:definition>
    </owl:Class>
    


    <!-- http://www.semanticweb.org/david/ontologies/2013/0/1.3.6.1.4.1.19376.1.8.2.1.1986 -->

    <owl:Class rdf:about="&pathLex;1986">
        <rdfs:subClassOf rdf:resource="&pathLex;99999"/>
        <skos:definition xml:lang="en">Skin (melanoma)-Infiltrating malignant neoplasm-Lymph node site-Subcapsular and intramedullary</skos:definition>
        <skos:prefLabel xml:lang="en">Subcapsular and intramedullary</skos:prefLabel>
    </owl:Class>
    


    <!-- http://www.semanticweb.org/david/ontologies/2013/0/1.3.6.1.4.1.19376.1.8.2.1.1987 -->

    <owl:Class rdf:about="&pathLex;1987">
        <rdfs:subClassOf rdf:resource="&pathLex;423"/>
        <skos:definition xml:lang="en">Breast-Infiltrating malignant neoplasm-Lymph node site-Supraclavicular</skos:definition>
        <skos:prefLabel xml:lang="en">Supraclavicular</skos:prefLabel>
    </owl:Class>
    


    <!-- http://www.semanticweb.org/david/ontologies/2013/0/1.3.6.1.4.1.19376.1.8.2.1.1988 -->

    <owl:Class rdf:about="&pathLex;1988">
        <rdfs:subClassOf rdf:resource="&pathLex;487"/>
        <skos:definition xml:lang="en">Cervix-Infiltrating malignant neoplasm-Margin site-Endocervical Margin</skos:definition>
        <skos:prefLabel xml:lang="en">Endocervical Margin</skos:prefLabel>
    </owl:Class>
    


    <!-- http://www.semanticweb.org/david/ontologies/2013/0/1.3.6.1.4.1.19376.1.8.2.1.1989 -->

    <owl:Class rdf:about="&pathLex;1989">
        <rdfs:subClassOf rdf:resource="&pathLex;487"/>
        <skos:definition xml:lang="en">Cervix-Infiltrating malignant neoplasm-Margin site-Exocervical Margin</skos:definition>
        <skos:prefLabel xml:lang="en">Exocervical Margin</skos:prefLabel>
    </owl:Class>
    


    <!-- http://www.semanticweb.org/david/ontologies/2013/0/1.3.6.1.4.1.19376.1.8.2.1.199 -->

    <owl:Class rdf:about="&pathLex;199">
        <rdfs:subClassOf rdf:resource="&pathLex;99999"/>
        <skos:prefLabel xml:lang="en">Lesion site</skos:prefLabel>
        <skos:definition xml:lang="en">Liver-Infiltrating malignant neoplasm-Lesion site</skos:definition>
    </owl:Class>
    


    <!-- http://www.semanticweb.org/david/ontologies/2013/0/1.3.6.1.4.1.19376.1.8.2.1.1990 -->

    <owl:Class rdf:about="&pathLex;1990">
        <rdfs:subClassOf rdf:resource="&pathLex;487"/>
        <skos:definition xml:lang="en">Cervix-Infiltrating malignant neoplasm-Margin site-Deep Margin</skos:definition>
        <skos:prefLabel xml:lang="en">Deep Margin</skos:prefLabel>
    </owl:Class>
    


    <!-- http://www.semanticweb.org/david/ontologies/2013/0/1.3.6.1.4.1.19376.1.8.2.1.1991 -->

    <owl:Class rdf:about="&pathLex;1991">
        <rdfs:subClassOf rdf:resource="&pathLex;99999"/>
        <skos:definition xml:lang="en">Colon-Infiltrating malignant neoplasm-Margin site-Deep Margin (Stalk Margin)</skos:definition>
        <skos:prefLabel xml:lang="en">Deep Margin (Stalk Margin)</skos:prefLabel>
    </owl:Class>
    


    <!-- http://www.semanticweb.org/david/ontologies/2013/0/1.3.6.1.4.1.19376.1.8.2.1.1992 -->

    <owl:Class rdf:about="&pathLex;1992">
        <rdfs:subClassOf rdf:resource="&pathLex;99999"/>
        <skos:definition xml:lang="en">Colon-Infiltrating malignant neoplasm-Margin site-Mucosal/Lateral Margin (for non-circumferential transanal disk excision)</skos:definition>
        <skos:prefLabel xml:lang="en">Mucosal/Lateral Margin (for non-circumferential transanal disk excision)</skos:prefLabel>
    </owl:Class>
    


    <!-- http://www.semanticweb.org/david/ontologies/2013/0/1.3.6.1.4.1.19376.1.8.2.1.1993 -->

    <owl:Class rdf:about="&pathLex;1993">
        <rdfs:subClassOf rdf:resource="&pathLex;99999"/>
        <skos:prefLabel xml:lang="en">Circumferential (Radial) or Mesenteric Margin</skos:prefLabel>
        <skos:definition xml:lang="en">Colon-Infiltrating malignant neoplasm-Margin site-Circumferential (Radial) or Mesenteric Margin</skos:definition>
    </owl:Class>
    


    <!-- http://www.semanticweb.org/david/ontologies/2013/0/1.3.6.1.4.1.19376.1.8.2.1.1994 -->

    <owl:Class rdf:about="&pathLex;1994">
        <rdfs:subClassOf rdf:resource="&pathLex;99999"/>
        <skos:prefLabel xml:lang="en">Omental (Radial) Margins</skos:prefLabel>
        <skos:definition xml:lang="en">Stomach-Infiltrating malignant neoplasm-Margin site-Omental (Radial) Margins</skos:definition>
    </owl:Class>
    


    <!-- http://www.semanticweb.org/david/ontologies/2013/0/1.3.6.1.4.1.19376.1.8.2.1.1995 -->

    <owl:Class rdf:about="&pathLex;1995">
        <rdfs:subClassOf rdf:resource="&pathLex;99999"/>
        <skos:prefLabel xml:lang="en">Deep Margin (applies to endoscopic resections)</skos:prefLabel>
        <skos:definition xml:lang="en">Stomach-Infiltrating malignant neoplasm-Margin site-Deep Margin (applies to endoscopic resections)</skos:definition>
    </owl:Class>
    


    <!-- http://www.semanticweb.org/david/ontologies/2013/0/1.3.6.1.4.1.19376.1.8.2.1.1996 -->

    <owl:Class rdf:about="&pathLex;1996">
        <rdfs:subClassOf rdf:resource="&pathLex;99999"/>
        <skos:definition xml:lang="en">Liver-Infiltrating malignant neoplasm-Margin site-Parenchymal margin</skos:definition>
        <skos:prefLabel xml:lang="en">Parenchymal margin</skos:prefLabel>
    </owl:Class>
    


    <!-- http://www.semanticweb.org/david/ontologies/2013/0/1.3.6.1.4.1.19376.1.8.2.1.1997 -->

    <owl:Class rdf:about="&pathLex;1997">
        <rdfs:subClassOf rdf:resource="&pathLex;99999"/>
        <skos:definition xml:lang="en">Liver-Infiltrating malignant neoplasm-Margin site-Other margin</skos:definition>
        <skos:prefLabel xml:lang="en">Other margin</skos:prefLabel>
    </owl:Class>
    


    <!-- http://www.semanticweb.org/david/ontologies/2013/0/1.3.6.1.4.1.19376.1.8.2.1.1998 -->

    <owl:Class rdf:about="&pathLex;1998">
        <rdfs:subClassOf rdf:resource="&pathLex;99999"/>
        <skos:prefLabel xml:lang="en">Circumferential (Adventitial) Margin (esophagectomy or esophagogastrectomy specimens)</skos:prefLabel>
        <skos:definition xml:lang="en">Esophagus-Infiltrating malignant neoplasm-Margin site-Circumferential (Adventitial) Margin (esophagectomy or esophagogastrectomy specimens)</skos:definition>
    </owl:Class>
    


    <!-- http://www.semanticweb.org/david/ontologies/2013/0/1.3.6.1.4.1.19376.1.8.2.1.1999 -->

    <owl:Class rdf:about="&pathLex;1999">
        <rdfs:subClassOf rdf:resource="&pathLex;99999"/>
        <skos:prefLabel xml:lang="en">Deep Margin (endoscopic resection specimens)</skos:prefLabel>
        <skos:definition xml:lang="en">Esophagus-Infiltrating malignant neoplasm-Margin site-Deep Margin (endoscopic resection specimens)</skos:definition>
    </owl:Class>
    


    <!-- http://www.semanticweb.org/david/ontologies/2013/0/1.3.6.1.4.1.19376.1.8.2.1.2 -->

    <owl:Class rdf:about="&pathLex;2">
        <rdfs:subClassOf rdf:resource="&pathLex;99999"/>
        <skos:definition xml:lang="en">Generic-Infiltrating malignant neoplasm-Specimen size, largest dimension</skos:definition>
        <skos:prefLabel xml:lang="en">Specimen size, largest dimension</skos:prefLabel>
    </owl:Class>
    


    <!-- http://www.semanticweb.org/david/ontologies/2013/0/1.3.6.1.4.1.19376.1.8.2.1.200 -->

    <owl:Class rdf:about="&pathLex;200">
        <rdfs:subClassOf rdf:resource="&pathLex;99999"/>
        <skos:definition xml:lang="en">Liver-Infiltrating malignant neoplasm-Margin site</skos:definition>
        <skos:prefLabel xml:lang="en">Margin site</skos:prefLabel>
    </owl:Class>
    


    <!-- http://www.semanticweb.org/david/ontologies/2013/0/1.3.6.1.4.1.19376.1.8.2.1.2000 -->

    <owl:Class rdf:about="&pathLex;2000">
        <rdfs:subClassOf rdf:resource="&pathLex;99999"/>
        <skos:definition xml:lang="en">Lung-Infiltrating malignant neoplasm-Margin site-Parietal Pleural Margin</skos:definition>
        <skos:prefLabel xml:lang="en">Parietal Pleural Margin</skos:prefLabel>
    </owl:Class>
    


    <!-- http://www.semanticweb.org/david/ontologies/2013/0/1.3.6.1.4.1.19376.1.8.2.1.2001 -->

    <owl:Class rdf:about="&pathLex;2001">
        <rdfs:subClassOf rdf:resource="&pathLex;99999"/>
        <skos:prefLabel xml:lang="en">Chest Wall Margin</skos:prefLabel>
        <skos:definition xml:lang="en">Lung-Infiltrating malignant neoplasm-Margin site-Chest Wall Margin</skos:definition>
    </owl:Class>
    


    <!-- http://www.semanticweb.org/david/ontologies/2013/0/1.3.6.1.4.1.19376.1.8.2.1.2008 -->

    <owl:Class rdf:about="&pathLex;2008">
        <rdfs:subClassOf rdf:resource="&pathLex;99999"/>
        <skos:definition xml:lang="en">Kidney-Infiltrating malignant neoplasm-Margin site-Renal capsular margin (partial nephrectomy only)</skos:definition>
        <skos:prefLabel xml:lang="en">Renal capsular margin (partial nephrectomy only)</skos:prefLabel>
    </owl:Class>
    


    <!-- http://www.semanticweb.org/david/ontologies/2013/0/1.3.6.1.4.1.19376.1.8.2.1.2009 -->

    <owl:Class rdf:about="&pathLex;2009">
        <rdfs:subClassOf rdf:resource="&pathLex;99999"/>
        <skos:definition xml:lang="en">Kidney-Infiltrating malignant neoplasm-Margin site-Perinephric fat margin (partial nephrectomy only)</skos:definition>
        <skos:prefLabel xml:lang="en">Perinephric fat margin (partial nephrectomy only)</skos:prefLabel>
    </owl:Class>
    


    <!-- http://www.semanticweb.org/david/ontologies/2013/0/1.3.6.1.4.1.19376.1.8.2.1.201 -->

    <owl:Class rdf:about="&pathLex;201">
        <rdfs:subClassOf rdf:resource="&pathLex;99999"/>
        <skos:definition xml:lang="en">Liver-Infiltrating malignant neoplasm-Number of lymph nodes involved</skos:definition>
        <skos:prefLabel xml:lang="en">Number of lymph nodes involved</skos:prefLabel>
    </owl:Class>
    


    <!-- http://www.semanticweb.org/david/ontologies/2013/0/1.3.6.1.4.1.19376.1.8.2.1.2010 -->

    <owl:Class rdf:about="&pathLex;2010">
        <rdfs:subClassOf rdf:resource="&pathLex;99999"/>
        <skos:prefLabel xml:lang="en">Gerota’s fascial margin</skos:prefLabel>
        <skos:definition xml:lang="en">Kidney-Infiltrating malignant neoplasm-Margin site-Gerota’s fascial margin</skos:definition>
    </owl:Class>
    


    <!-- http://www.semanticweb.org/david/ontologies/2013/0/1.3.6.1.4.1.19376.1.8.2.1.2011 -->

    <owl:Class rdf:about="&pathLex;2011">
        <rdfs:subClassOf rdf:resource="&pathLex;99999"/>
        <skos:definition xml:lang="en">Kidney-Infiltrating malignant neoplasm-Margin site-Ureteral margin</skos:definition>
        <skos:prefLabel xml:lang="en">Ureteral margin</skos:prefLabel>
    </owl:Class>
    


    <!-- http://www.semanticweb.org/david/ontologies/2013/0/1.3.6.1.4.1.19376.1.8.2.1.2012 -->

    <owl:Class rdf:about="&pathLex;2012">
        <rdfs:subClassOf rdf:resource="&pathLex;128"/>
        <skos:definition xml:lang="en">Cervix-Infiltrating malignant neoplasm-Lesion site-Right superior quadrant (12 to 3 o’clock)</skos:definition>
        <skos:prefLabel xml:lang="en">Right superior quadrant (12 to 3 o’clock)</skos:prefLabel>
    </owl:Class>
    


    <!-- http://www.semanticweb.org/david/ontologies/2013/0/1.3.6.1.4.1.19376.1.8.2.1.2013 -->

    <owl:Class rdf:about="&pathLex;2013">
        <rdfs:subClassOf rdf:resource="&pathLex;128"/>
        <skos:definition xml:lang="en">Cervix-Infiltrating malignant neoplasm-Lesion site-Right inferior quadrant (3 to 6 o’clock)</skos:definition>
        <skos:prefLabel xml:lang="en">Right inferior quadrant (3 to 6 o’clock)</skos:prefLabel>
    </owl:Class>
    


    <!-- http://www.semanticweb.org/david/ontologies/2013/0/1.3.6.1.4.1.19376.1.8.2.1.2014 -->

    <owl:Class rdf:about="&pathLex;2014">
        <rdfs:subClassOf rdf:resource="&pathLex;128"/>
        <skos:definition xml:lang="en">Cervix-Infiltrating malignant neoplasm-Lesion site-Left inferior quadrant (6 to 9 o’clock)</skos:definition>
        <skos:prefLabel xml:lang="en">Left inferior quadrant (6 to 9 o’clock)</skos:prefLabel>
    </owl:Class>
    


    <!-- http://www.semanticweb.org/david/ontologies/2013/0/1.3.6.1.4.1.19376.1.8.2.1.2015 -->

    <owl:Class rdf:about="&pathLex;2015">
        <rdfs:subClassOf rdf:resource="&pathLex;128"/>
        <skos:definition xml:lang="en">Cervix-Infiltrating malignant neoplasm-Lesion site-Left superior quadrant (9 to 12 o’clock)</skos:definition>
        <skos:prefLabel xml:lang="en">Left superior quadrant (9 to 12 o’clock)</skos:prefLabel>
    </owl:Class>
    


    <!-- http://www.semanticweb.org/david/ontologies/2013/0/1.3.6.1.4.1.19376.1.8.2.1.2016 -->

    <owl:Class rdf:about="&pathLex;2016">
        <rdfs:subClassOf rdf:resource="&pathLex;99999"/>
        <skos:prefLabel xml:lang="en">Cecum</skos:prefLabel>
        <skos:definition xml:lang="en">Colon-Infiltrating malignant neoplasm-Lesion site-Cecum</skos:definition>
    </owl:Class>
    


    <!-- http://www.semanticweb.org/david/ontologies/2013/0/1.3.6.1.4.1.19376.1.8.2.1.2017 -->

    <owl:Class rdf:about="&pathLex;2017">
        <rdfs:subClassOf rdf:resource="&pathLex;99999"/>
        <skos:definition xml:lang="en">Colon-Infiltrating malignant neoplasm-Lesion site-Rectosigmoid</skos:definition>
        <skos:prefLabel xml:lang="en">Rectosigmoid</skos:prefLabel>
    </owl:Class>
    


    <!-- http://www.semanticweb.org/david/ontologies/2013/0/1.3.6.1.4.1.19376.1.8.2.1.2018 -->

    <owl:Class rdf:about="&pathLex;2018">
        <rdfs:subClassOf rdf:resource="&pathLex;99999"/>
        <skos:prefLabel xml:lang="en">Colon, not otherwise specified</skos:prefLabel>
        <skos:definition xml:lang="en">Colon-Infiltrating malignant neoplasm-Lesion site-Colon, not otherwise specified</skos:definition>
    </owl:Class>
    


    <!-- http://www.semanticweb.org/david/ontologies/2013/0/1.3.6.1.4.1.19376.1.8.2.1.2019 -->

    <owl:Class rdf:about="&pathLex;2019">
        <rdfs:subClassOf rdf:resource="&pathLex;99999"/>
        <skos:definition xml:lang="en">Colon-Infiltrating malignant neoplasm-Lesion site-Terminal ileum</skos:definition>
        <skos:prefLabel xml:lang="en">Terminal ileum</skos:prefLabel>
    </owl:Class>
    


    <!-- http://www.semanticweb.org/david/ontologies/2013/0/1.3.6.1.4.1.19376.1.8.2.1.202 -->

    <owl:Class rdf:about="&pathLex;202">
        <rdfs:subClassOf rdf:resource="&pathLex;99999"/>
        <skos:definition xml:lang="en">Liver-Infiltrating malignant neoplasm-Number of lymph nodes examined</skos:definition>
        <skos:prefLabel xml:lang="en">Number of lymph nodes examined</skos:prefLabel>
    </owl:Class>
    


    <!-- http://www.semanticweb.org/david/ontologies/2013/0/1.3.6.1.4.1.19376.1.8.2.1.2020 -->

    <owl:Class rdf:about="&pathLex;2020">
        <rdfs:subClassOf rdf:resource="&pathLex;99999"/>
        <skos:prefLabel xml:lang="en">Appendix</skos:prefLabel>
        <skos:definition xml:lang="en">Colon-Infiltrating malignant neoplasm-Lesion site-Appendix</skos:definition>
    </owl:Class>
    


    <!-- http://www.semanticweb.org/david/ontologies/2013/0/1.3.6.1.4.1.19376.1.8.2.1.2021 -->

    <owl:Class rdf:about="&pathLex;2021">
        <rdfs:subClassOf rdf:resource="&pathLex;99999"/>
        <skos:prefLabel xml:lang="en">Anus</skos:prefLabel>
        <skos:definition xml:lang="en">Colon-Infiltrating malignant neoplasm-Lesion site-Anus</skos:definition>
    </owl:Class>
    


    <!-- http://www.semanticweb.org/david/ontologies/2013/0/1.3.6.1.4.1.19376.1.8.2.1.2022 -->

    <owl:Class rdf:about="&pathLex;2022">
        <rdfs:subClassOf rdf:resource="&pathLex;99999"/>
        <skos:prefLabel xml:lang="en">Anterior endometrium</skos:prefLabel>
        <skos:definition xml:lang="en">Endometrium-Infiltrating malignant neoplasm-Lesion site-Anterior endometrium</skos:definition>
    </owl:Class>
    


    <!-- http://www.semanticweb.org/david/ontologies/2013/0/1.3.6.1.4.1.19376.1.8.2.1.2023 -->

    <owl:Class rdf:about="&pathLex;2023">
        <rdfs:subClassOf rdf:resource="&pathLex;99999"/>
        <skos:definition xml:lang="en">Endometrium-Infiltrating malignant neoplasm-Lesion site-Posterior endometrium</skos:definition>
        <skos:prefLabel xml:lang="en">Posterior endometrium</skos:prefLabel>
    </owl:Class>
    


    <!-- http://www.semanticweb.org/david/ontologies/2013/0/1.3.6.1.4.1.19376.1.8.2.1.2024 -->

    <owl:Class rdf:about="&pathLex;2024">
        <rdfs:subClassOf rdf:resource="&pathLex;99999"/>
        <skos:prefLabel xml:lang="en">Body: Anterior wall</skos:prefLabel>
        <skos:definition xml:lang="en">Stomach-Infiltrating malignant neoplasm-Lesion site-Body: Anterior wall</skos:definition>
    </owl:Class>
    


    <!-- http://www.semanticweb.org/david/ontologies/2013/0/1.3.6.1.4.1.19376.1.8.2.1.2025 -->

    <owl:Class rdf:about="&pathLex;2025">
        <rdfs:subClassOf rdf:resource="&pathLex;99999"/>
        <skos:prefLabel xml:lang="en">Body: Posterior wall</skos:prefLabel>
        <skos:definition xml:lang="en">Stomach-Infiltrating malignant neoplasm-Lesion site-Body: Posterior wall</skos:definition>
    </owl:Class>
    


    <!-- http://www.semanticweb.org/david/ontologies/2013/0/1.3.6.1.4.1.19376.1.8.2.1.2026 -->

    <owl:Class rdf:about="&pathLex;2026">
        <rdfs:subClassOf rdf:resource="&pathLex;99999"/>
        <skos:prefLabel xml:lang="en">Body: Lesser curvature</skos:prefLabel>
        <skos:definition xml:lang="en">Stomach-Infiltrating malignant neoplasm-Lesion site-Body: Lesser curvature</skos:definition>
    </owl:Class>
    


    <!-- http://www.semanticweb.org/david/ontologies/2013/0/1.3.6.1.4.1.19376.1.8.2.1.2027 -->

    <owl:Class rdf:about="&pathLex;2027">
        <rdfs:subClassOf rdf:resource="&pathLex;99999"/>
        <skos:prefLabel xml:lang="en">Body: Greater curvature</skos:prefLabel>
        <skos:definition xml:lang="en">Stomach-Infiltrating malignant neoplasm-Lesion site-Body: Greater curvature</skos:definition>
    </owl:Class>
    


    <!-- http://www.semanticweb.org/david/ontologies/2013/0/1.3.6.1.4.1.19376.1.8.2.1.2028 -->

    <owl:Class rdf:about="&pathLex;2028">
        <rdfs:subClassOf rdf:resource="&pathLex;99999"/>
        <skos:prefLabel xml:lang="en">Antrum: Anterior wall</skos:prefLabel>
        <skos:definition xml:lang="en">Stomach-Infiltrating malignant neoplasm-Lesion site-Antrum: Anterior wall</skos:definition>
    </owl:Class>
    


    <!-- http://www.semanticweb.org/david/ontologies/2013/0/1.3.6.1.4.1.19376.1.8.2.1.2029 -->

    <owl:Class rdf:about="&pathLex;2029">
        <rdfs:subClassOf rdf:resource="&pathLex;99999"/>
        <skos:prefLabel xml:lang="en">Antrum: Posterior wall</skos:prefLabel>
        <skos:definition xml:lang="en">Stomach-Infiltrating malignant neoplasm-Lesion site-Antrum: Posterior wall</skos:definition>
    </owl:Class>
    


    <!-- http://www.semanticweb.org/david/ontologies/2013/0/1.3.6.1.4.1.19376.1.8.2.1.2030 -->

    <owl:Class rdf:about="&pathLex;2030">
        <rdfs:subClassOf rdf:resource="&pathLex;99999"/>
        <skos:prefLabel xml:lang="en">Antrum: Lesser curvature</skos:prefLabel>
        <skos:definition xml:lang="en">Stomach-Infiltrating malignant neoplasm-Lesion site-Antrum: Lesser curvature</skos:definition>
    </owl:Class>
    


    <!-- http://www.semanticweb.org/david/ontologies/2013/0/1.3.6.1.4.1.19376.1.8.2.1.2031 -->

    <owl:Class rdf:about="&pathLex;2031">
        <rdfs:subClassOf rdf:resource="&pathLex;99999"/>
        <skos:prefLabel xml:lang="en">Antrum: Greater curvature</skos:prefLabel>
        <skos:definition xml:lang="en">Stomach-Infiltrating malignant neoplasm-Lesion site-Antrum: Greater curvature</skos:definition>
    </owl:Class>
    


    <!-- http://www.semanticweb.org/david/ontologies/2013/0/1.3.6.1.4.1.19376.1.8.2.1.2032 -->

    <owl:Class rdf:about="&pathLex;2032">
        <rdfs:subClassOf rdf:resource="&pathLex;99999"/>
        <skos:prefLabel xml:lang="en">Fundus: Anterior wall</skos:prefLabel>
        <skos:definition xml:lang="en">Stomach-Infiltrating malignant neoplasm-Lesion site-Fundus: Anterior wall</skos:definition>
    </owl:Class>
    


    <!-- http://www.semanticweb.org/david/ontologies/2013/0/1.3.6.1.4.1.19376.1.8.2.1.2033 -->

    <owl:Class rdf:about="&pathLex;2033">
        <rdfs:subClassOf rdf:resource="&pathLex;99999"/>
        <skos:prefLabel xml:lang="en">Fundus: Posterior wall</skos:prefLabel>
        <skos:definition xml:lang="en">Stomach-Infiltrating malignant neoplasm-Lesion site-Fundus: Posterior wall</skos:definition>
    </owl:Class>
    


    <!-- http://www.semanticweb.org/david/ontologies/2013/0/1.3.6.1.4.1.19376.1.8.2.1.2034 -->

    <owl:Class rdf:about="&pathLex;2034">
        <rdfs:subClassOf rdf:resource="&pathLex;99999"/>
        <skos:prefLabel xml:lang="en">Gallbladder</skos:prefLabel>
        <skos:definition xml:lang="en">Liver-Infiltrating malignant neoplasm-Lesion site-Gallbladder</skos:definition>
    </owl:Class>
    


    <!-- http://www.semanticweb.org/david/ontologies/2013/0/1.3.6.1.4.1.19376.1.8.2.1.2036 -->

    <owl:Class rdf:about="&pathLex;2036">
        <rdfs:subClassOf rdf:resource="&pathLex;99999"/>
        <skos:prefLabel xml:lang="en">Parotid gland</skos:prefLabel>
        <skos:definition xml:lang="en">Salivary gland-Infiltrating malignant neoplasm-Lesion site-Parotid gland</skos:definition>
    </owl:Class>
    


    <!-- http://www.semanticweb.org/david/ontologies/2013/0/1.3.6.1.4.1.19376.1.8.2.1.2037 -->

    <owl:Class rdf:about="&pathLex;2037">
        <rdfs:subClassOf rdf:resource="&pathLex;99999"/>
        <skos:definition xml:lang="en">Salivary gland-Infiltrating malignant neoplasm-Lesion site-Superficial lobe</skos:definition>
        <skos:prefLabel xml:lang="en">Superficial lobe</skos:prefLabel>
    </owl:Class>
    


    <!-- http://www.semanticweb.org/david/ontologies/2013/0/1.3.6.1.4.1.19376.1.8.2.1.2038 -->

    <owl:Class rdf:about="&pathLex;2038">
        <rdfs:subClassOf rdf:resource="&pathLex;99999"/>
        <skos:prefLabel xml:lang="en">Deep lobe</skos:prefLabel>
        <skos:definition xml:lang="en">Salivary gland-Infiltrating malignant neoplasm-Lesion site-Deep lobe</skos:definition>
    </owl:Class>
    


    <!-- http://www.semanticweb.org/david/ontologies/2013/0/1.3.6.1.4.1.19376.1.8.2.1.2039 -->

    <owl:Class rdf:about="&pathLex;2039">
        <rdfs:subClassOf rdf:resource="&pathLex;99999"/>
        <skos:prefLabel xml:lang="en">Entire parotid gland</skos:prefLabel>
        <skos:definition xml:lang="en">Salivary gland-Infiltrating malignant neoplasm-Lesion site-Entire parotid gland</skos:definition>
    </owl:Class>
    


    <!-- http://www.semanticweb.org/david/ontologies/2013/0/1.3.6.1.4.1.19376.1.8.2.1.204 -->

    <owl:Class rdf:about="&pathLex;204">
        <rdfs:subClassOf rdf:resource="&pathLex;99999"/>
        <skos:definition xml:lang="en">Liver-Infiltrating malignant neoplasm-pN</skos:definition>
        <skos:prefLabel xml:lang="en">pN</skos:prefLabel>
    </owl:Class>
    


    <!-- http://www.semanticweb.org/david/ontologies/2013/0/1.3.6.1.4.1.19376.1.8.2.1.2042 -->

    <owl:Class rdf:about="&pathLex;2042">
        <rdfs:subClassOf rdf:resource="&pathLex;99999"/>
        <skos:definition xml:lang="en">Salivary gland-Infiltrating malignant neoplasm-pM-pM1: Distant metastasis - Specify site(s)</skos:definition>
        <skos:prefLabel xml:lang="en">pM1: Distant metastasis - Specify site(s)</skos:prefLabel>
    </owl:Class>
    


    <!-- http://www.semanticweb.org/david/ontologies/2013/0/1.3.6.1.4.1.19376.1.8.2.1.2043 -->

    <owl:Class rdf:about="&pathLex;2043">
        <rdfs:subClassOf rdf:resource="&pathLex;99999"/>
        <skos:prefLabel xml:lang="en">Larynx, supraglottis</skos:prefLabel>
        <skos:definition xml:lang="en">Larynx-Infiltrating malignant neoplasm-Lesion site-Larynx, supraglottis</skos:definition>
    </owl:Class>
    


    <!-- http://www.semanticweb.org/david/ontologies/2013/0/1.3.6.1.4.1.19376.1.8.2.1.2044 -->

    <owl:Class rdf:about="&pathLex;2044">
        <rdfs:subClassOf rdf:resource="&pathLex;99999"/>
        <skos:definition xml:lang="en">Larynx-Infiltrating malignant neoplasm-Lesion site-Lingual aspect</skos:definition>
        <skos:prefLabel xml:lang="en">Lingual aspect</skos:prefLabel>
    </owl:Class>
    


    <!-- http://www.semanticweb.org/david/ontologies/2013/0/1.3.6.1.4.1.19376.1.8.2.1.2045 -->

    <owl:Class rdf:about="&pathLex;2045">
        <rdfs:subClassOf rdf:resource="&pathLex;99999"/>
        <skos:prefLabel xml:lang="en">Laryngeal aspect</skos:prefLabel>
        <skos:definition xml:lang="en">Larynx-Infiltrating malignant neoplasm-Lesion site-Laryngeal aspect</skos:definition>
    </owl:Class>
    


    <!-- http://www.semanticweb.org/david/ontologies/2013/0/1.3.6.1.4.1.19376.1.8.2.1.2046 -->

    <owl:Class rdf:about="&pathLex;2046">
        <rdfs:subClassOf rdf:resource="&pathLex;99999"/>
        <skos:prefLabel xml:lang="en">Larynx, glottis</skos:prefLabel>
        <skos:definition xml:lang="en">Larynx-Infiltrating malignant neoplasm-Lesion site-Larynx, glottis</skos:definition>
    </owl:Class>
    


    <!-- http://www.semanticweb.org/david/ontologies/2013/0/1.3.6.1.4.1.19376.1.8.2.1.2049 -->

    <owl:Class rdf:about="&pathLex;2049">
        <rdfs:subClassOf rdf:resource="&pathLex;99999"/>
        <skos:definition xml:lang="en">Lip, oral cavity-Infiltrating malignant neoplasm-Lesion site-Vermilion border upper lip (qualifier : right, left, medial)</skos:definition>
        <skos:prefLabel xml:lang="en">Vermilion border upper lip (qualifier : right, left, medial)</skos:prefLabel>
    </owl:Class>
    


    <!-- http://www.semanticweb.org/david/ontologies/2013/0/1.3.6.1.4.1.19376.1.8.2.1.2050 -->

    <owl:Class rdf:about="&pathLex;2050">
        <rdfs:subClassOf rdf:resource="&pathLex;99999"/>
        <skos:definition xml:lang="en">Lip, oral cavity-Infiltrating malignant neoplasm-Lesion site-Vermilion border lower lip (qualifier : right, left, medial)</skos:definition>
        <skos:prefLabel xml:lang="en">Vermilion border lower lip (qualifier : right, left, medial)</skos:prefLabel>
    </owl:Class>
    


    <!-- http://www.semanticweb.org/david/ontologies/2013/0/1.3.6.1.4.1.19376.1.8.2.1.2052 -->

    <owl:Class rdf:about="&pathLex;2052">
        <rdfs:subClassOf rdf:resource="&pathLex;99999"/>
        <skos:definition xml:lang="en">Lip, oral cavity-Infiltrating malignant neoplasm-Lesion site-Mucosa of lower lip (qualifier : right, left, medial)</skos:definition>
        <skos:prefLabel xml:lang="en">Mucosa of lower lip (qualifier : right, left, medial)</skos:prefLabel>
    </owl:Class>
    


    <!-- http://www.semanticweb.org/david/ontologies/2013/0/1.3.6.1.4.1.19376.1.8.2.1.2053 -->

    <owl:Class rdf:about="&pathLex;2053">
        <rdfs:subClassOf rdf:resource="&pathLex;99999"/>
        <skos:prefLabel xml:lang="en">Commissure of lip (qualifier : right, left, medial)</skos:prefLabel>
        <skos:definition xml:lang="en">Lip, oral cavity-Infiltrating malignant neoplasm-Lesion site-Commissure of lip (qualifier : right, left, medial)</skos:definition>
    </owl:Class>
    


    <!-- http://www.semanticweb.org/david/ontologies/2013/0/1.3.6.1.4.1.19376.1.8.2.1.2055 -->

    <owl:Class rdf:about="&pathLex;2055">
        <rdfs:subClassOf rdf:resource="&pathLex;99999"/>
        <skos:prefLabel xml:lang="en">Lateral border of tongue (qualifier : right, left, medial)</skos:prefLabel>
        <skos:definition xml:lang="en">Lip, oral cavity-Infiltrating malignant neoplasm-Lesion site-Lateral border of tongue (qualifier : right, left, medial)</skos:definition>
    </owl:Class>
    


    <!-- http://www.semanticweb.org/david/ontologies/2013/0/1.3.6.1.4.1.19376.1.8.2.1.2056 -->

    <owl:Class rdf:about="&pathLex;2056">
        <rdfs:subClassOf rdf:resource="&pathLex;99999"/>
        <skos:definition xml:lang="en">Lip, oral cavity-Infiltrating malignant neoplasm-Lesion site-Ventral surface of tongue, not otherwise specified (NOS) (qualifier : right, left, medial)</skos:definition>
        <skos:prefLabel xml:lang="en">Ventral surface of tongue, not otherwise specified (NOS) (qualifier : right, left, medial)</skos:prefLabel>
    </owl:Class>
    


    <!-- http://www.semanticweb.org/david/ontologies/2013/0/1.3.6.1.4.1.19376.1.8.2.1.2057 -->

    <owl:Class rdf:about="&pathLex;2057">
        <rdfs:subClassOf rdf:resource="&pathLex;99999"/>
        <skos:prefLabel xml:lang="en">Dorsal surface of tongue, NOS (qualifier : right, left, medial)</skos:prefLabel>
        <skos:definition xml:lang="en">Lip, oral cavity-Infiltrating malignant neoplasm-Lesion site-Dorsal surface of tongue, NOS (qualifier : right, left, medial)</skos:definition>
    </owl:Class>
    


    <!-- http://www.semanticweb.org/david/ontologies/2013/0/1.3.6.1.4.1.19376.1.8.2.1.2058 -->

    <owl:Class rdf:about="&pathLex;2058">
        <rdfs:subClassOf rdf:resource="&pathLex;99999"/>
        <skos:prefLabel xml:lang="en">Anterior two-thirds of tongue, NOS (qualifier : right, left, medial)</skos:prefLabel>
        <skos:definition xml:lang="en">Lip, oral cavity-Infiltrating malignant neoplasm-Lesion site-Anterior two-thirds of tongue, NOS (qualifier : right, left, medial)</skos:definition>
    </owl:Class>
    


    <!-- http://www.semanticweb.org/david/ontologies/2013/0/1.3.6.1.4.1.19376.1.8.2.1.2059 -->

    <owl:Class rdf:about="&pathLex;2059">
        <rdfs:subClassOf rdf:resource="&pathLex;99999"/>
        <skos:definition xml:lang="en">Lip, oral cavity-Infiltrating malignant neoplasm-Lesion site-Upper gingiva (gum) (qualifier : right, left, medial)</skos:definition>
        <skos:prefLabel xml:lang="en">Upper gingiva (gum) (qualifier : right, left, medial)</skos:prefLabel>
    </owl:Class>
    


    <!-- http://www.semanticweb.org/david/ontologies/2013/0/1.3.6.1.4.1.19376.1.8.2.1.206 -->

    <owl:Class rdf:about="&pathLex;206">
        <rdfs:subClassOf rdf:resource="&pathLex;99999"/>
        <skos:definition xml:lang="en">Liver-Infiltrating malignant neoplasm-pT</skos:definition>
        <skos:prefLabel xml:lang="en">pT</skos:prefLabel>
    </owl:Class>
    


    <!-- http://www.semanticweb.org/david/ontologies/2013/0/1.3.6.1.4.1.19376.1.8.2.1.2060 -->

    <owl:Class rdf:about="&pathLex;2060">
        <rdfs:subClassOf rdf:resource="&pathLex;99999"/>
        <skos:definition xml:lang="en">Lip, oral cavity-Infiltrating malignant neoplasm-Lesion site-Lower gingiva (gum) (qualifier : right, left, medial)</skos:definition>
        <skos:prefLabel xml:lang="en">Lower gingiva (gum) (qualifier : right, left, medial)</skos:prefLabel>
    </owl:Class>
    


    <!-- http://www.semanticweb.org/david/ontologies/2013/0/1.3.6.1.4.1.19376.1.8.2.1.2061 -->

    <owl:Class rdf:about="&pathLex;2061">
        <rdfs:subClassOf rdf:resource="&pathLex;99999"/>
        <skos:prefLabel xml:lang="en">Anterior floor of mouth (qualifier : right, left, medial)</skos:prefLabel>
        <skos:definition xml:lang="en">Lip, oral cavity-Infiltrating malignant neoplasm-Lesion site-Anterior floor of mouth (qualifier : right, left, medial)</skos:definition>
    </owl:Class>
    


    <!-- http://www.semanticweb.org/david/ontologies/2013/0/1.3.6.1.4.1.19376.1.8.2.1.2062 -->

    <owl:Class rdf:about="&pathLex;2062">
        <rdfs:subClassOf rdf:resource="&pathLex;99999"/>
        <skos:prefLabel xml:lang="en">Floor of mouth, NOS (qualifier : right, left, medial)</skos:prefLabel>
        <skos:definition xml:lang="en">Lip, oral cavity-Infiltrating malignant neoplasm-Lesion site-Floor of mouth, NOS (qualifier : right, left, medial)</skos:definition>
    </owl:Class>
    


    <!-- http://www.semanticweb.org/david/ontologies/2013/0/1.3.6.1.4.1.19376.1.8.2.1.2063 -->

    <owl:Class rdf:about="&pathLex;2063">
        <rdfs:subClassOf rdf:resource="&pathLex;99999"/>
        <skos:prefLabel xml:lang="en">Hard palate (qualifier : right, left, medial)</skos:prefLabel>
        <skos:definition xml:lang="en">Lip, oral cavity-Infiltrating malignant neoplasm-Lesion site-Hard palate (qualifier : right, left, medial)</skos:definition>
    </owl:Class>
    


    <!-- http://www.semanticweb.org/david/ontologies/2013/0/1.3.6.1.4.1.19376.1.8.2.1.2064 -->

    <owl:Class rdf:about="&pathLex;2064">
        <rdfs:subClassOf rdf:resource="&pathLex;99999"/>
        <skos:prefLabel xml:lang="en">Buccal mucosa (inner cheek) (qualifier : right, left, medial)</skos:prefLabel>
        <skos:definition xml:lang="en">Lip, oral cavity-Infiltrating malignant neoplasm-Lesion site-Buccal mucosa (inner cheek) (qualifier : right, left, medial)</skos:definition>
    </owl:Class>
    


    <!-- http://www.semanticweb.org/david/ontologies/2013/0/1.3.6.1.4.1.19376.1.8.2.1.2065 -->

    <owl:Class rdf:about="&pathLex;2065">
        <rdfs:subClassOf rdf:resource="&pathLex;99999"/>
        <skos:definition xml:lang="en">Lip, oral cavity-Infiltrating malignant neoplasm-Lesion site-Upper vestibule of mouth (qualifier : right, left, medial)</skos:definition>
        <skos:prefLabel xml:lang="en">Upper vestibule of mouth (qualifier : right, left, medial)</skos:prefLabel>
    </owl:Class>
    


    <!-- http://www.semanticweb.org/david/ontologies/2013/0/1.3.6.1.4.1.19376.1.8.2.1.2066 -->

    <owl:Class rdf:about="&pathLex;2066">
        <rdfs:subClassOf rdf:resource="&pathLex;99999"/>
        <skos:definition xml:lang="en">Lip, oral cavity-Infiltrating malignant neoplasm-Lesion site-Lower vestibule of mouth (qualifier : right, left, medial)</skos:definition>
        <skos:prefLabel xml:lang="en">Lower vestibule of mouth (qualifier : right, left, medial)</skos:prefLabel>
    </owl:Class>
    


    <!-- http://www.semanticweb.org/david/ontologies/2013/0/1.3.6.1.4.1.19376.1.8.2.1.2067 -->

    <owl:Class rdf:about="&pathLex;2067">
        <rdfs:subClassOf rdf:resource="&pathLex;99999"/>
        <skos:definition xml:lang="en">Lip, oral cavity-Infiltrating malignant neoplasm-Lesion site-Upper alveolar process (qualifier : right, left, medial)</skos:definition>
        <skos:prefLabel xml:lang="en">Upper alveolar process (qualifier : right, left, medial)</skos:prefLabel>
    </owl:Class>
    


    <!-- http://www.semanticweb.org/david/ontologies/2013/0/1.3.6.1.4.1.19376.1.8.2.1.2068 -->

    <owl:Class rdf:about="&pathLex;2068">
        <rdfs:subClassOf rdf:resource="&pathLex;99999"/>
        <skos:definition xml:lang="en">Lip, oral cavity-Infiltrating malignant neoplasm-Lesion site-Lower alveolar process (qualifier : right, left, medial)</skos:definition>
        <skos:prefLabel xml:lang="en">Lower alveolar process (qualifier : right, left, medial)</skos:prefLabel>
    </owl:Class>
    


    <!-- http://www.semanticweb.org/david/ontologies/2013/0/1.3.6.1.4.1.19376.1.8.2.1.2069 -->

    <owl:Class rdf:about="&pathLex;2069">
        <rdfs:subClassOf rdf:resource="&pathLex;99999"/>
        <skos:definition xml:lang="en">Lip, oral cavity-Infiltrating malignant neoplasm-Lesion site-Mandible (qualifier : right, left, medial)</skos:definition>
        <skos:prefLabel xml:lang="en">Mandible (qualifier : right, left, medial)</skos:prefLabel>
    </owl:Class>
    


    <!-- http://www.semanticweb.org/david/ontologies/2013/0/1.3.6.1.4.1.19376.1.8.2.1.207 -->

    <owl:Class rdf:about="&pathLex;207">
        <rdfs:subClassOf rdf:resource="&pathLex;99999"/>
        <skos:prefLabel xml:lang="en">Lesion size, largest dimension</skos:prefLabel>
        <skos:definition xml:lang="en">Liver-Infiltrating malignant neoplasm-Lesion size, largest dimension</skos:definition>
    </owl:Class>
    


    <!-- http://www.semanticweb.org/david/ontologies/2013/0/1.3.6.1.4.1.19376.1.8.2.1.2070 -->

    <owl:Class rdf:about="&pathLex;2070">
        <rdfs:subClassOf rdf:resource="&pathLex;99999"/>
        <skos:definition xml:lang="en">Lip, oral cavity-Infiltrating malignant neoplasm-Lesion site-Maxilla (qualifier : right, left, medial)</skos:definition>
        <skos:prefLabel xml:lang="en">Maxilla (qualifier : right, left, medial)</skos:prefLabel>
    </owl:Class>
    


    <!-- http://www.semanticweb.org/david/ontologies/2013/0/1.3.6.1.4.1.19376.1.8.2.1.2071 -->

    <owl:Class rdf:about="&pathLex;2071">
        <rdfs:subClassOf rdf:resource="&pathLex;99999"/>
        <skos:definition xml:lang="en">Lip, oral cavity-Infiltrating malignant neoplasm-pM-pM1: Distant metastasis - Specify site(s)</skos:definition>
        <skos:prefLabel xml:lang="en">pM1: Distant metastasis - Specify site(s)</skos:prefLabel>
    </owl:Class>
    


    <!-- http://www.semanticweb.org/david/ontologies/2013/0/1.3.6.1.4.1.19376.1.8.2.1.2072 -->

    <owl:Class rdf:about="&pathLex;2072">
        <rdfs:subClassOf rdf:resource="&pathLex;99999"/>
        <skos:definition xml:lang="en">Esophagus-Infiltrating malignant neoplasm-Lesion site-Midesophagus: Upper thoracic esophagus</skos:definition>
        <skos:prefLabel xml:lang="en">Midesophagus: Upper thoracic esophagus</skos:prefLabel>
    </owl:Class>
    


    <!-- http://www.semanticweb.org/david/ontologies/2013/0/1.3.6.1.4.1.19376.1.8.2.1.2073 -->

    <owl:Class rdf:about="&pathLex;2073">
        <rdfs:subClassOf rdf:resource="&pathLex;99999"/>
        <skos:definition xml:lang="en">Esophagus-Infiltrating malignant neoplasm-Lesion site-Midesophagus: Midthoracic esophagus</skos:definition>
        <skos:prefLabel xml:lang="en">Midesophagus: Midthoracic esophagus</skos:prefLabel>
    </owl:Class>
    


    <!-- http://www.semanticweb.org/david/ontologies/2013/0/1.3.6.1.4.1.19376.1.8.2.1.2074 -->

    <owl:Class rdf:about="&pathLex;2074">
        <rdfs:subClassOf rdf:resource="&pathLex;99999"/>
        <skos:prefLabel xml:lang="en">Distal esophagus (lower thoracic esophagus)</skos:prefLabel>
        <skos:definition xml:lang="en">Esophagus-Infiltrating malignant neoplasm-Lesion site-Distal esophagus (lower thoracic esophagus)</skos:definition>
    </owl:Class>
    


    <!-- http://www.semanticweb.org/david/ontologies/2013/0/1.3.6.1.4.1.19376.1.8.2.1.2075 -->

    <owl:Class rdf:about="&pathLex;2075">
        <rdfs:subClassOf rdf:resource="&pathLex;99999"/>
        <skos:definition xml:lang="en">Esophagus-Infiltrating malignant neoplasm-Lesion site-Proximal stomach and esophagogastric junction</skos:definition>
        <skos:prefLabel xml:lang="en">Proximal stomach and esophagogastric junction</skos:prefLabel>
    </owl:Class>
    


    <!-- http://www.semanticweb.org/david/ontologies/2013/0/1.3.6.1.4.1.19376.1.8.2.1.2077 -->

    <owl:Class rdf:about="&pathLex;2077">
        <rdfs:subClassOf rdf:resource="&pathLex;99999"/>
        <skos:prefLabel xml:lang="en">Nasopharynx: Nasopharyngeal tonsils (adenoids)</skos:prefLabel>
        <skos:definition xml:lang="en">Pharynx-Infiltrating malignant neoplasm-Lesion site-Nasopharynx: Nasopharyngeal tonsils (adenoids)</skos:definition>
    </owl:Class>
    


    <!-- http://www.semanticweb.org/david/ontologies/2013/0/1.3.6.1.4.1.19376.1.8.2.1.2078 -->

    <owl:Class rdf:about="&pathLex;2078">
        <rdfs:subClassOf rdf:resource="&pathLex;99999"/>
        <skos:prefLabel xml:lang="en">Oropharynx: Palatine tonsil</skos:prefLabel>
        <skos:definition xml:lang="en">Pharynx-Infiltrating malignant neoplasm-Lesion site-Oropharynx: Palatine tonsil</skos:definition>
    </owl:Class>
    


    <!-- http://www.semanticweb.org/david/ontologies/2013/0/1.3.6.1.4.1.19376.1.8.2.1.2079 -->

    <owl:Class rdf:about="&pathLex;2079">
        <rdfs:subClassOf rdf:resource="&pathLex;99999"/>
        <skos:prefLabel xml:lang="en">Oropharynx: Base of tongue, including lingual tonsil</skos:prefLabel>
        <skos:definition xml:lang="en">Pharynx-Infiltrating malignant neoplasm-Lesion site-Oropharynx: Base of tongue, including lingual tonsil</skos:definition>
    </owl:Class>
    


    <!-- http://www.semanticweb.org/david/ontologies/2013/0/1.3.6.1.4.1.19376.1.8.2.1.208 -->

    <owl:Class rdf:about="&pathLex;208">
        <rdfs:subClassOf rdf:resource="&pathLex;99999"/>
        <skos:prefLabel xml:lang="en">Histologic type</skos:prefLabel>
        <skos:definition xml:lang="en">Liver-Infiltrating malignant neoplasm-Histologic type</skos:definition>
    </owl:Class>
    


    <!-- http://www.semanticweb.org/david/ontologies/2013/0/1.3.6.1.4.1.19376.1.8.2.1.2080 -->

    <owl:Class rdf:about="&pathLex;2080">
        <rdfs:subClassOf rdf:resource="&pathLex;99999"/>
        <skos:prefLabel xml:lang="en">Oropharynx: Soft palate</skos:prefLabel>
        <skos:definition xml:lang="en">Pharynx-Infiltrating malignant neoplasm-Lesion site-Oropharynx: Soft palate</skos:definition>
    </owl:Class>
    


    <!-- http://www.semanticweb.org/david/ontologies/2013/0/1.3.6.1.4.1.19376.1.8.2.1.2081 -->

    <owl:Class rdf:about="&pathLex;2081">
        <rdfs:subClassOf rdf:resource="&pathLex;99999"/>
        <skos:prefLabel xml:lang="en">Oropharynx: Uvula</skos:prefLabel>
        <skos:definition xml:lang="en">Pharynx-Infiltrating malignant neoplasm-Lesion site-Oropharynx: Uvula</skos:definition>
    </owl:Class>
    


    <!-- http://www.semanticweb.org/david/ontologies/2013/0/1.3.6.1.4.1.19376.1.8.2.1.2082 -->

    <owl:Class rdf:about="&pathLex;2082">
        <rdfs:subClassOf rdf:resource="&pathLex;99999"/>
        <skos:prefLabel xml:lang="en">Oropharynx: Pharyngeal wall (posterior)</skos:prefLabel>
        <skos:definition xml:lang="en">Pharynx-Infiltrating malignant neoplasm-Lesion site-Oropharynx: Pharyngeal wall (posterior)</skos:definition>
    </owl:Class>
    


    <!-- http://www.semanticweb.org/david/ontologies/2013/0/1.3.6.1.4.1.19376.1.8.2.1.2083 -->

    <owl:Class rdf:about="&pathLex;2083">
        <rdfs:subClassOf rdf:resource="&pathLex;99999"/>
        <skos:prefLabel xml:lang="en">Oropharynx: Other</skos:prefLabel>
        <skos:definition xml:lang="en">Pharynx-Infiltrating malignant neoplasm-Lesion site-Oropharynx: Other</skos:definition>
    </owl:Class>
    


    <!-- http://www.semanticweb.org/david/ontologies/2013/0/1.3.6.1.4.1.19376.1.8.2.1.2085 -->

    <owl:Class rdf:about="&pathLex;2085">
        <rdfs:subClassOf rdf:resource="&pathLex;99999"/>
        <skos:prefLabel xml:lang="en">Lung upper lobe</skos:prefLabel>
        <skos:definition xml:lang="en">Lung-Infiltrating malignant neoplasm-Lesion site-Lung upper lobe</skos:definition>
    </owl:Class>
    


    <!-- http://www.semanticweb.org/david/ontologies/2013/0/1.3.6.1.4.1.19376.1.8.2.1.2086 -->

    <owl:Class rdf:about="&pathLex;2086">
        <rdfs:subClassOf rdf:resource="&pathLex;99999"/>
        <skos:prefLabel xml:lang="en">Lung middle lobe</skos:prefLabel>
        <skos:definition xml:lang="en">Lung-Infiltrating malignant neoplasm-Lesion site-Lung middle lobe</skos:definition>
    </owl:Class>
    


    <!-- http://www.semanticweb.org/david/ontologies/2013/0/1.3.6.1.4.1.19376.1.8.2.1.2087 -->

    <owl:Class rdf:about="&pathLex;2087">
        <rdfs:subClassOf rdf:resource="&pathLex;99999"/>
        <skos:prefLabel xml:lang="en">Lung lower lobe</skos:prefLabel>
        <skos:definition xml:lang="en">Lung-Infiltrating malignant neoplasm-Lesion site-Lung lower lobe</skos:definition>
    </owl:Class>
    


    <!-- http://www.semanticweb.org/david/ontologies/2013/0/1.3.6.1.4.1.19376.1.8.2.1.2088 -->

    <owl:Class rdf:about="&pathLex;2088">
        <rdfs:subClassOf rdf:resource="&pathLex;99999"/>
        <skos:prefLabel xml:lang="en">Bronchus (specify)</skos:prefLabel>
        <skos:definition xml:lang="en">Lung-Infiltrating malignant neoplasm-Lesion site-Bronchus (specify)</skos:definition>
    </owl:Class>
    


    <!-- http://www.semanticweb.org/david/ontologies/2013/0/1.3.6.1.4.1.19376.1.8.2.1.2089 -->

    <owl:Class rdf:about="&pathLex;2089">
        <rdfs:subClassOf rdf:resource="&pathLex;99999"/>
        <skos:prefLabel xml:lang="en">Prostate</skos:prefLabel>
        <skos:definition xml:lang="en">Prostate-Infiltrating malignant neoplasm-Lesion site-Prostate</skos:definition>
    </owl:Class>
    


    <!-- http://www.semanticweb.org/david/ontologies/2013/0/1.3.6.1.4.1.19376.1.8.2.1.209 -->

    <owl:Class rdf:about="&pathLex;209">
        <rdfs:subClassOf rdf:resource="&pathLex;10010"/>
        <skos:definition xml:lang="en">Generic-Infiltrating malignant neoplasm-Lymph node sampling</skos:definition>
        <skos:prefLabel xml:lang="en">Lymph node sampling</skos:prefLabel>
    </owl:Class>
    


    <!-- http://www.semanticweb.org/david/ontologies/2013/0/1.3.6.1.4.1.19376.1.8.2.1.2090 -->

    <owl:Class rdf:about="&pathLex;2090">
        <rdfs:subClassOf rdf:resource="&pathLex;99999"/>
        <skos:prefLabel xml:lang="en">Lobe</skos:prefLabel>
        <skos:definition xml:lang="en">Thyroid-Infiltrating malignant neoplasm-Lesion site-Lobe</skos:definition>
    </owl:Class>
    


    <!-- http://www.semanticweb.org/david/ontologies/2013/0/1.3.6.1.4.1.19376.1.8.2.1.2093 -->

    <owl:Class rdf:about="&pathLex;2093">
        <rdfs:subClassOf rdf:resource="&pathLex;10008"/>
        <skos:definition xml:lang="en">Cervix-Specimen-Target site-Fallopian tube (qualifier : right, left)</skos:definition>
        <skos:prefLabel xml:lang="en">Fallopian tube (qualifier : right, left)</skos:prefLabel>
    </owl:Class>
    


    <!-- http://www.semanticweb.org/david/ontologies/2013/0/1.3.6.1.4.1.19376.1.8.2.1.2094 -->

    <owl:Class rdf:about="&pathLex;2094">
        <rdfs:subClassOf rdf:resource="&pathLex;10008"/>
        <skos:definition xml:lang="en">Cervix-Specimen-Target site-Vagina</skos:definition>
        <skos:prefLabel xml:lang="en">Vagina</skos:prefLabel>
    </owl:Class>
    


    <!-- http://www.semanticweb.org/david/ontologies/2013/0/1.3.6.1.4.1.19376.1.8.2.1.2095 -->

    <owl:Class rdf:about="&pathLex;2095">
        <rdfs:subClassOf rdf:resource="&pathLex;10008"/>
        <skos:definition xml:lang="en">Cervix-Specimen-Target site-Urinary bladder</skos:definition>
        <skos:prefLabel xml:lang="en">Urinary bladder</skos:prefLabel>
    </owl:Class>
    


    <!-- http://www.semanticweb.org/david/ontologies/2013/0/1.3.6.1.4.1.19376.1.8.2.1.21 -->

    <owl:Class rdf:about="&pathLex;21">
        <rdfs:subClassOf rdf:resource="&pathLex;10010"/>
        <skos:definition xml:lang="en">Generic-Infiltrating malignant neoplasm-Histologic type</skos:definition>
        <skos:prefLabel xml:lang="en">Histologic type</skos:prefLabel>
    </owl:Class>
    


    <!-- http://www.semanticweb.org/david/ontologies/2013/0/1.3.6.1.4.1.19376.1.8.2.1.210 -->

    <owl:Class rdf:about="&pathLex;210">
        <rdfs:subClassOf rdf:resource="&pathLex;10005"/>
        <skos:definition xml:lang="en">Generic-Infiltrating malignant neoplasm-Histologic grade (Two-Tier Grading System)</skos:definition>
        <skos:prefLabel xml:lang="en">Histologic grade (Two-Tier Grading System)</skos:prefLabel>
    </owl:Class>
    


    <!-- http://www.semanticweb.org/david/ontologies/2013/0/1.3.6.1.4.1.19376.1.8.2.1.2101 -->

    <owl:Class rdf:about="&pathLex;2101">
        <rdfs:subClassOf rdf:resource="&pathLex;99999"/>
        <skos:prefLabel xml:lang="en">Appendix</skos:prefLabel>
        <skos:definition xml:lang="en">Colon-Specimen-Target site-Appendix</skos:definition>
    </owl:Class>
    


    <!-- http://www.semanticweb.org/david/ontologies/2013/0/1.3.6.1.4.1.19376.1.8.2.1.2102 -->

    <owl:Class rdf:about="&pathLex;2102">
        <rdfs:subClassOf rdf:resource="&pathLex;99999"/>
        <skos:prefLabel xml:lang="en">Anus</skos:prefLabel>
        <skos:definition xml:lang="en">Colon-Specimen-Target site-Anus</skos:definition>
    </owl:Class>
    


    <!-- http://www.semanticweb.org/david/ontologies/2013/0/1.3.6.1.4.1.19376.1.8.2.1.2105 -->

    <owl:Class rdf:about="&pathLex;2105">
        <rdfs:subClassOf rdf:resource="&pathLex;99999"/>
        <skos:definition xml:lang="en">Endometrium-Specimen-Target site-Parametrium (qualifier : right, left)</skos:definition>
        <skos:prefLabel xml:lang="en">Parametrium (qualifier : right, left)</skos:prefLabel>
    </owl:Class>
    


    <!-- http://www.semanticweb.org/david/ontologies/2013/0/1.3.6.1.4.1.19376.1.8.2.1.2106 -->

    <owl:Class rdf:about="&pathLex;2106">
        <rdfs:subClassOf rdf:resource="&pathLex;99999"/>
        <skos:definition xml:lang="en">Endometrium-Specimen-Target site-Vaginal cuff</skos:definition>
        <skos:prefLabel xml:lang="en">Vaginal cuff</skos:prefLabel>
    </owl:Class>
    


    <!-- http://www.semanticweb.org/david/ontologies/2013/0/1.3.6.1.4.1.19376.1.8.2.1.2107 -->

    <owl:Class rdf:about="&pathLex;2107">
        <rdfs:subClassOf rdf:resource="&pathLex;99999"/>
        <skos:definition xml:lang="en">Endometrium-Specimen-Target site-Omentum</skos:definition>
        <skos:prefLabel xml:lang="en">Omentum</skos:prefLabel>
    </owl:Class>
    


    <!-- http://www.semanticweb.org/david/ontologies/2013/0/1.3.6.1.4.1.19376.1.8.2.1.2108 -->

    <owl:Class rdf:about="&pathLex;2108">
        <rdfs:subClassOf rdf:resource="&pathLex;99999"/>
        <skos:prefLabel xml:lang="en">Portion of stomach</skos:prefLabel>
        <skos:definition xml:lang="en">Stomach-Specimen-Target site-Portion of stomach</skos:definition>
    </owl:Class>
    


    <!-- http://www.semanticweb.org/david/ontologies/2013/0/1.3.6.1.4.1.19376.1.8.2.1.2109 -->

    <owl:Class rdf:about="&pathLex;2109">
        <rdfs:subClassOf rdf:resource="&pathLex;99999"/>
        <skos:prefLabel xml:lang="en">Gastric body</skos:prefLabel>
        <skos:definition xml:lang="en">Stomach-Specimen-Target site-Gastric body</skos:definition>
    </owl:Class>
    


    <!-- http://www.semanticweb.org/david/ontologies/2013/0/1.3.6.1.4.1.19376.1.8.2.1.2110 -->

    <owl:Class rdf:about="&pathLex;2110">
        <rdfs:subClassOf rdf:resource="&pathLex;99999"/>
        <skos:prefLabel xml:lang="en">Gastric antrum</skos:prefLabel>
        <skos:definition xml:lang="en">Stomach-Specimen-Target site-Gastric antrum</skos:definition>
    </owl:Class>
    


    <!-- http://www.semanticweb.org/david/ontologies/2013/0/1.3.6.1.4.1.19376.1.8.2.1.2111 -->

    <owl:Class rdf:about="&pathLex;2111">
        <rdfs:subClassOf rdf:resource="&pathLex;99999"/>
        <skos:prefLabel xml:lang="en">Distal esophagus</skos:prefLabel>
        <skos:definition xml:lang="en">Stomach-Specimen-Target site-Distal esophagus</skos:definition>
    </owl:Class>
    


    <!-- http://www.semanticweb.org/david/ontologies/2013/0/1.3.6.1.4.1.19376.1.8.2.1.2112 -->

    <owl:Class rdf:about="&pathLex;2112">
        <rdfs:subClassOf rdf:resource="&pathLex;99999"/>
        <skos:prefLabel xml:lang="en">Proximal duodenum</skos:prefLabel>
        <skos:definition xml:lang="en">Stomach-Specimen-Target site-Proximal duodenum</skos:definition>
    </owl:Class>
    


    <!-- http://www.semanticweb.org/david/ontologies/2013/0/1.3.6.1.4.1.19376.1.8.2.1.2115 -->

    <owl:Class rdf:about="&pathLex;2115">
        <rdfs:subClassOf rdf:resource="&pathLex;99999"/>
        <skos:definition xml:lang="en">Salivary gland-Specimen-Target site-Superficial lobe of parotid gland only (qualifier : right, left)</skos:definition>
        <skos:prefLabel xml:lang="en">Superficial lobe of parotid gland only (qualifier : right, left)</skos:prefLabel>
    </owl:Class>
    


    <!-- http://www.semanticweb.org/david/ontologies/2013/0/1.3.6.1.4.1.19376.1.8.2.1.2116 -->

    <owl:Class rdf:about="&pathLex;2116">
        <rdfs:subClassOf rdf:resource="&pathLex;99999"/>
        <skos:prefLabel xml:lang="en">Deep lobe of parotid gland only (qualifier : right, left)</skos:prefLabel>
        <skos:definition xml:lang="en">Salivary gland-Specimen-Target site-Deep lobe of parotid gland only (qualifier : right, left)</skos:definition>
    </owl:Class>
    


    <!-- http://www.semanticweb.org/david/ontologies/2013/0/1.3.6.1.4.1.19376.1.8.2.1.2127 -->

    <owl:Class rdf:about="&pathLex;2127">
        <rdfs:subClassOf rdf:resource="&pathLex;99999"/>
        <skos:prefLabel xml:lang="en">Dorsal surface of tongue, NOS (qualifier : right, left, medial)</skos:prefLabel>
        <skos:definition xml:lang="en">Lip, oral cavity-Specimen-Target site-Dorsal surface of tongue, NOS (qualifier : right, left, medial)</skos:definition>
    </owl:Class>
    


    <!-- http://www.semanticweb.org/david/ontologies/2013/0/1.3.6.1.4.1.19376.1.8.2.1.2128 -->

    <owl:Class rdf:about="&pathLex;2128">
        <rdfs:subClassOf rdf:resource="&pathLex;99999"/>
        <skos:prefLabel xml:lang="en">Anterior two-thirds of tongue, NOS (qualifier : right, left, medial)</skos:prefLabel>
        <skos:definition xml:lang="en">Lip, oral cavity-Specimen-Target site-Anterior two-thirds of tongue, NOS (qualifier : right, left, medial)</skos:definition>
    </owl:Class>
    


    <!-- http://www.semanticweb.org/david/ontologies/2013/0/1.3.6.1.4.1.19376.1.8.2.1.213 -->

    <owl:Class rdf:about="&pathLex;213">
        <rdfs:subClassOf rdf:resource="&pathLex;99999"/>
        <skos:definition xml:lang="en">Generic-Infiltrating malignant neoplasm-Macroscopic type</skos:definition>
        <skos:prefLabel xml:lang="en">Macroscopic type</skos:prefLabel>
    </owl:Class>
    


    <!-- http://www.semanticweb.org/david/ontologies/2013/0/1.3.6.1.4.1.19376.1.8.2.1.2131 -->

    <owl:Class rdf:about="&pathLex;2131">
        <rdfs:subClassOf rdf:resource="&pathLex;99999"/>
        <skos:prefLabel xml:lang="en">Anterior floor of mouth (qualifier : right, left, medial)</skos:prefLabel>
        <skos:definition xml:lang="en">Lip, oral cavity-Specimen-Target site-Anterior floor of mouth (qualifier : right, left, medial)</skos:definition>
    </owl:Class>
    


    <!-- http://www.semanticweb.org/david/ontologies/2013/0/1.3.6.1.4.1.19376.1.8.2.1.2134 -->

    <owl:Class rdf:about="&pathLex;2134">
        <rdfs:subClassOf rdf:resource="&pathLex;99999"/>
        <skos:prefLabel xml:lang="en">Buccal mucosa (inner cheek) (qualifier : right, left, medial)</skos:prefLabel>
        <skos:definition xml:lang="en">Lip, oral cavity-Specimen-Target site-Buccal mucosa (inner cheek) (qualifier : right, left, medial)</skos:definition>
    </owl:Class>
    


    <!-- http://www.semanticweb.org/david/ontologies/2013/0/1.3.6.1.4.1.19376.1.8.2.1.2136 -->

    <owl:Class rdf:about="&pathLex;2136">
        <rdfs:subClassOf rdf:resource="&pathLex;99999"/>
        <skos:definition xml:lang="en">Lip, oral cavity-Specimen-Target site-Lower vestibule of mouth (qualifier : right, left, medial)</skos:definition>
        <skos:prefLabel xml:lang="en">Lower vestibule of mouth (qualifier : right, left, medial)</skos:prefLabel>
    </owl:Class>
    


    <!-- http://www.semanticweb.org/david/ontologies/2013/0/1.3.6.1.4.1.19376.1.8.2.1.214 -->

    <owl:Class rdf:about="&pathLex;214">
        <rdfs:subClassOf rdf:resource="&pathLex;99999"/>
        <skos:prefLabel xml:lang="en">Margins involvement</skos:prefLabel>
        <skos:definition xml:lang="en">Salivary gland-Infiltrating malignant neoplasm-Margins involvement</skos:definition>
    </owl:Class>
    


    <!-- http://www.semanticweb.org/david/ontologies/2013/0/1.3.6.1.4.1.19376.1.8.2.1.2141 -->

    <owl:Class rdf:about="&pathLex;2141">
        <rdfs:subClassOf rdf:resource="&pathLex;99999"/>
        <skos:definition xml:lang="en">Esophagus-Specimen-Target site-Proximal stomach</skos:definition>
        <skos:prefLabel xml:lang="en">Proximal stomach</skos:prefLabel>
    </owl:Class>
    


    <!-- http://www.semanticweb.org/david/ontologies/2013/0/1.3.6.1.4.1.19376.1.8.2.1.2144 -->

    <owl:Class rdf:about="&pathLex;2144">
        <rdfs:subClassOf rdf:resource="&pathLex;99999"/>
        <skos:prefLabel xml:lang="en">Cervix</skos:prefLabel>
        <skos:definition xml:lang="en">Ovary-Specimen-Target site-Cervix</skos:definition>
    </owl:Class>
    


    <!-- http://www.semanticweb.org/david/ontologies/2013/0/1.3.6.1.4.1.19376.1.8.2.1.2146 -->

    <owl:Class rdf:about="&pathLex;2146">
        <rdfs:subClassOf rdf:resource="&pathLex;99999"/>
        <skos:definition xml:lang="en">Ovary-Specimen-Target site-Peritoneum</skos:definition>
        <skos:prefLabel xml:lang="en">Peritoneum</skos:prefLabel>
    </owl:Class>
    


    <!-- http://www.semanticweb.org/david/ontologies/2013/0/1.3.6.1.4.1.19376.1.8.2.1.2147 -->

    <owl:Class rdf:about="&pathLex;2147">
        <rdfs:subClassOf rdf:resource="&pathLex;99999"/>
        <skos:prefLabel xml:lang="en">Head of pancreas</skos:prefLabel>
        <skos:definition xml:lang="en">Pancreas-Specimen-Target site-Head of pancreas</skos:definition>
    </owl:Class>
    


    <!-- http://www.semanticweb.org/david/ontologies/2013/0/1.3.6.1.4.1.19376.1.8.2.1.2148 -->

    <owl:Class rdf:about="&pathLex;2148">
        <rdfs:subClassOf rdf:resource="&pathLex;99999"/>
        <skos:prefLabel xml:lang="en">Body of pancreas</skos:prefLabel>
        <skos:definition xml:lang="en">Pancreas-Specimen-Target site-Body of pancreas</skos:definition>
    </owl:Class>
    


    <!-- http://www.semanticweb.org/david/ontologies/2013/0/1.3.6.1.4.1.19376.1.8.2.1.2149 -->

    <owl:Class rdf:about="&pathLex;2149">
        <rdfs:subClassOf rdf:resource="&pathLex;99999"/>
        <skos:definition xml:lang="en">Pancreas-Specimen-Target site-Tail of pancreas</skos:definition>
        <skos:prefLabel xml:lang="en">Tail of pancreas</skos:prefLabel>
    </owl:Class>
    


    <!-- http://www.semanticweb.org/david/ontologies/2013/0/1.3.6.1.4.1.19376.1.8.2.1.215 -->

    <owl:Class rdf:about="&pathLex;215">
        <rdfs:subClassOf rdf:resource="&pathLex;99999"/>
        <skos:prefLabel xml:lang="en">Distance of lesion from closest uninvolved margin</skos:prefLabel>
        <skos:definition xml:lang="en">Salivary gland-Infiltrating malignant neoplasm-Distance of lesion from closest uninvolved margin</skos:definition>
    </owl:Class>
    


    <!-- http://www.semanticweb.org/david/ontologies/2013/0/1.3.6.1.4.1.19376.1.8.2.1.2150 -->

    <owl:Class rdf:about="&pathLex;2150">
        <rdfs:subClassOf rdf:resource="&pathLex;99999"/>
        <skos:prefLabel xml:lang="en">Duodenum</skos:prefLabel>
        <skos:definition xml:lang="en">Pancreas-Specimen-Target site-Duodenum</skos:definition>
    </owl:Class>
    


    <!-- http://www.semanticweb.org/david/ontologies/2013/0/1.3.6.1.4.1.19376.1.8.2.1.2152 -->

    <owl:Class rdf:about="&pathLex;2152">
        <rdfs:subClassOf rdf:resource="&pathLex;99999"/>
        <skos:prefLabel xml:lang="en">Common bile duct</skos:prefLabel>
        <skos:definition xml:lang="en">Pancreas-Specimen-Target site-Common bile duct</skos:definition>
    </owl:Class>
    


    <!-- http://www.semanticweb.org/david/ontologies/2013/0/1.3.6.1.4.1.19376.1.8.2.1.2154 -->

    <owl:Class rdf:about="&pathLex;2154">
        <rdfs:subClassOf rdf:resource="&pathLex;99999"/>
        <skos:definition xml:lang="en">Pancreas-Specimen-Target site-Spleen</skos:definition>
        <skos:prefLabel xml:lang="en">Spleen</skos:prefLabel>
    </owl:Class>
    


    <!-- http://www.semanticweb.org/david/ontologies/2013/0/1.3.6.1.4.1.19376.1.8.2.1.2155 -->

    <owl:Class rdf:about="&pathLex;2155">
        <rdfs:subClassOf rdf:resource="&pathLex;99999"/>
        <skos:prefLabel xml:lang="en">Adjacent large vessels</skos:prefLabel>
        <skos:definition xml:lang="en">Pancreas-Specimen-Target site-Adjacent large vessels</skos:definition>
    </owl:Class>
    


    <!-- http://www.semanticweb.org/david/ontologies/2013/0/1.3.6.1.4.1.19376.1.8.2.1.2156 -->

    <owl:Class rdf:about="&pathLex;2156">
        <rdfs:subClassOf rdf:resource="&pathLex;99999"/>
        <skos:definition xml:lang="en">Pancreas-Specimen-Target site-Portal vein</skos:definition>
        <skos:prefLabel xml:lang="en">Portal vein</skos:prefLabel>
    </owl:Class>
    


    <!-- http://www.semanticweb.org/david/ontologies/2013/0/1.3.6.1.4.1.19376.1.8.2.1.2157 -->

    <owl:Class rdf:about="&pathLex;2157">
        <rdfs:subClassOf rdf:resource="&pathLex;99999"/>
        <skos:definition xml:lang="en">Pancreas-Specimen-Target site-Superior mesenteric vein</skos:definition>
        <skos:prefLabel xml:lang="en">Superior mesenteric vein</skos:prefLabel>
    </owl:Class>
    


    <!-- http://www.semanticweb.org/david/ontologies/2013/0/1.3.6.1.4.1.19376.1.8.2.1.2158 -->

    <owl:Class rdf:about="&pathLex;2158">
        <rdfs:subClassOf rdf:resource="&pathLex;99999"/>
        <skos:prefLabel xml:lang="en">Oropharynx</skos:prefLabel>
        <skos:definition xml:lang="en">Pharynx-Specimen-Target site-Oropharynx</skos:definition>
    </owl:Class>
    


    <!-- http://www.semanticweb.org/david/ontologies/2013/0/1.3.6.1.4.1.19376.1.8.2.1.216 -->

    <owl:Class rdf:about="&pathLex;216">
        <rdfs:subClassOf rdf:resource="&pathLex;99999"/>
        <skos:prefLabel xml:lang="en">Lymph-vascular invasion</skos:prefLabel>
        <skos:definition xml:lang="en">Salivary gland-Infiltrating malignant neoplasm-Lymph-vascular invasion</skos:definition>
    </owl:Class>
    


    <!-- http://www.semanticweb.org/david/ontologies/2013/0/1.3.6.1.4.1.19376.1.8.2.1.2162 -->

    <owl:Class rdf:about="&pathLex;2162">
        <rdfs:subClassOf rdf:resource="&pathLex;99999"/>
        <skos:prefLabel xml:lang="en">Bronchus (specify)</skos:prefLabel>
        <skos:definition xml:lang="en">Lung-Specimen-Target site-Bronchus (specify)</skos:definition>
    </owl:Class>
    


    <!-- http://www.semanticweb.org/david/ontologies/2013/0/1.3.6.1.4.1.19376.1.8.2.1.2166 -->

    <owl:Class rdf:about="&pathLex;2166">
        <rdfs:subClassOf rdf:resource="&pathLex;10008"/>
        <skos:definition xml:lang="en">Breast-Specimen-Target site-Partial breast</skos:definition>
        <skos:prefLabel xml:lang="en">Partial breast</skos:prefLabel>
    </owl:Class>
    


    <!-- http://www.semanticweb.org/david/ontologies/2013/0/1.3.6.1.4.1.19376.1.8.2.1.2168 -->

    <owl:Class rdf:about="&pathLex;2168">
        <rdfs:subClassOf rdf:resource="&pathLex;98"/>
        <skos:definition xml:lang="en">Breast-Infiltrating malignant neoplasm-Necrosis of ductal carcinoma in situ (DCIS)-Not identified</skos:definition>
        <skos:prefLabel xml:lang="en">Not identified</skos:prefLabel>
    </owl:Class>
    


    <!-- http://www.semanticweb.org/david/ontologies/2013/0/1.3.6.1.4.1.19376.1.8.2.1.2169 -->

    <owl:Class rdf:about="&pathLex;2169">
        <rdfs:subClassOf rdf:resource="&pathLex;98"/>
        <skos:definition xml:lang="en">Breast-Infiltrating malignant neoplasm-Necrosis of ductal carcinoma in situ (DCIS)-Present, focal (small foci or single cell necrosis)</skos:definition>
        <skos:prefLabel xml:lang="en">Present, focal (small foci or single cell necrosis)</skos:prefLabel>
    </owl:Class>
    


    <!-- http://www.semanticweb.org/david/ontologies/2013/0/1.3.6.1.4.1.19376.1.8.2.1.217 -->

    <owl:Class rdf:about="&pathLex;217">
        <rdfs:subClassOf rdf:resource="&pathLex;99999"/>
        <skos:prefLabel xml:lang="en">Extent</skos:prefLabel>
        <skos:definition xml:lang="en">Salivary gland-Infiltrating malignant neoplasm-Extent</skos:definition>
    </owl:Class>
    


    <!-- http://www.semanticweb.org/david/ontologies/2013/0/1.3.6.1.4.1.19376.1.8.2.1.2170 -->

    <owl:Class rdf:about="&pathLex;2170">
        <rdfs:subClassOf rdf:resource="&pathLex;98"/>
        <skos:definition xml:lang="en">Breast-Infiltrating malignant neoplasm-Necrosis of ductal carcinoma in situ (DCIS)-Present, central (expansive “comedo” necrosis)</skos:definition>
        <skos:prefLabel xml:lang="en">Present, central (expansive “comedo” necrosis)</skos:prefLabel>
    </owl:Class>
    


    <!-- http://www.semanticweb.org/david/ontologies/2013/0/1.3.6.1.4.1.19376.1.8.2.1.2171 -->

    <owl:Class rdf:about="&pathLex;2171">
        <rdfs:subClassOf rdf:resource="&pathLex;489"/>
        <skos:definition xml:lang="en">Cervix-Infiltrating malignant neoplasm-pM-pM1 [IVB] - Distant metastasis site(s)</skos:definition>
        <skos:prefLabel xml:lang="en">pM1 [IVB] - Distant metastasis site(s)</skos:prefLabel>
    </owl:Class>
    


    <!-- http://www.semanticweb.org/david/ontologies/2013/0/1.3.6.1.4.1.19376.1.8.2.1.2172 -->

    <owl:Class rdf:about="&pathLex;2172">
        <rdfs:subClassOf rdf:resource="&pathLex;99999"/>
        <skos:definition xml:lang="en">Colon-Infiltrating malignant neoplasm-pM-pM1: Distant metastasis</skos:definition>
        <skos:prefLabel xml:lang="en">pM1: Distant metastasis</skos:prefLabel>
    </owl:Class>
    


    <!-- http://www.semanticweb.org/david/ontologies/2013/0/1.3.6.1.4.1.19376.1.8.2.1.2173 -->

    <owl:Class rdf:about="&pathLex;2173">
        <rdfs:subClassOf rdf:resource="&pathLex;99999"/>
        <skos:definition xml:lang="en">Colon-Infiltrating malignant neoplasm-pM-pM1a: Metastasis to single organ or site (eg, liver, lung, ovary, nonregional lymph node)</skos:definition>
        <skos:prefLabel xml:lang="en">pM1a: Metastasis to single organ or site (eg, liver, lung, ovary, nonregional lymph node)</skos:prefLabel>
    </owl:Class>
    


    <!-- http://www.semanticweb.org/david/ontologies/2013/0/1.3.6.1.4.1.19376.1.8.2.1.2174 -->

    <owl:Class rdf:about="&pathLex;2174">
        <rdfs:subClassOf rdf:resource="&pathLex;99999"/>
        <skos:definition xml:lang="en">Colon-Infiltrating malignant neoplasm-pM-pM1b: Metastasis to more than one organ/site or to the peritoneum - Specify site(s)</skos:definition>
        <skos:prefLabel xml:lang="en">pM1b: Metastasis to more than one organ/site or to the peritoneum - Specify site(s)</skos:prefLabel>
    </owl:Class>
    


    <!-- http://www.semanticweb.org/david/ontologies/2013/0/1.3.6.1.4.1.19376.1.8.2.1.2175 -->

    <owl:Class rdf:about="&pathLex;2175">
        <rdfs:subClassOf rdf:resource="&pathLex;99999"/>
        <skos:definition xml:lang="en">Endometrium-Infiltrating malignant neoplasm-pM-pM1 [IVB]: Distant metastasis (includes metastasis to inguinal lymph nodes, intraperitoneal disease, or lung, liver, or bone metastasis. It excludes metastasis to para-aortic lymph nodes, vagina, pelvic serosa, or adnexa) - Specify site(s)</skos:definition>
        <skos:prefLabel xml:lang="en">pM1 [IVB]: Distant metastasis (includes metastasis to inguinal lymph nodes, intraperitoneal disease, or lung, liver, or bone metastasis. It excludes metastasis to para-aortic lymph nodes, vagina, pelvic serosa, or adnexa) - Specify site(s)</skos:prefLabel>
    </owl:Class>
    


    <!-- http://www.semanticweb.org/david/ontologies/2013/0/1.3.6.1.4.1.19376.1.8.2.1.2176 -->

    <owl:Class rdf:about="&pathLex;2176">
        <rdfs:subClassOf rdf:resource="&pathLex;99999"/>
        <skos:definition xml:lang="en">Stomach-Infiltrating malignant neoplasm-pM-pM1: Distant metastasis - Specify site(s)</skos:definition>
        <skos:prefLabel xml:lang="en">pM1: Distant metastasis - Specify site(s)</skos:prefLabel>
    </owl:Class>
    


    <!-- http://www.semanticweb.org/david/ontologies/2013/0/1.3.6.1.4.1.19376.1.8.2.1.2177 -->

    <owl:Class rdf:about="&pathLex;2177">
        <rdfs:subClassOf rdf:resource="&pathLex;99999"/>
        <skos:definition xml:lang="en">Liver-Infiltrating malignant neoplasm-PM-pM1: Distant metastasis - Specify site(s)</skos:definition>
        <skos:prefLabel xml:lang="en">pM1: Distant metastasis - Specify site(s)</skos:prefLabel>
    </owl:Class>
    


    <!-- http://www.semanticweb.org/david/ontologies/2013/0/1.3.6.1.4.1.19376.1.8.2.1.2178 -->

    <owl:Class rdf:about="&pathLex;2178">
        <rdfs:subClassOf rdf:resource="&pathLex;99999"/>
        <skos:definition xml:lang="en">Larynx-Infiltrating malignant neoplasm-pM-pM1: Distant metastasis - Specify site(s)</skos:definition>
        <skos:prefLabel xml:lang="en">pM1: Distant metastasis - Specify site(s)</skos:prefLabel>
    </owl:Class>
    


    <!-- http://www.semanticweb.org/david/ontologies/2013/0/1.3.6.1.4.1.19376.1.8.2.1.2179 -->

    <owl:Class rdf:about="&pathLex;2179">
        <rdfs:subClassOf rdf:resource="&pathLex;99999"/>
        <skos:definition xml:lang="en">Esophagus-Infiltrating malignant neoplasm-pM-pM1: Distant metastasis. Specify site(s)</skos:definition>
        <skos:prefLabel xml:lang="en">pM1: Distant metastasis. Specify site(s)</skos:prefLabel>
    </owl:Class>
    


    <!-- http://www.semanticweb.org/david/ontologies/2013/0/1.3.6.1.4.1.19376.1.8.2.1.218 -->

    <owl:Class rdf:about="&pathLex;218">
        <rdfs:subClassOf rdf:resource="&pathLex;99999"/>
        <skos:prefLabel xml:lang="en">Perineural invasion</skos:prefLabel>
        <skos:definition xml:lang="en">Salivary gland-Infiltrating malignant neoplasm-Perineural invasion</skos:definition>
    </owl:Class>
    


    <!-- http://www.semanticweb.org/david/ontologies/2013/0/1.3.6.1.4.1.19376.1.8.2.1.2180 -->

    <owl:Class rdf:about="&pathLex;2180">
        <rdfs:subClassOf rdf:resource="&pathLex;99999"/>
        <skos:definition xml:lang="en">Ovary-Infiltrating malignant neoplasm-pM-pM1 [IV]: Distant metastases (includes extraperitoneal sites such as liver parenchyma, lung, skeletal metastases, and supraclavicular and axillary nodes)</skos:definition>
        <skos:prefLabel xml:lang="en">pM1 [IV]: Distant metastases (includes extraperitoneal sites such as liver parenchyma, lung, skeletal metastases, and supraclavicular and axillary nodes)</skos:prefLabel>
    </owl:Class>
    


    <!-- http://www.semanticweb.org/david/ontologies/2013/0/1.3.6.1.4.1.19376.1.8.2.1.2182 -->

    <owl:Class rdf:about="&pathLex;2182">
        <rdfs:subClassOf rdf:resource="&pathLex;99999"/>
        <skos:definition xml:lang="en">Skin (melanoma)-Infiltrating malignant neoplasm-pM-pM1: Distant metastasis (documented in this specimen)</skos:definition>
        <skos:prefLabel xml:lang="en">pM1: Distant metastasis (documented in this specimen)</skos:prefLabel>
    </owl:Class>
    


    <!-- http://www.semanticweb.org/david/ontologies/2013/0/1.3.6.1.4.1.19376.1.8.2.1.2183 -->

    <owl:Class rdf:about="&pathLex;2183">
        <rdfs:subClassOf rdf:resource="&pathLex;99999"/>
        <skos:definition xml:lang="en">Skin (melanoma)-Infiltrating malignant neoplasm-pM-pM1a: Metastasis in skin, subcutaneous tissues, or distant lymph nodes</skos:definition>
        <skos:prefLabel xml:lang="en">pM1a: Metastasis in skin, subcutaneous tissues, or distant lymph nodes</skos:prefLabel>
    </owl:Class>
    


    <!-- http://www.semanticweb.org/david/ontologies/2013/0/1.3.6.1.4.1.19376.1.8.2.1.2184 -->

    <owl:Class rdf:about="&pathLex;2184">
        <rdfs:subClassOf rdf:resource="&pathLex;99999"/>
        <skos:definition xml:lang="en">Skin (melanoma)-Infiltrating malignant neoplasm-pM-pM1b: Metastasis to lung</skos:definition>
        <skos:prefLabel xml:lang="en">pM1b: Metastasis to lung</skos:prefLabel>
    </owl:Class>
    


    <!-- http://www.semanticweb.org/david/ontologies/2013/0/1.3.6.1.4.1.19376.1.8.2.1.2185 -->

    <owl:Class rdf:about="&pathLex;2185">
        <rdfs:subClassOf rdf:resource="&pathLex;99999"/>
        <skos:definition xml:lang="en">Skin (melanoma)-Infiltrating malignant neoplasm-pM-pM1c: Metastasis to all other visceral sites or distant metastasis at any site associated with an elevated serum lactic dehydrogenase (LDH)</skos:definition>
        <skos:prefLabel xml:lang="en">pM1c: Metastasis to all other visceral sites or distant metastasis at any site associated with an elevated serum lactic dehydrogenase (LDH)</skos:prefLabel>
    </owl:Class>
    


    <!-- http://www.semanticweb.org/david/ontologies/2013/0/1.3.6.1.4.1.19376.1.8.2.1.2186 -->

    <owl:Class rdf:about="&pathLex;2186">
        <rdfs:subClassOf rdf:resource="&pathLex;99999"/>
        <skos:definition xml:lang="en">Pharynx-Infiltrating malignant neoplasm-pM-pM1: Distant metastasis - Specify site(s)</skos:definition>
        <skos:prefLabel xml:lang="en">pM1: Distant metastasis - Specify site(s)</skos:prefLabel>
    </owl:Class>
    


    <!-- http://www.semanticweb.org/david/ontologies/2013/0/1.3.6.1.4.1.19376.1.8.2.1.2187 -->

    <owl:Class rdf:about="&pathLex;2187">
        <rdfs:subClassOf rdf:resource="&pathLex;99999"/>
        <skos:definition xml:lang="en">Lung-Infiltrating malignant neoplasm-pM-pM1a: Separate tumor nodule(s) in contralateral lung; tumor with pleural nodules or malignant pleural (or pericardial) effusion (Note A)</skos:definition>
        <skos:prefLabel xml:lang="en">pM1a: Separate tumor nodule(s) in contralateral lung; tumor with pleural nodules or malignant pleural (or pericardial) effusion (Note A)</skos:prefLabel>
    </owl:Class>
    


    <!-- http://www.semanticweb.org/david/ontologies/2013/0/1.3.6.1.4.1.19376.1.8.2.1.2188 -->

    <owl:Class rdf:about="&pathLex;2188">
        <rdfs:subClassOf rdf:resource="&pathLex;99999"/>
        <skos:definition xml:lang="en">Lung-Infiltrating malignant neoplasm-pM-pM1b: Distant metastases outside the lung/pleura</skos:definition>
        <skos:prefLabel xml:lang="en">pM1b: Distant metastases outside the lung/pleura</skos:prefLabel>
    </owl:Class>
    


    <!-- http://www.semanticweb.org/david/ontologies/2013/0/1.3.6.1.4.1.19376.1.8.2.1.2189 -->

    <owl:Class rdf:about="&pathLex;2189">
        <rdfs:subClassOf rdf:resource="&pathLex;99999"/>
        <skos:definition xml:lang="en">Prostate-Infiltrating malignant neoplasm-pM-pM1: Distant metastasis</skos:definition>
        <skos:prefLabel xml:lang="en">pM1: Distant metastasis</skos:prefLabel>
    </owl:Class>
    


    <!-- http://www.semanticweb.org/david/ontologies/2013/0/1.3.6.1.4.1.19376.1.8.2.1.219 -->

    <owl:Class rdf:about="&pathLex;219">
        <rdfs:subClassOf rdf:resource="&pathLex;99999"/>
        <skos:prefLabel xml:lang="en">Lymph node capsule involvement</skos:prefLabel>
        <skos:definition xml:lang="en">Salivary gland-Infiltrating malignant neoplasm-Lymph node capsule involvement</skos:definition>
    </owl:Class>
    


    <!-- http://www.semanticweb.org/david/ontologies/2013/0/1.3.6.1.4.1.19376.1.8.2.1.2190 -->

    <owl:Class rdf:about="&pathLex;2190">
        <rdfs:subClassOf rdf:resource="&pathLex;99999"/>
        <skos:definition xml:lang="en">Prostate-Infiltrating malignant neoplasm-pM-pM1a: Nonregional lymph nodes(s)</skos:definition>
        <skos:prefLabel xml:lang="en">pM1a: Nonregional lymph nodes(s)</skos:prefLabel>
    </owl:Class>
    


    <!-- http://www.semanticweb.org/david/ontologies/2013/0/1.3.6.1.4.1.19376.1.8.2.1.2191 -->

    <owl:Class rdf:about="&pathLex;2191">
        <rdfs:subClassOf rdf:resource="&pathLex;99999"/>
        <skos:definition xml:lang="en">Prostate-Infiltrating malignant neoplasm-pM-pM1b: Bone(s)</skos:definition>
        <skos:prefLabel xml:lang="en">pM1b: Bone(s)</skos:prefLabel>
    </owl:Class>
    


    <!-- http://www.semanticweb.org/david/ontologies/2013/0/1.3.6.1.4.1.19376.1.8.2.1.2192 -->

    <owl:Class rdf:about="&pathLex;2192">
        <rdfs:subClassOf rdf:resource="&pathLex;99999"/>
        <skos:definition xml:lang="en">Prostate-Infiltrating malignant neoplasm-pM-pM1c: Other site(s) with or without bone disease</skos:definition>
        <skos:prefLabel xml:lang="en">pM1c: Other site(s) with or without bone disease</skos:prefLabel>
    </owl:Class>
    


    <!-- http://www.semanticweb.org/david/ontologies/2013/0/1.3.6.1.4.1.19376.1.8.2.1.2193 -->

    <owl:Class rdf:about="&pathLex;2193">
        <rdfs:subClassOf rdf:resource="&pathLex;99999"/>
        <skos:definition xml:lang="en">Kidney-Infiltrating malignant neoplasm-pM-pM1: Distant metastasis</skos:definition>
        <skos:prefLabel xml:lang="en">pM1: Distant metastasis</skos:prefLabel>
    </owl:Class>
    


    <!-- http://www.semanticweb.org/david/ontologies/2013/0/1.3.6.1.4.1.19376.1.8.2.1.2194 -->

    <owl:Class rdf:about="&pathLex;2194">
        <rdfs:subClassOf rdf:resource="&pathLex;1903"/>
        <skos:definition xml:lang="en">Breast-Infiltrating malignant neoplasm-pM-cM0(i+) - No clinical or radiographic evidence of distant metastasis, but deposits of molecularly or microscopically detected tumor cells in circulating blood, bone marrow, or other nonregional nodal tissue that are &lt; = 0.2 mm in a patient without symptoms or signs of metastasis</skos:definition>
        <skos:prefLabel xml:lang="en">cM0(i+) - No clinical or radiographic evidence of distant metastasis, but deposits of molecularly or microscopically detected tumor cells in circulating blood, bone marrow, or other nonregional nodal tissue that are &lt; = 0.2 mm in a patient without symptoms or signs of metastasis</skos:prefLabel>
    </owl:Class>
    


    <!-- http://www.semanticweb.org/david/ontologies/2013/0/1.3.6.1.4.1.19376.1.8.2.1.2195 -->

    <owl:Class rdf:about="&pathLex;2195">
        <rdfs:subClassOf rdf:resource="&pathLex;1903"/>
        <skos:definition xml:lang="en">Breast-Infiltrating malignant neoplasm-pM-pM1 - Distant detectable metastasis as determined by classic clinical and radiographic means and/or histologically proven &gt;0.2 mm</skos:definition>
        <skos:prefLabel xml:lang="en">pM1 - Distant detectable metastasis as determined by classic clinical and radiographic means and/or histologically proven &gt;0.2 mm</skos:prefLabel>
    </owl:Class>
    


    <!-- http://www.semanticweb.org/david/ontologies/2013/0/1.3.6.1.4.1.19376.1.8.2.1.2197 -->

    <owl:Class rdf:about="&pathLex;2197">
        <rdfs:subClassOf rdf:resource="&pathLex;99999"/>
        <skos:definition xml:lang="en">Thyroid-Infiltrating malignant neoplasm-pM-pM1: Distant metastasis</skos:definition>
        <skos:prefLabel xml:lang="en">pM1: Distant metastasis</skos:prefLabel>
    </owl:Class>
    


    <!-- http://www.semanticweb.org/david/ontologies/2013/0/1.3.6.1.4.1.19376.1.8.2.1.2199 -->

    <owl:Class rdf:about="&pathLex;2199">
        <rdfs:subClassOf rdf:resource="&pathLex;209"/>
        <skos:definition xml:lang="en">Generic-Infiltrating malignant neoplasm-Lymph node sampling-Performed</skos:definition>
        <skos:prefLabel xml:lang="en">Performed</skos:prefLabel>
    </owl:Class>
    


    <!-- http://www.semanticweb.org/david/ontologies/2013/0/1.3.6.1.4.1.19376.1.8.2.1.220 -->

    <owl:Class rdf:about="&pathLex;220">
        <rdfs:subClassOf rdf:resource="&pathLex;99999"/>
        <skos:prefLabel xml:lang="en">Lymph node site</skos:prefLabel>
        <skos:definition xml:lang="en">Salivary gland-Infiltrating malignant neoplasm-Lymph node site</skos:definition>
    </owl:Class>
    


    <!-- http://www.semanticweb.org/david/ontologies/2013/0/1.3.6.1.4.1.19376.1.8.2.1.2200 -->

    <owl:Class rdf:about="&pathLex;2200">
        <rdfs:subClassOf rdf:resource="&pathLex;209"/>
        <skos:definition xml:lang="en">Generic-Infiltrating malignant neoplasm-Lymph node sampling-Sentinel lymph node(s)</skos:definition>
        <skos:prefLabel xml:lang="en">Sentinel lymph node(s)</skos:prefLabel>
    </owl:Class>
    


    <!-- http://www.semanticweb.org/david/ontologies/2013/0/1.3.6.1.4.1.19376.1.8.2.1.2201 -->

    <owl:Class rdf:about="&pathLex;2201">
        <rdfs:subClassOf rdf:resource="&pathLex;209"/>
        <skos:definition xml:lang="en">Generic-Infiltrating malignant neoplasm-Lymph node sampling-Not performed</skos:definition>
        <skos:prefLabel xml:lang="en">Not performed</skos:prefLabel>
    </owl:Class>
    


    <!-- http://www.semanticweb.org/david/ontologies/2013/0/1.3.6.1.4.1.19376.1.8.2.1.2202 -->

    <owl:Class rdf:about="&pathLex;2202">
        <rdfs:subClassOf rdf:resource="&pathLex;10009"/>
        <skos:definition xml:lang="en">Cervix-Specimen-Specimen collection procedure-Pelvic Exenteration</skos:definition>
        <skos:prefLabel xml:lang="en">Pelvic Exenteration</skos:prefLabel>
    </owl:Class>
    


    <!-- http://www.semanticweb.org/david/ontologies/2013/0/1.3.6.1.4.1.19376.1.8.2.1.2203 -->

    <owl:Class rdf:about="&pathLex;2203">
        <rdfs:subClassOf rdf:resource="&pathLex;10009"/>
        <skos:definition xml:lang="en">Cervix-Specimen-Specimen collection procedure-Cold knife cone excision</skos:definition>
        <skos:prefLabel xml:lang="en">Cold knife cone excision</skos:prefLabel>
    </owl:Class>
    


    <!-- http://www.semanticweb.org/david/ontologies/2013/0/1.3.6.1.4.1.19376.1.8.2.1.2204 -->

    <owl:Class rdf:about="&pathLex;2204">
        <rdfs:subClassOf rdf:resource="&pathLex;10009"/>
        <skos:definition xml:lang="en">Cervix-Specimen-Specimen collection procedure-Loop electrical excision procedure (LEEP)</skos:definition>
        <skos:prefLabel xml:lang="en">Loop electrical excision procedure (LEEP)</skos:prefLabel>
    </owl:Class>
    


    <!-- http://www.semanticweb.org/david/ontologies/2013/0/1.3.6.1.4.1.19376.1.8.2.1.2205 -->

    <owl:Class rdf:about="&pathLex;2205">
        <rdfs:subClassOf rdf:resource="&pathLex;10009"/>
        <skos:definition xml:lang="en">Cervix-Specimen-Specimen collection procedure-Large loop excision of the transformation zone (LLETZ)</skos:definition>
        <skos:prefLabel xml:lang="en">Large loop excision of the transformation zone (LLETZ)</skos:prefLabel>
    </owl:Class>
    


    <!-- http://www.semanticweb.org/david/ontologies/2013/0/1.3.6.1.4.1.19376.1.8.2.1.2206 -->

    <owl:Class rdf:about="&pathLex;2206">
        <rdfs:subClassOf rdf:resource="&pathLex;10009"/>
        <skos:definition xml:lang="en">Cervix-Specimen-Specimen collection procedure-Radical trachelectomy</skos:definition>
        <skos:prefLabel xml:lang="en">Radical trachelectomy</skos:prefLabel>
    </owl:Class>
    


    <!-- http://www.semanticweb.org/david/ontologies/2013/0/1.3.6.1.4.1.19376.1.8.2.1.2207 -->

    <owl:Class rdf:about="&pathLex;2207">
        <rdfs:subClassOf rdf:resource="&pathLex;99999"/>
        <skos:definition xml:lang="en">Colon-Specimen-Specimen collection procedure-Resection</skos:definition>
        <skos:prefLabel xml:lang="en">Resection</skos:prefLabel>
    </owl:Class>
    


    <!-- http://www.semanticweb.org/david/ontologies/2013/0/1.3.6.1.4.1.19376.1.8.2.1.2208 -->

    <owl:Class rdf:about="&pathLex;2208">
        <rdfs:subClassOf rdf:resource="&pathLex;99999"/>
        <skos:definition xml:lang="en">Colon-Specimen-Specimen collection procedure-Excisional Biopsy (Polypectomy)</skos:definition>
        <skos:prefLabel xml:lang="en">Excisional Biopsy (Polypectomy)</skos:prefLabel>
    </owl:Class>
    


    <!-- http://www.semanticweb.org/david/ontologies/2013/0/1.3.6.1.4.1.19376.1.8.2.1.2209 -->

    <owl:Class rdf:about="&pathLex;2209">
        <rdfs:subClassOf rdf:resource="&pathLex;99999"/>
        <skos:definition xml:lang="en">Colon-Specimen-Specimen collection procedure-Transanal Disk Excision of Rectal Neoplasms</skos:definition>
        <skos:prefLabel xml:lang="en">Transanal Disk Excision of Rectal Neoplasms</skos:prefLabel>
    </owl:Class>
    


    <!-- http://www.semanticweb.org/david/ontologies/2013/0/1.3.6.1.4.1.19376.1.8.2.1.221 -->

    <owl:Class rdf:about="&pathLex;221">
        <rdfs:subClassOf rdf:resource="&pathLex;99999"/>
        <skos:prefLabel xml:lang="en">Number of lymph nodes involved</skos:prefLabel>
        <skos:definition xml:lang="en">Salivary gland-Infiltrating malignant neoplasm-Number of lymph nodes involved</skos:definition>
    </owl:Class>
    


    <!-- http://www.semanticweb.org/david/ontologies/2013/0/1.3.6.1.4.1.19376.1.8.2.1.2210 -->

    <owl:Class rdf:about="&pathLex;2210">
        <rdfs:subClassOf rdf:resource="&pathLex;99999"/>
        <skos:definition xml:lang="en">Endometrium-Specimen-Specimen collection procedure-Simple hysterectomy</skos:definition>
        <skos:prefLabel xml:lang="en">Simple hysterectomy</skos:prefLabel>
    </owl:Class>
    


    <!-- http://www.semanticweb.org/david/ontologies/2013/0/1.3.6.1.4.1.19376.1.8.2.1.2211 -->

    <owl:Class rdf:about="&pathLex;2211">
        <rdfs:subClassOf rdf:resource="&pathLex;99999"/>
        <skos:definition xml:lang="en">Endometrium-Specimen-Specimen collection procedure-Oophorectomy (Qualifier: laterality - Right,Left) Bilateral?</skos:definition>
        <skos:prefLabel xml:lang="en">Oophorectomy (Qualifier: laterality - Right,Left) Bilateral?</skos:prefLabel>
    </owl:Class>
    


    <!-- http://www.semanticweb.org/david/ontologies/2013/0/1.3.6.1.4.1.19376.1.8.2.1.2212 -->

    <owl:Class rdf:about="&pathLex;2212">
        <rdfs:subClassOf rdf:resource="&pathLex;99999"/>
        <skos:definition xml:lang="en">Endometrium-Specimen-Specimen collection procedure-Salpingectomy (Qualifier: laterality - Right,Left) Bilateral?</skos:definition>
        <skos:prefLabel xml:lang="en">Salpingectomy (Qualifier: laterality - Right,Left) Bilateral?</skos:prefLabel>
    </owl:Class>
    


    <!-- http://www.semanticweb.org/david/ontologies/2013/0/1.3.6.1.4.1.19376.1.8.2.1.2213 -->

    <owl:Class rdf:about="&pathLex;2213">
        <rdfs:subClassOf rdf:resource="&pathLex;99999"/>
        <skos:definition xml:lang="en">Endometrium-Specimen-Specimen collection procedure-Salpingo-oophorectomy (Qualifier: laterality - Right,Left, Bilateral)</skos:definition>
        <skos:prefLabel xml:lang="en">Salpingo-oophorectomy (Qualifier: laterality - Right,Left, Bilateral)</skos:prefLabel>
    </owl:Class>
    


    <!-- http://www.semanticweb.org/david/ontologies/2013/0/1.3.6.1.4.1.19376.1.8.2.1.2214 -->

    <owl:Class rdf:about="&pathLex;2214">
        <rdfs:subClassOf rdf:resource="&pathLex;99999"/>
        <skos:definition xml:lang="en">Endometrium-Specimen-Specimen collection procedure-Omentectomy</skos:definition>
        <skos:prefLabel xml:lang="en">Omentectomy</skos:prefLabel>
    </owl:Class>
    


    <!-- http://www.semanticweb.org/david/ontologies/2013/0/1.3.6.1.4.1.19376.1.8.2.1.2215 -->

    <owl:Class rdf:about="&pathLex;2215">
        <rdfs:subClassOf rdf:resource="&pathLex;99999"/>
        <skos:definition xml:lang="en">Endometrium-Specimen-Specimen collection procedure-Peritoneal biopsies</skos:definition>
        <skos:prefLabel xml:lang="en">Peritoneal biopsies</skos:prefLabel>
    </owl:Class>
    


    <!-- http://www.semanticweb.org/david/ontologies/2013/0/1.3.6.1.4.1.19376.1.8.2.1.2216 -->

    <owl:Class rdf:about="&pathLex;2216">
        <rdfs:subClassOf rdf:resource="&pathLex;99999"/>
        <skos:prefLabel xml:lang="en">Partial gastrectomy, Other</skos:prefLabel>
        <skos:definition xml:lang="en">Stomach-Specimen-Specimen collection procedure-Partial gastrectomy, Other</skos:definition>
    </owl:Class>
    


    <!-- http://www.semanticweb.org/david/ontologies/2013/0/1.3.6.1.4.1.19376.1.8.2.1.2217 -->

    <owl:Class rdf:about="&pathLex;2217">
        <rdfs:subClassOf rdf:resource="&pathLex;99999"/>
        <skos:definition xml:lang="en">Liver-Specimen-Specimen collection procedure-Wedge resection</skos:definition>
        <skos:prefLabel xml:lang="en">Wedge resection</skos:prefLabel>
    </owl:Class>
    


    <!-- http://www.semanticweb.org/david/ontologies/2013/0/1.3.6.1.4.1.19376.1.8.2.1.2218 -->

    <owl:Class rdf:about="&pathLex;2218">
        <rdfs:subClassOf rdf:resource="&pathLex;99999"/>
        <skos:definition xml:lang="en">Liver-Specimen-Specimen collection procedure-Partial hepatectomy: Major hepatectomy (3 segments or more)</skos:definition>
        <skos:prefLabel xml:lang="en">Partial hepatectomy: Major hepatectomy (3 segments or more)</skos:prefLabel>
    </owl:Class>
    


    <!-- http://www.semanticweb.org/david/ontologies/2013/0/1.3.6.1.4.1.19376.1.8.2.1.2219 -->

    <owl:Class rdf:about="&pathLex;2219">
        <rdfs:subClassOf rdf:resource="&pathLex;99999"/>
        <skos:definition xml:lang="en">Liver-Specimen-Specimen collection procedure-Partial hepatectomy: Minor hepatectomy (less than 3 segments)</skos:definition>
        <skos:prefLabel xml:lang="en">Partial hepatectomy: Minor hepatectomy (less than 3 segments)</skos:prefLabel>
    </owl:Class>
    


    <!-- http://www.semanticweb.org/david/ontologies/2013/0/1.3.6.1.4.1.19376.1.8.2.1.222 -->

    <owl:Class rdf:about="&pathLex;222">
        <rdfs:subClassOf rdf:resource="&pathLex;99999"/>
        <skos:prefLabel xml:lang="en">Number of lymph nodes examined</skos:prefLabel>
        <skos:definition xml:lang="en">Salivary gland-Infiltrating malignant neoplasm-Number of lymph nodes examined</skos:definition>
    </owl:Class>
    


    <!-- http://www.semanticweb.org/david/ontologies/2013/0/1.3.6.1.4.1.19376.1.8.2.1.2221 -->

    <owl:Class rdf:about="&pathLex;2221">
        <rdfs:subClassOf rdf:resource="&pathLex;99999"/>
        <skos:prefLabel xml:lang="en">Incisional biopsy (qualifier: right, left)</skos:prefLabel>
        <skos:definition xml:lang="en">Salivary gland-Specimen-Specimen collection procedure-Incisional biopsy (qualifier: right, left)</skos:definition>
    </owl:Class>
    


    <!-- http://www.semanticweb.org/david/ontologies/2013/0/1.3.6.1.4.1.19376.1.8.2.1.2222 -->

    <owl:Class rdf:about="&pathLex;2222">
        <rdfs:subClassOf rdf:resource="&pathLex;99999"/>
        <skos:prefLabel xml:lang="en">Excisional biopsy (qualifier: right, left)</skos:prefLabel>
        <skos:definition xml:lang="en">Salivary gland-Specimen-Specimen collection procedure-Excisional biopsy (qualifier: right, left)</skos:definition>
    </owl:Class>
    


    <!-- http://www.semanticweb.org/david/ontologies/2013/0/1.3.6.1.4.1.19376.1.8.2.1.2223 -->

    <owl:Class rdf:about="&pathLex;2223">
        <rdfs:subClassOf rdf:resource="&pathLex;99999"/>
        <skos:prefLabel xml:lang="en">Resection, parotid gland (qualifier: right, left)</skos:prefLabel>
        <skos:definition xml:lang="en">Salivary gland-Specimen-Specimen collection procedure-Resection, parotid gland (qualifier: right, left)</skos:definition>
    </owl:Class>
    


    <!-- http://www.semanticweb.org/david/ontologies/2013/0/1.3.6.1.4.1.19376.1.8.2.1.2224 -->

    <owl:Class rdf:about="&pathLex;2224">
        <rdfs:subClassOf rdf:resource="&pathLex;99999"/>
        <skos:prefLabel xml:lang="en">Resection, submandibular gland (qualifier: right, left)</skos:prefLabel>
        <skos:definition xml:lang="en">Salivary gland-Specimen-Specimen collection procedure-Resection, submandibular gland (qualifier: right, left)</skos:definition>
    </owl:Class>
    


    <!-- http://www.semanticweb.org/david/ontologies/2013/0/1.3.6.1.4.1.19376.1.8.2.1.2225 -->

    <owl:Class rdf:about="&pathLex;2225">
        <rdfs:subClassOf rdf:resource="&pathLex;99999"/>
        <skos:prefLabel xml:lang="en">Resection, sublingual gland (qualifier: right, left)</skos:prefLabel>
        <skos:definition xml:lang="en">Salivary gland-Specimen-Specimen collection procedure-Resection, sublingual gland (qualifier: right, left)</skos:definition>
    </owl:Class>
    


    <!-- http://www.semanticweb.org/david/ontologies/2013/0/1.3.6.1.4.1.19376.1.8.2.1.2226 -->

    <owl:Class rdf:about="&pathLex;2226">
        <rdfs:subClassOf rdf:resource="&pathLex;99999"/>
        <skos:prefLabel xml:lang="en">Neck (lymph node) dissection (specify)</skos:prefLabel>
        <skos:definition xml:lang="en">Salivary gland-Specimen-Specimen collection procedure-Neck (lymph node) dissection (specify)</skos:definition>
    </owl:Class>
    


    <!-- http://www.semanticweb.org/david/ontologies/2013/0/1.3.6.1.4.1.19376.1.8.2.1.2227 -->

    <owl:Class rdf:about="&pathLex;2227">
        <rdfs:subClassOf rdf:resource="&pathLex;99999"/>
        <skos:prefLabel xml:lang="en">Incisional biopsy</skos:prefLabel>
        <skos:definition xml:lang="en">Larynx-Specimen-Specimen collection procedure-Incisional biopsy</skos:definition>
    </owl:Class>
    


    <!-- http://www.semanticweb.org/david/ontologies/2013/0/1.3.6.1.4.1.19376.1.8.2.1.2228 -->

    <owl:Class rdf:about="&pathLex;2228">
        <rdfs:subClassOf rdf:resource="&pathLex;99999"/>
        <skos:prefLabel xml:lang="en">Excisional biopsy</skos:prefLabel>
        <skos:definition xml:lang="en">Larynx-Specimen-Specimen collection procedure-Excisional biopsy</skos:definition>
    </owl:Class>
    


    <!-- http://www.semanticweb.org/david/ontologies/2013/0/1.3.6.1.4.1.19376.1.8.2.1.2229 -->

    <owl:Class rdf:about="&pathLex;2229">
        <rdfs:subClassOf rdf:resource="&pathLex;99999"/>
        <skos:definition xml:lang="en">Larynx-Specimen-Specimen collection procedure-Resection</skos:definition>
        <skos:prefLabel xml:lang="en">Resection</skos:prefLabel>
    </owl:Class>
    


    <!-- http://www.semanticweb.org/david/ontologies/2013/0/1.3.6.1.4.1.19376.1.8.2.1.2230 -->

    <owl:Class rdf:about="&pathLex;2230">
        <rdfs:subClassOf rdf:resource="&pathLex;99999"/>
        <skos:definition xml:lang="en">Larynx-Specimen-Specimen collection procedure-Stripping (glottis)</skos:definition>
        <skos:prefLabel xml:lang="en">Stripping (glottis)</skos:prefLabel>
    </owl:Class>
    


    <!-- http://www.semanticweb.org/david/ontologies/2013/0/1.3.6.1.4.1.19376.1.8.2.1.2231 -->

    <owl:Class rdf:about="&pathLex;2231">
        <rdfs:subClassOf rdf:resource="&pathLex;99999"/>
        <skos:definition xml:lang="en">Larynx-Specimen-Specimen collection procedure-Transoral laser excision (glottis)</skos:definition>
        <skos:prefLabel xml:lang="en">Transoral laser excision (glottis)</skos:prefLabel>
    </owl:Class>
    


    <!-- http://www.semanticweb.org/david/ontologies/2013/0/1.3.6.1.4.1.19376.1.8.2.1.2232 -->

    <owl:Class rdf:about="&pathLex;2232">
        <rdfs:subClassOf rdf:resource="&pathLex;99999"/>
        <skos:definition xml:lang="en">Larynx-Specimen-Specimen collection procedure-Supraglottic laryngectomy</skos:definition>
        <skos:prefLabel xml:lang="en">Supraglottic laryngectomy</skos:prefLabel>
    </owl:Class>
    


    <!-- http://www.semanticweb.org/david/ontologies/2013/0/1.3.6.1.4.1.19376.1.8.2.1.2233 -->

    <owl:Class rdf:about="&pathLex;2233">
        <rdfs:subClassOf rdf:resource="&pathLex;99999"/>
        <skos:definition xml:lang="en">Larynx-Specimen-Specimen collection procedure-Supracricoid laryngectomy</skos:definition>
        <skos:prefLabel xml:lang="en">Supracricoid laryngectomy</skos:prefLabel>
    </owl:Class>
    


    <!-- http://www.semanticweb.org/david/ontologies/2013/0/1.3.6.1.4.1.19376.1.8.2.1.2234 -->

    <owl:Class rdf:about="&pathLex;2234">
        <rdfs:subClassOf rdf:resource="&pathLex;99999"/>
        <skos:definition xml:lang="en">Larynx-Specimen-Specimen collection procedure-Vertical hemilaryngectomy (qualifier: right, left)</skos:definition>
        <skos:prefLabel xml:lang="en">Vertical hemilaryngectomy (qualifier: right, left)</skos:prefLabel>
    </owl:Class>
    


    <!-- http://www.semanticweb.org/david/ontologies/2013/0/1.3.6.1.4.1.19376.1.8.2.1.2235 -->

    <owl:Class rdf:about="&pathLex;2235">
        <rdfs:subClassOf rdf:resource="&pathLex;99999"/>
        <skos:definition xml:lang="en">Larynx-Specimen-Specimen collection procedure-Neck (lymph node) dissection (specify)</skos:definition>
        <skos:prefLabel xml:lang="en">Neck (lymph node) dissection (specify)</skos:prefLabel>
    </owl:Class>
    


    <!-- http://www.semanticweb.org/david/ontologies/2013/0/1.3.6.1.4.1.19376.1.8.2.1.2236 -->

    <owl:Class rdf:about="&pathLex;2236">
        <rdfs:subClassOf rdf:resource="&pathLex;99999"/>
        <skos:prefLabel xml:lang="en">Esophagogastrectomy</skos:prefLabel>
        <skos:definition xml:lang="en">Esophagus-Specimen-Specimen collection procedure-Esophagogastrectomy</skos:definition>
    </owl:Class>
    


    <!-- http://www.semanticweb.org/david/ontologies/2013/0/1.3.6.1.4.1.19376.1.8.2.1.2237 -->

    <owl:Class rdf:about="&pathLex;2237">
        <rdfs:subClassOf rdf:resource="&pathLex;99999"/>
        <skos:prefLabel xml:lang="en">Esophagectomy</skos:prefLabel>
        <skos:definition xml:lang="en">Esophagus-Specimen-Specimen collection procedure-Esophagectomy</skos:definition>
    </owl:Class>
    


    <!-- http://www.semanticweb.org/david/ontologies/2013/0/1.3.6.1.4.1.19376.1.8.2.1.2238 -->

    <owl:Class rdf:about="&pathLex;2238">
        <rdfs:subClassOf rdf:resource="&pathLex;99999"/>
        <skos:definition xml:lang="en">Ovary-Specimen-Specimen collection procedure-Subtotal oophorectomy</skos:definition>
        <skos:prefLabel xml:lang="en">Subtotal oophorectomy</skos:prefLabel>
    </owl:Class>
    


    <!-- http://www.semanticweb.org/david/ontologies/2013/0/1.3.6.1.4.1.19376.1.8.2.1.2239 -->

    <owl:Class rdf:about="&pathLex;2239">
        <rdfs:subClassOf rdf:resource="&pathLex;99999"/>
        <skos:definition xml:lang="en">Ovary-Specimen-Specimen collection procedure-Supracervical hysterectomy</skos:definition>
        <skos:prefLabel xml:lang="en">Supracervical hysterectomy</skos:prefLabel>
    </owl:Class>
    


    <!-- http://www.semanticweb.org/david/ontologies/2013/0/1.3.6.1.4.1.19376.1.8.2.1.224 -->

    <owl:Class rdf:about="&pathLex;224">
        <rdfs:subClassOf rdf:resource="&pathLex;99999"/>
        <skos:definition xml:lang="en">Salivary gland-Infiltrating malignant neoplasm-pN</skos:definition>
        <skos:prefLabel xml:lang="en">pN</skos:prefLabel>
    </owl:Class>
    


    <!-- http://www.semanticweb.org/david/ontologies/2013/0/1.3.6.1.4.1.19376.1.8.2.1.2240 -->

    <owl:Class rdf:about="&pathLex;2240">
        <rdfs:subClassOf rdf:resource="&pathLex;99999"/>
        <skos:prefLabel xml:lang="en">Hysterectomy</skos:prefLabel>
        <skos:definition xml:lang="en">Ovary-Specimen-Specimen collection procedure-Hysterectomy</skos:definition>
    </owl:Class>
    


    <!-- http://www.semanticweb.org/david/ontologies/2013/0/1.3.6.1.4.1.19376.1.8.2.1.2241 -->

    <owl:Class rdf:about="&pathLex;2241">
        <rdfs:subClassOf rdf:resource="&pathLex;99999"/>
        <skos:definition xml:lang="en">Ovary-Specimen-Specimen collection procedure-Peritoneal biopsies</skos:definition>
        <skos:prefLabel xml:lang="en">Peritoneal biopsies</skos:prefLabel>
    </owl:Class>
    


    <!-- http://www.semanticweb.org/david/ontologies/2013/0/1.3.6.1.4.1.19376.1.8.2.1.2242 -->

    <owl:Class rdf:about="&pathLex;2242">
        <rdfs:subClassOf rdf:resource="&pathLex;99999"/>
        <skos:definition xml:lang="en">Pancreas-Specimen-Specimen collection procedure-Pancreaticoduodenectomy (Whipple resection), partial pancreatectomy</skos:definition>
        <skos:prefLabel xml:lang="en">Pancreaticoduodenectomy (Whipple resection), partial pancreatectomy</skos:prefLabel>
    </owl:Class>
    


    <!-- http://www.semanticweb.org/david/ontologies/2013/0/1.3.6.1.4.1.19376.1.8.2.1.2243 -->

    <owl:Class rdf:about="&pathLex;2243">
        <rdfs:subClassOf rdf:resource="&pathLex;99999"/>
        <skos:prefLabel xml:lang="en">Biopsy, shave</skos:prefLabel>
        <skos:definition xml:lang="en">Skin (melanoma)-Specimen-Specimen collection procedure-Biopsy, shave</skos:definition>
    </owl:Class>
    


    <!-- http://www.semanticweb.org/david/ontologies/2013/0/1.3.6.1.4.1.19376.1.8.2.1.2244 -->

    <owl:Class rdf:about="&pathLex;2244">
        <rdfs:subClassOf rdf:resource="&pathLex;99999"/>
        <skos:prefLabel xml:lang="en">Biopsy, punch</skos:prefLabel>
        <skos:definition xml:lang="en">Skin (melanoma)-Specimen-Specimen collection procedure-Biopsy, punch</skos:definition>
    </owl:Class>
    


    <!-- http://www.semanticweb.org/david/ontologies/2013/0/1.3.6.1.4.1.19376.1.8.2.1.2245 -->

    <owl:Class rdf:about="&pathLex;2245">
        <rdfs:subClassOf rdf:resource="&pathLex;99999"/>
        <skos:prefLabel xml:lang="en">Biopsy, incisional</skos:prefLabel>
        <skos:definition xml:lang="en">Skin (melanoma)-Specimen-Specimen collection procedure-Biopsy, incisional</skos:definition>
    </owl:Class>
    


    <!-- http://www.semanticweb.org/david/ontologies/2013/0/1.3.6.1.4.1.19376.1.8.2.1.2246 -->

    <owl:Class rdf:about="&pathLex;2246">
        <rdfs:subClassOf rdf:resource="&pathLex;99999"/>
        <skos:prefLabel xml:lang="en">Re-excision</skos:prefLabel>
        <skos:definition xml:lang="en">Skin (melanoma)-Specimen-Specimen collection procedure-Re-excision</skos:definition>
    </owl:Class>
    


    <!-- http://www.semanticweb.org/david/ontologies/2013/0/1.3.6.1.4.1.19376.1.8.2.1.2247 -->

    <owl:Class rdf:about="&pathLex;2247">
        <rdfs:subClassOf rdf:resource="&pathLex;99999"/>
        <skos:prefLabel xml:lang="en">Incisional biopsy</skos:prefLabel>
        <skos:definition xml:lang="en">Pharynx-Specimen-Specimen collection procedure-Incisional biopsy</skos:definition>
    </owl:Class>
    


    <!-- http://www.semanticweb.org/david/ontologies/2013/0/1.3.6.1.4.1.19376.1.8.2.1.2248 -->

    <owl:Class rdf:about="&pathLex;2248">
        <rdfs:subClassOf rdf:resource="&pathLex;99999"/>
        <skos:prefLabel xml:lang="en">Excisional biopsy</skos:prefLabel>
        <skos:definition xml:lang="en">Pharynx-Specimen-Specimen collection procedure-Excisional biopsy</skos:definition>
    </owl:Class>
    


    <!-- http://www.semanticweb.org/david/ontologies/2013/0/1.3.6.1.4.1.19376.1.8.2.1.2249 -->

    <owl:Class rdf:about="&pathLex;2249">
        <rdfs:subClassOf rdf:resource="&pathLex;99999"/>
        <skos:definition xml:lang="en">Pharynx-Specimen-Specimen collection procedure-Resection</skos:definition>
        <skos:prefLabel xml:lang="en">Resection</skos:prefLabel>
    </owl:Class>
    


    <!-- http://www.semanticweb.org/david/ontologies/2013/0/1.3.6.1.4.1.19376.1.8.2.1.2250 -->

    <owl:Class rdf:about="&pathLex;2250">
        <rdfs:subClassOf rdf:resource="&pathLex;99999"/>
        <skos:definition xml:lang="en">Pharynx-Specimen-Specimen collection procedure-Tonsillectomy</skos:definition>
        <skos:prefLabel xml:lang="en">Tonsillectomy</skos:prefLabel>
    </owl:Class>
    


    <!-- http://www.semanticweb.org/david/ontologies/2013/0/1.3.6.1.4.1.19376.1.8.2.1.2251 -->

    <owl:Class rdf:about="&pathLex;2251">
        <rdfs:subClassOf rdf:resource="&pathLex;99999"/>
        <skos:definition xml:lang="en">Lung-Specimen-Specimen collection procedure-Major airway resection</skos:definition>
        <skos:prefLabel xml:lang="en">Major airway resection</skos:prefLabel>
    </owl:Class>
    


    <!-- http://www.semanticweb.org/david/ontologies/2013/0/1.3.6.1.4.1.19376.1.8.2.1.2252 -->

    <owl:Class rdf:about="&pathLex;2252">
        <rdfs:subClassOf rdf:resource="&pathLex;99999"/>
        <skos:definition xml:lang="en">Lung-Specimen-Specimen collection procedure-Wedge resection</skos:definition>
        <skos:prefLabel xml:lang="en">Wedge resection</skos:prefLabel>
    </owl:Class>
    


    <!-- http://www.semanticweb.org/david/ontologies/2013/0/1.3.6.1.4.1.19376.1.8.2.1.2253 -->

    <owl:Class rdf:about="&pathLex;2253">
        <rdfs:subClassOf rdf:resource="&pathLex;99999"/>
        <skos:definition xml:lang="en">Prostate-Specimen-Specimen collection procedure-Transurethral prostatic resection (enucleation)</skos:definition>
        <skos:prefLabel xml:lang="en">Transurethral prostatic resection (enucleation)</skos:prefLabel>
    </owl:Class>
    


    <!-- http://www.semanticweb.org/david/ontologies/2013/0/1.3.6.1.4.1.19376.1.8.2.1.2254 -->

    <owl:Class rdf:about="&pathLex;2254">
        <rdfs:subClassOf rdf:resource="&pathLex;99999"/>
        <skos:prefLabel xml:lang="en">Incisional biopsy, needle</skos:prefLabel>
        <skos:definition xml:lang="en">Kidney-Specimen-Specimen collection procedure-Incisional biopsy, needle</skos:definition>
    </owl:Class>
    


    <!-- http://www.semanticweb.org/david/ontologies/2013/0/1.3.6.1.4.1.19376.1.8.2.1.2255 -->

    <owl:Class rdf:about="&pathLex;2255">
        <rdfs:subClassOf rdf:resource="&pathLex;99999"/>
        <skos:prefLabel xml:lang="en">Incisional biopsy, wedge</skos:prefLabel>
        <skos:definition xml:lang="en">Kidney-Specimen-Specimen collection procedure-Incisional biopsy, wedge</skos:definition>
    </owl:Class>
    


    <!-- http://www.semanticweb.org/david/ontologies/2013/0/1.3.6.1.4.1.19376.1.8.2.1.2256 -->

    <owl:Class rdf:about="&pathLex;2256">
        <rdfs:subClassOf rdf:resource="&pathLex;10009"/>
        <skos:definition xml:lang="en">Breast-Specimen-Specimen collection procedure-Excision without wire-guided localization</skos:definition>
        <skos:prefLabel xml:lang="en">Excision without wire-guided localization</skos:prefLabel>
    </owl:Class>
    


    <!-- http://www.semanticweb.org/david/ontologies/2013/0/1.3.6.1.4.1.19376.1.8.2.1.2257 -->

    <owl:Class rdf:about="&pathLex;2257">
        <rdfs:subClassOf rdf:resource="&pathLex;10009"/>
        <skos:definition xml:lang="en">Breast-Specimen-Specimen collection procedure-Excision with wire-guided localization</skos:definition>
        <skos:prefLabel xml:lang="en">Excision with wire-guided localization</skos:prefLabel>
    </owl:Class>
    


    <!-- http://www.semanticweb.org/david/ontologies/2013/0/1.3.6.1.4.1.19376.1.8.2.1.2258 -->

    <owl:Class rdf:about="&pathLex;2258">
        <rdfs:subClassOf rdf:resource="&pathLex;99999"/>
        <skos:definition xml:lang="en">Thyroid-Specimen-Specimen collection procedure-Total thyroidectomy with central compartment dissection</skos:definition>
        <skos:prefLabel xml:lang="en">Total thyroidectomy with central compartment dissection</skos:prefLabel>
    </owl:Class>
    


    <!-- http://www.semanticweb.org/david/ontologies/2013/0/1.3.6.1.4.1.19376.1.8.2.1.2259 -->

    <owl:Class rdf:about="&pathLex;2259">
        <rdfs:subClassOf rdf:resource="&pathLex;99999"/>
        <skos:definition xml:lang="en">Thyroid-Specimen-Specimen collection procedure-Total thyroidectomy with neck dissection</skos:definition>
        <skos:prefLabel xml:lang="en">Total thyroidectomy with neck dissection</skos:prefLabel>
    </owl:Class>
    


    <!-- http://www.semanticweb.org/david/ontologies/2013/0/1.3.6.1.4.1.19376.1.8.2.1.226 -->

    <owl:Class rdf:about="&pathLex;226">
        <rdfs:subClassOf rdf:resource="&pathLex;99999"/>
        <skos:definition xml:lang="en">Salivary gland-Infiltrating malignant neoplasm-pT</skos:definition>
        <skos:prefLabel xml:lang="en">pT</skos:prefLabel>
    </owl:Class>
    


    <!-- http://www.semanticweb.org/david/ontologies/2013/0/1.3.6.1.4.1.19376.1.8.2.1.2260 -->

    <owl:Class rdf:about="&pathLex;2260">
        <rdfs:subClassOf rdf:resource="&pathLex;99999"/>
        <skos:definition xml:lang="en">Pharynx-Infiltrating malignant neoplasm-pT oropharynx carcinoma-pT0: No evidence of primary tumor</skos:definition>
        <skos:prefLabel xml:lang="en">pT0: No evidence of primary tumor</skos:prefLabel>
    </owl:Class>
    


    <!-- http://www.semanticweb.org/david/ontologies/2013/0/1.3.6.1.4.1.19376.1.8.2.1.2261 -->

    <owl:Class rdf:about="&pathLex;2261">
        <rdfs:subClassOf rdf:resource="&pathLex;99999"/>
        <skos:definition xml:lang="en">Pharynx-Infiltrating malignant neoplasm-pT oropharynx carcinoma-pTis: Carcinoma in situ</skos:definition>
        <skos:prefLabel xml:lang="en">pTis: Carcinoma in situ</skos:prefLabel>
    </owl:Class>
    


    <!-- http://www.semanticweb.org/david/ontologies/2013/0/1.3.6.1.4.1.19376.1.8.2.1.2262 -->

    <owl:Class rdf:about="&pathLex;2262">
        <rdfs:subClassOf rdf:resource="&pathLex;99999"/>
        <skos:definition xml:lang="en">Pharynx-Infiltrating malignant neoplasm-pT oropharynx carcinoma-pT1: Tumor 2 cm or less in greatest dimension</skos:definition>
        <skos:prefLabel xml:lang="en">pT1: Tumor 2 cm or less in greatest dimension</skos:prefLabel>
    </owl:Class>
    


    <!-- http://www.semanticweb.org/david/ontologies/2013/0/1.3.6.1.4.1.19376.1.8.2.1.2263 -->

    <owl:Class rdf:about="&pathLex;2263">
        <rdfs:subClassOf rdf:resource="&pathLex;99999"/>
        <skos:definition xml:lang="en">Pharynx-Infiltrating malignant neoplasm-pT oropharynx carcinoma-pT2: Tumor more than 2 cm but not more than 4 cm in greatest dimension</skos:definition>
        <skos:prefLabel xml:lang="en">pT2: Tumor more than 2 cm but not more than 4 cm in greatest dimension</skos:prefLabel>
    </owl:Class>
    


    <!-- http://www.semanticweb.org/david/ontologies/2013/0/1.3.6.1.4.1.19376.1.8.2.1.2264 -->

    <owl:Class rdf:about="&pathLex;2264">
        <rdfs:subClassOf rdf:resource="&pathLex;99999"/>
        <skos:definition xml:lang="en">Pharynx-Infiltrating malignant neoplasm-pT oropharynx carcinoma-pT3: Tumor more than 4 cm in greatest dimension or extension to lingual surface of epiglottis</skos:definition>
        <skos:prefLabel xml:lang="en">pT3: Tumor more than 4 cm in greatest dimension or extension to lingual surface of epiglottis</skos:prefLabel>
    </owl:Class>
    


    <!-- http://www.semanticweb.org/david/ontologies/2013/0/1.3.6.1.4.1.19376.1.8.2.1.2265 -->

    <owl:Class rdf:about="&pathLex;2265">
        <rdfs:subClassOf rdf:resource="&pathLex;99999"/>
        <skos:definition xml:lang="en">Pharynx-Infiltrating malignant neoplasm-pT oropharynx carcinoma-pT4a: Moderately advanced local disease. Tumor invades larynx, deep/extrinsic muscle of tongue, medial pterygoid muscles, hard palate, or mandible</skos:definition>
        <skos:prefLabel xml:lang="en">pT4a: Moderately advanced local disease. Tumor invades larynx, deep/extrinsic muscle of tongue, medial pterygoid muscles, hard palate, or mandible</skos:prefLabel>
    </owl:Class>
    


    <!-- http://www.semanticweb.org/david/ontologies/2013/0/1.3.6.1.4.1.19376.1.8.2.1.2266 -->

    <owl:Class rdf:about="&pathLex;2266">
        <rdfs:subClassOf rdf:resource="&pathLex;99999"/>
        <skos:definition xml:lang="en">Pharynx-Infiltrating malignant neoplasm-pT oropharynx carcinoma-pT4b: Very advanced local disease. Tumor invades lateral pterygoid muscle, pterygoid plates, lateral nasopharynx, or skull base, or encases carotid artery</skos:definition>
        <skos:prefLabel xml:lang="en">pT4b: Very advanced local disease. Tumor invades lateral pterygoid muscle, pterygoid plates, lateral nasopharynx, or skull base, or encases carotid artery</skos:prefLabel>
    </owl:Class>
    


    <!-- http://www.semanticweb.org/david/ontologies/2013/0/1.3.6.1.4.1.19376.1.8.2.1.2267 -->

    <owl:Class rdf:about="&pathLex;2267">
        <rdfs:subClassOf rdf:resource="&pathLex;431"/>
        <skos:definition xml:lang="en">Breast-Infiltrating malignant neoplasm-Progesterone receptor-Immunoreactive tumor cells present (&gt; = 1%) (Specify Quantitation)</skos:definition>
        <skos:prefLabel xml:lang="en">Immunoreactive tumor cells present (&gt; = 1%) (Specify Quantitation)</skos:prefLabel>
    </owl:Class>
    


    <!-- http://www.semanticweb.org/david/ontologies/2013/0/1.3.6.1.4.1.19376.1.8.2.1.2268 -->

    <owl:Class rdf:about="&pathLex;2268">
        <rdfs:subClassOf rdf:resource="&pathLex;431"/>
        <skos:definition xml:lang="en">Breast-Infiltrating malignant neoplasm-Progesterone receptor-Less than 1% immunoreactive cells present</skos:definition>
        <skos:prefLabel xml:lang="en">Less than 1% immunoreactive cells present</skos:prefLabel>
    </owl:Class>
    


    <!-- http://www.semanticweb.org/david/ontologies/2013/0/1.3.6.1.4.1.19376.1.8.2.1.2269 -->

    <owl:Class rdf:about="&pathLex;2269">
        <rdfs:subClassOf rdf:resource="&pathLex;432"/>
        <skos:definition xml:lang="en">Breast-Infiltrating malignant neoplasm-Estrogen receptor-Immunoreactive tumor cells present (&gt; = 1%) (Specify Quantitation)</skos:definition>
        <skos:prefLabel xml:lang="en">Immunoreactive tumor cells present (&gt; = 1%) (Specify Quantitation)</skos:prefLabel>
    </owl:Class>
    


    <!-- http://www.semanticweb.org/david/ontologies/2013/0/1.3.6.1.4.1.19376.1.8.2.1.227 -->

    <owl:Class rdf:about="&pathLex;227">
        <rdfs:subClassOf rdf:resource="&pathLex;99999"/>
        <skos:prefLabel xml:lang="en">Lymph node metastasis size</skos:prefLabel>
        <skos:definition xml:lang="en">Salivary gland-Infiltrating malignant neoplasm-Lymph node metastasis size</skos:definition>
    </owl:Class>
    


    <!-- http://www.semanticweb.org/david/ontologies/2013/0/1.3.6.1.4.1.19376.1.8.2.1.2270 -->

    <owl:Class rdf:about="&pathLex;2270">
        <rdfs:subClassOf rdf:resource="&pathLex;432"/>
        <skos:definition xml:lang="en">Breast-Infiltrating malignant neoplasm-Estrogen receptor-Less than 1% immunoreactive cells present</skos:definition>
        <skos:prefLabel xml:lang="en">Less than 1% immunoreactive cells present</skos:prefLabel>
    </owl:Class>
    


    <!-- http://www.semanticweb.org/david/ontologies/2013/0/1.3.6.1.4.1.19376.1.8.2.1.2271 -->

    <owl:Class rdf:about="&pathLex;2271">
        <rdfs:subClassOf rdf:resource="&pathLex;99999"/>
        <skos:definition xml:lang="en">Generic-Infiltrating malignant neoplasm-Treatment effect-Marked response (grade 1, minimal residual cancer)</skos:definition>
        <skos:prefLabel xml:lang="en">Marked response (grade 1, minimal residual cancer)</skos:prefLabel>
    </owl:Class>
    


    <!-- http://www.semanticweb.org/david/ontologies/2013/0/1.3.6.1.4.1.19376.1.8.2.1.2272 -->

    <owl:Class rdf:about="&pathLex;2272">
        <rdfs:subClassOf rdf:resource="&pathLex;99999"/>
        <skos:definition xml:lang="en">Colon-Infiltrating malignant neoplasm-Histologic Features Suggestive of Microsatellite Instability-No Intratumoral Lymphocytic Response (tumor-infiltrating lymphocytes)</skos:definition>
        <skos:prefLabel xml:lang="en">No Intratumoral Lymphocytic Response (tumor-infiltrating lymphocytes)</skos:prefLabel>
    </owl:Class>
    


    <!-- http://www.semanticweb.org/david/ontologies/2013/0/1.3.6.1.4.1.19376.1.8.2.1.2273 -->

    <owl:Class rdf:about="&pathLex;2273">
        <rdfs:subClassOf rdf:resource="&pathLex;99999"/>
        <skos:definition xml:lang="en">Colon-Infiltrating malignant neoplasm-Histologic Features Suggestive of Microsatellite Instability-Mild to moderate (0-2 per high-power [X400] field) Intratumoral Lymphocytic Response (tumor-infiltrating lymphocytes)</skos:definition>
        <skos:prefLabel xml:lang="en">Mild to moderate (0-2 per high-power [X400] field) Intratumoral Lymphocytic Response (tumor-infiltrating lymphocytes)</skos:prefLabel>
    </owl:Class>
    


    <!-- http://www.semanticweb.org/david/ontologies/2013/0/1.3.6.1.4.1.19376.1.8.2.1.2274 -->

    <owl:Class rdf:about="&pathLex;2274">
        <rdfs:subClassOf rdf:resource="&pathLex;99999"/>
        <skos:definition xml:lang="en">Colon-Infiltrating malignant neoplasm-Histologic Features Suggestive of Microsatellite Instability-Marked (3 or more per high-power field) Intratumoral Lymphocytic Response (tumor-infiltrating lymphocytes)</skos:definition>
        <skos:prefLabel xml:lang="en">Marked (3 or more per high-power field) Intratumoral Lymphocytic Response (tumor-infiltrating lymphocytes)</skos:prefLabel>
    </owl:Class>
    


    <!-- http://www.semanticweb.org/david/ontologies/2013/0/1.3.6.1.4.1.19376.1.8.2.1.2275 -->

    <owl:Class rdf:about="&pathLex;2275">
        <rdfs:subClassOf rdf:resource="&pathLex;99999"/>
        <skos:definition xml:lang="en">Colon-Infiltrating malignant neoplasm-Histologic Features Suggestive of Microsatellite Instability-No Peritumor Lymphocytic Response (Crohn-like response)</skos:definition>
        <skos:prefLabel xml:lang="en">No Peritumor Lymphocytic Response (Crohn-like response)</skos:prefLabel>
    </owl:Class>
    


    <!-- http://www.semanticweb.org/david/ontologies/2013/0/1.3.6.1.4.1.19376.1.8.2.1.2276 -->

    <owl:Class rdf:about="&pathLex;2276">
        <rdfs:subClassOf rdf:resource="&pathLex;99999"/>
        <skos:definition xml:lang="en">Colon-Infiltrating malignant neoplasm-Histologic Features Suggestive of Microsatellite Instability-Mild to moderate Peritumor Lymphocytic Response (Crohn-like response)</skos:definition>
        <skos:prefLabel xml:lang="en">Mild to moderate Peritumor Lymphocytic Response (Crohn-like response)</skos:prefLabel>
    </owl:Class>
    


    <!-- http://www.semanticweb.org/david/ontologies/2013/0/1.3.6.1.4.1.19376.1.8.2.1.2277 -->

    <owl:Class rdf:about="&pathLex;2277">
        <rdfs:subClassOf rdf:resource="&pathLex;99999"/>
        <skos:definition xml:lang="en">Colon-Infiltrating malignant neoplasm-Histologic Features Suggestive of Microsatellite Instability-Marked Peritumor Lymphocytic Response (Crohn-like response)</skos:definition>
        <skos:prefLabel xml:lang="en">Marked Peritumor Lymphocytic Response (Crohn-like response)</skos:prefLabel>
    </owl:Class>
    


    <!-- http://www.semanticweb.org/david/ontologies/2013/0/1.3.6.1.4.1.19376.1.8.2.1.2278 -->

    <owl:Class rdf:about="&pathLex;2278">
        <rdfs:subClassOf rdf:resource="&pathLex;99999"/>
        <skos:definition xml:lang="en">Colon-Infiltrating malignant neoplasm-Histologic Features Suggestive of Microsatellite Instability-Mucinous tumor component (specify percentage: ____)</skos:definition>
        <skos:prefLabel xml:lang="en">Mucinous tumor component (specify percentage: ____)</skos:prefLabel>
    </owl:Class>
    


    <!-- http://www.semanticweb.org/david/ontologies/2013/0/1.3.6.1.4.1.19376.1.8.2.1.2279 -->

    <owl:Class rdf:about="&pathLex;2279">
        <rdfs:subClassOf rdf:resource="&pathLex;99999"/>
        <skos:definition xml:lang="en">Colon-Infiltrating malignant neoplasm-Histologic Features Suggestive of Microsatellite Instability-Medullary tumor component</skos:definition>
        <skos:prefLabel xml:lang="en">Medullary tumor component</skos:prefLabel>
    </owl:Class>
    


    <!-- http://www.semanticweb.org/david/ontologies/2013/0/1.3.6.1.4.1.19376.1.8.2.1.228 -->

    <owl:Class rdf:about="&pathLex;228">
        <rdfs:subClassOf rdf:resource="&pathLex;99999"/>
        <skos:prefLabel xml:lang="en">Lesion size, largest dimension</skos:prefLabel>
        <skos:definition xml:lang="en">Salivary gland-Infiltrating malignant neoplasm-Lesion size, largest dimension</skos:definition>
    </owl:Class>
    


    <!-- http://www.semanticweb.org/david/ontologies/2013/0/1.3.6.1.4.1.19376.1.8.2.1.2280 -->

    <owl:Class rdf:about="&pathLex;2280">
        <rdfs:subClassOf rdf:resource="&pathLex;99999"/>
        <skos:definition xml:lang="en">Colon-Infiltrating malignant neoplasm-Histologic Features Suggestive of Microsatellite Instability-High histologic grade (poorly differentiated)</skos:definition>
        <skos:prefLabel xml:lang="en">High histologic grade (poorly differentiated)</skos:prefLabel>
    </owl:Class>
    


    <!-- http://www.semanticweb.org/david/ontologies/2013/0/1.3.6.1.4.1.19376.1.8.2.1.2281 -->

    <owl:Class rdf:about="&pathLex;2281">
        <rdfs:subClassOf rdf:resource="&pathLex;141"/>
        <skos:definition xml:lang="en">Cervix-Infiltrating malignant neoplasm-Histologic type-Nonkeratinizing squamous cell carcinoma</skos:definition>
        <skos:prefLabel xml:lang="en">Nonkeratinizing squamous cell carcinoma</skos:prefLabel>
    </owl:Class>
    


    <!-- http://www.semanticweb.org/david/ontologies/2013/0/1.3.6.1.4.1.19376.1.8.2.1.2282 -->

    <owl:Class rdf:about="&pathLex;2282">
        <rdfs:subClassOf rdf:resource="&pathLex;99999"/>
        <skos:definition xml:lang="en">Colon-Infiltrating malignant neoplasm-Histologic type-Small cell carcinoma</skos:definition>
        <skos:prefLabel xml:lang="en">Small cell carcinoma</skos:prefLabel>
    </owl:Class>
    


    <!-- http://www.semanticweb.org/david/ontologies/2013/0/1.3.6.1.4.1.19376.1.8.2.1.2283 -->

    <owl:Class rdf:about="&pathLex;2283">
        <rdfs:subClassOf rdf:resource="&pathLex;99999"/>
        <skos:definition xml:lang="en">Colon-Infiltrating malignant neoplasm-Histologic type-Squamous cell carcinoma</skos:definition>
        <skos:prefLabel xml:lang="en">Squamous cell carcinoma</skos:prefLabel>
    </owl:Class>
    


    <!-- http://www.semanticweb.org/david/ontologies/2013/0/1.3.6.1.4.1.19376.1.8.2.1.2284 -->

    <owl:Class rdf:about="&pathLex;2284">
        <rdfs:subClassOf rdf:resource="&pathLex;99999"/>
        <skos:prefLabel xml:lang="en">Adenosquamous carcinoma</skos:prefLabel>
        <skos:definition xml:lang="en">Colon-Infiltrating malignant neoplasm-Histologic type-Adenosquamous carcinoma</skos:definition>
    </owl:Class>
    


    <!-- http://www.semanticweb.org/david/ontologies/2013/0/1.3.6.1.4.1.19376.1.8.2.1.2285 -->

    <owl:Class rdf:about="&pathLex;2285">
        <rdfs:subClassOf rdf:resource="&pathLex;99999"/>
        <skos:prefLabel xml:lang="en">Carcinoma, type cannot be determinedd</skos:prefLabel>
        <skos:definition xml:lang="en">Colon-Infiltrating malignant neoplasm-Histologic type-Carcinoma, type cannot be determinedd</skos:definition>
    </owl:Class>
    


    <!-- http://www.semanticweb.org/david/ontologies/2013/0/1.3.6.1.4.1.19376.1.8.2.1.2286 -->

    <owl:Class rdf:about="&pathLex;2286">
        <rdfs:subClassOf rdf:resource="&pathLex;99999"/>
        <skos:prefLabel xml:lang="en">Active inflammatory bowel disease</skos:prefLabel>
        <skos:definition xml:lang="en">Colon-Lesion-Histologic type-Active inflammatory bowel disease</skos:definition>
    </owl:Class>
    


    <!-- http://www.semanticweb.org/david/ontologies/2013/0/1.3.6.1.4.1.19376.1.8.2.1.2287 -->

    <owl:Class rdf:about="&pathLex;2287">
        <rdfs:subClassOf rdf:resource="&pathLex;99999"/>
        <skos:definition xml:lang="en">Colon-Lesion-Histologic type-Quiescent inflammatory bowel disease</skos:definition>
        <skos:prefLabel xml:lang="en">Quiescent inflammatory bowel disease</skos:prefLabel>
    </owl:Class>
    


    <!-- http://www.semanticweb.org/david/ontologies/2013/0/1.3.6.1.4.1.19376.1.8.2.1.2288 -->

    <owl:Class rdf:about="&pathLex;2288">
        <rdfs:subClassOf rdf:resource="&pathLex;99999"/>
        <skos:definition xml:lang="en">Colon-Lesion-Histologic type-Dysplasia arising in inflammatory bowel disease</skos:definition>
        <skos:prefLabel xml:lang="en">Dysplasia arising in inflammatory bowel disease</skos:prefLabel>
    </owl:Class>
    


    <!-- http://www.semanticweb.org/david/ontologies/2013/0/1.3.6.1.4.1.19376.1.8.2.1.2289 -->

    <owl:Class rdf:about="&pathLex;2289">
        <rdfs:subClassOf rdf:resource="&pathLex;99999"/>
        <skos:prefLabel xml:lang="en">Chronic ulcerative proctocolitis</skos:prefLabel>
        <skos:definition xml:lang="en">Colon-Lesion-Histologic type-Chronic ulcerative proctocolitis</skos:definition>
    </owl:Class>
    


    <!-- http://www.semanticweb.org/david/ontologies/2013/0/1.3.6.1.4.1.19376.1.8.2.1.229 -->

    <owl:Class rdf:about="&pathLex;229">
        <rdfs:subClassOf rdf:resource="&pathLex;99999"/>
        <skos:definition xml:lang="en">Salivary gland-Infiltrating malignant neoplasm-Specimen size, largest dimension</skos:definition>
        <skos:prefLabel xml:lang="en">Specimen size, largest dimension</skos:prefLabel>
    </owl:Class>
    


    <!-- http://www.semanticweb.org/david/ontologies/2013/0/1.3.6.1.4.1.19376.1.8.2.1.2290 -->

    <owl:Class rdf:about="&pathLex;2290">
        <rdfs:subClassOf rdf:resource="&pathLex;99999"/>
        <skos:definition xml:lang="en">Colon-Lesion-Histologic type-Crohn disease</skos:definition>
        <skos:prefLabel xml:lang="en">Crohn disease</skos:prefLabel>
    </owl:Class>
    


    <!-- http://www.semanticweb.org/david/ontologies/2013/0/1.3.6.1.4.1.19376.1.8.2.1.2291 -->

    <owl:Class rdf:about="&pathLex;2291">
        <rdfs:subClassOf rdf:resource="&pathLex;99999"/>
        <skos:prefLabel xml:lang="en">Adenoma(s)</skos:prefLabel>
        <skos:definition xml:lang="en">Colon-Lesion-Histologic type-Adenoma(s)</skos:definition>
    </owl:Class>
    


    <!-- http://www.semanticweb.org/david/ontologies/2013/0/1.3.6.1.4.1.19376.1.8.2.1.2292 -->

    <owl:Class rdf:about="&pathLex;2292">
        <rdfs:subClassOf rdf:resource="&pathLex;99999"/>
        <skos:definition xml:lang="en">Colon-Lesion-Histologic type-Other polyps (specify)</skos:definition>
        <skos:prefLabel xml:lang="en">Other polyps (specify)</skos:prefLabel>
    </owl:Class>
    


    <!-- http://www.semanticweb.org/david/ontologies/2013/0/1.3.6.1.4.1.19376.1.8.2.1.2293 -->

    <owl:Class rdf:about="&pathLex;2293">
        <rdfs:subClassOf rdf:resource="&pathLex;99999"/>
        <skos:definition xml:lang="en">Endometrium-Infiltrating malignant neoplasm-Histologic type-Small cell carcinoma</skos:definition>
        <skos:prefLabel xml:lang="en">Small cell carcinoma</skos:prefLabel>
    </owl:Class>
    


    <!-- http://www.semanticweb.org/david/ontologies/2013/0/1.3.6.1.4.1.19376.1.8.2.1.2294 -->

    <owl:Class rdf:about="&pathLex;2294">
        <rdfs:subClassOf rdf:resource="&pathLex;99999"/>
        <skos:definition xml:lang="en">Endometrium-Infiltrating malignant neoplasm-Histologic type-Mixed carcinoma (specify types and percentages)</skos:definition>
        <skos:prefLabel xml:lang="en">Mixed carcinoma (specify types and percentages)</skos:prefLabel>
    </owl:Class>
    


    <!-- http://www.semanticweb.org/david/ontologies/2013/0/1.3.6.1.4.1.19376.1.8.2.1.2295 -->

    <owl:Class rdf:about="&pathLex;2295">
        <rdfs:subClassOf rdf:resource="&pathLex;99999"/>
        <skos:definition xml:lang="en">Endometrium-Infiltrating malignant neoplasm-Histologic type-Transitional cell carcinoma</skos:definition>
        <skos:prefLabel xml:lang="en">Transitional cell carcinoma</skos:prefLabel>
    </owl:Class>
    


    <!-- http://www.semanticweb.org/david/ontologies/2013/0/1.3.6.1.4.1.19376.1.8.2.1.2296 -->

    <owl:Class rdf:about="&pathLex;2296">
        <rdfs:subClassOf rdf:resource="&pathLex;99999"/>
        <skos:definition xml:lang="en">Endometrium-Lesion-Histologic type-Simple hyperplasia without cytologic atypia</skos:definition>
        <skos:prefLabel xml:lang="en">Simple hyperplasia without cytologic atypia</skos:prefLabel>
    </owl:Class>
    


    <!-- http://www.semanticweb.org/david/ontologies/2013/0/1.3.6.1.4.1.19376.1.8.2.1.2297 -->

    <owl:Class rdf:about="&pathLex;2297">
        <rdfs:subClassOf rdf:resource="&pathLex;99999"/>
        <skos:prefLabel xml:lang="en">Complex hyperplasia without cytologic atypia</skos:prefLabel>
        <skos:definition xml:lang="en">Endometrium-Lesion-Histologic type-Complex hyperplasia without cytologic atypia</skos:definition>
    </owl:Class>
    


    <!-- http://www.semanticweb.org/david/ontologies/2013/0/1.3.6.1.4.1.19376.1.8.2.1.2298 -->

    <owl:Class rdf:about="&pathLex;2298">
        <rdfs:subClassOf rdf:resource="&pathLex;99999"/>
        <skos:definition xml:lang="en">Endometrium-Lesion-Histologic type-Simple atypical hyperplasia</skos:definition>
        <skos:prefLabel xml:lang="en">Simple atypical hyperplasia</skos:prefLabel>
    </owl:Class>
    


    <!-- http://www.semanticweb.org/david/ontologies/2013/0/1.3.6.1.4.1.19376.1.8.2.1.2299 -->

    <owl:Class rdf:about="&pathLex;2299">
        <rdfs:subClassOf rdf:resource="&pathLex;99999"/>
        <skos:prefLabel xml:lang="en">Complex atypical hyperplasia</skos:prefLabel>
        <skos:definition xml:lang="en">Endometrium-Lesion-Histologic type-Complex atypical hyperplasia</skos:definition>
    </owl:Class>
    


    <!-- http://www.semanticweb.org/david/ontologies/2013/0/1.3.6.1.4.1.19376.1.8.2.1.23 -->

    <owl:Class rdf:about="&pathLex;23">
        <rdfs:subClassOf rdf:resource="&pathLex;10012"/>
        <skos:definition xml:lang="en">Generic-Lesion-Histologic type</skos:definition>
        <skos:prefLabel xml:lang="en">Histologic type</skos:prefLabel>
    </owl:Class>
    


    <!-- http://www.semanticweb.org/david/ontologies/2013/0/1.3.6.1.4.1.19376.1.8.2.1.230 -->

    <owl:Class rdf:about="&pathLex;230">
        <rdfs:subClassOf rdf:resource="&pathLex;99999"/>
        <skos:prefLabel xml:lang="en">Histologic type</skos:prefLabel>
        <skos:definition xml:lang="en">Salivary gland-Infiltrating malignant neoplasm-Histologic type</skos:definition>
    </owl:Class>
    


    <!-- http://www.semanticweb.org/david/ontologies/2013/0/1.3.6.1.4.1.19376.1.8.2.1.2300 -->

    <owl:Class rdf:about="&pathLex;2300">
        <rdfs:subClassOf rdf:resource="&pathLex;99999"/>
        <skos:prefLabel xml:lang="en">Endometrial intraepithelial neoplasia (EIN)</skos:prefLabel>
        <skos:definition xml:lang="en">Endometrium-Lesion-Histologic type-Endometrial intraepithelial neoplasia (EIN)</skos:definition>
    </owl:Class>
    


    <!-- http://www.semanticweb.org/david/ontologies/2013/0/1.3.6.1.4.1.19376.1.8.2.1.2301 -->

    <owl:Class rdf:about="&pathLex;2301">
        <rdfs:subClassOf rdf:resource="&pathLex;437"/>
        <skos:definition xml:lang="en">Breast-Infiltrating malignant neoplasm-Histologic type-Invasive mucinous carcinoma</skos:definition>
        <skos:prefLabel xml:lang="en">Invasive mucinous carcinoma</skos:prefLabel>
    </owl:Class>
    


    <!-- http://www.semanticweb.org/david/ontologies/2013/0/1.3.6.1.4.1.19376.1.8.2.1.2302 -->

    <owl:Class rdf:about="&pathLex;2302">
        <rdfs:subClassOf rdf:resource="&pathLex;437"/>
        <skos:definition xml:lang="en">Breast-Infiltrating malignant neoplasm-Histologic type-Invasive medullary carcinoma</skos:definition>
        <skos:prefLabel xml:lang="en">Invasive medullary carcinoma</skos:prefLabel>
    </owl:Class>
    


    <!-- http://www.semanticweb.org/david/ontologies/2013/0/1.3.6.1.4.1.19376.1.8.2.1.2303 -->

    <owl:Class rdf:about="&pathLex;2303">
        <rdfs:subClassOf rdf:resource="&pathLex;437"/>
        <skos:definition xml:lang="en">Breast-Infiltrating malignant neoplasm-Histologic type-Invasive papillary carcinoma</skos:definition>
        <skos:prefLabel xml:lang="en">Invasive papillary carcinoma</skos:prefLabel>
    </owl:Class>
    


    <!-- http://www.semanticweb.org/david/ontologies/2013/0/1.3.6.1.4.1.19376.1.8.2.1.2304 -->

    <owl:Class rdf:about="&pathLex;2304">
        <rdfs:subClassOf rdf:resource="&pathLex;437"/>
        <skos:definition xml:lang="en">Breast-Infiltrating malignant neoplasm-Histologic type-Invasive micropapillary carcinoma</skos:definition>
        <skos:prefLabel xml:lang="en">Invasive micropapillary carcinoma</skos:prefLabel>
    </owl:Class>
    


    <!-- http://www.semanticweb.org/david/ontologies/2013/0/1.3.6.1.4.1.19376.1.8.2.1.2305 -->

    <owl:Class rdf:about="&pathLex;2305">
        <rdfs:subClassOf rdf:resource="&pathLex;437"/>
        <skos:definition xml:lang="en">Breast-Infiltrating malignant neoplasm-Histologic type-Invasive tubular carcinoma</skos:definition>
        <skos:prefLabel xml:lang="en">Invasive tubular carcinoma</skos:prefLabel>
    </owl:Class>
    


    <!-- http://www.semanticweb.org/david/ontologies/2013/0/1.3.6.1.4.1.19376.1.8.2.1.2306 -->

    <owl:Class rdf:about="&pathLex;2306">
        <rdfs:subClassOf rdf:resource="&pathLex;437"/>
        <skos:definition xml:lang="en">Breast-Infiltrating malignant neoplasm-Histologic type-Invasive cribriform carcinoma</skos:definition>
        <skos:prefLabel xml:lang="en">Invasive cribriform carcinoma</skos:prefLabel>
    </owl:Class>
    


    <!-- http://www.semanticweb.org/david/ontologies/2013/0/1.3.6.1.4.1.19376.1.8.2.1.2308 -->

    <owl:Class rdf:about="&pathLex;2308">
        <rdfs:subClassOf rdf:resource="&pathLex;436"/>
        <skos:definition xml:lang="en">Breast-In situ neoplasm-Histologic type-Ductal carcinoma in situ with microinvasion</skos:definition>
        <skos:prefLabel xml:lang="en">Ductal carcinoma in situ with microinvasion</skos:prefLabel>
    </owl:Class>
    


    <!-- http://www.semanticweb.org/david/ontologies/2013/0/1.3.6.1.4.1.19376.1.8.2.1.2309 -->

    <owl:Class rdf:about="&pathLex;2309">
        <rdfs:subClassOf rdf:resource="&pathLex;436"/>
        <skos:definition xml:lang="en">Breast-In situ neoplasm-Histologic type-Lobular carcinoma in situ with microinvasion</skos:definition>
        <skos:prefLabel xml:lang="en">Lobular carcinoma in situ with microinvasion</skos:prefLabel>
    </owl:Class>
    


    <!-- http://www.semanticweb.org/david/ontologies/2013/0/1.3.6.1.4.1.19376.1.8.2.1.231 -->

    <owl:Class rdf:about="&pathLex;231">
        <rdfs:subClassOf rdf:resource="&pathLex;99999"/>
        <skos:definition xml:lang="en">Larynx-Infiltrating malignant neoplasm-Margins involvement</skos:definition>
        <skos:prefLabel xml:lang="en">Margins involvement</skos:prefLabel>
    </owl:Class>
    


    <!-- http://www.semanticweb.org/david/ontologies/2013/0/1.3.6.1.4.1.19376.1.8.2.1.2310 -->

    <owl:Class rdf:about="&pathLex;2310">
        <rdfs:subClassOf rdf:resource="&pathLex;436"/>
        <skos:definition xml:lang="en">Breast-In situ neoplasm-Histologic type-Ductal carcinoma in situ involving nipple skin (Paget disease) with microinvasion</skos:definition>
        <skos:prefLabel xml:lang="en">Ductal carcinoma in situ involving nipple skin (Paget disease) with microinvasion</skos:prefLabel>
    </owl:Class>
    


    <!-- http://www.semanticweb.org/david/ontologies/2013/0/1.3.6.1.4.1.19376.1.8.2.1.2311 -->

    <owl:Class rdf:about="&pathLex;2311">
        <rdfs:subClassOf rdf:resource="&pathLex;436"/>
        <skos:definition xml:lang="en">Breast-In situ neoplasm-Histologic type-Invasive carcinoma with ductal and lobular features (“mixed type carcinoma”)</skos:definition>
        <skos:prefLabel xml:lang="en">Invasive carcinoma with ductal and lobular features (“mixed type carcinoma”)</skos:prefLabel>
    </owl:Class>
    


    <!-- http://www.semanticweb.org/david/ontologies/2013/0/1.3.6.1.4.1.19376.1.8.2.1.2312 -->

    <owl:Class rdf:about="&pathLex;2312">
        <rdfs:subClassOf rdf:resource="&pathLex;139"/>
        <skos:definition xml:lang="en">Cervix-Lesion-Histologic type-Koilocytosis</skos:definition>
        <skos:prefLabel xml:lang="en">Koilocytosis</skos:prefLabel>
    </owl:Class>
    


    <!-- http://www.semanticweb.org/david/ontologies/2013/0/1.3.6.1.4.1.19376.1.8.2.1.2313 -->

    <owl:Class rdf:about="&pathLex;2313">
        <rdfs:subClassOf rdf:resource="&pathLex;99999"/>
        <skos:prefLabel xml:lang="en">Adenocarcinoma, diffuse type</skos:prefLabel>
        <skos:definition xml:lang="en">Stomach-Infiltrating malignant neoplasm-Histologic type-Adenocarcinoma, diffuse type</skos:definition>
    </owl:Class>
    


    <!-- http://www.semanticweb.org/david/ontologies/2013/0/1.3.6.1.4.1.19376.1.8.2.1.2314 -->

    <owl:Class rdf:about="&pathLex;2314">
        <rdfs:subClassOf rdf:resource="&pathLex;99999"/>
        <skos:prefLabel xml:lang="en">Signet-ring cell carcinoma (greater than 50% signet-ring cells)</skos:prefLabel>
        <skos:definition xml:lang="en">Stomach-Infiltrating malignant neoplasm-Histologic type-Signet-ring cell carcinoma (greater than 50% signet-ring cells)</skos:definition>
    </owl:Class>
    


    <!-- http://www.semanticweb.org/david/ontologies/2013/0/1.3.6.1.4.1.19376.1.8.2.1.2315 -->

    <owl:Class rdf:about="&pathLex;2315">
        <rdfs:subClassOf rdf:resource="&pathLex;99999"/>
        <skos:prefLabel xml:lang="en">Adenocarcinoma, intestinal type</skos:prefLabel>
        <skos:definition xml:lang="en">Stomach-Infiltrating malignant neoplasm-Histologic type-Adenocarcinoma, intestinal type</skos:definition>
    </owl:Class>
    


    <!-- http://www.semanticweb.org/david/ontologies/2013/0/1.3.6.1.4.1.19376.1.8.2.1.2316 -->

    <owl:Class rdf:about="&pathLex;2316">
        <rdfs:subClassOf rdf:resource="&pathLex;99999"/>
        <skos:prefLabel xml:lang="en">Intestinal metaplasia</skos:prefLabel>
        <skos:definition xml:lang="en">Stomach-Lesion-Histologic type-Intestinal metaplasia</skos:definition>
    </owl:Class>
    


    <!-- http://www.semanticweb.org/david/ontologies/2013/0/1.3.6.1.4.1.19376.1.8.2.1.2317 -->

    <owl:Class rdf:about="&pathLex;2317">
        <rdfs:subClassOf rdf:resource="&pathLex;99999"/>
        <skos:prefLabel xml:lang="en">Dysplasia</skos:prefLabel>
        <skos:definition xml:lang="en">Stomach-Lesion-Histologic type-Dysplasia</skos:definition>
    </owl:Class>
    


    <!-- http://www.semanticweb.org/david/ontologies/2013/0/1.3.6.1.4.1.19376.1.8.2.1.2318 -->

    <owl:Class rdf:about="&pathLex;2318">
        <rdfs:subClassOf rdf:resource="&pathLex;99999"/>
        <skos:prefLabel xml:lang="en">Helicobacter pylori-type gastritis</skos:prefLabel>
        <skos:definition xml:lang="en">Stomach-Lesion-Histologic type-Helicobacter pylori-type gastritis</skos:definition>
    </owl:Class>
    


    <!-- http://www.semanticweb.org/david/ontologies/2013/0/1.3.6.1.4.1.19376.1.8.2.1.2319 -->

    <owl:Class rdf:about="&pathLex;2319">
        <rdfs:subClassOf rdf:resource="&pathLex;99999"/>
        <skos:prefLabel xml:lang="en">Other gastritis (specify)</skos:prefLabel>
        <skos:definition xml:lang="en">Stomach-Lesion-Histologic type-Other gastritis (specify)</skos:definition>
    </owl:Class>
    


    <!-- http://www.semanticweb.org/david/ontologies/2013/0/1.3.6.1.4.1.19376.1.8.2.1.2320 -->

    <owl:Class rdf:about="&pathLex;2320">
        <rdfs:subClassOf rdf:resource="&pathLex;99999"/>
        <skos:prefLabel xml:lang="en">Polyp(s) (specify)</skos:prefLabel>
        <skos:definition xml:lang="en">Stomach-Lesion-Histologic type-Polyp(s) (specify)</skos:definition>
    </owl:Class>
    


    <!-- http://www.semanticweb.org/david/ontologies/2013/0/1.3.6.1.4.1.19376.1.8.2.1.2321 -->

    <owl:Class rdf:about="&pathLex;2321">
        <rdfs:subClassOf rdf:resource="&pathLex;99999"/>
        <skos:prefLabel xml:lang="en">Fibrolamellar hepatocellular carcinoma</skos:prefLabel>
        <skos:definition xml:lang="en">Liver-Infiltrating malignant neoplasm-Histologic type-Fibrolamellar hepatocellular carcinoma</skos:definition>
    </owl:Class>
    


    <!-- http://www.semanticweb.org/david/ontologies/2013/0/1.3.6.1.4.1.19376.1.8.2.1.2322 -->

    <owl:Class rdf:about="&pathLex;2322">
        <rdfs:subClassOf rdf:resource="&pathLex;99999"/>
        <skos:definition xml:lang="en">Liver-Infiltrating malignant neoplasm-Histologic type-Undifferentiated carcinoma</skos:definition>
        <skos:prefLabel xml:lang="en">Undifferentiated carcinoma</skos:prefLabel>
    </owl:Class>
    


    <!-- http://www.semanticweb.org/david/ontologies/2013/0/1.3.6.1.4.1.19376.1.8.2.1.2323 -->

    <owl:Class rdf:about="&pathLex;2323">
        <rdfs:subClassOf rdf:resource="&pathLex;99999"/>
        <skos:prefLabel xml:lang="en">Carcinoma, type cannot be determinedd</skos:prefLabel>
        <skos:definition xml:lang="en">Liver-Infiltrating malignant neoplasm-Histologic type-Carcinoma, type cannot be determinedd</skos:definition>
    </owl:Class>
    


    <!-- http://www.semanticweb.org/david/ontologies/2013/0/1.3.6.1.4.1.19376.1.8.2.1.2324 -->

    <owl:Class rdf:about="&pathLex;2324">
        <rdfs:subClassOf rdf:resource="&pathLex;99999"/>
        <skos:prefLabel xml:lang="en">Cirrhosis/severe fibrosis (Ishak score 5-6) (F1)</skos:prefLabel>
        <skos:definition xml:lang="en">Liver-Lesion-Histologic type-Cirrhosis/severe fibrosis (Ishak score 5-6) (F1)</skos:definition>
    </owl:Class>
    


    <!-- http://www.semanticweb.org/david/ontologies/2013/0/1.3.6.1.4.1.19376.1.8.2.1.2325 -->

    <owl:Class rdf:about="&pathLex;2325">
        <rdfs:subClassOf rdf:resource="&pathLex;99999"/>
        <skos:definition xml:lang="en">Liver-Lesion-Histologic type-None to moderate fibrosis (Ishak score 0-4) (F2)</skos:definition>
        <skos:prefLabel xml:lang="en">None to moderate fibrosis (Ishak score 0-4) (F2)</skos:prefLabel>
    </owl:Class>
    


    <!-- http://www.semanticweb.org/david/ontologies/2013/0/1.3.6.1.4.1.19376.1.8.2.1.2326 -->

    <owl:Class rdf:about="&pathLex;2326">
        <rdfs:subClassOf rdf:resource="&pathLex;99999"/>
        <skos:definition xml:lang="en">Liver-Lesion-Histologic type-Low-grade hepatocellular dysplastic nodule</skos:definition>
        <skos:prefLabel xml:lang="en">Low-grade hepatocellular dysplastic nodule</skos:prefLabel>
    </owl:Class>
    


    <!-- http://www.semanticweb.org/david/ontologies/2013/0/1.3.6.1.4.1.19376.1.8.2.1.2327 -->

    <owl:Class rdf:about="&pathLex;2327">
        <rdfs:subClassOf rdf:resource="&pathLex;99999"/>
        <skos:prefLabel xml:lang="en">High-grade  hepatocellular dysplastic nodule</skos:prefLabel>
        <skos:definition xml:lang="en">Liver-Lesion-Histologic type-High-grade  hepatocellular dysplastic nodule</skos:definition>
    </owl:Class>
    


    <!-- http://www.semanticweb.org/david/ontologies/2013/0/1.3.6.1.4.1.19376.1.8.2.1.2328 -->

    <owl:Class rdf:about="&pathLex;2328">
        <rdfs:subClassOf rdf:resource="&pathLex;99999"/>
        <skos:definition xml:lang="en">Liver-Lesion-Histologic type-Steatosis</skos:definition>
        <skos:prefLabel xml:lang="en">Steatosis</skos:prefLabel>
    </owl:Class>
    


    <!-- http://www.semanticweb.org/david/ontologies/2013/0/1.3.6.1.4.1.19376.1.8.2.1.2329 -->

    <owl:Class rdf:about="&pathLex;2329">
        <rdfs:subClassOf rdf:resource="&pathLex;99999"/>
        <skos:prefLabel xml:lang="en">Iron overload</skos:prefLabel>
        <skos:definition xml:lang="en">Liver-Lesion-Histologic type-Iron overload</skos:definition>
    </owl:Class>
    


    <!-- http://www.semanticweb.org/david/ontologies/2013/0/1.3.6.1.4.1.19376.1.8.2.1.233 -->

    <owl:Class rdf:about="&pathLex;233">
        <rdfs:subClassOf rdf:resource="&pathLex;99999"/>
        <skos:prefLabel xml:lang="en">Distance of lesion from closest uninvolved margin</skos:prefLabel>
        <skos:definition xml:lang="en">Larynx-Infiltrating malignant neoplasm-Distance of lesion from closest uninvolved margin</skos:definition>
    </owl:Class>
    


    <!-- http://www.semanticweb.org/david/ontologies/2013/0/1.3.6.1.4.1.19376.1.8.2.1.2330 -->

    <owl:Class rdf:about="&pathLex;2330">
        <rdfs:subClassOf rdf:resource="&pathLex;99999"/>
        <skos:prefLabel xml:lang="en">Chronic hepatitis (specify)</skos:prefLabel>
        <skos:definition xml:lang="en">Liver-Lesion-Histologic type-Chronic hepatitis (specify)</skos:definition>
    </owl:Class>
    


    <!-- http://www.semanticweb.org/david/ontologies/2013/0/1.3.6.1.4.1.19376.1.8.2.1.2333 -->

    <owl:Class rdf:about="&pathLex;2333">
        <rdfs:subClassOf rdf:resource="&pathLex;99999"/>
        <skos:prefLabel xml:lang="en">Acinic cell carcinoma</skos:prefLabel>
        <skos:definition xml:lang="en">Salivary gland-Infiltrating malignant neoplasm-Histologic type-Acinic cell carcinoma</skos:definition>
    </owl:Class>
    


    <!-- http://www.semanticweb.org/david/ontologies/2013/0/1.3.6.1.4.1.19376.1.8.2.1.2334 -->

    <owl:Class rdf:about="&pathLex;2334">
        <rdfs:subClassOf rdf:resource="&pathLex;99999"/>
        <skos:prefLabel xml:lang="en">Clear cell adenocarcinoma</skos:prefLabel>
        <skos:definition xml:lang="en">Salivary gland-Infiltrating malignant neoplasm-Histologic type-Clear cell adenocarcinoma</skos:definition>
    </owl:Class>
    


    <!-- http://www.semanticweb.org/david/ontologies/2013/0/1.3.6.1.4.1.19376.1.8.2.1.2335 -->

    <owl:Class rdf:about="&pathLex;2335">
        <rdfs:subClassOf rdf:resource="&pathLex;99999"/>
        <skos:prefLabel xml:lang="en">Cystadenocarcinoma</skos:prefLabel>
        <skos:definition xml:lang="en">Salivary gland-Infiltrating malignant neoplasm-Histologic type-Cystadenocarcinoma</skos:definition>
    </owl:Class>
    


    <!-- http://www.semanticweb.org/david/ontologies/2013/0/1.3.6.1.4.1.19376.1.8.2.1.2336 -->

    <owl:Class rdf:about="&pathLex;2336">
        <rdfs:subClassOf rdf:resource="&pathLex;99999"/>
        <skos:prefLabel xml:lang="en">Large cell carcinoma</skos:prefLabel>
        <skos:definition xml:lang="en">Salivary gland-Infiltrating malignant neoplasm-Histologic type-Large cell carcinoma</skos:definition>
    </owl:Class>
    


    <!-- http://www.semanticweb.org/david/ontologies/2013/0/1.3.6.1.4.1.19376.1.8.2.1.2337 -->

    <owl:Class rdf:about="&pathLex;2337">
        <rdfs:subClassOf rdf:resource="&pathLex;99999"/>
        <skos:prefLabel xml:lang="en">Low-grade cribriform cystadenocarcinoma</skos:prefLabel>
        <skos:definition xml:lang="en">Salivary gland-Infiltrating malignant neoplasm-Histologic type-Low-grade cribriform cystadenocarcinoma</skos:definition>
    </owl:Class>
    


    <!-- http://www.semanticweb.org/david/ontologies/2013/0/1.3.6.1.4.1.19376.1.8.2.1.2338 -->

    <owl:Class rdf:about="&pathLex;2338">
        <rdfs:subClassOf rdf:resource="&pathLex;99999"/>
        <skos:prefLabel xml:lang="en">Lymphoepithelial carcinoma</skos:prefLabel>
        <skos:definition xml:lang="en">Salivary gland-Infiltrating malignant neoplasm-Histologic type-Lymphoepithelial carcinoma</skos:definition>
    </owl:Class>
    


    <!-- http://www.semanticweb.org/david/ontologies/2013/0/1.3.6.1.4.1.19376.1.8.2.1.2339 -->

    <owl:Class rdf:about="&pathLex;2339">
        <rdfs:subClassOf rdf:resource="&pathLex;99999"/>
        <skos:prefLabel xml:lang="en">Metastasizing pleomorphic adenoma</skos:prefLabel>
        <skos:definition xml:lang="en">Salivary gland-Infiltrating malignant neoplasm-Histologic type-Metastasizing pleomorphic adenoma</skos:definition>
    </owl:Class>
    


    <!-- http://www.semanticweb.org/david/ontologies/2013/0/1.3.6.1.4.1.19376.1.8.2.1.234 -->

    <owl:Class rdf:about="&pathLex;234">
        <rdfs:subClassOf rdf:resource="&pathLex;99999"/>
        <skos:prefLabel xml:lang="en">Distance of lesion from closest uninvolved margin</skos:prefLabel>
        <skos:definition xml:lang="en">Larynx-Infiltrating malignant neoplasm-Distance of lesion from closest uninvolved margin</skos:definition>
    </owl:Class>
    


    <!-- http://www.semanticweb.org/david/ontologies/2013/0/1.3.6.1.4.1.19376.1.8.2.1.2340 -->

    <owl:Class rdf:about="&pathLex;2340">
        <rdfs:subClassOf rdf:resource="&pathLex;99999"/>
        <skos:prefLabel xml:lang="en">Mucinous adenocarcinoma (colloid carcinoma)</skos:prefLabel>
        <skos:definition xml:lang="en">Salivary gland-Infiltrating malignant neoplasm-Histologic type-Mucinous adenocarcinoma (colloid carcinoma)</skos:definition>
    </owl:Class>
    


    <!-- http://www.semanticweb.org/david/ontologies/2013/0/1.3.6.1.4.1.19376.1.8.2.1.2341 -->

    <owl:Class rdf:about="&pathLex;2341">
        <rdfs:subClassOf rdf:resource="&pathLex;99999"/>
        <skos:prefLabel xml:lang="en">Myoepithelial carcinoma (malignant myoepithelioma)</skos:prefLabel>
        <skos:definition xml:lang="en">Salivary gland-Infiltrating malignant neoplasm-Histologic type-Myoepithelial carcinoma (malignant myoepithelioma)</skos:definition>
    </owl:Class>
    


    <!-- http://www.semanticweb.org/david/ontologies/2013/0/1.3.6.1.4.1.19376.1.8.2.1.2342 -->

    <owl:Class rdf:about="&pathLex;2342">
        <rdfs:subClassOf rdf:resource="&pathLex;99999"/>
        <skos:prefLabel xml:lang="en">Oncocytic carcinoma</skos:prefLabel>
        <skos:definition xml:lang="en">Salivary gland-Infiltrating malignant neoplasm-Histologic type-Oncocytic carcinoma</skos:definition>
    </owl:Class>
    


    <!-- http://www.semanticweb.org/david/ontologies/2013/0/1.3.6.1.4.1.19376.1.8.2.1.2343 -->

    <owl:Class rdf:about="&pathLex;2343">
        <rdfs:subClassOf rdf:resource="&pathLex;99999"/>
        <skos:prefLabel xml:lang="en">Polymorphous low-grade adenocarcinoma</skos:prefLabel>
        <skos:definition xml:lang="en">Salivary gland-Infiltrating malignant neoplasm-Histologic type-Polymorphous low-grade adenocarcinoma</skos:definition>
    </owl:Class>
    


    <!-- http://www.semanticweb.org/david/ontologies/2013/0/1.3.6.1.4.1.19376.1.8.2.1.2344 -->

    <owl:Class rdf:about="&pathLex;2344">
        <rdfs:subClassOf rdf:resource="&pathLex;99999"/>
        <skos:prefLabel xml:lang="en">Salivary duct carcinoma</skos:prefLabel>
        <skos:definition xml:lang="en">Salivary gland-Infiltrating malignant neoplasm-Histologic type-Salivary duct carcinoma</skos:definition>
    </owl:Class>
    


    <!-- http://www.semanticweb.org/david/ontologies/2013/0/1.3.6.1.4.1.19376.1.8.2.1.2345 -->

    <owl:Class rdf:about="&pathLex;2345">
        <rdfs:subClassOf rdf:resource="&pathLex;99999"/>
        <skos:definition xml:lang="en">Salivary gland-Infiltrating malignant neoplasm-Histologic type-Sebaceous lymphadenocarcinoma</skos:definition>
        <skos:prefLabel xml:lang="en">Sebaceous lymphadenocarcinoma</skos:prefLabel>
    </owl:Class>
    


    <!-- http://www.semanticweb.org/david/ontologies/2013/0/1.3.6.1.4.1.19376.1.8.2.1.2346 -->

    <owl:Class rdf:about="&pathLex;2346">
        <rdfs:subClassOf rdf:resource="&pathLex;99999"/>
        <skos:definition xml:lang="en">Salivary gland-Infiltrating malignant neoplasm-Histologic type-Sialoblastoma</skos:definition>
        <skos:prefLabel xml:lang="en">Sialoblastoma</skos:prefLabel>
    </owl:Class>
    


    <!-- http://www.semanticweb.org/david/ontologies/2013/0/1.3.6.1.4.1.19376.1.8.2.1.2347 -->

    <owl:Class rdf:about="&pathLex;2347">
        <rdfs:subClassOf rdf:resource="&pathLex;99999"/>
        <skos:definition xml:lang="en">Salivary gland-Infiltrating malignant neoplasm-Histologic type-Squamous cell carcinoma, primary</skos:definition>
        <skos:prefLabel xml:lang="en">Squamous cell carcinoma, primary</skos:prefLabel>
    </owl:Class>
    


    <!-- http://www.semanticweb.org/david/ontologies/2013/0/1.3.6.1.4.1.19376.1.8.2.1.2348 -->

    <owl:Class rdf:about="&pathLex;2348">
        <rdfs:subClassOf rdf:resource="&pathLex;99999"/>
        <skos:prefLabel xml:lang="en">Other</skos:prefLabel>
        <skos:definition xml:lang="en">Salivary gland-Infiltrating malignant neoplasm-Histologic type-Other</skos:definition>
    </owl:Class>
    


    <!-- http://www.semanticweb.org/david/ontologies/2013/0/1.3.6.1.4.1.19376.1.8.2.1.2349 -->

    <owl:Class rdf:about="&pathLex;2349">
        <rdfs:subClassOf rdf:resource="&pathLex;99999"/>
        <skos:prefLabel xml:lang="en">Carcinoma, type cannot be determinedd</skos:prefLabel>
        <skos:definition xml:lang="en">Salivary gland-Infiltrating malignant neoplasm-Histologic type-Carcinoma, type cannot be determinedd</skos:definition>
    </owl:Class>
    


    <!-- http://www.semanticweb.org/david/ontologies/2013/0/1.3.6.1.4.1.19376.1.8.2.1.235 -->

    <owl:Class rdf:about="&pathLex;235">
        <rdfs:subClassOf rdf:resource="&pathLex;99999"/>
        <skos:definition xml:lang="en">Larynx-Infiltrating malignant neoplasm-Lymph-vascular invasion</skos:definition>
        <skos:prefLabel xml:lang="en">Lymph-vascular invasion</skos:prefLabel>
    </owl:Class>
    


    <!-- http://www.semanticweb.org/david/ontologies/2013/0/1.3.6.1.4.1.19376.1.8.2.1.2350 -->

    <owl:Class rdf:about="&pathLex;2350">
        <rdfs:subClassOf rdf:resource="&pathLex;99999"/>
        <skos:definition xml:lang="en">Salivary gland-Lesion-Histologic type-Sialadenitis</skos:definition>
        <skos:prefLabel xml:lang="en">Sialadenitis</skos:prefLabel>
    </owl:Class>
    


    <!-- http://www.semanticweb.org/david/ontologies/2013/0/1.3.6.1.4.1.19376.1.8.2.1.2351 -->

    <owl:Class rdf:about="&pathLex;2351">
        <rdfs:subClassOf rdf:resource="&pathLex;99999"/>
        <skos:definition xml:lang="en">Salivary gland-Lesion-Histologic type-Tumor associated lymphoid proliferation (TALP)</skos:definition>
        <skos:prefLabel xml:lang="en">Tumor associated lymphoid proliferation (TALP)</skos:prefLabel>
    </owl:Class>
    


    <!-- http://www.semanticweb.org/david/ontologies/2013/0/1.3.6.1.4.1.19376.1.8.2.1.2352 -->

    <owl:Class rdf:about="&pathLex;2352">
        <rdfs:subClassOf rdf:resource="&pathLex;99999"/>
        <skos:definition xml:lang="en">Salivary gland-Lesion-Histologic type-Severe keratinizing dysplasia (carcinoma in situ)</skos:definition>
        <skos:prefLabel xml:lang="en">Severe keratinizing dysplasia (carcinoma in situ)</skos:prefLabel>
    </owl:Class>
    


    <!-- http://www.semanticweb.org/david/ontologies/2013/0/1.3.6.1.4.1.19376.1.8.2.1.2353 -->

    <owl:Class rdf:about="&pathLex;2353">
        <rdfs:subClassOf rdf:resource="&pathLex;99999"/>
        <skos:prefLabel xml:lang="en">Mild keratinizing dysplasia</skos:prefLabel>
        <skos:definition xml:lang="en">Salivary gland-Lesion-Histologic type-Mild keratinizing dysplasia</skos:definition>
    </owl:Class>
    


    <!-- http://www.semanticweb.org/david/ontologies/2013/0/1.3.6.1.4.1.19376.1.8.2.1.2354 -->

    <owl:Class rdf:about="&pathLex;2354">
        <rdfs:subClassOf rdf:resource="&pathLex;99999"/>
        <skos:prefLabel xml:lang="en">Moderate keratinizing dysplasia</skos:prefLabel>
        <skos:definition xml:lang="en">Salivary gland-Lesion-Histologic type-Moderate keratinizing dysplasia</skos:definition>
    </owl:Class>
    


    <!-- http://www.semanticweb.org/david/ontologies/2013/0/1.3.6.1.4.1.19376.1.8.2.1.2355 -->

    <owl:Class rdf:about="&pathLex;2355">
        <rdfs:subClassOf rdf:resource="&pathLex;99999"/>
        <skos:definition xml:lang="en">Larynx-Infiltrating malignant neoplasm-Histologic type-Variants of Squamous Cell Carcinoma</skos:definition>
        <skos:prefLabel xml:lang="en">Variants of Squamous Cell Carcinoma</skos:prefLabel>
    </owl:Class>
    


    <!-- http://www.semanticweb.org/david/ontologies/2013/0/1.3.6.1.4.1.19376.1.8.2.1.2356 -->

    <owl:Class rdf:about="&pathLex;2356">
        <rdfs:subClassOf rdf:resource="&pathLex;99999"/>
        <skos:prefLabel xml:lang="en">Acantholytic squamous cell carcinoma</skos:prefLabel>
        <skos:definition xml:lang="en">Larynx-Infiltrating malignant neoplasm-Histologic type-Acantholytic squamous cell carcinoma</skos:definition>
    </owl:Class>
    


    <!-- http://www.semanticweb.org/david/ontologies/2013/0/1.3.6.1.4.1.19376.1.8.2.1.2357 -->

    <owl:Class rdf:about="&pathLex;2357">
        <rdfs:subClassOf rdf:resource="&pathLex;99999"/>
        <skos:definition xml:lang="en">Larynx-Infiltrating malignant neoplasm-Histologic type-Papillary squamous cell carcinoma</skos:definition>
        <skos:prefLabel xml:lang="en">Papillary squamous cell carcinoma</skos:prefLabel>
    </owl:Class>
    


    <!-- http://www.semanticweb.org/david/ontologies/2013/0/1.3.6.1.4.1.19376.1.8.2.1.2358 -->

    <owl:Class rdf:about="&pathLex;2358">
        <rdfs:subClassOf rdf:resource="&pathLex;99999"/>
        <skos:prefLabel xml:lang="en">Giant cell carcinoma</skos:prefLabel>
        <skos:definition xml:lang="en">Larynx-Infiltrating malignant neoplasm-Histologic type-Giant cell carcinoma</skos:definition>
    </owl:Class>
    


    <!-- http://www.semanticweb.org/david/ontologies/2013/0/1.3.6.1.4.1.19376.1.8.2.1.2359 -->

    <owl:Class rdf:about="&pathLex;2359">
        <rdfs:subClassOf rdf:resource="&pathLex;99999"/>
        <skos:definition xml:lang="en">Larynx-Infiltrating malignant neoplasm-Histologic type-Neuroendocrine Carcinoma</skos:definition>
        <skos:prefLabel xml:lang="en">Neuroendocrine Carcinoma</skos:prefLabel>
    </owl:Class>
    


    <!-- http://www.semanticweb.org/david/ontologies/2013/0/1.3.6.1.4.1.19376.1.8.2.1.236 -->

    <owl:Class rdf:about="&pathLex;236">
        <rdfs:subClassOf rdf:resource="&pathLex;99999"/>
        <skos:definition xml:lang="en">Larynx-Infiltrating malignant neoplasm-Lymph node sampling</skos:definition>
        <skos:prefLabel xml:lang="en">Lymph node sampling</skos:prefLabel>
    </owl:Class>
    


    <!-- http://www.semanticweb.org/david/ontologies/2013/0/1.3.6.1.4.1.19376.1.8.2.1.2360 -->

    <owl:Class rdf:about="&pathLex;2360">
        <rdfs:subClassOf rdf:resource="&pathLex;99999"/>
        <skos:definition xml:lang="en">Larynx-Infiltrating malignant neoplasm-Histologic type-Typical carcinoid tumor (well differentiated neuroendocrine carcinoma)</skos:definition>
        <skos:prefLabel xml:lang="en">Typical carcinoid tumor (well differentiated neuroendocrine carcinoma)</skos:prefLabel>
    </owl:Class>
    


    <!-- http://www.semanticweb.org/david/ontologies/2013/0/1.3.6.1.4.1.19376.1.8.2.1.2361 -->

    <owl:Class rdf:about="&pathLex;2361">
        <rdfs:subClassOf rdf:resource="&pathLex;99999"/>
        <skos:prefLabel xml:lang="en">Atypical carcinoid tumor (moderately differentiated neuroendocrine carcinoma)</skos:prefLabel>
        <skos:definition xml:lang="en">Larynx-Infiltrating malignant neoplasm-Histologic type-Atypical carcinoid tumor (moderately differentiated neuroendocrine carcinoma)</skos:definition>
    </owl:Class>
    


    <!-- http://www.semanticweb.org/david/ontologies/2013/0/1.3.6.1.4.1.19376.1.8.2.1.2362 -->

    <owl:Class rdf:about="&pathLex;2362">
        <rdfs:subClassOf rdf:resource="&pathLex;99999"/>
        <skos:definition xml:lang="en">Larynx-Infiltrating malignant neoplasm-Histologic type-Small cell carcinoma, neuroendocrine type (poorly differentiated neuroendocrine</skos:definition>
        <skos:prefLabel xml:lang="en">Small cell carcinoma, neuroendocrine type (poorly differentiated neuroendocrine</skos:prefLabel>
    </owl:Class>
    


    <!-- http://www.semanticweb.org/david/ontologies/2013/0/1.3.6.1.4.1.19376.1.8.2.1.2363 -->

    <owl:Class rdf:about="&pathLex;2363">
        <rdfs:subClassOf rdf:resource="&pathLex;99999"/>
        <skos:definition xml:lang="en">Larynx-Infiltrating malignant neoplasm-Histologic type-carcinoma)</skos:definition>
        <skos:prefLabel xml:lang="en">carcinoma)</skos:prefLabel>
    </owl:Class>
    


    <!-- http://www.semanticweb.org/david/ontologies/2013/0/1.3.6.1.4.1.19376.1.8.2.1.2364 -->

    <owl:Class rdf:about="&pathLex;2364">
        <rdfs:subClassOf rdf:resource="&pathLex;99999"/>
        <skos:prefLabel xml:lang="en">Combined (or composite) small cell carcinoma, neuroendocrine type</skos:prefLabel>
        <skos:definition xml:lang="en">Larynx-Infiltrating malignant neoplasm-Histologic type-Combined (or composite) small cell carcinoma, neuroendocrine type</skos:definition>
    </owl:Class>
    


    <!-- http://www.semanticweb.org/david/ontologies/2013/0/1.3.6.1.4.1.19376.1.8.2.1.2365 -->

    <owl:Class rdf:about="&pathLex;2365">
        <rdfs:subClassOf rdf:resource="&pathLex;99999"/>
        <skos:definition xml:lang="en">Larynx-Infiltrating malignant neoplasm-Histologic type-Mucosal malignant melanoma</skos:definition>
        <skos:prefLabel xml:lang="en">Mucosal malignant melanoma</skos:prefLabel>
    </owl:Class>
    


    <!-- http://www.semanticweb.org/david/ontologies/2013/0/1.3.6.1.4.1.19376.1.8.2.1.2366 -->

    <owl:Class rdf:about="&pathLex;2366">
        <rdfs:subClassOf rdf:resource="&pathLex;99999"/>
        <skos:prefLabel xml:lang="en">Adenoid cystic carcinoma</skos:prefLabel>
        <skos:definition xml:lang="en">Larynx-Infiltrating malignant neoplasm-Histologic type-Adenoid cystic carcinoma</skos:definition>
    </owl:Class>
    


    <!-- http://www.semanticweb.org/david/ontologies/2013/0/1.3.6.1.4.1.19376.1.8.2.1.2367 -->

    <owl:Class rdf:about="&pathLex;2367">
        <rdfs:subClassOf rdf:resource="&pathLex;99999"/>
        <skos:definition xml:lang="en">Larynx-Infiltrating malignant neoplasm-Histologic type-Mucoepidermoid carcinoma</skos:definition>
        <skos:prefLabel xml:lang="en">Mucoepidermoid carcinoma</skos:prefLabel>
    </owl:Class>
    


    <!-- http://www.semanticweb.org/david/ontologies/2013/0/1.3.6.1.4.1.19376.1.8.2.1.2368 -->

    <owl:Class rdf:about="&pathLex;2368">
        <rdfs:subClassOf rdf:resource="&pathLex;99999"/>
        <skos:definition xml:lang="en">Larynx-Infiltrating malignant neoplasm-Histologic type-Other carcinoma (specify)</skos:definition>
        <skos:prefLabel xml:lang="en">Other carcinoma (specify)</skos:prefLabel>
    </owl:Class>
    


    <!-- http://www.semanticweb.org/david/ontologies/2013/0/1.3.6.1.4.1.19376.1.8.2.1.2369 -->

    <owl:Class rdf:about="&pathLex;2369">
        <rdfs:subClassOf rdf:resource="&pathLex;99999"/>
        <skos:prefLabel xml:lang="en">Carcinoma, type cannot be determinedd</skos:prefLabel>
        <skos:definition xml:lang="en">Larynx-Infiltrating malignant neoplasm-Histologic type-Carcinoma, type cannot be determinedd</skos:definition>
    </owl:Class>
    


    <!-- http://www.semanticweb.org/david/ontologies/2013/0/1.3.6.1.4.1.19376.1.8.2.1.237 -->

    <owl:Class rdf:about="&pathLex;237">
        <rdfs:subClassOf rdf:resource="&pathLex;99999"/>
        <skos:prefLabel xml:lang="en">Extent</skos:prefLabel>
        <skos:definition xml:lang="en">Larynx-Infiltrating malignant neoplasm-Extent</skos:definition>
    </owl:Class>
    


    <!-- http://www.semanticweb.org/david/ontologies/2013/0/1.3.6.1.4.1.19376.1.8.2.1.2370 -->

    <owl:Class rdf:about="&pathLex;2370">
        <rdfs:subClassOf rdf:resource="&pathLex;99999"/>
        <skos:prefLabel xml:lang="en">Acantholytic squamous cell carcinoma</skos:prefLabel>
        <skos:definition xml:lang="en">Lip, oral cavity-Infiltrating malignant neoplasm-Histologic type-Acantholytic squamous cell carcinoma</skos:definition>
    </owl:Class>
    


    <!-- http://www.semanticweb.org/david/ontologies/2013/0/1.3.6.1.4.1.19376.1.8.2.1.2371 -->

    <owl:Class rdf:about="&pathLex;2371">
        <rdfs:subClassOf rdf:resource="&pathLex;99999"/>
        <skos:prefLabel xml:lang="en">Carcinoma cuniculatum</skos:prefLabel>
        <skos:definition xml:lang="en">Lip, oral cavity-Infiltrating malignant neoplasm-Histologic type-Carcinoma cuniculatum</skos:definition>
    </owl:Class>
    


    <!-- http://www.semanticweb.org/david/ontologies/2013/0/1.3.6.1.4.1.19376.1.8.2.1.2372 -->

    <owl:Class rdf:about="&pathLex;2372">
        <rdfs:subClassOf rdf:resource="&pathLex;99999"/>
        <skos:definition xml:lang="en">Lip, oral cavity-Infiltrating malignant neoplasm-Histologic type-Papillary squamous cell carcinoma</skos:definition>
        <skos:prefLabel xml:lang="en">Papillary squamous cell carcinoma</skos:prefLabel>
    </owl:Class>
    


    <!-- http://www.semanticweb.org/david/ontologies/2013/0/1.3.6.1.4.1.19376.1.8.2.1.2373 -->

    <owl:Class rdf:about="&pathLex;2373">
        <rdfs:subClassOf rdf:resource="&pathLex;99999"/>
        <skos:definition xml:lang="en">Lip, oral cavity-Infiltrating malignant neoplasm-Histologic type-Lymphoepithelial carcinoma (non-nasopharyngeal)</skos:definition>
        <skos:prefLabel xml:lang="en">Lymphoepithelial carcinoma (non-nasopharyngeal)</skos:prefLabel>
    </owl:Class>
    


    <!-- http://www.semanticweb.org/david/ontologies/2013/0/1.3.6.1.4.1.19376.1.8.2.1.2374 -->

    <owl:Class rdf:about="&pathLex;2374">
        <rdfs:subClassOf rdf:resource="&pathLex;99999"/>
        <skos:prefLabel xml:lang="en">Carcinoma of Minor Salivary Glands: Acinic cell carcinoma</skos:prefLabel>
        <skos:definition xml:lang="en">Lip, oral cavity-Infiltrating malignant neoplasm-Histologic type-Carcinoma of Minor Salivary Glands: Acinic cell carcinoma</skos:definition>
    </owl:Class>
    


    <!-- http://www.semanticweb.org/david/ontologies/2013/0/1.3.6.1.4.1.19376.1.8.2.1.2375 -->

    <owl:Class rdf:about="&pathLex;2375">
        <rdfs:subClassOf rdf:resource="&pathLex;99999"/>
        <skos:prefLabel xml:lang="en">Carcinoma of Minor Salivary Glands: Adenoid cystic carcinoma</skos:prefLabel>
        <skos:definition xml:lang="en">Lip, oral cavity-Infiltrating malignant neoplasm-Histologic type-Carcinoma of Minor Salivary Glands: Adenoid cystic carcinoma</skos:definition>
    </owl:Class>
    


    <!-- http://www.semanticweb.org/david/ontologies/2013/0/1.3.6.1.4.1.19376.1.8.2.1.2376 -->

    <owl:Class rdf:about="&pathLex;2376">
        <rdfs:subClassOf rdf:resource="&pathLex;99999"/>
        <skos:prefLabel xml:lang="en">Carcinoma of Minor Salivary Glands: Adenocarcinoma, not otherwise specified (NOS)</skos:prefLabel>
        <skos:definition xml:lang="en">Lip, oral cavity-Infiltrating malignant neoplasm-Histologic type-Carcinoma of Minor Salivary Glands: Adenocarcinoma, not otherwise specified (NOS)</skos:definition>
    </owl:Class>
    


    <!-- http://www.semanticweb.org/david/ontologies/2013/0/1.3.6.1.4.1.19376.1.8.2.1.2377 -->

    <owl:Class rdf:about="&pathLex;2377">
        <rdfs:subClassOf rdf:resource="&pathLex;99999"/>
        <skos:prefLabel xml:lang="en">Carcinoma of Minor Salivary Glands: Basal cell adenocarcinoma</skos:prefLabel>
        <skos:definition xml:lang="en">Lip, oral cavity-Infiltrating malignant neoplasm-Histologic type-Carcinoma of Minor Salivary Glands: Basal cell adenocarcinoma</skos:definition>
    </owl:Class>
    


    <!-- http://www.semanticweb.org/david/ontologies/2013/0/1.3.6.1.4.1.19376.1.8.2.1.2378 -->

    <owl:Class rdf:about="&pathLex;2378">
        <rdfs:subClassOf rdf:resource="&pathLex;99999"/>
        <skos:prefLabel xml:lang="en">Carcinoma of Minor Salivary Glands: Carcinoma ex pleomorphic adenoma (malignant mixed tumor)</skos:prefLabel>
        <skos:definition xml:lang="en">Lip, oral cavity-Infiltrating malignant neoplasm-Histologic type-Carcinoma of Minor Salivary Glands: Carcinoma ex pleomorphic adenoma (malignant mixed tumor)</skos:definition>
    </owl:Class>
    


    <!-- http://www.semanticweb.org/david/ontologies/2013/0/1.3.6.1.4.1.19376.1.8.2.1.2379 -->

    <owl:Class rdf:about="&pathLex;2379">
        <rdfs:subClassOf rdf:resource="&pathLex;99999"/>
        <skos:prefLabel xml:lang="en">Carcinoma of Minor Salivary Glands: Carcinoma, type cannot be determinedd</skos:prefLabel>
        <skos:definition xml:lang="en">Lip, oral cavity-Infiltrating malignant neoplasm-Histologic type-Carcinoma of Minor Salivary Glands: Carcinoma, type cannot be determinedd</skos:definition>
    </owl:Class>
    


    <!-- http://www.semanticweb.org/david/ontologies/2013/0/1.3.6.1.4.1.19376.1.8.2.1.238 -->

    <owl:Class rdf:about="&pathLex;238">
        <rdfs:subClassOf rdf:resource="&pathLex;99999"/>
        <skos:definition xml:lang="en">Larynx-Infiltrating malignant neoplasm-Perineural invasion</skos:definition>
        <skos:prefLabel xml:lang="en">Perineural invasion</skos:prefLabel>
    </owl:Class>
    


    <!-- http://www.semanticweb.org/david/ontologies/2013/0/1.3.6.1.4.1.19376.1.8.2.1.2380 -->

    <owl:Class rdf:about="&pathLex;2380">
        <rdfs:subClassOf rdf:resource="&pathLex;99999"/>
        <skos:prefLabel xml:lang="en">Carcinoma of Minor Salivary Glands: Carcinosarcoma</skos:prefLabel>
        <skos:definition xml:lang="en">Lip, oral cavity-Infiltrating malignant neoplasm-Histologic type-Carcinoma of Minor Salivary Glands: Carcinosarcoma</skos:definition>
    </owl:Class>
    


    <!-- http://www.semanticweb.org/david/ontologies/2013/0/1.3.6.1.4.1.19376.1.8.2.1.2381 -->

    <owl:Class rdf:about="&pathLex;2381">
        <rdfs:subClassOf rdf:resource="&pathLex;99999"/>
        <skos:prefLabel xml:lang="en">Carcinoma of Minor Salivary Glands: Clear cell adenocarcinoma</skos:prefLabel>
        <skos:definition xml:lang="en">Lip, oral cavity-Infiltrating malignant neoplasm-Histologic type-Carcinoma of Minor Salivary Glands: Clear cell adenocarcinoma</skos:definition>
    </owl:Class>
    


    <!-- http://www.semanticweb.org/david/ontologies/2013/0/1.3.6.1.4.1.19376.1.8.2.1.2382 -->

    <owl:Class rdf:about="&pathLex;2382">
        <rdfs:subClassOf rdf:resource="&pathLex;99999"/>
        <skos:prefLabel xml:lang="en">Carcinoma of Minor Salivary Glands: Cystadenocarcinoma</skos:prefLabel>
        <skos:definition xml:lang="en">Lip, oral cavity-Infiltrating malignant neoplasm-Histologic type-Carcinoma of Minor Salivary Glands: Cystadenocarcinoma</skos:definition>
    </owl:Class>
    


    <!-- http://www.semanticweb.org/david/ontologies/2013/0/1.3.6.1.4.1.19376.1.8.2.1.2383 -->

    <owl:Class rdf:about="&pathLex;2383">
        <rdfs:subClassOf rdf:resource="&pathLex;99999"/>
        <skos:prefLabel xml:lang="en">Carcinoma of Minor Salivary Glands: Epithelial-myoepithelial carcinoma</skos:prefLabel>
        <skos:definition xml:lang="en">Lip, oral cavity-Infiltrating malignant neoplasm-Histologic type-Carcinoma of Minor Salivary Glands: Epithelial-myoepithelial carcinoma</skos:definition>
    </owl:Class>
    


    <!-- http://www.semanticweb.org/david/ontologies/2013/0/1.3.6.1.4.1.19376.1.8.2.1.2384 -->

    <owl:Class rdf:about="&pathLex;2384">
        <rdfs:subClassOf rdf:resource="&pathLex;99999"/>
        <skos:prefLabel xml:lang="en">Carcinoma of Minor Salivary Glands: Mucoepidermoid carcinoma</skos:prefLabel>
        <skos:definition xml:lang="en">Lip, oral cavity-Infiltrating malignant neoplasm-Histologic type-Carcinoma of Minor Salivary Glands: Mucoepidermoid carcinoma</skos:definition>
    </owl:Class>
    


    <!-- http://www.semanticweb.org/david/ontologies/2013/0/1.3.6.1.4.1.19376.1.8.2.1.2385 -->

    <owl:Class rdf:about="&pathLex;2385">
        <rdfs:subClassOf rdf:resource="&pathLex;99999"/>
        <skos:prefLabel xml:lang="en">Carcinoma of Minor Salivary Glands: Mucinous adenocarcinoma (colloid carcinoma)</skos:prefLabel>
        <skos:definition xml:lang="en">Lip, oral cavity-Infiltrating malignant neoplasm-Histologic type-Carcinoma of Minor Salivary Glands: Mucinous adenocarcinoma (colloid carcinoma)</skos:definition>
    </owl:Class>
    


    <!-- http://www.semanticweb.org/david/ontologies/2013/0/1.3.6.1.4.1.19376.1.8.2.1.2386 -->

    <owl:Class rdf:about="&pathLex;2386">
        <rdfs:subClassOf rdf:resource="&pathLex;99999"/>
        <skos:prefLabel xml:lang="en">Carcinoma of Minor Salivary Glands: Myoepithelial carcinoma (malignant myoepithelioma)</skos:prefLabel>
        <skos:definition xml:lang="en">Lip, oral cavity-Infiltrating malignant neoplasm-Histologic type-Carcinoma of Minor Salivary Glands: Myoepithelial carcinoma (malignant myoepithelioma)</skos:definition>
    </owl:Class>
    


    <!-- http://www.semanticweb.org/david/ontologies/2013/0/1.3.6.1.4.1.19376.1.8.2.1.2387 -->

    <owl:Class rdf:about="&pathLex;2387">
        <rdfs:subClassOf rdf:resource="&pathLex;99999"/>
        <skos:prefLabel xml:lang="en">Carcinoma of Minor Salivary Glands: Oncocytic carcinoma</skos:prefLabel>
        <skos:definition xml:lang="en">Lip, oral cavity-Infiltrating malignant neoplasm-Histologic type-Carcinoma of Minor Salivary Glands: Oncocytic carcinoma</skos:definition>
    </owl:Class>
    


    <!-- http://www.semanticweb.org/david/ontologies/2013/0/1.3.6.1.4.1.19376.1.8.2.1.2388 -->

    <owl:Class rdf:about="&pathLex;2388">
        <rdfs:subClassOf rdf:resource="&pathLex;99999"/>
        <skos:prefLabel xml:lang="en">Carcinoma of Minor Salivary Glands: Polymorphous low-grade adenocarcinoma</skos:prefLabel>
        <skos:definition xml:lang="en">Lip, oral cavity-Infiltrating malignant neoplasm-Histologic type-Carcinoma of Minor Salivary Glands: Polymorphous low-grade adenocarcinoma</skos:definition>
    </owl:Class>
    


    <!-- http://www.semanticweb.org/david/ontologies/2013/0/1.3.6.1.4.1.19376.1.8.2.1.2389 -->

    <owl:Class rdf:about="&pathLex;2389">
        <rdfs:subClassOf rdf:resource="&pathLex;99999"/>
        <skos:prefLabel xml:lang="en">Carcinoma of Minor Salivary Glands: Salivary duct carcinoma</skos:prefLabel>
        <skos:definition xml:lang="en">Lip, oral cavity-Infiltrating malignant neoplasm-Histologic type-Carcinoma of Minor Salivary Glands: Salivary duct carcinoma</skos:definition>
    </owl:Class>
    


    <!-- http://www.semanticweb.org/david/ontologies/2013/0/1.3.6.1.4.1.19376.1.8.2.1.239 -->

    <owl:Class rdf:about="&pathLex;239">
        <rdfs:subClassOf rdf:resource="&pathLex;99999"/>
        <skos:definition xml:lang="en">Larynx-Infiltrating malignant neoplasm-Lymph node capsule involvement</skos:definition>
        <skos:prefLabel xml:lang="en">Lymph node capsule involvement</skos:prefLabel>
    </owl:Class>
    


    <!-- http://www.semanticweb.org/david/ontologies/2013/0/1.3.6.1.4.1.19376.1.8.2.1.2390 -->

    <owl:Class rdf:about="&pathLex;2390">
        <rdfs:subClassOf rdf:resource="&pathLex;99999"/>
        <skos:prefLabel xml:lang="en">Carcinoma of Minor Salivary Glands: Other</skos:prefLabel>
        <skos:definition xml:lang="en">Lip, oral cavity-Infiltrating malignant neoplasm-Histologic type-Carcinoma of Minor Salivary Glands: Other</skos:definition>
    </owl:Class>
    


    <!-- http://www.semanticweb.org/david/ontologies/2013/0/1.3.6.1.4.1.19376.1.8.2.1.2391 -->

    <owl:Class rdf:about="&pathLex;2391">
        <rdfs:subClassOf rdf:resource="&pathLex;99999"/>
        <skos:prefLabel xml:lang="en">Adenocarcinoma, Non-Salivary Gland Type: Adenocarcinoma, not otherwise specified (NOS)</skos:prefLabel>
        <skos:definition xml:lang="en">Lip, oral cavity-Infiltrating malignant neoplasm-Histologic type-Adenocarcinoma, Non-Salivary Gland Type: Adenocarcinoma, not otherwise specified (NOS)</skos:definition>
    </owl:Class>
    


    <!-- http://www.semanticweb.org/david/ontologies/2013/0/1.3.6.1.4.1.19376.1.8.2.1.2392 -->

    <owl:Class rdf:about="&pathLex;2392">
        <rdfs:subClassOf rdf:resource="&pathLex;99999"/>
        <skos:prefLabel xml:lang="en">Adenocarcinoma, Non-Salivary Gland Type: Other</skos:prefLabel>
        <skos:definition xml:lang="en">Lip, oral cavity-Infiltrating malignant neoplasm-Histologic type-Adenocarcinoma, Non-Salivary Gland Type: Other</skos:definition>
    </owl:Class>
    


    <!-- http://www.semanticweb.org/david/ontologies/2013/0/1.3.6.1.4.1.19376.1.8.2.1.2393 -->

    <owl:Class rdf:about="&pathLex;2393">
        <rdfs:subClassOf rdf:resource="&pathLex;99999"/>
        <skos:definition xml:lang="en">Lip, oral cavity-Infiltrating malignant neoplasm-Histologic type-Neuroendocrine Carcinoma</skos:definition>
        <skos:prefLabel xml:lang="en">Neuroendocrine Carcinoma</skos:prefLabel>
    </owl:Class>
    


    <!-- http://www.semanticweb.org/david/ontologies/2013/0/1.3.6.1.4.1.19376.1.8.2.1.2394 -->

    <owl:Class rdf:about="&pathLex;2394">
        <rdfs:subClassOf rdf:resource="&pathLex;99999"/>
        <skos:definition xml:lang="en">Lip, oral cavity-Infiltrating malignant neoplasm-Histologic type-Neuroendocrine Carcinoma: Typical carcinoid tumor (well differentiated neuroendocrine carcinoma)</skos:definition>
        <skos:prefLabel xml:lang="en">Neuroendocrine Carcinoma: Typical carcinoid tumor (well differentiated neuroendocrine carcinoma)</skos:prefLabel>
    </owl:Class>
    


    <!-- http://www.semanticweb.org/david/ontologies/2013/0/1.3.6.1.4.1.19376.1.8.2.1.2395 -->

    <owl:Class rdf:about="&pathLex;2395">
        <rdfs:subClassOf rdf:resource="&pathLex;99999"/>
        <skos:definition xml:lang="en">Lip, oral cavity-Infiltrating malignant neoplasm-Histologic type-Neuroendocrine Carcinoma: Atypical carcinoid tumor (moderately differentiated neuroendocrine carcinoma)</skos:definition>
        <skos:prefLabel xml:lang="en">Neuroendocrine Carcinoma: Atypical carcinoid tumor (moderately differentiated neuroendocrine carcinoma)</skos:prefLabel>
    </owl:Class>
    


    <!-- http://www.semanticweb.org/david/ontologies/2013/0/1.3.6.1.4.1.19376.1.8.2.1.2396 -->

    <owl:Class rdf:about="&pathLex;2396">
        <rdfs:subClassOf rdf:resource="&pathLex;99999"/>
        <skos:definition xml:lang="en">Lip, oral cavity-Infiltrating malignant neoplasm-Histologic type-Neuroendocrine Carcinoma: Small cell carcinoma (poorly differentiated neuroendocrine carcinoma)</skos:definition>
        <skos:prefLabel xml:lang="en">Neuroendocrine Carcinoma: Small cell carcinoma (poorly differentiated neuroendocrine carcinoma)</skos:prefLabel>
    </owl:Class>
    


    <!-- http://www.semanticweb.org/david/ontologies/2013/0/1.3.6.1.4.1.19376.1.8.2.1.2397 -->

    <owl:Class rdf:about="&pathLex;2397">
        <rdfs:subClassOf rdf:resource="&pathLex;99999"/>
        <skos:definition xml:lang="en">Lip, oral cavity-Infiltrating malignant neoplasm-Histologic type-Neuroendocrine Carcinoma: Combined (or composite) small cell carcinoma, neuroendocrine type</skos:definition>
        <skos:prefLabel xml:lang="en">Neuroendocrine Carcinoma: Combined (or composite) small cell carcinoma, neuroendocrine type</skos:prefLabel>
    </owl:Class>
    


    <!-- http://www.semanticweb.org/david/ontologies/2013/0/1.3.6.1.4.1.19376.1.8.2.1.2398 -->

    <owl:Class rdf:about="&pathLex;2398">
        <rdfs:subClassOf rdf:resource="&pathLex;99999"/>
        <skos:definition xml:lang="en">Lip, oral cavity-Infiltrating malignant neoplasm-Histologic type-Neuroendocrine Carcinoma: Other</skos:definition>
        <skos:prefLabel xml:lang="en">Neuroendocrine Carcinoma: Other</skos:prefLabel>
    </owl:Class>
    


    <!-- http://www.semanticweb.org/david/ontologies/2013/0/1.3.6.1.4.1.19376.1.8.2.1.2399 -->

    <owl:Class rdf:about="&pathLex;2399">
        <rdfs:subClassOf rdf:resource="&pathLex;99999"/>
        <skos:prefLabel xml:lang="en">Carcinoma, type cannot be determined</skos:prefLabel>
        <skos:definition xml:lang="en">Lip, oral cavity-Infiltrating malignant neoplasm-Histologic type-Carcinoma, type cannot be determined</skos:definition>
    </owl:Class>
    


    <!-- http://www.semanticweb.org/david/ontologies/2013/0/1.3.6.1.4.1.19376.1.8.2.1.240 -->

    <owl:Class rdf:about="&pathLex;240">
        <rdfs:subClassOf rdf:resource="&pathLex;99999"/>
        <skos:definition xml:lang="en">Larynx-Infiltrating malignant neoplasm-Lesion site</skos:definition>
        <skos:prefLabel xml:lang="en">Lesion site</skos:prefLabel>
    </owl:Class>
    


    <!-- http://www.semanticweb.org/david/ontologies/2013/0/1.3.6.1.4.1.19376.1.8.2.1.2400 -->

    <owl:Class rdf:about="&pathLex;2400">
        <rdfs:subClassOf rdf:resource="&pathLex;99999"/>
        <skos:definition xml:lang="en">Lip, oral cavity-Infiltrating malignant neoplasm-Histologic type-Mucosal malignant melanoma</skos:definition>
        <skos:prefLabel xml:lang="en">Mucosal malignant melanoma</skos:prefLabel>
    </owl:Class>
    


    <!-- http://www.semanticweb.org/david/ontologies/2013/0/1.3.6.1.4.1.19376.1.8.2.1.2401 -->

    <owl:Class rdf:about="&pathLex;2401">
        <rdfs:subClassOf rdf:resource="&pathLex;99999"/>
        <skos:definition xml:lang="en">Lip, oral cavity-Lesion-Histologic type-Severe keratinizing dysplasia (carcinoma in situ)</skos:definition>
        <skos:prefLabel xml:lang="en">Severe keratinizing dysplasia (carcinoma in situ)</skos:prefLabel>
    </owl:Class>
    


    <!-- http://www.semanticweb.org/david/ontologies/2013/0/1.3.6.1.4.1.19376.1.8.2.1.2402 -->

    <owl:Class rdf:about="&pathLex;2402">
        <rdfs:subClassOf rdf:resource="&pathLex;99999"/>
        <skos:definition xml:lang="en">Lip, oral cavity-Lesion-Histologic type-Mild non-keratinizing dysplasia</skos:definition>
        <skos:prefLabel xml:lang="en">Mild non-keratinizing dysplasia</skos:prefLabel>
    </owl:Class>
    


    <!-- http://www.semanticweb.org/david/ontologies/2013/0/1.3.6.1.4.1.19376.1.8.2.1.2403 -->

    <owl:Class rdf:about="&pathLex;2403">
        <rdfs:subClassOf rdf:resource="&pathLex;99999"/>
        <skos:definition xml:lang="en">Lip, oral cavity-Lesion-Histologic type-Moderate non-keratinizing dysplasia</skos:definition>
        <skos:prefLabel xml:lang="en">Moderate non-keratinizing dysplasia</skos:prefLabel>
    </owl:Class>
    


    <!-- http://www.semanticweb.org/david/ontologies/2013/0/1.3.6.1.4.1.19376.1.8.2.1.2404 -->

    <owl:Class rdf:about="&pathLex;2404">
        <rdfs:subClassOf rdf:resource="&pathLex;99999"/>
        <skos:definition xml:lang="en">Lip, oral cavity-Lesion-Histologic type-Severe non-keratinizing dysplasia (carcinoma in situ)</skos:definition>
        <skos:prefLabel xml:lang="en">Severe non-keratinizing dysplasia (carcinoma in situ)</skos:prefLabel>
    </owl:Class>
    


    <!-- http://www.semanticweb.org/david/ontologies/2013/0/1.3.6.1.4.1.19376.1.8.2.1.2405 -->

    <owl:Class rdf:about="&pathLex;2405">
        <rdfs:subClassOf rdf:resource="&pathLex;99999"/>
        <skos:prefLabel xml:lang="en">Inflammation (specify)</skos:prefLabel>
        <skos:definition xml:lang="en">Lip, oral cavity-Lesion-Histologic type-Inflammation (specify)</skos:definition>
    </owl:Class>
    


    <!-- http://www.semanticweb.org/david/ontologies/2013/0/1.3.6.1.4.1.19376.1.8.2.1.2406 -->

    <owl:Class rdf:about="&pathLex;2406">
        <rdfs:subClassOf rdf:resource="&pathLex;99999"/>
        <skos:prefLabel xml:lang="en">Epithelial hyperplasia</skos:prefLabel>
        <skos:definition xml:lang="en">Lip, oral cavity-Lesion-Histologic type-Epithelial hyperplasia</skos:definition>
    </owl:Class>
    


    <!-- http://www.semanticweb.org/david/ontologies/2013/0/1.3.6.1.4.1.19376.1.8.2.1.2407 -->

    <owl:Class rdf:about="&pathLex;2407">
        <rdfs:subClassOf rdf:resource="&pathLex;99999"/>
        <skos:prefLabel xml:lang="en">Fungal colonization</skos:prefLabel>
        <skos:definition xml:lang="en">Lip, oral cavity-Lesion-Histologic type-Fungal colonization</skos:definition>
    </owl:Class>
    


    <!-- http://www.semanticweb.org/david/ontologies/2013/0/1.3.6.1.4.1.19376.1.8.2.1.2408 -->

    <owl:Class rdf:about="&pathLex;2408">
        <rdfs:subClassOf rdf:resource="&pathLex;99999"/>
        <skos:prefLabel xml:lang="en">Bacterial colonization</skos:prefLabel>
        <skos:definition xml:lang="en">Lip, oral cavity-Lesion-Histologic type-Bacterial colonization</skos:definition>
    </owl:Class>
    


    <!-- http://www.semanticweb.org/david/ontologies/2013/0/1.3.6.1.4.1.19376.1.8.2.1.2409 -->

    <owl:Class rdf:about="&pathLex;2409">
        <rdfs:subClassOf rdf:resource="&pathLex;99999"/>
        <skos:definition xml:lang="en">Esophagus-Infiltrating malignant neoplasm-Histologic type-Small cell carcinoma</skos:definition>
        <skos:prefLabel xml:lang="en">Small cell carcinoma</skos:prefLabel>
    </owl:Class>
    


    <!-- http://www.semanticweb.org/david/ontologies/2013/0/1.3.6.1.4.1.19376.1.8.2.1.241 -->

    <owl:Class rdf:about="&pathLex;241">
        <rdfs:subClassOf rdf:resource="&pathLex;99999"/>
        <skos:definition xml:lang="en">Larynx-Infiltrating malignant neoplasm-Lymph node site</skos:definition>
        <skos:prefLabel xml:lang="en">Lymph node site</skos:prefLabel>
    </owl:Class>
    


    <!-- http://www.semanticweb.org/david/ontologies/2013/0/1.3.6.1.4.1.19376.1.8.2.1.2410 -->

    <owl:Class rdf:about="&pathLex;2410">
        <rdfs:subClassOf rdf:resource="&pathLex;99999"/>
        <skos:definition xml:lang="en">Esophagus-Infiltrating malignant neoplasm-Histologic type-Undifferentiated carcinoma</skos:definition>
        <skos:prefLabel xml:lang="en">Undifferentiated carcinoma</skos:prefLabel>
    </owl:Class>
    


    <!-- http://www.semanticweb.org/david/ontologies/2013/0/1.3.6.1.4.1.19376.1.8.2.1.2411 -->

    <owl:Class rdf:about="&pathLex;2411">
        <rdfs:subClassOf rdf:resource="&pathLex;99999"/>
        <skos:prefLabel xml:lang="en">Carcinoma, type cannot be determinedd</skos:prefLabel>
        <skos:definition xml:lang="en">Esophagus-Infiltrating malignant neoplasm-Histologic type-Carcinoma, type cannot be determinedd</skos:definition>
    </owl:Class>
    


    <!-- http://www.semanticweb.org/david/ontologies/2013/0/1.3.6.1.4.1.19376.1.8.2.1.2412 -->

    <owl:Class rdf:about="&pathLex;2412">
        <rdfs:subClassOf rdf:resource="&pathLex;99999"/>
        <skos:definition xml:lang="en">Esophagus-Lesion-Histologic type-Intestinal metaplasia (Barrett’s esophagus)</skos:definition>
        <skos:prefLabel xml:lang="en">Intestinal metaplasia (Barrett’s esophagus)</skos:prefLabel>
    </owl:Class>
    


    <!-- http://www.semanticweb.org/david/ontologies/2013/0/1.3.6.1.4.1.19376.1.8.2.1.2413 -->

    <owl:Class rdf:about="&pathLex;2413">
        <rdfs:subClassOf rdf:resource="&pathLex;99999"/>
        <skos:definition xml:lang="en">Esophagus-Lesion-Histologic type-Low grade dysplasia</skos:definition>
        <skos:prefLabel xml:lang="en">Low grade dysplasia</skos:prefLabel>
    </owl:Class>
    


    <!-- http://www.semanticweb.org/david/ontologies/2013/0/1.3.6.1.4.1.19376.1.8.2.1.2414 -->

    <owl:Class rdf:about="&pathLex;2414">
        <rdfs:subClassOf rdf:resource="&pathLex;99999"/>
        <skos:definition xml:lang="en">Esophagus-Lesion-Histologic type-High grade dysplasia</skos:definition>
        <skos:prefLabel xml:lang="en">High grade dysplasia</skos:prefLabel>
    </owl:Class>
    


    <!-- http://www.semanticweb.org/david/ontologies/2013/0/1.3.6.1.4.1.19376.1.8.2.1.2415 -->

    <owl:Class rdf:about="&pathLex;2415">
        <rdfs:subClassOf rdf:resource="&pathLex;99999"/>
        <skos:prefLabel xml:lang="en">Esophagitis (specify)</skos:prefLabel>
        <skos:definition xml:lang="en">Esophagus-Lesion-Histologic type-Esophagitis (specify)</skos:definition>
    </owl:Class>
    


    <!-- http://www.semanticweb.org/david/ontologies/2013/0/1.3.6.1.4.1.19376.1.8.2.1.2416 -->

    <owl:Class rdf:about="&pathLex;2416">
        <rdfs:subClassOf rdf:resource="&pathLex;99999"/>
        <skos:definition xml:lang="en">Esophagus-Lesion-Histologic type-Gastritis (specify)</skos:definition>
        <skos:prefLabel xml:lang="en">Gastritis (specify)</skos:prefLabel>
    </owl:Class>
    


    <!-- http://www.semanticweb.org/david/ontologies/2013/0/1.3.6.1.4.1.19376.1.8.2.1.2417 -->

    <owl:Class rdf:about="&pathLex;2417">
        <rdfs:subClassOf rdf:resource="&pathLex;99999"/>
        <skos:prefLabel xml:lang="en">Mucinous, borderline tumor, intestinal type</skos:prefLabel>
        <skos:definition xml:lang="en">Ovary-Infiltrating malignant neoplasm-Histologic type-Mucinous, borderline tumor, intestinal type</skos:definition>
    </owl:Class>
    


    <!-- http://www.semanticweb.org/david/ontologies/2013/0/1.3.6.1.4.1.19376.1.8.2.1.2418 -->

    <owl:Class rdf:about="&pathLex;2418">
        <rdfs:subClassOf rdf:resource="&pathLex;99999"/>
        <skos:prefLabel xml:lang="en">Mucinous, borderline tumor, endocervical type (seromucinous type)</skos:prefLabel>
        <skos:definition xml:lang="en">Ovary-Infiltrating malignant neoplasm-Histologic type-Mucinous, borderline tumor, endocervical type (seromucinous type)</skos:definition>
    </owl:Class>
    


    <!-- http://www.semanticweb.org/david/ontologies/2013/0/1.3.6.1.4.1.19376.1.8.2.1.2419 -->

    <owl:Class rdf:about="&pathLex;2419">
        <rdfs:subClassOf rdf:resource="&pathLex;99999"/>
        <skos:prefLabel xml:lang="en">Brenner tumor, malignant type</skos:prefLabel>
        <skos:definition xml:lang="en">Ovary-Infiltrating malignant neoplasm-Histologic type-Brenner tumor, malignant type</skos:definition>
    </owl:Class>
    


    <!-- http://www.semanticweb.org/david/ontologies/2013/0/1.3.6.1.4.1.19376.1.8.2.1.242 -->

    <owl:Class rdf:about="&pathLex;242">
        <rdfs:subClassOf rdf:resource="&pathLex;99999"/>
        <skos:definition xml:lang="en">Larynx-Infiltrating malignant neoplasm-Number of lymph nodes involved</skos:definition>
        <skos:prefLabel xml:lang="en">Number of lymph nodes involved</skos:prefLabel>
    </owl:Class>
    


    <!-- http://www.semanticweb.org/david/ontologies/2013/0/1.3.6.1.4.1.19376.1.8.2.1.2420 -->

    <owl:Class rdf:about="&pathLex;2420">
        <rdfs:subClassOf rdf:resource="&pathLex;99999"/>
        <skos:definition xml:lang="en">Ovary-Infiltrating malignant neoplasm-Histologic type-Squamous cell carcinoma</skos:definition>
        <skos:prefLabel xml:lang="en">Squamous cell carcinoma</skos:prefLabel>
    </owl:Class>
    


    <!-- http://www.semanticweb.org/david/ontologies/2013/0/1.3.6.1.4.1.19376.1.8.2.1.2421 -->

    <owl:Class rdf:about="&pathLex;2421">
        <rdfs:subClassOf rdf:resource="&pathLex;99999"/>
        <skos:prefLabel xml:lang="en">Mixed epithelial borderline tumor (specify types and percentages)</skos:prefLabel>
        <skos:definition xml:lang="en">Ovary-Infiltrating malignant neoplasm-Histologic type-Mixed epithelial borderline tumor (specify types and percentages)</skos:definition>
    </owl:Class>
    


    <!-- http://www.semanticweb.org/david/ontologies/2013/0/1.3.6.1.4.1.19376.1.8.2.1.2422 -->

    <owl:Class rdf:about="&pathLex;2422">
        <rdfs:subClassOf rdf:resource="&pathLex;99999"/>
        <skos:prefLabel xml:lang="en">Mixed epithelial carcinoma (specify types and percentages)</skos:prefLabel>
        <skos:definition xml:lang="en">Ovary-Infiltrating malignant neoplasm-Histologic type-Mixed epithelial carcinoma (specify types and percentages)</skos:definition>
    </owl:Class>
    


    <!-- http://www.semanticweb.org/david/ontologies/2013/0/1.3.6.1.4.1.19376.1.8.2.1.2423 -->

    <owl:Class rdf:about="&pathLex;2423">
        <rdfs:subClassOf rdf:resource="&pathLex;99999"/>
        <skos:definition xml:lang="en">Ovary-Infiltrating malignant neoplasm-Histologic type-Undifferentiated carcinoma</skos:definition>
        <skos:prefLabel xml:lang="en">Undifferentiated carcinoma</skos:prefLabel>
    </owl:Class>
    


    <!-- http://www.semanticweb.org/david/ontologies/2013/0/1.3.6.1.4.1.19376.1.8.2.1.2424 -->

    <owl:Class rdf:about="&pathLex;2424">
        <rdfs:subClassOf rdf:resource="&pathLex;99999"/>
        <skos:prefLabel xml:lang="en">Carcinosarcoma (Malignant müllerian mixed tumor)</skos:prefLabel>
        <skos:definition xml:lang="en">Ovary-Infiltrating malignant neoplasm-Histologic type-Carcinosarcoma (Malignant müllerian mixed tumor)</skos:definition>
    </owl:Class>
    


    <!-- http://www.semanticweb.org/david/ontologies/2013/0/1.3.6.1.4.1.19376.1.8.2.1.2425 -->

    <owl:Class rdf:about="&pathLex;2425">
        <rdfs:subClassOf rdf:resource="&pathLex;99999"/>
        <skos:prefLabel xml:lang="en">Granulosa cell tumor</skos:prefLabel>
        <skos:definition xml:lang="en">Ovary-Infiltrating malignant neoplasm-Histologic type-Granulosa cell tumor</skos:definition>
    </owl:Class>
    


    <!-- http://www.semanticweb.org/david/ontologies/2013/0/1.3.6.1.4.1.19376.1.8.2.1.2426 -->

    <owl:Class rdf:about="&pathLex;2426">
        <rdfs:subClassOf rdf:resource="&pathLex;99999"/>
        <skos:prefLabel xml:lang="en">Ovarian endometriosis</skos:prefLabel>
        <skos:definition xml:lang="en">Ovary-Lesion-Histologic type-Ovarian endometriosis</skos:definition>
    </owl:Class>
    


    <!-- http://www.semanticweb.org/david/ontologies/2013/0/1.3.6.1.4.1.19376.1.8.2.1.2427 -->

    <owl:Class rdf:about="&pathLex;2427">
        <rdfs:subClassOf rdf:resource="&pathLex;99999"/>
        <skos:prefLabel xml:lang="en">Extraovarian endometriosis</skos:prefLabel>
        <skos:definition xml:lang="en">Ovary-Lesion-Histologic type-Extraovarian endometriosis</skos:definition>
    </owl:Class>
    


    <!-- http://www.semanticweb.org/david/ontologies/2013/0/1.3.6.1.4.1.19376.1.8.2.1.2428 -->

    <owl:Class rdf:about="&pathLex;2428">
        <rdfs:subClassOf rdf:resource="&pathLex;99999"/>
        <skos:prefLabel xml:lang="en">Endosalpingiosis</skos:prefLabel>
        <skos:definition xml:lang="en">Ovary-Lesion-Histologic type-Endosalpingiosis</skos:definition>
    </owl:Class>
    


    <!-- http://www.semanticweb.org/david/ontologies/2013/0/1.3.6.1.4.1.19376.1.8.2.1.2429 -->

    <owl:Class rdf:about="&pathLex;2429">
        <rdfs:subClassOf rdf:resource="&pathLex;99999"/>
        <skos:definition xml:lang="en">Pancreas-Infiltrating malignant neoplasm-Histologic type-Undifferentiated (anaplastic) carcinoma</skos:definition>
        <skos:prefLabel xml:lang="en">Undifferentiated (anaplastic) carcinoma</skos:prefLabel>
    </owl:Class>
    


    <!-- http://www.semanticweb.org/david/ontologies/2013/0/1.3.6.1.4.1.19376.1.8.2.1.243 -->

    <owl:Class rdf:about="&pathLex;243">
        <rdfs:subClassOf rdf:resource="&pathLex;99999"/>
        <skos:definition xml:lang="en">Larynx-Infiltrating malignant neoplasm-Number of lymph nodes examined</skos:definition>
        <skos:prefLabel xml:lang="en">Number of lymph nodes examined</skos:prefLabel>
    </owl:Class>
    


    <!-- http://www.semanticweb.org/david/ontologies/2013/0/1.3.6.1.4.1.19376.1.8.2.1.2430 -->

    <owl:Class rdf:about="&pathLex;2430">
        <rdfs:subClassOf rdf:resource="&pathLex;99999"/>
        <skos:definition xml:lang="en">Pancreas-Infiltrating malignant neoplasm-Histologic type-Undifferentiated carcinoma with osteoclast-like giant cells</skos:definition>
        <skos:prefLabel xml:lang="en">Undifferentiated carcinoma with osteoclast-like giant cells</skos:prefLabel>
    </owl:Class>
    


    <!-- http://www.semanticweb.org/david/ontologies/2013/0/1.3.6.1.4.1.19376.1.8.2.1.2431 -->

    <owl:Class rdf:about="&pathLex;2431">
        <rdfs:subClassOf rdf:resource="&pathLex;99999"/>
        <skos:prefLabel xml:lang="en">Mixed ductal-endocrine carcinoma</skos:prefLabel>
        <skos:definition xml:lang="en">Pancreas-Infiltrating malignant neoplasm-Histologic type-Mixed ductal-endocrine carcinoma</skos:definition>
    </owl:Class>
    


    <!-- http://www.semanticweb.org/david/ontologies/2013/0/1.3.6.1.4.1.19376.1.8.2.1.2432 -->

    <owl:Class rdf:about="&pathLex;2432">
        <rdfs:subClassOf rdf:resource="&pathLex;99999"/>
        <skos:prefLabel xml:lang="en">Noninvasive mucinous cystic neoplasm</skos:prefLabel>
        <skos:definition xml:lang="en">Pancreas-Infiltrating malignant neoplasm-Histologic type-Noninvasive mucinous cystic neoplasm</skos:definition>
    </owl:Class>
    


    <!-- http://www.semanticweb.org/david/ontologies/2013/0/1.3.6.1.4.1.19376.1.8.2.1.2433 -->

    <owl:Class rdf:about="&pathLex;2433">
        <rdfs:subClassOf rdf:resource="&pathLex;99999"/>
        <skos:prefLabel xml:lang="en">Noninvasive intraductal papillary-mucinous carcinoma</skos:prefLabel>
        <skos:definition xml:lang="en">Pancreas-Infiltrating malignant neoplasm-Histologic type-Noninvasive intraductal papillary-mucinous carcinoma</skos:definition>
    </owl:Class>
    


    <!-- http://www.semanticweb.org/david/ontologies/2013/0/1.3.6.1.4.1.19376.1.8.2.1.2434 -->

    <owl:Class rdf:about="&pathLex;2434">
        <rdfs:subClassOf rdf:resource="&pathLex;99999"/>
        <skos:prefLabel xml:lang="en">Mixed acinar-endocrine carcinoma</skos:prefLabel>
        <skos:definition xml:lang="en">Pancreas-Infiltrating malignant neoplasm-Histologic type-Mixed acinar-endocrine carcinoma</skos:definition>
    </owl:Class>
    


    <!-- http://www.semanticweb.org/david/ontologies/2013/0/1.3.6.1.4.1.19376.1.8.2.1.2435 -->

    <owl:Class rdf:about="&pathLex;2435">
        <rdfs:subClassOf rdf:resource="&pathLex;99999"/>
        <skos:definition xml:lang="en">Pancreas-Lesion-Histologic type-Pancreatic intraepithelial neoplasia</skos:definition>
        <skos:prefLabel xml:lang="en">Pancreatic intraepithelial neoplasia</skos:prefLabel>
    </owl:Class>
    


    <!-- http://www.semanticweb.org/david/ontologies/2013/0/1.3.6.1.4.1.19376.1.8.2.1.2436 -->

    <owl:Class rdf:about="&pathLex;2436">
        <rdfs:subClassOf rdf:resource="&pathLex;99999"/>
        <skos:prefLabel xml:lang="en">Malignant melanoma</skos:prefLabel>
        <skos:definition xml:lang="en">Skin (melanoma)-Infiltrating malignant neoplasm-Histologic type-Malignant melanoma</skos:definition>
    </owl:Class>
    


    <!-- http://www.semanticweb.org/david/ontologies/2013/0/1.3.6.1.4.1.19376.1.8.2.1.2437 -->

    <owl:Class rdf:about="&pathLex;2437">
        <rdfs:subClassOf rdf:resource="&pathLex;99999"/>
        <skos:prefLabel xml:lang="en">Melanoma, not otherwise classified</skos:prefLabel>
        <skos:definition xml:lang="en">Skin (melanoma)-Infiltrating malignant neoplasm-Histologic type-Melanoma, not otherwise classified</skos:definition>
    </owl:Class>
    


    <!-- http://www.semanticweb.org/david/ontologies/2013/0/1.3.6.1.4.1.19376.1.8.2.1.2438 -->

    <owl:Class rdf:about="&pathLex;2438">
        <rdfs:subClassOf rdf:resource="&pathLex;99999"/>
        <skos:prefLabel xml:lang="en">Lentigo maligna melanoma</skos:prefLabel>
        <skos:definition xml:lang="en">Skin (melanoma)-Infiltrating malignant neoplasm-Histologic type-Lentigo maligna melanoma</skos:definition>
    </owl:Class>
    


    <!-- http://www.semanticweb.org/david/ontologies/2013/0/1.3.6.1.4.1.19376.1.8.2.1.2439 -->

    <owl:Class rdf:about="&pathLex;2439">
        <rdfs:subClassOf rdf:resource="&pathLex;99999"/>
        <skos:prefLabel xml:lang="en">Acral-lentiginous melanoma</skos:prefLabel>
        <skos:definition xml:lang="en">Skin (melanoma)-Infiltrating malignant neoplasm-Histologic type-Acral-lentiginous melanoma</skos:definition>
    </owl:Class>
    


    <!-- http://www.semanticweb.org/david/ontologies/2013/0/1.3.6.1.4.1.19376.1.8.2.1.2440 -->

    <owl:Class rdf:about="&pathLex;2440">
        <rdfs:subClassOf rdf:resource="&pathLex;99999"/>
        <skos:prefLabel xml:lang="en">Desmoplastic and/or desmoplastic neurotropic melanoma</skos:prefLabel>
        <skos:definition xml:lang="en">Skin (melanoma)-Infiltrating malignant neoplasm-Histologic type-Desmoplastic and/or desmoplastic neurotropic melanoma</skos:definition>
    </owl:Class>
    


    <!-- http://www.semanticweb.org/david/ontologies/2013/0/1.3.6.1.4.1.19376.1.8.2.1.2441 -->

    <owl:Class rdf:about="&pathLex;2441">
        <rdfs:subClassOf rdf:resource="&pathLex;99999"/>
        <skos:prefLabel xml:lang="en">Melanoma arising from blue nevus</skos:prefLabel>
        <skos:definition xml:lang="en">Skin (melanoma)-Infiltrating malignant neoplasm-Histologic type-Melanoma arising from blue nevus</skos:definition>
    </owl:Class>
    


    <!-- http://www.semanticweb.org/david/ontologies/2013/0/1.3.6.1.4.1.19376.1.8.2.1.2442 -->

    <owl:Class rdf:about="&pathLex;2442">
        <rdfs:subClassOf rdf:resource="&pathLex;99999"/>
        <skos:prefLabel xml:lang="en">Melanoma arising in a giant congenital nevus</skos:prefLabel>
        <skos:definition xml:lang="en">Skin (melanoma)-Infiltrating malignant neoplasm-Histologic type-Melanoma arising in a giant congenital nevus</skos:definition>
    </owl:Class>
    


    <!-- http://www.semanticweb.org/david/ontologies/2013/0/1.3.6.1.4.1.19376.1.8.2.1.2443 -->

    <owl:Class rdf:about="&pathLex;2443">
        <rdfs:subClassOf rdf:resource="&pathLex;99999"/>
        <skos:prefLabel xml:lang="en">Melanoma of childhood</skos:prefLabel>
        <skos:definition xml:lang="en">Skin (melanoma)-Infiltrating malignant neoplasm-Histologic type-Melanoma of childhood</skos:definition>
    </owl:Class>
    


    <!-- http://www.semanticweb.org/david/ontologies/2013/0/1.3.6.1.4.1.19376.1.8.2.1.2444 -->

    <owl:Class rdf:about="&pathLex;2444">
        <rdfs:subClassOf rdf:resource="&pathLex;99999"/>
        <skos:prefLabel xml:lang="en">Nevoid melanoma</skos:prefLabel>
        <skos:definition xml:lang="en">Skin (melanoma)-Infiltrating malignant neoplasm-Histologic type-Nevoid melanoma</skos:definition>
    </owl:Class>
    


    <!-- http://www.semanticweb.org/david/ontologies/2013/0/1.3.6.1.4.1.19376.1.8.2.1.2445 -->

    <owl:Class rdf:about="&pathLex;2445">
        <rdfs:subClassOf rdf:resource="&pathLex;99999"/>
        <skos:prefLabel xml:lang="en">Persistent melanoma</skos:prefLabel>
        <skos:definition xml:lang="en">Skin (melanoma)-Infiltrating malignant neoplasm-Histologic type-Persistent melanoma</skos:definition>
    </owl:Class>
    


    <!-- http://www.semanticweb.org/david/ontologies/2013/0/1.3.6.1.4.1.19376.1.8.2.1.2446 -->

    <owl:Class rdf:about="&pathLex;2446">
        <rdfs:subClassOf rdf:resource="&pathLex;99999"/>
        <skos:prefLabel xml:lang="en">Carcinoma of the Oropharynx and Hypopharynx: Squamous cell carcinoma, conventional</skos:prefLabel>
        <skos:definition xml:lang="en">Pharynx-Infiltrating malignant neoplasm-Histologic type-Carcinoma of the Oropharynx and Hypopharynx: Squamous cell carcinoma, conventional</skos:definition>
    </owl:Class>
    


    <!-- http://www.semanticweb.org/david/ontologies/2013/0/1.3.6.1.4.1.19376.1.8.2.1.2447 -->

    <owl:Class rdf:about="&pathLex;2447">
        <rdfs:subClassOf rdf:resource="&pathLex;99999"/>
        <skos:prefLabel xml:lang="en">Carcinoma of the Oropharynx and Hypopharynx: Acantholytic squamous cell carcinoma</skos:prefLabel>
        <skos:definition xml:lang="en">Pharynx-Infiltrating malignant neoplasm-Histologic type-Carcinoma of the Oropharynx and Hypopharynx: Acantholytic squamous cell carcinoma</skos:definition>
    </owl:Class>
    


    <!-- http://www.semanticweb.org/david/ontologies/2013/0/1.3.6.1.4.1.19376.1.8.2.1.2448 -->

    <owl:Class rdf:about="&pathLex;2448">
        <rdfs:subClassOf rdf:resource="&pathLex;99999"/>
        <skos:prefLabel xml:lang="en">Carcinoma of the Oropharynx and Hypopharynx: Adenosquamous carcinoma</skos:prefLabel>
        <skos:definition xml:lang="en">Pharynx-Infiltrating malignant neoplasm-Histologic type-Carcinoma of the Oropharynx and Hypopharynx: Adenosquamous carcinoma</skos:definition>
    </owl:Class>
    


    <!-- http://www.semanticweb.org/david/ontologies/2013/0/1.3.6.1.4.1.19376.1.8.2.1.2449 -->

    <owl:Class rdf:about="&pathLex;2449">
        <rdfs:subClassOf rdf:resource="&pathLex;99999"/>
        <skos:prefLabel xml:lang="en">Carcinoma of the Oropharynx and Hypopharynx: Basaloid squamous cell carcinoma</skos:prefLabel>
        <skos:definition xml:lang="en">Pharynx-Infiltrating malignant neoplasm-Histologic type-Carcinoma of the Oropharynx and Hypopharynx: Basaloid squamous cell carcinoma</skos:definition>
    </owl:Class>
    


    <!-- http://www.semanticweb.org/david/ontologies/2013/0/1.3.6.1.4.1.19376.1.8.2.1.2450 -->

    <owl:Class rdf:about="&pathLex;2450">
        <rdfs:subClassOf rdf:resource="&pathLex;99999"/>
        <skos:prefLabel xml:lang="en">Carcinoma of the Oropharynx and Hypopharynx: Papillary squamous cell carcinoma</skos:prefLabel>
        <skos:definition xml:lang="en">Pharynx-Infiltrating malignant neoplasm-Histologic type-Carcinoma of the Oropharynx and Hypopharynx: Papillary squamous cell carcinoma</skos:definition>
    </owl:Class>
    


    <!-- http://www.semanticweb.org/david/ontologies/2013/0/1.3.6.1.4.1.19376.1.8.2.1.2451 -->

    <owl:Class rdf:about="&pathLex;2451">
        <rdfs:subClassOf rdf:resource="&pathLex;99999"/>
        <skos:prefLabel xml:lang="en">Carcinoma of the Oropharynx and Hypopharynx: Spindle cell squamous carcinoma</skos:prefLabel>
        <skos:definition xml:lang="en">Pharynx-Infiltrating malignant neoplasm-Histologic type-Carcinoma of the Oropharynx and Hypopharynx: Spindle cell squamous carcinoma</skos:definition>
    </owl:Class>
    


    <!-- http://www.semanticweb.org/david/ontologies/2013/0/1.3.6.1.4.1.19376.1.8.2.1.2452 -->

    <owl:Class rdf:about="&pathLex;2452">
        <rdfs:subClassOf rdf:resource="&pathLex;99999"/>
        <skos:prefLabel xml:lang="en">Carcinoma of the Oropharynx and Hypopharynx: Verrucous carcinoma</skos:prefLabel>
        <skos:definition xml:lang="en">Pharynx-Infiltrating malignant neoplasm-Histologic type-Carcinoma of the Oropharynx and Hypopharynx: Verrucous carcinoma</skos:definition>
    </owl:Class>
    


    <!-- http://www.semanticweb.org/david/ontologies/2013/0/1.3.6.1.4.1.19376.1.8.2.1.2453 -->

    <owl:Class rdf:about="&pathLex;2453">
        <rdfs:subClassOf rdf:resource="&pathLex;99999"/>
        <skos:prefLabel xml:lang="en">Carcinoma of the Oropharynx and Hypopharynx: Lymphoepithelial carcinoma (non-nasopharyngeal)</skos:prefLabel>
        <skos:definition xml:lang="en">Pharynx-Infiltrating malignant neoplasm-Histologic type-Carcinoma of the Oropharynx and Hypopharynx: Lymphoepithelial carcinoma (non-nasopharyngeal)</skos:definition>
    </owl:Class>
    


    <!-- http://www.semanticweb.org/david/ontologies/2013/0/1.3.6.1.4.1.19376.1.8.2.1.2454 -->

    <owl:Class rdf:about="&pathLex;2454">
        <rdfs:subClassOf rdf:resource="&pathLex;99999"/>
        <skos:prefLabel xml:lang="en">Keratinizing squamous cell carcinoma (formerly WHO-1) of the Nasopharynx</skos:prefLabel>
        <skos:definition xml:lang="en">Pharynx-Infiltrating malignant neoplasm-Histologic type-Keratinizing squamous cell carcinoma (formerly WHO-1) of the Nasopharynx</skos:definition>
    </owl:Class>
    


    <!-- http://www.semanticweb.org/david/ontologies/2013/0/1.3.6.1.4.1.19376.1.8.2.1.2455 -->

    <owl:Class rdf:about="&pathLex;2455">
        <rdfs:subClassOf rdf:resource="&pathLex;99999"/>
        <skos:prefLabel xml:lang="en">Nonkeratinizing carcinoma of the Nasopharynx</skos:prefLabel>
        <skos:definition xml:lang="en">Pharynx-Infiltrating malignant neoplasm-Histologic type-Nonkeratinizing carcinoma of the Nasopharynx</skos:definition>
    </owl:Class>
    


    <!-- http://www.semanticweb.org/david/ontologies/2013/0/1.3.6.1.4.1.19376.1.8.2.1.2456 -->

    <owl:Class rdf:about="&pathLex;2456">
        <rdfs:subClassOf rdf:resource="&pathLex;99999"/>
        <skos:prefLabel xml:lang="en">Differentiated carcinoma (formerly WHO-2; transitional carcinoma) of the Nasopharynx</skos:prefLabel>
        <skos:definition xml:lang="en">Pharynx-Infiltrating malignant neoplasm-Histologic type-Differentiated carcinoma (formerly WHO-2; transitional carcinoma) of the Nasopharynx</skos:definition>
    </owl:Class>
    


    <!-- http://www.semanticweb.org/david/ontologies/2013/0/1.3.6.1.4.1.19376.1.8.2.1.2457 -->

    <owl:Class rdf:about="&pathLex;2457">
        <rdfs:subClassOf rdf:resource="&pathLex;99999"/>
        <skos:definition xml:lang="en">Pharynx-Infiltrating malignant neoplasm-Histologic type-Undifferentiated carcinoma (formerly WHO-3; lymphoepithelioma) of the Nasopharynx</skos:definition>
        <skos:prefLabel xml:lang="en">Undifferentiated carcinoma (formerly WHO-3; lymphoepithelioma) of the Nasopharynx</skos:prefLabel>
    </owl:Class>
    


    <!-- http://www.semanticweb.org/david/ontologies/2013/0/1.3.6.1.4.1.19376.1.8.2.1.2458 -->

    <owl:Class rdf:about="&pathLex;2458">
        <rdfs:subClassOf rdf:resource="&pathLex;99999"/>
        <skos:prefLabel xml:lang="en">Basaloid squamous cell carcinoma of the Nasopharynx</skos:prefLabel>
        <skos:definition xml:lang="en">Pharynx-Infiltrating malignant neoplasm-Histologic type-Basaloid squamous cell carcinoma of the Nasopharynx</skos:definition>
    </owl:Class>
    


    <!-- http://www.semanticweb.org/david/ontologies/2013/0/1.3.6.1.4.1.19376.1.8.2.1.2459 -->

    <owl:Class rdf:about="&pathLex;2459">
        <rdfs:subClassOf rdf:resource="&pathLex;99999"/>
        <skos:prefLabel xml:lang="en">AdenoCarcinoma (Non-Salivary Gland Type): Nasopharyngeal papillary adenocarcinoma</skos:prefLabel>
        <skos:definition xml:lang="en">Pharynx-Infiltrating malignant neoplasm-Histologic type-AdenoCarcinoma (Non-Salivary Gland Type): Nasopharyngeal papillary adenocarcinoma</skos:definition>
    </owl:Class>
    


    <!-- http://www.semanticweb.org/david/ontologies/2013/0/1.3.6.1.4.1.19376.1.8.2.1.246 -->

    <owl:Class rdf:about="&pathLex;246">
        <rdfs:subClassOf rdf:resource="&pathLex;99999"/>
        <skos:definition xml:lang="en">Larynx-Infiltrating malignant neoplasm-Lesion size, largest dimension</skos:definition>
        <skos:prefLabel xml:lang="en">Lesion size, largest dimension</skos:prefLabel>
    </owl:Class>
    


    <!-- http://www.semanticweb.org/david/ontologies/2013/0/1.3.6.1.4.1.19376.1.8.2.1.2460 -->

    <owl:Class rdf:about="&pathLex;2460">
        <rdfs:subClassOf rdf:resource="&pathLex;99999"/>
        <skos:prefLabel xml:lang="en">AdenoCarcinoma (Non-Salivary Gland Type): Adenocarcinoma, not otherwise specified (NOS)</skos:prefLabel>
        <skos:definition xml:lang="en">Pharynx-Infiltrating malignant neoplasm-Histologic type-AdenoCarcinoma (Non-Salivary Gland Type): Adenocarcinoma, not otherwise specified (NOS)</skos:definition>
    </owl:Class>
    


    <!-- http://www.semanticweb.org/david/ontologies/2013/0/1.3.6.1.4.1.19376.1.8.2.1.2461 -->

    <owl:Class rdf:about="&pathLex;2461">
        <rdfs:subClassOf rdf:resource="&pathLex;99999"/>
        <skos:prefLabel xml:lang="en">AdenoCarcinoma (Non-Salivary Gland Type): Other:</skos:prefLabel>
        <skos:definition xml:lang="en">Pharynx-Infiltrating malignant neoplasm-Histologic type-AdenoCarcinoma (Non-Salivary Gland Type): Other:</skos:definition>
    </owl:Class>
    


    <!-- http://www.semanticweb.org/david/ontologies/2013/0/1.3.6.1.4.1.19376.1.8.2.1.2462 -->

    <owl:Class rdf:about="&pathLex;2462">
        <rdfs:subClassOf rdf:resource="&pathLex;99999"/>
        <skos:prefLabel xml:lang="en">Carcinoma of Minor Salivary Glands: Acinic cell carcinoma</skos:prefLabel>
        <skos:definition xml:lang="en">Pharynx-Infiltrating malignant neoplasm-Histologic type-Carcinoma of Minor Salivary Glands: Acinic cell carcinoma</skos:definition>
    </owl:Class>
    


    <!-- http://www.semanticweb.org/david/ontologies/2013/0/1.3.6.1.4.1.19376.1.8.2.1.2463 -->

    <owl:Class rdf:about="&pathLex;2463">
        <rdfs:subClassOf rdf:resource="&pathLex;99999"/>
        <skos:prefLabel xml:lang="en">Carcinoma of Minor Salivary Glands: Adenoid cystic carcinoma</skos:prefLabel>
        <skos:definition xml:lang="en">Pharynx-Infiltrating malignant neoplasm-Histologic type-Carcinoma of Minor Salivary Glands: Adenoid cystic carcinoma</skos:definition>
    </owl:Class>
    


    <!-- http://www.semanticweb.org/david/ontologies/2013/0/1.3.6.1.4.1.19376.1.8.2.1.2464 -->

    <owl:Class rdf:about="&pathLex;2464">
        <rdfs:subClassOf rdf:resource="&pathLex;99999"/>
        <skos:prefLabel xml:lang="en">Carcinoma of Minor Salivary Glands: Adenocarcinoma, not otherwise specified (NOS)</skos:prefLabel>
        <skos:definition xml:lang="en">Pharynx-Infiltrating malignant neoplasm-Histologic type-Carcinoma of Minor Salivary Glands: Adenocarcinoma, not otherwise specified (NOS)</skos:definition>
    </owl:Class>
    


    <!-- http://www.semanticweb.org/david/ontologies/2013/0/1.3.6.1.4.1.19376.1.8.2.1.2465 -->

    <owl:Class rdf:about="&pathLex;2465">
        <rdfs:subClassOf rdf:resource="&pathLex;99999"/>
        <skos:prefLabel xml:lang="en">Carcinoma of Minor Salivary Glands: Basal cell adenocarcinoma</skos:prefLabel>
        <skos:definition xml:lang="en">Pharynx-Infiltrating malignant neoplasm-Histologic type-Carcinoma of Minor Salivary Glands: Basal cell adenocarcinoma</skos:definition>
    </owl:Class>
    


    <!-- http://www.semanticweb.org/david/ontologies/2013/0/1.3.6.1.4.1.19376.1.8.2.1.2466 -->

    <owl:Class rdf:about="&pathLex;2466">
        <rdfs:subClassOf rdf:resource="&pathLex;99999"/>
        <skos:prefLabel xml:lang="en">Carcinoma of Minor Salivary Glands: Carcinoma ex pleomorphic adenoma (malignant mixed tumor)</skos:prefLabel>
        <skos:definition xml:lang="en">Pharynx-Infiltrating malignant neoplasm-Histologic type-Carcinoma of Minor Salivary Glands: Carcinoma ex pleomorphic adenoma (malignant mixed tumor)</skos:definition>
    </owl:Class>
    


    <!-- http://www.semanticweb.org/david/ontologies/2013/0/1.3.6.1.4.1.19376.1.8.2.1.2467 -->

    <owl:Class rdf:about="&pathLex;2467">
        <rdfs:subClassOf rdf:resource="&pathLex;99999"/>
        <skos:prefLabel xml:lang="en">Carcinoma of Minor Salivary Glands: Carcinoma, type cannot be determinedd</skos:prefLabel>
        <skos:definition xml:lang="en">Pharynx-Infiltrating malignant neoplasm-Histologic type-Carcinoma of Minor Salivary Glands: Carcinoma, type cannot be determinedd</skos:definition>
    </owl:Class>
    


    <!-- http://www.semanticweb.org/david/ontologies/2013/0/1.3.6.1.4.1.19376.1.8.2.1.2468 -->

    <owl:Class rdf:about="&pathLex;2468">
        <rdfs:subClassOf rdf:resource="&pathLex;99999"/>
        <skos:prefLabel xml:lang="en">Carcinoma of Minor Salivary Glands: Clear cell adenocarcinoma</skos:prefLabel>
        <skos:definition xml:lang="en">Pharynx-Infiltrating malignant neoplasm-Histologic type-Carcinoma of Minor Salivary Glands: Clear cell adenocarcinoma</skos:definition>
    </owl:Class>
    


    <!-- http://www.semanticweb.org/david/ontologies/2013/0/1.3.6.1.4.1.19376.1.8.2.1.2469 -->

    <owl:Class rdf:about="&pathLex;2469">
        <rdfs:subClassOf rdf:resource="&pathLex;99999"/>
        <skos:prefLabel xml:lang="en">Carcinoma of Minor Salivary Glands: Cystadenocarcinoma</skos:prefLabel>
        <skos:definition xml:lang="en">Pharynx-Infiltrating malignant neoplasm-Histologic type-Carcinoma of Minor Salivary Glands: Cystadenocarcinoma</skos:definition>
    </owl:Class>
    


    <!-- http://www.semanticweb.org/david/ontologies/2013/0/1.3.6.1.4.1.19376.1.8.2.1.247 -->

    <owl:Class rdf:about="&pathLex;247">
        <rdfs:subClassOf rdf:resource="&pathLex;99999"/>
        <skos:definition xml:lang="en">Larynx-Infiltrating malignant neoplasm-Specimen size, largest dimension</skos:definition>
        <skos:prefLabel xml:lang="en">Specimen size, largest dimension</skos:prefLabel>
    </owl:Class>
    


    <!-- http://www.semanticweb.org/david/ontologies/2013/0/1.3.6.1.4.1.19376.1.8.2.1.2470 -->

    <owl:Class rdf:about="&pathLex;2470">
        <rdfs:subClassOf rdf:resource="&pathLex;99999"/>
        <skos:prefLabel xml:lang="en">Carcinoma of Minor Salivary Glands: Epithelial-myoepithelial carcinoma</skos:prefLabel>
        <skos:definition xml:lang="en">Pharynx-Infiltrating malignant neoplasm-Histologic type-Carcinoma of Minor Salivary Glands: Epithelial-myoepithelial carcinoma</skos:definition>
    </owl:Class>
    


    <!-- http://www.semanticweb.org/david/ontologies/2013/0/1.3.6.1.4.1.19376.1.8.2.1.2471 -->

    <owl:Class rdf:about="&pathLex;2471">
        <rdfs:subClassOf rdf:resource="&pathLex;99999"/>
        <skos:prefLabel xml:lang="en">Carcinoma of Minor Salivary Glands: Mucoepidermoid carcinoma</skos:prefLabel>
        <skos:definition xml:lang="en">Pharynx-Infiltrating malignant neoplasm-Histologic type-Carcinoma of Minor Salivary Glands: Mucoepidermoid carcinoma</skos:definition>
    </owl:Class>
    


    <!-- http://www.semanticweb.org/david/ontologies/2013/0/1.3.6.1.4.1.19376.1.8.2.1.2472 -->

    <owl:Class rdf:about="&pathLex;2472">
        <rdfs:subClassOf rdf:resource="&pathLex;99999"/>
        <skos:prefLabel xml:lang="en">Carcinoma of Minor Salivary Glands: Mucinous adenocarcinoma (colloid carcinoma)</skos:prefLabel>
        <skos:definition xml:lang="en">Pharynx-Infiltrating malignant neoplasm-Histologic type-Carcinoma of Minor Salivary Glands: Mucinous adenocarcinoma (colloid carcinoma)</skos:definition>
    </owl:Class>
    


    <!-- http://www.semanticweb.org/david/ontologies/2013/0/1.3.6.1.4.1.19376.1.8.2.1.2473 -->

    <owl:Class rdf:about="&pathLex;2473">
        <rdfs:subClassOf rdf:resource="&pathLex;99999"/>
        <skos:prefLabel xml:lang="en">Carcinoma of Minor Salivary Glands: Myoepithelial carcinoma (malignant myoepithelioma)</skos:prefLabel>
        <skos:definition xml:lang="en">Pharynx-Infiltrating malignant neoplasm-Histologic type-Carcinoma of Minor Salivary Glands: Myoepithelial carcinoma (malignant myoepithelioma)</skos:definition>
    </owl:Class>
    


    <!-- http://www.semanticweb.org/david/ontologies/2013/0/1.3.6.1.4.1.19376.1.8.2.1.2474 -->

    <owl:Class rdf:about="&pathLex;2474">
        <rdfs:subClassOf rdf:resource="&pathLex;99999"/>
        <skos:prefLabel xml:lang="en">Carcinoma of Minor Salivary Glands: Oncocytic carcinoma</skos:prefLabel>
        <skos:definition xml:lang="en">Pharynx-Infiltrating malignant neoplasm-Histologic type-Carcinoma of Minor Salivary Glands: Oncocytic carcinoma</skos:definition>
    </owl:Class>
    


    <!-- http://www.semanticweb.org/david/ontologies/2013/0/1.3.6.1.4.1.19376.1.8.2.1.2475 -->

    <owl:Class rdf:about="&pathLex;2475">
        <rdfs:subClassOf rdf:resource="&pathLex;99999"/>
        <skos:prefLabel xml:lang="en">Carcinoma of Minor Salivary Glands: Polymorphous low-grade adenocarcinoma</skos:prefLabel>
        <skos:definition xml:lang="en">Pharynx-Infiltrating malignant neoplasm-Histologic type-Carcinoma of Minor Salivary Glands: Polymorphous low-grade adenocarcinoma</skos:definition>
    </owl:Class>
    


    <!-- http://www.semanticweb.org/david/ontologies/2013/0/1.3.6.1.4.1.19376.1.8.2.1.2476 -->

    <owl:Class rdf:about="&pathLex;2476">
        <rdfs:subClassOf rdf:resource="&pathLex;99999"/>
        <skos:prefLabel xml:lang="en">Carcinoma of Minor Salivary Glands: Salivary duct carcinoma</skos:prefLabel>
        <skos:definition xml:lang="en">Pharynx-Infiltrating malignant neoplasm-Histologic type-Carcinoma of Minor Salivary Glands: Salivary duct carcinoma</skos:definition>
    </owl:Class>
    


    <!-- http://www.semanticweb.org/david/ontologies/2013/0/1.3.6.1.4.1.19376.1.8.2.1.2477 -->

    <owl:Class rdf:about="&pathLex;2477">
        <rdfs:subClassOf rdf:resource="&pathLex;99999"/>
        <skos:prefLabel xml:lang="en">Carcinoma of Minor Salivary Glands: Other</skos:prefLabel>
        <skos:definition xml:lang="en">Pharynx-Infiltrating malignant neoplasm-Histologic type-Carcinoma of Minor Salivary Glands: Other</skos:definition>
    </owl:Class>
    


    <!-- http://www.semanticweb.org/david/ontologies/2013/0/1.3.6.1.4.1.19376.1.8.2.1.2478 -->

    <owl:Class rdf:about="&pathLex;2478">
        <rdfs:subClassOf rdf:resource="&pathLex;99999"/>
        <skos:prefLabel xml:lang="en">Neuroendocrine Carcinoma: Typical carcinoid tumor (well differentiated neuroendocrine carcinoma)</skos:prefLabel>
        <skos:definition xml:lang="en">Pharynx-Infiltrating malignant neoplasm-Histologic type-Neuroendocrine Carcinoma: Typical carcinoid tumor (well differentiated neuroendocrine carcinoma)</skos:definition>
    </owl:Class>
    


    <!-- http://www.semanticweb.org/david/ontologies/2013/0/1.3.6.1.4.1.19376.1.8.2.1.2479 -->

    <owl:Class rdf:about="&pathLex;2479">
        <rdfs:subClassOf rdf:resource="&pathLex;99999"/>
        <skos:prefLabel xml:lang="en">Neuroendocrine Carcinoma: Atypical carcinoid tumor (moderately differentiated neuroendocrine carcinoma)</skos:prefLabel>
        <skos:definition xml:lang="en">Pharynx-Infiltrating malignant neoplasm-Histologic type-Neuroendocrine Carcinoma: Atypical carcinoid tumor (moderately differentiated neuroendocrine carcinoma)</skos:definition>
    </owl:Class>
    


    <!-- http://www.semanticweb.org/david/ontologies/2013/0/1.3.6.1.4.1.19376.1.8.2.1.248 -->

    <owl:Class rdf:about="&pathLex;248">
        <rdfs:subClassOf rdf:resource="&pathLex;99999"/>
        <skos:prefLabel xml:lang="en">Histologic type</skos:prefLabel>
        <skos:definition xml:lang="en">Larynx-Infiltrating malignant neoplasm-Histologic type</skos:definition>
    </owl:Class>
    


    <!-- http://www.semanticweb.org/david/ontologies/2013/0/1.3.6.1.4.1.19376.1.8.2.1.2480 -->

    <owl:Class rdf:about="&pathLex;2480">
        <rdfs:subClassOf rdf:resource="&pathLex;99999"/>
        <skos:prefLabel xml:lang="en">Neuroendocrine Carcinoma: Small cell carcinoma (poorly differentiated neuroendocrine carcinoma)</skos:prefLabel>
        <skos:definition xml:lang="en">Pharynx-Infiltrating malignant neoplasm-Histologic type-Neuroendocrine Carcinoma: Small cell carcinoma (poorly differentiated neuroendocrine carcinoma)</skos:definition>
    </owl:Class>
    


    <!-- http://www.semanticweb.org/david/ontologies/2013/0/1.3.6.1.4.1.19376.1.8.2.1.2481 -->

    <owl:Class rdf:about="&pathLex;2481">
        <rdfs:subClassOf rdf:resource="&pathLex;99999"/>
        <skos:prefLabel xml:lang="en">Neuroendocrine Carcinoma: Combined (or composite) small cell carcinoma, neuroendocrine type</skos:prefLabel>
        <skos:definition xml:lang="en">Pharynx-Infiltrating malignant neoplasm-Histologic type-Neuroendocrine Carcinoma: Combined (or composite) small cell carcinoma, neuroendocrine type</skos:definition>
    </owl:Class>
    


    <!-- http://www.semanticweb.org/david/ontologies/2013/0/1.3.6.1.4.1.19376.1.8.2.1.2482 -->

    <owl:Class rdf:about="&pathLex;2482">
        <rdfs:subClassOf rdf:resource="&pathLex;99999"/>
        <skos:prefLabel xml:lang="en">Mucosal malignant melanoma</skos:prefLabel>
        <skos:definition xml:lang="en">Pharynx-Infiltrating malignant neoplasm-Histologic type-Mucosal malignant melanoma</skos:definition>
    </owl:Class>
    


    <!-- http://www.semanticweb.org/david/ontologies/2013/0/1.3.6.1.4.1.19376.1.8.2.1.2483 -->

    <owl:Class rdf:about="&pathLex;2483">
        <rdfs:subClassOf rdf:resource="&pathLex;99999"/>
        <skos:prefLabel xml:lang="en">Other carcinoma (specify)</skos:prefLabel>
        <skos:definition xml:lang="en">Pharynx-Infiltrating malignant neoplasm-Histologic type-Other carcinoma (specify)</skos:definition>
    </owl:Class>
    


    <!-- http://www.semanticweb.org/david/ontologies/2013/0/1.3.6.1.4.1.19376.1.8.2.1.2484 -->

    <owl:Class rdf:about="&pathLex;2484">
        <rdfs:subClassOf rdf:resource="&pathLex;99999"/>
        <skos:prefLabel xml:lang="en">Carcinoma, type cannot be determinedd</skos:prefLabel>
        <skos:definition xml:lang="en">Pharynx-Infiltrating malignant neoplasm-Histologic type-Carcinoma, type cannot be determinedd</skos:definition>
    </owl:Class>
    


    <!-- http://www.semanticweb.org/david/ontologies/2013/0/1.3.6.1.4.1.19376.1.8.2.1.2485 -->

    <owl:Class rdf:about="&pathLex;2485">
        <rdfs:subClassOf rdf:resource="&pathLex;99999"/>
        <skos:prefLabel xml:lang="en">Mild Keratinizing dysplasia</skos:prefLabel>
        <skos:definition xml:lang="en">Pharynx-Lesion-Histologic type-Mild Keratinizing dysplasia</skos:definition>
    </owl:Class>
    


    <!-- http://www.semanticweb.org/david/ontologies/2013/0/1.3.6.1.4.1.19376.1.8.2.1.2486 -->

    <owl:Class rdf:about="&pathLex;2486">
        <rdfs:subClassOf rdf:resource="&pathLex;99999"/>
        <skos:prefLabel xml:lang="en">Moderate Keratinizing dysplasia</skos:prefLabel>
        <skos:definition xml:lang="en">Pharynx-Lesion-Histologic type-Moderate Keratinizing dysplasia</skos:definition>
    </owl:Class>
    


    <!-- http://www.semanticweb.org/david/ontologies/2013/0/1.3.6.1.4.1.19376.1.8.2.1.2487 -->

    <owl:Class rdf:about="&pathLex;2487">
        <rdfs:subClassOf rdf:resource="&pathLex;99999"/>
        <skos:definition xml:lang="en">Pharynx-Lesion-Histologic type-Severe Keratinizing dysplasia (carcinoma in situ)</skos:definition>
        <skos:prefLabel xml:lang="en">Severe Keratinizing dysplasia (carcinoma in situ)</skos:prefLabel>
    </owl:Class>
    


    <!-- http://www.semanticweb.org/david/ontologies/2013/0/1.3.6.1.4.1.19376.1.8.2.1.2488 -->

    <owl:Class rdf:about="&pathLex;2488">
        <rdfs:subClassOf rdf:resource="&pathLex;99999"/>
        <skos:prefLabel xml:lang="en">Mild Nonkeratinizing dysplasia</skos:prefLabel>
        <skos:definition xml:lang="en">Pharynx-Lesion-Histologic type-Mild Nonkeratinizing dysplasia</skos:definition>
    </owl:Class>
    


    <!-- http://www.semanticweb.org/david/ontologies/2013/0/1.3.6.1.4.1.19376.1.8.2.1.2489 -->

    <owl:Class rdf:about="&pathLex;2489">
        <rdfs:subClassOf rdf:resource="&pathLex;99999"/>
        <skos:prefLabel xml:lang="en">Moderate Nonkeratinizing dysplasia</skos:prefLabel>
        <skos:definition xml:lang="en">Pharynx-Lesion-Histologic type-Moderate Nonkeratinizing dysplasia</skos:definition>
    </owl:Class>
    


    <!-- http://www.semanticweb.org/david/ontologies/2013/0/1.3.6.1.4.1.19376.1.8.2.1.249 -->

    <owl:Class rdf:about="&pathLex;249">
        <rdfs:subClassOf rdf:resource="&pathLex;99999"/>
        <skos:definition xml:lang="en">Lip, oral cavity-Infiltrating malignant neoplasm-Margins involvement</skos:definition>
        <skos:prefLabel xml:lang="en">Margins involvement</skos:prefLabel>
    </owl:Class>
    


    <!-- http://www.semanticweb.org/david/ontologies/2013/0/1.3.6.1.4.1.19376.1.8.2.1.2490 -->

    <owl:Class rdf:about="&pathLex;2490">
        <rdfs:subClassOf rdf:resource="&pathLex;99999"/>
        <skos:definition xml:lang="en">Pharynx-Lesion-Histologic type-Severe Nonkeratinizing dysplasia (carcinoma in situ)</skos:definition>
        <skos:prefLabel xml:lang="en">Severe Nonkeratinizing dysplasia (carcinoma in situ)</skos:prefLabel>
    </owl:Class>
    


    <!-- http://www.semanticweb.org/david/ontologies/2013/0/1.3.6.1.4.1.19376.1.8.2.1.2491 -->

    <owl:Class rdf:about="&pathLex;2491">
        <rdfs:subClassOf rdf:resource="&pathLex;99999"/>
        <skos:prefLabel xml:lang="en">Inflammation (specify type)</skos:prefLabel>
        <skos:definition xml:lang="en">Pharynx-Lesion-Histologic type-Inflammation (specify type)</skos:definition>
    </owl:Class>
    


    <!-- http://www.semanticweb.org/david/ontologies/2013/0/1.3.6.1.4.1.19376.1.8.2.1.2492 -->

    <owl:Class rdf:about="&pathLex;2492">
        <rdfs:subClassOf rdf:resource="&pathLex;99999"/>
        <skos:definition xml:lang="en">Pharynx-Lesion-Histologic type-Squamous metaplasia</skos:definition>
        <skos:prefLabel xml:lang="en">Squamous metaplasia</skos:prefLabel>
    </owl:Class>
    


    <!-- http://www.semanticweb.org/david/ontologies/2013/0/1.3.6.1.4.1.19376.1.8.2.1.2493 -->

    <owl:Class rdf:about="&pathLex;2493">
        <rdfs:subClassOf rdf:resource="&pathLex;99999"/>
        <skos:prefLabel xml:lang="en">Epithelial hyperplasia</skos:prefLabel>
        <skos:definition xml:lang="en">Pharynx-Lesion-Histologic type-Epithelial hyperplasia</skos:definition>
    </owl:Class>
    


    <!-- http://www.semanticweb.org/david/ontologies/2013/0/1.3.6.1.4.1.19376.1.8.2.1.2494 -->

    <owl:Class rdf:about="&pathLex;2494">
        <rdfs:subClassOf rdf:resource="&pathLex;99999"/>
        <skos:prefLabel xml:lang="en">Fungal Colonization</skos:prefLabel>
        <skos:definition xml:lang="en">Pharynx-Lesion-Histologic type-Fungal Colonization</skos:definition>
    </owl:Class>
    


    <!-- http://www.semanticweb.org/david/ontologies/2013/0/1.3.6.1.4.1.19376.1.8.2.1.2495 -->

    <owl:Class rdf:about="&pathLex;2495">
        <rdfs:subClassOf rdf:resource="&pathLex;99999"/>
        <skos:prefLabel xml:lang="en">Bacterial Colonization</skos:prefLabel>
        <skos:definition xml:lang="en">Pharynx-Lesion-Histologic type-Bacterial Colonization</skos:definition>
    </owl:Class>
    


    <!-- http://www.semanticweb.org/david/ontologies/2013/0/1.3.6.1.4.1.19376.1.8.2.1.2496 -->

    <owl:Class rdf:about="&pathLex;2496">
        <rdfs:subClassOf rdf:resource="&pathLex;99999"/>
        <skos:prefLabel xml:lang="en">Carcinoma, type cannot be determinedd</skos:prefLabel>
        <skos:definition xml:lang="en">Lung-Infiltrating malignant neoplasm-Histologic type-Carcinoma, type cannot be determinedd</skos:definition>
    </owl:Class>
    


    <!-- http://www.semanticweb.org/david/ontologies/2013/0/1.3.6.1.4.1.19376.1.8.2.1.2497 -->

    <owl:Class rdf:about="&pathLex;2497">
        <rdfs:subClassOf rdf:resource="&pathLex;99999"/>
        <skos:definition xml:lang="en">Lung-Infiltrating malignant neoplasm-Histologic type-Non-small cell carcinoma, subtype cannot be determined</skos:definition>
        <skos:prefLabel xml:lang="en">Non-small cell carcinoma, subtype cannot be determined</skos:prefLabel>
    </owl:Class>
    


    <!-- http://www.semanticweb.org/david/ontologies/2013/0/1.3.6.1.4.1.19376.1.8.2.1.2498 -->

    <owl:Class rdf:about="&pathLex;2498">
        <rdfs:subClassOf rdf:resource="&pathLex;99999"/>
        <skos:prefLabel xml:lang="en">Combined small cell carcinoma (small cell carcinoma and non-small cell component)</skos:prefLabel>
        <skos:definition xml:lang="en">Lung-Infiltrating malignant neoplasm-Histologic type-Combined small cell carcinoma (small cell carcinoma and non-small cell component)</skos:definition>
    </owl:Class>
    


    <!-- http://www.semanticweb.org/david/ontologies/2013/0/1.3.6.1.4.1.19376.1.8.2.1.2499 -->

    <owl:Class rdf:about="&pathLex;2499">
        <rdfs:subClassOf rdf:resource="&pathLex;99999"/>
        <skos:definition xml:lang="en">Lung-Infiltrating malignant neoplasm-Histologic type-Squamous cell carcinoma</skos:definition>
        <skos:prefLabel xml:lang="en">Squamous cell carcinoma</skos:prefLabel>
    </owl:Class>
    


    <!-- http://www.semanticweb.org/david/ontologies/2013/0/1.3.6.1.4.1.19376.1.8.2.1.250 -->

    <owl:Class rdf:about="&pathLex;250">
        <rdfs:subClassOf rdf:resource="&pathLex;99999"/>
        <skos:definition xml:lang="en">Lip, oral cavity-Infiltrating malignant neoplasm-Margins involvement</skos:definition>
        <skos:prefLabel xml:lang="en">Margins involvement</skos:prefLabel>
    </owl:Class>
    


    <!-- http://www.semanticweb.org/david/ontologies/2013/0/1.3.6.1.4.1.19376.1.8.2.1.2500 -->

    <owl:Class rdf:about="&pathLex;2500">
        <rdfs:subClassOf rdf:resource="&pathLex;99999"/>
        <skos:definition xml:lang="en">Lung-Infiltrating malignant neoplasm-Histologic type-Squamous cell carcinoma, papillary variant</skos:definition>
        <skos:prefLabel xml:lang="en">Squamous cell carcinoma, papillary variant</skos:prefLabel>
    </owl:Class>
    


    <!-- http://www.semanticweb.org/david/ontologies/2013/0/1.3.6.1.4.1.19376.1.8.2.1.2501 -->

    <owl:Class rdf:about="&pathLex;2501">
        <rdfs:subClassOf rdf:resource="&pathLex;99999"/>
        <skos:definition xml:lang="en">Lung-Infiltrating malignant neoplasm-Histologic type-Squamous cell carcinoma, clear cell variant</skos:definition>
        <skos:prefLabel xml:lang="en">Squamous cell carcinoma, clear cell variant</skos:prefLabel>
    </owl:Class>
    


    <!-- http://www.semanticweb.org/david/ontologies/2013/0/1.3.6.1.4.1.19376.1.8.2.1.2502 -->

    <owl:Class rdf:about="&pathLex;2502">
        <rdfs:subClassOf rdf:resource="&pathLex;99999"/>
        <skos:definition xml:lang="en">Lung-Infiltrating malignant neoplasm-Histologic type-Squamous cell carcinoma, small cell variant</skos:definition>
        <skos:prefLabel xml:lang="en">Squamous cell carcinoma, small cell variant</skos:prefLabel>
    </owl:Class>
    


    <!-- http://www.semanticweb.org/david/ontologies/2013/0/1.3.6.1.4.1.19376.1.8.2.1.2503 -->

    <owl:Class rdf:about="&pathLex;2503">
        <rdfs:subClassOf rdf:resource="&pathLex;99999"/>
        <skos:definition xml:lang="en">Lung-Infiltrating malignant neoplasm-Histologic type-Squamous cell carcinoma, basaloid variant</skos:definition>
        <skos:prefLabel xml:lang="en">Squamous cell carcinoma, basaloid variant</skos:prefLabel>
    </owl:Class>
    


    <!-- http://www.semanticweb.org/david/ontologies/2013/0/1.3.6.1.4.1.19376.1.8.2.1.2504 -->

    <owl:Class rdf:about="&pathLex;2504">
        <rdfs:subClassOf rdf:resource="&pathLex;99999"/>
        <skos:prefLabel xml:lang="en">Adenocarcinoma, mixed subtype</skos:prefLabel>
        <skos:definition xml:lang="en">Lung-Infiltrating malignant neoplasm-Histologic type-Adenocarcinoma, mixed subtype</skos:definition>
    </owl:Class>
    


    <!-- http://www.semanticweb.org/david/ontologies/2013/0/1.3.6.1.4.1.19376.1.8.2.1.2505 -->

    <owl:Class rdf:about="&pathLex;2505">
        <rdfs:subClassOf rdf:resource="&pathLex;99999"/>
        <skos:prefLabel xml:lang="en">Acinar adenocarcinoma</skos:prefLabel>
        <skos:definition xml:lang="en">Lung-Infiltrating malignant neoplasm-Histologic type-Acinar adenocarcinoma</skos:definition>
    </owl:Class>
    


    <!-- http://www.semanticweb.org/david/ontologies/2013/0/1.3.6.1.4.1.19376.1.8.2.1.2506 -->

    <owl:Class rdf:about="&pathLex;2506">
        <rdfs:subClassOf rdf:resource="&pathLex;99999"/>
        <skos:definition xml:lang="en">Lung-Infiltrating malignant neoplasm-Histologic type-Papillary adenocarcinoma</skos:definition>
        <skos:prefLabel xml:lang="en">Papillary adenocarcinoma</skos:prefLabel>
    </owl:Class>
    


    <!-- http://www.semanticweb.org/david/ontologies/2013/0/1.3.6.1.4.1.19376.1.8.2.1.2507 -->

    <owl:Class rdf:about="&pathLex;2507">
        <rdfs:subClassOf rdf:resource="&pathLex;99999"/>
        <skos:prefLabel xml:lang="en">Bronchioloalveolar carcinoma</skos:prefLabel>
        <skos:definition xml:lang="en">Lung-Infiltrating malignant neoplasm-Histologic type-Bronchioloalveolar carcinoma</skos:definition>
    </owl:Class>
    


    <!-- http://www.semanticweb.org/david/ontologies/2013/0/1.3.6.1.4.1.19376.1.8.2.1.2508 -->

    <owl:Class rdf:about="&pathLex;2508">
        <rdfs:subClassOf rdf:resource="&pathLex;99999"/>
        <skos:prefLabel xml:lang="en">Bronchioloalveolar carcinoma, nonmucinous</skos:prefLabel>
        <skos:definition xml:lang="en">Lung-Infiltrating malignant neoplasm-Histologic type-Bronchioloalveolar carcinoma, nonmucinous</skos:definition>
    </owl:Class>
    


    <!-- http://www.semanticweb.org/david/ontologies/2013/0/1.3.6.1.4.1.19376.1.8.2.1.2509 -->

    <owl:Class rdf:about="&pathLex;2509">
        <rdfs:subClassOf rdf:resource="&pathLex;99999"/>
        <skos:prefLabel xml:lang="en">Bronchioloalveolar carcinoma, mucinous</skos:prefLabel>
        <skos:definition xml:lang="en">Lung-Infiltrating malignant neoplasm-Histologic type-Bronchioloalveolar carcinoma, mucinous</skos:definition>
    </owl:Class>
    


    <!-- http://www.semanticweb.org/david/ontologies/2013/0/1.3.6.1.4.1.19376.1.8.2.1.251 -->

    <owl:Class rdf:about="&pathLex;251">
        <rdfs:subClassOf rdf:resource="&pathLex;99999"/>
        <skos:definition xml:lang="en">Lip, oral cavity-Infiltrating malignant neoplasm-Margins involvement</skos:definition>
        <skos:prefLabel xml:lang="en">Margins involvement</skos:prefLabel>
    </owl:Class>
    


    <!-- http://www.semanticweb.org/david/ontologies/2013/0/1.3.6.1.4.1.19376.1.8.2.1.2510 -->

    <owl:Class rdf:about="&pathLex;2510">
        <rdfs:subClassOf rdf:resource="&pathLex;99999"/>
        <skos:prefLabel xml:lang="en">Bronchioloalveolar carcinoma, mixed nonmucinous and mucinous</skos:prefLabel>
        <skos:definition xml:lang="en">Lung-Infiltrating malignant neoplasm-Histologic type-Bronchioloalveolar carcinoma, mixed nonmucinous and mucinous</skos:definition>
    </owl:Class>
    


    <!-- http://www.semanticweb.org/david/ontologies/2013/0/1.3.6.1.4.1.19376.1.8.2.1.2511 -->

    <owl:Class rdf:about="&pathLex;2511">
        <rdfs:subClassOf rdf:resource="&pathLex;99999"/>
        <skos:definition xml:lang="en">Lung-Infiltrating malignant neoplasm-Histologic type-Solid adenocarcinoma</skos:definition>
        <skos:prefLabel xml:lang="en">Solid adenocarcinoma</skos:prefLabel>
    </owl:Class>
    


    <!-- http://www.semanticweb.org/david/ontologies/2013/0/1.3.6.1.4.1.19376.1.8.2.1.2512 -->

    <owl:Class rdf:about="&pathLex;2512">
        <rdfs:subClassOf rdf:resource="&pathLex;99999"/>
        <skos:prefLabel xml:lang="en">Fetal adenocarcinoma</skos:prefLabel>
        <skos:definition xml:lang="en">Lung-Infiltrating malignant neoplasm-Histologic type-Fetal adenocarcinoma</skos:definition>
    </owl:Class>
    


    <!-- http://www.semanticweb.org/david/ontologies/2013/0/1.3.6.1.4.1.19376.1.8.2.1.2513 -->

    <owl:Class rdf:about="&pathLex;2513">
        <rdfs:subClassOf rdf:resource="&pathLex;99999"/>
        <skos:definition xml:lang="en">Lung-Infiltrating malignant neoplasm-Histologic type-Mucinous (colloid) adenocarcinoma</skos:definition>
        <skos:prefLabel xml:lang="en">Mucinous (colloid) adenocarcinoma</skos:prefLabel>
    </owl:Class>
    


    <!-- http://www.semanticweb.org/david/ontologies/2013/0/1.3.6.1.4.1.19376.1.8.2.1.2514 -->

    <owl:Class rdf:about="&pathLex;2514">
        <rdfs:subClassOf rdf:resource="&pathLex;99999"/>
        <skos:definition xml:lang="en">Lung-Infiltrating malignant neoplasm-Histologic type-Mucinous cystadenocarcinoma</skos:definition>
        <skos:prefLabel xml:lang="en">Mucinous cystadenocarcinoma</skos:prefLabel>
    </owl:Class>
    


    <!-- http://www.semanticweb.org/david/ontologies/2013/0/1.3.6.1.4.1.19376.1.8.2.1.2515 -->

    <owl:Class rdf:about="&pathLex;2515">
        <rdfs:subClassOf rdf:resource="&pathLex;99999"/>
        <skos:definition xml:lang="en">Lung-Infiltrating malignant neoplasm-Histologic type-Signet ring adenocarcinoma</skos:definition>
        <skos:prefLabel xml:lang="en">Signet ring adenocarcinoma</skos:prefLabel>
    </owl:Class>
    


    <!-- http://www.semanticweb.org/david/ontologies/2013/0/1.3.6.1.4.1.19376.1.8.2.1.2516 -->

    <owl:Class rdf:about="&pathLex;2516">
        <rdfs:subClassOf rdf:resource="&pathLex;99999"/>
        <skos:prefLabel xml:lang="en">Clear cell adenocarcinoma</skos:prefLabel>
        <skos:definition xml:lang="en">Lung-Infiltrating malignant neoplasm-Histologic type-Clear cell adenocarcinoma</skos:definition>
    </owl:Class>
    


    <!-- http://www.semanticweb.org/david/ontologies/2013/0/1.3.6.1.4.1.19376.1.8.2.1.2517 -->

    <owl:Class rdf:about="&pathLex;2517">
        <rdfs:subClassOf rdf:resource="&pathLex;99999"/>
        <skos:prefLabel xml:lang="en">Large cell neuroendocrine carcinoma</skos:prefLabel>
        <skos:definition xml:lang="en">Lung-Infiltrating malignant neoplasm-Histologic type-Large cell neuroendocrine carcinoma</skos:definition>
    </owl:Class>
    


    <!-- http://www.semanticweb.org/david/ontologies/2013/0/1.3.6.1.4.1.19376.1.8.2.1.2518 -->

    <owl:Class rdf:about="&pathLex;2518">
        <rdfs:subClassOf rdf:resource="&pathLex;99999"/>
        <skos:prefLabel xml:lang="en">Combined large cell neuroendocrine carcinoma (specify type of other non-small cell carcinoma component)</skos:prefLabel>
        <skos:definition xml:lang="en">Lung-Infiltrating malignant neoplasm-Histologic type-Combined large cell neuroendocrine carcinoma (specify type of other non-small cell carcinoma component)</skos:definition>
    </owl:Class>
    


    <!-- http://www.semanticweb.org/david/ontologies/2013/0/1.3.6.1.4.1.19376.1.8.2.1.2519 -->

    <owl:Class rdf:about="&pathLex;2519">
        <rdfs:subClassOf rdf:resource="&pathLex;99999"/>
        <skos:prefLabel xml:lang="en">Basaloid carcinoma</skos:prefLabel>
        <skos:definition xml:lang="en">Lung-Infiltrating malignant neoplasm-Histologic type-Basaloid carcinoma</skos:definition>
    </owl:Class>
    


    <!-- http://www.semanticweb.org/david/ontologies/2013/0/1.3.6.1.4.1.19376.1.8.2.1.252 -->

    <owl:Class rdf:about="&pathLex;252">
        <rdfs:subClassOf rdf:resource="&pathLex;99999"/>
        <skos:prefLabel xml:lang="en">Distance of lesion from closest uninvolved margin</skos:prefLabel>
        <skos:definition xml:lang="en">Lip, oral cavity-Infiltrating malignant neoplasm-Distance of lesion from closest uninvolved margin</skos:definition>
    </owl:Class>
    


    <!-- http://www.semanticweb.org/david/ontologies/2013/0/1.3.6.1.4.1.19376.1.8.2.1.2520 -->

    <owl:Class rdf:about="&pathLex;2520">
        <rdfs:subClassOf rdf:resource="&pathLex;99999"/>
        <skos:definition xml:lang="en">Lung-Infiltrating malignant neoplasm-Histologic type-Lymphoepithelioma-like carcinoma</skos:definition>
        <skos:prefLabel xml:lang="en">Lymphoepithelioma-like carcinoma</skos:prefLabel>
    </owl:Class>
    


    <!-- http://www.semanticweb.org/david/ontologies/2013/0/1.3.6.1.4.1.19376.1.8.2.1.2521 -->

    <owl:Class rdf:about="&pathLex;2521">
        <rdfs:subClassOf rdf:resource="&pathLex;99999"/>
        <skos:prefLabel xml:lang="en">Clear cell carcinoma</skos:prefLabel>
        <skos:definition xml:lang="en">Lung-Infiltrating malignant neoplasm-Histologic type-Clear cell carcinoma</skos:definition>
    </owl:Class>
    


    <!-- http://www.semanticweb.org/david/ontologies/2013/0/1.3.6.1.4.1.19376.1.8.2.1.2522 -->

    <owl:Class rdf:about="&pathLex;2522">
        <rdfs:subClassOf rdf:resource="&pathLex;99999"/>
        <skos:prefLabel xml:lang="en">Large cell carcinoma with rhabdoid phenotype</skos:prefLabel>
        <skos:definition xml:lang="en">Lung-Infiltrating malignant neoplasm-Histologic type-Large cell carcinoma with rhabdoid phenotype</skos:definition>
    </owl:Class>
    


    <!-- http://www.semanticweb.org/david/ontologies/2013/0/1.3.6.1.4.1.19376.1.8.2.1.2523 -->

    <owl:Class rdf:about="&pathLex;2523">
        <rdfs:subClassOf rdf:resource="&pathLex;99999"/>
        <skos:definition xml:lang="en">Lung-Infiltrating malignant neoplasm-Histologic type-Pleomorphic carcinoma</skos:definition>
        <skos:prefLabel xml:lang="en">Pleomorphic carcinoma</skos:prefLabel>
    </owl:Class>
    


    <!-- http://www.semanticweb.org/david/ontologies/2013/0/1.3.6.1.4.1.19376.1.8.2.1.2524 -->

    <owl:Class rdf:about="&pathLex;2524">
        <rdfs:subClassOf rdf:resource="&pathLex;99999"/>
        <skos:definition xml:lang="en">Lung-Infiltrating malignant neoplasm-Histologic type-Spindle cell carcinoma</skos:definition>
        <skos:prefLabel xml:lang="en">Spindle cell carcinoma</skos:prefLabel>
    </owl:Class>
    


    <!-- http://www.semanticweb.org/david/ontologies/2013/0/1.3.6.1.4.1.19376.1.8.2.1.2525 -->

    <owl:Class rdf:about="&pathLex;2525">
        <rdfs:subClassOf rdf:resource="&pathLex;99999"/>
        <skos:prefLabel xml:lang="en">Giant cell carcinoma</skos:prefLabel>
        <skos:definition xml:lang="en">Lung-Infiltrating malignant neoplasm-Histologic type-Giant cell carcinoma</skos:definition>
    </owl:Class>
    


    <!-- http://www.semanticweb.org/david/ontologies/2013/0/1.3.6.1.4.1.19376.1.8.2.1.2526 -->

    <owl:Class rdf:about="&pathLex;2526">
        <rdfs:subClassOf rdf:resource="&pathLex;99999"/>
        <skos:prefLabel xml:lang="en">Carcinosarcoma</skos:prefLabel>
        <skos:definition xml:lang="en">Lung-Infiltrating malignant neoplasm-Histologic type-Carcinosarcoma</skos:definition>
    </owl:Class>
    


    <!-- http://www.semanticweb.org/david/ontologies/2013/0/1.3.6.1.4.1.19376.1.8.2.1.2527 -->

    <owl:Class rdf:about="&pathLex;2527">
        <rdfs:subClassOf rdf:resource="&pathLex;99999"/>
        <skos:definition xml:lang="en">Lung-Infiltrating malignant neoplasm-Histologic type-Pulmonary blastoma</skos:definition>
        <skos:prefLabel xml:lang="en">Pulmonary blastoma</skos:prefLabel>
    </owl:Class>
    


    <!-- http://www.semanticweb.org/david/ontologies/2013/0/1.3.6.1.4.1.19376.1.8.2.1.2528 -->

    <owl:Class rdf:about="&pathLex;2528">
        <rdfs:subClassOf rdf:resource="&pathLex;99999"/>
        <skos:prefLabel xml:lang="en">Atypical carcinoid tumor</skos:prefLabel>
        <skos:definition xml:lang="en">Lung-Infiltrating malignant neoplasm-Histologic type-Atypical carcinoid tumor</skos:definition>
    </owl:Class>
    


    <!-- http://www.semanticweb.org/david/ontologies/2013/0/1.3.6.1.4.1.19376.1.8.2.1.2529 -->

    <owl:Class rdf:about="&pathLex;2529">
        <rdfs:subClassOf rdf:resource="&pathLex;99999"/>
        <skos:definition xml:lang="en">Lung-Infiltrating malignant neoplasm-Histologic type-Mucoepidermoid carcinoma</skos:definition>
        <skos:prefLabel xml:lang="en">Mucoepidermoid carcinoma</skos:prefLabel>
    </owl:Class>
    


    <!-- http://www.semanticweb.org/david/ontologies/2013/0/1.3.6.1.4.1.19376.1.8.2.1.253 -->

    <owl:Class rdf:about="&pathLex;253">
        <rdfs:subClassOf rdf:resource="&pathLex;99999"/>
        <skos:prefLabel xml:lang="en">Distance of lesion from closest uninvolved margin</skos:prefLabel>
        <skos:definition xml:lang="en">Lip, oral cavity-Infiltrating malignant neoplasm-Distance of lesion from closest uninvolved margin</skos:definition>
    </owl:Class>
    


    <!-- http://www.semanticweb.org/david/ontologies/2013/0/1.3.6.1.4.1.19376.1.8.2.1.2530 -->

    <owl:Class rdf:about="&pathLex;2530">
        <rdfs:subClassOf rdf:resource="&pathLex;99999"/>
        <skos:prefLabel xml:lang="en">Adenoid cystic carcinoma</skos:prefLabel>
        <skos:definition xml:lang="en">Lung-Infiltrating malignant neoplasm-Histologic type-Adenoid cystic carcinoma</skos:definition>
    </owl:Class>
    


    <!-- http://www.semanticweb.org/david/ontologies/2013/0/1.3.6.1.4.1.19376.1.8.2.1.2531 -->

    <owl:Class rdf:about="&pathLex;2531">
        <rdfs:subClassOf rdf:resource="&pathLex;99999"/>
        <skos:prefLabel xml:lang="en">Epithelial-myoepithelial carcinoma</skos:prefLabel>
        <skos:definition xml:lang="en">Lung-Infiltrating malignant neoplasm-Histologic type-Epithelial-myoepithelial carcinoma</skos:definition>
    </owl:Class>
    


    <!-- http://www.semanticweb.org/david/ontologies/2013/0/1.3.6.1.4.1.19376.1.8.2.1.2532 -->

    <owl:Class rdf:about="&pathLex;2532">
        <rdfs:subClassOf rdf:resource="&pathLex;99999"/>
        <skos:prefLabel xml:lang="en">Atelectasis Extends to the hilar region but does not involve entire lung</skos:prefLabel>
        <skos:definition xml:lang="en">Lung-Lesion-Histologic type-Atelectasis Extends to the hilar region but does not involve entire lung</skos:definition>
    </owl:Class>
    


    <!-- http://www.semanticweb.org/david/ontologies/2013/0/1.3.6.1.4.1.19376.1.8.2.1.2533 -->

    <owl:Class rdf:about="&pathLex;2533">
        <rdfs:subClassOf rdf:resource="&pathLex;99999"/>
        <skos:prefLabel xml:lang="en">Atelectasis involves entire lung</skos:prefLabel>
        <skos:definition xml:lang="en">Lung-Lesion-Histologic type-Atelectasis involves entire lung</skos:definition>
    </owl:Class>
    


    <!-- http://www.semanticweb.org/david/ontologies/2013/0/1.3.6.1.4.1.19376.1.8.2.1.2534 -->

    <owl:Class rdf:about="&pathLex;2534">
        <rdfs:subClassOf rdf:resource="&pathLex;99999"/>
        <skos:definition xml:lang="en">Lung-Lesion-Histologic type-Obstructive Pneumonitis extends to the hilar region but does not involve entire lung</skos:definition>
        <skos:prefLabel xml:lang="en">Obstructive Pneumonitis extends to the hilar region but does not involve entire lung</skos:prefLabel>
    </owl:Class>
    


    <!-- http://www.semanticweb.org/david/ontologies/2013/0/1.3.6.1.4.1.19376.1.8.2.1.2535 -->

    <owl:Class rdf:about="&pathLex;2535">
        <rdfs:subClassOf rdf:resource="&pathLex;99999"/>
        <skos:definition xml:lang="en">Lung-Lesion-Histologic type-Obstructive Pneumonitis involves entire lung</skos:definition>
        <skos:prefLabel xml:lang="en">Obstructive Pneumonitis involves entire lung</skos:prefLabel>
    </owl:Class>
    


    <!-- http://www.semanticweb.org/david/ontologies/2013/0/1.3.6.1.4.1.19376.1.8.2.1.2536 -->

    <owl:Class rdf:about="&pathLex;2536">
        <rdfs:subClassOf rdf:resource="&pathLex;99999"/>
        <skos:prefLabel xml:lang="en">Atypical adenomatous hyperplasia</skos:prefLabel>
        <skos:definition xml:lang="en">Lung-Lesion-Histologic type-Atypical adenomatous hyperplasia</skos:definition>
    </owl:Class>
    


    <!-- http://www.semanticweb.org/david/ontologies/2013/0/1.3.6.1.4.1.19376.1.8.2.1.2537 -->

    <owl:Class rdf:about="&pathLex;2537">
        <rdfs:subClassOf rdf:resource="&pathLex;99999"/>
        <skos:definition xml:lang="en">Lung-Lesion-Histologic type-Squamous dysplasia</skos:definition>
        <skos:prefLabel xml:lang="en">Squamous dysplasia</skos:prefLabel>
    </owl:Class>
    


    <!-- http://www.semanticweb.org/david/ontologies/2013/0/1.3.6.1.4.1.19376.1.8.2.1.2538 -->

    <owl:Class rdf:about="&pathLex;2538">
        <rdfs:subClassOf rdf:resource="&pathLex;99999"/>
        <skos:definition xml:lang="en">Lung-Lesion-Histologic type-Metaplasia (specify)</skos:definition>
        <skos:prefLabel xml:lang="en">Metaplasia (specify)</skos:prefLabel>
    </owl:Class>
    


    <!-- http://www.semanticweb.org/david/ontologies/2013/0/1.3.6.1.4.1.19376.1.8.2.1.2539 -->

    <owl:Class rdf:about="&pathLex;2539">
        <rdfs:subClassOf rdf:resource="&pathLex;99999"/>
        <skos:prefLabel xml:lang="en">Diffuse neuroendocrine hyperplasia</skos:prefLabel>
        <skos:definition xml:lang="en">Lung-Lesion-Histologic type-Diffuse neuroendocrine hyperplasia</skos:definition>
    </owl:Class>
    


    <!-- http://www.semanticweb.org/david/ontologies/2013/0/1.3.6.1.4.1.19376.1.8.2.1.254 -->

    <owl:Class rdf:about="&pathLex;254">
        <rdfs:subClassOf rdf:resource="&pathLex;99999"/>
        <skos:definition xml:lang="en">Lip, oral cavity-Infiltrating malignant neoplasm-Lymph-vascular invasion</skos:definition>
        <skos:prefLabel xml:lang="en">Lymph-vascular invasion</skos:prefLabel>
    </owl:Class>
    


    <!-- http://www.semanticweb.org/david/ontologies/2013/0/1.3.6.1.4.1.19376.1.8.2.1.2540 -->

    <owl:Class rdf:about="&pathLex;2540">
        <rdfs:subClassOf rdf:resource="&pathLex;99999"/>
        <skos:prefLabel xml:lang="en">Inflammation</skos:prefLabel>
        <skos:definition xml:lang="en">Lung-Lesion-Histologic type-Inflammation</skos:definition>
    </owl:Class>
    


    <!-- http://www.semanticweb.org/david/ontologies/2013/0/1.3.6.1.4.1.19376.1.8.2.1.2541 -->

    <owl:Class rdf:about="&pathLex;2541">
        <rdfs:subClassOf rdf:resource="&pathLex;99999"/>
        <skos:prefLabel xml:lang="en">High-grade prostatic intraepithelial neoplasia (PIN)</skos:prefLabel>
        <skos:definition xml:lang="en">Prostate-Lesion-Histologic type-High-grade prostatic intraepithelial neoplasia (PIN)</skos:definition>
    </owl:Class>
    


    <!-- http://www.semanticweb.org/david/ontologies/2013/0/1.3.6.1.4.1.19376.1.8.2.1.2542 -->

    <owl:Class rdf:about="&pathLex;2542">
        <rdfs:subClassOf rdf:resource="&pathLex;99999"/>
        <skos:prefLabel xml:lang="en">Atypical adenomatous hyperplasia (adenosis)</skos:prefLabel>
        <skos:definition xml:lang="en">Prostate-Lesion-Histologic type-Atypical adenomatous hyperplasia (adenosis)</skos:definition>
    </owl:Class>
    


    <!-- http://www.semanticweb.org/david/ontologies/2013/0/1.3.6.1.4.1.19376.1.8.2.1.2543 -->

    <owl:Class rdf:about="&pathLex;2543">
        <rdfs:subClassOf rdf:resource="&pathLex;99999"/>
        <skos:prefLabel xml:lang="en">Nodular prostatic hyperplasia</skos:prefLabel>
        <skos:definition xml:lang="en">Prostate-Lesion-Histologic type-Nodular prostatic hyperplasia</skos:definition>
    </owl:Class>
    


    <!-- http://www.semanticweb.org/david/ontologies/2013/0/1.3.6.1.4.1.19376.1.8.2.1.2544 -->

    <owl:Class rdf:about="&pathLex;2544">
        <rdfs:subClassOf rdf:resource="&pathLex;99999"/>
        <skos:prefLabel xml:lang="en">Inflammation</skos:prefLabel>
        <skos:definition xml:lang="en">Prostate-Lesion-Histologic type-Inflammation</skos:definition>
    </owl:Class>
    


    <!-- http://www.semanticweb.org/david/ontologies/2013/0/1.3.6.1.4.1.19376.1.8.2.1.2545 -->

    <owl:Class rdf:about="&pathLex;2545">
        <rdfs:subClassOf rdf:resource="&pathLex;99999"/>
        <skos:definition xml:lang="en">Kidney-Infiltrating malignant neoplasm-Histologic type-Multilocular clear cell renal cell carcinoma</skos:definition>
        <skos:prefLabel xml:lang="en">Multilocular clear cell renal cell carcinoma</skos:prefLabel>
    </owl:Class>
    


    <!-- http://www.semanticweb.org/david/ontologies/2013/0/1.3.6.1.4.1.19376.1.8.2.1.2546 -->

    <owl:Class rdf:about="&pathLex;2546">
        <rdfs:subClassOf rdf:resource="&pathLex;99999"/>
        <skos:definition xml:lang="en">Kidney-Infiltrating malignant neoplasm-Histologic type-Papillary renal cell carcinoma</skos:definition>
        <skos:prefLabel xml:lang="en">Papillary renal cell carcinoma</skos:prefLabel>
    </owl:Class>
    


    <!-- http://www.semanticweb.org/david/ontologies/2013/0/1.3.6.1.4.1.19376.1.8.2.1.2547 -->

    <owl:Class rdf:about="&pathLex;2547">
        <rdfs:subClassOf rdf:resource="&pathLex;99999"/>
        <skos:definition xml:lang="en">Kidney-Infiltrating malignant neoplasm-Histologic type-Translocation carcinoma (Xp11 or others)</skos:definition>
        <skos:prefLabel xml:lang="en">Translocation carcinoma (Xp11 or others)</skos:prefLabel>
    </owl:Class>
    


    <!-- http://www.semanticweb.org/david/ontologies/2013/0/1.3.6.1.4.1.19376.1.8.2.1.2548 -->

    <owl:Class rdf:about="&pathLex;2548">
        <rdfs:subClassOf rdf:resource="&pathLex;99999"/>
        <skos:prefLabel xml:lang="en">Carcinoma associated with neuroblastoma</skos:prefLabel>
        <skos:definition xml:lang="en">Kidney-Infiltrating malignant neoplasm-Histologic type-Carcinoma associated with neuroblastoma</skos:definition>
    </owl:Class>
    


    <!-- http://www.semanticweb.org/david/ontologies/2013/0/1.3.6.1.4.1.19376.1.8.2.1.2549 -->

    <owl:Class rdf:about="&pathLex;2549">
        <rdfs:subClassOf rdf:resource="&pathLex;99999"/>
        <skos:definition xml:lang="en">Kidney-Infiltrating malignant neoplasm-Histologic type-Mucinous tubular and spindle cell carcinoma</skos:definition>
        <skos:prefLabel xml:lang="en">Mucinous tubular and spindle cell carcinoma</skos:prefLabel>
    </owl:Class>
    


    <!-- http://www.semanticweb.org/david/ontologies/2013/0/1.3.6.1.4.1.19376.1.8.2.1.255 -->

    <owl:Class rdf:about="&pathLex;255">
        <rdfs:subClassOf rdf:resource="&pathLex;99999"/>
        <skos:prefLabel xml:lang="en">Extent</skos:prefLabel>
        <skos:definition xml:lang="en">Lip, oral cavity-Infiltrating malignant neoplasm-Extent</skos:definition>
    </owl:Class>
    


    <!-- http://www.semanticweb.org/david/ontologies/2013/0/1.3.6.1.4.1.19376.1.8.2.1.2550 -->

    <owl:Class rdf:about="&pathLex;2550">
        <rdfs:subClassOf rdf:resource="&pathLex;99999"/>
        <skos:definition xml:lang="en">Kidney-Infiltrating malignant neoplasm-Histologic type-Tubulocystic renal cell carcinoma</skos:definition>
        <skos:prefLabel xml:lang="en">Tubulocystic renal cell carcinoma</skos:prefLabel>
    </owl:Class>
    


    <!-- http://www.semanticweb.org/david/ontologies/2013/0/1.3.6.1.4.1.19376.1.8.2.1.2551 -->

    <owl:Class rdf:about="&pathLex;2551">
        <rdfs:subClassOf rdf:resource="&pathLex;99999"/>
        <skos:definition xml:lang="en">Kidney-Infiltrating malignant neoplasm-Histologic type-Renal cell carcinoma, unclassified</skos:definition>
        <skos:prefLabel xml:lang="en">Renal cell carcinoma, unclassified</skos:prefLabel>
    </owl:Class>
    


    <!-- http://www.semanticweb.org/david/ontologies/2013/0/1.3.6.1.4.1.19376.1.8.2.1.2552 -->

    <owl:Class rdf:about="&pathLex;2552">
        <rdfs:subClassOf rdf:resource="&pathLex;99999"/>
        <skos:prefLabel xml:lang="en">Glomerular disease (specify)</skos:prefLabel>
        <skos:definition xml:lang="en">Kidney-Lesion-Histologic type-Glomerular disease (specify)</skos:definition>
    </owl:Class>
    


    <!-- http://www.semanticweb.org/david/ontologies/2013/0/1.3.6.1.4.1.19376.1.8.2.1.2553 -->

    <owl:Class rdf:about="&pathLex;2553">
        <rdfs:subClassOf rdf:resource="&pathLex;99999"/>
        <skos:definition xml:lang="en">Kidney-Lesion-Histologic type-Tubulointerstitial disease (specify)</skos:definition>
        <skos:prefLabel xml:lang="en">Tubulointerstitial disease (specify)</skos:prefLabel>
    </owl:Class>
    


    <!-- http://www.semanticweb.org/david/ontologies/2013/0/1.3.6.1.4.1.19376.1.8.2.1.2554 -->

    <owl:Class rdf:about="&pathLex;2554">
        <rdfs:subClassOf rdf:resource="&pathLex;99999"/>
        <skos:definition xml:lang="en">Kidney-Lesion-Histologic type-Vascular disease (specify)</skos:definition>
        <skos:prefLabel xml:lang="en">Vascular disease (specify)</skos:prefLabel>
    </owl:Class>
    


    <!-- http://www.semanticweb.org/david/ontologies/2013/0/1.3.6.1.4.1.19376.1.8.2.1.2555 -->

    <owl:Class rdf:about="&pathLex;2555">
        <rdfs:subClassOf rdf:resource="&pathLex;99999"/>
        <skos:prefLabel xml:lang="en">Cyst(s) (specify)</skos:prefLabel>
        <skos:definition xml:lang="en">Kidney-Lesion-Histologic type-Cyst(s) (specify)</skos:definition>
    </owl:Class>
    


    <!-- http://www.semanticweb.org/david/ontologies/2013/0/1.3.6.1.4.1.19376.1.8.2.1.2556 -->

    <owl:Class rdf:about="&pathLex;2556">
        <rdfs:subClassOf rdf:resource="&pathLex;99999"/>
        <skos:definition xml:lang="en">Kidney-Lesion-Histologic type-Tubular (papillary) adenoma(s)</skos:definition>
        <skos:prefLabel xml:lang="en">Tubular (papillary) adenoma(s)</skos:prefLabel>
    </owl:Class>
    


    <!-- http://www.semanticweb.org/david/ontologies/2013/0/1.3.6.1.4.1.19376.1.8.2.1.2557 -->

    <owl:Class rdf:about="&pathLex;2557">
        <rdfs:subClassOf rdf:resource="&pathLex;436"/>
        <skos:definition xml:lang="en">Breast-In situ neoplasm-Histologic type-DCIS Comedo</skos:definition>
        <skos:prefLabel xml:lang="en">DCIS Comedo</skos:prefLabel>
    </owl:Class>
    


    <!-- http://www.semanticweb.org/david/ontologies/2013/0/1.3.6.1.4.1.19376.1.8.2.1.2558 -->

    <owl:Class rdf:about="&pathLex;2558">
        <rdfs:subClassOf rdf:resource="&pathLex;436"/>
        <skos:definition xml:lang="en">Breast-In situ neoplasm-Histologic type-DCIS Paget disease (DCIS involving nipple skin)</skos:definition>
        <skos:prefLabel xml:lang="en">DCIS Paget disease (DCIS involving nipple skin)</skos:prefLabel>
    </owl:Class>
    


    <!-- http://www.semanticweb.org/david/ontologies/2013/0/1.3.6.1.4.1.19376.1.8.2.1.2559 -->

    <owl:Class rdf:about="&pathLex;2559">
        <rdfs:subClassOf rdf:resource="&pathLex;436"/>
        <skos:definition xml:lang="en">Breast-In situ neoplasm-Histologic type-DCIS Cribriform</skos:definition>
        <skos:prefLabel xml:lang="en">DCIS Cribriform</skos:prefLabel>
    </owl:Class>
    


    <!-- http://www.semanticweb.org/david/ontologies/2013/0/1.3.6.1.4.1.19376.1.8.2.1.256 -->

    <owl:Class rdf:about="&pathLex;256">
        <rdfs:subClassOf rdf:resource="&pathLex;99999"/>
        <skos:definition xml:lang="en">Lip, oral cavity-Infiltrating malignant neoplasm-Perineural invasion</skos:definition>
        <skos:prefLabel xml:lang="en">Perineural invasion</skos:prefLabel>
    </owl:Class>
    


    <!-- http://www.semanticweb.org/david/ontologies/2013/0/1.3.6.1.4.1.19376.1.8.2.1.2560 -->

    <owl:Class rdf:about="&pathLex;2560">
        <rdfs:subClassOf rdf:resource="&pathLex;436"/>
        <skos:definition xml:lang="en">Breast-In situ neoplasm-Histologic type-DCIS Micropapillary</skos:definition>
        <skos:prefLabel xml:lang="en">DCIS Micropapillary</skos:prefLabel>
    </owl:Class>
    


    <!-- http://www.semanticweb.org/david/ontologies/2013/0/1.3.6.1.4.1.19376.1.8.2.1.2561 -->

    <owl:Class rdf:about="&pathLex;2561">
        <rdfs:subClassOf rdf:resource="&pathLex;436"/>
        <skos:definition xml:lang="en">Breast-In situ neoplasm-Histologic type-DCIS Papillary</skos:definition>
        <skos:prefLabel xml:lang="en">DCIS Papillary</skos:prefLabel>
    </owl:Class>
    


    <!-- http://www.semanticweb.org/david/ontologies/2013/0/1.3.6.1.4.1.19376.1.8.2.1.2562 -->

    <owl:Class rdf:about="&pathLex;2562">
        <rdfs:subClassOf rdf:resource="&pathLex;436"/>
        <skos:definition xml:lang="en">Breast-In situ neoplasm-Histologic type-DCIS Solid</skos:definition>
        <skos:prefLabel xml:lang="en">DCIS Solid</skos:prefLabel>
    </owl:Class>
    


    <!-- http://www.semanticweb.org/david/ontologies/2013/0/1.3.6.1.4.1.19376.1.8.2.1.2563 -->

    <owl:Class rdf:about="&pathLex;2563">
        <rdfs:subClassOf rdf:resource="&pathLex;99999"/>
        <skos:prefLabel xml:lang="en">Intratubular germ cell neoplasia</skos:prefLabel>
        <skos:definition xml:lang="en">Testis-Lesion-Histologic type-Intratubular germ cell neoplasia</skos:definition>
    </owl:Class>
    


    <!-- http://www.semanticweb.org/david/ontologies/2013/0/1.3.6.1.4.1.19376.1.8.2.1.2564 -->

    <owl:Class rdf:about="&pathLex;2564">
        <rdfs:subClassOf rdf:resource="&pathLex;99999"/>
        <skos:prefLabel xml:lang="en">Adenoma</skos:prefLabel>
        <skos:definition xml:lang="en">Thyroid-Lesion-Histologic type-Adenoma</skos:definition>
    </owl:Class>
    


    <!-- http://www.semanticweb.org/david/ontologies/2013/0/1.3.6.1.4.1.19376.1.8.2.1.2565 -->

    <owl:Class rdf:about="&pathLex;2565">
        <rdfs:subClassOf rdf:resource="&pathLex;99999"/>
        <skos:prefLabel xml:lang="en">Adenomatoid nodule(s)</skos:prefLabel>
        <skos:definition xml:lang="en">Thyroid-Lesion-Histologic type-Adenomatoid nodule(s)</skos:definition>
    </owl:Class>
    


    <!-- http://www.semanticweb.org/david/ontologies/2013/0/1.3.6.1.4.1.19376.1.8.2.1.2566 -->

    <owl:Class rdf:about="&pathLex;2566">
        <rdfs:subClassOf rdf:resource="&pathLex;99999"/>
        <skos:prefLabel xml:lang="en">Nodular follicular disease (eg, nodular hyperplasia,goitrous thyroid)</skos:prefLabel>
        <skos:definition xml:lang="en">Thyroid-Lesion-Histologic type-Nodular follicular disease (eg, nodular hyperplasia,goitrous thyroid)</skos:definition>
    </owl:Class>
    


    <!-- http://www.semanticweb.org/david/ontologies/2013/0/1.3.6.1.4.1.19376.1.8.2.1.2567 -->

    <owl:Class rdf:about="&pathLex;2567">
        <rdfs:subClassOf rdf:resource="&pathLex;99999"/>
        <skos:prefLabel xml:lang="en">Diffuse hyperplasia (Graves’ disease)</skos:prefLabel>
        <skos:definition xml:lang="en">Thyroid-Lesion-Histologic type-Diffuse hyperplasia (Graves’ disease)</skos:definition>
    </owl:Class>
    


    <!-- http://www.semanticweb.org/david/ontologies/2013/0/1.3.6.1.4.1.19376.1.8.2.1.2568 -->

    <owl:Class rdf:about="&pathLex;2568">
        <rdfs:subClassOf rdf:resource="&pathLex;99999"/>
        <skos:prefLabel xml:lang="en">Advanced thyroiditis</skos:prefLabel>
        <skos:definition xml:lang="en">Thyroid-Lesion-Histologic type-Advanced thyroiditis</skos:definition>
    </owl:Class>
    


    <!-- http://www.semanticweb.org/david/ontologies/2013/0/1.3.6.1.4.1.19376.1.8.2.1.2569 -->

    <owl:Class rdf:about="&pathLex;2569">
        <rdfs:subClassOf rdf:resource="&pathLex;99999"/>
        <skos:prefLabel xml:lang="en">Focal (nonspecific) thyroiditis</skos:prefLabel>
        <skos:definition xml:lang="en">Thyroid-Lesion-Histologic type-Focal (nonspecific) thyroiditis</skos:definition>
    </owl:Class>
    


    <!-- http://www.semanticweb.org/david/ontologies/2013/0/1.3.6.1.4.1.19376.1.8.2.1.257 -->

    <owl:Class rdf:about="&pathLex;257">
        <rdfs:subClassOf rdf:resource="&pathLex;99999"/>
        <skos:definition xml:lang="en">Lip, oral cavity-Infiltrating malignant neoplasm-Lymph node capsule involvement</skos:definition>
        <skos:prefLabel xml:lang="en">Lymph node capsule involvement</skos:prefLabel>
    </owl:Class>
    


    <!-- http://www.semanticweb.org/david/ontologies/2013/0/1.3.6.1.4.1.19376.1.8.2.1.2570 -->

    <owl:Class rdf:about="&pathLex;2570">
        <rdfs:subClassOf rdf:resource="&pathLex;99999"/>
        <skos:prefLabel xml:lang="en">Parathyroid gland(s) within normal limits</skos:prefLabel>
        <skos:definition xml:lang="en">Thyroid-Lesion-Histologic type-Parathyroid gland(s) within normal limits</skos:definition>
    </owl:Class>
    


    <!-- http://www.semanticweb.org/david/ontologies/2013/0/1.3.6.1.4.1.19376.1.8.2.1.2571 -->

    <owl:Class rdf:about="&pathLex;2571">
        <rdfs:subClassOf rdf:resource="&pathLex;99999"/>
        <skos:prefLabel xml:lang="en">Hypercellular parathyroid gland(s)</skos:prefLabel>
        <skos:definition xml:lang="en">Thyroid-Lesion-Histologic type-Hypercellular parathyroid gland(s)</skos:definition>
    </owl:Class>
    


    <!-- http://www.semanticweb.org/david/ontologies/2013/0/1.3.6.1.4.1.19376.1.8.2.1.2572 -->

    <owl:Class rdf:about="&pathLex;2572">
        <rdfs:subClassOf rdf:resource="&pathLex;99999"/>
        <skos:prefLabel xml:lang="en">C-cell hyperplasia</skos:prefLabel>
        <skos:definition xml:lang="en">Thyroid-Lesion-Histologic type-C-cell hyperplasia</skos:definition>
    </owl:Class>
    


    <!-- http://www.semanticweb.org/david/ontologies/2013/0/1.3.6.1.4.1.19376.1.8.2.1.2573 -->

    <owl:Class rdf:about="&pathLex;2573">
        <rdfs:subClassOf rdf:resource="&pathLex;99999"/>
        <skos:prefLabel xml:lang="en">Inflammation/regenerative changes</skos:prefLabel>
        <skos:definition xml:lang="en">Urinary bladder-Lesion-Histologic type-Inflammation/regenerative changes</skos:definition>
    </owl:Class>
    


    <!-- http://www.semanticweb.org/david/ontologies/2013/0/1.3.6.1.4.1.19376.1.8.2.1.2574 -->

    <owl:Class rdf:about="&pathLex;2574">
        <rdfs:subClassOf rdf:resource="&pathLex;99999"/>
        <skos:prefLabel xml:lang="en">Therapy-related changes</skos:prefLabel>
        <skos:definition xml:lang="en">Urinary bladder-Lesion-Histologic type-Therapy-related changes</skos:definition>
    </owl:Class>
    


    <!-- http://www.semanticweb.org/david/ontologies/2013/0/1.3.6.1.4.1.19376.1.8.2.1.2575 -->

    <owl:Class rdf:about="&pathLex;2575">
        <rdfs:subClassOf rdf:resource="&pathLex;99999"/>
        <skos:prefLabel xml:lang="en">Cautery artifact</skos:prefLabel>
        <skos:definition xml:lang="en">Urinary bladder-Lesion-Histologic type-Cautery artifact</skos:definition>
    </owl:Class>
    


    <!-- http://www.semanticweb.org/david/ontologies/2013/0/1.3.6.1.4.1.19376.1.8.2.1.2576 -->

    <owl:Class rdf:about="&pathLex;2576">
        <rdfs:subClassOf rdf:resource="&pathLex;99999"/>
        <skos:prefLabel xml:lang="en">Cystitis cystica glandularis</skos:prefLabel>
        <skos:definition xml:lang="en">Urinary bladder-Lesion-Histologic type-Cystitis cystica glandularis</skos:definition>
    </owl:Class>
    


    <!-- http://www.semanticweb.org/david/ontologies/2013/0/1.3.6.1.4.1.19376.1.8.2.1.2577 -->

    <owl:Class rdf:about="&pathLex;2577">
        <rdfs:subClassOf rdf:resource="&pathLex;99999"/>
        <skos:prefLabel xml:lang="en">Keratinizing squamous metaplasia</skos:prefLabel>
        <skos:definition xml:lang="en">Urinary bladder-Lesion-Histologic type-Keratinizing squamous metaplasia</skos:definition>
    </owl:Class>
    


    <!-- http://www.semanticweb.org/david/ontologies/2013/0/1.3.6.1.4.1.19376.1.8.2.1.2578 -->

    <owl:Class rdf:about="&pathLex;2578">
        <rdfs:subClassOf rdf:resource="&pathLex;99999"/>
        <skos:prefLabel xml:lang="en">Intestinal metaplasia</skos:prefLabel>
        <skos:definition xml:lang="en">Urinary bladder-Lesion-Histologic type-Intestinal metaplasia</skos:definition>
    </owl:Class>
    


    <!-- http://www.semanticweb.org/david/ontologies/2013/0/1.3.6.1.4.1.19376.1.8.2.1.2579 -->

    <owl:Class rdf:about="&pathLex;2579">
        <rdfs:subClassOf rdf:resource="&pathLex;99999"/>
        <skos:definition xml:lang="en">Colon-Infiltrating malignant neoplasm-Macroscopic type-Tubular adenoma</skos:definition>
        <skos:prefLabel xml:lang="en">Tubular adenoma</skos:prefLabel>
    </owl:Class>
    


    <!-- http://www.semanticweb.org/david/ontologies/2013/0/1.3.6.1.4.1.19376.1.8.2.1.258 -->

    <owl:Class rdf:about="&pathLex;258">
        <rdfs:subClassOf rdf:resource="&pathLex;99999"/>
        <skos:definition xml:lang="en">Lip, oral cavity-Infiltrating malignant neoplasm-Lymph node site</skos:definition>
        <skos:prefLabel xml:lang="en">Lymph node site</skos:prefLabel>
    </owl:Class>
    


    <!-- http://www.semanticweb.org/david/ontologies/2013/0/1.3.6.1.4.1.19376.1.8.2.1.2580 -->

    <owl:Class rdf:about="&pathLex;2580">
        <rdfs:subClassOf rdf:resource="&pathLex;99999"/>
        <skos:definition xml:lang="en">Colon-Infiltrating malignant neoplasm-Macroscopic type-Villous adenoma</skos:definition>
        <skos:prefLabel xml:lang="en">Villous adenoma</skos:prefLabel>
    </owl:Class>
    


    <!-- http://www.semanticweb.org/david/ontologies/2013/0/1.3.6.1.4.1.19376.1.8.2.1.2581 -->

    <owl:Class rdf:about="&pathLex;2581">
        <rdfs:subClassOf rdf:resource="&pathLex;99999"/>
        <skos:definition xml:lang="en">Colon-Infiltrating malignant neoplasm-Macroscopic type-Tubulovillous adenoma</skos:definition>
        <skos:prefLabel xml:lang="en">Tubulovillous adenoma</skos:prefLabel>
    </owl:Class>
    


    <!-- http://www.semanticweb.org/david/ontologies/2013/0/1.3.6.1.4.1.19376.1.8.2.1.2582 -->

    <owl:Class rdf:about="&pathLex;2582">
        <rdfs:subClassOf rdf:resource="&pathLex;99999"/>
        <skos:definition xml:lang="en">Colon-Infiltrating malignant neoplasm-Macroscopic type-Traditional serrated adenoma</skos:definition>
        <skos:prefLabel xml:lang="en">Traditional serrated adenoma</skos:prefLabel>
    </owl:Class>
    


    <!-- http://www.semanticweb.org/david/ontologies/2013/0/1.3.6.1.4.1.19376.1.8.2.1.2583 -->

    <owl:Class rdf:about="&pathLex;2583">
        <rdfs:subClassOf rdf:resource="&pathLex;99999"/>
        <skos:definition xml:lang="en">Colon-Infiltrating malignant neoplasm-Macroscopic type-Sessile serrated adenoma</skos:definition>
        <skos:prefLabel xml:lang="en">Sessile serrated adenoma</skos:prefLabel>
    </owl:Class>
    


    <!-- http://www.semanticweb.org/david/ontologies/2013/0/1.3.6.1.4.1.19376.1.8.2.1.2584 -->

    <owl:Class rdf:about="&pathLex;2584">
        <rdfs:subClassOf rdf:resource="&pathLex;99999"/>
        <skos:definition xml:lang="en">Colon-Infiltrating malignant neoplasm-Macroscopic type-Hamartomatous polyp</skos:definition>
        <skos:prefLabel xml:lang="en">Hamartomatous polyp</skos:prefLabel>
    </owl:Class>
    


    <!-- http://www.semanticweb.org/david/ontologies/2013/0/1.3.6.1.4.1.19376.1.8.2.1.2585 -->

    <owl:Class rdf:about="&pathLex;2585">
        <rdfs:subClassOf rdf:resource="&pathLex;99999"/>
        <skos:definition xml:lang="en">Colon-Infiltrating malignant neoplasm-Macroscopic type-Indeterminate</skos:definition>
        <skos:prefLabel xml:lang="en">Indeterminate</skos:prefLabel>
    </owl:Class>
    


    <!-- http://www.semanticweb.org/david/ontologies/2013/0/1.3.6.1.4.1.19376.1.8.2.1.2586 -->

    <owl:Class rdf:about="&pathLex;2586">
        <rdfs:subClassOf rdf:resource="&pathLex;99999"/>
        <skos:definition xml:lang="en">Colon-Lesion-Macroscopic type-Pedunculated polyp with stalk (Stalk length: cm)</skos:definition>
        <skos:prefLabel xml:lang="en">Pedunculated polyp with stalk (Stalk length: cm)</skos:prefLabel>
    </owl:Class>
    


    <!-- http://www.semanticweb.org/david/ontologies/2013/0/1.3.6.1.4.1.19376.1.8.2.1.2587 -->

    <owl:Class rdf:about="&pathLex;2587">
        <rdfs:subClassOf rdf:resource="&pathLex;99999"/>
        <skos:definition xml:lang="en">Colon-Lesion-Macroscopic type-Sessile polyp</skos:definition>
        <skos:prefLabel xml:lang="en">Sessile polyp</skos:prefLabel>
    </owl:Class>
    


    <!-- http://www.semanticweb.org/david/ontologies/2013/0/1.3.6.1.4.1.19376.1.8.2.1.2589 -->

    <owl:Class rdf:about="&pathLex;2589">
        <rdfs:subClassOf rdf:resource="&pathLex;99999"/>
        <skos:prefLabel xml:lang="en">Encapsulated/circumscribed lesion</skos:prefLabel>
        <skos:definition xml:lang="en">Salivary gland-Infiltrating malignant neoplasm-Macroscopic type-Encapsulated/circumscribed lesion</skos:definition>
    </owl:Class>
    


    <!-- http://www.semanticweb.org/david/ontologies/2013/0/1.3.6.1.4.1.19376.1.8.2.1.259 -->

    <owl:Class rdf:about="&pathLex;259">
        <rdfs:subClassOf rdf:resource="&pathLex;99999"/>
        <skos:definition xml:lang="en">Lip, oral cavity-Infiltrating malignant neoplasm-Number of lymph nodes involved</skos:definition>
        <skos:prefLabel xml:lang="en">Number of lymph nodes involved</skos:prefLabel>
    </owl:Class>
    


    <!-- http://www.semanticweb.org/david/ontologies/2013/0/1.3.6.1.4.1.19376.1.8.2.1.2590 -->

    <owl:Class rdf:about="&pathLex;2590">
        <rdfs:subClassOf rdf:resource="&pathLex;99999"/>
        <skos:prefLabel xml:lang="en">Invasive lesion</skos:prefLabel>
        <skos:definition xml:lang="en">Salivary gland-Infiltrating malignant neoplasm-Macroscopic type-Invasive lesion</skos:definition>
    </owl:Class>
    


    <!-- http://www.semanticweb.org/david/ontologies/2013/0/1.3.6.1.4.1.19376.1.8.2.1.2591 -->

    <owl:Class rdf:about="&pathLex;2591">
        <rdfs:subClassOf rdf:resource="&pathLex;99999"/>
        <skos:definition xml:lang="en">Salivary gland-Infiltrating malignant neoplasm-Macroscopic type-Solid lesion</skos:definition>
        <skos:prefLabel xml:lang="en">Solid lesion</skos:prefLabel>
    </owl:Class>
    


    <!-- http://www.semanticweb.org/david/ontologies/2013/0/1.3.6.1.4.1.19376.1.8.2.1.2592 -->

    <owl:Class rdf:about="&pathLex;2592">
        <rdfs:subClassOf rdf:resource="&pathLex;99999"/>
        <skos:prefLabel xml:lang="en">Cystic lesion</skos:prefLabel>
        <skos:definition xml:lang="en">Salivary gland-Infiltrating malignant neoplasm-Macroscopic type-Cystic lesion</skos:definition>
    </owl:Class>
    


    <!-- http://www.semanticweb.org/david/ontologies/2013/0/1.3.6.1.4.1.19376.1.8.2.1.2593 -->

    <owl:Class rdf:about="&pathLex;2593">
        <rdfs:subClassOf rdf:resource="&pathLex;99999"/>
        <skos:prefLabel xml:lang="en">Epithelial-myoepithelial carcinoma</skos:prefLabel>
        <skos:definition xml:lang="en">Salivary gland-Infiltrating malignant neoplasm-Macroscopic type-Epithelial-myoepithelial carcinoma</skos:definition>
    </owl:Class>
    


    <!-- http://www.semanticweb.org/david/ontologies/2013/0/1.3.6.1.4.1.19376.1.8.2.1.2594 -->

    <owl:Class rdf:about="&pathLex;2594">
        <rdfs:subClassOf rdf:resource="&pathLex;99999"/>
        <skos:definition xml:lang="en">Larynx-Infiltrating malignant neoplasm-Macroscopic type-Sessile lesion</skos:definition>
        <skos:prefLabel xml:lang="en">Sessile lesion</skos:prefLabel>
    </owl:Class>
    


    <!-- http://www.semanticweb.org/david/ontologies/2013/0/1.3.6.1.4.1.19376.1.8.2.1.2595 -->

    <owl:Class rdf:about="&pathLex;2595">
        <rdfs:subClassOf rdf:resource="&pathLex;99999"/>
        <skos:definition xml:lang="en">Larynx-Infiltrating malignant neoplasm-Macroscopic type-Polypoid lesion</skos:definition>
        <skos:prefLabel xml:lang="en">Polypoid lesion</skos:prefLabel>
    </owl:Class>
    


    <!-- http://www.semanticweb.org/david/ontologies/2013/0/1.3.6.1.4.1.19376.1.8.2.1.2596 -->

    <owl:Class rdf:about="&pathLex;2596">
        <rdfs:subClassOf rdf:resource="&pathLex;99999"/>
        <skos:prefLabel xml:lang="en">Exophytic lesion</skos:prefLabel>
        <skos:definition xml:lang="en">Larynx-Infiltrating malignant neoplasm-Macroscopic type-Exophytic lesion</skos:definition>
    </owl:Class>
    


    <!-- http://www.semanticweb.org/david/ontologies/2013/0/1.3.6.1.4.1.19376.1.8.2.1.2597 -->

    <owl:Class rdf:about="&pathLex;2597">
        <rdfs:subClassOf rdf:resource="&pathLex;99999"/>
        <skos:prefLabel xml:lang="en">Endophytic lesion</skos:prefLabel>
        <skos:definition xml:lang="en">Larynx-Infiltrating malignant neoplasm-Macroscopic type-Endophytic lesion</skos:definition>
    </owl:Class>
    


    <!-- http://www.semanticweb.org/david/ontologies/2013/0/1.3.6.1.4.1.19376.1.8.2.1.2598 -->

    <owl:Class rdf:about="&pathLex;2598">
        <rdfs:subClassOf rdf:resource="&pathLex;99999"/>
        <skos:definition xml:lang="en">Larynx-Infiltrating malignant neoplasm-Macroscopic type-Ulcerated lesion</skos:definition>
        <skos:prefLabel xml:lang="en">Ulcerated lesion</skos:prefLabel>
    </owl:Class>
    


    <!-- http://www.semanticweb.org/david/ontologies/2013/0/1.3.6.1.4.1.19376.1.8.2.1.2599 -->

    <owl:Class rdf:about="&pathLex;2599">
        <rdfs:subClassOf rdf:resource="&pathLex;99999"/>
        <skos:definition xml:lang="en">Larynx-Infiltrating malignant neoplasm-Macroscopic type-Mild keratinizing dysplasia</skos:definition>
        <skos:prefLabel xml:lang="en">Mild keratinizing dysplasia</skos:prefLabel>
    </owl:Class>
    


    <!-- http://www.semanticweb.org/david/ontologies/2013/0/1.3.6.1.4.1.19376.1.8.2.1.260 -->

    <owl:Class rdf:about="&pathLex;260">
        <rdfs:subClassOf rdf:resource="&pathLex;99999"/>
        <skos:definition xml:lang="en">Lip, oral cavity-Infiltrating malignant neoplasm-Number of lymph nodes examined</skos:definition>
        <skos:prefLabel xml:lang="en">Number of lymph nodes examined</skos:prefLabel>
    </owl:Class>
    


    <!-- http://www.semanticweb.org/david/ontologies/2013/0/1.3.6.1.4.1.19376.1.8.2.1.2600 -->

    <owl:Class rdf:about="&pathLex;2600">
        <rdfs:subClassOf rdf:resource="&pathLex;99999"/>
        <skos:definition xml:lang="en">Larynx-Infiltrating malignant neoplasm-Macroscopic type-Moderate keratinizing dysplasia</skos:definition>
        <skos:prefLabel xml:lang="en">Moderate keratinizing dysplasia</skos:prefLabel>
    </owl:Class>
    


    <!-- http://www.semanticweb.org/david/ontologies/2013/0/1.3.6.1.4.1.19376.1.8.2.1.2601 -->

    <owl:Class rdf:about="&pathLex;2601">
        <rdfs:subClassOf rdf:resource="&pathLex;99999"/>
        <skos:definition xml:lang="en">Larynx-Infiltrating malignant neoplasm-Macroscopic type-Severe keratinizing dysplasia (carcinoma in situ)</skos:definition>
        <skos:prefLabel xml:lang="en">Severe keratinizing dysplasia (carcinoma in situ)</skos:prefLabel>
    </owl:Class>
    


    <!-- http://www.semanticweb.org/david/ontologies/2013/0/1.3.6.1.4.1.19376.1.8.2.1.2602 -->

    <owl:Class rdf:about="&pathLex;2602">
        <rdfs:subClassOf rdf:resource="&pathLex;99999"/>
        <skos:definition xml:lang="en">Larynx-Infiltrating malignant neoplasm-Macroscopic type-Mild non-keratinizing dysplasia</skos:definition>
        <skos:prefLabel xml:lang="en">Mild non-keratinizing dysplasia</skos:prefLabel>
    </owl:Class>
    


    <!-- http://www.semanticweb.org/david/ontologies/2013/0/1.3.6.1.4.1.19376.1.8.2.1.2603 -->

    <owl:Class rdf:about="&pathLex;2603">
        <rdfs:subClassOf rdf:resource="&pathLex;99999"/>
        <skos:definition xml:lang="en">Larynx-Infiltrating malignant neoplasm-Macroscopic type-Moderate non-keratinizing dysplasia</skos:definition>
        <skos:prefLabel xml:lang="en">Moderate non-keratinizing dysplasia</skos:prefLabel>
    </owl:Class>
    


    <!-- http://www.semanticweb.org/david/ontologies/2013/0/1.3.6.1.4.1.19376.1.8.2.1.2604 -->

    <owl:Class rdf:about="&pathLex;2604">
        <rdfs:subClassOf rdf:resource="&pathLex;99999"/>
        <skos:definition xml:lang="en">Larynx-Infiltrating malignant neoplasm-Macroscopic type-Severe non-keratinizing dysplasia (carcinoma in situ)</skos:definition>
        <skos:prefLabel xml:lang="en">Severe non-keratinizing dysplasia (carcinoma in situ)</skos:prefLabel>
    </owl:Class>
    


    <!-- http://www.semanticweb.org/david/ontologies/2013/0/1.3.6.1.4.1.19376.1.8.2.1.2605 -->

    <owl:Class rdf:about="&pathLex;2605">
        <rdfs:subClassOf rdf:resource="&pathLex;99999"/>
        <skos:prefLabel xml:lang="en">Inflammation (specify)</skos:prefLabel>
        <skos:definition xml:lang="en">Larynx-Infiltrating malignant neoplasm-Macroscopic type-Inflammation (specify)</skos:definition>
    </owl:Class>
    


    <!-- http://www.semanticweb.org/david/ontologies/2013/0/1.3.6.1.4.1.19376.1.8.2.1.2606 -->

    <owl:Class rdf:about="&pathLex;2606">
        <rdfs:subClassOf rdf:resource="&pathLex;99999"/>
        <skos:definition xml:lang="en">Larynx-Infiltrating malignant neoplasm-Macroscopic type-Squamous metaplasia</skos:definition>
        <skos:prefLabel xml:lang="en">Squamous metaplasia</skos:prefLabel>
    </owl:Class>
    


    <!-- http://www.semanticweb.org/david/ontologies/2013/0/1.3.6.1.4.1.19376.1.8.2.1.2607 -->

    <owl:Class rdf:about="&pathLex;2607">
        <rdfs:subClassOf rdf:resource="&pathLex;99999"/>
        <skos:prefLabel xml:lang="en">Epithelial hyperplasia</skos:prefLabel>
        <skos:definition xml:lang="en">Larynx-Infiltrating malignant neoplasm-Macroscopic type-Epithelial hyperplasia</skos:definition>
    </owl:Class>
    


    <!-- http://www.semanticweb.org/david/ontologies/2013/0/1.3.6.1.4.1.19376.1.8.2.1.2608 -->

    <owl:Class rdf:about="&pathLex;2608">
        <rdfs:subClassOf rdf:resource="&pathLex;99999"/>
        <skos:prefLabel xml:lang="en">Fungal colonization</skos:prefLabel>
        <skos:definition xml:lang="en">Larynx-Infiltrating malignant neoplasm-Macroscopic type-Fungal colonization</skos:definition>
    </owl:Class>
    


    <!-- http://www.semanticweb.org/david/ontologies/2013/0/1.3.6.1.4.1.19376.1.8.2.1.2609 -->

    <owl:Class rdf:about="&pathLex;2609">
        <rdfs:subClassOf rdf:resource="&pathLex;99999"/>
        <skos:prefLabel xml:lang="en">Bacterial colonization</skos:prefLabel>
        <skos:definition xml:lang="en">Larynx-Infiltrating malignant neoplasm-Macroscopic type-Bacterial colonization</skos:definition>
    </owl:Class>
    


    <!-- http://www.semanticweb.org/david/ontologies/2013/0/1.3.6.1.4.1.19376.1.8.2.1.2610 -->

    <owl:Class rdf:about="&pathLex;2610">
        <rdfs:subClassOf rdf:resource="&pathLex;99999"/>
        <skos:definition xml:lang="en">Pharynx-Infiltrating malignant neoplasm-Macroscopic type-Polypoid lesion</skos:definition>
        <skos:prefLabel xml:lang="en">Polypoid lesion</skos:prefLabel>
    </owl:Class>
    


    <!-- http://www.semanticweb.org/david/ontologies/2013/0/1.3.6.1.4.1.19376.1.8.2.1.2611 -->

    <owl:Class rdf:about="&pathLex;2611">
        <rdfs:subClassOf rdf:resource="&pathLex;99999"/>
        <skos:prefLabel xml:lang="en">Exophytic  lesion</skos:prefLabel>
        <skos:definition xml:lang="en">Pharynx-Infiltrating malignant neoplasm-Macroscopic type-Exophytic  lesion</skos:definition>
    </owl:Class>
    


    <!-- http://www.semanticweb.org/david/ontologies/2013/0/1.3.6.1.4.1.19376.1.8.2.1.2612 -->

    <owl:Class rdf:about="&pathLex;2612">
        <rdfs:subClassOf rdf:resource="&pathLex;99999"/>
        <skos:prefLabel xml:lang="en">Endophytic lesion</skos:prefLabel>
        <skos:definition xml:lang="en">Pharynx-Infiltrating malignant neoplasm-Macroscopic type-Endophytic lesion</skos:definition>
    </owl:Class>
    


    <!-- http://www.semanticweb.org/david/ontologies/2013/0/1.3.6.1.4.1.19376.1.8.2.1.2613 -->

    <owl:Class rdf:about="&pathLex;2613">
        <rdfs:subClassOf rdf:resource="&pathLex;99999"/>
        <skos:definition xml:lang="en">Pharynx-Infiltrating malignant neoplasm-Macroscopic type-Ulcerated lesion</skos:definition>
        <skos:prefLabel xml:lang="en">Ulcerated lesion</skos:prefLabel>
    </owl:Class>
    


    <!-- http://www.semanticweb.org/david/ontologies/2013/0/1.3.6.1.4.1.19376.1.8.2.1.2614 -->

    <owl:Class rdf:about="&pathLex;2614">
        <rdfs:subClassOf rdf:resource="&pathLex;99999"/>
        <skos:definition xml:lang="en">Pharynx-Infiltrating malignant neoplasm-Macroscopic type-Sessile lesion</skos:definition>
        <skos:prefLabel xml:lang="en">Sessile lesion</skos:prefLabel>
    </owl:Class>
    


    <!-- http://www.semanticweb.org/david/ontologies/2013/0/1.3.6.1.4.1.19376.1.8.2.1.2615 -->

    <owl:Class rdf:about="&pathLex;2615">
        <rdfs:subClassOf rdf:resource="&pathLex;99999"/>
        <skos:prefLabel xml:lang="en">Papillary</skos:prefLabel>
        <skos:definition xml:lang="en">Urinary bladder-Infiltrating malignant neoplasm-Macroscopic type-Papillary</skos:definition>
    </owl:Class>
    


    <!-- http://www.semanticweb.org/david/ontologies/2013/0/1.3.6.1.4.1.19376.1.8.2.1.2616 -->

    <owl:Class rdf:about="&pathLex;2616">
        <rdfs:subClassOf rdf:resource="&pathLex;99999"/>
        <skos:prefLabel xml:lang="en">Solid/nodule</skos:prefLabel>
        <skos:definition xml:lang="en">Urinary bladder-Infiltrating malignant neoplasm-Macroscopic type-Solid/nodule</skos:definition>
    </owl:Class>
    


    <!-- http://www.semanticweb.org/david/ontologies/2013/0/1.3.6.1.4.1.19376.1.8.2.1.2617 -->

    <owl:Class rdf:about="&pathLex;2617">
        <rdfs:subClassOf rdf:resource="&pathLex;99999"/>
        <skos:prefLabel xml:lang="en">Flat</skos:prefLabel>
        <skos:definition xml:lang="en">Urinary bladder-Infiltrating malignant neoplasm-Macroscopic type-Flat</skos:definition>
    </owl:Class>
    


    <!-- http://www.semanticweb.org/david/ontologies/2013/0/1.3.6.1.4.1.19376.1.8.2.1.2618 -->

    <owl:Class rdf:about="&pathLex;2618">
        <rdfs:subClassOf rdf:resource="&pathLex;99999"/>
        <skos:prefLabel xml:lang="en">Ulcerated</skos:prefLabel>
        <skos:definition xml:lang="en">Urinary bladder-Infiltrating malignant neoplasm-Macroscopic type-Ulcerated</skos:definition>
    </owl:Class>
    


    <!-- http://www.semanticweb.org/david/ontologies/2013/0/1.3.6.1.4.1.19376.1.8.2.1.2619 -->

    <owl:Class rdf:about="&pathLex;2619">
        <rdfs:subClassOf rdf:resource="&pathLex;99999"/>
        <skos:prefLabel xml:lang="en">Indeterminate</skos:prefLabel>
        <skos:definition xml:lang="en">Urinary bladder-Infiltrating malignant neoplasm-Macroscopic type-Indeterminate</skos:definition>
    </owl:Class>
    


    <!-- http://www.semanticweb.org/david/ontologies/2013/0/1.3.6.1.4.1.19376.1.8.2.1.262 -->

    <owl:Class rdf:about="&pathLex;262">
        <rdfs:subClassOf rdf:resource="&pathLex;99999"/>
        <skos:definition xml:lang="en">Lip, oral cavity-Infiltrating malignant neoplasm-pN</skos:definition>
        <skos:prefLabel xml:lang="en">pN</skos:prefLabel>
    </owl:Class>
    


    <!-- http://www.semanticweb.org/david/ontologies/2013/0/1.3.6.1.4.1.19376.1.8.2.1.2620 -->

    <owl:Class rdf:about="&pathLex;2620">
        <rdfs:subClassOf rdf:resource="&pathLex;99999"/>
        <skos:definition xml:lang="en">Cervix-In situ neoplasm-Histologic type-</skos:definition>
        <skos:prefLabel xml:lang="en">Intraepithelial neoplasia</skos:prefLabel>
    </owl:Class>
    


    <!-- http://www.semanticweb.org/david/ontologies/2013/0/1.3.6.1.4.1.19376.1.8.2.1.2621 -->

    <owl:Class rdf:about="&pathLex;2621">
        <rdfs:subClassOf rdf:resource="&pathLex;99999"/>
        <skos:definition xml:lang="en">Prostate-Infiltrating malignant neoplasm-Histologic type-Signet-ring cell carcinoma</skos:definition>
        <skos:prefLabel xml:lang="en">Signet-ring cell carcinoma</skos:prefLabel>
    </owl:Class>
    


    <!-- http://www.semanticweb.org/david/ontologies/2013/0/1.3.6.1.4.1.19376.1.8.2.1.2622 -->

    <owl:Class rdf:about="&pathLex;2622">
        <rdfs:subClassOf rdf:resource="&pathLex;99999"/>
        <skos:prefLabel xml:lang="en">Adenosquamous carcinoma</skos:prefLabel>
        <skos:definition xml:lang="en">Prostate-Infiltrating malignant neoplasm-Histologic type-Adenosquamous carcinoma</skos:definition>
    </owl:Class>
    


    <!-- http://www.semanticweb.org/david/ontologies/2013/0/1.3.6.1.4.1.19376.1.8.2.1.2623 -->

    <owl:Class rdf:about="&pathLex;2623">
        <rdfs:subClassOf rdf:resource="&pathLex;99999"/>
        <skos:definition xml:lang="en">Prostate-Infiltrating malignant neoplasm-Histologic type-Small cell carcinoma</skos:definition>
        <skos:prefLabel xml:lang="en">Small cell carcinoma</skos:prefLabel>
    </owl:Class>
    


    <!-- http://www.semanticweb.org/david/ontologies/2013/0/1.3.6.1.4.1.19376.1.8.2.1.2624 -->

    <owl:Class rdf:about="&pathLex;2624">
        <rdfs:subClassOf rdf:resource="&pathLex;99999"/>
        <skos:definition xml:lang="en">Prostate-Infiltrating malignant neoplasm-Histologic type-Sarcomatoid carcinoma</skos:definition>
        <skos:prefLabel xml:lang="en">Sarcomatoid carcinoma</skos:prefLabel>
    </owl:Class>
    


    <!-- http://www.semanticweb.org/david/ontologies/2013/0/1.3.6.1.4.1.19376.1.8.2.1.2625 -->

    <owl:Class rdf:about="&pathLex;2625">
        <rdfs:subClassOf rdf:resource="&pathLex;99999"/>
        <skos:definition xml:lang="en">Prostate-Infiltrating malignant neoplasm-Histologic type-Undifferentiated carcinoma, not otherwise specified</skos:definition>
        <skos:prefLabel xml:lang="en">Undifferentiated carcinoma, not otherwise specified</skos:prefLabel>
    </owl:Class>
    


    <!-- http://www.semanticweb.org/david/ontologies/2013/0/1.3.6.1.4.1.19376.1.8.2.1.2626 -->

    <owl:Class rdf:about="&pathLex;2626">
        <rdfs:subClassOf rdf:resource="&pathLex;99999"/>
        <skos:prefLabel xml:lang="en">Seminoma with associated scar</skos:prefLabel>
        <skos:definition xml:lang="en">Testis-Infiltrating malignant neoplasm-Histologic type-Seminoma with associated scar</skos:definition>
    </owl:Class>
    


    <!-- http://www.semanticweb.org/david/ontologies/2013/0/1.3.6.1.4.1.19376.1.8.2.1.2627 -->

    <owl:Class rdf:about="&pathLex;2627">
        <rdfs:subClassOf rdf:resource="&pathLex;99999"/>
        <skos:prefLabel xml:lang="en">Seminoma with syncytiotrophoblastic cells</skos:prefLabel>
        <skos:definition xml:lang="en">Testis-Infiltrating malignant neoplasm-Histologic type-Seminoma with syncytiotrophoblastic cells</skos:definition>
    </owl:Class>
    


    <!-- http://www.semanticweb.org/david/ontologies/2013/0/1.3.6.1.4.1.19376.1.8.2.1.2628 -->

    <owl:Class rdf:about="&pathLex;2628">
        <rdfs:subClassOf rdf:resource="&pathLex;99999"/>
        <skos:prefLabel xml:lang="en">Embryonal carcinoma</skos:prefLabel>
        <skos:definition xml:lang="en">Testis-Infiltrating malignant neoplasm-Histologic type-Embryonal carcinoma</skos:definition>
    </owl:Class>
    


    <!-- http://www.semanticweb.org/david/ontologies/2013/0/1.3.6.1.4.1.19376.1.8.2.1.2629 -->

    <owl:Class rdf:about="&pathLex;2629">
        <rdfs:subClassOf rdf:resource="&pathLex;99999"/>
        <skos:prefLabel xml:lang="en">Choriocarcinoma, biphasic</skos:prefLabel>
        <skos:definition xml:lang="en">Testis-Infiltrating malignant neoplasm-Histologic type-Choriocarcinoma, biphasic</skos:definition>
    </owl:Class>
    


    <!-- http://www.semanticweb.org/david/ontologies/2013/0/1.3.6.1.4.1.19376.1.8.2.1.2630 -->

    <owl:Class rdf:about="&pathLex;2630">
        <rdfs:subClassOf rdf:resource="&pathLex;99999"/>
        <skos:prefLabel xml:lang="en">Choriocarcinoma, monophasic</skos:prefLabel>
        <skos:definition xml:lang="en">Testis-Infiltrating malignant neoplasm-Histologic type-Choriocarcinoma, monophasic</skos:definition>
    </owl:Class>
    


    <!-- http://www.semanticweb.org/david/ontologies/2013/0/1.3.6.1.4.1.19376.1.8.2.1.2631 -->

    <owl:Class rdf:about="&pathLex;2631">
        <rdfs:subClassOf rdf:resource="&pathLex;99999"/>
        <skos:prefLabel xml:lang="en">Placental site trophoblastic tumor</skos:prefLabel>
        <skos:definition xml:lang="en">Testis-Infiltrating malignant neoplasm-Histologic type-Placental site trophoblastic tumor</skos:definition>
    </owl:Class>
    


    <!-- http://www.semanticweb.org/david/ontologies/2013/0/1.3.6.1.4.1.19376.1.8.2.1.2632 -->

    <owl:Class rdf:about="&pathLex;2632">
        <rdfs:subClassOf rdf:resource="&pathLex;99999"/>
        <skos:prefLabel xml:lang="en">Teratoma with a secondary somatic-type malignant component (specify type)</skos:prefLabel>
        <skos:definition xml:lang="en">Testis-Infiltrating malignant neoplasm-Histologic type-Teratoma with a secondary somatic-type malignant component (specify type)</skos:definition>
    </owl:Class>
    


    <!-- http://www.semanticweb.org/david/ontologies/2013/0/1.3.6.1.4.1.19376.1.8.2.1.2633 -->

    <owl:Class rdf:about="&pathLex;2633">
        <rdfs:subClassOf rdf:resource="&pathLex;99999"/>
        <skos:prefLabel xml:lang="en">Monodermal teratoma, carcinoid</skos:prefLabel>
        <skos:definition xml:lang="en">Testis-Infiltrating malignant neoplasm-Histologic type-Monodermal teratoma, carcinoid</skos:definition>
    </owl:Class>
    


    <!-- http://www.semanticweb.org/david/ontologies/2013/0/1.3.6.1.4.1.19376.1.8.2.1.2634 -->

    <owl:Class rdf:about="&pathLex;2634">
        <rdfs:subClassOf rdf:resource="&pathLex;99999"/>
        <skos:prefLabel xml:lang="en">Monodermal teratoma, primitive neuroectodermal tumor</skos:prefLabel>
        <skos:definition xml:lang="en">Testis-Infiltrating malignant neoplasm-Histologic type-Monodermal teratoma, primitive neuroectodermal tumor</skos:definition>
    </owl:Class>
    


    <!-- http://www.semanticweb.org/david/ontologies/2013/0/1.3.6.1.4.1.19376.1.8.2.1.2635 -->

    <owl:Class rdf:about="&pathLex;2635">
        <rdfs:subClassOf rdf:resource="&pathLex;99999"/>
        <skos:prefLabel xml:lang="en">Monodermal teratoma, Other</skos:prefLabel>
        <skos:definition xml:lang="en">Testis-Infiltrating malignant neoplasm-Histologic type-Monodermal teratoma, Other</skos:definition>
    </owl:Class>
    


    <!-- http://www.semanticweb.org/david/ontologies/2013/0/1.3.6.1.4.1.19376.1.8.2.1.2636 -->

    <owl:Class rdf:about="&pathLex;2636">
        <rdfs:subClassOf rdf:resource="&pathLex;99999"/>
        <skos:prefLabel xml:lang="en">Spermatocytic seminoma</skos:prefLabel>
        <skos:definition xml:lang="en">Testis-Infiltrating malignant neoplasm-Histologic type-Spermatocytic seminoma</skos:definition>
    </owl:Class>
    


    <!-- http://www.semanticweb.org/david/ontologies/2013/0/1.3.6.1.4.1.19376.1.8.2.1.2637 -->

    <owl:Class rdf:about="&pathLex;2637">
        <rdfs:subClassOf rdf:resource="&pathLex;99999"/>
        <skos:prefLabel xml:lang="en">Spermatocytic seminoma with a sarcomatous component</skos:prefLabel>
        <skos:definition xml:lang="en">Testis-Infiltrating malignant neoplasm-Histologic type-Spermatocytic seminoma with a sarcomatous component</skos:definition>
    </owl:Class>
    


    <!-- http://www.semanticweb.org/david/ontologies/2013/0/1.3.6.1.4.1.19376.1.8.2.1.2638 -->

    <owl:Class rdf:about="&pathLex;2638">
        <rdfs:subClassOf rdf:resource="&pathLex;99999"/>
        <skos:prefLabel xml:lang="en">Mixed germ cell-sex cord-stromal tumor, gonadoblastoma</skos:prefLabel>
        <skos:definition xml:lang="en">Testis-Infiltrating malignant neoplasm-Histologic type-Mixed germ cell-sex cord-stromal tumor, gonadoblastoma</skos:definition>
    </owl:Class>
    


    <!-- http://www.semanticweb.org/david/ontologies/2013/0/1.3.6.1.4.1.19376.1.8.2.1.2639 -->

    <owl:Class rdf:about="&pathLex;2639">
        <rdfs:subClassOf rdf:resource="&pathLex;99999"/>
        <skos:prefLabel xml:lang="en">Mixed germ cell-sex cord-stromal tumor, others (specify)</skos:prefLabel>
        <skos:definition xml:lang="en">Testis-Infiltrating malignant neoplasm-Histologic type-Mixed germ cell-sex cord-stromal tumor, others (specify)</skos:definition>
    </owl:Class>
    


    <!-- http://www.semanticweb.org/david/ontologies/2013/0/1.3.6.1.4.1.19376.1.8.2.1.264 -->

    <owl:Class rdf:about="&pathLex;264">
        <rdfs:subClassOf rdf:resource="&pathLex;99999"/>
        <skos:definition xml:lang="en">Lip, oral cavity-Infiltrating malignant neoplasm-pT mucosal malignant melanoma</skos:definition>
        <skos:prefLabel xml:lang="en">pT mucosal malignant melanoma</skos:prefLabel>
    </owl:Class>
    


    <!-- http://www.semanticweb.org/david/ontologies/2013/0/1.3.6.1.4.1.19376.1.8.2.1.2640 -->

    <owl:Class rdf:about="&pathLex;2640">
        <rdfs:subClassOf rdf:resource="&pathLex;99999"/>
        <skos:prefLabel xml:lang="en">Testicular scar with intratubular germ cell neoplasia</skos:prefLabel>
        <skos:definition xml:lang="en">Testis-Infiltrating malignant neoplasm-Histologic type-Testicular scar with intratubular germ cell neoplasia</skos:definition>
    </owl:Class>
    


    <!-- http://www.semanticweb.org/david/ontologies/2013/0/1.3.6.1.4.1.19376.1.8.2.1.2641 -->

    <owl:Class rdf:about="&pathLex;2641">
        <rdfs:subClassOf rdf:resource="&pathLex;99999"/>
        <skos:prefLabel xml:lang="en">Sex cord-stromal tumor: Leydig cell tumor</skos:prefLabel>
        <skos:definition xml:lang="en">Testis-Infiltrating malignant neoplasm-Histologic type-Sex cord-stromal tumor: Leydig cell tumor</skos:definition>
    </owl:Class>
    


    <!-- http://www.semanticweb.org/david/ontologies/2013/0/1.3.6.1.4.1.19376.1.8.2.1.2642 -->

    <owl:Class rdf:about="&pathLex;2642">
        <rdfs:subClassOf rdf:resource="&pathLex;99999"/>
        <skos:prefLabel xml:lang="en">Sex cord-stromal tumor: Classic Sertoli cell tumor</skos:prefLabel>
        <skos:definition xml:lang="en">Testis-Infiltrating malignant neoplasm-Histologic type-Sex cord-stromal tumor: Classic Sertoli cell tumor</skos:definition>
    </owl:Class>
    


    <!-- http://www.semanticweb.org/david/ontologies/2013/0/1.3.6.1.4.1.19376.1.8.2.1.2643 -->

    <owl:Class rdf:about="&pathLex;2643">
        <rdfs:subClassOf rdf:resource="&pathLex;99999"/>
        <skos:prefLabel xml:lang="en">Sex cord-stromal tumor: Sclerosing Sertoli cell tumor</skos:prefLabel>
        <skos:definition xml:lang="en">Testis-Infiltrating malignant neoplasm-Histologic type-Sex cord-stromal tumor: Sclerosing Sertoli cell tumor</skos:definition>
    </owl:Class>
    


    <!-- http://www.semanticweb.org/david/ontologies/2013/0/1.3.6.1.4.1.19376.1.8.2.1.2644 -->

    <owl:Class rdf:about="&pathLex;2644">
        <rdfs:subClassOf rdf:resource="&pathLex;99999"/>
        <skos:prefLabel xml:lang="en">Sex cord-stromal tumor: Large cell calcifying Sertoli cell tumor</skos:prefLabel>
        <skos:definition xml:lang="en">Testis-Infiltrating malignant neoplasm-Histologic type-Sex cord-stromal tumor: Large cell calcifying Sertoli cell tumor</skos:definition>
    </owl:Class>
    


    <!-- http://www.semanticweb.org/david/ontologies/2013/0/1.3.6.1.4.1.19376.1.8.2.1.2645 -->

    <owl:Class rdf:about="&pathLex;2645">
        <rdfs:subClassOf rdf:resource="&pathLex;99999"/>
        <skos:prefLabel xml:lang="en">Sex cord-stromal tumor: Adult-type Granulosa cell tumor</skos:prefLabel>
        <skos:definition xml:lang="en">Testis-Infiltrating malignant neoplasm-Histologic type-Sex cord-stromal tumor: Adult-type Granulosa cell tumor</skos:definition>
    </owl:Class>
    


    <!-- http://www.semanticweb.org/david/ontologies/2013/0/1.3.6.1.4.1.19376.1.8.2.1.2646 -->

    <owl:Class rdf:about="&pathLex;2646">
        <rdfs:subClassOf rdf:resource="&pathLex;99999"/>
        <skos:prefLabel xml:lang="en">Sex cord-stromal tumor: Juvenile-type Granulosa cell tumor</skos:prefLabel>
        <skos:definition xml:lang="en">Testis-Infiltrating malignant neoplasm-Histologic type-Sex cord-stromal tumor: Juvenile-type Granulosa cell tumor</skos:definition>
    </owl:Class>
    


    <!-- http://www.semanticweb.org/david/ontologies/2013/0/1.3.6.1.4.1.19376.1.8.2.1.2647 -->

    <owl:Class rdf:about="&pathLex;2647">
        <rdfs:subClassOf rdf:resource="&pathLex;99999"/>
        <skos:prefLabel xml:lang="en">Sex cord-stromal tumor: Mixed, with components</skos:prefLabel>
        <skos:definition xml:lang="en">Testis-Infiltrating malignant neoplasm-Histologic type-Sex cord-stromal tumor: Mixed, with components</skos:definition>
    </owl:Class>
    


    <!-- http://www.semanticweb.org/david/ontologies/2013/0/1.3.6.1.4.1.19376.1.8.2.1.2648 -->

    <owl:Class rdf:about="&pathLex;2648">
        <rdfs:subClassOf rdf:resource="&pathLex;99999"/>
        <skos:prefLabel xml:lang="en">Sex cord-stromal tumor: Unclassified</skos:prefLabel>
        <skos:definition xml:lang="en">Testis-Infiltrating malignant neoplasm-Histologic type-Sex cord-stromal tumor: Unclassified</skos:definition>
    </owl:Class>
    


    <!-- http://www.semanticweb.org/david/ontologies/2013/0/1.3.6.1.4.1.19376.1.8.2.1.2649 -->

    <owl:Class rdf:about="&pathLex;2649">
        <rdfs:subClassOf rdf:resource="&pathLex;99999"/>
        <skos:prefLabel xml:lang="en">Malignant neoplasm, type cannot be determined</skos:prefLabel>
        <skos:definition xml:lang="en">Testis-Infiltrating malignant neoplasm-Histologic type-Malignant neoplasm, type cannot be determined</skos:definition>
    </owl:Class>
    


    <!-- http://www.semanticweb.org/david/ontologies/2013/0/1.3.6.1.4.1.19376.1.8.2.1.265 -->

    <owl:Class rdf:about="&pathLex;265">
        <rdfs:subClassOf rdf:resource="&pathLex;99999"/>
        <skos:definition xml:lang="en">Lip, oral cavity-Infiltrating malignant neoplasm-Lymph node metastasis size</skos:definition>
        <skos:prefLabel xml:lang="en">Lymph node metastasis size</skos:prefLabel>
    </owl:Class>
    


    <!-- http://www.semanticweb.org/david/ontologies/2013/0/1.3.6.1.4.1.19376.1.8.2.1.2650 -->

    <owl:Class rdf:about="&pathLex;2650">
        <rdfs:subClassOf rdf:resource="&pathLex;99999"/>
        <skos:prefLabel xml:lang="en">Hemosiderin-laden macrophages</skos:prefLabel>
        <skos:definition xml:lang="en">Testis-Lesion-Histologic type-Hemosiderin-laden macrophages</skos:definition>
    </owl:Class>
    


    <!-- http://www.semanticweb.org/david/ontologies/2013/0/1.3.6.1.4.1.19376.1.8.2.1.2651 -->

    <owl:Class rdf:about="&pathLex;2651">
        <rdfs:subClassOf rdf:resource="&pathLex;99999"/>
        <skos:prefLabel xml:lang="en">Atrophy</skos:prefLabel>
        <skos:definition xml:lang="en">Testis-Lesion-Histologic type-Atrophy</skos:definition>
    </owl:Class>
    


    <!-- http://www.semanticweb.org/david/ontologies/2013/0/1.3.6.1.4.1.19376.1.8.2.1.2652 -->

    <owl:Class rdf:about="&pathLex;2652">
        <rdfs:subClassOf rdf:resource="&pathLex;99999"/>
        <skos:definition xml:lang="en">Urinary bladder-Infiltrating malignant neoplasm-Histologic type-Urothelial (transitional cell) carcinoma with squamous differentiation</skos:definition>
        <skos:prefLabel xml:lang="en">Urothelial (transitional cell) carcinoma with squamous differentiation</skos:prefLabel>
    </owl:Class>
    


    <!-- http://www.semanticweb.org/david/ontologies/2013/0/1.3.6.1.4.1.19376.1.8.2.1.2653 -->

    <owl:Class rdf:about="&pathLex;2653">
        <rdfs:subClassOf rdf:resource="&pathLex;99999"/>
        <skos:definition xml:lang="en">Urinary bladder-Infiltrating malignant neoplasm-Histologic type-Urothelial (transitional cell) carcinoma with glandular differentiation</skos:definition>
        <skos:prefLabel xml:lang="en">Urothelial (transitional cell) carcinoma with glandular differentiation</skos:prefLabel>
    </owl:Class>
    


    <!-- http://www.semanticweb.org/david/ontologies/2013/0/1.3.6.1.4.1.19376.1.8.2.1.2654 -->

    <owl:Class rdf:about="&pathLex;2654">
        <rdfs:subClassOf rdf:resource="&pathLex;99999"/>
        <skos:definition xml:lang="en">Urinary bladder-Infiltrating malignant neoplasm-Histologic type-Urothelial (transitional cell) carcinoma with variant histology - Specify</skos:definition>
        <skos:prefLabel xml:lang="en">Urothelial (transitional cell) carcinoma with variant histology - Specify</skos:prefLabel>
    </owl:Class>
    


    <!-- http://www.semanticweb.org/david/ontologies/2013/0/1.3.6.1.4.1.19376.1.8.2.1.2655 -->

    <owl:Class rdf:about="&pathLex;2655">
        <rdfs:subClassOf rdf:resource="&pathLex;99999"/>
        <skos:prefLabel xml:lang="en">Squamous cell carcinoma, typical</skos:prefLabel>
        <skos:definition xml:lang="en">Urinary bladder-Infiltrating malignant neoplasm-Histologic type-Squamous cell carcinoma, typical</skos:definition>
    </owl:Class>
    


    <!-- http://www.semanticweb.org/david/ontologies/2013/0/1.3.6.1.4.1.19376.1.8.2.1.2656 -->

    <owl:Class rdf:about="&pathLex;2656">
        <rdfs:subClassOf rdf:resource="&pathLex;99999"/>
        <skos:prefLabel xml:lang="en">Squamous cell carcinoma, variant histology - Specify</skos:prefLabel>
        <skos:definition xml:lang="en">Urinary bladder-Infiltrating malignant neoplasm-Histologic type-Squamous cell carcinoma, variant histology - Specify</skos:definition>
    </owl:Class>
    


    <!-- http://www.semanticweb.org/david/ontologies/2013/0/1.3.6.1.4.1.19376.1.8.2.1.2657 -->

    <owl:Class rdf:about="&pathLex;2657">
        <rdfs:subClassOf rdf:resource="&pathLex;99999"/>
        <skos:prefLabel xml:lang="en">Adenocarcinoma, typical</skos:prefLabel>
        <skos:definition xml:lang="en">Urinary bladder-Infiltrating malignant neoplasm-Histologic type-Adenocarcinoma, typical</skos:definition>
    </owl:Class>
    


    <!-- http://www.semanticweb.org/david/ontologies/2013/0/1.3.6.1.4.1.19376.1.8.2.1.2658 -->

    <owl:Class rdf:about="&pathLex;2658">
        <rdfs:subClassOf rdf:resource="&pathLex;99999"/>
        <skos:prefLabel xml:lang="en">Adenocarcinoma, variant histology - Specify</skos:prefLabel>
        <skos:definition xml:lang="en">Urinary bladder-Infiltrating malignant neoplasm-Histologic type-Adenocarcinoma, variant histology - Specify</skos:definition>
    </owl:Class>
    


    <!-- http://www.semanticweb.org/david/ontologies/2013/0/1.3.6.1.4.1.19376.1.8.2.1.2659 -->

    <owl:Class rdf:about="&pathLex;2659">
        <rdfs:subClassOf rdf:resource="&pathLex;99999"/>
        <skos:prefLabel xml:lang="en">Undifferentiated carcinoma - Specify</skos:prefLabel>
        <skos:definition xml:lang="en">Urinary bladder-Infiltrating malignant neoplasm-Histologic type-Undifferentiated carcinoma - Specify</skos:definition>
    </owl:Class>
    


    <!-- http://www.semanticweb.org/david/ontologies/2013/0/1.3.6.1.4.1.19376.1.8.2.1.266 -->

    <owl:Class rdf:about="&pathLex;266">
        <rdfs:subClassOf rdf:resource="&pathLex;99999"/>
        <skos:prefLabel xml:lang="en">Lesion size, largest dimension</skos:prefLabel>
        <skos:definition xml:lang="en">Lip, oral cavity-Infiltrating malignant neoplasm-Lesion size, largest dimension</skos:definition>
    </owl:Class>
    


    <!-- http://www.semanticweb.org/david/ontologies/2013/0/1.3.6.1.4.1.19376.1.8.2.1.2660 -->

    <owl:Class rdf:about="&pathLex;2660">
        <rdfs:subClassOf rdf:resource="&pathLex;99999"/>
        <skos:prefLabel xml:lang="en">Mixed cell type - Specify</skos:prefLabel>
        <skos:definition xml:lang="en">Urinary bladder-Infiltrating malignant neoplasm-Histologic type-Mixed cell type - Specify</skos:definition>
    </owl:Class>
    


    <!-- http://www.semanticweb.org/david/ontologies/2013/0/1.3.6.1.4.1.19376.1.8.2.1.2661 -->

    <owl:Class rdf:about="&pathLex;2661">
        <rdfs:subClassOf rdf:resource="&pathLex;99999"/>
        <skos:prefLabel xml:lang="en">Chronic pancreatitis</skos:prefLabel>
        <skos:definition xml:lang="en">Pancreas-Lesion-Histologic type-Chronic pancreatitis</skos:definition>
    </owl:Class>
    


    <!-- http://www.semanticweb.org/david/ontologies/2013/0/1.3.6.1.4.1.19376.1.8.2.1.2662 -->

    <owl:Class rdf:about="&pathLex;2662">
        <rdfs:subClassOf rdf:resource="&pathLex;99999"/>
        <skos:prefLabel xml:lang="en">Acute pancreatitis</skos:prefLabel>
        <skos:definition xml:lang="en">Pancreas-Lesion-Histologic type-Acute pancreatitis</skos:definition>
    </owl:Class>
    


    <!-- http://www.semanticweb.org/david/ontologies/2013/0/1.3.6.1.4.1.19376.1.8.2.1.267 -->

    <owl:Class rdf:about="&pathLex;267">
        <rdfs:subClassOf rdf:resource="&pathLex;99999"/>
        <skos:definition xml:lang="en">Lip, oral cavity-Infiltrating malignant neoplasm-Specimen size, largest dimension</skos:definition>
        <skos:prefLabel xml:lang="en">Specimen size, largest dimension</skos:prefLabel>
    </owl:Class>
    


    <!-- http://www.semanticweb.org/david/ontologies/2013/0/1.3.6.1.4.1.19376.1.8.2.1.268 -->

    <owl:Class rdf:about="&pathLex;268">
        <rdfs:subClassOf rdf:resource="&pathLex;99999"/>
        <skos:prefLabel xml:lang="en">Histologic type</skos:prefLabel>
        <skos:definition xml:lang="en">Lip, oral cavity-Infiltrating malignant neoplasm-Histologic type</skos:definition>
    </owl:Class>
    


    <!-- http://www.semanticweb.org/david/ontologies/2013/0/1.3.6.1.4.1.19376.1.8.2.1.269 -->

    <owl:Class rdf:about="&pathLex;269">
        <rdfs:subClassOf rdf:resource="&pathLex;99999"/>
        <skos:prefLabel xml:lang="en">Margins involvement</skos:prefLabel>
        <skos:definition xml:lang="en">Skin (melanoma)-Infiltrating malignant neoplasm-Margins involvement</skos:definition>
    </owl:Class>
    


    <!-- http://www.semanticweb.org/david/ontologies/2013/0/1.3.6.1.4.1.19376.1.8.2.1.270 -->

    <owl:Class rdf:about="&pathLex;270">
        <rdfs:subClassOf rdf:resource="&pathLex;99999"/>
        <skos:definition xml:lang="en">Esophagus-Infiltrating malignant neoplasm-Margins involvement</skos:definition>
        <skos:prefLabel xml:lang="en">Margins involvement</skos:prefLabel>
    </owl:Class>
    


    <!-- http://www.semanticweb.org/david/ontologies/2013/0/1.3.6.1.4.1.19376.1.8.2.1.271 -->

    <owl:Class rdf:about="&pathLex;271">
        <rdfs:subClassOf rdf:resource="&pathLex;99999"/>
        <skos:prefLabel xml:lang="en">Distance of lesion from closest uninvolved margin</skos:prefLabel>
        <skos:definition xml:lang="en">Esophagus-Infiltrating malignant neoplasm-Distance of lesion from closest uninvolved margin</skos:definition>
    </owl:Class>
    


    <!-- http://www.semanticweb.org/david/ontologies/2013/0/1.3.6.1.4.1.19376.1.8.2.1.272 -->

    <owl:Class rdf:about="&pathLex;272">
        <rdfs:subClassOf rdf:resource="&pathLex;99999"/>
        <skos:definition xml:lang="en">Esophagus-Infiltrating malignant neoplasm-Lymph-vascular invasion</skos:definition>
        <skos:prefLabel xml:lang="en">Lymph-vascular invasion</skos:prefLabel>
    </owl:Class>
    


    <!-- http://www.semanticweb.org/david/ontologies/2013/0/1.3.6.1.4.1.19376.1.8.2.1.273 -->

    <owl:Class rdf:about="&pathLex;273">
        <rdfs:subClassOf rdf:resource="&pathLex;99999"/>
        <skos:definition xml:lang="en">Esophagus-Infiltrating malignant neoplasm-Extent</skos:definition>
        <skos:prefLabel xml:lang="en">Extent</skos:prefLabel>
    </owl:Class>
    


    <!-- http://www.semanticweb.org/david/ontologies/2013/0/1.3.6.1.4.1.19376.1.8.2.1.274 -->

    <owl:Class rdf:about="&pathLex;274">
        <rdfs:subClassOf rdf:resource="&pathLex;99999"/>
        <skos:definition xml:lang="en">Esophagus-Infiltrating malignant neoplasm-Perineural invasion</skos:definition>
        <skos:prefLabel xml:lang="en">Perineural invasion</skos:prefLabel>
    </owl:Class>
    


    <!-- http://www.semanticweb.org/david/ontologies/2013/0/1.3.6.1.4.1.19376.1.8.2.1.275 -->

    <owl:Class rdf:about="&pathLex;275">
        <rdfs:subClassOf rdf:resource="&pathLex;99999"/>
        <skos:definition xml:lang="en">Esophagus-Infiltrating malignant neoplasm-Lesion site</skos:definition>
        <skos:prefLabel xml:lang="en">Lesion site</skos:prefLabel>
    </owl:Class>
    


    <!-- http://www.semanticweb.org/david/ontologies/2013/0/1.3.6.1.4.1.19376.1.8.2.1.276 -->

    <owl:Class rdf:about="&pathLex;276">
        <rdfs:subClassOf rdf:resource="&pathLex;99999"/>
        <skos:definition xml:lang="en">Esophagus-Infiltrating malignant neoplasm-Margin site</skos:definition>
        <skos:prefLabel xml:lang="en">Margin site</skos:prefLabel>
    </owl:Class>
    


    <!-- http://www.semanticweb.org/david/ontologies/2013/0/1.3.6.1.4.1.19376.1.8.2.1.277 -->

    <owl:Class rdf:about="&pathLex;277">
        <rdfs:subClassOf rdf:resource="&pathLex;99999"/>
        <skos:definition xml:lang="en">Esophagus-Infiltrating malignant neoplasm-Number of lymph nodes involved</skos:definition>
        <skos:prefLabel xml:lang="en">Number of lymph nodes involved</skos:prefLabel>
    </owl:Class>
    


    <!-- http://www.semanticweb.org/david/ontologies/2013/0/1.3.6.1.4.1.19376.1.8.2.1.278 -->

    <owl:Class rdf:about="&pathLex;278">
        <rdfs:subClassOf rdf:resource="&pathLex;99999"/>
        <skos:definition xml:lang="en">Esophagus-Infiltrating malignant neoplasm-Number of lymph nodes examined</skos:definition>
        <skos:prefLabel xml:lang="en">Number of lymph nodes examined</skos:prefLabel>
    </owl:Class>
    


    <!-- http://www.semanticweb.org/david/ontologies/2013/0/1.3.6.1.4.1.19376.1.8.2.1.280 -->

    <owl:Class rdf:about="&pathLex;280">
        <rdfs:subClassOf rdf:resource="&pathLex;99999"/>
        <skos:definition xml:lang="en">Esophagus-Infiltrating malignant neoplasm-pN</skos:definition>
        <skos:prefLabel xml:lang="en">pN</skos:prefLabel>
    </owl:Class>
    


    <!-- http://www.semanticweb.org/david/ontologies/2013/0/1.3.6.1.4.1.19376.1.8.2.1.282 -->

    <owl:Class rdf:about="&pathLex;282">
        <rdfs:subClassOf rdf:resource="&pathLex;99999"/>
        <skos:definition xml:lang="en">Esophagus-Infiltrating malignant neoplasm-pT</skos:definition>
        <skos:prefLabel xml:lang="en">pT</skos:prefLabel>
    </owl:Class>
    


    <!-- http://www.semanticweb.org/david/ontologies/2013/0/1.3.6.1.4.1.19376.1.8.2.1.283 -->

    <owl:Class rdf:about="&pathLex;283">
        <rdfs:subClassOf rdf:resource="&pathLex;99999"/>
        <skos:definition xml:lang="en">Esophagus-Infiltrating malignant neoplasm-Lesion size, largest dimension</skos:definition>
        <skos:prefLabel xml:lang="en">Lesion size, largest dimension</skos:prefLabel>
    </owl:Class>
    


    <!-- http://www.semanticweb.org/david/ontologies/2013/0/1.3.6.1.4.1.19376.1.8.2.1.284 -->

    <owl:Class rdf:about="&pathLex;284">
        <rdfs:subClassOf rdf:resource="&pathLex;99999"/>
        <skos:definition xml:lang="en">Esophagus-Infiltrating malignant neoplasm-Histologic type</skos:definition>
        <skos:prefLabel xml:lang="en">Histologic type</skos:prefLabel>
    </owl:Class>
    


    <!-- http://www.semanticweb.org/david/ontologies/2013/0/1.3.6.1.4.1.19376.1.8.2.1.285 -->

    <owl:Class rdf:about="&pathLex;285">
        <rdfs:subClassOf rdf:resource="&pathLex;99999"/>
        <skos:prefLabel xml:lang="en">Extent</skos:prefLabel>
        <skos:definition xml:lang="en">Ovary-Infiltrating malignant neoplasm-Extent</skos:definition>
    </owl:Class>
    


    <!-- http://www.semanticweb.org/david/ontologies/2013/0/1.3.6.1.4.1.19376.1.8.2.1.286 -->

    <owl:Class rdf:about="&pathLex;286">
        <rdfs:subClassOf rdf:resource="&pathLex;99999"/>
        <skos:prefLabel xml:lang="en">Histologic grade of ovary mucinous carcinoma</skos:prefLabel>
        <skos:definition xml:lang="en">Ovary-Infiltrating malignant neoplasm-Histologic grade of ovary mucinous carcinoma</skos:definition>
    </owl:Class>
    


    <!-- http://www.semanticweb.org/david/ontologies/2013/0/1.3.6.1.4.1.19376.1.8.2.1.287 -->

    <owl:Class rdf:about="&pathLex;287">
        <rdfs:subClassOf rdf:resource="&pathLex;99999"/>
        <skos:prefLabel xml:lang="en">Histologic grade (FIGO)</skos:prefLabel>
        <skos:definition xml:lang="en">Ovary-Infiltrating malignant neoplasm-Histologic grade (FIGO)</skos:definition>
    </owl:Class>
    


    <!-- http://www.semanticweb.org/david/ontologies/2013/0/1.3.6.1.4.1.19376.1.8.2.1.288 -->

    <owl:Class rdf:about="&pathLex;288">
        <rdfs:subClassOf rdf:resource="&pathLex;99999"/>
        <skos:prefLabel xml:lang="en">Histologic grade of ovarry immature teratoma</skos:prefLabel>
        <skos:definition xml:lang="en">Ovary-Infiltrating malignant neoplasm-Histologic grade of ovarry immature teratoma</skos:definition>
    </owl:Class>
    


    <!-- http://www.semanticweb.org/david/ontologies/2013/0/1.3.6.1.4.1.19376.1.8.2.1.289 -->

    <owl:Class rdf:about="&pathLex;289">
        <rdfs:subClassOf rdf:resource="&pathLex;99999"/>
        <skos:prefLabel xml:lang="en">Lymph node site</skos:prefLabel>
        <skos:definition xml:lang="en">Ovary-Infiltrating malignant neoplasm-Lymph node site</skos:definition>
    </owl:Class>
    


    <!-- http://www.semanticweb.org/david/ontologies/2013/0/1.3.6.1.4.1.19376.1.8.2.1.291 -->

    <owl:Class rdf:about="&pathLex;291">
        <rdfs:subClassOf rdf:resource="&pathLex;99999"/>
        <skos:definition xml:lang="en">Ovary-Infiltrating malignant neoplasm-pN</skos:definition>
        <skos:prefLabel xml:lang="en">pN</skos:prefLabel>
    </owl:Class>
    


    <!-- http://www.semanticweb.org/david/ontologies/2013/0/1.3.6.1.4.1.19376.1.8.2.1.293 -->

    <owl:Class rdf:about="&pathLex;293">
        <rdfs:subClassOf rdf:resource="&pathLex;99999"/>
        <skos:definition xml:lang="en">Ovary-Infiltrating malignant neoplasm-pT</skos:definition>
        <skos:prefLabel xml:lang="en">pT</skos:prefLabel>
    </owl:Class>
    


    <!-- http://www.semanticweb.org/david/ontologies/2013/0/1.3.6.1.4.1.19376.1.8.2.1.294 -->

    <owl:Class rdf:about="&pathLex;294">
        <rdfs:subClassOf rdf:resource="&pathLex;99999"/>
        <skos:prefLabel xml:lang="en">Lymph-vascular invasion</skos:prefLabel>
        <skos:definition xml:lang="en">Ovary-Infiltrating malignant neoplasm-Lymph-vascular invasion</skos:definition>
    </owl:Class>
    


    <!-- http://www.semanticweb.org/david/ontologies/2013/0/1.3.6.1.4.1.19376.1.8.2.1.295 -->

    <owl:Class rdf:about="&pathLex;295">
        <rdfs:subClassOf rdf:resource="&pathLex;99999"/>
        <skos:prefLabel xml:lang="en">Lymph node sampling</skos:prefLabel>
        <skos:definition xml:lang="en">Ovary-Infiltrating malignant neoplasm-Lymph node sampling</skos:definition>
    </owl:Class>
    


    <!-- http://www.semanticweb.org/david/ontologies/2013/0/1.3.6.1.4.1.19376.1.8.2.1.296 -->

    <owl:Class rdf:about="&pathLex;296">
        <rdfs:subClassOf rdf:resource="&pathLex;99999"/>
        <skos:prefLabel xml:lang="en">Number of lymph nodes involved</skos:prefLabel>
        <skos:definition xml:lang="en">Ovary-Infiltrating malignant neoplasm-Number of lymph nodes involved</skos:definition>
    </owl:Class>
    


    <!-- http://www.semanticweb.org/david/ontologies/2013/0/1.3.6.1.4.1.19376.1.8.2.1.297 -->

    <owl:Class rdf:about="&pathLex;297">
        <rdfs:subClassOf rdf:resource="&pathLex;99999"/>
        <skos:prefLabel xml:lang="en">Number of lymph nodes examined</skos:prefLabel>
        <skos:definition xml:lang="en">Ovary-Infiltrating malignant neoplasm-Number of lymph nodes examined</skos:definition>
    </owl:Class>
    


    <!-- http://www.semanticweb.org/david/ontologies/2013/0/1.3.6.1.4.1.19376.1.8.2.1.298 -->

    <owl:Class rdf:about="&pathLex;298">
        <rdfs:subClassOf rdf:resource="&pathLex;99999"/>
        <skos:prefLabel xml:lang="en">Lesion size, largest dimension</skos:prefLabel>
        <skos:definition xml:lang="en">Ovary-Infiltrating malignant neoplasm-Lesion size, largest dimension</skos:definition>
    </owl:Class>
    


    <!-- http://www.semanticweb.org/david/ontologies/2013/0/1.3.6.1.4.1.19376.1.8.2.1.299 -->

    <owl:Class rdf:about="&pathLex;299">
        <rdfs:subClassOf rdf:resource="&pathLex;99999"/>
        <skos:prefLabel xml:lang="en">Histologic type</skos:prefLabel>
        <skos:definition xml:lang="en">Ovary-Infiltrating malignant neoplasm-Histologic type</skos:definition>
    </owl:Class>
    


    <!-- http://www.semanticweb.org/david/ontologies/2013/0/1.3.6.1.4.1.19376.1.8.2.1.3 -->

    <owl:Class rdf:about="&pathLex;3">
        <rdfs:subClassOf rdf:resource="&pathLex;99999"/>
        <skos:definition xml:lang="en">Generic-Infiltrating malignant neoplasm-Specimen size, additional dimension</skos:definition>
        <skos:prefLabel xml:lang="en">Specimen size, additional dimension</skos:prefLabel>
    </owl:Class>
    


    <!-- http://www.semanticweb.org/david/ontologies/2013/0/1.3.6.1.4.1.19376.1.8.2.1.300 -->

    <owl:Class rdf:about="&pathLex;300">
        <rdfs:subClassOf rdf:resource="&pathLex;99999"/>
        <skos:prefLabel xml:lang="en">Margins involvement</skos:prefLabel>
        <skos:definition xml:lang="en">Pancreas-Infiltrating malignant neoplasm-Margins involvement</skos:definition>
    </owl:Class>
    


    <!-- http://www.semanticweb.org/david/ontologies/2013/0/1.3.6.1.4.1.19376.1.8.2.1.301 -->

    <owl:Class rdf:about="&pathLex;301">
        <rdfs:subClassOf rdf:resource="&pathLex;99999"/>
        <skos:prefLabel xml:lang="en">Margins involvement</skos:prefLabel>
        <skos:definition xml:lang="en">Pancreas-Infiltrating malignant neoplasm-Margins involvement</skos:definition>
    </owl:Class>
    


    <!-- http://www.semanticweb.org/david/ontologies/2013/0/1.3.6.1.4.1.19376.1.8.2.1.302 -->

    <owl:Class rdf:about="&pathLex;302">
        <rdfs:subClassOf rdf:resource="&pathLex;99999"/>
        <skos:prefLabel xml:lang="en">Distance of lesion from closest uninvolved margin</skos:prefLabel>
        <skos:definition xml:lang="en">Pancreas-Infiltrating malignant neoplasm-Distance of lesion from closest uninvolved margin</skos:definition>
    </owl:Class>
    


    <!-- http://www.semanticweb.org/david/ontologies/2013/0/1.3.6.1.4.1.19376.1.8.2.1.303 -->

    <owl:Class rdf:about="&pathLex;303">
        <rdfs:subClassOf rdf:resource="&pathLex;99999"/>
        <skos:prefLabel xml:lang="en">Lymph-vascular invasion</skos:prefLabel>
        <skos:definition xml:lang="en">Pancreas-Infiltrating malignant neoplasm-Lymph-vascular invasion</skos:definition>
    </owl:Class>
    


    <!-- http://www.semanticweb.org/david/ontologies/2013/0/1.3.6.1.4.1.19376.1.8.2.1.304 -->

    <owl:Class rdf:about="&pathLex;304">
        <rdfs:subClassOf rdf:resource="&pathLex;99999"/>
        <skos:prefLabel xml:lang="en">Extent</skos:prefLabel>
        <skos:definition xml:lang="en">Pancreas-Infiltrating malignant neoplasm-Extent</skos:definition>
    </owl:Class>
    


    <!-- http://www.semanticweb.org/david/ontologies/2013/0/1.3.6.1.4.1.19376.1.8.2.1.305 -->

    <owl:Class rdf:about="&pathLex;305">
        <rdfs:subClassOf rdf:resource="&pathLex;99999"/>
        <skos:definition xml:lang="en">Pancreas-Infiltrating malignant neoplasm-Perineural invasion</skos:definition>
        <skos:prefLabel xml:lang="en">Perineural invasion</skos:prefLabel>
    </owl:Class>
    


    <!-- http://www.semanticweb.org/david/ontologies/2013/0/1.3.6.1.4.1.19376.1.8.2.1.306 -->

    <owl:Class rdf:about="&pathLex;306">
        <rdfs:subClassOf rdf:resource="&pathLex;99999"/>
        <skos:prefLabel xml:lang="en">Lesion site</skos:prefLabel>
        <skos:definition xml:lang="en">Pancreas-Infiltrating malignant neoplasm-Lesion site</skos:definition>
    </owl:Class>
    


    <!-- http://www.semanticweb.org/david/ontologies/2013/0/1.3.6.1.4.1.19376.1.8.2.1.307 -->

    <owl:Class rdf:about="&pathLex;307">
        <rdfs:subClassOf rdf:resource="&pathLex;99999"/>
        <skos:prefLabel xml:lang="en">Margin site</skos:prefLabel>
        <skos:definition xml:lang="en">Pancreas-Infiltrating malignant neoplasm-Margin site</skos:definition>
    </owl:Class>
    


    <!-- http://www.semanticweb.org/david/ontologies/2013/0/1.3.6.1.4.1.19376.1.8.2.1.308 -->

    <owl:Class rdf:about="&pathLex;308">
        <rdfs:subClassOf rdf:resource="&pathLex;99999"/>
        <skos:prefLabel xml:lang="en">Number of lymph nodes involved</skos:prefLabel>
        <skos:definition xml:lang="en">Pancreas-Infiltrating malignant neoplasm-Number of lymph nodes involved</skos:definition>
    </owl:Class>
    


    <!-- http://www.semanticweb.org/david/ontologies/2013/0/1.3.6.1.4.1.19376.1.8.2.1.309 -->

    <owl:Class rdf:about="&pathLex;309">
        <rdfs:subClassOf rdf:resource="&pathLex;99999"/>
        <skos:prefLabel xml:lang="en">Number of lymph nodes examined</skos:prefLabel>
        <skos:definition xml:lang="en">Pancreas-Infiltrating malignant neoplasm-Number of lymph nodes examined</skos:definition>
    </owl:Class>
    


    <!-- http://www.semanticweb.org/david/ontologies/2013/0/1.3.6.1.4.1.19376.1.8.2.1.31 -->

    <owl:Class rdf:about="&pathLex;31">
        <rdfs:subClassOf rdf:resource="&pathLex;10005"/>
        <skos:definition xml:lang="en">Generic-Infiltrating malignant neoplasm-Histologic grade (WHO)</skos:definition>
        <skos:prefLabel xml:lang="en">Histologic grade (WHO)</skos:prefLabel>
    </owl:Class>
    


    <!-- http://www.semanticweb.org/david/ontologies/2013/0/1.3.6.1.4.1.19376.1.8.2.1.311 -->

    <owl:Class rdf:about="&pathLex;311">
        <rdfs:subClassOf rdf:resource="&pathLex;99999"/>
        <skos:definition xml:lang="en">Pancreas-Infiltrating malignant neoplasm-pN</skos:definition>
        <skos:prefLabel xml:lang="en">pN</skos:prefLabel>
    </owl:Class>
    


    <!-- http://www.semanticweb.org/david/ontologies/2013/0/1.3.6.1.4.1.19376.1.8.2.1.313 -->

    <owl:Class rdf:about="&pathLex;313">
        <rdfs:subClassOf rdf:resource="&pathLex;99999"/>
        <skos:definition xml:lang="en">Pancreas-Infiltrating malignant neoplasm-pT</skos:definition>
        <skos:prefLabel xml:lang="en">pT</skos:prefLabel>
    </owl:Class>
    


    <!-- http://www.semanticweb.org/david/ontologies/2013/0/1.3.6.1.4.1.19376.1.8.2.1.314 -->

    <owl:Class rdf:about="&pathLex;314">
        <rdfs:subClassOf rdf:resource="&pathLex;99999"/>
        <skos:prefLabel xml:lang="en">Lesion size, largest dimension</skos:prefLabel>
        <skos:definition xml:lang="en">Pancreas-Infiltrating malignant neoplasm-Lesion size, largest dimension</skos:definition>
    </owl:Class>
    


    <!-- http://www.semanticweb.org/david/ontologies/2013/0/1.3.6.1.4.1.19376.1.8.2.1.315 -->

    <owl:Class rdf:about="&pathLex;315">
        <rdfs:subClassOf rdf:resource="&pathLex;99999"/>
        <skos:prefLabel xml:lang="en">Histologic type</skos:prefLabel>
        <skos:definition xml:lang="en">Pancreas-Infiltrating malignant neoplasm-Histologic type</skos:definition>
    </owl:Class>
    


    <!-- http://www.semanticweb.org/david/ontologies/2013/0/1.3.6.1.4.1.19376.1.8.2.1.316 -->

    <owl:Class rdf:about="&pathLex;316">
        <rdfs:subClassOf rdf:resource="&pathLex;99999"/>
        <skos:prefLabel xml:lang="en">Margins involvement</skos:prefLabel>
        <skos:definition xml:lang="en">Skin (melanoma)-Infiltrating malignant neoplasm-Margins involvement</skos:definition>
    </owl:Class>
    


    <!-- http://www.semanticweb.org/david/ontologies/2013/0/1.3.6.1.4.1.19376.1.8.2.1.317 -->

    <owl:Class rdf:about="&pathLex;317">
        <rdfs:subClassOf rdf:resource="&pathLex;99999"/>
        <skos:prefLabel xml:lang="en">Distance of lesion from closest uninvolved margin</skos:prefLabel>
        <skos:definition xml:lang="en">Skin (melanoma)-Infiltrating malignant neoplasm-Distance of lesion from closest uninvolved margin</skos:definition>
    </owl:Class>
    


    <!-- http://www.semanticweb.org/david/ontologies/2013/0/1.3.6.1.4.1.19376.1.8.2.1.318 -->

    <owl:Class rdf:about="&pathLex;318">
        <rdfs:subClassOf rdf:resource="&pathLex;99999"/>
        <skos:prefLabel xml:lang="en">Lymph-vascular invasion</skos:prefLabel>
        <skos:definition xml:lang="en">Skin (melanoma)-Infiltrating malignant neoplasm-Lymph-vascular invasion</skos:definition>
    </owl:Class>
    


    <!-- http://www.semanticweb.org/david/ontologies/2013/0/1.3.6.1.4.1.19376.1.8.2.1.319 -->

    <owl:Class rdf:about="&pathLex;319">
        <rdfs:subClassOf rdf:resource="&pathLex;99999"/>
        <skos:prefLabel xml:lang="en">Lymph node sampling</skos:prefLabel>
        <skos:definition xml:lang="en">Skin (melanoma)-Infiltrating malignant neoplasm-Lymph node sampling</skos:definition>
    </owl:Class>
    


    <!-- http://www.semanticweb.org/david/ontologies/2013/0/1.3.6.1.4.1.19376.1.8.2.1.320 -->

    <owl:Class rdf:about="&pathLex;320">
        <rdfs:subClassOf rdf:resource="&pathLex;99999"/>
        <skos:prefLabel xml:lang="en">Perineural invasion</skos:prefLabel>
        <skos:definition xml:lang="en">Skin (melanoma)-Infiltrating malignant neoplasm-Perineural invasion</skos:definition>
    </owl:Class>
    


    <!-- http://www.semanticweb.org/david/ontologies/2013/0/1.3.6.1.4.1.19376.1.8.2.1.321 -->

    <owl:Class rdf:about="&pathLex;321">
        <rdfs:subClassOf rdf:resource="&pathLex;99999"/>
        <skos:prefLabel xml:lang="en">Lymph node capsule involvement</skos:prefLabel>
        <skos:definition xml:lang="en">Skin (melanoma)-Infiltrating malignant neoplasm-Lymph node capsule involvement</skos:definition>
    </owl:Class>
    


    <!-- http://www.semanticweb.org/david/ontologies/2013/0/1.3.6.1.4.1.19376.1.8.2.1.322 -->

    <owl:Class rdf:about="&pathLex;322">
        <rdfs:subClassOf rdf:resource="&pathLex;99999"/>
        <skos:prefLabel xml:lang="en">Lesion site</skos:prefLabel>
        <skos:definition xml:lang="en">Skin (melanoma)-Infiltrating malignant neoplasm-Lesion site</skos:definition>
    </owl:Class>
    


    <!-- http://www.semanticweb.org/david/ontologies/2013/0/1.3.6.1.4.1.19376.1.8.2.1.323 -->

    <owl:Class rdf:about="&pathLex;323">
        <rdfs:subClassOf rdf:resource="&pathLex;99999"/>
        <skos:prefLabel xml:lang="en">Margin site</skos:prefLabel>
        <skos:definition xml:lang="en">Skin (melanoma)-Infiltrating malignant neoplasm-Margin site</skos:definition>
    </owl:Class>
    


    <!-- http://www.semanticweb.org/david/ontologies/2013/0/1.3.6.1.4.1.19376.1.8.2.1.324 -->

    <owl:Class rdf:about="&pathLex;324">
        <rdfs:subClassOf rdf:resource="&pathLex;99999"/>
        <skos:prefLabel xml:lang="en">Number of lymph nodes involved</skos:prefLabel>
        <skos:definition xml:lang="en">Skin (melanoma)-Infiltrating malignant neoplasm-Number of lymph nodes involved</skos:definition>
    </owl:Class>
    


    <!-- http://www.semanticweb.org/david/ontologies/2013/0/1.3.6.1.4.1.19376.1.8.2.1.325 -->

    <owl:Class rdf:about="&pathLex;325">
        <rdfs:subClassOf rdf:resource="&pathLex;99999"/>
        <skos:prefLabel xml:lang="en">Number of lymph nodes examined</skos:prefLabel>
        <skos:definition xml:lang="en">Skin (melanoma)-Infiltrating malignant neoplasm-Number of lymph nodes examined</skos:definition>
    </owl:Class>
    


    <!-- http://www.semanticweb.org/david/ontologies/2013/0/1.3.6.1.4.1.19376.1.8.2.1.327 -->

    <owl:Class rdf:about="&pathLex;327">
        <rdfs:subClassOf rdf:resource="&pathLex;99999"/>
        <skos:definition xml:lang="en">Skin (melanoma)-Infiltrating malignant neoplasm-pN</skos:definition>
        <skos:prefLabel xml:lang="en">pN</skos:prefLabel>
    </owl:Class>
    


    <!-- http://www.semanticweb.org/david/ontologies/2013/0/1.3.6.1.4.1.19376.1.8.2.1.329 -->

    <owl:Class rdf:about="&pathLex;329">
        <rdfs:subClassOf rdf:resource="&pathLex;99999"/>
        <skos:definition xml:lang="en">Skin (melanoma)-Infiltrating malignant neoplasm-pT</skos:definition>
        <skos:prefLabel xml:lang="en">pT</skos:prefLabel>
    </owl:Class>
    


    <!-- http://www.semanticweb.org/david/ontologies/2013/0/1.3.6.1.4.1.19376.1.8.2.1.330 -->

    <owl:Class rdf:about="&pathLex;330">
        <rdfs:subClassOf rdf:resource="&pathLex;99999"/>
        <skos:prefLabel xml:lang="en">Lymph node metastasis size</skos:prefLabel>
        <skos:definition xml:lang="en">Skin (melanoma)-Infiltrating malignant neoplasm-Lymph node metastasis size</skos:definition>
    </owl:Class>
    


    <!-- http://www.semanticweb.org/david/ontologies/2013/0/1.3.6.1.4.1.19376.1.8.2.1.331 -->

    <owl:Class rdf:about="&pathLex;331">
        <rdfs:subClassOf rdf:resource="&pathLex;99999"/>
        <skos:prefLabel xml:lang="en">Lesion size, largest dimension</skos:prefLabel>
        <skos:definition xml:lang="en">Skin (melanoma)-Infiltrating malignant neoplasm-Lesion size, largest dimension</skos:definition>
    </owl:Class>
    


    <!-- http://www.semanticweb.org/david/ontologies/2013/0/1.3.6.1.4.1.19376.1.8.2.1.332 -->

    <owl:Class rdf:about="&pathLex;332">
        <rdfs:subClassOf rdf:resource="&pathLex;99999"/>
        <skos:definition xml:lang="en">Skin (melanoma)-Infiltrating malignant neoplasm-Specimen size, largest dimension</skos:definition>
        <skos:prefLabel xml:lang="en">Specimen size, largest dimension</skos:prefLabel>
    </owl:Class>
    


    <!-- http://www.semanticweb.org/david/ontologies/2013/0/1.3.6.1.4.1.19376.1.8.2.1.333 -->

    <owl:Class rdf:about="&pathLex;333">
        <rdfs:subClassOf rdf:resource="&pathLex;99999"/>
        <skos:prefLabel xml:lang="en">Histologic type</skos:prefLabel>
        <skos:definition xml:lang="en">Skin (melanoma)-Infiltrating malignant neoplasm-Histologic type</skos:definition>
    </owl:Class>
    


    <!-- http://www.semanticweb.org/david/ontologies/2013/0/1.3.6.1.4.1.19376.1.8.2.1.334 -->

    <owl:Class rdf:about="&pathLex;334">
        <rdfs:subClassOf rdf:resource="&pathLex;99999"/>
        <skos:prefLabel xml:lang="en">Lesion ulceration</skos:prefLabel>
        <skos:definition xml:lang="en">Skin (melanoma)-Infiltrating malignant neoplasm-Lesion ulceration</skos:definition>
    </owl:Class>
    


    <!-- http://www.semanticweb.org/david/ontologies/2013/0/1.3.6.1.4.1.19376.1.8.2.1.335 -->

    <owl:Class rdf:about="&pathLex;335">
        <rdfs:subClassOf rdf:resource="&pathLex;99999"/>
        <skos:prefLabel xml:lang="en">Margins involvement</skos:prefLabel>
        <skos:definition xml:lang="en">Pharynx-Infiltrating malignant neoplasm-Margins involvement</skos:definition>
    </owl:Class>
    


    <!-- http://www.semanticweb.org/david/ontologies/2013/0/1.3.6.1.4.1.19376.1.8.2.1.337 -->

    <owl:Class rdf:about="&pathLex;337">
        <rdfs:subClassOf rdf:resource="&pathLex;99999"/>
        <skos:prefLabel xml:lang="en">Distance of lesion from closest uninvolved margin</skos:prefLabel>
        <skos:definition xml:lang="en">Pharynx-Infiltrating malignant neoplasm-Distance of lesion from closest uninvolved margin</skos:definition>
    </owl:Class>
    


    <!-- http://www.semanticweb.org/david/ontologies/2013/0/1.3.6.1.4.1.19376.1.8.2.1.338 -->

    <owl:Class rdf:about="&pathLex;338">
        <rdfs:subClassOf rdf:resource="&pathLex;99999"/>
        <skos:prefLabel xml:lang="en">Distance of lesion from closest uninvolved margin</skos:prefLabel>
        <skos:definition xml:lang="en">Pharynx-Infiltrating malignant neoplasm-Distance of lesion from closest uninvolved margin</skos:definition>
    </owl:Class>
    


    <!-- http://www.semanticweb.org/david/ontologies/2013/0/1.3.6.1.4.1.19376.1.8.2.1.339 -->

    <owl:Class rdf:about="&pathLex;339">
        <rdfs:subClassOf rdf:resource="&pathLex;99999"/>
        <skos:prefLabel xml:lang="en">Lymph-vascular invasion</skos:prefLabel>
        <skos:definition xml:lang="en">Pharynx-Infiltrating malignant neoplasm-Lymph-vascular invasion</skos:definition>
    </owl:Class>
    


    <!-- http://www.semanticweb.org/david/ontologies/2013/0/1.3.6.1.4.1.19376.1.8.2.1.340 -->

    <owl:Class rdf:about="&pathLex;340">
        <rdfs:subClassOf rdf:resource="&pathLex;99999"/>
        <skos:prefLabel xml:lang="en">Extent</skos:prefLabel>
        <skos:definition xml:lang="en">Pharynx-Infiltrating malignant neoplasm-Extent</skos:definition>
    </owl:Class>
    


    <!-- http://www.semanticweb.org/david/ontologies/2013/0/1.3.6.1.4.1.19376.1.8.2.1.341 -->

    <owl:Class rdf:about="&pathLex;341">
        <rdfs:subClassOf rdf:resource="&pathLex;99999"/>
        <skos:prefLabel xml:lang="en">Perineural invasion</skos:prefLabel>
        <skos:definition xml:lang="en">Pharynx-Infiltrating malignant neoplasm-Perineural invasion</skos:definition>
    </owl:Class>
    


    <!-- http://www.semanticweb.org/david/ontologies/2013/0/1.3.6.1.4.1.19376.1.8.2.1.342 -->

    <owl:Class rdf:about="&pathLex;342">
        <rdfs:subClassOf rdf:resource="&pathLex;99999"/>
        <skos:prefLabel xml:lang="en">Lymph node capsule involvement</skos:prefLabel>
        <skos:definition xml:lang="en">Pharynx-Infiltrating malignant neoplasm-Lymph node capsule involvement</skos:definition>
    </owl:Class>
    


    <!-- http://www.semanticweb.org/david/ontologies/2013/0/1.3.6.1.4.1.19376.1.8.2.1.343 -->

    <owl:Class rdf:about="&pathLex;343">
        <rdfs:subClassOf rdf:resource="&pathLex;99999"/>
        <skos:prefLabel xml:lang="en">Lesion site</skos:prefLabel>
        <skos:definition xml:lang="en">Pharynx-Infiltrating malignant neoplasm-Lesion site</skos:definition>
    </owl:Class>
    


    <!-- http://www.semanticweb.org/david/ontologies/2013/0/1.3.6.1.4.1.19376.1.8.2.1.344 -->

    <owl:Class rdf:about="&pathLex;344">
        <rdfs:subClassOf rdf:resource="&pathLex;99999"/>
        <skos:prefLabel xml:lang="en">Lymph node site</skos:prefLabel>
        <skos:definition xml:lang="en">Pharynx-Infiltrating malignant neoplasm-Lymph node site</skos:definition>
    </owl:Class>
    


    <!-- http://www.semanticweb.org/david/ontologies/2013/0/1.3.6.1.4.1.19376.1.8.2.1.345 -->

    <owl:Class rdf:about="&pathLex;345">
        <rdfs:subClassOf rdf:resource="&pathLex;99999"/>
        <skos:prefLabel xml:lang="en">Number of lymph nodes involved</skos:prefLabel>
        <skos:definition xml:lang="en">Pharynx-Infiltrating malignant neoplasm-Number of lymph nodes involved</skos:definition>
    </owl:Class>
    


    <!-- http://www.semanticweb.org/david/ontologies/2013/0/1.3.6.1.4.1.19376.1.8.2.1.346 -->

    <owl:Class rdf:about="&pathLex;346">
        <rdfs:subClassOf rdf:resource="&pathLex;99999"/>
        <skos:prefLabel xml:lang="en">Number of lymph nodes examined</skos:prefLabel>
        <skos:definition xml:lang="en">Pharynx-Infiltrating malignant neoplasm-Number of lymph nodes examined</skos:definition>
    </owl:Class>
    


    <!-- http://www.semanticweb.org/david/ontologies/2013/0/1.3.6.1.4.1.19376.1.8.2.1.348 -->

    <owl:Class rdf:about="&pathLex;348">
        <rdfs:subClassOf rdf:resource="&pathLex;99999"/>
        <skos:definition xml:lang="en">Pharynx-Infiltrating malignant neoplasm-pN hypopharynx carcinoma</skos:definition>
        <skos:prefLabel xml:lang="en">pN hypopharynx carcinoma</skos:prefLabel>
    </owl:Class>
    


    <!-- http://www.semanticweb.org/david/ontologies/2013/0/1.3.6.1.4.1.19376.1.8.2.1.349 -->

    <owl:Class rdf:about="&pathLex;349">
        <rdfs:subClassOf rdf:resource="&pathLex;99999"/>
        <skos:definition xml:lang="en">Pharynx-Infiltrating malignant neoplasm-pN nasopharynx carcinoma</skos:definition>
        <skos:prefLabel xml:lang="en">pN nasopharynx carcinoma</skos:prefLabel>
    </owl:Class>
    


    <!-- http://www.semanticweb.org/david/ontologies/2013/0/1.3.6.1.4.1.19376.1.8.2.1.35 -->

    <owl:Class rdf:about="&pathLex;35">
        <rdfs:subClassOf rdf:resource="&pathLex;99999"/>
        <skos:definition xml:lang="en">Colon-Infiltrating malignant neoplasm-Tumor deposits</skos:definition>
        <skos:prefLabel xml:lang="en">Tumor deposits</skos:prefLabel>
    </owl:Class>
    


    <!-- http://www.semanticweb.org/david/ontologies/2013/0/1.3.6.1.4.1.19376.1.8.2.1.350 -->

    <owl:Class rdf:about="&pathLex;350">
        <rdfs:subClassOf rdf:resource="&pathLex;99999"/>
        <skos:definition xml:lang="en">Pharynx-Infiltrating malignant neoplasm-pN mucosal malignant melanoma</skos:definition>
        <skos:prefLabel xml:lang="en">pN mucosal malignant melanoma</skos:prefLabel>
    </owl:Class>
    


    <!-- http://www.semanticweb.org/david/ontologies/2013/0/1.3.6.1.4.1.19376.1.8.2.1.352 -->

    <owl:Class rdf:about="&pathLex;352">
        <rdfs:subClassOf rdf:resource="&pathLex;99999"/>
        <skos:definition xml:lang="en">Pharynx-Infiltrating malignant neoplasm-pT hypopharynx carcinoma</skos:definition>
        <skos:prefLabel xml:lang="en">pT hypopharynx carcinoma</skos:prefLabel>
    </owl:Class>
    


    <!-- http://www.semanticweb.org/david/ontologies/2013/0/1.3.6.1.4.1.19376.1.8.2.1.353 -->

    <owl:Class rdf:about="&pathLex;353">
        <rdfs:subClassOf rdf:resource="&pathLex;99999"/>
        <skos:definition xml:lang="en">Pharynx-Infiltrating malignant neoplasm-pT nasopharynx carcinoma</skos:definition>
        <skos:prefLabel xml:lang="en">pT nasopharynx carcinoma</skos:prefLabel>
    </owl:Class>
    


    <!-- http://www.semanticweb.org/david/ontologies/2013/0/1.3.6.1.4.1.19376.1.8.2.1.354 -->

    <owl:Class rdf:about="&pathLex;354">
        <rdfs:subClassOf rdf:resource="&pathLex;99999"/>
        <skos:definition xml:lang="en">Pharynx-Infiltrating malignant neoplasm-pT mucosal malignant melanoma</skos:definition>
        <skos:prefLabel xml:lang="en">pT mucosal malignant melanoma</skos:prefLabel>
    </owl:Class>
    


    <!-- http://www.semanticweb.org/david/ontologies/2013/0/1.3.6.1.4.1.19376.1.8.2.1.355 -->

    <owl:Class rdf:about="&pathLex;355">
        <rdfs:subClassOf rdf:resource="&pathLex;99999"/>
        <skos:prefLabel xml:lang="en">Lymph node metastasis size</skos:prefLabel>
        <skos:definition xml:lang="en">Pharynx-Infiltrating malignant neoplasm-Lymph node metastasis size</skos:definition>
    </owl:Class>
    


    <!-- http://www.semanticweb.org/david/ontologies/2013/0/1.3.6.1.4.1.19376.1.8.2.1.356 -->

    <owl:Class rdf:about="&pathLex;356">
        <rdfs:subClassOf rdf:resource="&pathLex;99999"/>
        <skos:prefLabel xml:lang="en">Lesion size, largest dimension</skos:prefLabel>
        <skos:definition xml:lang="en">Pharynx-Infiltrating malignant neoplasm-Lesion size, largest dimension</skos:definition>
    </owl:Class>
    


    <!-- http://www.semanticweb.org/david/ontologies/2013/0/1.3.6.1.4.1.19376.1.8.2.1.357 -->

    <owl:Class rdf:about="&pathLex;357">
        <rdfs:subClassOf rdf:resource="&pathLex;99999"/>
        <skos:definition xml:lang="en">Pharynx-Infiltrating malignant neoplasm-Specimen size, largest dimension</skos:definition>
        <skos:prefLabel xml:lang="en">Specimen size, largest dimension</skos:prefLabel>
    </owl:Class>
    


    <!-- http://www.semanticweb.org/david/ontologies/2013/0/1.3.6.1.4.1.19376.1.8.2.1.358 -->

    <owl:Class rdf:about="&pathLex;358">
        <rdfs:subClassOf rdf:resource="&pathLex;99999"/>
        <skos:prefLabel xml:lang="en">Histologic type</skos:prefLabel>
        <skos:definition xml:lang="en">Pharynx-Infiltrating malignant neoplasm-Histologic type</skos:definition>
    </owl:Class>
    


    <!-- http://www.semanticweb.org/david/ontologies/2013/0/1.3.6.1.4.1.19376.1.8.2.1.359 -->

    <owl:Class rdf:about="&pathLex;359">
        <rdfs:subClassOf rdf:resource="&pathLex;99999"/>
        <skos:definition xml:lang="en">Lung-Infiltrating malignant neoplasm-Margins involvement</skos:definition>
        <skos:prefLabel xml:lang="en">Margins involvement</skos:prefLabel>
    </owl:Class>
    


    <!-- http://www.semanticweb.org/david/ontologies/2013/0/1.3.6.1.4.1.19376.1.8.2.1.36 -->

    <owl:Class rdf:about="&pathLex;36">
        <rdfs:subClassOf rdf:resource="&pathLex;10010"/>
        <skos:prefLabel xml:lang="en">Extent</skos:prefLabel>
        <skos:definition xml:lang="en">Generic-Infiltrating malignant neoplasm-Extent</skos:definition>
    </owl:Class>
    


    <!-- http://www.semanticweb.org/david/ontologies/2013/0/1.3.6.1.4.1.19376.1.8.2.1.360 -->

    <owl:Class rdf:about="&pathLex;360">
        <rdfs:subClassOf rdf:resource="&pathLex;99999"/>
        <skos:definition xml:lang="en">Lung-Infiltrating malignant neoplasm-Margins involvement</skos:definition>
        <skos:prefLabel xml:lang="en">Margins involvement</skos:prefLabel>
    </owl:Class>
    


    <!-- http://www.semanticweb.org/david/ontologies/2013/0/1.3.6.1.4.1.19376.1.8.2.1.361 -->

    <owl:Class rdf:about="&pathLex;361">
        <rdfs:subClassOf rdf:resource="&pathLex;99999"/>
        <skos:prefLabel xml:lang="en">Distance of lesion from closest uninvolved margin</skos:prefLabel>
        <skos:definition xml:lang="en">Lung-Infiltrating malignant neoplasm-Distance of lesion from closest uninvolved margin</skos:definition>
    </owl:Class>
    


    <!-- http://www.semanticweb.org/david/ontologies/2013/0/1.3.6.1.4.1.19376.1.8.2.1.362 -->

    <owl:Class rdf:about="&pathLex;362">
        <rdfs:subClassOf rdf:resource="&pathLex;99999"/>
        <skos:definition xml:lang="en">Lung-Infiltrating malignant neoplasm-Lymph-vascular invasion</skos:definition>
        <skos:prefLabel xml:lang="en">Lymph-vascular invasion</skos:prefLabel>
    </owl:Class>
    


    <!-- http://www.semanticweb.org/david/ontologies/2013/0/1.3.6.1.4.1.19376.1.8.2.1.363 -->

    <owl:Class rdf:about="&pathLex;363">
        <rdfs:subClassOf rdf:resource="&pathLex;99999"/>
        <skos:prefLabel xml:lang="en">Extent</skos:prefLabel>
        <skos:definition xml:lang="en">Lung-Infiltrating malignant neoplasm-Extent</skos:definition>
    </owl:Class>
    


    <!-- http://www.semanticweb.org/david/ontologies/2013/0/1.3.6.1.4.1.19376.1.8.2.1.364 -->

    <owl:Class rdf:about="&pathLex;364">
        <rdfs:subClassOf rdf:resource="&pathLex;99999"/>
        <skos:definition xml:lang="en">Lung-Infiltrating malignant neoplasm-Perineural invasion</skos:definition>
        <skos:prefLabel xml:lang="en">Perineural invasion</skos:prefLabel>
    </owl:Class>
    


    <!-- http://www.semanticweb.org/david/ontologies/2013/0/1.3.6.1.4.1.19376.1.8.2.1.365 -->

    <owl:Class rdf:about="&pathLex;365">
        <rdfs:subClassOf rdf:resource="&pathLex;99999"/>
        <skos:definition xml:lang="en">Lung-Infiltrating malignant neoplasm-Lymph node capsule involvement</skos:definition>
        <skos:prefLabel xml:lang="en">Lymph node capsule involvement</skos:prefLabel>
    </owl:Class>
    


    <!-- http://www.semanticweb.org/david/ontologies/2013/0/1.3.6.1.4.1.19376.1.8.2.1.366 -->

    <owl:Class rdf:about="&pathLex;366">
        <rdfs:subClassOf rdf:resource="&pathLex;99999"/>
        <skos:definition xml:lang="en">Lung-Infiltrating malignant neoplasm-Lymph node site</skos:definition>
        <skos:prefLabel xml:lang="en">Lymph node site</skos:prefLabel>
    </owl:Class>
    


    <!-- http://www.semanticweb.org/david/ontologies/2013/0/1.3.6.1.4.1.19376.1.8.2.1.367 -->

    <owl:Class rdf:about="&pathLex;367">
        <rdfs:subClassOf rdf:resource="&pathLex;99999"/>
        <skos:definition xml:lang="en">Lung-Infiltrating malignant neoplasm-Margin site</skos:definition>
        <skos:prefLabel xml:lang="en">Margin site</skos:prefLabel>
    </owl:Class>
    


    <!-- http://www.semanticweb.org/david/ontologies/2013/0/1.3.6.1.4.1.19376.1.8.2.1.368 -->

    <owl:Class rdf:about="&pathLex;368">
        <rdfs:subClassOf rdf:resource="&pathLex;99999"/>
        <skos:definition xml:lang="en">Lung-Infiltrating malignant neoplasm-Number of lymph nodes involved</skos:definition>
        <skos:prefLabel xml:lang="en">Number of lymph nodes involved</skos:prefLabel>
    </owl:Class>
    


    <!-- http://www.semanticweb.org/david/ontologies/2013/0/1.3.6.1.4.1.19376.1.8.2.1.369 -->

    <owl:Class rdf:about="&pathLex;369">
        <rdfs:subClassOf rdf:resource="&pathLex;99999"/>
        <skos:definition xml:lang="en">Lung-Infiltrating malignant neoplasm-Number of lymph nodes examined</skos:definition>
        <skos:prefLabel xml:lang="en">Number of lymph nodes examined</skos:prefLabel>
    </owl:Class>
    


    <!-- http://www.semanticweb.org/david/ontologies/2013/0/1.3.6.1.4.1.19376.1.8.2.1.371 -->

    <owl:Class rdf:about="&pathLex;371">
        <rdfs:subClassOf rdf:resource="&pathLex;99999"/>
        <skos:definition xml:lang="en">Lung-Infiltrating malignant neoplasm-pN</skos:definition>
        <skos:prefLabel xml:lang="en">pN</skos:prefLabel>
    </owl:Class>
    


    <!-- http://www.semanticweb.org/david/ontologies/2013/0/1.3.6.1.4.1.19376.1.8.2.1.373 -->

    <owl:Class rdf:about="&pathLex;373">
        <rdfs:subClassOf rdf:resource="&pathLex;99999"/>
        <skos:definition xml:lang="en">Lung-Infiltrating malignant neoplasm-pT</skos:definition>
        <skos:prefLabel xml:lang="en">pT</skos:prefLabel>
    </owl:Class>
    


    <!-- http://www.semanticweb.org/david/ontologies/2013/0/1.3.6.1.4.1.19376.1.8.2.1.374 -->

    <owl:Class rdf:about="&pathLex;374">
        <rdfs:subClassOf rdf:resource="&pathLex;99999"/>
        <skos:prefLabel xml:lang="en">Lesion size, largest dimension</skos:prefLabel>
        <skos:definition xml:lang="en">Lung-Infiltrating malignant neoplasm-Lesion size, largest dimension</skos:definition>
    </owl:Class>
    


    <!-- http://www.semanticweb.org/david/ontologies/2013/0/1.3.6.1.4.1.19376.1.8.2.1.375 -->

    <owl:Class rdf:about="&pathLex;375">
        <rdfs:subClassOf rdf:resource="&pathLex;99999"/>
        <skos:prefLabel xml:lang="en">Lesion size, largest dimension</skos:prefLabel>
        <skos:definition xml:lang="en">Lung-Infiltrating malignant neoplasm-Lesion size, largest dimension</skos:definition>
    </owl:Class>
    


    <!-- http://www.semanticweb.org/david/ontologies/2013/0/1.3.6.1.4.1.19376.1.8.2.1.376 -->

    <owl:Class rdf:about="&pathLex;376">
        <rdfs:subClassOf rdf:resource="&pathLex;99999"/>
        <skos:prefLabel xml:lang="en">Histologic type</skos:prefLabel>
        <skos:definition xml:lang="en">Lung-Infiltrating malignant neoplasm-Histologic type</skos:definition>
    </owl:Class>
    


    <!-- http://www.semanticweb.org/david/ontologies/2013/0/1.3.6.1.4.1.19376.1.8.2.1.377 -->

    <owl:Class rdf:about="&pathLex;377">
        <rdfs:subClassOf rdf:resource="&pathLex;99999"/>
        <skos:prefLabel xml:lang="en">Margins involvement</skos:prefLabel>
        <skos:definition xml:lang="en">Prostate-Infiltrating malignant neoplasm-Margins involvement</skos:definition>
    </owl:Class>
    


    <!-- http://www.semanticweb.org/david/ontologies/2013/0/1.3.6.1.4.1.19376.1.8.2.1.378 -->

    <owl:Class rdf:about="&pathLex;378">
        <rdfs:subClassOf rdf:resource="&pathLex;99999"/>
        <skos:prefLabel xml:lang="en">Distance of lesion from closest uninvolved margin</skos:prefLabel>
        <skos:definition xml:lang="en">Prostate-Infiltrating malignant neoplasm-Distance of lesion from closest uninvolved margin</skos:definition>
    </owl:Class>
    


    <!-- http://www.semanticweb.org/david/ontologies/2013/0/1.3.6.1.4.1.19376.1.8.2.1.379 -->

    <owl:Class rdf:about="&pathLex;379">
        <rdfs:subClassOf rdf:resource="&pathLex;99999"/>
        <skos:prefLabel xml:lang="en">Lymph-vascular invasion</skos:prefLabel>
        <skos:definition xml:lang="en">Prostate-Infiltrating malignant neoplasm-Lymph-vascular invasion</skos:definition>
    </owl:Class>
    


    <!-- http://www.semanticweb.org/david/ontologies/2013/0/1.3.6.1.4.1.19376.1.8.2.1.38 -->

    <owl:Class rdf:about="&pathLex;38">
        <rdfs:subClassOf rdf:resource="&pathLex;10010"/>
        <skos:definition xml:lang="en">Generic-Infiltrating malignant neoplasm-Number of lymph nodes examined</skos:definition>
        <skos:prefLabel xml:lang="en">Number of lymph nodes examined</skos:prefLabel>
    </owl:Class>
    


    <!-- http://www.semanticweb.org/david/ontologies/2013/0/1.3.6.1.4.1.19376.1.8.2.1.380 -->

    <owl:Class rdf:about="&pathLex;380">
        <rdfs:subClassOf rdf:resource="&pathLex;99999"/>
        <skos:prefLabel xml:lang="en">Lymph node sampling</skos:prefLabel>
        <skos:definition xml:lang="en">Prostate-Infiltrating malignant neoplasm-Lymph node sampling</skos:definition>
    </owl:Class>
    


    <!-- http://www.semanticweb.org/david/ontologies/2013/0/1.3.6.1.4.1.19376.1.8.2.1.381 -->

    <owl:Class rdf:about="&pathLex;381">
        <rdfs:subClassOf rdf:resource="&pathLex;99999"/>
        <skos:prefLabel xml:lang="en">Extent</skos:prefLabel>
        <skos:definition xml:lang="en">Prostate-Infiltrating malignant neoplasm-Extent</skos:definition>
    </owl:Class>
    


    <!-- http://www.semanticweb.org/david/ontologies/2013/0/1.3.6.1.4.1.19376.1.8.2.1.382 -->

    <owl:Class rdf:about="&pathLex;382">
        <rdfs:subClassOf rdf:resource="&pathLex;99999"/>
        <skos:prefLabel xml:lang="en">Histologic grade (Gleason-Primary (Predominant) Pattern)</skos:prefLabel>
        <skos:definition xml:lang="en">Prostate-Infiltrating malignant neoplasm-Histologic grade (Gleason-Primary (Predominant) Pattern)</skos:definition>
    </owl:Class>
    


    <!-- http://www.semanticweb.org/david/ontologies/2013/0/1.3.6.1.4.1.19376.1.8.2.1.383 -->

    <owl:Class rdf:about="&pathLex;383">
        <rdfs:subClassOf rdf:resource="&pathLex;99999"/>
        <skos:prefLabel xml:lang="en">Histologic grade (Gleason-Secondary (Worst Remaining) Pattern)</skos:prefLabel>
        <skos:definition xml:lang="en">Prostate-Infiltrating malignant neoplasm-Histologic grade (Gleason-Secondary (Worst Remaining) Pattern)</skos:definition>
    </owl:Class>
    


    <!-- http://www.semanticweb.org/david/ontologies/2013/0/1.3.6.1.4.1.19376.1.8.2.1.384 -->

    <owl:Class rdf:about="&pathLex;384">
        <rdfs:subClassOf rdf:resource="&pathLex;99999"/>
        <skos:prefLabel xml:lang="en">Histologic grade (Gleason-Tertiary Pattern)</skos:prefLabel>
        <skos:definition xml:lang="en">Prostate-Infiltrating malignant neoplasm-Histologic grade (Gleason-Tertiary Pattern)</skos:definition>
    </owl:Class>
    


    <!-- http://www.semanticweb.org/david/ontologies/2013/0/1.3.6.1.4.1.19376.1.8.2.1.385 -->

    <owl:Class rdf:about="&pathLex;385">
        <rdfs:subClassOf rdf:resource="&pathLex;99999"/>
        <skos:prefLabel xml:lang="en">Histologic grade (Gleason-Total Gleason Score)</skos:prefLabel>
        <skos:definition xml:lang="en">Prostate-Infiltrating malignant neoplasm-Histologic grade (Gleason-Total Gleason Score)</skos:definition>
    </owl:Class>
    


    <!-- http://www.semanticweb.org/david/ontologies/2013/0/1.3.6.1.4.1.19376.1.8.2.1.386 -->

    <owl:Class rdf:about="&pathLex;386">
        <rdfs:subClassOf rdf:resource="&pathLex;99999"/>
        <skos:prefLabel xml:lang="en">Perineural invasion</skos:prefLabel>
        <skos:definition xml:lang="en">Prostate-Infiltrating malignant neoplasm-Perineural invasion</skos:definition>
    </owl:Class>
    


    <!-- http://www.semanticweb.org/david/ontologies/2013/0/1.3.6.1.4.1.19376.1.8.2.1.387 -->

    <owl:Class rdf:about="&pathLex;387">
        <rdfs:subClassOf rdf:resource="&pathLex;99999"/>
        <skos:prefLabel xml:lang="en">Lesion site</skos:prefLabel>
        <skos:definition xml:lang="en">Prostate-Infiltrating malignant neoplasm-Lesion site</skos:definition>
    </owl:Class>
    


    <!-- http://www.semanticweb.org/david/ontologies/2013/0/1.3.6.1.4.1.19376.1.8.2.1.388 -->

    <owl:Class rdf:about="&pathLex;388">
        <rdfs:subClassOf rdf:resource="&pathLex;99999"/>
        <skos:prefLabel xml:lang="en">Number of lymph nodes involved</skos:prefLabel>
        <skos:definition xml:lang="en">Prostate-Infiltrating malignant neoplasm-Number of lymph nodes involved</skos:definition>
    </owl:Class>
    


    <!-- http://www.semanticweb.org/david/ontologies/2013/0/1.3.6.1.4.1.19376.1.8.2.1.389 -->

    <owl:Class rdf:about="&pathLex;389">
        <rdfs:subClassOf rdf:resource="&pathLex;99999"/>
        <skos:prefLabel xml:lang="en">Number of lymph nodes examined</skos:prefLabel>
        <skos:definition xml:lang="en">Prostate-Infiltrating malignant neoplasm-Number of lymph nodes examined</skos:definition>
    </owl:Class>
    


    <!-- http://www.semanticweb.org/david/ontologies/2013/0/1.3.6.1.4.1.19376.1.8.2.1.39 -->

    <owl:Class rdf:about="&pathLex;39">
        <rdfs:subClassOf rdf:resource="&pathLex;10010"/>
        <skos:definition xml:lang="en">Generic-Infiltrating malignant neoplasm-Number of lymph nodes involved</skos:definition>
        <skos:prefLabel xml:lang="en">Number of lymph nodes involved</skos:prefLabel>
    </owl:Class>
    


    <!-- http://www.semanticweb.org/david/ontologies/2013/0/1.3.6.1.4.1.19376.1.8.2.1.391 -->

    <owl:Class rdf:about="&pathLex;391">
        <rdfs:subClassOf rdf:resource="&pathLex;99999"/>
        <skos:definition xml:lang="en">Prostate-Infiltrating malignant neoplasm-pN</skos:definition>
        <skos:prefLabel xml:lang="en">pN</skos:prefLabel>
    </owl:Class>
    


    <!-- http://www.semanticweb.org/david/ontologies/2013/0/1.3.6.1.4.1.19376.1.8.2.1.392 -->

    <owl:Class rdf:about="&pathLex;392">
        <rdfs:subClassOf rdf:resource="&pathLex;99999"/>
        <skos:definition xml:lang="en">Prostate-Infiltrating malignant neoplasm-Specimen weight</skos:definition>
        <skos:prefLabel xml:lang="en">Specimen weight</skos:prefLabel>
    </owl:Class>
    


    <!-- http://www.semanticweb.org/david/ontologies/2013/0/1.3.6.1.4.1.19376.1.8.2.1.394 -->

    <owl:Class rdf:about="&pathLex;394">
        <rdfs:subClassOf rdf:resource="&pathLex;99999"/>
        <skos:definition xml:lang="en">Prostate-Infiltrating malignant neoplasm-pT</skos:definition>
        <skos:prefLabel xml:lang="en">pT</skos:prefLabel>
    </owl:Class>
    


    <!-- http://www.semanticweb.org/david/ontologies/2013/0/1.3.6.1.4.1.19376.1.8.2.1.395 -->

    <owl:Class rdf:about="&pathLex;395">
        <rdfs:subClassOf rdf:resource="&pathLex;99999"/>
        <skos:prefLabel xml:lang="en">Lymph node metastasis size</skos:prefLabel>
        <skos:definition xml:lang="en">Prostate-Infiltrating malignant neoplasm-Lymph node metastasis size</skos:definition>
    </owl:Class>
    


    <!-- http://www.semanticweb.org/david/ontologies/2013/0/1.3.6.1.4.1.19376.1.8.2.1.396 -->

    <owl:Class rdf:about="&pathLex;396">
        <rdfs:subClassOf rdf:resource="&pathLex;99999"/>
        <skos:definition xml:lang="en">Prostate-Infiltrating malignant neoplasm-Specimen size, largest dimension</skos:definition>
        <skos:prefLabel xml:lang="en">Specimen size, largest dimension</skos:prefLabel>
    </owl:Class>
    


    <!-- http://www.semanticweb.org/david/ontologies/2013/0/1.3.6.1.4.1.19376.1.8.2.1.397 -->

    <owl:Class rdf:about="&pathLex;397">
        <rdfs:subClassOf rdf:resource="&pathLex;99999"/>
        <skos:prefLabel xml:lang="en">Histologic type</skos:prefLabel>
        <skos:definition xml:lang="en">Prostate-Infiltrating malignant neoplasm-Histologic type</skos:definition>
    </owl:Class>
    


    <!-- http://www.semanticweb.org/david/ontologies/2013/0/1.3.6.1.4.1.19376.1.8.2.1.398 -->

    <owl:Class rdf:about="&pathLex;398">
        <rdfs:subClassOf rdf:resource="&pathLex;99999"/>
        <skos:definition xml:lang="en">Kidney-Infiltrating malignant neoplasm-Margins involvement</skos:definition>
        <skos:prefLabel xml:lang="en">Margins involvement</skos:prefLabel>
    </owl:Class>
    


    <!-- http://www.semanticweb.org/david/ontologies/2013/0/1.3.6.1.4.1.19376.1.8.2.1.399 -->

    <owl:Class rdf:about="&pathLex;399">
        <rdfs:subClassOf rdf:resource="&pathLex;99999"/>
        <skos:prefLabel xml:lang="en">Distance of lesion from closest uninvolved margin</skos:prefLabel>
        <skos:definition xml:lang="en">Kidney-Infiltrating malignant neoplasm-Distance of lesion from closest uninvolved margin</skos:definition>
    </owl:Class>
    


    <!-- http://www.semanticweb.org/david/ontologies/2013/0/1.3.6.1.4.1.19376.1.8.2.1.4 -->

    <owl:Class rdf:about="&pathLex;4">
        <rdfs:subClassOf rdf:resource="&pathLex;99999"/>
        <skos:definition xml:lang="en">Generic-Specimen-Specimen integrity</skos:definition>
        <skos:prefLabel xml:lang="en">Specimen integrity</skos:prefLabel>
    </owl:Class>
    


    <!-- http://www.semanticweb.org/david/ontologies/2013/0/1.3.6.1.4.1.19376.1.8.2.1.40 -->

    <owl:Class rdf:about="&pathLex;40">
        <rdfs:subClassOf rdf:resource="&pathLex;425"/>
        <skos:definition xml:lang="en">Breast-Infiltrating malignant neoplasm-Number of lymph nodes with isolated tumor cells (&lt; = 0.2 mm and &lt; = 200 cells)</skos:definition>
        <skos:prefLabel xml:lang="en">Number of lymph nodes with isolated tumor cells (&lt; = 0.2 mm and &lt; = 200 cells)</skos:prefLabel>
    </owl:Class>
    


    <!-- http://www.semanticweb.org/david/ontologies/2013/0/1.3.6.1.4.1.19376.1.8.2.1.400 -->

    <owl:Class rdf:about="&pathLex;400">
        <rdfs:subClassOf rdf:resource="&pathLex;99999"/>
        <skos:definition xml:lang="en">Kidney-Infiltrating malignant neoplasm-Lymph-vascular invasion</skos:definition>
        <skos:prefLabel xml:lang="en">Lymph-vascular invasion</skos:prefLabel>
    </owl:Class>
    


    <!-- http://www.semanticweb.org/david/ontologies/2013/0/1.3.6.1.4.1.19376.1.8.2.1.401 -->

    <owl:Class rdf:about="&pathLex;401">
        <rdfs:subClassOf rdf:resource="&pathLex;99999"/>
        <skos:prefLabel xml:lang="en">Extent</skos:prefLabel>
        <skos:definition xml:lang="en">Kidney-Infiltrating malignant neoplasm-Extent</skos:definition>
    </owl:Class>
    


    <!-- http://www.semanticweb.org/david/ontologies/2013/0/1.3.6.1.4.1.19376.1.8.2.1.402 -->

    <owl:Class rdf:about="&pathLex;402">
        <rdfs:subClassOf rdf:resource="&pathLex;99999"/>
        <skos:prefLabel xml:lang="en">Histologic grade (Fuhrman Nuclear Grade)</skos:prefLabel>
        <skos:definition xml:lang="en">Kidney-Infiltrating malignant neoplasm-Histologic grade (Fuhrman Nuclear Grade)</skos:definition>
    </owl:Class>
    


    <!-- http://www.semanticweb.org/david/ontologies/2013/0/1.3.6.1.4.1.19376.1.8.2.1.403 -->

    <owl:Class rdf:about="&pathLex;403">
        <rdfs:subClassOf rdf:resource="&pathLex;99999"/>
        <skos:definition xml:lang="en">Kidney-Infiltrating malignant neoplasm-Lesion site</skos:definition>
        <skos:prefLabel xml:lang="en">Lesion site</skos:prefLabel>
    </owl:Class>
    


    <!-- http://www.semanticweb.org/david/ontologies/2013/0/1.3.6.1.4.1.19376.1.8.2.1.404 -->

    <owl:Class rdf:about="&pathLex;404">
        <rdfs:subClassOf rdf:resource="&pathLex;99999"/>
        <skos:definition xml:lang="en">Kidney-Infiltrating malignant neoplasm-Margin site</skos:definition>
        <skos:prefLabel xml:lang="en">Margin site</skos:prefLabel>
    </owl:Class>
    


    <!-- http://www.semanticweb.org/david/ontologies/2013/0/1.3.6.1.4.1.19376.1.8.2.1.405 -->

    <owl:Class rdf:about="&pathLex;405">
        <rdfs:subClassOf rdf:resource="&pathLex;99999"/>
        <skos:definition xml:lang="en">Kidney-Infiltrating malignant neoplasm-Number of lymph nodes involved</skos:definition>
        <skos:prefLabel xml:lang="en">Number of lymph nodes involved</skos:prefLabel>
    </owl:Class>
    


    <!-- http://www.semanticweb.org/david/ontologies/2013/0/1.3.6.1.4.1.19376.1.8.2.1.406 -->

    <owl:Class rdf:about="&pathLex;406">
        <rdfs:subClassOf rdf:resource="&pathLex;99999"/>
        <skos:definition xml:lang="en">Kidney-Infiltrating malignant neoplasm-Number of lymph nodes examined</skos:definition>
        <skos:prefLabel xml:lang="en">Number of lymph nodes examined</skos:prefLabel>
    </owl:Class>
    


    <!-- http://www.semanticweb.org/david/ontologies/2013/0/1.3.6.1.4.1.19376.1.8.2.1.408 -->

    <owl:Class rdf:about="&pathLex;408">
        <rdfs:subClassOf rdf:resource="&pathLex;99999"/>
        <skos:definition xml:lang="en">Kidney-Infiltrating malignant neoplasm-pN</skos:definition>
        <skos:prefLabel xml:lang="en">pN</skos:prefLabel>
    </owl:Class>
    


    <!-- http://www.semanticweb.org/david/ontologies/2013/0/1.3.6.1.4.1.19376.1.8.2.1.41 -->

    <owl:Class rdf:about="&pathLex;41">
        <rdfs:subClassOf rdf:resource="&pathLex;425"/>
        <skos:definition xml:lang="en">Breast-Infiltrating malignant neoplasm-Number of lymph nodes with macrometastases (&gt;0.2 cm)</skos:definition>
        <skos:prefLabel xml:lang="en">Number of lymph nodes with macrometastases (&gt;0.2 cm)</skos:prefLabel>
    </owl:Class>
    


    <!-- http://www.semanticweb.org/david/ontologies/2013/0/1.3.6.1.4.1.19376.1.8.2.1.410 -->

    <owl:Class rdf:about="&pathLex;410">
        <rdfs:subClassOf rdf:resource="&pathLex;99999"/>
        <skos:definition xml:lang="en">Kidney-Infiltrating malignant neoplasm-pT</skos:definition>
        <skos:prefLabel xml:lang="en">pT</skos:prefLabel>
    </owl:Class>
    


    <!-- http://www.semanticweb.org/david/ontologies/2013/0/1.3.6.1.4.1.19376.1.8.2.1.411 -->

    <owl:Class rdf:about="&pathLex;411">
        <rdfs:subClassOf rdf:resource="&pathLex;99999"/>
        <skos:definition xml:lang="en">Kidney-Infiltrating malignant neoplasm-Lesion size, largest dimension</skos:definition>
        <skos:prefLabel xml:lang="en">Lesion size, largest dimension</skos:prefLabel>
    </owl:Class>
    


    <!-- http://www.semanticweb.org/david/ontologies/2013/0/1.3.6.1.4.1.19376.1.8.2.1.412 -->

    <owl:Class rdf:about="&pathLex;412">
        <rdfs:subClassOf rdf:resource="&pathLex;99999"/>
        <skos:prefLabel xml:lang="en">Histologic type</skos:prefLabel>
        <skos:definition xml:lang="en">Kidney-Infiltrating malignant neoplasm-Histologic type</skos:definition>
    </owl:Class>
    


    <!-- http://www.semanticweb.org/david/ontologies/2013/0/1.3.6.1.4.1.19376.1.8.2.1.413 -->

    <owl:Class rdf:about="&pathLex;413">
        <rdfs:subClassOf rdf:resource="&pathLex;69"/>
        <skos:definition xml:lang="en">Breast-In situ neoplasm-Margins involvement</skos:definition>
        <skos:prefLabel xml:lang="en">Breast-Margins involvement</skos:prefLabel>
        <skos:altLabel xml:lang="en">Margins involvement</skos:altLabel>
    </owl:Class>
    


    <!-- http://www.semanticweb.org/david/ontologies/2013/0/1.3.6.1.4.1.19376.1.8.2.1.414 -->

    <owl:Class rdf:about="&pathLex;414">
        <rdfs:subClassOf rdf:resource="&pathLex;99999"/>
        <skos:definition xml:lang="en">Breast-In situ neoplasm-Distance of lesion from closest uninvolved margin</skos:definition>
        <skos:prefLabel xml:lang="en">Distance of lesion from closest uninvolved margin</skos:prefLabel>
    </owl:Class>
    


    <!-- http://www.semanticweb.org/david/ontologies/2013/0/1.3.6.1.4.1.19376.1.8.2.1.415 -->

    <owl:Class rdf:about="&pathLex;415">
        <rdfs:subClassOf rdf:resource="&pathLex;62"/>
        <skos:definition xml:lang="en">Breast-Infiltrating malignant neoplasm-Lymph-vascular invasion</skos:definition>
        <skos:prefLabel xml:lang="en">Breast-Lymph-vascular invasion</skos:prefLabel>
        <skos:altLabel xml:lang="en">Lymph-vascular invasion</skos:altLabel>
    </owl:Class>
    


    <!-- http://www.semanticweb.org/david/ontologies/2013/0/1.3.6.1.4.1.19376.1.8.2.1.416 -->

    <owl:Class rdf:about="&pathLex;416">
        <rdfs:subClassOf rdf:resource="&pathLex;209"/>
        <skos:definition xml:lang="en">Breast-Infiltrating malignant neoplasm-Lymph node sampling</skos:definition>
        <skos:prefLabel xml:lang="en">Breast-Lymph node sampling</skos:prefLabel>
        <skos:altLabel xml:lang="en">Lymph node sampling</skos:altLabel>
    </owl:Class>
    


    <!-- http://www.semanticweb.org/david/ontologies/2013/0/1.3.6.1.4.1.19376.1.8.2.1.417 -->

    <owl:Class rdf:about="&pathLex;417">
        <rdfs:subClassOf rdf:resource="&pathLex;10000"/>
        <skos:definition xml:lang="en">Breast-In situ neoplasm-Histologic grade of ductal carcinoma in situ (DCIS)</skos:definition>
        <skos:prefLabel xml:lang="en">Histologic grade of ductal carcinoma in situ (DCIS)</skos:prefLabel>
    </owl:Class>
    


    <!-- http://www.semanticweb.org/david/ontologies/2013/0/1.3.6.1.4.1.19376.1.8.2.1.418 -->

    <owl:Class rdf:about="&pathLex;418">
        <rdfs:subClassOf rdf:resource="&pathLex;421"/>
        <skos:definition xml:lang="en">Breast-Infiltrating malignant neoplasm-Histologic grade (Nottingham Histologic Score-Glandular (Acinar)/Tubular Differentiation)</skos:definition>
        <skos:prefLabel xml:lang="en">Histologic grade (Nottingham Histologic Score-Glandular (Acinar)/Tubular Differentiation)</skos:prefLabel>
    </owl:Class>
    


    <!-- http://www.semanticweb.org/david/ontologies/2013/0/1.3.6.1.4.1.19376.1.8.2.1.419 -->

    <owl:Class rdf:about="&pathLex;419">
        <rdfs:subClassOf rdf:resource="&pathLex;421"/>
        <skos:definition xml:lang="en">Breast-Infiltrating malignant neoplasm-Histologic grade (Nottingham Histologic Score-Mitotic Count)</skos:definition>
        <skos:prefLabel xml:lang="en">Histologic grade (Nottingham Histologic Score-Mitotic Count)</skos:prefLabel>
    </owl:Class>
    


    <!-- http://www.semanticweb.org/david/ontologies/2013/0/1.3.6.1.4.1.19376.1.8.2.1.42 -->

    <owl:Class rdf:about="&pathLex;42">
        <rdfs:subClassOf rdf:resource="&pathLex;425"/>
        <skos:definition xml:lang="en">Breast-Infiltrating malignant neoplasm-Number of lymph nodes with micrometastases (&gt;0.2 mm to 0.2 cm and/or &gt;200 cells): </skos:definition>
        <skos:prefLabel xml:lang="en">Number of lymph nodes with micrometastases (&gt;0.2 mm to 0.2 cm and/or &gt;200 cells): </skos:prefLabel>
    </owl:Class>
    


    <!-- http://www.semanticweb.org/david/ontologies/2013/0/1.3.6.1.4.1.19376.1.8.2.1.420 -->

    <owl:Class rdf:about="&pathLex;420">
        <rdfs:subClassOf rdf:resource="&pathLex;421"/>
        <skos:definition xml:lang="en">Breast-Infiltrating malignant neoplasm-Histologic grade (Nottingham Histologic Score-Nuclear Pleomorphism)</skos:definition>
        <skos:prefLabel xml:lang="en">Histologic grade (Nottingham Histologic Score-Nuclear Pleomorphism)</skos:prefLabel>
    </owl:Class>
    


    <!-- http://www.semanticweb.org/david/ontologies/2013/0/1.3.6.1.4.1.19376.1.8.2.1.421 -->

    <owl:Class rdf:about="&pathLex;421">
        <rdfs:subClassOf rdf:resource="&pathLex;10005"/>
        <skos:definition xml:lang="en">Breast-Infiltrating malignant neoplasm-Histologic grade (Nottingham)</skos:definition>
        <skos:prefLabel xml:lang="en">Histologic grade (Nottingham)</skos:prefLabel>
    </owl:Class>
    


    <!-- http://www.semanticweb.org/david/ontologies/2013/0/1.3.6.1.4.1.19376.1.8.2.1.422 -->

    <owl:Class rdf:about="&pathLex;422">
        <rdfs:subClassOf rdf:resource="&pathLex;7"/>
        <skos:definition xml:lang="en">Breast-Infiltrating malignant neoplasm-Lesion site</skos:definition>
        <skos:prefLabel xml:lang="en">Breast-Lesion site</skos:prefLabel>
        <skos:altLabel xml:lang="en">Lesion site</skos:altLabel>
    </owl:Class>
    


    <!-- http://www.semanticweb.org/david/ontologies/2013/0/1.3.6.1.4.1.19376.1.8.2.1.423 -->

    <owl:Class rdf:about="&pathLex;423">
        <rdfs:subClassOf rdf:resource="&pathLex;45"/>
        <skos:definition xml:lang="en">Breast-Infiltrating malignant neoplasm-Lymph node site</skos:definition>
        <skos:prefLabel xml:lang="en">Breast-Lymph node site</skos:prefLabel>
        <skos:altLabel xml:lang="en">Lymph node site</skos:altLabel>
    </owl:Class>
    


    <!-- http://www.semanticweb.org/david/ontologies/2013/0/1.3.6.1.4.1.19376.1.8.2.1.424 -->

    <owl:Class rdf:about="&pathLex;424">
        <rdfs:subClassOf rdf:resource="&pathLex;1836"/>
        <skos:definition xml:lang="en">Breast-Infiltrating malignant neoplasm-Margin site</skos:definition>
        <skos:prefLabel xml:lang="en">Breast-Margin site</skos:prefLabel>
        <skos:altLabel xml:lang="en">Margin site</skos:altLabel>
    </owl:Class>
    


    <!-- http://www.semanticweb.org/david/ontologies/2013/0/1.3.6.1.4.1.19376.1.8.2.1.425 -->

    <owl:Class rdf:about="&pathLex;425">
        <rdfs:subClassOf rdf:resource="&pathLex;39"/>
        <skos:definition xml:lang="en">Breast-Infiltrating malignant neoplasm-Number of lymph nodes involved</skos:definition>
        <skos:prefLabel xml:lang="en">Breast-Number of lymph nodes involved</skos:prefLabel>
        <skos:altLabel xml:lang="en">Number of lymph nodes involved</skos:altLabel>
    </owl:Class>
    


    <!-- http://www.semanticweb.org/david/ontologies/2013/0/1.3.6.1.4.1.19376.1.8.2.1.426 -->

    <owl:Class rdf:about="&pathLex;426">
        <rdfs:subClassOf rdf:resource="&pathLex;38"/>
        <skos:definition xml:lang="en">Breast-Infiltrating malignant neoplasm-Number of lymph nodes examined</skos:definition>
        <skos:prefLabel xml:lang="en">Breast-Number of lymph nodes examined</skos:prefLabel>
        <skos:altLabel xml:lang="en">Number of lymph nodes examined</skos:altLabel>
    </owl:Class>
    


    <!-- http://www.semanticweb.org/david/ontologies/2013/0/1.3.6.1.4.1.19376.1.8.2.1.428 -->

    <owl:Class rdf:about="&pathLex;428">
        <rdfs:subClassOf rdf:resource="&pathLex;1432"/>
        <skos:definition xml:lang="en">Breast-Infiltrating malignant neoplasm-pN</skos:definition>
        <skos:prefLabel xml:lang="en">Breast-Infiltrating malignant neoplasm-pN</skos:prefLabel>
        <skos:altLabel xml:lang="en">pN</skos:altLabel>
    </owl:Class>
    


    <!-- http://www.semanticweb.org/david/ontologies/2013/0/1.3.6.1.4.1.19376.1.8.2.1.43 -->

    <owl:Class rdf:about="&pathLex;43">
        <rdfs:subClassOf rdf:resource="&pathLex;99999"/>
        <skos:definition xml:lang="en">Larynx-Infiltrating malignant neoplasm-Lymph node metastasis size</skos:definition>
        <skos:prefLabel xml:lang="en">Lymph node metastasis size</skos:prefLabel>
    </owl:Class>
    


    <!-- http://www.semanticweb.org/david/ontologies/2013/0/1.3.6.1.4.1.19376.1.8.2.1.430 -->

    <owl:Class rdf:about="&pathLex;430">
        <rdfs:subClassOf rdf:resource="&pathLex;1431"/>
        <skos:prefLabel xml:lang="en">Breast-Infiltrating malignant neoplasm-pT</skos:prefLabel>
        <skos:definition xml:lang="en">Breast-Infiltrating malignant neoplasm-pT</skos:definition>
        <skos:altLabel xml:lang="en">pT</skos:altLabel>
    </owl:Class>
    


    <!-- http://www.semanticweb.org/david/ontologies/2013/0/1.3.6.1.4.1.19376.1.8.2.1.431 -->

    <owl:Class rdf:about="&pathLex;431">
        <rdfs:subClassOf rdf:resource="&pathLex;10003"/>
        <skos:definition xml:lang="en">Breast-Infiltrating malignant neoplasm-Progesterone receptor</skos:definition>
        <skos:prefLabel xml:lang="en">Progesterone receptor</skos:prefLabel>
    </owl:Class>
    


    <!-- http://www.semanticweb.org/david/ontologies/2013/0/1.3.6.1.4.1.19376.1.8.2.1.432 -->

    <owl:Class rdf:about="&pathLex;432">
        <rdfs:subClassOf rdf:resource="&pathLex;10003"/>
        <skos:definition xml:lang="en">Breast-Infiltrating malignant neoplasm-Estrogen receptor</skos:definition>
        <skos:prefLabel xml:lang="en">Estrogen receptor</skos:prefLabel>
    </owl:Class>
    


    <!-- http://www.semanticweb.org/david/ontologies/2013/0/1.3.6.1.4.1.19376.1.8.2.1.433 -->

    <owl:Class rdf:about="&pathLex;433">
        <rdfs:subClassOf rdf:resource="&pathLex;10003"/>
        <skos:definition xml:lang="en">Breast-Infiltrating malignant neoplasm-HER2/neu (FISH method)</skos:definition>
        <skos:prefLabel xml:lang="en">HER2/neu (FISH method)</skos:prefLabel>
    </owl:Class>
    


    <!-- http://www.semanticweb.org/david/ontologies/2013/0/1.3.6.1.4.1.19376.1.8.2.1.434 -->

    <owl:Class rdf:about="&pathLex;434">
        <rdfs:subClassOf rdf:resource="&pathLex;10003"/>
        <skos:definition xml:lang="en">Breast-Infiltrating malignant neoplasm-HER2/neu (immunoperoxidase study)</skos:definition>
        <skos:prefLabel xml:lang="en">Specimen size, largest dimension</skos:prefLabel>
    </owl:Class>
    


    <!-- http://www.semanticweb.org/david/ontologies/2013/0/1.3.6.1.4.1.19376.1.8.2.1.435 -->

    <owl:Class rdf:about="&pathLex;435">
        <rdfs:subClassOf rdf:resource="&pathLex;10011"/>
        <skos:definition xml:lang="en">Breast-In situ neoplasm-Lesion size, largest dimension</skos:definition>
        <skos:prefLabel xml:lang="en">Lesion size, largest dimension</skos:prefLabel>
    </owl:Class>
    


    <!-- http://www.semanticweb.org/david/ontologies/2013/0/1.3.6.1.4.1.19376.1.8.2.1.436 -->

    <owl:Class rdf:about="&pathLex;436">
        <rdfs:subClassOf rdf:resource="&pathLex;1840"/>
        <skos:prefLabel xml:lang="en">Breast-Histologic type</skos:prefLabel>
        <skos:definition xml:lang="en">Breast-In situ neoplasm-Histologic type</skos:definition>
        <skos:altLabel xml:lang="en">Histologic type</skos:altLabel>
    </owl:Class>
    


    <!-- http://www.semanticweb.org/david/ontologies/2013/0/1.3.6.1.4.1.19376.1.8.2.1.437 -->

    <owl:Class rdf:about="&pathLex;437">
        <rdfs:subClassOf rdf:resource="&pathLex;21"/>
        <skos:prefLabel xml:lang="en">Breast-Histologic type</skos:prefLabel>
        <skos:definition xml:lang="en">Breast-Infiltrating malignant neoplasm-Histologic type</skos:definition>
        <skos:altLabel xml:lang="en">Histologic type</skos:altLabel>
    </owl:Class>
    


    <!-- http://www.semanticweb.org/david/ontologies/2013/0/1.3.6.1.4.1.19376.1.8.2.1.438 -->

    <owl:Class rdf:about="&pathLex;438">
        <rdfs:subClassOf rdf:resource="&pathLex;99999"/>
        <skos:prefLabel xml:lang="en">Margins involvement</skos:prefLabel>
        <skos:definition xml:lang="en">Testis-Infiltrating malignant neoplasm-Margins involvement</skos:definition>
    </owl:Class>
    


    <!-- http://www.semanticweb.org/david/ontologies/2013/0/1.3.6.1.4.1.19376.1.8.2.1.439 -->

    <owl:Class rdf:about="&pathLex;439">
        <rdfs:subClassOf rdf:resource="&pathLex;99999"/>
        <skos:prefLabel xml:lang="en">Distance of lesion from closest uninvolved margin</skos:prefLabel>
        <skos:definition xml:lang="en">Testis-Infiltrating malignant neoplasm-Distance of lesion from closest uninvolved margin</skos:definition>
    </owl:Class>
    


    <!-- http://www.semanticweb.org/david/ontologies/2013/0/1.3.6.1.4.1.19376.1.8.2.1.44 -->

    <owl:Class rdf:about="&pathLex;44">
        <rdfs:subClassOf rdf:resource="&pathLex;10010"/>
        <skos:definition xml:lang="en">Cervix-Infiltrating malignant neoplasm-Lymph node capsule involvement</skos:definition>
        <skos:prefLabel xml:lang="en">Lymph node capsule involvement</skos:prefLabel>
    </owl:Class>
    


    <!-- http://www.semanticweb.org/david/ontologies/2013/0/1.3.6.1.4.1.19376.1.8.2.1.440 -->

    <owl:Class rdf:about="&pathLex;440">
        <rdfs:subClassOf rdf:resource="&pathLex;99999"/>
        <skos:prefLabel xml:lang="en">Lymph-vascular invasion</skos:prefLabel>
        <skos:definition xml:lang="en">Testis-Infiltrating malignant neoplasm-Lymph-vascular invasion</skos:definition>
    </owl:Class>
    


    <!-- http://www.semanticweb.org/david/ontologies/2013/0/1.3.6.1.4.1.19376.1.8.2.1.441 -->

    <owl:Class rdf:about="&pathLex;441">
        <rdfs:subClassOf rdf:resource="&pathLex;99999"/>
        <skos:prefLabel xml:lang="en">Extent</skos:prefLabel>
        <skos:definition xml:lang="en">Testis-Infiltrating malignant neoplasm-Extent</skos:definition>
    </owl:Class>
    


    <!-- http://www.semanticweb.org/david/ontologies/2013/0/1.3.6.1.4.1.19376.1.8.2.1.442 -->

    <owl:Class rdf:about="&pathLex;442">
        <rdfs:subClassOf rdf:resource="&pathLex;99999"/>
        <skos:prefLabel xml:lang="en">Margin site</skos:prefLabel>
        <skos:definition xml:lang="en">Testis-Infiltrating malignant neoplasm-Margin site</skos:definition>
    </owl:Class>
    


    <!-- http://www.semanticweb.org/david/ontologies/2013/0/1.3.6.1.4.1.19376.1.8.2.1.443 -->

    <owl:Class rdf:about="&pathLex;443">
        <rdfs:subClassOf rdf:resource="&pathLex;99999"/>
        <skos:prefLabel xml:lang="en">Number of lymph nodes involved</skos:prefLabel>
        <skos:definition xml:lang="en">Testis-Infiltrating malignant neoplasm-Number of lymph nodes involved</skos:definition>
    </owl:Class>
    


    <!-- http://www.semanticweb.org/david/ontologies/2013/0/1.3.6.1.4.1.19376.1.8.2.1.444 -->

    <owl:Class rdf:about="&pathLex;444">
        <rdfs:subClassOf rdf:resource="&pathLex;99999"/>
        <skos:prefLabel xml:lang="en">Number of lymph nodes examined</skos:prefLabel>
        <skos:definition xml:lang="en">Testis-Infiltrating malignant neoplasm-Number of lymph nodes examined</skos:definition>
    </owl:Class>
    


    <!-- http://www.semanticweb.org/david/ontologies/2013/0/1.3.6.1.4.1.19376.1.8.2.1.446 -->

    <owl:Class rdf:about="&pathLex;446">
        <rdfs:subClassOf rdf:resource="&pathLex;99999"/>
        <skos:definition xml:lang="en">Testis-Infiltrating malignant neoplasm-pN</skos:definition>
        <skos:prefLabel xml:lang="en">pN</skos:prefLabel>
    </owl:Class>
    


    <!-- http://www.semanticweb.org/david/ontologies/2013/0/1.3.6.1.4.1.19376.1.8.2.1.448 -->

    <owl:Class rdf:about="&pathLex;448">
        <rdfs:subClassOf rdf:resource="&pathLex;99999"/>
        <skos:definition xml:lang="en">Testis-Infiltrating malignant neoplasm-pT</skos:definition>
        <skos:prefLabel xml:lang="en">pT</skos:prefLabel>
    </owl:Class>
    


    <!-- http://www.semanticweb.org/david/ontologies/2013/0/1.3.6.1.4.1.19376.1.8.2.1.449 -->

    <owl:Class rdf:about="&pathLex;449">
        <rdfs:subClassOf rdf:resource="&pathLex;99999"/>
        <skos:prefLabel xml:lang="en">Lesion size, largest dimension</skos:prefLabel>
        <skos:definition xml:lang="en">Testis-Infiltrating malignant neoplasm-Lesion size, largest dimension</skos:definition>
    </owl:Class>
    


    <!-- http://www.semanticweb.org/david/ontologies/2013/0/1.3.6.1.4.1.19376.1.8.2.1.45 -->

    <owl:Class rdf:about="&pathLex;45">
        <rdfs:subClassOf rdf:resource="&pathLex;10010"/>
        <skos:definition xml:lang="en">Generic-Infiltrating malignant neoplasm-Lymph node site</skos:definition>
        <skos:prefLabel xml:lang="en">Lymph node site</skos:prefLabel>
    </owl:Class>
    


    <!-- http://www.semanticweb.org/david/ontologies/2013/0/1.3.6.1.4.1.19376.1.8.2.1.450 -->

    <owl:Class rdf:about="&pathLex;450">
        <rdfs:subClassOf rdf:resource="&pathLex;99999"/>
        <skos:prefLabel xml:lang="en">Histologic type</skos:prefLabel>
        <skos:definition xml:lang="en">Testis-Infiltrating malignant neoplasm-Histologic type</skos:definition>
    </owl:Class>
    


    <!-- http://www.semanticweb.org/david/ontologies/2013/0/1.3.6.1.4.1.19376.1.8.2.1.451 -->

    <owl:Class rdf:about="&pathLex;451">
        <rdfs:subClassOf rdf:resource="&pathLex;99999"/>
        <skos:prefLabel xml:lang="en">Margins involvement</skos:prefLabel>
        <skos:definition xml:lang="en">Thyroid-Infiltrating malignant neoplasm-Margins involvement</skos:definition>
    </owl:Class>
    


    <!-- http://www.semanticweb.org/david/ontologies/2013/0/1.3.6.1.4.1.19376.1.8.2.1.452 -->

    <owl:Class rdf:about="&pathLex;452">
        <rdfs:subClassOf rdf:resource="&pathLex;99999"/>
        <skos:prefLabel xml:lang="en">Distance of lesion from closest uninvolved margin</skos:prefLabel>
        <skos:definition xml:lang="en">Thyroid-Infiltrating malignant neoplasm-Distance of lesion from closest uninvolved margin</skos:definition>
    </owl:Class>
    


    <!-- http://www.semanticweb.org/david/ontologies/2013/0/1.3.6.1.4.1.19376.1.8.2.1.453 -->

    <owl:Class rdf:about="&pathLex;453">
        <rdfs:subClassOf rdf:resource="&pathLex;99999"/>
        <skos:prefLabel xml:lang="en">Lymph-vascular invasion</skos:prefLabel>
        <skos:definition xml:lang="en">Thyroid-Infiltrating malignant neoplasm-Lymph-vascular invasion</skos:definition>
    </owl:Class>
    


    <!-- http://www.semanticweb.org/david/ontologies/2013/0/1.3.6.1.4.1.19376.1.8.2.1.454 -->

    <owl:Class rdf:about="&pathLex;454">
        <rdfs:subClassOf rdf:resource="&pathLex;99999"/>
        <skos:prefLabel xml:lang="en">Extent</skos:prefLabel>
        <skos:definition xml:lang="en">Thyroid-Infiltrating malignant neoplasm-Extent</skos:definition>
    </owl:Class>
    


    <!-- http://www.semanticweb.org/david/ontologies/2013/0/1.3.6.1.4.1.19376.1.8.2.1.455 -->

    <owl:Class rdf:about="&pathLex;455">
        <rdfs:subClassOf rdf:resource="&pathLex;99999"/>
        <skos:prefLabel xml:lang="en">Perineural invasion</skos:prefLabel>
        <skos:definition xml:lang="en">Thyroid-Infiltrating malignant neoplasm-Perineural invasion</skos:definition>
    </owl:Class>
    


    <!-- http://www.semanticweb.org/david/ontologies/2013/0/1.3.6.1.4.1.19376.1.8.2.1.456 -->

    <owl:Class rdf:about="&pathLex;456">
        <rdfs:subClassOf rdf:resource="&pathLex;99999"/>
        <skos:prefLabel xml:lang="en">Lymph node capsule involvement</skos:prefLabel>
        <skos:definition xml:lang="en">Thyroid-Infiltrating malignant neoplasm-Lymph node capsule involvement</skos:definition>
    </owl:Class>
    


    <!-- http://www.semanticweb.org/david/ontologies/2013/0/1.3.6.1.4.1.19376.1.8.2.1.457 -->

    <owl:Class rdf:about="&pathLex;457">
        <rdfs:subClassOf rdf:resource="&pathLex;99999"/>
        <skos:prefLabel xml:lang="en">Lesion site</skos:prefLabel>
        <skos:definition xml:lang="en">Thyroid-Infiltrating malignant neoplasm-Lesion site</skos:definition>
    </owl:Class>
    


    <!-- http://www.semanticweb.org/david/ontologies/2013/0/1.3.6.1.4.1.19376.1.8.2.1.458 -->

    <owl:Class rdf:about="&pathLex;458">
        <rdfs:subClassOf rdf:resource="&pathLex;99999"/>
        <skos:prefLabel xml:lang="en">Number of lymph nodes involved</skos:prefLabel>
        <skos:definition xml:lang="en">Thyroid-Infiltrating malignant neoplasm-Number of lymph nodes involved</skos:definition>
    </owl:Class>
    


    <!-- http://www.semanticweb.org/david/ontologies/2013/0/1.3.6.1.4.1.19376.1.8.2.1.459 -->

    <owl:Class rdf:about="&pathLex;459">
        <rdfs:subClassOf rdf:resource="&pathLex;99999"/>
        <skos:prefLabel xml:lang="en">Number of lymph nodes examined</skos:prefLabel>
        <skos:definition xml:lang="en">Thyroid-Infiltrating malignant neoplasm-Number of lymph nodes examined</skos:definition>
    </owl:Class>
    


    <!-- http://www.semanticweb.org/david/ontologies/2013/0/1.3.6.1.4.1.19376.1.8.2.1.461 -->

    <owl:Class rdf:about="&pathLex;461">
        <rdfs:subClassOf rdf:resource="&pathLex;99999"/>
        <skos:definition xml:lang="en">Thyroid-Infiltrating malignant neoplasm-pN</skos:definition>
        <skos:prefLabel xml:lang="en">pN</skos:prefLabel>
    </owl:Class>
    


    <!-- http://www.semanticweb.org/david/ontologies/2013/0/1.3.6.1.4.1.19376.1.8.2.1.462 -->

    <owl:Class rdf:about="&pathLex;462">
        <rdfs:subClassOf rdf:resource="&pathLex;99999"/>
        <skos:prefLabel xml:lang="en">Specimen weight</skos:prefLabel>
        <skos:definition xml:lang="en">Thyroid-Infiltrating malignant neoplasm-Specimen weight</skos:definition>
    </owl:Class>
    


    <!-- http://www.semanticweb.org/david/ontologies/2013/0/1.3.6.1.4.1.19376.1.8.2.1.464 -->

    <owl:Class rdf:about="&pathLex;464">
        <rdfs:subClassOf rdf:resource="&pathLex;99999"/>
        <skos:definition xml:lang="en">Thyroid-Infiltrating malignant neoplasm-pT anaplasic carcinoma</skos:definition>
        <skos:prefLabel xml:lang="en">pT anaplasic carcinoma</skos:prefLabel>
    </owl:Class>
    


    <!-- http://www.semanticweb.org/david/ontologies/2013/0/1.3.6.1.4.1.19376.1.8.2.1.465 -->

    <owl:Class rdf:about="&pathLex;465">
        <rdfs:subClassOf rdf:resource="&pathLex;99999"/>
        <skos:definition xml:lang="en">Thyroid-Infiltrating malignant neoplasm-pT exept anaplasic carcinoma</skos:definition>
        <skos:prefLabel xml:lang="en">pT exept anaplasic carcinoma</skos:prefLabel>
    </owl:Class>
    


    <!-- http://www.semanticweb.org/david/ontologies/2013/0/1.3.6.1.4.1.19376.1.8.2.1.466 -->

    <owl:Class rdf:about="&pathLex;466">
        <rdfs:subClassOf rdf:resource="&pathLex;99999"/>
        <skos:prefLabel xml:lang="en">Lesion size, largest dimension</skos:prefLabel>
        <skos:definition xml:lang="en">Thyroid-Infiltrating malignant neoplasm-Lesion size, largest dimension</skos:definition>
    </owl:Class>
    


    <!-- http://www.semanticweb.org/david/ontologies/2013/0/1.3.6.1.4.1.19376.1.8.2.1.467 -->

    <owl:Class rdf:about="&pathLex;467">
        <rdfs:subClassOf rdf:resource="&pathLex;99999"/>
        <skos:prefLabel xml:lang="en">Lesion size, largest dimension</skos:prefLabel>
        <skos:definition xml:lang="en">Thyroid-Infiltrating malignant neoplasm-Lesion size, largest dimension</skos:definition>
    </owl:Class>
    


    <!-- http://www.semanticweb.org/david/ontologies/2013/0/1.3.6.1.4.1.19376.1.8.2.1.468 -->

    <owl:Class rdf:about="&pathLex;468">
        <rdfs:subClassOf rdf:resource="&pathLex;99999"/>
        <skos:prefLabel xml:lang="en">Specimen size, largest dimension</skos:prefLabel>
        <skos:definition xml:lang="en">Thyroid-Infiltrating malignant neoplasm-Specimen size, largest dimension</skos:definition>
    </owl:Class>
    


    <!-- http://www.semanticweb.org/david/ontologies/2013/0/1.3.6.1.4.1.19376.1.8.2.1.469 -->

    <owl:Class rdf:about="&pathLex;469">
        <rdfs:subClassOf rdf:resource="&pathLex;99999"/>
        <skos:prefLabel xml:lang="en">Histologic type</skos:prefLabel>
        <skos:definition xml:lang="en">Thyroid-Infiltrating malignant neoplasm-Histologic type</skos:definition>
    </owl:Class>
    


    <!-- http://www.semanticweb.org/david/ontologies/2013/0/1.3.6.1.4.1.19376.1.8.2.1.47 -->

    <owl:Class rdf:about="&pathLex;47">
        <rdfs:subClassOf rdf:resource="&pathLex;99999"/>
        <skos:definition xml:lang="en">Colon-Infiltrating malignant neoplasm-Margins involvement</skos:definition>
        <skos:prefLabel xml:lang="en">Margins involvement</skos:prefLabel>
    </owl:Class>
    


    <!-- http://www.semanticweb.org/david/ontologies/2013/0/1.3.6.1.4.1.19376.1.8.2.1.470 -->

    <owl:Class rdf:about="&pathLex;470">
        <rdfs:subClassOf rdf:resource="&pathLex;99999"/>
        <skos:prefLabel xml:lang="en">Margins involvement</skos:prefLabel>
        <skos:definition xml:lang="en">Urinary bladder-Infiltrating malignant neoplasm-Margins involvement</skos:definition>
    </owl:Class>
    


    <!-- http://www.semanticweb.org/david/ontologies/2013/0/1.3.6.1.4.1.19376.1.8.2.1.471 -->

    <owl:Class rdf:about="&pathLex;471">
        <rdfs:subClassOf rdf:resource="&pathLex;99999"/>
        <skos:prefLabel xml:lang="en">Margins involvement</skos:prefLabel>
        <skos:definition xml:lang="en">Urinary bladder-Infiltrating malignant neoplasm-Margins involvement</skos:definition>
    </owl:Class>
    


    <!-- http://www.semanticweb.org/david/ontologies/2013/0/1.3.6.1.4.1.19376.1.8.2.1.472 -->

    <owl:Class rdf:about="&pathLex;472">
        <rdfs:subClassOf rdf:resource="&pathLex;99999"/>
        <skos:prefLabel xml:lang="en">Distance of lesion from closest uninvolved margin</skos:prefLabel>
        <skos:definition xml:lang="en">Urinary bladder-Infiltrating malignant neoplasm-Distance of lesion from closest uninvolved margin</skos:definition>
    </owl:Class>
    


    <!-- http://www.semanticweb.org/david/ontologies/2013/0/1.3.6.1.4.1.19376.1.8.2.1.473 -->

    <owl:Class rdf:about="&pathLex;473">
        <rdfs:subClassOf rdf:resource="&pathLex;99999"/>
        <skos:prefLabel xml:lang="en">Lymph-vascular invasion</skos:prefLabel>
        <skos:definition xml:lang="en">Urinary bladder-Infiltrating malignant neoplasm-Lymph-vascular invasion</skos:definition>
    </owl:Class>
    


    <!-- http://www.semanticweb.org/david/ontologies/2013/0/1.3.6.1.4.1.19376.1.8.2.1.474 -->

    <owl:Class rdf:about="&pathLex;474">
        <rdfs:subClassOf rdf:resource="&pathLex;99999"/>
        <skos:prefLabel xml:lang="en">Extent</skos:prefLabel>
        <skos:definition xml:lang="en">Urinary bladder-Infiltrating malignant neoplasm-Extent</skos:definition>
    </owl:Class>
    


    <!-- http://www.semanticweb.org/david/ontologies/2013/0/1.3.6.1.4.1.19376.1.8.2.1.475 -->

    <owl:Class rdf:about="&pathLex;475">
        <rdfs:subClassOf rdf:resource="&pathLex;99999"/>
        <skos:prefLabel xml:lang="en">Histologic grade (WHO 2004)</skos:prefLabel>
        <skos:definition xml:lang="en">Urinary bladder-Infiltrating malignant neoplasm-Histologic grade (WHO 2004)</skos:definition>
    </owl:Class>
    


    <!-- http://www.semanticweb.org/david/ontologies/2013/0/1.3.6.1.4.1.19376.1.8.2.1.476 -->

    <owl:Class rdf:about="&pathLex;476">
        <rdfs:subClassOf rdf:resource="&pathLex;99999"/>
        <skos:prefLabel xml:lang="en">Lesion site</skos:prefLabel>
        <skos:definition xml:lang="en">Urinary bladder-Infiltrating malignant neoplasm-Lesion site</skos:definition>
    </owl:Class>
    


    <!-- http://www.semanticweb.org/david/ontologies/2013/0/1.3.6.1.4.1.19376.1.8.2.1.477 -->

    <owl:Class rdf:about="&pathLex;477">
        <rdfs:subClassOf rdf:resource="&pathLex;99999"/>
        <skos:prefLabel xml:lang="en">Margin site</skos:prefLabel>
        <skos:definition xml:lang="en">Urinary bladder-Infiltrating malignant neoplasm-Margin site</skos:definition>
    </owl:Class>
    


    <!-- http://www.semanticweb.org/david/ontologies/2013/0/1.3.6.1.4.1.19376.1.8.2.1.478 -->

    <owl:Class rdf:about="&pathLex;478">
        <rdfs:subClassOf rdf:resource="&pathLex;99999"/>
        <skos:prefLabel xml:lang="en">Number of lymph nodes involved</skos:prefLabel>
        <skos:definition xml:lang="en">Urinary bladder-Infiltrating malignant neoplasm-Number of lymph nodes involved</skos:definition>
    </owl:Class>
    


    <!-- http://www.semanticweb.org/david/ontologies/2013/0/1.3.6.1.4.1.19376.1.8.2.1.479 -->

    <owl:Class rdf:about="&pathLex;479">
        <rdfs:subClassOf rdf:resource="&pathLex;99999"/>
        <skos:prefLabel xml:lang="en">Number of lymph nodes examined</skos:prefLabel>
        <skos:definition xml:lang="en">Urinary bladder-Infiltrating malignant neoplasm-Number of lymph nodes examined</skos:definition>
    </owl:Class>
    


    <!-- http://www.semanticweb.org/david/ontologies/2013/0/1.3.6.1.4.1.19376.1.8.2.1.481 -->

    <owl:Class rdf:about="&pathLex;481">
        <rdfs:subClassOf rdf:resource="&pathLex;99999"/>
        <skos:definition xml:lang="en">Urinary bladder-Infiltrating malignant neoplasm-pN</skos:definition>
        <skos:prefLabel xml:lang="en">pN</skos:prefLabel>
    </owl:Class>
    


    <!-- http://www.semanticweb.org/david/ontologies/2013/0/1.3.6.1.4.1.19376.1.8.2.1.483 -->

    <owl:Class rdf:about="&pathLex;483">
        <rdfs:subClassOf rdf:resource="&pathLex;99999"/>
        <skos:definition xml:lang="en">Urinary bladder-Infiltrating malignant neoplasm-pT</skos:definition>
        <skos:prefLabel xml:lang="en">pT</skos:prefLabel>
    </owl:Class>
    


    <!-- http://www.semanticweb.org/david/ontologies/2013/0/1.3.6.1.4.1.19376.1.8.2.1.484 -->

    <owl:Class rdf:about="&pathLex;484">
        <rdfs:subClassOf rdf:resource="&pathLex;99999"/>
        <skos:prefLabel xml:lang="en">Lesion size, largest dimension</skos:prefLabel>
        <skos:definition xml:lang="en">Urinary bladder-Infiltrating malignant neoplasm-Lesion size, largest dimension</skos:definition>
    </owl:Class>
    


    <!-- http://www.semanticweb.org/david/ontologies/2013/0/1.3.6.1.4.1.19376.1.8.2.1.485 -->

    <owl:Class rdf:about="&pathLex;485">
        <rdfs:subClassOf rdf:resource="&pathLex;99999"/>
        <skos:prefLabel xml:lang="en">Histologic type</skos:prefLabel>
        <skos:definition xml:lang="en">Urinary bladder-Infiltrating malignant neoplasm-Histologic type</skos:definition>
    </owl:Class>
    


    <!-- http://www.semanticweb.org/david/ontologies/2013/0/1.3.6.1.4.1.19376.1.8.2.1.486 -->

    <owl:Class rdf:about="&pathLex;486">
        <rdfs:subClassOf rdf:resource="&pathLex;10005"/>
        <skos:prefLabel xml:lang="en">Cervix-Histologic grade (WHO)</skos:prefLabel>
        <skos:definition xml:lang="en">Cervix-Infiltrating malignant neoplasm-Histologic grade (WHO)</skos:definition>
        <skos:altLabel xml:lang="en">Histologic grade (WHO)</skos:altLabel>
    </owl:Class>
    


    <!-- http://www.semanticweb.org/david/ontologies/2013/0/1.3.6.1.4.1.19376.1.8.2.1.487 -->

    <owl:Class rdf:about="&pathLex;487">
        <rdfs:subClassOf rdf:resource="&pathLex;1836"/>
        <skos:definition xml:lang="en">Cervix-Infiltrating malignant neoplasm-Margin site</skos:definition>
        <skos:prefLabel xml:lang="en">Cervix-Margin site</skos:prefLabel>
        <skos:altLabel xml:lang="en">Margin site</skos:altLabel>
    </owl:Class>
    


    <!-- http://www.semanticweb.org/david/ontologies/2013/0/1.3.6.1.4.1.19376.1.8.2.1.489 -->

    <owl:Class rdf:about="&pathLex;489">
        <rdfs:subClassOf rdf:resource="&pathLex;1433"/>
        <skos:prefLabel xml:lang="en">Cervix-Infiltrating malignant neoplasm-pM</skos:prefLabel>
        <skos:definition xml:lang="en">Cervix-Infiltrating malignant neoplasm-pM</skos:definition>
        <skos:altLabel xml:lang="en">pM</skos:altLabel>
    </owl:Class>
    


    <!-- http://www.semanticweb.org/david/ontologies/2013/0/1.3.6.1.4.1.19376.1.8.2.1.49 -->

    <owl:Class rdf:about="&pathLex;49">
        <rdfs:subClassOf rdf:resource="&pathLex;54"/>
        <skos:definition xml:lang="en">Breast-Infiltrating malignant neoplasm-Margins involvement</skos:definition>
        <skos:prefLabel xml:lang="en">Breast-Margins involvement</skos:prefLabel>
        <skos:altLabel xml:lang="en">Margins involvement</skos:altLabel>
    </owl:Class>
    


    <!-- http://www.semanticweb.org/david/ontologies/2013/0/1.3.6.1.4.1.19376.1.8.2.1.491 -->

    <owl:Class rdf:about="&pathLex;491">
        <rdfs:subClassOf rdf:resource="&pathLex;6"/>
        <skos:prefLabel xml:lang="en">Cervix-Lesion site</skos:prefLabel>
        <skos:definition xml:lang="en">Cervix-Lesion-Lesion site</skos:definition>
        <skos:altLabel xml:lang="en">Lesion site</skos:altLabel>
    </owl:Class>
    


    <!-- http://www.semanticweb.org/david/ontologies/2013/0/1.3.6.1.4.1.19376.1.8.2.1.492 -->

    <owl:Class rdf:about="&pathLex;492">
        <rdfs:subClassOf rdf:resource="&pathLex;1841"/>
        <skos:definition xml:lang="en">Cervix-In situ neoplasm-Lesion site</skos:definition>
        <skos:prefLabel xml:lang="en">Cervix-Lesion site</skos:prefLabel>
        <skos:altLabel xml:lang="en">Lesion site</skos:altLabel>
    </owl:Class>
    


    <!-- http://www.semanticweb.org/david/ontologies/2013/0/1.3.6.1.4.1.19376.1.8.2.1.493 -->

    <owl:Class rdf:about="&pathLex;493">
        <rdfs:subClassOf rdf:resource="&pathLex;99999"/>
        <skos:definition xml:lang="en">Colon-Infiltrating malignant neoplasm-Microsatellite instability</skos:definition>
        <skos:prefLabel xml:lang="en">Microsatellite instability</skos:prefLabel>
    </owl:Class>
    


    <!-- http://www.semanticweb.org/david/ontologies/2013/0/1.3.6.1.4.1.19376.1.8.2.1.494 -->

    <owl:Class rdf:about="&pathLex;494">
        <rdfs:subClassOf rdf:resource="&pathLex;99999"/>
        <skos:definition xml:lang="en">Colon-Infiltrating malignant neoplasm-Mismatch Repair Proteins-MLH1 (Immunohistochemistry Study)</skos:definition>
        <skos:prefLabel xml:lang="en">Mismatch Repair Proteins-MLH1 (Immunohistochemistry Study)</skos:prefLabel>
    </owl:Class>
    


    <!-- http://www.semanticweb.org/david/ontologies/2013/0/1.3.6.1.4.1.19376.1.8.2.1.495 -->

    <owl:Class rdf:about="&pathLex;495">
        <rdfs:subClassOf rdf:resource="&pathLex;99999"/>
        <skos:definition xml:lang="en">Colon-Infiltrating malignant neoplasm-Mismatch Repair Proteins-MLH2 (Immunohistochemistry Study)</skos:definition>
        <skos:prefLabel xml:lang="en">Mismatch Repair Proteins-MLH2 (Immunohistochemistry Study)</skos:prefLabel>
    </owl:Class>
    


    <!-- http://www.semanticweb.org/david/ontologies/2013/0/1.3.6.1.4.1.19376.1.8.2.1.496 -->

    <owl:Class rdf:about="&pathLex;496">
        <rdfs:subClassOf rdf:resource="&pathLex;99999"/>
        <skos:definition xml:lang="en">Colon-Infiltrating malignant neoplasm-Mismatch Repair Proteins-MLH6 (Immunohistochemistry Study)</skos:definition>
        <skos:prefLabel xml:lang="en">Mismatch Repair Proteins-MLH6 (Immunohistochemistry Study)</skos:prefLabel>
    </owl:Class>
    


    <!-- http://www.semanticweb.org/david/ontologies/2013/0/1.3.6.1.4.1.19376.1.8.2.1.497 -->

    <owl:Class rdf:about="&pathLex;497">
        <rdfs:subClassOf rdf:resource="&pathLex;99999"/>
        <skos:prefLabel xml:lang="en">BRAF V600E mutational analysis</skos:prefLabel>
        <skos:definition xml:lang="en">Colon-Infiltrating malignant neoplasm-BRAF V600E mutational analysis</skos:definition>
    </owl:Class>
    


    <!-- http://www.semanticweb.org/david/ontologies/2013/0/1.3.6.1.4.1.19376.1.8.2.1.498 -->

    <owl:Class rdf:about="&pathLex;498">
        <rdfs:subClassOf rdf:resource="&pathLex;99999"/>
        <skos:definition xml:lang="en">Colon-Infiltrating malignant neoplasm-KRAS mutational analysis</skos:definition>
        <skos:prefLabel xml:lang="en">KRAS mutational analysis</skos:prefLabel>
    </owl:Class>
    


    <!-- http://www.semanticweb.org/david/ontologies/2013/0/1.3.6.1.4.1.19376.1.8.2.1.499 -->

    <owl:Class rdf:about="&pathLex;499">
        <rdfs:subClassOf rdf:resource="&pathLex;99999"/>
        <skos:definition xml:lang="en">Colon-Infiltrating malignant neoplasm-Mismatch Repair Proteins-PMS2 (Immunohistochemistry Study)</skos:definition>
        <skos:prefLabel xml:lang="en">Mismatch Repair Proteins-PMS2 (Immunohistochemistry Study)</skos:prefLabel>
    </owl:Class>
    


    <!-- http://www.semanticweb.org/david/ontologies/2013/0/1.3.6.1.4.1.19376.1.8.2.1.50 -->

    <owl:Class rdf:about="&pathLex;50">
        <rdfs:subClassOf rdf:resource="&pathLex;99999"/>
        <skos:definition xml:lang="en">Esophagus-Infiltrating malignant neoplasm-Margins involvement</skos:definition>
        <skos:prefLabel xml:lang="en">Margins involvement</skos:prefLabel>
    </owl:Class>
    


    <!-- http://www.semanticweb.org/david/ontologies/2013/0/1.3.6.1.4.1.19376.1.8.2.1.500 -->

    <owl:Class rdf:about="&pathLex;500">
        <rdfs:subClassOf rdf:resource="&pathLex;10008"/>
        <skos:prefLabel xml:lang="en">Cervix</skos:prefLabel>
        <skos:definition xml:lang="en">Cervix-Specimen-Target site-Col utérin</skos:definition>
    </owl:Class>
    


    <!-- http://www.semanticweb.org/david/ontologies/2013/0/1.3.6.1.4.1.19376.1.8.2.1.501 -->

    <owl:Class rdf:about="&pathLex;501">
        <rdfs:subClassOf rdf:resource="&pathLex;10009"/>
        <skos:definition xml:lang="en">Cervix-Specimen-Specimen collection procedure-Radical hysterectomy</skos:definition>
        <skos:prefLabel xml:lang="en">Radical hysterectomy</skos:prefLabel>
    </owl:Class>
    


    <!-- http://www.semanticweb.org/david/ontologies/2013/0/1.3.6.1.4.1.19376.1.8.2.1.507 -->

    <owl:Class rdf:about="&pathLex;507">
        <rdfs:subClassOf rdf:resource="&pathLex;138"/>
        <skos:definition xml:lang="en">Cervix-Infiltrating malignant neoplasm-Cytologic type-Invasive carcinoma</skos:definition>
        <skos:prefLabel xml:lang="en">Invasive carcinoma</skos:prefLabel>
    </owl:Class>
    


    <!-- http://www.semanticweb.org/david/ontologies/2013/0/1.3.6.1.4.1.19376.1.8.2.1.508 -->

    <owl:Class rdf:about="&pathLex;508">
        <rdfs:subClassOf rdf:resource="&pathLex;141"/>
        <skos:definition xml:lang="en">Cervix-Infiltrating malignant neoplasm-Histologic type-Endocervical type Mucinous Adenocarcinoma</skos:definition>
        <skos:prefLabel xml:lang="en">Endocervical type Mucinous Adenocarcinoma</skos:prefLabel>
    </owl:Class>
    


    <!-- http://www.semanticweb.org/david/ontologies/2013/0/1.3.6.1.4.1.19376.1.8.2.1.509 -->

    <owl:Class rdf:about="&pathLex;509">
        <rdfs:subClassOf rdf:resource="&pathLex;141"/>
        <skos:definition xml:lang="en">Cervix-Infiltrating malignant neoplasm-Histologic type-Intestinal type Mucinous Adenocarcinoma</skos:definition>
        <skos:prefLabel xml:lang="en">Intestinal type Mucinous Adenocarcinoma</skos:prefLabel>
    </owl:Class>
    


    <!-- http://www.semanticweb.org/david/ontologies/2013/0/1.3.6.1.4.1.19376.1.8.2.1.51 -->

    <owl:Class rdf:about="&pathLex;51">
        <rdfs:subClassOf rdf:resource="&pathLex;99999"/>
        <skos:definition xml:lang="en">Esophagus-Infiltrating malignant neoplasm-Margins involvement</skos:definition>
        <skos:prefLabel xml:lang="en">Margins involvement</skos:prefLabel>
    </owl:Class>
    


    <!-- http://www.semanticweb.org/david/ontologies/2013/0/1.3.6.1.4.1.19376.1.8.2.1.510 -->

    <owl:Class rdf:about="&pathLex;510">
        <rdfs:subClassOf rdf:resource="&pathLex;141"/>
        <skos:definition xml:lang="en">Cervix-Infiltrating malignant neoplasm-Histologic type-Other Mucinous Adenocarcinoma</skos:definition>
        <skos:prefLabel xml:lang="en">Other Mucinous Adenocarcinoma</skos:prefLabel>
    </owl:Class>
    


    <!-- http://www.semanticweb.org/david/ontologies/2013/0/1.3.6.1.4.1.19376.1.8.2.1.513 -->

    <owl:Class rdf:about="&pathLex;513">
        <rdfs:subClassOf rdf:resource="&pathLex;141"/>
        <skos:definition xml:lang="en">Cervix-Infiltrating malignant neoplasm-Histologic type-Endometrioid Adenocarcinoma</skos:definition>
        <skos:prefLabel xml:lang="en">Endometrioid Adenocarcinoma</skos:prefLabel>
    </owl:Class>
    


    <!-- http://www.semanticweb.org/david/ontologies/2013/0/1.3.6.1.4.1.19376.1.8.2.1.514 -->

    <owl:Class rdf:about="&pathLex;514">
        <rdfs:subClassOf rdf:resource="&pathLex;141"/>
        <skos:definition xml:lang="en">Cervix-Infiltrating malignant neoplasm-Histologic type-Clear cell Adenocarcinoma</skos:definition>
        <skos:prefLabel xml:lang="en">Clear cell Adenocarcinoma</skos:prefLabel>
    </owl:Class>
    


    <!-- http://www.semanticweb.org/david/ontologies/2013/0/1.3.6.1.4.1.19376.1.8.2.1.519 -->

    <owl:Class rdf:about="&pathLex;519">
        <rdfs:subClassOf rdf:resource="&pathLex;73"/>
        <skos:definition xml:lang="en">Cervix-Infiltrating malignant neoplasm-Histologic grade (FIGO)-FIGO grade 1</skos:definition>
        <skos:prefLabel xml:lang="en">FIGO grade 1</skos:prefLabel>
    </owl:Class>
    


    <!-- http://www.semanticweb.org/david/ontologies/2013/0/1.3.6.1.4.1.19376.1.8.2.1.52 -->

    <owl:Class rdf:about="&pathLex;52">
        <rdfs:subClassOf rdf:resource="&pathLex;99999"/>
        <skos:definition xml:lang="en">Esophagus-Infiltrating malignant neoplasm-Margins involvement</skos:definition>
        <skos:prefLabel xml:lang="en">Margins involvement</skos:prefLabel>
    </owl:Class>
    


    <!-- http://www.semanticweb.org/david/ontologies/2013/0/1.3.6.1.4.1.19376.1.8.2.1.520 -->

    <owl:Class rdf:about="&pathLex;520">
        <rdfs:subClassOf rdf:resource="&pathLex;73"/>
        <skos:definition xml:lang="en">Cervix-Infiltrating malignant neoplasm-Histologic grade (FIGO)-FIGO grade 2</skos:definition>
        <skos:prefLabel xml:lang="en">FIGO grade 2</skos:prefLabel>
    </owl:Class>
    


    <!-- http://www.semanticweb.org/david/ontologies/2013/0/1.3.6.1.4.1.19376.1.8.2.1.521 -->

    <owl:Class rdf:about="&pathLex;521">
        <rdfs:subClassOf rdf:resource="&pathLex;73"/>
        <skos:definition xml:lang="en">Cervix-Infiltrating malignant neoplasm-Histologic grade (FIGO)-FIGO grade 3</skos:definition>
        <skos:prefLabel xml:lang="en">FIGO grade 3</skos:prefLabel>
    </owl:Class>
    


    <!-- http://www.semanticweb.org/david/ontologies/2013/0/1.3.6.1.4.1.19376.1.8.2.1.532 -->

    <owl:Class rdf:about="&pathLex;532">
        <rdfs:subClassOf rdf:resource="&pathLex;135"/>
        <skos:definition xml:lang="en">Cervix-Infiltrating malignant neoplasm-pT-pT1 [I]: Cervical carcinoma confined to uterus (extension to corpus should be disregarded)</skos:definition>
        <skos:prefLabel xml:lang="en">pT1 [I]: Cervical carcinoma confined to uterus (extension to corpus should be disregarded)</skos:prefLabel>
    </owl:Class>
    


    <!-- http://www.semanticweb.org/david/ontologies/2013/0/1.3.6.1.4.1.19376.1.8.2.1.533 -->

    <owl:Class rdf:about="&pathLex;533">
        <rdfs:subClassOf rdf:resource="&pathLex;135"/>
        <skos:definition xml:lang="en">Cervix-Infiltrating malignant neoplasm-pT-pT1a [IA]: Invasive carcinoma diagnosed by microscopy only. All macroscopically visible lesions (even with superficial invasion) are pT1b/1B.</skos:definition>
        <skos:prefLabel xml:lang="en">pT1a [IA]: Invasive carcinoma diagnosed by microscopy only. All macroscopically visible lesions (even with superficial invasion) are pT1b/1B.</skos:prefLabel>
    </owl:Class>
    


    <!-- http://www.semanticweb.org/david/ontologies/2013/0/1.3.6.1.4.1.19376.1.8.2.1.534 -->

    <owl:Class rdf:about="&pathLex;534">
        <rdfs:subClassOf rdf:resource="&pathLex;135"/>
        <skos:definition xml:lang="en">Cervix-Infiltrating malignant neoplasm-pT-pT1a1 [IA1]: Stromal invasion &lt; =3.0 mm in depth and horizontal spread &lt; =7.0 mm</skos:definition>
        <skos:prefLabel xml:lang="en">pT1a1 [IA1]: Stromal invasion &lt; =3.0 mm in depth and horizontal spread &lt; =7.0 mm</skos:prefLabel>
    </owl:Class>
    


    <!-- http://www.semanticweb.org/david/ontologies/2013/0/1.3.6.1.4.1.19376.1.8.2.1.535 -->

    <owl:Class rdf:about="&pathLex;535">
        <rdfs:subClassOf rdf:resource="&pathLex;135"/>
        <skos:definition xml:lang="en">Cervix-Infiltrating malignant neoplasm-pT-pT1a2 [IA2]: Stromal invasion &gt;3.0 mm but not more than 5.0 mm in depth and horizontal spread 􀀁7.0 mm</skos:definition>
        <skos:prefLabel xml:lang="en">pT1a2 [IA2]: Stromal invasion &gt;3.0 mm but not more than 5.0 mm in depth and horizontal spread 􀀁7.0 mm</skos:prefLabel>
    </owl:Class>
    


    <!-- http://www.semanticweb.org/david/ontologies/2013/0/1.3.6.1.4.1.19376.1.8.2.1.536 -->

    <owl:Class rdf:about="&pathLex;536">
        <rdfs:subClassOf rdf:resource="&pathLex;135"/>
        <skos:definition xml:lang="en">Cervix-Infiltrating malignant neoplasm-pT-pT1b [IB]: Clinically visible lesion confined to the cervix or microscopic lesion greater than T1a2/IA2</skos:definition>
        <skos:prefLabel xml:lang="en">pT1b [IB]: Clinically visible lesion confined to the cervix or microscopic lesion greater than T1a2/IA2</skos:prefLabel>
    </owl:Class>
    


    <!-- http://www.semanticweb.org/david/ontologies/2013/0/1.3.6.1.4.1.19376.1.8.2.1.537 -->

    <owl:Class rdf:about="&pathLex;537">
        <rdfs:subClassOf rdf:resource="&pathLex;135"/>
        <skos:definition xml:lang="en">Cervix-Infiltrating malignant neoplasm-pT-pT1b1 [IB1]: Clinically visible lesion 􀀁4.0 cm in greatest dimension</skos:definition>
        <skos:prefLabel xml:lang="en">pT1b1 [IB1]: Clinically visible lesion 􀀁4.0 cm in greatest dimension</skos:prefLabel>
    </owl:Class>
    


    <!-- http://www.semanticweb.org/david/ontologies/2013/0/1.3.6.1.4.1.19376.1.8.2.1.538 -->

    <owl:Class rdf:about="&pathLex;538">
        <rdfs:subClassOf rdf:resource="&pathLex;135"/>
        <skos:definition xml:lang="en">Cervix-Infiltrating malignant neoplasm-pT-pT1b2 [IB2]: Clinically visible lesion &gt;4.0 cm in greatest dimension</skos:definition>
        <skos:prefLabel xml:lang="en">pT1b2 [IB2]: Clinically visible lesion &gt;4.0 cm in greatest dimension</skos:prefLabel>
    </owl:Class>
    


    <!-- http://www.semanticweb.org/david/ontologies/2013/0/1.3.6.1.4.1.19376.1.8.2.1.539 -->

    <owl:Class rdf:about="&pathLex;539">
        <rdfs:subClassOf rdf:resource="&pathLex;135"/>
        <skos:definition xml:lang="en">Cervix-Infiltrating malignant neoplasm-pT-pT2 [II]: Tumor invades beyond the uterus but not to pelvic wall or to lower third of vagina</skos:definition>
        <skos:prefLabel xml:lang="en">pT2 [II]: Tumor invades beyond the uterus but not to pelvic wall or to lower third of vagina</skos:prefLabel>
    </owl:Class>
    


    <!-- http://www.semanticweb.org/david/ontologies/2013/0/1.3.6.1.4.1.19376.1.8.2.1.54 -->

    <owl:Class rdf:about="&pathLex;54">
        <rdfs:subClassOf rdf:resource="&pathLex;10010"/>
        <skos:definition xml:lang="en">Generic-Infiltrating malignant neoplasm-Margins involvement</skos:definition>
        <skos:prefLabel xml:lang="en">Margins involvement</skos:prefLabel>
    </owl:Class>
    


    <!-- http://www.semanticweb.org/david/ontologies/2013/0/1.3.6.1.4.1.19376.1.8.2.1.540 -->

    <owl:Class rdf:about="&pathLex;540">
        <rdfs:subClassOf rdf:resource="&pathLex;135"/>
        <skos:definition xml:lang="en">Cervix-Infiltrating malignant neoplasm-pT-pT2a [IIA]: Tumor without parametrial invasion</skos:definition>
        <skos:prefLabel xml:lang="en">pT2a [IIA]: Tumor without parametrial invasion</skos:prefLabel>
    </owl:Class>
    


    <!-- http://www.semanticweb.org/david/ontologies/2013/0/1.3.6.1.4.1.19376.1.8.2.1.541 -->

    <owl:Class rdf:about="&pathLex;541">
        <rdfs:subClassOf rdf:resource="&pathLex;135"/>
        <skos:definition xml:lang="en">Cervix-Infiltrating malignant neoplasm-pT-pT2a1 [IIA1]: Clinically visible lesion 􀀁4.0 cm in greatest dimension</skos:definition>
        <skos:prefLabel xml:lang="en">pT2a1 [IIA1]: Clinically visible lesion 􀀁4.0 cm in greatest dimension</skos:prefLabel>
    </owl:Class>
    


    <!-- http://www.semanticweb.org/david/ontologies/2013/0/1.3.6.1.4.1.19376.1.8.2.1.542 -->

    <owl:Class rdf:about="&pathLex;542">
        <rdfs:subClassOf rdf:resource="&pathLex;135"/>
        <skos:definition xml:lang="en">Cervix-Infiltrating malignant neoplasm-pT-pT2a2 [IIA2] Clinically visible lesion &gt;4.0 cm in greatest dimension</skos:definition>
        <skos:prefLabel xml:lang="en">pT2a2 [IIA2] Clinically visible lesion &gt;4.0 cm in greatest dimension</skos:prefLabel>
    </owl:Class>
    


    <!-- http://www.semanticweb.org/david/ontologies/2013/0/1.3.6.1.4.1.19376.1.8.2.1.543 -->

    <owl:Class rdf:about="&pathLex;543">
        <rdfs:subClassOf rdf:resource="&pathLex;135"/>
        <skos:definition xml:lang="en">Cervix-Infiltrating malignant neoplasm-pT-pT2b [IIB]: Tumor with parametrial invasion</skos:definition>
        <skos:prefLabel xml:lang="en">pT2b [IIB]: Tumor with parametrial invasion</skos:prefLabel>
    </owl:Class>
    


    <!-- http://www.semanticweb.org/david/ontologies/2013/0/1.3.6.1.4.1.19376.1.8.2.1.544 -->

    <owl:Class rdf:about="&pathLex;544">
        <rdfs:subClassOf rdf:resource="&pathLex;135"/>
        <skos:definition xml:lang="en">Cervix-Infiltrating malignant neoplasm-pT-pT3 [III]: Tumor extends to the pelvic wall and/or involves the lower third of the vagina and/or causes hydronephrosis or non-functioning kidney</skos:definition>
        <skos:prefLabel xml:lang="en">pT3 [III]: Tumor extends to the pelvic wall and/or involves the lower third of the vagina and/or causes hydronephrosis or non-functioning kidney</skos:prefLabel>
    </owl:Class>
    


    <!-- http://www.semanticweb.org/david/ontologies/2013/0/1.3.6.1.4.1.19376.1.8.2.1.545 -->

    <owl:Class rdf:about="&pathLex;545">
        <rdfs:subClassOf rdf:resource="&pathLex;135"/>
        <skos:definition xml:lang="en">Cervix-Infiltrating malignant neoplasm-pT-pT3a [IIIA]: Tumor involves lower third of vagina, but not pelvic wall</skos:definition>
        <skos:prefLabel xml:lang="en">pT3a [IIIA]: Tumor involves lower third of vagina, but not pelvic wall</skos:prefLabel>
    </owl:Class>
    


    <!-- http://www.semanticweb.org/david/ontologies/2013/0/1.3.6.1.4.1.19376.1.8.2.1.546 -->

    <owl:Class rdf:about="&pathLex;546">
        <rdfs:subClassOf rdf:resource="&pathLex;135"/>
        <skos:definition xml:lang="en">Cervix-Infiltrating malignant neoplasm-pT-pT3b [IIIB]: Tumor extends to pelvic wall and/or causes hydronephrosis or non-functioning kidney</skos:definition>
        <skos:prefLabel xml:lang="en">pT3b [IIIB]: Tumor extends to pelvic wall and/or causes hydronephrosis or non-functioning kidney</skos:prefLabel>
    </owl:Class>
    


    <!-- http://www.semanticweb.org/david/ontologies/2013/0/1.3.6.1.4.1.19376.1.8.2.1.547 -->

    <owl:Class rdf:about="&pathLex;547">
        <rdfs:subClassOf rdf:resource="&pathLex;135"/>
        <skos:definition xml:lang="en">Cervix-Infiltrating malignant neoplasm-pT-pT4 [IVA]: Tumor invades the mucosa of bladder or rectum and/or extends beyond true pelvis (bullous edema is not sufficient evidence to classify a tumor as pT4)</skos:definition>
        <skos:prefLabel xml:lang="en">pT4 [IVA]: Tumor invades the mucosa of bladder or rectum and/or extends beyond true pelvis (bullous edema is not sufficient evidence to classify a tumor as pT4)</skos:prefLabel>
    </owl:Class>
    


    <!-- http://www.semanticweb.org/david/ontologies/2013/0/1.3.6.1.4.1.19376.1.8.2.1.548 -->

    <owl:Class rdf:about="&pathLex;548">
        <rdfs:subClassOf rdf:resource="&pathLex;133"/>
        <skos:definition xml:lang="en">Cervix-Infiltrating malignant neoplasm-pN-pN0: No regional lymph node metastasis</skos:definition>
        <skos:prefLabel xml:lang="en">pN0: No regional lymph node metastasis</skos:prefLabel>
    </owl:Class>
    


    <!-- http://www.semanticweb.org/david/ontologies/2013/0/1.3.6.1.4.1.19376.1.8.2.1.549 -->

    <owl:Class rdf:about="&pathLex;549">
        <rdfs:subClassOf rdf:resource="&pathLex;133"/>
        <skos:definition xml:lang="en">Cervix-Infiltrating malignant neoplasm-pN-pN1: Regional lymph node metastasis</skos:definition>
        <skos:prefLabel xml:lang="en">pN1: Regional lymph node metastasis</skos:prefLabel>
    </owl:Class>
    


    <!-- http://www.semanticweb.org/david/ontologies/2013/0/1.3.6.1.4.1.19376.1.8.2.1.550 -->

    <owl:Class rdf:about="&pathLex;550">
        <rdfs:subClassOf rdf:resource="&pathLex;10008"/>
        <skos:definition xml:lang="en">Cervix-Specimen-Target site-Uterine corpus</skos:definition>
        <skos:prefLabel xml:lang="en">Uterine corpus</skos:prefLabel>
    </owl:Class>
    


    <!-- http://www.semanticweb.org/david/ontologies/2013/0/1.3.6.1.4.1.19376.1.8.2.1.552 -->

    <owl:Class rdf:about="&pathLex;552">
        <rdfs:subClassOf rdf:resource="&pathLex;99999"/>
        <skos:definition xml:lang="en">Endometrium-Specimen-Specimen collection procedure-Supracervical hysterectomy</skos:definition>
        <skos:prefLabel xml:lang="en">Supracervical hysterectomy</skos:prefLabel>
    </owl:Class>
    


    <!-- http://www.semanticweb.org/david/ontologies/2013/0/1.3.6.1.4.1.19376.1.8.2.1.553 -->

    <owl:Class rdf:about="&pathLex;553">
        <rdfs:subClassOf rdf:resource="&pathLex;99999"/>
        <skos:definition xml:lang="en">Endometrium-Specimen-Specimen collection procedure-Radical hysterectomy</skos:definition>
        <skos:prefLabel xml:lang="en">Radical hysterectomy</skos:prefLabel>
    </owl:Class>
    


    <!-- http://www.semanticweb.org/david/ontologies/2013/0/1.3.6.1.4.1.19376.1.8.2.1.556 -->

    <owl:Class rdf:about="&pathLex;556">
        <rdfs:subClassOf rdf:resource="&pathLex;99999"/>
        <skos:prefLabel xml:lang="en">Endometrioid adenocarcinoma, not otherwise characterized</skos:prefLabel>
        <skos:definition xml:lang="en">Endometrium-Infiltrating malignant neoplasm-Histologic type-Endometrioid adenocarcinoma, not otherwise characterized</skos:definition>
    </owl:Class>
    


    <!-- http://www.semanticweb.org/david/ontologies/2013/0/1.3.6.1.4.1.19376.1.8.2.1.557 -->

    <owl:Class rdf:about="&pathLex;557">
        <rdfs:subClassOf rdf:resource="&pathLex;99999"/>
        <skos:definition xml:lang="en">Endometrium-Infiltrating malignant neoplasm-Histologic type-Mucinous adenocarcinoma</skos:definition>
        <skos:prefLabel xml:lang="en">Mucinous adenocarcinoma</skos:prefLabel>
    </owl:Class>
    


    <!-- http://www.semanticweb.org/david/ontologies/2013/0/1.3.6.1.4.1.19376.1.8.2.1.558 -->

    <owl:Class rdf:about="&pathLex;558">
        <rdfs:subClassOf rdf:resource="&pathLex;99999"/>
        <skos:definition xml:lang="en">Endometrium-Infiltrating malignant neoplasm-Histologic type-Serous adenocarcinoma</skos:definition>
        <skos:prefLabel xml:lang="en">Serous adenocarcinoma</skos:prefLabel>
    </owl:Class>
    


    <!-- http://www.semanticweb.org/david/ontologies/2013/0/1.3.6.1.4.1.19376.1.8.2.1.559 -->

    <owl:Class rdf:about="&pathLex;559">
        <rdfs:subClassOf rdf:resource="&pathLex;99999"/>
        <skos:prefLabel xml:lang="en">Clear cell adenocarcinoma</skos:prefLabel>
        <skos:definition xml:lang="en">Endometrium-Infiltrating malignant neoplasm-Histologic type-Clear cell adenocarcinoma</skos:definition>
    </owl:Class>
    


    <!-- http://www.semanticweb.org/david/ontologies/2013/0/1.3.6.1.4.1.19376.1.8.2.1.560 -->

    <owl:Class rdf:about="&pathLex;560">
        <rdfs:subClassOf rdf:resource="&pathLex;99999"/>
        <skos:definition xml:lang="en">Endometrium-Infiltrating malignant neoplasm-Histologic type-Squamous cell carcinoma</skos:definition>
        <skos:prefLabel xml:lang="en">Squamous cell carcinoma</skos:prefLabel>
    </owl:Class>
    


    <!-- http://www.semanticweb.org/david/ontologies/2013/0/1.3.6.1.4.1.19376.1.8.2.1.561 -->

    <owl:Class rdf:about="&pathLex;561">
        <rdfs:subClassOf rdf:resource="&pathLex;99999"/>
        <skos:definition xml:lang="en">Endometrium-Infiltrating malignant neoplasm-Histologic type-Undifferentiated carcinoma</skos:definition>
        <skos:prefLabel xml:lang="en">Undifferentiated carcinoma</skos:prefLabel>
    </owl:Class>
    


    <!-- http://www.semanticweb.org/david/ontologies/2013/0/1.3.6.1.4.1.19376.1.8.2.1.562 -->

    <owl:Class rdf:about="&pathLex;562">
        <rdfs:subClassOf rdf:resource="&pathLex;99999"/>
        <skos:prefLabel xml:lang="en">Carcinosarcoma (malignant müllerian mixed tumor)</skos:prefLabel>
        <skos:definition xml:lang="en">Endometrium-Infiltrating malignant neoplasm-Histologic type-Carcinosarcoma (malignant müllerian mixed tumor)</skos:definition>
    </owl:Class>
    


    <!-- http://www.semanticweb.org/david/ontologies/2013/0/1.3.6.1.4.1.19376.1.8.2.1.563 -->

    <owl:Class rdf:about="&pathLex;563">
        <rdfs:subClassOf rdf:resource="&pathLex;99999"/>
        <skos:prefLabel xml:lang="en">Endometrioid adenocarcinoma, variant (specify)</skos:prefLabel>
        <skos:definition xml:lang="en">Endometrium-Infiltrating malignant neoplasm-Histologic type-Endometrioid adenocarcinoma, variant (specify)</skos:definition>
    </owl:Class>
    


    <!-- http://www.semanticweb.org/david/ontologies/2013/0/1.3.6.1.4.1.19376.1.8.2.1.564 -->

    <owl:Class rdf:about="&pathLex;564">
        <rdfs:subClassOf rdf:resource="&pathLex;99999"/>
        <skos:prefLabel xml:lang="en">Endometrioid adenocarcinoma, variant (specify)</skos:prefLabel>
        <skos:definition xml:lang="en">Endometrium-Infiltrating malignant neoplasm-Histologic type-Endometrioid adenocarcinoma, variant (specify)</skos:definition>
    </owl:Class>
    


    <!-- http://www.semanticweb.org/david/ontologies/2013/0/1.3.6.1.4.1.19376.1.8.2.1.565 -->

    <owl:Class rdf:about="&pathLex;565">
        <rdfs:subClassOf rdf:resource="&pathLex;99999"/>
        <skos:prefLabel xml:lang="en">Endometrioid adenocarcinoma, variant (specify)</skos:prefLabel>
        <skos:definition xml:lang="en">Endometrium-Infiltrating malignant neoplasm-Histologic type-Endometrioid adenocarcinoma, variant (specify)</skos:definition>
    </owl:Class>
    


    <!-- http://www.semanticweb.org/david/ontologies/2013/0/1.3.6.1.4.1.19376.1.8.2.1.566 -->

    <owl:Class rdf:about="&pathLex;566">
        <rdfs:subClassOf rdf:resource="&pathLex;99999"/>
        <skos:definition xml:lang="en">Endometrium-Infiltrating malignant neoplasm-Histologic grade (FIGO)-FIGO grade 1</skos:definition>
        <skos:prefLabel xml:lang="en">FIGO grade 1</skos:prefLabel>
    </owl:Class>
    


    <!-- http://www.semanticweb.org/david/ontologies/2013/0/1.3.6.1.4.1.19376.1.8.2.1.567 -->

    <owl:Class rdf:about="&pathLex;567">
        <rdfs:subClassOf rdf:resource="&pathLex;99999"/>
        <skos:definition xml:lang="en">Endometrium-Infiltrating malignant neoplasm-Histologic grade (FIGO)-FIGO grade 2</skos:definition>
        <skos:prefLabel xml:lang="en">FIGO grade 2</skos:prefLabel>
    </owl:Class>
    


    <!-- http://www.semanticweb.org/david/ontologies/2013/0/1.3.6.1.4.1.19376.1.8.2.1.568 -->

    <owl:Class rdf:about="&pathLex;568">
        <rdfs:subClassOf rdf:resource="&pathLex;99999"/>
        <skos:definition xml:lang="en">Endometrium-Infiltrating malignant neoplasm-Histologic grade (FIGO)-FIGO grade 3</skos:definition>
        <skos:prefLabel xml:lang="en">FIGO grade 3</skos:prefLabel>
    </owl:Class>
    


    <!-- http://www.semanticweb.org/david/ontologies/2013/0/1.3.6.1.4.1.19376.1.8.2.1.569 -->

    <owl:Class rdf:about="&pathLex;569">
        <rdfs:subClassOf rdf:resource="&pathLex;31"/>
        <skos:prefLabel xml:lang="en">G1: Well differentiated</skos:prefLabel>
        <skos:definition xml:lang="en">Generic-Infiltrating malignant neoplasm-Histologic grade (WHO)-G1: Well differentiated</skos:definition>
    </owl:Class>
    


    <!-- http://www.semanticweb.org/david/ontologies/2013/0/1.3.6.1.4.1.19376.1.8.2.1.570 -->

    <owl:Class rdf:about="&pathLex;570">
        <rdfs:subClassOf rdf:resource="&pathLex;31"/>
        <skos:prefLabel xml:lang="en">G2: Moderately differentiated</skos:prefLabel>
        <skos:definition xml:lang="en">Generic-Infiltrating malignant neoplasm-Histologic grade (WHO)-G2: Moderately differentiated</skos:definition>
    </owl:Class>
    


    <!-- http://www.semanticweb.org/david/ontologies/2013/0/1.3.6.1.4.1.19376.1.8.2.1.571 -->

    <owl:Class rdf:about="&pathLex;571">
        <rdfs:subClassOf rdf:resource="&pathLex;31"/>
        <skos:prefLabel xml:lang="en">G3: Poorly differentiated&quot;</skos:prefLabel>
        <skos:definition xml:lang="en">Generic-Infiltrating malignant neoplasm-Histologic grade (WHO)-G3: Poorly differentiated&quot;</skos:definition>
    </owl:Class>
    


    <!-- http://www.semanticweb.org/david/ontologies/2013/0/1.3.6.1.4.1.19376.1.8.2.1.582 -->

    <owl:Class rdf:about="&pathLex;582">
        <rdfs:subClassOf rdf:resource="&pathLex;99999"/>
        <skos:definition xml:lang="en">Endometrium-Infiltrating malignant neoplasm-Lymph node site-Pelvic lymph nodes</skos:definition>
        <skos:prefLabel xml:lang="en">Pelvic lymph nodes</skos:prefLabel>
    </owl:Class>
    


    <!-- http://www.semanticweb.org/david/ontologies/2013/0/1.3.6.1.4.1.19376.1.8.2.1.583 -->

    <owl:Class rdf:about="&pathLex;583">
        <rdfs:subClassOf rdf:resource="&pathLex;99999"/>
        <skos:definition xml:lang="en">Endometrium-Infiltrating malignant neoplasm-Lymph node site-Para-aortic lymph nodes</skos:definition>
        <skos:prefLabel xml:lang="en">Para-aortic lymph nodes</skos:prefLabel>
    </owl:Class>
    


    <!-- http://www.semanticweb.org/david/ontologies/2013/0/1.3.6.1.4.1.19376.1.8.2.1.585 -->

    <owl:Class rdf:about="&pathLex;585">
        <rdfs:subClassOf rdf:resource="&pathLex;99999"/>
        <skos:definition xml:lang="en">Endometrium-Infiltrating malignant neoplasm-pT-pT0 [--]: No evidence of primary tumor</skos:definition>
        <skos:prefLabel xml:lang="en">pT0 [--]: No evidence of primary tumor</skos:prefLabel>
    </owl:Class>
    


    <!-- http://www.semanticweb.org/david/ontologies/2013/0/1.3.6.1.4.1.19376.1.8.2.1.586 -->

    <owl:Class rdf:about="&pathLex;586">
        <rdfs:subClassOf rdf:resource="&pathLex;99999"/>
        <skos:definition xml:lang="en">Endometrium-Infiltrating malignant neoplasm-pT-pT1a [IA]: Tumor limited to endometrium or invades less than one-half of the myometrium</skos:definition>
        <skos:prefLabel xml:lang="en">pT1a [IA]: Tumor limited to endometrium or invades less than one-half of the myometrium</skos:prefLabel>
    </owl:Class>
    


    <!-- http://www.semanticweb.org/david/ontologies/2013/0/1.3.6.1.4.1.19376.1.8.2.1.587 -->

    <owl:Class rdf:about="&pathLex;587">
        <rdfs:subClassOf rdf:resource="&pathLex;99999"/>
        <skos:definition xml:lang="en">Endometrium-Infiltrating malignant neoplasm-pT-pT1b [IB]: Tumor invades greater than or equal to one-half of the myometrium</skos:definition>
        <skos:prefLabel xml:lang="en">pT1b [IB]: Tumor invades greater than or equal to one-half of the myometrium</skos:prefLabel>
    </owl:Class>
    


    <!-- http://www.semanticweb.org/david/ontologies/2013/0/1.3.6.1.4.1.19376.1.8.2.1.588 -->

    <owl:Class rdf:about="&pathLex;588">
        <rdfs:subClassOf rdf:resource="&pathLex;99999"/>
        <skos:definition xml:lang="en">Endometrium-Infiltrating malignant neoplasm-pT-pT2 [II]: Tumor invades stromal connective tissue of the cervix, but does not extend beyond uterus</skos:definition>
        <skos:prefLabel xml:lang="en">pT2 [II]: Tumor invades stromal connective tissue of the cervix, but does not extend beyond uterus</skos:prefLabel>
    </owl:Class>
    


    <!-- http://www.semanticweb.org/david/ontologies/2013/0/1.3.6.1.4.1.19376.1.8.2.1.589 -->

    <owl:Class rdf:about="&pathLex;589">
        <rdfs:subClassOf rdf:resource="&pathLex;99999"/>
        <skos:definition xml:lang="en">Endometrium-Infiltrating malignant neoplasm-pT-pT3a [IIIA]: Tumor involves serosa and/or adnexa (direct extension or metastasis)</skos:definition>
        <skos:prefLabel xml:lang="en">pT3a [IIIA]: Tumor involves serosa and/or adnexa (direct extension or metastasis)</skos:prefLabel>
    </owl:Class>
    


    <!-- http://www.semanticweb.org/david/ontologies/2013/0/1.3.6.1.4.1.19376.1.8.2.1.590 -->

    <owl:Class rdf:about="&pathLex;590">
        <rdfs:subClassOf rdf:resource="&pathLex;99999"/>
        <skos:definition xml:lang="en">Endometrium-Infiltrating malignant neoplasm-pT-pT3b [IIIB]: Vaginal involvement (direct extension or metastasis) or parametrial involvement</skos:definition>
        <skos:prefLabel xml:lang="en">pT3b [IIIB]: Vaginal involvement (direct extension or metastasis) or parametrial involvement</skos:prefLabel>
    </owl:Class>
    


    <!-- http://www.semanticweb.org/david/ontologies/2013/0/1.3.6.1.4.1.19376.1.8.2.1.591 -->

    <owl:Class rdf:about="&pathLex;591">
        <rdfs:subClassOf rdf:resource="&pathLex;99999"/>
        <skos:definition xml:lang="en">Endometrium-Infiltrating malignant neoplasm-pT-pT4 [IVA]: Tumor invades bladder mucosa and/or bowel mucosa (bullous edema is not sufficient to classify a tumor as T4)</skos:definition>
        <skos:prefLabel xml:lang="en">pT4 [IVA]: Tumor invades bladder mucosa and/or bowel mucosa (bullous edema is not sufficient to classify a tumor as T4)</skos:prefLabel>
    </owl:Class>
    


    <!-- http://www.semanticweb.org/david/ontologies/2013/0/1.3.6.1.4.1.19376.1.8.2.1.592 -->

    <owl:Class rdf:about="&pathLex;592">
        <rdfs:subClassOf rdf:resource="&pathLex;99999"/>
        <skos:definition xml:lang="en">Endometrium-Infiltrating malignant neoplasm-pN-pN0: No regional lymph node metastasis</skos:definition>
        <skos:prefLabel xml:lang="en">pN0: No regional lymph node metastasis</skos:prefLabel>
    </owl:Class>
    


    <!-- http://www.semanticweb.org/david/ontologies/2013/0/1.3.6.1.4.1.19376.1.8.2.1.593 -->

    <owl:Class rdf:about="&pathLex;593">
        <rdfs:subClassOf rdf:resource="&pathLex;99999"/>
        <skos:definition xml:lang="en">Endometrium-Infiltrating malignant neoplasm-pN-pN1 [IIIC1]: Regional lymph node metastasis to pelvic lymph nodes</skos:definition>
        <skos:prefLabel xml:lang="en">pN1 [IIIC1]: Regional lymph node metastasis to pelvic lymph nodes</skos:prefLabel>
    </owl:Class>
    


    <!-- http://www.semanticweb.org/david/ontologies/2013/0/1.3.6.1.4.1.19376.1.8.2.1.594 -->

    <owl:Class rdf:about="&pathLex;594">
        <rdfs:subClassOf rdf:resource="&pathLex;99999"/>
        <skos:definition xml:lang="en">Endometrium-Infiltrating malignant neoplasm-pN-pN2 [IIIC2]: Regional lymph node metastasis to para-aortic lymph nodes, with or without positive pelvic lymph nodes</skos:definition>
        <skos:prefLabel xml:lang="en">pN2 [IIIC2]: Regional lymph node metastasis to para-aortic lymph nodes, with or without positive pelvic lymph nodes</skos:prefLabel>
    </owl:Class>
    


    <!-- http://www.semanticweb.org/david/ontologies/2013/0/1.3.6.1.4.1.19376.1.8.2.1.595 -->

    <owl:Class rdf:about="&pathLex;595">
        <rdfs:subClassOf rdf:resource="&pathLex;10008"/>
        <skos:definition xml:lang="en">Cervix-Specimen-Target site-Ovary (qualifier : right, left)</skos:definition>
        <skos:prefLabel xml:lang="en">Ovary (qualifier : right, left)</skos:prefLabel>
    </owl:Class>
    


    <!-- http://www.semanticweb.org/david/ontologies/2013/0/1.3.6.1.4.1.19376.1.8.2.1.596 -->

    <owl:Class rdf:about="&pathLex;596">
        <rdfs:subClassOf rdf:resource="&pathLex;99999"/>
        <skos:prefLabel xml:lang="en">Oophorectomy</skos:prefLabel>
        <skos:definition xml:lang="en">Ovary-Specimen-Specimen collection procedure-Oophorectomy</skos:definition>
    </owl:Class>
    


    <!-- http://www.semanticweb.org/david/ontologies/2013/0/1.3.6.1.4.1.19376.1.8.2.1.597 -->

    <owl:Class rdf:about="&pathLex;597">
        <rdfs:subClassOf rdf:resource="&pathLex;99999"/>
        <skos:definition xml:lang="en">Ovary-Specimen-Specimen collection procedure-Salpingo-oophorectomy</skos:definition>
        <skos:prefLabel xml:lang="en">Salpingo-oophorectomy</skos:prefLabel>
    </owl:Class>
    


    <!-- http://www.semanticweb.org/david/ontologies/2013/0/1.3.6.1.4.1.19376.1.8.2.1.6 -->

    <owl:Class rdf:about="&pathLex;6">
        <rdfs:subClassOf rdf:resource="&pathLex;10012"/>
        <skos:definition xml:lang="en">Generic-Lesion-Lesion site</skos:definition>
        <skos:prefLabel xml:lang="en">Lesion site</skos:prefLabel>
    </owl:Class>
    


    <!-- http://www.semanticweb.org/david/ontologies/2013/0/1.3.6.1.4.1.19376.1.8.2.1.60 -->

    <owl:Class rdf:about="&pathLex;60">
        <rdfs:subClassOf rdf:resource="&pathLex;10010"/>
        <skos:prefLabel xml:lang="en">Distance of lesion from closest uninvolved margin</skos:prefLabel>
        <skos:definition xml:lang="en">Generic-Infiltrating malignant neoplasm-Distance of lesion from closest uninvolved margin</skos:definition>
    </owl:Class>
    


    <!-- http://www.semanticweb.org/david/ontologies/2013/0/1.3.6.1.4.1.19376.1.8.2.1.600 -->

    <owl:Class rdf:about="&pathLex;600">
        <rdfs:subClassOf rdf:resource="&pathLex;99999"/>
        <skos:prefLabel xml:lang="en">Omentectomy</skos:prefLabel>
        <skos:definition xml:lang="en">Ovary-Specimen-Specimen collection procedure-Omentectomy</skos:definition>
    </owl:Class>
    


    <!-- http://www.semanticweb.org/david/ontologies/2013/0/1.3.6.1.4.1.19376.1.8.2.1.602 -->

    <owl:Class rdf:about="&pathLex;602">
        <rdfs:subClassOf rdf:resource="&pathLex;99999"/>
        <skos:definition xml:lang="en">Ovary-Infiltrating malignant neoplasm-Histologic type-Serous, borderline tumor</skos:definition>
        <skos:prefLabel xml:lang="en">Serous, borderline tumor</skos:prefLabel>
    </owl:Class>
    


    <!-- http://www.semanticweb.org/david/ontologies/2013/0/1.3.6.1.4.1.19376.1.8.2.1.603 -->

    <owl:Class rdf:about="&pathLex;603">
        <rdfs:subClassOf rdf:resource="&pathLex;99999"/>
        <skos:definition xml:lang="en">Ovary-Infiltrating malignant neoplasm-Histologic type-Serous, carcinoma</skos:definition>
        <skos:prefLabel xml:lang="en">Serous, carcinoma</skos:prefLabel>
    </owl:Class>
    


    <!-- http://www.semanticweb.org/david/ontologies/2013/0/1.3.6.1.4.1.19376.1.8.2.1.605 -->

    <owl:Class rdf:about="&pathLex;605">
        <rdfs:subClassOf rdf:resource="&pathLex;99999"/>
        <skos:prefLabel xml:lang="en">Mucinous carcinoma</skos:prefLabel>
        <skos:definition xml:lang="en">Ovary-Infiltrating malignant neoplasm-Histologic type-Mucinous carcinoma</skos:definition>
    </owl:Class>
    


    <!-- http://www.semanticweb.org/david/ontologies/2013/0/1.3.6.1.4.1.19376.1.8.2.1.606 -->

    <owl:Class rdf:about="&pathLex;606">
        <rdfs:subClassOf rdf:resource="&pathLex;99999"/>
        <skos:prefLabel xml:lang="en">Endometrioid borderline tumor</skos:prefLabel>
        <skos:definition xml:lang="en">Ovary-Infiltrating malignant neoplasm-Histologic type-Endometrioid borderline tumor</skos:definition>
    </owl:Class>
    


    <!-- http://www.semanticweb.org/david/ontologies/2013/0/1.3.6.1.4.1.19376.1.8.2.1.607 -->

    <owl:Class rdf:about="&pathLex;607">
        <rdfs:subClassOf rdf:resource="&pathLex;99999"/>
        <skos:prefLabel xml:lang="en">Endometrioid carcinoma</skos:prefLabel>
        <skos:definition xml:lang="en">Ovary-Infiltrating malignant neoplasm-Histologic type-Endometrioid carcinoma</skos:definition>
    </owl:Class>
    


    <!-- http://www.semanticweb.org/david/ontologies/2013/0/1.3.6.1.4.1.19376.1.8.2.1.608 -->

    <owl:Class rdf:about="&pathLex;608">
        <rdfs:subClassOf rdf:resource="&pathLex;99999"/>
        <skos:prefLabel xml:lang="en">Clear cell borderline tumor</skos:prefLabel>
        <skos:definition xml:lang="en">Ovary-Infiltrating malignant neoplasm-Histologic type-Clear cell borderline tumor</skos:definition>
    </owl:Class>
    


    <!-- http://www.semanticweb.org/david/ontologies/2013/0/1.3.6.1.4.1.19376.1.8.2.1.609 -->

    <owl:Class rdf:about="&pathLex;609">
        <rdfs:subClassOf rdf:resource="&pathLex;99999"/>
        <skos:prefLabel xml:lang="en">Clear cell carcinoma</skos:prefLabel>
        <skos:definition xml:lang="en">Ovary-Infiltrating malignant neoplasm-Histologic type-Clear cell carcinoma</skos:definition>
    </owl:Class>
    


    <!-- http://www.semanticweb.org/david/ontologies/2013/0/1.3.6.1.4.1.19376.1.8.2.1.61 -->

    <owl:Class rdf:about="&pathLex;61">
        <rdfs:subClassOf rdf:resource="&pathLex;99999"/>
        <skos:prefLabel xml:lang="en">Distance of lesion from closest uninvolved margin</skos:prefLabel>
        <skos:definition xml:lang="en">Generic-In situ neoplasm-Distance of lesion from closest uninvolved margin</skos:definition>
    </owl:Class>
    


    <!-- http://www.semanticweb.org/david/ontologies/2013/0/1.3.6.1.4.1.19376.1.8.2.1.610 -->

    <owl:Class rdf:about="&pathLex;610">
        <rdfs:subClassOf rdf:resource="&pathLex;99999"/>
        <skos:definition xml:lang="en">Ovary-Infiltrating malignant neoplasm-Histologic type-Transitional cell borderline tumor</skos:definition>
        <skos:prefLabel xml:lang="en">Transitional cell borderline tumor</skos:prefLabel>
    </owl:Class>
    


    <!-- http://www.semanticweb.org/david/ontologies/2013/0/1.3.6.1.4.1.19376.1.8.2.1.611 -->

    <owl:Class rdf:about="&pathLex;611">
        <rdfs:subClassOf rdf:resource="&pathLex;99999"/>
        <skos:definition xml:lang="en">Ovary-Infiltrating malignant neoplasm-Histologic type-Transitional cell carcinoma</skos:definition>
        <skos:prefLabel xml:lang="en">Transitional cell carcinoma</skos:prefLabel>
    </owl:Class>
    


    <!-- http://www.semanticweb.org/david/ontologies/2013/0/1.3.6.1.4.1.19376.1.8.2.1.617 -->

    <owl:Class rdf:about="&pathLex;617">
        <rdfs:subClassOf rdf:resource="&pathLex;99999"/>
        <skos:prefLabel xml:lang="en">Other sex cord-stromal tumor (specify type)</skos:prefLabel>
        <skos:definition xml:lang="en">Ovary-Infiltrating malignant neoplasm-Histologic type-Other sex cord-stromal tumor (specify type)</skos:definition>
    </owl:Class>
    


    <!-- http://www.semanticweb.org/david/ontologies/2013/0/1.3.6.1.4.1.19376.1.8.2.1.618 -->

    <owl:Class rdf:about="&pathLex;618">
        <rdfs:subClassOf rdf:resource="&pathLex;99999"/>
        <skos:prefLabel xml:lang="en">Malignant germ cell tumor (specify types and percentages)</skos:prefLabel>
        <skos:definition xml:lang="en">Ovary-Infiltrating malignant neoplasm-Histologic type-Malignant germ cell tumor (specify types and percentages)</skos:definition>
    </owl:Class>
    


    <!-- http://www.semanticweb.org/david/ontologies/2013/0/1.3.6.1.4.1.19376.1.8.2.1.62 -->

    <owl:Class rdf:about="&pathLex;62">
        <rdfs:subClassOf rdf:resource="&pathLex;10010"/>
        <skos:definition xml:lang="en">Generic-Infiltrating malignant neoplasm-Lymph-vascular invasion</skos:definition>
        <skos:prefLabel xml:lang="en">Lymph-vascular invasion</skos:prefLabel>
    </owl:Class>
    


    <!-- http://www.semanticweb.org/david/ontologies/2013/0/1.3.6.1.4.1.19376.1.8.2.1.623 -->

    <owl:Class rdf:about="&pathLex;623">
        <rdfs:subClassOf rdf:resource="&pathLex;210"/>
        <skos:definition xml:lang="en">Generic-Infiltrating malignant neoplasm-Histologic grade (Two-Tier Grading System)-High grade</skos:definition>
        <skos:prefLabel xml:lang="en">High grade</skos:prefLabel>
    </owl:Class>
    


    <!-- http://www.semanticweb.org/david/ontologies/2013/0/1.3.6.1.4.1.19376.1.8.2.1.624 -->

    <owl:Class rdf:about="&pathLex;624">
        <rdfs:subClassOf rdf:resource="&pathLex;210"/>
        <skos:definition xml:lang="en">Generic-Infiltrating malignant neoplasm-Histologic grade (Two-Tier Grading System)-Low grade</skos:definition>
        <skos:prefLabel xml:lang="en">Low grade</skos:prefLabel>
    </owl:Class>
    


    <!-- http://www.semanticweb.org/david/ontologies/2013/0/1.3.6.1.4.1.19376.1.8.2.1.63 -->

    <owl:Class rdf:about="&pathLex;63">
        <rdfs:subClassOf rdf:resource="&pathLex;99999"/>
        <skos:definition xml:lang="en">Generic-Infiltrating malignant neoplasm-Perineural invasion</skos:definition>
        <skos:prefLabel xml:lang="en">Perineural invasion</skos:prefLabel>
    </owl:Class>
    


    <!-- http://www.semanticweb.org/david/ontologies/2013/0/1.3.6.1.4.1.19376.1.8.2.1.640 -->

    <owl:Class rdf:about="&pathLex;640">
        <rdfs:subClassOf rdf:resource="&pathLex;99999"/>
        <skos:definition xml:lang="en">Ovary-Infiltrating malignant neoplasm-pT-pT0 [--]: No evidence of primary tumor</skos:definition>
        <skos:prefLabel xml:lang="en">pT0 [--]: No evidence of primary tumor</skos:prefLabel>
    </owl:Class>
    


    <!-- http://www.semanticweb.org/david/ontologies/2013/0/1.3.6.1.4.1.19376.1.8.2.1.641 -->

    <owl:Class rdf:about="&pathLex;641">
        <rdfs:subClassOf rdf:resource="&pathLex;99999"/>
        <skos:definition xml:lang="en">Ovary-Infiltrating malignant neoplasm-pT-pT1a [IA]: Tumor limited to one ovary; capsule intact, no tumor on ovarian surface. No malignant cells in ascites or peritoneal washings</skos:definition>
        <skos:prefLabel xml:lang="en">pT1a [IA]: Tumor limited to one ovary; capsule intact, no tumor on ovarian surface. No malignant cells in ascites or peritoneal washings</skos:prefLabel>
    </owl:Class>
    


    <!-- http://www.semanticweb.org/david/ontologies/2013/0/1.3.6.1.4.1.19376.1.8.2.1.642 -->

    <owl:Class rdf:about="&pathLex;642">
        <rdfs:subClassOf rdf:resource="&pathLex;99999"/>
        <skos:definition xml:lang="en">Ovary-Infiltrating malignant neoplasm-pT-pT1b [IB]: Tumor limited to both ovaries; capsule intact, no tumor on ovarian surface. No malignant cells in ascites or peritoneal washings</skos:definition>
        <skos:prefLabel xml:lang="en">pT1b [IB]: Tumor limited to both ovaries; capsule intact, no tumor on ovarian surface. No malignant cells in ascites or peritoneal washings</skos:prefLabel>
    </owl:Class>
    


    <!-- http://www.semanticweb.org/david/ontologies/2013/0/1.3.6.1.4.1.19376.1.8.2.1.643 -->

    <owl:Class rdf:about="&pathLex;643">
        <rdfs:subClassOf rdf:resource="&pathLex;99999"/>
        <skos:definition xml:lang="en">Ovary-Infiltrating malignant neoplasm-pT-pT1c [IC]: Tumor limited to one or both ovaries with any of the following: capsule ruptured, tumor on ovarian surface, malignant cells in ascites or peritoneal washings</skos:definition>
        <skos:prefLabel xml:lang="en">pT1c [IC]: Tumor limited to one or both ovaries with any of the following: capsule ruptured, tumor on ovarian surface, malignant cells in ascites or peritoneal washings</skos:prefLabel>
    </owl:Class>
    


    <!-- http://www.semanticweb.org/david/ontologies/2013/0/1.3.6.1.4.1.19376.1.8.2.1.644 -->

    <owl:Class rdf:about="&pathLex;644">
        <rdfs:subClassOf rdf:resource="&pathLex;99999"/>
        <skos:definition xml:lang="en">Ovary-Infiltrating malignant neoplasm-pT-pT2a [IIA]: Extension and/or implants on uterus and/or tube(s). No malignant cells in ascites or peritoneal washings</skos:definition>
        <skos:prefLabel xml:lang="en">pT2a [IIA]: Extension and/or implants on uterus and/or tube(s). No malignant cells in ascites or peritoneal washings</skos:prefLabel>
    </owl:Class>
    


    <!-- http://www.semanticweb.org/david/ontologies/2013/0/1.3.6.1.4.1.19376.1.8.2.1.645 -->

    <owl:Class rdf:about="&pathLex;645">
        <rdfs:subClassOf rdf:resource="&pathLex;99999"/>
        <skos:definition xml:lang="en">Ovary-Infiltrating malignant neoplasm-pT-pT2b [IIB]: Extension to other pelvic tissues. No malignant cells in ascites or peritoneal washings</skos:definition>
        <skos:prefLabel xml:lang="en">pT2b [IIB]: Extension to other pelvic tissues. No malignant cells in ascites or peritoneal washings</skos:prefLabel>
    </owl:Class>
    


    <!-- http://www.semanticweb.org/david/ontologies/2013/0/1.3.6.1.4.1.19376.1.8.2.1.646 -->

    <owl:Class rdf:about="&pathLex;646">
        <rdfs:subClassOf rdf:resource="&pathLex;99999"/>
        <skos:definition xml:lang="en">Ovary-Infiltrating malignant neoplasm-pT-pT2c [IIC]: Pelvic extension and/or implants (T2a or T2b / IIa or IIb) with malignant cells in ascites or peritoneal washings</skos:definition>
        <skos:prefLabel xml:lang="en">pT2c [IIC]: Pelvic extension and/or implants (T2a or T2b / IIa or IIb) with malignant cells in ascites or peritoneal washings</skos:prefLabel>
    </owl:Class>
    


    <!-- http://www.semanticweb.org/david/ontologies/2013/0/1.3.6.1.4.1.19376.1.8.2.1.647 -->

    <owl:Class rdf:about="&pathLex;647">
        <rdfs:subClassOf rdf:resource="&pathLex;99999"/>
        <skos:definition xml:lang="en">Ovary-Infiltrating malignant neoplasm-pT-pT3a [IIIA]: Microscopic peritoneal metastasis beyond pelvis (no macroscopic tumor)</skos:definition>
        <skos:prefLabel xml:lang="en">pT3a [IIIA]: Microscopic peritoneal metastasis beyond pelvis (no macroscopic tumor)</skos:prefLabel>
    </owl:Class>
    


    <!-- http://www.semanticweb.org/david/ontologies/2013/0/1.3.6.1.4.1.19376.1.8.2.1.648 -->

    <owl:Class rdf:about="&pathLex;648">
        <rdfs:subClassOf rdf:resource="&pathLex;99999"/>
        <skos:definition xml:lang="en">Ovary-Infiltrating malignant neoplasm-pT-pT3b [IIIB]: Macroscopic peritoneal metastasis beyond pelvis ≤ 2 cm in greatest dimension</skos:definition>
        <skos:prefLabel xml:lang="en">pT3b [IIIB]: Macroscopic peritoneal metastasis beyond pelvis ≤ 2 cm in greatest dimension</skos:prefLabel>
    </owl:Class>
    


    <!-- http://www.semanticweb.org/david/ontologies/2013/0/1.3.6.1.4.1.19376.1.8.2.1.649 -->

    <owl:Class rdf:about="&pathLex;649">
        <rdfs:subClassOf rdf:resource="&pathLex;99999"/>
        <skos:definition xml:lang="en">Ovary-Infiltrating malignant neoplasm-pT-pT3c [IIIC]: Peritoneal metastasis beyond pelvis &gt; 2 cm in greatest dimension and/or regional lymph node metastasis</skos:definition>
        <skos:prefLabel xml:lang="en">pT3c [IIIC]: Peritoneal metastasis beyond pelvis &gt; 2 cm in greatest dimension and/or regional lymph node metastasis</skos:prefLabel>
    </owl:Class>
    


    <!-- http://www.semanticweb.org/david/ontologies/2013/0/1.3.6.1.4.1.19376.1.8.2.1.65 -->

    <owl:Class rdf:about="&pathLex;65">
        <rdfs:subClassOf rdf:resource="&pathLex;99999"/>
        <skos:definition xml:lang="en">Generic-Infiltrating malignant neoplasm-pT</skos:definition>
        <skos:prefLabel xml:lang="en">pT</skos:prefLabel>
    </owl:Class>
    


    <!-- http://www.semanticweb.org/david/ontologies/2013/0/1.3.6.1.4.1.19376.1.8.2.1.650 -->

    <owl:Class rdf:about="&pathLex;650">
        <rdfs:subClassOf rdf:resource="&pathLex;99999"/>
        <skos:definition xml:lang="en">Ovary-Infiltrating malignant neoplasm-pN-pN0: No regional lymph node metastasis</skos:definition>
        <skos:prefLabel xml:lang="en">pN0: No regional lymph node metastasis</skos:prefLabel>
    </owl:Class>
    


    <!-- http://www.semanticweb.org/david/ontologies/2013/0/1.3.6.1.4.1.19376.1.8.2.1.651 -->

    <owl:Class rdf:about="&pathLex;651">
        <rdfs:subClassOf rdf:resource="&pathLex;99999"/>
        <skos:definition xml:lang="en">Ovary-Infiltrating malignant neoplasm-pN-pN1 [IIIC]: Regional lymph node metastasis</skos:definition>
        <skos:prefLabel xml:lang="en">pN1 [IIIC]: Regional lymph node metastasis</skos:prefLabel>
    </owl:Class>
    


    <!-- http://www.semanticweb.org/david/ontologies/2013/0/1.3.6.1.4.1.19376.1.8.2.1.652 -->

    <owl:Class rdf:about="&pathLex;652">
        <rdfs:subClassOf rdf:resource="&pathLex;10008"/>
        <skos:definition xml:lang="en">Breast-Specimen-Target site-Total breast (including nipple and skin)</skos:definition>
        <skos:prefLabel xml:lang="en">Total breast (including nipple and skin)</skos:prefLabel>
    </owl:Class>
    


    <!-- http://www.semanticweb.org/david/ontologies/2013/0/1.3.6.1.4.1.19376.1.8.2.1.66 -->

    <owl:Class rdf:about="&pathLex;66">
        <rdfs:subClassOf rdf:resource="&pathLex;99999"/>
        <skos:definition xml:lang="en">Generic-Infiltrating malignant neoplasm-pN</skos:definition>
        <skos:prefLabel xml:lang="en">pN</skos:prefLabel>
    </owl:Class>
    


    <!-- http://www.semanticweb.org/david/ontologies/2013/0/1.3.6.1.4.1.19376.1.8.2.1.662 -->

    <owl:Class rdf:about="&pathLex;662">
        <rdfs:subClassOf rdf:resource="&pathLex;10009"/>
        <skos:definition xml:lang="en">Breast-Specimen-Specimen collection procedure-Total mastectomy (including nipple and skin)</skos:definition>
        <skos:prefLabel xml:lang="en">Total mastectomy (including nipple and skin)</skos:prefLabel>
    </owl:Class>
    


    <!-- http://www.semanticweb.org/david/ontologies/2013/0/1.3.6.1.4.1.19376.1.8.2.1.663 -->

    <owl:Class rdf:about="&pathLex;663">
        <rdfs:subClassOf rdf:resource="&pathLex;422"/>
        <skos:definition xml:lang="en">Breast-Infiltrating malignant neoplasm-Lesion site-Upper outer quadrant</skos:definition>
        <skos:prefLabel xml:lang="en">Upper outer quadrant</skos:prefLabel>
    </owl:Class>
    


    <!-- http://www.semanticweb.org/david/ontologies/2013/0/1.3.6.1.4.1.19376.1.8.2.1.664 -->

    <owl:Class rdf:about="&pathLex;664">
        <rdfs:subClassOf rdf:resource="&pathLex;422"/>
        <skos:definition xml:lang="en">Breast-Infiltrating malignant neoplasm-Lesion site-Lower outer quadrant</skos:definition>
        <skos:prefLabel xml:lang="en">Lower outer quadrant</skos:prefLabel>
    </owl:Class>
    


    <!-- http://www.semanticweb.org/david/ontologies/2013/0/1.3.6.1.4.1.19376.1.8.2.1.665 -->

    <owl:Class rdf:about="&pathLex;665">
        <rdfs:subClassOf rdf:resource="&pathLex;422"/>
        <skos:definition xml:lang="en">Breast-Infiltrating malignant neoplasm-Lesion site-Upper inner quadrant</skos:definition>
        <skos:prefLabel xml:lang="en">Upper inner quadrant</skos:prefLabel>
    </owl:Class>
    


    <!-- http://www.semanticweb.org/david/ontologies/2013/0/1.3.6.1.4.1.19376.1.8.2.1.666 -->

    <owl:Class rdf:about="&pathLex;666">
        <rdfs:subClassOf rdf:resource="&pathLex;422"/>
        <skos:definition xml:lang="en">Breast-Infiltrating malignant neoplasm-Lesion site-Lower inner quadrant</skos:definition>
        <skos:prefLabel xml:lang="en">Lower inner quadrant</skos:prefLabel>
    </owl:Class>
    


    <!-- http://www.semanticweb.org/david/ontologies/2013/0/1.3.6.1.4.1.19376.1.8.2.1.67 -->

    <owl:Class rdf:about="&pathLex;67">
        <rdfs:subClassOf rdf:resource="&pathLex;99999"/>
        <skos:definition xml:lang="en">Generic-Infiltrating malignant neoplasm-pM</skos:definition>
        <skos:prefLabel xml:lang="en">pM</skos:prefLabel>
    </owl:Class>
    


    <!-- http://www.semanticweb.org/david/ontologies/2013/0/1.3.6.1.4.1.19376.1.8.2.1.671 -->

    <owl:Class rdf:about="&pathLex;671">
        <rdfs:subClassOf rdf:resource="&pathLex;422"/>
        <skos:definition xml:lang="en">Breast-Infiltrating malignant neoplasm-Lesion site-Nipple</skos:definition>
        <skos:prefLabel xml:lang="en">Nipple</skos:prefLabel>
    </owl:Class>
    


    <!-- http://www.semanticweb.org/david/ontologies/2013/0/1.3.6.1.4.1.19376.1.8.2.1.672 -->

    <owl:Class rdf:about="&pathLex;672">
        <rdfs:subClassOf rdf:resource="&pathLex;422"/>
        <skos:definition xml:lang="en">Breast-Infiltrating malignant neoplasm-Lesion site-Central</skos:definition>
        <skos:prefLabel xml:lang="en">Central</skos:prefLabel>
    </owl:Class>
    


    <!-- http://www.semanticweb.org/david/ontologies/2013/0/1.3.6.1.4.1.19376.1.8.2.1.68 -->

    <owl:Class rdf:about="&pathLex;68">
        <rdfs:subClassOf rdf:resource="&pathLex;99999"/>
        <skos:definition xml:lang="en">Generic-Infiltrating malignant neoplasm-Treatment effect</skos:definition>
        <skos:prefLabel xml:lang="en">Treatment effect</skos:prefLabel>
    </owl:Class>
    


    <!-- http://www.semanticweb.org/david/ontologies/2013/0/1.3.6.1.4.1.19376.1.8.2.1.688 -->

    <owl:Class rdf:about="&pathLex;688">
        <rdfs:subClassOf rdf:resource="&pathLex;437"/>
        <skos:definition xml:lang="en">Breast-Infiltrating malignant neoplasm-Histologic type-Invasive ductal carcinoma (no special type or not otherwise specified)</skos:definition>
        <skos:prefLabel xml:lang="en">Invasive ductal carcinoma (no special type or not otherwise specified)</skos:prefLabel>
    </owl:Class>
    


    <!-- http://www.semanticweb.org/david/ontologies/2013/0/1.3.6.1.4.1.19376.1.8.2.1.689 -->

    <owl:Class rdf:about="&pathLex;689">
        <rdfs:subClassOf rdf:resource="&pathLex;437"/>
        <skos:definition xml:lang="en">Breast-Infiltrating malignant neoplasm-Histologic type-Invasive lobular carcinoma</skos:definition>
        <skos:prefLabel xml:lang="en">Invasive lobular carcinoma</skos:prefLabel>
    </owl:Class>
    


    <!-- http://www.semanticweb.org/david/ontologies/2013/0/1.3.6.1.4.1.19376.1.8.2.1.69 -->

    <owl:Class rdf:about="&pathLex;69">
        <rdfs:subClassOf rdf:resource="&pathLex;10011"/>
        <skos:definition xml:lang="en">Generic-In situ neoplasm-Margins involvement</skos:definition>
        <skos:prefLabel xml:lang="en">Margins involvement</skos:prefLabel>
    </owl:Class>
    


    <!-- http://www.semanticweb.org/david/ontologies/2013/0/1.3.6.1.4.1.19376.1.8.2.1.690 -->

    <owl:Class rdf:about="&pathLex;690">
        <rdfs:subClassOf rdf:resource="&pathLex;437"/>
        <skos:definition xml:lang="en">Breast-Infiltrating malignant neoplasm-Histologic type-Invasive Carcinoma, type cannot be determinedd</skos:definition>
        <skos:prefLabel xml:lang="en">Invasive Carcinoma, type cannot be determinedd</skos:prefLabel>
    </owl:Class>
    


    <!-- http://www.semanticweb.org/david/ontologies/2013/0/1.3.6.1.4.1.19376.1.8.2.1.7 -->

    <owl:Class rdf:about="&pathLex;7">
        <rdfs:subClassOf rdf:resource="&pathLex;10010"/>
        <skos:definition xml:lang="en">Generic-Infiltrating malignant neoplasm-Lesion site</skos:definition>
        <skos:prefLabel xml:lang="en">Lesion site</skos:prefLabel>
    </owl:Class>
    


    <!-- http://www.semanticweb.org/david/ontologies/2013/0/1.3.6.1.4.1.19376.1.8.2.1.70 -->

    <owl:Class rdf:about="&pathLex;70">
        <rdfs:subClassOf rdf:resource="&pathLex;60"/>
        <skos:definition xml:lang="en">Breast-Infiltrating malignant neoplasm-Distance of lesion from closest uninvolved margin</skos:definition>
        <skos:prefLabel xml:lang="en">Distance of lesion from closest uninvolved margin</skos:prefLabel>
    </owl:Class>
    


    <!-- http://www.semanticweb.org/david/ontologies/2013/0/1.3.6.1.4.1.19376.1.8.2.1.700 -->

    <owl:Class rdf:about="&pathLex;700">
        <rdfs:subClassOf rdf:resource="&pathLex;424"/>
        <skos:definition xml:lang="en">Breast-Infiltrating malignant neoplasm-Margin site-Superior</skos:definition>
        <skos:prefLabel xml:lang="en">Superior</skos:prefLabel>
    </owl:Class>
    


    <!-- http://www.semanticweb.org/david/ontologies/2013/0/1.3.6.1.4.1.19376.1.8.2.1.701 -->

    <owl:Class rdf:about="&pathLex;701">
        <rdfs:subClassOf rdf:resource="&pathLex;424"/>
        <skos:definition xml:lang="en">Breast-Infiltrating malignant neoplasm-Margin site-Inferior</skos:definition>
        <skos:prefLabel xml:lang="en">Inferior</skos:prefLabel>
    </owl:Class>
    


    <!-- http://www.semanticweb.org/david/ontologies/2013/0/1.3.6.1.4.1.19376.1.8.2.1.702 -->

    <owl:Class rdf:about="&pathLex;702">
        <rdfs:subClassOf rdf:resource="&pathLex;424"/>
        <skos:definition xml:lang="en">Breast-Infiltrating malignant neoplasm-Margin site-Medial</skos:definition>
        <skos:prefLabel xml:lang="en">Medial</skos:prefLabel>
    </owl:Class>
    


    <!-- http://www.semanticweb.org/david/ontologies/2013/0/1.3.6.1.4.1.19376.1.8.2.1.703 -->

    <owl:Class rdf:about="&pathLex;703">
        <rdfs:subClassOf rdf:resource="&pathLex;424"/>
        <skos:definition xml:lang="en">Breast-Infiltrating malignant neoplasm-Margin site-Lateral</skos:definition>
        <skos:prefLabel xml:lang="en">Lateral</skos:prefLabel>
    </owl:Class>
    


    <!-- http://www.semanticweb.org/david/ontologies/2013/0/1.3.6.1.4.1.19376.1.8.2.1.704 -->

    <owl:Class rdf:about="&pathLex;704">
        <rdfs:subClassOf rdf:resource="&pathLex;424"/>
        <skos:prefLabel xml:lang="en">Anterior</skos:prefLabel>
        <skos:definition xml:lang="en">Breast-Infiltrating malignant neoplasm-Margin site-Anterior</skos:definition>
    </owl:Class>
    


    <!-- http://www.semanticweb.org/david/ontologies/2013/0/1.3.6.1.4.1.19376.1.8.2.1.705 -->

    <owl:Class rdf:about="&pathLex;705">
        <rdfs:subClassOf rdf:resource="&pathLex;424"/>
        <skos:definition xml:lang="en">Breast-Infiltrating malignant neoplasm-Margin site-Posterior</skos:definition>
        <skos:prefLabel xml:lang="en">Posterior</skos:prefLabel>
    </owl:Class>
    


    <!-- http://www.semanticweb.org/david/ontologies/2013/0/1.3.6.1.4.1.19376.1.8.2.1.707 -->

    <owl:Class rdf:about="&pathLex;707">
        <rdfs:subClassOf rdf:resource="&pathLex;423"/>
        <skos:definition xml:lang="en">Breast-Infiltrating malignant neoplasm-Lymph node site-Intramammary lymph nodes)</skos:definition>
        <skos:prefLabel xml:lang="en">Intramammary lymph nodes)</skos:prefLabel>
    </owl:Class>
    


    <!-- http://www.semanticweb.org/david/ontologies/2013/0/1.3.6.1.4.1.19376.1.8.2.1.708 -->

    <owl:Class rdf:about="&pathLex;708">
        <rdfs:subClassOf rdf:resource="&pathLex;423"/>
        <skos:definition xml:lang="en">Breast-Infiltrating malignant neoplasm-Lymph node site-Sentinel lymph node(s)</skos:definition>
        <skos:prefLabel xml:lang="en">Sentinel lymph node(s)</skos:prefLabel>
    </owl:Class>
    


    <!-- http://www.semanticweb.org/david/ontologies/2013/0/1.3.6.1.4.1.19376.1.8.2.1.709 -->

    <owl:Class rdf:about="&pathLex;709">
        <rdfs:subClassOf rdf:resource="&pathLex;430"/>
        <skos:definition xml:lang="en">Breast-Infiltrating malignant neoplasm-pT-pT0: No evidence of primary tumor</skos:definition>
        <skos:prefLabel xml:lang="en">pT0: No evidence of primary tumor</skos:prefLabel>
    </owl:Class>
    


    <!-- http://www.semanticweb.org/david/ontologies/2013/0/1.3.6.1.4.1.19376.1.8.2.1.710 -->

    <owl:Class rdf:about="&pathLex;710">
        <rdfs:subClassOf rdf:resource="&pathLex;430"/>
        <skos:definition xml:lang="en">Breast-Infiltrating malignant neoplasm-pT-pTis (DCIS): Ductal carcinoma in situ</skos:definition>
        <skos:prefLabel xml:lang="en">pTis (DCIS): Ductal carcinoma in situ</skos:prefLabel>
    </owl:Class>
    


    <!-- http://www.semanticweb.org/david/ontologies/2013/0/1.3.6.1.4.1.19376.1.8.2.1.711 -->

    <owl:Class rdf:about="&pathLex;711">
        <rdfs:subClassOf rdf:resource="&pathLex;430"/>
        <skos:definition xml:lang="en">Breast-Infiltrating malignant neoplasm-pT-pTis (LCIS): Lobular carcinoma in situ</skos:definition>
        <skos:prefLabel xml:lang="en">pTis (LCIS): Lobular carcinoma in situ</skos:prefLabel>
    </owl:Class>
    


    <!-- http://www.semanticweb.org/david/ontologies/2013/0/1.3.6.1.4.1.19376.1.8.2.1.712 -->

    <owl:Class rdf:about="&pathLex;712">
        <rdfs:subClassOf rdf:resource="&pathLex;430"/>
        <skos:definition xml:lang="en">Breast-Infiltrating malignant neoplasm-pT-pTis (Paget): Paget disease of the nipple not associated with invasive carcinoma and/or carcinoma in situ (DCIS and/or LCIS) in the underlying breast parenchyma</skos:definition>
        <skos:prefLabel xml:lang="en">pTis (Paget): Paget disease of the nipple not associated with invasive carcinoma and/or carcinoma in situ (DCIS and/or LCIS) in the underlying breast parenchyma</skos:prefLabel>
    </owl:Class>
    


    <!-- http://www.semanticweb.org/david/ontologies/2013/0/1.3.6.1.4.1.19376.1.8.2.1.713 -->

    <owl:Class rdf:about="&pathLex;713">
        <rdfs:subClassOf rdf:resource="&pathLex;430"/>
        <skos:definition xml:lang="en">Breast-Infiltrating malignant neoplasm-pT-pT1: Tumor &lt; =20 mm in greatest dimension</skos:definition>
        <skos:prefLabel xml:lang="en">pT1: Tumor &lt; =20 mm in greatest dimension</skos:prefLabel>
    </owl:Class>
    


    <!-- http://www.semanticweb.org/david/ontologies/2013/0/1.3.6.1.4.1.19376.1.8.2.1.714 -->

    <owl:Class rdf:about="&pathLex;714">
        <rdfs:subClassOf rdf:resource="&pathLex;430"/>
        <skos:definition xml:lang="en">Breast-Infiltrating malignant neoplasm-pT-pT1mi: Tumor &lt; =1 mm in greatest dimension (microinvasion)</skos:definition>
        <skos:prefLabel xml:lang="en">pT1mi: Tumor &lt; =1 mm in greatest dimension (microinvasion)</skos:prefLabel>
    </owl:Class>
    


    <!-- http://www.semanticweb.org/david/ontologies/2013/0/1.3.6.1.4.1.19376.1.8.2.1.715 -->

    <owl:Class rdf:about="&pathLex;715">
        <rdfs:subClassOf rdf:resource="&pathLex;430"/>
        <skos:definition xml:lang="en">Breast-Infiltrating malignant neoplasm-pT-pT1a: Tumor &gt;1 mm but &lt; = 5 mm in greatest dimension</skos:definition>
        <skos:prefLabel xml:lang="en">pT1a: Tumor &gt;1 mm but &lt; = 5 mm in greatest dimension</skos:prefLabel>
    </owl:Class>
    


    <!-- http://www.semanticweb.org/david/ontologies/2013/0/1.3.6.1.4.1.19376.1.8.2.1.716 -->

    <owl:Class rdf:about="&pathLex;716">
        <rdfs:subClassOf rdf:resource="&pathLex;430"/>
        <skos:definition xml:lang="en">Breast-Infiltrating malignant neoplasm-pT-pT1b: Tumor &gt;5 mm but &lt; = 10 mm in greatest dimension</skos:definition>
        <skos:prefLabel xml:lang="en">pT1b: Tumor &gt;5 mm but &lt; = 10 mm in greatest dimension</skos:prefLabel>
    </owl:Class>
    


    <!-- http://www.semanticweb.org/david/ontologies/2013/0/1.3.6.1.4.1.19376.1.8.2.1.717 -->

    <owl:Class rdf:about="&pathLex;717">
        <rdfs:subClassOf rdf:resource="&pathLex;430"/>
        <skos:definition xml:lang="en">Breast-Infiltrating malignant neoplasm-pT-pT1c: Tumor &gt;10 mm but &lt; = 20 mm in greatest dimension</skos:definition>
        <skos:prefLabel xml:lang="en">pT1c: Tumor &gt;10 mm but &lt; = 20 mm in greatest dimension</skos:prefLabel>
    </owl:Class>
    


    <!-- http://www.semanticweb.org/david/ontologies/2013/0/1.3.6.1.4.1.19376.1.8.2.1.718 -->

    <owl:Class rdf:about="&pathLex;718">
        <rdfs:subClassOf rdf:resource="&pathLex;430"/>
        <skos:definition xml:lang="en">Breast-Infiltrating malignant neoplasm-pT-pT2: Tumor &gt;20 mm but &lt; = 50 mm in greatest dimension</skos:definition>
        <skos:prefLabel xml:lang="en">pT2: Tumor &gt;20 mm but &lt; = 50 mm in greatest dimension</skos:prefLabel>
    </owl:Class>
    


    <!-- http://www.semanticweb.org/david/ontologies/2013/0/1.3.6.1.4.1.19376.1.8.2.1.719 -->

    <owl:Class rdf:about="&pathLex;719">
        <rdfs:subClassOf rdf:resource="&pathLex;430"/>
        <skos:definition xml:lang="en">Breast-Infiltrating malignant neoplasm-pT-pT3: Tumor &gt;50 mm in greatest dimension</skos:definition>
        <skos:prefLabel xml:lang="en">pT3: Tumor &gt;50 mm in greatest dimension</skos:prefLabel>
    </owl:Class>
    


    <!-- http://www.semanticweb.org/david/ontologies/2013/0/1.3.6.1.4.1.19376.1.8.2.1.72 -->

    <owl:Class rdf:about="&pathLex;72">
        <rdfs:subClassOf rdf:resource="&pathLex;99999"/>
        <skos:prefLabel xml:lang="en">Histologic grade (Clark)</skos:prefLabel>
        <skos:definition xml:lang="en">Skin (melanoma)-Infiltrating malignant neoplasm-Histologic grade (Clark)</skos:definition>
    </owl:Class>
    


    <!-- http://www.semanticweb.org/david/ontologies/2013/0/1.3.6.1.4.1.19376.1.8.2.1.720 -->

    <owl:Class rdf:about="&pathLex;720">
        <rdfs:subClassOf rdf:resource="&pathLex;430"/>
        <skos:definition xml:lang="en">Breast-Infiltrating malignant neoplasm-pT-pT4: Tumor of any size with direct extension to the chest wall and/or to the skin (ulceration or skin nodules). Note: Invasion of the dermis alone does not qualify as pT4.</skos:definition>
        <skos:prefLabel xml:lang="en">pT4: Tumor of any size with direct extension to the chest wall and/or to the skin (ulceration or skin nodules). Note: Invasion of the dermis alone does not qualify as pT4.</skos:prefLabel>
    </owl:Class>
    


    <!-- http://www.semanticweb.org/david/ontologies/2013/0/1.3.6.1.4.1.19376.1.8.2.1.721 -->

    <owl:Class rdf:about="&pathLex;721">
        <rdfs:subClassOf rdf:resource="&pathLex;430"/>
        <skos:definition xml:lang="en">Breast-Infiltrating malignant neoplasm-pT-pT4a: Extension to chest wall, not including only pectoralis muscle adherence/invasion</skos:definition>
        <skos:prefLabel xml:lang="en">pT4a: Extension to chest wall, not including only pectoralis muscle adherence/invasion</skos:prefLabel>
    </owl:Class>
    


    <!-- http://www.semanticweb.org/david/ontologies/2013/0/1.3.6.1.4.1.19376.1.8.2.1.722 -->

    <owl:Class rdf:about="&pathLex;722">
        <rdfs:subClassOf rdf:resource="&pathLex;430"/>
        <skos:definition xml:lang="en">Breast-Infiltrating malignant neoplasm-pT-pT4b: Ulceration and/or ipsilateral satellite nodules and/or edema (including peau d’orange) of the skin which do not meet the criteria for inflammatory carcinoma</skos:definition>
        <skos:prefLabel xml:lang="en">pT4b: Ulceration and/or ipsilateral satellite nodules and/or edema (including peau d’orange) of the skin which do not meet the criteria for inflammatory carcinoma</skos:prefLabel>
    </owl:Class>
    


    <!-- http://www.semanticweb.org/david/ontologies/2013/0/1.3.6.1.4.1.19376.1.8.2.1.723 -->

    <owl:Class rdf:about="&pathLex;723">
        <rdfs:subClassOf rdf:resource="&pathLex;430"/>
        <skos:definition xml:lang="en">Breast-Infiltrating malignant neoplasm-pT-pT4c: Both T4a and T4b</skos:definition>
        <skos:prefLabel xml:lang="en">pT4c: Both T4a and T4b</skos:prefLabel>
    </owl:Class>
    


    <!-- http://www.semanticweb.org/david/ontologies/2013/0/1.3.6.1.4.1.19376.1.8.2.1.724 -->

    <owl:Class rdf:about="&pathLex;724">
        <rdfs:subClassOf rdf:resource="&pathLex;430"/>
        <skos:definition xml:lang="en">Breast-Infiltrating malignant neoplasm-pT-pT4d: Inflammatory carcinoma</skos:definition>
        <skos:prefLabel xml:lang="en">pT4d: Inflammatory carcinoma</skos:prefLabel>
    </owl:Class>
    


    <!-- http://www.semanticweb.org/david/ontologies/2013/0/1.3.6.1.4.1.19376.1.8.2.1.725 -->

    <owl:Class rdf:about="&pathLex;725">
        <rdfs:subClassOf rdf:resource="&pathLex;428"/>
        <skos:definition xml:lang="en">Breast-Infiltrating malignant neoplasm-pN-pN0: No regional lymph node metastasis identified histologically Note: Isolated tumor cell (ITC) clusters are defined as small clusters of cells not greater than 0.2 mm or single tumor cells, or a cluster of fewer than 200 cells in a single histologic cross-section. ITCs may be detected by routine histology or by immunohistochemical (IHC) methods. Nodes containing only ITCs are excluded from the total positive node count for purposes of N classification but should be included in the total number of nodes evaluated.</skos:definition>
        <skos:prefLabel xml:lang="en">pN0: No regional lymph node metastasis identified histologically Note: Isolated tumor cell (ITC) clusters are defined as small clusters of cells not greater than 0.2 mm or single tumor cells, or a cluster of fewer than 200 cells in a single histologic cross-section. ITCs may be detected by routine histology or by immunohistochemical (IHC) methods. Nodes containing only ITCs are excluded from the total positive node count for purposes of N classification but should be included in the total number of nodes evaluated.</skos:prefLabel>
    </owl:Class>
    


    <!-- http://www.semanticweb.org/david/ontologies/2013/0/1.3.6.1.4.1.19376.1.8.2.1.726 -->

    <owl:Class rdf:about="&pathLex;726">
        <rdfs:subClassOf rdf:resource="&pathLex;428"/>
        <skos:definition xml:lang="en">Breast-Infiltrating malignant neoplasm-pN-pN0 (i-): No regional lymph node metastases histologically, negative IHC</skos:definition>
        <skos:prefLabel xml:lang="en">pN0 (i-): No regional lymph node metastases histologically, negative IHC</skos:prefLabel>
    </owl:Class>
    


    <!-- http://www.semanticweb.org/david/ontologies/2013/0/1.3.6.1.4.1.19376.1.8.2.1.727 -->

    <owl:Class rdf:about="&pathLex;727">
        <rdfs:subClassOf rdf:resource="&pathLex;428"/>
        <skos:definition xml:lang="en">Breast-Infiltrating malignant neoplasm-pN-pN0 (i+): Malignant cells in regional lymph node(s) no greater than 0.2 mm and no more than 200 cells (detected by H&amp;E or IHC including ITC)</skos:definition>
        <skos:prefLabel xml:lang="en">pN0 (i+): Malignant cells in regional lymph node(s) no greater than 0.2 mm and no more than 200 cells (detected by H&amp;E or IHC including ITC)</skos:prefLabel>
    </owl:Class>
    


    <!-- http://www.semanticweb.org/david/ontologies/2013/0/1.3.6.1.4.1.19376.1.8.2.1.728 -->

    <owl:Class rdf:about="&pathLex;728">
        <rdfs:subClassOf rdf:resource="&pathLex;428"/>
        <skos:definition xml:lang="en">Breast-Infiltrating malignant neoplasm-pN-pN0 (mol-): No regional lymph node metastases histologically, negative molecular findings (reverse transcriptase polymerase chain reaction [RT-PCR])</skos:definition>
        <skos:prefLabel xml:lang="en">pN0 (mol-): No regional lymph node metastases histologically, negative molecular findings (reverse transcriptase polymerase chain reaction [RT-PCR])</skos:prefLabel>
    </owl:Class>
    


    <!-- http://www.semanticweb.org/david/ontologies/2013/0/1.3.6.1.4.1.19376.1.8.2.1.729 -->

    <owl:Class rdf:about="&pathLex;729">
        <rdfs:subClassOf rdf:resource="&pathLex;428"/>
        <skos:definition xml:lang="en">Breast-Infiltrating malignant neoplasm-pN-pN0 (mol+): Positive molecular findings (RT-PCR), but no regional lymph node metastases detected by histology or IHC</skos:definition>
        <skos:prefLabel xml:lang="en">pN0 (mol+): Positive molecular findings (RT-PCR), but no regional lymph node metastases detected by histology or IHC</skos:prefLabel>
    </owl:Class>
    


    <!-- http://www.semanticweb.org/david/ontologies/2013/0/1.3.6.1.4.1.19376.1.8.2.1.73 -->

    <owl:Class rdf:about="&pathLex;73">
        <rdfs:subClassOf rdf:resource="&pathLex;10005"/>
        <skos:definition xml:lang="en">Cervix-Infiltrating malignant neoplasm-Histologic grade (FIGO)</skos:definition>
        <skos:prefLabel xml:lang="en">Histologic grade (FIGO)</skos:prefLabel>
    </owl:Class>
    


    <!-- http://www.semanticweb.org/david/ontologies/2013/0/1.3.6.1.4.1.19376.1.8.2.1.730 -->

    <owl:Class rdf:about="&pathLex;730">
        <rdfs:subClassOf rdf:resource="&pathLex;428"/>
        <skos:definition xml:lang="en">Breast-Infiltrating malignant neoplasm-pN-pN1mi: Micrometastases (greater than 0.2 mm and/or more than 200 cells, but none greater than 2.0 mm).</skos:definition>
        <skos:prefLabel xml:lang="en">pN1mi: Micrometastases (greater than 0.2 mm and/or more than 200 cells, but none greater than 2.0 mm).</skos:prefLabel>
    </owl:Class>
    


    <!-- http://www.semanticweb.org/david/ontologies/2013/0/1.3.6.1.4.1.19376.1.8.2.1.731 -->

    <owl:Class rdf:about="&pathLex;731">
        <rdfs:subClassOf rdf:resource="&pathLex;428"/>
        <skos:definition xml:lang="en">Breast-Infiltrating malignant neoplasm-pN-pN1a: Metastases in 1 to 3 axillary lymph nodes, at least 1 metastasis greater than 2.0 mm</skos:definition>
        <skos:prefLabel xml:lang="en">pN1a: Metastases in 1 to 3 axillary lymph nodes, at least 1 metastasis greater than 2.0 mm</skos:prefLabel>
    </owl:Class>
    


    <!-- http://www.semanticweb.org/david/ontologies/2013/0/1.3.6.1.4.1.19376.1.8.2.1.732 -->

    <owl:Class rdf:about="&pathLex;732">
        <rdfs:subClassOf rdf:resource="&pathLex;428"/>
        <skos:definition xml:lang="en">Breast-Infiltrating malignant neoplasm-pN-pN2a: Metastases in 4 to 9 axillary lymph nodes (at least 1 tumor deposit greater than 2.0 mm)</skos:definition>
        <skos:prefLabel xml:lang="en">pN2a: Metastases in 4 to 9 axillary lymph nodes (at least 1 tumor deposit greater than 2.0 mm)</skos:prefLabel>
    </owl:Class>
    


    <!-- http://www.semanticweb.org/david/ontologies/2013/0/1.3.6.1.4.1.19376.1.8.2.1.733 -->

    <owl:Class rdf:about="&pathLex;733">
        <rdfs:subClassOf rdf:resource="&pathLex;428"/>
        <skos:definition xml:lang="en">Breast-Infiltrating malignant neoplasm-pN-pN3a: Metastases in 10 or more axillary lymph nodes (at least 1 tumor deposit greater than 2.0 mm)</skos:definition>
        <skos:prefLabel xml:lang="en">pN3a: Metastases in 10 or more axillary lymph nodes (at least 1 tumor deposit greater than 2.0 mm)</skos:prefLabel>
    </owl:Class>
    


    <!-- http://www.semanticweb.org/david/ontologies/2013/0/1.3.6.1.4.1.19376.1.8.2.1.734 -->

    <owl:Class rdf:about="&pathLex;734">
        <rdfs:subClassOf rdf:resource="&pathLex;99999"/>
        <skos:definition xml:lang="en">Generic-Infiltrating malignant neoplasm-Treatment effect-No residual tumor (complete response, grade 0)</skos:definition>
        <skos:prefLabel xml:lang="en">No residual tumor (complete response, grade 0)</skos:prefLabel>
    </owl:Class>
    


    <!-- http://www.semanticweb.org/david/ontologies/2013/0/1.3.6.1.4.1.19376.1.8.2.1.735 -->

    <owl:Class rdf:about="&pathLex;735">
        <rdfs:subClassOf rdf:resource="&pathLex;99999"/>
        <skos:definition xml:lang="en">Generic-Infiltrating malignant neoplasm-Treatment effect-Moderate response (grade 2)</skos:definition>
        <skos:prefLabel xml:lang="en">Moderate response (grade 2)</skos:prefLabel>
    </owl:Class>
    


    <!-- http://www.semanticweb.org/david/ontologies/2013/0/1.3.6.1.4.1.19376.1.8.2.1.736 -->

    <owl:Class rdf:about="&pathLex;736">
        <rdfs:subClassOf rdf:resource="&pathLex;99999"/>
        <skos:definition xml:lang="en">Generic-Infiltrating malignant neoplasm-Treatment effect-No definite response identified (grade 3, poor or no response)</skos:definition>
        <skos:prefLabel xml:lang="en">No definite response identified (grade 3, poor or no response)</skos:prefLabel>
    </owl:Class>
    


    <!-- http://www.semanticweb.org/david/ontologies/2013/0/1.3.6.1.4.1.19376.1.8.2.1.740 -->

    <owl:Class rdf:about="&pathLex;740">
        <rdfs:subClassOf rdf:resource="&pathLex;431"/>
        <skos:definition xml:lang="en">Breast-Infiltrating malignant neoplasm-Progesterone receptor-No immunoreactive tumor cells present</skos:definition>
        <skos:prefLabel xml:lang="en">No immunoreactive tumor cells present</skos:prefLabel>
    </owl:Class>
    


    <!-- http://www.semanticweb.org/david/ontologies/2013/0/1.3.6.1.4.1.19376.1.8.2.1.741 -->

    <owl:Class rdf:about="&pathLex;741">
        <rdfs:subClassOf rdf:resource="&pathLex;433"/>
        <skos:prefLabel xml:lang="en">Amplified (HER2 gene copy &gt;6.0 or ratio &gt;2.2)</skos:prefLabel>
        <skos:definition xml:lang="en">Breast-Infiltrating malignant neoplasm-HER2/neu (FISH method)-Amplified (HER2 gene copy &gt;6.0 or ratio &gt;2.2)</skos:definition>
    </owl:Class>
    


    <!-- http://www.semanticweb.org/david/ontologies/2013/0/1.3.6.1.4.1.19376.1.8.2.1.742 -->

    <owl:Class rdf:about="&pathLex;742">
        <rdfs:subClassOf rdf:resource="&pathLex;433"/>
        <skos:definition xml:lang="en">Breast-Infiltrating malignant neoplasm-HER2/neu (FISH method)-Not amplified (HER2 gene copy &lt;4.0 or ratio &lt;1.8)</skos:definition>
        <skos:prefLabel xml:lang="en">Not amplified (HER2 gene copy &lt;4.0 or ratio &lt;1.8)</skos:prefLabel>
    </owl:Class>
    


    <!-- http://www.semanticweb.org/david/ontologies/2013/0/1.3.6.1.4.1.19376.1.8.2.1.743 -->

    <owl:Class rdf:about="&pathLex;743">
        <rdfs:subClassOf rdf:resource="&pathLex;417"/>
        <skos:definition xml:lang="en">Breast-In situ neoplasm-Histologic grade of ductal carcinoma in situ (DCIS)-Grade I (low)</skos:definition>
        <skos:prefLabel xml:lang="en">Grade I (low)</skos:prefLabel>
    </owl:Class>
    


    <!-- http://www.semanticweb.org/david/ontologies/2013/0/1.3.6.1.4.1.19376.1.8.2.1.744 -->

    <owl:Class rdf:about="&pathLex;744">
        <rdfs:subClassOf rdf:resource="&pathLex;417"/>
        <skos:definition xml:lang="en">Breast-In situ neoplasm-Histologic grade of ductal carcinoma in situ (DCIS)-Grade II (intermediate)</skos:definition>
        <skos:prefLabel xml:lang="en">Grade II (intermediate)</skos:prefLabel>
    </owl:Class>
    


    <!-- http://www.semanticweb.org/david/ontologies/2013/0/1.3.6.1.4.1.19376.1.8.2.1.745 -->

    <owl:Class rdf:about="&pathLex;745">
        <rdfs:subClassOf rdf:resource="&pathLex;417"/>
        <skos:definition xml:lang="en">Breast-In situ neoplasm-Histologic grade of ductal carcinoma in situ (DCIS)-Grade III (high)</skos:definition>
        <skos:prefLabel xml:lang="en">Grade III (high)</skos:prefLabel>
    </owl:Class>
    


    <!-- http://www.semanticweb.org/david/ontologies/2013/0/1.3.6.1.4.1.19376.1.8.2.1.749 -->

    <owl:Class rdf:about="&pathLex;749">
        <rdfs:subClassOf rdf:resource="&pathLex;418"/>
        <skos:definition xml:lang="en">Breast-Infiltrating malignant neoplasm-Histologic grade (Nottingham Histologic Score-Glandular (Acinar)/Tubular Differentiation)-Score 1: &gt;75% of tumor area forming glandular/tubular structures</skos:definition>
        <skos:prefLabel xml:lang="en">Score 1: &gt;75% of tumor area forming glandular/tubular structures</skos:prefLabel>
    </owl:Class>
    


    <!-- http://www.semanticweb.org/david/ontologies/2013/0/1.3.6.1.4.1.19376.1.8.2.1.750 -->

    <owl:Class rdf:about="&pathLex;750">
        <rdfs:subClassOf rdf:resource="&pathLex;418"/>
        <skos:definition xml:lang="en">Breast-Infiltrating malignant neoplasm-Histologic grade (Nottingham Histologic Score-Glandular (Acinar)/Tubular Differentiation)-Score 2: 10% to 75% of tumor area forming glandular/tubular structures</skos:definition>
        <skos:prefLabel xml:lang="en">Score 2: 10% to 75% of tumor area forming glandular/tubular structures</skos:prefLabel>
    </owl:Class>
    


    <!-- http://www.semanticweb.org/david/ontologies/2013/0/1.3.6.1.4.1.19376.1.8.2.1.751 -->

    <owl:Class rdf:about="&pathLex;751">
        <rdfs:subClassOf rdf:resource="&pathLex;418"/>
        <skos:definition xml:lang="en">Breast-Infiltrating malignant neoplasm-Histologic grade (Nottingham Histologic Score-Glandular (Acinar)/Tubular Differentiation)-Score 3: &lt;10% of tumor area forming glandular/tubular structures</skos:definition>
        <skos:prefLabel xml:lang="en">Score 3: &lt;10% of tumor area forming glandular/tubular structures</skos:prefLabel>
    </owl:Class>
    


    <!-- http://www.semanticweb.org/david/ontologies/2013/0/1.3.6.1.4.1.19376.1.8.2.1.752 -->

    <owl:Class rdf:about="&pathLex;752">
        <rdfs:subClassOf rdf:resource="&pathLex;420"/>
        <skos:definition xml:lang="en">Breast-Infiltrating malignant neoplasm-Histologic grade (Nottingham Histologic Score-Nuclear Pleomorphism)-Score 1: Nuclei small with little increase in size in comparison with normal breast</skos:definition>
        <skos:prefLabel xml:lang="en">Score 1: Nuclei small with little increase in size in comparison with normal breast</skos:prefLabel>
    </owl:Class>
    


    <!-- http://www.semanticweb.org/david/ontologies/2013/0/1.3.6.1.4.1.19376.1.8.2.1.753 -->

    <owl:Class rdf:about="&pathLex;753">
        <rdfs:subClassOf rdf:resource="&pathLex;99999"/>
        <skos:definition xml:lang="en">Breast-Infiltrating malignant neoplasm-Histologic grade (Nottingham Histologic Score-Nuclear Pleomorphism)-epithelial cells, regular outlines, uniform nuclear chromatin, little variation in size</skos:definition>
        <skos:prefLabel xml:lang="en">epithelial cells, regular outlines, uniform nuclear chromatin, little variation in size</skos:prefLabel>
    </owl:Class>
    


    <!-- http://www.semanticweb.org/david/ontologies/2013/0/1.3.6.1.4.1.19376.1.8.2.1.754 -->

    <owl:Class rdf:about="&pathLex;754">
        <rdfs:subClassOf rdf:resource="&pathLex;420"/>
        <skos:definition xml:lang="en">Breast-Infiltrating malignant neoplasm-Histologic grade (Nottingham Histologic Score-Nuclear Pleomorphism)-Score 2: Cells larger than normal with open vesicular nuclei, visible nucleoli, and</skos:definition>
        <skos:prefLabel xml:lang="en">Score 2: Cells larger than normal with open vesicular nuclei, visible nucleoli, and</skos:prefLabel>
    </owl:Class>
    


    <!-- http://www.semanticweb.org/david/ontologies/2013/0/1.3.6.1.4.1.19376.1.8.2.1.755 -->

    <owl:Class rdf:about="&pathLex;755">
        <rdfs:subClassOf rdf:resource="&pathLex;419"/>
        <skos:definition xml:lang="en">Breast-Infiltrating malignant neoplasm-Histologic grade (Nottingham Histologic Score-Mitotic Count)-Score 1</skos:definition>
        <skos:prefLabel xml:lang="en">Score 1</skos:prefLabel>
    </owl:Class>
    


    <!-- http://www.semanticweb.org/david/ontologies/2013/0/1.3.6.1.4.1.19376.1.8.2.1.756 -->

    <owl:Class rdf:about="&pathLex;756">
        <rdfs:subClassOf rdf:resource="&pathLex;419"/>
        <skos:definition xml:lang="en">Breast-Infiltrating malignant neoplasm-Histologic grade (Nottingham Histologic Score-Mitotic Count)-Score 2</skos:definition>
        <skos:prefLabel xml:lang="en">Score 2</skos:prefLabel>
    </owl:Class>
    


    <!-- http://www.semanticweb.org/david/ontologies/2013/0/1.3.6.1.4.1.19376.1.8.2.1.757 -->

    <owl:Class rdf:about="&pathLex;757">
        <rdfs:subClassOf rdf:resource="&pathLex;419"/>
        <skos:definition xml:lang="en">Breast-Infiltrating malignant neoplasm-Histologic grade (Nottingham Histologic Score-Mitotic Count)-Score 3</skos:definition>
        <skos:prefLabel xml:lang="en">Score 3</skos:prefLabel>
    </owl:Class>
    


    <!-- http://www.semanticweb.org/david/ontologies/2013/0/1.3.6.1.4.1.19376.1.8.2.1.758 -->

    <owl:Class rdf:about="&pathLex;758">
        <rdfs:subClassOf rdf:resource="&pathLex;99999"/>
        <skos:definition xml:lang="en">Breast-Infiltrating malignant neoplasm-Histologic grade (Nottingham)-moderate variability in both size and shape</skos:definition>
        <skos:prefLabel xml:lang="en">moderate variability in both size and shape</skos:prefLabel>
    </owl:Class>
    


    <!-- http://www.semanticweb.org/david/ontologies/2013/0/1.3.6.1.4.1.19376.1.8.2.1.759 -->

    <owl:Class rdf:about="&pathLex;759">
        <rdfs:subClassOf rdf:resource="&pathLex;420"/>
        <skos:definition xml:lang="en">Breast-Infiltrating malignant neoplasm-Histologic grade (Nottingham)-Score 3: Vesicular nuclei, often with prominent nucleoli, exhibiting marked variation</skos:definition>
        <skos:prefLabel xml:lang="en">Score 3: Vesicular nuclei, often with prominent nucleoli, exhibiting marked variation</skos:prefLabel>
    </owl:Class>
    


    <!-- http://www.semanticweb.org/david/ontologies/2013/0/1.3.6.1.4.1.19376.1.8.2.1.760 -->

    <owl:Class rdf:about="&pathLex;760">
        <rdfs:subClassOf rdf:resource="&pathLex;99999"/>
        <skos:definition xml:lang="en">Breast-Infiltrating malignant neoplasm-Histologic grade (Nottingham)-in size and shape, occasionally with very large and bizarre forms</skos:definition>
        <skos:prefLabel xml:lang="en">in size and shape, occasionally with very large and bizarre forms</skos:prefLabel>
    </owl:Class>
    


    <!-- http://www.semanticweb.org/david/ontologies/2013/0/1.3.6.1.4.1.19376.1.8.2.1.761 -->

    <owl:Class rdf:about="&pathLex;761">
        <rdfs:subClassOf rdf:resource="&pathLex;99999"/>
        <skos:prefLabel xml:lang="en">Esophagus</skos:prefLabel>
        <skos:definition xml:lang="en">Esophagus-Specimen-Target site-Esophagus</skos:definition>
    </owl:Class>
    


    <!-- http://www.semanticweb.org/david/ontologies/2013/0/1.3.6.1.4.1.19376.1.8.2.1.764 -->

    <owl:Class rdf:about="&pathLex;764">
        <rdfs:subClassOf rdf:resource="&pathLex;99999"/>
        <skos:prefLabel xml:lang="en">Cervical (proximal) esophagus</skos:prefLabel>
        <skos:definition xml:lang="en">Esophagus-Infiltrating malignant neoplasm-Lesion site-Cervical (proximal) esophagus</skos:definition>
    </owl:Class>
    


    <!-- http://www.semanticweb.org/david/ontologies/2013/0/1.3.6.1.4.1.19376.1.8.2.1.769 -->

    <owl:Class rdf:about="&pathLex;769">
        <rdfs:subClassOf rdf:resource="&pathLex;99999"/>
        <skos:prefLabel xml:lang="en">Esophagogastric junction (EGJ)</skos:prefLabel>
        <skos:definition xml:lang="en">Esophagus-Infiltrating malignant neoplasm-Lesion site-Esophagogastric junction (EGJ)</skos:definition>
    </owl:Class>
    


    <!-- http://www.semanticweb.org/david/ontologies/2013/0/1.3.6.1.4.1.19376.1.8.2.1.771 -->

    <owl:Class rdf:about="&pathLex;771">
        <rdfs:subClassOf rdf:resource="&pathLex;99999"/>
        <skos:definition xml:lang="en">Esophagus-Infiltrating malignant neoplasm-Histologic type-Squamous cell carcinoma</skos:definition>
        <skos:prefLabel xml:lang="en">Squamous cell carcinoma</skos:prefLabel>
    </owl:Class>
    


    <!-- http://www.semanticweb.org/david/ontologies/2013/0/1.3.6.1.4.1.19376.1.8.2.1.775 -->

    <owl:Class rdf:about="&pathLex;775">
        <rdfs:subClassOf rdf:resource="&pathLex;99999"/>
        <skos:prefLabel xml:lang="en">Adenocarcinoma</skos:prefLabel>
        <skos:definition xml:lang="en">Esophagus-Infiltrating malignant neoplasm-Histologic type-Adenocarcinoma</skos:definition>
    </owl:Class>
    


    <!-- http://www.semanticweb.org/david/ontologies/2013/0/1.3.6.1.4.1.19376.1.8.2.1.776 -->

    <owl:Class rdf:about="&pathLex;776">
        <rdfs:subClassOf rdf:resource="&pathLex;99999"/>
        <skos:prefLabel xml:lang="en">Adenosquamous carcinoma</skos:prefLabel>
        <skos:definition xml:lang="en">Esophagus-Infiltrating malignant neoplasm-Histologic type-Adenosquamous carcinoma</skos:definition>
    </owl:Class>
    


    <!-- http://www.semanticweb.org/david/ontologies/2013/0/1.3.6.1.4.1.19376.1.8.2.1.781 -->

    <owl:Class rdf:about="&pathLex;781">
        <rdfs:subClassOf rdf:resource="&pathLex;99999"/>
        <skos:definition xml:lang="en">Esophagus-Infiltrating malignant neoplasm-Margin site-Proximal Margin</skos:definition>
        <skos:prefLabel xml:lang="en">Proximal Margin</skos:prefLabel>
    </owl:Class>
    


    <!-- http://www.semanticweb.org/david/ontologies/2013/0/1.3.6.1.4.1.19376.1.8.2.1.782 -->

    <owl:Class rdf:about="&pathLex;782">
        <rdfs:subClassOf rdf:resource="&pathLex;99999"/>
        <skos:prefLabel xml:lang="en">Distal Margin</skos:prefLabel>
        <skos:definition xml:lang="en">Esophagus-Infiltrating malignant neoplasm-Margin site-Distal Margin</skos:definition>
    </owl:Class>
    


    <!-- http://www.semanticweb.org/david/ontologies/2013/0/1.3.6.1.4.1.19376.1.8.2.1.783 -->

    <owl:Class rdf:about="&pathLex;783">
        <rdfs:subClassOf rdf:resource="&pathLex;99999"/>
        <skos:definition xml:lang="en">Esophagus-Infiltrating malignant neoplasm-pT-pT0: No evidence of primary tumor</skos:definition>
        <skos:prefLabel xml:lang="en">pT0: No evidence of primary tumor</skos:prefLabel>
    </owl:Class>
    


    <!-- http://www.semanticweb.org/david/ontologies/2013/0/1.3.6.1.4.1.19376.1.8.2.1.784 -->

    <owl:Class rdf:about="&pathLex;784">
        <rdfs:subClassOf rdf:resource="&pathLex;99999"/>
        <skos:definition xml:lang="en">Esophagus-Infiltrating malignant neoplasm-pT-pTis: High-grade dysplasia</skos:definition>
        <skos:prefLabel xml:lang="en">pTis: High-grade dysplasia</skos:prefLabel>
    </owl:Class>
    


    <!-- http://www.semanticweb.org/david/ontologies/2013/0/1.3.6.1.4.1.19376.1.8.2.1.785 -->

    <owl:Class rdf:about="&pathLex;785">
        <rdfs:subClassOf rdf:resource="&pathLex;99999"/>
        <skos:definition xml:lang="en">Esophagus-Infiltrating malignant neoplasm-pT-pT1: Tumor invades lamina propria, muscularis mucosae, or submucosa</skos:definition>
        <skos:prefLabel xml:lang="en">pT1: Tumor invades lamina propria, muscularis mucosae, or submucosa</skos:prefLabel>
    </owl:Class>
    


    <!-- http://www.semanticweb.org/david/ontologies/2013/0/1.3.6.1.4.1.19376.1.8.2.1.786 -->

    <owl:Class rdf:about="&pathLex;786">
        <rdfs:subClassOf rdf:resource="&pathLex;99999"/>
        <skos:definition xml:lang="en">Esophagus-Infiltrating malignant neoplasm-pT-pT1a: Tumor invades lamina propria or muscularis mucosae</skos:definition>
        <skos:prefLabel xml:lang="en">pT1a: Tumor invades lamina propria or muscularis mucosae</skos:prefLabel>
    </owl:Class>
    


    <!-- http://www.semanticweb.org/david/ontologies/2013/0/1.3.6.1.4.1.19376.1.8.2.1.787 -->

    <owl:Class rdf:about="&pathLex;787">
        <rdfs:subClassOf rdf:resource="&pathLex;99999"/>
        <skos:definition xml:lang="en">Esophagus-Infiltrating malignant neoplasm-pT-pT1b: Tumor invades submucosa</skos:definition>
        <skos:prefLabel xml:lang="en">pT1b: Tumor invades submucosa</skos:prefLabel>
    </owl:Class>
    


    <!-- http://www.semanticweb.org/david/ontologies/2013/0/1.3.6.1.4.1.19376.1.8.2.1.788 -->

    <owl:Class rdf:about="&pathLex;788">
        <rdfs:subClassOf rdf:resource="&pathLex;99999"/>
        <skos:definition xml:lang="en">Esophagus-Infiltrating malignant neoplasm-pT-pT2: Tumor invades muscularis propria</skos:definition>
        <skos:prefLabel xml:lang="en">pT2: Tumor invades muscularis propria</skos:prefLabel>
    </owl:Class>
    


    <!-- http://www.semanticweb.org/david/ontologies/2013/0/1.3.6.1.4.1.19376.1.8.2.1.789 -->

    <owl:Class rdf:about="&pathLex;789">
        <rdfs:subClassOf rdf:resource="&pathLex;99999"/>
        <skos:definition xml:lang="en">Esophagus-Infiltrating malignant neoplasm-pT-pT3: Tumor invades adventitia</skos:definition>
        <skos:prefLabel xml:lang="en">pT3: Tumor invades adventitia</skos:prefLabel>
    </owl:Class>
    


    <!-- http://www.semanticweb.org/david/ontologies/2013/0/1.3.6.1.4.1.19376.1.8.2.1.790 -->

    <owl:Class rdf:about="&pathLex;790">
        <rdfs:subClassOf rdf:resource="&pathLex;99999"/>
        <skos:definition xml:lang="en">Esophagus-Infiltrating malignant neoplasm-pT-pT4: Tumor invades adjacent structures (specify)</skos:definition>
        <skos:prefLabel xml:lang="en">pT4: Tumor invades adjacent structures (specify)</skos:prefLabel>
    </owl:Class>
    


    <!-- http://www.semanticweb.org/david/ontologies/2013/0/1.3.6.1.4.1.19376.1.8.2.1.791 -->

    <owl:Class rdf:about="&pathLex;791">
        <rdfs:subClassOf rdf:resource="&pathLex;99999"/>
        <skos:definition xml:lang="en">Esophagus-Infiltrating malignant neoplasm-pT-pT4a: Resectable tumor invading pleura, pericardium, or diaphragm</skos:definition>
        <skos:prefLabel xml:lang="en">pT4a: Resectable tumor invading pleura, pericardium, or diaphragm</skos:prefLabel>
    </owl:Class>
    


    <!-- http://www.semanticweb.org/david/ontologies/2013/0/1.3.6.1.4.1.19376.1.8.2.1.792 -->

    <owl:Class rdf:about="&pathLex;792">
        <rdfs:subClassOf rdf:resource="&pathLex;99999"/>
        <skos:definition xml:lang="en">Esophagus-Infiltrating malignant neoplasm-pT-pT4b: Unresectable tumor invading other adjacent structures, such as aorta, vertebral body, trachea, etc</skos:definition>
        <skos:prefLabel xml:lang="en">pT4b: Unresectable tumor invading other adjacent structures, such as aorta, vertebral body, trachea, etc</skos:prefLabel>
    </owl:Class>
    


    <!-- http://www.semanticweb.org/david/ontologies/2013/0/1.3.6.1.4.1.19376.1.8.2.1.793 -->

    <owl:Class rdf:about="&pathLex;793">
        <rdfs:subClassOf rdf:resource="&pathLex;99999"/>
        <skos:definition xml:lang="en">Esophagus-Infiltrating malignant neoplasm-pN-pN0: No regional lymph node metastasis</skos:definition>
        <skos:prefLabel xml:lang="en">pN0: No regional lymph node metastasis</skos:prefLabel>
    </owl:Class>
    


    <!-- http://www.semanticweb.org/david/ontologies/2013/0/1.3.6.1.4.1.19376.1.8.2.1.794 -->

    <owl:Class rdf:about="&pathLex;794">
        <rdfs:subClassOf rdf:resource="&pathLex;99999"/>
        <skos:definition xml:lang="en">Esophagus-Infiltrating malignant neoplasm-pN-pN1: Regional lymph node metastasis involving 1 to 2 nodes</skos:definition>
        <skos:prefLabel xml:lang="en">pN1: Regional lymph node metastasis involving 1 to 2 nodes</skos:prefLabel>
    </owl:Class>
    


    <!-- http://www.semanticweb.org/david/ontologies/2013/0/1.3.6.1.4.1.19376.1.8.2.1.795 -->

    <owl:Class rdf:about="&pathLex;795">
        <rdfs:subClassOf rdf:resource="&pathLex;99999"/>
        <skos:definition xml:lang="en">Esophagus-Infiltrating malignant neoplasm-pN-pN2: 3 to 6 nodes involved</skos:definition>
        <skos:prefLabel xml:lang="en">pN2: 3 to 6 nodes involved</skos:prefLabel>
    </owl:Class>
    


    <!-- http://www.semanticweb.org/david/ontologies/2013/0/1.3.6.1.4.1.19376.1.8.2.1.796 -->

    <owl:Class rdf:about="&pathLex;796">
        <rdfs:subClassOf rdf:resource="&pathLex;99999"/>
        <skos:definition xml:lang="en">Esophagus-Infiltrating malignant neoplasm-pN-pN3: 7 or more nodes involved</skos:definition>
        <skos:prefLabel xml:lang="en">pN3: 7 or more nodes involved</skos:prefLabel>
    </owl:Class>
    


    <!-- http://www.semanticweb.org/david/ontologies/2013/0/1.3.6.1.4.1.19376.1.8.2.1.797 -->

    <owl:Class rdf:about="&pathLex;797">
        <rdfs:subClassOf rdf:resource="&pathLex;99999"/>
        <skos:definition xml:lang="en">Generic-Specimen-Specimen integrity -Intact specimen(s) (Unopened, Capsule intact, Single intact specimen, Multiple intact, designated specimens (margins can be evaluated))</skos:definition>
        <skos:prefLabel xml:lang="en">Intact specimen(s) (Unopened, Capsule intact, Single intact specimen, Multiple intact, designated specimens (margins can be evaluated))</skos:prefLabel>
    </owl:Class>
    


    <!-- http://www.semanticweb.org/david/ontologies/2013/0/1.3.6.1.4.1.19376.1.8.2.1.798 -->

    <owl:Class rdf:about="&pathLex;798">
        <rdfs:subClassOf rdf:resource="&pathLex;99999"/>
        <skos:definition xml:lang="en">Generic-Specimen-Specimen integrity -Non intact specimen (Open, Capsule ruptured specimen, Multiple non designated specimens (Fragmented, Morcellated)(margins cannot be evaluated with certainty)</skos:definition>
        <skos:prefLabel xml:lang="en">Non intact specimen (Open, Capsule ruptured specimen, Multiple non designated specimens (Fragmented, Morcellated)(margins cannot be evaluated with certainty)</skos:prefLabel>
    </owl:Class>
    


    <!-- http://www.semanticweb.org/david/ontologies/2013/0/1.3.6.1.4.1.19376.1.8.2.1.799 -->

    <owl:Class rdf:about="&pathLex;799">
        <rdfs:subClassOf rdf:resource="&pathLex;99999"/>
        <skos:definition xml:lang="en">Generic-Lesion-Lesion focality-Single focus (Solitary - Unifocal)</skos:definition>
        <skos:prefLabel xml:lang="en">Single focus (Solitary - Unifocal)</skos:prefLabel>
    </owl:Class>
    


    <!-- http://www.semanticweb.org/david/ontologies/2013/0/1.3.6.1.4.1.19376.1.8.2.1.8 -->

    <owl:Class rdf:about="&pathLex;8">
        <rdfs:subClassOf rdf:resource="&pathLex;99999"/>
        <skos:definition xml:lang="en">Generic-Lesion-Lesion focality</skos:definition>
        <skos:prefLabel xml:lang="en">Lesion focality</skos:prefLabel>
    </owl:Class>
    


    <!-- http://www.semanticweb.org/david/ontologies/2013/0/1.3.6.1.4.1.19376.1.8.2.1.800 -->

    <owl:Class rdf:about="&pathLex;800">
        <rdfs:subClassOf rdf:resource="&pathLex;99999"/>
        <skos:definition xml:lang="en">Generic-Lesion-Lesion focality-Multiple foci (Multifocal - (Ipsilateral – Bilateral))(specify location)</skos:definition>
        <skos:prefLabel xml:lang="en">Multiple foci (Multifocal - (Ipsilateral – Bilateral))(specify location)</skos:prefLabel>
    </owl:Class>
    


    <!-- http://www.semanticweb.org/david/ontologies/2013/0/1.3.6.1.4.1.19376.1.8.2.1.801 -->

    <owl:Class rdf:about="&pathLex;801">
        <rdfs:subClassOf rdf:resource="&pathLex;99999"/>
        <skos:definition xml:lang="en">Generic-Infiltrating malignant neoplasm-Lesion focality-Single focus (Solitary - Unifocal)</skos:definition>
        <skos:prefLabel xml:lang="en">Single focus (Solitary - Unifocal)</skos:prefLabel>
    </owl:Class>
    


    <!-- http://www.semanticweb.org/david/ontologies/2013/0/1.3.6.1.4.1.19376.1.8.2.1.802 -->

    <owl:Class rdf:about="&pathLex;802">
        <rdfs:subClassOf rdf:resource="&pathLex;99999"/>
        <skos:definition xml:lang="en">Generic-Infiltrating malignant neoplasm-Lesion focality-Multiple foci (Multifocal - (Ipsilateral – Bilateral))(specify location)</skos:definition>
        <skos:prefLabel xml:lang="en">Multiple foci (Multifocal - (Ipsilateral – Bilateral))(specify location)</skos:prefLabel>
    </owl:Class>
    


    <!-- http://www.semanticweb.org/david/ontologies/2013/0/1.3.6.1.4.1.19376.1.8.2.1.803 -->

    <owl:Class rdf:about="&pathLex;803">
        <rdfs:subClassOf rdf:resource="&pathLex;99999"/>
        <skos:definition xml:lang="en">Pancreas-Specimen-Target site-Stomach</skos:definition>
        <skos:prefLabel xml:lang="en">Stomach</skos:prefLabel>
    </owl:Class>
    


    <!-- http://www.semanticweb.org/david/ontologies/2013/0/1.3.6.1.4.1.19376.1.8.2.1.805 -->

    <owl:Class rdf:about="&pathLex;805">
        <rdfs:subClassOf rdf:resource="&pathLex;99999"/>
        <skos:definition xml:lang="en">Stomach-Specimen-Specimen collection procedure-Total gastrectomy</skos:definition>
        <skos:prefLabel xml:lang="en">Total gastrectomy</skos:prefLabel>
    </owl:Class>
    


    <!-- http://www.semanticweb.org/david/ontologies/2013/0/1.3.6.1.4.1.19376.1.8.2.1.806 -->

    <owl:Class rdf:about="&pathLex;806">
        <rdfs:subClassOf rdf:resource="&pathLex;99999"/>
        <skos:prefLabel xml:lang="en">Partial gastrectomy, proximal</skos:prefLabel>
        <skos:definition xml:lang="en">Stomach-Specimen-Specimen collection procedure-Partial gastrectomy, proximal</skos:definition>
    </owl:Class>
    


    <!-- http://www.semanticweb.org/david/ontologies/2013/0/1.3.6.1.4.1.19376.1.8.2.1.807 -->

    <owl:Class rdf:about="&pathLex;807">
        <rdfs:subClassOf rdf:resource="&pathLex;99999"/>
        <skos:prefLabel xml:lang="en">Partial gastrectomy, distal</skos:prefLabel>
        <skos:definition xml:lang="en">Stomach-Specimen-Specimen collection procedure-Partial gastrectomy, distal</skos:definition>
    </owl:Class>
    


    <!-- http://www.semanticweb.org/david/ontologies/2013/0/1.3.6.1.4.1.19376.1.8.2.1.808 -->

    <owl:Class rdf:about="&pathLex;808">
        <rdfs:subClassOf rdf:resource="&pathLex;99999"/>
        <skos:prefLabel xml:lang="en">Endoscopic resection</skos:prefLabel>
        <skos:definition xml:lang="en">Stomach-Specimen-Specimen collection procedure-Endoscopic resection</skos:definition>
    </owl:Class>
    


    <!-- http://www.semanticweb.org/david/ontologies/2013/0/1.3.6.1.4.1.19376.1.8.2.1.81 -->

    <owl:Class rdf:about="&pathLex;81">
        <rdfs:subClassOf rdf:resource="&pathLex;99999"/>
        <skos:definition xml:lang="en">Larynx-Infiltrating malignant neoplasm-pN mucosal malignant melanoma</skos:definition>
        <skos:prefLabel xml:lang="en">pN mucosal malignant melanoma</skos:prefLabel>
    </owl:Class>
    


    <!-- http://www.semanticweb.org/david/ontologies/2013/0/1.3.6.1.4.1.19376.1.8.2.1.814 -->

    <owl:Class rdf:about="&pathLex;814">
        <rdfs:subClassOf rdf:resource="&pathLex;99999"/>
        <skos:definition xml:lang="en">Stomach-Infiltrating malignant neoplasm-Histologic type-Tubular adenocarcinoma</skos:definition>
        <skos:prefLabel xml:lang="en">Tubular adenocarcinoma</skos:prefLabel>
    </owl:Class>
    


    <!-- http://www.semanticweb.org/david/ontologies/2013/0/1.3.6.1.4.1.19376.1.8.2.1.815 -->

    <owl:Class rdf:about="&pathLex;815">
        <rdfs:subClassOf rdf:resource="&pathLex;99999"/>
        <skos:prefLabel xml:lang="en">Papillary adenocarcinoma</skos:prefLabel>
        <skos:definition xml:lang="en">Stomach-Infiltrating malignant neoplasm-Histologic type-Papillary adenocarcinoma</skos:definition>
    </owl:Class>
    


    <!-- http://www.semanticweb.org/david/ontologies/2013/0/1.3.6.1.4.1.19376.1.8.2.1.816 -->

    <owl:Class rdf:about="&pathLex;816">
        <rdfs:subClassOf rdf:resource="&pathLex;99999"/>
        <skos:prefLabel xml:lang="en">Mucinous adenocarcinoma (greater than 50% mucinous)</skos:prefLabel>
        <skos:definition xml:lang="en">Stomach-Infiltrating malignant neoplasm-Histologic type-Mucinous adenocarcinoma (greater than 50% mucinous)</skos:definition>
    </owl:Class>
    


    <!-- http://www.semanticweb.org/david/ontologies/2013/0/1.3.6.1.4.1.19376.1.8.2.1.82 -->

    <owl:Class rdf:about="&pathLex;82">
        <rdfs:subClassOf rdf:resource="&pathLex;99999"/>
        <skos:definition xml:lang="en">Larynx-Infiltrating malignant neoplasm-pN carcinoma</skos:definition>
        <skos:prefLabel xml:lang="en">pN carcinoma</skos:prefLabel>
    </owl:Class>
    


    <!-- http://www.semanticweb.org/david/ontologies/2013/0/1.3.6.1.4.1.19376.1.8.2.1.822 -->

    <owl:Class rdf:about="&pathLex;822">
        <rdfs:subClassOf rdf:resource="&pathLex;99999"/>
        <skos:prefLabel xml:lang="en">Carcinoma, not otherwise specified</skos:prefLabel>
        <skos:definition xml:lang="en">Stomach-Infiltrating malignant neoplasm-Histologic type-Carcinoma, not otherwise specified</skos:definition>
    </owl:Class>
    


    <!-- http://www.semanticweb.org/david/ontologies/2013/0/1.3.6.1.4.1.19376.1.8.2.1.825 -->

    <owl:Class rdf:about="&pathLex;825">
        <rdfs:subClassOf rdf:resource="&pathLex;99999"/>
        <skos:prefLabel xml:lang="en">Proximal Margin</skos:prefLabel>
        <skos:definition xml:lang="en">Stomach-Infiltrating malignant neoplasm-Margin site-Proximal Margin</skos:definition>
    </owl:Class>
    


    <!-- http://www.semanticweb.org/david/ontologies/2013/0/1.3.6.1.4.1.19376.1.8.2.1.826 -->

    <owl:Class rdf:about="&pathLex;826">
        <rdfs:subClassOf rdf:resource="&pathLex;99999"/>
        <skos:prefLabel xml:lang="en">Distal Margin</skos:prefLabel>
        <skos:definition xml:lang="en">Stomach-Infiltrating malignant neoplasm-Margin site-Distal Margin</skos:definition>
    </owl:Class>
    


    <!-- http://www.semanticweb.org/david/ontologies/2013/0/1.3.6.1.4.1.19376.1.8.2.1.827 -->

    <owl:Class rdf:about="&pathLex;827">
        <rdfs:subClassOf rdf:resource="&pathLex;99999"/>
        <skos:definition xml:lang="en">Stomach-Infiltrating malignant neoplasm-pT-pT0: No evidence of primary tumor</skos:definition>
        <skos:prefLabel xml:lang="en">pT0: No evidence of primary tumor</skos:prefLabel>
    </owl:Class>
    


    <!-- http://www.semanticweb.org/david/ontologies/2013/0/1.3.6.1.4.1.19376.1.8.2.1.828 -->

    <owl:Class rdf:about="&pathLex;828">
        <rdfs:subClassOf rdf:resource="&pathLex;99999"/>
        <skos:definition xml:lang="en">Stomach-Infiltrating malignant neoplasm-pT-pTis: Carcinoma in situ</skos:definition>
        <skos:prefLabel xml:lang="en">pTis: Carcinoma in situ</skos:prefLabel>
    </owl:Class>
    


    <!-- http://www.semanticweb.org/david/ontologies/2013/0/1.3.6.1.4.1.19376.1.8.2.1.829 -->

    <owl:Class rdf:about="&pathLex;829">
        <rdfs:subClassOf rdf:resource="&pathLex;99999"/>
        <skos:definition xml:lang="en">Stomach-Infiltrating malignant neoplasm-pT-pT1: Tumor invades lamina propria, muscularis mucosae, or submucosa</skos:definition>
        <skos:prefLabel xml:lang="en">pT1: Tumor invades lamina propria, muscularis mucosae, or submucosa</skos:prefLabel>
    </owl:Class>
    


    <!-- http://www.semanticweb.org/david/ontologies/2013/0/1.3.6.1.4.1.19376.1.8.2.1.830 -->

    <owl:Class rdf:about="&pathLex;830">
        <rdfs:subClassOf rdf:resource="&pathLex;99999"/>
        <skos:definition xml:lang="en">Stomach-Infiltrating malignant neoplasm-pT-pT1a: Tumor invades lamina propria or muscularis mucosae</skos:definition>
        <skos:prefLabel xml:lang="en">pT1a: Tumor invades lamina propria or muscularis mucosae</skos:prefLabel>
    </owl:Class>
    


    <!-- http://www.semanticweb.org/david/ontologies/2013/0/1.3.6.1.4.1.19376.1.8.2.1.831 -->

    <owl:Class rdf:about="&pathLex;831">
        <rdfs:subClassOf rdf:resource="&pathLex;99999"/>
        <skos:definition xml:lang="en">Stomach-Infiltrating malignant neoplasm-pT-pT1b: Tumor invades submucosa</skos:definition>
        <skos:prefLabel xml:lang="en">pT1b: Tumor invades submucosa</skos:prefLabel>
    </owl:Class>
    


    <!-- http://www.semanticweb.org/david/ontologies/2013/0/1.3.6.1.4.1.19376.1.8.2.1.832 -->

    <owl:Class rdf:about="&pathLex;832">
        <rdfs:subClassOf rdf:resource="&pathLex;99999"/>
        <skos:definition xml:lang="en">Stomach-Infiltrating malignant neoplasm-pT-pT2: Tumor invades muscularis propria</skos:definition>
        <skos:prefLabel xml:lang="en">pT2: Tumor invades muscularis propria</skos:prefLabel>
    </owl:Class>
    


    <!-- http://www.semanticweb.org/david/ontologies/2013/0/1.3.6.1.4.1.19376.1.8.2.1.833 -->

    <owl:Class rdf:about="&pathLex;833">
        <rdfs:subClassOf rdf:resource="&pathLex;99999"/>
        <skos:definition xml:lang="en">Stomach-Infiltrating malignant neoplasm-pT-pT3: Tumor invades subserosal connective tissue, without involvement of visceral peritoneum or adjacent structures</skos:definition>
        <skos:prefLabel xml:lang="en">pT3: Tumor invades subserosal connective tissue, without involvement of visceral peritoneum or adjacent structures</skos:prefLabel>
    </owl:Class>
    


    <!-- http://www.semanticweb.org/david/ontologies/2013/0/1.3.6.1.4.1.19376.1.8.2.1.834 -->

    <owl:Class rdf:about="&pathLex;834">
        <rdfs:subClassOf rdf:resource="&pathLex;99999"/>
        <skos:definition xml:lang="en">Stomach-Infiltrating malignant neoplasm-pT-pT4: Tumor involves serosa (visceral peritoneum) or adjacent structures</skos:definition>
        <skos:prefLabel xml:lang="en">pT4: Tumor involves serosa (visceral peritoneum) or adjacent structures</skos:prefLabel>
    </owl:Class>
    


    <!-- http://www.semanticweb.org/david/ontologies/2013/0/1.3.6.1.4.1.19376.1.8.2.1.835 -->

    <owl:Class rdf:about="&pathLex;835">
        <rdfs:subClassOf rdf:resource="&pathLex;99999"/>
        <skos:definition xml:lang="en">Stomach-Infiltrating malignant neoplasm-pT-pT4a: Tumor invades serosa (visceral peritoneum)</skos:definition>
        <skos:prefLabel xml:lang="en">pT4a: Tumor invades serosa (visceral peritoneum)</skos:prefLabel>
    </owl:Class>
    


    <!-- http://www.semanticweb.org/david/ontologies/2013/0/1.3.6.1.4.1.19376.1.8.2.1.836 -->

    <owl:Class rdf:about="&pathLex;836">
        <rdfs:subClassOf rdf:resource="&pathLex;99999"/>
        <skos:definition xml:lang="en">Stomach-Infiltrating malignant neoplasm-pT-pT4b: Tumor invades adjacent structures</skos:definition>
        <skos:prefLabel xml:lang="en">pT4b: Tumor invades adjacent structures</skos:prefLabel>
    </owl:Class>
    


    <!-- http://www.semanticweb.org/david/ontologies/2013/0/1.3.6.1.4.1.19376.1.8.2.1.837 -->

    <owl:Class rdf:about="&pathLex;837">
        <rdfs:subClassOf rdf:resource="&pathLex;99999"/>
        <skos:definition xml:lang="en">Stomach-Infiltrating malignant neoplasm-pN-pN0: No regional lymph node metastasis</skos:definition>
        <skos:prefLabel xml:lang="en">pN0: No regional lymph node metastasis</skos:prefLabel>
    </owl:Class>
    


    <!-- http://www.semanticweb.org/david/ontologies/2013/0/1.3.6.1.4.1.19376.1.8.2.1.838 -->

    <owl:Class rdf:about="&pathLex;838">
        <rdfs:subClassOf rdf:resource="&pathLex;99999"/>
        <skos:definition xml:lang="en">Stomach-Infiltrating malignant neoplasm-pN-pN1: Metastasis in 1 to 2 perigastric lymph nodes</skos:definition>
        <skos:prefLabel xml:lang="en">pN1: Metastasis in 1 to 2 perigastric lymph nodes</skos:prefLabel>
    </owl:Class>
    


    <!-- http://www.semanticweb.org/david/ontologies/2013/0/1.3.6.1.4.1.19376.1.8.2.1.839 -->

    <owl:Class rdf:about="&pathLex;839">
        <rdfs:subClassOf rdf:resource="&pathLex;99999"/>
        <skos:definition xml:lang="en">Stomach-Infiltrating malignant neoplasm-pN-pN2: Metastasis in 3 to 6 perigastric lymph nodes</skos:definition>
        <skos:prefLabel xml:lang="en">pN2: Metastasis in 3 to 6 perigastric lymph nodes</skos:prefLabel>
    </owl:Class>
    


    <!-- http://www.semanticweb.org/david/ontologies/2013/0/1.3.6.1.4.1.19376.1.8.2.1.840 -->

    <owl:Class rdf:about="&pathLex;840">
        <rdfs:subClassOf rdf:resource="&pathLex;99999"/>
        <skos:definition xml:lang="en">Stomach-Infiltrating malignant neoplasm-pN-pN3: Metastasis in 7 or more perigastric lymph nodes</skos:definition>
        <skos:prefLabel xml:lang="en">pN3: Metastasis in 7 or more perigastric lymph nodes</skos:prefLabel>
    </owl:Class>
    


    <!-- http://www.semanticweb.org/david/ontologies/2013/0/1.3.6.1.4.1.19376.1.8.2.1.841 -->

    <owl:Class rdf:about="&pathLex;841">
        <rdfs:subClassOf rdf:resource="&pathLex;99999"/>
        <skos:definition xml:lang="en">Stomach-Infiltrating malignant neoplasm-pN-pN3a: Metastasis in 7 to 15 perigastric lymph nodes</skos:definition>
        <skos:prefLabel xml:lang="en">pN3a: Metastasis in 7 to 15 perigastric lymph nodes</skos:prefLabel>
    </owl:Class>
    


    <!-- http://www.semanticweb.org/david/ontologies/2013/0/1.3.6.1.4.1.19376.1.8.2.1.842 -->

    <owl:Class rdf:about="&pathLex;842">
        <rdfs:subClassOf rdf:resource="&pathLex;99999"/>
        <skos:definition xml:lang="en">Stomach-Infiltrating malignant neoplasm-pN-pN3b: Metastassis in 16 or more perigastric lymph nodes</skos:definition>
        <skos:prefLabel xml:lang="en">pN3b: Metastassis in 16 or more perigastric lymph nodes</skos:prefLabel>
    </owl:Class>
    


    <!-- http://www.semanticweb.org/david/ontologies/2013/0/1.3.6.1.4.1.19376.1.8.2.1.85 -->

    <owl:Class rdf:about="&pathLex;85">
        <rdfs:subClassOf rdf:resource="&pathLex;99999"/>
        <skos:definition xml:lang="en">Lip, oral cavity-Infiltrating malignant neoplasm-pT carcinoma</skos:definition>
        <skos:prefLabel xml:lang="en">pT carcinoma</skos:prefLabel>
    </owl:Class>
    


    <!-- http://www.semanticweb.org/david/ontologies/2013/0/1.3.6.1.4.1.19376.1.8.2.1.851 -->

    <owl:Class rdf:about="&pathLex;851">
        <rdfs:subClassOf rdf:resource="&pathLex;99999"/>
        <skos:definition xml:lang="en">Colon-Infiltrating malignant neoplasm-Lesion site-Right (ascending) colon</skos:definition>
        <skos:prefLabel xml:lang="en">Right (ascending) colon</skos:prefLabel>
    </owl:Class>
    


    <!-- http://www.semanticweb.org/david/ontologies/2013/0/1.3.6.1.4.1.19376.1.8.2.1.852 -->

    <owl:Class rdf:about="&pathLex;852">
        <rdfs:subClassOf rdf:resource="&pathLex;99999"/>
        <skos:definition xml:lang="en">Colon-Infiltrating malignant neoplasm-Lesion site-Hepatic flexure</skos:definition>
        <skos:prefLabel xml:lang="en">Hepatic flexure</skos:prefLabel>
    </owl:Class>
    


    <!-- http://www.semanticweb.org/david/ontologies/2013/0/1.3.6.1.4.1.19376.1.8.2.1.853 -->

    <owl:Class rdf:about="&pathLex;853">
        <rdfs:subClassOf rdf:resource="&pathLex;99999"/>
        <skos:definition xml:lang="en">Colon-Infiltrating malignant neoplasm-Lesion site-Transverse colon</skos:definition>
        <skos:prefLabel xml:lang="en">Transverse colon</skos:prefLabel>
    </owl:Class>
    


    <!-- http://www.semanticweb.org/david/ontologies/2013/0/1.3.6.1.4.1.19376.1.8.2.1.854 -->

    <owl:Class rdf:about="&pathLex;854">
        <rdfs:subClassOf rdf:resource="&pathLex;99999"/>
        <skos:definition xml:lang="en">Colon-Infiltrating malignant neoplasm-Lesion site-Splenic flexure</skos:definition>
        <skos:prefLabel xml:lang="en">Splenic flexure</skos:prefLabel>
    </owl:Class>
    


    <!-- http://www.semanticweb.org/david/ontologies/2013/0/1.3.6.1.4.1.19376.1.8.2.1.855 -->

    <owl:Class rdf:about="&pathLex;855">
        <rdfs:subClassOf rdf:resource="&pathLex;99999"/>
        <skos:definition xml:lang="en">Colon-Infiltrating malignant neoplasm-Lesion site-Left (descending) colon</skos:definition>
        <skos:prefLabel xml:lang="en">Left (descending) colon</skos:prefLabel>
    </owl:Class>
    


    <!-- http://www.semanticweb.org/david/ontologies/2013/0/1.3.6.1.4.1.19376.1.8.2.1.856 -->

    <owl:Class rdf:about="&pathLex;856">
        <rdfs:subClassOf rdf:resource="&pathLex;99999"/>
        <skos:definition xml:lang="en">Colon-Infiltrating malignant neoplasm-Lesion site-Sigmoid colon</skos:definition>
        <skos:prefLabel xml:lang="en">Sigmoid colon</skos:prefLabel>
    </owl:Class>
    


    <!-- http://www.semanticweb.org/david/ontologies/2013/0/1.3.6.1.4.1.19376.1.8.2.1.857 -->

    <owl:Class rdf:about="&pathLex;857">
        <rdfs:subClassOf rdf:resource="&pathLex;10008"/>
        <skos:definition xml:lang="en">Cervix-Specimen-Target site-Rectum</skos:definition>
        <skos:prefLabel xml:lang="en">Rectum</skos:prefLabel>
    </owl:Class>
    


    <!-- http://www.semanticweb.org/david/ontologies/2013/0/1.3.6.1.4.1.19376.1.8.2.1.858 -->

    <owl:Class rdf:about="&pathLex;858">
        <rdfs:subClassOf rdf:resource="&pathLex;99999"/>
        <skos:prefLabel xml:lang="en">Adenocarcinoma</skos:prefLabel>
        <skos:definition xml:lang="en">Colon-Infiltrating malignant neoplasm-Histologic type-Adenocarcinoma</skos:definition>
    </owl:Class>
    


    <!-- http://www.semanticweb.org/david/ontologies/2013/0/1.3.6.1.4.1.19376.1.8.2.1.859 -->

    <owl:Class rdf:about="&pathLex;859">
        <rdfs:subClassOf rdf:resource="&pathLex;99999"/>
        <skos:definition xml:lang="en">Colon-Infiltrating malignant neoplasm-Histologic type-Mucinous adenocarcinoma</skos:definition>
        <skos:prefLabel xml:lang="en">Mucinous adenocarcinoma</skos:prefLabel>
    </owl:Class>
    


    <!-- http://www.semanticweb.org/david/ontologies/2013/0/1.3.6.1.4.1.19376.1.8.2.1.86 -->

    <owl:Class rdf:about="&pathLex;86">
        <rdfs:subClassOf rdf:resource="&pathLex;99999"/>
        <skos:definition xml:lang="en">Larynx-Infiltrating malignant neoplasm-pT glottis carcinoma</skos:definition>
        <skos:prefLabel xml:lang="en">pT glottis carcinoma</skos:prefLabel>
    </owl:Class>
    


    <!-- http://www.semanticweb.org/david/ontologies/2013/0/1.3.6.1.4.1.19376.1.8.2.1.860 -->

    <owl:Class rdf:about="&pathLex;860">
        <rdfs:subClassOf rdf:resource="&pathLex;99999"/>
        <skos:definition xml:lang="en">Colon-Infiltrating malignant neoplasm-Histologic type-Signet-ring cell carcinoma</skos:definition>
        <skos:prefLabel xml:lang="en">Signet-ring cell carcinoma</skos:prefLabel>
    </owl:Class>
    


    <!-- http://www.semanticweb.org/david/ontologies/2013/0/1.3.6.1.4.1.19376.1.8.2.1.861 -->

    <owl:Class rdf:about="&pathLex;861">
        <rdfs:subClassOf rdf:resource="&pathLex;99999"/>
        <skos:definition xml:lang="en">Colon-Infiltrating malignant neoplasm-Histologic type-Medullary carcinoma</skos:definition>
        <skos:prefLabel xml:lang="en">Medullary carcinoma</skos:prefLabel>
    </owl:Class>
    


    <!-- http://www.semanticweb.org/david/ontologies/2013/0/1.3.6.1.4.1.19376.1.8.2.1.862 -->

    <owl:Class rdf:about="&pathLex;862">
        <rdfs:subClassOf rdf:resource="&pathLex;99999"/>
        <skos:definition xml:lang="en">Colon-Infiltrating malignant neoplasm-Histologic type-Undifferentiated carcinoma</skos:definition>
        <skos:prefLabel xml:lang="en">Undifferentiated carcinoma</skos:prefLabel>
    </owl:Class>
    


    <!-- http://www.semanticweb.org/david/ontologies/2013/0/1.3.6.1.4.1.19376.1.8.2.1.865 -->

    <owl:Class rdf:about="&pathLex;865">
        <rdfs:subClassOf rdf:resource="&pathLex;99999"/>
        <skos:definition xml:lang="en">Colon-Infiltrating malignant neoplasm-Margin site-Proximal Margin</skos:definition>
        <skos:prefLabel xml:lang="en">Proximal Margin</skos:prefLabel>
    </owl:Class>
    


    <!-- http://www.semanticweb.org/david/ontologies/2013/0/1.3.6.1.4.1.19376.1.8.2.1.866 -->

    <owl:Class rdf:about="&pathLex;866">
        <rdfs:subClassOf rdf:resource="&pathLex;99999"/>
        <skos:definition xml:lang="en">Colon-Infiltrating malignant neoplasm-Margin site-Distal Margin</skos:definition>
        <skos:prefLabel xml:lang="en">Distal Margin</skos:prefLabel>
    </owl:Class>
    


    <!-- http://www.semanticweb.org/david/ontologies/2013/0/1.3.6.1.4.1.19376.1.8.2.1.867 -->

    <owl:Class rdf:about="&pathLex;867">
        <rdfs:subClassOf rdf:resource="&pathLex;99999"/>
        <skos:definition xml:lang="en">Colon-Infiltrating malignant neoplasm-pT-pT0: No evidence of primary tumor</skos:definition>
        <skos:prefLabel xml:lang="en">pT0: No evidence of primary tumor</skos:prefLabel>
    </owl:Class>
    


    <!-- http://www.semanticweb.org/david/ontologies/2013/0/1.3.6.1.4.1.19376.1.8.2.1.868 -->

    <owl:Class rdf:about="&pathLex;868">
        <rdfs:subClassOf rdf:resource="&pathLex;99999"/>
        <skos:definition xml:lang="en">Colon-Infiltrating malignant neoplasm-pT-pTis: Carcinoma in situ, intraepithelial (no invasion)</skos:definition>
        <skos:prefLabel xml:lang="en">pTis: Carcinoma in situ, intraepithelial (no invasion)</skos:prefLabel>
    </owl:Class>
    


    <!-- http://www.semanticweb.org/david/ontologies/2013/0/1.3.6.1.4.1.19376.1.8.2.1.869 -->

    <owl:Class rdf:about="&pathLex;869">
        <rdfs:subClassOf rdf:resource="&pathLex;99999"/>
        <skos:definition xml:lang="en">Colon-Infiltrating malignant neoplasm-pT-pTis: Carcinoma in situ, invasion of lamina propria</skos:definition>
        <skos:prefLabel xml:lang="en">pTis: Carcinoma in situ, invasion of lamina propria</skos:prefLabel>
    </owl:Class>
    


    <!-- http://www.semanticweb.org/david/ontologies/2013/0/1.3.6.1.4.1.19376.1.8.2.1.87 -->

    <owl:Class rdf:about="&pathLex;87">
        <rdfs:subClassOf rdf:resource="&pathLex;99999"/>
        <skos:definition xml:lang="en">Larynx-Infiltrating malignant neoplasm-pT supra glottis carcinoma</skos:definition>
        <skos:prefLabel xml:lang="en">pT supra glottis carcinoma</skos:prefLabel>
    </owl:Class>
    


    <!-- http://www.semanticweb.org/david/ontologies/2013/0/1.3.6.1.4.1.19376.1.8.2.1.870 -->

    <owl:Class rdf:about="&pathLex;870">
        <rdfs:subClassOf rdf:resource="&pathLex;99999"/>
        <skos:definition xml:lang="en">Colon-Infiltrating malignant neoplasm-pT-pT1: Tumor invades submucosa</skos:definition>
        <skos:prefLabel xml:lang="en">pT1: Tumor invades submucosa</skos:prefLabel>
    </owl:Class>
    


    <!-- http://www.semanticweb.org/david/ontologies/2013/0/1.3.6.1.4.1.19376.1.8.2.1.871 -->

    <owl:Class rdf:about="&pathLex;871">
        <rdfs:subClassOf rdf:resource="&pathLex;99999"/>
        <skos:definition xml:lang="en">Colon-Infiltrating malignant neoplasm-pT-pT2: Tumor invades muscularis propria</skos:definition>
        <skos:prefLabel xml:lang="en">pT2: Tumor invades muscularis propria</skos:prefLabel>
    </owl:Class>
    


    <!-- http://www.semanticweb.org/david/ontologies/2013/0/1.3.6.1.4.1.19376.1.8.2.1.872 -->

    <owl:Class rdf:about="&pathLex;872">
        <rdfs:subClassOf rdf:resource="&pathLex;99999"/>
        <skos:definition xml:lang="en">Colon-Infiltrating malignant neoplasm-pT-pT3: Tumor invades through the muscularis propria into pericolorectal tissues</skos:definition>
        <skos:prefLabel xml:lang="en">pT3: Tumor invades through the muscularis propria into pericolorectal tissues</skos:prefLabel>
    </owl:Class>
    


    <!-- http://www.semanticweb.org/david/ontologies/2013/0/1.3.6.1.4.1.19376.1.8.2.1.873 -->

    <owl:Class rdf:about="&pathLex;873">
        <rdfs:subClassOf rdf:resource="&pathLex;99999"/>
        <skos:definition xml:lang="en">Colon-Infiltrating malignant neoplasm-pT-pT4a: Tumor penetrates the visceral peritoneum</skos:definition>
        <skos:prefLabel xml:lang="en">pT4a: Tumor penetrates the visceral peritoneum</skos:prefLabel>
    </owl:Class>
    


    <!-- http://www.semanticweb.org/david/ontologies/2013/0/1.3.6.1.4.1.19376.1.8.2.1.874 -->

    <owl:Class rdf:about="&pathLex;874">
        <rdfs:subClassOf rdf:resource="&pathLex;99999"/>
        <skos:definition xml:lang="en">Colon-Infiltrating malignant neoplasm-pT-pT4b: Tumor directly invades or is adherent to other organs or structures</skos:definition>
        <skos:prefLabel xml:lang="en">pT4b: Tumor directly invades or is adherent to other organs or structures</skos:prefLabel>
    </owl:Class>
    


    <!-- http://www.semanticweb.org/david/ontologies/2013/0/1.3.6.1.4.1.19376.1.8.2.1.875 -->

    <owl:Class rdf:about="&pathLex;875">
        <rdfs:subClassOf rdf:resource="&pathLex;99999"/>
        <skos:definition xml:lang="en">Colon-Infiltrating malignant neoplasm-pN-pN0: No regional lymph node metastasis</skos:definition>
        <skos:prefLabel xml:lang="en">pN0: No regional lymph node metastasis</skos:prefLabel>
    </owl:Class>
    


    <!-- http://www.semanticweb.org/david/ontologies/2013/0/1.3.6.1.4.1.19376.1.8.2.1.876 -->

    <owl:Class rdf:about="&pathLex;876">
        <rdfs:subClassOf rdf:resource="&pathLex;99999"/>
        <skos:definition xml:lang="en">Colon-Infiltrating malignant neoplasm-pN-pN1a: Metastasis in 1 regional lymph node</skos:definition>
        <skos:prefLabel xml:lang="en">pN1a: Metastasis in 1 regional lymph node</skos:prefLabel>
    </owl:Class>
    


    <!-- http://www.semanticweb.org/david/ontologies/2013/0/1.3.6.1.4.1.19376.1.8.2.1.877 -->

    <owl:Class rdf:about="&pathLex;877">
        <rdfs:subClassOf rdf:resource="&pathLex;99999"/>
        <skos:definition xml:lang="en">Colon-Infiltrating malignant neoplasm-pN-pN1b: Metastasis in 2 to 3 regional lymph nodes</skos:definition>
        <skos:prefLabel xml:lang="en">pN1b: Metastasis in 2 to 3 regional lymph nodes</skos:prefLabel>
    </owl:Class>
    


    <!-- http://www.semanticweb.org/david/ontologies/2013/0/1.3.6.1.4.1.19376.1.8.2.1.878 -->

    <owl:Class rdf:about="&pathLex;878">
        <rdfs:subClassOf rdf:resource="&pathLex;99999"/>
        <skos:definition xml:lang="en">Colon-Infiltrating malignant neoplasm-pN-pN1c: Tumor deposit(s) in the subserosa, or non-peritonealized pericolic or perirectal tissues without regional lymph node metastasis</skos:definition>
        <skos:prefLabel xml:lang="en">pN1c: Tumor deposit(s) in the subserosa, or non-peritonealized pericolic or perirectal tissues without regional lymph node metastasis</skos:prefLabel>
    </owl:Class>
    


    <!-- http://www.semanticweb.org/david/ontologies/2013/0/1.3.6.1.4.1.19376.1.8.2.1.879 -->

    <owl:Class rdf:about="&pathLex;879">
        <rdfs:subClassOf rdf:resource="&pathLex;99999"/>
        <skos:definition xml:lang="en">Colon-Infiltrating malignant neoplasm-pN-pN2a: Metastasis in 4 to 6 regional lymph nodes</skos:definition>
        <skos:prefLabel xml:lang="en">pN2a: Metastasis in 4 to 6 regional lymph nodes</skos:prefLabel>
    </owl:Class>
    


    <!-- http://www.semanticweb.org/david/ontologies/2013/0/1.3.6.1.4.1.19376.1.8.2.1.88 -->

    <owl:Class rdf:about="&pathLex;88">
        <rdfs:subClassOf rdf:resource="&pathLex;99999"/>
        <skos:definition xml:lang="en">Larynx-Infiltrating malignant neoplasm-pT sub glottis carcinoma</skos:definition>
        <skos:prefLabel xml:lang="en">pT sub glottis carcinoma</skos:prefLabel>
    </owl:Class>
    


    <!-- http://www.semanticweb.org/david/ontologies/2013/0/1.3.6.1.4.1.19376.1.8.2.1.880 -->

    <owl:Class rdf:about="&pathLex;880">
        <rdfs:subClassOf rdf:resource="&pathLex;99999"/>
        <skos:definition xml:lang="en">Colon-Infiltrating malignant neoplasm-pN-pN2b: Metastasis in 7 or more regional lymph nodes</skos:definition>
        <skos:prefLabel xml:lang="en">pN2b: Metastasis in 7 or more regional lymph nodes</skos:prefLabel>
    </owl:Class>
    


    <!-- http://www.semanticweb.org/david/ontologies/2013/0/1.3.6.1.4.1.19376.1.8.2.1.881 -->

    <owl:Class rdf:about="&pathLex;881">
        <rdfs:subClassOf rdf:resource="&pathLex;99999"/>
        <skos:prefLabel xml:lang="en">Liver</skos:prefLabel>
        <skos:definition xml:lang="en">Liver-Infiltrating malignant neoplasm-Lesion site-Liver</skos:definition>
    </owl:Class>
    


    <!-- http://www.semanticweb.org/david/ontologies/2013/0/1.3.6.1.4.1.19376.1.8.2.1.885 -->

    <owl:Class rdf:about="&pathLex;885">
        <rdfs:subClassOf rdf:resource="&pathLex;99999"/>
        <skos:definition xml:lang="en">Liver-Specimen-Specimen collection procedure-Total hepatectomy</skos:definition>
        <skos:prefLabel xml:lang="en">Total hepatectomy</skos:prefLabel>
    </owl:Class>
    


    <!-- http://www.semanticweb.org/david/ontologies/2013/0/1.3.6.1.4.1.19376.1.8.2.1.898 -->

    <owl:Class rdf:about="&pathLex;898">
        <rdfs:subClassOf rdf:resource="&pathLex;99999"/>
        <skos:prefLabel xml:lang="en">Hepatocellular carcinoma</skos:prefLabel>
        <skos:definition xml:lang="en">Liver-Infiltrating malignant neoplasm-Histologic type-Hepatocellular carcinoma</skos:definition>
    </owl:Class>
    


    <!-- http://www.semanticweb.org/david/ontologies/2013/0/1.3.6.1.4.1.19376.1.8.2.1.9 -->

    <owl:Class rdf:about="&pathLex;9">
        <rdfs:subClassOf rdf:resource="&pathLex;99999"/>
        <skos:definition xml:lang="en">Generic-Infiltrating malignant neoplasm-Lesion focality</skos:definition>
        <skos:prefLabel xml:lang="en">Lesion focality</skos:prefLabel>
    </owl:Class>
    


    <!-- http://www.semanticweb.org/david/ontologies/2013/0/1.3.6.1.4.1.19376.1.8.2.1.906 -->

    <owl:Class rdf:about="&pathLex;906">
        <rdfs:subClassOf rdf:resource="&pathLex;99999"/>
        <skos:definition xml:lang="en">Liver-Infiltrating malignant neoplasm-pT-pT0: No evidence of primary tumor</skos:definition>
        <skos:prefLabel xml:lang="en">pT0: No evidence of primary tumor</skos:prefLabel>
    </owl:Class>
    


    <!-- http://www.semanticweb.org/david/ontologies/2013/0/1.3.6.1.4.1.19376.1.8.2.1.907 -->

    <owl:Class rdf:about="&pathLex;907">
        <rdfs:subClassOf rdf:resource="&pathLex;99999"/>
        <skos:definition xml:lang="en">Liver-Infiltrating malignant neoplasm-pT-pT1: Solitary tumor without vascular invasion</skos:definition>
        <skos:prefLabel xml:lang="en">pT1: Solitary tumor without vascular invasion</skos:prefLabel>
    </owl:Class>
    


    <!-- http://www.semanticweb.org/david/ontologies/2013/0/1.3.6.1.4.1.19376.1.8.2.1.908 -->

    <owl:Class rdf:about="&pathLex;908">
        <rdfs:subClassOf rdf:resource="&pathLex;99999"/>
        <skos:definition xml:lang="en">Liver-Infiltrating malignant neoplasm-pT-pT2: Solitary tumor with vascular invasion or multiple tumors none more than 5 cm</skos:definition>
        <skos:prefLabel xml:lang="en">pT2: Solitary tumor with vascular invasion or multiple tumors none more than 5 cm</skos:prefLabel>
    </owl:Class>
    


    <!-- http://www.semanticweb.org/david/ontologies/2013/0/1.3.6.1.4.1.19376.1.8.2.1.909 -->

    <owl:Class rdf:about="&pathLex;909">
        <rdfs:subClassOf rdf:resource="&pathLex;99999"/>
        <skos:definition xml:lang="en">Liver-Infiltrating malignant neoplasm-pT-pT3a: Multiple tumors more than 5 cm</skos:definition>
        <skos:prefLabel xml:lang="en">pT3a: Multiple tumors more than 5 cm</skos:prefLabel>
    </owl:Class>
    


    <!-- http://www.semanticweb.org/david/ontologies/2013/0/1.3.6.1.4.1.19376.1.8.2.1.91 -->

    <owl:Class rdf:about="&pathLex;91">
        <rdfs:subClassOf rdf:resource="&pathLex;99999"/>
        <skos:definition xml:lang="en">Larynx-Infiltrating malignant neoplasm-pT mucosal malignant melanoma</skos:definition>
        <skos:prefLabel xml:lang="en">pT mucosal malignant melanoma</skos:prefLabel>
    </owl:Class>
    


    <!-- http://www.semanticweb.org/david/ontologies/2013/0/1.3.6.1.4.1.19376.1.8.2.1.910 -->

    <owl:Class rdf:about="&pathLex;910">
        <rdfs:subClassOf rdf:resource="&pathLex;99999"/>
        <skos:definition xml:lang="en">Liver-Infiltrating malignant neoplasm-pT-pT3b: Single tumor or multiple tumors of any size involving a major branch of the portal vein or hepatic veins</skos:definition>
        <skos:prefLabel xml:lang="en">pT3b: Single tumor or multiple tumors of any size involving a major branch of the portal vein or hepatic veins</skos:prefLabel>
    </owl:Class>
    


    <!-- http://www.semanticweb.org/david/ontologies/2013/0/1.3.6.1.4.1.19376.1.8.2.1.911 -->

    <owl:Class rdf:about="&pathLex;911">
        <rdfs:subClassOf rdf:resource="&pathLex;99999"/>
        <skos:definition xml:lang="en">Liver-Infiltrating malignant neoplasm-pT-pT4: Tumor(s) with direct invasion of adjacent organs other than the gallbladder or with perforation of visceral peritoneum</skos:definition>
        <skos:prefLabel xml:lang="en">pT4: Tumor(s) with direct invasion of adjacent organs other than the gallbladder or with perforation of visceral peritoneum</skos:prefLabel>
    </owl:Class>
    


    <!-- http://www.semanticweb.org/david/ontologies/2013/0/1.3.6.1.4.1.19376.1.8.2.1.912 -->

    <owl:Class rdf:about="&pathLex;912">
        <rdfs:subClassOf rdf:resource="&pathLex;99999"/>
        <skos:definition xml:lang="en">Liver-Infiltrating malignant neoplasm-pN-pN0: No regional lymph node metastasis</skos:definition>
        <skos:prefLabel xml:lang="en">pN0: No regional lymph node metastasis</skos:prefLabel>
    </owl:Class>
    


    <!-- http://www.semanticweb.org/david/ontologies/2013/0/1.3.6.1.4.1.19376.1.8.2.1.913 -->

    <owl:Class rdf:about="&pathLex;913">
        <rdfs:subClassOf rdf:resource="&pathLex;99999"/>
        <skos:definition xml:lang="en">Liver-Infiltrating malignant neoplasm-pN-pN1: Regional lymph node metastasis</skos:definition>
        <skos:prefLabel xml:lang="en">pN1: Regional lymph node metastasis</skos:prefLabel>
    </owl:Class>
    


    <!-- http://www.semanticweb.org/david/ontologies/2013/0/1.3.6.1.4.1.19376.1.8.2.1.915 -->

    <owl:Class rdf:about="&pathLex;915">
        <rdfs:subClassOf rdf:resource="&pathLex;99999"/>
        <skos:definition xml:lang="en">Pancreas-Specimen-Specimen collection procedure-Partial pancreatectomy, pancreatic tail</skos:definition>
        <skos:prefLabel xml:lang="en">Partial pancreatectomy, pancreatic tail</skos:prefLabel>
    </owl:Class>
    


    <!-- http://www.semanticweb.org/david/ontologies/2013/0/1.3.6.1.4.1.19376.1.8.2.1.916 -->

    <owl:Class rdf:about="&pathLex;916">
        <rdfs:subClassOf rdf:resource="&pathLex;99999"/>
        <skos:definition xml:lang="en">Pancreas-Specimen-Specimen collection procedure-Pancreaticoduodenectomy (Whipple resection), total pancreatectomy</skos:definition>
        <skos:prefLabel xml:lang="en">Pancreaticoduodenectomy (Whipple resection), total pancreatectomy</skos:prefLabel>
    </owl:Class>
    


    <!-- http://www.semanticweb.org/david/ontologies/2013/0/1.3.6.1.4.1.19376.1.8.2.1.918 -->

    <owl:Class rdf:about="&pathLex;918">
        <rdfs:subClassOf rdf:resource="&pathLex;99999"/>
        <skos:definition xml:lang="en">Pancreas-Specimen-Specimen collection procedure-Partial pancreatectomy, pancreatic body</skos:definition>
        <skos:prefLabel xml:lang="en">Partial pancreatectomy, pancreatic body</skos:prefLabel>
    </owl:Class>
    


    <!-- http://www.semanticweb.org/david/ontologies/2013/0/1.3.6.1.4.1.19376.1.8.2.1.920 -->

    <owl:Class rdf:about="&pathLex;920">
        <rdfs:subClassOf rdf:resource="&pathLex;99999"/>
        <skos:definition xml:lang="en">Pancreas-Infiltrating malignant neoplasm-Lesion site-Pancreatic head</skos:definition>
        <skos:prefLabel xml:lang="en">Pancreatic head</skos:prefLabel>
    </owl:Class>
    


    <!-- http://www.semanticweb.org/david/ontologies/2013/0/1.3.6.1.4.1.19376.1.8.2.1.921 -->

    <owl:Class rdf:about="&pathLex;921">
        <rdfs:subClassOf rdf:resource="&pathLex;99999"/>
        <skos:definition xml:lang="en">Pancreas-Infiltrating malignant neoplasm-Lesion site-Uncinate process</skos:definition>
        <skos:prefLabel xml:lang="en">Uncinate process</skos:prefLabel>
    </owl:Class>
    


    <!-- http://www.semanticweb.org/david/ontologies/2013/0/1.3.6.1.4.1.19376.1.8.2.1.923 -->

    <owl:Class rdf:about="&pathLex;923">
        <rdfs:subClassOf rdf:resource="&pathLex;99999"/>
        <skos:definition xml:lang="en">Pancreas-Infiltrating malignant neoplasm-Lesion site-Pancreatic body</skos:definition>
        <skos:prefLabel xml:lang="en">Pancreatic body</skos:prefLabel>
    </owl:Class>
    


    <!-- http://www.semanticweb.org/david/ontologies/2013/0/1.3.6.1.4.1.19376.1.8.2.1.924 -->

    <owl:Class rdf:about="&pathLex;924">
        <rdfs:subClassOf rdf:resource="&pathLex;99999"/>
        <skos:definition xml:lang="en">Pancreas-Infiltrating malignant neoplasm-Lesion site-Pancreatic tail</skos:definition>
        <skos:prefLabel xml:lang="en">Pancreatic tail</skos:prefLabel>
    </owl:Class>
    


    <!-- http://www.semanticweb.org/david/ontologies/2013/0/1.3.6.1.4.1.19376.1.8.2.1.925 -->

    <owl:Class rdf:about="&pathLex;925">
        <rdfs:subClassOf rdf:resource="&pathLex;99999"/>
        <skos:prefLabel xml:lang="en">Ductal adenocarcinoma</skos:prefLabel>
        <skos:definition xml:lang="en">Pancreas-Infiltrating malignant neoplasm-Histologic type-Ductal adenocarcinoma</skos:definition>
    </owl:Class>
    


    <!-- http://www.semanticweb.org/david/ontologies/2013/0/1.3.6.1.4.1.19376.1.8.2.1.926 -->

    <owl:Class rdf:about="&pathLex;926">
        <rdfs:subClassOf rdf:resource="&pathLex;99999"/>
        <skos:prefLabel xml:lang="en">Mucinous noncystic carcinoma</skos:prefLabel>
        <skos:definition xml:lang="en">Pancreas-Infiltrating malignant neoplasm-Histologic type-Mucinous noncystic carcinoma</skos:definition>
    </owl:Class>
    


    <!-- http://www.semanticweb.org/david/ontologies/2013/0/1.3.6.1.4.1.19376.1.8.2.1.927 -->

    <owl:Class rdf:about="&pathLex;927">
        <rdfs:subClassOf rdf:resource="&pathLex;99999"/>
        <skos:definition xml:lang="en">Pancreas-Infiltrating malignant neoplasm-Histologic type-Signet-ring cell carcinoma</skos:definition>
        <skos:prefLabel xml:lang="en">Signet-ring cell carcinoma</skos:prefLabel>
    </owl:Class>
    


    <!-- http://www.semanticweb.org/david/ontologies/2013/0/1.3.6.1.4.1.19376.1.8.2.1.928 -->

    <owl:Class rdf:about="&pathLex;928">
        <rdfs:subClassOf rdf:resource="&pathLex;99999"/>
        <skos:prefLabel xml:lang="en">Acinar cell carcinoma</skos:prefLabel>
        <skos:definition xml:lang="en">Pancreas-Infiltrating malignant neoplasm-Histologic type-Acinar cell carcinoma</skos:definition>
    </owl:Class>
    


    <!-- http://www.semanticweb.org/david/ontologies/2013/0/1.3.6.1.4.1.19376.1.8.2.1.930 -->

    <owl:Class rdf:about="&pathLex;930">
        <rdfs:subClassOf rdf:resource="&pathLex;99999"/>
        <skos:definition xml:lang="en">Pancreas-Infiltrating malignant neoplasm-Histologic type-Serous cystadenocarcinoma</skos:definition>
        <skos:prefLabel xml:lang="en">Serous cystadenocarcinoma</skos:prefLabel>
    </owl:Class>
    


    <!-- http://www.semanticweb.org/david/ontologies/2013/0/1.3.6.1.4.1.19376.1.8.2.1.931 -->

    <owl:Class rdf:about="&pathLex;931">
        <rdfs:subClassOf rdf:resource="&pathLex;99999"/>
        <skos:prefLabel xml:lang="en">Invasive mucinous cystic neoplasm</skos:prefLabel>
        <skos:definition xml:lang="en">Pancreas-Infiltrating malignant neoplasm-Histologic type-Invasive mucinous cystic neoplasm</skos:definition>
    </owl:Class>
    


    <!-- http://www.semanticweb.org/david/ontologies/2013/0/1.3.6.1.4.1.19376.1.8.2.1.932 -->

    <owl:Class rdf:about="&pathLex;932">
        <rdfs:subClassOf rdf:resource="&pathLex;99999"/>
        <skos:prefLabel xml:lang="en">Acinar cell cystadenocarcinoma</skos:prefLabel>
        <skos:definition xml:lang="en">Pancreas-Infiltrating malignant neoplasm-Histologic type-Acinar cell cystadenocarcinoma</skos:definition>
    </owl:Class>
    


    <!-- http://www.semanticweb.org/david/ontologies/2013/0/1.3.6.1.4.1.19376.1.8.2.1.935 -->

    <owl:Class rdf:about="&pathLex;935">
        <rdfs:subClassOf rdf:resource="&pathLex;99999"/>
        <skos:prefLabel xml:lang="en">Adenosquamous carcinoma</skos:prefLabel>
        <skos:definition xml:lang="en">Pancreas-Infiltrating malignant neoplasm-Histologic type-Adenosquamous carcinoma</skos:definition>
    </owl:Class>
    


    <!-- http://www.semanticweb.org/david/ontologies/2013/0/1.3.6.1.4.1.19376.1.8.2.1.938 -->

    <owl:Class rdf:about="&pathLex;938">
        <rdfs:subClassOf rdf:resource="&pathLex;99999"/>
        <skos:prefLabel xml:lang="en">Invasive intraductal papillary-mucinous carcinoma</skos:prefLabel>
        <skos:definition xml:lang="en">Pancreas-Infiltrating malignant neoplasm-Histologic type-Invasive intraductal papillary-mucinous carcinoma</skos:definition>
    </owl:Class>
    


    <!-- http://www.semanticweb.org/david/ontologies/2013/0/1.3.6.1.4.1.19376.1.8.2.1.944 -->

    <owl:Class rdf:about="&pathLex;944">
        <rdfs:subClassOf rdf:resource="&pathLex;99999"/>
        <skos:definition xml:lang="en">Pancreas-Infiltrating malignant neoplasm-Margin site-Proximal pancreatic margin</skos:definition>
        <skos:prefLabel xml:lang="en">Proximal pancreatic margin</skos:prefLabel>
    </owl:Class>
    


    <!-- http://www.semanticweb.org/david/ontologies/2013/0/1.3.6.1.4.1.19376.1.8.2.1.945 -->

    <owl:Class rdf:about="&pathLex;945">
        <rdfs:subClassOf rdf:resource="&pathLex;99999"/>
        <skos:prefLabel xml:lang="en">Common bile duct margin</skos:prefLabel>
        <skos:definition xml:lang="en">Pancreas-Infiltrating malignant neoplasm-Margin site-Common bile duct margin</skos:definition>
    </owl:Class>
    


    <!-- http://www.semanticweb.org/david/ontologies/2013/0/1.3.6.1.4.1.19376.1.8.2.1.946 -->

    <owl:Class rdf:about="&pathLex;946">
        <rdfs:subClassOf rdf:resource="&pathLex;99999"/>
        <skos:prefLabel xml:lang="en">Distal pancreatic margin</skos:prefLabel>
        <skos:definition xml:lang="en">Pancreas-Infiltrating malignant neoplasm-Margin site-Distal pancreatic margin</skos:definition>
    </owl:Class>
    


    <!-- http://www.semanticweb.org/david/ontologies/2013/0/1.3.6.1.4.1.19376.1.8.2.1.947 -->

    <owl:Class rdf:about="&pathLex;947">
        <rdfs:subClassOf rdf:resource="&pathLex;99999"/>
        <skos:definition xml:lang="en">Pancreas-Infiltrating malignant neoplasm-Margin site-Posterior retroperitoneal surface of pancreas (Uncinate process (retroperitoneal) margin (nonperitonealized surface of the uncinate process)</skos:definition>
        <skos:prefLabel xml:lang="en">Posterior retroperitoneal surface of pancreas (Uncinate process (retroperitoneal) margin (nonperitonealized surface of the uncinate process)</skos:prefLabel>
    </owl:Class>
    


    <!-- http://www.semanticweb.org/david/ontologies/2013/0/1.3.6.1.4.1.19376.1.8.2.1.948 -->

    <owl:Class rdf:about="&pathLex;948">
        <rdfs:subClassOf rdf:resource="&pathLex;99999"/>
        <skos:definition xml:lang="en">Pancreas-Infiltrating malignant neoplasm-pT-pT0: No evidence of primary tumor</skos:definition>
        <skos:prefLabel xml:lang="en">pT0: No evidence of primary tumor</skos:prefLabel>
    </owl:Class>
    


    <!-- http://www.semanticweb.org/david/ontologies/2013/0/1.3.6.1.4.1.19376.1.8.2.1.949 -->

    <owl:Class rdf:about="&pathLex;949">
        <rdfs:subClassOf rdf:resource="&pathLex;99999"/>
        <skos:definition xml:lang="en">Pancreas-Infiltrating malignant neoplasm-pT-pTis: Carcinoma in situ</skos:definition>
        <skos:prefLabel xml:lang="en">pTis: Carcinoma in situ</skos:prefLabel>
    </owl:Class>
    


    <!-- http://www.semanticweb.org/david/ontologies/2013/0/1.3.6.1.4.1.19376.1.8.2.1.95 -->

    <owl:Class rdf:about="&pathLex;95">
        <rdfs:subClassOf rdf:resource="&pathLex;10"/>
        <skos:definition xml:lang="en">Breast-Infiltrating malignant neoplasm-Lesion size, largest dimension</skos:definition>
        <skos:prefLabel xml:lang="en">Breast-Lesion size, largest dimension</skos:prefLabel>
        <skos:altLabel xml:lang="en">Lesion size, largest dimension</skos:altLabel>
    </owl:Class>
    


    <!-- http://www.semanticweb.org/david/ontologies/2013/0/1.3.6.1.4.1.19376.1.8.2.1.950 -->

    <owl:Class rdf:about="&pathLex;950">
        <rdfs:subClassOf rdf:resource="&pathLex;99999"/>
        <skos:definition xml:lang="en">Pancreas-Infiltrating malignant neoplasm-pT-pT1: Tumor limited to the pancreas, 2 cm or less in greatest dimension</skos:definition>
        <skos:prefLabel xml:lang="en">pT1: Tumor limited to the pancreas, 2 cm or less in greatest dimension</skos:prefLabel>
    </owl:Class>
    


    <!-- http://www.semanticweb.org/david/ontologies/2013/0/1.3.6.1.4.1.19376.1.8.2.1.951 -->

    <owl:Class rdf:about="&pathLex;951">
        <rdfs:subClassOf rdf:resource="&pathLex;99999"/>
        <skos:definition xml:lang="en">Pancreas-Infiltrating malignant neoplasm-pT-pT2: Tumor limited to the pancreas, more than 2 cm in greatest dimension</skos:definition>
        <skos:prefLabel xml:lang="en">pT2: Tumor limited to the pancreas, more than 2 cm in greatest dimension</skos:prefLabel>
    </owl:Class>
    


    <!-- http://www.semanticweb.org/david/ontologies/2013/0/1.3.6.1.4.1.19376.1.8.2.1.952 -->

    <owl:Class rdf:about="&pathLex;952">
        <rdfs:subClassOf rdf:resource="&pathLex;99999"/>
        <skos:definition xml:lang="en">Pancreas-Infiltrating malignant neoplasm-pT-pT3: Tumor extends beyond the pancreas but without involvement of the celiac axis or the superior mesenteric artery</skos:definition>
        <skos:prefLabel xml:lang="en">pT3: Tumor extends beyond the pancreas but without involvement of the celiac axis or the superior mesenteric artery</skos:prefLabel>
    </owl:Class>
    


    <!-- http://www.semanticweb.org/david/ontologies/2013/0/1.3.6.1.4.1.19376.1.8.2.1.953 -->

    <owl:Class rdf:about="&pathLex;953">
        <rdfs:subClassOf rdf:resource="&pathLex;99999"/>
        <skos:definition xml:lang="en">Pancreas-Infiltrating malignant neoplasm-pT-pT4: Tumor involves the celiac axis or the superior mesenteric artery</skos:definition>
        <skos:prefLabel xml:lang="en">pT4: Tumor involves the celiac axis or the superior mesenteric artery</skos:prefLabel>
    </owl:Class>
    


    <!-- http://www.semanticweb.org/david/ontologies/2013/0/1.3.6.1.4.1.19376.1.8.2.1.956 -->

    <owl:Class rdf:about="&pathLex;956">
        <rdfs:subClassOf rdf:resource="&pathLex;99999"/>
        <skos:prefLabel xml:lang="en">Lung</skos:prefLabel>
        <skos:definition xml:lang="en">Lung-Infiltrating malignant neoplasm-Lesion site-Lung</skos:definition>
    </owl:Class>
    


    <!-- http://www.semanticweb.org/david/ontologies/2013/0/1.3.6.1.4.1.19376.1.8.2.1.957 -->

    <owl:Class rdf:about="&pathLex;957">
        <rdfs:subClassOf rdf:resource="&pathLex;99999"/>
        <skos:definition xml:lang="en">Lung-Specimen-Specimen collection procedure-Pneumonectomy</skos:definition>
        <skos:prefLabel xml:lang="en">Pneumonectomy</skos:prefLabel>
    </owl:Class>
    


    <!-- http://www.semanticweb.org/david/ontologies/2013/0/1.3.6.1.4.1.19376.1.8.2.1.959 -->

    <owl:Class rdf:about="&pathLex;959">
        <rdfs:subClassOf rdf:resource="&pathLex;99999"/>
        <skos:prefLabel xml:lang="en">Lobectomy</skos:prefLabel>
        <skos:definition xml:lang="en">Lung-Specimen-Specimen collection procedure-Lobectomy</skos:definition>
    </owl:Class>
    


    <!-- http://www.semanticweb.org/david/ontologies/2013/0/1.3.6.1.4.1.19376.1.8.2.1.960 -->

    <owl:Class rdf:about="&pathLex;960">
        <rdfs:subClassOf rdf:resource="&pathLex;99999"/>
        <skos:prefLabel xml:lang="en">Bilobectomy</skos:prefLabel>
        <skos:definition xml:lang="en">Lung-Specimen-Specimen collection procedure-Bilobectomy</skos:definition>
    </owl:Class>
    


    <!-- http://www.semanticweb.org/david/ontologies/2013/0/1.3.6.1.4.1.19376.1.8.2.1.961 -->

    <owl:Class rdf:about="&pathLex;961">
        <rdfs:subClassOf rdf:resource="&pathLex;99999"/>
        <skos:definition xml:lang="en">Lung-Specimen-Specimen collection procedure-Segmentectomy</skos:definition>
        <skos:prefLabel xml:lang="en">Segmentectomy</skos:prefLabel>
    </owl:Class>
    


    <!-- http://www.semanticweb.org/david/ontologies/2013/0/1.3.6.1.4.1.19376.1.8.2.1.964 -->

    <owl:Class rdf:about="&pathLex;964">
        <rdfs:subClassOf rdf:resource="&pathLex;99999"/>
        <skos:definition xml:lang="en">Lung-Infiltrating malignant neoplasm-Margin site-Parenchymal Margin</skos:definition>
        <skos:prefLabel xml:lang="en">Parenchymal Margin</skos:prefLabel>
    </owl:Class>
    


    <!-- http://www.semanticweb.org/david/ontologies/2013/0/1.3.6.1.4.1.19376.1.8.2.1.966 -->

    <owl:Class rdf:about="&pathLex;966">
        <rdfs:subClassOf rdf:resource="&pathLex;99999"/>
        <skos:prefLabel xml:lang="en">Adenocarcinoma</skos:prefLabel>
        <skos:definition xml:lang="en">Lung-Infiltrating malignant neoplasm-Histologic type-Adenocarcinoma</skos:definition>
    </owl:Class>
    


    <!-- http://www.semanticweb.org/david/ontologies/2013/0/1.3.6.1.4.1.19376.1.8.2.1.967 -->

    <owl:Class rdf:about="&pathLex;967">
        <rdfs:subClassOf rdf:resource="&pathLex;99999"/>
        <skos:prefLabel xml:lang="en">Large cell carcinoma</skos:prefLabel>
        <skos:definition xml:lang="en">Lung-Infiltrating malignant neoplasm-Histologic type-Large cell carcinoma</skos:definition>
    </owl:Class>
    


    <!-- http://www.semanticweb.org/david/ontologies/2013/0/1.3.6.1.4.1.19376.1.8.2.1.968 -->

    <owl:Class rdf:about="&pathLex;968">
        <rdfs:subClassOf rdf:resource="&pathLex;99999"/>
        <skos:definition xml:lang="en">Lung-Infiltrating malignant neoplasm-Histologic type-Small cell carcinoma</skos:definition>
        <skos:prefLabel xml:lang="en">Small cell carcinoma</skos:prefLabel>
    </owl:Class>
    


    <!-- http://www.semanticweb.org/david/ontologies/2013/0/1.3.6.1.4.1.19376.1.8.2.1.969 -->

    <owl:Class rdf:about="&pathLex;969">
        <rdfs:subClassOf rdf:resource="&pathLex;99999"/>
        <skos:prefLabel xml:lang="en">Adenosquamous carcinoma</skos:prefLabel>
        <skos:definition xml:lang="en">Lung-Infiltrating malignant neoplasm-Histologic type-Adenosquamous carcinoma</skos:definition>
    </owl:Class>
    


    <!-- http://www.semanticweb.org/david/ontologies/2013/0/1.3.6.1.4.1.19376.1.8.2.1.97 -->

    <owl:Class rdf:about="&pathLex;97">
        <rdfs:subClassOf rdf:resource="&pathLex;99999"/>
        <skos:definition xml:lang="en">Endometrium-Infiltrating malignant neoplasm-Lesion ulceration</skos:definition>
        <skos:prefLabel xml:lang="en">Lesion ulceration</skos:prefLabel>
    </owl:Class>
    


    <!-- http://www.semanticweb.org/david/ontologies/2013/0/1.3.6.1.4.1.19376.1.8.2.1.970 -->

    <owl:Class rdf:about="&pathLex;970">
        <rdfs:subClassOf rdf:resource="&pathLex;99999"/>
        <skos:definition xml:lang="en">Lung-Infiltrating malignant neoplasm-Histologic type-Sarcomatoid carcinoma</skos:definition>
        <skos:prefLabel xml:lang="en">Sarcomatoid carcinoma</skos:prefLabel>
    </owl:Class>
    


    <!-- http://www.semanticweb.org/david/ontologies/2013/0/1.3.6.1.4.1.19376.1.8.2.1.971 -->

    <owl:Class rdf:about="&pathLex;971">
        <rdfs:subClassOf rdf:resource="&pathLex;99999"/>
        <skos:definition xml:lang="en">Lung-Infiltrating malignant neoplasm-Histologic type-Typical carcinoid tumor</skos:definition>
        <skos:prefLabel xml:lang="en">Typical carcinoid tumor</skos:prefLabel>
    </owl:Class>
    


    <!-- http://www.semanticweb.org/david/ontologies/2013/0/1.3.6.1.4.1.19376.1.8.2.1.976 -->

    <owl:Class rdf:about="&pathLex;976">
        <rdfs:subClassOf rdf:resource="&pathLex;99999"/>
        <skos:prefLabel xml:lang="en">Bronchial Margin</skos:prefLabel>
        <skos:definition xml:lang="en">Lung-Infiltrating malignant neoplasm-Margin site-Bronchial Margin</skos:definition>
    </owl:Class>
    


    <!-- http://www.semanticweb.org/david/ontologies/2013/0/1.3.6.1.4.1.19376.1.8.2.1.977 -->

    <owl:Class rdf:about="&pathLex;977">
        <rdfs:subClassOf rdf:resource="&pathLex;99999"/>
        <skos:definition xml:lang="en">Lung-Infiltrating malignant neoplasm-Margin site-Vascular Margin</skos:definition>
        <skos:prefLabel xml:lang="en">Vascular Margin</skos:prefLabel>
    </owl:Class>
    


    <!-- http://www.semanticweb.org/david/ontologies/2013/0/1.3.6.1.4.1.19376.1.8.2.1.98 -->

    <owl:Class rdf:about="&pathLex;98">
        <rdfs:subClassOf rdf:resource="&pathLex;21"/>
        <skos:definition xml:lang="en">Breast-Infiltrating malignant neoplasm-Microinvasion (DCIS)</skos:definition>
        <skos:prefLabel xml:lang="en">Microinvasion (DCIS)</skos:prefLabel>
    </owl:Class>
    


    <!-- http://www.semanticweb.org/david/ontologies/2013/0/1.3.6.1.4.1.19376.1.8.2.1.981 -->

    <owl:Class rdf:about="&pathLex;981">
        <rdfs:subClassOf rdf:resource="&pathLex;99999"/>
        <skos:definition xml:lang="en">Lung-Infiltrating malignant neoplasm-pT-pT0: No evidence of primary tumor</skos:definition>
        <skos:prefLabel xml:lang="en">pT0: No evidence of primary tumor</skos:prefLabel>
    </owl:Class>
    


    <!-- http://www.semanticweb.org/david/ontologies/2013/0/1.3.6.1.4.1.19376.1.8.2.1.982 -->

    <owl:Class rdf:about="&pathLex;982">
        <rdfs:subClassOf rdf:resource="&pathLex;99999"/>
        <skos:definition xml:lang="en">Lung-Infiltrating malignant neoplasm-pT-pTis: Carcinoma in situ</skos:definition>
        <skos:prefLabel xml:lang="en">pTis: Carcinoma in situ</skos:prefLabel>
    </owl:Class>
    


    <!-- http://www.semanticweb.org/david/ontologies/2013/0/1.3.6.1.4.1.19376.1.8.2.1.983 -->

    <owl:Class rdf:about="&pathLex;983">
        <rdfs:subClassOf rdf:resource="&pathLex;99999"/>
        <skos:definition xml:lang="en">Lung-Infiltrating malignant neoplasm-pT-pT1a: Tumor 2 cm or less in greatest dimension, surrounded by lung or visceral pleura, without bronchoscopic evidence of invasion more proximal than the lobar bronchus (ie, not in the main bronchus); or Superficial spreading tumor of any size with its invasive component limited to the bronchial wall, which may extend proximally to the main bronchus</skos:definition>
        <skos:prefLabel xml:lang="en">pT1a: Tumor 2 cm or less in greatest dimension, surrounded by lung or visceral pleura, without bronchoscopic evidence of invasion more proximal than the lobar bronchus (ie, not in the main bronchus); or Superficial spreading tumor of any size with its invasive component limited to the bronchial wall, which may extend proximally to the main bronchus</skos:prefLabel>
    </owl:Class>
    


    <!-- http://www.semanticweb.org/david/ontologies/2013/0/1.3.6.1.4.1.19376.1.8.2.1.984 -->

    <owl:Class rdf:about="&pathLex;984">
        <rdfs:subClassOf rdf:resource="&pathLex;99999"/>
        <skos:definition xml:lang="en">Lung-Infiltrating malignant neoplasm-pT-pT1b: Tumor greater than 2 cm, but 3 cm or less in greatest dimension, surrounded by lung or visceral pleura, without bronchoscopic evidence of invasion more proximal than the lobar bronchus (ie, not in the main bronchus)</skos:definition>
        <skos:prefLabel xml:lang="en">pT1b: Tumor greater than 2 cm, but 3 cm or less in greatest dimension, surrounded by lung or visceral pleura, without bronchoscopic evidence of invasion more proximal than the lobar bronchus (ie, not in the main bronchus)</skos:prefLabel>
    </owl:Class>
    


    <!-- http://www.semanticweb.org/david/ontologies/2013/0/1.3.6.1.4.1.19376.1.8.2.1.985 -->

    <owl:Class rdf:about="&pathLex;985">
        <rdfs:subClassOf rdf:resource="&pathLex;99999"/>
        <skos:definition xml:lang="en">Lung-Infiltrating malignant neoplasm-pT-pT2a: Tumor greater than 3 cm, but 5 cm or less in greatest dimension surrounded by lung or visceral pleura, without bronchoscopic evidence of invasion more proximal than the lobar bronchus (ie, not in the main bronchus); or Tumor 5 cm or less in greatest dimension with any of the following features of extent: involves main bronchus, 2 cm or more distal to the carina; invades the visceral pleura; associated with atelectasi  or obstructive pneumonitis that extends to the hilar region but does not involve the entire lung</skos:definition>
        <skos:prefLabel xml:lang="en">pT2a: Tumor greater than 3 cm, but 5 cm or less in greatest dimension surrounded by lung or visceral pleura, without bronchoscopic evidence of invasion more proximal than the lobar bronchus (ie, not in the main bronchus); or Tumor 5 cm or less in greatest dimension with any of the following features of extent: involves main bronchus, 2 cm or more distal to the carina; invades the visceral pleura; associated with atelectasi  or obstructive pneumonitis that extends to the hilar region but does not involve the entire lung</skos:prefLabel>
    </owl:Class>
    


    <!-- http://www.semanticweb.org/david/ontologies/2013/0/1.3.6.1.4.1.19376.1.8.2.1.986 -->

    <owl:Class rdf:about="&pathLex;986">
        <rdfs:subClassOf rdf:resource="&pathLex;99999"/>
        <skos:definition xml:lang="en">Lung-Infiltrating malignant neoplasm-pT-pT2b: Tumor greater than 5 cm, but 7 cm or less in greatest dimension</skos:definition>
        <skos:prefLabel xml:lang="en">pT2b: Tumor greater than 5 cm, but 7 cm or less in greatest dimension</skos:prefLabel>
    </owl:Class>
    


    <!-- http://www.semanticweb.org/david/ontologies/2013/0/1.3.6.1.4.1.19376.1.8.2.1.987 -->

    <owl:Class rdf:about="&pathLex;987">
        <rdfs:subClassOf rdf:resource="&pathLex;99999"/>
        <skos:definition xml:lang="en">Lung-Infiltrating malignant neoplasm-pT-pT3: Tumor greater than 7 cm in greatest dimension; or Tumor of any size that directly invades any of the following: chest wall (including superior sulcus tumors), diaphragm, phrenic nerve, mediastinal pleura, parietal pericardium; or Tumor of any size in the main bronchus less than 2 cm distal to the carina but without involvement of the carina; or Tumor of any size associated with atelectasis or obstructive pneumonitis of the entire lung; or Tumors of any size with separate tumor nodule(s) in same lobe</skos:definition>
        <skos:prefLabel xml:lang="en">pT3: Tumor greater than 7 cm in greatest dimension; or Tumor of any size that directly invades any of the following: chest wall (including superior sulcus tumors), diaphragm, phrenic nerve, mediastinal pleura, parietal pericardium; or Tumor of any size in the main bronchus less than 2 cm distal to the carina but without involvement of the carina; or Tumor of any size associated with atelectasis or obstructive pneumonitis of the entire lung; or Tumors of any size with separate tumor nodule(s) in same lobe</skos:prefLabel>
    </owl:Class>
    


    <!-- http://www.semanticweb.org/david/ontologies/2013/0/1.3.6.1.4.1.19376.1.8.2.1.989 -->

    <owl:Class rdf:about="&pathLex;989">
        <rdfs:subClassOf rdf:resource="&pathLex;99999"/>
        <skos:definition xml:lang="en">Lung-Infiltrating malignant neoplasm-pT-pT4: Tumor of any size that invades any of the following: mediastinum, heart, great vessels, trachea, recurrent laryngeal nerve, esophagus, vertebral body, carina; or Tumor of any size with separate tumor nodule(s) in a different lobe of ipsilateral lung</skos:definition>
        <skos:prefLabel xml:lang="en">pT4: Tumor of any size that invades any of the following: mediastinum, heart, great vessels, trachea, recurrent laryngeal nerve, esophagus, vertebral body, carina; or Tumor of any size with separate tumor nodule(s) in a different lobe of ipsilateral lung</skos:prefLabel>
    </owl:Class>
    


    <!-- http://www.semanticweb.org/david/ontologies/2013/0/1.3.6.1.4.1.19376.1.8.2.1.990 -->

    <owl:Class rdf:about="&pathLex;990">
        <rdfs:subClassOf rdf:resource="&pathLex;99999"/>
        <skos:definition xml:lang="en">Lung-Infiltrating malignant neoplasm-pN-pN0: No regional lymph node metastasis</skos:definition>
        <skos:prefLabel xml:lang="en">pN0: No regional lymph node metastasis</skos:prefLabel>
    </owl:Class>
    


    <!-- http://www.semanticweb.org/david/ontologies/2013/0/1.3.6.1.4.1.19376.1.8.2.1.991 -->

    <owl:Class rdf:about="&pathLex;991">
        <rdfs:subClassOf rdf:resource="&pathLex;99999"/>
        <skos:definition xml:lang="en">Lung-Infiltrating malignant neoplasm-pN-pN1: Metastasis in ipsilateral peribronchial and/or ipsilateral hilar lymph nodes, and intrapulmonary nodes, including involvement by direct extension</skos:definition>
        <skos:prefLabel xml:lang="en">pN1: Metastasis in ipsilateral peribronchial and/or ipsilateral hilar lymph nodes, and intrapulmonary nodes, including involvement by direct extension</skos:prefLabel>
    </owl:Class>
    


    <!-- http://www.semanticweb.org/david/ontologies/2013/0/1.3.6.1.4.1.19376.1.8.2.1.992 -->

    <owl:Class rdf:about="&pathLex;992">
        <rdfs:subClassOf rdf:resource="&pathLex;99999"/>
        <skos:definition xml:lang="en">Lung-Infiltrating malignant neoplasm-pN-pN2: Metastasis in ipsilateral mediastinal and/or subcarinal lymph node(s)</skos:definition>
        <skos:prefLabel xml:lang="en">pN2: Metastasis in ipsilateral mediastinal and/or subcarinal lymph node(s)</skos:prefLabel>
    </owl:Class>
    


    <!-- http://www.semanticweb.org/david/ontologies/2013/0/1.3.6.1.4.1.19376.1.8.2.1.993 -->

    <owl:Class rdf:about="&pathLex;993">
        <rdfs:subClassOf rdf:resource="&pathLex;99999"/>
        <skos:definition xml:lang="en">Lung-Infiltrating malignant neoplasm-pN-pN3: Metastasis in contralateral mediastinal, contralateral hilar, ipsilateral or contralateral scalene, or supraclavicular lymph node(s)</skos:definition>
        <skos:prefLabel xml:lang="en">pN3: Metastasis in contralateral mediastinal, contralateral hilar, ipsilateral or contralateral scalene, or supraclavicular lymph node(s)</skos:prefLabel>
    </owl:Class>
    


    <!-- http://www.semanticweb.org/david/ontologies/2013/0/1.3.6.1.4.1.19376.1.8.2.1.994 -->

    <owl:Class rdf:about="&pathLex;994">
        <rdfs:subClassOf rdf:resource="&pathLex;99999"/>
        <skos:prefLabel xml:lang="en">Prostate</skos:prefLabel>
        <skos:definition xml:lang="en">Prostate-Specimen-Target site-Prostate</skos:definition>
    </owl:Class>
    


    <!-- http://www.semanticweb.org/david/ontologies/2013/0/1.3.6.1.4.1.19376.1.8.2.1.995 -->

    <owl:Class rdf:about="&pathLex;995">
        <rdfs:subClassOf rdf:resource="&pathLex;99999"/>
        <skos:prefLabel xml:lang="en">Needle Biopsy</skos:prefLabel>
        <skos:definition xml:lang="en">Prostate-Specimen-Specimen collection procedure-Needle Biopsy</skos:definition>
    </owl:Class>
    


    <!-- http://www.semanticweb.org/david/ontologies/2013/0/1.3.6.1.4.1.19376.1.8.2.1.996 -->

    <owl:Class rdf:about="&pathLex;996">
        <rdfs:subClassOf rdf:resource="&pathLex;99999"/>
        <skos:definition xml:lang="en">Prostate-Specimen-Specimen collection procedure-Radical prostatectomy</skos:definition>
        <skos:prefLabel xml:lang="en">Radical prostatectomy</skos:prefLabel>
    </owl:Class>
    


    <!-- http://www.semanticweb.org/david/ontologies/2013/0/1.3.6.1.4.1.19376.1.8.2.1.99999 -->

    <owl:Class rdf:about="&pathLex;99999">
        <rdfs:subClassOf rdf:resource="&owl;Thing"/>
        <skos:prefLabel xml:lang="en">Not classified</skos:prefLabel>
    </owl:Class>
</rdf:RDF>



<!-- Generated by the OWL API (version 3.2.3.1824) http://owlapi.sourceforge.net -->

