<?xml version="1.0"?>

<!-- 
	This OWL Schema document is a minimalist schema for TMA data.
	It contains all of the concepts that might be deemed unique to a TMA. The classes for general concepts (size, etc.) will be specified in this header.
	The following are examples of external classes and properties that we recommend be used in the TMA OWL document.
	<Classes>
	Stains and Fixatives: "http://www.mindswap.org/2003/CancerOntology/nciOncology.owl#Fixative_Stain" 
	Should point to resources in the NCI metathesaurus.
	
	Organisms: "http://www.mindswap.org/2003/CancerOntology/nciOncology.owl#Organism"
	Clinical information: "http://www.mindswap.org/2003/CancerOntology/nciOncology.owl#Medical_Record"
	Pathology report: "http://www.mindswap.org/2003/CancerOntology/nciOncology.owl#Pathology_Report"
	<Properties>
	Dates: "http://purl.org/dc/terms/date"
    	Identifiers: "http://purl.org/dc/terms/identifier"
	Descriptions: "http://purl.org/dc/terms/description"
	Creator: "http://purl.org/dc/terms/creator"
-->

<rdf:RDF xml:base="http://bioontology.org/ontologies/tma-minimal#" xmlns:rdf="http://www.w3.org/1999/02/22-rdf-syntax-ns#" xmlns:rdfs="http://www.w3.org/2000/01/rdf-schema#" xmlns:tma="http://bioontology.org/ontologies/tma-minimal#" xmlns:owl="http://www.w3.org/2002/07/owl#">
	<owl:Class rdf:about="#tma">		
		<rdfs:comment>This class collects the blocks used to create a TMA.</rdfs:comment>
		<rdfs:label>tma</rdfs:label>
	</owl:Class>
	<owl:Class rdf:about="#block">		
		<rdfs:label>block</rdfs:label>
		<rdfs:subClassOf rdf:resource="#repository_product"/>
		<rdfs:subClassOf rdf:resource="#experimental_component"/>
	</owl:Class>
	<owl:Class rdf:about="#slide">		
		<rdfs:label>slide</rdfs:label>
		<rdfs:subClassOf rdf:resource="#experimental_component"/>
	</owl:Class>
	<owl:Class rdf:about="#core_in_block">		
		<rdfs:label>coreInBlock</rdfs:label>
		<rdfs:subClassOf rdf:resource="#repository_product"/>
		<rdfs:subClassOf rdf:resource="#experimental_component"/>
	</owl:Class>
	<owl:Class rdf:about="#core_on_slide">		
		<rdfs:label>coreOnSlide</rdfs:label>
		<rdfs:subClassOf rdf:resource="#core_in_block"/>
	</owl:Class>
	<owl:Class rdf:about="#repository_product">		
		<rdfs:label>repositoryProduct</rdfs:label>
		<rdfs:comment>This is an abstract parent class.  This class represents any item that is produced by a repository.</rdfs:comment>
	</owl:Class>
	<owl:Class rdf:about="#experimental_component">		
		<rdfs:label>experimentalComponent</rdfs:label>
		<rdfs:comment>This is an abstract parent class.  This class includes items that can be used in an experiment.</rdfs:comment>
	</owl:Class>
	<owl:DatatypeProperty rdf:about="#status">
		<rdfs:label>blockStatus</rdfs:label>
		<rdfs:comment>the current status if known for the block; Production, Retired, Exhausted, or Unknown</rdfs:comment>
		<rdfs:range rdf:resource="http://www.w3.org/2001/XMLSchema#string"/>
		<rdfs:domain rdf:resource="#block"/>
	</owl:DatatypeProperty>
	<owl:ObjectProperty rdf:about="#includes_block">
		<rdfs:label>includesBlock</rdfs:label>
		<rdfs:comment>This property describes the relationship between a TMA and the blocks it contains.</rdfs:comment>
		<rdfs:range rdf:resource="#block"/>
		<rdfs:domain rdf:resource="#tma"/>
		<owl:inverseOf rdf:resource="#included_in_tma"/>
	</owl:ObjectProperty>
	<owl:ObjectProperty rdf:about="#included_in_tma">
		<rdfs:label>includedInTMA</rdfs:label>
		<rdfs:comment>This property is used to refer from a block to the TMA that includes it.</rdfs:comment>
		<rdfs:range rdf:resource="#tma"/>
		<rdfs:domain rdf:resource="#block"/>
		<owl:inverseOf rdf:resource="#includes_block"/>
	</owl:ObjectProperty>
	<owl:ObjectProperty rdf:about="#block_includes_core">
		<rdfs:label>blockIncludesCore</rdfs:label>
		<rdfs:comment>This property describes the relationship between a block and the cores it contains.</rdfs:comment>
		<rdfs:range rdf:resource="#core_in_block"/>
		<rdfs:domain rdf:resource="#block"/>
		<owl:inverseOf rdf:resource="#included_in_block"/>
	</owl:ObjectProperty>
	<owl:ObjectProperty rdf:about="#included_in_block">
		<rdfs:label>includedInBlock</rdfs:label>
		<rdfs:comment>This property describes the relationship between a core and the block containing the core.</rdfs:comment>
		<rdfs:range rdf:resource="#block"/>
		<rdfs:domain rdf:resource="#core_in_block"/>
		<owl:inverseOf rdf:resource="#block_includes_core"/>
	</owl:ObjectProperty>
	<owl:ObjectProperty rdf:about="#slide_includes_core">
		<rdfs:label>slideIncludesCore</rdfs:label>
		<rdfs:comment>This property describes the relationship between a slide and the core sections it contains.</rdfs:comment>
		<rdfs:range rdf:resource="#core_on_slide"/>
		<rdfs:domain rdf:resource="#slide"/>
		<owl:inverseOf rdf:resource="#affixed_to_slide"/>
	</owl:ObjectProperty>
	<owl:ObjectProperty rdf:about="#affixed_to_slide">
		<rdfs:label>affixedToSlide</rdfs:label>
		<rdfs:comment>This property describes the relationship between a core and the slide it has been affixed to.</rdfs:comment>
		<rdfs:range rdf:resource="#slide"/>
		<rdfs:domain rdf:resource="#core_on_slide"/>
		<owl:inverseOf rdf:resource="#slide_includes_core"/>
	</owl:ObjectProperty>
	<owl:ObjectProperty rdf:about="#includes_slide">
		<rdfs:label>includesSlide</rdfs:label>
		<rdfs:comment>This property describes the relationship between a block and the slides that are derived from it.</rdfs:comment>
		<rdfs:range rdf:resource="#slide"/>
		<rdfs:domain rdf:resource="#block"/>
		<owl:inverseOf rdf:resource="#cut_from_block"/>
	</owl:ObjectProperty>
	<owl:ObjectProperty rdf:about="#cut_from_block">
		<rdfs:label>cutFromBlock</rdfs:label>
		<rdfs:comment>This property describes refer from a slide to the block it was cut from.</rdfs:comment>
		<rdfs:range rdf:resource="#block"/>
		<rdfs:domain rdf:resource="#slide"/>
		<owl:inverseOf rdf:resource="#includes_slide"/>
	</owl:ObjectProperty>
	<owl:ObjectProperty rdf:about="#derived_from_core">
		<rdfs:label>derivedFromCore</rdfs:label>
		<rdfs:comment>This property describes the relationship between a core section on a slide and the core it is derived from.</rdfs:comment>
		<rdfs:range rdf:resource="#core_in_block"/>
		<rdfs:domain rdf:resource="#core_on_slide"/>
	</owl:ObjectProperty>
	<owl:DatatypeProperty rdf:about="#control">
		<rdfs:label>control</rdfs:label>
		<rdfs:comment>the quality control review of the test performed on the slide. adequate/not adequate/no QA</rdfs:comment>
		<rdfs:label>control</rdfs:label>
		<rdfs:range rdf:resource="http://www.w3.org/2001/XMLSchema#string"/>
		<rdfs:domain rdf:resource="#slide"/>
	</owl:DatatypeProperty>
	<owl:ObjectProperty rdf:about="#donor_block">
		<rdfs:label>donorBlock</rdfs:label>
		<rdfs:range rdf:resource="#block"/>
		<rdfs:domain rdf:resource="#core_in_block"/>
	</owl:ObjectProperty>
	<owl:DatatypeProperty rdf:about="#level">
		<rdfs:comment>the level of the block for this slide, e.g. 25</rdfs:comment>
		<rdfs:label>slideLevel</rdfs:label>
		<rdfs:range rdf:resource="http://www.w3.org/2001/XMLSchema#integer"/>
		<rdfs:domain rdf:resource="#slide"/>
	</owl:DatatypeProperty>
	<owl:DatatypeProperty rdf:about="#location">
		<rdfs:comment>Please note that the domain of this property is core_in_block.  Therefore, this property
		can apply to instances of either core_in_block or core_on_slide (since core_on_slide is a subclass
		of core_in_block).</rdfs:comment>
		<rdfs:label>location</rdfs:label>
		<rdfs:range rdf:resource="http://www.w3.org/2001/XMLSchema#string"/>
		<rdfs:domain rdf:resource="#core_in_block"/>
	</owl:DatatypeProperty>
	<owl:DatatypeProperty rdf:about="#protocol">
		<rdfs:label>protocol</rdfs:label>
		<rdfs:label>Can be a character string or a URI</rdfs:label>
		<rdfs:range rdf:resource="http://www.w3.org/2001/XMLSchema#anyURI"/>
		<rdfs:domain rdf:resource="#experimental_component"/>
	</owl:DatatypeProperty>
	<owl:DatatypeProperty rdf:about="#report_link">
		<rdfs:comment>This is the identifier used by an instance of class Block to link to a unique report.  This will be the report accession number or some derivation of the report accession number.</rdfs:comment>
		<rdfs:label>reportLink</rdfs:label>
		<rdfs:range rdf:resource="http://www.w3.org/2001/XMLSchema#anyURI"/>
		<rdfs:domain rdf:resource="#block"/>
	</owl:DatatypeProperty>
	<owl:DatatypeProperty rdf:about="#result">
		<rdfs:comment>the result of a test procedure</rdfs:comment>
		<rdfs:label>result</rdfs:label>
		<rdfs:range rdf:resource="http://www.w3.org/2001/XMLSchema#anyURI"/>
		<rdfs:domain rdf:resource="#core_on_slide"/>
	</owl:DatatypeProperty>
	<owl:DatatypeProperty rdf:about="#size">
		<rdfs:comment>the diameter of a core or tissue, measured in millimeters</rdfs:comment>
		<rdfs:label>diameter</rdfs:label>
		<rdfs:range rdf:resource="http://www.w3.org/2001/XMLSchema#string"/>
		<rdfs:domain rdf:resource="#core_in_block"/>
	</owl:DatatypeProperty>
	<owl:DatatypeProperty rdf:about="#thickness">
		<rdfs:comment>the thickness of the section expressed as a real number in microns</rdfs:comment>
		<rdfs:label>sectionThickness</rdfs:label>
		<rdfs:range rdf:resource="http://www.w3.org/2001/XMLSchema#string"/>
		<rdfs:domain rdf:resource="#slide"/>
	</owl:DatatypeProperty>
	<owl:DatatypeProperty rdf:about="#core_spacing">
		<rdfs:comment>the spacings between cores in the TMA block expressed in millimeters (mm); this may be a single value or a series of numbers, each should be expressed as a decimal number with one decimal place, e.g. 3.5</rdfs:comment>
		<rdfs:label>coreSpacing</rdfs:label>
		<rdfs:range rdf:resource="http://www.w3.org/2001/XMLSchema#string"/>
		<rdfs:domain rdf:resource="#block"/>
	</owl:DatatypeProperty>
	<owl:DatatypeProperty rdf:about="#diagnosis">
		<rdfs:comment>Use this property to describe pathalogical diagnosis of original source or drill site.</rdfs:comment>
		<rdfs:label>diagnosis</rdfs:label>
		<rdfs:range rdf:resource="http://www.w3.org/2001/XMLSchema#anyURI"/>
		<rdfs:domain rdf:resource="#core_in_block"/>
	</owl:DatatypeProperty>
	<owl:DatatypeProperty rdf:about="#clinical_annotation">
		<rdfs:comment>The clinical information of the patient from which the core was taken.</rdfs:comment>
		<rdfs:label>clinicalAnnotation</rdfs:label>
		<rdfs:range rdf:resource="http://www.w3.org/2001/XMLSchema#anyURI"/>
		<rdfs:domain rdf:resource="#core_in_block"/>
	</owl:DatatypeProperty>
	<owl:DatatypeProperty rdf:about="#drill_site">
		<rdfs:comment>The location in the donor block from which the core was taken. (Coordinates or description)</rdfs:comment>
		<rdfs:label>drillSite</rdfs:label>
		<rdfs:range rdf:resource="http://www.w3.org/2001/XMLSchema#string"/>
		<rdfs:domain rdf:resource="#core_in_block"/>
	</owl:DatatypeProperty>
	<owl:DatatypeProperty rdf:about="#repository">
		<rdfs:comment>Name of the institution providing the core.  Should use unique identifier specified by HL7.</rdfs:comment>
		<rdfs:label>repository</rdfs:label>
		<rdfs:range rdf:resource="http://www.w3.org/2001/XMLSchema#anyURI"/>
		<rdfs:domain rdf:resource="#repository_product"/>
	</owl:DatatypeProperty>
	<owl:DatatypeProperty rdf:about="#assay">
		<rdfs:comment>The type of special study applied to this slide, e.g. FISH, Immunohistochemistry, in situ PCR, BLOT, regular stain, other.</rdfs:comment>
		<rdfs:label>assay</rdfs:label>
		<rdfs:range rdf:resource="http://www.w3.org/2001/XMLSchema#anyURI"/>
		<rdfs:domain rdf:resource="#slide"/>
	</owl:DatatypeProperty>
</rdf:RDF>
